@prefix dc: <http://purl.org/dc/elements/1.1/> .
@prefix rdf: <http://www.w3.org/1999/02/22-rdf-syntax-ns#> .
@prefix rdfs: <http://www.w3.org/2000/01/rdf-schema#> .
@prefix reg: <http://metadataregistry.org/uri/schema/registry/> .
@prefix skos: <http://www.w3.org/2004/02/skos/core#> .
@prefix xml: <http://www.w3.org/XML/1998/namespace> .
@prefix xsd: <http://www.w3.org/2001/XMLSchema#> .

<http://rdaregistry.info/termList/AspectRatio/1001> a skos:Concept ;
    reg:identifier <727> ;
    reg:status <http://metadataregistry.org/uri/RegStatus/1001> ;
    skos:definition "Aspect ratio for a moving image resource of less than 1.5:1."@en ;
    skos:inScheme <http://rdaregistry.info/termList/AspectRatio> ;
    skos:prefLabel "full screen"@en .

<http://rdaregistry.info/termList/AspectRatio/1002> a skos:Concept ;
    reg:identifier <728> ;
    reg:status <http://metadataregistry.org/uri/RegStatus/1001> ;
    skos:definition "Aspect ratio for a moving image resource of 1.5:1 or greater."@en ;
    skos:inScheme <http://rdaregistry.info/termList/AspectRatio> ;
    skos:prefLabel "wide screen"@en .

<http://rdaregistry.info/termList/AspectRatio/1003> a skos:Concept ;
    reg:identifier <729> ;
    reg:status <http://metadataregistry.org/uri/RegStatus/1001> ;
    skos:definition """Aspect ratio for a moving image resource that includes multiple aspect ratios within the
same resource."""@en ;
    skos:inScheme <http://rdaregistry.info/termList/AspectRatio> ;
    skos:prefLabel "mixed"@en .

<http://metadataregistry.org/uri/RegStatus/1001> a skos:Concept ;
    skos:prefLabel "Published"@en .

<http://rdaregistry.info/termList/AspectRatio> a skos:ConceptScheme ;
    dc:title "RDA Aspect Ratio" .

