@prefix dc: <http://purl.org/dc/elements/1.1/> .
@prefix rdf: <http://www.w3.org/1999/02/22-rdf-syntax-ns#> .
@prefix rdfs: <http://www.w3.org/2000/01/rdf-schema#> .
@prefix reg: <http://metadataregistry.org/uri/schema/registry/> .
@prefix skos: <http://www.w3.org/2004/02/skos/core#> .
@prefix xml: <http://www.w3.org/XML/1998/namespace> .
@prefix xsd: <http://www.w3.org/2001/XMLSchema#> .

<http://rdaregistry.info/termList/bookFormat/1001> a skos:Concept ;
    reg:identifier <850> ;
    reg:status <http://metadataregistry.org/uri/RegStatus/1001> ;
    skos:definition "A book format consisting of one or more leaves that are 1/2 of the whole sheet."@en ;
    skos:inScheme <http://rdaregistry.info/termList/bookFormat> ;
    skos:prefLabel "folio"@en .

<http://rdaregistry.info/termList/bookFormat/1002> a skos:Concept ;
    reg:identifier <851> ;
    reg:status <http://metadataregistry.org/uri/RegStatus/1001> ;
    skos:altLabel "quarto"@en ;
    skos:definition "Quarto; a book format consisting of one or more leaves that are 1/4 of the whole sheet."@en ;
    skos:inScheme <http://rdaregistry.info/termList/bookFormat> ;
    skos:prefLabel "4to"@en .

<http://rdaregistry.info/termList/bookFormat/1003> a skos:Concept ;
    reg:identifier <852> ;
    reg:status <http://metadataregistry.org/uri/RegStatus/1001> ;
    skos:altLabel "octavo"@en ;
    skos:definition "Octavo; a book format consisting of one or more leaves that are 1/8 of the whole sheet."@en ;
    skos:inScheme <http://rdaregistry.info/termList/bookFormat> ;
    skos:prefLabel "8vo"@en .

<http://rdaregistry.info/termList/bookFormat/1004> a skos:Concept ;
    reg:identifier <853> ;
    reg:status <http://metadataregistry.org/uri/RegStatus/1001> ;
    skos:altLabel "duodecimo"@en,
        "twelvemo"@en ;
    skos:definition "Duodecimo or twelvemo; a book format consisting of one or more leaves that are 1/12 of the whole sheet."@en ;
    skos:inScheme <http://rdaregistry.info/termList/bookFormat> ;
    skos:prefLabel "12mo"@en .

<http://rdaregistry.info/termList/bookFormat/1005> a skos:Concept ;
    reg:identifier <854> ;
    reg:status <http://metadataregistry.org/uri/RegStatus/1001> ;
    skos:altLabel "decimo-sexto"@en,
        "sexto-decimo"@en,
        "sixteenmo"@en ;
    skos:definition "Decimo-sexto, sexto-decimo, or sixteenmo; a book format consisting of one or more leaves that are 1/16 of the whole sheet."@en ;
    skos:inScheme <http://rdaregistry.info/termList/bookFormat> ;
    skos:prefLabel "16mo"@en .

<http://rdaregistry.info/termList/bookFormat/1006> a skos:Concept ;
    reg:identifier <855> ;
    reg:status <http://metadataregistry.org/uri/RegStatus/1001> ;
    skos:altLabel "twenty-fourmo"@en,
        "vigesimo-quarto"@en ;
    skos:definition "Vigesimo-quarto or twenty-fourmo; a book format consisting of one or more leaves that are 1/24 of the whole sheet."@en ;
    skos:inScheme <http://rdaregistry.info/termList/bookFormat> ;
    skos:prefLabel "24mo"@en .

<http://rdaregistry.info/termList/bookFormat/1007> a skos:Concept ;
    reg:identifier <856> ;
    reg:status <http://metadataregistry.org/uri/RegStatus/1001> ;
    skos:altLabel "thirty-twomo"@en,
        "trigesimo-secundo"@en ;
    skos:definition "Trigesimo-secundo or thirty-twomo; a book format consisting of one or more leaves that are 1/32 of the whole sheet."@en ;
    skos:inScheme <http://rdaregistry.info/termList/bookFormat> ;
    skos:prefLabel "32mo"@en .

<http://rdaregistry.info/termList/bookFormat/1008> a skos:Concept ;
    reg:identifier <857> ;
    reg:status <http://metadataregistry.org/uri/RegStatus/1001> ;
    skos:altLabel "Forty-eightmo"@en ;
    skos:definition "Forty-eightmo; a book format consisting of one or more leaves that are 1/48 of the whole sheet."@en ;
    skos:inScheme <http://rdaregistry.info/termList/bookFormat> ;
    skos:prefLabel "48mo"@en .

<http://rdaregistry.info/termList/bookFormat/1009> a skos:Concept ;
    reg:identifier <858> ;
    reg:status <http://metadataregistry.org/uri/RegStatus/1001> ;
    skos:altLabel "sixty-fourmo"@en ;
    skos:definition "Sixty-fourmo; a book format consisting of one or more leaves that are 1/64 of the whole sheet."@en ;
    skos:inScheme <http://rdaregistry.info/termList/bookFormat> ;
    skos:prefLabel "64mo"@en .

<http://metadataregistry.org/uri/RegStatus/1001> a skos:Concept ;
    skos:prefLabel "Published"@en .

<http://rdaregistry.info/termList/bookFormat> a skos:ConceptScheme ;
    dc:title "RDA Book Format" .

