@prefix dc: <http://purl.org/dc/elements/1.1/> .
@prefix rdf: <http://www.w3.org/1999/02/22-rdf-syntax-ns#> .
@prefix rdfs: <http://www.w3.org/2000/01/rdf-schema#> .
@prefix reg: <http://metadataregistry.org/uri/schema/registry/> .
@prefix skos: <http://www.w3.org/2004/02/skos/core#> .
@prefix xml: <http://www.w3.org/XML/1998/namespace> .
@prefix xsd: <http://www.w3.org/2001/XMLSchema#> .

<http://rdaregistry.info/termList/CollTitle/1001> a skos:Concept ;
    reg:identifier <583> ;
    reg:status <http://metadataregistry.org/uri/RegStatus/1001> ;
    skos:definition "Conventional collective title for compilations of all correspondence of a person, family, or corporate body."@en ;
    skos:inScheme <http://rdaregistry.info/termList/CollTitle> ;
    skos:prefLabel "Correspondence"@en .

<http://rdaregistry.info/termList/CollTitle/1002> a skos:Concept ;
    reg:identifier <584> ;
    reg:status <http://metadataregistry.org/uri/RegStatus/1001> ;
    skos:definition "Conventional collective title for compilations of all essays by a person."@en ;
    skos:inScheme <http://rdaregistry.info/termList/CollTitle> ;
    skos:prefLabel "Essays"@en .

<http://rdaregistry.info/termList/CollTitle/1003> a skos:Concept ;
    reg:identifier <585> ;
    reg:status <http://metadataregistry.org/uri/RegStatus/1001> ;
    skos:definition "Conventional collective title for compilations of all novels by a person, family, or corporate body."@en ;
    skos:inScheme <http://rdaregistry.info/termList/CollTitle> ;
    skos:prefLabel "Novels"@en .

<http://rdaregistry.info/termList/CollTitle/1004> a skos:Concept ;
    reg:identifier <586> ;
    reg:status <http://metadataregistry.org/uri/RegStatus/1001> ;
    skos:definition "Conventional collective title for compilations of all plays by a person, family, or corporate body."@en ;
    skos:inScheme <http://rdaregistry.info/termList/CollTitle> ;
    skos:prefLabel "Plays"@en .

<http://rdaregistry.info/termList/CollTitle/1005> a skos:Concept ;
    reg:identifier <587> ;
    reg:status <http://metadataregistry.org/uri/RegStatus/1001> ;
    skos:definition "Conventional collective title for compilations of all poems by a person, family, or corporate body."@en ;
    skos:inScheme <http://rdaregistry.info/termList/CollTitle> ;
    skos:prefLabel "Poems"@en .

<http://rdaregistry.info/termList/CollTitle/1006> a skos:Concept ;
    reg:identifier <588> ;
    reg:status <http://metadataregistry.org/uri/RegStatus/1001> ;
    skos:definition "Conventional collective title for compilations of all prose works by a person, family, or corporate body."@en ;
    skos:inScheme <http://rdaregistry.info/termList/CollTitle> ;
    skos:prefLabel "Prose works"@en .

<http://rdaregistry.info/termList/CollTitle/1007> a skos:Concept ;
    reg:identifier <589> ;
    reg:status <http://metadataregistry.org/uri/RegStatus/1001> ;
    skos:definition "Conventional collective title for compilations of all short stories by a person, family, or corporate body."@en ;
    skos:inScheme <http://rdaregistry.info/termList/CollTitle> ;
    skos:prefLabel "Short stories"@en .

<http://rdaregistry.info/termList/CollTitle/1008> a skos:Concept ;
    reg:identifier <590> ;
    reg:status <http://metadataregistry.org/uri/RegStatus/1001> ;
    skos:definition "Conventional collective title for compilations of all speeches by a person, family, or corporate body."@en ;
    skos:inScheme <http://rdaregistry.info/termList/CollTitle> ;
    skos:prefLabel "Speeches"@en .

<http://metadataregistry.org/uri/RegStatus/1001> a skos:Concept ;
    skos:prefLabel "Published"@en .

<http://rdaregistry.info/termList/CollTitle> a skos:ConceptScheme ;
    dc:title "RDA Conventional Collective Title" .

