@prefix dc: <http://purl.org/dc/elements/1.1/> .
@prefix rdakit: <http://metadataregistry.org/uri/profile/rdakit/> .
@prefix rdf: <http://www.w3.org/1999/02/22-rdf-syntax-ns#> .
@prefix rdfs: <http://www.w3.org/2000/01/rdf-schema#> .
@prefix reg: <http://metadataregistry.org/uri/profile/regap/> .
@prefix skos: <http://www.w3.org/2004/02/skos/core#> .
@prefix xml: <http://www.w3.org/XML/1998/namespace> .
@prefix xsd: <http://www.w3.org/2001/XMLSchema#> .

<http://rdaregistry.info/termList/configPlayback/1001> a skos:Concept ;
    rdakit:toolkitDefinition "A configuration of playback channels consisting of a single channel for monophonic sound."@en ;
    rdakit:toolkitLabel "mono"@en ;
    reg:identifier <http://metadataregistry.org/concepts/874> ;
    reg:status <http://metadataregistry.org/uri/RegStatus/1001> ;
    skos:definition "A configuration of playback channels consisting of a single channel for monophonic sound."@en ;
    skos:inScheme <http://rdaregistry.info/termList/configPlayback> ;
    skos:prefLabel "mono"@en .

<http://rdaregistry.info/termList/configPlayback/1002> a skos:Concept ;
    rdakit:toolkitDefinition "A configuration of playback channels consisting of two channels for stereophonic sound."@en ;
    rdakit:toolkitLabel "stereo"@en ;
    reg:identifier <http://metadataregistry.org/concepts/875> ;
    reg:status <http://metadataregistry.org/uri/RegStatus/1001> ;
    skos:definition "A configuration of playback channels consisting of two channels for stereophonic sound."@en ;
    skos:inScheme <http://rdaregistry.info/termList/configPlayback> ;
    skos:prefLabel "stereo"@en .

<http://rdaregistry.info/termList/configPlayback/1003> a skos:Concept ;
    rdakit:toolkitDefinition "A configuration of playback channels consisting of four channels for quadraphonic sound."@en ;
    rdakit:toolkitLabel "quadraphonic"@en ;
    reg:identifier <http://metadataregistry.org/concepts/876> ;
    reg:status <http://metadataregistry.org/uri/RegStatus/1001> ;
    skos:definition "A configuration of playback channels consisting of four channels for quadraphonic sound."@en ;
    skos:inScheme <http://rdaregistry.info/termList/configPlayback> ;
    skos:prefLabel "quadraphonic"@en .

<http://rdaregistry.info/termList/configPlayback/1004> a skos:Concept ;
    rdakit:toolkitDefinition "A configuration of playback channels consisting of more than four channels for surround sound."@en ;
    rdakit:toolkitLabel "surround"@en ;
    reg:identifier <http://metadataregistry.org/concepts/877> ;
    reg:status <http://metadataregistry.org/uri/RegStatus/1001> ;
    skos:definition "A configuration of playback channels consisting of more than four channels for surround sound."@en ;
    skos:inScheme <http://rdaregistry.info/termList/configPlayback> ;
    skos:prefLabel "surround"@en .

<http://metadataregistry.org/uri/RegStatus/1001> a skos:Concept ;
    skos:prefLabel "Published"@en .

<http://rdaregistry.info/termList/configPlayback> a skos:ConceptScheme ;
    dc:title "RDA Configuration of Playback Channels" .

