@prefix dc: <http://purl.org/dc/elements/1.1/> .
@prefix rdf: <http://www.w3.org/1999/02/22-rdf-syntax-ns#> .
@prefix rdfs: <http://www.w3.org/2000/01/rdf-schema#> .
@prefix reg: <http://metadataregistry.org/uri/schema/registry/> .
@prefix skos: <http://www.w3.org/2004/02/skos/core#> .
@prefix xml: <http://www.w3.org/XML/1998/namespace> .
@prefix xsd: <http://www.w3.org/2001/XMLSchema#> .

<http://rdaregistry.info/termList/fontSize/1001> a skos:Concept ;
    reg:identifier <859> ;
    reg:status <http://metadataregistry.org/uri/RegStatus/1001> ;
    skos:altLabel "Extra-Großdruck"@de,
        "Super-Großdruck"@de,
        "extra large print"@en,
        "super large print"@en,
        "impresión extra grande"@es,
        "impresión super grande"@es,
        "extra gros caractères"@fr ;
    skos:definition "Eine Schriftgröße, die sehr groß ist und dazu konzipiert ist, Leser zu unterstützen, die Schwierigkeiten beim Lesen von regulärem oder Großdruck haben."@de,
        "A font size that is very large, designed to aid readers who experience difficulty reading large print."@en,
        "Tipo de letra de gran tamaño definida para ayudar a los lectores que tienen dificultad para leer con tipos de letra normal o mayor."@es,
        "Très grande taille de police de caractères visant à aider les lecteurs qui ont de la difficulté à lire les caractères de taille ordinaire ou les gros caractères."@fr ;
    skos:inScheme <http://rdaregistry.info/termList/fontSize> ;
    skos:prefLabel "Riesendruck"@de,
        "giant print"@en,
        "impresión gigante"@es,
        "caractères géants"@fr ;
    skos:scopeNote "Used for:  Extra large print, Super large print."@en .

<http://rdaregistry.info/termList/fontSize/1002> a skos:Concept ;
    reg:identifier <860> ;
    reg:status <http://metadataregistry.org/uri/RegStatus/1001> ;
    skos:definition "Eine Schriftgröße, die dazu konzipiert ist, Lesern zu helfen, die Schwierigkeiten beim Lesen regulären Drucks haben."@de,
        "A font size designed to aid readers who experience difficulty reading regular print."@en,
        "Extra gros caractères."@fr ;
    skos:inScheme <http://rdaregistry.info/termList/fontSize> ;
    skos:prefLabel "Großdruck"@de,
        "large print"@en,
        "letra grande"@es,
        "gros caractères"@fr .

<http://rdaregistry.info/termList/fontSize/1003> a skos:Concept ;
    reg:identifier <6762> ;
    reg:status <http://metadataregistry.org/uri/RegStatus/1001> ;
    skos:definition "A font size of braille text where the individual cells are expanded to give wider spacing between standard size dots or between dots larger than standard size."@en ;
    skos:inScheme <http://rdaregistry.info/termList/fontSize> ;
    skos:prefLabel "Jumbo-Braille-Schrift"@de,
        "jumbo braille"@en,
        "braille jumbo"@es .

<http://metadataregistry.org/uri/RegStatus/1001> a skos:Concept ;
    skos:prefLabel "Published"@en .

<http://rdaregistry.info/termList/fontSize> a skos:ConceptScheme ;
    dc:title "RDA Font Size" .

