@prefix dc: <http://purl.org/dc/elements/1.1/> .
@prefix rdf: <http://www.w3.org/1999/02/22-rdf-syntax-ns#> .
@prefix rdfs: <http://www.w3.org/2000/01/rdf-schema#> .
@prefix reg: <http://metadataregistry.org/uri/schema/registry/> .
@prefix skos: <http://www.w3.org/2004/02/skos/core#> .
@prefix xml: <http://www.w3.org/XML/1998/namespace> .
@prefix xsd: <http://www.w3.org/2001/XMLSchema#> .

<http://rdaregistry.info/termList/frequency/1001> a skos:Concept ;
    reg:identifier <745> ;
    reg:status <http://metadataregistry.org/uri/RegStatus/1001> ;
    skos:definition "Frequency for a resource issued or updated once every day, usually exclusive of nonworking days."@en ;
    skos:inScheme <http://rdaregistry.info/termList/frequency> ;
    skos:prefLabel "daily"@en .

<http://rdaregistry.info/termList/frequency/1002> a skos:Concept ;
    reg:identifier <746> ;
    reg:status <http://metadataregistry.org/uri/RegStatus/1001> ;
    skos:definition "Frequency for a resource issued or updated three times every week."@en ;
    skos:inScheme <http://rdaregistry.info/termList/frequency> ;
    skos:prefLabel "three times a week"@en .

<http://rdaregistry.info/termList/frequency/1003> a skos:Concept ;
    reg:identifier <747> ;
    reg:status <http://metadataregistry.org/uri/RegStatus/1001> ;
    skos:altLabel "fortnightly"@en ;
    skos:definition "Frequency for a resource issued or updated once every two weeks."@en ;
    skos:inScheme <http://rdaregistry.info/termList/frequency> ;
    skos:prefLabel "biweekly"@en ;
    skos:scopeNote "Used for: Fortnightly."@en .

<http://rdaregistry.info/termList/frequency/1004> a skos:Concept ;
    reg:identifier <748> ;
    reg:status <http://metadataregistry.org/uri/RegStatus/1001> ;
    skos:definition "Frequency for a resource issued or updated once every week."@en ;
    skos:inScheme <http://rdaregistry.info/termList/frequency> ;
    skos:prefLabel "weekly"@en .

<http://rdaregistry.info/termList/frequency/1005> a skos:Concept ;
    reg:identifier <749> ;
    reg:status <http://metadataregistry.org/uri/RegStatus/1001> ;
    skos:definition "Frequency for a resource issued or updated twice every week."@en ;
    skos:inScheme <http://rdaregistry.info/termList/frequency> ;
    skos:prefLabel "semiweekly"@en .

<http://rdaregistry.info/termList/frequency/1006> a skos:Concept ;
    reg:identifier <750> ;
    reg:status <http://metadataregistry.org/uri/RegStatus/1001> ;
    skos:definition "Frequency for a resource issued or updated three times every month."@en ;
    skos:inScheme <http://rdaregistry.info/termList/frequency> ;
    skos:prefLabel "three times a month"@en .

<http://rdaregistry.info/termList/frequency/1007> a skos:Concept ;
    reg:identifier <751> ;
    reg:status <http://metadataregistry.org/uri/RegStatus/1001> ;
    skos:definition "Frequency for a resource issued or updated once every two months."@en ;
    skos:inScheme <http://rdaregistry.info/termList/frequency> ;
    skos:prefLabel "bimonthly"@en .

<http://rdaregistry.info/termList/frequency/1008> a skos:Concept ;
    reg:identifier <752> ;
    reg:status <http://metadataregistry.org/uri/RegStatus/1001> ;
    skos:definition "Frequency for a resource issued or updated once every month."@en ;
    skos:inScheme <http://rdaregistry.info/termList/frequency> ;
    skos:prefLabel "monthly"@en .

<http://rdaregistry.info/termList/frequency/1009> a skos:Concept ;
    reg:identifier <753> ;
    reg:status <http://metadataregistry.org/uri/RegStatus/1001> ;
    skos:definition "Frequency for a resource issued or updated twice every month."@en ;
    skos:inScheme <http://rdaregistry.info/termList/frequency> ;
    skos:prefLabel "semimonthly"@en .

<http://rdaregistry.info/termList/frequency/1010> a skos:Concept ;
    reg:identifier <754> ;
    reg:status <http://metadataregistry.org/uri/RegStatus/1001> ;
    skos:definition "Frequency for a resource issued or updated once every three months."@en ;
    skos:inScheme <http://rdaregistry.info/termList/frequency> ;
    skos:prefLabel "quarterly"@en .

<http://rdaregistry.info/termList/frequency/1011> a skos:Concept ;
    reg:identifier <755> ;
    reg:status <http://metadataregistry.org/uri/RegStatus/1001> ;
    skos:definition "Frequency for a resource issued or updated three times every year."@en ;
    skos:inScheme <http://rdaregistry.info/termList/frequency> ;
    skos:prefLabel "three times a year"@en .

<http://rdaregistry.info/termList/frequency/1012> a skos:Concept ;
    reg:identifier <756> ;
    reg:status <http://metadataregistry.org/uri/RegStatus/1001> ;
    skos:definition "Frequency for a resource issued or updated twice every year."@en ;
    skos:inScheme <http://rdaregistry.info/termList/frequency> ;
    skos:prefLabel "semiannual"@en .

<http://rdaregistry.info/termList/frequency/1013> a skos:Concept ;
    reg:identifier <757> ;
    reg:status <http://metadataregistry.org/uri/RegStatus/1001> ;
    skos:definition "Frequency for a resource issued or updated once every year."@en ;
    skos:inScheme <http://rdaregistry.info/termList/frequency> ;
    skos:prefLabel "annual"@en .

<http://rdaregistry.info/termList/frequency/1014> a skos:Concept ;
    reg:identifier <758> ;
    reg:status <http://metadataregistry.org/uri/RegStatus/1001> ;
    skos:definition "Frequency for a resource issued or updated once every two years."@en ;
    skos:inScheme <http://rdaregistry.info/termList/frequency> ;
    skos:prefLabel "biennial"@en .

<http://rdaregistry.info/termList/frequency/1015> a skos:Concept ;
    reg:identifier <759> ;
    reg:status <http://metadataregistry.org/uri/RegStatus/1001> ;
    skos:definition "Frequency for a resource issued or updated once every three years."@en ;
    skos:inScheme <http://rdaregistry.info/termList/frequency> ;
    skos:prefLabel "triennial"@en .

<http://rdaregistry.info/termList/frequency/1016> a skos:Concept ;
    reg:identifier <760> ;
    reg:status <http://metadataregistry.org/uri/RegStatus/1001> ;
    skos:definition "Frequency for a resource issued with no consistent interval between issues."@en ;
    skos:inScheme <http://rdaregistry.info/termList/frequency> ;
    skos:prefLabel "irregular"@en .

<http://metadataregistry.org/uri/RegStatus/1001> a skos:Concept ;
    skos:prefLabel "Published"@en .

<http://rdaregistry.info/termList/frequency> a skos:ConceptScheme ;
    dc:title "RDA Frequency" .

