@prefix dc: <http://purl.org/dc/elements/1.1/> .
@prefix rdakit: <http://metadataregistry.org/uri/profile/rdakit/> .
@prefix rdf: <http://www.w3.org/1999/02/22-rdf-syntax-ns#> .
@prefix rdfs: <http://www.w3.org/2000/01/rdf-schema#> .
@prefix reg: <http://metadataregistry.org/uri/profile/regap/> .
@prefix skos: <http://www.w3.org/2004/02/skos/core#> .
@prefix xml: <http://www.w3.org/XML/1998/namespace> .
@prefix xsd: <http://www.w3.org/2001/XMLSchema#> .

<http://rdaregistry.info/termList/layout/1001> a skos:Concept ;
    rdakit:toolkitDefinition "A layout that uses both sides of a sheet."@en ;
    rdakit:toolkitLabel "double sided"@en ;
    reg:identifier <http://metadataregistry.org/concepts/836> ;
    reg:status <http://metadataregistry.org/uri/RegStatus/1001> ;
    skos:definition "A layout that uses both sides of a sheet."@en ;
    skos:inScheme <http://rdaregistry.info/termList/layout> ;
    skos:prefLabel "double sided"@en ;
    skos:scopeNote "Applies to sheets and tactile text."@en .

<http://rdaregistry.info/termList/layout/1002> a skos:Concept ;
    rdakit:toolkitDefinition "A layout that uses only one side of a sheet."@en ;
    rdakit:toolkitLabel "single sided"@en ;
    reg:identifier <http://metadataregistry.org/concepts/837> ;
    reg:status <http://metadataregistry.org/uri/RegStatus/1001> ;
    skos:definition "A layout that uses only one side of a sheet."@en ;
    skos:inScheme <http://rdaregistry.info/termList/layout> ;
    skos:prefLabel "single sided"@en ;
    skos:scopeNote "Applies to sheets and tactile text."@en .

<http://rdaregistry.info/termList/layout/1003> a skos:Concept ;
    rdakit:toolkitDefinition "A layout in which the same image is represented in more than one language on each side of a sheet."@en ;
    rdakit:toolkitLabel "back to back"@en ;
    reg:identifier <http://metadataregistry.org/concepts/8436> ;
    reg:status <http://metadataregistry.org/uri/RegStatus/1001> ;
    skos:definition "A layout in which the same image is represented in more than one language on each side of a sheet."@en ;
    skos:inScheme <http://rdaregistry.info/termList/layout> ;
    skos:prefLabel "back to back"@en ;
    skos:scopeNote "Applies to cartographic images."@en .

<http://rdaregistry.info/termList/layout/1004> a skos:Concept ;
    rdakit:toolkitDefinition "A layout consisting of music displayed in indented paragraphs with all of the parts for each measure written consecutively."@en ;
    rdakit:toolkitLabel "bar by bar"@en ;
    reg:identifier <http://metadataregistry.org/concepts/8437> ;
    reg:status <http://metadataregistry.org/uri/RegStatus/1001> ;
    skos:definition "A layout consisting of music displayed in indented paragraphs with all of the parts for each measure written consecutively."@en ;
    skos:inScheme <http://rdaregistry.info/termList/layout> ;
    skos:prefLabel "bar by bar"@en ;
    skos:scopeNote "Applies to tactile music resources."@en .

<http://rdaregistry.info/termList/layout/1005> a skos:Concept ;
    rdakit:toolkitDefinition "A layout consisting of measures displayed in units called parallels and that the beginning of each part’s measure is vertically aligned with the beginning of the same measure for the other part or parts."@en ;
    rdakit:toolkitLabel "bar over bar"@en ;
    reg:identifier <http://metadataregistry.org/concepts/8438> ;
    reg:status <http://metadataregistry.org/uri/RegStatus/1001> ;
    skos:definition "A layout consisting of measures displayed in units called parallels and that the beginning of each part’s measure is vertically aligned with the beginning of the same measure for the other part or parts."@en ;
    skos:inScheme <http://rdaregistry.info/termList/layout> ;
    skos:prefLabel "bar over bar"@en ;
    skos:scopeNote "Applies to tactile music resources."@en .

<http://rdaregistry.info/termList/layout/1006> a skos:Concept ;
    rdakit:toolkitDefinition "A layout that is continued at the same scale on both sides of a sheet or sheets."@en ;
    rdakit:toolkitLabel "both sides"@en ;
    reg:identifier <http://metadataregistry.org/concepts/8439> ;
    reg:status <http://metadataregistry.org/uri/RegStatus/1001> ;
    skos:definition "A layout that is continued at the same scale on both sides of a sheet or sheets."@en ;
    skos:inScheme <http://rdaregistry.info/termList/layout> ;
    skos:prefLabel "both sides"@en ;
    skos:scopeNote "Applies to cartographic images."@en .

<http://rdaregistry.info/termList/layout/1007> a skos:Concept ;
    rdakit:toolkitDefinition "A layout consisting of lines of text that alternate with lines of music for the preceding text."@en ;
    rdakit:toolkitLabel "line by line"@en ;
    reg:identifier <http://metadataregistry.org/concepts/8440> ;
    reg:status <http://metadataregistry.org/uri/RegStatus/1001> ;
    skos:definition "A layout consisting of lines of text that alternate with lines of music for the preceding text."@en ;
    skos:inScheme <http://rdaregistry.info/termList/layout> ;
    skos:prefLabel "line by line"@en ;
    skos:scopeNote "Applies to tactile music resources."@en .

<http://rdaregistry.info/termList/layout/1008> a skos:Concept ;
    rdakit:toolkitDefinition "A layout consisting of measures displayed in parallels, but the measures are not necessarily aligned."@en ;
    rdakit:toolkitLabel "line over line"@en ;
    reg:identifier <http://metadataregistry.org/concepts/8441> ;
    reg:status <http://metadataregistry.org/uri/RegStatus/1001> ;
    skos:definition "A layout consisting of measures displayed in parallels, but the measures are not necessarily aligned."@en ;
    skos:inScheme <http://rdaregistry.info/termList/layout> ;
    skos:prefLabel "line over line"@en ;
    skos:scopeNote "Applies to tactile music resources."@en .

<http://rdaregistry.info/termList/layout/1009> a skos:Concept ;
    rdakit:toolkitDefinition "A layout consisting of chord symbols and melody presented in paragraphs with music braille used for the chord symbols."@en ;
    rdakit:toolkitLabel "melody chord system"@en ;
    reg:identifier <http://metadataregistry.org/concepts/8442> ;
    reg:status <http://metadataregistry.org/uri/RegStatus/1001> ;
    skos:definition "A layout consisting of chord symbols and melody presented in paragraphs with music braille used for the chord symbols."@en ;
    skos:inScheme <http://rdaregistry.info/termList/layout> ;
    skos:prefLabel "melody chord system"@en ;
    skos:scopeNote "Applies to tactile music resources."@en .

<http://rdaregistry.info/termList/layout/1010> a skos:Concept ;
    rdakit:toolkitDefinition "A layout consisting of music presented in parallels."@en ;
    rdakit:toolkitLabel "open score"@en ;
    reg:identifier <http://metadataregistry.org/concepts/8443> ;
    reg:status <http://metadataregistry.org/uri/RegStatus/1001> ;
    skos:definition "A layout consisting of music presented in parallels."@en ;
    skos:inScheme <http://rdaregistry.info/termList/layout> ;
    skos:prefLabel "open score"@en ;
    skos:scopeNote "Open score is similar to bar over bar, but used for ensemble scores. Applies to tactile music resources."@en .

<http://rdaregistry.info/termList/layout/1011> a skos:Concept ;
    rdakit:toolkitDefinition "A layout consisting of music in the outline format."@en ;
    rdakit:toolkitLabel "outline"@en ;
    reg:identifier <http://metadataregistry.org/concepts/8444> ;
    reg:status <http://metadataregistry.org/uri/RegStatus/1001> ;
    skos:definition "A layout consisting of music in the outline format."@en ;
    skos:inScheme <http://rdaregistry.info/termList/layout> ;
    skos:prefLabel "outline"@en ;
    skos:scopeNote "Applies to tactile music resources."@en .

<http://rdaregistry.info/termList/layout/1012> a skos:Concept ;
    rdakit:toolkitDefinition "A layout in braille consisting of music displayed in paragraphs with one part per paragraph."@en ;
    rdakit:toolkitLabel "paragraph"@en ;
    reg:identifier <http://metadataregistry.org/concepts/8445> ;
    reg:status <http://metadataregistry.org/uri/RegStatus/1001> ;
    skos:definition "A layout in braille consisting of music displayed in paragraphs with one part per paragraph."@en ;
    skos:inScheme <http://rdaregistry.info/termList/layout> ;
    skos:prefLabel "paragraph"@en ;
    skos:scopeNote "Applies to tactile music resources."@en .

<http://rdaregistry.info/termList/layout/1013> a skos:Concept ;
    rdakit:toolkitDefinition "A layout consisting of hand or part signs that are prominent in the left margin."@en ;
    rdakit:toolkitLabel "section by section"@en ;
    reg:identifier <http://metadataregistry.org/concepts/8446> ;
    reg:status <http://metadataregistry.org/uri/RegStatus/1001> ;
    skos:definition "A layout consisting of hand or part signs that are prominent in the left margin."@en ;
    skos:inScheme <http://rdaregistry.info/termList/layout> ;
    skos:prefLabel "section by section"@en ;
    skos:scopeNote "Applies to tactile music resources."@en .

<http://rdaregistry.info/termList/layout/1014> a skos:Concept ;
    rdakit:toolkitDefinition "A layout consisting of words, chord symbols, and melody presented in parallels with literary braille used for the chord symbols."@en ;
    rdakit:toolkitLabel "short form scoring"@en ;
    reg:identifier <http://metadataregistry.org/concepts/8447> ;
    reg:status <http://metadataregistry.org/uri/RegStatus/1001> ;
    skos:definition "A layout consisting of words, chord symbols, and melody presented in parallels with literary braille used for the chord symbols."@en ;
    skos:inScheme <http://rdaregistry.info/termList/layout> ;
    skos:prefLabel "short form scoring"@en ;
    skos:scopeNote "Short form scoring is used chiefly for popular and folk music. Applies to tactile music resources."@en .

<http://rdaregistry.info/termList/layout/1015> a skos:Concept ;
    rdakit:toolkitDefinition "A layout consisting of music for single instrumental parts or solos presented in segments of two to five lines, the initial line displaying a measure number or rehearsal designation."@en ;
    rdakit:toolkitLabel "single line"@en ;
    reg:identifier <http://metadataregistry.org/concepts/8448> ;
    reg:status <http://metadataregistry.org/uri/RegStatus/1001> ;
    skos:definition "A layout consisting of music for single instrumental parts or solos presented in segments of two to five lines, the initial line displaying a measure number or rehearsal designation."@en ;
    skos:inScheme <http://rdaregistry.info/termList/layout> ;
    skos:prefLabel "single line"@en ;
    skos:scopeNote "Applies to tactile music resources."@en .

<http://rdaregistry.info/termList/layout/1016> a skos:Concept ;
    rdakit:toolkitDefinition "A layout consisting of musical parts that are combined and written as chords."@en ;
    rdakit:toolkitLabel "vertical score"@en ;
    reg:identifier <http://metadataregistry.org/concepts/8449> ;
    reg:status <http://metadataregistry.org/uri/RegStatus/1001> ;
    skos:definition "A layout consisting of musical parts that are combined and written as chords."@en ;
    skos:inScheme <http://rdaregistry.info/termList/layout> ;
    skos:prefLabel "vertical score"@en ;
    skos:scopeNote "Applies to tactile music resources."@en .

<http://rdaregistry.info/termList/layout/1017> a skos:Concept ;
    rdakit:toolkitDefinition "A layout containing a full blank line between lines of text."@en ;
    rdakit:toolkitLabel "double line spacing"@en ;
    reg:identifier <http://metadataregistry.org/concepts/8450> ;
    reg:status <http://metadataregistry.org/uri/RegStatus/1001> ;
    skos:definition "A layout containing a full blank line between lines of text."@en ;
    skos:inScheme <http://rdaregistry.info/termList/layout> ;
    skos:prefLabel "double line spacing"@en ;
    skos:scopeNote "Applies to tactile text."@en .

<http://metadataregistry.org/uri/RegStatus/1001> a skos:Concept ;
    skos:prefLabel "Published"@en .

<http://rdaregistry.info/termList/layout> a skos:ConceptScheme ;
    dc:title "RDA Layout" .

