@prefix dc: <http://purl.org/dc/elements/1.1/> .
@prefix rdf: <http://www.w3.org/1999/02/22-rdf-syntax-ns#> .
@prefix rdfs: <http://www.w3.org/2000/01/rdf-schema#> .
@prefix reg: <http://metadataregistry.org/uri/schema/registry/> .
@prefix skos: <http://www.w3.org/2004/02/skos/core#> .
@prefix xml: <http://www.w3.org/XML/1998/namespace> .
@prefix xsd: <http://www.w3.org/2001/XMLSchema#> .

<http://rdaregistry.info/termList/ModeIssue/1001> a skos:Concept ;
    reg:identifier <741> ;
    reg:status <http://metadataregistry.org/uri/RegStatus/1001> ;
    skos:definition "A resource that is issued either as a single physical unit (e.g., as a single-volume monograph) or, in the case of an intangible resource, as a single logical unit (e.g., as a PDF file mounted on the Web)."@en ;
    skos:inScheme <http://rdaregistry.info/termList/ModeIssue> ;
    skos:prefLabel "single unit"@en .

<http://rdaregistry.info/termList/ModeIssue/1002> a skos:Concept ;
    reg:identifier <742> ;
    reg:status <http://metadataregistry.org/uri/RegStatus/1001> ;
    skos:definition "A resource issued in two or more parts (either simultaneously or successively) that is complete or intended to be completed within a finite number of parts (e.g., a dictionary in two volumes, three audiocassettes issued as a set)."@en ;
    skos:inScheme <http://rdaregistry.info/termList/ModeIssue> ;
    skos:prefLabel "multipart monograph"@en .

<http://rdaregistry.info/termList/ModeIssue/1003> a skos:Concept ;
    reg:identifier <743> ;
    reg:status <http://metadataregistry.org/uri/RegStatus/1001> ;
    skos:definition "A resource issued in successive parts, usually bearing numbering, that has no predetermined conclusion (e.g., a periodical, a monographic series, a newspaper)."@en ;
    skos:inScheme <http://rdaregistry.info/termList/ModeIssue> ;
    skos:prefLabel "serial"@en ;
    skos:scopeNote "Includes resources that exhibit characteristics of serials, such as successive issues, numbering, and frequency, but whose duration is limited (e.g., newsletters of events) and reproductions of serials."@en .

<http://rdaregistry.info/termList/ModeIssue/1004> a skos:Concept ;
    reg:identifier <744> ;
    reg:status <http://metadataregistry.org/uri/RegStatus/1001> ;
    skos:definition "A resource that is added to or changed by means of updates that do not remain discrete and are integrated into the whole. An integrating resource may be tangible (e.g., a loose-leaf manual that is updated by means of replacement pages) or intangible (e.g., a Web site that is updated either continuously or on a cyclical basis)."@en ;
    skos:inScheme <http://rdaregistry.info/termList/ModeIssue> ;
    skos:prefLabel "integrating resource"@en .

<http://metadataregistry.org/uri/RegStatus/1001> a skos:Concept ;
    skos:prefLabel "Published"@en .

<http://rdaregistry.info/termList/ModeIssue> a skos:ConceptScheme ;
    dc:title "RDA Mode of Issuance" .

