@prefix dc: <http://purl.org/dc/elements/1.1/> .
@prefix rdf: <http://www.w3.org/1999/02/22-rdf-syntax-ns#> .
@prefix rdfs: <http://www.w3.org/2000/01/rdf-schema#> .
@prefix reg: <http://metadataregistry.org/uri/schema/registry/> .
@prefix skos: <http://www.w3.org/2004/02/skos/core#> .
@prefix xml: <http://www.w3.org/XML/1998/namespace> .
@prefix xsd: <http://www.w3.org/2001/XMLSchema#> .

<http://rdaregistry.info/termList/MusNotation/1001> a skos:Concept ;
    reg:identifier <699> ;
    reg:status <http://metadataregistry.org/uri/RegStatus/1001> ;
    skos:definition "A form of musical notation that uses various suggestive lines, symbols, colour, etc., to prompt or guide the performers. It is used for music that is indeterminate in pitch, duration, temperament, etc., and also to depict electronic music in which no performer is involved."@en ;
    skos:inScheme <http://rdaregistry.info/termList/MusNotation> ;
    skos:prefLabel "graphic notation"@en .

<http://rdaregistry.info/termList/MusNotation/1002> a skos:Concept ;
    reg:identifier <700> ;
    reg:status <http://metadataregistry.org/uri/RegStatus/1001> ;
    skos:definition "Musical notation that uses the letters of the alphabet to designate pitches."@en ;
    skos:inScheme <http://rdaregistry.info/termList/MusNotation> ;
    skos:prefLabel "letter notation"@en .

<http://rdaregistry.info/termList/MusNotation/1003> a skos:Concept ;
    reg:identifier <701> ;
    reg:status <http://metadataregistry.org/uri/RegStatus/1001> ;
    skos:definition "A system of notating duration, beginning around 1260 and continuing through about 1600, employing four principal note-values and associated rests: long, breve, semibreve, and minim."@en ;
    skos:inScheme <http://rdaregistry.info/termList/MusNotation> ;
    skos:prefLabel "mensural notation"@en .

<http://rdaregistry.info/termList/MusNotation/1004> a skos:Concept ;
    reg:identifier <702> ;
    reg:status <http://metadataregistry.org/uri/RegStatus/1001> ;
    skos:definition "A system of musical notation conveying pitch by use of numbers, assigned to the notes of a scale, the keys of a keyboard, the finger positions or frets of a string instrument, or to the holes or valves of a wind instrument."@en ;
    skos:inScheme <http://rdaregistry.info/termList/MusNotation> ;
    skos:prefLabel "number notation"@en .

<http://rdaregistry.info/termList/MusNotation/1005> a skos:Concept ;
    reg:identifier <703> ;
    reg:status <http://metadataregistry.org/uri/RegStatus/1008> ;
    skos:inScheme <http://rdaregistry.info/termList/MusNotation> ;
    skos:prefLabel "plainsong notation"@en .

<http://rdaregistry.info/termList/MusNotation/1006> a skos:Concept ;
    reg:identifier <704> ;
    reg:status <http://metadataregistry.org/uri/RegStatus/1001> ;
    skos:definition "The designation of pitches by means of conventional syllables rather than letter names."@en ;
    skos:inScheme <http://rdaregistry.info/termList/MusNotation> ;
    skos:prefLabel "solmization"@en .

<http://rdaregistry.info/termList/MusNotation/1007> a skos:Concept ;
    reg:identifier <705> ;
    reg:status <http://metadataregistry.org/uri/RegStatus/1001> ;
    skos:definition "A system of musical notation in wide use for Western art music, conveying pitch and duration using a staff of multiple parallel lines (in 15th- to 21st-century music, usually five lines) often in combination with other staves."@en ;
    skos:inScheme <http://rdaregistry.info/termList/MusNotation> ;
    skos:prefLabel "staff notation"@en .

<http://rdaregistry.info/termList/MusNotation/1008> a skos:Concept ;
    reg:identifier <706> ;
    reg:status <http://metadataregistry.org/uri/RegStatus/1001> ;
    skos:definition "Any notational system from 1300 or later that uses letters, numbers or other signs as an alternative to conventional staff notation."@en ;
    skos:inScheme <http://rdaregistry.info/termList/MusNotation> ;
    skos:prefLabel "tablature"@en .

<http://rdaregistry.info/termList/MusNotation/1009> a skos:Concept ;
    reg:identifier <707> ;
    reg:status <http://metadataregistry.org/uri/RegStatus/1001> ;
    skos:definition "A system of musical notation that replaces staff notation with sol-fa syllables or their initials."@en ;
    skos:inScheme <http://rdaregistry.info/termList/MusNotation> ;
    skos:prefLabel "tonic sol-fa"@en .

<http://rdaregistry.info/termList/MusNotation/1010> a skos:Concept ;
    reg:identifier <1036> ;
    reg:status <http://metadataregistry.org/uri/RegStatus/1001> ;
    skos:definition "A system of musical notation using neumes, i.e., graphic signs that represent essentially the movement in pitch of a melody."@en ;
    skos:inScheme <http://rdaregistry.info/termList/MusNotation> ;
    skos:prefLabel "neumatic notation"@en .

<http://metadataregistry.org/uri/RegStatus/1008> a skos:Concept ;
    skos:prefLabel "Deprecated"@en .

<http://metadataregistry.org/uri/RegStatus/1001> a skos:Concept ;
    skos:prefLabel "Published"@en .

<http://rdaregistry.info/termList/MusNotation> a skos:ConceptScheme ;
    dc:title "RDA Form of Musical Notation" .

