@prefix dc: <http://purl.org/dc/elements/1.1/> .
@prefix rdf: <http://www.w3.org/1999/02/22-rdf-syntax-ns#> .
@prefix rdfs: <http://www.w3.org/2000/01/rdf-schema#> .
@prefix reg: <http://metadataregistry.org/uri/schema/registry/> .
@prefix skos: <http://www.w3.org/2004/02/skos/core#> .
@prefix xml: <http://www.w3.org/XML/1998/namespace> .
@prefix xsd: <http://www.w3.org/2001/XMLSchema#> .

<http://rdaregistry.info/termList/noteMove/1001> a skos:Concept ;
    reg:identifier <1027> ;
    reg:status <http://metadataregistry.org/uri/RegStatus/1001> ;
    skos:definition "A form of notated movement for dance using musical notation to represent movements by single parts of the body. It is recorded on a horizontal nine–line staff that represents the body."@en ;
    skos:inScheme <http://rdaregistry.info/termList/noteMove> ;
    skos:prefLabel "Stepanoy dance notation"@en .

<http://rdaregistry.info/termList/noteMove/1002> a skos:Concept ;
    reg:identifier <1028> ;
    reg:status <http://metadataregistry.org/uri/RegStatus/1001> ;
    skos:definition "A form of notated movement using abstract symbols to represent movement of the body and limbs as seen from the back. It is recorded on a vertical three–line staff that represents the body."@en ;
    skos:inScheme <http://rdaregistry.info/termList/noteMove> ;
    skos:note "Similar to Kinetography Laban."@en ;
    skos:prefLabel "Labanotation"@en .

<http://rdaregistry.info/termList/noteMove/1004> a skos:Concept ;
    reg:identifier <1030> ;
    reg:status <http://metadataregistry.org/uri/RegStatus/1001> ;
    skos:definition "A form of notated movement recording tactical movements during the course of a game, such as chess."@en ;
    skos:inScheme <http://rdaregistry.info/termList/noteMove> ;
    skos:prefLabel "game play notation"@en .

<http://rdaregistry.info/termList/noteMove/1005> a skos:Concept ;
    reg:identifier <1031> ;
    reg:status <http://metadataregistry.org/uri/RegStatus/1001> ;
    skos:definition "A form of notated movement using a spherical coordinate system to denote body and limb positions. It is recorded on a grid that represents the body."@en ;
    skos:inScheme <http://rdaregistry.info/termList/noteMove> ;
    skos:prefLabel "Eshkol-Wachman movement notation"@en .

<http://rdaregistry.info/termList/noteMove/1006> a skos:Concept ;
    reg:identifier <1032> ;
    reg:status <http://metadataregistry.org/uri/RegStatus/1001> ;
    skos:definition "A form of notated movement using figurative and abstract symbols to represent body and limb positions and movements. It is recorded on a five–line horizontal staff that represents the body."@en ;
    skos:inScheme <http://rdaregistry.info/termList/noteMove> ;
    skos:prefLabel "DanceWriting"@en .

<http://rdaregistry.info/termList/noteMove/1007> a skos:Concept ;
    reg:identifier <1033> ;
    reg:status <http://metadataregistry.org/uri/RegStatus/1001> ;
    skos:definition "A form of notated movement using abstract symbols to represent body and limb positions as seen from the back. It is recorded on a five–line horizontal staff that represents the body."@en ;
    skos:inScheme <http://rdaregistry.info/termList/noteMove> ;
    skos:prefLabel "Benesh movement notation"@en .

<http://rdaregistry.info/termList/noteMove/1008> a skos:Concept ;
    reg:identifier <1034> ;
    reg:status <http://metadataregistry.org/uri/RegStatus/1001> ;
    skos:definition "A form of notated movement using abstract symbols to represent movements of the feet during an associated passage of music. It is recorded on a track drawing that traces the path of the dancer across the floor."@en ;
    skos:inScheme <http://rdaregistry.info/termList/noteMove> ;
    skos:prefLabel "Beauchamp-Feuillet notation"@en .

<http://rdaregistry.info/termList/noteMove/1009> a skos:Concept ;
    reg:identifier <1035> ;
    reg:status <http://metadataregistry.org/uri/RegStatus/1001> ;
    skos:definition "A form of notated movement using abstract symbols to represent body and limb positions and movements.  It is recorded on separate vertical staffs representing the arms, legs, and trunk."@en ;
    skos:inScheme <http://rdaregistry.info/termList/noteMove> ;
    skos:prefLabel "action stroke dance notation"@en .

<http://rdaregistry.info/termList/noteMove/1010> a skos:Concept ;
    reg:identifier <5924> ;
    reg:status <http://metadataregistry.org/uri/RegStatus/1001> ;
    skos:definition "A form of notated movement using abstract symbols to represent movement of the body and limbs as seen from the back. It is recorded on a vertical three–line staff that represents the body."@en ;
    skos:inScheme <http://rdaregistry.info/termList/noteMove> ;
    skos:note "Similar to Labanotation."@en ;
    skos:prefLabel "Kinetography Laban"@en .

<http://metadataregistry.org/uri/RegStatus/1001> a skos:Concept ;
    skos:prefLabel "Published"@en .

<http://rdaregistry.info/termList/noteMove> a skos:ConceptScheme ;
    dc:title "RDA Form of Notated Movement" .

