@prefix dc: <http://purl.org/dc/elements/1.1/> .
@prefix rdf: <http://www.w3.org/1999/02/22-rdf-syntax-ns#> .
@prefix rdfs: <http://www.w3.org/2000/01/rdf-schema#> .
@prefix reg: <http://metadataregistry.org/uri/schema/registry/> .
@prefix skos: <http://www.w3.org/2004/02/skos/core#> .
@prefix xml: <http://www.w3.org/XML/1998/namespace> .
@prefix xsd: <http://www.w3.org/2001/XMLSchema#> .

<http://rdaregistry.info/termList/prodTactile/1001> a skos:Concept ;
    reg:identifier <811> ;
    reg:status <http://metadataregistry.org/uri/RegStatus/1001> ;
    skos:definition "A production method for tactile resources using either a metal or plastic sheet as a master or embossing equipment (often in combination with a computer and specialized software) to produce braille and Moon copies."@en ;
    skos:inScheme <http://rdaregistry.info/termList/prodTactile> ;
    skos:prefLabel "embossed"@en ;
    skos:scopeNote "Also use for \"dotty Moon\" (where the Moon characters are embossed as lines of dots), including use of Tiger Embosser equipment."@en,
        "Use for \"plate copy\" or \"press braille\" or braille generated using Braillo equipment."@en .

<http://rdaregistry.info/termList/prodTactile/1002> a skos:Concept ;
    reg:identifier <812> ;
    reg:status <http://metadataregistry.org/uri/RegStatus/1001> ;
    skos:definition "A production method for tactile resources in which solid plastic dots are heat sealed onto the surface of thin but strong paper."@en ;
    skos:inScheme <http://rdaregistry.info/termList/prodTactile> ;
    skos:prefLabel "solid dot"@en .

<http://rdaregistry.info/termList/prodTactile/1003> a skos:Concept ;
    reg:identifier <813> ;
    reg:status <http://metadataregistry.org/uri/RegStatus/1001> ;
    skos:altLabel "Minolta paper"@en,
        "hot spot"@en,
        "microcapsule paper"@en ;
    skos:definition "A production method for tactile resources in which an image is printed on a special type of paper with embedded microcapsules of alcohol which burst when exposed to heat to make the surface of the paper swell up."@en ;
    skos:inScheme <http://rdaregistry.info/termList/prodTactile> ;
    skos:note "Also known as: Minolta paper (brand name), microcapsule paper, hot spot."@en ;
    skos:prefLabel "swell paper"@en ;
    skos:scopeNote "Use for tactile graphics and for embossing text in Moon characters (linear Moon)."@en .

<http://rdaregistry.info/termList/prodTactile/1004> a skos:Concept ;
    reg:identifier <814> ;
    reg:status <http://metadataregistry.org/uri/RegStatus/1001> ;
    skos:altLabel "vacuum form"@en ;
    skos:definition "A production method for tactile resources in which a collage master is covered with a sheet of plastic, which is heated and vacuumed to generate a copy of a model or diagram."@en ;
    skos:inScheme <http://rdaregistry.info/termList/prodTactile> ;
    skos:note "Also known as: vacuum form."@en ;
    skos:prefLabel "thermoform"@en .

<http://metadataregistry.org/uri/RegStatus/1001> a skos:Concept ;
    skos:prefLabel "Published"@en .

<http://rdaregistry.info/termList/prodTactile> a skos:ConceptScheme ;
    dc:title "RDA Production Method for Tactile Resource" .

