@prefix dc: <http://purl.org/dc/elements/1.1/> .
@prefix rdakit: <http://metadataregistry.org/uri/profile/rdakit/> .
@prefix rdf: <http://www.w3.org/1999/02/22-rdf-syntax-ns#> .
@prefix rdfs: <http://www.w3.org/2000/01/rdf-schema#> .
@prefix reg: <http://metadataregistry.org/uri/profile/regap/> .
@prefix skos: <http://www.w3.org/2004/02/skos/core#> .
@prefix xml: <http://www.w3.org/XML/1998/namespace> .
@prefix xsd: <http://www.w3.org/2001/XMLSchema#> .

<http://rdaregistry.info/termList/RDAInteractivityMode/1001> a skos:Concept ;
    rdakit:toolkitDefinition "An interactivity mode that indicates that the content of an expression responds to actions performed by the user."@en ;
    rdakit:toolkitLabel "interactive"@en ;
    reg:identifier <http://metadataregistry.org/concepts/12584> ;
    reg:status <http://metadataregistry.org/uri/RegStatus/1001> ;
    skos:definition "An interactivity mode that indicates that the content of an expression responds to actions performed by the user."@en ;
    skos:inScheme <http://rdaregistry.info/termList/RDAInteractivityMode> ;
    skos:notation "1001"@en ;
    skos:prefLabel "interactive"@en ;
    skos:scopeNote "Actions include searching, using commands, and making selections."@en .

<http://rdaregistry.info/termList/RDAInteractivityMode/1002> a skos:Concept ;
    rdakit:toolkitDefinition "An interactivity mode that indicates that the content of an expression does not respond to actions performed by the user."@en ;
    rdakit:toolkitLabel "non-interactive"@en ;
    reg:identifier <http://metadataregistry.org/concepts/12585> ;
    reg:status <http://metadataregistry.org/uri/RegStatus/1001> ;
    skos:definition "An interactivity mode that indicates that the content of an expression does not respond to actions performed by the user."@en ;
    skos:inScheme <http://rdaregistry.info/termList/RDAInteractivityMode> ;
    skos:notation "1002"@en ;
    skos:prefLabel "non-interactive"@en .

<http://metadataregistry.org/uri/RegStatus/1001> a skos:Concept ;
    skos:prefLabel "Published"@en .

<http://rdaregistry.info/termList/RDAInteractivityMode> a skos:ConceptScheme ;
    dc:title "RDA Interactivity Mode" .

