@prefix dc: <http://purl.org/dc/elements/1.1/> .
@prefix rdf: <http://www.w3.org/1999/02/22-rdf-syntax-ns#> .
@prefix rdfs: <http://www.w3.org/2000/01/rdf-schema#> .
@prefix reg: <http://metadataregistry.org/uri/schema/registry/> .
@prefix skos: <http://www.w3.org/2004/02/skos/core#> .
@prefix xml: <http://www.w3.org/XML/1998/namespace> .
@prefix xsd: <http://www.w3.org/2001/XMLSchema#> .

<http://rdaregistry.info/termList/RDAPolarity/1001> a skos:Concept ;
    reg:identifier <483> ;
    reg:status <http://metadataregistry.org/uri/RegStatus/1001> ;
    skos:definition "A polarity in which colours and tones used for images are the same as those seen with the human eye."@en ;
    skos:inScheme <http://rdaregistry.info/termList/RDAPolarity> ;
    skos:prefLabel "positive"@en .

<http://rdaregistry.info/termList/RDAPolarity/1002> a skos:Concept ;
    reg:identifier <484> ;
    reg:status <http://metadataregistry.org/uri/RegStatus/1001> ;
    skos:definition "A polarity in which colours and tones used for images are opposite those seen with the human eye."@en ;
    skos:inScheme <http://rdaregistry.info/termList/RDAPolarity> ;
    skos:prefLabel "negative"@en .

<http://rdaregistry.info/termList/RDAPolarity/1003> a skos:Concept ;
    reg:identifier <485> ;
    reg:status <http://metadataregistry.org/uri/RegStatus/1001> ;
    skos:definition "A polarity in which colours and tones used for images are a mixture of those seen with the human eye and those opposite what the human eye would see."@en ;
    skos:inScheme <http://rdaregistry.info/termList/RDAPolarity> ;
    skos:prefLabel "mixed polarity"@en .

<http://metadataregistry.org/uri/RegStatus/1001> a skos:Concept ;
    skos:prefLabel "Published"@en .

<http://rdaregistry.info/termList/RDAPolarity> a skos:ConceptScheme ;
    dc:title "RDA Polarity" .

