@prefix dc: <http://purl.org/dc/elements/1.1/> .
@prefix rdakit: <http://metadataregistry.org/uri/profile/rdakit/> .
@prefix rdf: <http://www.w3.org/1999/02/22-rdf-syntax-ns#> .
@prefix rdfs: <http://www.w3.org/2000/01/rdf-schema#> .
@prefix reg: <http://metadataregistry.org/uri/profile/regap/> .
@prefix skos: <http://www.w3.org/2004/02/skos/core#> .
@prefix xml: <http://www.w3.org/XML/1998/namespace> .
@prefix xsd: <http://www.w3.org/2001/XMLSchema#> .

<http://rdaregistry.info/termList/RDARecordingSources/1001> a skos:Concept ;
    rdakit:toolkitDefinition "A source of information in a manifestation that is a housing that is physically separable from the manifestation. ."@en ;
    rdakit:toolkitLabel "container"@en ;
    reg:identifier <http://metadataregistry.org/concepts/12498> ;
    reg:status <http://metadataregistry.org/uri/RegStatus/1001> ;
    skos:definition "A source of information in a manifestation that is a housing that is physically separable from the manifestation. ."@en ;
    skos:inScheme <http://rdaregistry.info/termList/RDARecordingSources> ;
    skos:notation "1001"@en ;
    skos:prefLabel "container"@en .

<http://rdaregistry.info/termList/RDARecordingSources/1002> a skos:Concept ;
    rdakit:toolkitDefinition "A source of information in a manifestation that is a frame of a film that contains information about title proper, statement of responsibility, publication, or other aspect of the manifestation."@en ;
    rdakit:toolkitLabel "title frame"@en ;
    reg:identifier <http://metadataregistry.org/concepts/12597> ;
    reg:status <http://metadataregistry.org/uri/RegStatus/1001>,
        "Published"@en ;
    reg:uri "http://rdaregistry.info/termList/RDARecordingSources/1002"@en ;
    skos:definition "A source of information in a manifestation that is a frame of a film that contains information about title proper, statement of responsibility, publication, or other aspect of the manifestation."@en ;
    skos:inScheme <http://rdaregistry.info/termList/RDARecordingSources> ;
    skos:notation "1002"@en ;
    skos:prefLabel "title frame"@en .

<http://rdaregistry.info/termList/RDARecordingSources/1003> a skos:Concept ;
    rdakit:toolkitDefinition "A source of information in a manifestation that is a page of a volume that contains information about title proper, statement of responsibility, publication, or other aspect of the manifestation."@en ;
    rdakit:toolkitLabel "title page"@en ;
    reg:identifier <http://metadataregistry.org/concepts/12598> ;
    reg:status <http://metadataregistry.org/uri/RegStatus/1001>,
        "Published"@en ;
    reg:uri "http://rdaregistry.info/termList/RDARecordingSources/1003"@en ;
    skos:definition "A source of information in a manifestation that is a page of a volume that contains information about title proper, statement of responsibility, publication, or other aspect of the manifestation."@en ;
    skos:inScheme <http://rdaregistry.info/termList/RDARecordingSources> ;
    skos:notation "1003"@en ;
    skos:prefLabel "title page"@en .

<http://rdaregistry.info/termList/RDARecordingSources/1004> a skos:Concept ;
    rdakit:toolkitDefinition "A source of information in a manifestation that is a screen of a digital manifestation that contains information about title proper, statement of responsibility, publication, or other aspect of the manifestation."@en ;
    rdakit:toolkitLabel "title screen"@en ;
    reg:identifier <http://metadataregistry.org/concepts/12599> ;
    reg:status <http://metadataregistry.org/uri/RegStatus/1001>,
        "Published"@en ;
    reg:uri "http://rdaregistry.info/termList/RDARecordingSources/1004"@en ;
    skos:definition "A source of information in a manifestation that is a screen of a digital manifestation that contains information about title proper, statement of responsibility, publication, or other aspect of the manifestation."@en ;
    skos:inScheme <http://rdaregistry.info/termList/RDARecordingSources> ;
    skos:notation "1004"@en ;
    skos:prefLabel "title screen"@en .

<http://rdaregistry.info/termList/RDARecordingSources/1005> a skos:Concept ;
    rdakit:toolkitDefinition "A source of information in a manifestation that is a sheet in a set of sheets that contains information about title proper, statement of responsibility, publication, or other aspect of the manifestation."@en ;
    rdakit:toolkitLabel "title sheet"@en ;
    reg:identifier <http://metadataregistry.org/concepts/12600> ;
    reg:status <http://metadataregistry.org/uri/RegStatus/1001>,
        "Published"@en ;
    reg:uri "http://rdaregistry.info/termList/RDARecordingSources/1005"@en ;
    skos:definition "A source of information in a manifestation that is a sheet in a set of sheets that contains information about title proper, statement of responsibility, publication, or other aspect of the manifestation."@en ;
    skos:inScheme <http://rdaregistry.info/termList/RDARecordingSources> ;
    skos:notation "1005"@en ;
    skos:prefLabel "title sheet"@en .

<http://rdaregistry.info/termList/RDARecordingSources/1006> a skos:Concept ;
    rdakit:toolkitDefinition "A source of information in a manifestation that is a card in a set of cards that contains information about title proper, statement of responsibility, publication, or other aspect of the manifestation."@en ;
    rdakit:toolkitLabel "title card"@en ;
    reg:identifier <http://metadataregistry.org/concepts/12601> ;
    reg:status <http://metadataregistry.org/uri/RegStatus/1001>,
        "Published"@en ;
    reg:uri "http://rdaregistry.info/termList/RDARecordingSources/1006"@en ;
    skos:definition "A source of information in a manifestation that is a card in a set of cards that contains information about title proper, statement of responsibility, publication, or other aspect of the manifestation."@en ;
    skos:inScheme <http://rdaregistry.info/termList/RDARecordingSources> ;
    skos:notation "1006"@en ;
    skos:prefLabel "title card"@en .

<http://rdaregistry.info/termList/RDARecordingSources/1007> a skos:Concept ;
    rdakit:toolkitDefinition "A source of information in a manifestation that is a human-readable label that is permanently affixed to the manifestation."@en ;
    rdakit:toolkitLabel "label"@en ;
    reg:identifier <http://metadataregistry.org/concepts/12602> ;
    reg:status <http://metadataregistry.org/uri/RegStatus/1001>,
        "Published"@en ;
    reg:uri "http://rdaregistry.info/termList/RDARecordingSources/1007"@en ;
    skos:definition "A source of information in a manifestation that is a human-readable label that is permanently affixed to the manifestation."@en ;
    skos:inScheme <http://rdaregistry.info/termList/RDARecordingSources> ;
    skos:notation "1007"@en ;
    skos:prefLabel "label"@en .

<http://rdaregistry.info/termList/RDARecordingSources/1008> a skos:Concept ;
    rdakit:toolkitDefinition "A source of information in a manifestation that is a protective binding of a volume."@en ;
    rdakit:toolkitLabel "cover"@en ;
    reg:identifier <http://metadataregistry.org/concepts/12603> ;
    reg:status <http://metadataregistry.org/uri/RegStatus/1001>,
        "Published"@en ;
    reg:uri "http://rdaregistry.info/termList/RDARecordingSources/1008"@en ;
    skos:definition "A source of information in a manifestation that is a protective binding of a volume."@en ;
    skos:inScheme <http://rdaregistry.info/termList/RDARecordingSources> ;
    skos:notation "1008"@en ;
    skos:prefLabel "cover"@en .

<http://rdaregistry.info/termList/RDARecordingSources/1009> a skos:Concept ;
    rdakit:toolkitDefinition "A source of information in a manifestation that is a detachable, protective wrapping of a volume."@en ;
    rdakit:toolkitLabel "jacket"@en ;
    reg:identifier <http://metadataregistry.org/concepts/12604> ;
    reg:status <http://metadataregistry.org/uri/RegStatus/1001>,
        "Published"@en ;
    reg:uri "http://rdaregistry.info/termList/RDARecordingSources/1009"@en ;
    skos:altLabel "book jacket"@en ;
    skos:definition "A source of information in a manifestation that is a detachable, protective wrapping of a volume."@en ;
    skos:inScheme <http://rdaregistry.info/termList/RDARecordingSources> ;
    skos:notation "1009"@en ;
    skos:prefLabel "jacket"@en .

<http://rdaregistry.info/termList/RDARecordingSources/1010> a skos:Concept ;
    rdakit:toolkitDefinition "A source of information in a manifestation that is a part of an editorial page or first page, that appears in each issue of a manifestation of an indeterminate diachronic work, that contains information about title proper, statement of responsibility, publication, or other aspects of the manifestation."@en ;
    rdakit:toolkitLabel "masthead"@en ;
    reg:identifier <http://metadataregistry.org/concepts/12605> ;
    reg:status <http://metadataregistry.org/uri/RegStatus/1001>,
        "Published"@en ;
    reg:uri "http://rdaregistry.info/termList/RDARecordingSources/1010"@en ;
    skos:definition "A source of information in a manifestation that is a part of an editorial page or first page, that appears in each issue of a manifestation of an indeterminate diachronic work, that contains information about title proper, statement of responsibility, publication, or other aspects of the manifestation."@en ;
    skos:inScheme <http://rdaregistry.info/termList/RDARecordingSources> ;
    skos:notation "1010"@en ;
    skos:prefLabel "masthead"@en .

<http://rdaregistry.info/termList/RDARecordingSources/1011> a skos:Concept ;
    rdakit:toolkitDefinition "A source of information in a manifestation that is a textual augmentation of a still image that contains information about title, brief description, or other aspect of the manifestation.."@en ;
    rdakit:toolkitLabel "caption"@en ;
    reg:identifier <http://metadataregistry.org/concepts/12606> ;
    reg:status <http://metadataregistry.org/uri/RegStatus/1001>,
        "Published"@en ;
    reg:uri "http://rdaregistry.info/termList/RDARecordingSources/1011"@en ;
    skos:definition "A source of information in a manifestation that is a textual augmentation of a still image that contains information about title, brief description, or other aspect of the manifestation.."@en ;
    skos:inScheme <http://rdaregistry.info/termList/RDARecordingSources> ;
    skos:notation "1011"@en ;
    skos:prefLabel "caption"@en .

<http://rdaregistry.info/termList/RDARecordingSources/1012> a skos:Concept ;
    rdakit:toolkitDefinition "A source of information in a manifestation that is metadata embedded in an online manifestation."@en ;
    rdakit:toolkitLabel "embedded metadata"@en ;
    reg:identifier <http://metadataregistry.org/concepts/12607> ;
    reg:status <http://metadataregistry.org/uri/RegStatus/1001>,
        "Published"@en ;
    reg:uri "http://rdaregistry.info/termList/RDARecordingSources/1012"@en ;
    skos:definition "A source of information in a manifestation that is metadata embedded in an online manifestation."@en ;
    skos:inScheme <http://rdaregistry.info/termList/RDARecordingSources> ;
    skos:notation "1012"@en ;
    skos:prefLabel "embedded metadata"@en .

<http://metadataregistry.org/uri/RegStatus/1001> a skos:Concept ;
    skos:prefLabel "Published"@en .

<http://rdaregistry.info/termList/RDARecordingSources> a skos:ConceptScheme ;
    dc:title "RDA Recording Sources" .

