@prefix dc: <http://purl.org/dc/elements/1.1/> .
@prefix rdf: <http://www.w3.org/1999/02/22-rdf-syntax-ns#> .
@prefix rdfs: <http://www.w3.org/2000/01/rdf-schema#> .
@prefix reg: <http://metadataregistry.org/uri/schema/registry/> .
@prefix skos: <http://www.w3.org/2004/02/skos/core#> .
@prefix xml: <http://www.w3.org/XML/1998/namespace> .
@prefix xsd: <http://www.w3.org/2001/XMLSchema#> .

<http://rdaregistry.info/termList/recMedium/1001> a skos:Concept ;
    reg:identifier <863> ;
    reg:status <http://metadataregistry.org/uri/RegStatus/1001> ;
    skos:definition "Recording medium that relies on pole reversal in a ferromagnetic medium, typically ferromagnetic oxide particles bound to a continuous flexible surface (tape) or a rigid platter (disc)."@en ;
    skos:inScheme <http://rdaregistry.info/termList/recMedium> ;
    skos:prefLabel "magnetic"@en .

<http://rdaregistry.info/termList/recMedium/1002> a skos:Concept ;
    reg:identifier <864> ;
    reg:status <http://metadataregistry.org/uri/RegStatus/1001> ;
    skos:definition "Recording medium that uses a combination of laser heating with a varying magnetic field to write data to a disc. The Sony MiniDisc is the most prominent format."@en ;
    skos:inScheme <http://rdaregistry.info/termList/recMedium> ;
    skos:prefLabel "magneto-optical"@en .

<http://rdaregistry.info/termList/recMedium/1003> a skos:Concept ;
    reg:identifier <865> ;
    reg:status <http://metadataregistry.org/uri/RegStatus/1001> ;
    skos:definition "Recording medium for recording binary encoded data in a transparent medium with a reflective backing. A laser is used to read the changes in reflectivity as a binary data stream."@en ;
    skos:inScheme <http://rdaregistry.info/termList/recMedium> ;
    skos:prefLabel "optical"@en .

<http://metadataregistry.org/uri/RegStatus/1001> a skos:Concept ;
    skos:prefLabel "Published"@en .

<http://rdaregistry.info/termList/recMedium> a skos:ConceptScheme ;
    dc:title "RDA Recording Medium" .

