@prefix dc: <http://purl.org/dc/elements/1.1/> .
@prefix rdf: <http://www.w3.org/1999/02/22-rdf-syntax-ns#> .
@prefix rdfs: <http://www.w3.org/2000/01/rdf-schema#> .
@prefix reg: <http://metadataregistry.org/uri/schema/registry/> .
@prefix skos: <http://www.w3.org/2004/02/skos/core#> .
@prefix xml: <http://www.w3.org/XML/1998/namespace> .
@prefix xsd: <http://www.w3.org/2001/XMLSchema#> .

<http://rdaregistry.info/termList/statIdentification/1001> a skos:Concept ;
    reg:identifier <1008> ;
    reg:status <http://metadataregistry.org/uri/RegStatus/1001> ;
    skos:definition "Status of identification for an authorized access point when the data is sufficient to establish fully an authorized access point representing the entity."@en ;
    skos:inScheme <http://rdaregistry.info/termList/statIdentification> ;
    skos:prefLabel "fully established"@en .

<http://rdaregistry.info/termList/statIdentification/1002> a skos:Concept ;
    reg:identifier <1009> ;
    reg:status <http://metadataregistry.org/uri/RegStatus/1001> ;
    skos:definition "Status of identification for an authorized access point when the data is insufficient to establish satisfactorily an authorized access point representing the entity."@en ;
    skos:inScheme <http://rdaregistry.info/termList/statIdentification> ;
    skos:prefLabel "provisional"@en .

<http://rdaregistry.info/termList/statIdentification/1003> a skos:Concept ;
    reg:identifier <1010> ;
    reg:status <http://metadataregistry.org/uri/RegStatus/1001> ;
    skos:definition "Status of identification for an authorized access point when the data is taken from a description without the resource described in hand."@en ;
    skos:inScheme <http://rdaregistry.info/termList/statIdentification> ;
    skos:prefLabel "preliminary"@en .

<http://metadataregistry.org/uri/RegStatus/1001> a skos:Concept ;
    skos:prefLabel "Published"@en .

<http://rdaregistry.info/termList/statIdentification> a skos:ConceptScheme ;
    dc:title "RDA Status of Identification" .

