@prefix dc: <http://purl.org/dc/elements/1.1/> .
@prefix rdf: <http://www.w3.org/1999/02/22-rdf-syntax-ns#> .
@prefix rdfs: <http://www.w3.org/2000/01/rdf-schema#> .
@prefix reg: <http://metadataregistry.org/uri/schema/registry/> .
@prefix skos: <http://www.w3.org/2004/02/skos/core#> .
@prefix xml: <http://www.w3.org/XML/1998/namespace> .
@prefix xsd: <http://www.w3.org/2001/XMLSchema#> .

<http://rdaregistry.info/termList/TacNotation/1001> a skos:Concept ;
    reg:identifier <708> ;
    reg:status <http://metadataregistry.org/uri/RegStatus/1001> ;
    skos:definition "A form of tactile notation for text using embossed characters formed by raised dots in six-dot cells."@en ;
    skos:inScheme <http://rdaregistry.info/termList/TacNotation> ;
    skos:prefLabel "braille code"@en .

<http://rdaregistry.info/termList/TacNotation/1002> a skos:Concept ;
    reg:identifier <709> ;
    reg:status <http://metadataregistry.org/uri/RegStatus/1001> ;
    skos:altLabel "computer braille code"@en ;
    skos:definition "A form of tactile notation for computer related materials which enables the representation of symbols and ASCII code."@en ;
    skos:inScheme <http://rdaregistry.info/termList/TacNotation> ;
    skos:prefLabel "computing braille code"@en ;
    skos:scopeNote "Also called Computer braille code."@en .

<http://rdaregistry.info/termList/TacNotation/1003> a skos:Concept ;
    reg:identifier <710> ;
    reg:status <http://metadataregistry.org/uri/RegStatus/1001> ;
    skos:definition "A form of tactile notation used to transcribe mathematical and scientific information."@en ;
    skos:inScheme <http://rdaregistry.info/termList/TacNotation> ;
    skos:prefLabel "mathematics braille code"@en .

<http://rdaregistry.info/termList/TacNotation/1004> a skos:Concept ;
    reg:identifier <711> ;
    reg:status <http://metadataregistry.org/uri/RegStatus/1001> ;
    skos:definition "A form of tactile notation based on simplified letter forms."@en ;
    skos:inScheme <http://rdaregistry.info/termList/TacNotation> ;
    skos:prefLabel "Moon code"@en .

<http://rdaregistry.info/termList/TacNotation/1005> a skos:Concept ;
    reg:identifier <712> ;
    reg:status <http://metadataregistry.org/uri/RegStatus/1001> ;
    skos:definition "A form of tactile notation for music using braille cells."@en ;
    skos:inScheme <http://rdaregistry.info/termList/TacNotation> ;
    skos:prefLabel "music braille code"@en .

<http://rdaregistry.info/termList/TacNotation/1006> a skos:Concept ;
    reg:identifier <713> ;
    reg:status <http://metadataregistry.org/uri/RegStatus/1001> ;
    skos:definition "A form of tactile notation for music."@en ;
    skos:inScheme <http://rdaregistry.info/termList/TacNotation> ;
    skos:prefLabel "tactile musical notation"@en .

<http://rdaregistry.info/termList/TacNotation/1007> a skos:Concept ;
    reg:identifier <1026> ;
    reg:status <http://metadataregistry.org/uri/RegStatus/1001> ;
    skos:definition "A form of tactile notation using a raised version of a print graphic."@en ;
    skos:inScheme <http://rdaregistry.info/termList/TacNotation> ;
    skos:prefLabel "tactile graphic"@en .

<http://metadataregistry.org/uri/RegStatus/1001> a skos:Concept ;
    skos:prefLabel "Published"@en .

<http://rdaregistry.info/termList/TacNotation> a skos:ConceptScheme ;
    dc:title "RDA Form of Tactile Notation" .

