@prefix rdf: <http://www.w3.org/1999/02/22-rdf-syntax-ns#> .
@prefix dc: <http://purl.org/dc/elements/1.1/> .
@prefix rdakit: <http://metadataregistry.org/uri/profile/rdakit/> .
@prefix reg: <http://metadataregistry.org/uri/profile/regap/> .
@prefix skos: <http://www.w3.org/2004/02/skos/core#> .

<http://metadataregistry.org/uri/RegStatus/1001>
    a skos:Concept ;
    skos:prefLabel "Published"@en .

<http://rdaregistry.info/termList/fileType>
    dc:title "RDA File Type" ;
    a skos:ConceptScheme .

<http://rdaregistry.info/termList/fileType1001>
    rdakit:toolkitDefinition "A file type for storing electronically recorded audio content."@en ;
    rdakit:toolkitLabel "audio file"@en ;
    reg:identifier <http://metadataregistry.org/concepts/1116> ;
    reg:status <http://metadataregistry.org/uri/RegStatus/1001> ;
    a skos:Concept ;
    skos:definition "A file type for storing electronically recorded audio content."@en ;
    skos:inScheme <http://rdaregistry.info/termList/fileType> ;
    skos:prefLabel "audio file"@en .

<http://rdaregistry.info/termList/fileType1002>
    rdakit:toolkitDefinition "A file type for storing electronically recorded textual content."@en ;
    rdakit:toolkitLabel "text file"@en ;
    reg:identifier <http://metadataregistry.org/concepts/1117> ;
    reg:status <http://metadataregistry.org/uri/RegStatus/1001> ;
    a skos:Concept ;
    skos:definition "A file type for storing electronically recorded textual content."@en ;
    skos:inScheme <http://rdaregistry.info/termList/fileType> ;
    skos:prefLabel "text file"@en .

<http://rdaregistry.info/termList/fileType1003>
    rdakit:toolkitDefinition "A file type for storing electronically recorded programs consisting of organized lists of instructions to be executed by computer software."@en ;
    rdakit:toolkitLabel "program file"@en ;
    reg:identifier <http://metadataregistry.org/concepts/1118> ;
    reg:status <http://metadataregistry.org/uri/RegStatus/1001> ;
    a skos:Concept ;
    skos:definition "A file type for storing electronically recorded programs consisting of organized lists of instructions to be executed by computer software."@en ;
    skos:inScheme <http://rdaregistry.info/termList/fileType> ;
    skos:prefLabel "program file"@en .

<http://rdaregistry.info/termList/fileType1004>
    rdakit:toolkitDefinition "A file type for storing electronically recorded content representing still images."@en ;
    rdakit:toolkitLabel "image file"@en ;
    reg:identifier <http://metadataregistry.org/concepts/1119> ;
    reg:status <http://metadataregistry.org/uri/RegStatus/1001> ;
    a skos:Concept ;
    skos:definition "A file type for storing electronically recorded content representing still images."@en ;
    skos:inScheme <http://rdaregistry.info/termList/fileType> ;
    skos:prefLabel "image file"@en .

<http://rdaregistry.info/termList/fileType1005>
    rdakit:toolkitDefinition "A file type for storing electronically recorded content representing data values."@en ;
    rdakit:toolkitLabel "data file"@en ;
    reg:identifier <http://metadataregistry.org/concepts/1120> ;
    reg:status <http://metadataregistry.org/uri/RegStatus/1001> ;
    a skos:Concept ;
    skos:definition "A file type for storing electronically recorded content representing data values."@en ;
    skos:inScheme <http://rdaregistry.info/termList/fileType> ;
    skos:prefLabel "data file"@en .

<http://rdaregistry.info/termList/fileType1006>
    rdakit:toolkitDefinition "A file type for storing electronically recorded content representing moving images."@en ;
    rdakit:toolkitLabel "video file"@en ;
    reg:identifier <http://metadataregistry.org/concepts/1121> ;
    reg:status <http://metadataregistry.org/uri/RegStatus/1001> ;
    a skos:Concept ;
    skos:definition "A file type for storing electronically recorded content representing moving images."@en ;
    skos:inScheme <http://rdaregistry.info/termList/fileType> ;
    skos:prefLabel "video file"@en .

