@prefix rdf: <http://www.w3.org/1999/02/22-rdf-syntax-ns#> .
@prefix dc: <http://purl.org/dc/elements/1.1/> .
@prefix rdakit: <http://metadataregistry.org/uri/profile/rdakit/> .
@prefix reg: <http://metadataregistry.org/uri/profile/regap/> .
@prefix skos: <http://www.w3.org/2004/02/skos/core#> .

<http://metadataregistry.org/uri/RegStatus/1001>
    a skos:Concept ;
    skos:prefLabel "Published"@en .

<http://rdaregistry.info/termList/RDAExtensionPlan>
    dc:title "RDA Extension Plan" ;
    a skos:ConceptScheme .

<http://rdaregistry.info/termList/RDAExtensionPlan/1001>
    rdakit:toolkitDefinition "An extension plan for a work intended to be realized in one or more distinct expressions that are all embodied simultaneously."@en ;
    rdakit:toolkitLabel "static plan"@en ;
    reg:identifier <http://metadataregistry.org/concepts/12591> ;
    reg:status <http://metadataregistry.org/uri/RegStatus/1001> ;
    a skos:Concept ;
    skos:definition "An extension plan for a work intended to be realized in one or more distinct expressions that are all embodied simultaneously."@en ;
    skos:inScheme <http://rdaregistry.info/termList/RDAExtensionPlan> ;
    skos:notation "1001"@en ;
    skos:prefLabel "static plan"@en ;
    skos:scopeNote "Includes poems, photographs, and completed novels."@en .

<http://rdaregistry.info/termList/RDAExtensionPlan/1002>
    rdakit:toolkitDefinition "An extension plan for a work that is intended to be realized in one distinct expression that is embodied during a closed timespan."@en ;
    rdakit:toolkitLabel "integrating determinate plan"@en ;
    reg:identifier <http://metadataregistry.org/concepts/12592> ;
    reg:status <http://metadataregistry.org/uri/RegStatus/1001> ;
    a skos:Concept ;
    skos:definition "An extension plan for a work that is intended to be realized in one distinct expression that is embodied during a closed timespan."@en ;
    skos:inScheme <http://rdaregistry.info/termList/RDAExtensionPlan> ;
    skos:notation "1002"@en ;
    skos:prefLabel "integrating determinate plan"@en ;
    skos:scopeNote "Includes project wikis, and conference websites."@en .

<http://rdaregistry.info/termList/RDAExtensionPlan/1003>
    rdakit:toolkitDefinition "An extension plan for a work that is intended to be realized in one distinct expression that is embodied during an open timespan."@en ;
    rdakit:toolkitLabel "integrating indeterminate plan"@en ;
    reg:identifier <http://metadataregistry.org/concepts/12593> ;
    reg:status <http://metadataregistry.org/uri/RegStatus/1001> ;
    a skos:Concept ;
    skos:definition "An extension plan for a work that is intended to be realized in one distinct expression that is embodied during an open timespan."@en ;
    skos:inScheme <http://rdaregistry.info/termList/RDAExtensionPlan> ;
    skos:notation "1003"@en ;
    skos:prefLabel "integrating indeterminate plan"@en ;
    skos:scopeNote "Includes updated standards, laws, and wikis."@en .

<http://rdaregistry.info/termList/RDAExtensionPlan/1004>
    rdakit:toolkitDefinition "An extension plan for a work that is intended to be realized in multiple distinct expressions that are embodied during a closed timespan."@en ;
    rdakit:toolkitLabel "successive determinate plan "@en ;
    reg:identifier <http://metadataregistry.org/concepts/12594> ;
    reg:status <http://metadataregistry.org/uri/RegStatus/1001> ;
    a skos:Concept ;
    skos:definition "An extension plan for a work that is intended to be realized in multiple distinct expressions that are embodied during a closed timespan."@en ;
    skos:inScheme <http://rdaregistry.info/termList/RDAExtensionPlan> ;
    skos:notation "1004"@en ;
    skos:prefLabel "successive determinate plan "@en ;
    skos:scopeNote "Includes serialized versions of novels, dictionaries, and reference works."@en .

<http://rdaregistry.info/termList/RDAExtensionPlan/1005>
    rdakit:toolkitDefinition "An extension plan for a work that is intended to be realized in multiple distinct expressions that are embodied during an open timespan,"@en ;
    rdakit:toolkitLabel "successive indeterminate plan "@en ;
    reg:identifier <http://metadataregistry.org/concepts/12595> ;
    reg:status <http://metadataregistry.org/uri/RegStatus/1001> ;
    a skos:Concept ;
    skos:altLabel "serial work plan"@en ;
    skos:definition "An extension plan for a work that is intended to be realized in multiple distinct expressions that are embodied during an open timespan,"@en ;
    skos:inScheme <http://rdaregistry.info/termList/RDAExtensionPlan> ;
    skos:notation "1005"@en ;
    skos:prefLabel "successive indeterminate plan "@en ;
    skos:scopeNote "Includes periodicals, newspapers, series, newsletters, conference proceedings, annual reports, and archived copies of webpages."@en .

