@prefix rdf: <http://www.w3.org/1999/02/22-rdf-syntax-ns#> .
@prefix dc: <http://purl.org/dc/elements/1.1/> .
@prefix rdakit: <http://metadataregistry.org/uri/profile/rdakit/> .
@prefix reg: <http://metadataregistry.org/uri/profile/regap/> .
@prefix skos: <http://www.w3.org/2004/02/skos/core#> .

<http://metadataregistry.org/uri/RegStatus/1001>
    a skos:Concept ;
    skos:prefLabel "Published"@en .

<http://rdaregistry.info/termList/RDAMaterial>
    dc:title "RDA Material" ;
    a skos:ConceptScheme .

<http://rdaregistry.info/termList/RDAMaterial/1001>
    rdakit:toolkitDefinition "A material composed of the acetate ester of cellulose."@en ;
    rdakit:toolkitLabel "acetate"@en ;
    reg:identifier <http://metadataregistry.org/concepts/8455> ;
    reg:status <http://metadataregistry.org/uri/RegStatus/1001> ;
    a skos:Concept ;
    skos:altLabel "cellulose acetate"@en ;
    skos:definition "A material composed of the acetate ester of cellulose."@en ;
    skos:inScheme <http://rdaregistry.info/termList/RDAMaterial> ;
    skos:prefLabel "acetate"@en ;
    skos:related <http://rdaregistry.info/termList/RDAMaterial/1029>, <http://rdaregistry.info/termList/RDAMaterial/1040> .

<http://rdaregistry.info/termList/RDAMaterial/1002>
    rdakit:toolkitDefinition "A material consisting of pigment or dye bound in an emulsion of acrylic resin."@en ;
    rdakit:toolkitLabel "acrylic paint"@en ;
    reg:identifier <http://metadataregistry.org/concepts/8456> ;
    reg:status <http://metadataregistry.org/uri/RegStatus/1001> ;
    a skos:Concept ;
    skos:definition "A material consisting of pigment or dye bound in an emulsion of acrylic resin."@en ;
    skos:inScheme <http://rdaregistry.info/termList/RDAMaterial> ;
    skos:prefLabel "acrylic paint"@en .

<http://rdaregistry.info/termList/RDAMaterial/1003>
    rdakit:toolkitDefinition "A material of non-magnetic metal, usually alloyed, that is ductile and malleable with a lustre that ranges from grey to silver."@en ;
    rdakit:toolkitLabel "aluminium"@en ;
    reg:identifier <http://metadataregistry.org/concepts/8457> ;
    reg:status <http://metadataregistry.org/uri/RegStatus/1001> ;
    a skos:Concept ;
    skos:altLabel "aluminum"@en ;
    skos:definition "A material of non-magnetic metal, usually alloyed, that is ductile and malleable with a lustre that ranges from grey to silver."@en ;
    skos:inScheme <http://rdaregistry.info/termList/RDAMaterial> ;
    skos:prefLabel "aluminium"@en .

<http://rdaregistry.info/termList/RDAMaterial/1004>
    rdakit:toolkitDefinition "A material consisting of a high-grade white cardboard, most commonly made by pasting together sheets of heavy ledger paper."@en ;
    rdakit:toolkitLabel "Bristol board"@en ;
    reg:identifier <http://metadataregistry.org/concepts/8458> ;
    reg:status <http://metadataregistry.org/uri/RegStatus/1001> ;
    a skos:Concept ;
    skos:definition "A material consisting of a high-grade white cardboard, most commonly made by pasting together sheets of heavy ledger paper."@en ;
    skos:inScheme <http://rdaregistry.info/termList/RDAMaterial> ;
    skos:prefLabel "Bristol board"@en .

<http://rdaregistry.info/termList/RDAMaterial/1005>
    rdakit:toolkitDefinition "A material consisting of a closely woven textile made in various weights, usually of flax, hemp, jute, or cotton, used as a support for painting or printing; or a loosely woven, lattice-like mesh, usually of flax, hemp, jute, or cotton, used as a needlepoint foundation."@en ;
    rdakit:toolkitLabel "canvas"@en ;
    reg:identifier <http://metadataregistry.org/concepts/8459> ;
    reg:status <http://metadataregistry.org/uri/RegStatus/1001> ;
    a skos:Concept ;
    skos:definition "A material consisting of a closely woven textile made in various weights, usually of flax, hemp, jute, or cotton, used as a support for painting or printing; or a loosely woven, lattice-like mesh, usually of flax, hemp, jute, or cotton, used as a needlepoint foundation."@en ;
    skos:inScheme <http://rdaregistry.info/termList/RDAMaterial> ;
    skos:prefLabel "canvas"@en .

<http://rdaregistry.info/termList/RDAMaterial/1006>
    rdakit:toolkitDefinition "A material consisting of a type of stiff sheet typically made of good-quality chemical pulp or rag pulp, varying greatly in type and strength, and that is thicker than 0.1524 mm."@en ;
    rdakit:toolkitLabel "cardboard"@en ;
    reg:identifier <http://metadataregistry.org/concepts/8460> ;
    reg:status <http://metadataregistry.org/uri/RegStatus/1001> ;
    a skos:Concept ;
    skos:definition "A material consisting of a type of stiff sheet typically made of good-quality chemical pulp or rag pulp, varying greatly in type and strength, and that is thicker than 0.1524 mm."@en ;
    skos:inScheme <http://rdaregistry.info/termList/RDAMaterial> ;
    skos:prefLabel "cardboard"@en .

<http://rdaregistry.info/termList/RDAMaterial/1007>
    rdakit:toolkitDefinition "A material consisting of a nonmetallic mineral, such as clay, fired at a high temperature to form a hard, brittle, heat- and corrosion-resistant material."@en ;
    rdakit:toolkitLabel "ceramic"@en ;
    reg:identifier <http://metadataregistry.org/concepts/8461> ;
    reg:status <http://metadataregistry.org/uri/RegStatus/1001> ;
    a skos:Concept ;
    skos:definition "A material consisting of a nonmetallic mineral, such as clay, fired at a high temperature to form a hard, brittle, heat- and corrosion-resistant material."@en ;
    skos:inScheme <http://rdaregistry.info/termList/RDAMaterial> ;
    skos:prefLabel "ceramic"@en .

<http://rdaregistry.info/termList/RDAMaterial/1008>
    rdakit:toolkitDefinition "A material consisting of fine-grained limestone, or a soft, earthy form of calcium carbonate."@en ;
    rdakit:toolkitLabel "chalk"@en ;
    reg:identifier <http://metadataregistry.org/concepts/8462> ;
    reg:status <http://metadataregistry.org/uri/RegStatus/1001> ;
    a skos:Concept ;
    skos:definition "A material consisting of fine-grained limestone, or a soft, earthy form of calcium carbonate."@en ;
    skos:inScheme <http://rdaregistry.info/termList/RDAMaterial> ;
    skos:prefLabel "chalk"@en .

<http://rdaregistry.info/termList/RDAMaterial/1009>
    rdakit:toolkitDefinition "A material consisting of the dark grey residue made of carbon, and any remaining ash, obtained by removing water and other volatile constituents from animal and plant substances."@en ;
    rdakit:toolkitLabel "charcoal"@en ;
    reg:identifier <http://metadataregistry.org/concepts/8463> ;
    reg:status <http://metadataregistry.org/uri/RegStatus/1001> ;
    a skos:Concept ;
    skos:definition "A material consisting of the dark grey residue made of carbon, and any remaining ash, obtained by removing water and other volatile constituents from animal and plant substances."@en ;
    skos:inScheme <http://rdaregistry.info/termList/RDAMaterial> ;
    skos:prefLabel "charcoal"@en .

<http://rdaregistry.info/termList/RDAMaterial/1010>
    rdakit:toolkitDefinition "A material made by treating cellulose with acetic acid."@en ;
    rdakit:toolkitLabel "diacetate"@en ;
    reg:identifier <http://metadataregistry.org/concepts/8464> ;
    reg:status <http://metadataregistry.org/uri/RegStatus/1001> ;
    a skos:Concept ;
    skos:altLabel "cellulose diacetate"@en ;
    skos:definition "A material made by treating cellulose with acetic acid."@en ;
    skos:inScheme <http://rdaregistry.info/termList/RDAMaterial> ;
    skos:prefLabel "diacetate"@en ;
    skos:related <http://rdaregistry.info/termList/RDAMaterial/1029>, <http://rdaregistry.info/termList/RDAMaterial/1033>, <http://rdaregistry.info/termList/RDAMaterial/1040> .

<http://rdaregistry.info/termList/RDAMaterial/1011>
    rdakit:toolkitDefinition "A material consisting of a coloured substance dissolved or suspended in a liquid that can be absorbed by the base material."@en ;
    rdakit:toolkitLabel "dye"@en ;
    reg:identifier <http://metadataregistry.org/concepts/8465> ;
    reg:status <http://metadataregistry.org/uri/RegStatus/1001> ;
    a skos:Concept ;
    skos:definition "A material consisting of a coloured substance dissolved or suspended in a liquid that can be absorbed by the base material."@en ;
    skos:inScheme <http://rdaregistry.info/termList/RDAMaterial> ;
    skos:prefLabel "dye"@en .

<http://rdaregistry.info/termList/RDAMaterial/1012>
    rdakit:toolkitDefinition "A material consisting of silicon dioxide, known as silica, fused with one or more basic oxides; generally transparent but often translucent or opaque."@en ;
    rdakit:toolkitLabel "glass"@en ;
    reg:identifier <http://metadataregistry.org/concepts/8466> ;
    reg:status <http://metadataregistry.org/uri/RegStatus/1001> ;
    a skos:Concept ;
    skos:definition "A material consisting of silicon dioxide, known as silica, fused with one or more basic oxides; generally transparent but often translucent or opaque."@en ;
    skos:inScheme <http://rdaregistry.info/termList/RDAMaterial> ;
    skos:prefLabel "glass"@en .

<http://rdaregistry.info/termList/RDAMaterial/1013>
    rdakit:toolkitDefinition "A material consisting of pigment and a binding agent, and sometimes added inert materials, to form an opaque, coloured, water-soluble paint."@en ;
    rdakit:toolkitLabel "gouache"@en ;
    reg:identifier <http://metadataregistry.org/concepts/8467> ;
    reg:status <http://metadataregistry.org/uri/RegStatus/1001> ;
    a skos:Concept ;
    skos:definition "A material consisting of pigment and a binding agent, and sometimes added inert materials, to form an opaque, coloured, water-soluble paint."@en ;
    skos:inScheme <http://rdaregistry.info/termList/RDAMaterial> ;
    skos:prefLabel "gouache"@en ;
    skos:scopeNote "Poster paints are included. The term originally referred to the technique of oil paint applied on top of tempera."@en .

<http://rdaregistry.info/termList/RDAMaterial/1014>
    rdakit:toolkitDefinition "A material consisting of a naturally occurring allotrope of carbon which is opaque, soft, greasy to the touch, and iron black to steel gray in color."@en ;
    rdakit:toolkitLabel "graphite"@en ;
    reg:identifier <http://metadataregistry.org/concepts/8468> ;
    reg:status <http://metadataregistry.org/uri/RegStatus/1001> ;
    a skos:Concept ;
    skos:definition "A material consisting of a naturally occurring allotrope of carbon which is opaque, soft, greasy to the touch, and iron black to steel gray in color."@en ;
    skos:inScheme <http://rdaregistry.info/termList/RDAMaterial> ;
    skos:prefLabel "graphite"@en ;
    skos:scopeNote "The material is used in the form of powder, sticks, or in pencils."@en .

<http://rdaregistry.info/termList/RDAMaterial/1015>
    rdakit:toolkitDefinition "A material consisting of any firm, dense, rigid board, often manufactured from fiber consolidated in a hot press."@en ;
    rdakit:toolkitLabel "hardboard"@en ;
    reg:identifier <http://metadataregistry.org/concepts/8469> ;
    reg:status <http://metadataregistry.org/uri/RegStatus/1001> ;
    a skos:Concept ;
    skos:altLabel "fibreboard"@en ;
    skos:definition "A material consisting of any firm, dense, rigid board, often manufactured from fiber consolidated in a hot press."@en ;
    skos:inScheme <http://rdaregistry.info/termList/RDAMaterial> ;
    skos:prefLabel "hardboard"@en .

<http://rdaregistry.info/termList/RDAMaterial/1016>
    rdakit:toolkitDefinition "A material consisting of laminated paper board that has paper layers glued to its surface."@en ;
    rdakit:toolkitLabel "illustration board"@en ;
    reg:identifier <http://metadataregistry.org/concepts/8470> ;
    reg:status <http://metadataregistry.org/uri/RegStatus/1001> ;
    a skos:Concept ;
    skos:definition "A material consisting of laminated paper board that has paper layers glued to its surface."@en ;
    skos:inScheme <http://rdaregistry.info/termList/RDAMaterial> ;
    skos:prefLabel "illustration board"@en .

<http://rdaregistry.info/termList/RDAMaterial/1017>
    rdakit:toolkitDefinition "A material consisting of pigment or dye contained in a liquid or paste."@en ;
    rdakit:toolkitLabel "ink"@en ;
    reg:identifier <http://metadataregistry.org/concepts/8471> ;
    reg:status <http://metadataregistry.org/uri/RegStatus/1001> ;
    a skos:Concept ;
    skos:definition "A material consisting of pigment or dye contained in a liquid or paste."@en ;
    skos:inScheme <http://rdaregistry.info/termList/RDAMaterial> ;
    skos:prefLabel "ink"@en .

<http://rdaregistry.info/termList/RDAMaterial/1018>
    rdakit:toolkitDefinition "A material consisting of the dentine forming the bulk of the teeth and tusks of animals such as elephants, walruses, and narwhals."@en ;
    rdakit:toolkitLabel "ivory"@en ;
    reg:identifier <http://metadataregistry.org/concepts/8472> ;
    reg:status <http://metadataregistry.org/uri/RegStatus/1001> ;
    a skos:Concept ;
    skos:definition "A material consisting of the dentine forming the bulk of the teeth and tusks of animals such as elephants, walruses, and narwhals."@en ;
    skos:inScheme <http://rdaregistry.info/termList/RDAMaterial> ;
    skos:prefLabel "ivory"@en .

<http://rdaregistry.info/termList/RDAMaterial/1019>
    rdakit:toolkitDefinition "A material generally used as a finish that may be clear or coloured, consisting of polymers or acrylic compounds dissolved in volatile organic compounds or other solvents, that when dry is a hard and durable material."@en ;
    rdakit:toolkitLabel "lacquer"@en ;
    reg:identifier <http://metadataregistry.org/concepts/8473> ;
    reg:status <http://metadataregistry.org/uri/RegStatus/1001> ;
    a skos:Concept ;
    skos:definition "A material generally used as a finish that may be clear or coloured, consisting of polymers or acrylic compounds dissolved in volatile organic compounds or other solvents, that when dry is a hard and durable material."@en ;
    skos:inScheme <http://rdaregistry.info/termList/RDAMaterial> ;
    skos:prefLabel "lacquer"@en .

<http://rdaregistry.info/termList/RDAMaterial/1020>
    rdakit:toolkitDefinition "A material consisting of the skin or hide of an animal that has been tanned to render it resistant to putrefaction and relatively soft and flexible when dry."@en ;
    rdakit:toolkitLabel "leather"@en ;
    reg:identifier <http://metadataregistry.org/concepts/8474> ;
    reg:status <http://metadataregistry.org/uri/RegStatus/1001> ;
    a skos:Concept ;
    skos:definition "A material consisting of the skin or hide of an animal that has been tanned to render it resistant to putrefaction and relatively soft and flexible when dry."@en ;
    skos:inScheme <http://rdaregistry.info/termList/RDAMaterial> ;
    skos:prefLabel "leather"@en ;
    skos:related <http://rdaregistry.info/termList/RDAMaterial/1035> .

<http://rdaregistry.info/termList/RDAMaterial/1021>
    rdakit:toolkitDefinition "A material that is a natural or synthetic inorganic compound consisting of particles that are highly magnetic and are commonly used to store binary or analog information."@en ;
    rdakit:toolkitLabel "magnetic particles"@en ;
    reg:identifier <http://metadataregistry.org/concepts/8475> ;
    reg:status <http://metadataregistry.org/uri/RegStatus/1001> ;
    a skos:Concept ;
    skos:definition "A material that is a natural or synthetic inorganic compound consisting of particles that are highly magnetic and are commonly used to store binary or analog information."@en ;
    skos:inScheme <http://rdaregistry.info/termList/RDAMaterial> ;
    skos:prefLabel "magnetic particles"@en .

<http://rdaregistry.info/termList/RDAMaterial/1022>
    rdakit:toolkitDefinition "A material consisting of a substance typified by being a good conductor of electricity and heat, opaque with a characteristic lustre, fusible, and usually malleable or ductile."@en ;
    rdakit:toolkitLabel "metal"@en ;
    reg:identifier <http://metadataregistry.org/concepts/8476> ;
    reg:status <http://metadataregistry.org/uri/RegStatus/1001> ;
    a skos:Concept ;
    skos:definition "A material consisting of a substance typified by being a good conductor of electricity and heat, opaque with a characteristic lustre, fusible, and usually malleable or ductile."@en ;
    skos:inScheme <http://rdaregistry.info/termList/RDAMaterial> ;
    skos:prefLabel "metal"@en .

<http://rdaregistry.info/termList/RDAMaterial/1023>
    rdakit:toolkitDefinition "A material of cellulose nitrate plasticized with camphor."@en ;
    rdakit:toolkitLabel "nitrate"@en ;
    reg:identifier <http://metadataregistry.org/concepts/8477> ;
    reg:status <http://metadataregistry.org/uri/RegStatus/1001> ;
    a skos:Concept ;
    skos:altLabel "celluloid"@en ;
    skos:definition "A material of cellulose nitrate plasticized with camphor."@en ;
    skos:inScheme <http://rdaregistry.info/termList/RDAMaterial> ;
    skos:prefLabel "nitrate"@en ;
    skos:related <http://rdaregistry.info/termList/RDAMaterial/1029>, <http://rdaregistry.info/termList/RDAMaterial/1033> .

<http://rdaregistry.info/termList/RDAMaterial/1024>
    rdakit:toolkitDefinition "A material consisting of pigment suspended in a drying oil."@en ;
    rdakit:toolkitLabel "oil paint"@en ;
    reg:identifier <http://metadataregistry.org/concepts/8478> ;
    reg:status <http://metadataregistry.org/uri/RegStatus/1001> ;
    a skos:Concept ;
    skos:definition "A material consisting of pigment suspended in a drying oil."@en ;
    skos:inScheme <http://rdaregistry.info/termList/RDAMaterial> ;
    skos:prefLabel "oil paint"@en .

<http://rdaregistry.info/termList/RDAMaterial/1025>
    rdakit:toolkitDefinition "A material consisting of thin material made from felted sheets or webs of animal, plant, mineral, or synthetic fibres formed and dried from a suspension in water."@en ;
    rdakit:toolkitLabel "paper"@en ;
    reg:identifier <http://metadataregistry.org/concepts/8479> ;
    reg:status <http://metadataregistry.org/uri/RegStatus/1001> ;
    a skos:Concept ;
    skos:definition "A material consisting of thin material made from felted sheets or webs of animal, plant, mineral, or synthetic fibres formed and dried from a suspension in water."@en ;
    skos:inScheme <http://rdaregistry.info/termList/RDAMaterial> ;
    skos:prefLabel "paper"@en .

<http://rdaregistry.info/termList/RDAMaterial/1026>
    rdakit:toolkitDefinition "A material consisting of calf, sheep, or goat skin which has been prepared to produce a thin, strong, translucent or opaque substance for writing, bookbinding, or other uses."@en ;
    rdakit:toolkitLabel "parchment"@en ;
    reg:identifier <http://metadataregistry.org/concepts/8480> ;
    reg:status <http://metadataregistry.org/uri/RegStatus/1001> ;
    a skos:Concept ;
    skos:definition "A material consisting of calf, sheep, or goat skin which has been prepared to produce a thin, strong, translucent or opaque substance for writing, bookbinding, or other uses."@en ;
    skos:inScheme <http://rdaregistry.info/termList/RDAMaterial> ;
    skos:prefLabel "parchment"@en ;
    skos:related <http://rdaregistry.info/termList/RDAMaterial/1035>, <http://rdaregistry.info/termList/RDAMaterial/1041> .

<http://rdaregistry.info/termList/RDAMaterial/1027>
    rdakit:toolkitDefinition "A material consisting of pigment mixed with a binder, usually in the form of a stick."@en ;
    rdakit:toolkitLabel "pastel"@en ;
    reg:identifier <http://metadataregistry.org/concepts/8481> ;
    reg:status <http://metadataregistry.org/uri/RegStatus/1001> ;
    a skos:Concept ;
    skos:definition "A material consisting of pigment mixed with a binder, usually in the form of a stick."@en ;
    skos:inScheme <http://rdaregistry.info/termList/RDAMaterial> ;
    skos:prefLabel "pastel"@en .

<http://rdaregistry.info/termList/RDAMaterial/1028>
    rdakit:toolkitDefinition "A material consisting of a powder prepared from calcium sulphate dihydrate, known as gypsum, or calcium carbonate and mixed with water and sometimes a filler to form a paste that liberates heat and then hardens."@en ;
    rdakit:toolkitLabel "plaster"@en ;
    reg:identifier <http://metadataregistry.org/concepts/8482> ;
    reg:status <http://metadataregistry.org/uri/RegStatus/1001> ;
    a skos:Concept ;
    skos:definition "A material consisting of a powder prepared from calcium sulphate dihydrate, known as gypsum, or calcium carbonate and mixed with water and sometimes a filler to form a paste that liberates heat and then hardens."@en ;
    skos:inScheme <http://rdaregistry.info/termList/RDAMaterial> ;
    skos:prefLabel "plaster"@en .

<http://rdaregistry.info/termList/RDAMaterial/1029>
    rdakit:toolkitDefinition "A material consisting of synthetic or semi-synthetic organic polymers of high molecular weight that are moldable."@en ;
    rdakit:toolkitLabel "plastic"@en ;
    reg:identifier <http://metadataregistry.org/concepts/8483> ;
    reg:status <http://metadataregistry.org/uri/RegStatus/1001> ;
    a skos:Concept ;
    skos:definition "A material consisting of synthetic or semi-synthetic organic polymers of high molecular weight that are moldable."@en ;
    skos:inScheme <http://rdaregistry.info/termList/RDAMaterial> ;
    skos:prefLabel "plastic"@en ;
    skos:related <http://rdaregistry.info/termList/RDAMaterial/1001>, <http://rdaregistry.info/termList/RDAMaterial/1010>, <http://rdaregistry.info/termList/RDAMaterial/1023>, <http://rdaregistry.info/termList/RDAMaterial/1030>, <http://rdaregistry.info/termList/RDAMaterial/1040> .

<http://rdaregistry.info/termList/RDAMaterial/1030>
    rdakit:toolkitDefinition "A material that is a category of polymers that contain the ester functional group in their main chain."@en ;
    rdakit:toolkitLabel "polyester"@en ;
    reg:identifier <http://metadataregistry.org/concepts/8484> ;
    reg:status <http://metadataregistry.org/uri/RegStatus/1001> ;
    a skos:Concept ;
    skos:definition "A material that is a category of polymers that contain the ester functional group in their main chain."@en ;
    skos:inScheme <http://rdaregistry.info/termList/RDAMaterial> ;
    skos:prefLabel "polyester"@en ;
    skos:related <http://rdaregistry.info/termList/RDAMaterial/1029>, <http://rdaregistry.info/termList/RDAMaterial/1033>, <http://rdaregistry.info/termList/RDAMaterial/1040> .

<http://rdaregistry.info/termList/RDAMaterial/1031>
    rdakit:toolkitDefinition "A material consisting of a refractory white clay, known as kaolin, and a feldspathic rock that is heated to form a ceramic material."@en ;
    rdakit:toolkitLabel "porcelain"@en ;
    reg:identifier <http://metadataregistry.org/concepts/8485> ;
    reg:status <http://metadataregistry.org/uri/RegStatus/1001> ;
    a skos:Concept ;
    skos:definition "A material consisting of a refractory white clay, known as kaolin, and a feldspathic rock that is heated to form a ceramic material."@en ;
    skos:inScheme <http://rdaregistry.info/termList/RDAMaterial> ;
    skos:prefLabel "porcelain"@en .

<http://rdaregistry.info/termList/RDAMaterial/1032>
    rdakit:toolkitDefinition "A material consisting of natural or synthetic polymers that have a high degree of resilience and elasticity."@en ;
    rdakit:toolkitLabel "rubber"@en ;
    reg:identifier <http://metadataregistry.org/concepts/8486> ;
    reg:status <http://metadataregistry.org/uri/RegStatus/1001> ;
    a skos:Concept ;
    skos:definition "A material consisting of natural or synthetic polymers that have a high degree of resilience and elasticity."@en ;
    skos:inScheme <http://rdaregistry.info/termList/RDAMaterial> ;
    skos:prefLabel "rubber"@en .

<http://rdaregistry.info/termList/RDAMaterial/1033>
    rdakit:toolkitDefinition "A material consisting of nonflammable cellulose acetate or polyester."@en ;
    rdakit:toolkitLabel "safety base"@en ;
    reg:identifier <http://metadataregistry.org/concepts/8487> ;
    reg:status <http://metadataregistry.org/uri/RegStatus/1001> ;
    a skos:Concept ;
    skos:definition "A material consisting of nonflammable cellulose acetate or polyester."@en ;
    skos:inScheme <http://rdaregistry.info/termList/RDAMaterial> ;
    skos:prefLabel "safety base"@en ;
    skos:related <http://rdaregistry.info/termList/RDAMaterial/1010>, <http://rdaregistry.info/termList/RDAMaterial/1023>, <http://rdaregistry.info/termList/RDAMaterial/1030>, <http://rdaregistry.info/termList/RDAMaterial/1040> .

<http://rdaregistry.info/termList/RDAMaterial/1034>
    rdakit:toolkitDefinition "A material consisting of lac, a resinous substance excreted by the female lac insect, that can be dissolved in ethyl alcohol to form a liquid that can be applied with a brush."@en ;
    rdakit:toolkitLabel "shellac"@en ;
    reg:identifier <http://metadataregistry.org/concepts/8488> ;
    reg:status <http://metadataregistry.org/uri/RegStatus/1001> ;
    a skos:Concept ;
    skos:definition "A material consisting of lac, a resinous substance excreted by the female lac insect, that can be dissolved in ethyl alcohol to form a liquid that can be applied with a brush."@en ;
    skos:inScheme <http://rdaregistry.info/termList/RDAMaterial> ;
    skos:prefLabel "shellac"@en .

<http://rdaregistry.info/termList/RDAMaterial/1035>
    rdakit:toolkitDefinition "A material consisting of the integument of animals, such as sheep, goats, or calves, separated from the body and variously processed to remove hair, dry, tan, or otherwise dress."@en ;
    rdakit:toolkitLabel "skin"@en ;
    reg:identifier <http://metadataregistry.org/concepts/8489> ;
    reg:status <http://metadataregistry.org/uri/RegStatus/1001> ;
    a skos:Concept ;
    skos:definition "A material consisting of the integument of animals, such as sheep, goats, or calves, separated from the body and variously processed to remove hair, dry, tan, or otherwise dress."@en ;
    skos:inScheme <http://rdaregistry.info/termList/RDAMaterial> ;
    skos:prefLabel "skin"@en ;
    skos:related <http://rdaregistry.info/termList/RDAMaterial/1020>, <http://rdaregistry.info/termList/RDAMaterial/1026> .

<http://rdaregistry.info/termList/RDAMaterial/1036>
    rdakit:toolkitDefinition "A material consisting of rock in its naturally occurring shape or that has been cut, shaped, crushed, or otherwise formed."@en ;
    rdakit:toolkitLabel "stone"@en ;
    reg:identifier <http://metadataregistry.org/concepts/8490> ;
    reg:status <http://metadataregistry.org/uri/RegStatus/1001> ;
    a skos:Concept ;
    skos:definition "A material consisting of rock in its naturally occurring shape or that has been cut, shaped, crushed, or otherwise formed."@en ;
    skos:inScheme <http://rdaregistry.info/termList/RDAMaterial> ;
    skos:prefLabel "stone"@en .

<http://rdaregistry.info/termList/RDAMaterial/1037>
    rdakit:toolkitDefinition "A material created by processing man-made materials, usually as a substitute for a natural material."@en ;
    rdakit:toolkitLabel "synthetic"@en ;
    reg:identifier <http://metadataregistry.org/concepts/8491> ;
    reg:status <http://metadataregistry.org/uri/RegStatus/1001> ;
    a skos:Concept ;
    skos:definition "A material created by processing man-made materials, usually as a substitute for a natural material."@en ;
    skos:inScheme <http://rdaregistry.info/termList/RDAMaterial> ;
    skos:prefLabel "synthetic"@en .

<http://rdaregistry.info/termList/RDAMaterial/1038>
    rdakit:toolkitDefinition "A material consisting of pigment mixed with a water-soluble binder medium, usually a glutinous material such as egg yolk or some other size, to form a permanent fast-drying painting medium."@en ;
    rdakit:toolkitLabel "tempera"@en ;
    reg:identifier <http://metadataregistry.org/concepts/8492> ;
    reg:status <http://metadataregistry.org/uri/RegStatus/1001> ;
    a skos:Concept ;
    skos:definition "A material consisting of pigment mixed with a water-soluble binder medium, usually a glutinous material such as egg yolk or some other size, to form a permanent fast-drying painting medium."@en ;
    skos:inScheme <http://rdaregistry.info/termList/RDAMaterial> ;
    skos:prefLabel "tempera"@en .

<http://rdaregistry.info/termList/RDAMaterial/1039>
    rdakit:toolkitDefinition "A material produced by weaving, felting, knotting, twining, or otherwise processing natural or synthetic fibers so that they cohere."@en ;
    rdakit:toolkitLabel "textile"@en ;
    reg:identifier <http://metadataregistry.org/concepts/8493> ;
    reg:status <http://metadataregistry.org/uri/RegStatus/1001> ;
    a skos:Concept ;
    skos:definition "A material produced by weaving, felting, knotting, twining, or otherwise processing natural or synthetic fibers so that they cohere."@en ;
    skos:inScheme <http://rdaregistry.info/termList/RDAMaterial> ;
    skos:prefLabel "textile"@en ;
    skos:scopeNote "Excludes fibreboard, paper, papier-mâché, and papyrus."@en .

<http://rdaregistry.info/termList/RDAMaterial/1040>
    rdakit:toolkitDefinition "A material manufactured from cellulose and a source of acetate esters, typically acetic anhydride."@en ;
    rdakit:toolkitLabel "triacetate"@en ;
    reg:identifier <http://metadataregistry.org/concepts/8494> ;
    reg:status <http://metadataregistry.org/uri/RegStatus/1001> ;
    a skos:Concept ;
    skos:altLabel "cellulose triacetate"@en ;
    skos:definition "A material manufactured from cellulose and a source of acetate esters, typically acetic anhydride."@en ;
    skos:inScheme <http://rdaregistry.info/termList/RDAMaterial> ;
    skos:prefLabel "triacetate"@en ;
    skos:related <http://rdaregistry.info/termList/RDAMaterial/1001>, <http://rdaregistry.info/termList/RDAMaterial/1010>, <http://rdaregistry.info/termList/RDAMaterial/1029>, <http://rdaregistry.info/termList/RDAMaterial/1030>, <http://rdaregistry.info/termList/RDAMaterial/1033> .

<http://rdaregistry.info/termList/RDAMaterial/1041>
    rdakit:toolkitDefinition "A material consisting of fine-quality calf or lamb parchment."@en ;
    rdakit:toolkitLabel "vellum"@en ;
    reg:identifier <http://metadataregistry.org/concepts/8495> ;
    reg:status <http://metadataregistry.org/uri/RegStatus/1001> ;
    a skos:Concept ;
    skos:definition "A material consisting of fine-quality calf or lamb parchment."@en ;
    skos:inScheme <http://rdaregistry.info/termList/RDAMaterial> ;
    skos:prefLabel "vellum"@en ;
    skos:related <http://rdaregistry.info/termList/RDAMaterial/1026> .

<http://rdaregistry.info/termList/RDAMaterial/1042>
    rdakit:toolkitDefinition "A material consisting of a polymer or copolymer derived from a vinyl group, typically vinyl chloride."@en ;
    rdakit:toolkitLabel "vinyl"@en ;
    reg:identifier <http://metadataregistry.org/concepts/8496> ;
    reg:status <http://metadataregistry.org/uri/RegStatus/1001> ;
    a skos:Concept ;
    skos:definition "A material consisting of a polymer or copolymer derived from a vinyl group, typically vinyl chloride."@en ;
    skos:inScheme <http://rdaregistry.info/termList/RDAMaterial> ;
    skos:prefLabel "vinyl"@en .

<http://rdaregistry.info/termList/RDAMaterial/1043>
    rdakit:toolkitDefinition "A material consisting of pigment suspended in water to form a transparent painting medium."@en ;
    rdakit:toolkitLabel "watercolour"@en ;
    reg:identifier <http://metadataregistry.org/concepts/8497> ;
    reg:status <http://metadataregistry.org/uri/RegStatus/1001> ;
    a skos:Concept ;
    skos:altLabel "watercolor"@en ;
    skos:definition "A material consisting of pigment suspended in water to form a transparent painting medium."@en ;
    skos:inScheme <http://rdaregistry.info/termList/RDAMaterial> ;
    skos:prefLabel "watercolour"@en .

<http://rdaregistry.info/termList/RDAMaterial/1044>
    rdakit:toolkitDefinition "A material consisting of a chemical compound from an animal, plant, mineral, or synthetic source that is malleable near ambient temperatures, slightly greasy to the touch, with a low melting point, and usually translucent, water-repellant, and soluble in organic solvents."@en ;
    rdakit:toolkitLabel "wax"@en ;
    reg:identifier <http://metadataregistry.org/concepts/8498> ;
    reg:status <http://metadataregistry.org/uri/RegStatus/1001> ;
    a skos:Concept ;
    skos:definition "A material consisting of a chemical compound from an animal, plant, mineral, or synthetic source that is malleable near ambient temperatures, slightly greasy to the touch, with a low melting point, and usually translucent, water-repellant, and soluble in organic solvents."@en ;
    skos:inScheme <http://rdaregistry.info/termList/RDAMaterial> ;
    skos:prefLabel "wax"@en .

<http://rdaregistry.info/termList/RDAMaterial/1045>
    rdakit:toolkitDefinition "A material consisting of the principal tissue of trees and similar plants."@en ;
    rdakit:toolkitLabel "wood"@en ;
    reg:identifier <http://metadataregistry.org/concepts/8499> ;
    reg:status <http://metadataregistry.org/uri/RegStatus/1001> ;
    a skos:Concept ;
    skos:definition "A material consisting of the principal tissue of trees and similar plants."@en ;
    skos:inScheme <http://rdaregistry.info/termList/RDAMaterial> ;
    skos:prefLabel "wood"@en .

<http://rdaregistry.info/termList/RDAMaterial/1046>
    rdakit:toolkitDefinition "A material consisting of an emulsion of one or more light-sensitive layers of diazonium salts in a polyester or acetate base that react with dye couplers when processed to produce azo dye images."@en ;
    rdakit:toolkitLabel "diazo emulsion"@en ;
    reg:identifier <http://metadataregistry.org/concepts/8500> ;
    reg:status <http://metadataregistry.org/uri/RegStatus/1001> ;
    a skos:Concept ;
    skos:definition "A material consisting of an emulsion of one or more light-sensitive layers of diazonium salts in a polyester or acetate base that react with dye couplers when processed to produce azo dye images."@en ;
    skos:inScheme <http://rdaregistry.info/termList/RDAMaterial> ;
    skos:prefLabel "diazo emulsion"@en ;
    skos:scopeNote "A material usually applied to the base material of a microfilm or microfiche."@en .

<http://rdaregistry.info/termList/RDAMaterial/1047>
    rdakit:toolkitDefinition "A material consisting of an emulsion of a light-sensitive compound of silver and chlorine, bromine, iodine or fluorine suspended in a colloidal medium, usually gelatin."@en ;
    rdakit:toolkitLabel "silver halide emulsion"@en ;
    reg:identifier <http://metadataregistry.org/concepts/8501> ;
    reg:status <http://metadataregistry.org/uri/RegStatus/1001> ;
    a skos:Concept ;
    skos:definition "A material consisting of an emulsion of a light-sensitive compound of silver and chlorine, bromine, iodine or fluorine suspended in a colloidal medium, usually gelatin."@en ;
    skos:inScheme <http://rdaregistry.info/termList/RDAMaterial> ;
    skos:prefLabel "silver halide emulsion"@en ;
    skos:scopeNote "A material usually applied to the base material of a microfilm or microfiche."@en .

<http://rdaregistry.info/termList/RDAMaterial/1048>
    rdakit:toolkitDefinition "A material consisting of an emulsion of one or more light-sensitive layers of diazonium salts in a polyester thermoplastic base that decompose on exposure to produce nitrogen bubbles, known as vesicles, that form a latent image, commonly blue or beige, which becomes visible and fixed when heated and allowed to cool."@en ;
    rdakit:toolkitLabel "vesicular emulsion"@en ;
    reg:identifier <http://metadataregistry.org/concepts/8502> ;
    reg:status <http://metadataregistry.org/uri/RegStatus/1001> ;
    a skos:Concept ;
    skos:definition "A material consisting of an emulsion of one or more light-sensitive layers of diazonium salts in a polyester thermoplastic base that decompose on exposure to produce nitrogen bubbles, known as vesicles, that form a latent image, commonly blue or beige, which becomes visible and fixed when heated and allowed to cool."@en ;
    skos:inScheme <http://rdaregistry.info/termList/RDAMaterial> ;
    skos:prefLabel "vesicular emulsion"@en ;
    skos:scopeNote "A material usually applied to the base material of a microfilm or microfiche."@en .

