@prefix rdf: <http://www.w3.org/1999/02/22-rdf-syntax-ns#> .
@prefix dc: <http://purl.org/dc/elements/1.1/> .
@prefix rdakit: <http://metadataregistry.org/uri/profile/rdakit/> .
@prefix reg: <http://metadataregistry.org/uri/profile/regap/> .
@prefix skos: <http://www.w3.org/2004/02/skos/core#> .

<http://metadataregistry.org/uri/RegStatus/1001>
    a skos:Concept ;
    skos:prefLabel "Published"@en .

<http://rdaregistry.info/termList/RDATasks>
    dc:title "RDA User Tasks" ;
    a skos:ConceptScheme .

<http://rdaregistry.info/termList/RDATasks/1001>
    rdakit:toolkitDefinition "A user task that is to bring together information about one or more RDA entities of interest by searching on any relevant criteria."@en ;
    rdakit:toolkitLabel "find"@en ;
    reg:identifier <http://metadataregistry.org/concepts/9780> ;
    reg:status <http://metadataregistry.org/uri/RegStatus/1001> ;
    a skos:Concept ;
    skos:definition "A user task that is to bring together information about one or more RDA entities of interest by searching on any relevant criteria."@en ;
    skos:inScheme <http://rdaregistry.info/termList/RDATasks> ;
    skos:notation "1001"@en ;
    skos:prefLabel "find"@en .

<http://rdaregistry.info/termList/RDATasks/1002>
    rdakit:toolkitDefinition "A user task that is to clearly understand the nature of RDA entities found by searching and to distinguish between similar entities."@en ;
    rdakit:toolkitLabel "identify"@en ;
    reg:identifier <http://metadataregistry.org/concepts/9781> ;
    reg:status <http://metadataregistry.org/uri/RegStatus/1001> ;
    a skos:Concept ;
    skos:definition "A user task that is to clearly understand the nature of RDA entities found by searching and to distinguish between similar entities."@en ;
    skos:inScheme <http://rdaregistry.info/termList/RDATasks> ;
    skos:notation "1002"@en ;
    skos:prefLabel "identify"@en .

<http://rdaregistry.info/termList/RDATasks/1003>
    rdakit:toolkitDefinition "A user task that is to determine the suitability of RDA entities found by searching, and to be enabled to either accept or reject specific entities."@en ;
    rdakit:toolkitLabel "select"@en ;
    reg:identifier <http://metadataregistry.org/concepts/9782> ;
    reg:status <http://metadataregistry.org/uri/RegStatus/1001> ;
    a skos:Concept ;
    skos:definition "A user task that is to determine the suitability of RDA entities found by searching, and to be enabled to either accept or reject specific entities."@en ;
    skos:inScheme <http://rdaregistry.info/termList/RDATasks> ;
    skos:notation "1003"@en ;
    skos:prefLabel "select"@en .

<http://rdaregistry.info/termList/RDATasks/1004>
    rdakit:toolkitDefinition "A user task that is to access the content of an RDA manifestation."@en ;
    rdakit:toolkitLabel "obtain"@en ;
    reg:identifier <http://metadataregistry.org/concepts/9783> ;
    reg:status <http://metadataregistry.org/uri/RegStatus/1001> ;
    a skos:Concept ;
    skos:definition "A user task that is to access the content of an RDA manifestation."@en ;
    skos:inScheme <http://rdaregistry.info/termList/RDATasks> ;
    skos:notation "1004"@en ;
    skos:prefLabel "obtain"@en .

<http://rdaregistry.info/termList/RDATasks/1005>
    rdakit:toolkitDefinition "A user task that is to discover RDA entities using the relationships between them and thus place the entities in a context."@en ;
    rdakit:toolkitLabel "explore"@en ;
    reg:identifier <http://metadataregistry.org/concepts/9784> ;
    reg:status <http://metadataregistry.org/uri/RegStatus/1001> ;
    a skos:Concept ;
    skos:definition "A user task that is to discover RDA entities using the relationships between them and thus place the entities in a context."@en ;
    skos:inScheme <http://rdaregistry.info/termList/RDATasks> ;
    skos:notation "1005"@en ;
    skos:prefLabel "explore"@en .

