@prefix rdf: <http://www.w3.org/1999/02/22-rdf-syntax-ns#> .
@prefix dc: <http://purl.org/dc/elements/1.1/> .
@prefix rdakit: <http://metadataregistry.org/uri/profile/rdakit/> .
@prefix reg: <http://metadataregistry.org/uri/profile/regap/> .
@prefix skos: <http://www.w3.org/2004/02/skos/core#> .

<http://metadataregistry.org/uri/RegStatus/1001>
    a skos:Concept ;
    skos:prefLabel "Published"@en .

<http://rdaregistry.info/termList/scale>
    dc:title "RDA Scale Designation" ;
    a skos:ConceptScheme .

<http://rdaregistry.info/termList/scale/1001>
    rdakit:toolkitDefinition "A scale designation for a resource consisting of more than one image, map, etc., with different scales."@en ;
    rdakit:toolkitLabel "scales differ"@en ;
    reg:identifier <http://metadataregistry.org/concepts/1141> ;
    reg:status <http://metadataregistry.org/uri/RegStatus/1001> ;
    a skos:Concept ;
    skos:definition "A scale designation for a resource consisting of more than one image, map, etc., with different scales."@en ;
    skos:inScheme <http://rdaregistry.info/termList/scale> ;
    skos:prefLabel "scales differ"@en .

<http://rdaregistry.info/termList/scale/1002>
    rdakit:toolkitDefinition "A scale designation for a resource when no scale can be determined."@en ;
    rdakit:toolkitLabel "scale not given"@en ;
    reg:identifier <http://metadataregistry.org/concepts/1142> ;
    reg:status <http://metadataregistry.org/uri/RegStatus/1001> ;
    a skos:Concept ;
    skos:definition "A scale designation for a resource when no scale can be determined."@en ;
    skos:inScheme <http://rdaregistry.info/termList/scale> ;
    skos:prefLabel "scale not given"@en .

<http://rdaregistry.info/termList/scale/1003>
    rdakit:toolkitDefinition "A scale designation for a resource whose scale is variable across the resource, when the range of values cannot be determined."@en ;
    rdakit:toolkitLabel "scale varies"@en ;
    reg:identifier <http://metadataregistry.org/concepts/1143> ;
    reg:status <http://metadataregistry.org/uri/RegStatus/1001> ;
    a skos:Concept ;
    skos:definition "A scale designation for a resource whose scale is variable across the resource, when the range of values cannot be determined."@en ;
    skos:inScheme <http://rdaregistry.info/termList/scale> ;
    skos:prefLabel "scale varies"@en .

<http://rdaregistry.info/termList/scale/1004>
    rdakit:toolkitDefinition "A scale designation for a still image or three-dimensional form that is not to scale."@en ;
    rdakit:toolkitLabel "not drawn to scale"@en ;
    reg:identifier <http://metadataregistry.org/concepts/3392> ;
    reg:status <http://metadataregistry.org/uri/RegStatus/1001> ;
    a skos:Concept ;
    skos:definition "A scale designation for a still image or three-dimensional form that is not to scale."@en ;
    skos:inScheme <http://rdaregistry.info/termList/scale> ;
    skos:prefLabel "not drawn to scale"@en .

