@prefix rdf: <http://www.w3.org/1999/02/22-rdf-syntax-ns#> .
@prefix dc: <http://purl.org/dc/elements/1.1/> .
@prefix foaf: <http://xmlns.com/foaf/0.1/> .
@prefix rdakit: <http://metadataregistry.org/uri/profile/rdakit/> .
@prefix rdfs: <http://www.w3.org/2000/01/rdf-schema#> .
@prefix reg: <http://metadataregistry.org/uri/profile/regap/> .
@prefix skos: <http://www.w3.org/2004/02/skos/core#> .

<http://metadataregistry.org/uri/RegStatus/1001>
    a skos:Concept ;
    skos:prefLabel "Published"@en .

<http://metadataregistry.org/uri/RegStatus/1008>
    a skos:Concept ;
    skos:prefLabel "Deprecated"@en .

<http://rdaregistry.info/Elements/a/>
    dc:title "RDA Agent properties"@en ;
    skos:note "Properties derived from RDA elements and relationship designators with the domain of RDA Agent and its sub-classes Person, Family, and Corporate Body."@en ;
    foaf:homepage <http://www.rdaregistry.info/Elements/a/> .

<http://rdaregistry.info/Elements/a/P50001>
    rdakit:instructionNumber "18.5" ;
    rdakit:toolkitDefinition "A thesis provided by the praeses in an academic disputation that is defended or opposed by a candidate for a degree."@en, "Candidat à un diplôme universitaire qui défend ou réfute la thèse proposée par le praeses lors d’une soutenance de thèse."@fr ;
    rdakit:toolkitLabel "respondent of"@en, "répondant de"@fr ;
    reg:hasSubproperty <http://rdaregistry.info/Elements/a/datatype/P50001>, <http://rdaregistry.info/Elements/a/object/P50001> ;
    reg:hasUnconstrained <http://rdaregistry.info/Elements/u/P60001> ;
    reg:lexicalAlias <http://rdaregistry.info/Elements/a/respondentOf.en> ;
    reg:name "respondentOf"@en ;
    reg:status <http://metadataregistry.org/uri/RegStatus/1001> ;
    a rdf:Property ;
    rdfs:domain <http://rdaregistry.info/Elements/c/C10004> ;
    rdfs:isDefinedBy <http://rdaregistry.info/Elements/a/> ;
    rdfs:label "est le répondant de"@fr, "is respondent of"@en ;
    rdfs:subPropertyOf <http://rdaregistry.info/Elements/a/P50204> ;
    skos:definition "Met un candidat à un diplôme universitaire qui défend ou réfute la thèse proposée par le praeses lors d’une soutenance de thèse en relation avec l’œuvre."@fr, "Relates a candidate for a degree who defends or opposes a thesis provided by the praeses in an academic disputation to a work."@en .

<http://rdaregistry.info/Elements/a/P50002>
    rdakit:instructionNumber "18.5" ;
    rdakit:toolkitDefinition "A legal work of a higher court recording a decision of a lower court that appeals against a corporate body."@en, "Collectivité contre laquelle un appel a été formé."@fr ;
    rdakit:toolkitLabel "appellee corporate body of"@en, "collectivité intimée de"@fr ;
    reg:hasSubproperty <http://rdaregistry.info/Elements/a/datatype/P50002>, <http://rdaregistry.info/Elements/a/object/P50002> ;
    reg:hasUnconstrained <http://rdaregistry.info/Elements/u/P60601> ;
    reg:lexicalAlias <http://rdaregistry.info/Elements/a/appelleeCorporateBodyOf.en> ;
    reg:name "appelleeCorporateBodyOf"@en ;
    reg:status <http://metadataregistry.org/uri/RegStatus/1001> ;
    a rdf:Property ;
    rdfs:domain <http://rdaregistry.info/Elements/c/C10005> ;
    rdfs:isDefinedBy <http://rdaregistry.info/Elements/a/> ;
    rdfs:label "est la collectivité intimée de"@fr, "is appellee corporate body of"@en ;
    rdfs:subPropertyOf <http://rdaregistry.info/Elements/a/P50087> ;
    skos:definition "Met une collectivité contre laquelle un appel a été formé en relation avec l’œuvre."@fr, "Relates a corporate body against whom an appeal is taken on a decision of a lower court recorded in a legal work of a higher court to a work."@en .

<http://rdaregistry.info/Elements/a/P50003>
    rdakit:instructionNumber "18.5" ;
    rdakit:toolkitDefinition "An academic degree that is granted to a corporate body."@en, "Collectivité conférant un diplôme universitaire."@fr ;
    rdakit:toolkitLabel "degree granting institution of"@en, "institution conférant des diplômes universitaires de"@fr ;
    reg:hasSubproperty <http://rdaregistry.info/Elements/a/datatype/P50003>, <http://rdaregistry.info/Elements/a/object/P50003> ;
    reg:hasUnconstrained <http://rdaregistry.info/Elements/u/P60002> ;
    reg:lexicalAlias <http://rdaregistry.info/Elements/a/degreeGrantingInstitutionOf.en> ;
    reg:name "degreeGrantingInstitutionOf"@en ;
    reg:status <http://metadataregistry.org/uri/RegStatus/1001> ;
    a rdf:Property ;
    rdfs:domain <http://rdaregistry.info/Elements/c/C10005> ;
    rdfs:isDefinedBy <http://rdaregistry.info/Elements/a/> ;
    rdfs:label "est l’institution conférant des diplômes universitaires de"@fr, "is degree granting institution of"@en ;
    rdfs:subPropertyOf <http://rdaregistry.info/Elements/a/P50131> ;
    skos:definition "Met une collectivité conférant un diplôme universitaire en relation avec l’œuvre."@fr, "Relates a corporate body granting an academic degree to a work."@en .

<http://rdaregistry.info/Elements/a/P50004>
    rdakit:instructionNumber "18.5" ;
    rdakit:toolkitDefinition "An event, exhibit, conference, etc., which gave rise to a work that is hosted by a corporate body having little or no responsibility for the content of the work."@en, "Collectivité accueillant l’événement, l’exposition, le congrès, etc."@fr ;
    rdakit:toolkitLabel "host institution of"@en, "institution hôte de"@fr ;
    reg:hasSubproperty <http://rdaregistry.info/Elements/a/datatype/P50004>, <http://rdaregistry.info/Elements/a/object/P50004> ;
    reg:hasUnconstrained <http://rdaregistry.info/Elements/u/P60003> ;
    reg:lexicalAlias <http://rdaregistry.info/Elements/a/hostInstitutionOf.en> ;
    reg:name "hostInstitutionOf"@en ;
    reg:status <http://metadataregistry.org/uri/RegStatus/1001> ;
    a rdf:Property ;
    rdfs:domain <http://rdaregistry.info/Elements/c/C10005> ;
    rdfs:isDefinedBy <http://rdaregistry.info/Elements/a/> ;
    rdfs:label "est l’institution hôte de"@fr, "is host institution of"@en ;
    rdfs:subPropertyOf <http://rdaregistry.info/Elements/a/P50131> ;
    skos:definition "Met une collectivité accueillant l’événement, l’exposition, le congrès, etc. en relation avec l’œuvre."@fr, "Relates a corporate body hosting an event, exhibit, conference, etc., which gave rise to a work to a work."@en .

<http://rdaregistry.info/Elements/a/P50005>
    rdakit:instructionNumber "18.5" ;
    rdakit:toolkitDefinition "A work that includes the financial, technical, and organizational management of a production for stage, screen, sound recording, television, webcast, etc."@en, "Collectivité responsable de la gestion financière, technique et organisationnelle de la production d’un spectacle, d’un film, d’un enregistrement audio, d’une émission de télévision, d’une webémission, etc."@fr ;
    rdakit:toolkitLabel "production company of"@en, "société de production de"@fr ;
    reg:hasSubproperty <http://rdaregistry.info/Elements/a/datatype/P50005>, <http://rdaregistry.info/Elements/a/object/P50005> ;
    reg:hasUnconstrained <http://rdaregistry.info/Elements/u/P60004> ;
    reg:lexicalAlias <http://rdaregistry.info/Elements/a/productionCompanyOf.en> ;
    reg:name "productionCompanyOf"@en ;
    reg:status <http://metadataregistry.org/uri/RegStatus/1001> ;
    a rdf:Property ;
    rdfs:domain <http://rdaregistry.info/Elements/c/C10005> ;
    rdfs:isDefinedBy <http://rdaregistry.info/Elements/a/> ;
    rdfs:label "est la société de production de"@fr, "is production company of"@en ;
    rdfs:subPropertyOf <http://rdaregistry.info/Elements/a/P50131> ;
    skos:definition "Met une collectivité responsable de la gestion financière, technique et organisationnelle de la production d’un spectacle, d’un film, d’un enregistrement audio, d’une émission de télévision, d’une webémission, etc. en relation avec l’œuvre."@fr, "Relates a corporate body that is responsible for financial, technical, and organizational management of a production for stage, screen, sound recording, television, webcast, etc to a work."@en .

<http://rdaregistry.info/Elements/a/P50006>
    rdakit:instructionNumber "11.12" ;
    rdakit:toolkitDefinition "A character string uniquely associated with a corporate body, or with a surrogate such as an authority record for a corporate body."@en, "Chaîne de caractères associée de manière unique à une collectivité ou à un substitut d’une collectivité (par exemple, une notice d’autorité)."@fr, "Una cadena de caracteres singularmente asociada con una entidad corporativa, o con un substituto de una entidad corporativa (p.ej., un registro de autoridad)."@es ;
    rdakit:toolkitLabel "identifiant de la collectivité"@fr, "identificador de la entidad corporativa"@es, "identifier for the corporate body"@en, "identifikator för institutionen"@sv ;
    reg:hasSubproperty <http://rdaregistry.info/Elements/a/datatype/P50006> ;
    reg:hasUnconstrained <http://rdaregistry.info/Elements/u/P60053> ;
    reg:lexicalAlias <http://rdaregistry.info/Elements/a/identifierForTheCorporateBody.en> ;
    reg:name "identifierForTheCorporateBody"@en ;
    reg:status <http://metadataregistry.org/uri/RegStatus/1001> ;
    a rdf:Property ;
    rdfs:domain <http://rdaregistry.info/Elements/c/C10005> ;
    rdfs:isDefinedBy <http://rdaregistry.info/Elements/a/> ;
    rdfs:label "a pour identifiant de la collectivité"@fr, "har identifikator för institutionen"@sv, "has identifier for the corporate body"@en ;
    skos:definition "Met une collectivité en relation avec une chaîne de caractères associée de manière unique à une collectivité ou à un substitut d’une collectivité (par exemple, une notice d’autorité)."@fr, "Relates a corporate body to a character string uniquely associated with a corporate body, or with a surrogate such as an authority record for a corporate body."@en ;
    skos:scopeNote "L’identifiant sert à distinguer cette collectivité d’autres collectivités."@fr, "The identifier serves to differentiate a corporate body from other corporate bodies."@en .

<http://rdaregistry.info/Elements/a/P50007>
    rdakit:instructionNumber "29.5" ;
    rdakit:toolkitDefinition "A corporate body that founded another corporate body."@en, "Collectivité qui a fondé l’autre collectivité."@fr, "Una entidad corporativa que fundó a otra entidad corporativa."@es ;
    rdakit:toolkitLabel "collectivité fondatrice"@fr, "entidad corporativa fundadora"@es, "founding corporate body"@en ;
    reg:hasSubproperty <http://rdaregistry.info/Elements/a/datatype/P50007>, <http://rdaregistry.info/Elements/a/object/P50007> ;
    reg:hasUnconstrained <http://rdaregistry.info/Elements/u/P60694> ;
    reg:lexicalAlias <http://rdaregistry.info/Elements/a/foundingCorporateBody.en> ;
    reg:name "foundingCorporateBody"@en ;
    reg:status <http://metadataregistry.org/uri/RegStatus/1001> ;
    a rdf:Property ;
    rdfs:domain <http://rdaregistry.info/Elements/c/C10005> ;
    rdfs:isDefinedBy <http://rdaregistry.info/Elements/a/> ;
    rdfs:label "a pour collectivité fondatrice"@fr, "has founding corporate body"@en ;
    skos:definition "Met une collectivité en relation avec une collectivité qui a fondé l’autre collectivité."@fr, "Relates a corporate body to a corporate body that founded another corporate body."@en .

<http://rdaregistry.info/Elements/a/P50008>
    rdakit:instructionNumber "29.5" ;
    rdakit:toolkitDefinition "A corporate body that is hierarchically superior to another corporate body."@en, "Collectivité qui est hiérarchiquement supérieure à l’autre collectivité."@fr, "Una entidad corporativa que es jerárquicamente superior a otra entidad corporativa."@es ;
    rdakit:toolkitLabel "hierarchical superior"@en, "superior jerárquica"@es, "supérieur hiérarchique"@fr ;
    reg:hasSubproperty <http://rdaregistry.info/Elements/a/datatype/P50008>, <http://rdaregistry.info/Elements/a/object/P50008> ;
    reg:hasUnconstrained <http://rdaregistry.info/Elements/u/P60680> ;
    reg:lexicalAlias <http://rdaregistry.info/Elements/a/hierarchicalSuperior.en> ;
    reg:name "hierarchicalSuperior"@en ;
    reg:status <http://metadataregistry.org/uri/RegStatus/1001> ;
    a rdf:Property ;
    rdfs:domain <http://rdaregistry.info/Elements/c/C10005> ;
    rdfs:isDefinedBy <http://rdaregistry.info/Elements/a/> ;
    rdfs:label "a pour supérieur hiérarchique"@fr, "has hierarchical superior"@en ;
    skos:definition "Met une collectivité en relation avec une collectivité qui est hiérarchiquement supérieure à l’autre collectivité."@fr, "Relates a corporate body to a corporate body that is hierarchically superior to another corporate body."@en .

<http://rdaregistry.info/Elements/a/P50009>
    rdakit:instructionNumber "29.5" ;
    rdakit:toolkitDefinition "A corporate body that is sponsored by another corporate body."@en, "Collectivité commanditée par l’autre collectivité."@fr, "Una entidad corporativa que es patrocinada por otra entidad corporativa."@es ;
    rdakit:toolkitLabel "collectivité commanditée"@fr, "entidad corporativa patrocinada"@es, "sponsored corporate body of corporate body"@en ;
    reg:hasSubproperty <http://rdaregistry.info/Elements/a/datatype/P50009>, <http://rdaregistry.info/Elements/a/object/P50009> ;
    reg:hasUnconstrained <http://rdaregistry.info/Elements/u/P60688> ;
    reg:lexicalAlias <http://rdaregistry.info/Elements/a/sponsoredCorporateBodyOfCorporateBody.en> ;
    reg:name "sponsoredCorporateBodyOfCorporateBody"@en ;
    reg:status <http://metadataregistry.org/uri/RegStatus/1001> ;
    a rdf:Property ;
    rdfs:domain <http://rdaregistry.info/Elements/c/C10005> ;
    rdfs:isDefinedBy <http://rdaregistry.info/Elements/a/> ;
    rdfs:label "a pour collectivité commanditée"@fr, "has sponsored corporate body of corporate body"@en ;
    skos:definition "Met une collectivité en relation avec une collectivité commanditée par l’autre collectivité."@fr, "Relates a corporate body to a corporate body that is sponsored by another corporate body."@en .

<http://rdaregistry.info/Elements/a/P50010>
    rdakit:instructionNumber "29.5" ;
    rdakit:toolkitDefinition "A corporate body that is subordinate to another corporate body."@en, "Collectivité qui est subordonnée à l’autre collectivité."@fr, "Una entidad corporativa que es subordinada a otra entidad corporativa."@es ;
    rdakit:toolkitLabel "hierarchical subordinate"@en, "subordinada jerárquica"@es, "subordonné hiérarchique"@fr ;
    reg:hasSubproperty <http://rdaregistry.info/Elements/a/datatype/P50010>, <http://rdaregistry.info/Elements/a/object/P50010> ;
    reg:hasUnconstrained <http://rdaregistry.info/Elements/u/P60681> ;
    reg:lexicalAlias <http://rdaregistry.info/Elements/a/hierarchicalSubordinate.en> ;
    reg:name "hierarchicalSubordinate"@en ;
    reg:status <http://metadataregistry.org/uri/RegStatus/1001> ;
    a rdf:Property ;
    rdfs:domain <http://rdaregistry.info/Elements/c/C10005> ;
    rdfs:isDefinedBy <http://rdaregistry.info/Elements/a/> ;
    rdfs:label "a pour subordonné hiérarchique"@fr, "has hierarchical subordinate"@en ;
    skos:definition "Met une collectivité en relation avec une collectivité qui est subordonnée à l’autre collectivité."@fr, "Relates a corporate body to a corporate body that is subordinate to another corporate body."@en .

<http://rdaregistry.info/Elements/a/P50011>
    rdakit:instructionNumber "29.5" ;
    rdakit:toolkitDefinition "A corporate body that merged with another corporate body to form a third."@en, "Collectivité qui a fusionné avec l’autre collectivité pour en former une troisième."@fr, "Una entidad corporativa que se fusionó con otra entidad corporativa para formar una tercera."@es ;
    rdakit:toolkitLabel "collectivité fusionnée"@fr, "fusionada con"@es, "mergee"@en ;
    reg:hasSubproperty <http://rdaregistry.info/Elements/a/datatype/P50011>, <http://rdaregistry.info/Elements/a/object/P50011> ;
    reg:hasUnconstrained <http://rdaregistry.info/Elements/u/P60682> ;
    reg:lexicalAlias <http://rdaregistry.info/Elements/a/mergee.en> ;
    reg:name "mergee"@en ;
    reg:status <http://metadataregistry.org/uri/RegStatus/1001> ;
    a rdf:Property ;
    rdfs:domain <http://rdaregistry.info/Elements/c/C10005> ;
    rdfs:isDefinedBy <http://rdaregistry.info/Elements/a/> ;
    rdfs:label "a pour collectivité fusionnée"@fr, "has mergee"@en ;
    skos:definition "Met une collectivité en relation avec une collectivité qui a fusionné avec l’autre collectivité pour en former une troisième."@fr, "Relates a corporate body to a corporate body that merged with another corporate body to form a third."@en .

<http://rdaregistry.info/Elements/a/P50012>
    rdakit:instructionNumber "29.5" ;
    rdakit:toolkitDefinition "A corporate body that precedes another corporate body."@en, "Collectivité qui précède l’autre collectivité."@fr, "Una entidad corporativa que precede a otra entidad corporativa"@es ;
    rdakit:toolkitLabel "predecesora"@es, "predecessor"@en, "prédécesseur"@fr ;
    reg:hasSubproperty <http://rdaregistry.info/Elements/a/datatype/P50012>, <http://rdaregistry.info/Elements/a/object/P50012> ;
    reg:hasUnconstrained <http://rdaregistry.info/Elements/u/P60683> ;
    reg:lexicalAlias <http://rdaregistry.info/Elements/a/predecessor.en> ;
    reg:name "predecessor"@en ;
    reg:status <http://metadataregistry.org/uri/RegStatus/1001> ;
    a rdf:Property ;
    rdfs:domain <http://rdaregistry.info/Elements/c/C10005> ;
    rdfs:isDefinedBy <http://rdaregistry.info/Elements/a/> ;
    rdfs:label "a pour prédécesseur"@fr, "has predecessor"@en ;
    skos:definition "Met une collectivité en relation avec une collectivité qui précède l’autre collectivité."@fr, "Relates a corporate body to a corporate body that precedes another corporate body."@en .

<http://rdaregistry.info/Elements/a/P50013>
    rdakit:instructionNumber "29.5" ;
    rdakit:toolkitDefinition "A corporate body that resulted from a merger of two or more other corporate bodies."@en, "Collectivité résultant d’une fusion entre deux ou plusieurs autres collectivités."@fr, "Una entidad corporativa que resulta de la fusión de dos o más entidades corporativas."@es ;
    rdakit:toolkitLabel "product of merger"@en, "producto de fusión de"@es, "résultat de fusion"@fr ;
    reg:hasSubproperty <http://rdaregistry.info/Elements/a/datatype/P50013>, <http://rdaregistry.info/Elements/a/object/P50013> ;
    reg:hasUnconstrained <http://rdaregistry.info/Elements/u/P60684> ;
    reg:lexicalAlias <http://rdaregistry.info/Elements/a/productOfAMerger.en> ;
    reg:name "productOfAMerger"@en ;
    reg:status <http://metadataregistry.org/uri/RegStatus/1001> ;
    a rdf:Property ;
    rdfs:domain <http://rdaregistry.info/Elements/c/C10005> ;
    rdfs:isDefinedBy <http://rdaregistry.info/Elements/a/> ;
    rdfs:label "a pour résultat de fusion"@fr, "has product of merger"@en ;
    skos:definition "Met une collectivité en relation avec une collectivité résultant d’une fusion entre deux ou plusieurs autres collectivités."@fr, "Relates a corporate body to a corporate body that resulted from a merger of two or more other corporate bodies."@en .

<http://rdaregistry.info/Elements/a/P50014>
    rdakit:instructionNumber "29.5" ;
    rdakit:toolkitDefinition "A corporate body that resulted from a split or division of another corporate body."@en, "Collectivité résultant d’une scission ou division de l’autre collectivité."@fr, "Una entidad corporativa que resulta de la escisión o división de otra entidad corporativa."@es ;
    rdakit:toolkitLabel "product of split"@en, "producto de escisión de"@es, "résultat de scission"@fr ;
    reg:hasSubproperty <http://rdaregistry.info/Elements/a/datatype/P50014>, <http://rdaregistry.info/Elements/a/object/P50014> ;
    reg:hasUnconstrained <http://rdaregistry.info/Elements/u/P60685> ;
    reg:lexicalAlias <http://rdaregistry.info/Elements/a/productOfASplit.en> ;
    reg:name "productOfASplit"@en ;
    reg:status <http://metadataregistry.org/uri/RegStatus/1001> ;
    a rdf:Property ;
    rdfs:domain <http://rdaregistry.info/Elements/c/C10005> ;
    rdfs:isDefinedBy <http://rdaregistry.info/Elements/a/> ;
    rdfs:label "a pour résultat de scission"@fr, "has product of split"@en ;
    skos:definition "Met une collectivité en relation avec une collectivité résultant d’une scission ou division de l’autre collectivité."@fr, "Relates a corporate body to a corporate body that resulted from a split or division of another corporate body."@en .

<http://rdaregistry.info/Elements/a/P50015>
    rdakit:instructionNumber "29.5" ;
    rdakit:toolkitDefinition "A corporate body that sponsors another corporate body."@en, "Collectivité qui commandite l’autre collectivité."@fr, "Una entidad corporativa que patrocina a otra entidad corporativa."@es ;
    rdakit:toolkitLabel "collectivité commanditaire"@fr, "entidad corporativa patrocinadora"@es, "sponsoring corporate body"@en ;
    reg:hasSubproperty <http://rdaregistry.info/Elements/a/datatype/P50015>, <http://rdaregistry.info/Elements/a/object/P50015> ;
    reg:hasUnconstrained <http://rdaregistry.info/Elements/u/P60676> ;
    reg:lexicalAlias <http://rdaregistry.info/Elements/a/sponsoringCorporateBody.en> ;
    reg:name "sponsoringCorporateBody"@en ;
    reg:status <http://metadataregistry.org/uri/RegStatus/1001> ;
    a rdf:Property ;
    rdfs:domain <http://rdaregistry.info/Elements/c/C10005> ;
    rdfs:isDefinedBy <http://rdaregistry.info/Elements/a/> ;
    rdfs:label "a pour collectivité commanditaire"@fr, "has sponsoring corporate body"@en ;
    skos:definition "Met une collectivité en relation avec une collectivité qui commandite l’autre collectivité."@fr, "Relates a corporate body to a corporate body that sponsors another corporate body."@en .

<http://rdaregistry.info/Elements/a/P50016>
    rdakit:instructionNumber "29.5" ;
    rdakit:toolkitDefinition "A corporate body that succeeds or follows another corporate body."@en, "Collectivité qui succède ou fait suite à l’autre collectivité."@fr, "Una entidad corporativa que sucede o continúa a otra entidad corporativa."@es ;
    rdakit:toolkitLabel "successeur"@fr, "successor"@en, "sucesora"@es ;
    reg:hasSubproperty <http://rdaregistry.info/Elements/a/datatype/P50016>, <http://rdaregistry.info/Elements/a/object/P50016> ;
    reg:hasUnconstrained <http://rdaregistry.info/Elements/u/P60686> ;
    reg:lexicalAlias <http://rdaregistry.info/Elements/a/successor.en> ;
    reg:name "successor"@en ;
    reg:status <http://metadataregistry.org/uri/RegStatus/1001> ;
    a rdf:Property ;
    rdfs:domain <http://rdaregistry.info/Elements/c/C10005> ;
    rdfs:isDefinedBy <http://rdaregistry.info/Elements/a/> ;
    rdfs:label "a pour successeur"@fr, "has successor"@en ;
    skos:definition "Met une collectivité en relation avec une collectivité qui succède ou fait suite à l’autre collectivité."@fr, "Relates a corporate body to a corporate body that succeeds or follows another corporate body."@en .

<http://rdaregistry.info/Elements/a/P50017>
    rdakit:instructionNumber "29.5" ;
    rdakit:toolkitDefinition "A corporate body that another corporate body founded."@en, "Collectivité que l’autre collectivité a fondée."@fr, "Una entidad corporativa fundada por la otra entidad corporativa."@es ;
    rdakit:toolkitLabel "collectivité fondée de la collectivité"@fr, "entidad corporativa fundada"@es, "founded corporate body of corporate body"@en ;
    reg:hasSubproperty <http://rdaregistry.info/Elements/a/datatype/P50017>, <http://rdaregistry.info/Elements/a/object/P50017> ;
    reg:hasUnconstrained <http://rdaregistry.info/Elements/u/P60687> ;
    reg:lexicalAlias <http://rdaregistry.info/Elements/a/foundedCorporateBodyOfCorporateBody.en> ;
    reg:name "foundedCorporateBodyOfCorporateBody"@en ;
    reg:status <http://metadataregistry.org/uri/RegStatus/1001> ;
    a rdf:Property ;
    rdfs:domain <http://rdaregistry.info/Elements/c/C10005> ;
    rdfs:isDefinedBy <http://rdaregistry.info/Elements/a/> ;
    rdfs:label "a pour collectivité fondée de la collectivité"@fr, "has founded corporate body of corporate body"@en ;
    skos:definition "Met une collectivité en relation avec une collectivité que l’autre collectivité a fondée."@fr, "Relates a corporate body to a corporate body that another corporate body founded."@en .

<http://rdaregistry.info/Elements/a/P50018>
    reg:status <http://metadataregistry.org/uri/RegStatus/1008> ;
    a rdf:Property ;
    rdfs:isDefinedBy <http://rdaregistry.info/Elements/a/> .

<http://rdaregistry.info/Elements/a/P50019>
    rdakit:instructionNumber "11.6" ;
    rdakit:toolkitDefinition "A designation of the sequencing of a conference, etc., within a series of conferences, etc."@en, "Indication d’ordre séquentiel d’un congrès, etc. à l’intérieur d’une série de congrès, etc."@fr, "Una designación de la secuencia de una conferencia, etc., dentro de una serie de conferencias, etc."@es ;
    rdakit:toolkitLabel "number of a conference, etc."@en, "numéro d’ordre d’un congrès, etc."@fr, "número de una conferencia, etc."@es, "ordningsnummer för konferens etc."@sv ;
    reg:hasSubproperty <http://rdaregistry.info/Elements/a/datatype/P50019> ;
    reg:hasUnconstrained <http://rdaregistry.info/Elements/u/P60079> ;
    reg:lexicalAlias <http://rdaregistry.info/Elements/a/numberOfAConferenceEtc.en> ;
    reg:name "numberOfAConferenceEtc"@en ;
    reg:status <http://metadataregistry.org/uri/RegStatus/1001> ;
    a rdf:Property ;
    rdfs:domain <http://rdaregistry.info/Elements/c/C10005> ;
    rdfs:isDefinedBy <http://rdaregistry.info/Elements/a/> ;
    rdfs:label "a pour numéro d’ordre d’un congrès, etc."@fr, "har ordningsnummer för konferens etc."@sv, "has number of a conference, etc."@en ;
    skos:definition "Met une collectivité en relation avec une indication d’ordre séquentiel d’un congrès, etc. à l’intérieur d’une série de congrès, etc."@fr, "Relates a corporate body to a designation of the sequencing of a conference, etc., within a series of conferences, etc."@en .

<http://rdaregistry.info/Elements/a/P50020>
    rdakit:instructionNumber "29.5" ;
    rdakit:toolkitDefinition "A family that founded a corporate body."@en, "Famille qui a fondé la collectivité."@fr, "Una familia que fundó la entidad corporativa."@es ;
    rdakit:toolkitLabel "familia fundadora"@es, "famille fondatrice"@fr, "founding family"@en ;
    reg:hasSubproperty <http://rdaregistry.info/Elements/a/datatype/P50020>, <http://rdaregistry.info/Elements/a/object/P50020> ;
    reg:hasUnconstrained <http://rdaregistry.info/Elements/u/P60694> ;
    reg:lexicalAlias <http://rdaregistry.info/Elements/a/foundingFamily.en> ;
    reg:name "foundingFamily"@en ;
    reg:status <http://metadataregistry.org/uri/RegStatus/1001> ;
    a rdf:Property ;
    rdfs:domain <http://rdaregistry.info/Elements/c/C10005> ;
    rdfs:isDefinedBy <http://rdaregistry.info/Elements/a/> ;
    rdfs:label "a pour famille fondatrice"@fr, "has founding family"@en ;
    skos:definition "Met une collectivité en relation avec une famille qui a fondé la collectivité."@fr, "Relates a corporate body to a family that founded a corporate body."@en .

<http://rdaregistry.info/Elements/a/P50021>
    rdakit:instructionNumber "29.5" ;
    rdakit:toolkitDefinition "A family that sponsors a corporate body."@en, "Famille qui commandite la collectivité."@fr, "Una familia que patrocina la entidad corporativa."@es ;
    rdakit:toolkitLabel "familia patrocinadora"@es, "famille commanditaire"@fr, "sponsoring family"@en ;
    reg:hasSubproperty <http://rdaregistry.info/Elements/a/datatype/P50021>, <http://rdaregistry.info/Elements/a/object/P50021> ;
    reg:hasUnconstrained <http://rdaregistry.info/Elements/u/P60676> ;
    reg:lexicalAlias <http://rdaregistry.info/Elements/a/sponsoringFamily.en> ;
    reg:name "sponsoringFamily"@en ;
    reg:status <http://metadataregistry.org/uri/RegStatus/1001> ;
    a rdf:Property ;
    rdfs:domain <http://rdaregistry.info/Elements/c/C10005> ;
    rdfs:isDefinedBy <http://rdaregistry.info/Elements/a/> ;
    rdfs:label "a pour famille commanditaire"@fr, "has sponsoring family"@en ;
    skos:definition "Met une collectivité en relation avec une famille qui commandite la collectivité."@fr, "Relates a corporate body to a family that sponsors a corporate body."@en .

<http://rdaregistry.info/Elements/a/P50022>
    rdakit:instructionNumber "11.1" ;
    rdakit:toolkitDefinition "A field of business in which a corporate body is engaged or an area of competence, responsibility, jurisdiction, etc. of a corporate body."@en, "Champ d’activité dans lequel s’investit la collectivité, sa zone de compétence, de responsabilité, de juridiction, etc."@fr, "Un campo de negocios al que la entidad corporativa está dedicada y/o su área de competencia, responsabilidad, jurisdicción, etc."@es ;
    rdakit:toolkitLabel "campo de actividad de la entidad corporativa"@es, "domaine d’activité de la collectivité"@fr, "field of activity of the corporate body"@en ;
    reg:hasSubproperty <http://rdaregistry.info/Elements/a/datatype/P50022> ;
    reg:hasUnconstrained <http://rdaregistry.info/Elements/u/P60089> ;
    reg:lexicalAlias <http://rdaregistry.info/Elements/a/fieldOfActivityOfTheCorporateBody.en> ;
    reg:name "fieldOfActivityOfTheCorporateBody"@en ;
    reg:status <http://metadataregistry.org/uri/RegStatus/1001> ;
    a rdf:Property ;
    rdfs:domain <http://rdaregistry.info/Elements/c/C10005> ;
    rdfs:isDefinedBy <http://rdaregistry.info/Elements/a/> ;
    rdfs:label "a pour domaine d’activité de la collectivité"@fr, "has field of activity of the corporate body"@en ;
    skos:definition "Met une collectivité en relation avec un champ d’activité dans lequel s’investit la collectivité, sa zone de compétence, de responsabilité, de juridiction, etc."@fr, "Relates a corporate body to a field of business in which a corporate body is engaged or an area of competence, responsibility, jurisdiction, etc. of a corporate body."@en .

<http://rdaregistry.info/Elements/a/P50023>
    rdakit:instructionNumber "11.8" ;
    rdakit:toolkitDefinition "A language a corporate body uses in its communications."@en, "Langue que la collectivité utilise pour sa communication."@fr, "Lengua o lenguas que usa la entidad corporativa en sus comunicaciones"@es ;
    rdakit:toolkitLabel "language of the corporate body"@en, "langue de la collectivité"@fr, "lengua de la entidad corporativa"@es ;
    reg:hasSubproperty <http://rdaregistry.info/Elements/a/datatype/P50023> ;
    reg:hasUnconstrained <http://rdaregistry.info/Elements/u/P60098> ;
    reg:lexicalAlias <http://rdaregistry.info/Elements/a/languageOfTheCorporateBody.en> ;
    reg:name "languageOfTheCorporateBody"@en ;
    reg:status <http://metadataregistry.org/uri/RegStatus/1001> ;
    a rdf:Property ;
    rdfs:domain <http://rdaregistry.info/Elements/c/C10005> ;
    rdfs:isDefinedBy <http://rdaregistry.info/Elements/a/> ;
    rdfs:label "a pour langue de la collectivité"@fr, "has language of the corporate body"@en ;
    skos:definition "Met une collectivité en relation avec une langue que la collectivité utilise pour sa communication."@fr, "Relates a corporate body to a language a corporate body uses in its communications."@en .

<http://rdaregistry.info/Elements/a/P50024>
    rdakit:instructionNumber "11.3.2" ;
    rdakit:toolkitDefinition "A place or places in which a conference, congress, meeting, exhibition, fair, festival, etc., was held."@en, "Localité où un congrès, une conférence, une réunion, une exposition, une foire, un festival, etc. s’est tenu."@fr, "Una localidad en la que se se realizó una conferencia, congreso, reunión, exposición, feria, festival, etc."@es ;
    rdakit:toolkitLabel "konferensort"@sv, "lieu du congrès, etc."@fr, "location of conference, etc."@en, "lugar de la conferencia, etc."@es ;
    reg:hasSubproperty <http://rdaregistry.info/Elements/a/datatype/P50024> ;
    reg:hasUnconstrained <http://rdaregistry.info/Elements/u/P60107> ;
    reg:lexicalAlias <http://rdaregistry.info/Elements/a/locationOfConferenceEtc.en> ;
    reg:name "locationOfConferenceEtc"@en ;
    reg:status <http://metadataregistry.org/uri/RegStatus/1001> ;
    a rdf:Property ;
    rdfs:domain <http://rdaregistry.info/Elements/c/C10005> ;
    rdfs:isDefinedBy <http://rdaregistry.info/Elements/a/> ;
    rdfs:label "a pour lieu du congrès, etc."@fr, "har konferensort"@sv, "has location of conference, etc."@en ;
    rdfs:subPropertyOf <http://rdaregistry.info/Elements/a/P50031> ;
    skos:definition "Met une collectivité en relation avec une localité où un congrès, une conférence, une réunion, une exposition, une foire, un festival, etc. s’est tenu."@fr, "Relates a corporate body to a place or places in which a conference, congress, meeting, exhibition, fair, festival, etc., was held."@en .

<http://rdaregistry.info/Elements/a/P50025>
    rdakit:instructionNumber "11.2.3" ;
    rdakit:toolkitDefinition "A name or form of name by which a corporate body is known that differs from a name or form of name chosen as a preferred name."@en, "Nom ou forme de nom sous laquelle une collectivité est connue et qui diffère du nom ou de la forme de nom choisie comme nom privilégié."@fr, "Un nombre o una forma de un nombre mediante el cual se conoce a una entidad corporativa que difiere del nombre o la forma del nombre escogido como el nombre preferido."@es ;
    rdakit:toolkitLabel "variant name for the corporate body"@en, "variante de nom de la collectivité"@fr, "variante del nombre de la entidad corporativa"@es, "variantnamn för institutionen"@sv ;
    reg:hasSubproperty <http://rdaregistry.info/Elements/a/datatype/P50025> ;
    reg:hasUnconstrained <http://rdaregistry.info/Elements/u/P60119> ;
    reg:lexicalAlias <http://rdaregistry.info/Elements/a/variantNameForTheCorporateBody.en> ;
    reg:name "variantNameForTheCorporateBody"@en ;
    reg:status <http://metadataregistry.org/uri/RegStatus/1001> ;
    a rdf:Property ;
    rdfs:domain <http://rdaregistry.info/Elements/c/C10005> ;
    rdfs:isDefinedBy <http://rdaregistry.info/Elements/a/> ;
    rdfs:label "a pour variante de nom de la collectivité"@fr, "har variantnamn för institutionen"@sv, "has variant name for the corporate body"@en ;
    rdfs:subPropertyOf <http://rdaregistry.info/Elements/a/P50032> ;
    skos:definition "Met une collectivité en relation avec un nom ou forme de nom sous laquelle une collectivité est connue et qui diffère du nom ou de la forme de nom choisie comme nom privilégié."@fr, "Relates a corporate body to a name or form of name by which a corporate body is known that differs from a name or form of name chosen as a preferred name."@en .

<http://rdaregistry.info/Elements/a/P50026>
    rdakit:instructionNumber "29.5" ;
    rdakit:toolkitDefinition "A person employed by a corporate body."@en, "Personne employée par la collectivité."@fr, "Una persona empleada por la entidad corporativa."@es ;
    rdakit:toolkitLabel "empleado"@es, "employee"@en, "employé"@fr ;
    reg:hasSubproperty <http://rdaregistry.info/Elements/a/datatype/P50026>, <http://rdaregistry.info/Elements/a/object/P50026> ;
    reg:hasUnconstrained <http://rdaregistry.info/Elements/u/P60629> ;
    reg:lexicalAlias <http://rdaregistry.info/Elements/a/employee.en> ;
    reg:name "employee"@en ;
    reg:status <http://metadataregistry.org/uri/RegStatus/1001> ;
    a rdf:Property ;
    rdfs:domain <http://rdaregistry.info/Elements/c/C10005> ;
    rdfs:isDefinedBy <http://rdaregistry.info/Elements/a/> ;
    rdfs:label "a pour employé"@fr, "has employee"@en ;
    skos:definition "Met une collectivité en relation avec une personne employée par la collectivité."@fr, "Relates a corporate body to a person employed by a corporate body."@en .

<http://rdaregistry.info/Elements/a/P50027>
    rdakit:instructionNumber "29.5" ;
    rdakit:toolkitDefinition "A person holding an office in or commanding a corporate body."@en, "Personne qui exerce une fonction administrative ou officielle dans la collectivité."@fr, "Una persona que tiene un cargo en la entidad corporativa."@es ;
    rdakit:toolkitLabel "funcionario"@es, "officer"@en, "titulaire"@fr ;
    reg:hasSubproperty <http://rdaregistry.info/Elements/a/datatype/P50027>, <http://rdaregistry.info/Elements/a/object/P50027>, <http://rdaregistry.info/Elements/a/object/P50284>, <http://rdaregistry.info/Elements/a/object/P50285> ;
    reg:hasUnconstrained <http://rdaregistry.info/Elements/u/P60633> ;
    reg:lexicalAlias <http://rdaregistry.info/Elements/a/officer.en> ;
    reg:name "officer"@en ;
    reg:status <http://metadataregistry.org/uri/RegStatus/1001> ;
    a rdf:Property ;
    rdfs:domain <http://rdaregistry.info/Elements/c/C10005> ;
    rdfs:isDefinedBy <http://rdaregistry.info/Elements/a/> ;
    rdfs:label "a pour titulaire"@fr, "has officer"@en ;
    skos:definition "Met une collectivité en relation avec une personne qui exerce une fonction administrative ou officielle dans la collectivité."@fr, "Relates a corporate body to a person holding an office in or commanding a corporate body."@en .

<http://rdaregistry.info/Elements/a/P50028>
    rdakit:instructionNumber "29.5" ;
    rdakit:toolkitDefinition "A person sponsoring a corporate body."@en, "Personne qui commandite la collectivité."@fr, "Una persona que patrocina la entidad corporativa"@es ;
    rdakit:toolkitLabel "patrocinador"@es, "personne commanditaire"@fr, "sponsor"@en ;
    reg:hasSubproperty <http://rdaregistry.info/Elements/a/datatype/P50028>, <http://rdaregistry.info/Elements/a/object/P50028> ;
    reg:hasUnconstrained <http://rdaregistry.info/Elements/u/P60676> ;
    reg:lexicalAlias <http://rdaregistry.info/Elements/a/sponsor.en> ;
    reg:name "sponsor"@en ;
    reg:status <http://metadataregistry.org/uri/RegStatus/1001> ;
    a rdf:Property ;
    rdfs:domain <http://rdaregistry.info/Elements/c/C10005> ;
    rdfs:isDefinedBy <http://rdaregistry.info/Elements/a/> ;
    rdfs:label "a pour personne commanditaire"@fr, "has sponsor"@en ;
    skos:definition "Met une collectivité en relation avec une personne qui commandite la collectivité."@fr, "Relates a corporate body to a person sponsoring a corporate body."@en .

<http://rdaregistry.info/Elements/a/P50029>
    rdakit:instructionNumber "29.5" ;
    rdakit:toolkitDefinition "A person who founded a corporate body."@en, "Personne qui a fondé la collectivité."@fr, "Una persona que fundó la entidad corporativa."@es ;
    rdakit:toolkitLabel "fondateur"@fr, "founder"@en, "fundador"@es ;
    reg:hasSubproperty <http://rdaregistry.info/Elements/a/datatype/P50029>, <http://rdaregistry.info/Elements/a/object/P50029> ;
    reg:hasUnconstrained <http://rdaregistry.info/Elements/u/P60694> ;
    reg:lexicalAlias <http://rdaregistry.info/Elements/a/founder.en> ;
    reg:name "founder"@en ;
    reg:status <http://metadataregistry.org/uri/RegStatus/1001> ;
    a rdf:Property ;
    rdfs:domain <http://rdaregistry.info/Elements/c/C10005> ;
    rdfs:isDefinedBy <http://rdaregistry.info/Elements/a/> ;
    rdfs:label "a pour fondateur"@fr, "has founder"@en ;
    skos:definition "Met une collectivité en relation avec une personne qui a fondé la collectivité."@fr, "Relates a corporate body to a person who founded a corporate body."@en .

<http://rdaregistry.info/Elements/a/P50030>
    rdakit:instructionNumber "29.5" ;
    rdakit:toolkitDefinition "A person who is a member of a corporate body."@en, "Personne qui est membre du groupe d’interprètes, de l’expédition, etc."@fr, "Una persona que es miembro de una entidad corporativa."@es ;
    rdakit:toolkitLabel "member"@en, "membre"@fr, "miembro"@es ;
    reg:hasSubproperty <http://rdaregistry.info/Elements/a/datatype/P50030>, <http://rdaregistry.info/Elements/a/object/P50030> ;
    reg:hasUnconstrained <http://rdaregistry.info/Elements/u/P60697> ;
    reg:lexicalAlias <http://rdaregistry.info/Elements/a/member.en> ;
    reg:name "member"@en ;
    reg:status <http://metadataregistry.org/uri/RegStatus/1001> ;
    a rdf:Property ;
    rdfs:domain <http://rdaregistry.info/Elements/c/C10005> ;
    rdfs:isDefinedBy <http://rdaregistry.info/Elements/a/> ;
    rdfs:label "a pour membre"@fr, "has member"@en ;
    skos:definition "Met une collectivité en relation avec une personne qui est membre du groupe d’interprètes, de l’expédition, etc."@fr, "Relates a corporate body to a person who is a member of a corporate body."@en .

<http://rdaregistry.info/Elements/a/P50031>
    rdakit:instructionNumber "11.3" ;
    rdakit:toolkitDefinition "A significant location associated with a corporate body."@en, "Localisation significative associée à une collectivité."@fr, "Un lugar significativo asociado con una entidad corporativa."@es ;
    rdakit:toolkitLabel "lieu associé à la collectivité"@fr, "lugar asociado con la entidad corporativa"@es, "ort förknippad med institutionen"@sv, "place associated with the corporate body"@en ;
    reg:hasSubproperty <http://rdaregistry.info/Elements/a/datatype/P50031> ;
    reg:hasUnconstrained <http://rdaregistry.info/Elements/u/P60325> ;
    reg:lexicalAlias <http://rdaregistry.info/Elements/a/placeAssociatedWithTheCorporateBody.en> ;
    reg:name "placeAssociatedWithTheCorporateBody"@en ;
    reg:status <http://metadataregistry.org/uri/RegStatus/1001> ;
    a rdf:Property ;
    rdfs:domain <http://rdaregistry.info/Elements/c/C10005> ;
    rdfs:isDefinedBy <http://rdaregistry.info/Elements/a/> ;
    rdfs:label "a pour lieu associé à la collectivité"@fr, "har ort förknippad med institutionen"@sv, "has place associated with the corporate body"@en ;
    skos:definition "Met une collectivité en relation avec une localisation significative associée à une collectivité."@fr, "Relates a corporate body to a significant location associated with a corporate body."@en .

<http://rdaregistry.info/Elements/a/P50032>
    rdakit:instructionNumber "11.2" ;
    rdakit:toolkitDefinition "A word, character, or group of words and/or characters by which a corporate body is known."@en, "Mot, caractère ou groupe de mots et/ou de caractères sous lequel une collectivité est connue."@fr, "Una palabra, carácter o grupo de palabras y/o caracteres mediante los cuales se conoce una entidad corporativa."@es ;
    rdakit:toolkitLabel "institutionsnamn"@sv, "name of the corporate body"@en, "nom de collectivité"@fr, "nombre de la entidad corporativa"@es ;
    reg:hasSubproperty <http://rdaregistry.info/Elements/a/P50041>, <http://rdaregistry.info/Elements/a/datatype/P50032> ;
    reg:hasUnconstrained <http://rdaregistry.info/Elements/u/P60368> ;
    reg:lexicalAlias <http://rdaregistry.info/Elements/a/nameOfTheCorporateBody.en> ;
    reg:name "nameOfTheCorporateBody"@en ;
    reg:status <http://metadataregistry.org/uri/RegStatus/1001> ;
    a rdf:Property ;
    rdfs:domain <http://rdaregistry.info/Elements/c/C10005> ;
    rdfs:isDefinedBy <http://rdaregistry.info/Elements/a/> ;
    rdfs:label "a pour nom de collectivité"@fr, "har institutionsnamn"@sv, "has name of the corporate body"@en ;
    skos:definition "Met une collectivité en relation avec un mot, un caractère ou un groupe de mots et/ou de caractères sous lequel une collectivité est connue."@fr, "Relates a corporate body to a word, character, or group of words and/or characters by which a corporate body is known."@en .

<http://rdaregistry.info/Elements/a/P50033>
    rdakit:instructionNumber "11.7" ;
    rdakit:toolkitDefinition "A word, phrase, or abbreviation indicating incorporation or legal status of a corporate body, or any term serving to differentiate a corporate body from other corporate bodies, persons, etc."@en, "Mot, locution ou abréviation indiquant le statut commercial ou juridique d’une collectivité ou tout terme permettant de différencier la collectivité d’autres collectivités, personnes, etc."@fr, "Una palabra, frase o abreviatura que indica la incorporación o la condición legal de una entidad corporativa, o cualquier término que diferencia la entidad de otras entidades corporativas, personas, etc."@es ;
    rdakit:toolkitLabel "autre information associée à la collectivité"@fr, "other designation associated with the corporate body"@en, "otra designación asociada con la entidad corporativa"@es, "övrig beteckning förknippad med institutionen"@sv ;
    reg:hasSubproperty <http://rdaregistry.info/Elements/a/datatype/P50033> ;
    reg:hasUnconstrained <http://rdaregistry.info/Elements/u/P60370> ;
    reg:lexicalAlias <http://rdaregistry.info/Elements/a/otherDesignationAssociatedWithTheCorporateBody.en> ;
    reg:name "otherDesignationAssociatedWithTheCorporateBody"@en ;
    reg:status <http://metadataregistry.org/uri/RegStatus/1001> ;
    a rdf:Property ;
    rdfs:domain <http://rdaregistry.info/Elements/c/C10005> ;
    rdfs:isDefinedBy <http://rdaregistry.info/Elements/a/> ;
    rdfs:label "a pour autre information associée à la collectivité"@fr, "har övrig beteckning förknippad med institutionen"@sv, "has other designation associated with the corporate body"@en ;
    skos:definition "Met une collectivité en relation avec un mot, une locution ou une abréviation indiquant le statut commercial ou juridique d’une collectivité ou tout terme permettant de différencier la collectivité d’autres collectivités, personnes, etc."@fr, "Relates a corporate body to a word, phrase, or abbreviation indicating incorporation or legal status of a corporate body, or any term serving to differentiate a corporate body from other corporate bodies, persons, etc."@en .

<http://rdaregistry.info/Elements/a/P50034>
    rdakit:instructionNumber "11.5" ;
    rdakit:toolkitDefinition "An institution commonly associated with a corporate body."@en, "Institution communément associée à une collectivité."@fr, "Una institución comúnmente asociada con una entidad corporativa."@es ;
    rdakit:toolkitLabel "associated institution"@en, "institución asociada"@es, "institution associée"@fr, "samhörande institution"@sv ;
    reg:hasSubproperty <http://rdaregistry.info/Elements/a/datatype/P50034> ;
    reg:hasUnconstrained <http://rdaregistry.info/Elements/u/P60482> ;
    reg:lexicalAlias <http://rdaregistry.info/Elements/a/associatedInstitution.en> ;
    reg:name "associatedInstitution"@en ;
    reg:status <http://metadataregistry.org/uri/RegStatus/1001> ;
    a rdf:Property ;
    rdfs:domain <http://rdaregistry.info/Elements/c/C10005> ;
    rdfs:isDefinedBy <http://rdaregistry.info/Elements/a/> ;
    rdfs:label "a pour institution associée"@fr, "har samhörande institution"@sv, "has associated institution"@en ;
    skos:definition "Met une collectivité en relation avec une institution communément associée à une collectivité."@fr, "Relates a corporate body to an institution commonly associated with a corporate body."@en .

<http://rdaregistry.info/Elements/a/P50035>
    rdakit:instructionNumber "11.11" ;
    rdakit:toolkitDefinition "A summary of historical information about a corporate body."@en, "Información histórica de una entidad corporativa"@es, "Information historique sur la collectivité."@fr ;
    rdakit:toolkitLabel "corporate history"@en, "historia corporativa"@es, "historique de la collectivité"@fr, "institutionshistoria"@sv ;
    reg:hasSubproperty <http://rdaregistry.info/Elements/a/datatype/P50035> ;
    reg:hasUnconstrained <http://rdaregistry.info/Elements/u/P60484> ;
    reg:lexicalAlias <http://rdaregistry.info/Elements/a/corporateHistory.en> ;
    reg:name "corporateHistory"@en ;
    reg:status <http://metadataregistry.org/uri/RegStatus/1001> ;
    a rdf:Property ;
    rdfs:domain <http://rdaregistry.info/Elements/c/C10005> ;
    rdfs:isDefinedBy <http://rdaregistry.info/Elements/a/> ;
    rdfs:label "a pour historique de la collectivité"@fr, "har institutionshistoria"@sv, "has corporate history"@en ;
    skos:definition "Met une collectivité en relation avec une information historique sur la collectivité."@fr, "Relates a corporate body to a summary of historical information about a corporate body."@en .

<http://rdaregistry.info/Elements/a/P50036>
    rdakit:instructionNumber "11.9" ;
    rdakit:toolkitDefinition "An address of a corporate body."@en, "La dirección de una entidad corporativa."@es, "L’adresse du siège social ou des bureaux, l’adresse électronique ou l’adresse du site Web de la collectivité."@fr ;
    rdakit:toolkitLabel "address of the corporate body"@en, "adresse de la collectivité"@fr, "dirección de la entidad corporativa"@es ;
    reg:hasSubproperty <http://rdaregistry.info/Elements/a/datatype/P50036> ;
    reg:hasUnconstrained <http://rdaregistry.info/Elements/u/P60512> ;
    reg:lexicalAlias <http://rdaregistry.info/Elements/a/addressOfTheCorporateBody.en> ;
    reg:name "addressOfTheCorporateBody"@en ;
    reg:status <http://metadataregistry.org/uri/RegStatus/1001> ;
    a rdf:Property ;
    rdfs:domain <http://rdaregistry.info/Elements/c/C10005> ;
    rdfs:isDefinedBy <http://rdaregistry.info/Elements/a/> ;
    rdfs:label "a pour adresse de la collectivité"@fr, "has address of the corporate body"@en ;
    skos:definition "Met une collectivité en relation avec l’adresse du siège social ou des bureaux, l’adresse électronique ou l’adresse du site Web de la collectivité."@fr, "Relates a corporate body to an address of a corporate body."@en .

<http://rdaregistry.info/Elements/a/P50037>
    rdakit:instructionNumber "11.4.3" ;
    rdakit:toolkitDefinition "A date on which a corporate body was established or founded."@en, "La date à laquelle une collectivité a été établie ou fondée."@fr, "La fecha en que se estableció o fundó una entidad corporativa."@es ;
    rdakit:toolkitLabel "date de fondation"@fr, "date of establishment"@en, "fecha de establecimiento"@es, "tid för institutionens grundande"@sv ;
    reg:hasSubproperty <http://rdaregistry.info/Elements/a/datatype/P50037> ;
    reg:hasUnconstrained <http://rdaregistry.info/Elements/u/P60524> ;
    reg:lexicalAlias <http://rdaregistry.info/Elements/a/dateOfEstablishment.en> ;
    reg:name "dateOfEstablishment"@en ;
    reg:status <http://metadataregistry.org/uri/RegStatus/1001> ;
    a rdf:Property ;
    rdfs:domain <http://rdaregistry.info/Elements/c/C10005> ;
    rdfs:isDefinedBy <http://rdaregistry.info/Elements/a/> ;
    rdfs:label "a pour date de fondation"@fr, "har tid för institutionens grundande"@sv, "has date of establishment"@en ;
    rdfs:subPropertyOf <http://rdaregistry.info/Elements/a/P50040> ;
    skos:definition "Met une collectivité en relation avec la date à laquelle une collectivité a été établie ou fondée."@fr, "Relates a corporate body to a date on which a corporate body was established or founded."@en .

<http://rdaregistry.info/Elements/a/P50038>
    rdakit:instructionNumber "11.4.4" ;
    rdakit:toolkitDefinition "A date on which a corporate body was terminated or dissolved."@en, "La date à laquelle une collectivité a cessé son activité ou a été dissoute."@fr, "La fecha en la que una entidad corporativa fue concluida o disuelta."@es ;
    rdakit:toolkitLabel "date de cessation"@fr, "date of termination"@en, "fecha de terminación"@es, "tid för institutionens upphörande"@sv ;
    reg:hasSubproperty <http://rdaregistry.info/Elements/a/datatype/P50038> ;
    reg:hasUnconstrained <http://rdaregistry.info/Elements/u/P60525> ;
    reg:lexicalAlias <http://rdaregistry.info/Elements/a/dateOfTermination.en> ;
    reg:name "dateOfTermination"@en ;
    reg:status <http://metadataregistry.org/uri/RegStatus/1001> ;
    a rdf:Property ;
    rdfs:domain <http://rdaregistry.info/Elements/c/C10005> ;
    rdfs:isDefinedBy <http://rdaregistry.info/Elements/a/> ;
    rdfs:label "a pour date de cessation"@fr, "har tid för institutionens upphörande"@sv, "has date of termination"@en ;
    rdfs:subPropertyOf <http://rdaregistry.info/Elements/a/P50040> ;
    skos:definition "Met une collectivité en relation avec la date à laquelle une collectivité a cessé son activité ou a été dissoute."@fr, "Relates a corporate body to a date on which a corporate body was terminated or dissolved."@en .

<http://rdaregistry.info/Elements/a/P50039>
    rdakit:instructionNumber "11.4.2" ;
    rdakit:toolkitDefinition "A date or range of dates on which a conference, congress, meeting, exhibition, fair, festival, etc., was held."@en, "La date ou la fourchette de dates à laquelle un congrès, une conférence, une réunion, une exposition, une foire, un festival, etc. s’est tenu."@fr, "La fecha o rango de fechas en las que se realizó una conferencia, congreso, reunión, exposición, feria, festival, etc."@es ;
    rdakit:toolkitLabel "date du congrès, etc."@fr, "date of conference, etc."@en, "fecha de la conferencia, etc."@es, "tid för konferens"@sv ;
    reg:hasSubproperty <http://rdaregistry.info/Elements/a/datatype/P50039> ;
    reg:hasUnconstrained <http://rdaregistry.info/Elements/u/P60526> ;
    reg:lexicalAlias <http://rdaregistry.info/Elements/a/dateOfConferenceEtc.en> ;
    reg:name "dateOfConferenceEtc"@en ;
    reg:status <http://metadataregistry.org/uri/RegStatus/1001> ;
    a rdf:Property ;
    rdfs:domain <http://rdaregistry.info/Elements/c/C10005> ;
    rdfs:isDefinedBy <http://rdaregistry.info/Elements/a/> ;
    rdfs:label "a pour date du congrès, etc."@fr, "har tid för konferens"@sv, "has date of conference, etc."@en ;
    rdfs:subPropertyOf <http://rdaregistry.info/Elements/a/P50040> ;
    skos:definition "Met une collectivité en relation avec la date ou la fourchette de dates à laquelle un congrès, une conférence, une réunion, une exposition, une foire, un festival, etc. s’est tenu."@fr, "Relates a corporate body to a date or range of dates on which a conference, congress, meeting, exhibition, fair, festival, etc., was held."@en .

<http://rdaregistry.info/Elements/a/P50040>
    rdakit:instructionNumber "11.4" ;
    rdakit:toolkitDefinition "A significant date associated with the history of a corporate body."@en, "Date importante associée à l’histoire d’une collectivité, telle que la date de fondation ou la date de cessation."@fr, "Una fecha significativa asociada con la historia de una entidad corporativa, incluyendo fechas de conferencia, fechas de terminación, y período de actividad."@es ;
    rdakit:toolkitLabel "date associated with the corporate body"@en, "date associée à la collectivité"@fr, "fecha asociada con la entidad corporativa"@es, "tid förknippad med institutionen"@sv ;
    reg:hasSubproperty <http://rdaregistry.info/Elements/a/P50037>, <http://rdaregistry.info/Elements/a/P50038>, <http://rdaregistry.info/Elements/a/P50039>, <http://rdaregistry.info/Elements/a/datatype/P50040> ;
    reg:hasUnconstrained <http://rdaregistry.info/Elements/u/P60324> ;
    reg:lexicalAlias <http://rdaregistry.info/Elements/a/dateAssociatedWithTheCorporateBody.en> ;
    reg:name "dateAssociatedWithTheCorporateBody"@en ;
    reg:status <http://metadataregistry.org/uri/RegStatus/1001> ;
    a rdf:Property ;
    rdfs:domain <http://rdaregistry.info/Elements/c/C10005> ;
    rdfs:isDefinedBy <http://rdaregistry.info/Elements/a/> ;
    rdfs:label "a pour date associée à la collectivité"@fr, "har tid förknippad med institutionen"@sv, "has date associated with the corporate body"@en ;
    skos:definition "Met une collectivité en relation avec une date importante associée à l’histoire d’une collectivité, telle que la date de fondation ou la date de cessation."@fr, "Relates a corporate body to a significant date associated with the history of a corporate body."@en .

<http://rdaregistry.info/Elements/a/P50041>
    rdakit:instructionNumber "11.2.2" ;
    rdakit:toolkitDefinition "A name or form of name chosen to identify a corporate body."@en, "El nombre o la forma del nombre elegida para identificar la entidad corporativa."@es, "Le nom ou la forme de nom choisie pour identifier la collectivité."@fr ;
    rdakit:toolkitLabel "föredraget namn för institutionen"@sv, "nom privilégié de la collectivité"@fr, "nombre preferido de la entidad corporativa"@es, "preferred name for the corporate body"@en ;
    reg:hasSubproperty <http://rdaregistry.info/Elements/a/datatype/P50041> ;
    reg:hasUnconstrained <http://rdaregistry.info/Elements/u/P60549> ;
    reg:lexicalAlias <http://rdaregistry.info/Elements/a/preferredNameForTheCorporateBody.en> ;
    reg:name "preferredNameForTheCorporateBody"@en ;
    reg:status <http://metadataregistry.org/uri/RegStatus/1001> ;
    a rdf:Property ;
    rdfs:domain <http://rdaregistry.info/Elements/c/C10005> ;
    rdfs:isDefinedBy <http://rdaregistry.info/Elements/a/> ;
    rdfs:label "a pour nom privilégié de la collectivité"@fr, "har föredraget namn för institutionen"@sv, "has preferred name for the corporate body"@en ;
    rdfs:subPropertyOf <http://rdaregistry.info/Elements/a/P50032> ;
    skos:definition "Met une collectivité en relation avec le nom ou la forme de nom choisie pour identifier la collectivité."@fr, "Relates a corporate body to a name or form of name chosen to identify a corporate body."@en .

<http://rdaregistry.info/Elements/a/P50042>
    rdakit:instructionNumber "18.5" ;
    rdakit:toolkitDefinition "A legal work of a higher court recording a decision of a lower court that is appealed by a corporate body."@en, "Collectivité qui en appelle de la décision d’un tribunal inférieur."@fr ;
    rdakit:toolkitLabel "appellant corporate body of"@en, "collectivité appelante de"@fr ;
    reg:hasSubproperty <http://rdaregistry.info/Elements/a/datatype/P50042>, <http://rdaregistry.info/Elements/a/object/P50042> ;
    reg:hasUnconstrained <http://rdaregistry.info/Elements/u/P60691> ;
    reg:lexicalAlias <http://rdaregistry.info/Elements/a/appellantCorporateBodyOf.en> ;
    reg:name "appellantCorporateBodyOf"@en ;
    reg:status <http://metadataregistry.org/uri/RegStatus/1001> ;
    a rdf:Property ;
    rdfs:domain <http://rdaregistry.info/Elements/c/C10005> ;
    rdfs:isDefinedBy <http://rdaregistry.info/Elements/a/> ;
    rdfs:label "est la collectivité appelante de"@fr, "is appellant corporate body of"@en ;
    rdfs:subPropertyOf <http://rdaregistry.info/Elements/a/P50088> ;
    skos:definition "Met une collectivité qui en appelle de la décision d’un tribunal inférieur en relation avec l’œuvre."@fr, "Relates a corporate body who appeals a decision of a lower court recorded in a legal work of a higher court to a work."@en .

<http://rdaregistry.info/Elements/a/P50043>
    rdakit:instructionNumber "18.5" ;
    rdakit:toolkitDefinition "A work that involves a responsibility for bringing a suit in a civil proceeding by a corporate body."@en, "Collectivité qui intente une poursuite civile."@fr ;
    rdakit:toolkitLabel "collectivité demanderesse de"@fr, "plaintiff corporate body of"@en ;
    reg:hasSubproperty <http://rdaregistry.info/Elements/a/datatype/P50043>, <http://rdaregistry.info/Elements/a/object/P50043> ;
    reg:hasUnconstrained <http://rdaregistry.info/Elements/u/P60693> ;
    reg:lexicalAlias <http://rdaregistry.info/Elements/a/plaintiffCorporateBodyOf.en> ;
    reg:name "plaintiffCorporateBodyOf"@en ;
    reg:status <http://metadataregistry.org/uri/RegStatus/1001> ;
    a rdf:Property ;
    rdfs:domain <http://rdaregistry.info/Elements/c/C10005> ;
    rdfs:isDefinedBy <http://rdaregistry.info/Elements/a/> ;
    rdfs:label "est la collectivité demanderesse de"@fr, "is plaintiff corporate body of"@en ;
    rdfs:subPropertyOf <http://rdaregistry.info/Elements/a/P50089> ;
    skos:definition "Met une collectivité qui intente une poursuite civile en relation avec l’œuvre."@fr, "Relates a corporate body who brings a suit in a civil proceeding to a work."@en .

<http://rdaregistry.info/Elements/a/P50044>
    rdakit:instructionNumber "18.5" ;
    rdakit:toolkitDefinition "A work of a court governed by court rules, regardless of their official nature."@en, "Tribunal régi par des règles de pratique, sans égard à leur nature officielle (par exemple, lois, règlements)."@fr ;
    rdakit:toolkitLabel "court governed of"@en, "tribunal régi de"@fr ;
    reg:hasSubproperty <http://rdaregistry.info/Elements/a/datatype/P50044>, <http://rdaregistry.info/Elements/a/object/P50044> ;
    reg:hasUnconstrained <http://rdaregistry.info/Elements/u/P60005> ;
    reg:lexicalAlias <http://rdaregistry.info/Elements/a/courtGovernedOf.en> ;
    reg:name "courtGovernedOf"@en ;
    reg:status <http://metadataregistry.org/uri/RegStatus/1001> ;
    a rdf:Property ;
    rdfs:domain <http://rdaregistry.info/Elements/c/C10005> ;
    rdfs:isDefinedBy <http://rdaregistry.info/Elements/a/> ;
    rdfs:label "est le tribunal régi de"@fr, "is court governed of"@en ;
    rdfs:subPropertyOf <http://rdaregistry.info/Elements/a/P50131> ;
    skos:definition "Met un tribunal régi par des règles de pratique, sans égard à leur nature officielle (par exemple, lois, règlements) en relation avec l’œuvre."@fr, "Relates a court governed by court rules, regardless of their official nature to a work."@en .

<http://rdaregistry.info/Elements/a/P50045>
    rdakit:instructionNumber "18.5" ;
    rdakit:toolkitDefinition "An item brought together with items from various sources that are then arranged, described, and cataloged as a collection."@en, "Conservateur qui rassemble des items de diverses sources qui sont subséquemment arrangés, décrits et catalogués comme une collection."@fr ;
    rdakit:toolkitLabel "collectionneur de"@fr, "collector of"@en ;
    reg:hasSubproperty <http://rdaregistry.info/Elements/a/datatype/P50045>, <http://rdaregistry.info/Elements/a/object/P50045> ;
    reg:hasUnconstrained <http://rdaregistry.info/Elements/u/P60006> ;
    reg:lexicalAlias <http://rdaregistry.info/Elements/a/collectorOf.en> ;
    reg:name "collectorOf"@en ;
    reg:status <http://metadataregistry.org/uri/RegStatus/1001> ;
    a rdf:Property ;
    rdfs:domain <http://rdaregistry.info/Elements/c/C10002> ;
    rdfs:isDefinedBy <http://rdaregistry.info/Elements/a/> ;
    rdfs:label "est le collectionneur de"@fr, "is collector of"@en ;
    rdfs:subPropertyOf <http://rdaregistry.info/Elements/a/P50133> ;
    skos:definition "Met un conservateur qui rassemble des items de diverses sources qui sont subséquemment arrangés, décrits et catalogués comme une collection en relation avec l’item."@fr, "Relates a curator who brings together items from various sources that are then arranged, described, and cataloged as a collection to an item."@en .

<http://rdaregistry.info/Elements/a/P50046>
    rdakit:instructionNumber "18.5" ;
    rdakit:toolkitDefinition "An item that is listed or inventoried in an aggregate work such as a collection of items or works."@en, "Conservateur qui dresse une liste et un inventaire des items faisant partie d’une œuvre agrégative telle qu’une collection d’items ou d’œuvres."@fr ;
    rdakit:toolkitLabel "collection registrar of"@en, "conservateur de collections de"@fr ;
    reg:hasSubproperty <http://rdaregistry.info/Elements/a/datatype/P50046>, <http://rdaregistry.info/Elements/a/object/P50046> ;
    reg:hasUnconstrained <http://rdaregistry.info/Elements/u/P60007> ;
    reg:lexicalAlias <http://rdaregistry.info/Elements/a/collectionRegistrarOf.en> ;
    reg:name "collectionRegistrarOf"@en ;
    reg:status <http://metadataregistry.org/uri/RegStatus/1001> ;
    a rdf:Property ;
    rdfs:domain <http://rdaregistry.info/Elements/c/C10002> ;
    rdfs:isDefinedBy <http://rdaregistry.info/Elements/a/> ;
    rdfs:label "est le conservateur de collections de"@fr, "is collection registrar of"@en ;
    rdfs:subPropertyOf <http://rdaregistry.info/Elements/a/P50133> ;
    skos:definition "Met un conservateur qui dresse une liste et un inventaire des items faisant partie d’une œuvre agrégative telle qu’une collection d’items ou d’œuvres en relation avec l’item."@fr, "Relates a curator who lists or inventories the items in an aggregate work such as a collection of items or works to an item."@en .

<http://rdaregistry.info/Elements/a/P50047>
    rdakit:instructionNumber "18.5" ;
    rdakit:toolkitDefinition "An item deposited into the custody of another agent, while still retaining ownership."@en, "Propriétaire actuel d’un item qui a déposé l’item sous la garde d’une autre personne, famille ou collectivité tout en en conservant la propriété."@fr ;
    rdakit:toolkitLabel "depositor of"@en, "déposant de"@fr ;
    reg:hasSubproperty <http://rdaregistry.info/Elements/a/datatype/P50047>, <http://rdaregistry.info/Elements/a/object/P50047> ;
    reg:hasUnconstrained <http://rdaregistry.info/Elements/u/P60008> ;
    reg:lexicalAlias <http://rdaregistry.info/Elements/a/depositorOf.en> ;
    reg:name "depositorOf"@en ;
    reg:status <http://metadataregistry.org/uri/RegStatus/1001> ;
    a rdf:Property ;
    rdfs:domain <http://rdaregistry.info/Elements/c/C10002> ;
    rdfs:isDefinedBy <http://rdaregistry.info/Elements/a/> ;
    rdfs:label "est le déposant de"@fr, "is depositor of"@en ;
    rdfs:subPropertyOf <http://rdaregistry.info/Elements/a/P50162> ;
    skos:definition "Met un propriétaire actuel d’un item qui a déposé l’item sous la garde d’une autre personne, famille ou collectivité tout en en conservant la propriété en relation avec l’item."@fr, "Relates a current owner of an item who deposited the item into the custody of another agent, while still retaining ownership to an item."@en .

<http://rdaregistry.info/Elements/a/P50048>
    rdakit:instructionNumber "18.5" ;
    rdakit:toolkitDefinition "A work that involves a responsibility for the general management and supervision of a filmed performance."@en, "Réalisateur responsable de la gestion et de la supervision générales d’une prestation filmée."@fr ;
    rdakit:toolkitLabel "film director of"@en, "réalisateur de films de"@fr ;
    reg:hasSubproperty <http://rdaregistry.info/Elements/a/datatype/P50048>, <http://rdaregistry.info/Elements/a/object/P50048> ;
    reg:hasUnconstrained <http://rdaregistry.info/Elements/u/P60009> ;
    reg:lexicalAlias <http://rdaregistry.info/Elements/a/filmDirectorOf.en> ;
    reg:name "filmDirectorOf"@en ;
    reg:status <http://metadataregistry.org/uri/RegStatus/1001> ;
    a rdf:Property ;
    rdfs:domain <http://rdaregistry.info/Elements/c/C10002> ;
    rdfs:isDefinedBy <http://rdaregistry.info/Elements/a/> ;
    rdfs:label "est le réalisateur de films de"@fr, "is film director of"@en ;
    rdfs:subPropertyOf <http://rdaregistry.info/Elements/a/P50205> ;
    skos:definition "Met un réalisateur responsable de la gestion et de la supervision générales d’une prestation filmée en relation avec l’œuvre."@fr, "Relates a director responsible for the general management and supervision of a filmed performance to a work."@en .

<http://rdaregistry.info/Elements/a/P50049>
    rdakit:instructionNumber "18.5" ;
    rdakit:toolkitDefinition "A work that involves a responsibility for the general management and supervision of a radio program."@en, "Réalisateur responsable de la gestion et de la supervision générales d’une émission de radio."@fr ;
    rdakit:toolkitLabel "radio director of"@en, "réalisateur d’émissions de radio de"@fr ;
    reg:hasSubproperty <http://rdaregistry.info/Elements/a/datatype/P50049>, <http://rdaregistry.info/Elements/a/object/P50049> ;
    reg:hasUnconstrained <http://rdaregistry.info/Elements/u/P60010> ;
    reg:lexicalAlias <http://rdaregistry.info/Elements/a/radioDirectorOf.en> ;
    reg:name "radioDirectorOf"@en ;
    reg:status <http://metadataregistry.org/uri/RegStatus/1001> ;
    a rdf:Property ;
    rdfs:domain <http://rdaregistry.info/Elements/c/C10002> ;
    rdfs:isDefinedBy <http://rdaregistry.info/Elements/a/> ;
    rdfs:label "est le réalisateur d’émissions de radio de"@fr, "is radio director of"@en ;
    rdfs:subPropertyOf <http://rdaregistry.info/Elements/a/P50205> ;
    skos:definition "Met un réalisateur responsable de la gestion et de la supervision générales d’une émission de radio en relation avec l’œuvre."@fr, "Relates a director responsible for the general management and supervision of a radio program to a work."@en .

<http://rdaregistry.info/Elements/a/P50050>
    rdakit:instructionNumber "18.5" ;
    rdakit:toolkitDefinition "A work that involves a responsibility for the general management and supervision of a television program."@en, "Réalisateur responsable de la gestion et de la supervision générales d’une émission de télévision."@fr ;
    rdakit:toolkitLabel "réalisateur d’émissions de télévision de"@fr, "television director of"@en ;
    reg:hasSubproperty <http://rdaregistry.info/Elements/a/datatype/P50050>, <http://rdaregistry.info/Elements/a/object/P50050> ;
    reg:hasUnconstrained <http://rdaregistry.info/Elements/u/P60011> ;
    reg:lexicalAlias <http://rdaregistry.info/Elements/a/televisionDirectorOf.en> ;
    reg:name "televisionDirectorOf"@en ;
    reg:status <http://metadataregistry.org/uri/RegStatus/1001> ;
    a rdf:Property ;
    rdfs:domain <http://rdaregistry.info/Elements/c/C10002> ;
    rdfs:isDefinedBy <http://rdaregistry.info/Elements/a/> ;
    rdfs:label "est le réalisateur d’émissions de télévision de"@fr, "is television director of"@en ;
    rdfs:subPropertyOf <http://rdaregistry.info/Elements/a/P50205> ;
    skos:definition "Met un réalisateur responsable de la gestion et de la supervision générales d’une émission de télévision en relation avec l’œuvre."@fr, "Relates a director responsible for the general management and supervision of a television program to a work."@en .

<http://rdaregistry.info/Elements/a/P50051>
    rdakit:instructionNumber "10.3" ;
    rdakit:toolkitDefinition "A categorization or generic descriptor for a type of family."@en, "Catégorie ou descripteur générique pour le type de famille."@fr, "Una categorización o descriptor genérico del tipo de familia."@es ;
    rdakit:toolkitLabel "tipo de familia"@es, "typ av familj/släkt"@sv, "type de famille"@fr, "type of family"@en ;
    reg:hasSubproperty <http://rdaregistry.info/Elements/a/datatype/P50051> ;
    reg:hasUnconstrained <http://rdaregistry.info/Elements/u/P60047> ;
    reg:lexicalAlias <http://rdaregistry.info/Elements/a/typeOfFamily.en> ;
    reg:name "typeOfFamily"@en ;
    reg:status <http://metadataregistry.org/uri/RegStatus/1001> ;
    a rdf:Property ;
    rdfs:domain <http://rdaregistry.info/Elements/c/C10008> ;
    rdfs:isDefinedBy <http://rdaregistry.info/Elements/a/> ;
    rdfs:label "a pour type de famille"@fr, "har typ av familj/släkt"@sv, "has type of family"@en ;
    skos:definition "Met une famille en relation avec une catégorie ou descripteur générique pour le type de famille."@fr, "Relates a family to a categorization or generic descriptor for a type of family."@en .

<http://rdaregistry.info/Elements/a/P50052>
    rdakit:instructionNumber "10.1" ;
    rdakit:toolkitDefinition "A character string uniquely associated with a family, or with a surrogate such as an authority record for a family."@en, "Chaîne de caractères associée de manière unique à une famille ou à un substitut d’une famille (par exemple, une notice d’autorité)."@fr, "Una cadena de caracteres solamente asociada con una familia, o con un sustituto de una familia (por ej., un registro de autoridad)."@es ;
    rdakit:toolkitLabel "identifiant de la famille"@fr, "identificador de la familia"@es, "identifier for the family"@en, "identifikator för familjen/släkten"@sv ;
    reg:hasSubproperty <http://rdaregistry.info/Elements/a/datatype/P50052> ;
    reg:hasUnconstrained <http://rdaregistry.info/Elements/u/P60053> ;
    reg:lexicalAlias <http://rdaregistry.info/Elements/a/identifierForTheFamily.en> ;
    reg:name "identifierForTheFamily"@en ;
    reg:status <http://metadataregistry.org/uri/RegStatus/1001> ;
    a rdf:Property ;
    rdfs:domain <http://rdaregistry.info/Elements/c/C10008> ;
    rdfs:isDefinedBy <http://rdaregistry.info/Elements/a/> ;
    rdfs:label "a pour identifiant de la famille"@fr, "har identifikator för familjen/släkten"@sv, "has identifier for the family"@en ;
    skos:definition "Met une famille en relation avec une chaîne de caractères associée de manière unique à une famille ou à un substitut d’une famille (par exemple, une notice d’autorité)."@fr, "Relates a family to a character string uniquely associated with a family, or with a surrogate such as an authority record for a family."@en ;
    skos:scopeNote "L’identifiant sert à distinguer cette famille d’autres familles."@fr, "The identifier serves to differentiate a family from other families."@en .

<http://rdaregistry.info/Elements/a/P50053>
    rdakit:instructionNumber "29.5" ;
    rdakit:toolkitDefinition "A family descended from another family."@en, "Famille descendant de l’autre famille."@fr, "Una familia que desciende de otra familia."@es ;
    rdakit:toolkitLabel "descendant family"@en, "familia descendiente"@es, "famille descendante"@fr ;
    reg:hasSubproperty <http://rdaregistry.info/Elements/a/datatype/P50053>, <http://rdaregistry.info/Elements/a/object/P50053> ;
    reg:hasUnconstrained <http://rdaregistry.info/Elements/u/P60686> ;
    reg:lexicalAlias <http://rdaregistry.info/Elements/a/descendantFamily.en> ;
    reg:name "descendantFamily"@en ;
    reg:status <http://metadataregistry.org/uri/RegStatus/1001> ;
    a rdf:Property ;
    rdfs:domain <http://rdaregistry.info/Elements/c/C10008> ;
    rdfs:isDefinedBy <http://rdaregistry.info/Elements/a/> ;
    rdfs:label "a pour famille descendante"@fr, "has descendant family"@en ;
    skos:definition "Met une famille en relation avec une famille descendant de l’autre famille."@fr, "Relates a family to a family descended from another family."@en .

<http://rdaregistry.info/Elements/a/P50054>
    rdakit:instructionNumber "10.2.3" ;
    rdakit:toolkitDefinition "A name or form of name by which a family is known that differs from a name or form of name chosen as a preferred name."@en, "Nom ou forme de nom sous laquelle une famille est connue et qui diffère du nom ou de la forme de nom choisie comme nom privilégié."@fr, "Un nombre o una forma del nombre mediante el cual se conoce una familia, que difiere del nombre o la forma del nombre elegida como el nombre preferido."@es ;
    rdakit:toolkitLabel "variant name for the family"@en, "variante de nom de la famille"@fr, "variante del nombre de la familia"@es, "variantnamn för familjen/släkten"@sv ;
    reg:hasSubproperty <http://rdaregistry.info/Elements/a/datatype/P50054> ;
    reg:hasUnconstrained <http://rdaregistry.info/Elements/u/P60119> ;
    reg:lexicalAlias <http://rdaregistry.info/Elements/a/variantNameForTheFamily.en> ;
    reg:name "variantNameForTheFamily"@en ;
    reg:status <http://metadataregistry.org/uri/RegStatus/1001> ;
    a rdf:Property ;
    rdfs:domain <http://rdaregistry.info/Elements/c/C10008> ;
    rdfs:isDefinedBy <http://rdaregistry.info/Elements/a/> ;
    rdfs:label "a pour variante de nom de la famille"@fr, "har variantnamn för familjen/släkten"@sv, "has variant name for the family"@en ;
    rdfs:subPropertyOf <http://rdaregistry.info/Elements/a/P50061> ;
    skos:definition "Met une famille en relation avec un nom ou une forme de nom sous laquelle une famille est connue et qui diffère du nom ou de la forme de nom choisie comme nom privilégié."@fr, "Relates a family to a name or form of name by which a family is known that differs from a name or form of name chosen as a preferred name."@en .

<http://rdaregistry.info/Elements/a/P50055>
    rdakit:instructionNumber "29.5" ;
    rdakit:toolkitDefinition "A person from whom a family is descended."@en, "Personne de qui la famille descend."@fr, "Una persona de la cual desciende la familia."@es ;
    rdakit:toolkitLabel "ancêtre"@fr, "progenitor"@en, "progenitor"@es ;
    reg:hasSubproperty <http://rdaregistry.info/Elements/a/datatype/P50055>, <http://rdaregistry.info/Elements/a/object/P50055> ;
    reg:hasUnconstrained <http://rdaregistry.info/Elements/u/P60683> ;
    reg:lexicalAlias <http://rdaregistry.info/Elements/a/progenitor.en> ;
    reg:name "progenitor"@en ;
    reg:status <http://metadataregistry.org/uri/RegStatus/1001> ;
    a rdf:Property ;
    rdfs:domain <http://rdaregistry.info/Elements/c/C10008> ;
    rdfs:isDefinedBy <http://rdaregistry.info/Elements/a/> ;
    rdfs:label "a pour ancêtre"@fr, "has progenitor"@en ;
    rdfs:subPropertyOf <http://rdaregistry.info/Elements/a/P50056> ;
    skos:definition "Met une famille en relation avec une personne de qui la famille descend."@fr, "Relates a family to a person from whom a family is descended."@en .

<http://rdaregistry.info/Elements/a/P50056>
    rdakit:instructionNumber "29.5" ;
    rdakit:toolkitDefinition "A person who is a member of a family."@en, "Personne qui est membre de la famille."@fr, "Una persona que es un miembro de la familia."@es ;
    rdakit:toolkitLabel "family member"@en, "membre de la famille"@fr, "miembro de la familia"@es ;
    reg:hasSubproperty <http://rdaregistry.info/Elements/a/P50055>, <http://rdaregistry.info/Elements/a/datatype/P50056>, <http://rdaregistry.info/Elements/a/object/P50056> ;
    reg:hasUnconstrained <http://rdaregistry.info/Elements/u/P60648> ;
    reg:lexicalAlias <http://rdaregistry.info/Elements/a/familyMember.en> ;
    reg:name "familyMember"@en ;
    reg:status <http://metadataregistry.org/uri/RegStatus/1001> ;
    a rdf:Property ;
    rdfs:domain <http://rdaregistry.info/Elements/c/C10008> ;
    rdfs:isDefinedBy <http://rdaregistry.info/Elements/a/> ;
    rdfs:label "a pour membre de la famille"@fr, "has family member"@en ;
    skos:definition "Met une famille en relation avec une personne qui est membre de la famille."@fr, "Relates a family to a person who is a member of a family."@en .

<http://rdaregistry.info/Elements/a/P50057>
    rdakit:instructionNumber "10.5" ;
    rdakit:toolkitDefinition "A place where a family resides or has resided or has some connection."@en, "Lieu où une famille réside ou a résidé ou avec lequel elle a une relation quelconque."@fr, "Un lugar donde reside la familia, o donde ha residido o que tiene alguna conexión."@es ;
    rdakit:toolkitLabel "lieu associé à la famille"@fr, "lugar asociado con la familia"@es, "ort förknippad med familjen/släkten"@sv, "place associated with the family"@en ;
    reg:hasSubproperty <http://rdaregistry.info/Elements/a/datatype/P50057> ;
    reg:hasUnconstrained <http://rdaregistry.info/Elements/u/P60325> ;
    reg:lexicalAlias <http://rdaregistry.info/Elements/a/placeAssociatedWithTheFamily.en> ;
    reg:name "placeAssociatedWithTheFamily"@en ;
    reg:status <http://metadataregistry.org/uri/RegStatus/1001> ;
    a rdf:Property ;
    rdfs:domain <http://rdaregistry.info/Elements/c/C10008> ;
    rdfs:isDefinedBy <http://rdaregistry.info/Elements/a/> ;
    rdfs:label "a pour lieu associé à la famille"@fr, "har ort förknippad med familjen/släkten"@sv, "has place associated with the family"@en ;
    skos:definition "Met une famille en relation avec un lieu où une famille réside ou a résidé ou avec lequel elle a une relation quelconque."@fr, "Relates a family to a place where a family resides or has resided or has some connection."@en .

<http://rdaregistry.info/Elements/a/P50058>
    rdakit:instructionNumber "10.4" ;
    rdakit:toolkitDefinition "A significant date associated with a family."@en, "Date importante associée à une famille."@fr, "Una fecha significativa asociada con la familia."@es ;
    rdakit:toolkitLabel "date associated with the family"@en, "date associée à la famille"@fr, "fecha asociada con la familia"@es, "tid förknippad med famliljen/släkten"@sv ;
    reg:hasSubproperty <http://rdaregistry.info/Elements/a/datatype/P50058> ;
    reg:hasUnconstrained <http://rdaregistry.info/Elements/u/P60324> ;
    reg:lexicalAlias <http://rdaregistry.info/Elements/a/dateAssociatedWithTheFamily.en> ;
    reg:name "dateAssociatedWithTheFamily"@en ;
    reg:status <http://metadataregistry.org/uri/RegStatus/1001> ;
    a rdf:Property ;
    rdfs:domain <http://rdaregistry.info/Elements/c/C10008> ;
    rdfs:isDefinedBy <http://rdaregistry.info/Elements/a/> ;
    rdfs:label "a pour date associée à la famille"@fr, "har tid förknippad med famliljen/släkten"@sv, "has date associated with the family"@en ;
    skos:definition "Met une famille en relation avec une date importante associée à une famille."@fr, "Relates a family to a significant date associated with a family."@en .

<http://rdaregistry.info/Elements/a/P50059>
    rdakit:instructionNumber "10.7" ;
    rdakit:toolkitDefinition "A title of nobility, etc., associated with a family."@en, "Titre de noblesse, etc. associé à une famille."@fr, "Un título de nobleza, etc., asociado con una familia."@es ;
    rdakit:toolkitLabel "hereditary title"@en, "titre héréditaire"@fr, "título hereditario"@es, "ärvd titel"@sv ;
    reg:hasSubproperty <http://rdaregistry.info/Elements/a/datatype/P50059> ;
    reg:hasUnconstrained <http://rdaregistry.info/Elements/u/P60356> ;
    reg:lexicalAlias <http://rdaregistry.info/Elements/a/hereditaryTitle.en> ;
    reg:name "hereditaryTitle"@en ;
    reg:status <http://metadataregistry.org/uri/RegStatus/1001> ;
    a rdf:Property ;
    rdfs:domain <http://rdaregistry.info/Elements/c/C10008> ;
    rdfs:isDefinedBy <http://rdaregistry.info/Elements/a/> ;
    rdfs:label "a pour titre héréditaire"@fr, "har ärvd titel"@sv, "has hereditary title"@en ;
    skos:definition "Met une famille en relation avec un titre de noblesse, etc. associé à une famille."@fr, "Relates a family to a title of nobility, etc., associated with a family."@en .

<http://rdaregistry.info/Elements/a/P50060>
    rdakit:instructionNumber "10.6" ;
    rdakit:toolkitDefinition "A well-known individual who is a member of a family."@en, "Individu jouissant d’une certaine notoriété et qui est membre d’une famille."@fr, "Un individuo ampliamente conocido, que es miembro de una familia."@es ;
    rdakit:toolkitLabel "membre illustre de la famille"@fr, "miembro prominente de la familia"@es, "prominent member of the family"@en, "välkänd medlem av familjen/släkten"@sv ;
    reg:hasSubproperty <http://rdaregistry.info/Elements/a/datatype/P50060> ;
    reg:hasUnconstrained <http://rdaregistry.info/Elements/u/P60362> ;
    reg:lexicalAlias <http://rdaregistry.info/Elements/a/prominentMemberOfTheFamily.en> ;
    reg:name "prominentMemberOfTheFamily"@en ;
    reg:status <http://metadataregistry.org/uri/RegStatus/1001> ;
    a rdf:Property ;
    rdfs:domain <http://rdaregistry.info/Elements/c/C10008> ;
    rdfs:isDefinedBy <http://rdaregistry.info/Elements/a/> ;
    rdfs:label "a pour membre illustre de la famille"@fr, "har välkänd medlem av familjen/släkten"@sv, "has prominent member of the family"@en ;
    skos:definition "Met une famille en relation avec un individu jouissant d’une certaine notoriété et qui est membre d’une famille."@fr, "Relates a family to a well-known individual who is a member of a family."@en .

<http://rdaregistry.info/Elements/a/P50061>
    rdakit:instructionNumber "10.2" ;
    rdakit:toolkitDefinition "A word, character, or group of words and/or characters by which a family is known."@en, "Mot, caractère ou groupe de mots et/ou de caractères sous lequel une famille est connue."@fr, "Una palabra, un carácter o grupo de palabras y/o caracteres mediante los cuales se conoce una familia."@es ;
    rdakit:toolkitLabel "name of the family"@en, "nom de famille"@fr, "nombre de la familia"@es ;
    reg:hasSubproperty <http://rdaregistry.info/Elements/a/P50054>, <http://rdaregistry.info/Elements/a/P50065>, <http://rdaregistry.info/Elements/a/datatype/P50061> ;
    reg:hasUnconstrained <http://rdaregistry.info/Elements/u/P60368> ;
    reg:lexicalAlias <http://rdaregistry.info/Elements/a/nameOfTheFamily.en> ;
    reg:name "nameOfTheFamily"@en ;
    reg:status <http://metadataregistry.org/uri/RegStatus/1001> ;
    a rdf:Property ;
    rdfs:domain <http://rdaregistry.info/Elements/c/C10008> ;
    rdfs:isDefinedBy <http://rdaregistry.info/Elements/a/> ;
    rdfs:label "a pour nom de famille"@fr, "has name of the family"@en ;
    skos:definition "Met une famille en relation avec un mot, un caractère ou un groupe de mots et/ou de caractères sous lequel une famille est connue."@fr, "Relates a family to a word, character, or group of words and/or characters by which a family is known."@en .

<http://rdaregistry.info/Elements/a/P50062>
    rdakit:instructionNumber "29.5" ;
    rdakit:toolkitDefinition "An organization that a family founded."@en, "Organisation que la famille a fondée."@fr, "Una entidad corporativa que la familia fundó."@es ;
    rdakit:toolkitLabel "collectivité fondée de la famille"@fr, "entidad corporativa fundada"@es, "founded corporate body of family"@en ;
    reg:hasSubproperty <http://rdaregistry.info/Elements/a/datatype/P50062>, <http://rdaregistry.info/Elements/a/object/P50062> ;
    reg:hasUnconstrained <http://rdaregistry.info/Elements/u/P60687> ;
    reg:lexicalAlias <http://rdaregistry.info/Elements/a/foundedCorporateBodyOfFamily.en> ;
    reg:name "foundedCorporateBodyOfFamily"@en ;
    reg:status <http://metadataregistry.org/uri/RegStatus/1001> ;
    a rdf:Property ;
    rdfs:domain <http://rdaregistry.info/Elements/c/C10008> ;
    rdfs:isDefinedBy <http://rdaregistry.info/Elements/a/> ;
    rdfs:label "a pour collectivité fondée de la famille"@fr, "has founded corporate body of family"@en ;
    skos:definition "Met une famille en relation avec une organisation que la famille a fondée."@fr, "Relates a family to an organization that a family founded."@en .

<http://rdaregistry.info/Elements/a/P50063>
    rdakit:instructionNumber "29.5" ;
    rdakit:toolkitDefinition "An organization that a family sponsors."@en, "Organisation que la famille commandite."@fr, "Una entidad corporativa que la familia patrocina."@es ;
    rdakit:toolkitLabel "collectivité commanditée"@fr, "entidad corporativa patrocinada"@es, "sponsored corporate body of family"@en ;
    reg:hasSubproperty <http://rdaregistry.info/Elements/a/datatype/P50063>, <http://rdaregistry.info/Elements/a/object/P50063> ;
    reg:hasUnconstrained <http://rdaregistry.info/Elements/u/P60688> ;
    reg:lexicalAlias <http://rdaregistry.info/Elements/a/sponsoredCorporateBodyOfFamily.en> ;
    reg:name "sponsoredCorporateBodyOfFamily"@en ;
    reg:status <http://metadataregistry.org/uri/RegStatus/1001> ;
    a rdf:Property ;
    rdfs:domain <http://rdaregistry.info/Elements/c/C10008> ;
    rdfs:isDefinedBy <http://rdaregistry.info/Elements/a/> ;
    rdfs:label "a pour collectivité commanditée"@fr, "has sponsored corporate body of family"@en ;
    skos:definition "Met une famille en relation avec une organisation que la famille commandite."@fr, "Relates a family to an organization that a family sponsors."@en .

<http://rdaregistry.info/Elements/a/P50064>
    rdakit:instructionNumber "10.9" ;
    rdakit:toolkitDefinition "A summary of information about the history of a family and/or its members."@en, "Información biográfica sobre la familia y sus miembros"@es, "Information biographique sur la famille et ses membres."@fr ;
    rdakit:toolkitLabel "family history"@en, "historia de la familia"@es, "historique de la famille"@fr ;
    reg:hasSubproperty <http://rdaregistry.info/Elements/a/datatype/P50064> ;
    reg:hasUnconstrained <http://rdaregistry.info/Elements/u/P60484> ;
    reg:lexicalAlias <http://rdaregistry.info/Elements/a/familyHistory.en> ;
    reg:name "familyHistory"@en ;
    reg:status <http://metadataregistry.org/uri/RegStatus/1001> ;
    a rdf:Property ;
    rdfs:domain <http://rdaregistry.info/Elements/c/C10008> ;
    rdfs:isDefinedBy <http://rdaregistry.info/Elements/a/> ;
    rdfs:label "a pour historique de la famille"@fr, "has family history"@en ;
    skos:definition "Met une famille en relation avec une information biographique sur la famille et ses membres."@fr, "Relates a family to a summary of information about the history of a family and/or its members."@en .

<http://rdaregistry.info/Elements/a/P50065>
    rdakit:instructionNumber "10.2.2" ;
    rdakit:toolkitDefinition "A name or form of name chosen to identify a family."@en, "El nombre o la forma del nombre elegida para identificar la familia."@es, "Le nom ou la forme de nom choisie pour identifier la famille."@fr ;
    rdakit:toolkitLabel "föredraget namn för familjen/släkten"@sv, "nom privilégié de la famille"@fr, "nombre preferido de la familia"@es, "preferred name for the family"@en ;
    reg:hasSubproperty <http://rdaregistry.info/Elements/a/datatype/P50065> ;
    reg:hasUnconstrained <http://rdaregistry.info/Elements/u/P60549> ;
    reg:lexicalAlias <http://rdaregistry.info/Elements/a/preferredNameForTheFamily.en> ;
    reg:name "preferredNameForTheFamily"@en ;
    reg:status <http://metadataregistry.org/uri/RegStatus/1001> ;
    a rdf:Property ;
    rdfs:domain <http://rdaregistry.info/Elements/c/C10008> ;
    rdfs:isDefinedBy <http://rdaregistry.info/Elements/a/> ;
    rdfs:label "a pour nom privilégié de la famille"@fr, "har föredraget namn för familjen/släkten"@sv, "has preferred name for the family"@en ;
    rdfs:subPropertyOf <http://rdaregistry.info/Elements/a/P50061> ;
    skos:definition "Met une famille en relation avec le nom ou la forme de nom choisie pour identifier la famille."@fr, "Relates a family to a name or form of name chosen to identify a family."@en .

<http://rdaregistry.info/Elements/a/P50066>
    rdakit:instructionNumber "18.5" ;
    rdakit:toolkitDefinition "An item donated to another owner."@en, "Ancien propriétaire d’un item qui a fait don de cet item à un autre propriétaire."@fr ;
    rdakit:toolkitLabel "donateur de"@fr, "donor of"@en ;
    reg:hasSubproperty <http://rdaregistry.info/Elements/a/datatype/P50066>, <http://rdaregistry.info/Elements/a/object/P50066> ;
    reg:hasUnconstrained <http://rdaregistry.info/Elements/u/P60012> ;
    reg:lexicalAlias <http://rdaregistry.info/Elements/a/donorOf.en> ;
    reg:name "donorOf"@en ;
    reg:status <http://metadataregistry.org/uri/RegStatus/1001> ;
    a rdf:Property ;
    rdfs:domain <http://rdaregistry.info/Elements/c/C10002> ;
    rdfs:isDefinedBy <http://rdaregistry.info/Elements/a/> ;
    rdfs:label "est le donateur de"@fr, "is donor of"@en ;
    rdfs:subPropertyOf <http://rdaregistry.info/Elements/a/P50163> ;
    skos:definition "Met un ancien propriétaire d’un item qui a fait don de cet item à un autre propriétaire en relation avec l’item."@fr, "Relates a former owner of an item who donated that item to another owner to an item."@en .

<http://rdaregistry.info/Elements/a/P50067>
    rdakit:instructionNumber "18.5" ;
    rdakit:toolkitDefinition "An item sold to another owner."@en, "Ancien propriétaire d’un item qui a vendu cet item à un autre propriétaire."@fr ;
    rdakit:toolkitLabel "seller of"@en, "vendeur de"@fr ;
    reg:hasSubproperty <http://rdaregistry.info/Elements/a/datatype/P50067>, <http://rdaregistry.info/Elements/a/object/P50067> ;
    reg:hasUnconstrained <http://rdaregistry.info/Elements/u/P60013> ;
    reg:lexicalAlias <http://rdaregistry.info/Elements/a/sellerOf.en> ;
    reg:name "sellerOf"@en ;
    reg:status <http://metadataregistry.org/uri/RegStatus/1001> ;
    a rdf:Property ;
    rdfs:domain <http://rdaregistry.info/Elements/c/C10002> ;
    rdfs:isDefinedBy <http://rdaregistry.info/Elements/a/> ;
    rdfs:label "est le vendeur de"@fr, "is seller of"@en ;
    rdfs:subPropertyOf <http://rdaregistry.info/Elements/a/P50163> ;
    skos:definition "Met un ancien propriétaire d’un item qui a vendu cet item à un autre propriétaire en relation avec l’item."@fr, "Relates a former owner of an item who sold that item to another owner to an item."@en .

<http://rdaregistry.info/Elements/a/P50068>
    rdakit:instructionNumber "18.5" ;
    rdakit:toolkitDefinition "A work enacting a law, regulation, constitution, court rule, etc."@en, "Juridiction promulguant une loi, un règlement, une constitution, une règle de pratique de tribunal, etc."@fr ;
    rdakit:toolkitLabel "enacting jurisdiction of"@en, "juridiction promulgatrice de"@fr ;
    reg:hasSubproperty <http://rdaregistry.info/Elements/a/datatype/P50068>, <http://rdaregistry.info/Elements/a/object/P50068> ;
    reg:hasUnconstrained <http://rdaregistry.info/Elements/u/P60014> ;
    reg:lexicalAlias <http://rdaregistry.info/Elements/a/enactingJurisdictionOf.en> ;
    reg:name "enactingJurisdictionOf"@en ;
    reg:status <http://metadataregistry.org/uri/RegStatus/1001> ;
    a rdf:Property ;
    rdfs:domain <http://rdaregistry.info/Elements/c/C10005> ;
    rdfs:isDefinedBy <http://rdaregistry.info/Elements/a/> ;
    rdfs:label "est la juridiction promulgatrice de"@fr, "is enacting jurisdiction of"@en ;
    rdfs:subPropertyOf <http://rdaregistry.info/Elements/a/P50204> ;
    skos:definition "Met une juridiction promulguant une loi, un règlement, une constitution, une règle de pratique de tribunal, etc. en relation avec l’œuvre."@fr, "Relates a jurisdiction enacting a law, regulation, constitution, court rule, etc. to a work."@en .

<http://rdaregistry.info/Elements/a/P50069>
    rdakit:instructionNumber "18.5" ;
    rdakit:toolkitDefinition "A law, regulation, etc., that was enacted by another jurisdiction."@en, "Juridiction régie par une loi, un règlement, etc. qui a été promulgué par une autre juridiction."@fr ;
    rdakit:toolkitLabel "juridiction régie de"@fr, "jurisdiction governed of"@en ;
    reg:hasSubproperty <http://rdaregistry.info/Elements/a/datatype/P50069>, <http://rdaregistry.info/Elements/a/object/P50069> ;
    reg:hasUnconstrained <http://rdaregistry.info/Elements/u/P60015> ;
    reg:lexicalAlias <http://rdaregistry.info/Elements/a/jurisdictionGovernedOf.en> ;
    reg:name "jurisdictionGovernedOf"@en ;
    reg:status <http://metadataregistry.org/uri/RegStatus/1001> ;
    a rdf:Property ;
    rdfs:domain <http://rdaregistry.info/Elements/c/C10005> ;
    rdfs:isDefinedBy <http://rdaregistry.info/Elements/a/> ;
    rdfs:label "est la juridiction régie de"@fr, "is jurisdiction governed of"@en ;
    rdfs:subPropertyOf <http://rdaregistry.info/Elements/a/P50131> ;
    skos:definition "Met une juridiction régie par une loi, un règlement, etc. qui a été promulgué par une autre juridiction en relation avec l’œuvre."@fr, "Relates a jurisdiction governed by a law, regulation, etc., that was enacted by another jurisdiction to a work."@en .

<http://rdaregistry.info/Elements/a/P50070>
    rdakit:instructionNumber "18.5" ;
    rdakit:toolkitDefinition "An expression of a musical work that incorporates a performance of leading of a performing group in a musical or dramatic presentation, etc."@en, "Interprète contribuant à une expression d’une œuvre musicale en dirigeant un groupe d’interprètes (orchestre, chorale, opéra, etc.) dans une représentation musicale ou dramatique, etc."@fr ;
    rdakit:toolkitLabel "chef d’orchestre de"@fr, "conductor of"@en ;
    reg:hasSubproperty <http://rdaregistry.info/Elements/a/datatype/P50070>, <http://rdaregistry.info/Elements/a/object/P50070>, <http://rdaregistry.info/Elements/a/object/P50268>, <http://rdaregistry.info/Elements/a/object/P50269> ;
    reg:hasUnconstrained <http://rdaregistry.info/Elements/u/P60016> ;
    reg:lexicalAlias <http://rdaregistry.info/Elements/a/conductorOf.en> ;
    reg:name "conductorOf"@en ;
    reg:status <http://metadataregistry.org/uri/RegStatus/1001> ;
    a rdf:Property ;
    rdfs:domain <http://rdaregistry.info/Elements/c/C10002> ;
    rdfs:isDefinedBy <http://rdaregistry.info/Elements/a/> ;
    rdfs:label "est le chef d’orchestre de"@fr, "is conductor of"@en ;
    rdfs:subPropertyOf <http://rdaregistry.info/Elements/a/P50147> ;
    skos:definition "Met un interprète contribuant à une expression d’une œuvre musicale en dirigeant un groupe d’interprètes (orchestre, chorale, opéra, etc.) dans une représentation musicale ou dramatique, etc. en relation avec l’expression."@fr, "Relates a performer contributing to an expression of a musical work by leading a performing group in a musical or dramatic presentation, etc. to an expression."@en .

<http://rdaregistry.info/Elements/a/P50071>
    rdakit:instructionNumber "18.5" ;
    rdakit:toolkitDefinition "An expression of a work that incorporates a performance of acting as a cast member or player in a musical or dramatic presentation, etc."@en, "Interprète contribuant à une expression d’une œuvre en agissant à titre de membre d’une distribution artistique ou de comédien dans une représentation musicale ou dramatique, etc."@fr ;
    rdakit:toolkitLabel "acteur de"@fr, "actor of"@en ;
    reg:hasSubproperty <http://rdaregistry.info/Elements/a/P50217>, <http://rdaregistry.info/Elements/a/datatype/P50071>, <http://rdaregistry.info/Elements/a/object/P50071> ;
    reg:hasUnconstrained <http://rdaregistry.info/Elements/u/P60017> ;
    reg:lexicalAlias <http://rdaregistry.info/Elements/a/actorOf.en> ;
    reg:name "actorOf"@en ;
    reg:status <http://metadataregistry.org/uri/RegStatus/1001> ;
    a rdf:Property ;
    rdfs:domain <http://rdaregistry.info/Elements/c/C10002> ;
    rdfs:isDefinedBy <http://rdaregistry.info/Elements/a/> ;
    rdfs:label "est l’acteur de"@fr, "is actor of"@en ;
    rdfs:subPropertyOf <http://rdaregistry.info/Elements/a/P50147> ;
    skos:definition "Met un interprète contribuant à une expression d’une œuvre en agissant à titre de membre d’une distribution artistique ou de comédien dans une représentation musicale ou dramatique, etc. en relation avec l’expression."@fr, "Relates a performer contributing to an expression of a work by acting as a cast member or player in a musical or dramatic presentation, etc. to an expression."@en .

<http://rdaregistry.info/Elements/a/P50072>
    rdakit:instructionNumber "18.5" ;
    rdakit:seeAlso <http://rdaregistry.info/Elements/a/P50261> ;
    rdakit:toolkitDefinition "An expression of a work that incorporates a performance of appearing on screen to provide contextual or background information."@en, "Interprète contribuant à une expression d’une œuvre en apparaissant à l’écran pour fournir de l’information contextuelle ou complémentaire."@fr ;
    rdakit:toolkitLabel "on-screen presenter of"@en, "présentateur à l’écran de"@fr ;
    reg:hasSubproperty <http://rdaregistry.info/Elements/a/datatype/P50072>, <http://rdaregistry.info/Elements/a/object/P50072> ;
    reg:hasUnconstrained <http://rdaregistry.info/Elements/u/P60018> ;
    reg:lexicalAlias <http://rdaregistry.info/Elements/a/onScreenPresenterOf.en> ;
    reg:name "onScreenPresenterOf"@en ;
    reg:status <http://metadataregistry.org/uri/RegStatus/1001> ;
    a rdf:Property ;
    rdfs:domain <http://rdaregistry.info/Elements/c/C10002> ;
    rdfs:isDefinedBy <http://rdaregistry.info/Elements/a/> ;
    rdfs:label "est le présentateur à l’écran de"@fr, "is on-screen presenter of"@en ;
    rdfs:subPropertyOf <http://rdaregistry.info/Elements/a/P50147> ;
    skos:definition "Met un interprète contribuant à une expression d’une œuvre en apparaissant à l’écran pour fournir de l’information contextuelle ou complémentaire en relation avec l’expression."@fr, "Relates a performer contributing to an expression of a work by appearing on screen to provide contextual or background information to an expression."@en ;
    skos:scopeNote "An on-screen presenter may appear in nonfiction moving image materials or in introductions to fiction moving image materials."@en, "Un présentateur à l’écran peut apparaître dans des images animées de non fiction ou dans des introductions à des images animées de fiction."@fr .

<http://rdaregistry.info/Elements/a/P50073>
    rdakit:instructionNumber "18.5" ;
    rdakit:toolkitDefinition "An expression of a work that incorporates a performance of dancing in a musical, dramatic, etc., presentation."@en, "Interprète contribuant à une expression d’une œuvre en dansant dans une représentation musicale ou dramatique, etc."@fr ;
    rdakit:toolkitLabel "dancer of"@en, "danseur de"@fr ;
    reg:hasSubproperty <http://rdaregistry.info/Elements/a/datatype/P50073>, <http://rdaregistry.info/Elements/a/object/P50073> ;
    reg:hasUnconstrained <http://rdaregistry.info/Elements/u/P60019> ;
    reg:lexicalAlias <http://rdaregistry.info/Elements/a/dancerOf.en> ;
    reg:name "dancerOf"@en ;
    reg:status <http://metadataregistry.org/uri/RegStatus/1001> ;
    a rdf:Property ;
    rdfs:domain <http://rdaregistry.info/Elements/c/C10002> ;
    rdfs:isDefinedBy <http://rdaregistry.info/Elements/a/> ;
    rdfs:label "est le danseur de"@fr, "is dancer of"@en ;
    rdfs:subPropertyOf <http://rdaregistry.info/Elements/a/P50147> ;
    skos:definition "Met un interprète contribuant à une expression d’une œuvre en dansant dans une représentation musicale ou dramatique, etc. en relation avec l’expression."@fr, "Relates a performer contributing to an expression of a work by dancing in a musical, dramatic, etc., presentation to an expression."@en .

<http://rdaregistry.info/Elements/a/P50074>
    rdakit:instructionNumber "18.5" ;
    rdakit:toolkitDefinition "An expression of a work that incorporates a performance of giving instruction or providing a demonstration."@en, "Interprète contribuant à une expression d’une œuvre en transmettant des connaissances par la théorie ou la pratique."@fr ;
    rdakit:toolkitLabel "enseignant de"@fr, "teacher of"@en ;
    reg:hasSubproperty <http://rdaregistry.info/Elements/a/datatype/P50074>, <http://rdaregistry.info/Elements/a/object/P50074> ;
    reg:hasUnconstrained <http://rdaregistry.info/Elements/u/P60020> ;
    reg:lexicalAlias <http://rdaregistry.info/Elements/a/teacherOf.en> ;
    reg:name "teacherOf"@en ;
    reg:status <http://metadataregistry.org/uri/RegStatus/1001> ;
    a rdf:Property ;
    rdfs:domain <http://rdaregistry.info/Elements/c/C10002> ;
    rdfs:isDefinedBy <http://rdaregistry.info/Elements/a/> ;
    rdfs:label "est l’enseignant de"@fr, "is teacher of"@en ;
    rdfs:subPropertyOf <http://rdaregistry.info/Elements/a/P50147> ;
    skos:definition "Met un interprète contribuant à une expression d’une œuvre en transmettant des connaissances par la théorie ou la pratique en relation avec l’expression."@fr, "Relates a performer contributing to an expression of a work by giving instruction or providing a demonstration to an expression."@en .

<http://rdaregistry.info/Elements/a/P50075>
    rdakit:instructionNumber "18.5" ;
    rdakit:toolkitDefinition "An expression of a work that incorporates a performance of leading a program, often broadcast, that includes other guests, performers, etc."@en, "Interprète contribuant à une expression d’une œuvre en dirigeant une émission (souvent diffusée) qui comprend d’autres invités, interprètes, etc. (par exemple, un animateur d’émission-débat)."@fr ;
    rdakit:toolkitLabel "host of"@en, "hôte de"@fr ;
    reg:hasSubproperty <http://rdaregistry.info/Elements/a/datatype/P50075>, <http://rdaregistry.info/Elements/a/object/P50075> ;
    reg:hasUnconstrained <http://rdaregistry.info/Elements/u/P60021> ;
    reg:lexicalAlias <http://rdaregistry.info/Elements/a/hostOf.en> ;
    reg:name "hostOf"@en ;
    reg:status <http://metadataregistry.org/uri/RegStatus/1001> ;
    a rdf:Property ;
    rdfs:domain <http://rdaregistry.info/Elements/c/C10002> ;
    rdfs:isDefinedBy <http://rdaregistry.info/Elements/a/> ;
    rdfs:label "est l’hôte de"@fr, "is host of"@en ;
    rdfs:subPropertyOf <http://rdaregistry.info/Elements/a/P50147> ;
    skos:definition "Met un interprète contribuant à une expression d’une œuvre en dirigeant une émission (souvent diffusée) qui comprend d’autres invités, interprètes, etc. (par exemple, un animateur d’émission-débat) en relation avec l’expression."@fr, "Relates a performer contributing to an expression of a work by leading a program, often broadcast, that includes other guests, performers, etc., to an expression."@en .

<http://rdaregistry.info/Elements/a/P50076>
    rdakit:instructionNumber "18.5" ;
    rdakit:toolkitDefinition "An expression of a work that incorporates a performance of leading a program, often broadcast, where topics are discussed, usually with participation of experts in fields related to the discussion."@en, "Interprète contribuant à une expression d’une œuvre en dirigeant une émission (souvent diffusée) où des sujets sont discutés, habituellement avec la participation d’experts dans les domaines reliés à la discussion."@fr ;
    rdakit:toolkitLabel "moderator of"@en, "modérateur de"@fr ;
    reg:hasSubproperty <http://rdaregistry.info/Elements/a/datatype/P50076>, <http://rdaregistry.info/Elements/a/object/P50076> ;
    reg:hasUnconstrained <http://rdaregistry.info/Elements/u/P60022> ;
    reg:lexicalAlias <http://rdaregistry.info/Elements/a/moderatorOf.en> ;
    reg:name "moderatorOf"@en ;
    reg:status <http://metadataregistry.org/uri/RegStatus/1001> ;
    a rdf:Property ;
    rdfs:domain <http://rdaregistry.info/Elements/c/C10002> ;
    rdfs:isDefinedBy <http://rdaregistry.info/Elements/a/> ;
    rdfs:label "est le modérateur de"@fr, "is moderator of"@en ;
    rdfs:subPropertyOf <http://rdaregistry.info/Elements/a/P50147> ;
    skos:definition "Met un interprète contribuant à une expression d’une œuvre en dirigeant une émission (souvent diffusée) où des sujets sont discutés, habituellement avec la participation d’experts dans les domaines reliés à la discussion en relation avec l’expression."@fr, "Relates a performer contributing to an expression of a work by leading a program, often broadcast, where topics are discussed, usually with participation of experts in fields related to the discussion to an expression."@en .

<http://rdaregistry.info/Elements/a/P50077>
    rdakit:instructionNumber "18.5" ;
    rdakit:toolkitDefinition "An expression of a work that incorporates a performance of manipulating, controlling, or directing puppets or marionettes in a moving image production or a musical or dramatic presentation or entertainment."@en, "Interprète contribuant à une expression d’une œuvre en manipulant, en contrôlant ou en dirigeant des marionnettes dans une production d’images animées ou bien dans une représentation ou un spectacle musical ou dramatique."@fr ;
    rdakit:toolkitLabel "marionnettiste de"@fr, "puppeteer of"@en ;
    reg:hasSubproperty <http://rdaregistry.info/Elements/a/datatype/P50077>, <http://rdaregistry.info/Elements/a/object/P50077> ;
    reg:hasUnconstrained <http://rdaregistry.info/Elements/u/P60023> ;
    reg:lexicalAlias <http://rdaregistry.info/Elements/a/puppeteerOf.en> ;
    reg:name "puppeteerOf"@en ;
    reg:status <http://metadataregistry.org/uri/RegStatus/1001> ;
    a rdf:Property ;
    rdfs:domain <http://rdaregistry.info/Elements/c/C10002> ;
    rdfs:isDefinedBy <http://rdaregistry.info/Elements/a/> ;
    rdfs:label "est le marionnettiste de"@fr, "is puppeteer of"@en ;
    rdfs:subPropertyOf <http://rdaregistry.info/Elements/a/P50147> ;
    skos:definition "Met un interprète contribuant à une expression d’une œuvre en manipulant, en contrôlant ou en dirigeant des marionnettes dans une production d’images animées ou bien dans une représentation ou un spectacle musical ou dramatique en relation avec l’expression."@fr, "Relates a performer contributing to an expression of a work by manipulating, controlling, or directing puppets or marionettes in a moving image production or a musical or dramatic presentation or entertainment to an expression."@en .

<http://rdaregistry.info/Elements/a/P50078>
    rdakit:instructionNumber "18.5" ;
    rdakit:toolkitDefinition "An expression of a work that incorporates a performance of participating in a program, often broadcast, where topics are discussed, usually with participation of experts in fields related to the discussion."@en, "Interprète contribuant à une expression d’une œuvre en participant à une émission (souvent diffusée) où des sujets sont discutés, habituellement avec la participation d’experts dans les domaines reliés à la discussion."@fr ;
    rdakit:toolkitLabel "panelist of"@en, "panéliste de"@fr ;
    reg:hasSubproperty <http://rdaregistry.info/Elements/a/datatype/P50078>, <http://rdaregistry.info/Elements/a/object/P50078> ;
    reg:hasUnconstrained <http://rdaregistry.info/Elements/u/P60024> ;
    reg:lexicalAlias <http://rdaregistry.info/Elements/a/panelistOf.en> ;
    reg:name "panelistOf"@en ;
    reg:status <http://metadataregistry.org/uri/RegStatus/1001> ;
    a rdf:Property ;
    rdfs:domain <http://rdaregistry.info/Elements/c/C10002> ;
    rdfs:isDefinedBy <http://rdaregistry.info/Elements/a/> ;
    rdfs:label "est le panéliste de"@fr, "is panelist of"@en ;
    rdfs:subPropertyOf <http://rdaregistry.info/Elements/a/P50147> ;
    skos:definition "Met un interprète contribuant à une expression d’une œuvre en participant à une émission (souvent diffusée) où des sujets sont discutés, habituellement avec la participation d’experts dans les domaines reliés à la discussion en relation avec l’expression."@fr, "Relates a performer contributing to an expression of a work by participating in a program, often broadcast, where topics are discussed, usually with participation of experts in fields related to the discussion to an expression."@en .

<http://rdaregistry.info/Elements/a/P50079>
    rdakit:instructionNumber "18.5" ;
    rdakit:toolkitDefinition "An expression of a work that incorporates a performance of playing a musical instrument."@en, "Interprète contribuant à une expression d’une œuvre en jouant d’un instrument de musique."@fr ;
    rdakit:toolkitLabel "instrumentalist of"@en, "instrumentiste de"@fr ;
    reg:hasSubproperty <http://rdaregistry.info/Elements/a/datatype/P50079>, <http://rdaregistry.info/Elements/a/object/P50079> ;
    reg:hasUnconstrained <http://rdaregistry.info/Elements/u/P60025> ;
    reg:lexicalAlias <http://rdaregistry.info/Elements/a/instrumentalistOf.en> ;
    reg:name "instrumentalistOf"@en ;
    reg:status <http://metadataregistry.org/uri/RegStatus/1001> ;
    a rdf:Property ;
    rdfs:domain <http://rdaregistry.info/Elements/c/C10002> ;
    rdfs:isDefinedBy <http://rdaregistry.info/Elements/a/> ;
    rdfs:label "est l’instrumentiste de"@fr, "is instrumentalist of"@en ;
    rdfs:subPropertyOf <http://rdaregistry.info/Elements/a/P50147> ;
    skos:definition "Met un interprète contribuant à une expression d’une œuvre en jouant d’un instrument de musique en relation avec l’expression."@fr, "Relates a performer contributing to an expression of a work by playing a musical instrument to an expression."@en .

<http://rdaregistry.info/Elements/a/P50080>
    rdakit:instructionNumber "18.5" ;
    rdakit:toolkitDefinition "An expression of a work that incorporates a performance of providing interpretation, analysis, or a discussion of the subject matter on a recording, film, or other audiovisual medium."@en, "Interprète contribuant à une expression d’une œuvre en fournissant une interprétation, une analyse ou une explication du sujet sur un enregistrement, un film ou un autre support audiovisuel."@fr ;
    rdakit:toolkitLabel "commentateur de"@fr, "commentator of"@en ;
    reg:hasSubproperty <http://rdaregistry.info/Elements/a/datatype/P50080>, <http://rdaregistry.info/Elements/a/object/P50080> ;
    reg:hasUnconstrained <http://rdaregistry.info/Elements/u/P60026> ;
    reg:lexicalAlias <http://rdaregistry.info/Elements/a/commentatorOf.en> ;
    reg:name "commentatorOf"@en ;
    reg:status <http://metadataregistry.org/uri/RegStatus/1001> ;
    a rdf:Property ;
    rdfs:domain <http://rdaregistry.info/Elements/c/C10002> ;
    rdfs:isDefinedBy <http://rdaregistry.info/Elements/a/> ;
    rdfs:label "est le commentateur de"@fr, "is commentator of"@en ;
    rdfs:subPropertyOf <http://rdaregistry.info/Elements/a/P50147> ;
    skos:definition "Met un interprète contribuant à une expression d’une œuvre en fournissant une interprétation, une analyse ou une explication du sujet sur un enregistrement, un film ou un autre support audiovisuel en relation avec l’expression."@fr, "Relates a performer contributing to an expression of a work by providing interpretation, analysis, or a discussion of the subject matter on a recording, film, or other audiovisual medium to an expression."@en .

<http://rdaregistry.info/Elements/a/P50081>
    rdakit:instructionNumber "18.5" ;
    rdakit:toolkitDefinition "An expression of a work that incorporates a performance of reading aloud or giving an account of an act, occurrence, course of events, etc."@en, "Interprète contribuant à une expression d’une œuvre en lisant à voix haute ou en rendant compte d’une action, d’une situation, du déroulement des événements, etc."@fr ;
    rdakit:toolkitLabel "narrateur de"@fr, "narrator of"@en ;
    reg:hasSubproperty <http://rdaregistry.info/Elements/a/datatype/P50081>, <http://rdaregistry.info/Elements/a/object/P50081> ;
    reg:hasUnconstrained <http://rdaregistry.info/Elements/u/P60028> ;
    reg:lexicalAlias <http://rdaregistry.info/Elements/a/narratorOf.en> ;
    reg:name "narratorOf"@en ;
    reg:status <http://metadataregistry.org/uri/RegStatus/1001> ;
    a rdf:Property ;
    rdfs:domain <http://rdaregistry.info/Elements/c/C10002> ;
    rdfs:isDefinedBy <http://rdaregistry.info/Elements/a/> ;
    rdfs:label "est le narrateur de"@fr, "is narrator of"@en ;
    rdfs:subPropertyOf <http://rdaregistry.info/Elements/a/P50147> ;
    skos:definition "Met un interprète contribuant à une expression d’une œuvre en lisant à voix haute ou en rendant compte d’une action, d’une situation, du déroulement des événements, etc. en relation avec l’expression."@fr, "Relates a performer contributing to an expression of a work by reading aloud or giving an account of an act, occurrence, course of events, etc. to an expression."@en .

<http://rdaregistry.info/Elements/a/P50082>
    rdakit:instructionNumber "18.5" ;
    rdakit:toolkitDefinition "An expression of a work that incorporates a performance of relaying a creator's original story with dramatic or theatrical interpretation."@en, "Interprète contribuant à une expression d’une œuvre en racontant l’histoire originale d’un créateur dans une interprétation dramatique ou théâtrale."@fr ;
    rdakit:toolkitLabel "conteur de"@fr, "storyteller of"@en ;
    reg:hasSubproperty <http://rdaregistry.info/Elements/a/datatype/P50082>, <http://rdaregistry.info/Elements/a/object/P50082> ;
    reg:hasUnconstrained <http://rdaregistry.info/Elements/u/P60029> ;
    reg:lexicalAlias <http://rdaregistry.info/Elements/a/storytellerOf.en> ;
    reg:name "storytellerOf"@en ;
    reg:status <http://metadataregistry.org/uri/RegStatus/1001> ;
    a rdf:Property ;
    rdfs:domain <http://rdaregistry.info/Elements/c/C10002> ;
    rdfs:isDefinedBy <http://rdaregistry.info/Elements/a/> ;
    rdfs:label "est le conteur de"@fr, "is storyteller of"@en ;
    rdfs:subPropertyOf <http://rdaregistry.info/Elements/a/P50147> ;
    skos:definition "Met un interprète contribuant à une expression d’une œuvre en racontant l’histoire originale d’un créateur dans une interprétation dramatique ou théâtrale en relation avec l’expression."@fr, "Relates a performer contributing to an expression of a work by relaying a creator's original story with dramatic or theatrical interpretation to an expression."@en .

<http://rdaregistry.info/Elements/a/P50083>
    rdakit:instructionNumber "18.5" ;
    rdakit:toolkitDefinition "An expression of a work that incorporates a performance of speaking words, such as a lecture, speech, etc."@en, "Interprète contribuant à une expression d’une œuvre en énonçant des paroles, telles qu’un exposé, un discours, etc."@fr ;
    rdakit:toolkitLabel "orateur de"@fr, "speaker of"@en ;
    reg:hasSubproperty <http://rdaregistry.info/Elements/a/datatype/P50083>, <http://rdaregistry.info/Elements/a/object/P50083> ;
    reg:hasUnconstrained <http://rdaregistry.info/Elements/u/P60030> ;
    reg:lexicalAlias <http://rdaregistry.info/Elements/a/speakerOf.en> ;
    reg:name "speakerOf"@en ;
    reg:status <http://metadataregistry.org/uri/RegStatus/1001> ;
    a rdf:Property ;
    rdfs:domain <http://rdaregistry.info/Elements/c/C10002> ;
    rdfs:isDefinedBy <http://rdaregistry.info/Elements/a/> ;
    rdfs:label "est l’orateur de"@fr, "is speaker of"@en ;
    rdfs:subPropertyOf <http://rdaregistry.info/Elements/a/P50147> ;
    skos:definition "Met un interprète contribuant à une expression d’une œuvre en énonçant des paroles, telles qu’un exposé, un discours, etc., en relation avec l’expression."@fr, "Relates a performer contributing to an expression of a work by speaking words, such as a lecture, speech, etc. to an expression."@en .

<http://rdaregistry.info/Elements/a/P50084>
    rdakit:instructionNumber "18.5" ;
    rdakit:toolkitDefinition "An expression of a work that incorporates a performance of using his/her/their voice, with or without instrumental accompaniment, to produce music."@en, "Interprète contribuant à une expression d’une œuvre en utilisant sa voix, avec ou sans accompagnement instrumental, pour produire de la musique."@fr ;
    rdakit:toolkitLabel "chanteur de"@fr, "singer of"@en ;
    reg:hasSubproperty <http://rdaregistry.info/Elements/a/datatype/P50084>, <http://rdaregistry.info/Elements/a/object/P50084> ;
    reg:hasUnconstrained <http://rdaregistry.info/Elements/u/P60031> ;
    reg:lexicalAlias <http://rdaregistry.info/Elements/a/singerOf.en> ;
    reg:name "singerOf"@en ;
    reg:status <http://metadataregistry.org/uri/RegStatus/1001> ;
    a rdf:Property ;
    rdfs:domain <http://rdaregistry.info/Elements/c/C10002> ;
    rdfs:isDefinedBy <http://rdaregistry.info/Elements/a/> ;
    rdfs:label "est le chanteur de"@fr, "is singer of"@en ;
    rdfs:subPropertyOf <http://rdaregistry.info/Elements/a/P50147> ;
    skos:definition "Met un interprète contribuant à une expression d’une œuvre en utilisant sa voix, avec ou sans accompagnement instrumental, pour produire de la musique en relation avec l’expression."@fr, "Relates a performer contributing to an expression of a work by using his/her/their voice, with or without instrumental accompaniment, to produce music to an expression."@en ;
    skos:scopeNote "A singer's performance may or may not include actual words."@en, "La prestation d’un chanteur peut inclure ou non des paroles."@fr .

<http://rdaregistry.info/Elements/a/P50085>
    rdakit:instructionNumber "18.5" ;
    rdakit:toolkitDefinition "A legal work of a higher court recording a decision of a lower court that appeals against a person."@en, "Personne contre laquelle un appel a été formé."@fr ;
    rdakit:toolkitLabel "appellee person of"@en, "personne intimée de"@fr ;
    reg:hasSubproperty <http://rdaregistry.info/Elements/a/datatype/P50085>, <http://rdaregistry.info/Elements/a/object/P50085> ;
    reg:hasUnconstrained <http://rdaregistry.info/Elements/u/P60601> ;
    reg:lexicalAlias <http://rdaregistry.info/Elements/a/appelleePersonOf.en> ;
    reg:name "appelleePersonOf"@en ;
    reg:status <http://metadataregistry.org/uri/RegStatus/1001> ;
    a rdf:Property ;
    rdfs:domain <http://rdaregistry.info/Elements/c/C10004> ;
    rdfs:isDefinedBy <http://rdaregistry.info/Elements/a/> ;
    rdfs:label "est la personne intimée de"@fr, "is appellee person of"@en ;
    rdfs:subPropertyOf <http://rdaregistry.info/Elements/a/P50087> ;
    skos:definition "Met une personne contre laquelle un appel a été formé en relation avec l’œuvre."@fr, "Relates a person against whom an appeal is taken on a decision of a lower court recorded in a legal work of a higher court to a work."@en .

<http://rdaregistry.info/Elements/a/P50086>
    rdakit:instructionNumber "18.5" ;
    rdakit:toolkitDefinition "A work that involves a responsibility for a communication between the earthly world and a world of spirits."@en, "Personne tenue pour être un canal de communication entre le monde terrestre et le monde des esprits."@fr ;
    rdakit:toolkitLabel "medium of"@en, "médium de"@fr ;
    reg:hasSubproperty <http://rdaregistry.info/Elements/a/datatype/P50086>, <http://rdaregistry.info/Elements/a/object/P50086> ;
    reg:hasUnconstrained <http://rdaregistry.info/Elements/u/P60032> ;
    reg:lexicalAlias <http://rdaregistry.info/Elements/a/mediumOf.en> ;
    reg:name "mediumOf"@en ;
    reg:status <http://metadataregistry.org/uri/RegStatus/1001> ;
    a rdf:Property ;
    rdfs:domain <http://rdaregistry.info/Elements/c/C10004> ;
    rdfs:isDefinedBy <http://rdaregistry.info/Elements/a/> ;
    rdfs:label "est le médium de"@fr, "is medium of"@en ;
    rdfs:subPropertyOf <http://rdaregistry.info/Elements/a/P50131> ;
    skos:definition "Met une personne tenue pour être un canal de communication entre le monde terrestre et le monde des esprits en relation avec l’œuvre."@fr, "Relates a person held to be a channel of communication between the earthly world and a world of spirits to a work."@en .

<http://rdaregistry.info/Elements/a/P50087>
    rdakit:instructionNumber "18.5" ;
    rdakit:toolkitDefinition "A legal work of a higher court recording a decision of a lower court that appeals against a person or corporate body."@en, "Personne ou collectivité contre laquelle un appel a été formé."@fr ;
    rdakit:toolkitLabel "appellee of"@en, "intimé de"@fr ;
    reg:hasSubproperty <http://rdaregistry.info/Elements/a/P50085>, <http://rdaregistry.info/Elements/a/datatype/P50087>, <http://rdaregistry.info/Elements/a/object/P50087> ;
    reg:hasUnconstrained <http://rdaregistry.info/Elements/u/P60601> ;
    reg:lexicalAlias <http://rdaregistry.info/Elements/a/appelleeOf.en> ;
    reg:name "appelleeOf"@en ;
    reg:status <http://metadataregistry.org/uri/RegStatus/1001> ;
    a rdf:Property ;
    rdfs:isDefinedBy <http://rdaregistry.info/Elements/a/> ;
    rdfs:label "est l’intimé de"@fr, "is appellee of"@en ;
    rdfs:subPropertyOf <http://rdaregistry.info/Elements/a/P50131> ;
    skos:definition "Met une personne ou collectivité contre laquelle un appel a été formé en relation avec l’œuvre."@fr, "Relates a person or corporate body against whom an appeal is taken on a decision of a lower court recorded in a legal work of a higher court to a work."@en .

<http://rdaregistry.info/Elements/a/P50088>
    rdakit:instructionNumber "18.5" ;
    rdakit:toolkitDefinition "A legal work of a higher court recording a decision of a lower court that is appealed by a person or corporate body."@en, "Personne ou collectivité qui en appelle de la décision d’un tribunal inférieur."@fr ;
    rdakit:toolkitLabel "appelant de"@fr, "appellant of"@en ;
    reg:hasSubproperty <http://rdaregistry.info/Elements/a/P50042>, <http://rdaregistry.info/Elements/a/datatype/P50088>, <http://rdaregistry.info/Elements/a/object/P50088>, <http://rdaregistry.info/Elements/a/object/P50122> ;
    reg:hasUnconstrained <http://rdaregistry.info/Elements/u/P60691> ;
    reg:lexicalAlias <http://rdaregistry.info/Elements/a/appellantOf.en> ;
    reg:name "appellantOf"@en ;
    reg:status <http://metadataregistry.org/uri/RegStatus/1001> ;
    a rdf:Property ;
    rdfs:isDefinedBy <http://rdaregistry.info/Elements/a/> ;
    rdfs:label "est l’appelant de"@fr, "is appellant of"@en ;
    rdfs:subPropertyOf <http://rdaregistry.info/Elements/a/P50131> ;
    skos:definition "Met une personne ou collectivité qui en appelle de la décision d’un tribunal inférieur en relation avec l’œuvre."@fr, "Relates a person or corporate body who appeals the decision of a lower court recorded in a legal work of a higher court to a work."@en .

<http://rdaregistry.info/Elements/a/P50089>
    rdakit:instructionNumber "18.5" ;
    rdakit:toolkitDefinition "A work that involves a responsibility for bringing a suit in a civil proceeding by a person or corporate body."@en, "Personne ou collectivité qui intente une poursuite civile."@fr ;
    rdakit:toolkitLabel "demandeur de"@fr, "plaintiff of"@en ;
    reg:hasSubproperty <http://rdaregistry.info/Elements/a/P50043>, <http://rdaregistry.info/Elements/a/P50124>, <http://rdaregistry.info/Elements/a/datatype/P50089>, <http://rdaregistry.info/Elements/a/object/P50089> ;
    reg:hasUnconstrained <http://rdaregistry.info/Elements/u/P60693> ;
    reg:lexicalAlias <http://rdaregistry.info/Elements/a/plaintiffOf.en> ;
    reg:name "plaintiffOf"@en ;
    reg:status <http://metadataregistry.org/uri/RegStatus/1001> ;
    a rdf:Property ;
    rdfs:isDefinedBy <http://rdaregistry.info/Elements/a/> ;
    rdfs:label "est le demandeur de"@fr, "is plaintiff of"@en ;
    rdfs:subPropertyOf <http://rdaregistry.info/Elements/a/P50131> ;
    skos:definition "Met une personne ou collectivité qui intente une poursuite civile en relation avec l’œuvre."@fr, "Relates a person or corporate body who brings a suit in a civil proceeding to a work."@en .

<http://rdaregistry.info/Elements/a/P50090>
    rdakit:instructionNumber "18.5" ;
    rdakit:toolkitDefinition "A work that involves a responsibility for being a person or corporate body accused in a criminal proceeding or sued in a civil proceeding."@en, "Personne ou collectivité qui est accusée dans une poursuite criminelle ou contre laquelle une poursuite civile est intentée."@fr ;
    rdakit:toolkitLabel "defendant of"@en, "défendeur de"@fr ;
    reg:hasSubproperty <http://rdaregistry.info/Elements/a/datatype/P50090>, <http://rdaregistry.info/Elements/a/object/P50090>, <http://rdaregistry.info/Elements/a/object/P50258>, <http://rdaregistry.info/Elements/a/object/P50259> ;
    reg:hasUnconstrained <http://rdaregistry.info/Elements/u/P60698> ;
    reg:lexicalAlias <http://rdaregistry.info/Elements/a/defendantOf.en> ;
    reg:name "defendantOf"@en ;
    reg:status <http://metadataregistry.org/uri/RegStatus/1001> ;
    a rdf:Property ;
    rdfs:isDefinedBy <http://rdaregistry.info/Elements/a/> ;
    rdfs:label "est le défendeur de"@fr, "is defendant of"@en ;
    rdfs:subPropertyOf <http://rdaregistry.info/Elements/a/P50131> ;
    skos:definition "Met une personne ou collectivité qui est accusée dans une poursuite criminelle ou contre laquelle une poursuite civile est intentée en relation avec l’œuvre."@fr, "Relates a person or corporate body who is accused in a criminal proceeding or sued in a civil proceeding to a work."@en .

<http://rdaregistry.info/Elements/a/P50091>
    rdakit:instructionNumber "18.5" ;
    rdakit:toolkitDefinition "A work that involves a responsibility as an advisor or supervisor of thesis or dissertation research, overseeing either an academic degree or thesis."@en, "Personne supervisant un diplôme universitaire de niveau supérieur."@fr ;
    rdakit:toolkitLabel "degree supervisor of"@en, "superviseur académique de"@fr ;
    reg:hasSubproperty <http://rdaregistry.info/Elements/a/datatype/P50091>, <http://rdaregistry.info/Elements/a/object/P50091> ;
    reg:hasUnconstrained <http://rdaregistry.info/Elements/u/P60649> ;
    reg:lexicalAlias <http://rdaregistry.info/Elements/a/degreeSupervisorOf.en> ;
    reg:name "degreeSupervisorOf"@en ;
    reg:status <http://metadataregistry.org/uri/RegStatus/1001> ;
    a rdf:Property ;
    rdfs:domain <http://rdaregistry.info/Elements/c/C10004> ;
    rdfs:isDefinedBy <http://rdaregistry.info/Elements/a/> ;
    rdfs:label "est le superviseur académique de"@fr, "is degree supervisor of"@en ;
    rdfs:subPropertyOf <http://rdaregistry.info/Elements/a/P50131> ;
    skos:definition "Met une personne supervisant un diplôme universitaire de niveau supérieur en relation avec l’œuvre."@fr, "Relates a person, such as an advisor or supervisor of thesis or dissertation research, overseeing either an academic degree or thesis to a work."@en .

<http://rdaregistry.info/Elements/a/P50092>
    rdakit:instructionNumber "18.5" ;
    rdakit:toolkitDefinition "An item decorated using precious metals or color, often with elaborate designs and motifs."@en, "Personne ornant un item spécifique en utilisant des métaux précieux ou de la couleur, souvent avec des dessins et des motifs élaborés."@fr ;
    rdakit:toolkitLabel "enlumineur de"@fr, "illuminator of"@en ;
    reg:hasSubproperty <http://rdaregistry.info/Elements/a/datatype/P50092>, <http://rdaregistry.info/Elements/a/object/P50092> ;
    reg:hasUnconstrained <http://rdaregistry.info/Elements/u/P60650> ;
    reg:lexicalAlias <http://rdaregistry.info/Elements/a/illuminatorOf.en> ;
    reg:name "illuminatorOf"@en ;
    reg:status <http://metadataregistry.org/uri/RegStatus/1001> ;
    a rdf:Property ;
    rdfs:domain <http://rdaregistry.info/Elements/c/C10004> ;
    rdfs:isDefinedBy <http://rdaregistry.info/Elements/a/> ;
    rdfs:label "est l’enlumineur de"@fr, "is illuminator of"@en ;
    rdfs:subPropertyOf <http://rdaregistry.info/Elements/a/P50182> ;
    skos:definition "Met une personne ornant un item spécifique en utilisant des métaux précieux ou de la couleur, souvent avec des dessins et des motifs élaborés, en relation avec l’item."@fr, "Relates a person providing decoration to a specific item using precious metals or color, often with elaborate designs and motifs to an item."@en .

<http://rdaregistry.info/Elements/a/P50093>
    rdakit:instructionNumber "8.11" ;
    rdakit:toolkitDefinition "A categorization indicating that the core elements recorded are insufficient to differentiate between two or more persons with the same name."@en, "Catégorisation indiquant que les éléments fondamentaux enregistrés sont insuffisants pour distinguer deux ou plusieurs personnes portant le même nom."@fr, "Una categorización que indica que los elementos núcleo registrados son insuficientes para diferenciar dos o más personas con el mismo nombre."@es ;
    rdakit:toolkitLabel "indicador de nombre no diferenciado"@es, "indicateur de nom indifférencié"@fr, "indikator för odifferentierat namn"@sv, "undifferentiated name indicator"@en ;
    reg:hasSubproperty <http://rdaregistry.info/Elements/a/datatype/P50093> ;
    reg:hasUnconstrained <http://rdaregistry.info/Elements/u/P60046> ;
    reg:lexicalAlias <http://rdaregistry.info/Elements/a/undifferentiatedNameIndicator.en> ;
    reg:name "undifferentiatedNameIndicator"@en ;
    reg:status <http://metadataregistry.org/uri/RegStatus/1001> ;
    a rdf:Property ;
    rdfs:domain <http://rdaregistry.info/Elements/c/C10004> ;
    rdfs:isDefinedBy <http://rdaregistry.info/Elements/a/> ;
    rdfs:label "a pour indicateur de nom indifférencié"@fr, "har indikator för odifferentierat namn"@sv, "has undifferentiated name indicator"@en ;
    skos:definition "Met une personne en relation avec une catégorisation indiquant que les éléments fondamentaux enregistrés sont insuffisants pour distinguer deux ou plusieurs personnes portant le même nom."@fr, "Relates a person to a categorization indicating that the core elements recorded are insufficient to differentiate between two or more persons with the same name."@en .

<http://rdaregistry.info/Elements/a/P50094>
    rdakit:instructionNumber "9.18" ;
    rdakit:toolkitDefinition "A character string uniquely associated with a person, or with a surrogate such as an authority record for a person."@en, "Chaîne de caractères associée de manière unique à une personne ou à un substitut d’une personne (par exemple, une notice d’autorité)."@fr, "Una cadena de caracteres asociados de manera unívoca con una persona, o un sustituto de la persona (p.ej., un registro de autoridad)."@es ;
    rdakit:toolkitLabel "identifiant de la personne"@fr, "identificador de la persona"@es, "identifier for the person"@en, "identifikator för personen"@sv ;
    reg:hasSubproperty <http://rdaregistry.info/Elements/a/datatype/P50094> ;
    reg:hasUnconstrained <http://rdaregistry.info/Elements/u/P60053> ;
    reg:lexicalAlias <http://rdaregistry.info/Elements/a/identifierForThePerson.en> ;
    reg:name "identifierForThePerson"@en ;
    reg:status <http://metadataregistry.org/uri/RegStatus/1001> ;
    a rdf:Property ;
    rdfs:domain <http://rdaregistry.info/Elements/c/C10004> ;
    rdfs:isDefinedBy <http://rdaregistry.info/Elements/a/> ;
    rdfs:label "a pour identifiant de la personne"@fr, "har identifikator för personen"@sv, "has identifier for the person"@en ;
    skos:definition "Met une personne en relation avec une chaîne de caractères associée de manière unique à une personne ou à un substitut d’une personne (par exemple, une notice d’autorité)."@fr, "Relates a person to a character string uniquely associated with a person, or with a surrogate such as an authority record for a person."@en ;
    skos:scopeNote "L’identifiant sert à distinguer cette personne d’autres personnes."@fr, "The identifier serves to differentiate that person from other persons."@en .

<http://rdaregistry.info/Elements/a/P50095>
    rdakit:instructionNumber "29.5" ;
    rdakit:toolkitDefinition "A corporate body of which a person is a member."@en, "Collectivité (groupe d’interprètes, expédition, etc) dont la personne est membre."@fr, "Una entidad corporativa de la cual es miembro una persona."@es ;
    rdakit:toolkitLabel "collectivité"@fr, "corporate body"@en, "entidad corporativa"@es ;
    reg:hasSubproperty <http://rdaregistry.info/Elements/a/datatype/P50095>, <http://rdaregistry.info/Elements/a/object/P50095> ;
    reg:hasUnconstrained <http://rdaregistry.info/Elements/u/P60648> ;
    reg:lexicalAlias <http://rdaregistry.info/Elements/a/corporateBody.en> ;
    reg:name "corporateBody"@en ;
    reg:status <http://metadataregistry.org/uri/RegStatus/1001> ;
    a rdf:Property ;
    rdfs:domain <http://rdaregistry.info/Elements/c/C10004> ;
    rdfs:isDefinedBy <http://rdaregistry.info/Elements/a/> ;
    rdfs:label "a pour collectivité"@fr, "has corporate body"@en ;
    skos:definition "Met une personne en relation avec une collectivité (groupe d’interprètes, expédition, etc) dont la personne est membre."@fr, "Relates a person to a corporate body of which a person is a member."@en .

<http://rdaregistry.info/Elements/a/P50096>
    rdakit:instructionNumber "29.5" ;
    rdakit:toolkitDefinition "A corporate body that employs a person."@en, "Collectivité qui emploie la personne."@fr, "Una entidad corporativa que emplea a la persona."@es ;
    rdakit:toolkitLabel "empleador"@es, "employer"@en, "employeur"@fr ;
    reg:hasSubproperty <http://rdaregistry.info/Elements/a/datatype/P50096>, <http://rdaregistry.info/Elements/a/object/P50096> ;
    reg:hasUnconstrained <http://rdaregistry.info/Elements/u/P60679> ;
    reg:lexicalAlias <http://rdaregistry.info/Elements/a/employer.en> ;
    reg:name "employer"@en ;
    reg:status <http://metadataregistry.org/uri/RegStatus/1001> ;
    a rdf:Property ;
    rdfs:domain <http://rdaregistry.info/Elements/c/C10004> ;
    rdfs:isDefinedBy <http://rdaregistry.info/Elements/a/> ;
    rdfs:label "a pour employeur"@fr, "has employer"@en ;
    skos:definition "Met une personne en relation avec une collectivité qui emploie la personne."@fr, "Relates a person to a corporate body that employs a person."@en .

<http://rdaregistry.info/Elements/a/P50097>
    rdakit:instructionNumber "9.1" ;
    rdakit:toolkitDefinition "A country with which a person is identified."@en, "Pays auquel une personne est identifiée."@fr, "Un país con el que se identifica la persona"@es ;
    rdakit:toolkitLabel "country associated with the person"@en, "land förknippat med personen"@sv, "pays associé à la personne"@fr, "país asociado con la persona"@es ;
    reg:hasSubproperty <http://rdaregistry.info/Elements/a/datatype/P50097> ;
    reg:hasUnconstrained <http://rdaregistry.info/Elements/u/P60063> ;
    reg:lexicalAlias <http://rdaregistry.info/Elements/a/countryAssociatedWithThePerson.en> ;
    reg:name "countryAssociatedWithThePerson"@en ;
    reg:status <http://metadataregistry.org/uri/RegStatus/1001> ;
    a rdf:Property ;
    rdfs:domain <http://rdaregistry.info/Elements/c/C10004> ;
    rdfs:isDefinedBy <http://rdaregistry.info/Elements/a/> ;
    rdfs:label "a pour pays associé à la personne"@fr, "har land förknippat med personen"@sv, "has country associated with the person"@en ;
    skos:definition "Met une personne en relation avec un pays auquel une personne est identifiée."@fr, "Relates a person to a country with which a person is identified."@en .

<http://rdaregistry.info/Elements/a/P50098>
    rdakit:instructionNumber "9.3.4" ;
    rdakit:toolkitDefinition "A date or range of dates indicative of the period in which a person was active in his or her primary field of endeavour."@en, "La date ou la fourchette de dates indicative de la période pendant laquelle une personne a été active dans son principal domaine d’activité."@fr, "La fecha o rango de fechas que indica el período en el que una persona fue activa en su campo primario de desempeño."@es ;
    rdakit:toolkitLabel "period of activity of the person"@en, "período de actividad de la persona"@es, "période d’activité de la personne"@fr, "verksamhetstid för personen"@sv ;
    reg:hasSubproperty <http://rdaregistry.info/Elements/a/datatype/P50098> ;
    reg:hasUnconstrained <http://rdaregistry.info/Elements/u/P60076> ;
    reg:lexicalAlias <http://rdaregistry.info/Elements/a/periodOfActivityOfThePerson.en> ;
    reg:name "periodOfActivityOfThePerson"@en ;
    reg:status <http://metadataregistry.org/uri/RegStatus/1001> ;
    a rdf:Property ;
    rdfs:domain <http://rdaregistry.info/Elements/c/C10004> ;
    rdfs:isDefinedBy <http://rdaregistry.info/Elements/a/> ;
    rdfs:label "a pour période d’activité de la personne"@fr, "har verksamhetstid för personen"@sv, "has period of activity of the person"@en ;
    rdfs:subPropertyOf <http://rdaregistry.info/Elements/a/P50107> ;
    skos:definition "Met une personne en relation avec la date ou la fourchette de dates indicative de la période pendant laquelle une personne a été active dans son principal domaine d’activité."@fr, "Relates a person to a date or range of dates indicative of the period in which a person was active in his or her primary field of endeavour."@en .

<http://rdaregistry.info/Elements/a/P50099>
    rdakit:instructionNumber "29.5" ;
    rdakit:toolkitDefinition "A family descended from a particular person."@en, "Famille descendant de la personne particulière."@fr, "Una familia que desciende de una persona determinada."@es ;
    rdakit:toolkitLabel "descendants"@en, "descendants"@fr, "descendientes"@es ;
    reg:hasSubproperty <http://rdaregistry.info/Elements/a/datatype/P50099>, <http://rdaregistry.info/Elements/a/object/P50099> ;
    reg:hasUnconstrained <http://rdaregistry.info/Elements/u/P60686> ;
    reg:lexicalAlias <http://rdaregistry.info/Elements/a/descendants.en> ;
    reg:name "descendants"@en ;
    reg:status <http://metadataregistry.org/uri/RegStatus/1001> ;
    a rdf:Property ;
    rdfs:domain <http://rdaregistry.info/Elements/c/C10004> ;
    rdfs:isDefinedBy <http://rdaregistry.info/Elements/a/> ;
    rdfs:label "a pour descendants"@fr, "has descendants"@en ;
    skos:definition "Met une personne en relation avec une famille descendant de la personne particulière."@fr, "Relates a person to a family descended from a particular person."@en .

<http://rdaregistry.info/Elements/a/P50100>
    rdakit:instructionNumber "9.15" ;
    rdakit:toolkitDefinition "A field of endeavour, area of expertise, etc., in which a person is engaged or was engaged."@en, "Champ d’action, domaine du savoir, etc. dans lequel s’investit ou s’est investie la personne."@fr, "Un área de trabajo, área de pericia, etc., en el que la persona está o estuvo involucrada."@es ;
    rdakit:toolkitLabel "campo de actividad de la persona"@es, "domaine d’activité de la personne"@fr, "field of activity of the person"@en ;
    reg:hasSubproperty <http://rdaregistry.info/Elements/a/datatype/P50100> ;
    reg:hasUnconstrained <http://rdaregistry.info/Elements/u/P60089> ;
    reg:lexicalAlias <http://rdaregistry.info/Elements/a/fieldOfActivityOfThePerson.en> ;
    reg:name "fieldOfActivityOfThePerson"@en ;
    reg:status <http://metadataregistry.org/uri/RegStatus/1001> ;
    a rdf:Property ;
    rdfs:domain <http://rdaregistry.info/Elements/c/C10004> ;
    rdfs:isDefinedBy <http://rdaregistry.info/Elements/a/> ;
    rdfs:label "a pour domaine d’activité de la personne"@fr, "has field of activity of the person"@en ;
    skos:definition "Met une personne en relation avec un champ d’action, un domaine du savoir, etc. dans lequel s’investit ou s’est investie la personne."@fr, "Relates a person to a field of endeavour, area of expertise, etc., in which a person is engaged or was engaged."@en .

<http://rdaregistry.info/Elements/a/P50101>
    rdakit:instructionNumber "9.13" ;
    rdakit:toolkitDefinition "A group with which a person is affiliated or has been affiliated through employment, membership, cultural identity, etc."@en, "Groupe auquel une personne est ou a été affiliée par recrutement, acquisition de la qualité de membre, identité culturelle, etc."@fr, "Un grupo con el que la persona está afiliada, o ha estado afiliada, mediante empleo, membresía, identidad cultural, etc."@es ;
    rdakit:toolkitLabel "affiliation"@en, "affiliation"@fr, "afiliación"@es, "organisatorisk tillhörighet"@sv ;
    reg:hasSubproperty <http://rdaregistry.info/Elements/a/datatype/P50101> ;
    reg:hasUnconstrained <http://rdaregistry.info/Elements/u/P60095> ;
    reg:lexicalAlias <http://rdaregistry.info/Elements/a/affiliation.en> ;
    reg:name "affiliation"@en ;
    reg:status <http://metadataregistry.org/uri/RegStatus/1001> ;
    a rdf:Property ;
    rdfs:domain <http://rdaregistry.info/Elements/c/C10004> ;
    rdfs:isDefinedBy <http://rdaregistry.info/Elements/a/> ;
    rdfs:label "a pour affiliation"@fr, "har organisatorisk tillhörighet"@sv, "has affiliation"@en ;
    skos:definition "Met une personne en relation avec un groupe auquel une personne est ou a été affiliée par recrutement, acquisition de la qualité de membre, identité culturelle, etc."@fr, "Relates a person to a group with which a person is affiliated or has been affiliated through employment, membership, cultural identity, etc."@en .

<http://rdaregistry.info/Elements/a/P50102>
    rdakit:instructionNumber "9.14" ;
    rdakit:toolkitDefinition "A language a person uses when writing for publication, broadcasting, etc."@en, "Langue utilisée par la personne quand elle écrit en vue d’une publication, d’une radiodiffusion, etc."@fr, "Una lengua que una persona utiliza cuando escribe para publicaciones, transmisiones, etc."@es ;
    rdakit:toolkitLabel "language of the person"@en, "langue de la personne"@fr, "lengua de la persona"@es ;
    reg:hasSubproperty <http://rdaregistry.info/Elements/a/datatype/P50102> ;
    reg:hasUnconstrained <http://rdaregistry.info/Elements/u/P60098> ;
    reg:lexicalAlias <http://rdaregistry.info/Elements/a/languageOfThePerson.en> ;
    reg:name "languageOfThePerson"@en ;
    reg:status <http://metadataregistry.org/uri/RegStatus/1001> ;
    a rdf:Property ;
    rdfs:domain <http://rdaregistry.info/Elements/c/C10004> ;
    rdfs:isDefinedBy <http://rdaregistry.info/Elements/a/> ;
    rdfs:label "a pour langue de la personne"@fr, "has language of the person"@en ;
    skos:definition "Met une personne en relation avec une langue utilisée par la personne quand elle écrit en vue d’une publication, d’une radiodiffusion, etc."@fr, "Relates a person to a language a person uses when writing for publication, broadcasting, etc."@en .

<http://rdaregistry.info/Elements/a/P50103>
    rdakit:instructionNumber "9.2.3" ;
    rdakit:toolkitDefinition "A name or form of name by which a person is known that differs from a name or form of name chosen as a preferred name."@en, "Nom ou forme de nom sous laquelle une personne est connue et qui diffère du nom ou de la forme de nom choisie comme nom privilégié."@fr, "Un nombre o forma del nombre mediante el cual se conoce una persona que difiere del nombre o forma del nombre elegido como el nombre preferido."@es ;
    rdakit:toolkitLabel "variant name for the person"@en, "variante de nom de la personne"@fr, "variante del nombre de la persona"@es, "variantnamn för personen"@sv ;
    reg:hasSubproperty <http://rdaregistry.info/Elements/a/datatype/P50103> ;
    reg:hasUnconstrained <http://rdaregistry.info/Elements/u/P60119> ;
    reg:lexicalAlias <http://rdaregistry.info/Elements/a/variantNameForThePerson.en> ;
    reg:name "variantNameForThePerson"@en ;
    reg:status <http://metadataregistry.org/uri/RegStatus/1001> ;
    a rdf:Property ;
    rdfs:domain <http://rdaregistry.info/Elements/c/C10004> ;
    rdfs:isDefinedBy <http://rdaregistry.info/Elements/a/> ;
    rdfs:label "a pour variante de nom de la personne"@fr, "har variantnamn för personen"@sv, "has variant name for the person"@en ;
    rdfs:subPropertyOf <http://rdaregistry.info/Elements/a/P50111> ;
    skos:definition "Met une personne en relation avec un nom ou une forme de nom sous laquelle une personne est connue et qui diffère du nom ou de la forme de nom choisie comme nom privilégié."@fr, "Relates a person to a name or form of name by which a person is known that differs from a name or form of name chosen as a preferred name."@en .

<http://rdaregistry.info/Elements/a/P50104>
    rdakit:instructionNumber "9.16" ;
    rdakit:toolkitDefinition "A person's vocation or avocation."@en, "La profession ou le passe-temps d’une personne."@fr, "Vocación o pasatiempo de una persona."@es ;
    rdakit:toolkitLabel "profesión u ocupación"@es, "profession or occupation"@en, "profession ou occupation"@fr, "yrke eller sysselsättning"@sv ;
    reg:hasSubproperty <http://rdaregistry.info/Elements/a/datatype/P50104> ;
    reg:hasUnconstrained <http://rdaregistry.info/Elements/u/P60468> ;
    reg:lexicalAlias <http://rdaregistry.info/Elements/a/professionOrOccupation.en> ;
    reg:name "professionOrOccupation"@en ;
    reg:status <http://metadataregistry.org/uri/RegStatus/1001> ;
    a rdf:Property ;
    rdfs:domain <http://rdaregistry.info/Elements/c/C10004> ;
    rdfs:isDefinedBy <http://rdaregistry.info/Elements/a/> ;
    rdfs:label "a pour profession ou occupation"@fr, "har yrke eller sysselsättning"@sv, "has profession or occupation"@en ;
    skos:definition "Met une personne en relation avec la profession ou le passe-temps d’une personne."@fr, "Relates a person to a person's vocation or avocation."@en .

<http://rdaregistry.info/Elements/a/P50105>
    rdakit:instructionNumber "29.5" ;
    rdakit:toolkitDefinition "A pseudonymous or other identity assumed by a person."@en, "Pseudonyme ou autre identité adoptée par la personne."@fr, "Un seudónimo u otra identidad asumida por la persona."@es ;
    rdakit:toolkitLabel "alternate identity"@en, "identidad alternativa"@es, "identité alternative"@fr ;
    reg:hasSubproperty <http://rdaregistry.info/Elements/a/datatype/P50105>, <http://rdaregistry.info/Elements/a/object/P50105> ;
    reg:hasUnconstrained <http://rdaregistry.info/Elements/u/P60036> ;
    reg:lexicalAlias <http://rdaregistry.info/Elements/a/alternateIdentity.en> ;
    reg:name "alternateIdentity"@en ;
    reg:status <http://metadataregistry.org/uri/RegStatus/1001> ;
    a rdf:Property ;
    rdfs:domain <http://rdaregistry.info/Elements/c/C10004> ;
    rdfs:isDefinedBy <http://rdaregistry.info/Elements/a/> ;
    rdfs:label "a pour identité alternative"@fr, "has alternate identity"@en ;
    skos:definition "Met une personne en relation avec un pseudonyme ou une autre identité adoptée par la personne."@fr, "Relates a person to a pseudonymous or other identity assumed by a person."@en .

<http://rdaregistry.info/Elements/a/P50106>
    rdakit:instructionNumber "29.5" ;
    rdakit:toolkitDefinition "A real person who assumes an alternate identity."@en, "Personne réelle qui adopte l’identité alternative."@fr, "Una persona real que asume la identidad alternativa."@es ;
    rdakit:toolkitLabel "identidad real"@es, "identité réelle"@fr, "real identity"@en ;
    reg:hasSubproperty <http://rdaregistry.info/Elements/a/datatype/P50106>, <http://rdaregistry.info/Elements/a/object/P50106> ;
    reg:hasUnconstrained <http://rdaregistry.info/Elements/u/P60037> ;
    reg:lexicalAlias <http://rdaregistry.info/Elements/a/realIdentity.en> ;
    reg:name "realIdentity"@en ;
    reg:status <http://metadataregistry.org/uri/RegStatus/1001> ;
    a rdf:Property ;
    rdfs:domain <http://rdaregistry.info/Elements/c/C10004> ;
    rdfs:isDefinedBy <http://rdaregistry.info/Elements/a/> ;
    rdfs:label "a pour identité réelle"@fr, "has real identity"@en ;
    skos:definition "Met une personne en relation avec une personne réelle qui adopte l’identité alternative."@fr, "Relates a person to a real person who assumes an alternate identity."@en .

<http://rdaregistry.info/Elements/a/P50107>
    rdakit:instructionNumber "9.3" ;
    rdakit:toolkitDefinition "A significant date associated with a person."@en, "Date importante associée à une personne (par exemple, date de naissance, date de décès)."@fr, "Una fecha significativa asociada con la persona (p.ej., fecha de nacimiento, fecha de fallecimiento)."@es ;
    rdakit:toolkitLabel "date associated with the person"@en, "date associée à la personne"@fr, "fecha asociada con la persona"@es, "tid förknippad med personen"@sv ;
    reg:hasSubproperty <http://rdaregistry.info/Elements/a/P50098>, <http://rdaregistry.info/Elements/a/P50120>, <http://rdaregistry.info/Elements/a/P50121>, <http://rdaregistry.info/Elements/a/datatype/P50107> ;
    reg:hasUnconstrained <http://rdaregistry.info/Elements/u/P60324> ;
    reg:lexicalAlias <http://rdaregistry.info/Elements/a/dateAssociatedWithThePerson.en> ;
    reg:name "dateAssociatedWithThePerson"@en ;
    reg:status <http://metadataregistry.org/uri/RegStatus/1001> ;
    a rdf:Property ;
    rdfs:domain <http://rdaregistry.info/Elements/c/C10004> ;
    rdfs:isDefinedBy <http://rdaregistry.info/Elements/a/> ;
    rdfs:label "a pour date associée à la personne"@fr, "har tid förknippad med personen"@sv, "has date associated with the person"@en ;
    skos:definition "Met une personne en relation avec une date importante associée à une personne (par exemple, date de naissance, date de décès)."@fr, "Relates a person to a significant date associated with a person."@en .

<http://rdaregistry.info/Elements/a/P50108>
    rdakit:instructionNumber "9.6" ;
    rdakit:toolkitDefinition "A term other than a title that is associated with a person."@en, "Terme, autre qu’un titre, associé à un nom de personne."@fr, "Un término diferente de un título que está asociado con el nombre de la persona."@es ;
    rdakit:toolkitLabel "autre information associée à la personne"@fr, "other designation associated with the person"@en, "otra designación asociada con la persona"@es, "övrig beteckning förknippad med personen"@sv ;
    reg:hasSubproperty <http://rdaregistry.info/Elements/a/datatype/P50108> ;
    reg:hasUnconstrained <http://rdaregistry.info/Elements/u/P60370> ;
    reg:lexicalAlias <http://rdaregistry.info/Elements/a/otherDesignationAssociatedWithThePerson.en> ;
    reg:name "otherDesignationAssociatedWithThePerson"@en ;
    reg:status <http://metadataregistry.org/uri/RegStatus/1001> ;
    a rdf:Property ;
    rdfs:domain <http://rdaregistry.info/Elements/c/C10004> ;
    rdfs:isDefinedBy <http://rdaregistry.info/Elements/a/> ;
    rdfs:label "a pour autre information associée à la personne"@fr, "har övrig beteckning förknippad med personen"@sv, "has other designation associated with the person"@en ;
    skos:definition "Met une personne en relation avec un terme, autre qu’un titre, associé à un nom de personne."@fr, "Relates a person to a term other than a title that is associated with a person's name."@en .

<http://rdaregistry.info/Elements/a/P50109>
    rdakit:instructionNumber "9.11" ;
    rdakit:toolkitDefinition "A town, city, province, state, and/or country in which a person resides or has resided, or another significant place associated with a person other than place of birth, place of death, or residence."@en, "Municipalité, ville, province, État et/ou pays où une personne réside ou a résidé, ou autre lieu important associé à la personne et autre qu’un lieu de naissance, de décès ou de résidence (par exemple, un lieu où la personne a travaillé ou étudié)."@fr, "Un poblado, ciudad, provincia, estado y/o país en el que residió o ha residido una persona, u otro lugar significativo asociado con la persona diferente del lugar de nacimiento, fallecimiento o residencia (por ej., un lugar donde la persona ha trabajado o estudiado)."@es ;
    rdakit:toolkitLabel "bostadsort"@sv, "lieu de résidence"@fr, "lugar de residencia"@es, "place of residence, etc."@en ;
    reg:hasSubproperty <http://rdaregistry.info/Elements/a/datatype/P50109> ;
    reg:hasUnconstrained <http://rdaregistry.info/Elements/u/P60360> ;
    reg:lexicalAlias <http://rdaregistry.info/Elements/a/placeOfResidenceEtc.en> ;
    reg:name "placeOfResidenceEtc"@en ;
    reg:status <http://metadataregistry.org/uri/RegStatus/1001> ;
    a rdf:Property ;
    rdfs:domain <http://rdaregistry.info/Elements/c/C10004> ;
    rdfs:isDefinedBy <http://rdaregistry.info/Elements/a/> ;
    rdfs:label "a pour lieu de résidence"@fr, "har bostadsort"@sv, "has place of residence, etc."@en ;
    skos:definition "Met une personne en relation avec une municipalité, une ville, une province, un État et/ou un pays où une personne réside ou a résidé, ou un autre lieu important associé à la personne et autre qu’un lieu de naissance, de décès ou de résidence (par exemple, un lieu où la personne a travaillé ou étudié)."@fr, "Relates a person to a town, city, province, state, and/or country in which a person resides or has resided, or another significant place associated with the person other than place of birth, place of death, or residence."@en ;
    skos:scopeNote "A place where a person has worked or studied is included."@en .

<http://rdaregistry.info/Elements/a/P50110>
    rdakit:instructionNumber "9.4" ;
    rdakit:toolkitDefinition "A word or phrase indicative of royalty, nobility, ecclesiastical rank or office, or a term of address for a person of religious vocation."@en, "Mot ou expression indiquant la royauté, la noblesse ou un rang ou une fonction ecclésiastiques, un terme de politesse pour une personne à vocation religieuse ou un autre terme indiquant un rang, un honneur ou une fonction."@fr, "Una palabra o frase que indica realeza, nobleza o rango o cargo eclesiástico o un término de tratamiento de una persona de vocación religiosa."@es ;
    rdakit:toolkitLabel "title of the person"@en, "titre de la personne"@fr, "título de la persona"@es ;
    reg:hasSubproperty <http://rdaregistry.info/Elements/a/datatype/P50110> ;
    reg:hasUnconstrained <http://rdaregistry.info/Elements/u/P60363> ;
    reg:lexicalAlias <http://rdaregistry.info/Elements/a/titleOfThePerson.en> ;
    reg:name "titleOfThePerson"@en ;
    reg:status <http://metadataregistry.org/uri/RegStatus/1001> ;
    a rdf:Property ;
    rdfs:domain <http://rdaregistry.info/Elements/c/C10004> ;
    rdfs:isDefinedBy <http://rdaregistry.info/Elements/a/> ;
    rdfs:label "a pour titre de la personne"@fr, "has title of the person"@en ;
    skos:definition "Met une personne en relation avec un mot ou une expression indiquant la royauté, la noblesse ou un rang ou une fonction ecclésiastiques, un terme de politesse pour une personne à vocation religieuse ou un autre terme indiquant un rang, un honneur ou une fonction."@fr, "Relates a person to a word or phrase indicative of royalty, nobility, ecclesiastical rank or office, or a term of address for a person of religious vocation."@en ;
    skos:scopeNote "A title of the person includes other terms indicative of rank, honour, or office, including initials or abbreviations representing an academic degree, or membership in an organization, and excludes terms of address that simply indicate gender or marital status such as Mr. or Mrs."@en, "Le titre de la personne exclut les termes de politesse qui indiquent simplement le sexe ou le statut marital (par exemple, M., Mme)."@fr .

<http://rdaregistry.info/Elements/a/P50111>
    rdakit:instructionNumber "9.2" ;
    rdakit:toolkitDefinition "A word, character, or group of words and/or characters by which a person is known."@en, "Mot, caractère ou groupe de mots et/ou de caractères sous lequel une personne est connue."@fr, "Una palabra, carácter o grupo de palabras y/o caracteres mediante el cual se conoce una persona."@es ;
    rdakit:toolkitLabel "name of the person"@en, "nom de personne"@fr, "nombre de la persona"@es, "personnamn"@sv ;
    reg:hasSubproperty <http://rdaregistry.info/Elements/a/P50103>, <http://rdaregistry.info/Elements/a/P50117>, <http://rdaregistry.info/Elements/a/datatype/P50111> ;
    reg:hasUnconstrained <http://rdaregistry.info/Elements/u/P60368> ;
    reg:lexicalAlias <http://rdaregistry.info/Elements/a/nameOfThePerson.en> ;
    reg:name "nameOfThePerson"@en ;
    reg:status <http://metadataregistry.org/uri/RegStatus/1001> ;
    a rdf:Property ;
    rdfs:domain <http://rdaregistry.info/Elements/c/C10004> ;
    rdfs:isDefinedBy <http://rdaregistry.info/Elements/a/> ;
    rdfs:label "a pour nom de personne"@fr, "har personnamn"@sv, "has name of the person"@en ;
    skos:definition "Met une personne en relation avec un mot, un caractère ou un groupe de mots et/ou de caractères sous lequel une personne est connue."@fr, "Relates a person to a word, character, or group of words and/or characters by which a person is known."@en .

<http://rdaregistry.info/Elements/a/P50112>
    rdakit:instructionNumber "29.5" ;
    rdakit:toolkitDefinition "An organization that a person founded."@en, "Organisation que la personne a fondée."@fr, "Una organización que la persona fundó."@es ;
    rdakit:toolkitLabel "collectivité fondée de la personne"@fr, "entidad corporativa fundada"@es, "founded corporate body of person"@en ;
    reg:hasSubproperty <http://rdaregistry.info/Elements/a/datatype/P50112>, <http://rdaregistry.info/Elements/a/object/P50112> ;
    reg:hasUnconstrained <http://rdaregistry.info/Elements/u/P60687> ;
    reg:lexicalAlias <http://rdaregistry.info/Elements/a/foundedCorporateBodyOfPerson.en> ;
    reg:name "foundedCorporateBodyOfPerson"@en ;
    reg:status <http://metadataregistry.org/uri/RegStatus/1001> ;
    a rdf:Property ;
    rdfs:domain <http://rdaregistry.info/Elements/c/C10004> ;
    rdfs:isDefinedBy <http://rdaregistry.info/Elements/a/> ;
    rdfs:label "a pour collectivité fondée de la personne"@fr, "has founded corporate body of person"@en ;
    skos:definition "Met une personne en relation avec une organisation que la personne a fondée."@fr, "Relates a person to an organization that a person founded."@en .

<http://rdaregistry.info/Elements/a/P50113>
    rdakit:instructionNumber "9.17" ;
    rdakit:toolkitDefinition "A summary of information about the life or history of a person."@en, "Información perteneciente a la vida o historia de una persona."@es, "Information relative à la vie ou à l’histoire d’une personne."@fr ;
    rdakit:toolkitLabel "biografisk information"@sv, "biographical information"@en, "información biográfica"@es, "information biographique"@fr ;
    reg:hasSubproperty <http://rdaregistry.info/Elements/a/datatype/P50113> ;
    reg:hasUnconstrained <http://rdaregistry.info/Elements/u/P60492> ;
    reg:lexicalAlias <http://rdaregistry.info/Elements/a/biographicalInformation.en> ;
    reg:name "biographicalInformation"@en ;
    reg:status <http://metadataregistry.org/uri/RegStatus/1001> ;
    a rdf:Property ;
    rdfs:domain <http://rdaregistry.info/Elements/c/C10004> ;
    rdfs:isDefinedBy <http://rdaregistry.info/Elements/a/> ;
    rdfs:label "a pour information biographique"@fr, "har biografisk information"@sv, "has biographical information"@en ;
    skos:definition "Met une personne en relation avec une information relative à la vie ou à l’histoire d’une personne."@fr, "Relates a person to a summary of information about the life or history of a person."@en .

<http://rdaregistry.info/Elements/a/P50114>
    rdakit:instructionNumber "9.12" ;
    rdakit:toolkitDefinition "An address of a person."@en, "La dirección de una persona."@es, "L’adresse du lieu de résidence, de travail, l’adresse de l’employeur d’une personne et/ou son adresse électronique ou son adresse de site Web."@fr ;
    rdakit:toolkitLabel "address of the person"@en, "adresse de la personne"@fr, "dirección de la persona"@es ;
    reg:hasSubproperty <http://rdaregistry.info/Elements/a/datatype/P50114> ;
    reg:hasUnconstrained <http://rdaregistry.info/Elements/u/P60512> ;
    reg:lexicalAlias <http://rdaregistry.info/Elements/a/addressOfThePerson.en> ;
    reg:name "addressOfThePerson"@en ;
    reg:status <http://metadataregistry.org/uri/RegStatus/1001> ;
    a rdf:Property ;
    rdfs:domain <http://rdaregistry.info/Elements/c/C10004> ;
    rdfs:isDefinedBy <http://rdaregistry.info/Elements/a/> ;
    rdfs:label "a pour adresse de la personne"@fr, "has address of the person"@en ;
    skos:definition "Met une personne en relation avec l’adresse du lieu de résidence, de travail, l’adresse de l’employeur d’une personne et/ou son adresse électronique ou son adresse de site Web."@fr, "Relates a person to an address of a person's place of residence, business, or employer, and/or an e-mail or internet address."@en .

<http://rdaregistry.info/Elements/a/P50115>
    rdakit:instructionNumber "9.5" ;
    rdakit:toolkitDefinition "A name or names associated with a person that includes the fuller form of a part of any name represented only by an initial, abbreviation, or shortened or otherwise modified variant in the form chosen as the preferred name and/or a part of the name not included in the form chosen as the preferred name."@en, "La forma completa de una parte de un nombre representado solo por una inicial o abreviatura en la forma escogida como el nombre preferido, o una parte del nombre no incluida en la forma elegida como el nombre preferido."@es, "La forme développée d’une partie d’un nom représentée seulement par une initiale ou une abréviation dans la forme choisie comme nom privilégié, ou une partie du nom non incluse dans la forme choisie comme nom privilégié."@fr ;
    rdakit:toolkitLabel "forma más completa del nombre"@es, "forme développée du nom"@fr, "fuller form of name"@en, "fullständig namnform"@sv ;
    reg:hasSubproperty <http://rdaregistry.info/Elements/a/datatype/P50115> ;
    reg:hasUnconstrained <http://rdaregistry.info/Elements/u/P60530> ;
    reg:lexicalAlias <http://rdaregistry.info/Elements/a/fullerFormOfName.en> ;
    reg:name "fullerFormOfName"@en ;
    reg:status <http://metadataregistry.org/uri/RegStatus/1001> ;
    a rdf:Property ;
    rdfs:domain <http://rdaregistry.info/Elements/c/C10004> ;
    rdfs:isDefinedBy <http://rdaregistry.info/Elements/a/> ;
    rdfs:label "a pour forme développée du nom"@fr, "har fullständig namnform"@sv, "has fuller form of name"@en ;
    skos:definition "Met une personne en relation avec la forme développée d’une partie d’un nom représentée seulement par une initiale ou une abréviation dans la forme choisie comme nom privilégié, ou une partie du nom non incluse dans la forme choisie comme nom privilégié."@fr, "Relates a person to a name or names associated with a person that includes the fuller form of a part of any name represented only by an initial, abbreviation, or shortened or otherwise modified variant in the form chosen as the preferred name and/or a part of the name not included in the form chosen as the preferred name."@en .

<http://rdaregistry.info/Elements/a/P50116>
    rdakit:instructionNumber "9.7" ;
    rdakit:toolkitDefinition "A gender with which a person identifies."@en, "El género con el que se identifica la persona."@es, "Le sexe auquel une personne s’identifie."@fr ;
    rdakit:toolkitLabel "gender"@en, "género"@es, "kön"@sv, "sexe"@fr ;
    reg:hasSubproperty <http://rdaregistry.info/Elements/a/datatype/P50116> ;
    reg:hasUnconstrained <http://rdaregistry.info/Elements/u/P60531> ;
    reg:lexicalAlias <http://rdaregistry.info/Elements/a/gender.en> ;
    reg:name "gender"@en ;
    reg:status <http://metadataregistry.org/uri/RegStatus/1001> ;
    a rdf:Property ;
    rdfs:domain <http://rdaregistry.info/Elements/c/C10004> ;
    rdfs:isDefinedBy <http://rdaregistry.info/Elements/a/> ;
    rdfs:label "a pour sexe"@fr, "har kön"@sv, "has gender"@en ;
    skos:definition "Met une personne en relation avec le sexe auquel une personne s’identifie."@fr, "Relates a person to a gender with which a person identifies."@en .

<http://rdaregistry.info/Elements/a/P50117>
    rdakit:instructionNumber "9.2.2" ;
    rdakit:toolkitDefinition "A name or form of name chosen to identify a person."@en, "El nombre o forma del nombre elegido para identificar la persona."@es, "Le nom ou la forme de nom choisie pour identifier la personne."@fr ;
    rdakit:toolkitLabel "nom privilégié de la personne"@fr, "nombre preferido de la persona"@es, "preferred name for the person"@en ;
    reg:hasSubproperty <http://rdaregistry.info/Elements/a/datatype/P50117> ;
    reg:hasUnconstrained <http://rdaregistry.info/Elements/u/P60549> ;
    reg:lexicalAlias <http://rdaregistry.info/Elements/a/preferredNameForThePerson.en> ;
    reg:name "preferredNameForThePerson"@en ;
    reg:status <http://metadataregistry.org/uri/RegStatus/1001> ;
    a rdf:Property ;
    rdfs:domain <http://rdaregistry.info/Elements/c/C10004> ;
    rdfs:isDefinedBy <http://rdaregistry.info/Elements/a/> ;
    rdfs:label "a pour nom privilégié de la personne"@fr, "has preferred name for the person"@en ;
    rdfs:subPropertyOf <http://rdaregistry.info/Elements/a/P50111> ;
    skos:definition "Met une personne en relation avec le nom ou la forme de nom choisie pour identifier la personne."@fr, "Relates a person to a name or form of name chosen to identify a person."@en .

<http://rdaregistry.info/Elements/a/P50118>
    rdakit:instructionNumber "9.9" ;
    rdakit:toolkitDefinition "A town, city, province, state, and/or country in which a person died."@en, "El poblado, ciudad, provincia, estado y/o país en el que murió la persona."@es, "La municipalité, la ville, la province, l’État et/ou le pays où une personne est morte."@fr ;
    rdakit:toolkitLabel "dödsort"@sv, "lieu de décès"@fr, "lugar de fallecimiento"@es, "place of death"@en ;
    reg:hasSubproperty <http://rdaregistry.info/Elements/a/datatype/P50118> ;
    reg:hasUnconstrained <http://rdaregistry.info/Elements/u/P60592> ;
    reg:lexicalAlias <http://rdaregistry.info/Elements/a/placeOfDeath.en> ;
    reg:name "placeOfDeath"@en ;
    reg:status <http://metadataregistry.org/uri/RegStatus/1001> ;
    a rdf:Property ;
    rdfs:domain <http://rdaregistry.info/Elements/c/C10004> ;
    rdfs:isDefinedBy <http://rdaregistry.info/Elements/a/> ;
    rdfs:label "a pour lieu de décès"@fr, "har dödsort"@sv, "has place of death"@en ;
    skos:definition "Met une personne en relation avec la municipalité, la ville, la province, l’État et/ou le pays où une personne est morte."@fr, "Relates a person to a town, city, province, state, and/or country in which a person died."@en .

<http://rdaregistry.info/Elements/a/P50119>
    rdakit:instructionNumber "9.8" ;
    rdakit:toolkitDefinition "A town, city, province, state, and/or country in which a person was born."@en, "El poblado, ciudad, provincia, estado y/o país en el que nació la persona."@es, "La municipalité, la ville, la province, l’État et/ou le pays où une personne est née."@fr ;
    rdakit:toolkitLabel "födelseort"@sv, "lieu de naissance"@fr, "lugar de nacimiento"@es, "place of birth"@en ;
    reg:hasSubproperty <http://rdaregistry.info/Elements/a/datatype/P50119> ;
    reg:hasUnconstrained <http://rdaregistry.info/Elements/u/P60593> ;
    reg:lexicalAlias <http://rdaregistry.info/Elements/a/placeOfBirth.en> ;
    reg:name "placeOfBirth"@en ;
    reg:status <http://metadataregistry.org/uri/RegStatus/1001> ;
    a rdf:Property ;
    rdfs:domain <http://rdaregistry.info/Elements/c/C10004> ;
    rdfs:isDefinedBy <http://rdaregistry.info/Elements/a/> ;
    rdfs:label "a pour lieu de naissance"@fr, "har födelseort"@sv, "has place of birth"@en ;
    skos:definition "Met une personne en relation avec la municipalité, la ville, la province, l’État et/ou le pays où une personne est née."@fr, "Relates a person to a town, city, province, state, and/or country in which a person was born."@en .

<http://rdaregistry.info/Elements/a/P50120>
    rdakit:instructionNumber "9.3.3" ;
    rdakit:toolkitDefinition "A year a person died."@en, "El año en que murió la persona."@es, "L’année de mort d’une personne."@fr ;
    rdakit:toolkitLabel "date de décès"@fr, "date of death"@en, "dödstid"@sv, "fecha de fallecimiento"@es ;
    reg:hasSubproperty <http://rdaregistry.info/Elements/a/datatype/P50120> ;
    reg:hasUnconstrained <http://rdaregistry.info/Elements/u/P60598> ;
    reg:lexicalAlias <http://rdaregistry.info/Elements/a/dateOfDeath.en> ;
    reg:name "dateOfDeath"@en ;
    reg:status <http://metadataregistry.org/uri/RegStatus/1001> ;
    a rdf:Property ;
    rdfs:domain <http://rdaregistry.info/Elements/c/C10004> ;
    rdfs:isDefinedBy <http://rdaregistry.info/Elements/a/> ;
    rdfs:label "a pour date de décès"@fr, "har dödstid"@sv, "has date of death"@en ;
    rdfs:subPropertyOf <http://rdaregistry.info/Elements/a/P50107> ;
    skos:definition "Met une personne en relation avec l’année de mort d’une personne."@fr, "Relates a person to a year a person died."@en ;
    skos:scopeNote "Date of death may also include the month or month and day of the person's death."@en, "La date de décès peut aussi inclure le mois et le jour de la mort de la personne."@fr .

<http://rdaregistry.info/Elements/a/P50121>
    rdakit:instructionNumber "9.3.2" ;
    rdakit:toolkitDefinition "A year a person was born."@en, "El año en que nació la persona."@es, "L’année de naissance d’une personne."@fr ;
    rdakit:toolkitLabel "date de naissance"@fr, "date of birth"@en, "fecha de nacimiento"@es, "födelsetid"@sv ;
    reg:hasSubproperty <http://rdaregistry.info/Elements/a/datatype/P50121> ;
    reg:hasUnconstrained <http://rdaregistry.info/Elements/u/P60599> ;
    reg:lexicalAlias <http://rdaregistry.info/Elements/a/dateOfBirth.en> ;
    reg:name "dateOfBirth"@en ;
    reg:status <http://metadataregistry.org/uri/RegStatus/1001> ;
    a rdf:Property ;
    rdfs:domain <http://rdaregistry.info/Elements/c/C10004> ;
    rdfs:isDefinedBy <http://rdaregistry.info/Elements/a/> ;
    rdfs:label "a pour date de naissance"@fr, "has date of birth"@en, "has date of birth"@sv ;
    rdfs:subPropertyOf <http://rdaregistry.info/Elements/a/P50107> ;
    skos:definition "Met une personne en relation avec l’année de naissance d’une personne."@fr, "Relates a person to a year a person was born."@en ;
    skos:scopeNote "Date of birth may also include the month or month and day of the person's birth."@en, "La date de naissance peut aussi inclure le mois et le jour de naissance de la personne."@fr .

<http://rdaregistry.info/Elements/a/P50122>
    rdakit:instructionNumber "18.5" ;
    rdakit:toolkitDefinition "A legal work of a higher court recording a decision of a lower court that is appealed by a person."@en, "Personne qui en appelle de la décision d’un tribunal inférieur."@fr ;
    rdakit:toolkitLabel "appellant person of"@en, "personne appelante de"@fr ;
    reg:hasSubproperty <http://rdaregistry.info/Elements/a/datatype/P50122>, <http://rdaregistry.info/Elements/a/object/P50122> ;
    reg:hasUnconstrained <http://rdaregistry.info/Elements/u/P60691> ;
    reg:lexicalAlias <http://rdaregistry.info/Elements/a/appellantPersonOf.en> ;
    reg:name "appellantPersonOf"@en ;
    reg:status <http://metadataregistry.org/uri/RegStatus/1001> ;
    a rdf:Property ;
    rdfs:domain <http://rdaregistry.info/Elements/c/C10004> ;
    rdfs:isDefinedBy <http://rdaregistry.info/Elements/a/> ;
    rdfs:label "est la personne appelante de"@fr, "is appellant person of"@en ;
    rdfs:subPropertyOf <http://rdaregistry.info/Elements/a/P50088> ;
    skos:definition "Met une personne qui en appelle de la décision d’un tribunal inférieur en relation avec l’œuvre."@fr, "Relates a person who appeals a decision of a lower court recorded in a legal work of a higher court to a work."@en .

<http://rdaregistry.info/Elements/a/P50123>
    rdakit:instructionNumber "18.5" ;
    rdakit:toolkitDefinition "An item that is bound."@en, "Personne qui relie un item."@fr ;
    rdakit:toolkitLabel "binder of"@en, "relieur de"@fr ;
    reg:hasSubproperty <http://rdaregistry.info/Elements/a/datatype/P50123>, <http://rdaregistry.info/Elements/a/object/P50123> ;
    reg:hasUnconstrained <http://rdaregistry.info/Elements/u/P60692> ;
    reg:lexicalAlias <http://rdaregistry.info/Elements/a/binderOf.en> ;
    reg:name "binderOf"@en ;
    reg:status <http://metadataregistry.org/uri/RegStatus/1001> ;
    a rdf:Property ;
    rdfs:domain <http://rdaregistry.info/Elements/c/C10004> ;
    rdfs:isDefinedBy <http://rdaregistry.info/Elements/a/> ;
    rdfs:label "est le relieur de"@fr, "is binder of"@en ;
    rdfs:subPropertyOf <http://rdaregistry.info/Elements/a/P50182> ;
    skos:definition "Met une personne qui relie un item en relation avec l’item."@fr, "Relates a person who binds an item to an item."@en .

<http://rdaregistry.info/Elements/a/P50124>
    rdakit:instructionNumber "18.5" ;
    rdakit:toolkitDefinition "A work that involves a responsibility for bringing a suit in a civil proceeding by a person."@en, "Personne qui intente une poursuite civile."@fr ;
    rdakit:toolkitLabel "personne demanderesse de"@fr, "plaintiff person of"@en ;
    reg:hasSubproperty <http://rdaregistry.info/Elements/a/datatype/P50124>, <http://rdaregistry.info/Elements/a/object/P50124> ;
    reg:hasUnconstrained <http://rdaregistry.info/Elements/u/P60693> ;
    reg:lexicalAlias <http://rdaregistry.info/Elements/a/plaintiffPersonOf.en> ;
    reg:name "plaintiffPersonOf"@en ;
    reg:status <http://metadataregistry.org/uri/RegStatus/1001> ;
    a rdf:Property ;
    rdfs:domain <http://rdaregistry.info/Elements/c/C10004> ;
    rdfs:isDefinedBy <http://rdaregistry.info/Elements/a/> ;
    rdfs:label "est la personne demanderesse de"@fr, "is plaintiff person of"@en ;
    rdfs:subPropertyOf <http://rdaregistry.info/Elements/a/P50089> ;
    skos:definition "Met une personne qui intente une poursuite civile en relation avec l’œuvre."@fr, "Relates a person who brings a suit in a civil proceeding to a work."@en .

<http://rdaregistry.info/Elements/a/P50125>
    rdakit:instructionNumber "18.5" ;
    rdakit:toolkitDefinition "An item with a statement of dedication or gift written on it."@en, "Personne qui a écrit une dédicace ou une mention de don sur un item."@fr ;
    rdakit:toolkitLabel "dédicateur (item) de"@fr, "inscriber of"@en ;
    reg:hasSubproperty <http://rdaregistry.info/Elements/a/datatype/P50125>, <http://rdaregistry.info/Elements/a/object/P50125> ;
    reg:hasUnconstrained <http://rdaregistry.info/Elements/u/P60695> ;
    reg:lexicalAlias <http://rdaregistry.info/Elements/a/inscriberOf.en> ;
    reg:name "inscriberOf"@en ;
    reg:status <http://metadataregistry.org/uri/RegStatus/1001> ;
    a rdf:Property ;
    rdfs:domain <http://rdaregistry.info/Elements/c/C10004> ;
    rdfs:isDefinedBy <http://rdaregistry.info/Elements/a/> ;
    rdfs:label "est le dédicateur (item) de"@fr, "is inscriber of"@en ;
    rdfs:subPropertyOf <http://rdaregistry.info/Elements/a/P50182> ;
    skos:definition "Met une personne qui a écrit une dédicace ou une mention de don sur un item en relation avec l’item."@fr, "Relates a person who has written a statement of dedication or gift on an item to an item."@en .

<http://rdaregistry.info/Elements/a/P50126>
    rdakit:instructionNumber "18.5" ;
    rdakit:toolkitDefinition "A work that involves a responsibility for hearing and decision on legal matters in court."@en, "Personne qui entend des causes juridiques et rend jugement dans un tribunal."@fr ;
    rdakit:toolkitLabel "judge of"@en, "juge de"@fr ;
    reg:hasSubproperty <http://rdaregistry.info/Elements/a/datatype/P50126>, <http://rdaregistry.info/Elements/a/object/P50126> ;
    reg:hasUnconstrained <http://rdaregistry.info/Elements/u/P60696> ;
    reg:lexicalAlias <http://rdaregistry.info/Elements/a/judgeOf.en> ;
    reg:name "judgeOf"@en ;
    reg:status <http://metadataregistry.org/uri/RegStatus/1001> ;
    a rdf:Property ;
    rdfs:domain <http://rdaregistry.info/Elements/c/C10004> ;
    rdfs:isDefinedBy <http://rdaregistry.info/Elements/a/> ;
    rdfs:label "est le juge de"@fr, "is judge of"@en ;
    rdfs:subPropertyOf <http://rdaregistry.info/Elements/a/P50131> ;
    skos:definition "Met une personne qui entend des causes juridiques et rend jugement dans un tribunal en relation avec l’œuvre."@fr, "Relates a person who hears and decides on legal matters in court to a work."@en .

<http://rdaregistry.info/Elements/a/P50127>
    rdakit:instructionNumber "18.5" ;
    rdakit:toolkitDefinition "A work that involves a responsibility as a faculty moderator of an academic disputation, normally proposing a thesis and participating in the ensuing disputation."@en, "Personne qui est le président d’une soutenance de thèse, proposant normalement la thèse et participant au débat qui s’ensuit."@fr ;
    rdakit:toolkitLabel "praeses de"@fr, "praeses of"@en ;
    reg:hasSubproperty <http://rdaregistry.info/Elements/a/datatype/P50127>, <http://rdaregistry.info/Elements/a/object/P50127> ;
    reg:hasUnconstrained <http://rdaregistry.info/Elements/u/P60699> ;
    reg:lexicalAlias <http://rdaregistry.info/Elements/a/praesesOf.en> ;
    reg:name "praesesOf"@en ;
    reg:status <http://metadataregistry.org/uri/RegStatus/1001> ;
    a rdf:Property ;
    rdfs:domain <http://rdaregistry.info/Elements/c/C10004> ;
    rdfs:isDefinedBy <http://rdaregistry.info/Elements/a/> ;
    rdfs:label "est le praeses de"@fr, "is praeses of"@en ;
    rdfs:subPropertyOf <http://rdaregistry.info/Elements/a/P50204> ;
    skos:definition "Met une personne qui est le président d’une soutenance de thèse, proposant normalement la thèse et participant au débat qui s’ensuit en relation avec l’œuvre."@fr, "Relates a person who is a faculty moderator of an academic disputation, normally proposing a thesis and participating in the ensuing disputation to a work."@en .

<http://rdaregistry.info/Elements/a/P50128>
    rdakit:instructionNumber "18.5" ;
    rdakit:toolkitDefinition "An item with manuscript annotations."@en, "Personne qui rédige des annotations manuscrites sur un item."@fr ;
    rdakit:toolkitLabel "annotateur de"@fr, "annotator of"@en ;
    reg:hasSubproperty <http://rdaregistry.info/Elements/a/datatype/P50128>, <http://rdaregistry.info/Elements/a/object/P50128> ;
    reg:hasUnconstrained <http://rdaregistry.info/Elements/u/P60700> ;
    reg:lexicalAlias <http://rdaregistry.info/Elements/a/annotatorOf.en> ;
    reg:name "annotatorOf"@en ;
    reg:status <http://metadataregistry.org/uri/RegStatus/1001> ;
    a rdf:Property ;
    rdfs:domain <http://rdaregistry.info/Elements/c/C10004> ;
    rdfs:isDefinedBy <http://rdaregistry.info/Elements/a/> ;
    rdfs:label "est l’annotateur de"@fr, "is annotator of"@en ;
    rdfs:subPropertyOf <http://rdaregistry.info/Elements/a/P50182> ;
    skos:definition "Met une personne qui rédige des annotations manuscrites sur un item en relation avec l’item."@fr, "Relates a person who makes manuscript annotations on an item to an item."@en .

<http://rdaregistry.info/Elements/a/P50129>
    rdakit:instructionNumber "18.5" ;
    rdakit:toolkitDefinition "An item with a manuscript signature appearing on it."@en, "Personne dont la signature manuscrite figure sur un item."@fr ;
    rdakit:toolkitLabel "autographer of"@en, "signataire autographe de"@fr ;
    reg:hasSubproperty <http://rdaregistry.info/Elements/a/datatype/P50129>, <http://rdaregistry.info/Elements/a/object/P50129> ;
    reg:hasUnconstrained <http://rdaregistry.info/Elements/u/P60702> ;
    reg:lexicalAlias <http://rdaregistry.info/Elements/a/autographerOf.en> ;
    reg:name "autographerOf"@en ;
    reg:status <http://metadataregistry.org/uri/RegStatus/1001> ;
    a rdf:Property ;
    rdfs:domain <http://rdaregistry.info/Elements/c/C10004> ;
    rdfs:isDefinedBy <http://rdaregistry.info/Elements/a/> ;
    rdfs:label "est le signataire autographe de"@fr, "is autographer of"@en ;
    rdfs:subPropertyOf <http://rdaregistry.info/Elements/a/P50182> ;
    skos:definition "Met une personne dont la signature manuscrite figure sur un item en relation avec l’item."@fr, "Relates a person whose manuscript signature appears on an item to an item."@en .

<http://rdaregistry.info/Elements/a/P50130>
    rdakit:instructionNumber "18.5" ;
    rdakit:toolkitDefinition "A work that involves a responsibility for issuing a work, such as an official organ of the body."@en, "Personne, famille ou collectivité publiant une œuvre, tel un organe officiel de l’organisme."@fr ;
    rdakit:toolkitLabel "issuing body of"@en, "organisme de publication de"@fr ;
    reg:hasSubproperty <http://rdaregistry.info/Elements/a/datatype/P50130>, <http://rdaregistry.info/Elements/a/object/P50130> ;
    reg:hasUnconstrained <http://rdaregistry.info/Elements/u/P60703> ;
    reg:lexicalAlias <http://rdaregistry.info/Elements/a/issuingBodyOf.en> ;
    reg:name "issuingBodyOf"@en ;
    reg:status <http://metadataregistry.org/uri/RegStatus/1001> ;
    a rdf:Property ;
    rdfs:domain <http://rdaregistry.info/Elements/c/C10002> ;
    rdfs:isDefinedBy <http://rdaregistry.info/Elements/a/> ;
    rdfs:label "est l’organisme de publication de"@fr, "is issuing body of"@en ;
    rdfs:subPropertyOf <http://rdaregistry.info/Elements/a/P50131> ;
    skos:definition "Met une personne, famille ou collectivité publiant une œuvre, tel un organe officiel de l’organisme, en relation avec l’œuvre."@fr, "Relates an agent issuing a work, such as an official organ of the body to a work."@en .

<http://rdaregistry.info/Elements/a/P50131>
    rdakit:toolkitDefinition "A work associated with an agent other than a creator."@en, "Personne, famille ou collectivité associée à une œuvre autrement que comme créateur."@fr ;
    rdakit:toolkitLabel "autre personne, famille ou collectivité associée à une œuvre de"@fr, "other person, family, or corporate body associated with a work of"@en ;
    reg:hasSubproperty <http://rdaregistry.info/Elements/a/P50044>, <http://rdaregistry.info/Elements/a/P50069>, <http://rdaregistry.info/Elements/a/P50086>, <http://rdaregistry.info/Elements/a/P50087>, <http://rdaregistry.info/Elements/a/P50088>, <http://rdaregistry.info/Elements/a/P50089>, <http://rdaregistry.info/Elements/a/P50090>, <http://rdaregistry.info/Elements/a/P50091>, <http://rdaregistry.info/Elements/a/P50126>, <http://rdaregistry.info/Elements/a/P50130>, <http://rdaregistry.info/Elements/a/P50132>, <http://rdaregistry.info/Elements/a/P50166>, <http://rdaregistry.info/Elements/a/P50201>, <http://rdaregistry.info/Elements/a/P50205>, <http://rdaregistry.info/Elements/a/P50207>, <http://rdaregistry.info/Elements/a/P50208>, <http://rdaregistry.info/Elements/a/P50209>, <http://rdaregistry.info/Elements/a/P50211>, <http://rdaregistry.info/Elements/a/P50226>, <http://rdaregistry.info/Elements/a/datatype/P50131>, <http://rdaregistry.info/Elements/a/object/P50131>, <http://rdaregistry.info/Elements/a/object/P50257>, <http://rdaregistry.info/Elements/a/object/P50262>, <http://rdaregistry.info/Elements/a/object/P50264>, <http://rdaregistry.info/Elements/a/object/P50265>, <http://rdaregistry.info/Elements/a/object/P50270>, <http://rdaregistry.info/Elements/a/object/P50289>, <http://rdaregistry.info/Elements/a/object/P50290> ;
    reg:hasUnconstrained <http://rdaregistry.info/Elements/u/P60602> ;
    reg:lexicalAlias <http://rdaregistry.info/Elements/a/otherPFCWorkOf.en> ;
    reg:name "otherPFCWorkOf"@en ;
    reg:status <http://metadataregistry.org/uri/RegStatus/1001> ;
    a rdf:Property ;
    rdfs:domain <http://rdaregistry.info/Elements/c/C10002> ;
    rdfs:isDefinedBy <http://rdaregistry.info/Elements/a/> ;
    rdfs:label "est l’autre personne, famille ou collectivité associée à une œuvre de"@fr, "is other person, family, or corporate body associated with a work of"@en ;
    rdfs:subPropertyOf <http://rdaregistry.info/Elements/a/P50305> ;
    skos:definition "Met une personne, famille ou collectivité associée à une œuvre autrement que comme créateur en relation avec l’œuvre."@fr, "Relates an agent associated with a work other than as a creator to a work."@en ;
    skos:scopeNote "Agents to whom correspondence is addressed, agents honoured by a festschrift, directors, cinematographers, sponsoring bodies, production companies, institutions, etc., hosting an exhibition or event, etc., are included."@en, "Comprend les personnes, etc. à qui une correspondance est adressée, les personnes, etc. à qui sont offerts des mélanges, les réalisateurs, les directeurs de la photographie, les commanditaires, les sociétés de production, les institutions, etc. accueillant une exposition ou un évènement, etc."@fr .

<http://rdaregistry.info/Elements/a/P50132>
    rdakit:instructionNumber "18.5" ;
    rdakit:toolkitDefinition "A work that is dedicated to an agent."@en, "Personne, famille ou collectivité par qui une œuvre est dédiée."@fr ;
    rdakit:toolkitLabel "dedicator of"@en, "dédicateur de"@fr ;
    reg:hasSubproperty <http://rdaregistry.info/Elements/a/datatype/P50132>, <http://rdaregistry.info/Elements/a/object/P50132> ;
    reg:hasUnconstrained <http://rdaregistry.info/Elements/u/P60603> ;
    reg:lexicalAlias <http://rdaregistry.info/Elements/a/dedicatorOf.en> ;
    reg:name "dedicatorOf"@en ;
    reg:status <http://metadataregistry.org/uri/RegStatus/1001> ;
    a rdf:Property ;
    rdfs:domain <http://rdaregistry.info/Elements/c/C10002> ;
    rdfs:isDefinedBy <http://rdaregistry.info/Elements/a/> ;
    rdfs:label "est le dédicateur de"@fr, "is dedicator of"@en ;
    rdfs:subPropertyOf <http://rdaregistry.info/Elements/a/P50131> ;
    skos:definition "Met une personne, famille ou collectivité par qui une œuvre est dédiée en relation avec l’œuvre."@fr, "Relates an agent by whom a work is dedicated to a work."@en .

<http://rdaregistry.info/Elements/a/P50133>
    rdakit:instructionNumber "18.5" ;
    rdakit:toolkitDefinition "An item that is conceived, aggregated, and/or organized in an exhibition, collection, or other item."@en, "Personne, famille ou collectivité concevant, regroupant et/ou organisant une exposition, une collection ou un autre item."@fr ;
    rdakit:toolkitLabel "conservateur de"@fr, "curator of"@en ;
    reg:hasSubproperty <http://rdaregistry.info/Elements/a/P50045>, <http://rdaregistry.info/Elements/a/P50046>, <http://rdaregistry.info/Elements/a/datatype/P50133>, <http://rdaregistry.info/Elements/a/object/P50133> ;
    reg:hasUnconstrained <http://rdaregistry.info/Elements/u/P60604> ;
    reg:lexicalAlias <http://rdaregistry.info/Elements/a/curatorOf.en> ;
    reg:name "curatorOf"@en ;
    reg:status <http://metadataregistry.org/uri/RegStatus/1001> ;
    a rdf:Property ;
    rdfs:domain <http://rdaregistry.info/Elements/c/C10002> ;
    rdfs:isDefinedBy <http://rdaregistry.info/Elements/a/> ;
    rdfs:label "est le conservateur de"@fr, "is curator of"@en ;
    rdfs:subPropertyOf <http://rdaregistry.info/Elements/a/P50182> ;
    skos:definition "Met une personne, famille ou collectivité concevant, regroupant et/ou organisant une exposition, une collection ou un autre item en relation avec l’item."@fr, "Relates an agent conceiving, aggregating, or organizing an exhibition, collection, or other item to an item."@en .

<http://rdaregistry.info/Elements/a/P50134>
    rdakit:instructionNumber "18.5" ;
    rdakit:toolkitDefinition "An expression that incorporates a contribution of adding music to a work that originally lacked it, by composing new music to substitute for original music, or by composing new music to supplement existing music."@en, "Personne, famille ou collectivité contribuant à une expression en ajoutant de la musique à une œuvre qui n’en avait pas à l’origine, en composant une nouvelle musique pour remplacer la musique originale ou en composant une nouvelle musique pour compléter la musique existante."@fr ;
    rdakit:toolkitLabel "composer (expression) of"@en, "compositeur (expression) de"@fr ;
    reg:hasSubproperty <http://rdaregistry.info/Elements/a/datatype/P50134>, <http://rdaregistry.info/Elements/a/object/P50134> ;
    reg:hasUnconstrained <http://rdaregistry.info/Elements/u/P60655> ;
    reg:lexicalAlias <http://rdaregistry.info/Elements/a/composerExpressionOf.en> ;
    reg:name "composerExpressionOf"@en ;
    reg:status <http://metadataregistry.org/uri/RegStatus/1001> ;
    a rdf:Property ;
    rdfs:domain <http://rdaregistry.info/Elements/c/C10002> ;
    rdfs:isDefinedBy <http://rdaregistry.info/Elements/a/> ;
    rdfs:label "est le compositeur (expression) de"@fr, "is composer (expression) of"@en ;
    rdfs:subPropertyOf <http://rdaregistry.info/Elements/a/P50161> ;
    skos:definition "Met une personne, famille ou collectivité contribuant à une expression en ajoutant de la musique à une œuvre qui n’en avait pas à l’origine, en composant une nouvelle musique pour remplacer la musique originale ou en composant une nouvelle musique pour compléter la musique existante en relation avec l’expression."@fr, "Relates an agent contributing to an expression by adding music to a work that originally lacked it, by composing new music to substitute for the original music, or by composing new music to supplement the existing music, to an expression."@en .

<http://rdaregistry.info/Elements/a/P50135>
    rdakit:instructionNumber "18.5" ;
    rdakit:toolkitDefinition "An expression of a cartographic work that incorporates a contribution of providing measurements or dimensional relationships for a geographic area represented."@en, "Personne, famille ou collectivité contribuant à une expression d’une œuvre cartographique en fournissant les mesures ou les relations dimensionnelles pour l’aire géographique représentée."@fr ;
    rdakit:toolkitLabel "arpenteur de"@fr, "surveyor of"@en ;
    reg:hasSubproperty <http://rdaregistry.info/Elements/a/datatype/P50135>, <http://rdaregistry.info/Elements/a/object/P50135> ;
    reg:hasUnconstrained <http://rdaregistry.info/Elements/u/P60605> ;
    reg:lexicalAlias <http://rdaregistry.info/Elements/a/surveyorOf.en> ;
    reg:name "surveyorOf"@en ;
    reg:status <http://metadataregistry.org/uri/RegStatus/1001> ;
    a rdf:Property ;
    rdfs:domain <http://rdaregistry.info/Elements/c/C10002> ;
    rdfs:isDefinedBy <http://rdaregistry.info/Elements/a/> ;
    rdfs:label "est l’arpenteur de"@fr, "is surveyor of"@en ;
    rdfs:subPropertyOf <http://rdaregistry.info/Elements/a/P50161> ;
    skos:definition "Met une personne, famille ou collectivité contribuant à une expression d’une œuvre cartographique en fournissant les mesures ou les relations dimensionnelles pour l’aire géographique représentée en relation avec l’expression."@fr, "Relates an agent contributing to an expression of a cartographic work by providing measurements or dimensional relationships for a geographic area represented to an expression."@en .

<http://rdaregistry.info/Elements/a/P50136>
    rdakit:instructionNumber "18.5" ;
    rdakit:seeAlso <http://rdaregistry.info/Elements/a/P50192> ;
    rdakit:toolkitDefinition "An expression of a moving image work or computer program that incorporates a contribution of giving apparent movement to inanimate objects or drawings."@en, "Personne, famille ou collectivité contribuant à une expression d’une œuvre d’images animées ou d’un programme informatique en donnant l’illusion du mouvement à des objets inanimés ou à des dessins."@fr ;
    rdakit:toolkitLabel "animateur de"@fr, "animator of"@en ;
    reg:hasSubproperty <http://rdaregistry.info/Elements/a/datatype/P50136>, <http://rdaregistry.info/Elements/a/object/P50136> ;
    reg:hasUnconstrained <http://rdaregistry.info/Elements/u/P60606> ;
    reg:lexicalAlias <http://rdaregistry.info/Elements/a/animatorOf.en> ;
    reg:name "animatorOf"@en ;
    reg:status <http://metadataregistry.org/uri/RegStatus/1001> ;
    a rdf:Property ;
    rdfs:domain <http://rdaregistry.info/Elements/c/C10002> ;
    rdfs:isDefinedBy <http://rdaregistry.info/Elements/a/> ;
    rdfs:label "est l’animateur de"@fr, "is animator of"@en ;
    rdfs:subPropertyOf <http://rdaregistry.info/Elements/a/P50161> ;
    skos:definition "Met une personne, famille ou collectivité contribuant à une expression d’une œuvre d’images animées ou d’un programme informatique en donnant l’illusion du mouvement à des objets inanimés ou à des dessins en relation avec l’expression."@fr, "Relates an agent contributing to an expression of a moving image work or computer program by giving apparent movement to inanimate objects or drawings to an expression."@en .

<http://rdaregistry.info/Elements/a/P50137>
    rdakit:instructionNumber "18.5" ;
    rdakit:seeAlso <http://rdaregistry.info/Elements/a/P50187> ;
    rdakit:toolkitDefinition "An expression of a musical work that incorporates a contribution of rewriting the composition for a medium of performance different from that for which the work was originally intended."@en, "Personne, famille ou collectivité contribuant à une expression d’une œuvre musicale en réécrivant la composition pour une distribution d’exécution différente de celle à laquelle l’œuvre est originellement destinée."@fr ;
    rdakit:toolkitLabel "arranger of music of"@en, "arrangeur de musique de"@fr ;
    reg:hasSubproperty <http://rdaregistry.info/Elements/a/datatype/P50137>, <http://rdaregistry.info/Elements/a/object/P50137> ;
    reg:hasUnconstrained <http://rdaregistry.info/Elements/u/P60607> ;
    reg:lexicalAlias <http://rdaregistry.info/Elements/a/arrangerOfMusicOf.en> ;
    reg:name "arrangerOfMusicOf"@en ;
    reg:status <http://metadataregistry.org/uri/RegStatus/1001> ;
    a rdf:Property ;
    rdfs:domain <http://rdaregistry.info/Elements/c/C10002> ;
    rdfs:isDefinedBy <http://rdaregistry.info/Elements/a/> ;
    rdfs:label "est l’arrangeur de musique de"@fr, "is arranger of music of"@en ;
    rdfs:subPropertyOf <http://rdaregistry.info/Elements/a/P50161> ;
    skos:definition "Met une personne, famille ou collectivité contribuant à une expression d’une œuvre musicale en réécrivant la composition pour une distribution d’exécution différente de celle à laquelle l’œuvre est originellement destinée en relation avec l’expression."@fr, "Relates an agent contributing to an expression of a musical work by rewriting the composition for a medium of performance different from that for which the work was originally intended to an expression."@en ;
    skos:scopeNote "An arranger of music may also modify the work for the same medium of performance, etc., keeping the musical substance of the original composition essentially unchanged."@en, "Un arrangeur de musique peut aussi modifier l’œuvre pour la même distribution d’exécution, etc. tout en gardant la substance musicale de la composition originale essentiellement inchangée."@fr .

<http://rdaregistry.info/Elements/a/P50138>
    rdakit:instructionNumber "18.5" ;
    rdakit:toolkitDefinition "An expression of a primarily non-textual work that incorporates a contribution of providing text, such as captions for photographs or descriptions of maps."@en, "Personne, famille ou collectivité contribuant à une expression d’une œuvre essentiellement non textuelle en fournissant un texte pour l’œuvre non textuelle (par exemple, en écrivant des légendes pour des photographies, des descriptions de cartes géographiques)."@fr ;
    rdakit:toolkitLabel "auteur de texte ajouté de"@fr, "writer of added text of"@en ;
    reg:hasSubproperty <http://rdaregistry.info/Elements/a/P50216>, <http://rdaregistry.info/Elements/a/datatype/P50138>, <http://rdaregistry.info/Elements/a/object/P50138> ;
    reg:hasUnconstrained <http://rdaregistry.info/Elements/u/P60608> ;
    reg:lexicalAlias <http://rdaregistry.info/Elements/a/writerOfAddedTextOf.en> ;
    reg:name "writerOfAddedTextOf"@en ;
    reg:status <http://metadataregistry.org/uri/RegStatus/1001> ;
    a rdf:Property ;
    rdfs:domain <http://rdaregistry.info/Elements/c/C10002> ;
    rdfs:isDefinedBy <http://rdaregistry.info/Elements/a/> ;
    rdfs:label "est l’auteur de texte ajouté de"@fr, "is writer of added text of"@en ;
    rdfs:subPropertyOf <http://rdaregistry.info/Elements/a/P50154> ;
    skos:definition "Met une personne, famille ou collectivité contribuant à une expression d’une œuvre essentiellement non textuelle en fournissant un texte pour l’œuvre non textuelle (par exemple, en écrivant des légendes pour des photographies, des descriptions de cartes géographiques) en relation avec l’expression."@fr, "Relates an agent contributing to an expression of a primarily non-textual work by providing text, such as captions for photographs or descriptions of maps, to an expression."@en .

<http://rdaregistry.info/Elements/a/P50139>
    rdakit:instructionNumber "18.5" ;
    rdakit:toolkitDefinition "An expression of a stage work that incorporates a contribution of the general management and supervision of a performance."@en, "Personne, famille ou collectivité contribuant à une expression d’une œuvre scénique par la gestion et la supervision générales d’une prestation."@fr ;
    rdakit:toolkitLabel "metteur en scène de"@fr, "stage director of"@en ;
    reg:hasSubproperty <http://rdaregistry.info/Elements/a/datatype/P50139>, <http://rdaregistry.info/Elements/a/object/P50139> ;
    reg:hasUnconstrained <http://rdaregistry.info/Elements/u/P60627> ;
    reg:lexicalAlias <http://rdaregistry.info/Elements/a/stageDirectorOf.en> ;
    reg:name "stageDirectorOf"@en ;
    reg:status <http://metadataregistry.org/uri/RegStatus/1001> ;
    a rdf:Property ;
    rdfs:domain <http://rdaregistry.info/Elements/c/C10002> ;
    rdfs:isDefinedBy <http://rdaregistry.info/Elements/a/> ;
    rdfs:label "est le metteur en scène de"@fr, "is stage director of"@en ;
    rdfs:subPropertyOf <http://rdaregistry.info/Elements/a/P50161> ;
    skos:definition "Met une personne, famille ou collectivité contribuant à une expression d’une œuvre scénique par la gestion et la supervision générales d’une prestation en relation avec l’expression."@fr, "Relates an agent contributing to an expression of a stage work through the general management and supervision of a performance to an expression."@en .

<http://rdaregistry.info/Elements/a/P50140>
    rdakit:instructionNumber "18.5" ;
    rdakit:toolkitDefinition "An expression of a work that incorporates a contribution of acting as an interviewer, reporter, pollster, or some other information gathering agent."@en, "Personne, famille ou collectivité contribuant à une expression d’une œuvre en agissant à titre d’intervieweur, de journaliste, de sondeur ou d’autre agent recueillant de l’information."@fr ;
    rdakit:toolkitLabel "interviewer (expression) of"@en, "intervieweur (expression) de"@fr ;
    reg:hasSubproperty <http://rdaregistry.info/Elements/a/datatype/P50140>, <http://rdaregistry.info/Elements/a/object/P50140> ;
    reg:hasUnconstrained <http://rdaregistry.info/Elements/u/P60659> ;
    reg:lexicalAlias <http://rdaregistry.info/Elements/a/interviewerExpressionOf.en> ;
    reg:name "interviewerExpressionOf"@en ;
    reg:status <http://metadataregistry.org/uri/RegStatus/1001> ;
    a rdf:Property ;
    rdfs:domain <http://rdaregistry.info/Elements/c/C10002> ;
    rdfs:isDefinedBy <http://rdaregistry.info/Elements/a/> ;
    rdfs:label "est l’intervieweur (expression) de"@fr, "is interviewer (expression) of"@en ;
    rdfs:subPropertyOf <http://rdaregistry.info/Elements/a/P50161> ;
    skos:definition "Met une personne, famille ou collectivité contribuant à une expression d’une œuvre en agissant à titre d’intervieweur, de journaliste, de sondeur ou d’autre agent recueillant de l’information en relation avec l’expression."@fr, "Relates an agent contributing to an expression of a work by acting as an interviewer, reporter, pollster, or some other information gathering agent to an expression."@en .

<http://rdaregistry.info/Elements/a/P50141>
    rdakit:instructionNumber "18.5" ;
    rdakit:toolkitDefinition "An expression of a work by an architect, inventor, etc., that incorporates a contribution of making detailed plans or drawings for buildings, ships, aircraft, machines, objects, etc."@en, "Personne, famille ou collectivité contribuant à une expression d’une œuvre par un architecte, un inventeur, etc. en effectuant des plans ou des dessins détaillés pour des bâtiments, des navires, des avions, des machines, des objets, etc."@fr ;
    rdakit:toolkitLabel "dessinateur industriel de"@fr, "draftsman of"@en ;
    reg:hasSubproperty <http://rdaregistry.info/Elements/a/datatype/P50141>, <http://rdaregistry.info/Elements/a/object/P50141> ;
    reg:hasUnconstrained <http://rdaregistry.info/Elements/u/P60609> ;
    reg:lexicalAlias <http://rdaregistry.info/Elements/a/draftsmanOf.en> ;
    reg:name "draftsmanOf"@en ;
    reg:status <http://metadataregistry.org/uri/RegStatus/1001> ;
    a rdf:Property ;
    rdfs:domain <http://rdaregistry.info/Elements/c/C10002> ;
    rdfs:isDefinedBy <http://rdaregistry.info/Elements/a/> ;
    rdfs:label "est le dessinateur industriel de"@fr, "is draftsman of"@en ;
    rdfs:subPropertyOf <http://rdaregistry.info/Elements/a/P50161> ;
    skos:definition "Met une personne, famille ou collectivité contribuant à une expression d’une œuvre par un architecte, un inventeur, etc. en effectuant des plans ou des dessins détaillés pour des bâtiments, des navires, des avions, des machines, des objets, etc. en relation avec l’expression."@fr, "Relates an agent contributing to an expression of a work by an architect, inventor, etc., by making detailed plans or drawings for buildings, ships, aircraft, machines, objects, etc. to an expression."@en .

<http://rdaregistry.info/Elements/a/P50142>
    rdakit:instructionNumber "18.5" ;
    rdakit:seeAlso <http://rdaregistry.info/Elements/a/P50137> ;
    rdakit:toolkitDefinition "An expression of a work that incorporates a contribution of writing down or notating previously unwritten or unnotated content, or by changing it from one system of notation to another."@en, "Personne, famille ou collectivité contribuant à une expression d’une œuvre en écrivant ou en notant un contenu auparavant non écrit ou non noté, ou bien en le transposant d’un système de notation à un autre."@fr ;
    rdakit:toolkitLabel "transcriber of"@en, "transcripteur de"@fr ;
    reg:hasSubproperty <http://rdaregistry.info/Elements/a/datatype/P50142>, <http://rdaregistry.info/Elements/a/object/P50142> ;
    reg:hasUnconstrained <http://rdaregistry.info/Elements/u/P60610> ;
    reg:lexicalAlias <http://rdaregistry.info/Elements/a/transcriberOf.en> ;
    reg:name "transcriberOf"@en ;
    reg:status <http://metadataregistry.org/uri/RegStatus/1001> ;
    a rdf:Property ;
    rdfs:domain <http://rdaregistry.info/Elements/c/C10002> ;
    rdfs:isDefinedBy <http://rdaregistry.info/Elements/a/> ;
    rdfs:label "est le transcripteur de"@fr, "is transcriber of"@en ;
    rdfs:subPropertyOf <http://rdaregistry.info/Elements/a/P50161> ;
    skos:definition "Met une personne, famille ou collectivité contribuant à une expression d’une œuvre en écrivant ou en notant un contenu auparavant non écrit ou non noté, ou bien en le transposant d’un système de notation à un autre en relation avec l’expression."@fr, "Relates an agent contributing to an expression of a work by writing down or notating previously unwritten or unnotated content, or by changing it from one system of notation to another to an expression."@en .

<http://rdaregistry.info/Elements/a/P50143>
    rdakit:instructionNumber "18.5" ;
    rdakit:toolkitDefinition "An expression of a work that incorporates a contribution of coordinating the activities of composers, sound editors, and sound mixers for a moving image production or for a musical or dramatic presentation or entertainment."@en, "Personne, famille ou collectivité contribuant à une expression d’une œuvre en coordonnant les activités du compositeur, du monteur son et des mixeurs de son pour une production d’images animées ou bien pour une représentation ou un spectacle dramatique ou musical."@fr ;
    rdakit:toolkitLabel "directeur musical de"@fr, "musical director of"@en ;
    reg:hasSubproperty <http://rdaregistry.info/Elements/a/datatype/P50143>, <http://rdaregistry.info/Elements/a/object/P50143> ;
    reg:hasUnconstrained <http://rdaregistry.info/Elements/u/P60611> ;
    reg:lexicalAlias <http://rdaregistry.info/Elements/a/musicalDirectorOf.en> ;
    reg:name "musicalDirectorOf"@en ;
    reg:status <http://metadataregistry.org/uri/RegStatus/1001> ;
    a rdf:Property ;
    rdfs:domain <http://rdaregistry.info/Elements/c/C10002> ;
    rdfs:isDefinedBy <http://rdaregistry.info/Elements/a/> ;
    rdfs:label "est le directeur musical de"@fr, "is musical director of"@en ;
    rdfs:subPropertyOf <http://rdaregistry.info/Elements/a/P50161> ;
    skos:definition "Met une personne, famille ou collectivité contribuant à une expression d’une œuvre en coordonnant les activités du compositeur, du monteur son et des mixeurs de son pour une production d’images animées ou bien pour une représentation ou un spectacle dramatique ou musical en relation avec l’expression."@fr, "Relates an agent contributing to an expression of a work by coordinating the activities of composers, sound editors, and sound mixers for a moving image production or for a musical or dramatic presentation or entertainment to an expression."@en .

<http://rdaregistry.info/Elements/a/P50144>
    rdakit:instructionNumber "18.5" ;
    rdakit:toolkitDefinition "An expression of a work that incorporates a contribution of designing costumes for a moving image production or for a musical or dramatic presentation or entertainment."@en, "Personne, famille ou collectivité contribuant à une expression d’une œuvre en créant les costumes pour une production d’images animées ou bien pour une représentation ou un spectacle musical ou dramatique."@fr ;
    rdakit:toolkitLabel "costume designer of"@en, "créateur de costumes de"@fr ;
    reg:hasSubproperty <http://rdaregistry.info/Elements/a/datatype/P50144>, <http://rdaregistry.info/Elements/a/object/P50144> ;
    reg:hasUnconstrained <http://rdaregistry.info/Elements/u/P60612> ;
    reg:lexicalAlias <http://rdaregistry.info/Elements/a/costumeDesignerOf.en> ;
    reg:name "costumeDesignerOf"@en ;
    reg:status <http://metadataregistry.org/uri/RegStatus/1001> ;
    a rdf:Property ;
    rdfs:domain <http://rdaregistry.info/Elements/c/C10002> ;
    rdfs:isDefinedBy <http://rdaregistry.info/Elements/a/> ;
    rdfs:label "est le créateur de costumes de"@fr, "is costume designer of"@en ;
    rdfs:subPropertyOf <http://rdaregistry.info/Elements/a/P50161> ;
    skos:definition "Met une personne, famille ou collectivité contribuant à une expression d’une œuvre en créant les costumes pour une production d’images animées ou bien pour une représentation ou un spectacle musical ou dramatique en relation avec l’expression."@fr, "Relates an agent contributing to an expression of a work by designing costumes for a moving image production or for a musical or dramatic presentation or entertainment to an expression."@en .

<http://rdaregistry.info/Elements/a/P50145>
    rdakit:instructionNumber "18.5" ;
    rdakit:toolkitDefinition "An expression of a work that incorporates a contribution of expressing the linguistic content of the work in a language different from that of previous expressions of an original work."@en, "Personne, famille ou collectivité contribuant à une expression d’une œuvre en exprimant le texte original de l’œuvre dans une langue différente de celle de l’œuvre originale."@fr ;
    rdakit:toolkitLabel "traducteur de"@fr, "translator of"@en ;
    reg:hasSubproperty <http://rdaregistry.info/Elements/a/datatype/P50145>, <http://rdaregistry.info/Elements/a/object/P50145> ;
    reg:hasUnconstrained <http://rdaregistry.info/Elements/u/P60613> ;
    reg:lexicalAlias <http://rdaregistry.info/Elements/a/translatorOf.en> ;
    reg:name "translatorOf"@en ;
    reg:status <http://metadataregistry.org/uri/RegStatus/1001> ;
    a rdf:Property ;
    rdfs:domain <http://rdaregistry.info/Elements/c/C10002> ;
    rdfs:isDefinedBy <http://rdaregistry.info/Elements/a/> ;
    rdfs:label "est le traducteur de"@fr, "is translator of"@en ;
    rdfs:subPropertyOf <http://rdaregistry.info/Elements/a/P50161> ;
    skos:definition "Met une personne, famille ou collectivité contribuant à une expression d’une œuvre en exprimant le texte original de l’œuvre dans une langue différente de celle de l’œuvre originale en relation avec l’expression."@fr, "Relates an agent contributing to an expression of a work by expressing the linguistic content of the work in a language different from that of previous expressions of an original work to an expression."@en ;
    skos:scopeNote "A translator may also translate linguistic content between forms of the same language from different time periods."@en, "Un traducteur peut aussi traduire un texte depuis une forme ancienne d’une langue vers la forme moderne."@fr .

<http://rdaregistry.info/Elements/a/P50146>
    rdakit:instructionNumber "18.5" ;
    rdakit:toolkitDefinition "An expression of a work that incorporates a contribution of overseeing artists and craftspeople who build sets for moving image productions."@en, "Personne, famille ou collectivité contribuant à une expression d’une œuvre en supervisant les artistes et les artisans qui construisent les décors pour des productions d’images animées."@fr ;
    rdakit:toolkitLabel "art director of"@en, "directeur artistique de"@fr ;
    reg:hasSubproperty <http://rdaregistry.info/Elements/a/datatype/P50146>, <http://rdaregistry.info/Elements/a/object/P50146> ;
    reg:hasUnconstrained <http://rdaregistry.info/Elements/u/P60614> ;
    reg:lexicalAlias <http://rdaregistry.info/Elements/a/artDirectorOf.en> ;
    reg:name "artDirectorOf"@en ;
    reg:status <http://metadataregistry.org/uri/RegStatus/1001> ;
    a rdf:Property ;
    rdfs:domain <http://rdaregistry.info/Elements/c/C10002> ;
    rdfs:isDefinedBy <http://rdaregistry.info/Elements/a/> ;
    rdfs:label "est le directeur artistique de"@fr, "is art director of"@en ;
    rdfs:subPropertyOf <http://rdaregistry.info/Elements/a/P50161> ;
    skos:definition "Met une personne, famille ou collectivité contribuant à une expression d’une œuvre en supervisant les artistes et les artisans qui construisent les décors pour des productions d’images animées en relation avec l’expression."@fr, "Relates an agent contributing to an expression of a work by overseeing artists and craftspeople who build sets for moving image productions to an expression."@en .

<http://rdaregistry.info/Elements/a/P50147>
    rdakit:instructionNumber "18.5" ;
    rdakit:toolkitDefinition "An expression of a work that incorporates a contribution of performing music, acting, dancing, speaking, etc."@en, "Personne, famille ou collectivité contribuant à une expression d’une œuvre en exécutant de la musique, en jouant, en dansant, en parlant, etc. souvent dans une représentation musicale ou dramatique, etc."@fr ;
    rdakit:toolkitLabel "interprète de"@fr, "performer of"@en ;
    reg:hasSubproperty <http://rdaregistry.info/Elements/a/P50070>, <http://rdaregistry.info/Elements/a/P50071>, <http://rdaregistry.info/Elements/a/P50072>, <http://rdaregistry.info/Elements/a/P50073>, <http://rdaregistry.info/Elements/a/P50074>, <http://rdaregistry.info/Elements/a/P50075>, <http://rdaregistry.info/Elements/a/P50076>, <http://rdaregistry.info/Elements/a/P50077>, <http://rdaregistry.info/Elements/a/P50078>, <http://rdaregistry.info/Elements/a/P50079>, <http://rdaregistry.info/Elements/a/P50080>, <http://rdaregistry.info/Elements/a/P50081>, <http://rdaregistry.info/Elements/a/P50082>, <http://rdaregistry.info/Elements/a/P50083>, <http://rdaregistry.info/Elements/a/P50084>, <http://rdaregistry.info/Elements/a/datatype/P50147>, <http://rdaregistry.info/Elements/a/object/P50147> ;
    reg:hasUnconstrained <http://rdaregistry.info/Elements/u/P60615> ;
    reg:lexicalAlias <http://rdaregistry.info/Elements/a/performerOf.en> ;
    reg:name "performerOf"@en ;
    reg:status <http://metadataregistry.org/uri/RegStatus/1001> ;
    a rdf:Property ;
    rdfs:domain <http://rdaregistry.info/Elements/c/C10002> ;
    rdfs:isDefinedBy <http://rdaregistry.info/Elements/a/> ;
    rdfs:label "est l’interprète de"@fr, "is performer of"@en ;
    rdfs:subPropertyOf <http://rdaregistry.info/Elements/a/P50161> ;
    skos:definition "Met une personne, famille ou collectivité contribuant à une expression d’une œuvre en exécutant de la musique, en jouant, en dansant, en parlant, etc. souvent dans une représentation musicale ou dramatique, etc. en relation avec l’expression."@fr, "Relates an agent contributing to an expression of a work by performing music, acting, dancing, speaking, etc. to an expression."@en .

<http://rdaregistry.info/Elements/a/P50148>
    rdakit:instructionNumber "18.5" ;
    rdakit:toolkitDefinition "An expression of a work that incorporates a contribution of preparing a court's opinions for publication."@en, "Personne, famille ou collectivité contribuant à une expression d’une œuvre en préparant les opinions d’un tribunal aux fins de publication."@fr ;
    rdakit:toolkitLabel "court reporter of"@en, "rapporteur judiciaire de"@fr ;
    reg:hasSubproperty <http://rdaregistry.info/Elements/a/datatype/P50148>, <http://rdaregistry.info/Elements/a/object/P50148> ;
    reg:hasUnconstrained <http://rdaregistry.info/Elements/u/P60616> ;
    reg:lexicalAlias <http://rdaregistry.info/Elements/a/courtReporterOf.en> ;
    reg:name "courtReporterOf"@en ;
    reg:status <http://metadataregistry.org/uri/RegStatus/1001> ;
    a rdf:Property ;
    rdfs:domain <http://rdaregistry.info/Elements/c/C10002> ;
    rdfs:isDefinedBy <http://rdaregistry.info/Elements/a/> ;
    rdfs:label "est le rapporteur judiciaire de"@fr, "is court reporter of"@en ;
    rdfs:subPropertyOf <http://rdaregistry.info/Elements/a/P50161> ;
    skos:definition "Met une personne, famille ou collectivité contribuant à une expression d’une œuvre en préparant les opinions d’un tribunal aux fins de publication en relation avec l’expression."@fr, "Relates an agent contributing to an expression of a work by preparing a court's opinions for publication to an expression."@en .

<http://rdaregistry.info/Elements/a/P50149>
    rdakit:instructionNumber "18.5" ;
    rdakit:toolkitDefinition "An expression of a work that incorporates a contribution of providing a preface to an original work."@en, "Personne, famille ou collectivité contribuant à une expression d’une œuvre en fournissant une préface à l’œuvre originale."@fr ;
    rdakit:toolkitLabel "préfacier de"@fr, "writer of preface of"@en ;
    reg:hasSubproperty <http://rdaregistry.info/Elements/a/datatype/P50149>, <http://rdaregistry.info/Elements/a/object/P50149> ;
    reg:hasUnconstrained <http://rdaregistry.info/Elements/u/P60617> ;
    reg:lexicalAlias <http://rdaregistry.info/Elements/a/writerOfPrefaceOf.en> ;
    reg:name "writerOfPrefaceOf"@en ;
    reg:status <http://metadataregistry.org/uri/RegStatus/1001> ;
    a rdf:Property ;
    rdfs:domain <http://rdaregistry.info/Elements/c/C10002> ;
    rdfs:isDefinedBy <http://rdaregistry.info/Elements/a/> ;
    rdfs:label "est le préfacier de"@fr, "is writer of preface of"@en ;
    rdfs:subPropertyOf <http://rdaregistry.info/Elements/a/P50154> ;
    skos:definition "Met une personne, famille ou collectivité contribuant à une expression d’une œuvre en fournissant une préface à l’œuvre originale en relation avec l’expression."@fr, "Relates an agent contributing to an expression of a work by providing a preface to an original work to an expression."@en .

<http://rdaregistry.info/Elements/a/P50150>
    rdakit:instructionNumber "18.5" ;
    rdakit:toolkitDefinition "An expression of a work that incorporates a contribution of providing additional cartography, or by modifying previous cartography."@en, "Personne, famille ou collectivité contribuant à une expression d’une œuvre en fournissant une cartographie additionnelle ou en modifiant la cartographie antérieure."@fr ;
    rdakit:toolkitLabel "cartographe (expression) de"@fr, "cartographer (expression) of"@en ;
    reg:hasSubproperty <http://rdaregistry.info/Elements/a/datatype/P50150>, <http://rdaregistry.info/Elements/a/object/P50150> ;
    reg:hasUnconstrained <http://rdaregistry.info/Elements/u/P60654> ;
    reg:lexicalAlias <http://rdaregistry.info/Elements/a/cartographerExpressionOf.en> ;
    reg:name "cartographerExpressionOf"@en ;
    reg:status <http://metadataregistry.org/uri/RegStatus/1001> ;
    a rdf:Property ;
    rdfs:domain <http://rdaregistry.info/Elements/c/C10002> ;
    rdfs:isDefinedBy <http://rdaregistry.info/Elements/a/> ;
    rdfs:label "est le cartographe (expression) de"@fr, "is cartographer (expression) of"@en ;
    rdfs:subPropertyOf <http://rdaregistry.info/Elements/a/P50161> ;
    skos:definition "Met une personne, famille ou collectivité contribuant à une expression d’une œuvre en fournissant une cartographie additionnelle ou en modifiant la cartographie antérieure en relation avec l’expression."@fr, "Relates an agent contributing to an expression of a work by providing additional cartography, or by modifying previous cartography to an expression."@en .

<http://rdaregistry.info/Elements/a/P50151>
    rdakit:instructionNumber "18.5" ;
    rdakit:toolkitDefinition "An expression of a work that incorporates a contribution of providing additional choreography, or by modifying previous choreography."@en, "Personne, famille ou collectivité contribuant à une expression d’une œuvre en fournissant une chorégraphie additionnelle ou en modifiant la chorégraphie antérieure."@fr ;
    rdakit:toolkitLabel "choreographer (expression) of"@en, "chorégraphe (expression) de"@fr ;
    reg:hasSubproperty <http://rdaregistry.info/Elements/a/datatype/P50151>, <http://rdaregistry.info/Elements/a/object/P50151> ;
    reg:hasUnconstrained <http://rdaregistry.info/Elements/u/P60662> ;
    reg:lexicalAlias <http://rdaregistry.info/Elements/a/choreographerExpressionOf.en> ;
    reg:name "choreographerExpressionOf"@en ;
    reg:status <http://metadataregistry.org/uri/RegStatus/1001> ;
    a rdf:Property ;
    rdfs:domain <http://rdaregistry.info/Elements/c/C10002> ;
    rdfs:isDefinedBy <http://rdaregistry.info/Elements/a/> ;
    rdfs:label "est le chorégraphe (expression) de"@fr, "is choreographer (expression) of"@en ;
    rdfs:subPropertyOf <http://rdaregistry.info/Elements/a/P50161> ;
    skos:definition "Met une personne, famille ou collectivité contribuant à une expression d’une œuvre en fournissant une chorégraphie additionnelle ou en modifiant la chorégraphie antérieure en relation avec l’expression."@fr, "Relates an agent contributing to an expression of a work by providing additional choreography, or by modifying previous choreography to an expression."@en .

<http://rdaregistry.info/Elements/a/P50152>
    rdakit:instructionNumber "18.5" ;
    rdakit:toolkitDefinition "An expression of a work that incorporates a contribution of providing an interpretation or critical explanation to an original work."@en, "Personne, famille ou collectivité contribuant à une expression d’une œuvre en fournissant une interprétation ou une critique de l’œuvre originale."@fr ;
    rdakit:toolkitLabel "auteur de commentaire ajouté de"@fr, "writer of added commentary of"@en ;
    reg:hasSubproperty <http://rdaregistry.info/Elements/a/datatype/P50152>, <http://rdaregistry.info/Elements/a/object/P50152> ;
    reg:hasUnconstrained <http://rdaregistry.info/Elements/u/P60618> ;
    reg:lexicalAlias <http://rdaregistry.info/Elements/a/writerOfAddedCommentaryOf.en> ;
    reg:name "writerOfAddedCommentaryOf"@en ;
    reg:status <http://metadataregistry.org/uri/RegStatus/1001> ;
    a rdf:Property ;
    rdfs:domain <http://rdaregistry.info/Elements/c/C10002> ;
    rdfs:isDefinedBy <http://rdaregistry.info/Elements/a/> ;
    rdfs:label "est l’auteur de commentaire ajouté de"@fr, "is writer of added commentary of"@en ;
    rdfs:subPropertyOf <http://rdaregistry.info/Elements/a/P50154> ;
    skos:definition "Met une personne, famille ou collectivité contribuant à une expression d’une œuvre en fournissant une interprétation ou une critique de l’œuvre originale en relation avec l’expression."@fr, "Relates an agent contributing to an expression of a work by providing an interpretation or critical explanation of an original work to an expression."@en .

<http://rdaregistry.info/Elements/a/P50153>
    rdakit:instructionNumber "18.5" ;
    rdakit:toolkitDefinition "An expression of a work that incorporates a contribution of providing an introduction to an original work."@en, "Personne, famille ou collectivité contribuant à une expression d’une œuvre en fournissant une introduction à l’œuvre originale."@fr ;
    rdakit:toolkitLabel "auteur d’introduction de"@fr, "writer of introduction of"@en ;
    reg:hasSubproperty <http://rdaregistry.info/Elements/a/datatype/P50153>, <http://rdaregistry.info/Elements/a/object/P50153> ;
    reg:hasUnconstrained <http://rdaregistry.info/Elements/u/P60619> ;
    reg:lexicalAlias <http://rdaregistry.info/Elements/a/writerOfIntroductionOf.en> ;
    reg:name "writerOfIntroductionOf"@en ;
    reg:status <http://metadataregistry.org/uri/RegStatus/1001> ;
    a rdf:Property ;
    rdfs:domain <http://rdaregistry.info/Elements/c/C10002> ;
    rdfs:isDefinedBy <http://rdaregistry.info/Elements/a/> ;
    rdfs:label "est l’auteur d’introduction de"@fr, "is writer of introduction of"@en ;
    rdfs:subPropertyOf <http://rdaregistry.info/Elements/a/P50154> ;
    skos:definition "Met une personne, famille ou collectivité contribuant à une expression d’une œuvre en fournissant une introduction à l’œuvre originale en relation avec l’expression."@fr, "Relates an agent contributing to an expression of a work by providing an introduction to an original work to an expression."@en .

<http://rdaregistry.info/Elements/a/P50154>
    rdakit:instructionNumber "18.5" ;
    rdakit:toolkitDefinition "An expression of a work that incorporates a contribution of providing supplementary textual content, such as an introduction or a preface, to an original work."@en, "Personne, famille ou collectivité contribuant à une expression d’une œuvre en fournissant du contenu textuel supplémentaire (par exemple, une introduction, une préface) à l’œuvre originale."@fr ;
    rdakit:toolkitLabel "auteur de contenu textuel supplémentaire de"@fr, "writer of supplementary textual content of"@en ;
    reg:hasSubproperty <http://rdaregistry.info/Elements/a/P50138>, <http://rdaregistry.info/Elements/a/P50149>, <http://rdaregistry.info/Elements/a/P50152>, <http://rdaregistry.info/Elements/a/P50153>, <http://rdaregistry.info/Elements/a/datatype/P50154>, <http://rdaregistry.info/Elements/a/object/P50154>, <http://rdaregistry.info/Elements/a/object/P50254> ;
    reg:hasUnconstrained <http://rdaregistry.info/Elements/u/P60620> ;
    reg:lexicalAlias <http://rdaregistry.info/Elements/a/writerOfSupplementaryTextualContentOf.en> ;
    reg:name "writerOfSupplementaryTextualContentOf"@en ;
    reg:status <http://metadataregistry.org/uri/RegStatus/1001> ;
    a rdf:Property ;
    rdfs:domain <http://rdaregistry.info/Elements/c/C10002> ;
    rdfs:isDefinedBy <http://rdaregistry.info/Elements/a/> ;
    rdfs:label "est l’auteur de contenu textuel supplémentaire de"@fr, "is writer of supplementary textual content of"@en ;
    rdfs:subPropertyOf <http://rdaregistry.info/Elements/a/P50161> ;
    skos:definition "Met une personne, famille ou collectivité contribuant à une expression d’une œuvre en fournissant du contenu textuel supplémentaire (par exemple, une introduction, une préface) à l’œuvre originale en relation avec l’expression."@fr, "Relates an agent contributing to an expression of a work by providing supplementary textual content, such as an introduction or a preface, to an original work to an expression."@en .

<http://rdaregistry.info/Elements/a/P50155>
    rdakit:instructionNumber "18.5" ;
    rdakit:toolkitDefinition "An expression of a work that incorporates a contribution of responding to an interviewer, usually a reporter, pollster, or some other information gathering agent."@en, "Personne, famille ou collectivité contribuant à une expression d’une œuvre en répondant à un intervieweur, habituellement un journaliste, un sondeur ou un autre agent recueillant de l’information."@fr ;
    rdakit:toolkitLabel "interviewee (expression) of"@en, "interviewé (expression) de"@fr ;
    reg:hasSubproperty <http://rdaregistry.info/Elements/a/datatype/P50155>, <http://rdaregistry.info/Elements/a/object/P50155> ;
    reg:hasUnconstrained <http://rdaregistry.info/Elements/u/P60661> ;
    reg:lexicalAlias <http://rdaregistry.info/Elements/a/intervieweeExpressionOf.en> ;
    reg:name "intervieweeExpressionOf"@en ;
    reg:status <http://metadataregistry.org/uri/RegStatus/1001> ;
    a rdf:Property ;
    rdfs:domain <http://rdaregistry.info/Elements/c/C10002> ;
    rdfs:isDefinedBy <http://rdaregistry.info/Elements/a/> ;
    rdfs:label "est l’interviewé (expression) de"@fr, "is interviewee (expression) of"@en ;
    rdfs:subPropertyOf <http://rdaregistry.info/Elements/a/P50161> ;
    skos:definition "Met une personne, famille ou collectivité contribuant à une expression d’une œuvre en répondant à un intervieweur, habituellement un journaliste, un sondeur ou un autre agent recueillant de l’information en relation avec l’expression."@fr, "Relates an agent contributing to an expression of a work by responding to an interviewer, usually a reporter, pollster, or some other information gathering agent to an expression."@en .

<http://rdaregistry.info/Elements/a/P50156>
    rdakit:instructionNumber "18.5" ;
    rdakit:seeAlso <http://rdaregistry.info/Elements/a/P50195> ;
    rdakit:toolkitDefinition "An expression of a work that incorporates a contribution of revising or clarifying the content, or by selecting and putting together works, or parts of works, by one or more creators."@en, "Personne, famille ou collectivité contribuant à une expression d’une œuvre en révisant ou en clarifiant le contenu, ou bien en choisissant et en rassemblant des œuvres, ou des parties d’œuvres, d’un ou de plusieurs créateurs."@fr ;
    rdakit:toolkitLabel "editor of"@en, "éditeur intellectuel de"@fr ;
    reg:hasSubproperty <http://rdaregistry.info/Elements/a/datatype/P50156>, <http://rdaregistry.info/Elements/a/object/P50156> ;
    reg:hasUnconstrained <http://rdaregistry.info/Elements/u/P60621> ;
    reg:lexicalAlias <http://rdaregistry.info/Elements/a/editorOf.en> ;
    reg:name "editorOf"@en ;
    reg:status <http://metadataregistry.org/uri/RegStatus/1001> ;
    a rdf:Property ;
    rdfs:domain <http://rdaregistry.info/Elements/c/C10002> ;
    rdfs:isDefinedBy <http://rdaregistry.info/Elements/a/> ;
    rdfs:label "est l’éditeur intellectuel de"@fr, "is editor of"@en ;
    rdfs:subPropertyOf <http://rdaregistry.info/Elements/a/P50161> ;
    skos:definition "Met une personne, famille ou collectivité contribuant à une expression d’une œuvre en révisant ou en clarifiant le contenu, ou bien en choisissant et en rassemblant des œuvres, ou des parties d’œuvres, d’un ou de plusieurs créateurs en relation avec l’expression."@fr, "Relates an agent contributing to an expression of a work by revising or clarifying the content, or by selecting and putting together works, or parts of works, by one or more creators to an expression."@en ;
    skos:scopeNote "Contributions may include adding an introduction, notes, or other critical matter, or preparing the expression of a work for production, publication, or distribution."@en, "Les contributions peuvent inclure l’ajout d’une introduction, de notes ou d’autres textes critiques, ou bien la préparation de l’expression d’une œuvre aux fins de production, de publication ou de diffusion/distribution."@fr .

<http://rdaregistry.info/Elements/a/P50157>
    rdakit:instructionNumber "18.5" ;
    rdakit:seeAlso <http://rdaregistry.info/Elements/a/P50195> ;
    rdakit:toolkitDefinition "An expression of a work that incorporates a contribution of shortening or condensing the original work but leaving the nature and content substantially unchanged."@en, "Personne, famille ou collectivité contribuant à une expression d’une œuvre en abrégeant ou en condensant l’œuvre originale tout en conservant la nature et le contenu de l’œuvre originale sensiblement inchangés."@fr ;
    rdakit:toolkitLabel "abridger of"@en, "abréviateur de"@fr ;
    reg:hasSubproperty <http://rdaregistry.info/Elements/a/datatype/P50157>, <http://rdaregistry.info/Elements/a/object/P50157> ;
    reg:hasUnconstrained <http://rdaregistry.info/Elements/u/P60622> ;
    reg:lexicalAlias <http://rdaregistry.info/Elements/a/abridgerOf.en> ;
    reg:name "abridgerOf"@en ;
    reg:status <http://metadataregistry.org/uri/RegStatus/1001> ;
    a rdf:Property ;
    rdfs:domain <http://rdaregistry.info/Elements/c/C10002> ;
    rdfs:isDefinedBy <http://rdaregistry.info/Elements/a/> ;
    rdfs:label "est l’abréviateur de"@fr, "is abridger of"@en ;
    rdfs:subPropertyOf <http://rdaregistry.info/Elements/a/P50161> ;
    skos:definition "Met une personne, famille ou collectivité contribuant à une expression d’une œuvre en abrégeant ou en condensant l’œuvre originale tout en conservant la nature et le contenu de l’œuvre originale sensiblement inchangés en relation avec l’expression."@fr, "Relates an agent contributing to an expression of a work by shortening or condensing the original work but leaving the nature and content substantially unchanged to an expression."@en .

<http://rdaregistry.info/Elements/a/P50158>
    rdakit:instructionNumber "18.5" ;
    rdakit:toolkitDefinition "An expression of a work that incorporates a contribution to the audio content of supervising the technical aspects of a recording session."@en, "Personne, famille ou collectivité contribuant à une expression d’une œuvre en supervisant les aspects techniques d’une séance d’enregistrement sonore ou vidéo."@fr ;
    rdakit:toolkitLabel "ingénieur du son de"@fr, "recording engineer of"@en ;
    reg:hasSubproperty <http://rdaregistry.info/Elements/a/datatype/P50158>, <http://rdaregistry.info/Elements/a/object/P50158> ;
    reg:hasUnconstrained <http://rdaregistry.info/Elements/u/P60623> ;
    reg:lexicalAlias <http://rdaregistry.info/Elements/a/recordingEngineerOf.en> ;
    reg:name "recordingEngineerOf"@en ;
    reg:status <http://metadataregistry.org/uri/RegStatus/1001> ;
    a rdf:Property ;
    rdfs:domain <http://rdaregistry.info/Elements/c/C10002> ;
    rdfs:isDefinedBy <http://rdaregistry.info/Elements/a/> ;
    rdfs:label "est l’ingénieur du son de"@fr, "is recording engineer of"@en ;
    rdfs:subPropertyOf <http://rdaregistry.info/Elements/a/P50296> ;
    skos:definition "Met une personne, famille ou collectivité contribuant à une expression d’une œuvre en supervisant les aspects techniques d’une séance d’enregistrement sonore ou vidéo en relation avec l’expression."@fr, "Relates an audio engineer contributing to the audio content of an expression by supervising the technical aspects of a recording session to an expression."@en .

<http://rdaregistry.info/Elements/a/P50159>
    rdakit:instructionNumber "18.5" ;
    rdakit:toolkitDefinition "An expression of a work that incorporates a contribution of supplementing the primary content with drawings, diagrams, photographs, etc."@en, "Personne, famille ou collectivité contribuant à une expression d’une œuvre en complétant le contenu principal avec des dessins, des diagrammes, des photographies, etc."@fr ;
    rdakit:toolkitLabel "illustrateur de"@fr, "illustrator of"@en ;
    reg:hasSubproperty <http://rdaregistry.info/Elements/a/datatype/P50159>, <http://rdaregistry.info/Elements/a/object/P50159>, <http://rdaregistry.info/Elements/a/object/P50245> ;
    reg:hasUnconstrained <http://rdaregistry.info/Elements/u/P60624> ;
    reg:lexicalAlias <http://rdaregistry.info/Elements/a/illustratorOf.en> ;
    reg:name "illustratorOf"@en ;
    reg:status <http://metadataregistry.org/uri/RegStatus/1001> ;
    a rdf:Property ;
    rdfs:domain <http://rdaregistry.info/Elements/c/C10002> ;
    rdfs:isDefinedBy <http://rdaregistry.info/Elements/a/> ;
    rdfs:label "est l’illustrateur de"@fr, "is illustrator of"@en ;
    rdfs:subPropertyOf <http://rdaregistry.info/Elements/a/P50161> ;
    skos:definition "Met une personne, famille ou collectivité contribuant à une expression d’une œuvre en complétant le contenu principal avec des dessins, des diagrammes, des photographies, etc. en relation avec l’expression."@fr, "Relates an agent contributing to an expression of a work by supplementing the primary content with drawings, diagrams, photographs, etc. to an expression."@en .

<http://rdaregistry.info/Elements/a/P50160>
    rdakit:instructionNumber "18.5" ;
    rdakit:toolkitDefinition "An expression of a work that incorporates a contribution of using a recording device to capture sound and/or video during a recording session, including field recordings of natural sounds, folkloric events, music, etc."@en, "Personne, famille ou collectivité contribuant à une expression d’une œuvre en utilisant un appareil d’enregistrement pour capter le son et/ou la vidéo durant une séance d’enregistrement, y compris les enregistrements de terrain de sons naturels, de prestations folkloriques, de musique, etc."@fr ;
    rdakit:toolkitLabel "opérateur d’enregistrement de"@fr, "recordist of"@en ;
    reg:hasSubproperty <http://rdaregistry.info/Elements/a/datatype/P50160>, <http://rdaregistry.info/Elements/a/object/P50160> ;
    reg:hasUnconstrained <http://rdaregistry.info/Elements/u/P60625> ;
    reg:lexicalAlias <http://rdaregistry.info/Elements/a/recordistOf.en> ;
    reg:name "recordistOf"@en ;
    reg:status <http://metadataregistry.org/uri/RegStatus/1001> ;
    a rdf:Property ;
    rdfs:domain <http://rdaregistry.info/Elements/c/C10002> ;
    rdfs:isDefinedBy <http://rdaregistry.info/Elements/a/> ;
    rdfs:label "est l’opérateur d’enregistrement de"@fr, "is recordist of"@en ;
    rdfs:subPropertyOf <http://rdaregistry.info/Elements/a/P50161> ;
    skos:definition "Met une personne, famille ou collectivité contribuant à une expression d’une œuvre en utilisant un appareil d’enregistrement pour capter le son et/ou la vidéo durant une séance d’enregistrement, y compris les enregistrements de terrain de sons naturels, de prestations folkloriques, de musique, etc., en relation avec l’expression."@fr, "Relates an agent contributing to an expression of a work by using a recording device to capture sound and/or video during a recording session, including field recordings of natural sounds, folkloric events, music, etc. to an expression."@en .

<http://rdaregistry.info/Elements/a/P50161>
    rdakit:toolkitDefinition "An expression that incorporates a contribution."@en, "Personne, famille ou collectivité contribuant à une expression."@fr ;
    rdakit:toolkitLabel "contributeur de"@fr, "contributor of"@en ;
    reg:hasSubproperty <http://rdaregistry.info/Elements/a/P50134>, <http://rdaregistry.info/Elements/a/P50135>, <http://rdaregistry.info/Elements/a/P50136>, <http://rdaregistry.info/Elements/a/P50137>, <http://rdaregistry.info/Elements/a/P50139>, <http://rdaregistry.info/Elements/a/P50140>, <http://rdaregistry.info/Elements/a/P50141>, <http://rdaregistry.info/Elements/a/P50142>, <http://rdaregistry.info/Elements/a/P50143>, <http://rdaregistry.info/Elements/a/P50144>, <http://rdaregistry.info/Elements/a/P50145>, <http://rdaregistry.info/Elements/a/P50146>, <http://rdaregistry.info/Elements/a/P50147>, <http://rdaregistry.info/Elements/a/P50150>, <http://rdaregistry.info/Elements/a/P50151>, <http://rdaregistry.info/Elements/a/P50154>, <http://rdaregistry.info/Elements/a/P50155>, <http://rdaregistry.info/Elements/a/P50156>, <http://rdaregistry.info/Elements/a/P50157>, <http://rdaregistry.info/Elements/a/P50158>, <http://rdaregistry.info/Elements/a/P50159>, <http://rdaregistry.info/Elements/a/P50160>, <http://rdaregistry.info/Elements/a/P50183>, <http://rdaregistry.info/Elements/a/P50198>, <http://rdaregistry.info/Elements/a/P50212>, <http://rdaregistry.info/Elements/a/datatype/P50161>, <http://rdaregistry.info/Elements/a/object/P50161>, <http://rdaregistry.info/Elements/a/object/P50180>, <http://rdaregistry.info/Elements/a/object/P50243>, <http://rdaregistry.info/Elements/a/object/P50244>, <http://rdaregistry.info/Elements/a/object/P50255>, <http://rdaregistry.info/Elements/a/object/P50256>, <http://rdaregistry.info/Elements/a/object/P50261>, <http://rdaregistry.info/Elements/a/object/P50263>, <http://rdaregistry.info/Elements/a/object/P50266>, <http://rdaregistry.info/Elements/a/object/P50267>, <http://rdaregistry.info/Elements/a/object/P50271>, <http://rdaregistry.info/Elements/a/object/P50272>, <http://rdaregistry.info/Elements/a/object/P50273>, <http://rdaregistry.info/Elements/a/object/P50296>, <http://rdaregistry.info/Elements/a/object/P50298>, <http://rdaregistry.info/Elements/a/object/P50299>, <http://rdaregistry.info/Elements/a/object/P50300> ;
    reg:hasUnconstrained <http://rdaregistry.info/Elements/u/P60626> ;
    reg:lexicalAlias <http://rdaregistry.info/Elements/a/contributorOf.en> ;
    reg:name "contributorOf"@en ;
    reg:status <http://metadataregistry.org/uri/RegStatus/1001> ;
    a rdf:Property ;
    rdfs:domain <http://rdaregistry.info/Elements/c/C10002> ;
    rdfs:isDefinedBy <http://rdaregistry.info/Elements/a/> ;
    rdfs:label "est le contributeur de"@fr, "is contributor of"@en ;
    rdfs:subPropertyOf <http://rdaregistry.info/Elements/a/P50306> ;
    skos:definition "Met une personne, famille ou collectivité contribuant à une expression en relation avec l’expression."@fr, "Relates an agent contributing to an expression to an expression."@en ;
    skos:scopeNote "Editors, translators, arrangers of music, performers, etc., are included."@en, "Les contributeurs incluent les éditeurs intellectuels, les traducteurs, les arrangeurs de musique, les interprètes, etc."@fr .

<http://rdaregistry.info/Elements/a/P50162>
    rdakit:instructionNumber "18.5" ;
    rdakit:toolkitDefinition "An item currently in the legal possession of an agent."@en, "Personne, famille ou collectivité possédant légalement un item."@fr ;
    rdakit:toolkitLabel "current owner of"@en, "propriétaire actuel de"@fr ;
    reg:hasSubproperty <http://rdaregistry.info/Elements/a/P50047>, <http://rdaregistry.info/Elements/a/datatype/P50162>, <http://rdaregistry.info/Elements/a/object/P50162> ;
    reg:hasUnconstrained <http://rdaregistry.info/Elements/u/P60628> ;
    reg:lexicalAlias <http://rdaregistry.info/Elements/a/currentOwnerOf.en> ;
    reg:name "currentOwnerOf"@en ;
    reg:status <http://metadataregistry.org/uri/RegStatus/1001> ;
    a rdf:Property ;
    rdfs:domain <http://rdaregistry.info/Elements/c/C10002> ;
    rdfs:isDefinedBy <http://rdaregistry.info/Elements/a/> ;
    rdfs:label "est le propriétaire actuel de"@fr, "is current owner of"@en ;
    rdfs:subPropertyOf <http://rdaregistry.info/Elements/a/P50165> ;
    skos:definition "Met une personne, famille ou collectivité possédant légalement un item en relation avec l’item."@fr, "Relates an agent currently having legal possession of an item to an item."@en .

<http://rdaregistry.info/Elements/a/P50163>
    rdakit:instructionNumber "18.5" ;
    rdakit:toolkitDefinition "An item formerly in the legal possession of an agent."@en, "Personne, famille ou collectivité ayant auparavant possédé légalement un item."@fr ;
    rdakit:toolkitLabel "ancien propriétaire de"@fr, "former owner of"@en ;
    reg:hasSubproperty <http://rdaregistry.info/Elements/a/P50066>, <http://rdaregistry.info/Elements/a/P50067>, <http://rdaregistry.info/Elements/a/datatype/P50163>, <http://rdaregistry.info/Elements/a/object/P50163> ;
    reg:hasUnconstrained <http://rdaregistry.info/Elements/u/P60630> ;
    reg:lexicalAlias <http://rdaregistry.info/Elements/a/formerOwnerOf.en> ;
    reg:name "formerOwnerOf"@en ;
    reg:status <http://metadataregistry.org/uri/RegStatus/1001> ;
    a rdf:Property ;
    rdfs:domain <http://rdaregistry.info/Elements/c/C10002> ;
    rdfs:isDefinedBy <http://rdaregistry.info/Elements/a/> ;
    rdfs:label "est l’ancien propriétaire de"@fr, "is former owner of"@en ;
    rdfs:subPropertyOf <http://rdaregistry.info/Elements/a/P50165> ;
    skos:definition "Met une personne, famille ou collectivité ayant auparavant possédé légalement un item en relation avec l’item."@fr, "Relates an agent formerly having legal possession of an item to an item."@en .

<http://rdaregistry.info/Elements/a/P50164>
    rdakit:instructionNumber "18.5" ;
    rdakit:toolkitDefinition "An item in the legal custody of an agent."@en, "Personne, famille ou collectivité à qui est confiée la garde légale d’un item."@fr ;
    rdakit:toolkitLabel "custodian of"@en, "dépositaire de"@fr ;
    reg:hasSubproperty <http://rdaregistry.info/Elements/a/datatype/P50164>, <http://rdaregistry.info/Elements/a/object/P50164> ;
    reg:hasUnconstrained <http://rdaregistry.info/Elements/u/P60631> ;
    reg:lexicalAlias <http://rdaregistry.info/Elements/a/custodianOf.en> ;
    reg:name "custodianOf"@en ;
    reg:status <http://metadataregistry.org/uri/RegStatus/1001> ;
    a rdf:Property ;
    rdfs:domain <http://rdaregistry.info/Elements/c/C10002> ;
    rdfs:isDefinedBy <http://rdaregistry.info/Elements/a/> ;
    rdfs:label "est le dépositaire de"@fr, "is custodian of"@en ;
    rdfs:subPropertyOf <http://rdaregistry.info/Elements/a/P50308> ;
    skos:definition "Met une personne, famille ou collectivité à qui est confiée la garde légale d’un item en relation avec l’item."@fr, "Relates an agent having legal custody of an item to an item."@en .

<http://rdaregistry.info/Elements/a/P50165>
    rdakit:toolkitDefinition "An item in the legal possession of an agent."@en, "Personne, famille ou collectivité possédant légalement un item."@fr ;
    rdakit:toolkitLabel "owner of"@en, "propriétaire de"@fr ;
    reg:hasSubproperty <http://rdaregistry.info/Elements/a/P50162>, <http://rdaregistry.info/Elements/a/P50163>, <http://rdaregistry.info/Elements/a/datatype/P50165>, <http://rdaregistry.info/Elements/a/object/P50165> ;
    reg:hasUnconstrained <http://rdaregistry.info/Elements/u/P60632> ;
    reg:lexicalAlias <http://rdaregistry.info/Elements/a/ownerOf.en> ;
    reg:name "ownerOf"@en ;
    reg:status <http://metadataregistry.org/uri/RegStatus/1001> ;
    a rdf:Property ;
    rdfs:domain <http://rdaregistry.info/Elements/c/C10002> ;
    rdfs:isDefinedBy <http://rdaregistry.info/Elements/a/> ;
    rdfs:label "est le propriétaire de"@fr, "is owner of"@en ;
    rdfs:subPropertyOf <http://rdaregistry.info/Elements/a/P50308> ;
    skos:definition "Met une personne, famille ou collectivité possédant légalement un item en relation avec l’item."@fr, "Relates an agent having legal possession of an item to an item."@en .

<http://rdaregistry.info/Elements/a/P50166>
    rdakit:instructionNumber "18.5" ;
    rdakit:toolkitDefinition "A work honouring an agent."@en, "Personne, famille ou collectivité honorée par une œuvre (par exemple, une personne à qui sont offerts des mélanges)."@fr ;
    rdakit:toolkitLabel "entité honorée de"@fr, "honouree of"@en ;
    reg:hasSubproperty <http://rdaregistry.info/Elements/a/datatype/P50166>, <http://rdaregistry.info/Elements/a/object/P50166> ;
    reg:hasUnconstrained <http://rdaregistry.info/Elements/u/P60634> ;
    reg:lexicalAlias <http://rdaregistry.info/Elements/a/honoureeOf.en> ;
    reg:name "honoureeOf"@en ;
    reg:status <http://metadataregistry.org/uri/RegStatus/1001> ;
    a rdf:Property ;
    rdfs:domain <http://rdaregistry.info/Elements/c/C10002> ;
    rdfs:isDefinedBy <http://rdaregistry.info/Elements/a/> ;
    rdfs:label "est l’entité honorée de"@fr, "is honouree of"@en ;
    rdfs:subPropertyOf <http://rdaregistry.info/Elements/a/P50131> ;
    skos:altLabel "honoree of"@en ;
    skos:definition "Met une personne, famille ou collectivité honorée par une œuvre (par exemple, une personne à qui sont offerts des mélanges) en relation avec l’œuvre."@fr, "Relates an agent honoured by a work to a work."@en .

<http://rdaregistry.info/Elements/a/P50167>
    rdakit:instructionNumber "18.5" ;
    rdakit:toolkitDefinition "An item honouring an agent."@en, "Personne, famille ou collectivité honorée par un item, par exemple, une personne à qui un exemplaire est offert."@fr ;
    rdakit:toolkitLabel "entité honorée (item) de"@fr, "honouree (item) of"@en ;
    reg:hasSubproperty <http://rdaregistry.info/Elements/a/datatype/P50167>, <http://rdaregistry.info/Elements/a/object/P50167> ;
    reg:hasUnconstrained <http://rdaregistry.info/Elements/u/P60634> ;
    reg:lexicalAlias <http://rdaregistry.info/Elements/a/honoureeOfItemOf.en> ;
    reg:name "honoureeOfItemOf"@en ;
    reg:status <http://metadataregistry.org/uri/RegStatus/1001> ;
    a rdf:Property ;
    rdfs:domain <http://rdaregistry.info/Elements/c/C10002> ;
    rdfs:isDefinedBy <http://rdaregistry.info/Elements/a/> ;
    rdfs:label "est l’entité honorée (item) de"@fr, "is honouree (item) of"@en ;
    rdfs:subPropertyOf <http://rdaregistry.info/Elements/a/P50182> ;
    skos:altLabel "honoree (item) of"@en ;
    skos:definition "Met une personne, famille ou collectivité honorée par un item, par exemple, une personne à qui un exemplaire est offert, en relation avec l’item."@fr, "Relates an agent honoured by an item to an item."@en .

<http://rdaregistry.info/Elements/a/P50168>
    rdakit:instructionNumber "18.5" ;
    rdakit:toolkitDefinition "A manifestation that is broadcast to an audience via radio, television, webcast, etc."@en, "Personne, famille ou collectivité prenant part à la diffusion d’une manifestation à un public par la radio, la télévision, la webdiffusion, etc."@fr ;
    rdakit:toolkitLabel "broadcaster of"@en, "diffuseur de"@fr ;
    reg:hasSubproperty <http://rdaregistry.info/Elements/a/datatype/P50168>, <http://rdaregistry.info/Elements/a/object/P50168> ;
    reg:hasUnconstrained <http://rdaregistry.info/Elements/u/P60635> ;
    reg:lexicalAlias <http://rdaregistry.info/Elements/a/broadcasterOf.en> ;
    reg:name "broadcasterOf"@en ;
    reg:status <http://metadataregistry.org/uri/RegStatus/1001> ;
    a rdf:Property ;
    rdfs:domain <http://rdaregistry.info/Elements/c/C10002> ;
    rdfs:isDefinedBy <http://rdaregistry.info/Elements/a/> ;
    rdfs:label "est le diffuseur de"@fr, "is broadcaster of"@en ;
    rdfs:subPropertyOf <http://rdaregistry.info/Elements/a/P50203> ;
    skos:definition "Met une personne, famille ou collectivité prenant part à la diffusion d’une manifestation à un public par la radio, la télévision, la webdiffusion, etc. en relation avec la manifestation."@fr, "Relates an agent involved in broadcasting a manifestation to an audience via radio, television, webcast, etc. to a manifestation."@en .

<http://rdaregistry.info/Elements/a/P50169>
    rdakit:instructionNumber "18.5" ;
    rdakit:toolkitDefinition "A moving image manifestation distributed to theatres or other distribution channels."@en, "Personne, famille ou collectivité prenant part à la distribution d’une manifestation d’images animées aux salles de cinéma ou aux autres réseaux de distribution."@fr ;
    rdakit:toolkitLabel "distributeur de films de"@fr, "film distributor of"@en ;
    reg:hasSubproperty <http://rdaregistry.info/Elements/a/datatype/P50169>, <http://rdaregistry.info/Elements/a/object/P50169> ;
    reg:hasUnconstrained <http://rdaregistry.info/Elements/u/P60636> ;
    reg:lexicalAlias <http://rdaregistry.info/Elements/a/filmDistributorOf.en> ;
    reg:name "filmDistributorOf"@en ;
    reg:status <http://metadataregistry.org/uri/RegStatus/1001> ;
    a rdf:Property ;
    rdfs:domain <http://rdaregistry.info/Elements/c/C10002> ;
    rdfs:isDefinedBy <http://rdaregistry.info/Elements/a/> ;
    rdfs:label "est le distributeur de films de"@fr, "is film distributor of"@en ;
    rdfs:subPropertyOf <http://rdaregistry.info/Elements/a/P50199> ;
    skos:definition "Met une personne, famille ou collectivité prenant part à la distribution d’une manifestation d’images animées aux salles de cinéma ou aux autres réseaux de distribution en relation avec la manifestation."@fr, "Relates an agent involved in distributing a moving image manifestation to theatres or other distribution channels to a manifestation."@en .

<http://rdaregistry.info/Elements/a/P50170>
    rdakit:instructionNumber "18.5" ;
    rdakit:toolkitDefinition "A manifestation manufactured by an agent responsible for the entire graphic design of a book, including arrangement of type and illustration, choice of materials, and process used."@en, "Personne, famille ou collectivité prenant part à la fabrication d’une manifestation en étant responsable de toute la conception graphique d’un livre, y compris la composition typographique, l’arrangement des illustrations, le choix des matériaux et le processus utilisé."@fr ;
    rdakit:toolkitLabel "book designer of"@en, "graphiste de"@fr ;
    reg:hasSubproperty <http://rdaregistry.info/Elements/a/datatype/P50170>, <http://rdaregistry.info/Elements/a/object/P50170> ;
    reg:hasUnconstrained <http://rdaregistry.info/Elements/u/P60637> ;
    reg:lexicalAlias <http://rdaregistry.info/Elements/a/bookDesignerOf.en> ;
    reg:name "bookDesignerOf"@en ;
    reg:status <http://metadataregistry.org/uri/RegStatus/1001> ;
    a rdf:Property ;
    rdfs:domain <http://rdaregistry.info/Elements/c/C10002> ;
    rdfs:isDefinedBy <http://rdaregistry.info/Elements/a/> ;
    rdfs:label "est le graphiste de"@fr, "is book designer of"@en ;
    rdfs:subPropertyOf <http://rdaregistry.info/Elements/a/P50202> ;
    skos:definition "Met une personne, famille ou collectivité prenant part à la fabrication d’une manifestation en étant responsable de toute la conception graphique d’un livre, y compris la composition typographique, l’arrangement des illustrations, le choix des matériaux et le processus utilisé, en relation avec la manifestation."@fr, "Relates an agent involved in manufacturing a manifestation by being responsible for the entire graphic design of a book, including arrangement of type and illustration, choice of materials, and process used to a manifestation."@en .

<http://rdaregistry.info/Elements/a/P50171>
    rdakit:instructionNumber "18.5" ;
    rdakit:toolkitDefinition "A manifestation manufactured by an agent responsible for cutting letters, figures, etc., on a surface such as a wooden or metal plate used for printing."@en, "Personne, famille ou collectivité prenant part à la fabrication d’une manifestation en gravant des lettres, des figures, etc. sur une surface telle qu’une plaque de bois ou de métal utilisée pour l’impression."@fr ;
    rdakit:toolkitLabel "engraver of"@en, "graveur de"@fr ;
    reg:hasSubproperty <http://rdaregistry.info/Elements/a/datatype/P50171>, <http://rdaregistry.info/Elements/a/object/P50171> ;
    reg:hasUnconstrained <http://rdaregistry.info/Elements/u/P60638> ;
    reg:lexicalAlias <http://rdaregistry.info/Elements/a/engraverOf.en> ;
    reg:name "engraverOf"@en ;
    reg:status <http://metadataregistry.org/uri/RegStatus/1001> ;
    a rdf:Property ;
    rdfs:domain <http://rdaregistry.info/Elements/c/C10002> ;
    rdfs:isDefinedBy <http://rdaregistry.info/Elements/a/> ;
    rdfs:label "est le graveur de"@fr, "is engraver of"@en ;
    rdfs:subPropertyOf <http://rdaregistry.info/Elements/a/P50202> ;
    skos:definition "Met une personne, famille ou collectivité prenant part à la fabrication d’une manifestation en gravant des lettres, des figures, etc. sur une surface telle qu’une plaque de bois ou de métal utilisée pour l’impression en relation avec la manifestation."@fr, "Relates an agent involved in manufacturing a manifestation by cutting letters, figures, etc., on a surface such as a wooden or metal plate used for printing to a manifestation."@en .

<http://rdaregistry.info/Elements/a/P50172>
    rdakit:instructionNumber "18.5" ;
    rdakit:toolkitDefinition "A manifestation manufactured by an agent responsible for embossing braille cells using a stylus, special embossing printer, or other device."@en, "Personne, famille ou collectivité prenant part à la fabrication d’une manifestation par l’embossage de cellules braille au moyen d’un poinçon, d’une imprimante spéciale ou d’un autre appareil."@fr ;
    rdakit:toolkitLabel "braille embosser of"@en, "producteur braille de"@fr ;
    reg:hasSubproperty <http://rdaregistry.info/Elements/a/datatype/P50172>, <http://rdaregistry.info/Elements/a/object/P50172> ;
    reg:hasUnconstrained <http://rdaregistry.info/Elements/u/P60639> ;
    reg:lexicalAlias <http://rdaregistry.info/Elements/a/brailleEmbosserOf.en> ;
    reg:name "brailleEmbosserOf"@en ;
    reg:status <http://metadataregistry.org/uri/RegStatus/1001> ;
    a rdf:Property ;
    rdfs:domain <http://rdaregistry.info/Elements/c/C10002> ;
    rdfs:isDefinedBy <http://rdaregistry.info/Elements/a/> ;
    rdfs:label "est le producteur braille de"@fr, "is braille embosser of"@en ;
    rdfs:subPropertyOf <http://rdaregistry.info/Elements/a/P50202> ;
    skos:definition "Met une personne, famille ou collectivité prenant part à la fabrication d’une manifestation par l’embossage de cellules braille au moyen d’un poinçon, d’une imprimante spéciale ou d’un autre appareil en relation avec la manifestation."@fr, "Relates an agent involved in manufacturing a manifestation by embossing braille cells using a stylus, special embossing printer, or other device to a manifestation."@en .

<http://rdaregistry.info/Elements/a/P50173>
    rdakit:instructionNumber "18.5" ;
    rdakit:toolkitDefinition "A manifestation manufactured by an agent responsible for making a relief, intaglio, or planographic printing surface."@en, "Personne, famille ou collectivité prenant part à la fabrication d’une manifestation en préparant un élément d’impression en relief, en creux ou planographique."@fr ;
    rdakit:toolkitLabel "graveur d’estampes de"@fr, "printmaker of"@en ;
    reg:hasSubproperty <http://rdaregistry.info/Elements/a/datatype/P50173>, <http://rdaregistry.info/Elements/a/object/P50173> ;
    reg:hasUnconstrained <http://rdaregistry.info/Elements/u/P60640> ;
    reg:lexicalAlias <http://rdaregistry.info/Elements/a/printmakerOf.en> ;
    reg:name "printmakerOf"@en ;
    reg:status <http://metadataregistry.org/uri/RegStatus/1001> ;
    a rdf:Property ;
    rdfs:domain <http://rdaregistry.info/Elements/c/C10002> ;
    rdfs:isDefinedBy <http://rdaregistry.info/Elements/a/> ;
    rdfs:label "est le graveur d’estampes de"@fr, "is printmaker of"@en ;
    rdfs:subPropertyOf <http://rdaregistry.info/Elements/a/P50202> ;
    skos:definition "Met une personne, famille ou collectivité prenant part à la fabrication d’une manifestation en préparant un élément d’impression en relief, en creux ou planographique en relation avec la manifestation."@fr, "Relates an agent involved in manufacturing a manifestation by making a relief, intaglio, or planographic printing surface to a manifestation."@en .

<http://rdaregistry.info/Elements/a/P50174>
    rdakit:instructionNumber "18.5" ;
    rdakit:toolkitDefinition "A manifestation manufactured by an agent responsible for pouring a liquid or molten substance into a mold and leaving it to solidify to take the shape of the mold."@en, "Personne, famille ou collectivité prenant part à la fabrication d’une manifestation en versant un liquide ou une substance fondue dans un moule et en laissant ce liquide ou cette substance se solidifier pour prendre la forme du moule."@fr ;
    rdakit:toolkitLabel "caster of"@en, "fondeur de"@fr ;
    reg:hasSubproperty <http://rdaregistry.info/Elements/a/datatype/P50174>, <http://rdaregistry.info/Elements/a/object/P50174> ;
    reg:hasUnconstrained <http://rdaregistry.info/Elements/u/P60641> ;
    reg:lexicalAlias <http://rdaregistry.info/Elements/a/casterOf.en> ;
    reg:name "casterOf"@en ;
    reg:status <http://metadataregistry.org/uri/RegStatus/1001> ;
    a rdf:Property ;
    rdfs:domain <http://rdaregistry.info/Elements/c/C10002> ;
    rdfs:isDefinedBy <http://rdaregistry.info/Elements/a/> ;
    rdfs:label "est le fondeur de"@fr, "is caster of"@en ;
    rdfs:subPropertyOf <http://rdaregistry.info/Elements/a/P50202> ;
    skos:definition "Met une personne, famille ou collectivité prenant part à la fabrication d’une manifestation en versant un liquide ou une substance fondue dans un moule et en laissant ce liquide ou cette substance se solidifier pour prendre la forme du moule en relation avec la manifestation."@fr, "Relates an agent involved in manufacturing a manifestation by pouring a liquid or molten substance into a mold and leaving it to solidify to take the shape of the mold to a manifestation."@en .

<http://rdaregistry.info/Elements/a/P50175>
    rdakit:instructionNumber "18.5" ;
    rdakit:toolkitDefinition "A manifestation manufactured by an agent responsible for preparing a stone or plate for lithographic printing, including a graphic artist creating a design directly on the surface from which printing will be done."@en, "Personne, famille ou collectivité prenant part à la fabrication d’une manifestation en préparant une pierre ou une plaque pour l’impression lithographique, y compris un artiste graphique créant un dessin directement sur la surface à partir de laquelle l’impression sera effectuée."@fr ;
    rdakit:toolkitLabel "lithographe de"@fr, "lithographer of"@en ;
    reg:hasSubproperty <http://rdaregistry.info/Elements/a/datatype/P50175>, <http://rdaregistry.info/Elements/a/object/P50175> ;
    reg:hasUnconstrained <http://rdaregistry.info/Elements/u/P60642> ;
    reg:lexicalAlias <http://rdaregistry.info/Elements/a/lithographerOf.en> ;
    reg:name "lithographerOf"@en ;
    reg:status <http://metadataregistry.org/uri/RegStatus/1001> ;
    a rdf:Property ;
    rdfs:domain <http://rdaregistry.info/Elements/c/C10002> ;
    rdfs:isDefinedBy <http://rdaregistry.info/Elements/a/> ;
    rdfs:label "est le lithographe de"@fr, "is lithographer of"@en ;
    rdfs:subPropertyOf <http://rdaregistry.info/Elements/a/P50202> ;
    skos:definition "Met une personne, famille ou collectivité prenant part à la fabrication d’une manifestation en préparant une pierre ou une plaque pour l’impression lithographique, y compris un artiste graphique créant un dessin directement sur la surface à partir de laquelle l’impression sera effectuée, en relation avec la manifestation."@fr, "Relates an agent involved in manufacturing a manifestation by preparing a stone or plate for lithographic printing, including a graphic artist creating a design directly on the surface from which printing will be done to a manifestation."@en .

<http://rdaregistry.info/Elements/a/P50176>
    rdakit:instructionNumber "18.5" ;
    rdakit:toolkitDefinition "A manifestation manufactured by an agent responsible for preparing plates used in the production of printed images and/or text."@en, "Personne, famille ou collectivité prenant part à la fabrication d’une manifestation en préparant les planches utilisées dans la production d’images et/ou de textes imprimés."@fr ;
    rdakit:toolkitLabel "graveur de planches de"@fr, "platemaker of"@en ;
    reg:hasSubproperty <http://rdaregistry.info/Elements/a/datatype/P50176>, <http://rdaregistry.info/Elements/a/object/P50176> ;
    reg:hasUnconstrained <http://rdaregistry.info/Elements/u/P60643> ;
    reg:lexicalAlias <http://rdaregistry.info/Elements/a/platemakerOf.en> ;
    reg:name "platemakerOf"@en ;
    reg:status <http://metadataregistry.org/uri/RegStatus/1001> ;
    a rdf:Property ;
    rdfs:domain <http://rdaregistry.info/Elements/c/C10002> ;
    rdfs:isDefinedBy <http://rdaregistry.info/Elements/a/> ;
    rdfs:label "est le graveur de planches de"@fr, "is platemaker of"@en ;
    rdfs:subPropertyOf <http://rdaregistry.info/Elements/a/P50202> ;
    skos:definition "Met une personne, famille ou collectivité prenant part à la fabrication d’une manifestation en préparant les planches utilisées dans la production d’images et/ou de textes imprimés en relation avec la manifestation."@fr, "Relates an agent involved in manufacturing a manifestation by preparing plates used in the production of printed images or text to a manifestation."@en .

<http://rdaregistry.info/Elements/a/P50177>
    rdakit:instructionNumber "18.5" ;
    rdakit:toolkitDefinition "A manifestation manufactured by an agent responsible for subjecting metal, glass, or some other surface used for printing, to acid or another corrosive substance."@en, "Personne, famille ou collectivité prenant part à la fabrication d’une manifestation en soumettant à l’acide ou à une autre substance corrosive du métal, du verre ou une autre surface utilisée pour l’impression."@fr ;
    rdakit:toolkitLabel "aquafortiste de"@fr, "etcher of"@en ;
    reg:hasSubproperty <http://rdaregistry.info/Elements/a/datatype/P50177>, <http://rdaregistry.info/Elements/a/object/P50177> ;
    reg:hasUnconstrained <http://rdaregistry.info/Elements/u/P60644> ;
    reg:lexicalAlias <http://rdaregistry.info/Elements/a/etcherOf.en> ;
    reg:name "etcherOf"@en ;
    reg:status <http://metadataregistry.org/uri/RegStatus/1001> ;
    a rdf:Property ;
    rdfs:domain <http://rdaregistry.info/Elements/c/C10002> ;
    rdfs:isDefinedBy <http://rdaregistry.info/Elements/a/> ;
    rdfs:label "est l’aquafortiste de"@fr, "is etcher of"@en ;
    rdfs:subPropertyOf <http://rdaregistry.info/Elements/a/P50202> ;
    skos:definition "Met une personne, famille ou collectivité prenant part à la fabrication d’une manifestation en soumettant à l’acide ou à une autre substance corrosive du métal, du verre ou une autre surface utilisée pour l’impression en relation avec la manifestation."@fr, "Relates an agent involved in manufacturing a manifestation by subjecting metal, glass, or some other surface used for printing, to acid or another corrosive substance to a manifestation."@en .

<http://rdaregistry.info/Elements/a/P50178>
    rdakit:instructionNumber "18.5" ;
    rdakit:toolkitDefinition "A manifestation manufactured by an agent responsible for using a photomechanical process for making prints directly from a hardened film of gelatin or other colloid that has ink-receptive and ink-repellent surfaces."@en, "Personne, famille ou collectivité prenant part à la fabrication d’une manifestation d’épreuves photographiques faites à partir d’un film de gélatine ou d’un autre colloïde ayant des surfaces acceptant ou repoussant l’encre."@fr ;
    rdakit:toolkitLabel "collotyper of"@en, "phototypeur de"@fr ;
    reg:hasSubproperty <http://rdaregistry.info/Elements/a/datatype/P50178>, <http://rdaregistry.info/Elements/a/object/P50178> ;
    reg:hasUnconstrained <http://rdaregistry.info/Elements/u/P60645> ;
    reg:lexicalAlias <http://rdaregistry.info/Elements/a/collotyperOf.en> ;
    reg:name "collotyperOf"@en ;
    reg:status <http://metadataregistry.org/uri/RegStatus/1001> ;
    a rdf:Property ;
    rdfs:domain <http://rdaregistry.info/Elements/c/C10002> ;
    rdfs:isDefinedBy <http://rdaregistry.info/Elements/a/> ;
    rdfs:label "est le phototypeur de"@fr, "is collotyper of"@en ;
    rdfs:subPropertyOf <http://rdaregistry.info/Elements/a/P50202> ;
    skos:definition "Met une personne, famille ou collectivité prenant part à la fabrication d’une manifestation d’épreuves photographiques faites à partir d’un film de gélatine ou d’un autre colloïde ayant des surfaces acceptant ou repoussant l’encre en relation avec la manifestation."@fr, "Relates an agent involved in manufacturing a manifestation using a photomechanical process for making prints directly from a hardened film of gelatin or other colloid that has ink-receptive and ink-repellent surfaces to a manifestation."@en .

<http://rdaregistry.info/Elements/a/P50179>
    rdakit:instructionNumber "18.5" ;
    rdakit:toolkitDefinition "A manifestation of printed text, notated music, etc., manufactured by an agent from type or plates, such as a book, newspaper, magazine, broadside, score, etc."@en, "Personne, famille ou collectivité prenant part à la fabrication d’une manifestation de texte imprimé, de musique notée, etc. à partir de caractères ou de planches, telle qu’un livre, un journal, une revue, un placard, une partition, etc."@fr ;
    rdakit:toolkitLabel "imprimeur de"@fr, "printer of"@en ;
    reg:hasSubproperty <http://rdaregistry.info/Elements/a/datatype/P50179>, <http://rdaregistry.info/Elements/a/object/P50179> ;
    reg:hasUnconstrained <http://rdaregistry.info/Elements/u/P60646> ;
    reg:lexicalAlias <http://rdaregistry.info/Elements/a/printerOf.en> ;
    reg:name "printerOf"@en ;
    reg:status <http://metadataregistry.org/uri/RegStatus/1001> ;
    a rdf:Property ;
    rdfs:domain <http://rdaregistry.info/Elements/c/C10002> ;
    rdfs:isDefinedBy <http://rdaregistry.info/Elements/a/> ;
    rdfs:label "est l’imprimeur de"@fr, "is printer of"@en ;
    rdfs:subPropertyOf <http://rdaregistry.info/Elements/a/P50202> ;
    skos:definition "Met une personne, famille ou collectivité prenant part à la fabrication d’une manifestation de texte imprimé, de musique notée, etc. à partir de caractères ou de planches, telle qu’un livre, un journal, une revue, un placard, une partition, etc., en relation avec la manifestation."@fr, "Relates an agent involved in manufacturing a manifestation of printed text, notated music, etc., from type or plates, such as a book, newspaper, magazine, broadside, score, etc. to a manifestation."@en .

<http://rdaregistry.info/Elements/a/P50180>
    rdakit:instructionNumber "18.5" ;
    rdakit:toolkitDefinition "A manifestation for moving image materials with an \"X presents:\" credit for an agent who is probably associated with production, finance, or distribution in some way."@en, "Personne, famille ou collectivité mentionnée dans un générique d’images animées sous la forme « X présente » et qui est probablement associée d’une façon quelconque à la production, au financement ou à la distribution."@fr ;
    rdakit:toolkitLabel "presenter of"@en, "présentateur de"@fr ;
    reg:hasSubproperty <http://rdaregistry.info/Elements/a/datatype/P50180>, <http://rdaregistry.info/Elements/a/object/P50180> ;
    reg:hasUnconstrained <http://rdaregistry.info/Elements/u/P60647> ;
    reg:lexicalAlias <http://rdaregistry.info/Elements/a/presenterOf.en> ;
    reg:name "presenterOf"@en ;
    reg:status <http://metadataregistry.org/uri/RegStatus/1001> ;
    a rdf:Property ;
    rdfs:domain <http://rdaregistry.info/Elements/c/C10002> ;
    rdfs:isDefinedBy <http://rdaregistry.info/Elements/a/> ;
    rdfs:label "est le présentateur de"@fr, "is presenter of"@en ;
    rdfs:subPropertyOf <http://rdaregistry.info/Elements/a/P50161> ;
    skos:definition "Met une personne, famille ou collectivité mentionnée dans un générique d’images animées sous la forme « X présente » et qui est probablement associée d’une façon quelconque à la production, au financement ou à la distribution en relation avec l’expression."@fr, "Relates an agent mentioned in an \"X presents:\" credit for moving image materials and who is probably associated with production, finance, or distribution in some way to an expression."@en .

<http://rdaregistry.info/Elements/a/P50181>
    rdakit:toolkitDefinition "A manifestation associated with an agent other than a producer, publisher, distributor, or manufacturer."@en, "Personne, famille ou collectivité, autre qu’un producteur, un éditeur, un diffuseur ou distributeur ou bien un fabricant, associée à une manifestation."@fr ;
    rdakit:toolkitLabel "autre personne, famille ou collectivité associée à une manifestation de"@fr, "other person, family, or corporate body associated with a manifestation of"@en ;
    reg:hasSubproperty <http://rdaregistry.info/Elements/a/datatype/P50181>, <http://rdaregistry.info/Elements/a/object/P50181> ;
    reg:hasUnconstrained <http://rdaregistry.info/Elements/u/P60602> ;
    reg:lexicalAlias <http://rdaregistry.info/Elements/a/otherPFCManifestationOf.en> ;
    reg:name "otherPFCManifestationOf"@en ;
    reg:status <http://metadataregistry.org/uri/RegStatus/1001> ;
    a rdf:Property ;
    rdfs:domain <http://rdaregistry.info/Elements/c/C10002> ;
    rdfs:isDefinedBy <http://rdaregistry.info/Elements/a/> ;
    rdfs:label "est l’autre personne, famille ou collectivité associée à une manifestation de"@fr, "is other person, family, or corporate body associated with a manifestation of"@en ;
    rdfs:subPropertyOf <http://rdaregistry.info/Elements/a/P50307> ;
    skos:definition "Met une personne, famille ou collectivité, autre qu’un producteur, un éditeur, un diffuseur ou distributeur ou bien un fabricant, associée à une manifestation en relation avec la manifestation."@fr, "Relates an agent other than a producer, publisher, distributor, or manufacturer associated with a manifestation to a manifestation."@en ;
    skos:scopeNote "Book designers, platemakers, etc., are included."@en, "Comprend les graphistes, les graveurs de planches, etc."@fr .

<http://rdaregistry.info/Elements/a/P50182>
    rdakit:toolkitDefinition "An item associated with an agent other than an owner or custodian."@en, "Personne, famille ou collectivité, autre qu’un propriétaire ou un dépositaire, associée à un item."@fr ;
    rdakit:toolkitLabel "autre personne, famille ou collectivité associée à un item de"@fr, "other person, family, or corporate body associated with an item of"@en ;
    reg:hasSubproperty <http://rdaregistry.info/Elements/a/P50092>, <http://rdaregistry.info/Elements/a/P50123>, <http://rdaregistry.info/Elements/a/P50125>, <http://rdaregistry.info/Elements/a/P50128>, <http://rdaregistry.info/Elements/a/P50129>, <http://rdaregistry.info/Elements/a/P50133>, <http://rdaregistry.info/Elements/a/P50167>, <http://rdaregistry.info/Elements/a/P50206>, <http://rdaregistry.info/Elements/a/P50210>, <http://rdaregistry.info/Elements/a/datatype/P50182>, <http://rdaregistry.info/Elements/a/object/P50182> ;
    reg:hasUnconstrained <http://rdaregistry.info/Elements/u/P60602> ;
    reg:lexicalAlias <http://rdaregistry.info/Elements/a/otherPFCItemOf.en> ;
    reg:name "otherPFCItemOf"@en ;
    reg:status <http://metadataregistry.org/uri/RegStatus/1001> ;
    a rdf:Property ;
    rdfs:domain <http://rdaregistry.info/Elements/c/C10002> ;
    rdfs:isDefinedBy <http://rdaregistry.info/Elements/a/> ;
    rdfs:label "est l’autre personne, famille ou collectivité associée à un item de"@fr, "is other person, family, or corporate body associated with an item of"@en ;
    rdfs:subPropertyOf <http://rdaregistry.info/Elements/a/P50308> ;
    skos:definition "Met une personne, famille ou collectivité, autre qu’un propriétaire ou un dépositaire, associée à un item en relation avec l’item."@fr, "Relates an agent other than an owner or custodian associated with an item to an item."@en ;
    skos:scopeNote "Comprend les conservateurs, les relieurs, les restaurateurs, etc."@fr, "Curators, binders, restorationists, etc., are included."@en .

<http://rdaregistry.info/Elements/a/P50183>
    rdakit:instructionNumber "18.5" ;
    rdakit:toolkitDefinition "An expression that incorporates a contribution of assembling, arranging, and trimming film, video, or other moving image formats, including both visual and audio aspects."@en, "Personne, famille ou collectivité responsable de l’assemblage, de l’arrangement et du découpage de film, de vidéo ou d’autres formats d’images animées, y compris les aspects visuels et sonores."@fr ;
    rdakit:toolkitLabel "editor of moving image work of"@en, "monteur d’œuvre d’images animées de"@fr ;
    reg:hasSubproperty <http://rdaregistry.info/Elements/a/datatype/P50183>, <http://rdaregistry.info/Elements/a/object/P50183> ;
    reg:hasUnconstrained <http://rdaregistry.info/Elements/u/P60651> ;
    reg:lexicalAlias <http://rdaregistry.info/Elements/a/editorOfMovingImageWorkOf.en> ;
    reg:name "editorOfMovingImageWorkOf"@en ;
    reg:status <http://metadataregistry.org/uri/RegStatus/1001> ;
    a rdf:Property ;
    rdfs:domain <http://rdaregistry.info/Elements/c/C10002> ;
    rdfs:isDefinedBy <http://rdaregistry.info/Elements/a/> ;
    rdfs:label "est le monteur d’œuvre d’images animées de"@fr, "is editor of moving image work of"@en ;
    rdfs:subPropertyOf <http://rdaregistry.info/Elements/a/P50161> ;
    skos:definition "Met une personne, famille ou collectivité responsable de l’assemblage, de l’arrangement et du découpage de film, de vidéo ou d’autres formats d’images animées, y compris les aspects visuels et sonores, en relation avec l’expression."@fr, "Relates an agent responsible for assembling, arranging, and trimming film, video, or other moving image formats, including both visual and audio aspects to an expression."@en .

<http://rdaregistry.info/Elements/a/P50184>
    rdakit:instructionNumber "18.5" ;
    rdakit:toolkitDefinition "A work that involves a creation responsibility for a computer program."@en, "Personne, famille ou collectivité responsable de la création d’un programme informatique."@fr ;
    rdakit:toolkitLabel "programmer of"@en, "programmeur de"@fr ;
    reg:hasSubproperty <http://rdaregistry.info/Elements/a/datatype/P50184>, <http://rdaregistry.info/Elements/a/object/P50184> ;
    reg:hasUnconstrained <http://rdaregistry.info/Elements/u/P60652> ;
    reg:lexicalAlias <http://rdaregistry.info/Elements/a/programmerOf.en> ;
    reg:name "programmerOf"@en ;
    reg:status <http://metadataregistry.org/uri/RegStatus/1001> ;
    a rdf:Property ;
    rdfs:domain <http://rdaregistry.info/Elements/c/C10002> ;
    rdfs:isDefinedBy <http://rdaregistry.info/Elements/a/> ;
    rdfs:label "est le programmeur de"@fr, "is programmer of"@en ;
    rdfs:subPropertyOf <http://rdaregistry.info/Elements/a/P50204> ;
    skos:definition "Met une personne, famille ou collectivité responsable de la création d’un programme informatique en relation avec l’œuvre."@fr, "Relates an agent responsible for creating a computer program to a work."@en .

<http://rdaregistry.info/Elements/a/P50185>
    rdakit:instructionNumber "18.5" ;
    rdakit:toolkitDefinition "A work that involves a creation responsibility for a design for an object."@en, "Personne, famille ou collectivité responsable de la conception d’un objet."@fr ;
    rdakit:toolkitLabel "designer de"@fr, "designer of"@en ;
    reg:hasSubproperty <http://rdaregistry.info/Elements/a/datatype/P50185>, <http://rdaregistry.info/Elements/a/object/P50185> ;
    reg:hasUnconstrained <http://rdaregistry.info/Elements/u/P60653> ;
    reg:lexicalAlias <http://rdaregistry.info/Elements/a/designerOf.en> ;
    reg:name "designerOf"@en ;
    reg:status <http://metadataregistry.org/uri/RegStatus/1001> ;
    a rdf:Property ;
    rdfs:domain <http://rdaregistry.info/Elements/c/C10002> ;
    rdfs:isDefinedBy <http://rdaregistry.info/Elements/a/> ;
    rdfs:label "est le designer de"@fr, "is designer of"@en ;
    rdfs:subPropertyOf <http://rdaregistry.info/Elements/a/P50204> ;
    skos:definition "Met une personne, famille ou collectivité responsable de la conception d’un objet en relation avec l’œuvre."@fr, "Relates an agent responsible for creating a design for an object to a work."@en .

<http://rdaregistry.info/Elements/a/P50186>
    rdakit:instructionNumber "18.5" ;
    rdakit:toolkitDefinition "A cartographic work that involves a creation responsibility for a map, atlas, globe, etc."@en, "Personne, famille ou collectivité responsable de la création d’une carte, d’un atlas, d’un globe ou d’une autre œuvre cartographique."@fr ;
    rdakit:toolkitLabel "cartographe de"@fr, "cartographer of"@en ;
    reg:hasSubproperty <http://rdaregistry.info/Elements/a/datatype/P50186>, <http://rdaregistry.info/Elements/a/object/P50186> ;
    reg:hasUnconstrained <http://rdaregistry.info/Elements/u/P60654> ;
    reg:lexicalAlias <http://rdaregistry.info/Elements/a/cartographerOf.en> ;
    reg:name "cartographerOf"@en ;
    reg:status <http://metadataregistry.org/uri/RegStatus/1001> ;
    a rdf:Property ;
    rdfs:domain <http://rdaregistry.info/Elements/c/C10002> ;
    rdfs:isDefinedBy <http://rdaregistry.info/Elements/a/> ;
    rdfs:label "est le cartographe de"@fr, "is cartographer of"@en ;
    rdfs:subPropertyOf <http://rdaregistry.info/Elements/a/P50204> ;
    skos:definition "Met une personne, famille ou collectivité responsable de la création d’une carte, d’un atlas, d’un globe ou d’une autre œuvre cartographique en relation avec l’œuvre."@fr, "Relates an agent responsible for creating a map, atlas, globe, or other cartographic work to a work."@en .

<http://rdaregistry.info/Elements/a/P50187>
    rdakit:instructionNumber "18.5" ;
    rdakit:toolkitDefinition "A musical work that involves a creation responsibility."@en, "Personne, famille ou collectivité responsable de la création d’une œuvre musicale."@fr ;
    rdakit:toolkitLabel "composer of"@en, "compositeur de"@fr ;
    reg:hasSubproperty <http://rdaregistry.info/Elements/a/datatype/P50187>, <http://rdaregistry.info/Elements/a/object/P50187> ;
    reg:hasUnconstrained <http://rdaregistry.info/Elements/u/P60655> ;
    reg:lexicalAlias <http://rdaregistry.info/Elements/a/composerOf.en> ;
    reg:name "composerOf"@en ;
    reg:status <http://metadataregistry.org/uri/RegStatus/1001> ;
    a rdf:Property ;
    rdfs:domain <http://rdaregistry.info/Elements/c/C10002> ;
    rdfs:isDefinedBy <http://rdaregistry.info/Elements/a/> ;
    rdfs:label "est le compositeur de"@fr, "is composer of"@en ;
    rdfs:subPropertyOf <http://rdaregistry.info/Elements/a/P50204> ;
    skos:definition "Met une personne, famille ou collectivité responsable de la création d’une œuvre musicale en relation avec l’œuvre."@fr, "Relates an agent responsible for creating a musical work to a work."@en .

<http://rdaregistry.info/Elements/a/P50188>
    rdakit:instructionNumber "18.5" ;
    rdakit:toolkitDefinition "A work that involves a creation responsibility for a new device or process."@en, "Personne, famille ou collectivité responsable de la création d’un nouveau dispositif ou procédé."@fr ;
    rdakit:toolkitLabel "inventeur de"@fr, "inventor of"@en ;
    reg:hasSubproperty <http://rdaregistry.info/Elements/a/datatype/P50188>, <http://rdaregistry.info/Elements/a/object/P50188> ;
    reg:hasUnconstrained <http://rdaregistry.info/Elements/u/P60656> ;
    reg:lexicalAlias <http://rdaregistry.info/Elements/a/inventorOf.en> ;
    reg:name "inventorOf"@en ;
    reg:status <http://metadataregistry.org/uri/RegStatus/1001> ;
    a rdf:Property ;
    rdfs:domain <http://rdaregistry.info/Elements/c/C10002> ;
    rdfs:isDefinedBy <http://rdaregistry.info/Elements/a/> ;
    rdfs:label "est l’inventeur de"@fr, "is inventor of"@en ;
    rdfs:subPropertyOf <http://rdaregistry.info/Elements/a/P50204> ;
    skos:definition "Met une personne, famille ou collectivité responsable de la création d’un nouveau dispositif ou procédé en relation avec l’œuvre."@fr, "Relates an agent responsible for creating a new device or process to a work."@en .

<http://rdaregistry.info/Elements/a/P50189>
    rdakit:instructionNumber "18.5" ;
    rdakit:seeAlso <http://rdaregistry.info/Elements/a/P50156> ;
    rdakit:toolkitDefinition "A work that involves a creation responsibility for a new work such as a bibliography or a directory by selecting, arranging, aggregating, and editing data, information, etc."@en, "Personne, famille ou collectivité responsable de la création d’une nouvelle œuvre (par exemple, une bibliographie, un répertoire) en sélectionnant, en organisant, en regroupant et en éditant des données, de l’information, etc."@fr ;
    rdakit:toolkitLabel "compilateur de"@fr, "compiler of"@en ;
    reg:hasSubproperty <http://rdaregistry.info/Elements/a/datatype/P50189>, <http://rdaregistry.info/Elements/a/object/P50189> ;
    reg:hasUnconstrained <http://rdaregistry.info/Elements/u/P60657> ;
    reg:lexicalAlias <http://rdaregistry.info/Elements/a/compilerOf.en> ;
    reg:name "compilerOf"@en ;
    reg:status <http://metadataregistry.org/uri/RegStatus/1001> ;
    a rdf:Property ;
    rdfs:domain <http://rdaregistry.info/Elements/c/C10002> ;
    rdfs:isDefinedBy <http://rdaregistry.info/Elements/a/> ;
    rdfs:label "est le compilateur de"@fr, "is compiler of"@en ;
    rdfs:subPropertyOf <http://rdaregistry.info/Elements/a/P50204> ;
    skos:definition "Met une personne, famille ou collectivité responsable de la création d’une nouvelle œuvre (par exemple, une bibliographie, un répertoire) en sélectionnant, en organisant, en regroupant et en éditant des données, de l’information, etc. en relation avec l’œuvre."@fr, "Relates an agent responsible for creating a new work such as a bibliography or a directory by selecting, arranging, aggregating, and editing data, information, etc., to a work."@en .

<http://rdaregistry.info/Elements/a/P50190>
    rdakit:instructionNumber "18.5" ;
    rdakit:toolkitDefinition "A photographic work that involves a creation responsibility."@en, "Personne, famille ou collectivité responsable de la création d’une œuvre photographique."@fr ;
    rdakit:toolkitLabel "photographe de"@fr, "photographer of"@en ;
    reg:hasSubproperty <http://rdaregistry.info/Elements/a/datatype/P50190>, <http://rdaregistry.info/Elements/a/object/P50190> ;
    reg:hasUnconstrained <http://rdaregistry.info/Elements/u/P60658> ;
    reg:lexicalAlias <http://rdaregistry.info/Elements/a/photographerOf.en> ;
    reg:name "photographerOf"@en ;
    reg:status <http://metadataregistry.org/uri/RegStatus/1001> ;
    a rdf:Property ;
    rdfs:domain <http://rdaregistry.info/Elements/c/C10002> ;
    rdfs:isDefinedBy <http://rdaregistry.info/Elements/a/> ;
    rdfs:label "est le photographe de"@fr, "is photographer of"@en ;
    rdfs:subPropertyOf <http://rdaregistry.info/Elements/a/P50204> ;
    skos:definition "Met une personne, famille ou collectivité responsable de la création d’une œuvre photographique en relation avec l’œuvre."@fr, "Relates an agent responsible for creating a photographic work to a work."@en .

<http://rdaregistry.info/Elements/a/P50191>
    rdakit:instructionNumber "18.5" ;
    rdakit:toolkitDefinition "A work that involves a creation responsibility for acting as an interviewer, reporter, pollster, or some other information gathering agent."@en, "Personne, famille ou collectivité responsable de la création d’une œuvre en agissant à titre d’intervieweur, de journaliste, de sondeur ou d’autre agent recueillant de l’information."@fr ;
    rdakit:toolkitLabel "interviewer of"@en, "intervieweur de"@fr ;
    reg:hasSubproperty <http://rdaregistry.info/Elements/a/datatype/P50191>, <http://rdaregistry.info/Elements/a/object/P50191> ;
    reg:hasUnconstrained <http://rdaregistry.info/Elements/u/P60659> ;
    reg:lexicalAlias <http://rdaregistry.info/Elements/a/interviewerOf.en> ;
    reg:name "interviewerOf"@en ;
    reg:status <http://metadataregistry.org/uri/RegStatus/1001> ;
    a rdf:Property ;
    rdfs:domain <http://rdaregistry.info/Elements/c/C10002> ;
    rdfs:isDefinedBy <http://rdaregistry.info/Elements/a/> ;
    rdfs:label "est l’intervieweur de"@fr, "is interviewer of"@en ;
    rdfs:subPropertyOf <http://rdaregistry.info/Elements/a/P50204> ;
    skos:definition "Met une personne, famille ou collectivité responsable de la création d’une œuvre en agissant à titre d’intervieweur, de journaliste, de sondeur ou d’autre agent recueillant de l’information en relation avec l’œuvre."@fr, "Relates an agent responsible for creating a work by acting as an interviewer, reporter, pollster, or some other information gathering agent to a work."@en .

<http://rdaregistry.info/Elements/a/P50192>
    rdakit:instructionNumber "18.5" ;
    rdakit:toolkitDefinition "A work that involves a creation responsibility for conceiving, and often implementing, an original graphic design, drawing, painting, etc."@en, "Personne, famille ou collectivité responsable de la création d’une œuvre par la conception et souvent par la réalisation d’un graphisme, d’une peinture, d’un dessin, etc. original."@fr ;
    rdakit:toolkitLabel "artist of"@en, "artiste de"@fr ;
    reg:hasSubproperty <http://rdaregistry.info/Elements/a/P50222>, <http://rdaregistry.info/Elements/a/datatype/P50192>, <http://rdaregistry.info/Elements/a/object/P50192>, <http://rdaregistry.info/Elements/a/object/P50246>, <http://rdaregistry.info/Elements/a/object/P50247> ;
    reg:hasUnconstrained <http://rdaregistry.info/Elements/u/P60660> ;
    reg:lexicalAlias <http://rdaregistry.info/Elements/a/artistOf.en> ;
    reg:name "artistOf"@en ;
    reg:status <http://metadataregistry.org/uri/RegStatus/1001> ;
    a rdf:Property ;
    rdfs:domain <http://rdaregistry.info/Elements/c/C10002> ;
    rdfs:isDefinedBy <http://rdaregistry.info/Elements/a/> ;
    rdfs:label "est l’artiste de"@fr, "is artist of"@en ;
    rdfs:subPropertyOf <http://rdaregistry.info/Elements/a/P50204> ;
    skos:definition "Met une personne, famille ou collectivité responsable de la création d’une œuvre par la conception et souvent par la réalisation d’un graphisme, d’une peinture, d’un dessin, etc. original en relation avec l’œuvre."@fr, "Relates an agent responsible for creating a work by conceiving, and often implementing, an original graphic design, drawing, painting, etc. to a work."@en .

<http://rdaregistry.info/Elements/a/P50193>
    rdakit:instructionNumber "18.5" ;
    rdakit:toolkitDefinition "A work that involves a creation responsibility for responding to an interviewer, usually a reporter, pollster, or some other information gathering agent."@en, "Personne, famille ou collectivité responsable de la création d’une œuvre en répondant à un intervieweur, habituellement un journaliste, un sondeur ou un autre agent recueillant de l’information."@fr ;
    rdakit:toolkitLabel "interviewee of"@en, "interviewé de"@fr ;
    reg:hasSubproperty <http://rdaregistry.info/Elements/a/datatype/P50193>, <http://rdaregistry.info/Elements/a/object/P50193> ;
    reg:hasUnconstrained <http://rdaregistry.info/Elements/u/P60661> ;
    reg:lexicalAlias <http://rdaregistry.info/Elements/a/intervieweeOf.en> ;
    reg:name "intervieweeOf"@en ;
    reg:status <http://metadataregistry.org/uri/RegStatus/1001> ;
    a rdf:Property ;
    rdfs:domain <http://rdaregistry.info/Elements/c/C10002> ;
    rdfs:isDefinedBy <http://rdaregistry.info/Elements/a/> ;
    rdfs:label "est l’interviewé de"@fr, "is interviewee of"@en ;
    rdfs:subPropertyOf <http://rdaregistry.info/Elements/a/P50204> ;
    skos:definition "Met une personne, famille ou collectivité responsable de la création d’une œuvre en répondant à un intervieweur, habituellement un journaliste, un sondeur ou un autre agent recueillant de l’information en relation avec l’œuvre."@fr, "Relates an agent responsible for creating a work by responding to an interviewer, usually a reporter, pollster, or some other information gathering agent to a work."@en .

<http://rdaregistry.info/Elements/a/P50194>
    rdakit:instructionNumber "18.5" ;
    rdakit:toolkitDefinition "A work of movement that involves a creation responsibility."@en, "Personne, famille ou collectivité responsable de la création d’une œuvre de mouvement."@fr ;
    rdakit:toolkitLabel "choreographer of"@en, "chorégraphe de"@fr ;
    reg:hasSubproperty <http://rdaregistry.info/Elements/a/datatype/P50194>, <http://rdaregistry.info/Elements/a/object/P50194> ;
    reg:hasUnconstrained <http://rdaregistry.info/Elements/u/P60662> ;
    reg:lexicalAlias <http://rdaregistry.info/Elements/a/choreographerOf.en> ;
    reg:name "choreographerOf"@en ;
    reg:status <http://metadataregistry.org/uri/RegStatus/1001> ;
    a rdf:Property ;
    rdfs:domain <http://rdaregistry.info/Elements/c/C10002> ;
    rdfs:isDefinedBy <http://rdaregistry.info/Elements/a/> ;
    rdfs:label "est le chorégraphe de"@fr, "is choreographer of"@en ;
    rdfs:subPropertyOf <http://rdaregistry.info/Elements/a/P50204> ;
    skos:definition "Met une personne, famille ou collectivité responsable de la création d’une œuvre de mouvement en relation avec l’œuvre."@fr, "Relates an agent responsible for creating a work of movement to a work."@en .

<http://rdaregistry.info/Elements/a/P50195>
    rdakit:instructionNumber "18.5" ;
    rdakit:toolkitDefinition "A work that is primarily textual in content, regardless of media  type or genre, that involves a creation responsibility."@en, "Personne, famille ou collectivité responsable de la création d’une œuvre dont le contenu est principalement textuel quel que soit le type de média (par exemple, texte imprimé, parole énoncée, texte électronique, texte tactile) ou le genre (par exemple, poèmes, romans, scénarios, blogues)."@fr ;
    rdakit:toolkitLabel "auteur de"@fr, "author of"@en ;
    reg:hasSubproperty <http://rdaregistry.info/Elements/a/P50223>, <http://rdaregistry.info/Elements/a/P50224>, <http://rdaregistry.info/Elements/a/P50225>, <http://rdaregistry.info/Elements/a/datatype/P50195>, <http://rdaregistry.info/Elements/a/object/P50195>, <http://rdaregistry.info/Elements/a/object/P50248> ;
    reg:hasUnconstrained <http://rdaregistry.info/Elements/u/P60663> ;
    reg:lexicalAlias <http://rdaregistry.info/Elements/a/authorOf.en> ;
    reg:name "authorOf"@en ;
    reg:status <http://metadataregistry.org/uri/RegStatus/1001> ;
    a rdf:Property ;
    rdfs:domain <http://rdaregistry.info/Elements/c/C10002> ;
    rdfs:isDefinedBy <http://rdaregistry.info/Elements/a/> ;
    rdfs:label "est l’auteur de"@fr, "is author of"@en ;
    rdfs:subPropertyOf <http://rdaregistry.info/Elements/a/P50204> ;
    skos:definition "Met une personne, famille ou collectivité responsable de la création d’une œuvre dont le contenu est principalement textuel quel que soit le type de média (par exemple, texte imprimé, parole énoncée, texte électronique, texte tactile) ou le genre (par exemple, poèmes, romans, scénarios, blogues) en relation avec l’œuvre."@fr, "Relates an agent responsible for creating a work that is primarily textual in content, regardless of media  type or genre to a work."@en .

<http://rdaregistry.info/Elements/a/P50196>
    rdakit:instructionNumber "18.5" ;
    rdakit:toolkitDefinition "A work that involves a responsibility for creating an architectural design, including a pictorial representation intended to show how a building, etc., will look when completed."@en, "Personne, famille ou collectivité responsable d’une création architecturale, y compris une représentation illustrée conçue pour montrer de quoi aura l’air un bâtiment, etc. une fois terminé."@fr ;
    rdakit:toolkitLabel "architect of"@en, "architecte de"@fr ;
    reg:hasSubproperty <http://rdaregistry.info/Elements/a/P50221>, <http://rdaregistry.info/Elements/a/datatype/P50196>, <http://rdaregistry.info/Elements/a/object/P50196> ;
    reg:hasUnconstrained <http://rdaregistry.info/Elements/u/P60664> ;
    reg:lexicalAlias <http://rdaregistry.info/Elements/a/architectOf.en> ;
    reg:name "architectOf"@en ;
    reg:status <http://metadataregistry.org/uri/RegStatus/1001> ;
    a rdf:Property ;
    rdfs:domain <http://rdaregistry.info/Elements/c/C10002> ;
    rdfs:isDefinedBy <http://rdaregistry.info/Elements/a/> ;
    rdfs:label "est l’architecte de"@fr, "is architect of"@en ;
    rdfs:subPropertyOf <http://rdaregistry.info/Elements/a/P50204> ;
    skos:definition "Met une personne, famille ou collectivité responsable d’une création architecturale, y compris une représentation illustrée conçue pour montrer de quoi aura l’air un bâtiment, etc. une fois terminé, en relation avec l’œuvre."@fr, "Relates an agent responsible for creating an architectural design, including a pictorial representation intended to show how a building, etc., will look when completed to a work."@en .

<http://rdaregistry.info/Elements/a/P50197>
    rdakit:instructionNumber "18.5" ;
    rdakit:toolkitDefinition "A work that involves a creation responsibility for an independent or personal film."@en, "Personne, famille ou collectivité responsable de la création d’un film indépendant ou personnel."@fr ;
    rdakit:toolkitLabel "cinéaste de"@fr, "filmmaker of"@en ;
    reg:hasSubproperty <http://rdaregistry.info/Elements/a/datatype/P50197>, <http://rdaregistry.info/Elements/a/object/P50197> ;
    reg:hasUnconstrained <http://rdaregistry.info/Elements/u/P60665> ;
    reg:lexicalAlias <http://rdaregistry.info/Elements/a/filmmakerOf.en> ;
    reg:name "filmmakerOf"@en ;
    reg:status <http://metadataregistry.org/uri/RegStatus/1001> ;
    a rdf:Property ;
    rdfs:domain <http://rdaregistry.info/Elements/c/C10002> ;
    rdfs:isDefinedBy <http://rdaregistry.info/Elements/a/> ;
    rdfs:label "est le cinéaste de"@fr, "is filmmaker of"@en ;
    rdfs:subPropertyOf <http://rdaregistry.info/Elements/a/P50204> ;
    skos:definition "Met une personne, famille ou collectivité responsable de la création d’un film indépendant ou personnel en relation avec l’œuvre."@fr, "Relates an agent responsible for creating an independent or personal film to a work."@en ;
    skos:scopeNote "A filmmaker is individually responsible for the conception and execution of all aspects of the film."@en, "Un cinéaste est responsable à titre individuel de la conception et de l’exécution de tous les aspects du film."@fr .

<http://rdaregistry.info/Elements/a/P50198>
    rdakit:instructionNumber "18.5" ;
    rdakit:toolkitDefinition "An expression that incorporates a contribution of designing the overall visual appearance of a moving image production."@en, "Personne, famille ou collectivité responsable de concevoir l’aspect visuel global d’une production d’images animées."@fr ;
    rdakit:toolkitLabel "chef décorateur de"@fr, "production designer of"@en ;
    reg:hasSubproperty <http://rdaregistry.info/Elements/a/datatype/P50198>, <http://rdaregistry.info/Elements/a/object/P50198> ;
    reg:hasUnconstrained <http://rdaregistry.info/Elements/u/P60666> ;
    reg:lexicalAlias <http://rdaregistry.info/Elements/a/productionDesignerOf.en> ;
    reg:name "productionDesignerOf"@en ;
    reg:status <http://metadataregistry.org/uri/RegStatus/1001> ;
    a rdf:Property ;
    rdfs:domain <http://rdaregistry.info/Elements/c/C10002> ;
    rdfs:isDefinedBy <http://rdaregistry.info/Elements/a/> ;
    rdfs:label "est le chef décorateur de"@fr, "is production designer of"@en ;
    rdfs:subPropertyOf <http://rdaregistry.info/Elements/a/P50161> ;
    skos:definition "Met une personne, famille ou collectivité responsable de concevoir l’aspect visuel global d’une production d’images animées en relation avec l’expression."@fr, "Relates an agent responsible for designing the overall visual appearance of a moving image production to an expression."@en .

<http://rdaregistry.info/Elements/a/P50199>
    rdakit:toolkitDefinition "A manifestation that is distributed."@en, "Personne, famille ou collectivité responsable de la diffusion ou de la distribution d’une ressource."@fr ;
    rdakit:toolkitLabel "diffuseur ou distributeur de"@fr, "distributor of"@en ;
    reg:hasSubproperty <http://rdaregistry.info/Elements/a/P50169>, <http://rdaregistry.info/Elements/a/datatype/P50199>, <http://rdaregistry.info/Elements/a/object/P50199> ;
    reg:hasUnconstrained <http://rdaregistry.info/Elements/u/P60667> ;
    reg:lexicalAlias <http://rdaregistry.info/Elements/a/distributorOf.en> ;
    reg:name "distributorOf"@en ;
    reg:status <http://metadataregistry.org/uri/RegStatus/1001> ;
    a rdf:Property ;
    rdfs:domain <http://rdaregistry.info/Elements/c/C10002> ;
    rdfs:isDefinedBy <http://rdaregistry.info/Elements/a/> ;
    rdfs:label "est le diffuseur ou distributeur de"@fr, "is distributor of"@en ;
    rdfs:subPropertyOf <http://rdaregistry.info/Elements/a/P50307> ;
    skos:definition "Met une personne, famille ou collectivité responsable de la diffusion ou de la distribution d’une ressource en relation avec la manifestation."@fr, "Relates an agent responsible for distributing a manifestation to a manifestation."@en .

<http://rdaregistry.info/Elements/a/P50200>
    rdakit:toolkitDefinition "A manifestation that is inscribed, fabricated, constructed, etc."@en, "Personne, famille ou collectivité responsable de la scription, de la fabrication, de la construction, etc. d’une ressource sous une forme non publiée."@fr ;
    rdakit:toolkitLabel "producer of an unpublished resource of"@en, "producteur d’une ressource non publiée de"@fr ;
    reg:hasSubproperty <http://rdaregistry.info/Elements/a/datatype/P50200>, <http://rdaregistry.info/Elements/a/object/P50200> ;
    reg:hasUnconstrained <http://rdaregistry.info/Elements/u/P60817> ;
    reg:lexicalAlias <http://rdaregistry.info/Elements/a/producerOfAnUnpublishedResourceOf.en> ;
    reg:name "producerOfAnUnpublishedResourceOf"@en ;
    reg:status <http://metadataregistry.org/uri/RegStatus/1001> ;
    a rdf:Property ;
    rdfs:domain <http://rdaregistry.info/Elements/c/C10002> ;
    rdfs:isDefinedBy <http://rdaregistry.info/Elements/a/> ;
    rdfs:label "est le producteur d’une ressource non publiée de"@fr, "is producer of an unpublished resource of"@en ;
    rdfs:subPropertyOf <http://rdaregistry.info/Elements/a/P50307> ;
    skos:definition "Met une personne, famille ou collectivité responsable de la scription, de la fabrication, de la construction, etc. d’une ressource sous une forme non publiée en relation avec la manifestation."@fr, "Relates an agent responsible for inscribing, fabricating, constructing, etc. to a manifestation."@en .

<http://rdaregistry.info/Elements/a/P50201>
    rdakit:toolkitDefinition "A work that involves a responsibility for most of the business aspects of a production for screen, sound recording, television, webcast, etc."@en, "Personne, famille ou collectivité responsable de la majeure partie des aspects financiers, techniques et artistiques de la production d’un film, d’un enregistrement audio, d’une émission de télévision, d’une webémission, etc."@fr ;
    rdakit:toolkitLabel "producer of"@en, "producteur de"@fr ;
    reg:hasSubproperty <http://rdaregistry.info/Elements/a/P50213>, <http://rdaregistry.info/Elements/a/P50214>, <http://rdaregistry.info/Elements/a/P50215>, <http://rdaregistry.info/Elements/a/datatype/P50201>, <http://rdaregistry.info/Elements/a/object/P50201>, <http://rdaregistry.info/Elements/a/object/P50295> ;
    reg:hasUnconstrained <http://rdaregistry.info/Elements/u/P60668> ;
    reg:lexicalAlias <http://rdaregistry.info/Elements/a/producerOf.en> ;
    reg:name "producerOf"@en ;
    reg:status <http://metadataregistry.org/uri/RegStatus/1001> ;
    a rdf:Property ;
    rdfs:domain <http://rdaregistry.info/Elements/c/C10002> ;
    rdfs:isDefinedBy <http://rdaregistry.info/Elements/a/> ;
    rdfs:label "est le producteur de"@fr, "is producer of"@en ;
    rdfs:subPropertyOf <http://rdaregistry.info/Elements/a/P50307> ;
    skos:definition "Met une personne, famille ou collectivité responsable de la majeure partie des aspects financiers, techniques et artistiques de la production d’un film, d’un enregistrement audio, d’une émission de télévision, d’une webémission, etc. en relation avec l’œuvre."@fr, "Relates an agent responsible for most of the business aspects of a production for screen, sound recording, television, webcast, etc. to a work."@en ;
    skos:scopeNote "A producer is generally responsible for fund raising, managing the production, hiring key personnel, arranging for distributors, etc."@en, "Le producteur est généralement responsable d’assurer le financement, de gérer la production, de recruter le personnel clé, d’organiser la distribution, etc."@fr .

<http://rdaregistry.info/Elements/a/P50202>
    rdakit:toolkitDefinition "A manifestation that is printed, duplicated, cast, etc."@en, "Personne, famille ou collectivité responsable de l’impression, de la reproduction, du moulage, etc. d’une ressource sous une forme publiée."@fr ;
    rdakit:toolkitLabel "fabricant de"@fr, "manufacturer of"@en ;
    reg:hasSubproperty <http://rdaregistry.info/Elements/a/P50170>, <http://rdaregistry.info/Elements/a/P50171>, <http://rdaregistry.info/Elements/a/P50172>, <http://rdaregistry.info/Elements/a/P50173>, <http://rdaregistry.info/Elements/a/P50174>, <http://rdaregistry.info/Elements/a/P50175>, <http://rdaregistry.info/Elements/a/P50176>, <http://rdaregistry.info/Elements/a/P50177>, <http://rdaregistry.info/Elements/a/P50178>, <http://rdaregistry.info/Elements/a/P50179>, <http://rdaregistry.info/Elements/a/datatype/P50202>, <http://rdaregistry.info/Elements/a/object/P50202>, <http://rdaregistry.info/Elements/a/object/P50242> ;
    reg:hasUnconstrained <http://rdaregistry.info/Elements/u/P60669> ;
    reg:lexicalAlias <http://rdaregistry.info/Elements/a/manufacturerOf.en> ;
    reg:name "manufacturerOf"@en ;
    reg:status <http://metadataregistry.org/uri/RegStatus/1001> ;
    a rdf:Property ;
    rdfs:domain <http://rdaregistry.info/Elements/c/C10002> ;
    rdfs:isDefinedBy <http://rdaregistry.info/Elements/a/> ;
    rdfs:label "est le fabricant de"@fr, "is manufacturer of"@en ;
    rdfs:subPropertyOf <http://rdaregistry.info/Elements/a/P50307> ;
    skos:definition "Met une personne, famille ou collectivité responsable de l’impression, de la reproduction, du moulage, etc. d’une ressource sous une forme publiée en relation avec la manifestation."@fr, "Relates an agent responsible for printing, duplicating, casting, etc. to a manifestation."@en .

<http://rdaregistry.info/Elements/a/P50203>
    rdakit:toolkitDefinition "A manifestation that is published, released, or issued."@en, "Personne, famille ou collectivité responsable de la publication, de la mise à disposition ou de l’édition d’une ressource."@fr ;
    rdakit:toolkitLabel "publisher of"@en, "éditeur de"@fr ;
    reg:hasSubproperty <http://rdaregistry.info/Elements/a/P50168>, <http://rdaregistry.info/Elements/a/datatype/P50203>, <http://rdaregistry.info/Elements/a/object/P50203> ;
    reg:hasUnconstrained <http://rdaregistry.info/Elements/u/P60670> ;
    reg:lexicalAlias <http://rdaregistry.info/Elements/a/publisherOf.en> ;
    reg:name "publisherOf"@en ;
    reg:status <http://metadataregistry.org/uri/RegStatus/1001> ;
    a rdf:Property ;
    rdfs:domain <http://rdaregistry.info/Elements/c/C10002> ;
    rdfs:isDefinedBy <http://rdaregistry.info/Elements/a/> ;
    rdfs:label "est l’éditeur de"@fr, "is publisher of"@en ;
    rdfs:subPropertyOf <http://rdaregistry.info/Elements/a/P50307> ;
    skos:definition "Met une personne, famille ou collectivité responsable de la publication, de la mise à disposition ou de l’édition d’une ressource en relation avec la manifestation."@fr, "Relates an agent responsible for publishing, releasing, or issuing a manifestation to a manifestation."@en .

<http://rdaregistry.info/Elements/a/P50204>
    rdakit:toolkitDefinition "A work that involves a creation responsibility."@en, "Personne, famille ou collectivité responsable de la création d’une œuvre."@fr ;
    rdakit:toolkitLabel "creator of"@en, "créateur de"@fr ;
    reg:hasSubproperty <http://rdaregistry.info/Elements/a/P50068>, <http://rdaregistry.info/Elements/a/P50127>, <http://rdaregistry.info/Elements/a/P50184>, <http://rdaregistry.info/Elements/a/P50185>, <http://rdaregistry.info/Elements/a/P50186>, <http://rdaregistry.info/Elements/a/P50187>, <http://rdaregistry.info/Elements/a/P50188>, <http://rdaregistry.info/Elements/a/P50189>, <http://rdaregistry.info/Elements/a/P50190>, <http://rdaregistry.info/Elements/a/P50191>, <http://rdaregistry.info/Elements/a/P50192>, <http://rdaregistry.info/Elements/a/P50193>, <http://rdaregistry.info/Elements/a/P50194>, <http://rdaregistry.info/Elements/a/P50195>, <http://rdaregistry.info/Elements/a/P50196>, <http://rdaregistry.info/Elements/a/P50197>, <http://rdaregistry.info/Elements/a/datatype/P50204>, <http://rdaregistry.info/Elements/a/object/P50204>, <http://rdaregistry.info/Elements/a/object/P50293>, <http://rdaregistry.info/Elements/a/object/P50294> ;
    reg:hasUnconstrained <http://rdaregistry.info/Elements/u/P60672> ;
    reg:lexicalAlias <http://rdaregistry.info/Elements/a/creatorOf.en> ;
    reg:name "creatorOf"@en ;
    reg:status <http://metadataregistry.org/uri/RegStatus/1001> ;
    a rdf:Property ;
    rdfs:domain <http://rdaregistry.info/Elements/c/C10002> ;
    rdfs:isDefinedBy <http://rdaregistry.info/Elements/a/> ;
    rdfs:label "est le créateur de"@fr, "is creator of"@en ;
    rdfs:subPropertyOf <http://rdaregistry.info/Elements/a/P50305> ;
    skos:definition "Met une personne, famille ou collectivité responsable de la création d’une œuvre en relation avec l’œuvre."@fr, "Relates an agent responsible for the creation of a work to a work."@en .

<http://rdaregistry.info/Elements/a/P50205>
    rdakit:instructionNumber "18.5" ;
    rdakit:toolkitDefinition "A work that involves a responsibility for the general management and supervision of a filmed performance, a radio or television program, etc."@en, "Personne, famille ou collectivité responsable de la gestion et de la supervision générales d’une prestation filmée, d’une émission de radio ou de télévision, etc."@fr ;
    rdakit:toolkitLabel "director of"@en, "réalisateur de"@fr ;
    reg:hasSubproperty <http://rdaregistry.info/Elements/a/P50048>, <http://rdaregistry.info/Elements/a/P50049>, <http://rdaregistry.info/Elements/a/P50050>, <http://rdaregistry.info/Elements/a/datatype/P50205>, <http://rdaregistry.info/Elements/a/object/P50205> ;
    reg:hasUnconstrained <http://rdaregistry.info/Elements/u/P60673> ;
    reg:lexicalAlias <http://rdaregistry.info/Elements/a/directorOf.en> ;
    reg:name "directorOf"@en ;
    reg:status <http://metadataregistry.org/uri/RegStatus/1001> ;
    a rdf:Property ;
    rdfs:domain <http://rdaregistry.info/Elements/c/C10002> ;
    rdfs:isDefinedBy <http://rdaregistry.info/Elements/a/> ;
    rdfs:label "est le réalisateur de"@fr, "is director of"@en ;
    rdfs:subPropertyOf <http://rdaregistry.info/Elements/a/P50131> ;
    skos:definition "Met une personne, famille ou collectivité responsable de la gestion et de la supervision générales d’une prestation filmée, d’une émission de radio ou de télévision, etc. en relation avec l’œuvre."@fr, "Relates an agent responsible for the general management and supervision of a filmed performance, a radio or television program, etc. to a work."@en .

<http://rdaregistry.info/Elements/a/P50206>
    rdakit:instructionNumber "18.5" ;
    rdakit:toolkitDefinition "An item compensated for degradation by bringing it back to a state as close as possible to its original condition using a set of technical, editorial, and intellectual procedures."@en, "Personne, famille ou collectivité responsable de l’ensemble des procédures techniques, éditoriales et intellectuelles destinées à compenser la dégradation d’un item en le ramenant à un état aussi près que possible de sa condition originelle."@fr ;
    rdakit:toolkitLabel "restaurateur de"@fr, "restorationist of"@en ;
    reg:hasSubproperty <http://rdaregistry.info/Elements/a/datatype/P50206>, <http://rdaregistry.info/Elements/a/object/P50206> ;
    reg:hasUnconstrained <http://rdaregistry.info/Elements/u/P60674> ;
    reg:lexicalAlias <http://rdaregistry.info/Elements/a/restorationistOf.en> ;
    reg:name "restorationistOf"@en ;
    reg:status <http://metadataregistry.org/uri/RegStatus/1001> ;
    a rdf:Property ;
    rdfs:domain <http://rdaregistry.info/Elements/c/C10002> ;
    rdfs:isDefinedBy <http://rdaregistry.info/Elements/a/> ;
    rdfs:label "est le restaurateur de"@fr, "is restorationist of"@en ;
    rdfs:subPropertyOf <http://rdaregistry.info/Elements/a/P50182> ;
    skos:definition "Met une personne, famille ou collectivité responsable de l’ensemble des procédures techniques, éditoriales et intellectuelles destinées à compenser la dégradation d’un item en le ramenant à un état aussi près que possible de sa condition originelle en relation avec l’item."@fr, "Relates an agent responsible for the set of technical, editorial, and intellectual procedures aimed at compensating for the degradation of an item by bringing it back to a state as close as possible to its original condition to an item."@en .

<http://rdaregistry.info/Elements/a/P50207>
    rdakit:instructionNumber "18.5" ;
    rdakit:toolkitDefinition "A work that involves a responsibility for capturing images, either electronically or on film or video stock, and often selecting and arranging the lighting."@en, "Personne, famille ou collectivité qui capte des images, de manière électronique ou bien sur film ou vidéo, et qui, souvent, choisit et dispose l’éclairage."@fr ;
    rdakit:toolkitLabel "directeur de la photographie de"@fr, "director of photography of"@en ;
    reg:hasSubproperty <http://rdaregistry.info/Elements/a/datatype/P50207>, <http://rdaregistry.info/Elements/a/object/P50207> ;
    reg:hasUnconstrained <http://rdaregistry.info/Elements/u/P60678> ;
    reg:lexicalAlias <http://rdaregistry.info/Elements/a/directorOfPhotographyOf.en> ;
    reg:name "directorOfPhotographyOf"@en ;
    reg:status <http://metadataregistry.org/uri/RegStatus/1001> ;
    a rdf:Property ;
    rdfs:domain <http://rdaregistry.info/Elements/c/C10002> ;
    rdfs:isDefinedBy <http://rdaregistry.info/Elements/a/> ;
    rdfs:label "est le directeur de la photographie de"@fr, "is director of photography of"@en ;
    rdfs:subPropertyOf <http://rdaregistry.info/Elements/a/P50131> ;
    skos:definition "Met une personne, famille ou collectivité qui capte des images, de manière électronique ou bien sur film ou vidéo, et qui, souvent, choisit et dispose l’éclairage en relation avec l’œuvre."@fr, "Relates an agent that captures images, either electronically or on film or video stock, and often selects and arranges the lighting to a work."@en ;
    skos:scopeNote "A director of photography for a movie is also called a chief cinematographer."@en, "Le directeur de la photographie pour un film est également appelé le chef opérateur de prise de vues."@fr .

<http://rdaregistry.info/Elements/a/P50208>
    rdakit:instructionNumber "18.5" ;
    rdakit:toolkitDefinition "A work that is dedicated to an agent."@en, "Personne, famille ou collectivité à qui une œuvre est dédiée."@fr ;
    rdakit:toolkitLabel "dedicatee of"@en, "dédicataire de"@fr ;
    reg:hasSubproperty <http://rdaregistry.info/Elements/a/datatype/P50208>, <http://rdaregistry.info/Elements/a/object/P50208> ;
    reg:hasUnconstrained <http://rdaregistry.info/Elements/u/P60689> ;
    reg:lexicalAlias <http://rdaregistry.info/Elements/a/dedicateeOf.en> ;
    reg:name "dedicateeOf"@en ;
    reg:status <http://metadataregistry.org/uri/RegStatus/1001> ;
    a rdf:Property ;
    rdfs:domain <http://rdaregistry.info/Elements/c/C10002> ;
    rdfs:isDefinedBy <http://rdaregistry.info/Elements/a/> ;
    rdfs:label "est le dédicataire de"@fr, "is dedicatee of"@en ;
    rdfs:subPropertyOf <http://rdaregistry.info/Elements/a/P50131> ;
    skos:definition "Met une personne, famille ou collectivité à qui une œuvre est dédiée en relation avec l’œuvre."@fr, "Relates an agent to whom a work is dedicated to a work."@en .

<http://rdaregistry.info/Elements/a/P50209>
    rdakit:instructionNumber "18.5" ;
    rdakit:toolkitDefinition "A work or part of a work that is addressed to an agent."@en, "Personne, famille ou collectivité à qui une œuvre ou une partie d’œuvre est adressée."@fr ;
    rdakit:toolkitLabel "addressee of"@en, "destinataire de"@fr ;
    reg:hasSubproperty <http://rdaregistry.info/Elements/a/datatype/P50209>, <http://rdaregistry.info/Elements/a/object/P50209> ;
    reg:hasUnconstrained <http://rdaregistry.info/Elements/u/P60690> ;
    reg:lexicalAlias <http://rdaregistry.info/Elements/a/addresseeOf.en> ;
    reg:name "addresseeOf"@en ;
    reg:status <http://metadataregistry.org/uri/RegStatus/1001> ;
    a rdf:Property ;
    rdfs:domain <http://rdaregistry.info/Elements/c/C10002> ;
    rdfs:isDefinedBy <http://rdaregistry.info/Elements/a/> ;
    rdfs:label "est le destinataire de"@fr, "is addressee of"@en ;
    rdfs:subPropertyOf <http://rdaregistry.info/Elements/a/P50131> ;
    skos:definition "Met une personne, famille ou collectivité à qui une œuvre ou une partie d’œuvre est adressée en relation avec l’œuvre."@fr, "Relates an agent to whom a work or part of a work is addressed to a work."@en .

<http://rdaregistry.info/Elements/a/P50210>
    rdakit:instructionNumber "18.5" ;
    rdakit:toolkitDefinition "An item that is dedicated to an agent."@en, "Personne, famille ou collectivité à qui un item est dédié."@fr ;
    rdakit:toolkitLabel "dedicatee (item) of"@en, "dédicataire (item) de"@fr ;
    reg:hasSubproperty <http://rdaregistry.info/Elements/a/datatype/P50210>, <http://rdaregistry.info/Elements/a/object/P50210> ;
    reg:hasUnconstrained <http://rdaregistry.info/Elements/u/P60689> ;
    reg:lexicalAlias <http://rdaregistry.info/Elements/a/dedicateeOfItemOf.en> ;
    reg:name "dedicateeOfItemOf"@en ;
    reg:status <http://metadataregistry.org/uri/RegStatus/1001> ;
    a rdf:Property ;
    rdfs:domain <http://rdaregistry.info/Elements/c/C10002> ;
    rdfs:isDefinedBy <http://rdaregistry.info/Elements/a/> ;
    rdfs:label "est le dédicataire (item) de"@fr, "is dedicatee (item) of"@en ;
    rdfs:subPropertyOf <http://rdaregistry.info/Elements/a/P50182> ;
    skos:definition "Met une personne, famille ou collectivité à qui un item est dédié en relation avec l’item."@fr, "Relates an agent to whom an item is dedicated to an item."@en .

<http://rdaregistry.info/Elements/a/P50211>
    rdakit:instructionNumber "18.5" ;
    rdakit:toolkitDefinition "A work that involves a responsibility for providing consultation services, and often making recommendations, for another agent that is represented as the creator of a work."@en, "Personne, famille ou collectivité qui fournit des services de consultation et fait souvent des recommandations à une autre personne, famille ou collectivité représentée comme créatrice de l’œuvre."@fr ;
    rdakit:toolkitLabel "consultant de"@fr, "consultant of"@en ;
    reg:hasSubproperty <http://rdaregistry.info/Elements/a/datatype/P50211>, <http://rdaregistry.info/Elements/a/object/P50211> ;
    reg:hasUnconstrained <http://rdaregistry.info/Elements/u/P60701> ;
    reg:lexicalAlias <http://rdaregistry.info/Elements/a/consultantOf.en> ;
    reg:name "consultantOf"@en ;
    reg:status <http://metadataregistry.org/uri/RegStatus/1001> ;
    a rdf:Property ;
    rdfs:domain <http://rdaregistry.info/Elements/c/C10002> ;
    rdfs:isDefinedBy <http://rdaregistry.info/Elements/a/> ;
    rdfs:label "est le consultant de"@fr, "is consultant of"@en ;
    rdfs:subPropertyOf <http://rdaregistry.info/Elements/a/P50131> ;
    skos:definition "Met une personne, famille ou collectivité qui fournit des services de consultation et fait souvent des recommandations à une autre personne, famille ou collectivité représentée comme créatrice de l’œuvre en relation avec l’œuvre."@fr, "Relates an agent who provides consultation services, and often makes recommendations, for another agent that is represented as the creator of a work to a work."@en .

<http://rdaregistry.info/Elements/a/P50212>
    rdakit:instructionNumber "18.5" ;
    rdakit:toolkitDefinition "An expression that incorporates a contribution of recording the minutes of a meeting."@en, "Personne, famille ou collectivité responsable de rédiger le procès-verbal d’une réunion."@fr ;
    rdakit:toolkitLabel "minute taker of"@en, "procès-verbaliste de"@fr ;
    reg:hasSubproperty <http://rdaregistry.info/Elements/a/datatype/P50212>, <http://rdaregistry.info/Elements/a/object/P50212> ;
    reg:hasUnconstrained <http://rdaregistry.info/Elements/u/P60671> ;
    reg:lexicalAlias <http://rdaregistry.info/Elements/a/minuteTakerOf.en> ;
    reg:name "minuteTakerOf"@en ;
    reg:status <http://metadataregistry.org/uri/RegStatus/1001> ;
    a rdf:Property ;
    rdfs:domain <http://rdaregistry.info/Elements/c/C10002> ;
    rdfs:isDefinedBy <http://rdaregistry.info/Elements/a/> ;
    rdfs:label "est le procès-verbaliste de"@fr, "is minute taker of"@en ;
    rdfs:subPropertyOf <http://rdaregistry.info/Elements/a/P50161> ;
    skos:definition "Met une personne, famille ou collectivité responsable de rédiger le procès-verbal d’une réunion en relation avec l’expression."@fr, "Relates an agent, responsible for recording the minutes of a meeting to an expression."@en .

<http://rdaregistry.info/Elements/a/P50213>
    rdakit:instructionNumber "18.5" ;
    rdakit:toolkitDefinition "A work that involves a production responsibility for most of the business aspects of a film."@en, "Producteur responsable de la majeure partie des aspects financiers, techniques et artistiques d’un film."@fr ;
    rdakit:toolkitLabel "film producer of"@en, "producteur de films de"@fr ;
    reg:hasSubproperty <http://rdaregistry.info/Elements/a/datatype/P50213>, <http://rdaregistry.info/Elements/a/object/P50213> ;
    reg:hasUnconstrained <http://rdaregistry.info/Elements/u/P60033> ;
    reg:lexicalAlias <http://rdaregistry.info/Elements/a/filmProducerOf.en> ;
    reg:name "filmProducerOf"@en ;
    reg:status <http://metadataregistry.org/uri/RegStatus/1001> ;
    a rdf:Property ;
    rdfs:domain <http://rdaregistry.info/Elements/c/C10002> ;
    rdfs:isDefinedBy <http://rdaregistry.info/Elements/a/> ;
    rdfs:label "est le producteur de films de"@fr, "is film producer of"@en ;
    rdfs:subPropertyOf <http://rdaregistry.info/Elements/a/P50201> ;
    skos:definition "Met un producteur responsable de la majeure partie des aspects financiers, techniques et artistiques d’un film en relation avec l’œuvre."@fr, "Relates a producer responsible for most of the business aspects of a film to a work."@en .

<http://rdaregistry.info/Elements/a/P50214>
    rdakit:instructionNumber "18.5" ;
    rdakit:toolkitDefinition "A work that involves a production responsibility for most of the business aspects of a radio program."@en, "Producteur responsable de la majeure partie des aspects financiers, techniques et artistiques d’une émission de radio."@fr ;
    rdakit:toolkitLabel "producteur d’émissions de radio de"@fr, "radio producer of"@en ;
    reg:hasSubproperty <http://rdaregistry.info/Elements/a/datatype/P50214>, <http://rdaregistry.info/Elements/a/object/P50214> ;
    reg:hasUnconstrained <http://rdaregistry.info/Elements/u/P60034> ;
    reg:lexicalAlias <http://rdaregistry.info/Elements/a/radioProducerOf.en> ;
    reg:name "radioProducerOf"@en ;
    reg:status <http://metadataregistry.org/uri/RegStatus/1001> ;
    a rdf:Property ;
    rdfs:domain <http://rdaregistry.info/Elements/c/C10002> ;
    rdfs:isDefinedBy <http://rdaregistry.info/Elements/a/> ;
    rdfs:label "est le producteur d’émissions de radio de"@fr, "is radio producer of"@en ;
    rdfs:subPropertyOf <http://rdaregistry.info/Elements/a/P50201> ;
    skos:definition "Met un producteur responsable de la majeure partie des aspects financiers, techniques et artistiques d’une émission de radio en relation avec l’œuvre."@fr, "Relates a producer responsible for most of the business aspects of a radio program to a work."@en .

<http://rdaregistry.info/Elements/a/P50215>
    rdakit:instructionNumber "18.5" ;
    rdakit:toolkitDefinition "A work that involves a production responsibility for most of the business aspects of a television program to a work."@en, "Producteur responsable de la majeure partie des aspects financiers, techniques et artistiques d’une émission de télévision."@fr ;
    rdakit:toolkitLabel "producteur d’émissions de télévision de"@fr, "television producer of"@en ;
    reg:hasSubproperty <http://rdaregistry.info/Elements/a/datatype/P50215>, <http://rdaregistry.info/Elements/a/object/P50215> ;
    reg:hasUnconstrained <http://rdaregistry.info/Elements/u/P60035> ;
    reg:lexicalAlias <http://rdaregistry.info/Elements/a/televisionProducerOf.en> ;
    reg:name "televisionProducerOf"@en ;
    reg:status <http://metadataregistry.org/uri/RegStatus/1001> ;
    a rdf:Property ;
    rdfs:domain <http://rdaregistry.info/Elements/c/C10002> ;
    rdfs:isDefinedBy <http://rdaregistry.info/Elements/a/> ;
    rdfs:label "est le producteur d’émissions de télévision de"@fr, "is television producer of"@en ;
    rdfs:subPropertyOf <http://rdaregistry.info/Elements/a/P50201> ;
    skos:definition "Met un producteur responsable de la majeure partie des aspects financiers, techniques et artistiques d’une émission de télévision en relation avec l’œuvre."@fr, "Relates a producer responsible for most of the business aspects of a television program to a work."@en .

<http://rdaregistry.info/Elements/a/P50216>
    rdakit:instructionNumber "18.5" ;
    rdakit:seeAlso <http://rdaregistry.info/Elements/a/P50224> ;
    rdakit:toolkitDefinition "An expression of a musical work that incorporates a contribution of writing words added to an expression."@en, "Auteur de paroles ajoutées à une expression d’une œuvre musicale."@fr ;
    rdakit:toolkitLabel "auteur de paroles ajoutées de"@fr, "writer of added lyrics of"@en ;
    reg:hasSubproperty <http://rdaregistry.info/Elements/a/datatype/P50216>, <http://rdaregistry.info/Elements/a/object/P50216> ;
    reg:hasUnconstrained <http://rdaregistry.info/Elements/u/P60600> ;
    reg:lexicalAlias <http://rdaregistry.info/Elements/a/writerOfAddedLyricsOf.en> ;
    reg:name "writerOfAddedLyricsOf"@en ;
    reg:status <http://metadataregistry.org/uri/RegStatus/1001> ;
    a rdf:Property ;
    rdfs:domain <http://rdaregistry.info/Elements/c/C10002> ;
    rdfs:isDefinedBy <http://rdaregistry.info/Elements/a/> ;
    rdfs:label "est l’auteur de paroles ajoutées de"@fr, "is writer of added lyrics of"@en ;
    rdfs:subPropertyOf <http://rdaregistry.info/Elements/a/P50138> ;
    skos:definition "Met un auteur de paroles ajoutées à une expression d’une œuvre musicale en relation avec l’expression."@fr, "Relates a writer of words added to an expression of a musical work to an expression."@en .

<http://rdaregistry.info/Elements/a/P50217>
    rdakit:instructionNumber "18.5" ;
    rdakit:toolkitDefinition "Acteur contribuant à une expression d’une œuvre en prêtant sa voix à des personnages dans des productions radiophoniques et audio et à des personnages animés dans des œuvres d’images animées, de même qu’en prêtant sa voix hors champ dans des messages publicitaires à la radio et à la télévision, du doublage, etc."@fr, "An expression that incorporates an acting contribution of providing the voice for characters in radio and audio productions and for animated characters in moving image works, as well as by providing voice-overs in radio and television commercials, dubbed expressions, etc."@en ;
    rdakit:toolkitLabel "voice actor of"@en, "voix de"@fr ;
    reg:hasSubproperty <http://rdaregistry.info/Elements/a/datatype/P50217>, <http://rdaregistry.info/Elements/a/object/P50217> ;
    reg:hasUnconstrained <http://rdaregistry.info/Elements/u/P60027> ;
    reg:lexicalAlias <http://rdaregistry.info/Elements/a/voiceActorOf.en> ;
    reg:name "voiceActorOf"@en ;
    reg:status <http://metadataregistry.org/uri/RegStatus/1001> ;
    a rdf:Property ;
    rdfs:domain <http://rdaregistry.info/Elements/c/C10002> ;
    rdfs:isDefinedBy <http://rdaregistry.info/Elements/a/> ;
    rdfs:label "est la voix de"@fr, "is voice actor of"@en ;
    rdfs:subPropertyOf <http://rdaregistry.info/Elements/a/P50071> ;
    skos:definition "Met un acteur contribuant à une expression d’une œuvre en prêtant sa voix à des personnages dans des productions radiophoniques et audio et à des personnages animés dans des œuvres d’images animées, de même qu’en prêtant sa voix hors champ dans des messages publicitaires à la radio et à la télévision, du doublage, etc. en relation avec l’expression."@fr, "Relates an actor contributing to an expression of a work by providing the voice for characters in radio and audio productions and for animated characters in moving image works, as well as by providing voice-overs in radio and television commercials, dubbed expressions, etc., to an expression."@en .

<http://rdaregistry.info/Elements/a/P50218>
    reg:hasSubproperty <http://rdaregistry.info/Elements/a/datatype/P50218>, <http://rdaregistry.info/Elements/a/object/P50218>, <http://rdaregistry.info/Elements/a/object/P50288> ;
    reg:lexicalAlias <http://rdaregistry.info/Elements/a/relatedCorporateBodyAgent.en> ;
    reg:name "relatedCorporateBodyAgent"@en ;
    reg:status <http://metadataregistry.org/uri/RegStatus/1001> ;
    a rdf:Property ;
    rdfs:domain <http://rdaregistry.info/Elements/c/C10002> ;
    rdfs:isDefinedBy <http://rdaregistry.info/Elements/a/> ;
    rdfs:label "has related corporate body (agent)"@en ;
    rdfs:subPropertyOf <http://rdaregistry.info/Elements/a/P50337>, <http://rdaregistry.info/Elements/x/P00006> ;
    skos:definition "Relates an agent to a corporate body associated with an agent being identified."@en .

<http://rdaregistry.info/Elements/a/P50219>
    reg:hasSubproperty <http://rdaregistry.info/Elements/a/datatype/P50219>, <http://rdaregistry.info/Elements/a/object/P50219> ;
    reg:lexicalAlias <http://rdaregistry.info/Elements/a/relatedFamilyAgent.en> ;
    reg:name "relatedFamilyAgent"@en ;
    reg:status <http://metadataregistry.org/uri/RegStatus/1001> ;
    a rdf:Property ;
    rdfs:domain <http://rdaregistry.info/Elements/c/C10002> ;
    rdfs:isDefinedBy <http://rdaregistry.info/Elements/a/> ;
    rdfs:label "has related family (agent)"@en ;
    rdfs:subPropertyOf <http://rdaregistry.info/Elements/a/P50337>, <http://rdaregistry.info/Elements/x/P00006> ;
    skos:definition "Relates an agent to a family associated with an agent being identified."@en .

<http://rdaregistry.info/Elements/a/P50220>
    reg:hasSubproperty <http://rdaregistry.info/Elements/a/datatype/P50220>, <http://rdaregistry.info/Elements/a/object/P50220>, <http://rdaregistry.info/Elements/a/object/P50274>, <http://rdaregistry.info/Elements/a/object/P50279>, <http://rdaregistry.info/Elements/a/object/P50280>, <http://rdaregistry.info/Elements/a/object/P50281>, <http://rdaregistry.info/Elements/a/object/P50282>, <http://rdaregistry.info/Elements/a/object/P50283> ;
    reg:lexicalAlias <http://rdaregistry.info/Elements/a/relatedPersonAgent.en> ;
    reg:name "relatedPersonAgent"@en ;
    reg:status <http://metadataregistry.org/uri/RegStatus/1001> ;
    a rdf:Property ;
    rdfs:domain <http://rdaregistry.info/Elements/c/C10002> ;
    rdfs:isDefinedBy <http://rdaregistry.info/Elements/a/> ;
    rdfs:label "has related person (agent)"@en ;
    rdfs:subPropertyOf <http://rdaregistry.info/Elements/a/P50309>, <http://rdaregistry.info/Elements/x/P00006> ;
    skos:definition "Relates an agent to a person who is associated with an agent being identified."@en .

<http://rdaregistry.info/Elements/a/P50221>
    rdakit:instructionNumber "18.5" ;
    rdakit:toolkitDefinition "A landscape work that involves an architectural responsibility."@en, "Architecte responsable de la création d’œuvres paysagères."@fr ;
    rdakit:toolkitLabel "architecte paysagiste de"@fr, "landscape architect of"@en ;
    reg:hasSubproperty <http://rdaregistry.info/Elements/a/datatype/P50221>, <http://rdaregistry.info/Elements/a/object/P50221> ;
    reg:hasUnconstrained <http://rdaregistry.info/Elements/u/P60704> ;
    reg:lexicalAlias <http://rdaregistry.info/Elements/a/landscapeArchitectOf.en> ;
    reg:name "landscapeArchitectOf"@en ;
    reg:status <http://metadataregistry.org/uri/RegStatus/1001> ;
    a rdf:Property ;
    rdfs:domain <http://rdaregistry.info/Elements/c/C10002> ;
    rdfs:isDefinedBy <http://rdaregistry.info/Elements/a/> ;
    rdfs:label "est l’architecte paysagiste de"@fr, "is landscape architect of"@en ;
    rdfs:subPropertyOf <http://rdaregistry.info/Elements/a/P50196> ;
    skos:definition "Met un architecte responsable de la création d’œuvres paysagères en relation avec l’œuvre."@fr, "Relates an architect responsible for creating landscape works to a work."@en .

<http://rdaregistry.info/Elements/a/P50222>
    rdakit:instructionNumber "18.5" ;
    rdakit:toolkitDefinition "A three-dimensional work that involves an artistic responsibility for modeling, carving, or similar technique."@en, "Artiste responsable de la création d’une œuvre tridimensionnelle par le modelage, la taille ou une technique similaire."@fr ;
    rdakit:toolkitLabel "sculpteur de"@fr, "sculptor of"@en ;
    reg:hasSubproperty <http://rdaregistry.info/Elements/a/datatype/P50222>, <http://rdaregistry.info/Elements/a/object/P50222> ;
    reg:hasUnconstrained <http://rdaregistry.info/Elements/u/P60705> ;
    reg:lexicalAlias <http://rdaregistry.info/Elements/a/sculptorOf.en> ;
    reg:name "sculptorOf"@en ;
    reg:status <http://metadataregistry.org/uri/RegStatus/1001> ;
    a rdf:Property ;
    rdfs:domain <http://rdaregistry.info/Elements/c/C10002> ;
    rdfs:isDefinedBy <http://rdaregistry.info/Elements/a/> ;
    rdfs:label "est le sculpteur de"@fr, "is sculptor of"@en ;
    rdfs:subPropertyOf <http://rdaregistry.info/Elements/a/P50192> ;
    skos:definition "Met un artiste responsable de la création d’une œuvre tridimensionnelle par le modelage, la taille ou une technique similaire en relation avec l’œuvre."@fr, "Relates an artist responsible for creating a three-dimensional work by modeling, carving, or similar technique to a work."@en .

<http://rdaregistry.info/Elements/a/P50223>
    rdakit:instructionNumber "18.5" ;
    rdakit:toolkitDefinition "A work that involves an authoring responsibility for a screenplay, script, or scene."@en, "Auteur d’un scénario, d’un script ou d’une scène."@fr ;
    rdakit:toolkitLabel "screenwriter of"@en, "scénariste de"@fr ;
    reg:hasSubproperty <http://rdaregistry.info/Elements/a/datatype/P50223>, <http://rdaregistry.info/Elements/a/object/P50223> ;
    reg:hasUnconstrained <http://rdaregistry.info/Elements/u/P60706> ;
    reg:lexicalAlias <http://rdaregistry.info/Elements/a/screenwriterOf.en> ;
    reg:name "screenwriterOf"@en ;
    reg:status <http://metadataregistry.org/uri/RegStatus/1001> ;
    a rdf:Property ;
    rdfs:domain <http://rdaregistry.info/Elements/c/C10002> ;
    rdfs:isDefinedBy <http://rdaregistry.info/Elements/a/> ;
    rdfs:label "est le scénariste de"@fr, "is screenwriter of"@en ;
    rdfs:subPropertyOf <http://rdaregistry.info/Elements/a/P50195> ;
    skos:definition "Met un auteur d’un scénario, d’un script ou d’une scène en relation avec l’œuvre."@fr, "Relates an author of a screenplay, script, or scene to a work."@en .

<http://rdaregistry.info/Elements/a/P50224>
    rdakit:instructionNumber "18.5" ;
    rdakit:seeAlso <http://rdaregistry.info/Elements/a/P50225> ;
    rdakit:toolkitDefinition "A work that involves an authoring responsibility for the words of a popular song, including a song or songs from a musical."@en, "Auteur des paroles d’une chanson populaire, y compris une ou plusieurs chansons d’une comédie musicale."@fr ;
    rdakit:toolkitLabel "lyricist of"@en, "parolier de"@fr ;
    reg:hasSubproperty <http://rdaregistry.info/Elements/a/datatype/P50224>, <http://rdaregistry.info/Elements/a/object/P50224> ;
    reg:hasUnconstrained <http://rdaregistry.info/Elements/u/P60707> ;
    reg:lexicalAlias <http://rdaregistry.info/Elements/a/lyricistOf.en> ;
    reg:name "lyricistOf"@en ;
    reg:status <http://metadataregistry.org/uri/RegStatus/1001> ;
    a rdf:Property ;
    rdfs:domain <http://rdaregistry.info/Elements/c/C10002> ;
    rdfs:isDefinedBy <http://rdaregistry.info/Elements/a/> ;
    rdfs:label "est le parolier de"@fr, "is lyricist of"@en ;
    rdfs:subPropertyOf <http://rdaregistry.info/Elements/a/P50195> ;
    skos:definition "Met un auteur des paroles d’une chanson populaire, y compris une ou plusieurs chansons d’une comédie musicale, en relation avec l’œuvre."@fr, "Relates an author of the words of a popular song, including a song or songs from a musical to a work."@en .

<http://rdaregistry.info/Elements/a/P50225>
    rdakit:instructionNumber "18.5" ;
    rdakit:seeAlso <http://rdaregistry.info/Elements/a/P50224> ;
    rdakit:toolkitDefinition "A work that involves an authoring responsibility for the words of an opera or other musical stage work, or an oratorio."@en, "Auteur des paroles d’un opéra ou d’une autre œuvre scénique ou d’un oratorio."@fr ;
    rdakit:toolkitLabel "librettist of"@en, "librettiste de"@fr ;
    reg:hasSubproperty <http://rdaregistry.info/Elements/a/datatype/P50225>, <http://rdaregistry.info/Elements/a/object/P50225> ;
    reg:hasUnconstrained <http://rdaregistry.info/Elements/u/P60708> ;
    reg:lexicalAlias <http://rdaregistry.info/Elements/a/librettistOf.en> ;
    reg:name "librettistOf"@en ;
    reg:status <http://metadataregistry.org/uri/RegStatus/1001> ;
    a rdf:Property ;
    rdfs:domain <http://rdaregistry.info/Elements/c/C10002> ;
    rdfs:isDefinedBy <http://rdaregistry.info/Elements/a/> ;
    rdfs:label "est le librettiste de"@fr, "is librettist of"@en ;
    rdfs:subPropertyOf <http://rdaregistry.info/Elements/a/P50195> ;
    skos:definition "Met un auteur des paroles d’un opéra ou d’une autre œuvre scénique ou d’un oratorio en relation avec l’œuvre."@fr, "Relates an author of the words of an opera or other musical stage work, or an oratorio to a work."@en .

<http://rdaregistry.info/Elements/a/P50226>
    rdakit:instructionNumber "18.5" ;
    rdakit:toolkitDefinition "A work that involves a responsibility for sponsoring some aspect of a work, e.g., funding research, sponsoring an event."@en, "Personne, famille ou collectivité commanditant certains aspects d’une œuvre, par exemple, le financement de la recherche, le parrainage d’un événement."@fr ;
    rdakit:toolkitLabel "commanditaire de"@fr, "sponsoring body of"@en ;
    reg:hasSubproperty <http://rdaregistry.info/Elements/a/datatype/P50226>, <http://rdaregistry.info/Elements/a/object/P50226> ;
    reg:hasUnconstrained <http://rdaregistry.info/Elements/u/P60675> ;
    reg:lexicalAlias <http://rdaregistry.info/Elements/a/sponsoringBodyOf.en> ;
    reg:name "sponsoringBodyOf"@en ;
    reg:status <http://metadataregistry.org/uri/RegStatus/1001> ;
    a rdf:Property ;
    rdfs:domain <http://rdaregistry.info/Elements/c/C10002> ;
    rdfs:isDefinedBy <http://rdaregistry.info/Elements/a/> ;
    rdfs:label "est le commanditaire de"@fr, "is sponsoring body of"@en ;
    rdfs:subPropertyOf <http://rdaregistry.info/Elements/a/P50131> ;
    skos:definition "Met une personne, famille ou collectivité commanditant certains aspects d’une œuvre, par exemple, le financement de la recherche, le parrainage d’un événement, en relation avec l’œuvre."@fr, "Relates an agent sponsoring some aspect of a work, e.g., funding research, sponsoring an event, to a work."@en .

<http://rdaregistry.info/Elements/a/P50227>
    rdakit:instructionNumber "18.5" ;
    rdakit:toolkitDefinition "An expression that incorporates a contribution of providing an afterword to an original work."@en, "Personne, famille ou collectivité contribuant à une expression d’une œuvre en fournissant un après-propos à l’œuvre originale."@fr ;
    rdakit:toolkitLabel "auteur d’après-propos de"@fr, "writer of afterword of"@en ;
    reg:hasSubproperty <http://rdaregistry.info/Elements/a/datatype/P50227>, <http://rdaregistry.info/Elements/a/object/P50227> ;
    reg:hasUnconstrained <http://rdaregistry.info/Elements/u/P60717> ;
    reg:lexicalAlias <http://rdaregistry.info/Elements/a/writerOfAfterwordOf.en> ;
    reg:name "writerOfAfterwordOf"@en ;
    reg:status <http://metadataregistry.org/uri/RegStatus/1001> ;
    a rdf:Property ;
    rdfs:domain <http://rdaregistry.info/Elements/c/C10002> ;
    rdfs:isDefinedBy <http://rdaregistry.info/Elements/a/> ;
    rdfs:label "est l’auteur d’après-propos de"@fr, "is writer of afterword of"@en ;
    rdfs:subPropertyOf <http://rdaregistry.info/Elements/a/P50154> ;
    skos:definition "Met une personne, famille ou collectivité contribuant à une expression d’une œuvre en fournissant un après-propos à l’œuvre originale en relation avec l’expression."@fr, "Relates an agent contributing to an expression of a work by providing an afterword to an original work to an expression."@en .

<http://rdaregistry.info/Elements/a/P50228>
    rdakit:instructionNumber "18.5" ;
    rdakit:toolkitDefinition "An expression that incorporates a contribution of providing a postface to an original work."@en, "Personne, famille ou collectivité contribuant à une expression d’une œuvre en fournissant une postface à l’œuvre originale."@fr ;
    rdakit:toolkitLabel "postfacier de"@fr, "writer of postface of"@en ;
    reg:hasSubproperty <http://rdaregistry.info/Elements/a/datatype/P50228>, <http://rdaregistry.info/Elements/a/object/P50228> ;
    reg:hasUnconstrained <http://rdaregistry.info/Elements/u/P60718> ;
    reg:lexicalAlias <http://rdaregistry.info/Elements/a/writerOfPostfaceOf.en> ;
    reg:name "writerOfPostfaceOf"@en ;
    reg:status <http://metadataregistry.org/uri/RegStatus/1001> ;
    a rdf:Property ;
    rdfs:domain <http://rdaregistry.info/Elements/c/C10002> ;
    rdfs:isDefinedBy <http://rdaregistry.info/Elements/a/> ;
    rdfs:label "est le postfacier de"@fr, "is writer of postface of"@en ;
    rdfs:subPropertyOf <http://rdaregistry.info/Elements/a/P50154> ;
    skos:definition "Met une personne, famille ou collectivité contribuant à une expression d’une œuvre en fournissant une postface à l’œuvre originale en relation avec l’expression."@fr, "Relates an agent contributing to an expression of a work by providing a postface to an original work to an expression."@en .

<http://rdaregistry.info/Elements/a/P50229>
    rdakit:instructionNumber "29.5" ;
    rdakit:toolkitDefinition "A corporate body that split or divided into another corporate body."@en, "Collectivité qui s’est scindée ou s’est divisée pour former l’autre collectivité."@fr, "Una entidad corporativa que se separa o divide en otra entidad corporativa."@es ;
    rdakit:toolkitLabel "predecesora de la división"@es, "predecessor of split"@en, "prédécesseur avant scission"@fr ;
    reg:hasSubproperty <http://rdaregistry.info/Elements/a/datatype/P50229>, <http://rdaregistry.info/Elements/a/object/P50229> ;
    reg:hasUnconstrained <http://rdaregistry.info/Elements/u/P60733> ;
    reg:lexicalAlias <http://rdaregistry.info/Elements/a/predecessorOfSplit.en> ;
    reg:name "predecessorOfSplit"@en ;
    reg:status <http://metadataregistry.org/uri/RegStatus/1001> ;
    a rdf:Property ;
    rdfs:domain <http://rdaregistry.info/Elements/c/C10005> ;
    rdfs:isDefinedBy <http://rdaregistry.info/Elements/a/> ;
    rdfs:label "a pour prédécesseur avant scission"@fr, "has predecessor of split"@en ;
    skos:definition "Met une collectivité en relation avec une collectivité qui s’est scindée ou s’est divisée pour former l’autre collectivité."@fr, "Relates a corporate body to a corporate body that split or divided into another corporate body."@en .

<http://rdaregistry.info/Elements/a/P50230>
    rdakit:instructionNumber "29.5" ;
    rdakit:toolkitDefinition "A corporate body formed from the membership of other corporate bodies."@en, "Collectivité formée par le regroupement de collectivités membres."@fr, "Una entidad corporativa formada de la membresía de otras entidades corporativas."@es ;
    rdakit:toolkitLabel "collectivité d’affiliation"@fr, "entidad corporativa por membresía"@es, "membership corporate body"@en ;
    reg:hasSubproperty <http://rdaregistry.info/Elements/a/datatype/P50230>, <http://rdaregistry.info/Elements/a/object/P50230> ;
    reg:hasUnconstrained <http://rdaregistry.info/Elements/u/P60648> ;
    reg:lexicalAlias <http://rdaregistry.info/Elements/a/membershipCorporateBody.en> ;
    reg:name "membershipCorporateBody"@en ;
    reg:status <http://metadataregistry.org/uri/RegStatus/1001> ;
    a rdf:Property ;
    rdfs:domain <http://rdaregistry.info/Elements/c/C10005> ;
    rdfs:isDefinedBy <http://rdaregistry.info/Elements/a/> ;
    rdfs:label "a pour collectivité d’affiliation"@fr, "has membership corporate body"@en ;
    skos:definition "Met une collectivité en relation avec une collectivité formée par le regroupement de collectivités membres."@fr, "Relates a corporate body to a corporate body formed from the membership of other corporate bodies."@en .

<http://rdaregistry.info/Elements/a/P50231>
    rdakit:instructionNumber "29.5" ;
    rdakit:toolkitDefinition "A corporate body that is a member of another corporate body."@en, "Collectivité qui est membre de l’autre collectivité."@fr, "Una entidad corporativa que es miembro de otra entidad corporativa."@es ;
    rdakit:toolkitLabel "collectivité membre"@fr, "corporate member"@en, "miembro corporativo"@es ;
    reg:hasSubproperty <http://rdaregistry.info/Elements/a/datatype/P50231>, <http://rdaregistry.info/Elements/a/object/P50231> ;
    reg:hasUnconstrained <http://rdaregistry.info/Elements/u/P60697> ;
    reg:lexicalAlias <http://rdaregistry.info/Elements/a/corporateMember.en> ;
    reg:name "corporateMember"@en ;
    reg:status <http://metadataregistry.org/uri/RegStatus/1001> ;
    a rdf:Property ;
    rdfs:domain <http://rdaregistry.info/Elements/c/C10005> ;
    rdfs:isDefinedBy <http://rdaregistry.info/Elements/a/> ;
    rdfs:label "a pour collectivité membre"@fr, "has corporate member"@en ;
    skos:definition "Met une collectivité en relation avec une collectivité qui est membre de l’autre collectivité."@fr, "Relates a corporate body to a corporate body that is a member of another corporate body."@en .

<http://rdaregistry.info/Elements/a/P50232>
    rdakit:instructionNumber "29.5" ;
    rdakit:toolkitDefinition "A corporate body that formed another corporate body by merging with one or more other corporate bodies."@en, "Collectivité qui a formé l’autre collectivité en fusionnant avec une ou plusieurs autres collectivités."@fr, "Una entidad corporativa que forma otra entidad corporativa mediante la fusión con otra u otras entidades corporativas."@es ;
    rdakit:toolkitLabel "component of merger"@en, "componente de una fusión"@es, "composante d’une fusion"@fr ;
    reg:hasSubproperty <http://rdaregistry.info/Elements/a/datatype/P50232>, <http://rdaregistry.info/Elements/a/object/P50232> ;
    reg:hasUnconstrained <http://rdaregistry.info/Elements/u/P60736> ;
    reg:lexicalAlias <http://rdaregistry.info/Elements/a/componentOfMerger.en> ;
    reg:name "componentOfAMerger"@en ;
    reg:status <http://metadataregistry.org/uri/RegStatus/1001> ;
    a rdf:Property ;
    rdfs:domain <http://rdaregistry.info/Elements/c/C10005> ;
    rdfs:isDefinedBy <http://rdaregistry.info/Elements/a/> ;
    rdfs:label "a pour composante d’une fusion"@fr, "has component of merger"@en ;
    skos:definition "Met une collectivité en relation avec une collectivité qui a formé l’autre collectivité en fusionnant avec une ou plusieurs autres collectivités."@fr, "Relates a corporate body to a corporate body that formed another corporate body by merging with one or more other corporate bodies."@en .

<http://rdaregistry.info/Elements/a/P50233>
    rdakit:instructionNumber "29.5" ;
    rdakit:toolkitDefinition "A family to which a person belongs."@en, "Famille à laquelle la personne appartient."@fr, "Una familia a la cual la persona pertenece."@es ;
    rdakit:toolkitLabel "familia"@es, "famille"@fr, "family"@en ;
    reg:hasSubproperty <http://rdaregistry.info/Elements/a/datatype/P50233>, <http://rdaregistry.info/Elements/a/object/P50233> ;
    reg:hasUnconstrained <http://rdaregistry.info/Elements/u/P60697> ;
    reg:lexicalAlias <http://rdaregistry.info/Elements/a/family.en> ;
    reg:name "family"@en ;
    reg:status <http://metadataregistry.org/uri/RegStatus/1001> ;
    a rdf:Property ;
    rdfs:domain <http://rdaregistry.info/Elements/c/C10004> ;
    rdfs:isDefinedBy <http://rdaregistry.info/Elements/a/> ;
    rdfs:label "a pour famille"@fr, "has family"@en ;
    skos:definition "Met une personne en relation avec une famille à laquelle la personne appartient."@fr, "Relates a person to a family to which a person belongs."@en .

<http://rdaregistry.info/Elements/a/P50234>
    rdakit:instructionNumber "29.5" ;
    rdakit:toolkitDefinition "A corporate body that a person commands or in which a person holds an office."@en, "Collectivité dans laquelle la personne exerce une fonction administrative ou officielle."@fr, "Una entidad corporativa en la cual una persona tiene un cargo."@es ;
    rdakit:toolkitLabel "collectivité administrée"@fr, "entidad corporativa sede"@es, "officer of"@en ;
    reg:hasSubproperty <http://rdaregistry.info/Elements/a/datatype/P50234>, <http://rdaregistry.info/Elements/a/object/P50234>, <http://rdaregistry.info/Elements/a/object/P50286>, <http://rdaregistry.info/Elements/a/object/P50287> ;
    reg:hasUnconstrained <http://rdaregistry.info/Elements/u/P60737> ;
    reg:lexicalAlias <http://rdaregistry.info/Elements/a/officerOf.en> ;
    reg:name "officerOf"@en ;
    reg:status <http://metadataregistry.org/uri/RegStatus/1001> ;
    a rdf:Property ;
    rdfs:domain <http://rdaregistry.info/Elements/c/C10004> ;
    rdfs:isDefinedBy <http://rdaregistry.info/Elements/a/> ;
    rdfs:label "a pour collectivité administrée"@fr, "is officer of"@en ;
    skos:definition "Met une personne en relation avec une collectivité dans laquelle la personne exerce une fonction administrative ou officielle."@fr, "Relates a person to a corporate body that a person commands or in which a person holds an office."@en .

<http://rdaregistry.info/Elements/a/P50235>
    rdakit:instructionNumber "10.8" ;
    rdakit:toolkitDefinition "A language a family uses in its communications."@en, "Langue que la famille utilise pour sa communication."@fr, "Una lengua que una familia usa para sus comunicaciones."@es ;
    rdakit:toolkitLabel "language of the family"@en, "langue de la famille"@fr, "lengua de la familia"@es ;
    reg:hasSubproperty <http://rdaregistry.info/Elements/a/datatype/P50235> ;
    reg:hasUnconstrained <http://rdaregistry.info/Elements/u/P60098> ;
    reg:lexicalAlias <http://rdaregistry.info/Elements/a/languageOfTheFamily.en> ;
    reg:name "languageOfTheFamily"@en ;
    reg:status <http://metadataregistry.org/uri/RegStatus/1001> ;
    a rdf:Property ;
    rdfs:domain <http://rdaregistry.info/Elements/c/C10008> ;
    rdfs:isDefinedBy <http://rdaregistry.info/Elements/a/> ;
    rdfs:label "a pour langue de la famille"@fr, "has language of the family"@en ;
    skos:definition "Met une famille en relation avec une langue que la famille utilise pour sa communication."@fr, "Relates a family to a language a family uses in its communications."@en .

<http://rdaregistry.info/Elements/a/P50236>
    rdakit:instructionNumber "11.4.5" ;
    rdakit:toolkitDefinition "A date or range of dates indicative of the period in which a corporate body was active."@en, "Una fecha o rango de fechas que indican el período en el que la entidad corporativa estaba activa."@es ;
    rdakit:toolkitLabel "period of activity of the corporate body"@en, "período de actividad de la entidad corporativa"@es, "verksamhetstid för institutionen"@sv ;
    reg:hasSubproperty <http://rdaregistry.info/Elements/a/datatype/P50236> ;
    reg:hasUnconstrained <http://rdaregistry.info/Elements/u/P60076> ;
    reg:lexicalAlias <http://rdaregistry.info/Elements/a/periodOfActivityOfTheCorporateBody.en> ;
    reg:name "periodOfActivityOfTheCorporateBody"@en ;
    reg:status <http://metadataregistry.org/uri/RegStatus/1001> ;
    a rdf:Property ;
    rdfs:domain <http://rdaregistry.info/Elements/c/C10005> ;
    rdfs:isDefinedBy <http://rdaregistry.info/Elements/a/> ;
    rdfs:label "har verksamhetstid för institutionen"@sv, "has period of activity of the corporate body"@en ;
    rdfs:subPropertyOf <http://rdaregistry.info/Elements/a/P50040> ;
    skos:definition "Relates a corporate body to a date or range of dates indicative of the period in which a corporate body was active."@en .

<http://rdaregistry.info/Elements/a/P50237>
    rdakit:instructionNumber "11.7.1.4" ;
    rdakit:toolkitDefinition "A categorization for a type of corporate body."@en, "Type de collectivité."@fr ;
    rdakit:toolkitLabel "tipo de entidad corporativa"@es, "type de collectivité"@fr, "type of corporate body"@en ;
    reg:hasSubproperty <http://rdaregistry.info/Elements/a/datatype/P50237> ;
    reg:hasUnconstrained <http://rdaregistry.info/Elements/u/P60047> ;
    reg:lexicalAlias <http://rdaregistry.info/Elements/a/typeOfCorporateBody.en> ;
    reg:name "typeOfCorporateBody"@en ;
    reg:status <http://metadataregistry.org/uri/RegStatus/1001> ;
    a rdf:Property ;
    rdfs:domain <http://rdaregistry.info/Elements/c/C10005> ;
    rdfs:isDefinedBy <http://rdaregistry.info/Elements/a/> ;
    rdfs:label "a pour type de collectivité"@fr, "has type of corporate body"@en ;
    rdfs:subPropertyOf <http://rdaregistry.info/Elements/a/P50033> ;
    skos:definition "Met une collectivité en relation avec le type de collectivité."@fr, "Relates a corporate body to a type of corporate body."@en .

<http://rdaregistry.info/Elements/a/P50238>
    rdakit:instructionNumber "11.7.1.5" ;
    rdakit:toolkitDefinition "A categorization for a type of corporate body."@en, "Type de juridiction."@fr ;
    rdakit:toolkitLabel "tipo de jurisdicción"@es, "type de juridiction"@fr, "type of jurisdiction"@en ;
    reg:hasSubproperty <http://rdaregistry.info/Elements/a/datatype/P50238> ;
    reg:hasUnconstrained <http://rdaregistry.info/Elements/u/P60047> ;
    reg:lexicalAlias <http://rdaregistry.info/Elements/a/typeOfJurisdiction.en> ;
    reg:name "typeOfJurisdiction"@en ;
    reg:status <http://metadataregistry.org/uri/RegStatus/1001> ;
    a rdf:Property ;
    rdfs:domain <http://rdaregistry.info/Elements/c/C10005> ;
    rdfs:isDefinedBy <http://rdaregistry.info/Elements/a/> ;
    rdfs:label "a pour type de juridiction"@fr, "has type of jurisdiction"@en ;
    rdfs:subPropertyOf <http://rdaregistry.info/Elements/a/P50033> ;
    skos:definition "Met une collectivité en relation avec le type de juridiction."@fr, "Relates a corporate body to a type of jurisdiction."@en .

<http://rdaregistry.info/Elements/a/P50239>
    rdakit:instructionNumber "11.7.1.6" ;
    rdakit:toolkitDefinition "A characteristic other than place associated with the corporate body, date associated with the corporate body, associated institution, type of corporate body, or type of jurisdiction."@en, "Autre information."@fr ;
    rdakit:toolkitLabel "autre information"@fr, "other designation"@en, "otra designación"@es ;
    reg:hasSubproperty <http://rdaregistry.info/Elements/a/datatype/P50239> ;
    reg:hasUnconstrained <http://rdaregistry.info/Elements/u/P60370> ;
    reg:lexicalAlias <http://rdaregistry.info/Elements/a/otherDesignation.en> ;
    reg:name "otherDesignation"@en ;
    reg:status <http://metadataregistry.org/uri/RegStatus/1001> ;
    a rdf:Property ;
    rdfs:domain <http://rdaregistry.info/Elements/c/C10005> ;
    rdfs:isDefinedBy <http://rdaregistry.info/Elements/a/> ;
    rdfs:label "a pour autre information"@fr, "has other designation"@en ;
    rdfs:subPropertyOf <http://rdaregistry.info/Elements/a/P50033> ;
    skos:definition "Met une collectivité en relation avec l’autre information."@fr, "Relates a corporate body to another designation."@en .

<http://rdaregistry.info/Elements/a/P50240>
    rdakit:instructionNumber "29.5" ;
    rdakit:toolkitDefinition "A corporate body that acts for a local affiliated body and others at a broader organizational level."@en, "Collectivité qui agit pour la collectivité affiliée locale et pour d’autres à un niveau organisationnel plus vaste."@fr, "Una entidad corporativa que actúa para la entidad afiliada local y otras en un nivel organizacional más amplio."@es ;
    rdakit:toolkitLabel "broader affiliated body"@en, "collectivité affiliée plus vaste"@fr, "entidad afiliada amplia"@es ;
    reg:hasSubproperty <http://rdaregistry.info/Elements/a/datatype/P50240>, <http://rdaregistry.info/Elements/a/object/P50240> ;
    reg:hasUnconstrained <http://rdaregistry.info/Elements/u/P60738> ;
    reg:lexicalAlias <http://rdaregistry.info/Elements/a/broaderAffiliatedBody.en> ;
    reg:name "broaderAffiliatedBody"@en ;
    reg:status <http://metadataregistry.org/uri/RegStatus/1001> ;
    a rdf:Property ;
    rdfs:domain <http://rdaregistry.info/Elements/c/C10005> ;
    rdfs:isDefinedBy <http://rdaregistry.info/Elements/a/> ;
    rdfs:label "a pour collectivité affiliée plus vaste"@fr, "has broader affiliated body"@en ;
    skos:definition "Met une collectivité en relation avec une collectivité qui agit pour la collectivité affiliée locale et pour d’autres à un niveau organisationnel plus vaste."@fr, "Relates a corporate body to a corporate body that acts for a local affiliated body and others at a broader organizational level."@en .

<http://rdaregistry.info/Elements/a/P50241>
    rdakit:instructionNumber "29.5" ;
    rdakit:toolkitDefinition "A local corporate body affiliated with a broader body which acts for it and others at a broader organizational level."@en, "Collectivité locale affiliée avec la collectivité plus vaste qui agit pour elle et pour d’autres à un niveau organisationnel plus vaste."@fr, "Una entidad corporativa afiliada a otra más amplia que actúa para ella y para otras en un nivel organizacional más amplio."@es ;
    rdakit:toolkitLabel "afiliado local"@es, "collectivité affiliée locale"@fr, "local affiliate"@en ;
    reg:hasSubproperty <http://rdaregistry.info/Elements/a/datatype/P50241>, <http://rdaregistry.info/Elements/a/object/P50241> ;
    reg:hasUnconstrained <http://rdaregistry.info/Elements/u/P60739> ;
    reg:lexicalAlias <http://rdaregistry.info/Elements/a/localAffiliate.en> ;
    reg:name "localAffiliate"@en ;
    reg:status <http://metadataregistry.org/uri/RegStatus/1001> ;
    a rdf:Property ;
    rdfs:domain <http://rdaregistry.info/Elements/c/C10005> ;
    rdfs:isDefinedBy <http://rdaregistry.info/Elements/a/> ;
    rdfs:label "a pour collectivité affiliée locale"@fr, "has local affiliate"@en ;
    skos:definition "Met une collectivité en relation avec une collectivité locale affiliée avec la collectivité plus vaste qui agit pour elle et pour d’autres à un niveau organisationnel plus vaste."@fr, "Relates a corporate body to a local corporate body affiliated with a broader body which acts for it and others at a broader organizational level."@en .

<http://rdaregistry.info/Elements/a/P50242>
    rdakit:instructionNumber "18.5" ;
    rdakit:toolkitDefinition "A manifestation using paper produced to manufacture a manifestation."@en, "Personne, famille ou collectivité responsable de la production du papier utilisé pour fabriquer une manifestation."@fr ;
    rdakit:toolkitLabel "papermaker of"@en, "papetier de"@fr ;
    reg:hasSubproperty <http://rdaregistry.info/Elements/a/datatype/P50242>, <http://rdaregistry.info/Elements/a/object/P50242> ;
    reg:hasUnconstrained <http://rdaregistry.info/Elements/u/P60747> ;
    reg:lexicalAlias <http://rdaregistry.info/Elements/a/papermakerOf.en> ;
    reg:name "papermakerOf"@en ;
    reg:status <http://metadataregistry.org/uri/RegStatus/1001> ;
    a rdf:Property ;
    rdfs:domain <http://rdaregistry.info/Elements/c/C10002> ;
    rdfs:isDefinedBy <http://rdaregistry.info/Elements/a/> ;
    rdfs:label "est le papetier de"@fr, "is papermaker of"@en ;
    rdfs:subPropertyOf <http://rdaregistry.info/Elements/a/P50202> ;
    skos:definition "Met une personne, famille ou collectivité responsable de la production du papier utilisé pour fabriquer une manifestation en relation avec la manifestation."@fr, "Relates an agent responsible for the production of paper used to manufacture a manifestation to a manifestation."@en .

<http://rdaregistry.info/Elements/a/P50243>
    rdakit:instructionNumber "18.5" ;
    rdakit:toolkitDefinition "An expression of a moving image work that involves a responsibility for designing and creating post-production visual effects."@en, "Personne, famille ou collectivité contribuant à une expression d’une œuvre d’images animées en concevant et en créant des effets visuels en postproduction."@fr ;
    rdakit:toolkitLabel "fournisseur d’effets visuels de"@fr, "visual effects provider of"@en ;
    reg:hasSubproperty <http://rdaregistry.info/Elements/a/datatype/P50243>, <http://rdaregistry.info/Elements/a/object/P50243> ;
    reg:hasUnconstrained <http://rdaregistry.info/Elements/u/P60754> ;
    reg:lexicalAlias <http://rdaregistry.info/Elements/a/visualEffectsProviderOf.en> ;
    reg:name "visualEffectsProviderOf"@en ;
    reg:status <http://metadataregistry.org/uri/RegStatus/1001> ;
    a rdf:Property ;
    rdfs:domain <http://rdaregistry.info/Elements/c/C10002> ;
    rdfs:isDefinedBy <http://rdaregistry.info/Elements/a/> ;
    rdfs:label "est le fournisseur d’effets visuels de"@fr, "is visual effects provider of"@en ;
    rdfs:subPropertyOf <http://rdaregistry.info/Elements/a/P50161> ;
    skos:definition "Met une personne, famille ou collectivité contribuant à une expression d’une œuvre d’images animées en concevant et en créant des effets visuels en postproduction en relation avec l’expression."@fr, "Relates an agent contributing to an expression of a moving image work by designing and creating post-production visual effects to an expression."@en .

<http://rdaregistry.info/Elements/a/P50244>
    rdakit:instructionNumber "18.5" ;
    rdakit:toolkitDefinition "An expression of a moving image or audio work that involves a responsibility for designing and creating on-set special effects, such as on-set mechanical effects and in-camera optical effects."@en, "Personne, famille ou collectivité contribuant à une expression d’une œuvre d’images animées ou d’une œuvre audio en concevant et en créant des effets spéciaux de plateau (effets mécaniques de plateau et effets d’optique dans la caméra)."@fr ;
    rdakit:toolkitLabel "fournisseur d’effets spéciaux de"@fr, "special effects provider of"@en ;
    reg:hasSubproperty <http://rdaregistry.info/Elements/a/datatype/P50244>, <http://rdaregistry.info/Elements/a/object/P50244> ;
    reg:hasUnconstrained <http://rdaregistry.info/Elements/u/P60755> ;
    reg:lexicalAlias <http://rdaregistry.info/Elements/a/specialEffectsProviderOf.en> ;
    reg:name "specialEffectsProviderOf"@en ;
    reg:status <http://metadataregistry.org/uri/RegStatus/1001> ;
    a rdf:Property ;
    rdfs:domain <http://rdaregistry.info/Elements/c/C10002> ;
    rdfs:isDefinedBy <http://rdaregistry.info/Elements/a/> ;
    rdfs:label "est le fournisseur d’effets spéciaux de"@fr, "is special effects provider of"@en ;
    rdfs:subPropertyOf <http://rdaregistry.info/Elements/a/P50161> ;
    skos:definition "Met une personne, famille ou collectivité contribuant à une expression d’une œuvre d’images animées ou d’une œuvre audio en concevant et en créant des effets spéciaux de plateau (effets mécaniques de plateau et effets d’optique dans la caméra) en relation avec l’expression."@fr, "Relates an agent contributing to an expression of a moving image or audio work by designing and creating on-set special effects, such as on-set mechanical effects and in-camera optical effects, to an expression."@en .

<http://rdaregistry.info/Elements/a/P50245>
    rdakit:instructionNumber "18.5" ;
    rdakit:toolkitDefinition "An expression of a comic book, graphic novel, etc. that incorporates an illustrating contribution."@en, "Illustrateur contribuant à une expression d’une bande dessinée, d’un roman graphique, etc. en dessinant le texte et les effets sonores graphiques."@fr ;
    rdakit:toolkitLabel "letterer of"@en, "lettreur de"@fr ;
    reg:hasSubproperty <http://rdaregistry.info/Elements/a/datatype/P50245>, <http://rdaregistry.info/Elements/a/object/P50245> ;
    reg:hasUnconstrained <http://rdaregistry.info/Elements/u/P60756> ;
    reg:lexicalAlias <http://rdaregistry.info/Elements/a/lettererOf.en> ;
    reg:name "lettererOf"@en ;
    reg:status <http://metadataregistry.org/uri/RegStatus/1001> ;
    a rdf:Property ;
    rdfs:domain <http://rdaregistry.info/Elements/c/C10002> ;
    rdfs:isDefinedBy <http://rdaregistry.info/Elements/a/> ;
    rdfs:label "est le lettreur de"@fr, "is letterer of"@en ;
    rdfs:subPropertyOf <http://rdaregistry.info/Elements/a/P50159> ;
    skos:definition "Met un illustrateur contribuant à une expression d’une bande dessinée, d’un roman graphique, etc. en dessinant le texte et les effets sonores graphiques en relation avec l’expression."@fr, "Relates an illustrator contributing to an expression of a comic book, graphic novel, etc. to an expression."@en .

<http://rdaregistry.info/Elements/a/P50246>
    rdakit:instructionNumber "18.5" ;
    rdakit:toolkitDefinition "A work of calligraphy that involves an artistic responsibility for the focus of interest in the aesthetic value of its penmanship or graphic artistry, regardless of whether the same person, etc. also authored the inscribed text."@en, "Artiste responsable de la création d’une œuvre de calligraphie où l’accent est mis sur la valeur esthétique de la calligraphie ou du graphisme, peu importe que la même personne, etc. soit aussi l’auteur du texte calligraphié."@fr ;
    rdakit:toolkitLabel "calligraphe de"@fr, "calligrapher of"@en ;
    reg:hasSubproperty <http://rdaregistry.info/Elements/a/datatype/P50246>, <http://rdaregistry.info/Elements/a/object/P50246> ;
    reg:hasUnconstrained <http://rdaregistry.info/Elements/u/P60758> ;
    reg:lexicalAlias <http://rdaregistry.info/Elements/a/calligrapherOf.en> ;
    reg:name "calligrapherOf"@en ;
    reg:status <http://metadataregistry.org/uri/RegStatus/1001> ;
    a rdf:Property ;
    rdfs:domain <http://rdaregistry.info/Elements/c/C10002> ;
    rdfs:isDefinedBy <http://rdaregistry.info/Elements/a/> ;
    rdfs:label "est le calligraphe de"@fr, "is calligrapher of"@en ;
    rdfs:subPropertyOf <http://rdaregistry.info/Elements/a/P50192> ;
    skos:definition "Met un artiste responsable de la création d’une œuvre de calligraphie où l’accent est mis sur la valeur esthétique de la calligraphie ou du graphisme, peu importe que la même personne, etc. soit aussi l’auteur du texte calligraphié, en relation avec l’œuvre."@fr, "Relates an artist responsible for creating a work of calligraphy where the focus of interest lies in the aesthetic value of its penmanship or graphic artistry, regardless of whether the same person, etc to a work."@en .

<http://rdaregistry.info/Elements/a/P50247>
    rdakit:instructionNumber "18.5" ;
    rdakit:toolkitDefinition "A work that involves an artistic responsibility for creating art works that exploit the book form or alter its physical structure as part of the content."@en, "Artiste responsable de la création d’œuvres d’art qui exploitent la forme livre ou qui modifient sa structure physique comme partie du contenu de l’œuvre."@fr ;
    rdakit:toolkitLabel "artiste du livre de"@fr, "book artist of"@en ;
    reg:hasSubproperty <http://rdaregistry.info/Elements/a/datatype/P50247>, <http://rdaregistry.info/Elements/a/object/P50247> ;
    reg:hasUnconstrained <http://rdaregistry.info/Elements/u/P60759> ;
    reg:lexicalAlias <http://rdaregistry.info/Elements/a/bookArtistOf.en> ;
    reg:name "bookArtistOf"@en ;
    reg:status <http://metadataregistry.org/uri/RegStatus/1001> ;
    a rdf:Property ;
    rdfs:domain <http://rdaregistry.info/Elements/c/C10002> ;
    rdfs:isDefinedBy <http://rdaregistry.info/Elements/a/> ;
    rdfs:label "est l’artiste du livre de"@fr, "is book artist of"@en ;
    rdfs:subPropertyOf <http://rdaregistry.info/Elements/a/P50192> ;
    skos:definition "Met un artiste responsable de la création d’œuvres d’art qui exploitent la forme livre ou qui modifient sa structure physique comme partie du contenu de l’œuvre en relation avec l’œuvre."@fr, "Relates an artist resonsible for creating art works that exploit the book form or alter its physical structure as part of the content to a work."@en .

<http://rdaregistry.info/Elements/a/P50248>
    rdakit:instructionNumber "18.5" ;
    rdakit:seeAlso <http://rdaregistry.info/Elements/a/P50212> ;
    rdakit:toolkitDefinition "A work that involves a responsibility for reporting on the proceedings of the meetings of an organization."@en, "Auteur nommé par une organisation pour rédiger les comptes rendus de ses réunions."@fr ;
    rdakit:toolkitLabel "rapporteur de"@fr, "rapporteur of"@en ;
    reg:hasSubproperty <http://rdaregistry.info/Elements/a/datatype/P50248>, <http://rdaregistry.info/Elements/a/object/P50248> ;
    reg:hasUnconstrained <http://rdaregistry.info/Elements/u/P60757> ;
    reg:lexicalAlias <http://rdaregistry.info/Elements/a/rapporteurOf.en> ;
    reg:name "rapporteurOf"@en ;
    reg:status <http://metadataregistry.org/uri/RegStatus/1001> ;
    a rdf:Property ;
    rdfs:domain <http://rdaregistry.info/Elements/c/C10002> ;
    rdfs:isDefinedBy <http://rdaregistry.info/Elements/a/> ;
    rdfs:label "est le rapporteur de"@fr, "is rapporteur of"@en ;
    rdfs:subPropertyOf <http://rdaregistry.info/Elements/a/P50195> ;
    skos:definition "Met un auteur nommé par une organisation pour rédiger les comptes rendus de ses réunions en relation avec l’œuvre."@fr, "Relates an author who is appointed by an organization to report on the proceedings of its meetings to a work."@en .

<http://rdaregistry.info/Elements/a/P50249>
    rdakit:toolkitDefinition "A work that is about a person."@en ;
    rdakit:toolkitLabel "subject of (person)"@en ;
    reg:hasSubproperty <http://rdaregistry.info/Elements/a/datatype/P50249>, <http://rdaregistry.info/Elements/a/object/P50249> ;
    reg:hasUnconstrained <http://rdaregistry.info/Elements/u/P60806> ;
    reg:lexicalAlias <http://rdaregistry.info/Elements/a/subjectOfPerson.en> ;
    reg:name "subjectOfPerson"@en ;
    reg:status <http://metadataregistry.org/uri/RegStatus/1001> ;
    a rdf:Property ;
    rdfs:domain <http://rdaregistry.info/Elements/c/C10004> ;
    rdfs:isDefinedBy <http://rdaregistry.info/Elements/a/> ;
    rdfs:label "is subject of (person)"@en ;
    rdfs:subPropertyOf <http://rdaregistry.info/Elements/a/P50366> ;
    skos:definition "Relates a person to a work that is about a person."@en .

<http://rdaregistry.info/Elements/a/P50250>
    rdakit:toolkitDefinition "A work that is about a family."@en ;
    rdakit:toolkitLabel "subject of (family)"@en ;
    reg:hasSubproperty <http://rdaregistry.info/Elements/a/datatype/P50250>, <http://rdaregistry.info/Elements/a/object/P50250> ;
    reg:hasUnconstrained <http://rdaregistry.info/Elements/u/P60806> ;
    reg:lexicalAlias <http://rdaregistry.info/Elements/a/subjectOfFamily.en> ;
    reg:name "subjectOfFamily"@en ;
    reg:status <http://metadataregistry.org/uri/RegStatus/1001> ;
    a rdf:Property ;
    rdfs:domain <http://rdaregistry.info/Elements/c/C10008> ;
    rdfs:isDefinedBy <http://rdaregistry.info/Elements/a/> ;
    rdfs:label "is subject of (family)"@en ;
    rdfs:subPropertyOf <http://rdaregistry.info/Elements/a/P50367> ;
    skos:definition "Relates a family to a work that is about a family."@en .

<http://rdaregistry.info/Elements/a/P50251>
    rdakit:toolkitDefinition "A work that is about a corporate body."@en ;
    rdakit:toolkitLabel "subject of (corporate body)"@en ;
    reg:hasSubproperty <http://rdaregistry.info/Elements/a/datatype/P50251>, <http://rdaregistry.info/Elements/a/object/P50251> ;
    reg:hasUnconstrained <http://rdaregistry.info/Elements/u/P60806> ;
    reg:lexicalAlias <http://rdaregistry.info/Elements/a/subjectOfCorporateBody.en> ;
    reg:name "subjectOfCorporateBody"@en ;
    reg:status <http://metadataregistry.org/uri/RegStatus/1001> ;
    a rdf:Property ;
    rdfs:domain <http://rdaregistry.info/Elements/c/C10005> ;
    rdfs:isDefinedBy <http://rdaregistry.info/Elements/a/> ;
    rdfs:label "is subject of (corporate body)"@en ;
    rdfs:subPropertyOf <http://rdaregistry.info/Elements/a/P50367> ;
    skos:definition "Relates a corporate body to a work that is about a corporate body."@en .

<http://rdaregistry.info/Elements/a/P50252>
    rdakit:instructionNumber "29.5" ;
    rdakit:toolkitDefinition "A person who receives an academic degree from a granting institution or faculty."@en, "Una persona que recibe un grado académico de una institución o facultad otorgante."@es ;
    rdakit:toolkitLabel "graduado"@es, "graduate"@en ;
    reg:hasSubproperty <http://rdaregistry.info/Elements/a/datatype/P50252>, <http://rdaregistry.info/Elements/a/object/P50252> ;
    reg:hasUnconstrained <http://rdaregistry.info/Elements/u/P60807> ;
    reg:lexicalAlias <http://rdaregistry.info/Elements/a/graduate.en> ;
    reg:name "graduate"@en ;
    reg:status <http://metadataregistry.org/uri/RegStatus/1001> ;
    a rdf:Property ;
    rdfs:domain <http://rdaregistry.info/Elements/c/C10005> ;
    rdfs:isDefinedBy <http://rdaregistry.info/Elements/a/> ;
    rdfs:label "has graduate"@en ;
    skos:definition "Relates a corporate body to a person who receives an academic degree from a granting institution or faculty."@en .

<http://rdaregistry.info/Elements/a/P50253>
    rdakit:instructionNumber "29.5" ;
    rdakit:toolkitDefinition "An institution or faculty that granted an academic degree to a person."@en, "Una institución o facultad que otorgó un grado académico a la persona."@es ;
    rdakit:toolkitLabel "graduado de"@es, "graduate of"@en ;
    reg:hasSubproperty <http://rdaregistry.info/Elements/a/datatype/P50253>, <http://rdaregistry.info/Elements/a/object/P50253> ;
    reg:hasUnconstrained <http://rdaregistry.info/Elements/u/P60808> ;
    reg:lexicalAlias <http://rdaregistry.info/Elements/a/graduateOf.en> ;
    reg:name "graduateOf"@en ;
    reg:status <http://metadataregistry.org/uri/RegStatus/1001> ;
    a rdf:Property ;
    rdfs:domain <http://rdaregistry.info/Elements/c/C10004> ;
    rdfs:isDefinedBy <http://rdaregistry.info/Elements/a/> ;
    rdfs:label "is graduate of"@en ;
    skos:definition "Relates a person to an institution or faculty that granted an academic degree to a person."@en .

<http://rdaregistry.info/Elements/a/P50254>
    rdakit:instructionNumber "18.5" ;
    rdakit:toolkitDefinition "An expression of a work that incorporates a contribution of providing a foreword to an original work."@en ;
    rdakit:toolkitLabel "writer of foreword of"@en ;
    reg:hasSubproperty <http://rdaregistry.info/Elements/a/datatype/P50254>, <http://rdaregistry.info/Elements/a/object/P50254> ;
    reg:hasUnconstrained <http://rdaregistry.info/Elements/u/P60810> ;
    reg:lexicalAlias <http://rdaregistry.info/Elements/a/writerOfForewordOf.en> ;
    reg:name "writerOfForewordOf"@en ;
    reg:status <http://metadataregistry.org/uri/RegStatus/1001> ;
    a rdf:Property ;
    rdfs:domain <http://rdaregistry.info/Elements/c/C10002> ;
    rdfs:isDefinedBy <http://rdaregistry.info/Elements/a/> ;
    rdfs:label "is writer of foreword of"@en ;
    rdfs:subPropertyOf <http://rdaregistry.info/Elements/a/P50154> ;
    skos:definition "Relates an agent contributing to an expression of a work by providing a foreword to an original work to an expression."@en .

<http://rdaregistry.info/Elements/a/P50255>
    rdakit:instructionNumber "18.5" ;
    rdakit:toolkitDefinition "An expression of a work that incorporates a contribution of designing and creating audio or sound components."@en ;
    rdakit:toolkitLabel "sound designer of"@en ;
    reg:hasSubproperty <http://rdaregistry.info/Elements/a/datatype/P50255>, <http://rdaregistry.info/Elements/a/object/P50255> ;
    reg:hasUnconstrained <http://rdaregistry.info/Elements/u/P60812> ;
    reg:lexicalAlias <http://rdaregistry.info/Elements/a/soundDesignerOf.en> ;
    reg:name "soundDesignerOf"@en ;
    reg:status <http://metadataregistry.org/uri/RegStatus/1001> ;
    a rdf:Property ;
    rdfs:domain <http://rdaregistry.info/Elements/c/C10002> ;
    rdfs:isDefinedBy <http://rdaregistry.info/Elements/a/> ;
    rdfs:label "is sound designer of"@en ;
    rdfs:subPropertyOf <http://rdaregistry.info/Elements/a/P50161> ;
    skos:definition "Relates an agent contributing to an expression of a work by designing and creating audio or sound components to an expression."@en .

<http://rdaregistry.info/Elements/a/P50256>
    rdakit:instructionNumber "18.5" ;
    rdakit:toolkitDefinition "An expression of a work that incorporates a contribution of designing and creating lighting components."@en ;
    rdakit:toolkitLabel "lighting designer of"@en ;
    reg:hasSubproperty <http://rdaregistry.info/Elements/a/datatype/P50256>, <http://rdaregistry.info/Elements/a/object/P50256> ;
    reg:hasUnconstrained <http://rdaregistry.info/Elements/u/P60814> ;
    reg:lexicalAlias <http://rdaregistry.info/Elements/a/lightingDesignerOf.en> ;
    reg:name "lightingDesignerOf"@en ;
    reg:status <http://metadataregistry.org/uri/RegStatus/1001> ;
    a rdf:Property ;
    rdfs:domain <http://rdaregistry.info/Elements/c/C10002> ;
    rdfs:isDefinedBy <http://rdaregistry.info/Elements/a/> ;
    rdfs:label "is lighting designer of"@en ;
    rdfs:subPropertyOf <http://rdaregistry.info/Elements/a/P50161> ;
    skos:definition "Relates an agent contributing to an expression of a work by designing and creating lighting components to an expression."@en .

<http://rdaregistry.info/Elements/a/P50257>
    rdakit:instructionNumber "18.5" ;
    rdakit:toolkitDefinition "A work that involves a responsibility for serving on a committee that supervises a student's thesis or dissertation."@en ;
    rdakit:toolkitLabel "degree committee member of"@en ;
    reg:hasSubproperty <http://rdaregistry.info/Elements/a/datatype/P50257>, <http://rdaregistry.info/Elements/a/object/P50257> ;
    reg:hasUnconstrained <http://rdaregistry.info/Elements/u/P60816> ;
    reg:lexicalAlias <http://rdaregistry.info/Elements/a/degreeCommitteeMemberOf.en> ;
    reg:name "degreeCommitteeMemberOf"@en ;
    reg:status <http://metadataregistry.org/uri/RegStatus/1001> ;
    a rdf:Property ;
    rdfs:domain <http://rdaregistry.info/Elements/c/C10004> ;
    rdfs:isDefinedBy <http://rdaregistry.info/Elements/a/> ;
    rdfs:label "is degree committee member of"@en ;
    rdfs:subPropertyOf <http://rdaregistry.info/Elements/a/P50131> ;
    skos:definition "Relates a person serving on a committee that supervises a student's thesis or dissertation to a work."@en .

<http://rdaregistry.info/Elements/a/P50258>
    rdakit:instructionNumber "18.5" ;
    rdakit:toolkitDefinition "A work that involves a responsibility for being a corporate body accused in a criminal proceeding or sued in a civil proceeding."@en, "Collectivité qui est accusée dans une poursuite criminelle ou contre laquelle une poursuite civile est intentée."@fr ;
    rdakit:toolkitLabel "collectivité défenderesse de"@fr, "defendant corporate body of"@en ;
    reg:hasSubproperty <http://rdaregistry.info/Elements/a/datatype/P50258>, <http://rdaregistry.info/Elements/a/object/P50258> ;
    reg:hasUnconstrained <http://rdaregistry.info/Elements/u/P60698> ;
    reg:lexicalAlias <http://rdaregistry.info/Elements/a/defendantCorporateBodyOf.en> ;
    reg:name "defendantCorporateBodyOf"@en ;
    reg:status <http://metadataregistry.org/uri/RegStatus/1001> ;
    a rdf:Property ;
    rdfs:domain <http://rdaregistry.info/Elements/c/C10005> ;
    rdfs:isDefinedBy <http://rdaregistry.info/Elements/a/> ;
    rdfs:label "est la collectivité défenderesse de"@fr, "is defendant corporate body of"@en ;
    rdfs:subPropertyOf <http://rdaregistry.info/Elements/a/P50090> ;
    skos:definition "Met une collectivité qui est accusée dans une poursuite criminelle ou contre laquelle une poursuite civile est intentée en relation avec l’œuvre."@fr, "Relates a corporate body who is accused in a criminal proceeding or sued in a civil proceeding to a work."@en .

<http://rdaregistry.info/Elements/a/P50259>
    rdakit:instructionNumber "18.5" ;
    rdakit:toolkitDefinition "A work that involves a responsibility for being a person accused in a criminal proceeding or sued in a civil proceeding."@en, "Personne qui est accusée dans une poursuite criminelle ou contre laquelle une poursuite civile est intentée."@fr ;
    rdakit:toolkitLabel "defendant person of"@en, "personne défenderesse de"@fr ;
    reg:hasSubproperty <http://rdaregistry.info/Elements/a/datatype/P50259>, <http://rdaregistry.info/Elements/a/object/P50259> ;
    reg:hasUnconstrained <http://rdaregistry.info/Elements/u/P60698> ;
    reg:lexicalAlias <http://rdaregistry.info/Elements/a/defendantPersonOf.en> ;
    reg:name "defendantPersonOf"@en ;
    reg:status <http://metadataregistry.org/uri/RegStatus/1001> ;
    a rdf:Property ;
    rdfs:domain <http://rdaregistry.info/Elements/c/C10004> ;
    rdfs:isDefinedBy <http://rdaregistry.info/Elements/a/> ;
    rdfs:label "est la personne défenderesse de"@fr, "is defendant person of"@en ;
    rdfs:subPropertyOf <http://rdaregistry.info/Elements/a/P50090> ;
    skos:definition "Met une personne qui est accusée dans une poursuite criminelle ou contre laquelle une poursuite civile est intentée en relation avec l’œuvre."@fr, "Relates a person who is accused in a criminal proceeding or sued in a civil proceeding to a work."@en .

<http://rdaregistry.info/Elements/a/P50260>
    rdakit:instructionNumber "11.3.3" ;
    rdakit:toolkitDefinition "A place associated with a corporate body other than location of a conference, etc."@en, "Un lugar asociado con una entidad corporativa diferente al lugar de una conferencia, etc."@es ;
    rdakit:toolkitLabel "other place associated with the corporate body"@en, "otro lugar asociado con la entidad corporativa"@es, "övrig ort förknippad med institutionen"@sv ;
    reg:hasSubproperty <http://rdaregistry.info/Elements/a/datatype/P50260> ;
    reg:hasUnconstrained <http://rdaregistry.info/Elements/u/P60325> ;
    reg:lexicalAlias <http://rdaregistry.info/Elements/a/otherPlaceAssociatedWithTheCorporateBody.en> ;
    reg:name "otherPlaceAssociatedWithTheCorporateBody"@en ;
    reg:status <http://metadataregistry.org/uri/RegStatus/1001> ;
    a rdf:Property ;
    rdfs:domain <http://rdaregistry.info/Elements/c/C10005> ;
    rdfs:isDefinedBy <http://rdaregistry.info/Elements/a/> ;
    rdfs:label "har övrig ort förknippad med institutionen"@sv, "has other place associated with the corporate body"@en ;
    rdfs:subPropertyOf <http://rdaregistry.info/Elements/a/P50031> ;
    skos:definition "Relates a corporate body to a place associated with a corporate body other than location of a conference, etc."@en ;
    skos:scopeNote "Other place associated with a corporate body includes a country, state, province, local place, etc., associated with a corporate body and the location of headquarters of a corporate body."@en .

<http://rdaregistry.info/Elements/a/P50261>
    rdakit:instructionNumber "18.5" ;
    rdakit:seeAlso <http://rdaregistry.info/Elements/a/P50072> ;
    rdakit:toolkitDefinition "An expression of a nonfiction moving image work that incorporates a contribution of taking an active role as a participant."@en ;
    rdakit:toolkitLabel "on-screen participant of"@en ;
    reg:hasSubproperty <http://rdaregistry.info/Elements/a/datatype/P50261>, <http://rdaregistry.info/Elements/a/object/P50261> ;
    reg:hasUnconstrained <http://rdaregistry.info/Elements/u/P60825> ;
    reg:lexicalAlias <http://rdaregistry.info/Elements/a/onScreenParticipantOf.en> ;
    reg:name "onscreenParticipantOf"@en ;
    reg:status <http://metadataregistry.org/uri/RegStatus/1001> ;
    a rdf:Property ;
    rdfs:domain <http://rdaregistry.info/Elements/c/C10002> ;
    rdfs:isDefinedBy <http://rdaregistry.info/Elements/a/> ;
    rdfs:label "is on-screen participant of"@en ;
    rdfs:subPropertyOf <http://rdaregistry.info/Elements/a/P50161> ;
    skos:definition "Relates an agent contributing to an expression of a nonfiction moving image work by taking an active role as a participant to an expression."@en .

<http://rdaregistry.info/Elements/a/P50262>
    rdakit:instructionNumber "18.5" ;
    rdakit:toolkitDefinition "A work that involves a responsibility for commissioning a work."@en ;
    rdakit:toolkitLabel "commissioning body of"@en ;
    reg:hasSubproperty <http://rdaregistry.info/Elements/a/datatype/P50262>, <http://rdaregistry.info/Elements/a/object/P50262> ;
    reg:hasUnconstrained <http://rdaregistry.info/Elements/u/P60827> ;
    reg:lexicalAlias <http://rdaregistry.info/Elements/a/commissioningBodyOf.en> ;
    reg:name "commissioningBodyOf"@en ;
    reg:status <http://metadataregistry.org/uri/RegStatus/1001> ;
    a rdf:Property ;
    rdfs:domain <http://rdaregistry.info/Elements/c/C10002> ;
    rdfs:isDefinedBy <http://rdaregistry.info/Elements/a/> ;
    rdfs:label "is commissioning body of"@en ;
    rdfs:subPropertyOf <http://rdaregistry.info/Elements/a/P50131> ;
    skos:definition "Relates an agent responsible for commissioning a work to a work."@en .

<http://rdaregistry.info/Elements/a/P50263>
    rdakit:instructionNumber "18.5" ;
    rdakit:toolkitDefinition "An expression of a work that incorporates a contribution of researching, designing, implementing, or testing the software."@en ;
    rdakit:toolkitLabel "software developer of"@en ;
    reg:hasSubproperty <http://rdaregistry.info/Elements/a/datatype/P50263>, <http://rdaregistry.info/Elements/a/object/P50263> ;
    reg:hasUnconstrained <http://rdaregistry.info/Elements/u/P60829> ;
    reg:lexicalAlias <http://rdaregistry.info/Elements/a/softwareDeveloperOf.en> ;
    reg:name "softwareDeveloperOf"@en ;
    reg:status <http://metadataregistry.org/uri/RegStatus/1001> ;
    a rdf:Property ;
    rdfs:domain <http://rdaregistry.info/Elements/c/C10002> ;
    rdfs:isDefinedBy <http://rdaregistry.info/Elements/a/> ;
    rdfs:label "is software developer of"@en ;
    rdfs:subPropertyOf <http://rdaregistry.info/Elements/a/P50161> ;
    skos:definition "Relates an agent contributing to an expression of a work by researching, designing, implementing, or testing the software to an expression."@en .

<http://rdaregistry.info/Elements/a/P50264>
    rdakit:instructionNumber "18.5" ;
    rdakit:toolkitDefinition "A work that is signed, ratified, or acceded to a treaty."@en, "Gouvernement, organisation internationale intergouvernementale ou autre collectivité qui a signé ou ratifié un traité ou y a adhéré."@fr ;
    rdakit:toolkitLabel "participant in a treaty of"@en, "participant à un traité de"@fr ;
    reg:hasSubproperty <http://rdaregistry.info/Elements/a/datatype/P50264>, <http://rdaregistry.info/Elements/a/object/P50264> ;
    reg:hasUnconstrained <http://rdaregistry.info/Elements/u/P60835> ;
    reg:lexicalAlias <http://rdaregistry.info/Elements/a/participantInATreatyOf.en> ;
    reg:name "participantInATreatyOf"@en ;
    reg:status <http://metadataregistry.org/uri/RegStatus/1001> ;
    a rdf:Property ;
    rdfs:domain <http://rdaregistry.info/Elements/c/C10005> ;
    rdfs:isDefinedBy <http://rdaregistry.info/Elements/a/> ;
    rdfs:label "est le participant à un traité de"@fr, "is participant in a treaty of"@en ;
    rdfs:subPropertyOf <http://rdaregistry.info/Elements/a/P50131> ;
    skos:definition "Met un gouvernement, une organisation internationale intergouvernementale ou une autre collectivité qui a signé ou ratifié un traité ou y a adhéré en relation avec l’œuvre."@fr, "Relates a government, international intergovernmental body, or other corporate body that has signed, ratified, or acceded to a treaty to a work."@en .

<http://rdaregistry.info/Elements/a/P50265>
    rdakit:instructionNumber "18.5" ;
    rdakit:toolkitDefinition "A work that involves a responsibility for research in support of the creation of a work."@en ;
    rdakit:toolkitLabel "researcher of"@en ;
    reg:hasSubproperty <http://rdaregistry.info/Elements/a/datatype/P50265>, <http://rdaregistry.info/Elements/a/object/P50265> ;
    reg:hasUnconstrained <http://rdaregistry.info/Elements/u/P60837> ;
    reg:lexicalAlias <http://rdaregistry.info/Elements/a/researcherOf.en> ;
    reg:name "researcherOf"@en ;
    reg:status <http://metadataregistry.org/uri/RegStatus/1001> ;
    a rdf:Property ;
    rdfs:domain <http://rdaregistry.info/Elements/c/C10002> ;
    rdfs:isDefinedBy <http://rdaregistry.info/Elements/a/> ;
    rdfs:label "is researcher of"@en ;
    rdfs:subPropertyOf <http://rdaregistry.info/Elements/a/P50131> ;
    skos:definition "Relates an agent who does research in support of the creation of a work to a work."@en .

<http://rdaregistry.info/Elements/a/P50266>
    rdakit:instructionNumber "18.5" ;
    rdakit:toolkitDefinition "An expression of a work that incorporates a contribution of applying colour to drawings, prints, photographs, maps, moving images, etc."@en ;
    rdakit:toolkitLabel "colourist of"@en ;
    reg:hasSubproperty <http://rdaregistry.info/Elements/a/datatype/P50266>, <http://rdaregistry.info/Elements/a/object/P50266> ;
    reg:hasUnconstrained <http://rdaregistry.info/Elements/u/P60839> ;
    reg:lexicalAlias <http://rdaregistry.info/Elements/a/colouristOf.en> ;
    reg:name "colouristOf"@en ;
    reg:status <http://metadataregistry.org/uri/RegStatus/1001> ;
    a rdf:Property ;
    rdfs:domain <http://rdaregistry.info/Elements/c/C10002> ;
    rdfs:isDefinedBy <http://rdaregistry.info/Elements/a/> ;
    rdfs:label "is colourist of"@en ;
    rdfs:subPropertyOf <http://rdaregistry.info/Elements/a/P50161> ;
    skos:definition "Relates an agent contributing to an expression of a work by applying colour to drawings, prints, photographs, maps, moving images, etc. to an expression."@en .

<http://rdaregistry.info/Elements/a/P50267>
    rdakit:instructionNumber "18.5" ;
    rdakit:toolkitDefinition "An expression of a work that incorporates a contribution of applying make-up and prosthetics for a moving image production or for a musical or dramatic presentation or entertainment."@en ;
    rdakit:toolkitLabel "make-up artist of"@en ;
    reg:hasSubproperty <http://rdaregistry.info/Elements/a/datatype/P50267>, <http://rdaregistry.info/Elements/a/object/P50267> ;
    reg:hasUnconstrained <http://rdaregistry.info/Elements/u/P60841> ;
    reg:lexicalAlias <http://rdaregistry.info/Elements/a/makeUpArtistOf.en> ;
    reg:name "makeUpArtistOf"@en ;
    reg:status <http://metadataregistry.org/uri/RegStatus/1001> ;
    a rdf:Property ;
    rdfs:domain <http://rdaregistry.info/Elements/c/C10002> ;
    rdfs:isDefinedBy <http://rdaregistry.info/Elements/a/> ;
    rdfs:label "is make-up artist of"@en ;
    rdfs:subPropertyOf <http://rdaregistry.info/Elements/a/P50161> ;
    skos:definition "Relates an agent contributing to an expression of a work by applying make-up and prosthetics for a moving image production or for a musical or dramatic presentation or entertainment to an expression."@en .

<http://rdaregistry.info/Elements/a/P50268>
    rdakit:instructionNumber "18.5" ;
    rdakit:toolkitDefinition "An expression of a musical work that incorporates a contribution of leading a choral performing group in a musical or dramatic presentation, etc."@en ;
    rdakit:toolkitLabel "choral conductor of"@en ;
    reg:hasSubproperty <http://rdaregistry.info/Elements/a/datatype/P50268>, <http://rdaregistry.info/Elements/a/object/P50268> ;
    reg:hasUnconstrained <http://rdaregistry.info/Elements/u/P60843> ;
    reg:lexicalAlias <http://rdaregistry.info/Elements/a/choralConductorOf.en> ;
    reg:name "choralConductorOf"@en ;
    reg:status <http://metadataregistry.org/uri/RegStatus/1001> ;
    a rdf:Property ;
    rdfs:domain <http://rdaregistry.info/Elements/c/C10002> ;
    rdfs:isDefinedBy <http://rdaregistry.info/Elements/a/> ;
    rdfs:label "is choral conductor of"@en ;
    rdfs:subPropertyOf <http://rdaregistry.info/Elements/a/P50070> ;
    skos:definition "Relates a conductor contributing to an expression of a musical work by leading a choral performing group in a musical or dramatic presentation, etc. to an expression."@en .

<http://rdaregistry.info/Elements/a/P50269>
    rdakit:instructionNumber "18.5" ;
    rdakit:toolkitDefinition "An expression of a musical work that incorporates a conducting contribution by leading an instrumental performing group in a musical or dramatic presentation, etc."@en ;
    rdakit:toolkitLabel "instrumental conductor of"@en ;
    reg:hasSubproperty <http://rdaregistry.info/Elements/a/datatype/P50269>, <http://rdaregistry.info/Elements/a/object/P50269> ;
    reg:hasUnconstrained <http://rdaregistry.info/Elements/u/P60845> ;
    reg:lexicalAlias <http://rdaregistry.info/Elements/a/instrumentalConductorOf.en> ;
    reg:name "instrumentalConductorOf"@en ;
    reg:status <http://metadataregistry.org/uri/RegStatus/1001> ;
    a rdf:Property ;
    rdfs:domain <http://rdaregistry.info/Elements/c/C10002> ;
    rdfs:isDefinedBy <http://rdaregistry.info/Elements/a/> ;
    rdfs:label "is instrumental conductor of"@en ;
    rdfs:subPropertyOf <http://rdaregistry.info/Elements/a/P50070> ;
    skos:definition "Relates a conductor contributing to an expression of a musical work by leading an instrumental performing group in a musical or dramatic presentation, etc. to an expression."@en .

<http://rdaregistry.info/Elements/a/P50270>
    rdakit:instructionNumber "18.5" ;
    rdakit:toolkitDefinition "A work that involves a responsibility for organizing an exhibit, event, conference, etc., which gave rise to a work."@en, "Personne, famille ou collectivité organisant l’exposition, l’événement, le congrès, etc. qui a donné lieu à la création d’une œuvre."@fr ;
    rdakit:toolkitLabel "organisateur de"@fr, "organizer of"@en ;
    reg:hasSubproperty <http://rdaregistry.info/Elements/a/datatype/P50270>, <http://rdaregistry.info/Elements/a/object/P50270> ;
    reg:hasUnconstrained <http://rdaregistry.info/Elements/u/P60850> ;
    reg:lexicalAlias <http://rdaregistry.info/Elements/a/organizerOf.en> ;
    reg:name "organizerOf"@en ;
    reg:status <http://metadataregistry.org/uri/RegStatus/1001> ;
    a rdf:Property ;
    rdfs:domain <http://rdaregistry.info/Elements/c/C10002> ;
    rdfs:isDefinedBy <http://rdaregistry.info/Elements/a/> ;
    rdfs:label "est l’organisateur de"@fr, "is organizer of"@en ;
    rdfs:subPropertyOf <http://rdaregistry.info/Elements/a/P50131> ;
    skos:definition "Met une personne, famille ou collectivité organisant l’exposition, l’événement, le congrès, etc. qui a donné lieu à la création d’une œuvre en relation avec l’œuvre."@fr, "Relates an agent organizing an exhibit, event, conference, etc., which gave rise to a work to a work."@en .

<http://rdaregistry.info/Elements/a/P50271>
    rdakit:instructionNumber "18.5" ;
    rdakit:seeAlso <http://rdaregistry.info/Elements/a/P50195> ;
    rdakit:toolkitDefinition "An expression of a work that involves a responsibility for revising the content for the purpose of suppressing parts deemed objectionable on moral, political, military, or other grounds, but leaving the nature and content substantially unchanged."@en ;
    rdakit:toolkitLabel "censor of"@en ;
    reg:hasSubproperty <http://rdaregistry.info/Elements/a/datatype/P50271>, <http://rdaregistry.info/Elements/a/object/P50271> ;
    reg:hasUnconstrained <http://rdaregistry.info/Elements/u/P60852> ;
    reg:lexicalAlias <http://rdaregistry.info/Elements/a/censorOf.en> ;
    reg:name "censorOf"@en ;
    reg:status <http://metadataregistry.org/uri/RegStatus/1001> ;
    a rdf:Property ;
    rdfs:domain <http://rdaregistry.info/Elements/c/C10002> ;
    rdfs:isDefinedBy <http://rdaregistry.info/Elements/a/> ;
    rdfs:label "is censor of"@en ;
    rdfs:subPropertyOf <http://rdaregistry.info/Elements/a/P50161> ;
    skos:definition "Relates an agent contributing to an expression of a work by revising the content for the purpose of suppressing parts deemed objectionable on moral, political, military, or other grounds, but leaving the nature and content substantially unchanged to an expression."@en .

<http://rdaregistry.info/Elements/a/P50272>
    rdakit:instructionNumber "18.5" ;
    rdakit:seeAlso <http://rdaregistry.info/Elements/a/P50190> ;
    rdakit:toolkitDefinition "An expression of a work that incorporates an illustrating contribution of providing supplementary photographic content to an original work."@en ;
    rdakit:toolkitLabel "photographer (expression) of"@en ;
    reg:hasSubproperty <http://rdaregistry.info/Elements/a/datatype/P50272>, <http://rdaregistry.info/Elements/a/object/P50272> ;
    reg:hasUnconstrained <http://rdaregistry.info/Elements/u/P60658> ;
    reg:lexicalAlias <http://rdaregistry.info/Elements/a/photographerExpressionOf.en> ;
    reg:name "photographerExpressionOf"@en ;
    reg:status <http://metadataregistry.org/uri/RegStatus/1001> ;
    a rdf:Property ;
    rdfs:domain <http://rdaregistry.info/Elements/c/C10002> ;
    rdfs:isDefinedBy <http://rdaregistry.info/Elements/a/> ;
    rdfs:label "is photographer (expression) of"@en ;
    rdfs:subPropertyOf <http://rdaregistry.info/Elements/a/P50161> ;
    skos:definition "Relates an illustrator contributing to an expression of a work by providing supplementary photographic content to an original work to an expression."@en .

<http://rdaregistry.info/Elements/a/P50273>
    rdakit:instructionNumber "18.5" ;
    rdakit:toolkitDefinition "An expression of a work that incorporates a contribution of restoring and/or combining earlier expressions, which may be damaged or fragmentary, to create a new expression."@en ;
    rdakit:toolkitLabel "restorationist (expression) of"@en ;
    reg:hasSubproperty <http://rdaregistry.info/Elements/a/datatype/P50273>, <http://rdaregistry.info/Elements/a/object/P50273> ;
    reg:hasUnconstrained <http://rdaregistry.info/Elements/u/P60674> ;
    reg:lexicalAlias <http://rdaregistry.info/Elements/a/restorationistExpressionOf.en> ;
    reg:name "restorationistExpressionOf"@en ;
    reg:status <http://metadataregistry.org/uri/RegStatus/1001> ;
    a rdf:Property ;
    rdfs:domain <http://rdaregistry.info/Elements/c/C10002> ;
    rdfs:isDefinedBy <http://rdaregistry.info/Elements/a/> ;
    rdfs:label "is restorationist (expression) of"@en ;
    rdfs:subPropertyOf <http://rdaregistry.info/Elements/a/P50161> ;
    skos:definition "Relates an agent who contributes to an expression of a work by restoring and/or combining earlier expressions, which may be damaged or fragmentary, to create a new expression to an expression."@en .

<http://rdaregistry.info/Elements/a/P50274>
    rdakit:instructionNumber "29.5" ;
    rdakit:toolkitDefinition "A fellow member of a profession, staff, or academic faculty."@en ;
    rdakit:toolkitLabel "colleague"@en ;
    reg:hasSubproperty <http://rdaregistry.info/Elements/a/datatype/P50274>, <http://rdaregistry.info/Elements/a/object/P50274>, <http://rdaregistry.info/Elements/a/object/P50275>, <http://rdaregistry.info/Elements/a/object/P50276>, <http://rdaregistry.info/Elements/a/object/P50277>, <http://rdaregistry.info/Elements/a/object/P50278> ;
    reg:hasUnconstrained <http://rdaregistry.info/Elements/u/P60853> ;
    reg:lexicalAlias <http://rdaregistry.info/Elements/a/colleague.en> ;
    reg:name "colleague"@en ;
    reg:status <http://metadataregistry.org/uri/RegStatus/1001> ;
    a rdf:Property ;
    rdfs:domain <http://rdaregistry.info/Elements/c/C10004> ;
    rdfs:isDefinedBy <http://rdaregistry.info/Elements/a/> ;
    rdfs:label "has colleague"@en ;
    rdfs:subPropertyOf <http://rdaregistry.info/Elements/a/P50220> ;
    skos:definition "Relates a person to a fellow member of a profession, staff, or academic faculty."@en .

<http://rdaregistry.info/Elements/a/P50275>
    rdakit:instructionNumber "29.5" ;
    rdakit:toolkitDefinition "A colleague who helps another person."@en ;
    rdakit:toolkitLabel "assistant"@en ;
    reg:hasSubproperty <http://rdaregistry.info/Elements/a/datatype/P50275>, <http://rdaregistry.info/Elements/a/object/P50275> ;
    reg:hasUnconstrained <http://rdaregistry.info/Elements/u/P60857> ;
    reg:lexicalAlias <http://rdaregistry.info/Elements/a/assistant.en> ;
    reg:name "assistant"@en ;
    reg:status <http://metadataregistry.org/uri/RegStatus/1001> ;
    a rdf:Property ;
    rdfs:domain <http://rdaregistry.info/Elements/c/C10004> ;
    rdfs:isDefinedBy <http://rdaregistry.info/Elements/a/> ;
    rdfs:label "has assistant"@en ;
    rdfs:subPropertyOf <http://rdaregistry.info/Elements/a/P50274> ;
    skos:definition "Relates a person to a colleague who helps another person."@en .

<http://rdaregistry.info/Elements/a/P50276>
    rdakit:instructionNumber "29.5" ;
    rdakit:toolkitDefinition "A colleague who is helped by another person."@en ;
    rdakit:toolkitLabel "assistant to"@en ;
    reg:hasSubproperty <http://rdaregistry.info/Elements/a/datatype/P50276>, <http://rdaregistry.info/Elements/a/object/P50276> ;
    reg:hasUnconstrained <http://rdaregistry.info/Elements/u/P60858> ;
    reg:lexicalAlias <http://rdaregistry.info/Elements/a/assistantTo.en> ;
    reg:name "assistantTo"@en ;
    reg:status <http://metadataregistry.org/uri/RegStatus/1001> ;
    a rdf:Property ;
    rdfs:domain <http://rdaregistry.info/Elements/c/C10004> ;
    rdfs:isDefinedBy <http://rdaregistry.info/Elements/a/> ;
    rdfs:label "is assistant to"@en ;
    rdfs:subPropertyOf <http://rdaregistry.info/Elements/a/P50274> ;
    skos:definition "Relates a person to a colleague who is helped by another person."@en .

<http://rdaregistry.info/Elements/a/P50277>
    rdakit:instructionNumber "29.5" ;
    rdakit:toolkitDefinition "A colleague who works with or shares a task with another person."@en ;
    rdakit:toolkitLabel "co-worker"@en ;
    reg:hasSubproperty <http://rdaregistry.info/Elements/a/datatype/P50277>, <http://rdaregistry.info/Elements/a/object/P50277> ;
    reg:hasUnconstrained <http://rdaregistry.info/Elements/u/P60859> ;
    reg:lexicalAlias <http://rdaregistry.info/Elements/a/coworker.en> ;
    reg:name "coworker"@en ;
    reg:status <http://metadataregistry.org/uri/RegStatus/1001> ;
    a rdf:Property ;
    rdfs:domain <http://rdaregistry.info/Elements/c/C10004> ;
    rdfs:isDefinedBy <http://rdaregistry.info/Elements/a/> ;
    rdfs:label "has co-worker"@en ;
    rdfs:subPropertyOf <http://rdaregistry.info/Elements/a/P50274> ;
    skos:definition "Relates a person to a colleague who works with or shares a task with another person."@en .

<http://rdaregistry.info/Elements/a/P50278>
    rdakit:instructionNumber "29.5" ;
    rdakit:toolkitDefinition "A colleague working with another person in an activity of common interest, most often, a business partnership."@en ;
    rdakit:toolkitLabel "partner"@en ;
    reg:hasSubproperty <http://rdaregistry.info/Elements/a/datatype/P50278>, <http://rdaregistry.info/Elements/a/object/P50278> ;
    reg:hasUnconstrained <http://rdaregistry.info/Elements/u/P60860> ;
    reg:lexicalAlias <http://rdaregistry.info/Elements/a/partner.en> ;
    reg:name "partner"@en ;
    reg:status <http://metadataregistry.org/uri/RegStatus/1001> ;
    a rdf:Property ;
    rdfs:domain <http://rdaregistry.info/Elements/c/C10004> ;
    rdfs:isDefinedBy <http://rdaregistry.info/Elements/a/> ;
    rdfs:label "has partner"@en ;
    rdfs:subPropertyOf <http://rdaregistry.info/Elements/a/P50274> ;
    skos:definition "Relates a person to a colleague working with another person in an activity of common interest, most often, a business partnership."@en .

<http://rdaregistry.info/Elements/a/P50279>
    rdakit:instructionNumber "29.5" ;
    rdakit:toolkitDefinition "An associate of another student who is also formally engaged in learning."@en ;
    rdakit:toolkitLabel "fellow student"@en ;
    reg:hasSubproperty <http://rdaregistry.info/Elements/a/datatype/P50279>, <http://rdaregistry.info/Elements/a/object/P50279> ;
    reg:hasUnconstrained <http://rdaregistry.info/Elements/u/P60861> ;
    reg:lexicalAlias <http://rdaregistry.info/Elements/a/fellowStudent.en> ;
    reg:name "fellowStudent"@en ;
    reg:status <http://metadataregistry.org/uri/RegStatus/1001> ;
    a rdf:Property ;
    rdfs:domain <http://rdaregistry.info/Elements/c/C10004> ;
    rdfs:isDefinedBy <http://rdaregistry.info/Elements/a/> ;
    rdfs:label "has fellow student"@en ;
    rdfs:subPropertyOf <http://rdaregistry.info/Elements/a/P50220> ;
    skos:definition "Relates a person to an associate of another student who is also formally engaged in learning."@en .

<http://rdaregistry.info/Elements/a/P50280>
    rdakit:instructionNumber "29.5" ;
    rdakit:toolkitDefinition "A person who shares a bond of mutual affection or regard with another person."@en ;
    rdakit:toolkitLabel "friend"@en ;
    reg:hasSubproperty <http://rdaregistry.info/Elements/a/datatype/P50280>, <http://rdaregistry.info/Elements/a/object/P50280> ;
    reg:hasUnconstrained <http://rdaregistry.info/Elements/u/P60854> ;
    reg:lexicalAlias <http://rdaregistry.info/Elements/a/friend.en> ;
    reg:name "friend"@en ;
    reg:status <http://metadataregistry.org/uri/RegStatus/1001> ;
    a rdf:Property ;
    rdfs:domain <http://rdaregistry.info/Elements/c/C10004> ;
    rdfs:isDefinedBy <http://rdaregistry.info/Elements/a/> ;
    rdfs:label "has friend"@en ;
    rdfs:subPropertyOf <http://rdaregistry.info/Elements/a/P50220> ;
    skos:definition "Relates a person to a person who shares a bond of mutual affection or regard with another person."@en .

<http://rdaregistry.info/Elements/a/P50281>
    rdakit:instructionNumber "29.5" ;
    rdakit:toolkitDefinition "A person who receives instruction from another person."@en ;
    rdakit:toolkitLabel "student"@en ;
    reg:hasSubproperty <http://rdaregistry.info/Elements/a/datatype/P50281>, <http://rdaregistry.info/Elements/a/object/P50281> ;
    reg:hasUnconstrained <http://rdaregistry.info/Elements/u/P60862> ;
    reg:lexicalAlias <http://rdaregistry.info/Elements/a/student.en> ;
    reg:name "student"@en ;
    reg:status <http://metadataregistry.org/uri/RegStatus/1001> ;
    a rdf:Property ;
    rdfs:domain <http://rdaregistry.info/Elements/c/C10004> ;
    rdfs:isDefinedBy <http://rdaregistry.info/Elements/a/> ;
    rdfs:label "has student"@en ;
    rdfs:subPropertyOf <http://rdaregistry.info/Elements/a/P50220> ;
    skos:definition "Relates a person to a person who receives instruction from another person."@en .

<http://rdaregistry.info/Elements/a/P50282>
    rdakit:instructionNumber "29.5" ;
    rdakit:toolkitDefinition "A person who instructs another person."@en ;
    rdakit:toolkitLabel "teacher"@en ;
    reg:hasSubproperty <http://rdaregistry.info/Elements/a/datatype/P50282>, <http://rdaregistry.info/Elements/a/object/P50282> ;
    reg:hasUnconstrained <http://rdaregistry.info/Elements/u/P60863> ;
    reg:lexicalAlias <http://rdaregistry.info/Elements/a/teacher.en> ;
    reg:name "teacher"@en ;
    reg:status <http://metadataregistry.org/uri/RegStatus/1001> ;
    a rdf:Property ;
    rdfs:domain <http://rdaregistry.info/Elements/c/C10004> ;
    rdfs:isDefinedBy <http://rdaregistry.info/Elements/a/> ;
    rdfs:label "has teacher"@en ;
    rdfs:subPropertyOf <http://rdaregistry.info/Elements/a/P50220> ;
    skos:definition "Relates a person to a person who instructs another person."@en .

<http://rdaregistry.info/Elements/a/P50283>
    rdakit:instructionNumber "29.5" ;
    rdakit:toolkitDefinition "A person who receives instruction at an educational institution."@en ;
    rdakit:toolkitLabel "enrolled student"@en ;
    reg:hasSubproperty <http://rdaregistry.info/Elements/a/datatype/P50283>, <http://rdaregistry.info/Elements/a/object/P50283> ;
    reg:hasUnconstrained <http://rdaregistry.info/Elements/u/P60855> ;
    reg:lexicalAlias <http://rdaregistry.info/Elements/a/enrolledStudent.en> ;
    reg:name "enrolledStudent"@en ;
    reg:status <http://metadataregistry.org/uri/RegStatus/1001> ;
    a rdf:Property ;
    rdfs:domain <http://rdaregistry.info/Elements/c/C10005> ;
    rdfs:isDefinedBy <http://rdaregistry.info/Elements/a/> ;
    rdfs:label "has enrolled student"@en ;
    rdfs:subPropertyOf <http://rdaregistry.info/Elements/a/P50220> ;
    skos:definition "Relates a corporate body to a person who receives instruction at an educational institution."@en .

<http://rdaregistry.info/Elements/a/P50284>
    rdakit:instructionNumber "29.5" ;
    rdakit:toolkitDefinition "An officer who is the top ranking official of a corporate body."@en ;
    rdakit:toolkitLabel "chief executive"@en ;
    reg:hasSubproperty <http://rdaregistry.info/Elements/a/datatype/P50284>, <http://rdaregistry.info/Elements/a/object/P50284> ;
    reg:hasUnconstrained <http://rdaregistry.info/Elements/u/P60864> ;
    reg:lexicalAlias <http://rdaregistry.info/Elements/a/chiefExecutive.en> ;
    reg:name "chiefExecutive"@en ;
    reg:status <http://metadataregistry.org/uri/RegStatus/1001> ;
    a rdf:Property ;
    rdfs:domain <http://rdaregistry.info/Elements/c/C10005> ;
    rdfs:isDefinedBy <http://rdaregistry.info/Elements/a/> ;
    rdfs:label "has chief executive"@en ;
    rdfs:subPropertyOf <http://rdaregistry.info/Elements/a/P50027> ;
    skos:definition "Relates a corporate body to an officer who is the top ranking official of a corporate body."@en .

<http://rdaregistry.info/Elements/a/P50285>
    rdakit:instructionNumber "29.5" ;
    rdakit:toolkitDefinition "An officer granted the powers of administration in a corporate body in order to act for its benefit."@en ;
    rdakit:toolkitLabel "trustee"@en ;
    reg:hasSubproperty <http://rdaregistry.info/Elements/a/datatype/P50285>, <http://rdaregistry.info/Elements/a/object/P50285> ;
    reg:hasUnconstrained <http://rdaregistry.info/Elements/u/P60866> ;
    reg:lexicalAlias <http://rdaregistry.info/Elements/a/trustee.en> ;
    reg:name "trustee"@en ;
    reg:status <http://metadataregistry.org/uri/RegStatus/1001> ;
    a rdf:Property ;
    rdfs:domain <http://rdaregistry.info/Elements/c/C10005> ;
    rdfs:isDefinedBy <http://rdaregistry.info/Elements/a/> ;
    rdfs:label "has trustee"@en ;
    rdfs:subPropertyOf <http://rdaregistry.info/Elements/a/P50027> ;
    skos:definition "Relates a corporate body to an officer granted the powers of administration in a corporate body in order to act for its benefit."@en .

<http://rdaregistry.info/Elements/a/P50286>
    rdakit:instructionNumber "29.5" ;
    rdakit:toolkitDefinition "A corporate body in which an officer is the top ranking official."@en ;
    rdakit:toolkitLabel "chief executive of"@en ;
    reg:hasSubproperty <http://rdaregistry.info/Elements/a/datatype/P50286>, <http://rdaregistry.info/Elements/a/object/P50286> ;
    reg:hasUnconstrained <http://rdaregistry.info/Elements/u/P60865> ;
    reg:lexicalAlias <http://rdaregistry.info/Elements/a/chiefExecutiveOf.en> ;
    reg:name "chiefExecutiveOf"@en ;
    reg:status <http://metadataregistry.org/uri/RegStatus/1001> ;
    a rdf:Property ;
    rdfs:domain <http://rdaregistry.info/Elements/c/C10004> ;
    rdfs:isDefinedBy <http://rdaregistry.info/Elements/a/> ;
    rdfs:label "is chief executive of"@en ;
    rdfs:subPropertyOf <http://rdaregistry.info/Elements/a/P50234> ;
    skos:definition "Relates a person to a corporate body in which an officer is the top ranking official."@en .

<http://rdaregistry.info/Elements/a/P50287>
    rdakit:instructionNumber "29.5" ;
    rdakit:toolkitDefinition "A corporate body that grants the powers of administration to an officer in order to act for its benefit."@en ;
    rdakit:toolkitLabel "trustee of"@en ;
    reg:hasSubproperty <http://rdaregistry.info/Elements/a/datatype/P50287>, <http://rdaregistry.info/Elements/a/object/P50287> ;
    reg:hasUnconstrained <http://rdaregistry.info/Elements/u/P60867> ;
    reg:lexicalAlias <http://rdaregistry.info/Elements/a/trusteeOf.en> ;
    reg:name "trusteeOf"@en ;
    reg:status <http://metadataregistry.org/uri/RegStatus/1001> ;
    a rdf:Property ;
    rdfs:domain <http://rdaregistry.info/Elements/c/C10004> ;
    rdfs:isDefinedBy <http://rdaregistry.info/Elements/a/> ;
    rdfs:label "is trustee of"@en ;
    rdfs:subPropertyOf <http://rdaregistry.info/Elements/a/P50234> ;
    skos:definition "Relates a person to a corporate body that grants the powers of administration to an officer in order to act for its benefit."@en .

<http://rdaregistry.info/Elements/a/P50288>
    rdakit:instructionNumber "29.5" ;
    rdakit:toolkitDefinition "An educational institution that provides instruction to a person."@en ;
    rdakit:toolkitLabel "student at"@en ;
    reg:hasSubproperty <http://rdaregistry.info/Elements/a/datatype/P50288>, <http://rdaregistry.info/Elements/a/object/P50288> ;
    reg:hasUnconstrained <http://rdaregistry.info/Elements/u/P60856> ;
    reg:lexicalAlias <http://rdaregistry.info/Elements/a/studentAt.en> ;
    reg:name "studentAt"@en ;
    reg:status <http://metadataregistry.org/uri/RegStatus/1001> ;
    a rdf:Property ;
    rdfs:domain <http://rdaregistry.info/Elements/c/C10004> ;
    rdfs:isDefinedBy <http://rdaregistry.info/Elements/a/> ;
    rdfs:label "is student at"@en ;
    rdfs:subPropertyOf <http://rdaregistry.info/Elements/a/P50218> ;
    skos:definition "Relates a person to an educational institution that provides instruction to a person."@en .

<http://rdaregistry.info/Elements/a/P50289>
    rdakit:instructionNumber "18.5" ;
    rdakit:seeAlso <http://rdaregistry.info/Elements/a/P50156> ;
    rdakit:toolkitDefinition "A work that includes a legal and/or intellectual responsibility other than creation for the content of a serial, integrating resource, or multipart monographic work."@en ;
    rdakit:toolkitLabel "editorial director of"@en ;
    reg:hasSubproperty <http://rdaregistry.info/Elements/a/datatype/P50289>, <http://rdaregistry.info/Elements/a/object/P50289> ;
    reg:hasUnconstrained <http://rdaregistry.info/Elements/u/P60870> ;
    reg:lexicalAlias <http://rdaregistry.info/Elements/a/editorialDirectorOf.en> ;
    reg:name "editorialDirectorOf"@en ;
    reg:status <http://metadataregistry.org/uri/RegStatus/1001> ;
    a rdf:Property ;
    rdfs:domain <http://rdaregistry.info/Elements/c/C10002> ;
    rdfs:isDefinedBy <http://rdaregistry.info/Elements/a/> ;
    rdfs:label "is editorial director of"@en ;
    rdfs:subPropertyOf <http://rdaregistry.info/Elements/a/P50131> ;
    skos:definition "Relates an agent responsible for the legal and/or intellectual responsibility other than creation for the content of a serial, integrating resource, or multipart monographic work to a work."@en, "Relates an agent responsible for the legal or intellectual responsibility other than creation for the content of a serial, integrating resource, or multipart monographic work to a work."@en .

<http://rdaregistry.info/Elements/a/P50290>
    rdakit:instructionNumber "18.5" ;
    rdakit:toolkitDefinition "A work that involves a responsibility for establishing a serial, integrating resource, or multipart monograph."@en ;
    rdakit:toolkitLabel "founder of work of"@en ;
    reg:hasSubproperty <http://rdaregistry.info/Elements/a/datatype/P50290>, <http://rdaregistry.info/Elements/a/object/P50290> ;
    reg:hasUnconstrained <http://rdaregistry.info/Elements/u/P60872> ;
    reg:lexicalAlias <http://rdaregistry.info/Elements/a/founderOfWorkOf.en> ;
    reg:name "founderOfWorkOf"@en ;
    reg:status <http://metadataregistry.org/uri/RegStatus/1001> ;
    a rdf:Property ;
    rdfs:domain <http://rdaregistry.info/Elements/c/C10002> ;
    rdfs:isDefinedBy <http://rdaregistry.info/Elements/a/> ;
    rdfs:label "is founder of work of"@en ;
    rdfs:subPropertyOf <http://rdaregistry.info/Elements/a/P50131> ;
    skos:definition "Relates an agent responsible for establishing a serial, integrating resource, or multipart monograph to a work."@en .

<http://rdaregistry.info/Elements/a/P50291>
    rdakit:instructionNumber "18.5" ;
    rdakit:toolkitDefinition "A name used as a family name."@en ;
    rdakit:toolkitLabel "surname"@en ;
    reg:hasSubproperty <http://rdaregistry.info/Elements/a/datatype/P50291> ;
    reg:hasUnconstrained <http://rdaregistry.info/Elements/u/P60878> ;
    reg:lexicalAlias <http://rdaregistry.info/Elements/a/surname.en> ;
    reg:name "surname"@en ;
    reg:status <http://metadataregistry.org/uri/RegStatus/1001> ;
    a rdf:Property ;
    rdfs:domain <http://rdaregistry.info/Elements/c/C10004> ;
    rdfs:isDefinedBy <http://rdaregistry.info/Elements/a/> ;
    rdfs:label "has surname"@en ;
    skos:definition "Relates a person to a name used as a family name."@en ;
    skos:scopeNote "Names used as family names by Romans of classical times are excluded."@en .

<http://rdaregistry.info/Elements/a/P50292>
    rdakit:instructionNumber "18.5" ;
    rdakit:toolkitDefinition "A name given to a person at birth or at some later point in addition to, or instead of, a surname."@en ;
    rdakit:toolkitLabel "given name"@en ;
    reg:hasSubproperty <http://rdaregistry.info/Elements/a/datatype/P50292> ;
    reg:hasUnconstrained <http://rdaregistry.info/Elements/u/P60879> ;
    reg:lexicalAlias <http://rdaregistry.info/Elements/a/givenName.en> ;
    reg:name "givenName"@en ;
    reg:status <http://metadataregistry.org/uri/RegStatus/1001> ;
    a rdf:Property ;
    rdfs:domain <http://rdaregistry.info/Elements/c/C10004> ;
    rdfs:isDefinedBy <http://rdaregistry.info/Elements/a/> ;
    rdfs:label "has given name"@en ;
    skos:definition "Relates a person to a name given to a person at birth or at some later point in addition to, or instead of, a surname."@en .

<http://rdaregistry.info/Elements/a/P50293>
    rdakit:instructionNumber "18.5" ;
    rdakit:seeAlso <http://rdaregistry.info/Elements/a/P50298> ;
    rdakit:toolkitDefinition "An audio work created by manipulating, recombining, mixing, and reproducing previously recorded sounds."@en ;
    rdakit:toolkitLabel "remix artist of"@en ;
    reg:hasSubproperty <http://rdaregistry.info/Elements/a/datatype/P50293>, <http://rdaregistry.info/Elements/a/object/P50293> ;
    reg:hasUnconstrained <http://rdaregistry.info/Elements/u/P60881> ;
    reg:lexicalAlias <http://rdaregistry.info/Elements/a/remixArtistOf.en> ;
    reg:name "remixArtistOf"@en ;
    reg:status <http://metadataregistry.org/uri/RegStatus/1001> ;
    a rdf:Property ;
    rdfs:domain <http://rdaregistry.info/Elements/c/C10002> ;
    rdfs:isDefinedBy <http://rdaregistry.info/Elements/a/> ;
    rdfs:label "is remix artist of"@en ;
    rdfs:subPropertyOf <http://rdaregistry.info/Elements/a/P50204> ;
    skos:definition "Relates an agent to an audio work created by manipulating, recombining, mixing, and reproducing previously recorded sounds."@en ;
    skos:scopeNote "Remixing activities that do not substantially change the nature and content of the original work, and mixing recorded tracks together to appear as one continuous track are excluded."@en .

<http://rdaregistry.info/Elements/a/P50294>
    rdakit:instructionNumber "18.5" ;
    rdakit:toolkitDefinition "A work that incorporates a contribution of responsibility for most aspects of assigning parts and duties to performers."@en ;
    rdakit:toolkitLabel "casting director of"@en ;
    reg:hasSubproperty <http://rdaregistry.info/Elements/a/datatype/P50294>, <http://rdaregistry.info/Elements/a/object/P50294> ;
    reg:hasUnconstrained <http://rdaregistry.info/Elements/u/P60882> ;
    reg:lexicalAlias <http://rdaregistry.info/Elements/a/castingDirectorOf.en> ;
    reg:name "castingDirectorOf"@en ;
    reg:status <http://metadataregistry.org/uri/RegStatus/1001> ;
    a rdf:Property ;
    rdfs:domain <http://rdaregistry.info/Elements/c/C10002> ;
    rdfs:isDefinedBy <http://rdaregistry.info/Elements/a/> ;
    rdfs:label "is casting director of"@en ;
    rdfs:subPropertyOf <http://rdaregistry.info/Elements/a/P50204> ;
    skos:definition "Relates an agent to a work that incorporates a contribution of responsibility for most aspects of assigning parts and duties to performers."@en .

<http://rdaregistry.info/Elements/a/P50295>
    rdakit:instructionNumber "18.5" ;
    rdakit:toolkitDefinition "A work that involves a responsibility for most of the business aspects of an audio recording."@en ;
    rdakit:toolkitLabel "audio producer of"@en ;
    reg:hasSubproperty <http://rdaregistry.info/Elements/a/datatype/P50295>, <http://rdaregistry.info/Elements/a/object/P50295> ;
    reg:hasUnconstrained <http://rdaregistry.info/Elements/u/P60883> ;
    reg:lexicalAlias <http://rdaregistry.info/Elements/a/audioProducerOf.en> ;
    reg:name "audioProducerOf"@en ;
    reg:status <http://metadataregistry.org/uri/RegStatus/1001> ;
    a rdf:Property ;
    rdfs:domain <http://rdaregistry.info/Elements/c/C10002> ;
    rdfs:isDefinedBy <http://rdaregistry.info/Elements/a/> ;
    rdfs:label "is audio producer of"@en ;
    rdfs:subPropertyOf <http://rdaregistry.info/Elements/a/P50201> ;
    skos:definition "Relates an agent to a work that involves a responsibility for most of the business aspects of an audio recording."@en .

<http://rdaregistry.info/Elements/a/P50296>
    rdakit:instructionNumber "18.5" ;
    rdakit:toolkitDefinition "An expression of a work that incorporates a contribution to the audio content of managing the technical aspects of sound during the processes of recording, mixing, and reproduction."@en ;
    rdakit:toolkitLabel "audio engineer of"@en ;
    reg:hasSubproperty <http://rdaregistry.info/Elements/a/datatype/P50296>, <http://rdaregistry.info/Elements/a/object/P50296>, <http://rdaregistry.info/Elements/a/object/P50297> ;
    reg:hasUnconstrained <http://rdaregistry.info/Elements/u/P60884> ;
    reg:lexicalAlias <http://rdaregistry.info/Elements/a/audioEngineerOf.en> ;
    reg:name "audioEngineerOf"@en ;
    reg:status <http://metadataregistry.org/uri/RegStatus/1001> ;
    a rdf:Property ;
    rdfs:domain <http://rdaregistry.info/Elements/c/C10002> ;
    rdfs:isDefinedBy <http://rdaregistry.info/Elements/a/> ;
    rdfs:label "is audio engineer of"@en ;
    rdfs:subPropertyOf <http://rdaregistry.info/Elements/a/P50161> ;
    skos:definition "Relates an agent to an expression of a work that incorporates a contribution to the audio content of managing the technical aspects of sound during the processes of recording, mixing, and reproduction."@en .

<http://rdaregistry.info/Elements/a/P50297>
    rdakit:instructionNumber "18.5" ;
    rdakit:seeAlso <http://rdaregistry.info/Elements/a/P50293> ;
    rdakit:toolkitDefinition "An expression of a work that incorporates a contribution to the audio content of manipulating, mixing and assembling the multiple tracks of a recording."@en ;
    rdakit:toolkitLabel "mixing engineer of"@en ;
    reg:hasSubproperty <http://rdaregistry.info/Elements/a/datatype/P50297>, <http://rdaregistry.info/Elements/a/object/P50297> ;
    reg:hasUnconstrained <http://rdaregistry.info/Elements/u/P60885> ;
    reg:lexicalAlias <http://rdaregistry.info/Elements/a/mixingEngineerOf.en> ;
    reg:name "mixingEngineerOf"@en ;
    reg:status <http://metadataregistry.org/uri/RegStatus/1001> ;
    a rdf:Property ;
    rdfs:domain <http://rdaregistry.info/Elements/c/C10002> ;
    rdfs:isDefinedBy <http://rdaregistry.info/Elements/a/> ;
    rdfs:label "is mixing engineer of"@en ;
    rdfs:subPropertyOf <http://rdaregistry.info/Elements/a/P50296> ;
    skos:definition "Relates an agent to an expression of a work that incorporates a contribution to the audio content of manipulating, mixing and assembling the multiple tracks of a recording."@en ;
    skos:scopeNote "Remixing activities that substantially change the nature and content of the original work, resulting in a new work, are excluded."@en .

<http://rdaregistry.info/Elements/a/P50298>
    rdakit:instructionNumber "18.5" ;
    rdakit:seeAlso <http://rdaregistry.info/Elements/a/P50297> ;
    rdakit:toolkitDefinition "An expression of a work that incorporates a contribution of mixing recorded tracks together during a live performance or in a recording studio to appear as one continuous track."@en ;
    rdakit:toolkitLabel "DJ of"@en ;
    reg:hasSubproperty <http://rdaregistry.info/Elements/a/datatype/P50298>, <http://rdaregistry.info/Elements/a/object/P50298> ;
    reg:hasUnconstrained <http://rdaregistry.info/Elements/u/P60886> ;
    reg:lexicalAlias <http://rdaregistry.info/Elements/a/DJOf.en> ;
    reg:name "DJOf"@en ;
    reg:status <http://metadataregistry.org/uri/RegStatus/1001> ;
    a rdf:Property ;
    rdfs:domain <http://rdaregistry.info/Elements/c/C10002> ;
    rdfs:isDefinedBy <http://rdaregistry.info/Elements/a/> ;
    rdfs:label "is DJ of"@en ;
    rdfs:subPropertyOf <http://rdaregistry.info/Elements/a/P50161> ;
    skos:definition "Relates an agent to an expression of a work that incorporates a contribution of mixing recorded tracks together during a live performance or in a recording studio to appear as one continuous track."@en ;
    skos:scopeNote "An expression of a work that incorporates a contribution of mixing recorded tracks together during a live performance or in a recording studio to appear as one continuous track."@en .

<http://rdaregistry.info/Elements/a/P50299>
    rdakit:instructionNumber "18.5" ;
    rdakit:toolkitDefinition "An expression of a work that incorporates a contribution of responsibility for the general management and supervision of the process of adding new dialogue or other sounds to complete the sound track."@en ;
    rdakit:toolkitLabel "dubbing director of"@en ;
    reg:hasSubproperty <http://rdaregistry.info/Elements/a/datatype/P50299>, <http://rdaregistry.info/Elements/a/object/P50299> ;
    reg:hasUnconstrained <http://rdaregistry.info/Elements/u/P60887> ;
    reg:lexicalAlias <http://rdaregistry.info/Elements/a/dubbingDirectorOf.en> ;
    reg:name "dubbingDirectorOf"@en ;
    reg:status <http://metadataregistry.org/uri/RegStatus/1001> ;
    a rdf:Property ;
    rdfs:domain <http://rdaregistry.info/Elements/c/C10002> ;
    rdfs:isDefinedBy <http://rdaregistry.info/Elements/a/> ;
    rdfs:label "is dubbing director of"@en ;
    rdfs:subPropertyOf <http://rdaregistry.info/Elements/a/P50161> ;
    skos:definition "Relates an agent to an expression of a work that incorporates a contribution of responsibility for the general management and supervision of the process of adding new dialogue or other sounds to complete the sound track."@en .

<http://rdaregistry.info/Elements/a/P50300>
    rdakit:instructionNumber "18.5" ;
    rdakit:seeAlso <http://rdaregistry.info/Elements/a/P50187> ;
    rdakit:toolkitDefinition "An expression of a musical work that incorporates a contribution of using electronic audio devices and/or computer software to generate sounds."@en ;
    rdakit:toolkitLabel "music programmer of"@en ;
    reg:hasSubproperty <http://rdaregistry.info/Elements/a/datatype/P50300>, <http://rdaregistry.info/Elements/a/object/P50300> ;
    reg:hasUnconstrained <http://rdaregistry.info/Elements/u/P60888> ;
    reg:lexicalAlias <http://rdaregistry.info/Elements/a/musicProgrammerOf.en> ;
    reg:name "musicProgrammerOf"@en ;
    reg:status <http://metadataregistry.org/uri/RegStatus/1001> ;
    a rdf:Property ;
    rdfs:domain <http://rdaregistry.info/Elements/c/C10002> ;
    rdfs:isDefinedBy <http://rdaregistry.info/Elements/a/> ;
    rdfs:label "is music programmer of"@en ;
    rdfs:subPropertyOf <http://rdaregistry.info/Elements/a/P50161> ;
    skos:definition "Relates an agent to an expression of a musical work that incorporates a contribution of using electronic audio devices and/or computer software to generate sounds."@en, "Relates an agent to an expression of a musical work that incorporates a contribution of using electronic audio devices or computer software to generate sounds."@en ;
    skos:scopeNote "The creation of a new musical work is excluded"@en .

<http://rdaregistry.info/Elements/a/P50301>
    rdakit:instructionNumber "29.5" ;
    rdakit:toolkitDefinition "A corporate body that was absorbed by another corporate body."@en ;
    rdakit:toolkitLabel "absorbed corporate body"@en ;
    reg:hasSubproperty <http://rdaregistry.info/Elements/a/datatype/P50301>, <http://rdaregistry.info/Elements/a/object/P50301> ;
    reg:hasUnconstrained <http://rdaregistry.info/Elements/u/P60901> ;
    reg:lexicalAlias <http://rdaregistry.info/Elements/a/absorbedCorporateBody.en> ;
    reg:name "absorbedCorporateBody"@en ;
    reg:status <http://metadataregistry.org/uri/RegStatus/1001> ;
    a rdf:Property ;
    rdfs:domain <http://rdaregistry.info/Elements/c/C10005> ;
    rdfs:isDefinedBy <http://rdaregistry.info/Elements/a/> ;
    rdfs:label "has absorbed corporate body"@en ;
    skos:definition "Relates a corporate body to a corporate body that was absorbed by another corporate body."@en .

<http://rdaregistry.info/Elements/a/P50302>
    rdakit:instructionNumber "29.5" ;
    rdakit:toolkitDefinition "A corporate body that absorbed another corporate body."@en ;
    rdakit:toolkitLabel "absorbing corporate body"@en ;
    reg:hasSubproperty <http://rdaregistry.info/Elements/a/datatype/P50302>, <http://rdaregistry.info/Elements/a/object/P50302> ;
    reg:hasUnconstrained <http://rdaregistry.info/Elements/u/P60902> ;
    reg:lexicalAlias <http://rdaregistry.info/Elements/a/absorbingCorporateBody.en> ;
    reg:name "absorbingCorporateBody"@en ;
    reg:status <http://metadataregistry.org/uri/RegStatus/1001> ;
    a rdf:Property ;
    rdfs:domain <http://rdaregistry.info/Elements/c/C10005> ;
    rdfs:isDefinedBy <http://rdaregistry.info/Elements/a/> ;
    rdfs:label "has absorbing corporate body"@en ;
    skos:definition "Relates a corporate body to a corporate body that absorbed another corporate body."@en .

<http://rdaregistry.info/Elements/a/P50303>
    rdakit:instructionNumber "29.5" ;
    rdakit:toolkitDefinition "A conference that is jointly held with another conference."@en ;
    rdakit:toolkitLabel "jointly held conference"@en ;
    reg:hasSubproperty <http://rdaregistry.info/Elements/a/datatype/P50303>, <http://rdaregistry.info/Elements/a/object/P50303> ;
    reg:hasUnconstrained <http://rdaregistry.info/Elements/u/P60903> ;
    reg:lexicalAlias <http://rdaregistry.info/Elements/a/jointlyHeldConference.en> ;
    reg:name "jointlyHeldConference"@en ;
    reg:status <http://metadataregistry.org/uri/RegStatus/1001> ;
    a rdf:Property ;
    rdfs:domain <http://rdaregistry.info/Elements/c/C10005> ;
    rdfs:isDefinedBy <http://rdaregistry.info/Elements/a/> ;
    rdfs:label "has jointly held conference"@en ;
    skos:definition "Relates a conference to a conference that is jointly held with another conference."@en .

<http://rdaregistry.info/Elements/a/P50304>
    reg:hasSubproperty <http://rdaregistry.info/Elements/a/P50305>, <http://rdaregistry.info/Elements/a/P50306>, <http://rdaregistry.info/Elements/a/P50307>, <http://rdaregistry.info/Elements/a/P50308>, <http://rdaregistry.info/Elements/a/P50309>, <http://rdaregistry.info/Elements/a/P50310>, <http://rdaregistry.info/Elements/a/P50319>, <http://rdaregistry.info/Elements/a/P50328>, <http://rdaregistry.info/Elements/a/P50338>, <http://rdaregistry.info/Elements/a/P50339>, <http://rdaregistry.info/Elements/a/P50340>, <http://rdaregistry.info/Elements/a/P50360>, <http://rdaregistry.info/Elements/a/datatype/P50304>, <http://rdaregistry.info/Elements/a/object/P50304> ;
    reg:lexicalAlias <http://rdaregistry.info/Elements/a/relatedEntityAgent.en> ;
    reg:name "relatedEntityAgent"@en ;
    reg:status <http://metadataregistry.org/uri/RegStatus/1001> ;
    a rdf:Property ;
    rdfs:domain <http://rdaregistry.info/Elements/c/C10002> ;
    rdfs:isDefinedBy <http://rdaregistry.info/Elements/a/> ;
    rdfs:label "has related entity (agent)"@en ;
    rdfs:subPropertyOf <http://rdaregistry.info/Elements/x/P00001> ;
    skos:definition "Relates an agent to an entity associated with an agent being described."@en .

<http://rdaregistry.info/Elements/a/P50305>
    reg:hasSubproperty <http://rdaregistry.info/Elements/a/P50329>, <http://rdaregistry.info/Elements/a/datatype/P50305>, <http://rdaregistry.info/Elements/a/object/P50305> ;
    reg:lexicalAlias <http://rdaregistry.info/Elements/a/relatedWorkAgent.en> ;
    reg:name "relatedWorkAgent"@en ;
    reg:status <http://metadataregistry.org/uri/RegStatus/1001> ;
    a rdf:Property ;
    rdfs:domain <http://rdaregistry.info/Elements/c/C10002> ;
    rdfs:isDefinedBy <http://rdaregistry.info/Elements/a/> ;
    rdfs:label "has related work (agent)"@en ;
    rdfs:subPropertyOf <http://rdaregistry.info/Elements/a/P50304>, <http://rdaregistry.info/Elements/x/P00006> ;
    skos:definition "Relates an agent to a work associated with an agent being described."@en .

<http://rdaregistry.info/Elements/a/P50306>
    reg:hasSubproperty <http://rdaregistry.info/Elements/a/P50330>, <http://rdaregistry.info/Elements/a/datatype/P50306>, <http://rdaregistry.info/Elements/a/object/P50306> ;
    reg:lexicalAlias <http://rdaregistry.info/Elements/a/relatedExpressionAgent.en> ;
    reg:name "relatedExpressionAgent"@en ;
    reg:status <http://metadataregistry.org/uri/RegStatus/1001> ;
    a rdf:Property ;
    rdfs:domain <http://rdaregistry.info/Elements/c/C10002> ;
    rdfs:isDefinedBy <http://rdaregistry.info/Elements/a/> ;
    rdfs:label "has related expression (agent)"@en ;
    rdfs:subPropertyOf <http://rdaregistry.info/Elements/a/P50304>, <http://rdaregistry.info/Elements/x/P00006> ;
    skos:definition "Relates an agent to an expression associated with an agent being described."@en .

<http://rdaregistry.info/Elements/a/P50307>
    reg:hasSubproperty <http://rdaregistry.info/Elements/a/P50331>, <http://rdaregistry.info/Elements/a/datatype/P50307>, <http://rdaregistry.info/Elements/a/object/P50307> ;
    reg:lexicalAlias <http://rdaregistry.info/Elements/a/relatedManifestationAgent.en> ;
    reg:name "relatedManifestationAgent"@en ;
    reg:status <http://metadataregistry.org/uri/RegStatus/1001> ;
    a rdf:Property ;
    rdfs:domain <http://rdaregistry.info/Elements/c/C10002> ;
    rdfs:isDefinedBy <http://rdaregistry.info/Elements/a/> ;
    rdfs:label "has related manifestation (agent)"@en ;
    rdfs:subPropertyOf <http://rdaregistry.info/Elements/a/P50304>, <http://rdaregistry.info/Elements/x/P00006> ;
    skos:definition "Relates an agent to a manifestation associated with an agent being described."@en .

<http://rdaregistry.info/Elements/a/P50308>
    reg:hasSubproperty <http://rdaregistry.info/Elements/a/P50332>, <http://rdaregistry.info/Elements/a/datatype/P50308>, <http://rdaregistry.info/Elements/a/object/P50308> ;
    reg:lexicalAlias <http://rdaregistry.info/Elements/a/relatedItemAgent.en> ;
    reg:name "relatedItemAgent"@en ;
    reg:status <http://metadataregistry.org/uri/RegStatus/1001> ;
    a rdf:Property ;
    rdfs:domain <http://rdaregistry.info/Elements/c/C10002> ;
    rdfs:isDefinedBy <http://rdaregistry.info/Elements/a/> ;
    rdfs:label "has related item (agent)"@en ;
    rdfs:subPropertyOf <http://rdaregistry.info/Elements/a/P50304>, <http://rdaregistry.info/Elements/x/P00006> ;
    skos:definition "Relates an agent to an item associated with an agent being described."@en .

<http://rdaregistry.info/Elements/a/P50309>
    reg:hasSubproperty <http://rdaregistry.info/Elements/a/P50220>, <http://rdaregistry.info/Elements/a/P50333>, <http://rdaregistry.info/Elements/a/P50337>, <http://rdaregistry.info/Elements/a/datatype/P50309>, <http://rdaregistry.info/Elements/a/object/P50309> ;
    reg:lexicalAlias <http://rdaregistry.info/Elements/a/relatedAgentAgent.en> ;
    reg:name "relatedAgentAgent"@en ;
    reg:status <http://metadataregistry.org/uri/RegStatus/1001> ;
    a rdf:Property ;
    rdfs:domain <http://rdaregistry.info/Elements/c/C10002> ;
    rdfs:isDefinedBy <http://rdaregistry.info/Elements/a/> ;
    rdfs:label "has related agent (agent)"@en ;
    rdfs:subPropertyOf <http://rdaregistry.info/Elements/a/P50304>, <http://rdaregistry.info/Elements/x/P00006> ;
    skos:definition "Relates an agent to an agent associated with an agent being described."@en .

<http://rdaregistry.info/Elements/a/P50310>
    reg:hasSubproperty <http://rdaregistry.info/Elements/a/P50311>, <http://rdaregistry.info/Elements/a/P50312>, <http://rdaregistry.info/Elements/a/P50313>, <http://rdaregistry.info/Elements/a/P50314>, <http://rdaregistry.info/Elements/a/P50315>, <http://rdaregistry.info/Elements/a/P50346>, <http://rdaregistry.info/Elements/a/P50347>, <http://rdaregistry.info/Elements/a/P50348>, <http://rdaregistry.info/Elements/a/datatype/P50310>, <http://rdaregistry.info/Elements/a/object/P50310> ;
    reg:lexicalAlias <http://rdaregistry.info/Elements/a/relatedEntityPerson.en> ;
    reg:name "relatedEntityPerson"@en ;
    reg:status <http://metadataregistry.org/uri/RegStatus/1001> ;
    a rdf:Property ;
    rdfs:domain <http://rdaregistry.info/Elements/c/C10004> ;
    rdfs:isDefinedBy <http://rdaregistry.info/Elements/a/> ;
    rdfs:label "has related entity (person)"@en ;
    rdfs:subPropertyOf <http://rdaregistry.info/Elements/a/P50304> ;
    skos:definition "Relates a person to an entity associated with a person being described."@en .

<http://rdaregistry.info/Elements/a/P50311>
    reg:hasSubproperty <http://rdaregistry.info/Elements/a/datatype/P50311>, <http://rdaregistry.info/Elements/a/object/P50311> ;
    reg:lexicalAlias <http://rdaregistry.info/Elements/a/relatedWorkPerson.en> ;
    reg:name "relatedWorkPerson"@en ;
    reg:status <http://metadataregistry.org/uri/RegStatus/1001> ;
    a rdf:Property ;
    rdfs:domain <http://rdaregistry.info/Elements/c/C10004> ;
    rdfs:isDefinedBy <http://rdaregistry.info/Elements/a/> ;
    rdfs:label "has related work (person)"@en ;
    rdfs:subPropertyOf <http://rdaregistry.info/Elements/a/P50305>, <http://rdaregistry.info/Elements/a/P50310> ;
    skos:definition "Relates a person to a work associated with a person being described."@en .

<http://rdaregistry.info/Elements/a/P50312>
    reg:hasSubproperty <http://rdaregistry.info/Elements/a/datatype/P50312>, <http://rdaregistry.info/Elements/a/object/P50312> ;
    reg:lexicalAlias <http://rdaregistry.info/Elements/a/relatedExpressionPerson.en> ;
    reg:name "relatedExpressionPerson"@en ;
    reg:status <http://metadataregistry.org/uri/RegStatus/1001> ;
    a rdf:Property ;
    rdfs:domain <http://rdaregistry.info/Elements/c/C10004> ;
    rdfs:isDefinedBy <http://rdaregistry.info/Elements/a/> ;
    rdfs:label "has related expression (person)"@en ;
    rdfs:subPropertyOf <http://rdaregistry.info/Elements/a/P50306>, <http://rdaregistry.info/Elements/a/P50310> ;
    skos:definition "Relates a person to an expression associated with a person being described."@en .

<http://rdaregistry.info/Elements/a/P50313>
    reg:hasSubproperty <http://rdaregistry.info/Elements/a/datatype/P50313>, <http://rdaregistry.info/Elements/a/object/P50313> ;
    reg:lexicalAlias <http://rdaregistry.info/Elements/a/relatedManifestationPerson.en> ;
    reg:name "relatedManifestationPerson"@en ;
    reg:status <http://metadataregistry.org/uri/RegStatus/1001> ;
    a rdf:Property ;
    rdfs:domain <http://rdaregistry.info/Elements/c/C10004> ;
    rdfs:isDefinedBy <http://rdaregistry.info/Elements/a/> ;
    rdfs:label "has related manifestation (person)"@en ;
    rdfs:subPropertyOf <http://rdaregistry.info/Elements/a/P50307>, <http://rdaregistry.info/Elements/a/P50310> ;
    skos:definition "Relates a person to a manifestation associated with a person being described."@en .

<http://rdaregistry.info/Elements/a/P50314>
    reg:hasSubproperty <http://rdaregistry.info/Elements/a/datatype/P50314>, <http://rdaregistry.info/Elements/a/object/P50314> ;
    reg:lexicalAlias <http://rdaregistry.info/Elements/a/relatedItemPerson.en> ;
    reg:name "relatedItemPerson"@en ;
    reg:status <http://metadataregistry.org/uri/RegStatus/1001> ;
    a rdf:Property ;
    rdfs:domain <http://rdaregistry.info/Elements/c/C10004> ;
    rdfs:isDefinedBy <http://rdaregistry.info/Elements/a/> ;
    rdfs:label "has related item (person)"@en ;
    rdfs:subPropertyOf <http://rdaregistry.info/Elements/a/P50308>, <http://rdaregistry.info/Elements/a/P50310> ;
    skos:definition "Relates a person to an item associated with a person being described."@en .

<http://rdaregistry.info/Elements/a/P50315>
    reg:hasSubproperty <http://rdaregistry.info/Elements/a/P50316>, <http://rdaregistry.info/Elements/a/P50345>, <http://rdaregistry.info/Elements/a/datatype/P50315>, <http://rdaregistry.info/Elements/a/object/P50315> ;
    reg:lexicalAlias <http://rdaregistry.info/Elements/a/relatedAgentPerson.en> ;
    reg:name "relatedAgentPerson"@en ;
    reg:status <http://metadataregistry.org/uri/RegStatus/1001> ;
    a rdf:Property ;
    rdfs:domain <http://rdaregistry.info/Elements/c/C10004> ;
    rdfs:isDefinedBy <http://rdaregistry.info/Elements/a/> ;
    rdfs:label "has related agent (person)"@en ;
    rdfs:subPropertyOf <http://rdaregistry.info/Elements/a/P50309>, <http://rdaregistry.info/Elements/a/P50310> ;
    skos:definition "Relates a person to an agent associated with a person being described."@en .

<http://rdaregistry.info/Elements/a/P50316>
    reg:hasSubproperty <http://rdaregistry.info/Elements/a/datatype/P50316>, <http://rdaregistry.info/Elements/a/object/P50316> ;
    reg:lexicalAlias <http://rdaregistry.info/Elements/a/relatedPersonPerson.en> ;
    reg:name "relatedPersonPerson"@en ;
    reg:status <http://metadataregistry.org/uri/RegStatus/1001> ;
    a rdf:Property ;
    rdfs:domain <http://rdaregistry.info/Elements/c/C10004> ;
    rdfs:isDefinedBy <http://rdaregistry.info/Elements/a/> ;
    rdfs:label "has related person (person)"@en ;
    rdfs:subPropertyOf <http://rdaregistry.info/Elements/a/P50220>, <http://rdaregistry.info/Elements/a/P50315> ;
    skos:definition "Relates a person to a person who is associated with a person being described."@en .

<http://rdaregistry.info/Elements/a/P50317>
    reg:hasSubproperty <http://rdaregistry.info/Elements/a/datatype/P50317>, <http://rdaregistry.info/Elements/a/object/P50317> ;
    reg:lexicalAlias <http://rdaregistry.info/Elements/a/relatedFamilyPerson.en> ;
    reg:name "relatedFamilyPerson"@en ;
    reg:status <http://metadataregistry.org/uri/RegStatus/1001> ;
    a rdf:Property ;
    rdfs:domain <http://rdaregistry.info/Elements/c/C10004> ;
    rdfs:isDefinedBy <http://rdaregistry.info/Elements/a/> ;
    rdfs:label "has related family (person)"@en ;
    rdfs:subPropertyOf <http://rdaregistry.info/Elements/a/P50219>, <http://rdaregistry.info/Elements/a/P50345> ;
    skos:definition "Relates a person to a family associated with a person being described."@en .

<http://rdaregistry.info/Elements/a/P50318>
    reg:hasSubproperty <http://rdaregistry.info/Elements/a/datatype/P50318>, <http://rdaregistry.info/Elements/a/object/P50318> ;
    reg:lexicalAlias <http://rdaregistry.info/Elements/a/relatedCorporateBodyPerson.en> ;
    reg:name "relatedCorporateBodyPerson"@en ;
    reg:status <http://metadataregistry.org/uri/RegStatus/1001> ;
    a rdf:Property ;
    rdfs:domain <http://rdaregistry.info/Elements/c/C10004> ;
    rdfs:isDefinedBy <http://rdaregistry.info/Elements/a/> ;
    rdfs:label "has related corporate body (person)"@en ;
    rdfs:subPropertyOf <http://rdaregistry.info/Elements/a/P50218>, <http://rdaregistry.info/Elements/a/P50345> ;
    skos:definition "Relates a person to a corporate body associated with a person being described."@en .

<http://rdaregistry.info/Elements/a/P50319>
    reg:hasSubproperty <http://rdaregistry.info/Elements/a/P50320>, <http://rdaregistry.info/Elements/a/P50321>, <http://rdaregistry.info/Elements/a/P50322>, <http://rdaregistry.info/Elements/a/P50323>, <http://rdaregistry.info/Elements/a/P50324>, <http://rdaregistry.info/Elements/a/P50354>, <http://rdaregistry.info/Elements/a/P50355>, <http://rdaregistry.info/Elements/a/P50356>, <http://rdaregistry.info/Elements/a/datatype/P50319>, <http://rdaregistry.info/Elements/a/object/P50319> ;
    reg:lexicalAlias <http://rdaregistry.info/Elements/a/relatedEntityFamily.en> ;
    reg:name "relatedEntityFamily"@en ;
    reg:status <http://metadataregistry.org/uri/RegStatus/1001> ;
    a rdf:Property ;
    rdfs:domain <http://rdaregistry.info/Elements/c/C10008> ;
    rdfs:isDefinedBy <http://rdaregistry.info/Elements/a/> ;
    rdfs:label "has related entity (family)"@en ;
    rdfs:subPropertyOf <http://rdaregistry.info/Elements/a/P50360> ;
    skos:definition "Relates a family to an entity associated with a family being described."@en .

<http://rdaregistry.info/Elements/a/P50320>
    reg:hasSubproperty <http://rdaregistry.info/Elements/a/datatype/P50320>, <http://rdaregistry.info/Elements/a/object/P50320> ;
    reg:lexicalAlias <http://rdaregistry.info/Elements/a/relatedWorkFamily.en> ;
    reg:name "relatedWorkFamily"@en ;
    reg:status <http://metadataregistry.org/uri/RegStatus/1001> ;
    a rdf:Property ;
    rdfs:domain <http://rdaregistry.info/Elements/c/C10008> ;
    rdfs:isDefinedBy <http://rdaregistry.info/Elements/a/> ;
    rdfs:label "has related work (family)"@en ;
    rdfs:subPropertyOf <http://rdaregistry.info/Elements/a/P50319>, <http://rdaregistry.info/Elements/a/P50357> ;
    skos:definition "Relates a family to a work associated with a family being described."@en .

<http://rdaregistry.info/Elements/a/P50321>
    reg:hasSubproperty <http://rdaregistry.info/Elements/a/datatype/P50321>, <http://rdaregistry.info/Elements/a/object/P50321> ;
    reg:lexicalAlias <http://rdaregistry.info/Elements/a/relatedExpressionFamily.en> ;
    reg:name "relatedExpressionFamily"@en ;
    reg:status <http://metadataregistry.org/uri/RegStatus/1001> ;
    a rdf:Property ;
    rdfs:domain <http://rdaregistry.info/Elements/c/C10008> ;
    rdfs:isDefinedBy <http://rdaregistry.info/Elements/a/> ;
    rdfs:label "has related expression (family)"@en ;
    rdfs:subPropertyOf <http://rdaregistry.info/Elements/a/P50319>, <http://rdaregistry.info/Elements/a/P50361> ;
    skos:definition "Relates a family to an expression associated with a family being described."@en .

<http://rdaregistry.info/Elements/a/P50322>
    reg:hasSubproperty <http://rdaregistry.info/Elements/a/datatype/P50322>, <http://rdaregistry.info/Elements/a/object/P50322> ;
    reg:lexicalAlias <http://rdaregistry.info/Elements/a/relatedManifestationFamily.en> ;
    reg:name "relatedManifestationFamily"@en ;
    reg:status <http://metadataregistry.org/uri/RegStatus/1001> ;
    a rdf:Property ;
    rdfs:domain <http://rdaregistry.info/Elements/c/C10008> ;
    rdfs:isDefinedBy <http://rdaregistry.info/Elements/a/> ;
    rdfs:label "has related manifestation (family)"@en ;
    rdfs:subPropertyOf <http://rdaregistry.info/Elements/a/P50319>, <http://rdaregistry.info/Elements/a/P50364> ;
    skos:definition "Relates a family to a manifestation associated with a family being described."@en .

<http://rdaregistry.info/Elements/a/P50323>
    reg:hasSubproperty <http://rdaregistry.info/Elements/a/datatype/P50323>, <http://rdaregistry.info/Elements/a/object/P50323> ;
    reg:lexicalAlias <http://rdaregistry.info/Elements/a/relatedItemFamily.en> ;
    reg:name "relatedItemFamily"@en ;
    reg:status <http://metadataregistry.org/uri/RegStatus/1001> ;
    a rdf:Property ;
    rdfs:domain <http://rdaregistry.info/Elements/c/C10008> ;
    rdfs:isDefinedBy <http://rdaregistry.info/Elements/a/> ;
    rdfs:label "has related item (family)"@en ;
    rdfs:subPropertyOf <http://rdaregistry.info/Elements/a/P50319>, <http://rdaregistry.info/Elements/a/P50363> ;
    skos:definition "Relates a family to an item associated with a family being described."@en .

<http://rdaregistry.info/Elements/a/P50324>
    reg:hasSubproperty <http://rdaregistry.info/Elements/a/P50325>, <http://rdaregistry.info/Elements/a/P50353>, <http://rdaregistry.info/Elements/a/datatype/P50324>, <http://rdaregistry.info/Elements/a/object/P50324> ;
    reg:lexicalAlias <http://rdaregistry.info/Elements/a/relatedAgentFamily.en> ;
    reg:name "relatedAgentFamily"@en ;
    reg:status <http://metadataregistry.org/uri/RegStatus/1001> ;
    a rdf:Property ;
    rdfs:domain <http://rdaregistry.info/Elements/c/C10008> ;
    rdfs:isDefinedBy <http://rdaregistry.info/Elements/a/> ;
    rdfs:label "has related agent (family)"@en ;
    rdfs:subPropertyOf <http://rdaregistry.info/Elements/a/P50319>, <http://rdaregistry.info/Elements/a/P50358> ;
    skos:definition "Relates a family to an agent associated with a family being described."@en .

<http://rdaregistry.info/Elements/a/P50325>
    reg:hasSubproperty <http://rdaregistry.info/Elements/a/datatype/P50325>, <http://rdaregistry.info/Elements/a/object/P50325> ;
    reg:lexicalAlias <http://rdaregistry.info/Elements/a/relatedPersonFamily.en> ;
    reg:name "relatedPersonFamily"@en ;
    reg:status <http://metadataregistry.org/uri/RegStatus/1001> ;
    a rdf:Property ;
    rdfs:domain <http://rdaregistry.info/Elements/c/C10008> ;
    rdfs:isDefinedBy <http://rdaregistry.info/Elements/a/> ;
    rdfs:label "has related person (family)"@en ;
    rdfs:subPropertyOf <http://rdaregistry.info/Elements/a/P50324>, <http://rdaregistry.info/Elements/a/P50365> ;
    skos:definition "Relates a family to a person who is associated with a family being described."@en .

<http://rdaregistry.info/Elements/a/P50326>
    reg:hasSubproperty <http://rdaregistry.info/Elements/a/datatype/P50326>, <http://rdaregistry.info/Elements/a/object/P50326> ;
    reg:lexicalAlias <http://rdaregistry.info/Elements/a/relatedFamilyFamily.en> ;
    reg:name "relatedFamilyFamily"@en ;
    reg:status <http://metadataregistry.org/uri/RegStatus/1001> ;
    a rdf:Property ;
    rdfs:domain <http://rdaregistry.info/Elements/c/C10008> ;
    rdfs:isDefinedBy <http://rdaregistry.info/Elements/a/> ;
    rdfs:label "has related family (family)"@en ;
    rdfs:subPropertyOf <http://rdaregistry.info/Elements/a/P50353>, <http://rdaregistry.info/Elements/a/P50362> ;
    skos:definition "Relates a family to a family associated with a family being described."@en .

<http://rdaregistry.info/Elements/a/P50327>
    reg:hasSubproperty <http://rdaregistry.info/Elements/a/datatype/P50327>, <http://rdaregistry.info/Elements/a/object/P50327> ;
    reg:lexicalAlias <http://rdaregistry.info/Elements/a/relatedCorporateBodyFamily.en> ;
    reg:name "relatedCorporateBodyFamily"@en ;
    reg:status <http://metadataregistry.org/uri/RegStatus/1001> ;
    a rdf:Property ;
    rdfs:domain <http://rdaregistry.info/Elements/c/C10008> ;
    rdfs:isDefinedBy <http://rdaregistry.info/Elements/a/> ;
    rdfs:label "has related corporate body (family)"@en ;
    rdfs:subPropertyOf <http://rdaregistry.info/Elements/a/P50353>, <http://rdaregistry.info/Elements/a/P50359> ;
    skos:definition "Relates a family to a corporate body associated with a family being described."@en .

<http://rdaregistry.info/Elements/a/P50328>
    reg:hasSubproperty <http://rdaregistry.info/Elements/a/P50349>, <http://rdaregistry.info/Elements/a/P50350>, <http://rdaregistry.info/Elements/a/P50351>, <http://rdaregistry.info/Elements/a/P50352>, <http://rdaregistry.info/Elements/a/datatype/P50328>, <http://rdaregistry.info/Elements/a/object/P50328> ;
    reg:lexicalAlias <http://rdaregistry.info/Elements/a/relatedEntityCorporateBody.en> ;
    reg:name "relatedEntityCorporateBody"@en ;
    reg:status <http://metadataregistry.org/uri/RegStatus/1001> ;
    a rdf:Property ;
    rdfs:domain <http://rdaregistry.info/Elements/c/C10005> ;
    rdfs:isDefinedBy <http://rdaregistry.info/Elements/a/> ;
    rdfs:label "has related entity (corporate body)"@en ;
    rdfs:subPropertyOf <http://rdaregistry.info/Elements/a/P50360> ;
    skos:definition "Relates a corporate body to an entity associated with a corporate body being described."@en .

<http://rdaregistry.info/Elements/a/P50329>
    reg:hasSubproperty <http://rdaregistry.info/Elements/a/datatype/P50329>, <http://rdaregistry.info/Elements/a/object/P50329> ;
    reg:lexicalAlias <http://rdaregistry.info/Elements/a/relatedWorkCorporateBody.en> ;
    reg:name "relatedWorkCorporateBody"@en ;
    reg:status <http://metadataregistry.org/uri/RegStatus/1001> ;
    a rdf:Property ;
    rdfs:domain <http://rdaregistry.info/Elements/c/C10005> ;
    rdfs:isDefinedBy <http://rdaregistry.info/Elements/a/> ;
    rdfs:label "has related work (corporate body)"@en ;
    rdfs:subPropertyOf <http://rdaregistry.info/Elements/a/P50305>, <http://rdaregistry.info/Elements/a/P50357> ;
    skos:definition "Relates a corporate body to a work associated with a corporate body being described."@en .

<http://rdaregistry.info/Elements/a/P50330>
    reg:hasSubproperty <http://rdaregistry.info/Elements/a/datatype/P50330>, <http://rdaregistry.info/Elements/a/object/P50330> ;
    reg:lexicalAlias <http://rdaregistry.info/Elements/a/relatedExpressionCorporateBody.en> ;
    reg:name "relatedExpressionCorporateBody"@en ;
    reg:status <http://metadataregistry.org/uri/RegStatus/1001> ;
    a rdf:Property ;
    rdfs:domain <http://rdaregistry.info/Elements/c/C10005> ;
    rdfs:isDefinedBy <http://rdaregistry.info/Elements/a/> ;
    rdfs:label "has related expression (corporate body)"@en ;
    rdfs:subPropertyOf <http://rdaregistry.info/Elements/a/P50306>, <http://rdaregistry.info/Elements/a/P50361> ;
    skos:definition "Relates a corporate body to an expression associated with a corporate body being described."@en .

<http://rdaregistry.info/Elements/a/P50331>
    reg:hasSubproperty <http://rdaregistry.info/Elements/a/datatype/P50331>, <http://rdaregistry.info/Elements/a/object/P50331> ;
    reg:lexicalAlias <http://rdaregistry.info/Elements/a/relatedManifestationCorporateBody.en> ;
    reg:name "relatedManifestationCorporateBody"@en ;
    reg:status <http://metadataregistry.org/uri/RegStatus/1001> ;
    a rdf:Property ;
    rdfs:domain <http://rdaregistry.info/Elements/c/C10005> ;
    rdfs:isDefinedBy <http://rdaregistry.info/Elements/a/> ;
    rdfs:label "has related manifestation (corporate body)"@en ;
    rdfs:subPropertyOf <http://rdaregistry.info/Elements/a/P50307>, <http://rdaregistry.info/Elements/a/P50364> ;
    skos:definition "Relates a corporate body to a manifestation associated with a corporate body being described."@en .

<http://rdaregistry.info/Elements/a/P50332>
    reg:hasSubproperty <http://rdaregistry.info/Elements/a/datatype/P50332>, <http://rdaregistry.info/Elements/a/object/P50332> ;
    reg:lexicalAlias <http://rdaregistry.info/Elements/a/relatedItemCorporateBody.en> ;
    reg:name "relatedItemCorporateBody"@en ;
    reg:status <http://metadataregistry.org/uri/RegStatus/1001> ;
    a rdf:Property ;
    rdfs:domain <http://rdaregistry.info/Elements/c/C10005> ;
    rdfs:isDefinedBy <http://rdaregistry.info/Elements/a/> ;
    rdfs:label "has related item (corporate body)"@en ;
    rdfs:subPropertyOf <http://rdaregistry.info/Elements/a/P50308>, <http://rdaregistry.info/Elements/a/P50363> ;
    skos:definition "Relates a corporate body to an item associated with a corporate body described."@en .

<http://rdaregistry.info/Elements/a/P50333>
    reg:hasSubproperty <http://rdaregistry.info/Elements/a/P50334>, <http://rdaregistry.info/Elements/a/P50335>, <http://rdaregistry.info/Elements/a/P50336>, <http://rdaregistry.info/Elements/a/datatype/P50333>, <http://rdaregistry.info/Elements/a/object/P50333> ;
    reg:lexicalAlias <http://rdaregistry.info/Elements/a/relatedAgentCorporateBody.en> ;
    reg:name "relatedAgentCorporateBody"@en ;
    reg:status <http://metadataregistry.org/uri/RegStatus/1001> ;
    a rdf:Property ;
    rdfs:domain <http://rdaregistry.info/Elements/c/C10005> ;
    rdfs:isDefinedBy <http://rdaregistry.info/Elements/a/> ;
    rdfs:label "has related agent (corporate body)"@en ;
    rdfs:subPropertyOf <http://rdaregistry.info/Elements/a/P50309>, <http://rdaregistry.info/Elements/a/P50358> ;
    skos:definition "Relates a corporate body to an agent associated with a corporate body being described."@en .

<http://rdaregistry.info/Elements/a/P50334>
    reg:hasSubproperty <http://rdaregistry.info/Elements/a/datatype/P50334>, <http://rdaregistry.info/Elements/a/object/P50334> ;
    reg:lexicalAlias <http://rdaregistry.info/Elements/a/relatedPersonCorporateBody.en> ;
    reg:name "relatedPersonCorporateBody"@en ;
    reg:status <http://metadataregistry.org/uri/RegStatus/1001> ;
    a rdf:Property ;
    rdfs:domain <http://rdaregistry.info/Elements/c/C10005> ;
    rdfs:isDefinedBy <http://rdaregistry.info/Elements/a/> ;
    rdfs:label "has related person (corporate body)"@en ;
    rdfs:subPropertyOf <http://rdaregistry.info/Elements/a/P50333>, <http://rdaregistry.info/Elements/a/P50365> ;
    skos:definition "Relates a corporate body to a person who is associated with a corporate body being described."@en .

<http://rdaregistry.info/Elements/a/P50335>
    reg:hasSubproperty <http://rdaregistry.info/Elements/a/datatype/P50335>, <http://rdaregistry.info/Elements/a/object/P50335> ;
    reg:lexicalAlias <http://rdaregistry.info/Elements/a/relatedFamilyCorporateBody.en> ;
    reg:name "relatedFamilyCorporateBody"@en ;
    reg:status <http://metadataregistry.org/uri/RegStatus/1001> ;
    a rdf:Property ;
    rdfs:domain <http://rdaregistry.info/Elements/c/C10005> ;
    rdfs:isDefinedBy <http://rdaregistry.info/Elements/a/> ;
    rdfs:label "has related family (corporate body)"@en ;
    rdfs:subPropertyOf <http://rdaregistry.info/Elements/a/P50333>, <http://rdaregistry.info/Elements/a/P50362> ;
    skos:definition "Relates a corporate body to a family associated with a corporate body being described."@en .

<http://rdaregistry.info/Elements/a/P50336>
    reg:hasSubproperty <http://rdaregistry.info/Elements/a/datatype/P50336>, <http://rdaregistry.info/Elements/a/object/P50336> ;
    reg:lexicalAlias <http://rdaregistry.info/Elements/a/relatedCorporateBodyCorporateBody.en> ;
    reg:name "relatedCorporateBodyCorporateBody"@en ;
    reg:status <http://metadataregistry.org/uri/RegStatus/1001> ;
    a rdf:Property ;
    rdfs:domain <http://rdaregistry.info/Elements/c/C10005> ;
    rdfs:isDefinedBy <http://rdaregistry.info/Elements/a/> ;
    rdfs:label "has related corporate body (corporate body)"@en ;
    rdfs:subPropertyOf <http://rdaregistry.info/Elements/a/P50333>, <http://rdaregistry.info/Elements/a/P50359> ;
    skos:definition "Relates a corporate body to a corporate body associated with a corporate body being described."@en .

<http://rdaregistry.info/Elements/a/P50337>
    reg:hasSubproperty <http://rdaregistry.info/Elements/a/P50218>, <http://rdaregistry.info/Elements/a/P50219>, <http://rdaregistry.info/Elements/a/datatype/P50337>, <http://rdaregistry.info/Elements/a/object/P50337> ;
    reg:lexicalAlias <http://rdaregistry.info/Elements/a/relatedCollectiveAgentAgent.en> ;
    reg:name "relatedCollectiveAgentAgent"@en ;
    reg:status <http://metadataregistry.org/uri/RegStatus/1001> ;
    a rdf:Property ;
    rdfs:domain <http://rdaregistry.info/Elements/c/C10002> ;
    rdfs:isDefinedBy <http://rdaregistry.info/Elements/a/> ;
    rdfs:label "has related collective agent (agent)"@en ;
    rdfs:subPropertyOf <http://rdaregistry.info/Elements/a/P50309>, <http://rdaregistry.info/Elements/x/P00006> ;
    skos:definition "Relates an agent to"@en .

<http://rdaregistry.info/Elements/a/P50338>
    reg:hasSubproperty <http://rdaregistry.info/Elements/a/datatype/P50338>, <http://rdaregistry.info/Elements/a/object/P50338> ;
    reg:lexicalAlias <http://rdaregistry.info/Elements/a/relatedPlaceAgent.en> ;
    reg:name "relatedPlaceAgent"@en ;
    reg:status <http://metadataregistry.org/uri/RegStatus/1001> ;
    a rdf:Property ;
    rdfs:domain <http://rdaregistry.info/Elements/c/C10002> ;
    rdfs:isDefinedBy <http://rdaregistry.info/Elements/a/> ;
    rdfs:label "has related place (agent)"@en ;
    rdfs:subPropertyOf <http://rdaregistry.info/Elements/a/P50304>, <http://rdaregistry.info/Elements/x/P00006> ;
    skos:definition "Relates an agent to"@en .

<http://rdaregistry.info/Elements/a/P50339>
    reg:hasSubproperty <http://rdaregistry.info/Elements/a/datatype/P50339>, <http://rdaregistry.info/Elements/a/object/P50339> ;
    reg:lexicalAlias <http://rdaregistry.info/Elements/a/relatedTimespanAgent.en> ;
    reg:name "relatedTimespanAgent"@en ;
    reg:status <http://metadataregistry.org/uri/RegStatus/1001> ;
    a rdf:Property ;
    rdfs:domain <http://rdaregistry.info/Elements/c/C10002> ;
    rdfs:isDefinedBy <http://rdaregistry.info/Elements/a/> ;
    rdfs:label "has related time-span (agent)"@en ;
    rdfs:subPropertyOf <http://rdaregistry.info/Elements/a/P50304>, <http://rdaregistry.info/Elements/x/P00006> ;
    skos:definition "Relates an agent to"@en .

<http://rdaregistry.info/Elements/a/P50340>
    reg:hasSubproperty <http://rdaregistry.info/Elements/a/datatype/P50340>, <http://rdaregistry.info/Elements/a/object/P50340> ;
    reg:lexicalAlias <http://rdaregistry.info/Elements/a/relatedNomenAgent.en> ;
    reg:name "relatedNomenAgent"@en ;
    reg:status <http://metadataregistry.org/uri/RegStatus/1001> ;
    a rdf:Property ;
    rdfs:domain <http://rdaregistry.info/Elements/c/C10002> ;
    rdfs:isDefinedBy <http://rdaregistry.info/Elements/a/> ;
    rdfs:label "has related nomen (agent)"@en ;
    rdfs:subPropertyOf <http://rdaregistry.info/Elements/a/P50304>, <http://rdaregistry.info/Elements/x/P00006> ;
    skos:definition "Relates an agent to"@en .

<http://rdaregistry.info/Elements/a/P50341>
    reg:hasSubproperty <http://rdaregistry.info/Elements/a/P50359>, <http://rdaregistry.info/Elements/a/P50362>, <http://rdaregistry.info/Elements/a/datatype/P50341>, <http://rdaregistry.info/Elements/a/object/P50341> ;
    reg:lexicalAlias <http://rdaregistry.info/Elements/a/relatedCollectiveAgentCollectiveAgent.en> ;
    reg:name "relatedCollectiveAgentCollectiveAgent"@en ;
    reg:status <http://metadataregistry.org/uri/RegStatus/1001> ;
    a rdf:Property ;
    rdfs:domain <http://rdaregistry.info/Elements/c/C10011> ;
    rdfs:isDefinedBy <http://rdaregistry.info/Elements/a/> ;
    rdfs:label "has related collective agent (collective agent)"@en ;
    rdfs:subPropertyOf <http://rdaregistry.info/Elements/a/P50337>, <http://rdaregistry.info/Elements/a/P50358> ;
    skos:definition "Relates a collective agent to"@en .

<http://rdaregistry.info/Elements/a/P50342>
    reg:hasSubproperty <http://rdaregistry.info/Elements/a/datatype/P50342>, <http://rdaregistry.info/Elements/a/object/P50342> ;
    reg:lexicalAlias <http://rdaregistry.info/Elements/a/relatedPlaceCollectiveAgent.en> ;
    reg:name "relatedPlaceCollectiveAgent"@en ;
    reg:status <http://metadataregistry.org/uri/RegStatus/1001> ;
    a rdf:Property ;
    rdfs:domain <http://rdaregistry.info/Elements/c/C10011> ;
    rdfs:isDefinedBy <http://rdaregistry.info/Elements/a/> ;
    rdfs:label "has related place (collective agent)"@en ;
    rdfs:subPropertyOf <http://rdaregistry.info/Elements/a/P50338>, <http://rdaregistry.info/Elements/a/P50360> ;
    skos:definition "Relates a collective agent to"@en .

<http://rdaregistry.info/Elements/a/P50343>
    reg:hasSubproperty <http://rdaregistry.info/Elements/a/datatype/P50343>, <http://rdaregistry.info/Elements/a/object/P50343> ;
    reg:lexicalAlias <http://rdaregistry.info/Elements/a/relatedTimespanCollectiveAgent.en> ;
    reg:name "relatedTimespanCollectiveAgent"@en ;
    reg:status <http://metadataregistry.org/uri/RegStatus/1001> ;
    a rdf:Property ;
    rdfs:domain <http://rdaregistry.info/Elements/c/C10011> ;
    rdfs:isDefinedBy <http://rdaregistry.info/Elements/a/> ;
    rdfs:label "has related time-span (collective agent)"@en ;
    rdfs:subPropertyOf <http://rdaregistry.info/Elements/a/P50339>, <http://rdaregistry.info/Elements/a/P50360> ;
    skos:definition "Relates a collective agent to"@en .

<http://rdaregistry.info/Elements/a/P50344>
    reg:hasSubproperty <http://rdaregistry.info/Elements/a/datatype/P50344>, <http://rdaregistry.info/Elements/a/object/P50344> ;
    reg:lexicalAlias <http://rdaregistry.info/Elements/a/relatedNomenCollectiveAgent.en> ;
    reg:name "relatedNomenCollectiveAgent"@en ;
    reg:status <http://metadataregistry.org/uri/RegStatus/1001> ;
    a rdf:Property ;
    rdfs:domain <http://rdaregistry.info/Elements/c/C10011> ;
    rdfs:isDefinedBy <http://rdaregistry.info/Elements/a/> ;
    rdfs:label "has related nomen (collective agent)"@en ;
    rdfs:subPropertyOf <http://rdaregistry.info/Elements/a/P50340>, <http://rdaregistry.info/Elements/a/P50360> ;
    skos:definition "Relates a collective agent to"@en .

<http://rdaregistry.info/Elements/a/P50345>
    reg:hasSubproperty <http://rdaregistry.info/Elements/a/P50317>, <http://rdaregistry.info/Elements/a/P50318>, <http://rdaregistry.info/Elements/a/datatype/P50345>, <http://rdaregistry.info/Elements/a/object/P50345> ;
    reg:lexicalAlias <http://rdaregistry.info/Elements/a/relatedCollectiveAgentPerson.en> ;
    reg:name "relatedCollectiveAgentPerson"@en ;
    reg:status <http://metadataregistry.org/uri/RegStatus/1001> ;
    a rdf:Property ;
    rdfs:domain <http://rdaregistry.info/Elements/c/C10004> ;
    rdfs:isDefinedBy <http://rdaregistry.info/Elements/a/> ;
    rdfs:label "has related collective agent (person)"@en ;
    rdfs:subPropertyOf <http://rdaregistry.info/Elements/a/P50315>, <http://rdaregistry.info/Elements/a/P50337> ;
    skos:definition "Relates a person to"@en .

<http://rdaregistry.info/Elements/a/P50346>
    reg:hasSubproperty <http://rdaregistry.info/Elements/a/datatype/P50346>, <http://rdaregistry.info/Elements/a/object/P50346> ;
    reg:lexicalAlias <http://rdaregistry.info/Elements/a/relatedPlacePerson.en> ;
    reg:name "relatedPlacePerson"@en ;
    reg:status <http://metadataregistry.org/uri/RegStatus/1001> ;
    a rdf:Property ;
    rdfs:domain <http://rdaregistry.info/Elements/c/C10004> ;
    rdfs:isDefinedBy <http://rdaregistry.info/Elements/a/> ;
    rdfs:label "has related place (person)"@en ;
    rdfs:subPropertyOf <http://rdaregistry.info/Elements/a/P50310>, <http://rdaregistry.info/Elements/a/P50338> ;
    skos:definition "Relates a person to"@en .

<http://rdaregistry.info/Elements/a/P50347>
    reg:hasSubproperty <http://rdaregistry.info/Elements/a/datatype/P50347>, <http://rdaregistry.info/Elements/a/object/P50347> ;
    reg:lexicalAlias <http://rdaregistry.info/Elements/a/relatedTimespanPerson.en> ;
    reg:name "relatedTimespanPerson"@en ;
    reg:status <http://metadataregistry.org/uri/RegStatus/1001> ;
    a rdf:Property ;
    rdfs:domain <http://rdaregistry.info/Elements/c/C10004> ;
    rdfs:isDefinedBy <http://rdaregistry.info/Elements/a/> ;
    rdfs:label "has related time-span (person)"@en ;
    rdfs:subPropertyOf <http://rdaregistry.info/Elements/a/P50310>, <http://rdaregistry.info/Elements/a/P50339> ;
    skos:definition "Relates a person to"@en .

<http://rdaregistry.info/Elements/a/P50348>
    reg:hasSubproperty <http://rdaregistry.info/Elements/a/datatype/P50348>, <http://rdaregistry.info/Elements/a/object/P50348> ;
    reg:lexicalAlias <http://rdaregistry.info/Elements/a/relatedNomenPerson.en> ;
    reg:name "relatedNomenPerson"@en ;
    reg:status <http://metadataregistry.org/uri/RegStatus/1001> ;
    a rdf:Property ;
    rdfs:domain <http://rdaregistry.info/Elements/c/C10004> ;
    rdfs:isDefinedBy <http://rdaregistry.info/Elements/a/> ;
    rdfs:label "has related nomen (person)"@en ;
    rdfs:subPropertyOf <http://rdaregistry.info/Elements/a/P50310>, <http://rdaregistry.info/Elements/a/P50340> ;
    skos:definition "Relates a person to"@en .

<http://rdaregistry.info/Elements/a/P50349>
    reg:hasSubproperty <http://rdaregistry.info/Elements/a/datatype/P50349>, <http://rdaregistry.info/Elements/a/object/P50349> ;
    reg:lexicalAlias <http://rdaregistry.info/Elements/a/relatedCollectiveAgentCorporateBody.en> ;
    reg:name "relatedCollectiveAgentCorporateBody"@en ;
    reg:status <http://metadataregistry.org/uri/RegStatus/1001> ;
    a rdf:Property ;
    rdfs:domain <http://rdaregistry.info/Elements/c/C10005> ;
    rdfs:isDefinedBy <http://rdaregistry.info/Elements/a/> ;
    rdfs:label "has related collective agent (corporate body)"@en ;
    rdfs:subPropertyOf <http://rdaregistry.info/Elements/a/P50328>, <http://rdaregistry.info/Elements/a/P50341> ;
    skos:definition "Relates a corporate body to"@en .

<http://rdaregistry.info/Elements/a/P50350>
    reg:hasSubproperty <http://rdaregistry.info/Elements/a/datatype/P50350>, <http://rdaregistry.info/Elements/a/object/P50350> ;
    reg:lexicalAlias <http://rdaregistry.info/Elements/a/relatedPlaceCorporateBody.en> ;
    reg:name "relatedPlaceCorporateBody"@en ;
    reg:status <http://metadataregistry.org/uri/RegStatus/1001> ;
    a rdf:Property ;
    rdfs:domain <http://rdaregistry.info/Elements/c/C10005> ;
    rdfs:isDefinedBy <http://rdaregistry.info/Elements/a/> ;
    rdfs:label "has related place (corporate body)"@en ;
    rdfs:subPropertyOf <http://rdaregistry.info/Elements/a/P50328>, <http://rdaregistry.info/Elements/a/P50342> ;
    skos:definition "Relates a corporate body to"@en .

<http://rdaregistry.info/Elements/a/P50351>
    reg:hasSubproperty <http://rdaregistry.info/Elements/a/datatype/P50351>, <http://rdaregistry.info/Elements/a/object/P50351> ;
    reg:lexicalAlias <http://rdaregistry.info/Elements/a/relatedTimespanCorporateBody.en> ;
    reg:name "relatedTimespanCorporateBody"@en ;
    reg:status <http://metadataregistry.org/uri/RegStatus/1001> ;
    a rdf:Property ;
    rdfs:domain <http://rdaregistry.info/Elements/c/C10005> ;
    rdfs:isDefinedBy <http://rdaregistry.info/Elements/a/> ;
    rdfs:label "has related time-span (corporate body)"@en ;
    rdfs:subPropertyOf <http://rdaregistry.info/Elements/a/P50328>, <http://rdaregistry.info/Elements/a/P50343> ;
    skos:definition "Relates a corporate body to"@en .

<http://rdaregistry.info/Elements/a/P50352>
    reg:hasSubproperty <http://rdaregistry.info/Elements/a/datatype/P50352>, <http://rdaregistry.info/Elements/a/object/P50352> ;
    reg:lexicalAlias <http://rdaregistry.info/Elements/a/relatedNomenCorporateBody.en> ;
    reg:name "relatedNomenCorporateBody"@en ;
    reg:status <http://metadataregistry.org/uri/RegStatus/1001> ;
    a rdf:Property ;
    rdfs:domain <http://rdaregistry.info/Elements/c/C10005> ;
    rdfs:isDefinedBy <http://rdaregistry.info/Elements/a/> ;
    rdfs:label "has related nomen (corporate body)"@en ;
    rdfs:subPropertyOf <http://rdaregistry.info/Elements/a/P50328>, <http://rdaregistry.info/Elements/a/P50344> ;
    skos:definition "Relates a corporate body to"@en .

<http://rdaregistry.info/Elements/a/P50353>
    reg:hasSubproperty <http://rdaregistry.info/Elements/a/P50326>, <http://rdaregistry.info/Elements/a/P50327>, <http://rdaregistry.info/Elements/a/datatype/P50353>, <http://rdaregistry.info/Elements/a/object/P50353> ;
    reg:lexicalAlias <http://rdaregistry.info/Elements/a/relatedCollectiveAgentFamily.en> ;
    reg:name "relatedCollectiveAgentFamily"@en ;
    reg:status <http://metadataregistry.org/uri/RegStatus/1001> ;
    a rdf:Property ;
    rdfs:domain <http://rdaregistry.info/Elements/c/C10008> ;
    rdfs:isDefinedBy <http://rdaregistry.info/Elements/a/> ;
    rdfs:label "has related collective agent (family)"@en ;
    rdfs:subPropertyOf <http://rdaregistry.info/Elements/a/P50324>, <http://rdaregistry.info/Elements/a/P50341> ;
    skos:definition "Relates a family to"@en .

<http://rdaregistry.info/Elements/a/P50354>
    reg:hasSubproperty <http://rdaregistry.info/Elements/a/datatype/P50354>, <http://rdaregistry.info/Elements/a/object/P50354> ;
    reg:lexicalAlias <http://rdaregistry.info/Elements/a/relatedPlaceFamily.en> ;
    reg:name "relatedPlaceFamily"@en ;
    reg:status <http://metadataregistry.org/uri/RegStatus/1001> ;
    a rdf:Property ;
    rdfs:domain <http://rdaregistry.info/Elements/c/C10008> ;
    rdfs:isDefinedBy <http://rdaregistry.info/Elements/a/> ;
    rdfs:label "has related place (family)"@en ;
    rdfs:subPropertyOf <http://rdaregistry.info/Elements/a/P50319>, <http://rdaregistry.info/Elements/a/P50342> ;
    skos:definition "Relates a family to"@en .

<http://rdaregistry.info/Elements/a/P50355>
    reg:hasSubproperty <http://rdaregistry.info/Elements/a/datatype/P50355>, <http://rdaregistry.info/Elements/a/object/P50355> ;
    reg:lexicalAlias <http://rdaregistry.info/Elements/a/relatedTimespanFamily.en> ;
    reg:name "relatedTimespanFamily"@en ;
    reg:status <http://metadataregistry.org/uri/RegStatus/1001> ;
    a rdf:Property ;
    rdfs:domain <http://rdaregistry.info/Elements/c/C10008> ;
    rdfs:isDefinedBy <http://rdaregistry.info/Elements/a/> ;
    rdfs:label "has related time-span (family)"@en ;
    rdfs:subPropertyOf <http://rdaregistry.info/Elements/a/P50319>, <http://rdaregistry.info/Elements/a/P50343> ;
    skos:definition "Relates a family to"@en .

<http://rdaregistry.info/Elements/a/P50356>
    reg:hasSubproperty <http://rdaregistry.info/Elements/a/datatype/P50356>, <http://rdaregistry.info/Elements/a/object/P50356> ;
    reg:lexicalAlias <http://rdaregistry.info/Elements/a/relatedNomenFamily.en> ;
    reg:name "relatedNomenFamily"@en ;
    reg:status <http://metadataregistry.org/uri/RegStatus/1001> ;
    a rdf:Property ;
    rdfs:domain <http://rdaregistry.info/Elements/c/C10008> ;
    rdfs:isDefinedBy <http://rdaregistry.info/Elements/a/> ;
    rdfs:label "has related nomen (family)"@en ;
    rdfs:subPropertyOf <http://rdaregistry.info/Elements/a/P50319>, <http://rdaregistry.info/Elements/a/P50344> ;
    skos:definition "Relates a family to"@en .

<http://rdaregistry.info/Elements/a/P50357>
    reg:hasSubproperty <http://rdaregistry.info/Elements/a/datatype/P50357>, <http://rdaregistry.info/Elements/a/object/P50357> ;
    reg:lexicalAlias <http://rdaregistry.info/Elements/a/relatedWorkCollectiveAgent.en> ;
    reg:name "relatedWorkCollectiveAgent"@en ;
    reg:status <http://metadataregistry.org/uri/RegStatus/1001> ;
    a rdf:Property ;
    rdfs:domain <http://rdaregistry.info/Elements/c/C10011> ;
    rdfs:isDefinedBy <http://rdaregistry.info/Elements/a/> ;
    rdfs:label "has related work (collective agent)"@en ;
    rdfs:subPropertyOf <http://rdaregistry.info/Elements/a/P50305>, <http://rdaregistry.info/Elements/a/P50360> ;
    skos:definition "Relates a collective agent to a work associated with a collective agent being described."@en .

<http://rdaregistry.info/Elements/a/P50358>
    reg:hasSubproperty <http://rdaregistry.info/Elements/a/P50218>, <http://rdaregistry.info/Elements/a/P50219>, <http://rdaregistry.info/Elements/a/P50341>, <http://rdaregistry.info/Elements/a/P50365>, <http://rdaregistry.info/Elements/a/datatype/P50358>, <http://rdaregistry.info/Elements/a/object/P50358> ;
    reg:lexicalAlias <http://rdaregistry.info/Elements/a/relatedAgentCollectiveAgent.en> ;
    reg:name "relatedAgentCollectiveAgent"@en ;
    reg:status <http://metadataregistry.org/uri/RegStatus/1001> ;
    a rdf:Property ;
    rdfs:domain <http://rdaregistry.info/Elements/c/C10011> ;
    rdfs:isDefinedBy <http://rdaregistry.info/Elements/a/> ;
    rdfs:label "has related agent (collective agent)"@en ;
    rdfs:subPropertyOf <http://rdaregistry.info/Elements/a/P50309>, <http://rdaregistry.info/Elements/a/P50360> ;
    skos:definition "Relates a collective agent to an agent associated with a collective agent,"@en .

<http://rdaregistry.info/Elements/a/P50359>
    reg:hasSubproperty <http://rdaregistry.info/Elements/a/datatype/P50359>, <http://rdaregistry.info/Elements/a/object/P50359> ;
    reg:lexicalAlias <http://rdaregistry.info/Elements/a/relatedCorporateBodyCollectiveAgent.en> ;
    reg:name "relatedCorporateBodyCollectiveAgent"@en ;
    reg:status <http://metadataregistry.org/uri/RegStatus/1001> ;
    a rdf:Property ;
    rdfs:domain <http://rdaregistry.info/Elements/c/C10011> ;
    rdfs:isDefinedBy <http://rdaregistry.info/Elements/a/> ;
    rdfs:label "has related corporate body (collective agent)"@en ;
    rdfs:subPropertyOf <http://rdaregistry.info/Elements/a/P50218>, <http://rdaregistry.info/Elements/a/P50341> ;
    skos:definition "Relastes a collective agent to a corporate body associated with a collective agent."@en .

<http://rdaregistry.info/Elements/a/P50360>
    reg:hasSubproperty <http://rdaregistry.info/Elements/a/P50342>, <http://rdaregistry.info/Elements/a/P50343>, <http://rdaregistry.info/Elements/a/P50344>, <http://rdaregistry.info/Elements/a/P50357>, <http://rdaregistry.info/Elements/a/P50358>, <http://rdaregistry.info/Elements/a/P50361>, <http://rdaregistry.info/Elements/a/P50363>, <http://rdaregistry.info/Elements/a/P50364>, <http://rdaregistry.info/Elements/a/datatype/P50360>, <http://rdaregistry.info/Elements/a/object/P50360> ;
    reg:lexicalAlias <http://rdaregistry.info/Elements/a/relatedEntityCollectiveAgent.en> ;
    reg:name "relatedEntityCollectiveAgent"@en ;
    reg:status <http://metadataregistry.org/uri/RegStatus/1001> ;
    a rdf:Property ;
    rdfs:domain <http://rdaregistry.info/Elements/c/C10011> ;
    rdfs:isDefinedBy <http://rdaregistry.info/Elements/a/> ;
    rdfs:label "has related entity (collective agent)"@en ;
    rdfs:subPropertyOf <http://rdaregistry.info/Elements/a/P50304> ;
    skos:definition "Relastes a collective agent to an entity associated with a collective agent."@en .

<http://rdaregistry.info/Elements/a/P50361>
    reg:hasSubproperty <http://rdaregistry.info/Elements/a/datatype/P50361>, <http://rdaregistry.info/Elements/a/object/P50361> ;
    reg:lexicalAlias <http://rdaregistry.info/Elements/a/relatedExpressionCollectiveAgent.en> ;
    reg:name "relatedExpressionCollectiveAgent"@en ;
    reg:status <http://metadataregistry.org/uri/RegStatus/1001> ;
    a rdf:Property ;
    rdfs:domain <http://rdaregistry.info/Elements/c/C10011> ;
    rdfs:isDefinedBy <http://rdaregistry.info/Elements/a/> ;
    rdfs:label "has related expression (collective agent)"@en ;
    rdfs:subPropertyOf <http://rdaregistry.info/Elements/a/P50306>, <http://rdaregistry.info/Elements/a/P50360> ;
    skos:definition "Relastes a collective agent to an expression associated with a collective agent."@en .

<http://rdaregistry.info/Elements/a/P50362>
    reg:hasSubproperty <http://rdaregistry.info/Elements/a/datatype/P50362>, <http://rdaregistry.info/Elements/a/object/P50362> ;
    reg:lexicalAlias <http://rdaregistry.info/Elements/a/relatedFamilyCollectiveAgent.en> ;
    reg:name "relatedFamilyCollectiveAgent"@en ;
    reg:status <http://metadataregistry.org/uri/RegStatus/1001> ;
    a rdf:Property ;
    rdfs:domain <http://rdaregistry.info/Elements/c/C10011> ;
    rdfs:isDefinedBy <http://rdaregistry.info/Elements/a/> ;
    rdfs:label "has related family (collective agent)"@en ;
    rdfs:subPropertyOf <http://rdaregistry.info/Elements/a/P50219>, <http://rdaregistry.info/Elements/a/P50341> ;
    skos:definition "Relastes a collective agent to a family associated with a collective agent."@en .

<http://rdaregistry.info/Elements/a/P50363>
    reg:hasSubproperty <http://rdaregistry.info/Elements/a/datatype/P50363>, <http://rdaregistry.info/Elements/a/object/P50363> ;
    reg:lexicalAlias <http://rdaregistry.info/Elements/a/relatedItemCollectiveAgent.en> ;
    reg:name "relatedItemCollectiveAgent"@en ;
    reg:status <http://metadataregistry.org/uri/RegStatus/1001> ;
    a rdf:Property ;
    rdfs:domain <http://rdaregistry.info/Elements/c/C10011> ;
    rdfs:isDefinedBy <http://rdaregistry.info/Elements/a/> ;
    rdfs:label "has related item (collective agent)"@en ;
    rdfs:subPropertyOf <http://rdaregistry.info/Elements/a/P50308>, <http://rdaregistry.info/Elements/a/P50360> ;
    skos:definition "Relastes a collective agent to an item associated with a collective agent."@en .

<http://rdaregistry.info/Elements/a/P50364>
    reg:hasSubproperty <http://rdaregistry.info/Elements/a/datatype/P50364>, <http://rdaregistry.info/Elements/a/object/P50364> ;
    reg:lexicalAlias <http://rdaregistry.info/Elements/a/relatedManifestationCollectiveAgent.en> ;
    reg:name "relatedManifestationCollectiveAgent"@en ;
    reg:status <http://metadataregistry.org/uri/RegStatus/1001> ;
    a rdf:Property ;
    rdfs:domain <http://rdaregistry.info/Elements/c/C10011> ;
    rdfs:isDefinedBy <http://rdaregistry.info/Elements/a/> ;
    rdfs:label "has related manifestation (collective agent)"@en ;
    rdfs:subPropertyOf <http://rdaregistry.info/Elements/a/P50307>, <http://rdaregistry.info/Elements/a/P50360> ;
    skos:definition "Relastes a collective agent to a manifestation associated with a collective agent."@en .

<http://rdaregistry.info/Elements/a/P50365>
    reg:hasSubproperty <http://rdaregistry.info/Elements/a/datatype/P50365>, <http://rdaregistry.info/Elements/a/object/P50365> ;
    reg:lexicalAlias <http://rdaregistry.info/Elements/a/relatedPersonCollectiveAgent.en> ;
    reg:name "relatedPersonCollectiveAgent"@en ;
    reg:status <http://metadataregistry.org/uri/RegStatus/1001> ;
    a rdf:Property ;
    rdfs:domain <http://rdaregistry.info/Elements/c/C10011> ;
    rdfs:isDefinedBy <http://rdaregistry.info/Elements/a/> ;
    rdfs:label "has related person (collective agent)"@en ;
    rdfs:subPropertyOf <http://rdaregistry.info/Elements/a/P50220>, <http://rdaregistry.info/Elements/a/P50358> ;
    skos:definition "Relastes a collective agent to a person associated with a collective agent."@en .

<http://rdaregistry.info/Elements/a/P50366>
    reg:lexicalAlias <http://rdaregistry.info/Elements/a/subjectOfAgent.en> ;
    reg:name "subjectOfAgent"@en ;
    reg:status <http://metadataregistry.org/uri/RegStatus/1001> ;
    a rdf:Property ;
    rdfs:domain <http://rdaregistry.info/Elements/c/C10011> ;
    rdfs:isDefinedBy <http://rdaregistry.info/Elements/a/> ;
    rdfs:label "is subject of (agent)"@en ;
    rdfs:subPropertyOf <http://rdaregistry.info/Elements/w/P10283> ;
    skos:definition "Relates an agent to a work that is about an agent."@en .

<http://rdaregistry.info/Elements/a/P50367>
    reg:lexicalAlias <http://rdaregistry.info/Elements/a/subjectOfCollectiveAgent.en> ;
    reg:name "subjectOfCollectiveAgent"@en ;
    reg:status <http://metadataregistry.org/uri/RegStatus/1001> ;
    a rdf:Property ;
    rdfs:domain <http://rdaregistry.info/Elements/c/C10011> ;
    rdfs:isDefinedBy <http://rdaregistry.info/Elements/a/> ;
    rdfs:label "is subject of (collective agent)"@en ;
    rdfs:subPropertyOf <http://rdaregistry.info/Elements/a/P50366> ;
    skos:definition "Relates a collective agent to a work that is about a collective agent."@en .

