@prefix rdf: <http://www.w3.org/1999/02/22-rdf-syntax-ns#> .
@prefix rdfs: <http://www.w3.org/2000/01/rdf-schema#> .
@prefix skos: <http://www.w3.org/2004/02/skos/core#> .
@prefix dc: <http://purl.org/dc/elements/1.1/> .
@prefix dct: <http://purl.org/dc/terms/> .
@prefix owl: <http://www.w3.org/2002/07/owl#> .
@prefix foaf: <http://xmlns.com/foaf/0.1/> .
@prefix reg: <http://metadataregistry.org/uri/profile/RegAp/> .
@prefix rdakit: <http://metadataregistry.org/uri/profile/rdakit/> .
@prefix status: <http://metadataregistry.org/uri/RegStatus/> .

<http://metadataregistry.org/uri/RegStatus/1001>
    a skos:Concept ;
    skos:prefLabel "Published"@en .

<http://metadataregistry.org/uri/RegStatus/1008>
    a skos:Concept ;
    skos:prefLabel "Deprecated"@en .

<http://rdaregistry.info/Elements/e/>
    dc:title "RDA Expression properties"@en ;
    skos:note "Properties derived from RDA elements and relationship designators with the domain of RDA Expression."@en ;
    foaf:homepage <http://www.rdaregistry.info/Elements/e/> .

<http://rdaregistry.info/Elements/e/P20001>
    reg:hasUnconstrained <http://rdaregistry.info/Elements/u/P60049> ;
    reg:lexicalAlias <http://rdaregistry.info/Elements/e/contentType.en> ;
    reg:name "contentType"@en ;
    reg:status <http://metadataregistry.org/uri/RegStatus/1001> ;
    rdakit:instructionNumber "6.9" ;
    rdakit:toolkitDefinition "A categorization reflecting the fundamental form of communication in which the content is expressed and the human sense through which it is intended to be perceived."@en ;
    rdakit:toolkitLabel "content type"@en ;
    a rdf:Property ;
    rdfs:domain <http://rdaregistry.info/Elements/c/C10006> ;
    rdfs:isDefinedBy <http://rdaregistry.info/Elements/e/> ;
    rdfs:label "has content type"@en ;
    skos:definition "Relates an expression to a categorization reflecting the fundamental form of communication in which the content is expressed and the human sense through which it is intended to be perceived."@en ;
    skos:scopeNote "For content expressed in the form of an image or images, content type also reflects the number of spatial dimensions in which the content is intended to be perceived and the perceived presence or absence of movement."@en .

<http://rdaregistry.info/Elements/e/P20002>
    reg:hasUnconstrained <http://rdaregistry.info/Elements/u/P60052> ;
    reg:lexicalAlias <http://rdaregistry.info/Elements/e/identifierForTheExpression.en> ;
    reg:name "identifierForTheExpression"@en ;
    reg:status <http://metadataregistry.org/uri/RegStatus/1001> ;
    rdakit:instructionNumber "6.13" ;
    rdakit:toolkitDefinition "A character string uniquely associated with an expression, or with a surrogate for an expression (e.g., an authority record)."@en ;
    rdakit:toolkitLabel "identifier for the expression"@en ;
    a rdf:Property ;
    rdfs:domain <http://rdaregistry.info/Elements/c/C10006> ;
    rdfs:isDefinedBy <http://rdaregistry.info/Elements/e/> ;
    rdfs:label "has identifier for the expression"@en ;
    skos:definition "Relates an expression to a character string uniquely associated with an expression, or with a surrogate for an expression (e.g., an authority record)."@en ;
    skos:scopeNote "The identifier serves to differentiate that expression from other expressions."@en .

<http://rdaregistry.info/Elements/e/P20003>
    reg:hasUnconstrained <http://rdaregistry.info/Elements/u/P60054> ;
    reg:lexicalAlias <http://rdaregistry.info/Elements/e/otherDistinguishingCharacteristicOfTheExpression.en> ;
    reg:name "otherDistinguishingCharacteristicOfTheExpression"@en ;
    reg:status <http://metadataregistry.org/uri/RegStatus/1001> ;
    rdakit:instructionNumber "6.12" ;
    rdakit:toolkitDefinition "A characteristic other than content type, language of expression, or date of expression."@en ;
    rdakit:toolkitLabel "other distinguishing characteristic of the expression"@en ;
    a rdf:Property ;
    rdfs:domain <http://rdaregistry.info/Elements/c/C10006> ;
    rdfs:isDefinedBy <http://rdaregistry.info/Elements/e/> ;
    rdfs:label "has other distinguishing characteristic of the expression"@en ;
    skos:definition "Relates an expression to a characteristic other than content type, language of expression, or date of expression."@en ;
    skos:scopeNote "It serves to differentiate an expression from another expression of the same work."@en .

<http://rdaregistry.info/Elements/e/P20004>
    reg:hasUnconstrained <http://rdaregistry.info/Elements/u/P60074> ;
    reg:lexicalAlias <http://rdaregistry.info/Elements/e/dateOfCapture.en> ;
    reg:name "dateOfCapture"@en ;
    reg:status <http://metadataregistry.org/uri/RegStatus/1001> ;
    rdakit:instructionNumber "7.11.3" ;
    rdakit:toolkitDefinition "A date or range of dates associated with the capture (i.e., recording, filming, etc.) of the content of a resource."@en ;
    rdakit:toolkitLabel "date of capture"@en ;
    a rdf:Property ;
    rdfs:domain <http://rdaregistry.info/Elements/c/C10006> ;
    rdfs:isDefinedBy <http://rdaregistry.info/Elements/e/> ;
    rdfs:label "has date of capture"@en ;
    skos:definition "Relates an expression to a date or range of dates associated with the capture (i.e., recording, filming, etc.) of the content of a resource."@en .

<http://rdaregistry.info/Elements/e/P20005>
    reg:hasUnconstrained <http://rdaregistry.info/Elements/u/P60090> ;
    reg:lexicalAlias <http://rdaregistry.info/Elements/e/award.en> ;
    reg:name "award"@en ;
    reg:status <http://metadataregistry.org/uri/RegStatus/1001> ;
    rdakit:instructionNumber "7.28" ;
    rdakit:toolkitDefinition "A formal recognition of excellence, etc., given by an award- or prize-granting body, for the content of a resource."@en ;
    rdakit:toolkitLabel "award"@en ;
    a rdf:Property ;
    rdfs:domain <http://rdaregistry.info/Elements/c/C10006> ;
    rdfs:isDefinedBy <http://rdaregistry.info/Elements/e/> ;
    rdfs:label "has award"@en ;
    skos:definition "Relates an expression to a formal recognition of excellence, etc., given by an award- or prize-granting body, for the content of a resource."@en .

<http://rdaregistry.info/Elements/e/P20006>
    reg:hasUnconstrained <http://rdaregistry.info/Elements/u/P60099> ;
    reg:lexicalAlias <http://rdaregistry.info/Elements/e/languageOfExpression.en> ;
    reg:name "languageOfExpression"@en ;
    reg:status <http://metadataregistry.org/uri/RegStatus/1001> ;
    rdakit:instructionNumber "6.11" ;
    rdakit:toolkitDefinition "A language in which a work is expressed."@en ;
    rdakit:toolkitLabel "language of expression"@en ;
    a rdf:Property ;
    rdfs:domain <http://rdaregistry.info/Elements/c/C10006> ;
    rdfs:isDefinedBy <http://rdaregistry.info/Elements/e/> ;
    rdfs:label "has language of expression"@en ;
    skos:definition "Relates an expression to a language in which a work is expressed."@en .

<http://rdaregistry.info/Elements/e/P20007>
    reg:hasUnconstrained <http://rdaregistry.info/Elements/u/P60099> ;
    reg:lexicalAlias <http://rdaregistry.info/Elements/e/languageOfTheContent.en> ;
    reg:name "languageOfTheContent"@en ;
    reg:status <http://metadataregistry.org/uri/RegStatus/1001> ;
    rdakit:instructionNumber "7.12" ;
    rdakit:toolkitDefinition "A language used to express the content of a resource."@en ;
    rdakit:toolkitLabel "language of the content"@en ;
    a rdf:Property ;
    rdfs:domain <http://rdaregistry.info/Elements/c/C10006> ;
    rdfs:isDefinedBy <http://rdaregistry.info/Elements/e/> ;
    rdfs:label "has language of the content"@en ;
    skos:definition "Relates an expression to a language used to express the content of a resource."@en .

<http://rdaregistry.info/Elements/e/P20008>
    reg:status <http://metadataregistry.org/uri/RegStatus/1008> ;
    a rdf:Property ;
    rdfs:isDefinedBy <http://rdaregistry.info/Elements/e/> .

<http://rdaregistry.info/Elements/e/P20009>
    reg:hasUnconstrained <http://rdaregistry.info/Elements/u/P60110> ;
    reg:lexicalAlias <http://rdaregistry.info/Elements/e/adaptedAsMotionPictureExpression.en> ;
    reg:name "adaptedAsMotionPictureExpression"@en ;
    reg:status <http://metadataregistry.org/uri/RegStatus/1001> ;
    rdakit:toolkitDefinition "A motion picture based on the source expression."@en ;
    rdakit:toolkitLabel "adapted as motion picture (expression)"@en ;
    a rdf:Property ;
    rdfs:domain <http://rdaregistry.info/Elements/c/C10006> ;
    rdfs:isDefinedBy <http://rdaregistry.info/Elements/e/> ;
    rdfs:label "is adapted as motion picture (expression)"@en ;
    rdfs:range <http://rdaregistry.info/Elements/c/C10006> ;
    rdfs:subPropertyOf <http://rdaregistry.info/Elements/e/P20153> ;
    owl:inverseOf <http://rdaregistry.info/Elements/e/P20125> ;
    skos:definition "Relates an expression to a motion picture based on the source expression."@en .

<http://rdaregistry.info/Elements/e/P20010>
    reg:hasUnconstrained <http://rdaregistry.info/Elements/u/P60123> ;
    reg:lexicalAlias <http://rdaregistry.info/Elements/e/noteOnChangesInContentCharacteristics.en> ;
    reg:name "noteOnChangesInContentCharacteristics"@en ;
    reg:status <http://metadataregistry.org/uri/RegStatus/1001> ;
    rdakit:instructionNumber "7.29.2" ;
    rdakit:toolkitDefinition "A note on changes in content characteristics that occur in subsequent issues or parts of a resource issued in successive parts or between iterations of an integrating resource."@en ;
    rdakit:toolkitLabel "note on changes in content characteristics"@en ;
    a rdf:Property ;
    rdfs:domain <http://rdaregistry.info/Elements/c/C10006> ;
    rdfs:isDefinedBy <http://rdaregistry.info/Elements/e/> ;
    rdfs:label "has note on changes in content characteristics"@en ;
    rdfs:subPropertyOf <http://rdaregistry.info/Elements/e/P20071> ;
    skos:definition "Relates an expression to a note on changes in content characteristics that occur in subsequent issues or parts of a resource issued in successive parts or between iterations of an integrating resource."@en .

<http://rdaregistry.info/Elements/e/P20011>
    reg:hasSubproperty <http://rdaregistry.info/Elements/e/P20285>, <http://rdaregistry.info/Elements/e/P20286> ;
    reg:hasUnconstrained <http://rdaregistry.info/Elements/u/P60141> ;
    reg:lexicalAlias <http://rdaregistry.info/Elements/e/conductor.en> ;
    reg:name "conductor"@en ;
    reg:status <http://metadataregistry.org/uri/RegStatus/1001> ;
    rdakit:toolkitDefinition "A performer contributing to an expression of a musical work by leading a performing group (orchestra, chorus, opera, etc.) in a musical or dramatic presentation, etc."@en ;
    rdakit:toolkitLabel "conductor"@en ;
    a rdf:Property ;
    rdfs:domain <http://rdaregistry.info/Elements/c/C10006> ;
    rdfs:isDefinedBy <http://rdaregistry.info/Elements/e/> ;
    rdfs:label "has conductor"@en ;
    rdfs:range <http://rdaregistry.info/Elements/c/C10002> ;
    rdfs:subPropertyOf <http://rdaregistry.info/Elements/e/P20039> ;
    owl:inverseOf <http://rdaregistry.info/Elements/a/P50070> ;
    skos:definition "Relates an expression to a performer contributing to an expression of a musical work by leading a performing group (orchestra, chorus, opera, etc.) in a musical or dramatic presentation, etc."@en .

<http://rdaregistry.info/Elements/e/P20012>
    reg:hasSubproperty <http://rdaregistry.info/Elements/e/P20070> ;
    reg:hasUnconstrained <http://rdaregistry.info/Elements/u/P60142> ;
    reg:lexicalAlias <http://rdaregistry.info/Elements/e/actor.en> ;
    reg:name "actor"@en ;
    reg:status <http://metadataregistry.org/uri/RegStatus/1001> ;
    rdakit:toolkitDefinition "A performer contributing to an expression of a work by acting as a cast member or player in a musical or dramatic presentation, etc."@en ;
    rdakit:toolkitLabel "actor"@en ;
    a rdf:Property ;
    rdfs:domain <http://rdaregistry.info/Elements/c/C10006> ;
    rdfs:isDefinedBy <http://rdaregistry.info/Elements/e/> ;
    rdfs:label "has actor"@en ;
    rdfs:range <http://rdaregistry.info/Elements/c/C10002> ;
    rdfs:subPropertyOf <http://rdaregistry.info/Elements/e/P20039> ;
    owl:inverseOf <http://rdaregistry.info/Elements/a/P50071> ;
    skos:definition "Relates an expression to a performer contributing to an expression of a work by acting as a cast member or player in a musical or dramatic presentation, etc."@en .

<http://rdaregistry.info/Elements/e/P20013>
    reg:hasUnconstrained <http://rdaregistry.info/Elements/u/P60143> ;
    reg:lexicalAlias <http://rdaregistry.info/Elements/e/onScreenPresenter.en> ;
    reg:name "onScreenPresenter"@en ;
    reg:status <http://metadataregistry.org/uri/RegStatus/1001> ;
    rdakit:toolkitDefinition "A performer contributing to an expression of a work by appearing on screen to provide contextual or background information."@en ;
    rdakit:toolkitLabel "on-screen presenter"@en ;
    a rdf:Property ;
    rdfs:domain <http://rdaregistry.info/Elements/c/C10006> ;
    rdfs:isDefinedBy <http://rdaregistry.info/Elements/e/> ;
    rdfs:label "has on-screen presenter"@en ;
    rdfs:range <http://rdaregistry.info/Elements/c/C10002> ;
    rdfs:subPropertyOf <http://rdaregistry.info/Elements/e/P20039> ;
    owl:inverseOf <http://rdaregistry.info/Elements/a/P50072> ;
    skos:definition "Relates an expression to a performer contributing to an expression of a work by appearing on screen to provide contextual or background information."@en ;
    skos:scopeNote "An on-screen presenter may appear in nonfiction moving image materials or in introductions to fiction moving image materials."@en .

<http://rdaregistry.info/Elements/e/P20014>
    reg:hasUnconstrained <http://rdaregistry.info/Elements/u/P60144> ;
    reg:lexicalAlias <http://rdaregistry.info/Elements/e/dancer.en> ;
    reg:name "dancer"@en ;
    reg:status <http://metadataregistry.org/uri/RegStatus/1001> ;
    rdakit:toolkitDefinition "A performer contributing to an expression of a work by dancing in a musical, dramatic, etc., presentation."@en ;
    rdakit:toolkitLabel "dancer"@en ;
    a rdf:Property ;
    rdfs:domain <http://rdaregistry.info/Elements/c/C10006> ;
    rdfs:isDefinedBy <http://rdaregistry.info/Elements/e/> ;
    rdfs:label "has dancer"@en ;
    rdfs:range <http://rdaregistry.info/Elements/c/C10002> ;
    rdfs:subPropertyOf <http://rdaregistry.info/Elements/e/P20039> ;
    owl:inverseOf <http://rdaregistry.info/Elements/a/P50073> ;
    skos:definition "Relates an expression to a performer contributing to an expression of a work by dancing in a musical, dramatic, etc., presentation."@en .

<http://rdaregistry.info/Elements/e/P20015>
    reg:hasUnconstrained <http://rdaregistry.info/Elements/u/P60145> ;
    reg:lexicalAlias <http://rdaregistry.info/Elements/e/teacher.en> ;
    reg:name "teacher"@en ;
    reg:status <http://metadataregistry.org/uri/RegStatus/1001> ;
    rdakit:toolkitDefinition "A performer contributing to an expression of a work by giving instruction or providing a demonstration."@en ;
    rdakit:toolkitLabel "teacher"@en ;
    a rdf:Property ;
    rdfs:domain <http://rdaregistry.info/Elements/c/C10006> ;
    rdfs:isDefinedBy <http://rdaregistry.info/Elements/e/> ;
    rdfs:label "has teacher"@en ;
    rdfs:range <http://rdaregistry.info/Elements/c/C10002> ;
    rdfs:subPropertyOf <http://rdaregistry.info/Elements/e/P20039> ;
    owl:inverseOf <http://rdaregistry.info/Elements/a/P50074> ;
    skos:definition "Relates an expression to a performer contributing to an expression of a work by giving instruction or providing a demonstration."@en .

<http://rdaregistry.info/Elements/e/P20016>
    reg:hasUnconstrained <http://rdaregistry.info/Elements/u/P60146> ;
    reg:lexicalAlias <http://rdaregistry.info/Elements/e/host.en> ;
    reg:name "host"@en ;
    reg:status <http://metadataregistry.org/uri/RegStatus/1001> ;
    rdakit:toolkitDefinition "A performer contributing to an expression of a work by leading a program (often broadcast) that includes other guests, performers, etc. (e.g., talk show host)."@en ;
    rdakit:toolkitLabel "host"@en ;
    a rdf:Property ;
    rdfs:domain <http://rdaregistry.info/Elements/c/C10006> ;
    rdfs:isDefinedBy <http://rdaregistry.info/Elements/e/> ;
    rdfs:label "has host"@en ;
    rdfs:range <http://rdaregistry.info/Elements/c/C10002> ;
    rdfs:subPropertyOf <http://rdaregistry.info/Elements/e/P20039> ;
    owl:inverseOf <http://rdaregistry.info/Elements/a/P50075> ;
    skos:definition "Relates an expression to a performer contributing to an expression of a work by leading a program (often broadcast) that includes other guests, performers, etc. (e.g., talk show host)."@en .

<http://rdaregistry.info/Elements/e/P20017>
    reg:hasUnconstrained <http://rdaregistry.info/Elements/u/P60147> ;
    reg:lexicalAlias <http://rdaregistry.info/Elements/e/moderator.en> ;
    reg:name "moderator"@en ;
    reg:status <http://metadataregistry.org/uri/RegStatus/1001> ;
    rdakit:toolkitDefinition "A performer contributing to an expression of a work by leading a program (often broadcast) where topics are discussed, usually with participation of experts in fields related to the discussion."@en ;
    rdakit:toolkitLabel "moderator"@en ;
    a rdf:Property ;
    rdfs:domain <http://rdaregistry.info/Elements/c/C10006> ;
    rdfs:isDefinedBy <http://rdaregistry.info/Elements/e/> ;
    rdfs:label "has moderator"@en ;
    rdfs:range <http://rdaregistry.info/Elements/c/C10002> ;
    rdfs:subPropertyOf <http://rdaregistry.info/Elements/e/P20039> ;
    owl:inverseOf <http://rdaregistry.info/Elements/a/P50076> ;
    skos:definition "Relates an expression to a performer contributing to an expression of a work by leading a program (often broadcast) where topics are discussed, usually with participation of experts in fields related to the discussion."@en .

<http://rdaregistry.info/Elements/e/P20018>
    reg:hasUnconstrained <http://rdaregistry.info/Elements/u/P60148> ;
    reg:lexicalAlias <http://rdaregistry.info/Elements/e/puppeteer.en> ;
    reg:name "puppeteer"@en ;
    reg:status <http://metadataregistry.org/uri/RegStatus/1001> ;
    rdakit:toolkitDefinition "A performer contributing to an expression of a work by manipulating, controlling, or directing puppets or marionettes in a moving image production or a musical or dramatic presentation or entertainment."@en ;
    rdakit:toolkitLabel "puppeteer"@en ;
    a rdf:Property ;
    rdfs:domain <http://rdaregistry.info/Elements/c/C10006> ;
    rdfs:isDefinedBy <http://rdaregistry.info/Elements/e/> ;
    rdfs:label "has puppeteer"@en ;
    rdfs:range <http://rdaregistry.info/Elements/c/C10002> ;
    rdfs:subPropertyOf <http://rdaregistry.info/Elements/e/P20039> ;
    owl:inverseOf <http://rdaregistry.info/Elements/a/P50077> ;
    skos:definition "Relates an expression to a performer contributing to an expression of a work by manipulating, controlling, or directing puppets or marionettes in a moving image production or a musical or dramatic presentation or entertainment."@en .

<http://rdaregistry.info/Elements/e/P20019>
    reg:hasUnconstrained <http://rdaregistry.info/Elements/u/P60149> ;
    reg:lexicalAlias <http://rdaregistry.info/Elements/e/panelist.en> ;
    reg:name "panelist"@en ;
    reg:status <http://metadataregistry.org/uri/RegStatus/1001> ;
    rdakit:toolkitDefinition "A performer contributing to an expression of a work by participating in a program (often broadcast) where topics are discussed, usually with participation of experts in fields related to the discussion."@en ;
    rdakit:toolkitLabel "panelist"@en ;
    a rdf:Property ;
    rdfs:domain <http://rdaregistry.info/Elements/c/C10006> ;
    rdfs:isDefinedBy <http://rdaregistry.info/Elements/e/> ;
    rdfs:label "has panelist"@en ;
    rdfs:range <http://rdaregistry.info/Elements/c/C10002> ;
    rdfs:subPropertyOf <http://rdaregistry.info/Elements/e/P20039> ;
    owl:inverseOf <http://rdaregistry.info/Elements/a/P50078> ;
    skos:definition "Relates an expression to a performer contributing to an expression of a work by participating in a program (often broadcast) where topics are discussed, usually with participation of experts in fields related to the discussion."@en .

<http://rdaregistry.info/Elements/e/P20020>
    reg:hasUnconstrained <http://rdaregistry.info/Elements/u/P60150> ;
    reg:lexicalAlias <http://rdaregistry.info/Elements/e/instrumentalist.en> ;
    reg:name "instrumentalist"@en ;
    reg:status <http://metadataregistry.org/uri/RegStatus/1001> ;
    rdakit:toolkitDefinition "A performer contributing to an expression of a work by playing a musical instrument."@en ;
    rdakit:toolkitLabel "instrumentalist"@en ;
    a rdf:Property ;
    rdfs:domain <http://rdaregistry.info/Elements/c/C10006> ;
    rdfs:isDefinedBy <http://rdaregistry.info/Elements/e/> ;
    rdfs:label "has instrumentalist"@en ;
    rdfs:range <http://rdaregistry.info/Elements/c/C10002> ;
    rdfs:subPropertyOf <http://rdaregistry.info/Elements/e/P20039> ;
    owl:inverseOf <http://rdaregistry.info/Elements/a/P50079> ;
    skos:definition "Relates an expression to a performer contributing to an expression of a work by playing a musical instrument."@en .

<http://rdaregistry.info/Elements/e/P20021>
    reg:hasUnconstrained <http://rdaregistry.info/Elements/u/P60151> ;
    reg:lexicalAlias <http://rdaregistry.info/Elements/e/commentator.en> ;
    reg:name "commentator"@en ;
    reg:status <http://metadataregistry.org/uri/RegStatus/1001> ;
    rdakit:toolkitDefinition "A performer contributing to an expression of a work by providing interpretation, analysis, or a discussion of the subject matter on a recording, film, or other audiovisual medium."@en ;
    rdakit:toolkitLabel "commentator"@en ;
    a rdf:Property ;
    rdfs:domain <http://rdaregistry.info/Elements/c/C10006> ;
    rdfs:isDefinedBy <http://rdaregistry.info/Elements/e/> ;
    rdfs:label "has commentator"@en ;
    rdfs:range <http://rdaregistry.info/Elements/c/C10002> ;
    rdfs:subPropertyOf <http://rdaregistry.info/Elements/e/P20039> ;
    owl:inverseOf <http://rdaregistry.info/Elements/a/P50080> ;
    skos:definition "Relates an expression to a performer contributing to an expression of a work by providing interpretation, analysis, or a discussion of the subject matter on a recording, film, or other audiovisual medium."@en .

<http://rdaregistry.info/Elements/e/P20022>
    reg:hasUnconstrained <http://rdaregistry.info/Elements/u/P60153> ;
    reg:lexicalAlias <http://rdaregistry.info/Elements/e/narrator.en> ;
    reg:name "narrator"@en ;
    reg:status <http://metadataregistry.org/uri/RegStatus/1001> ;
    rdakit:toolkitDefinition "A performer contributing to an expression of a work by reading alound or giving an account of an act, occurrence, course of events, etc."@en ;
    rdakit:toolkitLabel "narrator"@en ;
    a rdf:Property ;
    rdfs:domain <http://rdaregistry.info/Elements/c/C10006> ;
    rdfs:isDefinedBy <http://rdaregistry.info/Elements/e/> ;
    rdfs:label "has narrator"@en ;
    rdfs:range <http://rdaregistry.info/Elements/c/C10002> ;
    rdfs:subPropertyOf <http://rdaregistry.info/Elements/e/P20039> ;
    owl:inverseOf <http://rdaregistry.info/Elements/a/P50081> ;
    skos:definition "Relates an expression to a performer contributing to an expression of a work by reading aloud or giving an account of an act, occurrence, course of events, etc."@en .

<http://rdaregistry.info/Elements/e/P20023>
    reg:hasUnconstrained <http://rdaregistry.info/Elements/u/P60154> ;
    reg:lexicalAlias <http://rdaregistry.info/Elements/e/storyteller.en> ;
    reg:name "storyteller"@en ;
    reg:status <http://metadataregistry.org/uri/RegStatus/1001> ;
    rdakit:toolkitDefinition "A performer contributing to an expression of a work by relaying a creator"@en ;
    rdakit:toolkitLabel "storyteller"@en ;
    a rdf:Property ;
    rdfs:domain <http://rdaregistry.info/Elements/c/C10006> ;
    rdfs:isDefinedBy <http://rdaregistry.info/Elements/e/> ;
    rdfs:label "has storyteller"@en ;
    rdfs:range <http://rdaregistry.info/Elements/c/C10002> ;
    rdfs:subPropertyOf <http://rdaregistry.info/Elements/e/P20039> ;
    owl:inverseOf <http://rdaregistry.info/Elements/a/P50082> ;
    skos:definition "Relates an expression to a performer contributing to an expression of a work by relaying a creator's original story with dramatic or theatrical interpretation."@en .

<http://rdaregistry.info/Elements/e/P20024>
    reg:hasUnconstrained <http://rdaregistry.info/Elements/u/P60155> ;
    reg:lexicalAlias <http://rdaregistry.info/Elements/e/speaker.en> ;
    reg:name "speaker"@en ;
    reg:status <http://metadataregistry.org/uri/RegStatus/1001> ;
    rdakit:toolkitDefinition "A performer contributing to an expression of a work by speaking words, such as a lecture, speech, etc."@en ;
    rdakit:toolkitLabel "speaker"@en ;
    a rdf:Property ;
    rdfs:domain <http://rdaregistry.info/Elements/c/C10006> ;
    rdfs:isDefinedBy <http://rdaregistry.info/Elements/e/> ;
    rdfs:label "has speaker"@en ;
    rdfs:range <http://rdaregistry.info/Elements/c/C10002> ;
    rdfs:subPropertyOf <http://rdaregistry.info/Elements/e/P20039> ;
    owl:inverseOf <http://rdaregistry.info/Elements/a/P50083> ;
    skos:definition "Relates an expression to a performer contributing to an expression of a work by speaking words, such as a lecture, speech, etc."@en .

<http://rdaregistry.info/Elements/e/P20025>
    reg:hasUnconstrained <http://rdaregistry.info/Elements/u/P60156> ;
    reg:lexicalAlias <http://rdaregistry.info/Elements/e/singer.en> ;
    reg:name "singer"@en ;
    reg:status <http://metadataregistry.org/uri/RegStatus/1001> ;
    rdakit:toolkitDefinition "A performer contributing to an expression of a work by using his/her/their voice, with or without instrumental accompaniment, to produce music."@en ;
    rdakit:toolkitLabel "singer"@en ;
    a rdf:Property ;
    rdfs:domain <http://rdaregistry.info/Elements/c/C10006> ;
    rdfs:isDefinedBy <http://rdaregistry.info/Elements/e/> ;
    rdfs:label "has singer"@en ;
    rdfs:range <http://rdaregistry.info/Elements/c/C10002> ;
    rdfs:subPropertyOf <http://rdaregistry.info/Elements/e/P20039> ;
    owl:inverseOf <http://rdaregistry.info/Elements/a/P50084> ;
    skos:definition "Relates an expression to a performer contributing to an expression of a work by using his/her/their voice, with or without instrumental accompaniment, to produce music."@en ;
    skos:scopeNote "A singer's performance may or may not include actual words."@en .

<http://rdaregistry.info/Elements/e/P20026>
    reg:hasUnconstrained <http://rdaregistry.info/Elements/u/P60426> ;
    reg:lexicalAlias <http://rdaregistry.info/Elements/e/composerExpression.en> ;
    reg:name "composerExpression"@en ;
    reg:status <http://metadataregistry.org/uri/RegStatus/1001> ;
    rdakit:toolkitDefinition "A person, family, or corporate body contributing to an expression by adding music to a work that originally lacked it, by composing new music to substitute for the original music, or by composing new music to supplement the existing music."@en ;
    rdakit:toolkitLabel "composer (expression)"@en ;
    a rdf:Property ;
    rdfs:domain <http://rdaregistry.info/Elements/c/C10006> ;
    rdfs:isDefinedBy <http://rdaregistry.info/Elements/e/> ;
    rdfs:label "has composer (expression)"@en ;
    rdfs:range <http://rdaregistry.info/Elements/c/C10002> ;
    rdfs:subPropertyOf <http://rdaregistry.info/Elements/e/P20053> ;
    owl:inverseOf <http://rdaregistry.info/Elements/a/P50134> ;
    skos:definition "Relates an expression to a person, family, or corporate body contributing to an expression by adding music to a work that originally lacked it, by composing new music to substitute for the original music, or by composing new music to supplement the existing music."@en .

<http://rdaregistry.info/Elements/e/P20027>
    reg:hasUnconstrained <http://rdaregistry.info/Elements/u/P60377> ;
    reg:lexicalAlias <http://rdaregistry.info/Elements/e/surveyor.en> ;
    reg:name "surveyor"@en ;
    reg:status <http://metadataregistry.org/uri/RegStatus/1001> ;
    rdakit:toolkitDefinition "A person, family, or corporate body contributing to an expression of a cartographic work by providing measurements or dimensional relationships for the geographic area represented."@en ;
    rdakit:toolkitLabel "surveyor"@en ;
    a rdf:Property ;
    rdfs:domain <http://rdaregistry.info/Elements/c/C10006> ;
    rdfs:isDefinedBy <http://rdaregistry.info/Elements/e/> ;
    rdfs:label "has surveyor"@en ;
    rdfs:range <http://rdaregistry.info/Elements/c/C10002> ;
    rdfs:subPropertyOf <http://rdaregistry.info/Elements/e/P20053> ;
    owl:inverseOf <http://rdaregistry.info/Elements/a/P50135> ;
    skos:definition "Relates an expression to a person, family, or corporate body contributing to an expression of a cartographic work by providing measurements or dimensional relationships for the geographic area represented."@en .

<http://rdaregistry.info/Elements/e/P20028>
    reg:hasUnconstrained <http://rdaregistry.info/Elements/u/P60378> ;
    reg:lexicalAlias <http://rdaregistry.info/Elements/e/animator.en> ;
    reg:name "animator"@en ;
    reg:status <http://metadataregistry.org/uri/RegStatus/1001> ;
    rdakit:toolkitDefinition "A person, family, or corporate body contributing to an expression of a moving image work or computer program by giving apparent movement to inanimate objects or drawings."@en ;
    rdakit:toolkitLabel "animator"@en ;
    a rdf:Property ;
    rdfs:domain <http://rdaregistry.info/Elements/c/C10006> ;
    rdfs:isDefinedBy <http://rdaregistry.info/Elements/e/> ;
    rdfs:label "has animator"@en ;
    rdfs:range <http://rdaregistry.info/Elements/c/C10002> ;
    rdfs:subPropertyOf <http://rdaregistry.info/Elements/e/P20053> ;
    owl:inverseOf <http://rdaregistry.info/Elements/a/P50136> ;
    skos:definition "Relates an expression to a person, family, or corporate body contributing to an expression of a moving image work or computer program by giving apparent movement to inanimate objects or drawings."@en .

<http://rdaregistry.info/Elements/e/P20029>
    reg:hasUnconstrained <http://rdaregistry.info/Elements/u/P60379> ;
    reg:lexicalAlias <http://rdaregistry.info/Elements/e/arrangerOfMusic.en> ;
    reg:name "arrangerOfMusic"@en ;
    reg:status <http://metadataregistry.org/uri/RegStatus/1001> ;
    rdakit:toolkitDefinition "A person, family, or corporate body contributing to an expression of a musical work by rewriting the composition for a medium of performance different from that for which the work was originally intended."@en ;
    rdakit:toolkitLabel "arranger of music"@en ;
    a rdf:Property ;
    rdfs:domain <http://rdaregistry.info/Elements/c/C10006> ;
    rdfs:isDefinedBy <http://rdaregistry.info/Elements/e/> ;
    rdfs:label "has arranger of music"@en ;
    rdfs:range <http://rdaregistry.info/Elements/c/C10002> ;
    rdfs:subPropertyOf <http://rdaregistry.info/Elements/e/P20053> ;
    owl:inverseOf <http://rdaregistry.info/Elements/a/P50137> ;
    skos:definition "Relates an expression to a person, family, or corporate body contributing to an expression of a musical work by rewriting the composition for a medium of performance different from that for which the work was originally intended."@en ;
    skos:scopeNote "An arranger of music may also modify the work for the same medium of performance, etc., keeping the musical substance of the original composition essentially unchanged."@en .

<http://rdaregistry.info/Elements/e/P20030>
    reg:hasSubproperty <http://rdaregistry.info/Elements/e/P20068> ;
    reg:hasUnconstrained <http://rdaregistry.info/Elements/u/P60380> ;
    reg:lexicalAlias <http://rdaregistry.info/Elements/e/writerOfAddedText.en> ;
    reg:name "writerOfAddedText"@en ;
    reg:status <http://metadataregistry.org/uri/RegStatus/1001> ;
    rdakit:toolkitDefinition "A person, family, or corporate body contributing to an expression of a primarily non-textual work by providing text for the non-textual work (e.g., writing captions for photographs, descriptions of maps)."@en ;
    rdakit:toolkitLabel "writer of added text"@en ;
    a rdf:Property ;
    rdfs:domain <http://rdaregistry.info/Elements/c/C10006> ;
    rdfs:isDefinedBy <http://rdaregistry.info/Elements/e/> ;
    rdfs:label "has writer of added text"@en ;
    rdfs:range <http://rdaregistry.info/Elements/c/C10002> ;
    rdfs:subPropertyOf <http://rdaregistry.info/Elements/e/P20046> ;
    owl:inverseOf <http://rdaregistry.info/Elements/a/P50138> ;
    skos:definition "Relates an expression to a person, family, or corporate body contributing to an expression of a primarily non-textual work by providing text for the non-textual work (e.g., writing captions for photographs, descriptions of maps)."@en .

<http://rdaregistry.info/Elements/e/P20031>
    reg:hasUnconstrained <http://rdaregistry.info/Elements/u/P60399> ;
    reg:lexicalAlias <http://rdaregistry.info/Elements/e/stageDirector.en> ;
    reg:name "stageDirector"@en ;
    reg:status <http://metadataregistry.org/uri/RegStatus/1001> ;
    rdakit:toolkitDefinition "A person, family, or corporate body contributing to an expression of a stage work through the general management and supervision of a performance."@en ;
    rdakit:toolkitLabel "stage director"@en ;
    a rdf:Property ;
    rdfs:domain <http://rdaregistry.info/Elements/c/C10006> ;
    rdfs:isDefinedBy <http://rdaregistry.info/Elements/e/> ;
    rdfs:label "has stage director"@en ;
    rdfs:range <http://rdaregistry.info/Elements/c/C10002> ;
    rdfs:subPropertyOf <http://rdaregistry.info/Elements/e/P20053> ;
    owl:inverseOf <http://rdaregistry.info/Elements/a/P50139> ;
    skos:definition "Relates an expression to a person, family, or corporate body contributing to an expression of a stage work through the general management and supervision of a performance."@en .

<http://rdaregistry.info/Elements/e/P20032>
    reg:hasUnconstrained <http://rdaregistry.info/Elements/u/P60430> ;
    reg:lexicalAlias <http://rdaregistry.info/Elements/e/interviewerExpression.en> ;
    reg:name "interviewerExpression"@en ;
    reg:status <http://metadataregistry.org/uri/RegStatus/1001> ;
    rdakit:toolkitDefinition "A person, family, or corporate body contributing to an expression of a work by acting as an interviewer, reporter, pollster, or some other information gathering agent."@en ;
    rdakit:toolkitLabel "interviewer (expression)"@en ;
    a rdf:Property ;
    rdfs:domain <http://rdaregistry.info/Elements/c/C10006> ;
    rdfs:isDefinedBy <http://rdaregistry.info/Elements/e/> ;
    rdfs:label "has interviewer (expression)"@en ;
    rdfs:range <http://rdaregistry.info/Elements/c/C10002> ;
    rdfs:subPropertyOf <http://rdaregistry.info/Elements/e/P20053> ;
    owl:inverseOf <http://rdaregistry.info/Elements/a/P50140> ;
    skos:definition "Relates an expression to a person, family, or corporate body contributing to an expression of a work by acting as an interviewer, reporter, pollster, or some other information gathering agent."@en .

<http://rdaregistry.info/Elements/e/P20033>
    reg:hasUnconstrained <http://rdaregistry.info/Elements/u/P60381> ;
    reg:lexicalAlias <http://rdaregistry.info/Elements/e/draftsman.en> ;
    reg:name "draftsman"@en ;
    reg:status <http://metadataregistry.org/uri/RegStatus/1001> ;
    rdakit:toolkitDefinition "A person, family, or corporate body contributing to an expression of a work by an architect, inventor, etc., by making detailed plans or drawings for buildings, ships, aircraft, machines, objects, etc."@en ;
    rdakit:toolkitLabel "draftsman"@en ;
    a rdf:Property ;
    rdfs:domain <http://rdaregistry.info/Elements/c/C10006> ;
    rdfs:isDefinedBy <http://rdaregistry.info/Elements/e/> ;
    rdfs:label "has draftsman"@en ;
    rdfs:range <http://rdaregistry.info/Elements/c/C10002> ;
    rdfs:subPropertyOf <http://rdaregistry.info/Elements/e/P20053> ;
    owl:inverseOf <http://rdaregistry.info/Elements/a/P50141> ;
    skos:definition "Relates an expression to a person, family, or corporate body contributing to an expression of a work by an architect, inventor, etc., by making detailed plans or drawings for buildings, ships, aircraft, machines, objects, etc."@en .

<http://rdaregistry.info/Elements/e/P20034>
    reg:hasUnconstrained <http://rdaregistry.info/Elements/u/P60382> ;
    reg:lexicalAlias <http://rdaregistry.info/Elements/e/transcriber.en> ;
    reg:name "transcriber"@en ;
    reg:status <http://metadataregistry.org/uri/RegStatus/1001> ;
    rdakit:toolkitDefinition "A person, family, or corporate body contributing to an expression of a work by writing down or notating unwritten or unnotated content, or by changing it from one system of notation to another."@en ;
    rdakit:toolkitLabel "transcriber"@en ;
    a rdf:Property ;
    rdfs:domain <http://rdaregistry.info/Elements/c/C10006> ;
    rdfs:isDefinedBy <http://rdaregistry.info/Elements/e/> ;
    rdfs:label "has transcriber"@en ;
    rdfs:range <http://rdaregistry.info/Elements/c/C10002> ;
    rdfs:subPropertyOf <http://rdaregistry.info/Elements/e/P20053> ;
    owl:inverseOf <http://rdaregistry.info/Elements/a/P50142> ;
    skos:definition "Relates an expression to a person, family, or corporate body contributing to an expression of a work by writing down or notating unwritten or unnotated content, or by changing it from one system of notation to another."@en .

<http://rdaregistry.info/Elements/e/P20035>
    reg:hasUnconstrained <http://rdaregistry.info/Elements/u/P60383> ;
    reg:lexicalAlias <http://rdaregistry.info/Elements/e/musicalDirector.en> ;
    reg:name "musicalDirector"@en ;
    reg:status <http://metadataregistry.org/uri/RegStatus/1001> ;
    rdakit:toolkitDefinition "A person, family, or corporate body contributing to an expression of a work by coordinating the activities of the composer, the sound editor, and sound mixers for a moving image production or for a musical or dramatic presentation or entertainment."@en ;
    rdakit:toolkitLabel "musical director"@en ;
    a rdf:Property ;
    rdfs:domain <http://rdaregistry.info/Elements/c/C10006> ;
    rdfs:isDefinedBy <http://rdaregistry.info/Elements/e/> ;
    rdfs:label "has musical director"@en ;
    rdfs:range <http://rdaregistry.info/Elements/c/C10002> ;
    rdfs:subPropertyOf <http://rdaregistry.info/Elements/e/P20053> ;
    owl:inverseOf <http://rdaregistry.info/Elements/a/P50143> ;
    skos:definition "Relates an expression to a person, family, or corporate body contributing to an expression of a work by coordinating the activities of the composer, the sound editor, and sound mixers for a moving image production or for a musical or dramatic presentation or entertainment."@en .

<http://rdaregistry.info/Elements/e/P20036>
    reg:hasUnconstrained <http://rdaregistry.info/Elements/u/P60384> ;
    reg:lexicalAlias <http://rdaregistry.info/Elements/e/costumeDesigner.en> ;
    reg:name "costumeDesigner"@en ;
    reg:status <http://metadataregistry.org/uri/RegStatus/1001> ;
    rdakit:toolkitDefinition "A person, family, or corporate body contributing to an expression of a work by designing the costumes for a moving image production or for a musical or dramatic presentation or entertainment."@en ;
    rdakit:toolkitLabel "costume designer"@en ;
    a rdf:Property ;
    rdfs:domain <http://rdaregistry.info/Elements/c/C10006> ;
    rdfs:isDefinedBy <http://rdaregistry.info/Elements/e/> ;
    rdfs:label "has costume designer"@en ;
    rdfs:range <http://rdaregistry.info/Elements/c/C10002> ;
    rdfs:subPropertyOf <http://rdaregistry.info/Elements/e/P20053> ;
    owl:inverseOf <http://rdaregistry.info/Elements/a/P50144> ;
    skos:definition "Relates an expression to a person, family, or corporate body contributing to an expression of a work by designing the costumes for a moving image production or for a musical or dramatic presentation or entertainment."@en .

<http://rdaregistry.info/Elements/e/P20037>
    reg:hasUnconstrained <http://rdaregistry.info/Elements/u/P60385> ;
    reg:lexicalAlias <http://rdaregistry.info/Elements/e/translator.en> ;
    reg:name "translator"@en ;
    reg:status <http://metadataregistry.org/uri/RegStatus/1001> ;
    rdakit:toolkitDefinition "A person, family, or corporate body contributing to an expression of a work by expressing the linguistic content of the work in a language different from that of previous expressions of the original work."@en ;
    rdakit:toolkitLabel "translator"@en ;
    a rdf:Property ;
    rdfs:domain <http://rdaregistry.info/Elements/c/C10006> ;
    rdfs:isDefinedBy <http://rdaregistry.info/Elements/e/> ;
    rdfs:label "has translator"@en ;
    rdfs:range <http://rdaregistry.info/Elements/c/C10002> ;
    rdfs:subPropertyOf <http://rdaregistry.info/Elements/e/P20053> ;
    owl:inverseOf <http://rdaregistry.info/Elements/a/P50145> ;
    skos:definition "Relates an expression to a person, family, or corporate body contributing to an expression of a work by expressing the linguistic content of the work in a language different from that of previous expressions of the original work."@en ;
    skos:scopeNote "A translator may also translate linguistic content between forms of the same language from different time periods."@en .

<http://rdaregistry.info/Elements/e/P20038>
    reg:hasUnconstrained <http://rdaregistry.info/Elements/u/P60386> ;
    reg:lexicalAlias <http://rdaregistry.info/Elements/e/artDirector.en> ;
    reg:name "artDirector"@en ;
    reg:status <http://metadataregistry.org/uri/RegStatus/1001> ;
    rdakit:toolkitDefinition "A person, family, or corporate body contributing to an expression of a work by overseeing the artists and craftspeople who build the sets for moving image productions."@en ;
    rdakit:toolkitLabel "art director"@en ;
    a rdf:Property ;
    rdfs:domain <http://rdaregistry.info/Elements/c/C10006> ;
    rdfs:isDefinedBy <http://rdaregistry.info/Elements/e/> ;
    rdfs:label "has art director"@en ;
    rdfs:range <http://rdaregistry.info/Elements/c/C10002> ;
    rdfs:subPropertyOf <http://rdaregistry.info/Elements/e/P20053> ;
    owl:inverseOf <http://rdaregistry.info/Elements/a/P50146> ;
    skos:definition "Relates an expression to a person, family, or corporate body contributing to an expression of a work by overseeing the artists and craftspeople who build the sets for moving image productions."@en .

<http://rdaregistry.info/Elements/e/P20039>
    reg:hasSubproperty <http://rdaregistry.info/Elements/e/P20011>, <http://rdaregistry.info/Elements/e/P20012>, <http://rdaregistry.info/Elements/e/P20013>, <http://rdaregistry.info/Elements/e/P20014>, <http://rdaregistry.info/Elements/e/P20015>, <http://rdaregistry.info/Elements/e/P20016>, <http://rdaregistry.info/Elements/e/P20017>, <http://rdaregistry.info/Elements/e/P20018>, <http://rdaregistry.info/Elements/e/P20019>, <http://rdaregistry.info/Elements/e/P20020>, <http://rdaregistry.info/Elements/e/P20021>, <http://rdaregistry.info/Elements/e/P20022>, <http://rdaregistry.info/Elements/e/P20023>, <http://rdaregistry.info/Elements/e/P20024>, <http://rdaregistry.info/Elements/e/P20025> ;
    reg:hasUnconstrained <http://rdaregistry.info/Elements/u/P60387> ;
    reg:lexicalAlias <http://rdaregistry.info/Elements/e/performer.en> ;
    reg:name "performer"@en ;
    reg:status <http://metadataregistry.org/uri/RegStatus/1001> ;
    rdakit:toolkitDefinition "A person, family, or corporate body contributing to an expression of a work by performing music, acting, dancing, speaking, etc., often in a musical or dramatic presentation, etc."@en ;
    rdakit:toolkitLabel "performer"@en ;
    a rdf:Property ;
    rdfs:domain <http://rdaregistry.info/Elements/c/C10006> ;
    rdfs:isDefinedBy <http://rdaregistry.info/Elements/e/> ;
    rdfs:label "has performer"@en ;
    rdfs:range <http://rdaregistry.info/Elements/c/C10002> ;
    rdfs:subPropertyOf <http://rdaregistry.info/Elements/e/P20053> ;
    owl:inverseOf <http://rdaregistry.info/Elements/a/P50147> ;
    skos:definition "Relates an expression to a person, family, or corporate body contributing to an expression of a work by performing music, acting, dancing, speaking, etc., often in a musical or dramatic presentation, etc."@en .

<http://rdaregistry.info/Elements/e/P20040>
    reg:hasUnconstrained <http://rdaregistry.info/Elements/u/P60388> ;
    reg:lexicalAlias <http://rdaregistry.info/Elements/e/courtReporter.en> ;
    reg:name "courtReporter"@en ;
    reg:status <http://metadataregistry.org/uri/RegStatus/1001> ;
    rdakit:toolkitDefinition "A person, family, or corporate body contributing to an expression of a work by preparing a court's opinions for publication."@en ;
    rdakit:toolkitLabel "court reporter"@en ;
    a rdf:Property ;
    rdfs:domain <http://rdaregistry.info/Elements/c/C10006> ;
    rdfs:isDefinedBy <http://rdaregistry.info/Elements/e/> ;
    rdfs:label "has court reporter"@en ;
    rdfs:range <http://rdaregistry.info/Elements/c/C10002> ;
    rdfs:subPropertyOf <http://rdaregistry.info/Elements/e/P20053> ;
    owl:inverseOf <http://rdaregistry.info/Elements/a/P50148> ;
    skos:definition "Relates an expression to a person, family, or corporate body contributing to an expression of a work by preparing a court's opinions for publication."@en .

<http://rdaregistry.info/Elements/e/P20041>
    reg:hasUnconstrained <http://rdaregistry.info/Elements/u/P60389> ;
    reg:lexicalAlias <http://rdaregistry.info/Elements/e/writerOfPreface.en> ;
    reg:name "writerOfPreface"@en ;
    reg:status <http://metadataregistry.org/uri/RegStatus/1001> ;
    rdakit:toolkitDefinition "A person, family, or corporate body contributing to an expression of a work by providing a preface to the original work."@en ;
    rdakit:toolkitLabel "writer of preface"@en ;
    a rdf:Property ;
    rdfs:domain <http://rdaregistry.info/Elements/c/C10006> ;
    rdfs:isDefinedBy <http://rdaregistry.info/Elements/e/> ;
    rdfs:label "has writer of preface"@en ;
    rdfs:range <http://rdaregistry.info/Elements/c/C10002> ;
    rdfs:subPropertyOf <http://rdaregistry.info/Elements/e/P20046> ;
    owl:inverseOf <http://rdaregistry.info/Elements/a/P50149> ;
    skos:definition "Relates an expression to a person, family, or corporate body contributing to an expression of a work by providing a preface to the original work."@en .

<http://rdaregistry.info/Elements/e/P20042>
    reg:hasUnconstrained <http://rdaregistry.info/Elements/u/P60425> ;
    reg:lexicalAlias <http://rdaregistry.info/Elements/e/cartographerExpression.en> ;
    reg:name "cartographerExpression"@en ;
    reg:status <http://metadataregistry.org/uri/RegStatus/1001> ;
    rdakit:toolkitDefinition "A person, family, or corporate body contributing to an expression of a work by providing additional cartography, or by modifying the previous cartography."@en ;
    rdakit:toolkitLabel "cartographer (expression)"@en ;
    a rdf:Property ;
    rdfs:domain <http://rdaregistry.info/Elements/c/C10006> ;
    rdfs:isDefinedBy <http://rdaregistry.info/Elements/e/> ;
    rdfs:label "has cartographer (expression)"@en ;
    rdfs:range <http://rdaregistry.info/Elements/c/C10002> ;
    rdfs:subPropertyOf <http://rdaregistry.info/Elements/e/P20053> ;
    owl:inverseOf <http://rdaregistry.info/Elements/a/P50150> ;
    skos:definition "Relates an expression to a person, family, or corporate body contributing to an expression of a work by providing additional cartography, or by modifying the previous cartography."@en .

<http://rdaregistry.info/Elements/e/P20043>
    reg:hasUnconstrained <http://rdaregistry.info/Elements/u/P60433> ;
    reg:lexicalAlias <http://rdaregistry.info/Elements/e/choreographerExpression.en> ;
    reg:name "choreographerExpression"@en ;
    reg:status <http://metadataregistry.org/uri/RegStatus/1001> ;
    rdakit:toolkitDefinition "A person, family, or corporate body contributing to an expression of a work by providing additional choreography, or by modifying the previous choreography."@en ;
    rdakit:toolkitLabel "choreographer (expression)"@en ;
    a rdf:Property ;
    rdfs:domain <http://rdaregistry.info/Elements/c/C10006> ;
    rdfs:isDefinedBy <http://rdaregistry.info/Elements/e/> ;
    rdfs:label "has choreographer (expression)"@en ;
    rdfs:range <http://rdaregistry.info/Elements/c/C10002> ;
    rdfs:subPropertyOf <http://rdaregistry.info/Elements/e/P20053> ;
    owl:inverseOf <http://rdaregistry.info/Elements/a/P50151> ;
    skos:definition "Relates an expression to a person, family, or corporate body contributing to an expression of a work by providing additional choreography, or by modifying the previous choreography."@en .

<http://rdaregistry.info/Elements/e/P20044>
    reg:hasUnconstrained <http://rdaregistry.info/Elements/u/P60390> ;
    reg:lexicalAlias <http://rdaregistry.info/Elements/e/writerOfAddedCommentary.en> ;
    reg:name "writerOfAddedCommentary"@en ;
    reg:status <http://metadataregistry.org/uri/RegStatus/1001> ;
    rdakit:toolkitDefinition "A person, family, or corporate body contributing to an expression of a work by providing an interpretation or critical explanation of the original work."@en ;
    rdakit:toolkitLabel "writer of added commentary"@en ;
    a rdf:Property ;
    rdfs:domain <http://rdaregistry.info/Elements/c/C10006> ;
    rdfs:isDefinedBy <http://rdaregistry.info/Elements/e/> ;
    rdfs:label "has writer of added commentary"@en ;
    rdfs:range <http://rdaregistry.info/Elements/c/C10002> ;
    rdfs:subPropertyOf <http://rdaregistry.info/Elements/e/P20046> ;
    owl:inverseOf <http://rdaregistry.info/Elements/a/P50152> ;
    skos:definition "Relates an expression to a person, family, or corporate body contributing to an expression of a work by providing an interpretation or critical explanation of the original work."@en .

<http://rdaregistry.info/Elements/e/P20045>
    reg:hasUnconstrained <http://rdaregistry.info/Elements/u/P60391> ;
    reg:lexicalAlias <http://rdaregistry.info/Elements/e/writerOfIntroduction.en> ;
    reg:name "writerOfIntroduction"@en ;
    reg:status <http://metadataregistry.org/uri/RegStatus/1001> ;
    rdakit:toolkitDefinition "A person, family, or corporate body contributing to an expression of a work by providing an introduction to the original work."@en ;
    rdakit:toolkitLabel "writer of introduction"@en ;
    a rdf:Property ;
    rdfs:domain <http://rdaregistry.info/Elements/c/C10006> ;
    rdfs:isDefinedBy <http://rdaregistry.info/Elements/e/> ;
    rdfs:label "has writer of introduction"@en ;
    rdfs:range <http://rdaregistry.info/Elements/c/C10002> ;
    rdfs:subPropertyOf <http://rdaregistry.info/Elements/e/P20046> ;
    owl:inverseOf <http://rdaregistry.info/Elements/a/P50153> ;
    skos:definition "Relates an expression to a person, family, or corporate body contributing to an expression of a work by providing an introduction to the original work."@en .

<http://rdaregistry.info/Elements/e/P20046>
    reg:hasSubproperty <http://rdaregistry.info/Elements/e/P20030>, <http://rdaregistry.info/Elements/e/P20041>, <http://rdaregistry.info/Elements/e/P20044>, <http://rdaregistry.info/Elements/e/P20045>, <http://rdaregistry.info/Elements/e/P20275> ;
    reg:hasUnconstrained <http://rdaregistry.info/Elements/u/P60392> ;
    reg:lexicalAlias <http://rdaregistry.info/Elements/e/writerOfSupplementaryTextualContent.en> ;
    reg:name "writerOfSupplementaryTextualContent"@en ;
    reg:status <http://metadataregistry.org/uri/RegStatus/1001> ;
    rdakit:toolkitDefinition "A person, family, or corporate body contributing to an expression of a work by providing supplementary textual content (e.g., an appendix, an introduction, a preface) to the original work."@en ;
    rdakit:toolkitLabel "writer of supplementary textual content"@en ;
    a rdf:Property ;
    rdfs:domain <http://rdaregistry.info/Elements/c/C10006> ;
    rdfs:isDefinedBy <http://rdaregistry.info/Elements/e/> ;
    rdfs:label "has writer of supplementary textual content"@en ;
    rdfs:range <http://rdaregistry.info/Elements/c/C10002> ;
    rdfs:subPropertyOf <http://rdaregistry.info/Elements/e/P20053> ;
    owl:inverseOf <http://rdaregistry.info/Elements/a/P50154> ;
    skos:definition "Relates an expression to a person, family, or corporate body contributing to an expression of a work by providing supplementary textual content (e.g., an appendix, an introduction, a preface) to the original work."@en .

<http://rdaregistry.info/Elements/e/P20047>
    reg:hasUnconstrained <http://rdaregistry.info/Elements/u/P60432> ;
    reg:lexicalAlias <http://rdaregistry.info/Elements/e/intervieweeExpression.en> ;
    reg:name "intervieweeExpression"@en ;
    reg:status <http://metadataregistry.org/uri/RegStatus/1001> ;
    rdakit:toolkitDefinition "A person, family, or corporate body contributing to an expression of a work by responding to an interviewer, usually a reporter, pollster, or some other information gathering agent."@en ;
    rdakit:toolkitLabel "interviewee (expression)"@en ;
    a rdf:Property ;
    rdfs:domain <http://rdaregistry.info/Elements/c/C10006> ;
    rdfs:isDefinedBy <http://rdaregistry.info/Elements/e/> ;
    rdfs:label "has interviewee (expression)"@en ;
    rdfs:range <http://rdaregistry.info/Elements/c/C10002> ;
    rdfs:subPropertyOf <http://rdaregistry.info/Elements/e/P20053> ;
    owl:inverseOf <http://rdaregistry.info/Elements/a/P50155> ;
    skos:definition "Relates an expression to a person, family, or corporate body contributing to an expression of a work by responding to an interviewer, usually a reporter, pollster, or some other information gathering agent."@en .

<http://rdaregistry.info/Elements/e/P20048>
    reg:hasUnconstrained <http://rdaregistry.info/Elements/u/P60393> ;
    reg:lexicalAlias <http://rdaregistry.info/Elements/e/editor.en> ;
    reg:name "editor"@en ;
    reg:status <http://metadataregistry.org/uri/RegStatus/1001> ;
    rdakit:toolkitDefinition "A person, family, or corporate body contributing to an expression of a work by revising or clarifying the content, e.g., adding an introduction, notes, or other critical matter."@en ;
    rdakit:toolkitLabel "editor"@en ;
    a rdf:Property ;
    rdfs:domain <http://rdaregistry.info/Elements/c/C10006> ;
    rdfs:isDefinedBy <http://rdaregistry.info/Elements/e/> ;
    rdfs:label "has editor"@en ;
    rdfs:range <http://rdaregistry.info/Elements/c/C10002> ;
    rdfs:subPropertyOf <http://rdaregistry.info/Elements/e/P20053> ;
    owl:inverseOf <http://rdaregistry.info/Elements/a/P50156> ;
    skos:definition "Relates an expression to a person, family, or corporate body contributing to an expression of a work by revising or clarifying the content, e.g., adding an introduction, notes, or other critical matter."@en ;
    skos:scopeNote "An editor may also prepare an expression of a work for production, publication, or distribution."@en .

<http://rdaregistry.info/Elements/e/P20049>
    reg:hasUnconstrained <http://rdaregistry.info/Elements/u/P60394> ;
    reg:lexicalAlias <http://rdaregistry.info/Elements/e/abridger.en> ;
    reg:name "abridger"@en ;
    reg:status <http://metadataregistry.org/uri/RegStatus/1001> ;
    rdakit:toolkitDefinition "A person, family, or corporate body contributing to an expression of a work by shortening or condensing the original work but leaving the nature and content of the original work substantially unchanged."@en ;
    rdakit:toolkitLabel "abridger"@en ;
    a rdf:Property ;
    rdfs:domain <http://rdaregistry.info/Elements/c/C10006> ;
    rdfs:isDefinedBy <http://rdaregistry.info/Elements/e/> ;
    rdfs:label "has abridger"@en ;
    rdfs:range <http://rdaregistry.info/Elements/c/C10002> ;
    rdfs:subPropertyOf <http://rdaregistry.info/Elements/e/P20053> ;
    owl:inverseOf <http://rdaregistry.info/Elements/a/P50157> ;
    skos:definition "Relates an expression to a person, family, or corporate body contributing to an expression of a work by shortening or condensing the original work but leaving the nature and content of the original work substantially unchanged."@en .

<http://rdaregistry.info/Elements/e/P20050>
    reg:hasUnconstrained <http://rdaregistry.info/Elements/u/P60395> ;
    reg:lexicalAlias <http://rdaregistry.info/Elements/e/recordingEngineer.en> ;
    reg:name "recordingEngineer"@en ;
    reg:status <http://metadataregistry.org/uri/RegStatus/1001> ;
    rdakit:toolkitDefinition "A person, family, or corporate body contributing to an expression of a work by supervising the technical aspects of a sound or video recording session."@en ;
    rdakit:toolkitLabel "recording engineer"@en ;
    a rdf:Property ;
    rdfs:domain <http://rdaregistry.info/Elements/c/C10006> ;
    rdfs:isDefinedBy <http://rdaregistry.info/Elements/e/> ;
    rdfs:label "has recording engineer"@en ;
    rdfs:range <http://rdaregistry.info/Elements/c/C10002> ;
    rdfs:subPropertyOf <http://rdaregistry.info/Elements/e/P20053> ;
    owl:inverseOf <http://rdaregistry.info/Elements/a/P50158> ;
    skos:definition "Relates an expression to a person, family, or corporate body contributing to an expression of a work by supervising the technical aspects of a sound or video recording session."@en .

<http://rdaregistry.info/Elements/e/P20051>
    reg:hasSubproperty <http://rdaregistry.info/Elements/e/P20259> ;
    reg:hasUnconstrained <http://rdaregistry.info/Elements/u/P60396> ;
    reg:lexicalAlias <http://rdaregistry.info/Elements/e/illustrator.en> ;
    reg:name "illustrator"@en ;
    reg:status <http://metadataregistry.org/uri/RegStatus/1001> ;
    rdakit:toolkitDefinition "A person, family, or corporate body contributing to an expression of a work by supplementing the primary content with drawings, diagrams, photographs, etc."@en ;
    rdakit:toolkitLabel "illustrator"@en ;
    a rdf:Property ;
    rdfs:domain <http://rdaregistry.info/Elements/c/C10006> ;
    rdfs:isDefinedBy <http://rdaregistry.info/Elements/e/> ;
    rdfs:label "has illustrator"@en ;
    rdfs:range <http://rdaregistry.info/Elements/c/C10002> ;
    rdfs:subPropertyOf <http://rdaregistry.info/Elements/e/P20053> ;
    owl:inverseOf <http://rdaregistry.info/Elements/a/P50159> ;
    skos:definition "Relates an expression to a person, family, or corporate body contributing to an expression of a work by supplementing the primary content with drawings, diagrams, photographs, etc."@en .

<http://rdaregistry.info/Elements/e/P20052>
    reg:hasUnconstrained <http://rdaregistry.info/Elements/u/P60397> ;
    reg:lexicalAlias <http://rdaregistry.info/Elements/e/recordist.en> ;
    reg:name "recordist"@en ;
    reg:status <http://metadataregistry.org/uri/RegStatus/1001> ;
    rdakit:toolkitDefinition "A person, family, or corporate body contributing to an expression of a work by using a recording device to capture sound and/or video during a recording session, including field recordings of natural sounds, folkloric events, music, etc."@en ;
    rdakit:toolkitLabel "recordist"@en ;
    a rdf:Property ;
    rdfs:domain <http://rdaregistry.info/Elements/c/C10006> ;
    rdfs:isDefinedBy <http://rdaregistry.info/Elements/e/> ;
    rdfs:label "has recordist"@en ;
    rdfs:range <http://rdaregistry.info/Elements/c/C10002> ;
    rdfs:subPropertyOf <http://rdaregistry.info/Elements/e/P20053> ;
    owl:inverseOf <http://rdaregistry.info/Elements/a/P50160> ;
    skos:definition "Relates an expression to a person, family, or corporate body contributing to an expression of a work by using a recording device to capture sound and/or video during a recording session, including field recordings of natural sounds, folkloric events, music, etc."@en .

<http://rdaregistry.info/Elements/e/P20053>
    reg:hasSubproperty <http://rdaregistry.info/Elements/e/P20026>, <http://rdaregistry.info/Elements/e/P20027>, <http://rdaregistry.info/Elements/e/P20028>, <http://rdaregistry.info/Elements/e/P20029>, <http://rdaregistry.info/Elements/e/P20031>, <http://rdaregistry.info/Elements/e/P20032>, <http://rdaregistry.info/Elements/e/P20033>, <http://rdaregistry.info/Elements/e/P20034>, <http://rdaregistry.info/Elements/e/P20035>, <http://rdaregistry.info/Elements/e/P20036>, <http://rdaregistry.info/Elements/e/P20037>, <http://rdaregistry.info/Elements/e/P20038>, <http://rdaregistry.info/Elements/e/P20039>, <http://rdaregistry.info/Elements/e/P20040>, <http://rdaregistry.info/Elements/e/P20042>, <http://rdaregistry.info/Elements/e/P20043>, <http://rdaregistry.info/Elements/e/P20046>, <http://rdaregistry.info/Elements/e/P20047>, <http://rdaregistry.info/Elements/e/P20048>, <http://rdaregistry.info/Elements/e/P20049>, <http://rdaregistry.info/Elements/e/P20050>, <http://rdaregistry.info/Elements/e/P20051>, <http://rdaregistry.info/Elements/e/P20052>, <http://rdaregistry.info/Elements/e/P20054>, <http://rdaregistry.info/Elements/e/P20055>, <http://rdaregistry.info/Elements/e/P20056>, <http://rdaregistry.info/Elements/e/P20058>, <http://rdaregistry.info/Elements/e/P20257>, <http://rdaregistry.info/Elements/e/P20258>, <http://rdaregistry.info/Elements/e/P20276>, <http://rdaregistry.info/Elements/e/P20277>, <http://rdaregistry.info/Elements/e/P20279>, <http://rdaregistry.info/Elements/e/P20280>, <http://rdaregistry.info/Elements/e/P20283>, <http://rdaregistry.info/Elements/e/P20284> ;
    reg:hasUnconstrained <http://rdaregistry.info/Elements/u/P60398> ;
    reg:lexicalAlias <http://rdaregistry.info/Elements/e/contributor.en> ;
    reg:name "contributor"@en ;
    reg:status <http://metadataregistry.org/uri/RegStatus/1001> ;
    rdakit:instructionNumber "20.2" ;
    rdakit:toolkitDefinition "A person, family, or corporate body contributing to an expression."@en ;
    rdakit:toolkitLabel "contributor"@en ;
    a rdf:Property ;
    rdfs:domain <http://rdaregistry.info/Elements/c/C10006> ;
    rdfs:isDefinedBy <http://rdaregistry.info/Elements/e/> ;
    rdfs:label "has contributor"@en ;
    rdfs:range <http://rdaregistry.info/Elements/c/C10002> ;
    owl:inverseOf <http://rdaregistry.info/Elements/a/P50161> ;
    skos:definition "Relates an expression to a person, family, or corporate body contributing to an expression."@en ;
    skos:scopeNote "Contributors include editors, translators, arrangers of music, performers, etc."@en .

<http://rdaregistry.info/Elements/e/P20054>
    reg:hasUnconstrained <http://rdaregistry.info/Elements/u/P60419> ;
    reg:lexicalAlias <http://rdaregistry.info/Elements/e/presenter.en> ;
    reg:name "presenter"@en ;
    reg:status <http://metadataregistry.org/uri/RegStatus/1001> ;
    rdakit:toolkitDefinition "A person, family, or corporate body mentioned in an"@en ;
    rdakit:toolkitLabel "presenter"@en ;
    a rdf:Property ;
    rdfs:domain <http://rdaregistry.info/Elements/c/C10006> ;
    rdfs:isDefinedBy <http://rdaregistry.info/Elements/e/> ;
    rdfs:label "has presenter"@en ;
    rdfs:range <http://rdaregistry.info/Elements/c/C10002> ;
    rdfs:subPropertyOf <http://rdaregistry.info/Elements/e/P20053> ;
    owl:inverseOf <http://rdaregistry.info/Elements/a/P50180> ;
    skos:definition "Relates an expression to a person, family, or corporate body mentioned in an \"X presents&quot: credit for moving image materials and who is probably associated with production, finance, or distribution in some way."@en .

<http://rdaregistry.info/Elements/e/P20055>
    reg:hasUnconstrained <http://rdaregistry.info/Elements/u/P60422> ;
    reg:lexicalAlias <http://rdaregistry.info/Elements/e/editorOfMovingImageWork.en> ;
    reg:name "editorOfMovingImageWork"@en ;
    reg:status <http://metadataregistry.org/uri/RegStatus/1001> ;
    rdakit:toolkitDefinition "A person, family, or corporate body responsible for assembling, arranging, and trimming film, video, or other moving image formats, including both visual and audio aspects."@en ;
    rdakit:toolkitLabel "editor of moving image work"@en ;
    a rdf:Property ;
    rdfs:domain <http://rdaregistry.info/Elements/c/C10006> ;
    rdfs:isDefinedBy <http://rdaregistry.info/Elements/e/> ;
    rdfs:label "has editor of moving image work"@en ;
    rdfs:range <http://rdaregistry.info/Elements/c/C10002> ;
    rdfs:subPropertyOf <http://rdaregistry.info/Elements/e/P20053> ;
    owl:inverseOf <http://rdaregistry.info/Elements/a/P50183> ;
    skos:definition "Relates an expression to a person, family, or corporate body responsible for assembling, arranging, and trimming film, video, or other moving image formats, including both visual and audio aspects."@en .

<http://rdaregistry.info/Elements/e/P20056>
    reg:hasUnconstrained <http://rdaregistry.info/Elements/u/P60437> ;
    reg:lexicalAlias <http://rdaregistry.info/Elements/e/productionDesigner.en> ;
    reg:name "productionDesigner"@en ;
    reg:status <http://metadataregistry.org/uri/RegStatus/1001> ;
    rdakit:toolkitDefinition "A person, family, or corporate body responsible for designing the overall visual appearance of a moving image production."@en ;
    rdakit:toolkitLabel "production designer"@en ;
    a rdf:Property ;
    rdfs:domain <http://rdaregistry.info/Elements/c/C10006> ;
    rdfs:isDefinedBy <http://rdaregistry.info/Elements/e/> ;
    rdfs:label "has production designer"@en ;
    rdfs:range <http://rdaregistry.info/Elements/c/C10002> ;
    rdfs:subPropertyOf <http://rdaregistry.info/Elements/e/P20053> ;
    owl:inverseOf <http://rdaregistry.info/Elements/a/P50198> ;
    skos:definition "Relates an expression to a person, family, or corporate body responsible for designing the overall visual appearance of a moving image production."@en .

<http://rdaregistry.info/Elements/e/P20057>
    reg:status <http://metadataregistry.org/uri/RegStatus/1008> ;
    a rdf:Property ;
    rdfs:isDefinedBy <http://rdaregistry.info/Elements/e/> .

<http://rdaregistry.info/Elements/e/P20058>
    reg:hasUnconstrained <http://rdaregistry.info/Elements/u/P60446> ;
    reg:lexicalAlias <http://rdaregistry.info/Elements/e/minuteTaker.en> ;
    reg:name "minuteTaker"@en ;
    reg:status <http://metadataregistry.org/uri/RegStatus/1001> ;
    rdakit:toolkitDefinition "A person, family, or corporate body, responsible for recording the minutes of a meeting."@en ;
    rdakit:toolkitLabel "minute taker"@en ;
    a rdf:Property ;
    rdfs:domain <http://rdaregistry.info/Elements/c/C10006> ;
    rdfs:isDefinedBy <http://rdaregistry.info/Elements/e/> ;
    rdfs:label "has minute taker"@en ;
    rdfs:range <http://rdaregistry.info/Elements/c/C10002> ;
    rdfs:subPropertyOf <http://rdaregistry.info/Elements/e/P20053> ;
    owl:inverseOf <http://rdaregistry.info/Elements/a/P50212> ;
    skos:definition "Relates an expression to a person, family, or corporate body, responsible for recording the minutes of a meeting."@en .

<http://rdaregistry.info/Elements/e/P20059>
    reg:lexicalAlias <http://rdaregistry.info/Elements/e/manifestationOfExpression.en> ;
    reg:name "manifestationOfExpression"@en ;
    reg:status <http://metadataregistry.org/uri/RegStatus/1001> ;
    rdakit:instructionNumber "17.9" ;
    rdakit:toolkitDefinition "A physical embodiment of an expression."@en ;
    rdakit:toolkitLabel "manifestation of expression"@en ;
    a rdf:Property ;
    rdfs:domain <http://rdaregistry.info/Elements/c/C10006> ;
    rdfs:isDefinedBy <http://rdaregistry.info/Elements/e/> ;
    rdfs:label "has manifestation of expression"@en ;
    rdfs:range <http://rdaregistry.info/Elements/c/C10007> ;
    owl:inverseOf <http://rdaregistry.info/Elements/m/P30139> ;
    skos:definition "Relates an expression to a physical embodiment of an expression."@en .

<http://rdaregistry.info/Elements/e/P20060>
    reg:hasUnconstrained <http://rdaregistry.info/Elements/u/P60174> ;
    reg:lexicalAlias <http://rdaregistry.info/Elements/e/adaptedAsRadioProgramExpression.en> ;
    reg:name "adaptedAsRadioProgramExpression"@en ;
    reg:status <http://metadataregistry.org/uri/RegStatus/1001> ;
    rdakit:toolkitDefinition "A radio program based on the source expression."@en ;
    rdakit:toolkitLabel "adapted as radio program (expression)"@en ;
    a rdf:Property ;
    rdfs:domain <http://rdaregistry.info/Elements/c/C10006> ;
    rdfs:isDefinedBy <http://rdaregistry.info/Elements/e/> ;
    rdfs:label "is adapted as radio program (expression)"@en ;
    rdfs:range <http://rdaregistry.info/Elements/c/C10006> ;
    rdfs:subPropertyOf <http://rdaregistry.info/Elements/e/P20153> ;
    owl:inverseOf <http://rdaregistry.info/Elements/e/P20127> ;
    skos:definition "Relates an expression to a radio program based on the source expression."@en .

<http://rdaregistry.info/Elements/e/P20061>
    reg:hasUnconstrained <http://rdaregistry.info/Elements/u/P60318> ;
    reg:lexicalAlias <http://rdaregistry.info/Elements/e/formOfTactileNotation.en> ;
    reg:name "formOfTactileNotation"@en ;
    reg:status <http://metadataregistry.org/uri/RegStatus/1001> ;
    rdakit:instructionNumber "7.13.4" ;
    rdakit:toolkitDefinition "A set of characters and/or symbols used to express the content of a resource in a form that can be perceived through touch."@en ;
    rdakit:toolkitLabel "form of tactile notation"@en ;
    a rdf:Property ;
    rdfs:domain <http://rdaregistry.info/Elements/c/C10006> ;
    rdfs:isDefinedBy <http://rdaregistry.info/Elements/e/> ;
    rdfs:label "has form of tactile notation"@en ;
    rdfs:subPropertyOf <http://rdaregistry.info/Elements/e/P20062> ;
    skos:definition "Relates an expression to a set of characters and/or symbols used to express the content of a resource in a form that can be perceived through touch."@en .

<http://rdaregistry.info/Elements/e/P20062>
    reg:hasSubproperty <http://rdaregistry.info/Elements/e/P20061>, <http://rdaregistry.info/Elements/e/P20063>, <http://rdaregistry.info/Elements/e/P20064>, <http://rdaregistry.info/Elements/e/P20065> ;
    reg:hasUnconstrained <http://rdaregistry.info/Elements/u/P60319> ;
    reg:lexicalAlias <http://rdaregistry.info/Elements/e/formOfNotation.en> ;
    reg:name "formOfNotation"@en ;
    reg:status <http://metadataregistry.org/uri/RegStatus/1001> ;
    rdakit:instructionNumber "7.13" ;
    rdakit:toolkitDefinition "A set of characters and/or symbols used to express the content of a resource."@en ;
    rdakit:toolkitLabel "form of notation"@en ;
    a rdf:Property ;
    rdfs:domain <http://rdaregistry.info/Elements/c/C10006> ;
    rdfs:isDefinedBy <http://rdaregistry.info/Elements/e/> ;
    rdfs:label "has form of notation"@en ;
    skos:definition "Relates an expression to a set of characters and/or symbols used to express the content of a resource."@en .

<http://rdaregistry.info/Elements/e/P20063>
    reg:hasUnconstrained <http://rdaregistry.info/Elements/u/P60320> ;
    reg:lexicalAlias <http://rdaregistry.info/Elements/e/formOfNotatedMovement.en> ;
    reg:name "formOfNotatedMovement"@en ;
    reg:status <http://metadataregistry.org/uri/RegStatus/1001> ;
    rdakit:instructionNumber "7.13.5" ;
    rdakit:toolkitDefinition "A set of characters and/or symbols used to express the movement content of a resource."@en ;
    rdakit:toolkitLabel "form of notated movement"@en ;
    a rdf:Property ;
    rdfs:domain <http://rdaregistry.info/Elements/c/C10006> ;
    rdfs:isDefinedBy <http://rdaregistry.info/Elements/e/> ;
    rdfs:label "has form of notated movement"@en ;
    rdfs:subPropertyOf <http://rdaregistry.info/Elements/e/P20062> ;
    skos:definition "Relates an expression to a set of characters and/or symbols used to express the movement content of a resource."@en .

<http://rdaregistry.info/Elements/e/P20064>
    reg:hasUnconstrained <http://rdaregistry.info/Elements/u/P60321> ;
    reg:lexicalAlias <http://rdaregistry.info/Elements/e/formOfMusicalNotation.en> ;
    reg:name "formOfMusicalNotation"@en ;
    reg:status <http://metadataregistry.org/uri/RegStatus/1001> ;
    rdakit:instructionNumber "7.13.3" ;
    rdakit:toolkitDefinition "A set of characters and/or symbols used to express the musical content of a resource."@en ;
    rdakit:toolkitLabel "form of musical notation"@en ;
    a rdf:Property ;
    rdfs:domain <http://rdaregistry.info/Elements/c/C10006> ;
    rdfs:isDefinedBy <http://rdaregistry.info/Elements/e/> ;
    rdfs:label "has form of musical notation"@en ;
    rdfs:subPropertyOf <http://rdaregistry.info/Elements/e/P20062> ;
    skos:definition "Relates an expression to a set of characters and/or symbols used to express the musical content of a resource."@en .

<http://rdaregistry.info/Elements/e/P20065>
    reg:hasUnconstrained <http://rdaregistry.info/Elements/u/P60322> ;
    reg:lexicalAlias <http://rdaregistry.info/Elements/e/script.en> ;
    reg:name "script"@en ;
    reg:status <http://metadataregistry.org/uri/RegStatus/1001> ;
    rdakit:instructionNumber "7.13.2" ;
    rdakit:toolkitDefinition "A set of characters and/or symbols used to express the written language content of a resource."@en ;
    rdakit:toolkitLabel "script"@en ;
    a rdf:Property ;
    rdfs:domain <http://rdaregistry.info/Elements/c/C10006> ;
    rdfs:isDefinedBy <http://rdaregistry.info/Elements/e/> ;
    rdfs:label "has script"@en ;
    rdfs:subPropertyOf <http://rdaregistry.info/Elements/e/P20062> ;
    skos:definition "Relates an expression to a set of characters and/or symbols used to express the written language content of a resource."@en .

<http://rdaregistry.info/Elements/e/P20066>
    reg:hasUnconstrained <http://rdaregistry.info/Elements/u/P60354> ;
    reg:lexicalAlias <http://rdaregistry.info/Elements/e/adaptedAsTelevisionProgramExpression.en> ;
    reg:name "adaptedAsTelevisionProgramExpression"@en ;
    reg:status <http://metadataregistry.org/uri/RegStatus/1001> ;
    rdakit:toolkitDefinition "A television program based on the source expression."@en ;
    rdakit:toolkitLabel "adapted as television program (expression)"@en ;
    a rdf:Property ;
    rdfs:domain <http://rdaregistry.info/Elements/c/C10006> ;
    rdfs:isDefinedBy <http://rdaregistry.info/Elements/e/> ;
    rdfs:label "is adapted as television program (expression)"@en ;
    rdfs:range <http://rdaregistry.info/Elements/c/C10006> ;
    rdfs:subPropertyOf <http://rdaregistry.info/Elements/e/P20153> ;
    owl:inverseOf <http://rdaregistry.info/Elements/e/P20128> ;
    skos:definition "Relates an expression to a television program based on the source expression."@en .

<http://rdaregistry.info/Elements/e/P20067>
    reg:hasUnconstrained <http://rdaregistry.info/Elements/u/P60361> ;
    reg:lexicalAlias <http://rdaregistry.info/Elements/e/adaptedAsVideoExpression.en> ;
    reg:name "adaptedAsVideoExpression"@en ;
    reg:status <http://metadataregistry.org/uri/RegStatus/1001> ;
    rdakit:toolkitDefinition "A video based on the source expression."@en ;
    rdakit:toolkitLabel "adapted as video (expression)"@en ;
    a rdf:Property ;
    rdfs:domain <http://rdaregistry.info/Elements/c/C10006> ;
    rdfs:isDefinedBy <http://rdaregistry.info/Elements/e/> ;
    rdfs:label "is adapted as video (expression)"@en ;
    rdfs:range <http://rdaregistry.info/Elements/c/C10006> ;
    rdfs:subPropertyOf <http://rdaregistry.info/Elements/e/P20153> ;
    owl:inverseOf <http://rdaregistry.info/Elements/e/P20134> ;
    skos:definition "Relates an expression to a video based on the source expression."@en .

<http://rdaregistry.info/Elements/e/P20068>
    reg:hasUnconstrained <http://rdaregistry.info/Elements/u/P60371> ;
    reg:lexicalAlias <http://rdaregistry.info/Elements/e/writerOfAddedLyrics.en> ;
    reg:name "writerOfAddedLyrics"@en ;
    reg:status <http://metadataregistry.org/uri/RegStatus/1001> ;
    rdakit:toolkitDefinition "A writer of words added to an expression of a musical work."@en ;
    rdakit:toolkitLabel "writer of added lyrics"@en ;
    a rdf:Property ;
    rdfs:domain <http://rdaregistry.info/Elements/c/C10006> ;
    rdfs:isDefinedBy <http://rdaregistry.info/Elements/e/> ;
    rdfs:label "has writer of added lyrics"@en ;
    rdfs:range <http://rdaregistry.info/Elements/c/C10002> ;
    rdfs:subPropertyOf <http://rdaregistry.info/Elements/e/P20030> ;
    owl:inverseOf <http://rdaregistry.info/Elements/a/P50216> ;
    skos:definition "Relates an expression to a writer of words added to an expression of a musical work."@en .

<http://rdaregistry.info/Elements/e/P20069>
    reg:hasUnconstrained <http://rdaregistry.info/Elements/u/P60372> ;
    reg:lexicalAlias <http://rdaregistry.info/Elements/e/summarizationOfTheContent.en> ;
    reg:name "summarizationOfTheContent"@en ;
    reg:status <http://metadataregistry.org/uri/RegStatus/1001> ;
    rdakit:instructionNumber "7.1" ;
    rdakit:toolkitDefinition "An abstract, summary, synopsis, etc., of the content of a resource."@en ;
    rdakit:toolkitLabel "summarization of the content"@en ;
    a rdf:Property ;
    rdfs:domain <http://rdaregistry.info/Elements/c/C10006> ;
    rdfs:isDefinedBy <http://rdaregistry.info/Elements/e/> ;
    rdfs:label "has summarization of the content"@en ;
    skos:definition "Relates an expression to an abstract, summary, synopsis, etc., of the content of a resource."@en .

<http://rdaregistry.info/Elements/e/P20070>
    reg:hasUnconstrained <http://rdaregistry.info/Elements/u/P60152> ;
    reg:lexicalAlias <http://rdaregistry.info/Elements/e/voiceActor.en> ;
    reg:name "voiceActor"@en ;
    reg:status <http://metadataregistry.org/uri/RegStatus/1001> ;
    rdakit:toolkitDefinition "An actor contributing to an expression of a work by providing the voice for characters in radio and audio productions and for animated characters in moving image works, as well as by providing voice-overs in radio and television commercials, dubbed resources, etc."@en ;
    rdakit:toolkitLabel "voice actor"@en ;
    a rdf:Property ;
    rdfs:domain <http://rdaregistry.info/Elements/c/C10006> ;
    rdfs:isDefinedBy <http://rdaregistry.info/Elements/e/> ;
    rdfs:label "has voice actor"@en ;
    rdfs:range <http://rdaregistry.info/Elements/c/C10002> ;
    rdfs:subPropertyOf <http://rdaregistry.info/Elements/e/P20012> ;
    owl:inverseOf <http://rdaregistry.info/Elements/a/P50217> ;
    skos:definition "Relates an expression to an actor contributing to an expression of a work by providing the voice for characters in radio and audio productions and for animated characters in moving image works, as well as by providing voice-overs in radio and television commercials, dubbed resources, etc."@en .

<http://rdaregistry.info/Elements/e/P20071>
    reg:hasSubproperty <http://rdaregistry.info/Elements/e/P20010> ;
    reg:hasUnconstrained <http://rdaregistry.info/Elements/u/P60470> ;
    reg:lexicalAlias <http://rdaregistry.info/Elements/e/noteOnExpression.en> ;
    reg:name "noteOnExpression"@en ;
    reg:status <http://metadataregistry.org/uri/RegStatus/1001> ;
    rdakit:instructionNumber "7.29" ;
    rdakit:toolkitDefinition "An annotation providing additional information about content recorded as an expression attribute."@en ;
    rdakit:toolkitLabel "note on expression"@en ;
    a rdf:Property ;
    rdfs:domain <http://rdaregistry.info/Elements/c/C10006> ;
    rdfs:isDefinedBy <http://rdaregistry.info/Elements/e/> ;
    rdfs:label "has note on expression"@en ;
    skos:definition "Relates an expression to an annotation providing additional information about content recorded as an expression attribute."@en .

<http://rdaregistry.info/Elements/e/P20072>
    reg:status <http://metadataregistry.org/uri/RegStatus/1008> ;
    a rdf:Property ;
    rdfs:isDefinedBy <http://rdaregistry.info/Elements/e/> .

<http://rdaregistry.info/Elements/e/P20073>
    reg:hasUnconstrained <http://rdaregistry.info/Elements/u/P60088> ;
    reg:lexicalAlias <http://rdaregistry.info/Elements/e/dramatizedAsExpression.en> ;
    reg:name "dramatizedAsExpression"@en ;
    reg:status <http://metadataregistry.org/uri/RegStatus/1001> ;
    rdakit:toolkitDefinition "An expression of a dramatic work adapted from the source expression."@en ;
    rdakit:toolkitLabel "dramatized as (expression)"@en ;
    a rdf:Property ;
    rdfs:domain <http://rdaregistry.info/Elements/c/C10006> ;
    rdfs:isDefinedBy <http://rdaregistry.info/Elements/e/> ;
    rdfs:label "is dramatized as (expression)"@en ;
    rdfs:range <http://rdaregistry.info/Elements/c/C10006> ;
    rdfs:subPropertyOf <http://rdaregistry.info/Elements/e/P20153> ;
    owl:inverseOf <http://rdaregistry.info/Elements/e/P20123> ;
    skos:definition "Relates an expression to an expression of a dramatic work adapted from the source expression."@en .

<http://rdaregistry.info/Elements/e/P20074>
    reg:hasUnconstrained <http://rdaregistry.info/Elements/u/P60101> ;
    reg:lexicalAlias <http://rdaregistry.info/Elements/e/containedInExpression.en> ;
    reg:name "containedInExpression"@en ;
    reg:status <http://metadataregistry.org/uri/RegStatus/1001> ;
    rdakit:toolkitDefinition "An expression of a larger work of which the expression is a discrete component."@en ;
    rdakit:toolkitLabel "contained in (expression)"@en ;
    a rdf:Property ;
    rdfs:domain <http://rdaregistry.info/Elements/c/C10006> ;
    rdfs:isDefinedBy <http://rdaregistry.info/Elements/e/> ;
    rdfs:label "is contained in (expression)"@en ;
    rdfs:range <http://rdaregistry.info/Elements/c/C10006> ;
    rdfs:subPropertyOf <http://rdaregistry.info/Elements/e/P20236> ;
    owl:inverseOf <http://rdaregistry.info/Elements/e/P20145> ;
    skos:definition "Relates an expression to an expression of a larger work of which the expression is a discrete component."@en .

<http://rdaregistry.info/Elements/e/P20075>
    reg:hasUnconstrained <http://rdaregistry.info/Elements/u/P60103> ;
    reg:lexicalAlias <http://rdaregistry.info/Elements/e/replacedInPartByExpression.en> ;
    reg:name "replacedInPartByExpression"@en ;
    reg:status <http://metadataregistry.org/uri/RegStatus/1001> ;
    rdakit:toolkitDefinition "An expression of a later work used in part in place of the earlier expression usually because the later work contains updated or new information that makes part of the earlier expression obsolete."@en ;
    rdakit:toolkitLabel "replaced in part by (expression)"@en ;
    a rdf:Property ;
    rdfs:domain <http://rdaregistry.info/Elements/c/C10006> ;
    rdfs:isDefinedBy <http://rdaregistry.info/Elements/e/> ;
    rdfs:label "is replaced in part by (expression)"@en ;
    rdfs:range <http://rdaregistry.info/Elements/c/C10006> ;
    rdfs:subPropertyOf <http://rdaregistry.info/Elements/e/P20169> ;
    owl:inverseOf <http://rdaregistry.info/Elements/e/P20198> ;
    skos:definition "Relates an expression to an expression of a later work used in part in place of the earlier expression usually because the later work contains updated or new information that makes part of the earlier expression obsolete."@en .

<http://rdaregistry.info/Elements/e/P20076>
    reg:hasUnconstrained <http://rdaregistry.info/Elements/u/P60104> ;
    reg:lexicalAlias <http://rdaregistry.info/Elements/e/replacedByExpression.en> ;
    reg:name "replacedByExpression"@en ;
    reg:status <http://metadataregistry.org/uri/RegStatus/1001> ;
    rdakit:toolkitDefinition "An expression of a later work used in place of the earlier expression, usually because the later work contains updated or new information that makes the earlier expression obsolete."@en ;
    rdakit:toolkitLabel "replaced by (expression)"@en ;
    a rdf:Property ;
    rdfs:domain <http://rdaregistry.info/Elements/c/C10006> ;
    rdfs:isDefinedBy <http://rdaregistry.info/Elements/e/> ;
    rdfs:label "is replaced by (expression)"@en ;
    rdfs:range <http://rdaregistry.info/Elements/c/C10006> ;
    rdfs:subPropertyOf <http://rdaregistry.info/Elements/e/P20169> ;
    owl:inverseOf <http://rdaregistry.info/Elements/e/P20199> ;
    skos:definition "Relates an expression to an expression of a later work used in place of the earlier expression, usually because the later work contains updated or new information that makes the earlier expression obsolete."@en .

<http://rdaregistry.info/Elements/e/P20077>
    reg:hasUnconstrained <http://rdaregistry.info/Elements/u/P60106> ;
    reg:lexicalAlias <http://rdaregistry.info/Elements/e/adaptedInVerseAsExpression.en> ;
    reg:name "adaptedInVerseAsExpression"@en ;
    reg:status <http://metadataregistry.org/uri/RegStatus/1001> ;
    rdakit:toolkitDefinition "An expression of a literary composition in verse form adapted from the source expression."@en ;
    rdakit:toolkitLabel "adapted in verse as (expression)"@en ;
    a rdf:Property ;
    rdfs:domain <http://rdaregistry.info/Elements/c/C10006> ;
    rdfs:isDefinedBy <http://rdaregistry.info/Elements/e/> ;
    rdfs:label "is adapted in verse as (expression)"@en ;
    rdfs:range <http://rdaregistry.info/Elements/c/C10006> ;
    rdfs:subPropertyOf <http://rdaregistry.info/Elements/e/P20153> ;
    owl:inverseOf <http://rdaregistry.info/Elements/e/P20124> ;
    skos:definition "Relates an expression to an expression of a literary composition in verse form adapted from the source expression."@en .

<http://rdaregistry.info/Elements/e/P20078>
    reg:hasUnconstrained <http://rdaregistry.info/Elements/u/P60111> ;
    reg:lexicalAlias <http://rdaregistry.info/Elements/e/dubbedVersionOf.en> ;
    reg:name "dubbedVersionOf"@en ;
    reg:status <http://metadataregistry.org/uri/RegStatus/1001> ;
    rdakit:toolkitDefinition "An expression of a moving image work in which the spoken dialogue has been translated into a language different from that of the original work."@en ;
    rdakit:toolkitLabel "dubbed version of"@en ;
    a rdf:Property ;
    rdfs:domain <http://rdaregistry.info/Elements/c/C10006> ;
    rdfs:isDefinedBy <http://rdaregistry.info/Elements/e/> ;
    rdfs:label "is dubbed version of"@en ;
    rdfs:range <http://rdaregistry.info/Elements/c/C10006> ;
    rdfs:subPropertyOf <http://rdaregistry.info/Elements/e/P20141> ;
    owl:inverseOf <http://rdaregistry.info/Elements/e/P20079> ;
    skos:definition "Relates an expression to an expression of a moving image work in which the spoken dialogue has been translated into a language different from that of the original work."@en .

<http://rdaregistry.info/Elements/e/P20079>
    reg:hasUnconstrained <http://rdaregistry.info/Elements/u/P60112> ;
    reg:lexicalAlias <http://rdaregistry.info/Elements/e/dubbedVersion.en> ;
    reg:name "dubbedVersion"@en ;
    reg:status <http://metadataregistry.org/uri/RegStatus/1001> ;
    rdakit:toolkitDefinition "An expression of a moving image work that translates the spoken dialogue of the original work into a different language."@en ;
    rdakit:toolkitLabel "dubbed version"@en ;
    a rdf:Property ;
    rdfs:domain <http://rdaregistry.info/Elements/c/C10006> ;
    rdfs:isDefinedBy <http://rdaregistry.info/Elements/e/> ;
    rdfs:label "is dubbed version"@en ;
    rdfs:range <http://rdaregistry.info/Elements/c/C10006> ;
    rdfs:subPropertyOf <http://rdaregistry.info/Elements/e/P20171> ;
    owl:inverseOf <http://rdaregistry.info/Elements/e/P20078> ;
    skos:definition "Relates an expression to an expression of a moving image work that translates the spoken dialogue of the original work into a different language."@en .

<http://rdaregistry.info/Elements/e/P20080>
    reg:hasUnconstrained <http://rdaregistry.info/Elements/u/P60113> ;
    reg:lexicalAlias <http://rdaregistry.info/Elements/e/cadenzaExpression.en> ;
    reg:name "cadenzaExpression"@en ;
    reg:status <http://metadataregistry.org/uri/RegStatus/1001> ;
    rdakit:toolkitDefinition "An expression of a musical work consisting of an ornamental passage for a soloist, added to a musical work such as a concerto, either by the same or a different composer."@en ;
    rdakit:toolkitLabel "cadenza (expression)"@en ;
    a rdf:Property ;
    rdfs:domain <http://rdaregistry.info/Elements/c/C10006> ;
    rdfs:isDefinedBy <http://rdaregistry.info/Elements/e/> ;
    rdfs:label "is cadenza (expression)"@en ;
    rdfs:range <http://rdaregistry.info/Elements/c/C10006> ;
    rdfs:subPropertyOf <http://rdaregistry.info/Elements/e/P20105> ;
    owl:inverseOf <http://rdaregistry.info/Elements/e/P20083> ;
    skos:definition "Relates an expression to an expression of a musical work consisting of an ornamental passage for a soloist, added to a musical work such as a concerto, either by the same or a different composer."@en .

<http://rdaregistry.info/Elements/e/P20081>
    reg:hasUnconstrained <http://rdaregistry.info/Elements/u/P60114> ;
    reg:lexicalAlias <http://rdaregistry.info/Elements/e/variationsBasedOnExpression.en> ;
    reg:name "variationsBasedOnExpression"@en ;
    reg:status <http://metadataregistry.org/uri/RegStatus/1001> ;
    rdakit:toolkitDefinition "An expression of a musical work from which melodic, thematic, or harmonic material is taken to form a discrete theme, which is repeated one or more times with subsequent modifications."@en ;
    rdakit:toolkitLabel "variations based on (expression)"@en ;
    a rdf:Property ;
    rdfs:domain <http://rdaregistry.info/Elements/c/C10006> ;
    rdfs:isDefinedBy <http://rdaregistry.info/Elements/e/> ;
    rdfs:label "is variations based on (expression)"@en ;
    rdfs:range <http://rdaregistry.info/Elements/c/C10006> ;
    rdfs:subPropertyOf <http://rdaregistry.info/Elements/e/P20204> ;
    owl:inverseOf <http://rdaregistry.info/Elements/e/P20082> ;
    skos:definition "Relates an expression to an expression of a musical work from which melodic, thematic, or harmonic material is taken to form a discrete theme, which is repeated one or more times with subsequent modifications."@en .

<http://rdaregistry.info/Elements/e/P20082>
    reg:hasUnconstrained <http://rdaregistry.info/Elements/u/P60115> ;
    reg:lexicalAlias <http://rdaregistry.info/Elements/e/modifiedByVariationAsExpression.en> ;
    reg:name "modifiedByVariationAsExpression"@en ;
    reg:status <http://metadataregistry.org/uri/RegStatus/1001> ;
    rdakit:toolkitDefinition "An expression of a musical work in which melodic, thematic, or harmonic material is taken from the source work to form a discrete theme, which is repeated one or more times with subsequent modifications."@en ;
    rdakit:toolkitLabel "modified by variation as (expression)"@en ;
    a rdf:Property ;
    rdfs:domain <http://rdaregistry.info/Elements/c/C10006> ;
    rdfs:isDefinedBy <http://rdaregistry.info/Elements/e/> ;
    rdfs:label "is modified by variation as (expression)"@en ;
    rdfs:range <http://rdaregistry.info/Elements/c/C10006> ;
    rdfs:subPropertyOf <http://rdaregistry.info/Elements/e/P20203> ;
    owl:inverseOf <http://rdaregistry.info/Elements/e/P20081> ;
    skos:definition "Relates an expression to an expression of a musical work in which melodic, thematic, or harmonic material is taken from the source work to form a discrete theme, which is repeated one or more times with subsequent modifications."@en .

<http://rdaregistry.info/Elements/e/P20083>
    reg:hasUnconstrained <http://rdaregistry.info/Elements/u/P60116> ;
    reg:lexicalAlias <http://rdaregistry.info/Elements/e/cadenzaComposedForExpression.en> ;
    reg:name "cadenzaComposedForExpression"@en ;
    reg:status <http://metadataregistry.org/uri/RegStatus/1001> ;
    rdakit:toolkitDefinition "An expression of a musical work such as a concerto for which an ornamental passage for a soloist has been composed, either by the same or a different composer."@en ;
    rdakit:toolkitLabel "cadenza composed for (expression)"@en ;
    a rdf:Property ;
    rdfs:domain <http://rdaregistry.info/Elements/c/C10006> ;
    rdfs:isDefinedBy <http://rdaregistry.info/Elements/e/> ;
    rdfs:label "is cadenza composed for (expression)"@en ;
    rdfs:range <http://rdaregistry.info/Elements/c/C10006> ;
    rdfs:subPropertyOf <http://rdaregistry.info/Elements/e/P20192> ;
    owl:inverseOf <http://rdaregistry.info/Elements/e/P20080> ;
    skos:definition "Relates an expression to an expression of a musical work such as a concerto for which an ornamental passage for a soloist has been composed, either by the same or a different composer."@en .

<http://rdaregistry.info/Elements/e/P20084>
    reg:hasUnconstrained <http://rdaregistry.info/Elements/u/P60117> ;
    reg:lexicalAlias <http://rdaregistry.info/Elements/e/librettoForExpression.en> ;
    reg:name "librettoForExpression"@en ;
    reg:status <http://metadataregistry.org/uri/RegStatus/1001> ;
    rdakit:toolkitDefinition "An expression of a musical work such as an opera or other work for the musical stage, or an oratorio, that uses the text of the related work."@en ;
    rdakit:toolkitLabel "libretto for (expression)"@en ;
    a rdf:Property ;
    rdfs:domain <http://rdaregistry.info/Elements/c/C10006> ;
    rdfs:isDefinedBy <http://rdaregistry.info/Elements/e/> ;
    rdfs:label "is libretto for (expression)"@en ;
    rdfs:range <http://rdaregistry.info/Elements/c/C10006> ;
    rdfs:subPropertyOf <http://rdaregistry.info/Elements/e/P20100> ;
    owl:inverseOf <http://rdaregistry.info/Elements/e/P20163> ;
    skos:definition "Relates an expression to an expression of a musical work such as an opera or other work for the musical stage, or an oratorio, that uses the text of the related work."@en .

<http://rdaregistry.info/Elements/e/P20085>
    reg:hasUnconstrained <http://rdaregistry.info/Elements/u/P60118> ;
    reg:lexicalAlias <http://rdaregistry.info/Elements/e/incidentalMusicExpression.en> ;
    reg:name "incidentalMusicExpression"@en ;
    reg:status <http://metadataregistry.org/uri/RegStatus/1001> ;
    rdakit:toolkitDefinition "An expression of a musical work that that provides the incidental music for a play or other spoken work for the stage."@en ;
    rdakit:toolkitLabel "incidental music (expression)"@en ;
    a rdf:Property ;
    rdfs:domain <http://rdaregistry.info/Elements/c/C10006> ;
    rdfs:isDefinedBy <http://rdaregistry.info/Elements/e/> ;
    rdfs:label "is incidental music (expression)"@en ;
    rdfs:range <http://rdaregistry.info/Elements/c/C10006> ;
    rdfs:subPropertyOf <http://rdaregistry.info/Elements/e/P20243> ;
    owl:inverseOf <http://rdaregistry.info/Elements/e/P20103> ;
    skos:definition "Relates an expression to an expression of a musical work that that provides the incidental music for a play or other spoken work for the stage."@en .

<http://rdaregistry.info/Elements/e/P20086>
    reg:hasUnconstrained <http://rdaregistry.info/Elements/u/P60120> ;
    reg:lexicalAlias <http://rdaregistry.info/Elements/e/remadeAsExpression.en> ;
    reg:name "remadeAsExpression"@en ;
    reg:status <http://metadataregistry.org/uri/RegStatus/1001> ;
    rdakit:toolkitDefinition "An expression of a new motion picture, radio program, television program, or video based on an earlier work."@en ;
    rdakit:toolkitLabel "remade as (expression)"@en ;
    a rdf:Property ;
    rdfs:domain <http://rdaregistry.info/Elements/c/C10006> ;
    rdfs:isDefinedBy <http://rdaregistry.info/Elements/e/> ;
    rdfs:label "is remade as (expression)"@en ;
    rdfs:range <http://rdaregistry.info/Elements/c/C10006> ;
    rdfs:subPropertyOf <http://rdaregistry.info/Elements/e/P20203> ;
    owl:inverseOf <http://rdaregistry.info/Elements/e/P20185> ;
    skos:definition "Relates an expression to an expression of a new motion picture, radio program, television program, or video based on an earlier work."@en .

<http://rdaregistry.info/Elements/e/P20087>
    reg:hasUnconstrained <http://rdaregistry.info/Elements/u/P60121> ;
    reg:lexicalAlias <http://rdaregistry.info/Elements/e/setToMusicAsExpression.en> ;
    reg:name "setToMusicAsExpression"@en ;
    reg:status <http://metadataregistry.org/uri/RegStatus/1001> ;
    rdakit:toolkitDefinition "An expression of a non-dramatic musical work, other than an oratorio, that uses the text of the source work."@en ;
    rdakit:toolkitLabel "set to music as (expression)"@en ;
    a rdf:Property ;
    rdfs:domain <http://rdaregistry.info/Elements/c/C10006> ;
    rdfs:isDefinedBy <http://rdaregistry.info/Elements/e/> ;
    rdfs:label "is set to music as (expression)"@en ;
    rdfs:range <http://rdaregistry.info/Elements/c/C10006> ;
    rdfs:subPropertyOf <http://rdaregistry.info/Elements/e/P20203> ;
    owl:inverseOf <http://rdaregistry.info/Elements/e/P20159> ;
    skos:definition "Relates an expression to an expression of a non-dramatic musical work, other than an oratorio, that uses the text of the source work."@en .

<http://rdaregistry.info/Elements/e/P20088>
    reg:hasUnconstrained <http://rdaregistry.info/Elements/u/P60138> ;
    reg:lexicalAlias <http://rdaregistry.info/Elements/e/adaptedAsNovelExpression.en> ;
    reg:name "adaptedAsNovelExpression"@en ;
    reg:status <http://metadataregistry.org/uri/RegStatus/1001> ;
    rdakit:toolkitDefinition "An expression of a novel adapted from the source expression."@en ;
    rdakit:toolkitLabel "adapted as novel (expression)"@en ;
    a rdf:Property ;
    rdfs:domain <http://rdaregistry.info/Elements/c/C10006> ;
    rdfs:isDefinedBy <http://rdaregistry.info/Elements/e/> ;
    rdfs:label "is adapted as novel (expression)"@en ;
    rdfs:range <http://rdaregistry.info/Elements/c/C10006> ;
    rdfs:subPropertyOf <http://rdaregistry.info/Elements/e/P20153> ;
    owl:inverseOf <http://rdaregistry.info/Elements/e/P20126> ;
    skos:definition "Relates an expression to an expression of a novel adapted from the source expression."@en .

<http://rdaregistry.info/Elements/e/P20089>
    reg:hasUnconstrained <http://rdaregistry.info/Elements/u/P60253> ;
    reg:lexicalAlias <http://rdaregistry.info/Elements/e/appendixToExpression.en> ;
    reg:name "appendixToExpression"@en ;
    reg:status <http://metadataregistry.org/uri/RegStatus/1001> ;
    rdakit:toolkitDefinition "An expression of a predominant work that is augmented by another work that consists of material that is not essential to the completeness of the content, such as a list of references, statistical tables, and explanatory matter; the augmenting work can either come at the end of the content, or be issued separately."@en ;
    rdakit:toolkitLabel "appendix to (expression)"@en ;
    a rdf:Property ;
    rdfs:domain <http://rdaregistry.info/Elements/c/C10006> ;
    rdfs:isDefinedBy <http://rdaregistry.info/Elements/e/> ;
    rdfs:label "is appendix to (expression)"@en ;
    rdfs:range <http://rdaregistry.info/Elements/c/C10006> ;
    rdfs:subPropertyOf <http://rdaregistry.info/Elements/e/P20192> ;
    owl:inverseOf <http://rdaregistry.info/Elements/e/P20118> ;
    skos:definition "Relates an expression to an expression of a predominant work that is augmented by another work that consists of material that is not essential to the completeness of the content, such as a list of references, statistical tables, and explanatory matter; the augmenting work can either come at the end of the content, or be issued separately."@en .

<http://rdaregistry.info/Elements/e/P20090>
    reg:hasUnconstrained <http://rdaregistry.info/Elements/u/P60177> ;
    reg:lexicalAlias <http://rdaregistry.info/Elements/e/abstractedInExpression.en> ;
    reg:name "abstractedInExpression"@en ;
    reg:status <http://metadataregistry.org/uri/RegStatus/1001> ;
    rdakit:toolkitDefinition "An expression of a work (an abstracting and indexing service) that abstracts the contents of a source expression."@en ;
    rdakit:toolkitLabel "abstracted in (expression)"@en ;
    a rdf:Property ;
    rdfs:domain <http://rdaregistry.info/Elements/c/C10006> ;
    rdfs:isDefinedBy <http://rdaregistry.info/Elements/e/> ;
    rdfs:label "is abstracted in (expression)"@en ;
    rdfs:range <http://rdaregistry.info/Elements/c/C10006> ;
    rdfs:subPropertyOf <http://rdaregistry.info/Elements/e/P20203> ;
    owl:inverseOf <http://rdaregistry.info/Elements/e/P20193> ;
    skos:definition "Relates an expression to an expression of a work (an abstracting and indexing service) that abstracts the contents of a source expression."@en .

<http://rdaregistry.info/Elements/e/P20091>
    reg:hasUnconstrained <http://rdaregistry.info/Elements/u/P60178> ;
    reg:lexicalAlias <http://rdaregistry.info/Elements/e/indexedInExpression.en> ;
    reg:name "indexedInExpression"@en ;
    reg:status <http://metadataregistry.org/uri/RegStatus/1001> ;
    rdakit:toolkitDefinition "An expression of a work (an abstracting and indexing service) that indexes the contents of a source expression."@en ;
    rdakit:toolkitLabel "indexed in (expression)"@en ;
    a rdf:Property ;
    rdfs:domain <http://rdaregistry.info/Elements/c/C10006> ;
    rdfs:isDefinedBy <http://rdaregistry.info/Elements/e/> ;
    rdfs:label "is indexed in (expression)"@en ;
    rdfs:range <http://rdaregistry.info/Elements/c/C10006> ;
    rdfs:subPropertyOf <http://rdaregistry.info/Elements/e/P20203> ;
    owl:inverseOf <http://rdaregistry.info/Elements/e/P20194> ;
    skos:definition "Relates an expression to an expression of a work (an abstracting and indexing service) that indexes the contents of a source expression."@en .

<http://rdaregistry.info/Elements/e/P20092>
    reg:hasUnconstrained <http://rdaregistry.info/Elements/u/P60180> ;
    reg:lexicalAlias <http://rdaregistry.info/Elements/e/adaptedAsChoreographyExpression.en> ;
    reg:name "adaptedAsChoreographyExpression"@en ;
    reg:status <http://metadataregistry.org/uri/RegStatus/1001> ;
    rdakit:toolkitDefinition "An expression of a work consisting of movement (e.g., dance) based on the source work."@en ;
    rdakit:toolkitLabel "adapted as choreography (expression)"@en ;
    a rdf:Property ;
    rdfs:domain <http://rdaregistry.info/Elements/c/C10006> ;
    rdfs:isDefinedBy <http://rdaregistry.info/Elements/e/> ;
    rdfs:label "is adapted as choreography (expression)"@en ;
    rdfs:range <http://rdaregistry.info/Elements/c/C10006> ;
    rdfs:subPropertyOf <http://rdaregistry.info/Elements/e/P20153> ;
    owl:inverseOf <http://rdaregistry.info/Elements/e/P20183> ;
    skos:definition "Relates an expression to an expression of a work consisting of movement (e.g., dance) based on the source work."@en .

<http://rdaregistry.info/Elements/e/P20093>
    reg:hasUnconstrained <http://rdaregistry.info/Elements/u/P60181> ;
    reg:lexicalAlias <http://rdaregistry.info/Elements/e/errataExpression.en> ;
    reg:name "errataExpression"@en ;
    reg:status <http://metadataregistry.org/uri/RegStatus/1001> ;
    rdakit:toolkitDefinition "An expression of a work consisting of errors discovered after the publication of the predominant work, with their corrections."@en ;
    rdakit:toolkitLabel "errata (expression)"@en ;
    a rdf:Property ;
    rdfs:domain <http://rdaregistry.info/Elements/c/C10006> ;
    rdfs:isDefinedBy <http://rdaregistry.info/Elements/e/> ;
    rdfs:label "is errata (expression)"@en ;
    rdfs:range <http://rdaregistry.info/Elements/c/C10006> ;
    rdfs:subPropertyOf <http://rdaregistry.info/Elements/e/P20105> ;
    owl:inverseOf <http://rdaregistry.info/Elements/e/P20146> ;
    skos:definition "Relates an expression to an expression of a work consisting of errors discovered after the publication of the predominant work, with their corrections."@en .

<http://rdaregistry.info/Elements/e/P20094>
    reg:hasUnconstrained <http://rdaregistry.info/Elements/u/P60182> ;
    reg:lexicalAlias <http://rdaregistry.info/Elements/e/illustrationsExpression.en> ;
    reg:name "illustrationsExpression"@en ;
    reg:status <http://metadataregistry.org/uri/RegStatus/1001> ;
    rdakit:toolkitDefinition "An expression of a work consisting of pictorial content designed to explain or decorate the augmented expression."@en ;
    rdakit:toolkitLabel "illustrations (expression)"@en ;
    a rdf:Property ;
    rdfs:domain <http://rdaregistry.info/Elements/c/C10006> ;
    rdfs:isDefinedBy <http://rdaregistry.info/Elements/e/> ;
    rdfs:label "is illustrations (expression)"@en ;
    rdfs:range <http://rdaregistry.info/Elements/c/C10006> ;
    rdfs:subPropertyOf <http://rdaregistry.info/Elements/e/P20105> ;
    owl:inverseOf <http://rdaregistry.info/Elements/e/P20148> ;
    skos:definition "Relates an expression to an expression of a work consisting of pictorial content designed to explain or decorate the augmented expression."@en .

<http://rdaregistry.info/Elements/e/P20095>
    reg:hasUnconstrained <http://rdaregistry.info/Elements/u/P60184> ;
    reg:lexicalAlias <http://rdaregistry.info/Elements/e/adaptedAsMotionPictureScreenplayExpression.en> ;
    reg:name "adaptedAsMotionPictureScreenplayExpression"@en ;
    reg:status <http://metadataregistry.org/uri/RegStatus/1001> ;
    rdakit:toolkitDefinition "An expression of a work consisting of the screenplay for a motion picture, based on the source work."@en ;
    rdakit:toolkitLabel "adapted as motion picture screenplay (expression)"@en ;
    a rdf:Property ;
    rdfs:domain <http://rdaregistry.info/Elements/c/C10006> ;
    rdfs:isDefinedBy <http://rdaregistry.info/Elements/e/> ;
    rdfs:label "is adapted as motion picture screenplay (expression)"@en ;
    rdfs:range <http://rdaregistry.info/Elements/c/C10006> ;
    rdfs:subPropertyOf <http://rdaregistry.info/Elements/e/P20096> ;
    owl:inverseOf <http://rdaregistry.info/Elements/e/P20130> ;
    skos:definition "Relates an expression to an expression of a work consisting of the screenplay for a motion picture, based on the source work."@en .

<http://rdaregistry.info/Elements/e/P20096>
    reg:hasSubproperty <http://rdaregistry.info/Elements/e/P20095>, <http://rdaregistry.info/Elements/e/P20097>, <http://rdaregistry.info/Elements/e/P20098> ;
    reg:hasUnconstrained <http://rdaregistry.info/Elements/u/P60185> ;
    reg:lexicalAlias <http://rdaregistry.info/Elements/e/adaptedAsScreenplayExpression.en> ;
    reg:name "adaptedAsScreenplayExpression"@en ;
    reg:status <http://metadataregistry.org/uri/RegStatus/1001> ;
    rdakit:toolkitDefinition "An expression of a work consisting of the screenplay for a motion picture, television program, or video, based on the source work."@en ;
    rdakit:toolkitLabel "adapted as screenplay (expression)"@en ;
    a rdf:Property ;
    rdfs:domain <http://rdaregistry.info/Elements/c/C10006> ;
    rdfs:isDefinedBy <http://rdaregistry.info/Elements/e/> ;
    rdfs:label "is adapted as screenplay (expression)"@en ;
    rdfs:range <http://rdaregistry.info/Elements/c/C10006> ;
    rdfs:subPropertyOf <http://rdaregistry.info/Elements/e/P20153> ;
    owl:inverseOf <http://rdaregistry.info/Elements/e/P20129> ;
    skos:definition "Relates an expression to an expression of a work consisting of the screenplay for a motion picture, television program, or video, based on the source work."@en .

<http://rdaregistry.info/Elements/e/P20097>
    reg:hasUnconstrained <http://rdaregistry.info/Elements/u/P60186> ;
    reg:lexicalAlias <http://rdaregistry.info/Elements/e/adaptedAsTelevisionScreenplayExpression.en> ;
    reg:name "adaptedAsTelevisionScreenplayExpression"@en ;
    reg:status <http://metadataregistry.org/uri/RegStatus/1001> ;
    rdakit:toolkitDefinition "An expression of a work consisting of the screenplay for a television program, based on the source work."@en ;
    rdakit:toolkitLabel "adapted as television screenplay (expression)"@en ;
    a rdf:Property ;
    rdfs:domain <http://rdaregistry.info/Elements/c/C10006> ;
    rdfs:isDefinedBy <http://rdaregistry.info/Elements/e/> ;
    rdfs:label "is adapted as television screenplay (expression)"@en ;
    rdfs:range <http://rdaregistry.info/Elements/c/C10006> ;
    rdfs:subPropertyOf <http://rdaregistry.info/Elements/e/P20096> ;
    owl:inverseOf <http://rdaregistry.info/Elements/e/P20131> ;
    skos:definition "Relates an expression to an expression of a work consisting of the screenplay for a television program, based on the source work."@en .

<http://rdaregistry.info/Elements/e/P20098>
    reg:hasUnconstrained <http://rdaregistry.info/Elements/u/P60187> ;
    reg:lexicalAlias <http://rdaregistry.info/Elements/e/adaptedAsVideoScreenplayExpression.en> ;
    reg:name "adaptedAsVideoScreenplayExpression"@en ;
    reg:status <http://metadataregistry.org/uri/RegStatus/1001> ;
    rdakit:toolkitDefinition "An expression of a work consisting of the screenplay for a video, based on the source work."@en ;
    rdakit:toolkitLabel "adapted as video screenplay (expression)"@en ;
    a rdf:Property ;
    rdfs:domain <http://rdaregistry.info/Elements/c/C10006> ;
    rdfs:isDefinedBy <http://rdaregistry.info/Elements/e/> ;
    rdfs:label "is adapted as video screenplay (expression)"@en ;
    rdfs:range <http://rdaregistry.info/Elements/c/C10006> ;
    rdfs:subPropertyOf <http://rdaregistry.info/Elements/e/P20096> ;
    owl:inverseOf <http://rdaregistry.info/Elements/e/P20132> ;
    skos:definition "Relates an expression to an expression of a work consisting of the screenplay for a video, based on the source work."@en .

<http://rdaregistry.info/Elements/e/P20099>
    reg:hasUnconstrained <http://rdaregistry.info/Elements/u/P60188> ;
    reg:lexicalAlias <http://rdaregistry.info/Elements/e/adaptedAsRadioScriptExpression.en> ;
    reg:name "adaptedAsRadioScriptExpression"@en ;
    reg:status <http://metadataregistry.org/uri/RegStatus/1001> ;
    rdakit:toolkitDefinition "An expression of a work consisting of the script for a radio program, based on the source work."@en ;
    rdakit:toolkitLabel "adapted as radio script (expression)"@en ;
    a rdf:Property ;
    rdfs:domain <http://rdaregistry.info/Elements/c/C10006> ;
    rdfs:isDefinedBy <http://rdaregistry.info/Elements/e/> ;
    rdfs:label "is adapted as radio script (expression)"@en ;
    rdfs:range <http://rdaregistry.info/Elements/c/C10006> ;
    rdfs:subPropertyOf <http://rdaregistry.info/Elements/e/P20153> ;
    owl:inverseOf <http://rdaregistry.info/Elements/e/P20133> ;
    skos:definition "Relates an expression to an expression of a work consisting of the script for a radio program, based on the source work."@en .

<http://rdaregistry.info/Elements/e/P20100>
    reg:hasSubproperty <http://rdaregistry.info/Elements/e/P20084>, <http://rdaregistry.info/Elements/e/P20102>, <http://rdaregistry.info/Elements/e/P20157>, <http://rdaregistry.info/Elements/e/P20160>, <http://rdaregistry.info/Elements/e/P20163>, <http://rdaregistry.info/Elements/e/P20176>, <http://rdaregistry.info/Elements/e/P20253>, <http://rdaregistry.info/Elements/e/P20254> ;
    reg:hasUnconstrained <http://rdaregistry.info/Elements/u/P60198> ;
    reg:lexicalAlias <http://rdaregistry.info/Elements/e/complementedByExpression.en> ;
    reg:name "complementedByExpression"@en ;
    reg:status <http://metadataregistry.org/uri/RegStatus/1001> ;
    rdakit:toolkitDefinition "An expression of a work paired with another expression without either expression being considered to predominate."@en ;
    rdakit:toolkitLabel "complemented by (expression)"@en ;
    a rdf:Property ;
    rdfs:domain <http://rdaregistry.info/Elements/c/C10006> ;
    rdfs:isDefinedBy <http://rdaregistry.info/Elements/e/> ;
    rdfs:label "is complemented by (expression)"@en ;
    rdfs:range <http://rdaregistry.info/Elements/c/C10006> ;
    rdfs:subPropertyOf <http://rdaregistry.info/Elements/e/P20232> ;
    owl:inverseOf <http://rdaregistry.info/Elements/e/P20100> ;
    skos:definition "Relates an expression to an expression of a work paired with another expression without either expression being considered to predominate."@en .

<http://rdaregistry.info/Elements/e/P20101>
    reg:hasUnconstrained <http://rdaregistry.info/Elements/u/P60199> ;
    reg:lexicalAlias <http://rdaregistry.info/Elements/e/continuedInPartByExpression.en> ;
    reg:name "continuedInPartByExpression"@en ;
    reg:status <http://metadataregistry.org/uri/RegStatus/1001> ;
    rdakit:toolkitDefinition "An expression of a work part of whose content separated from an earlier expression to form a new expression."@en ;
    rdakit:toolkitLabel "continued in part by (expression)"@en ;
    a rdf:Property ;
    rdfs:domain <http://rdaregistry.info/Elements/c/C10006> ;
    rdfs:isDefinedBy <http://rdaregistry.info/Elements/e/> ;
    rdfs:label "is continued in part by (expression)"@en ;
    rdfs:range <http://rdaregistry.info/Elements/c/C10006> ;
    rdfs:subPropertyOf <http://rdaregistry.info/Elements/e/P20169> ;
    owl:inverseOf <http://rdaregistry.info/Elements/e/P20168> ;
    skos:definition "Relates an expression to an expression of a work part of whose content separated from an earlier expression to form a new expression."@en .

<http://rdaregistry.info/Elements/e/P20102>
    reg:hasSubproperty <http://rdaregistry.info/Elements/e/P20173>, <http://rdaregistry.info/Elements/e/P20174>, <http://rdaregistry.info/Elements/e/P20175> ;
    reg:hasUnconstrained <http://rdaregistry.info/Elements/u/P60201> ;
    reg:lexicalAlias <http://rdaregistry.info/Elements/e/screenplayForExpression.en> ;
    reg:name "screenplayForExpression"@en ;
    reg:status <http://metadataregistry.org/uri/RegStatus/1001> ;
    rdakit:toolkitDefinition "An expression of a work such as a motion picture, television program, or video, that uses the text of the work as a screenplay."@en ;
    rdakit:toolkitLabel "screenplay for (expression)"@en ;
    a rdf:Property ;
    rdfs:domain <http://rdaregistry.info/Elements/c/C10006> ;
    rdfs:isDefinedBy <http://rdaregistry.info/Elements/e/> ;
    rdfs:label "is screenplay for (expression)"@en ;
    rdfs:range <http://rdaregistry.info/Elements/c/C10006> ;
    rdfs:subPropertyOf <http://rdaregistry.info/Elements/e/P20100> ;
    owl:inverseOf <http://rdaregistry.info/Elements/e/P20157> ;
    skos:definition "Relates an expression to an expression of a work such as a motion picture, television program, or video, that uses the text of the work as a screenplay."@en .

<http://rdaregistry.info/Elements/e/P20103>
    reg:hasUnconstrained <http://rdaregistry.info/Elements/u/P60202> ;
    reg:lexicalAlias <http://rdaregistry.info/Elements/e/incidentalMusicForExpression.en> ;
    reg:name "incidentalMusicForExpression"@en ;
    reg:status <http://metadataregistry.org/uri/RegStatus/1001> ;
    rdakit:toolkitDefinition "An expression of a work such as a play or other spoken work for the stage that uses the musical work as incidental music."@en ;
    rdakit:toolkitLabel "incidental music for (expression)"@en ;
    a rdf:Property ;
    rdfs:domain <http://rdaregistry.info/Elements/c/C10006> ;
    rdfs:isDefinedBy <http://rdaregistry.info/Elements/e/> ;
    rdfs:label "is incidental music for (expression)"@en ;
    rdfs:range <http://rdaregistry.info/Elements/c/C10006> ;
    rdfs:subPropertyOf <http://rdaregistry.info/Elements/e/P20244> ;
    owl:inverseOf <http://rdaregistry.info/Elements/e/P20085> ;
    skos:definition "Relates an expression to an expression of a work such as a play or other spoken work for the stage that uses the musical work as incidental music."@en .

<http://rdaregistry.info/Elements/e/P20104>
    reg:hasUnconstrained <http://rdaregistry.info/Elements/u/P60203> ;
    reg:lexicalAlias <http://rdaregistry.info/Elements/e/abstractedAsExpression.en> ;
    reg:name "abstractedAsExpression"@en ;
    reg:status <http://metadataregistry.org/uri/RegStatus/1001> ;
    rdakit:toolkitDefinition "An expression of a work that abbreviates the source expression in a brief, objective manner."@en ;
    rdakit:toolkitLabel "abstracted as (expression)"@en ;
    a rdf:Property ;
    rdfs:domain <http://rdaregistry.info/Elements/c/C10006> ;
    rdfs:isDefinedBy <http://rdaregistry.info/Elements/e/> ;
    rdfs:label "is abstracted as (expression)"@en ;
    rdfs:range <http://rdaregistry.info/Elements/c/C10006> ;
    rdfs:subPropertyOf <http://rdaregistry.info/Elements/e/P20203> ;
    owl:inverseOf <http://rdaregistry.info/Elements/e/P20122> ;
    skos:definition "Relates an expression to an expression of a work that abbreviates the source expression in a brief, objective manner."@en .

<http://rdaregistry.info/Elements/e/P20105>
    reg:hasSubproperty <http://rdaregistry.info/Elements/e/P20080>, <http://rdaregistry.info/Elements/e/P20093>, <http://rdaregistry.info/Elements/e/P20094>, <http://rdaregistry.info/Elements/e/P20107>, <http://rdaregistry.info/Elements/e/P20108>, <http://rdaregistry.info/Elements/e/P20109>, <http://rdaregistry.info/Elements/e/P20118>, <http://rdaregistry.info/Elements/e/P20120>, <http://rdaregistry.info/Elements/e/P20155>, <http://rdaregistry.info/Elements/e/P20156>, <http://rdaregistry.info/Elements/e/P20172> ;
    reg:hasUnconstrained <http://rdaregistry.info/Elements/u/P60204> ;
    reg:lexicalAlias <http://rdaregistry.info/Elements/e/augmentedByExpression.en> ;
    reg:name "augmentedByExpression"@en ;
    reg:status <http://metadataregistry.org/uri/RegStatus/1001> ;
    rdakit:toolkitDefinition "An expression of a work that adds to the content of a predominant expression."@en ;
    rdakit:toolkitLabel "augmented by (expression)"@en ;
    a rdf:Property ;
    rdfs:domain <http://rdaregistry.info/Elements/c/C10006> ;
    rdfs:isDefinedBy <http://rdaregistry.info/Elements/e/> ;
    rdfs:label "is augmented by (expression)"@en ;
    rdfs:range <http://rdaregistry.info/Elements/c/C10006> ;
    rdfs:subPropertyOf <http://rdaregistry.info/Elements/e/P20232> ;
    owl:inverseOf <http://rdaregistry.info/Elements/e/P20192> ;
    skos:definition "Relates an expression to an expression of a work that adds to the content of a predominant expression."@en .

<http://rdaregistry.info/Elements/e/P20106>
    reg:hasUnconstrained <http://rdaregistry.info/Elements/u/P60205> ;
    reg:lexicalAlias <http://rdaregistry.info/Elements/e/summarizedAsExpression.en> ;
    reg:name "summarizedAsExpression"@en ;
    reg:status <http://metadataregistry.org/uri/RegStatus/1001> ;
    rdakit:toolkitDefinition "An expression of a work that consists of a brief recapitulation of the content of the source expression."@en ;
    rdakit:toolkitLabel "summarized as (expression)"@en ;
    a rdf:Property ;
    rdfs:domain <http://rdaregistry.info/Elements/c/C10006> ;
    rdfs:isDefinedBy <http://rdaregistry.info/Elements/e/> ;
    rdfs:label "is summarized as (expression)"@en ;
    rdfs:range <http://rdaregistry.info/Elements/c/C10006> ;
    rdfs:subPropertyOf <http://rdaregistry.info/Elements/e/P20203> ;
    owl:inverseOf <http://rdaregistry.info/Elements/e/P20179> ;
    skos:definition "Relates an expression to an expression of a work that consists of a brief recapitulation of the content of the source expression."@en .

<http://rdaregistry.info/Elements/e/P20107>
    reg:hasUnconstrained <http://rdaregistry.info/Elements/u/P60206> ;
    reg:lexicalAlias <http://rdaregistry.info/Elements/e/catalogueExpression.en> ;
    reg:name "catalogueExpression"@en ;
    reg:status <http://metadataregistry.org/uri/RegStatus/1001> ;
    rdakit:toolkitDefinition "An expression of a work that consists of a complete enumeration of items arranged systematically."@en ;
    rdakit:toolkitLabel "catalogue (expression)"@en ;
    a rdf:Property ;
    rdfs:domain <http://rdaregistry.info/Elements/c/C10006> ;
    rdfs:isDefinedBy <http://rdaregistry.info/Elements/e/> ;
    rdfs:label "is catalogue (expression)"@en ;
    rdfs:range <http://rdaregistry.info/Elements/c/C10006> ;
    rdfs:subPropertyOf <http://rdaregistry.info/Elements/e/P20105> ;
    owl:inverseOf <http://rdaregistry.info/Elements/e/P20180> ;
    skos:definition "Relates an expression to an expression of a work that consists of a complete enumeration of items arranged systematically."@en .

<http://rdaregistry.info/Elements/e/P20108>
    reg:hasUnconstrained <http://rdaregistry.info/Elements/u/P60208> ;
    reg:lexicalAlias <http://rdaregistry.info/Elements/e/concordanceExpression.en> ;
    reg:name "concordanceExpression"@en ;
    reg:status <http://metadataregistry.org/uri/RegStatus/1001> ;
    rdakit:toolkitDefinition "An expression of a work that consists of an index of all the words in the predominant expression."@en ;
    rdakit:toolkitLabel "concordance (expression)"@en ;
    a rdf:Property ;
    rdfs:domain <http://rdaregistry.info/Elements/c/C10006> ;
    rdfs:isDefinedBy <http://rdaregistry.info/Elements/e/> ;
    rdfs:label "is concordance (expression)"@en ;
    rdfs:range <http://rdaregistry.info/Elements/c/C10006> ;
    rdfs:subPropertyOf <http://rdaregistry.info/Elements/e/P20105> ;
    owl:inverseOf <http://rdaregistry.info/Elements/e/P20181> ;
    skos:definition "Relates an expression to an expression of a work that consists of an index of all the words in the predominant expression."@en .

<http://rdaregistry.info/Elements/e/P20109>
    reg:hasUnconstrained <http://rdaregistry.info/Elements/u/P60209> ;
    reg:lexicalAlias <http://rdaregistry.info/Elements/e/addendaExpression.en> ;
    reg:name "addendaExpression"@en ;
    reg:status <http://metadataregistry.org/uri/RegStatus/1001> ;
    rdakit:toolkitDefinition "An expression of a work that consists of brief additional material, less extensive than a supplement, but essential to the completeness of the text of the predominant work; it is usually added at the end of the content, but is sometimes issued separately."@en ;
    rdakit:toolkitLabel "addenda (expression)"@en ;
    a rdf:Property ;
    rdfs:domain <http://rdaregistry.info/Elements/c/C10006> ;
    rdfs:isDefinedBy <http://rdaregistry.info/Elements/e/> ;
    rdfs:label "is addenda (expression)"@en ;
    rdfs:range <http://rdaregistry.info/Elements/c/C10006> ;
    rdfs:subPropertyOf <http://rdaregistry.info/Elements/e/P20105> ;
    owl:inverseOf <http://rdaregistry.info/Elements/e/P20177> ;
    skos:definition "Relates an expression to an expression of a work that consists of brief additional material, less extensive than a supplement, but essential to the completeness of the text of the predominant work; it is usually added at the end of the content, but is sometimes issued separately."@en .

<http://rdaregistry.info/Elements/e/P20110>
    reg:hasUnconstrained <http://rdaregistry.info/Elements/u/P60210> ;
    reg:lexicalAlias <http://rdaregistry.info/Elements/e/adaptedAsLibrettoExpression.en> ;
    reg:name "adaptedAsLibrettoExpression"@en ;
    reg:status <http://metadataregistry.org/uri/RegStatus/1001> ;
    rdakit:toolkitDefinition "An expression of a work that consists of the text of an opera or other work for the musical stage, or an oratorio, based on the source work."@en ;
    rdakit:toolkitLabel "adapted as libretto (expression)"@en ;
    a rdf:Property ;
    rdfs:domain <http://rdaregistry.info/Elements/c/C10006> ;
    rdfs:isDefinedBy <http://rdaregistry.info/Elements/e/> ;
    rdfs:label "is adapted as libretto (expression)"@en ;
    rdfs:range <http://rdaregistry.info/Elements/c/C10006> ;
    rdfs:subPropertyOf <http://rdaregistry.info/Elements/e/P20153> ;
    owl:inverseOf <http://rdaregistry.info/Elements/e/P20190> ;
    skos:definition "Relates an expression to an expression of a work consisting of the text of an opera or other work for the musical stage, or an oratorio, based on the source work."@en .

<http://rdaregistry.info/Elements/e/P20111>
    reg:status <http://metadataregistry.org/uri/RegStatus/1008> ;
    a rdf:Property ;
    rdfs:isDefinedBy <http://rdaregistry.info/Elements/e/> .

<http://rdaregistry.info/Elements/e/P20112>
    reg:status <http://metadataregistry.org/uri/RegStatus/1008> ;
    a rdf:Property ;
    rdfs:isDefinedBy <http://rdaregistry.info/Elements/e/> .

<http://rdaregistry.info/Elements/e/P20113>
    reg:status <http://metadataregistry.org/uri/RegStatus/1008> ;
    a rdf:Property ;
    rdfs:isDefinedBy <http://rdaregistry.info/Elements/e/> .

<http://rdaregistry.info/Elements/e/P20114>
    reg:hasSubproperty <http://rdaregistry.info/Elements/e/P20142> ;
    reg:hasUnconstrained <http://rdaregistry.info/Elements/u/P60214> ;
    reg:lexicalAlias <http://rdaregistry.info/Elements/e/imitatedAsExpression.en> ;
    reg:name "imitatedAsExpression"@en ;
    reg:status <http://metadataregistry.org/uri/RegStatus/1001> ;
    rdakit:toolkitDefinition "An expression of a work that copies the style or content of the source work."@en ;
    rdakit:toolkitLabel "imitated as (expression)"@en ;
    a rdf:Property ;
    rdfs:domain <http://rdaregistry.info/Elements/c/C10006> ;
    rdfs:isDefinedBy <http://rdaregistry.info/Elements/e/> ;
    rdfs:label "is imitated as (expression)"@en ;
    rdfs:range <http://rdaregistry.info/Elements/c/C10006> ;
    rdfs:subPropertyOf <http://rdaregistry.info/Elements/e/P20203> ;
    owl:inverseOf <http://rdaregistry.info/Elements/e/P20195> ;
    skos:definition "Relates an expression to an expression of a work that copies the style or content of the source work."@en .

<http://rdaregistry.info/Elements/e/P20115>
    reg:hasUnconstrained <http://rdaregistry.info/Elements/u/P60216> ;
    reg:lexicalAlias <http://rdaregistry.info/Elements/e/expandedAsExpression.en> ;
    reg:name "expandedAsExpression"@en ;
    reg:status <http://metadataregistry.org/uri/RegStatus/1001> ;
    rdakit:toolkitDefinition "An expression of a work that enlarges upon the content of the source work."@en ;
    rdakit:toolkitLabel "expanded as (expression)"@en ;
    a rdf:Property ;
    rdfs:domain <http://rdaregistry.info/Elements/c/C10006> ;
    rdfs:isDefinedBy <http://rdaregistry.info/Elements/e/> ;
    rdfs:label "is expanded as (expression)"@en ;
    rdfs:range <http://rdaregistry.info/Elements/c/C10006> ;
    rdfs:subPropertyOf <http://rdaregistry.info/Elements/e/P20203> ;
    owl:inverseOf <http://rdaregistry.info/Elements/e/P20184> ;
    skos:definition "Relates an expression to an expression of a work that enlarges upon the content of the source work."@en .

<http://rdaregistry.info/Elements/e/P20116>
    reg:status <http://metadataregistry.org/uri/RegStatus/1008> ;
    a rdf:Property ;
    rdfs:isDefinedBy <http://rdaregistry.info/Elements/e/> .

<http://rdaregistry.info/Elements/e/P20117>
    reg:status <http://metadataregistry.org/uri/RegStatus/1008> ;
    a rdf:Property ;
    rdfs:isDefinedBy <http://rdaregistry.info/Elements/e/> .

<http://rdaregistry.info/Elements/e/P20118>
    reg:hasUnconstrained <http://rdaregistry.info/Elements/u/P60221> ;
    reg:lexicalAlias <http://rdaregistry.info/Elements/e/appendixExpression.en> ;
    reg:name "appendixExpression"@en ;
    reg:status <http://metadataregistry.org/uri/RegStatus/1001> ;
    rdakit:toolkitDefinition "An expression of a work that forms an augmenting part of another work which is not essential to the completeness of the content, such as a list of references, statistical tables, and explanatory matter; it can be material which either comes at the end of the content of the predominant work, or is issued separately."@en ;
    rdakit:toolkitLabel "appendix (expression)"@en ;
    a rdf:Property ;
    rdfs:domain <http://rdaregistry.info/Elements/c/C10006> ;
    rdfs:isDefinedBy <http://rdaregistry.info/Elements/e/> ;
    rdfs:label "is appendix (expression)"@en ;
    rdfs:range <http://rdaregistry.info/Elements/c/C10006> ;
    rdfs:subPropertyOf <http://rdaregistry.info/Elements/e/P20105> ;
    owl:inverseOf <http://rdaregistry.info/Elements/e/P20089> ;
    skos:definition "Relates an expression to an expression of a work that forms an augmenting part of another work which is not essential to the completeness of the content, such as a list of references, statistical tables, and explanatory matter; it can be material which either comes at the end of the content of the predominant work, or is issued separately."@en .

<http://rdaregistry.info/Elements/e/P20119>
    reg:hasUnconstrained <http://rdaregistry.info/Elements/u/P60189> ;
    reg:lexicalAlias <http://rdaregistry.info/Elements/e/freelyTranslatedAsExpression.en> ;
    reg:name "freelyTranslatedAsExpression"@en ;
    reg:status <http://metadataregistry.org/uri/RegStatus/1001> ;
    rdakit:toolkitDefinition "An expression of a work that freely translates the text into another language, preserving the spirit of the original, but not its linguistic details."@en ;
    rdakit:toolkitLabel "freely translated as (expression)"@en ;
    a rdf:Property ;
    rdfs:domain <http://rdaregistry.info/Elements/c/C10006> ;
    rdfs:isDefinedBy <http://rdaregistry.info/Elements/e/> ;
    rdfs:label "is freely translated as (expression)"@en ;
    rdfs:range <http://rdaregistry.info/Elements/c/C10006> ;
    rdfs:subPropertyOf <http://rdaregistry.info/Elements/e/P20203> ;
    owl:inverseOf <http://rdaregistry.info/Elements/e/P20140> ;
    skos:definition "Relates an expression to an expression of a work that freely translates the text into another language, preserving the spirit of the original, but not its linguistic details."@en .

<http://rdaregistry.info/Elements/e/P20120>
    reg:hasUnconstrained <http://rdaregistry.info/Elements/u/P60222> ;
    reg:lexicalAlias <http://rdaregistry.info/Elements/e/guideExpression.en> ;
    reg:name "guideExpression"@en ;
    reg:status <http://metadataregistry.org/uri/RegStatus/1001> ;
    rdakit:toolkitDefinition "An expression of a work that guides a user through the use of the predominant work, using notes, learning and study aids, exercises, problems, questions and answers, instructor or student materials, etc."@en ;
    rdakit:toolkitLabel "guide (expression)"@en ;
    a rdf:Property ;
    rdfs:domain <http://rdaregistry.info/Elements/c/C10006> ;
    rdfs:isDefinedBy <http://rdaregistry.info/Elements/e/> ;
    rdfs:label "is guide (expression)"@en ;
    rdfs:range <http://rdaregistry.info/Elements/c/C10006> ;
    rdfs:subPropertyOf <http://rdaregistry.info/Elements/e/P20105> ;
    owl:inverseOf <http://rdaregistry.info/Elements/e/P20147> ;
    skos:definition "Relates an expression to an expression of a work that guides a user through the use of the predominant work, using notes, learning and study aids, exercises, problems, questions and answers, instructor or student materials, etc."@en .

<http://rdaregistry.info/Elements/e/P20121>
    reg:hasUnconstrained <http://rdaregistry.info/Elements/u/P60223> ;
    reg:lexicalAlias <http://rdaregistry.info/Elements/e/abridgementOfExpression.en> ;
    reg:name "abridgementOfExpression"@en ;
    reg:status <http://metadataregistry.org/uri/RegStatus/1001> ;
    rdakit:toolkitDefinition "An expression of a work that has been abridged, i.e., shortened without changing the general meaning or manner of presentation of the source work."@en ;
    rdakit:toolkitLabel "abridgement of (expression)"@en ;
    a rdf:Property ;
    rdfs:domain <http://rdaregistry.info/Elements/c/C10006> ;
    rdfs:isDefinedBy <http://rdaregistry.info/Elements/e/> ;
    rdfs:label "is abridgement of (expression)"@en ;
    rdfs:range <http://rdaregistry.info/Elements/c/C10006> ;
    rdfs:subPropertyOf <http://rdaregistry.info/Elements/e/P20204> ;
    owl:inverseOf <http://rdaregistry.info/Elements/e/P20166> ;
    skos:definition "Relates an expression to an expression of a work that has been abridged, i.e., shortened without changing the general meaning or manner of presentation of the source work."@en .

<http://rdaregistry.info/Elements/e/P20122>
    reg:hasUnconstrained <http://rdaregistry.info/Elements/u/P60224> ;
    reg:lexicalAlias <http://rdaregistry.info/Elements/e/abstractOfExpression.en> ;
    reg:name "abstractOfExpression"@en ;
    reg:status <http://metadataregistry.org/uri/RegStatus/1001> ;
    rdakit:toolkitDefinition "An expression of a work that has been abstracted, i.e., abbreviated in a brief, objective manner."@en ;
    rdakit:toolkitLabel "abstract of (expression)"@en ;
    a rdf:Property ;
    rdfs:domain <http://rdaregistry.info/Elements/c/C10006> ;
    rdfs:isDefinedBy <http://rdaregistry.info/Elements/e/> ;
    rdfs:label "is abstract of (expression)"@en ;
    rdfs:range <http://rdaregistry.info/Elements/c/C10006> ;
    rdfs:subPropertyOf <http://rdaregistry.info/Elements/e/P20204> ;
    owl:inverseOf <http://rdaregistry.info/Elements/e/P20104> ;
    skos:definition "Relates an expression to an expression of a work that has been abstracted, i.e., abbreviated in a brief, objective manner."@en .

<http://rdaregistry.info/Elements/e/P20123>
    reg:hasUnconstrained <http://rdaregistry.info/Elements/u/P60225> ;
    reg:lexicalAlias <http://rdaregistry.info/Elements/e/dramatizationOfExpression.en> ;
    reg:name "dramatizationOfExpression"@en ;
    reg:status <http://metadataregistry.org/uri/RegStatus/1001> ;
    rdakit:toolkitDefinition "An expression of a work that has been adapted as a drama."@en ;
    rdakit:toolkitLabel "dramatization of (expression)"@en ;
    a rdf:Property ;
    rdfs:domain <http://rdaregistry.info/Elements/c/C10006> ;
    rdfs:isDefinedBy <http://rdaregistry.info/Elements/e/> ;
    rdfs:label "is dramatization of (expression)"@en ;
    rdfs:range <http://rdaregistry.info/Elements/c/C10006> ;
    rdfs:subPropertyOf <http://rdaregistry.info/Elements/e/P20152> ;
    owl:inverseOf <http://rdaregistry.info/Elements/e/P20073> ;
    skos:definition "Relates an expression to an expression of a work that has been adapted as a drama."@en .

<http://rdaregistry.info/Elements/e/P20124>
    reg:hasUnconstrained <http://rdaregistry.info/Elements/u/P60226> ;
    reg:lexicalAlias <http://rdaregistry.info/Elements/e/verseAdaptationOfExpression.en> ;
    reg:name "verseAdaptationOfExpression"@en ;
    reg:status <http://metadataregistry.org/uri/RegStatus/1001> ;
    rdakit:toolkitDefinition "An expression of a work that has been adapted as a literary composition in verse form."@en ;
    rdakit:toolkitLabel "verse adaptation of (expression)"@en ;
    a rdf:Property ;
    rdfs:domain <http://rdaregistry.info/Elements/c/C10006> ;
    rdfs:isDefinedBy <http://rdaregistry.info/Elements/e/> ;
    rdfs:label "is verse adaptation of (expression)"@en ;
    rdfs:range <http://rdaregistry.info/Elements/c/C10006> ;
    rdfs:subPropertyOf <http://rdaregistry.info/Elements/e/P20152> ;
    owl:inverseOf <http://rdaregistry.info/Elements/e/P20077> ;
    skos:definition "Relates an expression to an expression of a work that has been adapted as a literary composition in verse form."@en .

<http://rdaregistry.info/Elements/e/P20125>
    reg:hasUnconstrained <http://rdaregistry.info/Elements/u/P60227> ;
    reg:lexicalAlias <http://rdaregistry.info/Elements/e/motionPictureAdaptationOfExpression.en> ;
    reg:name "motionPictureAdaptationOfExpression"@en ;
    reg:status <http://metadataregistry.org/uri/RegStatus/1001> ;
    rdakit:toolkitDefinition "An expression of a work that has been adapted as a motion picture."@en ;
    rdakit:toolkitLabel "motion picture adaptation of (expression)"@en ;
    a rdf:Property ;
    rdfs:domain <http://rdaregistry.info/Elements/c/C10006> ;
    rdfs:isDefinedBy <http://rdaregistry.info/Elements/e/> ;
    rdfs:label "is motion picture adaptation of (expression)"@en ;
    rdfs:range <http://rdaregistry.info/Elements/c/C10006> ;
    rdfs:subPropertyOf <http://rdaregistry.info/Elements/e/P20152> ;
    owl:inverseOf <http://rdaregistry.info/Elements/e/P20009> ;
    skos:definition "Relates an expression to an expression of a work that has been adapted as a motion picture."@en .

<http://rdaregistry.info/Elements/e/P20126>
    reg:hasUnconstrained <http://rdaregistry.info/Elements/u/P60228> ;
    reg:lexicalAlias <http://rdaregistry.info/Elements/e/novelizationOfExpression.en> ;
    reg:name "novelizationOfExpression"@en ;
    reg:status <http://metadataregistry.org/uri/RegStatus/1001> ;
    rdakit:toolkitDefinition "An expression of a work that has been adapted as a novel."@en ;
    rdakit:toolkitLabel "novelization of (expression)"@en ;
    a rdf:Property ;
    rdfs:domain <http://rdaregistry.info/Elements/c/C10006> ;
    rdfs:isDefinedBy <http://rdaregistry.info/Elements/e/> ;
    rdfs:label "is novelization of (expression)"@en ;
    rdfs:range <http://rdaregistry.info/Elements/c/C10006> ;
    rdfs:subPropertyOf <http://rdaregistry.info/Elements/e/P20152> ;
    owl:inverseOf <http://rdaregistry.info/Elements/e/P20088> ;
    skos:definition "Relates an expression to an expression of a work that has been adapted as a novel."@en .

<http://rdaregistry.info/Elements/e/P20127>
    reg:hasUnconstrained <http://rdaregistry.info/Elements/u/P60229> ;
    reg:lexicalAlias <http://rdaregistry.info/Elements/e/radioAdaptationOfExpression.en> ;
    reg:name "radioAdaptationOfExpression"@en ;
    reg:status <http://metadataregistry.org/uri/RegStatus/1001> ;
    rdakit:toolkitDefinition "An expression of a work that has been adapted as a radio program."@en ;
    rdakit:toolkitLabel "radio adaptation of (expression)"@en ;
    a rdf:Property ;
    rdfs:domain <http://rdaregistry.info/Elements/c/C10006> ;
    rdfs:isDefinedBy <http://rdaregistry.info/Elements/e/> ;
    rdfs:label "is radio adaptation of (expression)"@en ;
    rdfs:range <http://rdaregistry.info/Elements/c/C10006> ;
    rdfs:subPropertyOf <http://rdaregistry.info/Elements/e/P20152> ;
    owl:inverseOf <http://rdaregistry.info/Elements/e/P20060> ;
    skos:definition "Relates an expression to an expression of a work that has been adapted as a radio program."@en .

<http://rdaregistry.info/Elements/e/P20128>
    reg:hasUnconstrained <http://rdaregistry.info/Elements/u/P60230> ;
    reg:lexicalAlias <http://rdaregistry.info/Elements/e/televisionAdaptationOfExpression.en> ;
    reg:name "televisionAdaptationOfExpression"@en ;
    reg:status <http://metadataregistry.org/uri/RegStatus/1001> ;
    rdakit:toolkitDefinition "An expression of a work that has been adapted as a television program."@en ;
    rdakit:toolkitLabel "television adaptation of (expression)"@en ;
    a rdf:Property ;
    rdfs:domain <http://rdaregistry.info/Elements/c/C10006> ;
    rdfs:isDefinedBy <http://rdaregistry.info/Elements/e/> ;
    rdfs:label "is television adaptation of (expression)"@en ;
    rdfs:range <http://rdaregistry.info/Elements/c/C10006> ;
    rdfs:subPropertyOf <http://rdaregistry.info/Elements/e/P20152> ;
    owl:inverseOf <http://rdaregistry.info/Elements/e/P20066> ;
    skos:definition "Relates an expression to an expression of a work that has been adapted as a television program."@en .

<http://rdaregistry.info/Elements/e/P20129>
    reg:hasSubproperty <http://rdaregistry.info/Elements/e/P20130>, <http://rdaregistry.info/Elements/e/P20131>, <http://rdaregistry.info/Elements/e/P20132> ;
    reg:hasUnconstrained <http://rdaregistry.info/Elements/u/P60231> ;
    reg:lexicalAlias <http://rdaregistry.info/Elements/e/screenplayBasedOnExpression.en> ;
    reg:name "screenplayBasedOnExpression"@en ;
    reg:status <http://metadataregistry.org/uri/RegStatus/1001> ;
    rdakit:toolkitDefinition "An expression of a work that has been adapted as the screenplay for a motion picture, television program, or video."@en ;
    rdakit:toolkitLabel "screenplay based on (expression)"@en ;
    a rdf:Property ;
    rdfs:domain <http://rdaregistry.info/Elements/c/C10006> ;
    rdfs:isDefinedBy <http://rdaregistry.info/Elements/e/> ;
    rdfs:label "is screenplay based on (expression)"@en ;
    rdfs:range <http://rdaregistry.info/Elements/c/C10006> ;
    rdfs:subPropertyOf <http://rdaregistry.info/Elements/e/P20152> ;
    owl:inverseOf <http://rdaregistry.info/Elements/e/P20096> ;
    skos:definition "Relates an expression to an expression of a work that has been adapted as the screenplay for a motion picture, television program, or video."@en .

<http://rdaregistry.info/Elements/e/P20130>
    reg:hasUnconstrained <http://rdaregistry.info/Elements/u/P60232> ;
    reg:lexicalAlias <http://rdaregistry.info/Elements/e/motionPictureScreenplayBasedOnExpression.en> ;
    reg:name "motionPictureScreenplayBasedOnExpression"@en ;
    reg:status <http://metadataregistry.org/uri/RegStatus/1001> ;
    rdakit:toolkitDefinition "An expression of a work that has been adapted as the screenplay for a motion picture."@en ;
    rdakit:toolkitLabel "motion picture screenplay based on (expression)"@en ;
    a rdf:Property ;
    rdfs:domain <http://rdaregistry.info/Elements/c/C10006> ;
    rdfs:isDefinedBy <http://rdaregistry.info/Elements/e/> ;
    rdfs:label "is motion picture screenplay based on (expression)"@en ;
    rdfs:range <http://rdaregistry.info/Elements/c/C10006> ;
    rdfs:subPropertyOf <http://rdaregistry.info/Elements/e/P20129> ;
    owl:inverseOf <http://rdaregistry.info/Elements/e/P20095> ;
    skos:definition "Relates an expression to an expression of a work that has been adapted as the screenplay for a motion picture."@en .

<http://rdaregistry.info/Elements/e/P20131>
    reg:hasUnconstrained <http://rdaregistry.info/Elements/u/P60233> ;
    reg:lexicalAlias <http://rdaregistry.info/Elements/e/televisionScreenplayBasedOnExpression.en> ;
    reg:name "televisionScreenplayBasedOnExpression"@en ;
    reg:status <http://metadataregistry.org/uri/RegStatus/1001> ;
    rdakit:toolkitDefinition "An expression of a work that has been adapted as the screenplay for a television program."@en ;
    rdakit:toolkitLabel "television screenplay based on (expression)"@en ;
    a rdf:Property ;
    rdfs:domain <http://rdaregistry.info/Elements/c/C10006> ;
    rdfs:isDefinedBy <http://rdaregistry.info/Elements/e/> ;
    rdfs:label "is television screenplay based on (expression)"@en ;
    rdfs:range <http://rdaregistry.info/Elements/c/C10006> ;
    rdfs:subPropertyOf <http://rdaregistry.info/Elements/e/P20129> ;
    owl:inverseOf <http://rdaregistry.info/Elements/e/P20097> ;
    skos:definition "Relates an expression to an expression of a work that has been adapted as the screenplay for a television program."@en .

<http://rdaregistry.info/Elements/e/P20132>
    reg:hasUnconstrained <http://rdaregistry.info/Elements/u/P60234> ;
    reg:lexicalAlias <http://rdaregistry.info/Elements/e/videoScreenplayBasedOnExpression.en> ;
    reg:name "videoScreenplayBasedOnExpression"@en ;
    reg:status <http://metadataregistry.org/uri/RegStatus/1001> ;
    rdakit:toolkitDefinition "An expression of a work that has been adapted as the screenplay for a video."@en ;
    rdakit:toolkitLabel "video screenplay based on (expression)"@en ;
    a rdf:Property ;
    rdfs:domain <http://rdaregistry.info/Elements/c/C10006> ;
    rdfs:isDefinedBy <http://rdaregistry.info/Elements/e/> ;
    rdfs:label "is video screenplay based on (expression)"@en ;
    rdfs:range <http://rdaregistry.info/Elements/c/C10006> ;
    rdfs:subPropertyOf <http://rdaregistry.info/Elements/e/P20129> ;
    owl:inverseOf <http://rdaregistry.info/Elements/e/P20098> ;
    skos:definition "Relates an expression to an expression of a work that has been adapted as the screenplay for a video."@en .

<http://rdaregistry.info/Elements/e/P20133>
    reg:hasUnconstrained <http://rdaregistry.info/Elements/u/P60235> ;
    reg:lexicalAlias <http://rdaregistry.info/Elements/e/radioScriptBasedOnExpression.en> ;
    reg:name "radioScriptBasedOnExpression"@en ;
    reg:status <http://metadataregistry.org/uri/RegStatus/1001> ;
    rdakit:toolkitDefinition "An expression of a work that has been adapted as the script for a radio program."@en ;
    rdakit:toolkitLabel "radio script based on (expression)"@en ;
    a rdf:Property ;
    rdfs:domain <http://rdaregistry.info/Elements/c/C10006> ;
    rdfs:isDefinedBy <http://rdaregistry.info/Elements/e/> ;
    rdfs:label "is radio script based on (expression)"@en ;
    rdfs:range <http://rdaregistry.info/Elements/c/C10006> ;
    rdfs:subPropertyOf <http://rdaregistry.info/Elements/e/P20152> ;
    owl:inverseOf <http://rdaregistry.info/Elements/e/P20099> ;
    skos:definition "Relates an expression to an expression of a work that has been adapted as the script for a radio program."@en .

<http://rdaregistry.info/Elements/e/P20134>
    reg:hasUnconstrained <http://rdaregistry.info/Elements/u/P60236> ;
    reg:lexicalAlias <http://rdaregistry.info/Elements/e/videoAdaptationOfExpression.en> ;
    reg:name "videoAdaptationOfExpression"@en ;
    reg:status <http://metadataregistry.org/uri/RegStatus/1001> ;
    rdakit:toolkitDefinition "An expression of a work that has been adapted for video."@en ;
    rdakit:toolkitLabel "video adaptation of (expression)"@en ;
    a rdf:Property ;
    rdfs:domain <http://rdaregistry.info/Elements/c/C10006> ;
    rdfs:isDefinedBy <http://rdaregistry.info/Elements/e/> ;
    rdfs:label "is video adaptation of (expression)"@en ;
    rdfs:range <http://rdaregistry.info/Elements/c/C10006> ;
    rdfs:subPropertyOf <http://rdaregistry.info/Elements/e/P20152> ;
    owl:inverseOf <http://rdaregistry.info/Elements/e/P20067> ;
    skos:definition "Relates an expression to an expression of a work that has been adapted for video."@en .

<http://rdaregistry.info/Elements/e/P20135>
    reg:hasUnconstrained <http://rdaregistry.info/Elements/u/P60238> ;
    reg:lexicalAlias <http://rdaregistry.info/Elements/e/digestOfExpression.en> ;
    reg:name "digestOfExpression"@en ;
    reg:status <http://metadataregistry.org/uri/RegStatus/1001> ;
    rdakit:toolkitDefinition "An expression of a work that has been digested, i.e., systematically and comprehensively condensed."@en ;
    rdakit:toolkitLabel "digest of (expression)"@en ;
    a rdf:Property ;
    rdfs:domain <http://rdaregistry.info/Elements/c/C10006> ;
    rdfs:isDefinedBy <http://rdaregistry.info/Elements/e/> ;
    rdfs:label "is digest of (expression)"@en ;
    rdfs:range <http://rdaregistry.info/Elements/c/C10006> ;
    rdfs:subPropertyOf <http://rdaregistry.info/Elements/e/P20204> ;
    owl:inverseOf <http://rdaregistry.info/Elements/e/P20170> ;
    skos:definition "Relates an expression to an expression of a work that has been digested, i.e., systematically and comprehensively condensed."@en .

<http://rdaregistry.info/Elements/e/P20136>
    reg:status <http://metadataregistry.org/uri/RegStatus/1008> ;
    a rdf:Property ;
    rdfs:isDefinedBy <http://rdaregistry.info/Elements/e/> .

<http://rdaregistry.info/Elements/e/P20137>
    reg:hasUnconstrained <http://rdaregistry.info/Elements/u/P60574> ;
    reg:lexicalAlias <http://rdaregistry.info/Elements/e/absorptionOfExpression.en> ;
    reg:name "absorptionOfExpression"@en ;
    reg:status <http://metadataregistry.org/uri/RegStatus/1001> ;
    rdakit:toolkitDefinition "An expression of a work that has been incorporated into another expression."@en ;
    rdakit:toolkitLabel "absorption of (expression)"@en ;
    a rdf:Property ;
    rdfs:domain <http://rdaregistry.info/Elements/c/C10006> ;
    rdfs:isDefinedBy <http://rdaregistry.info/Elements/e/> ;
    rdfs:label "is absorption of (expression)"@en ;
    rdfs:range <http://rdaregistry.info/Elements/c/C10006> ;
    rdfs:subPropertyOf <http://rdaregistry.info/Elements/e/P20154> ;
    owl:inverseOf <http://rdaregistry.info/Elements/e/P20143> ;
    skos:definition "Relates an expression to an expression of a work that has been incorporated into another expression."@en .

<http://rdaregistry.info/Elements/e/P20138>
    reg:hasUnconstrained <http://rdaregistry.info/Elements/u/P60575> ;
    reg:lexicalAlias <http://rdaregistry.info/Elements/e/absorptionInPartOfExpression.en> ;
    reg:name "absorptionInPartOfExpression"@en ;
    reg:status <http://metadataregistry.org/uri/RegStatus/1001> ;
    rdakit:toolkitDefinition "An expression of a work that has been partially incorporated into another expression."@en ;
    rdakit:toolkitLabel "absorption in part of (expression)"@en ;
    a rdf:Property ;
    rdfs:domain <http://rdaregistry.info/Elements/c/C10006> ;
    rdfs:isDefinedBy <http://rdaregistry.info/Elements/e/> ;
    rdfs:label "is absorption in part of (expression)"@en ;
    rdfs:range <http://rdaregistry.info/Elements/c/C10006> ;
    rdfs:subPropertyOf <http://rdaregistry.info/Elements/e/P20154> ;
    owl:inverseOf <http://rdaregistry.info/Elements/e/P20144> ;
    skos:definition "Relates an expression to an expression of a work that has been partially incorporated into another expression."@en .

<http://rdaregistry.info/Elements/e/P20139>
    reg:hasUnconstrained <http://rdaregistry.info/Elements/u/P60242> ;
    reg:lexicalAlias <http://rdaregistry.info/Elements/e/arrangementOf.en> ;
    reg:name "arrangementOf"@en ;
    reg:status <http://metadataregistry.org/uri/RegStatus/1001> ;
    rdakit:toolkitDefinition "An expression of a musical work that has been rewritten for a medium of performance different from that for which the work was originally intended."@en ;
    rdakit:toolkitLabel "arrangement of"@en ;
    a rdf:Property ;
    rdfs:domain <http://rdaregistry.info/Elements/c/C10006> ;
    rdfs:isDefinedBy <http://rdaregistry.info/Elements/e/> ;
    rdfs:label "is arrangement of"@en ;
    rdfs:range <http://rdaregistry.info/Elements/c/C10006> ;
    rdfs:subPropertyOf <http://rdaregistry.info/Elements/e/P20204> ;
    owl:inverseOf <http://rdaregistry.info/Elements/e/P20165> ;
    skos:definition "Relates an expression to an expression of a musical work that has been rewritten for a medium of performance different from that for which the work was originally intended."@en .

<http://rdaregistry.info/Elements/e/P20140>
    reg:hasUnconstrained <http://rdaregistry.info/Elements/u/P60243> ;
    reg:lexicalAlias <http://rdaregistry.info/Elements/e/freeTranslationOfExpression.en> ;
    reg:name "freeTranslationOfExpression"@en ;
    reg:status <http://metadataregistry.org/uri/RegStatus/1001> ;
    rdakit:toolkitDefinition "An expression of a work that has been translated freely, preserving the spirit of the original, but not its linguistic details."@en ;
    rdakit:toolkitLabel "free translation of (expression)"@en ;
    a rdf:Property ;
    rdfs:domain <http://rdaregistry.info/Elements/c/C10006> ;
    rdfs:isDefinedBy <http://rdaregistry.info/Elements/e/> ;
    rdfs:label "is free translation of (expression)"@en ;
    rdfs:range <http://rdaregistry.info/Elements/c/C10006> ;
    rdfs:subPropertyOf <http://rdaregistry.info/Elements/e/P20204> ;
    owl:inverseOf <http://rdaregistry.info/Elements/e/P20119> ;
    skos:definition "Relates an expression to an expression of a work that has been translated freely, preserving the spirit of the original, but not its linguistic details."@en .

<http://rdaregistry.info/Elements/e/P20141>
    reg:hasSubproperty <http://rdaregistry.info/Elements/e/P20078> ;
    reg:hasUnconstrained <http://rdaregistry.info/Elements/u/P60244> ;
    reg:lexicalAlias <http://rdaregistry.info/Elements/e/translationOf.en> ;
    reg:name "translationOf"@en ;
    reg:status <http://metadataregistry.org/uri/RegStatus/1001> ;
    rdakit:toolkitDefinition "An expression of a work that has been translated, i.e., the text expressed in a language different from that of the original work."@en ;
    rdakit:toolkitLabel "translation of"@en ;
    a rdf:Property ;
    rdfs:domain <http://rdaregistry.info/Elements/c/C10006> ;
    rdfs:isDefinedBy <http://rdaregistry.info/Elements/e/> ;
    rdfs:label "is translation of"@en ;
    rdfs:range <http://rdaregistry.info/Elements/c/C10006> ;
    rdfs:subPropertyOf <http://rdaregistry.info/Elements/e/P20204> ;
    owl:inverseOf <http://rdaregistry.info/Elements/e/P20171> ;
    skos:definition "Relates an expression to an expression of a work that has been translated, i.e., the text expressed in a language different from that of the original work."@en .

<http://rdaregistry.info/Elements/e/P20142>
    reg:hasUnconstrained <http://rdaregistry.info/Elements/u/P60246> ;
    reg:lexicalAlias <http://rdaregistry.info/Elements/e/parodiedAsExpression.en> ;
    reg:name "parodiedAsExpression"@en ;
    reg:status <http://metadataregistry.org/uri/RegStatus/1001> ;
    rdakit:toolkitDefinition "An expression of a work that imitates the style or content of the source work for comic effect."@en ;
    rdakit:toolkitLabel "parodied as (expression)"@en ;
    a rdf:Property ;
    rdfs:domain <http://rdaregistry.info/Elements/c/C10006> ;
    rdfs:isDefinedBy <http://rdaregistry.info/Elements/e/> ;
    rdfs:label "is parodied as (expression)"@en ;
    rdfs:range <http://rdaregistry.info/Elements/c/C10006> ;
    rdfs:subPropertyOf <http://rdaregistry.info/Elements/e/P20114> ;
    owl:inverseOf <http://rdaregistry.info/Elements/e/P20196> ;
    skos:definition "Relates an expression to an expression of a work that imitates the style or content of the source work for comic effect."@en .

<http://rdaregistry.info/Elements/e/P20143>
    reg:hasUnconstrained <http://rdaregistry.info/Elements/u/P60247> ;
    reg:lexicalAlias <http://rdaregistry.info/Elements/e/absorbedByExpression.en> ;
    reg:name "absorbedByExpression"@en ;
    reg:status <http://metadataregistry.org/uri/RegStatus/1001> ;
    rdakit:toolkitDefinition "An expression of a work that incorporates another expression."@en ;
    rdakit:toolkitLabel "absorbed by (expression)"@en ;
    a rdf:Property ;
    rdfs:domain <http://rdaregistry.info/Elements/c/C10006> ;
    rdfs:isDefinedBy <http://rdaregistry.info/Elements/e/> ;
    rdfs:label "is absorbed by (expression)"@en ;
    rdfs:range <http://rdaregistry.info/Elements/c/C10006> ;
    rdfs:subPropertyOf <http://rdaregistry.info/Elements/e/P20169> ;
    owl:inverseOf <http://rdaregistry.info/Elements/e/P20137> ;
    skos:definition "Relates an expression to an expression of a work that incorporates another expression."@en .

<http://rdaregistry.info/Elements/e/P20144>
    reg:hasUnconstrained <http://rdaregistry.info/Elements/u/P60248> ;
    reg:lexicalAlias <http://rdaregistry.info/Elements/e/absorbedInPartByExpression.en> ;
    reg:name "absorbedInPartByExpression"@en ;
    reg:status <http://metadataregistry.org/uri/RegStatus/1001> ;
    rdakit:toolkitDefinition "An expression of a work that incorporates part of the content of another expression."@en ;
    rdakit:toolkitLabel "absorbed in part by (expression)"@en ;
    a rdf:Property ;
    rdfs:domain <http://rdaregistry.info/Elements/c/C10006> ;
    rdfs:isDefinedBy <http://rdaregistry.info/Elements/e/> ;
    rdfs:label "is absorbed in part by (expression)"@en ;
    rdfs:range <http://rdaregistry.info/Elements/c/C10006> ;
    rdfs:subPropertyOf <http://rdaregistry.info/Elements/e/P20169> ;
    owl:inverseOf <http://rdaregistry.info/Elements/e/P20138> ;
    skos:definition "Relates an expression to an expression of a work that incorporates part of the content of another expression."@en .

<http://rdaregistry.info/Elements/e/P20145>
    reg:hasUnconstrained <http://rdaregistry.info/Elements/u/P60249> ;
    reg:lexicalAlias <http://rdaregistry.info/Elements/e/containerOfExpression.en> ;
    reg:name "containerOfExpression"@en ;
    reg:status <http://metadataregistry.org/uri/RegStatus/1001> ;
    rdakit:toolkitDefinition "An expression of a work that is a discrete component of a larger expression."@en ;
    rdakit:toolkitLabel "container of (expression)"@en ;
    a rdf:Property ;
    rdfs:domain <http://rdaregistry.info/Elements/c/C10006> ;
    rdfs:isDefinedBy <http://rdaregistry.info/Elements/e/> ;
    rdfs:label "is container of (expression)"@en ;
    rdfs:range <http://rdaregistry.info/Elements/c/C10006> ;
    rdfs:subPropertyOf <http://rdaregistry.info/Elements/e/P20236> ;
    owl:inverseOf <http://rdaregistry.info/Elements/e/P20074> ;
    skos:definition "Relates an expression to an expression of a work that is a discrete component of a larger expression."@en .

<http://rdaregistry.info/Elements/e/P20146>
    reg:hasUnconstrained <http://rdaregistry.info/Elements/u/P60251> ;
    reg:lexicalAlias <http://rdaregistry.info/Elements/e/errataToExpression.en> ;
    reg:name "errataToExpression"@en ;
    reg:status <http://metadataregistry.org/uri/RegStatus/1001> ;
    rdakit:toolkitDefinition "An expression of a work that is augmented by a list of errors in the predominant work, discovered after publication, with their corrections."@en ;
    rdakit:toolkitLabel "errata to (expression)"@en ;
    a rdf:Property ;
    rdfs:domain <http://rdaregistry.info/Elements/c/C10006> ;
    rdfs:isDefinedBy <http://rdaregistry.info/Elements/e/> ;
    rdfs:label "is errata to (expression)"@en ;
    rdfs:range <http://rdaregistry.info/Elements/c/C10006> ;
    rdfs:subPropertyOf <http://rdaregistry.info/Elements/e/P20192> ;
    owl:inverseOf <http://rdaregistry.info/Elements/e/P20093> ;
    skos:definition "Relates an expression to an expression of a work that is augmented by a list of errors in the predominant work, discovered after publication, with their corrections."@en .

<http://rdaregistry.info/Elements/e/P20147>
    reg:hasUnconstrained <http://rdaregistry.info/Elements/u/P60252> ;
    reg:lexicalAlias <http://rdaregistry.info/Elements/e/guideToExpression.en> ;
    reg:name "guideToExpression"@en ;
    reg:status <http://metadataregistry.org/uri/RegStatus/1001> ;
    rdakit:toolkitDefinition "An expression of a work that is augmented by another work consisting of material to help the user of the predominant work, such as notes, learning and study aids, exercises, problems, questions and answers, instructor or student materials, etc."@en ;
    rdakit:toolkitLabel "guide to (expression)"@en ;
    a rdf:Property ;
    rdfs:domain <http://rdaregistry.info/Elements/c/C10006> ;
    rdfs:isDefinedBy <http://rdaregistry.info/Elements/e/> ;
    rdfs:label "is guide to (expression)"@en ;
    rdfs:range <http://rdaregistry.info/Elements/c/C10006> ;
    rdfs:subPropertyOf <http://rdaregistry.info/Elements/e/P20192> ;
    owl:inverseOf <http://rdaregistry.info/Elements/e/P20120> ;
    skos:definition "Relates an expression to an expression of a work that is augmented by another work consisting of material to help the user of the predominant work, such as notes, learning and study aids, exercises, problems, questions and answers, instructor or student materials, etc."@en .

<http://rdaregistry.info/Elements/e/P20148>
    reg:hasUnconstrained <http://rdaregistry.info/Elements/u/P60254> ;
    reg:lexicalAlias <http://rdaregistry.info/Elements/e/illustrationsForExpression.en> ;
    reg:name "illustrationsForExpression"@en ;
    reg:status <http://metadataregistry.org/uri/RegStatus/1001> ;
    rdakit:toolkitDefinition "An expression of a work that is augmented by pictorial content designed to explain or decorate it."@en ;
    rdakit:toolkitLabel "illustrations for (expression)"@en ;
    a rdf:Property ;
    rdfs:domain <http://rdaregistry.info/Elements/c/C10006> ;
    rdfs:isDefinedBy <http://rdaregistry.info/Elements/e/> ;
    rdfs:label "is illustrations for (expression)"@en ;
    rdfs:range <http://rdaregistry.info/Elements/c/C10006> ;
    rdfs:subPropertyOf <http://rdaregistry.info/Elements/e/P20192> ;
    owl:inverseOf <http://rdaregistry.info/Elements/e/P20094> ;
    skos:definition "Relates an expression to an expression of a work that is augmented by pictorial content designed to explain or decorate it."@en .

<http://rdaregistry.info/Elements/e/P20149>
    reg:hasUnconstrained <http://rdaregistry.info/Elements/u/P60576> ;
    reg:lexicalAlias <http://rdaregistry.info/Elements/e/continuationOfExpression.en> ;
    reg:name "continuationOfExpression"@en ;
    reg:status <http://metadataregistry.org/uri/RegStatus/1001> ;
    rdakit:toolkitDefinition "An expression of a work that is continued by the content of an expression of a later work."@en ;
    rdakit:toolkitLabel "continuation of (expression)"@en ;
    a rdf:Property ;
    rdfs:domain <http://rdaregistry.info/Elements/c/C10006> ;
    rdfs:isDefinedBy <http://rdaregistry.info/Elements/e/> ;
    rdfs:label "is continuation of (expression)"@en ;
    rdfs:range <http://rdaregistry.info/Elements/c/C10006> ;
    rdfs:subPropertyOf <http://rdaregistry.info/Elements/e/P20154> ;
    owl:inverseOf <http://rdaregistry.info/Elements/e/P20191> ;
    skos:definition "Relates an expression to an expression of a work that is continued by the content of an expression of a later work."@en .

<http://rdaregistry.info/Elements/e/P20150>
    reg:status <http://metadataregistry.org/uri/RegStatus/1008> ;
    a rdf:Property ;
    rdfs:isDefinedBy <http://rdaregistry.info/Elements/e/> .

<http://rdaregistry.info/Elements/e/P20151>
    reg:hasUnconstrained <http://rdaregistry.info/Elements/u/P60259> ;
    reg:lexicalAlias <http://rdaregistry.info/Elements/e/supplementToExpression.en> ;
    reg:name "supplementToExpression"@en ;
    reg:status <http://metadataregistry.org/uri/RegStatus/1001> ;
    rdakit:toolkitDefinition "An expression of a work that is updated or otherwise complemented by the augmenting expression."@en ;
    rdakit:toolkitLabel "supplement to (expression)"@en ;
    a rdf:Property ;
    rdfs:domain <http://rdaregistry.info/Elements/c/C10006> ;
    rdfs:isDefinedBy <http://rdaregistry.info/Elements/e/> ;
    rdfs:label "is supplement to (expression)"@en ;
    rdfs:range <http://rdaregistry.info/Elements/c/C10006> ;
    rdfs:subPropertyOf <http://rdaregistry.info/Elements/e/P20192> ;
    owl:inverseOf <http://rdaregistry.info/Elements/e/P20172> ;
    skos:definition "Relates an expression to an expression of a work that is updated or otherwise complemented by the augmenting expression."@en .

<http://rdaregistry.info/Elements/e/P20152>
    reg:hasSubproperty <http://rdaregistry.info/Elements/e/P20123>, <http://rdaregistry.info/Elements/e/P20124>, <http://rdaregistry.info/Elements/e/P20125>, <http://rdaregistry.info/Elements/e/P20126>, <http://rdaregistry.info/Elements/e/P20127>, <http://rdaregistry.info/Elements/e/P20128>, <http://rdaregistry.info/Elements/e/P20129>, <http://rdaregistry.info/Elements/e/P20133>, <http://rdaregistry.info/Elements/e/P20134>, <http://rdaregistry.info/Elements/e/P20256>, <http://rdaregistry.info/Elements/e/P20281> ;
    reg:hasUnconstrained <http://rdaregistry.info/Elements/u/P60241> ;
    reg:lexicalAlias <http://rdaregistry.info/Elements/e/adaptationOfExpression.en> ;
    reg:name "adaptationOfExpression"@en ;
    reg:status <http://metadataregistry.org/uri/RegStatus/1001> ;
    rdakit:toolkitDefinition "An expression of a work that has been modified for a purpose, use, or medium other than that for which it was originally intended."@en ;
    rdakit:toolkitLabel "adaptation of (expression)"@en ;
    a rdf:Property ;
    rdfs:domain <http://rdaregistry.info/Elements/c/C10006> ;
    rdfs:isDefinedBy <http://rdaregistry.info/Elements/e/> ;
    rdfs:label "is adaptation of (expression)"@en ;
    rdfs:range <http://rdaregistry.info/Elements/c/C10006> ;
    rdfs:subPropertyOf <http://rdaregistry.info/Elements/e/P20204> ;
    owl:inverseOf <http://rdaregistry.info/Elements/e/P20153> ;
    skos:definition "Relates an expression to an expression of a work that has been modified for a purpose, use, or medium other than that for which it was originally intended."@en .

<http://rdaregistry.info/Elements/e/P20153>
    reg:hasSubproperty <http://rdaregistry.info/Elements/e/P20009>, <http://rdaregistry.info/Elements/e/P20060>, <http://rdaregistry.info/Elements/e/P20066>, <http://rdaregistry.info/Elements/e/P20067>, <http://rdaregistry.info/Elements/e/P20073>, <http://rdaregistry.info/Elements/e/P20077>, <http://rdaregistry.info/Elements/e/P20088>, <http://rdaregistry.info/Elements/e/P20096>, <http://rdaregistry.info/Elements/e/P20099>, <http://rdaregistry.info/Elements/e/P20255>, <http://rdaregistry.info/Elements/e/P20282> ;
    reg:hasUnconstrained <http://rdaregistry.info/Elements/u/P60260> ;
    reg:lexicalAlias <http://rdaregistry.info/Elements/e/adaptedAsExpression.en> ;
    reg:name "adaptedAsExpression"@en ;
    reg:status <http://metadataregistry.org/uri/RegStatus/1001> ;
    rdakit:toolkitDefinition "An expression of a work that modifies the source expression for a purpose, use, or medium other than that for which it was originally intended."@en ;
    rdakit:toolkitLabel "adapted as (expression)"@en ;
    a rdf:Property ;
    rdfs:domain <http://rdaregistry.info/Elements/c/C10006> ;
    rdfs:isDefinedBy <http://rdaregistry.info/Elements/e/> ;
    rdfs:label "is adapted as (expression)"@en ;
    rdfs:range <http://rdaregistry.info/Elements/c/C10006> ;
    rdfs:subPropertyOf <http://rdaregistry.info/Elements/e/P20203> ;
    owl:inverseOf <http://rdaregistry.info/Elements/e/P20152> ;
    skos:definition "Relates an expression to an expression of a work based on the source expression."@en .

<http://rdaregistry.info/Elements/e/P20154>
    reg:hasSubproperty <http://rdaregistry.info/Elements/e/P20137>, <http://rdaregistry.info/Elements/e/P20138>, <http://rdaregistry.info/Elements/e/P20149>, <http://rdaregistry.info/Elements/e/P20167>, <http://rdaregistry.info/Elements/e/P20168>, <http://rdaregistry.info/Elements/e/P20198>, <http://rdaregistry.info/Elements/e/P20199>, <http://rdaregistry.info/Elements/e/P20201> ;
    reg:hasUnconstrained <http://rdaregistry.info/Elements/u/P60261> ;
    reg:lexicalAlias <http://rdaregistry.info/Elements/e/precededByExpression.en> ;
    reg:name "precededByExpression"@en ;
    reg:status <http://metadataregistry.org/uri/RegStatus/1001> ;
    rdakit:toolkitDefinition "An expression of a work that precedes (e.g., is earlier in time or before in narrative) the succeeding expression."@en ;
    rdakit:toolkitLabel "preceded by (expression)"@en ;
    a rdf:Property ;
    rdfs:domain <http://rdaregistry.info/Elements/c/C10006> ;
    rdfs:isDefinedBy <http://rdaregistry.info/Elements/e/> ;
    rdfs:label "is preceded by (expression)"@en ;
    rdfs:range <http://rdaregistry.info/Elements/c/C10006> ;
    rdfs:subPropertyOf <http://rdaregistry.info/Elements/e/P20235> ;
    owl:inverseOf <http://rdaregistry.info/Elements/e/P20169> ;
    skos:definition "Relates an expression to an expression of a work that precedes (e.g., is earlier in time or before in narrative) the succeeding expression."@en .

<http://rdaregistry.info/Elements/e/P20155>
    reg:hasUnconstrained <http://rdaregistry.info/Elements/u/P60262> ;
    reg:lexicalAlias <http://rdaregistry.info/Elements/e/findingAidExpression.en> ;
    reg:name "findingAidExpression"@en ;
    reg:status <http://metadataregistry.org/uri/RegStatus/1001> ;
    rdakit:toolkitDefinition "An expression of a work that provides a guide to the organization, arrangement, and contents of an archival collection."@en ;
    rdakit:toolkitLabel "finding aid (expression)"@en ;
    a rdf:Property ;
    rdfs:domain <http://rdaregistry.info/Elements/c/C10006> ;
    rdfs:isDefinedBy <http://rdaregistry.info/Elements/e/> ;
    rdfs:label "is finding aid (expression)"@en ;
    rdfs:range <http://rdaregistry.info/Elements/c/C10006> ;
    rdfs:subPropertyOf <http://rdaregistry.info/Elements/e/P20105> ;
    owl:inverseOf <http://rdaregistry.info/Elements/e/P20197> ;
    skos:definition "Relates an expression to an expression of a work that provides a guide to the organization, arrangement, and contents of an archival collection."@en .

<http://rdaregistry.info/Elements/e/P20156>
    reg:hasUnconstrained <http://rdaregistry.info/Elements/u/P60263> ;
    reg:lexicalAlias <http://rdaregistry.info/Elements/e/indexExpression.en> ;
    reg:name "indexExpression"@en ;
    reg:status <http://metadataregistry.org/uri/RegStatus/1001> ;
    rdakit:toolkitDefinition "An expression of a work that provides a systematic, alphabetical guide to the contents of the predominant expression, usually keyed to page numbers or other reference codes."@en ;
    rdakit:toolkitLabel "index (expression)"@en ;
    a rdf:Property ;
    rdfs:domain <http://rdaregistry.info/Elements/c/C10006> ;
    rdfs:isDefinedBy <http://rdaregistry.info/Elements/e/> ;
    rdfs:label "is index (expression)"@en ;
    rdfs:range <http://rdaregistry.info/Elements/c/C10006> ;
    rdfs:subPropertyOf <http://rdaregistry.info/Elements/e/P20105> ;
    owl:inverseOf <http://rdaregistry.info/Elements/e/P20188> ;
    skos:definition "Relates an expression to an expression of a work that provides a systematic, alphabetical guide to the contents of the predominant expression, usually keyed to page numbers or other reference codes."@en .

<http://rdaregistry.info/Elements/e/P20157>
    reg:hasSubproperty <http://rdaregistry.info/Elements/e/P20158>, <http://rdaregistry.info/Elements/e/P20161>, <http://rdaregistry.info/Elements/e/P20162> ;
    reg:hasUnconstrained <http://rdaregistry.info/Elements/u/P60264> ;
    reg:lexicalAlias <http://rdaregistry.info/Elements/e/screenplayExpression.en> ;
    reg:name "screenplayExpression"@en ;
    reg:status <http://metadataregistry.org/uri/RegStatus/1001> ;
    rdakit:toolkitDefinition "An expression of a work that provides the text for a motion picture, television program or video."@en ;
    rdakit:toolkitLabel "screenplay (expression)"@en ;
    a rdf:Property ;
    rdfs:domain <http://rdaregistry.info/Elements/c/C10006> ;
    rdfs:isDefinedBy <http://rdaregistry.info/Elements/e/> ;
    rdfs:label "is screenplay (expression)"@en ;
    rdfs:range <http://rdaregistry.info/Elements/c/C10006> ;
    rdfs:subPropertyOf <http://rdaregistry.info/Elements/e/P20100> ;
    owl:inverseOf <http://rdaregistry.info/Elements/e/P20102> ;
    skos:definition "Relates an expression to an expression of a work that provides the text for a motion picture, television program or video."@en .

<http://rdaregistry.info/Elements/e/P20158>
    reg:hasUnconstrained <http://rdaregistry.info/Elements/u/P60265> ;
    reg:lexicalAlias <http://rdaregistry.info/Elements/e/motionPictureScreenplayExpression.en> ;
    reg:name "motionPictureScreenplayExpression"@en ;
    reg:status <http://metadataregistry.org/uri/RegStatus/1001> ;
    rdakit:toolkitDefinition "An expression of a work that provides the text for a motion picture."@en ;
    rdakit:toolkitLabel "motion picture screenplay (expression)"@en ;
    a rdf:Property ;
    rdfs:domain <http://rdaregistry.info/Elements/c/C10006> ;
    rdfs:isDefinedBy <http://rdaregistry.info/Elements/e/> ;
    rdfs:label "is motion picture screenplay (expression)"@en ;
    rdfs:range <http://rdaregistry.info/Elements/c/C10006> ;
    rdfs:subPropertyOf <http://rdaregistry.info/Elements/e/P20157> ;
    owl:inverseOf <http://rdaregistry.info/Elements/e/P20173> ;
    skos:definition "Relates an expression to an expression of a work that provides the text for a motion picture."@en .

<http://rdaregistry.info/Elements/e/P20159>
    reg:hasUnconstrained <http://rdaregistry.info/Elements/u/P60266> ;
    reg:lexicalAlias <http://rdaregistry.info/Elements/e/musicalSettingOfExpression.en> ;
    reg:name "musicalSettingOfExpression"@en ;
    reg:status <http://metadataregistry.org/uri/RegStatus/1001> ;
    rdakit:toolkitDefinition "An expression of a work that provides the text for a non-dramatic musical work, other than an oratorio."@en ;
    rdakit:toolkitLabel "musical setting of (expression)"@en ;
    a rdf:Property ;
    rdfs:domain <http://rdaregistry.info/Elements/c/C10006> ;
    rdfs:isDefinedBy <http://rdaregistry.info/Elements/e/> ;
    rdfs:label "is musical setting of (expression)"@en ;
    rdfs:range <http://rdaregistry.info/Elements/c/C10006> ;
    rdfs:subPropertyOf <http://rdaregistry.info/Elements/e/P20204> ;
    owl:inverseOf <http://rdaregistry.info/Elements/e/P20087> ;
    skos:definition "Relates an expression to an expression of a work that provides the text for a non-dramatic musical work, other than an oratorio."@en .

<http://rdaregistry.info/Elements/e/P20160>
    reg:hasUnconstrained <http://rdaregistry.info/Elements/u/P60267> ;
    reg:lexicalAlias <http://rdaregistry.info/Elements/e/radioScriptExpression.en> ;
    reg:name "radioScriptExpression"@en ;
    reg:status <http://metadataregistry.org/uri/RegStatus/1001> ;
    rdakit:toolkitDefinition "An expression of a work that provides the text for a radio program."@en ;
    rdakit:toolkitLabel "radio script (expression)"@en ;
    a rdf:Property ;
    rdfs:domain <http://rdaregistry.info/Elements/c/C10006> ;
    rdfs:isDefinedBy <http://rdaregistry.info/Elements/e/> ;
    rdfs:label "is radio script (expression)"@en ;
    rdfs:range <http://rdaregistry.info/Elements/c/C10006> ;
    rdfs:subPropertyOf <http://rdaregistry.info/Elements/e/P20100> ;
    owl:inverseOf <http://rdaregistry.info/Elements/e/P20176> ;
    skos:definition "Relates an expression to an expression of a work that provides the text for a radio program."@en .

<http://rdaregistry.info/Elements/e/P20161>
    reg:hasUnconstrained <http://rdaregistry.info/Elements/u/P60268> ;
    reg:lexicalAlias <http://rdaregistry.info/Elements/e/televisionScreenplayExpression.en> ;
    reg:name "televisionScreenplayExpression"@en ;
    reg:status <http://metadataregistry.org/uri/RegStatus/1001> ;
    rdakit:toolkitDefinition "An expression of a work that provides the text for a television program."@en ;
    rdakit:toolkitLabel "television screenplay (expression)"@en ;
    a rdf:Property ;
    rdfs:domain <http://rdaregistry.info/Elements/c/C10006> ;
    rdfs:isDefinedBy <http://rdaregistry.info/Elements/e/> ;
    rdfs:label "is television screenplay (expression)"@en ;
    rdfs:range <http://rdaregistry.info/Elements/c/C10006> ;
    rdfs:subPropertyOf <http://rdaregistry.info/Elements/e/P20157> ;
    owl:inverseOf <http://rdaregistry.info/Elements/e/P20174> ;
    skos:definition "Relates an expression to an expression of a work that provides the text for a television program."@en .

<http://rdaregistry.info/Elements/e/P20162>
    reg:hasUnconstrained <http://rdaregistry.info/Elements/u/P60269> ;
    reg:lexicalAlias <http://rdaregistry.info/Elements/e/videoScreenplayExpression.en> ;
    reg:name "videoScreenplayExpression"@en ;
    reg:status <http://metadataregistry.org/uri/RegStatus/1001> ;
    rdakit:toolkitDefinition "An expression of a work that provides the text for a video."@en ;
    rdakit:toolkitLabel "video screenplay (expression)"@en ;
    a rdf:Property ;
    rdfs:domain <http://rdaregistry.info/Elements/c/C10006> ;
    rdfs:isDefinedBy <http://rdaregistry.info/Elements/e/> ;
    rdfs:label "is video screenplay (expression)"@en ;
    rdfs:range <http://rdaregistry.info/Elements/c/C10006> ;
    rdfs:subPropertyOf <http://rdaregistry.info/Elements/e/P20157> ;
    owl:inverseOf <http://rdaregistry.info/Elements/e/P20175> ;
    skos:definition "Relates an expression to an expression of a work that provides the text for a video."@en .

<http://rdaregistry.info/Elements/e/P20163>
    reg:hasUnconstrained <http://rdaregistry.info/Elements/u/P60270> ;
    reg:lexicalAlias <http://rdaregistry.info/Elements/e/librettoExpression.en> ;
    reg:name "librettoExpression"@en ;
    reg:status <http://metadataregistry.org/uri/RegStatus/1001> ;
    rdakit:toolkitDefinition "An expression of a work that provides the text of an opera or other work for the musical stage, or an oratorio."@en ;
    rdakit:toolkitLabel "libretto (expression)"@en ;
    a rdf:Property ;
    rdfs:domain <http://rdaregistry.info/Elements/c/C10006> ;
    rdfs:isDefinedBy <http://rdaregistry.info/Elements/e/> ;
    rdfs:label "is libretto (expression)"@en ;
    rdfs:range <http://rdaregistry.info/Elements/c/C10006> ;
    rdfs:subPropertyOf <http://rdaregistry.info/Elements/e/P20100> ;
    owl:inverseOf <http://rdaregistry.info/Elements/e/P20084> ;
    skos:definition "Relates an expression to an expression of a work that provides the text of an opera or other work for the musical stage, or an oratorio."@en .

<http://rdaregistry.info/Elements/e/P20164>
    reg:hasUnconstrained <http://rdaregistry.info/Elements/u/P60273> ;
    reg:lexicalAlias <http://rdaregistry.info/Elements/e/paraphrasedAsExpression.en> ;
    reg:name "paraphrasedAsExpression"@en ;
    reg:status <http://metadataregistry.org/uri/RegStatus/1001> ;
    rdakit:toolkitDefinition "An expression of a work that restates the content of the source work in a different form."@en ;
    rdakit:toolkitLabel "paraphrased as (expression)"@en ;
    a rdf:Property ;
    rdfs:domain <http://rdaregistry.info/Elements/c/C10006> ;
    rdfs:isDefinedBy <http://rdaregistry.info/Elements/e/> ;
    rdfs:label "is paraphrased as (expression)"@en ;
    rdfs:range <http://rdaregistry.info/Elements/c/C10006> ;
    rdfs:subPropertyOf <http://rdaregistry.info/Elements/e/P20203> ;
    owl:inverseOf <http://rdaregistry.info/Elements/e/P20186> ;
    skos:definition "Relates an expression to an expression of a work that restates the content of the source work in a different form."@en .

<http://rdaregistry.info/Elements/e/P20165>
    reg:hasUnconstrained <http://rdaregistry.info/Elements/u/P60274> ;
    reg:lexicalAlias <http://rdaregistry.info/Elements/e/arrangedAs.en> ;
    reg:name "arrangedAs"@en ;
    reg:status <http://metadataregistry.org/uri/RegStatus/1001> ;
    rdakit:toolkitDefinition "An expression of a musical work that rewrites the source expression for a medium of performance different from that for which the work was originally intended."@en ;
    rdakit:toolkitLabel "arranged as"@en ;
    a rdf:Property ;
    rdfs:domain <http://rdaregistry.info/Elements/c/C10006> ;
    rdfs:isDefinedBy <http://rdaregistry.info/Elements/e/> ;
    rdfs:label "is arranged as"@en ;
    rdfs:range <http://rdaregistry.info/Elements/c/C10006> ;
    rdfs:subPropertyOf <http://rdaregistry.info/Elements/e/P20203> ;
    owl:inverseOf <http://rdaregistry.info/Elements/e/P20139> ;
    skos:definition "Relates an expression to an expression of a musical work that rewrites the source expression for a medium of performance different from that for which the work was originally intended."@en .

<http://rdaregistry.info/Elements/e/P20166>
    reg:hasUnconstrained <http://rdaregistry.info/Elements/u/P60275> ;
    reg:lexicalAlias <http://rdaregistry.info/Elements/e/abridgedAsExpression.en> ;
    reg:name "abridgedAsExpression"@en ;
    reg:status <http://metadataregistry.org/uri/RegStatus/1001> ;
    rdakit:toolkitDefinition "An expression of a work that shortens the source expression without changing the general meaning or manner of presentation."@en ;
    rdakit:toolkitLabel "abridged as (expression)"@en ;
    a rdf:Property ;
    rdfs:domain <http://rdaregistry.info/Elements/c/C10006> ;
    rdfs:isDefinedBy <http://rdaregistry.info/Elements/e/> ;
    rdfs:label "is abridged as (expression)"@en ;
    rdfs:range <http://rdaregistry.info/Elements/c/C10006> ;
    rdfs:subPropertyOf <http://rdaregistry.info/Elements/e/P20203> ;
    owl:inverseOf <http://rdaregistry.info/Elements/e/P20121> ;
    skos:definition "Relates an expression to an expression of a work that shortens the source expression without changing the general meaning or manner of presentation."@en .

<http://rdaregistry.info/Elements/e/P20167>
    reg:hasUnconstrained <http://rdaregistry.info/Elements/u/P60276> ;
    reg:lexicalAlias <http://rdaregistry.info/Elements/e/continuationInPartOfExpression.en> ;
    reg:name "continuationInPartOfExpression"@en ;
    reg:status <http://metadataregistry.org/uri/RegStatus/1001> ;
    rdakit:toolkitDefinition "An expression of a work that split into two or more separate expressions with new titles."@en ;
    rdakit:toolkitLabel "continuation in part of (expression)"@en ;
    a rdf:Property ;
    rdfs:domain <http://rdaregistry.info/Elements/c/C10006> ;
    rdfs:isDefinedBy <http://rdaregistry.info/Elements/e/> ;
    rdfs:label "is continuation in part of (expression)"@en ;
    rdfs:range <http://rdaregistry.info/Elements/c/C10006> ;
    rdfs:subPropertyOf <http://rdaregistry.info/Elements/e/P20154> ;
    owl:inverseOf <http://rdaregistry.info/Elements/e/P20200> ;
    skos:definition "Relates an expression to an expression of a work that split into two or more separate expressions with new titles."@en .

<http://rdaregistry.info/Elements/e/P20168>
    reg:hasUnconstrained <http://rdaregistry.info/Elements/u/P60277> ;
    reg:lexicalAlias <http://rdaregistry.info/Elements/e/separatedFromExpression.en> ;
    reg:name "separatedFromExpression"@en ;
    reg:status <http://metadataregistry.org/uri/RegStatus/1001> ;
    rdakit:toolkitDefinition "An expression of a work that spun off a part of its content to form a new expression."@en ;
    rdakit:toolkitLabel "separated from (expression)"@en ;
    a rdf:Property ;
    rdfs:domain <http://rdaregistry.info/Elements/c/C10006> ;
    rdfs:isDefinedBy <http://rdaregistry.info/Elements/e/> ;
    rdfs:label "is separated from (expression)"@en ;
    rdfs:range <http://rdaregistry.info/Elements/c/C10006> ;
    rdfs:subPropertyOf <http://rdaregistry.info/Elements/e/P20154> ;
    owl:inverseOf <http://rdaregistry.info/Elements/e/P20101> ;
    skos:definition "Relates an expression to an expression of a work that spun off a part of its content to form a new expression."@en .

<http://rdaregistry.info/Elements/e/P20169>
    reg:hasSubproperty <http://rdaregistry.info/Elements/e/P20075>, <http://rdaregistry.info/Elements/e/P20076>, <http://rdaregistry.info/Elements/e/P20101>, <http://rdaregistry.info/Elements/e/P20143>, <http://rdaregistry.info/Elements/e/P20144>, <http://rdaregistry.info/Elements/e/P20191>, <http://rdaregistry.info/Elements/e/P20200>, <http://rdaregistry.info/Elements/e/P20212> ;
    reg:hasUnconstrained <http://rdaregistry.info/Elements/u/P60278> ;
    reg:lexicalAlias <http://rdaregistry.info/Elements/e/succeededByExpression.en> ;
    reg:name "succeededByExpression"@en ;
    reg:status <http://metadataregistry.org/uri/RegStatus/1001> ;
    rdakit:toolkitDefinition "An expression of a work that succeeds (e.g., later in time or after in a narrative) the preceding expression."@en ;
    rdakit:toolkitLabel "succeeded by (expression)"@en ;
    a rdf:Property ;
    rdfs:domain <http://rdaregistry.info/Elements/c/C10006> ;
    rdfs:isDefinedBy <http://rdaregistry.info/Elements/e/> ;
    rdfs:label "is succeeded by (expression)"@en ;
    rdfs:range <http://rdaregistry.info/Elements/c/C10006> ;
    rdfs:subPropertyOf <http://rdaregistry.info/Elements/e/P20235> ;
    owl:inverseOf <http://rdaregistry.info/Elements/e/P20154> ;
    skos:definition "Relates an expression to an expression of a work that succeeds (e.g., later in time or after in a narrative) the preceding expression."@en .

<http://rdaregistry.info/Elements/e/P20170>
    reg:hasUnconstrained <http://rdaregistry.info/Elements/u/P60279> ;
    reg:lexicalAlias <http://rdaregistry.info/Elements/e/digestedAsExpression.en> ;
    reg:name "digestedAsExpression"@en ;
    reg:status <http://metadataregistry.org/uri/RegStatus/1001> ;
    rdakit:toolkitDefinition "An expression of a work that systematically and comprehensively condenses the source expression."@en ;
    rdakit:toolkitLabel "digested as (expression)"@en ;
    a rdf:Property ;
    rdfs:domain <http://rdaregistry.info/Elements/c/C10006> ;
    rdfs:isDefinedBy <http://rdaregistry.info/Elements/e/> ;
    rdfs:label "is digested as (expression)"@en ;
    rdfs:range <http://rdaregistry.info/Elements/c/C10006> ;
    rdfs:subPropertyOf <http://rdaregistry.info/Elements/e/P20203> ;
    owl:inverseOf <http://rdaregistry.info/Elements/e/P20135> ;
    skos:definition "Relates an expression to an expression of a work that systematically and comprehensively condenses the source expression."@en .

<http://rdaregistry.info/Elements/e/P20171>
    reg:hasSubproperty <http://rdaregistry.info/Elements/e/P20079> ;
    reg:hasUnconstrained <http://rdaregistry.info/Elements/u/P60280> ;
    reg:lexicalAlias <http://rdaregistry.info/Elements/e/translatedAs.en> ;
    reg:name "translatedAs"@en ;
    reg:status <http://metadataregistry.org/uri/RegStatus/1001> ;
    rdakit:toolkitDefinition "An expression of a work that translates the text of the source expression into a language different from that of the original work."@en ;
    rdakit:toolkitLabel "translated as"@en ;
    a rdf:Property ;
    rdfs:domain <http://rdaregistry.info/Elements/c/C10006> ;
    rdfs:isDefinedBy <http://rdaregistry.info/Elements/e/> ;
    rdfs:label "is translated as"@en ;
    rdfs:range <http://rdaregistry.info/Elements/c/C10006> ;
    rdfs:subPropertyOf <http://rdaregistry.info/Elements/e/P20203> ;
    owl:inverseOf <http://rdaregistry.info/Elements/e/P20141> ;
    skos:definition "Relates an expression to an expression of a work that translates the text of the source expression into a language different from that of the original work."@en .

<http://rdaregistry.info/Elements/e/P20172>
    reg:hasUnconstrained <http://rdaregistry.info/Elements/u/P60281> ;
    reg:lexicalAlias <http://rdaregistry.info/Elements/e/supplementExpression.en> ;
    reg:name "supplementExpression"@en ;
    reg:status <http://metadataregistry.org/uri/RegStatus/1001> ;
    rdakit:toolkitDefinition "An expression of a work that updates or otherwise complements the predominant expression."@en ;
    rdakit:toolkitLabel "supplement (expression)"@en ;
    a rdf:Property ;
    rdfs:domain <http://rdaregistry.info/Elements/c/C10006> ;
    rdfs:isDefinedBy <http://rdaregistry.info/Elements/e/> ;
    rdfs:label "is supplement (expression)"@en ;
    rdfs:range <http://rdaregistry.info/Elements/c/C10006> ;
    rdfs:subPropertyOf <http://rdaregistry.info/Elements/e/P20105> ;
    owl:inverseOf <http://rdaregistry.info/Elements/e/P20151> ;
    skos:definition "Relates an expression to an expression of a work that updates or otherwise complements the predominant expression."@en .

<http://rdaregistry.info/Elements/e/P20173>
    reg:hasUnconstrained <http://rdaregistry.info/Elements/u/P60282> ;
    reg:lexicalAlias <http://rdaregistry.info/Elements/e/screenplayForMotionPictureExpression.en> ;
    reg:name "screenplayForMotionPictureExpression"@en ;
    reg:status <http://metadataregistry.org/uri/RegStatus/1001> ;
    rdakit:toolkitDefinition "An expression of a work that uses the text as a screenplay for a motion picture."@en ;
    rdakit:toolkitLabel "screenplay for motion picture (expression)"@en ;
    a rdf:Property ;
    rdfs:domain <http://rdaregistry.info/Elements/c/C10006> ;
    rdfs:isDefinedBy <http://rdaregistry.info/Elements/e/> ;
    rdfs:label "is screenplay for motion picture (expression)"@en ;
    rdfs:range <http://rdaregistry.info/Elements/c/C10006> ;
    rdfs:subPropertyOf <http://rdaregistry.info/Elements/e/P20102> ;
    owl:inverseOf <http://rdaregistry.info/Elements/e/P20158> ;
    skos:definition "Relates an expression to an expression of a work that uses the text as a screenplay for a motion picture."@en .

<http://rdaregistry.info/Elements/e/P20174>
    reg:hasUnconstrained <http://rdaregistry.info/Elements/u/P60283> ;
    reg:lexicalAlias <http://rdaregistry.info/Elements/e/screenplayForTelevisionProgramExpression.en> ;
    reg:name "screenplayForTelevisionProgramExpression"@en ;
    reg:status <http://metadataregistry.org/uri/RegStatus/1001> ;
    rdakit:toolkitDefinition "An expression of a work that uses the text as a screenplay for a television program."@en ;
    rdakit:toolkitLabel "screenplay for television program (expression)"@en ;
    a rdf:Property ;
    rdfs:domain <http://rdaregistry.info/Elements/c/C10006> ;
    rdfs:isDefinedBy <http://rdaregistry.info/Elements/e/> ;
    rdfs:label "is screenplay for television program (expression)"@en ;
    rdfs:range <http://rdaregistry.info/Elements/c/C10006> ;
    rdfs:subPropertyOf <http://rdaregistry.info/Elements/e/P20102> ;
    owl:inverseOf <http://rdaregistry.info/Elements/e/P20161> ;
    skos:definition "Relates an expression to an expression of a work that uses the text as a screenplay for a television program."@en .

<http://rdaregistry.info/Elements/e/P20175>
    reg:hasUnconstrained <http://rdaregistry.info/Elements/u/P60284> ;
    reg:lexicalAlias <http://rdaregistry.info/Elements/e/screenplayForVideoExpression.en> ;
    reg:name "screenplayForVideoExpression"@en ;
    reg:status <http://metadataregistry.org/uri/RegStatus/1001> ;
    rdakit:toolkitDefinition "An expression of a work that uses the text as a screenplay for a video."@en ;
    rdakit:toolkitLabel "screenplay for video (expression)"@en ;
    a rdf:Property ;
    rdfs:domain <http://rdaregistry.info/Elements/c/C10006> ;
    rdfs:isDefinedBy <http://rdaregistry.info/Elements/e/> ;
    rdfs:label "is screenplay for video (expression)"@en ;
    rdfs:range <http://rdaregistry.info/Elements/c/C10006> ;
    rdfs:subPropertyOf <http://rdaregistry.info/Elements/e/P20102> ;
    owl:inverseOf <http://rdaregistry.info/Elements/e/P20162> ;
    skos:definition "Relates an expression to an expression of a work that uses the text as a screenplay for a video."@en .

<http://rdaregistry.info/Elements/e/P20176>
    reg:hasUnconstrained <http://rdaregistry.info/Elements/u/P60285> ;
    reg:lexicalAlias <http://rdaregistry.info/Elements/e/scriptForRadioProgramExpression.en> ;
    reg:name "scriptForRadioProgramExpression"@en ;
    reg:status <http://metadataregistry.org/uri/RegStatus/1001> ;
    rdakit:toolkitDefinition "An expression of a work that uses the text of the source work as the script for a radio program."@en ;
    rdakit:toolkitLabel "script for radio program (expression)"@en ;
    a rdf:Property ;
    rdfs:domain <http://rdaregistry.info/Elements/c/C10006> ;
    rdfs:isDefinedBy <http://rdaregistry.info/Elements/e/> ;
    rdfs:label "is script for radio program (expression)"@en ;
    rdfs:range <http://rdaregistry.info/Elements/c/C10006> ;
    rdfs:subPropertyOf <http://rdaregistry.info/Elements/e/P20100> ;
    owl:inverseOf <http://rdaregistry.info/Elements/e/P20160> ;
    skos:definition "Relates an expression to an expression of a work that uses the text of the source work as the script for a radio program."@en .

<http://rdaregistry.info/Elements/e/P20177>
    reg:hasUnconstrained <http://rdaregistry.info/Elements/u/P60286> ;
    reg:lexicalAlias <http://rdaregistry.info/Elements/e/addendaToExpression.en> ;
    reg:name "addendaToExpression"@en ;
    reg:status <http://metadataregistry.org/uri/RegStatus/1001> ;
    rdakit:toolkitDefinition "An expression of a work to which is added brief additional material, less extensive than a supplement, but essential to the completeness of the content of the work; it is usually added at the end of the content but is sometimes issued separately from it."@en ;
    rdakit:toolkitLabel "addenda to (expression)"@en ;
    a rdf:Property ;
    rdfs:domain <http://rdaregistry.info/Elements/c/C10006> ;
    rdfs:isDefinedBy <http://rdaregistry.info/Elements/e/> ;
    rdfs:label "is addenda to (expression)"@en ;
    rdfs:range <http://rdaregistry.info/Elements/c/C10006> ;
    rdfs:subPropertyOf <http://rdaregistry.info/Elements/e/P20192> ;
    owl:inverseOf <http://rdaregistry.info/Elements/e/P20109> ;
    skos:definition "Relates an expression to an expression of a work to which is added brief additional material, less extensive than a supplement, but essential to the completeness of the content of the work; it is usually added at the end of the content but is sometimes issued separately from it."@en .

<http://rdaregistry.info/Elements/e/P20178>
    reg:status <http://metadataregistry.org/uri/RegStatus/1008> ;
    a rdf:Property ;
    rdfs:isDefinedBy <http://rdaregistry.info/Elements/e/> .

<http://rdaregistry.info/Elements/e/P20179>
    reg:hasUnconstrained <http://rdaregistry.info/Elements/u/P60289> ;
    reg:lexicalAlias <http://rdaregistry.info/Elements/e/summaryOfExpression.en> ;
    reg:name "summaryOfExpression"@en ;
    reg:status <http://metadataregistry.org/uri/RegStatus/1001> ;
    rdakit:toolkitDefinition "An expression of a work used as the basis for a brief recapitulation of its content."@en ;
    rdakit:toolkitLabel "summary of (expression)"@en ;
    a rdf:Property ;
    rdfs:domain <http://rdaregistry.info/Elements/c/C10006> ;
    rdfs:isDefinedBy <http://rdaregistry.info/Elements/e/> ;
    rdfs:label "is summary of (expression)"@en ;
    rdfs:range <http://rdaregistry.info/Elements/c/C10006> ;
    rdfs:subPropertyOf <http://rdaregistry.info/Elements/e/P20204> ;
    owl:inverseOf <http://rdaregistry.info/Elements/e/P20106> ;
    skos:definition "Relates an expression to an expression of a work used as the basis for a brief recapitulation of its content."@en .

<http://rdaregistry.info/Elements/e/P20180>
    reg:hasUnconstrained <http://rdaregistry.info/Elements/u/P60290> ;
    reg:lexicalAlias <http://rdaregistry.info/Elements/e/catalogueOfExpression.en> ;
    reg:name "catalogueOfExpression"@en ;
    reg:status <http://metadataregistry.org/uri/RegStatus/1001> ;
    rdakit:toolkitDefinition "An expression of a work used as the basis for a catalogue, i.e., a complete enumeration of items arranged systematically."@en ;
    rdakit:toolkitLabel "catalogue of (expression)"@en ;
    a rdf:Property ;
    rdfs:domain <http://rdaregistry.info/Elements/c/C10006> ;
    rdfs:isDefinedBy <http://rdaregistry.info/Elements/e/> ;
    rdfs:label "is catalogue of (expression)"@en ;
    rdfs:range <http://rdaregistry.info/Elements/c/C10006> ;
    rdfs:subPropertyOf <http://rdaregistry.info/Elements/e/P20192> ;
    owl:inverseOf <http://rdaregistry.info/Elements/e/P20107> ;
    skos:definition "Relates an expression to an expression of a work used as the basis for a catalogue, i.e., a complete enumeration of items arranged systematically."@en .

<http://rdaregistry.info/Elements/e/P20181>
    reg:hasUnconstrained <http://rdaregistry.info/Elements/u/P60291> ;
    reg:lexicalAlias <http://rdaregistry.info/Elements/e/concordanceToExpression.en> ;
    reg:name "concordanceToExpression"@en ;
    reg:status <http://metadataregistry.org/uri/RegStatus/1001> ;
    rdakit:toolkitDefinition "An expression of a work used as the basis for a concordance, i.e., an index of all the words in the predominant expression."@en ;
    rdakit:toolkitLabel "concordance to (expression)"@en ;
    a rdf:Property ;
    rdfs:domain <http://rdaregistry.info/Elements/c/C10006> ;
    rdfs:isDefinedBy <http://rdaregistry.info/Elements/e/> ;
    rdfs:label "is concordance to (expression)"@en ;
    rdfs:range <http://rdaregistry.info/Elements/c/C10006> ;
    rdfs:subPropertyOf <http://rdaregistry.info/Elements/e/P20192> ;
    owl:inverseOf <http://rdaregistry.info/Elements/e/P20108> ;
    skos:definition "Relates an expression to an expression of a work used as the basis for a concordance, i.e., an index of all the words in the predominant expression."@en .

<http://rdaregistry.info/Elements/e/P20182>
    reg:status <http://metadataregistry.org/uri/RegStatus/1008> ;
    a rdf:Property ;
    rdfs:isDefinedBy <http://rdaregistry.info/Elements/e/> .

<http://rdaregistry.info/Elements/e/P20183>
    reg:hasUnconstrained <http://rdaregistry.info/Elements/u/P60293> ;
    reg:lexicalAlias <http://rdaregistry.info/Elements/e/choreographicAdaptationOfExpression.en> ;
    reg:name "choreographicAdaptationOfExpression"@en ;
    reg:status <http://metadataregistry.org/uri/RegStatus/1001> ;
    rdakit:toolkitDefinition "An expression of a work that has been adapted as a work consisting of movement (e.g., dance)."@en ;
    rdakit:toolkitLabel "choreographic adaptation of (expression)"@en ;
    a rdf:Property ;
    rdfs:domain <http://rdaregistry.info/Elements/c/C10006> ;
    rdfs:isDefinedBy <http://rdaregistry.info/Elements/e/> ;
    rdfs:label "is choreographic adaptation of (expression)"@en ;
    rdfs:range <http://rdaregistry.info/Elements/c/C10006> ;
    rdfs:subPropertyOf <http://rdaregistry.info/Elements/e/P20152> ;
    owl:inverseOf <http://rdaregistry.info/Elements/e/P20092> ;
    skos:definition "Relates an expression to an expression of a work that has been adapted as a work consisting of movement (e.g., dance)."@en .

<http://rdaregistry.info/Elements/e/P20184>
    reg:hasUnconstrained <http://rdaregistry.info/Elements/u/P60294> ;
    reg:lexicalAlias <http://rdaregistry.info/Elements/e/expandedVersionOfExpression.en> ;
    reg:name "expandedVersionOfExpression"@en ;
    reg:status <http://metadataregistry.org/uri/RegStatus/1001> ;
    rdakit:toolkitDefinition "An expression of a work used as the basis for a derivative work that enlarges upon the content of the source work."@en ;
    rdakit:toolkitLabel "expanded version of (expression)"@en ;
    a rdf:Property ;
    rdfs:domain <http://rdaregistry.info/Elements/c/C10006> ;
    rdfs:isDefinedBy <http://rdaregistry.info/Elements/e/> ;
    rdfs:label "is expanded version of (expression)"@en ;
    rdfs:range <http://rdaregistry.info/Elements/c/C10006> ;
    rdfs:subPropertyOf <http://rdaregistry.info/Elements/e/P20204> ;
    owl:inverseOf <http://rdaregistry.info/Elements/e/P20115> ;
    skos:definition "Relates an expression to an expression of a work used as the basis for a derivative work that enlarges upon the content of the source work."@en .

<http://rdaregistry.info/Elements/e/P20185>
    reg:hasUnconstrained <http://rdaregistry.info/Elements/u/P60295> ;
    reg:lexicalAlias <http://rdaregistry.info/Elements/e/remakeOfExpression.en> ;
    reg:name "remakeOfExpression"@en ;
    reg:status <http://metadataregistry.org/uri/RegStatus/1001> ;
    rdakit:toolkitDefinition "An expression of a work used as the basis for a new motion picture, radio program, television program, or video."@en ;
    rdakit:toolkitLabel "remake of (expression)"@en ;
    a rdf:Property ;
    rdfs:domain <http://rdaregistry.info/Elements/c/C10006> ;
    rdfs:isDefinedBy <http://rdaregistry.info/Elements/e/> ;
    rdfs:label "is remake of (expression)"@en ;
    rdfs:range <http://rdaregistry.info/Elements/c/C10006> ;
    rdfs:subPropertyOf <http://rdaregistry.info/Elements/e/P20204> ;
    owl:inverseOf <http://rdaregistry.info/Elements/e/P20086> ;
    skos:definition "Relates an expression to an expression of a work used as the basis for a new motion picture, radio program, television program, or video."@en .

<http://rdaregistry.info/Elements/e/P20186>
    reg:hasUnconstrained <http://rdaregistry.info/Elements/u/P60296> ;
    reg:lexicalAlias <http://rdaregistry.info/Elements/e/paraphraseOfExpression.en> ;
    reg:name "paraphraseOfExpression"@en ;
    reg:status <http://metadataregistry.org/uri/RegStatus/1001> ;
    rdakit:toolkitDefinition "An expression of a work used as the basis for a paraphrase, i.e., a restating of the content of the source work in a different form."@en ;
    rdakit:toolkitLabel "paraphrase of (expression)"@en ;
    a rdf:Property ;
    rdfs:domain <http://rdaregistry.info/Elements/c/C10006> ;
    rdfs:isDefinedBy <http://rdaregistry.info/Elements/e/> ;
    rdfs:label "is paraphrase of (expression)"@en ;
    rdfs:range <http://rdaregistry.info/Elements/c/C10006> ;
    rdfs:subPropertyOf <http://rdaregistry.info/Elements/e/P20204> ;
    owl:inverseOf <http://rdaregistry.info/Elements/e/P20164> ;
    skos:definition "Relates an expression to an expression of a work used as the basis for a paraphrase, i.e., a restating of the content of the source work in a different form."@en .

<http://rdaregistry.info/Elements/e/P20187>
    reg:status <http://metadataregistry.org/uri/RegStatus/1008> ;
    a rdf:Property ;
    rdfs:isDefinedBy <http://rdaregistry.info/Elements/e/> .

<http://rdaregistry.info/Elements/e/P20188>
    reg:hasUnconstrained <http://rdaregistry.info/Elements/u/P60302> ;
    reg:lexicalAlias <http://rdaregistry.info/Elements/e/indexToExpression.en> ;
    reg:name "indexToExpression"@en ;
    reg:status <http://metadataregistry.org/uri/RegStatus/1001> ;
    rdakit:toolkitDefinition "An expression of a work used as the basis for an index, i.e., a systematic, alphabetical guide to the contents of the predominant expression, usually keyed to page numbers or other reference codes."@en ;
    rdakit:toolkitLabel "index to (expression)"@en ;
    a rdf:Property ;
    rdfs:domain <http://rdaregistry.info/Elements/c/C10006> ;
    rdfs:isDefinedBy <http://rdaregistry.info/Elements/e/> ;
    rdfs:label "is index to (expression)"@en ;
    rdfs:range <http://rdaregistry.info/Elements/c/C10006> ;
    rdfs:subPropertyOf <http://rdaregistry.info/Elements/e/P20192> ;
    owl:inverseOf <http://rdaregistry.info/Elements/e/P20156> ;
    skos:definition "Relates an expression to an expression of a work used as the basis for an index, i.e., a systematic, alphabetical guide to the contents of the predominant expression, usually keyed to page numbers or other reference codes."@en .

<http://rdaregistry.info/Elements/e/P20189>
    reg:hasUnconstrained <http://rdaregistry.info/Elements/u/P60303> ;
    reg:lexicalAlias <http://rdaregistry.info/Elements/e/revisionOf.en> ;
    reg:name "revisionOf"@en ;
    reg:status <http://metadataregistry.org/uri/RegStatus/1001> ;
    rdakit:toolkitDefinition "An expression of a work used as the basis for an updated, corrected, or expanded version."@en ;
    rdakit:toolkitLabel "revision of"@en ;
    a rdf:Property ;
    rdfs:domain <http://rdaregistry.info/Elements/c/C10006> ;
    rdfs:isDefinedBy <http://rdaregistry.info/Elements/e/> ;
    rdfs:label "is revision of"@en ;
    rdfs:range <http://rdaregistry.info/Elements/c/C10006> ;
    rdfs:subPropertyOf <http://rdaregistry.info/Elements/e/P20204> ;
    owl:inverseOf <http://rdaregistry.info/Elements/e/P20211> ;
    skos:definition "Relates an expression to an expression of a work used as the basis for an updated, corrected, or expanded version."@en .

<http://rdaregistry.info/Elements/e/P20190>
    reg:hasUnconstrained <http://rdaregistry.info/Elements/u/P60304> ;
    reg:lexicalAlias <http://rdaregistry.info/Elements/e/librettoBasedOnExpression.en> ;
    reg:name "librettoBasedOnExpression"@en ;
    reg:status <http://metadataregistry.org/uri/RegStatus/1001> ;
    rdakit:toolkitDefinition "An expression of a work used as the basis for the text of an opera or other work for the musical stage, or an oratorio."@en ;
    rdakit:toolkitLabel "libretto based on (expression)"@en ;
    a rdf:Property ;
    rdfs:domain <http://rdaregistry.info/Elements/c/C10006> ;
    rdfs:isDefinedBy <http://rdaregistry.info/Elements/e/> ;
    rdfs:label "is libretto based on (expression)"@en ;
    rdfs:range <http://rdaregistry.info/Elements/c/C10006> ;
    rdfs:subPropertyOf <http://rdaregistry.info/Elements/e/P20152> ;
    owl:inverseOf <http://rdaregistry.info/Elements/e/P20110> ;
    skos:definition "Relates an expression to an expression of a work that has been adapted as the text of an opera or other work for the musical stage, or an oratorio."@en .

<http://rdaregistry.info/Elements/e/P20191>
    reg:hasUnconstrained <http://rdaregistry.info/Elements/u/P60306> ;
    reg:lexicalAlias <http://rdaregistry.info/Elements/e/continuedByExpression.en> ;
    reg:name "continuedByExpression"@en ;
    reg:status <http://metadataregistry.org/uri/RegStatus/1001> ;
    rdakit:toolkitDefinition "An expression of a work whose content continues an expression of an earlier work."@en ;
    rdakit:toolkitLabel "continued by (expression)"@en ;
    a rdf:Property ;
    rdfs:domain <http://rdaregistry.info/Elements/c/C10006> ;
    rdfs:isDefinedBy <http://rdaregistry.info/Elements/e/> ;
    rdfs:label "is continued by (expression)"@en ;
    rdfs:range <http://rdaregistry.info/Elements/c/C10006> ;
    rdfs:subPropertyOf <http://rdaregistry.info/Elements/e/P20169> ;
    owl:inverseOf <http://rdaregistry.info/Elements/e/P20149> ;
    skos:definition "Relates an expression to an expression of a work whose content continues an expression of an earlier work."@en .

<http://rdaregistry.info/Elements/e/P20192>
    reg:hasSubproperty <http://rdaregistry.info/Elements/e/P20083>, <http://rdaregistry.info/Elements/e/P20089>, <http://rdaregistry.info/Elements/e/P20146>, <http://rdaregistry.info/Elements/e/P20147>, <http://rdaregistry.info/Elements/e/P20148>, <http://rdaregistry.info/Elements/e/P20151>, <http://rdaregistry.info/Elements/e/P20177>, <http://rdaregistry.info/Elements/e/P20180>, <http://rdaregistry.info/Elements/e/P20181>, <http://rdaregistry.info/Elements/e/P20188>, <http://rdaregistry.info/Elements/e/P20197> ;
    reg:hasUnconstrained <http://rdaregistry.info/Elements/u/P60307> ;
    reg:lexicalAlias <http://rdaregistry.info/Elements/e/augmentationOfExpression.en> ;
    reg:name "augmentationOfExpression"@en ;
    reg:status <http://metadataregistry.org/uri/RegStatus/1001> ;
    rdakit:toolkitDefinition "An expression of a work whose content is added to by another expression."@en ;
    rdakit:toolkitLabel "augmentation of (expression)"@en ;
    a rdf:Property ;
    rdfs:domain <http://rdaregistry.info/Elements/c/C10006> ;
    rdfs:isDefinedBy <http://rdaregistry.info/Elements/e/> ;
    rdfs:label "is augmentation of (expression)"@en ;
    rdfs:range <http://rdaregistry.info/Elements/c/C10006> ;
    rdfs:subPropertyOf <http://rdaregistry.info/Elements/e/P20232> ;
    owl:inverseOf <http://rdaregistry.info/Elements/e/P20105> ;
    skos:definition "Relates an expression to an expression of a work whose content is added to by another expression."@en .

<http://rdaregistry.info/Elements/e/P20193>
    reg:hasUnconstrained <http://rdaregistry.info/Elements/u/P60308> ;
    reg:lexicalAlias <http://rdaregistry.info/Elements/e/abstractsForExpression.en> ;
    reg:name "abstractsForExpression"@en ;
    reg:status <http://metadataregistry.org/uri/RegStatus/1001> ;
    rdakit:toolkitDefinition "An expression of a work whose contents have been abstracted by an abstracting and indexing service."@en ;
    rdakit:toolkitLabel "abstracts for (expression)"@en ;
    a rdf:Property ;
    rdfs:domain <http://rdaregistry.info/Elements/c/C10006> ;
    rdfs:isDefinedBy <http://rdaregistry.info/Elements/e/> ;
    rdfs:label "is abstracts for (expression)"@en ;
    rdfs:range <http://rdaregistry.info/Elements/c/C10006> ;
    rdfs:subPropertyOf <http://rdaregistry.info/Elements/e/P20204> ;
    owl:inverseOf <http://rdaregistry.info/Elements/e/P20090> ;
    skos:definition "Relates an expression to an expression of a work whose contents have been abstracted by an abstracting and indexing service."@en .

<http://rdaregistry.info/Elements/e/P20194>
    reg:hasUnconstrained <http://rdaregistry.info/Elements/u/P60309> ;
    reg:lexicalAlias <http://rdaregistry.info/Elements/e/indexingForExpression.en> ;
    reg:name "indexingForExpression"@en ;
    reg:status <http://metadataregistry.org/uri/RegStatus/1001> ;
    rdakit:toolkitDefinition "An expression of a work whose contents have been indexed by an abstracting and indexing service."@en ;
    rdakit:toolkitLabel "indexing for (expression)"@en ;
    a rdf:Property ;
    rdfs:domain <http://rdaregistry.info/Elements/c/C10006> ;
    rdfs:isDefinedBy <http://rdaregistry.info/Elements/e/> ;
    rdfs:label "is indexing for (expression)"@en ;
    rdfs:range <http://rdaregistry.info/Elements/c/C10006> ;
    rdfs:subPropertyOf <http://rdaregistry.info/Elements/e/P20204> ;
    owl:inverseOf <http://rdaregistry.info/Elements/e/P20091> ;
    skos:definition "Relates an expression to an expression of a work whose contents have been indexed by an abstracting and indexing service."@en .

<http://rdaregistry.info/Elements/e/P20195>
    reg:hasSubproperty <http://rdaregistry.info/Elements/e/P20196> ;
    reg:hasUnconstrained <http://rdaregistry.info/Elements/u/P60311> ;
    reg:lexicalAlias <http://rdaregistry.info/Elements/e/imitationOfExpression.en> ;
    reg:name "imitationOfExpression"@en ;
    reg:status <http://metadataregistry.org/uri/RegStatus/1001> ;
    rdakit:toolkitDefinition "An expression of a work whose style or content is copied in a derivative work."@en ;
    rdakit:toolkitLabel "imitation of (expression)"@en ;
    a rdf:Property ;
    rdfs:domain <http://rdaregistry.info/Elements/c/C10006> ;
    rdfs:isDefinedBy <http://rdaregistry.info/Elements/e/> ;
    rdfs:label "is imitation of (expression)"@en ;
    rdfs:range <http://rdaregistry.info/Elements/c/C10006> ;
    rdfs:subPropertyOf <http://rdaregistry.info/Elements/e/P20204> ;
    owl:inverseOf <http://rdaregistry.info/Elements/e/P20114> ;
    skos:definition "Relates an expression to an expression of a work whose style or content is copied in a derivative work."@en .

<http://rdaregistry.info/Elements/e/P20196>
    reg:hasUnconstrained <http://rdaregistry.info/Elements/u/P60312> ;
    reg:lexicalAlias <http://rdaregistry.info/Elements/e/parodyOfExpression.en> ;
    reg:name "parodyOfExpression"@en ;
    reg:status <http://metadataregistry.org/uri/RegStatus/1001> ;
    rdakit:toolkitDefinition "An expression of a work whose style or content is imitated for comic effect."@en ;
    rdakit:toolkitLabel "parody of (expression)"@en ;
    a rdf:Property ;
    rdfs:domain <http://rdaregistry.info/Elements/c/C10006> ;
    rdfs:isDefinedBy <http://rdaregistry.info/Elements/e/> ;
    rdfs:label "is parody of (expression)"@en ;
    rdfs:range <http://rdaregistry.info/Elements/c/C10006> ;
    rdfs:subPropertyOf <http://rdaregistry.info/Elements/e/P20195> ;
    owl:inverseOf <http://rdaregistry.info/Elements/e/P20142> ;
    skos:definition "Relates an expression to an expression of a work whose style or content is imitated for comic effect."@en .

<http://rdaregistry.info/Elements/e/P20197>
    reg:hasUnconstrained <http://rdaregistry.info/Elements/u/P60474> ;
    reg:lexicalAlias <http://rdaregistry.info/Elements/e/findingAidForExpression.en> ;
    reg:name "findingAidForExpression"@en ;
    reg:status <http://metadataregistry.org/uri/RegStatus/1001> ;
    rdakit:toolkitDefinition "An expression of an archival collection that is described in a finding aid, i.e., a guide to the organization, arrangement, and contents of the collection."@en ;
    rdakit:toolkitLabel "finding aid for (expression)"@en ;
    a rdf:Property ;
    rdfs:domain <http://rdaregistry.info/Elements/c/C10006> ;
    rdfs:isDefinedBy <http://rdaregistry.info/Elements/e/> ;
    rdfs:label "is finding aid for (expression)"@en ;
    rdfs:range <http://rdaregistry.info/Elements/c/C10006> ;
    rdfs:subPropertyOf <http://rdaregistry.info/Elements/e/P20192> ;
    owl:inverseOf <http://rdaregistry.info/Elements/e/P20155> ;
    skos:definition "Relates an expression to an expression of an archival collection that is described in a finding aid, i.e., a guide to the organization, arrangement, and contents of the collection."@en .

<http://rdaregistry.info/Elements/e/P20198>
    reg:hasUnconstrained <http://rdaregistry.info/Elements/u/P60479> ;
    reg:lexicalAlias <http://rdaregistry.info/Elements/e/replacementInPartOfExpression.en> ;
    reg:name "replacementInPartOfExpression"@en ;
    reg:status <http://metadataregistry.org/uri/RegStatus/1001> ;
    rdakit:toolkitDefinition "An expression of an earlier work whose content has been partially replaced by a later expression, usually because the later work contains updated or new information that makes the earlier expression obsolete."@en ;
    rdakit:toolkitLabel "replacement in part of (expression)"@en ;
    a rdf:Property ;
    rdfs:domain <http://rdaregistry.info/Elements/c/C10006> ;
    rdfs:isDefinedBy <http://rdaregistry.info/Elements/e/> ;
    rdfs:label "is replacement in part of (expression)"@en ;
    rdfs:range <http://rdaregistry.info/Elements/c/C10006> ;
    rdfs:subPropertyOf <http://rdaregistry.info/Elements/e/P20154> ;
    owl:inverseOf <http://rdaregistry.info/Elements/e/P20075> ;
    skos:definition "Relates an expression to an expression of an earlier work whose content has been partially replaced by a later expression, usually because the later work contains updated or new information that makes the earlier expression obsolete."@en .

<http://rdaregistry.info/Elements/e/P20199>
    reg:hasUnconstrained <http://rdaregistry.info/Elements/u/P60480> ;
    reg:lexicalAlias <http://rdaregistry.info/Elements/e/replacementOfExpression.en> ;
    reg:name "replacementOfExpression"@en ;
    reg:status <http://metadataregistry.org/uri/RegStatus/1001> ;
    rdakit:toolkitDefinition "An expression of an earlier work whose content has been replaced by a later expression, usually because the later work contains updated or new information that makes the earlier expression obsolete."@en ;
    rdakit:toolkitLabel "replacement of (expression)"@en ;
    a rdf:Property ;
    rdfs:domain <http://rdaregistry.info/Elements/c/C10006> ;
    rdfs:isDefinedBy <http://rdaregistry.info/Elements/e/> ;
    rdfs:label "is replacement of (expression)"@en ;
    rdfs:range <http://rdaregistry.info/Elements/c/C10006> ;
    rdfs:subPropertyOf <http://rdaregistry.info/Elements/e/P20154> ;
    owl:inverseOf <http://rdaregistry.info/Elements/e/P20076> ;
    skos:definition "Relates an expression to an expression of an earlier work whose content has been replaced by a later expression, usually because the later work contains updated or new information that makes the earlier expression obsolete."@en .

<http://rdaregistry.info/Elements/e/P20200>
    reg:hasUnconstrained <http://rdaregistry.info/Elements/u/P60503> ;
    reg:lexicalAlias <http://rdaregistry.info/Elements/e/splitIntoExpression.en> ;
    reg:name "splitIntoExpression"@en ;
    reg:status <http://metadataregistry.org/uri/RegStatus/1001> ;
    rdakit:toolkitDefinition "An expression of one of two or more works resulting from the division of an earlier expression into separate expressions."@en ;
    rdakit:toolkitLabel "split into (expression)"@en ;
    a rdf:Property ;
    rdfs:domain <http://rdaregistry.info/Elements/c/C10006> ;
    rdfs:isDefinedBy <http://rdaregistry.info/Elements/e/> ;
    rdfs:label "is split into (expression)"@en ;
    rdfs:range <http://rdaregistry.info/Elements/c/C10006> ;
    rdfs:subPropertyOf <http://rdaregistry.info/Elements/e/P20169> ;
    owl:inverseOf <http://rdaregistry.info/Elements/e/P20167> ;
    skos:definition "Relates an expression to an expression of one of two or more works resulting from the division of an earlier expression into separate expressions."@en .

<http://rdaregistry.info/Elements/e/P20201>
    reg:hasUnconstrained <http://rdaregistry.info/Elements/u/P60505> ;
    reg:lexicalAlias <http://rdaregistry.info/Elements/e/mergerOfExpression.en> ;
    reg:name "mergerOfExpression"@en ;
    reg:status <http://metadataregistry.org/uri/RegStatus/1001> ;
    rdakit:toolkitDefinition "An expression of a work that came together with one or more other expressions to form the new expression."@en ;
    rdakit:toolkitLabel "merger of (expression)"@en ;
    a rdf:Property ;
    rdfs:domain <http://rdaregistry.info/Elements/c/C10006> ;
    rdfs:isDefinedBy <http://rdaregistry.info/Elements/e/> ;
    rdfs:label "is merger of (expression)"@en ;
    rdfs:range <http://rdaregistry.info/Elements/c/C10006> ;
    rdfs:subPropertyOf <http://rdaregistry.info/Elements/e/P20154> ;
    owl:inverseOf <http://rdaregistry.info/Elements/e/P20212> ;
    skos:definition "Relates an expression to an expression of a work that came together with one or more other expressions to form the new expression."@en .

<http://rdaregistry.info/Elements/e/P20202>
    reg:status <http://metadataregistry.org/uri/RegStatus/1008> ;
    a rdf:Property ;
    rdfs:isDefinedBy <http://rdaregistry.info/Elements/e/> .

<http://rdaregistry.info/Elements/e/P20203>
    reg:hasSubproperty <http://rdaregistry.info/Elements/e/P20082>, <http://rdaregistry.info/Elements/e/P20086>, <http://rdaregistry.info/Elements/e/P20087>, <http://rdaregistry.info/Elements/e/P20090>, <http://rdaregistry.info/Elements/e/P20091>, <http://rdaregistry.info/Elements/e/P20092>, <http://rdaregistry.info/Elements/e/P20104>, <http://rdaregistry.info/Elements/e/P20106>, <http://rdaregistry.info/Elements/e/P20110>, <http://rdaregistry.info/Elements/e/P20114>, <http://rdaregistry.info/Elements/e/P20115>, <http://rdaregistry.info/Elements/e/P20119>, <http://rdaregistry.info/Elements/e/P20153>, <http://rdaregistry.info/Elements/e/P20164>, <http://rdaregistry.info/Elements/e/P20165>, <http://rdaregistry.info/Elements/e/P20166>, <http://rdaregistry.info/Elements/e/P20170>, <http://rdaregistry.info/Elements/e/P20171>, <http://rdaregistry.info/Elements/e/P20204>, <http://rdaregistry.info/Elements/e/P20211> ;
    reg:hasUnconstrained <http://rdaregistry.info/Elements/u/P60250> ;
    reg:lexicalAlias <http://rdaregistry.info/Elements/e/derivativeExpression.en> ;
    reg:name "derivativeExpression"@en ;
    reg:status <http://metadataregistry.org/uri/RegStatus/1001> ;
    rdakit:toolkitDefinition "An expression that is a modification of a source expression."@en ;
    rdakit:toolkitLabel "derivative (expression)"@en ;
    a rdf:Property ;
    rdfs:domain <http://rdaregistry.info/Elements/c/C10006> ;
    rdfs:isDefinedBy <http://rdaregistry.info/Elements/e/> ;
    rdfs:label "is derivative (expression)"@en ;
    rdfs:range <http://rdaregistry.info/Elements/c/C10006> ;
    rdfs:subPropertyOf <http://rdaregistry.info/Elements/e/P20233> ;
    owl:inverseOf <http://rdaregistry.info/Elements/e/P20204> ;
    skos:definition "Relates an expression to an expression that is a modification of a source expression."@en .

<http://rdaregistry.info/Elements/e/P20204>
    reg:hasSubproperty <http://rdaregistry.info/Elements/e/P20081>, <http://rdaregistry.info/Elements/e/P20121>, <http://rdaregistry.info/Elements/e/P20122>, <http://rdaregistry.info/Elements/e/P20135>, <http://rdaregistry.info/Elements/e/P20139>, <http://rdaregistry.info/Elements/e/P20140>, <http://rdaregistry.info/Elements/e/P20141>, <http://rdaregistry.info/Elements/e/P20152>, <http://rdaregistry.info/Elements/e/P20159>, <http://rdaregistry.info/Elements/e/P20179>, <http://rdaregistry.info/Elements/e/P20183>, <http://rdaregistry.info/Elements/e/P20184>, <http://rdaregistry.info/Elements/e/P20185>, <http://rdaregistry.info/Elements/e/P20186>, <http://rdaregistry.info/Elements/e/P20189>, <http://rdaregistry.info/Elements/e/P20190>, <http://rdaregistry.info/Elements/e/P20193>, <http://rdaregistry.info/Elements/e/P20194>, <http://rdaregistry.info/Elements/e/P20195> ;
    reg:hasUnconstrained <http://rdaregistry.info/Elements/u/P60305> ;
    reg:lexicalAlias <http://rdaregistry.info/Elements/e/basedOnExpression.en> ;
    reg:name "basedOnExpression"@en ;
    reg:status <http://metadataregistry.org/uri/RegStatus/1001> ;
    rdakit:toolkitDefinition "An expression used as the basis for a derivative expression"@en ;
    rdakit:toolkitLabel "based on (expression)"@en ;
    a rdf:Property ;
    rdfs:domain <http://rdaregistry.info/Elements/c/C10006> ;
    rdfs:isDefinedBy <http://rdaregistry.info/Elements/e/> ;
    rdfs:label "is based on (expression)"@en ;
    rdfs:range <http://rdaregistry.info/Elements/c/C10006> ;
    rdfs:subPropertyOf <http://rdaregistry.info/Elements/e/P20233> ;
    owl:inverseOf <http://rdaregistry.info/Elements/e/P20203> ;
    skos:definition "Relates an expression to an expression used as the basis for a derivative expression"@en .

<http://rdaregistry.info/Elements/e/P20205>
    reg:hasSubproperty <http://rdaregistry.info/Elements/e/P20232>, <http://rdaregistry.info/Elements/e/P20233>, <http://rdaregistry.info/Elements/e/P20235>, <http://rdaregistry.info/Elements/e/P20236> ;
    reg:hasUnconstrained <http://rdaregistry.info/Elements/u/P60313> ;
    reg:lexicalAlias <http://rdaregistry.info/Elements/e/relatedExpression.en> ;
    reg:name "relatedExpression"@en ;
    reg:status <http://metadataregistry.org/uri/RegStatus/1001> ;
    rdakit:instructionNumber "26.1" ;
    rdakit:toolkitDefinition "An expression, represented by an identifier, an authorized access point, or a description, that is related to the expression being described (e.g., a revised version, a translation)."@en ;
    rdakit:toolkitLabel "related expression"@en ;
    a rdf:Property ;
    rdfs:domain <http://rdaregistry.info/Elements/c/C10006> ;
    rdfs:isDefinedBy <http://rdaregistry.info/Elements/e/> ;
    rdfs:label "has related expression"@en ;
    rdfs:range <http://rdaregistry.info/Elements/c/C10006> ;
    owl:inverseOf <http://rdaregistry.info/Elements/e/P20205> ;
    skos:definition "Relates an expression to an expression, represented by an identifier, an authorized access point, or a description, that is related to the expression being described (e.g., a revised version, a translation)."@en .

<http://rdaregistry.info/Elements/e/P20206>
    reg:hasUnconstrained <http://rdaregistry.info/Elements/u/P60485> ;
    reg:lexicalAlias <http://rdaregistry.info/Elements/e/supplementaryContent.en> ;
    reg:name "supplementaryContent"@en ;
    reg:status <http://metadataregistry.org/uri/RegStatus/1001> ;
    rdakit:instructionNumber "7.16" ;
    rdakit:toolkitDefinition "Content (e.g., an index, a bibliography, an appendix) intended to supplement the primary content of a resource."@en ;
    rdakit:toolkitLabel "supplementary content"@en ;
    a rdf:Property ;
    rdfs:domain <http://rdaregistry.info/Elements/c/C10006> ;
    rdfs:isDefinedBy <http://rdaregistry.info/Elements/e/> ;
    rdfs:label "has supplementary content"@en ;
    skos:definition "Relates an expression to content (e.g., an index, a bibliography, an appendix) intended to supplement the primary content of a resource."@en .

<http://rdaregistry.info/Elements/e/P20207>
    reg:hasUnconstrained <http://rdaregistry.info/Elements/u/P60486> ;
    reg:lexicalAlias <http://rdaregistry.info/Elements/e/illustrativeContent.en> ;
    reg:name "illustrativeContent"@en ;
    reg:status <http://metadataregistry.org/uri/RegStatus/1001> ;
    rdakit:instructionNumber "7.15" ;
    rdakit:toolkitDefinition "Content intended to illustrate the primary content of a resource."@en ;
    rdakit:toolkitLabel "illustrative content"@en ;
    a rdf:Property ;
    rdfs:domain <http://rdaregistry.info/Elements/c/C10006> ;
    rdfs:isDefinedBy <http://rdaregistry.info/Elements/e/> ;
    rdfs:label "has illustrative content"@en ;
    skos:definition "Relates an expression to content intended to illustrate the primary content of a resource."@en .

<http://rdaregistry.info/Elements/e/P20208>
    reg:hasUnconstrained <http://rdaregistry.info/Elements/u/P60487> ;
    reg:lexicalAlias <http://rdaregistry.info/Elements/e/accessibilityContent.en> ;
    reg:name "accessibilityContent"@en ;
    reg:status <http://metadataregistry.org/uri/RegStatus/1001> ;
    rdakit:instructionNumber "7.14" ;
    rdakit:toolkitDefinition "Content that assists those with a sensory impairment in the greater understanding of content which their impairment prevents them fully seeing or hearing."@en ;
    rdakit:toolkitLabel "accessibility content"@en ;
    a rdf:Property ;
    rdfs:domain <http://rdaregistry.info/Elements/c/C10006> ;
    rdfs:isDefinedBy <http://rdaregistry.info/Elements/e/> ;
    rdfs:label "has accessibility content"@en ;
    skos:definition "Relates an expression to content that assists those with a sensory impairment in the greater understanding of content which their impairment prevents them fully seeing or hearing."@en .

<http://rdaregistry.info/Elements/e/P20209>
    reg:hasUnconstrained <http://rdaregistry.info/Elements/u/P60488> ;
    reg:lexicalAlias <http://rdaregistry.info/Elements/e/formatOfNotatedMusic.en> ;
    reg:name "formatOfNotatedMusic"@en ;
    reg:status <http://metadataregistry.org/uri/RegStatus/1001> ;
    rdakit:instructionNumber "7.2" ;
    rdakit:toolkitDefinition "The musical or physical layout of the content of a resource that is presented in the form of musical notation."@en ;
    rdakit:toolkitLabel "format of notated music"@en ;
    a rdf:Property ;
    rdfs:domain <http://rdaregistry.info/Elements/c/C10006> ;
    rdfs:isDefinedBy <http://rdaregistry.info/Elements/e/> ;
    rdfs:label "has format of notated music"@en ;
    skos:definition "Relates an expression to the musical or physical layout of the content of a resource that is presented in the form of musical notation."@en .

<http://rdaregistry.info/Elements/e/P20210>
    reg:hasUnconstrained <http://rdaregistry.info/Elements/u/P60498> ;
    reg:lexicalAlias <http://rdaregistry.info/Elements/e/otherDetailsOfCartographicContent.en> ;
    reg:name "otherDetailsOfCartographicContent"@en ;
    reg:status <http://metadataregistry.org/uri/RegStatus/1001> ;
    rdakit:instructionNumber "7.27" ;
    rdakit:toolkitDefinition "Mathematical data and other features of the cartographic content of a resource not recorded in statements of scale, projection, and coordinates."@en ;
    rdakit:toolkitLabel "other details of cartographic content"@en ;
    a rdf:Property ;
    rdfs:domain <http://rdaregistry.info/Elements/c/C10006> ;
    rdfs:isDefinedBy <http://rdaregistry.info/Elements/e/> ;
    rdfs:label "has other details of cartographic content"@en ;
    skos:definition "Relates an expression to mathematical data and other features of the cartographic content of a resource not recorded in statements of scale, projection, and coordinates."@en .

<http://rdaregistry.info/Elements/e/P20211>
    reg:hasUnconstrained <http://rdaregistry.info/Elements/u/P60245> ;
    reg:lexicalAlias <http://rdaregistry.info/Elements/e/revisedAs.en> ;
    reg:name "revisedAs"@en ;
    reg:status <http://metadataregistry.org/uri/RegStatus/1001> ;
    rdakit:toolkitDefinition "An expression of a work that has been updated, corrected, or expanded."@en ;
    rdakit:toolkitLabel "revised as"@en ;
    a rdf:Property ;
    rdfs:domain <http://rdaregistry.info/Elements/c/C10006> ;
    rdfs:isDefinedBy <http://rdaregistry.info/Elements/e/> ;
    rdfs:label "is revised as"@en ;
    rdfs:range <http://rdaregistry.info/Elements/c/C10006> ;
    rdfs:subPropertyOf <http://rdaregistry.info/Elements/e/P20203> ;
    owl:inverseOf <http://rdaregistry.info/Elements/e/P20189> ;
    skos:definition "Relates an expression to an expression of a work that has been updated, corrected, or expanded."@en .

<http://rdaregistry.info/Elements/e/P20212>
    reg:hasUnconstrained <http://rdaregistry.info/Elements/u/P60504> ;
    reg:lexicalAlias <http://rdaregistry.info/Elements/e/mergedToFormExpression.en> ;
    reg:name "mergedToFormExpression"@en ;
    reg:status <http://metadataregistry.org/uri/RegStatus/1001> ;
    rdakit:toolkitDefinition "An expression of a work formed from the coming together of two or more expressions."@en ;
    rdakit:toolkitLabel "merged to form (expression)"@en ;
    a rdf:Property ;
    rdfs:domain <http://rdaregistry.info/Elements/c/C10006> ;
    rdfs:isDefinedBy <http://rdaregistry.info/Elements/e/> ;
    rdfs:label "is merged to form (expression)"@en ;
    rdfs:range <http://rdaregistry.info/Elements/c/C10006> ;
    rdfs:subPropertyOf <http://rdaregistry.info/Elements/e/P20169> ;
    owl:inverseOf <http://rdaregistry.info/Elements/e/P20201> ;
    skos:definition "Relates an expression to an expression of a work formed from the coming together of two or more expressions."@en .

<http://rdaregistry.info/Elements/e/P20213>
    reg:hasUnconstrained <http://rdaregistry.info/Elements/u/P60510> ;
    reg:lexicalAlias <http://rdaregistry.info/Elements/e/additionalScaleInformation.en> ;
    reg:name "additionalScaleInformation"@en ;
    reg:status <http://metadataregistry.org/uri/RegStatus/1001> ;
    rdakit:instructionNumber "7.25.5" ;
    rdakit:toolkitDefinition "Supplemental information about scale such as a statement of comparative measurements or limitation of the scale to particular parts of the content of a resource."@en ;
    rdakit:toolkitLabel "additional scale information"@en ;
    a rdf:Property ;
    rdfs:domain <http://rdaregistry.info/Elements/c/C10006> ;
    rdfs:isDefinedBy <http://rdaregistry.info/Elements/e/> ;
    rdfs:label "has additional scale information"@en ;
    rdfs:subPropertyOf <http://rdaregistry.info/Elements/e/P20228> ;
    skos:definition "Relates an expression to supplemental information about scale such as a statement of comparative measurements or limitation of the scale to particular parts of the content of a resource."@en .

<http://rdaregistry.info/Elements/e/P20214>
    reg:hasUnconstrained <http://rdaregistry.info/Elements/u/P60527> ;
    reg:lexicalAlias <http://rdaregistry.info/Elements/e/dateOfExpression.en> ;
    reg:name "dateOfExpression"@en ;
    reg:status <http://metadataregistry.org/uri/RegStatus/1001> ;
    rdakit:instructionNumber "6.1" ;
    rdakit:toolkitDefinition "The earliest date associated with an expression."@en ;
    rdakit:toolkitLabel "date of expression"@en ;
    a rdf:Property ;
    rdfs:domain <http://rdaregistry.info/Elements/c/C10006> ;
    rdfs:isDefinedBy <http://rdaregistry.info/Elements/e/> ;
    rdfs:label "has date of expression"@en ;
    skos:definition "Relates an expression to the earliest date associated with an expression."@en .

<http://rdaregistry.info/Elements/e/P20215>
    reg:hasUnconstrained <http://rdaregistry.info/Elements/u/P60537> ;
    reg:lexicalAlias <http://rdaregistry.info/Elements/e/mediumOfPerformanceOfMusicalContent.en> ;
    reg:name "mediumOfPerformanceOfMusicalContent"@en ;
    reg:status <http://metadataregistry.org/uri/RegStatus/1001> ;
    rdakit:instructionNumber "7.21" ;
    rdakit:toolkitDefinition "The instrument, instruments, voice, voices, etc., used (or intended to be used) for performance of musical content."@en ;
    rdakit:toolkitLabel "medium of performance of musical content"@en ;
    a rdf:Property ;
    rdfs:domain <http://rdaregistry.info/Elements/c/C10006> ;
    rdfs:isDefinedBy <http://rdaregistry.info/Elements/e/> ;
    rdfs:label "has medium of performance of musical content"@en ;
    skos:definition "Relates an expression to the instrument, instruments, voice, voices, etc., used (or intended to be used) for performance of musical content."@en .

<http://rdaregistry.info/Elements/e/P20216>
    reg:hasUnconstrained <http://rdaregistry.info/Elements/u/P60542> ;
    reg:lexicalAlias <http://rdaregistry.info/Elements/e/projectionOfCartographicContent.en> ;
    reg:name "projectionOfCartographicContent"@en ;
    reg:status <http://metadataregistry.org/uri/RegStatus/1001> ;
    rdakit:instructionNumber "7.26" ;
    rdakit:toolkitDefinition "The method or system used to represent the surface of the Earth or of a celestial sphere on a plane."@en ;
    rdakit:toolkitLabel "projection of cartographic content"@en ;
    a rdf:Property ;
    rdfs:domain <http://rdaregistry.info/Elements/c/C10006> ;
    rdfs:isDefinedBy <http://rdaregistry.info/Elements/e/> ;
    rdfs:label "has projection of cartographic content"@en ;
    skos:definition "Relates an expression to the method or system used to represent the surface of the earth or of a celestial sphere on a plane."@en .

<http://rdaregistry.info/Elements/e/P20217>
    reg:hasUnconstrained <http://rdaregistry.info/Elements/u/P60555> ;
    reg:lexicalAlias <http://rdaregistry.info/Elements/e/placeAndDateOfCapture.en> ;
    reg:name "placeAndDateOfCapture"@en ;
    reg:status <http://metadataregistry.org/uri/RegStatus/1001> ;
    rdakit:instructionNumber "7.11" ;
    rdakit:toolkitDefinition "The place and date associated with the capture (i.e., recording, filming, etc.) of the content of a resource."@en ;
    rdakit:toolkitLabel "place and date of capture"@en ;
    a rdf:Property ;
    rdfs:domain <http://rdaregistry.info/Elements/c/C10006> ;
    rdfs:isDefinedBy <http://rdaregistry.info/Elements/e/> ;
    rdfs:label "has place and date of capture"@en ;
    skos:definition "Relates an expression to the place and date associated with the capture (i.e., recording, filming, etc.) of the content of a resource."@en .

<http://rdaregistry.info/Elements/e/P20218>
    reg:hasUnconstrained <http://rdaregistry.info/Elements/u/P60556> ;
    reg:lexicalAlias <http://rdaregistry.info/Elements/e/placeOfCapture.en> ;
    reg:name "placeOfCapture"@en ;
    reg:status <http://metadataregistry.org/uri/RegStatus/1001> ;
    rdakit:instructionNumber "7.11.2" ;
    rdakit:toolkitDefinition "The place associated with the capture (i.e., recording, filming, etc.) of the content of a resource."@en ;
    rdakit:toolkitLabel "place of capture"@en ;
    a rdf:Property ;
    rdfs:domain <http://rdaregistry.info/Elements/c/C10006> ;
    rdfs:isDefinedBy <http://rdaregistry.info/Elements/e/> ;
    rdfs:label "has place of capture"@en ;
    skos:definition "Relates an expression to the place associated with the capture (i.e., recording, filming, etc.) of the content of a resource."@en .

<http://rdaregistry.info/Elements/e/P20219>
    reg:hasUnconstrained <http://rdaregistry.info/Elements/u/P60557> ;
    reg:lexicalAlias <http://rdaregistry.info/Elements/e/duration.en> ;
    reg:name "duration"@en ;
    reg:status <http://metadataregistry.org/uri/RegStatus/1001> ;
    rdakit:instructionNumber "7.22" ;
    rdakit:toolkitDefinition "The playing time, performance time, running time, etc., of the content of a resource."@en ;
    rdakit:toolkitLabel "duration"@en ;
    a rdf:Property ;
    rdfs:domain <http://rdaregistry.info/Elements/c/C10006> ;
    rdfs:isDefinedBy <http://rdaregistry.info/Elements/e/> ;
    rdfs:label "has duration"@en ;
    skos:definition "Relates an expression to the playing time, performance time, running time, etc., of the content of a resource."@en .

<http://rdaregistry.info/Elements/e/P20220>
    reg:status <http://metadataregistry.org/uri/RegStatus/1008> ;
    a rdf:Property ;
    rdfs:isDefinedBy <http://rdaregistry.info/Elements/e/> .

<http://rdaregistry.info/Elements/e/P20221>
    reg:status <http://metadataregistry.org/uri/RegStatus/1008> ;
    a rdf:Property ;
    rdfs:isDefinedBy <http://rdaregistry.info/Elements/e/> .

<http://rdaregistry.info/Elements/e/P20222>
    reg:status <http://metadataregistry.org/uri/RegStatus/1008> ;
    a rdf:Property ;
    rdfs:isDefinedBy <http://rdaregistry.info/Elements/e/> .

<http://rdaregistry.info/Elements/e/P20223>
    reg:status <http://metadataregistry.org/uri/RegStatus/1008> ;
    a rdf:Property ;
    rdfs:isDefinedBy <http://rdaregistry.info/Elements/e/> .

<http://rdaregistry.info/Elements/e/P20224>
    reg:hasUnconstrained <http://rdaregistry.info/Elements/u/P60558> ;
    reg:lexicalAlias <http://rdaregistry.info/Elements/e/colourContent.en> ;
    reg:name "colourContent"@en ;
    reg:status <http://metadataregistry.org/uri/RegStatus/1001> ;
    rdakit:instructionNumber "7.17" ;
    rdakit:toolkitDefinition "The presence of colour, tone, etc., in the content of a resource."@en ;
    rdakit:toolkitLabel "colour content"@en ;
    a rdf:Property ;
    rdfs:domain <http://rdaregistry.info/Elements/c/C10006> ;
    rdfs:isDefinedBy <http://rdaregistry.info/Elements/e/> ;
    rdfs:label "has colour content"@en ;
    skos:altLabel "has color content"@en ;
    skos:definition "Relates an expression to the presence of colour, tone, etc., in the content of a resource."@en .

<http://rdaregistry.info/Elements/e/P20225>
    reg:hasUnconstrained <http://rdaregistry.info/Elements/u/P60559> ;
    reg:lexicalAlias <http://rdaregistry.info/Elements/e/soundContent.en> ;
    reg:name "soundContent"@en ;
    reg:status <http://metadataregistry.org/uri/RegStatus/1001> ;
    rdakit:instructionNumber "7.18" ;
    rdakit:toolkitDefinition "The presence of sound in a resource other than one that consists primarily of recorded sound."@en ;
    rdakit:toolkitLabel "sound content"@en ;
    a rdf:Property ;
    rdfs:domain <http://rdaregistry.info/Elements/c/C10006> ;
    rdfs:isDefinedBy <http://rdaregistry.info/Elements/e/> ;
    rdfs:label "has sound content"@en ;
    skos:definition "Relates an expression to the presence of sound in a resource other than one that consists primarily of recorded sound."@en .

<http://rdaregistry.info/Elements/e/P20226>
    reg:hasUnconstrained <http://rdaregistry.info/Elements/u/P60563> ;
    reg:lexicalAlias <http://rdaregistry.info/Elements/e/horizontalScaleOfCartographicContent.en> ;
    reg:name "horizontalScaleOfCartographicContent"@en ;
    reg:status <http://metadataregistry.org/uri/RegStatus/1001> ;
    rdakit:instructionNumber "7.25.3" ;
    rdakit:toolkitDefinition "The ratio of horizontal distances in the cartographic content of a resource to the actual distances they represent."@en ;
    rdakit:toolkitLabel "horizontal scale of cartographic content"@en ;
    a rdf:Property ;
    rdfs:domain <http://rdaregistry.info/Elements/c/C10006> ;
    rdfs:isDefinedBy <http://rdaregistry.info/Elements/e/> ;
    rdfs:label "has horizontal scale of cartographic content"@en ;
    rdfs:subPropertyOf <http://rdaregistry.info/Elements/e/P20228> ;
    skos:definition "Relates an expression to the ratio of horizontal distances in the cartographic content of a resource to the actual distances they represent."@en .

<http://rdaregistry.info/Elements/e/P20227>
    reg:hasUnconstrained <http://rdaregistry.info/Elements/u/P60564> ;
    reg:lexicalAlias <http://rdaregistry.info/Elements/e/scaleOfStillImageOrThreeDimensionalForm.en> ;
    reg:name "scaleOfStillImageOrThreeDimensionalForm"@en ;
    reg:status <http://metadataregistry.org/uri/RegStatus/1001> ;
    rdakit:instructionNumber "7.25.2" ;
    rdakit:toolkitDefinition "The ratio of the dimensions of a still image or three-dimensional form contained or embodied in a resource to the dimensions of the thing it represents."@en ;
    rdakit:toolkitLabel "scale of still image or three-dimensional form"@en ;
    a rdf:Property ;
    rdfs:domain <http://rdaregistry.info/Elements/c/C10006> ;
    rdfs:isDefinedBy <http://rdaregistry.info/Elements/e/> ;
    rdfs:label "has scale of still image or three-dimensional form"@en ;
    rdfs:subPropertyOf <http://rdaregistry.info/Elements/e/P20228> ;
    skos:definition "Relates an expression to the ratio of the dimensions of a still image or three-dimensional form contained or embodied in a resource to the dimensions of the thing it represents."@en .

<http://rdaregistry.info/Elements/e/P20228>
    reg:hasSubproperty <http://rdaregistry.info/Elements/e/P20213>, <http://rdaregistry.info/Elements/e/P20226>, <http://rdaregistry.info/Elements/e/P20227>, <http://rdaregistry.info/Elements/e/P20230> ;
    reg:hasUnconstrained <http://rdaregistry.info/Elements/u/P60565> ;
    reg:lexicalAlias <http://rdaregistry.info/Elements/e/scale.en> ;
    reg:name "scale"@en ;
    reg:status <http://metadataregistry.org/uri/RegStatus/1001> ;
    rdakit:instructionNumber "7.25" ;
    rdakit:toolkitDefinition "The ratio of the dimensions of an image or three-dimensional form contained or embodied in a resource to the dimensions of the thing it represents."@en ;
    rdakit:toolkitLabel "scale"@en ;
    a rdf:Property ;
    rdfs:domain <http://rdaregistry.info/Elements/c/C10006> ;
    rdfs:isDefinedBy <http://rdaregistry.info/Elements/e/> ;
    rdfs:label "has scale"@en ;
    skos:definition "Relates an expression to the ratio of the dimensions of an image or three-dimensional form contained or embodied in a resource to the dimensions of the thing it represents."@en ;
    skos:scopeNote "Scale can apply to horizontal, vertical, angular, and/or other measurements represented in the resource."@en .

<http://rdaregistry.info/Elements/e/P20229>
    reg:hasUnconstrained <http://rdaregistry.info/Elements/u/P60566> ;
    reg:lexicalAlias <http://rdaregistry.info/Elements/e/aspectRatio.en> ;
    reg:name "aspectRatio"@en ;
    reg:status <http://metadataregistry.org/uri/RegStatus/1001> ;
    rdakit:instructionNumber "7.19" ;
    rdakit:toolkitDefinition "The ratio of the width to the height of a moving image."@en ;
    rdakit:toolkitLabel "aspect ratio"@en ;
    a rdf:Property ;
    rdfs:domain <http://rdaregistry.info/Elements/c/C10006> ;
    rdfs:isDefinedBy <http://rdaregistry.info/Elements/e/> ;
    rdfs:label "has aspect ratio"@en ;
    skos:definition "Relates an expression to the ratio of the width to the height of a moving image."@en .

<http://rdaregistry.info/Elements/e/P20230>
    reg:hasUnconstrained <http://rdaregistry.info/Elements/u/P60579> ;
    reg:lexicalAlias <http://rdaregistry.info/Elements/e/verticalScaleOfCartographicContent.en> ;
    reg:name "verticalScaleOfCartographicContent"@en ;
    reg:status <http://metadataregistry.org/uri/RegStatus/1001> ;
    rdakit:instructionNumber "7.25.4" ;
    rdakit:toolkitDefinition "The scale of elevation or vertical dimension of the cartographic content of a resource."@en ;
    rdakit:toolkitLabel "vertical scale of cartographic content"@en ;
    a rdf:Property ;
    rdfs:domain <http://rdaregistry.info/Elements/c/C10006> ;
    rdfs:isDefinedBy <http://rdaregistry.info/Elements/e/> ;
    rdfs:label "has vertical scale of cartographic content"@en ;
    rdfs:subPropertyOf <http://rdaregistry.info/Elements/e/P20228> ;
    skos:definition "Relates an expression to the scale of elevation or vertical dimension of the cartographic content of a resource."@en .

<http://rdaregistry.info/Elements/e/P20231>
    reg:lexicalAlias <http://rdaregistry.info/Elements/e/workExpressed.en> ;
    reg:name "workExpressed"@en ;
    reg:status <http://metadataregistry.org/uri/RegStatus/1001> ;
    rdakit:instructionNumber "17.6" ;
    rdakit:toolkitDefinition "The work realized through an expression."@en ;
    rdakit:toolkitLabel "work expressed"@en ;
    a rdf:Property ;
    rdfs:domain <http://rdaregistry.info/Elements/c/C10006> ;
    rdfs:isDefinedBy <http://rdaregistry.info/Elements/e/> ;
    rdfs:label "has work expressed"@en ;
    rdfs:range <http://rdaregistry.info/Elements/c/C10001> ;
    owl:inverseOf <http://rdaregistry.info/Elements/w/P10078> ;
    skos:definition "Relates an expression to the work realized through an expression."@en .

<http://rdaregistry.info/Elements/e/P20232>
    reg:hasSubproperty <http://rdaregistry.info/Elements/e/P20100>, <http://rdaregistry.info/Elements/e/P20105>, <http://rdaregistry.info/Elements/e/P20192> ;
    reg:hasUnconstrained <http://rdaregistry.info/Elements/u/P60709> ;
    reg:lexicalAlias <http://rdaregistry.info/Elements/e/accompanyingExpressionRelationship.en> ;
    reg:name "accompanyingExpressionRelationship"@en ;
    reg:status <http://metadataregistry.org/uri/RegStatus/1001> ;
    rdakit:toolkitDefinition "An expression of a work that is an augmentation of, or is augmented by, or is complemented by the expression."@en ;
    rdakit:toolkitLabel "accompanying expression relationship"@en ;
    a rdf:Property ;
    rdfs:domain <http://rdaregistry.info/Elements/c/C10006> ;
    rdfs:isDefinedBy <http://rdaregistry.info/Elements/e/> ;
    rdfs:label "has accompanying expression relationship with"@en ;
    rdfs:range <http://rdaregistry.info/Elements/c/C10006> ;
    rdfs:subPropertyOf <http://rdaregistry.info/Elements/e/P20205> ;
    owl:inverseOf <http://rdaregistry.info/Elements/e/P20232> ;
    skos:definition "Relates an expression to an expression of a work that is an augmentation of, or is augmented by, or is complemented by the expression."@en .

<http://rdaregistry.info/Elements/e/P20233>
    reg:hasSubproperty <http://rdaregistry.info/Elements/e/P20203> ;
    reg:hasUnconstrained <http://rdaregistry.info/Elements/u/P60710> ;
    reg:lexicalAlias <http://rdaregistry.info/Elements/e/derivativeExpressionRelationship.en> ;
    reg:name "derivativeExpressionRelationship"@en ;
    reg:status <http://metadataregistry.org/uri/RegStatus/1001> ;
    rdakit:toolkitDefinition "An expression of a work that is based on or is a derivative of the expression."@en ;
    rdakit:toolkitLabel "derivative expression relationship"@en ;
    a rdf:Property ;
    rdfs:domain <http://rdaregistry.info/Elements/c/C10006> ;
    rdfs:isDefinedBy <http://rdaregistry.info/Elements/e/> ;
    rdfs:label "has derivative expression relationship with"@en ;
    rdfs:range <http://rdaregistry.info/Elements/c/C10006> ;
    rdfs:subPropertyOf <http://rdaregistry.info/Elements/e/P20205> ;
    owl:inverseOf <http://rdaregistry.info/Elements/e/P20233> ;
    skos:definition "Relates an expression to an expression of a work that is based on or is a derivative of the expression."@en .

<http://rdaregistry.info/Elements/e/P20234>
    reg:status <http://metadataregistry.org/uri/RegStatus/1008> ;
    a rdf:Property ;
    rdfs:isDefinedBy <http://rdaregistry.info/Elements/e/> .

<http://rdaregistry.info/Elements/e/P20235>
    reg:hasSubproperty <http://rdaregistry.info/Elements/e/P20154>, <http://rdaregistry.info/Elements/e/P20169> ;
    reg:hasUnconstrained <http://rdaregistry.info/Elements/u/P60713> ;
    reg:lexicalAlias <http://rdaregistry.info/Elements/e/sequentialExpressionRelationship.en> ;
    reg:name "sequentialExpressionRelationship"@en ;
    reg:status <http://metadataregistry.org/uri/RegStatus/1001> ;
    rdakit:toolkitDefinition "An expression of a work that is preceded by or succeeded by the expression."@en ;
    rdakit:toolkitLabel "sequential expression relationship"@en ;
    a rdf:Property ;
    rdfs:domain <http://rdaregistry.info/Elements/c/C10006> ;
    rdfs:isDefinedBy <http://rdaregistry.info/Elements/e/> ;
    rdfs:label "has sequential expression relationship with"@en ;
    rdfs:range <http://rdaregistry.info/Elements/c/C10006> ;
    rdfs:subPropertyOf <http://rdaregistry.info/Elements/e/P20205> ;
    skos:definition "Relates an expression to an expression of a work that is preceded by or succeeded by the expression."@en .

<http://rdaregistry.info/Elements/e/P20236>
    reg:hasSubproperty <http://rdaregistry.info/Elements/e/P20074>, <http://rdaregistry.info/Elements/e/P20145> ;
    reg:hasUnconstrained <http://rdaregistry.info/Elements/u/P60714> ;
    reg:lexicalAlias <http://rdaregistry.info/Elements/e/wholePartExpressionRelationship.en> ;
    reg:name "wholePartExpressionRelationship"@en ;
    reg:status <http://metadataregistry.org/uri/RegStatus/1001> ;
    rdakit:toolkitDefinition "An expression that is contained in or contains the expression."@en ;
    rdakit:toolkitLabel "whole-part expression relationship"@en ;
    a rdf:Property ;
    rdfs:domain <http://rdaregistry.info/Elements/c/C10006> ;
    rdfs:isDefinedBy <http://rdaregistry.info/Elements/e/> ;
    rdfs:label "has whole-part expression relationship with"@en ;
    rdfs:range <http://rdaregistry.info/Elements/c/C10006> ;
    rdfs:subPropertyOf <http://rdaregistry.info/Elements/e/P20205> ;
    skos:definition "Relates an expression to an expression that is contained in or contains the expression."@en .

<http://rdaregistry.info/Elements/e/P20237>
    reg:hasUnconstrained <http://rdaregistry.info/Elements/u/P60715> ;
    reg:lexicalAlias <http://rdaregistry.info/Elements/e/writerOfAfterword.en> ;
    reg:name "writerOfAfterword"@en ;
    reg:status <http://metadataregistry.org/uri/RegStatus/1001> ;
    rdakit:toolkitDefinition "A person, family, or corporate body contributing to an expression of a work by providing an afterword to the original work."@en ;
    rdakit:toolkitLabel "writer of afterword"@en ;
    a rdf:Property ;
    rdfs:domain <http://rdaregistry.info/Elements/c/C10006> ;
    rdfs:isDefinedBy <http://rdaregistry.info/Elements/e/> ;
    rdfs:label "has writer of afterword"@en ;
    rdfs:range <http://rdaregistry.info/Elements/c/C10002> ;
    rdfs:subPropertyOf <http://rdaregistry.info/Elements/e/P20046> ;
    owl:inverseOf <http://rdaregistry.info/Elements/a/P50227> ;
    skos:definition "Relates an expression to a person, family, or corporate body contributing to an expression of a work by providing an afterword to the original work."@en .

<http://rdaregistry.info/Elements/e/P20238>
    reg:hasUnconstrained <http://rdaregistry.info/Elements/u/P60716> ;
    reg:lexicalAlias <http://rdaregistry.info/Elements/e/writerOfPostface.en> ;
    reg:name "writerOfPostface"@en ;
    reg:status <http://metadataregistry.org/uri/RegStatus/1001> ;
    rdakit:toolkitDefinition "A person, family, or corporate body contributing to an expression of a work by providing a postface to the original work."@en ;
    rdakit:toolkitLabel "writer of postface"@en ;
    a rdf:Property ;
    rdfs:domain <http://rdaregistry.info/Elements/c/C10006> ;
    rdfs:isDefinedBy <http://rdaregistry.info/Elements/e/> ;
    rdfs:label "has writer of postface"@en ;
    rdfs:range <http://rdaregistry.info/Elements/c/C10002> ;
    rdfs:subPropertyOf <http://rdaregistry.info/Elements/e/P20046> ;
    owl:inverseOf <http://rdaregistry.info/Elements/a/P50228> ;
    skos:definition "Relates an expression to a person, family, or corporate body contributing to an expression of a work by providing a postface to the original work."@en .

<http://rdaregistry.info/Elements/e/P20239>
    reg:hasUnconstrained <http://rdaregistry.info/Elements/u/P60719> ;
    reg:lexicalAlias <http://rdaregistry.info/Elements/e/musicalTheatreAdaptationOfExpression.en> ;
    reg:name "musicalTheatreAdaptationOfExpression"@en ;
    reg:status <http://metadataregistry.org/uri/RegStatus/1001> ;
    rdakit:toolkitDefinition "An expression of a work that has been adapted as a musical theatre work."@en ;
    rdakit:toolkitLabel "musical theatre adaptation of (expression)"@en ;
    a rdf:Property ;
    rdfs:domain <http://rdaregistry.info/Elements/c/C10006> ;
    rdfs:isDefinedBy <http://rdaregistry.info/Elements/e/> ;
    rdfs:label "is musical theatre adaptation of (expression)"@en ;
    rdfs:range <http://rdaregistry.info/Elements/c/C10006> ;
    rdfs:subPropertyOf <http://rdaregistry.info/Elements/e/P20152> ;
    owl:inverseOf <http://rdaregistry.info/Elements/e/P20241> ;
    skos:definition "Relates an expression to an expression of a work that has been adapted as a musical theatre work."@en .

<http://rdaregistry.info/Elements/e/P20240>
    reg:hasUnconstrained <http://rdaregistry.info/Elements/u/P60720> ;
    reg:lexicalAlias <http://rdaregistry.info/Elements/e/operaAdaptationOfExpression.en> ;
    reg:name "operaAdaptationOfExpression"@en ;
    reg:status <http://metadataregistry.org/uri/RegStatus/1001> ;
    rdakit:toolkitDefinition "An expression of a work that has been adapted as an opera."@en ;
    rdakit:toolkitLabel "opera adaptation of (expression)"@en ;
    a rdf:Property ;
    rdfs:domain <http://rdaregistry.info/Elements/c/C10006> ;
    rdfs:isDefinedBy <http://rdaregistry.info/Elements/e/> ;
    rdfs:label "is opera adaptation of (expression)"@en ;
    rdfs:range <http://rdaregistry.info/Elements/c/C10006> ;
    rdfs:subPropertyOf <http://rdaregistry.info/Elements/e/P20152> ;
    owl:inverseOf <http://rdaregistry.info/Elements/e/P20242> ;
    skos:definition "Relates an expression to an expression of a work that has been adapted as an opera."@en .

<http://rdaregistry.info/Elements/e/P20241>
    reg:hasUnconstrained <http://rdaregistry.info/Elements/u/P60721> ;
    reg:lexicalAlias <http://rdaregistry.info/Elements/e/adaptedAsMusicalTheatreExpression.en> ;
    reg:name "adaptedAsMusicalTheatreExpression"@en ;
    reg:status <http://metadataregistry.org/uri/RegStatus/1001> ;
    rdakit:toolkitDefinition "An expression of a musical theatre work based on the source expression."@en ;
    rdakit:toolkitLabel "adapted as musical theatre (expression)"@en ;
    a rdf:Property ;
    rdfs:domain <http://rdaregistry.info/Elements/c/C10006> ;
    rdfs:isDefinedBy <http://rdaregistry.info/Elements/e/> ;
    rdfs:label "is adapted as musical theatre (expression)"@en ;
    rdfs:range <http://rdaregistry.info/Elements/c/C10006> ;
    rdfs:subPropertyOf <http://rdaregistry.info/Elements/e/P20153> ;
    owl:inverseOf <http://rdaregistry.info/Elements/e/P20239> ;
    skos:definition "Relates an expression to an expression of a musical theatre work based on the source expression."@en .

<http://rdaregistry.info/Elements/e/P20242>
    reg:hasUnconstrained <http://rdaregistry.info/Elements/u/P60722> ;
    reg:lexicalAlias <http://rdaregistry.info/Elements/e/adaptedAsOperaExpression.en> ;
    reg:name "adaptedAsOperaExpression"@en ;
    reg:status <http://metadataregistry.org/uri/RegStatus/1001> ;
    rdakit:toolkitDefinition "An expression of an opera based on the source expression."@en ;
    rdakit:toolkitLabel "adapted as opera (expression)"@en ;
    a rdf:Property ;
    rdfs:domain <http://rdaregistry.info/Elements/c/C10006> ;
    rdfs:isDefinedBy <http://rdaregistry.info/Elements/e/> ;
    rdfs:label "is adapted as opera (expression)"@en ;
    rdfs:range <http://rdaregistry.info/Elements/c/C10006> ;
    rdfs:subPropertyOf <http://rdaregistry.info/Elements/e/P20153> ;
    owl:inverseOf <http://rdaregistry.info/Elements/e/P20240> ;
    skos:definition "Relates an expression to an expression of an opera based on the source expression."@en .

<http://rdaregistry.info/Elements/e/P20243>
    reg:hasSubproperty <http://rdaregistry.info/Elements/e/P20085> ;
    reg:hasUnconstrained <http://rdaregistry.info/Elements/u/P60723> ;
    reg:lexicalAlias <http://rdaregistry.info/Elements/e/musicExpression.en> ;
    reg:name "musicExpression"@en ;
    reg:status <http://metadataregistry.org/uri/RegStatus/1001> ;
    rdakit:toolkitDefinition "An expression of a musical work that is used in a motion picture, play, television program, etc."@en ;
    rdakit:toolkitLabel "music (expression)"@en ;
    a rdf:Property ;
    rdfs:domain <http://rdaregistry.info/Elements/c/C10006> ;
    rdfs:isDefinedBy <http://rdaregistry.info/Elements/e/> ;
    rdfs:label "is music (expression)"@en ;
    rdfs:range <http://rdaregistry.info/Elements/c/C10006> ;
    rdfs:subPropertyOf <http://rdaregistry.info/Elements/e/P20100> ;
    owl:inverseOf <http://rdaregistry.info/Elements/e/P20244> ;
    skos:definition "Relates an expression to an expression of a musical work that is used in a motion picture, play, television program, etc."@en .

<http://rdaregistry.info/Elements/e/P20244>
    reg:hasSubproperty <http://rdaregistry.info/Elements/e/P20103> ;
    reg:hasUnconstrained <http://rdaregistry.info/Elements/u/P60724> ;
    reg:lexicalAlias <http://rdaregistry.info/Elements/e/musicForExpression.en> ;
    reg:name "musicForExpression"@en ;
    reg:status <http://metadataregistry.org/uri/RegStatus/1001> ;
    rdakit:toolkitDefinition "An expression of a work such as a motion picture, play, television program, etc. that uses the musical work."@en ;
    rdakit:toolkitLabel "music for (expression)"@en ;
    a rdf:Property ;
    rdfs:domain <http://rdaregistry.info/Elements/c/C10006> ;
    rdfs:isDefinedBy <http://rdaregistry.info/Elements/e/> ;
    rdfs:label "is music for (expression)"@en ;
    rdfs:range <http://rdaregistry.info/Elements/c/C10006> ;
    rdfs:subPropertyOf <http://rdaregistry.info/Elements/e/P20100> ;
    owl:inverseOf <http://rdaregistry.info/Elements/e/P20243> ;
    skos:definition "Relates an expression to an expression of a work such as a motion picture, play, television program, etc. that uses the musical work."@en .

<http://rdaregistry.info/Elements/e/P20245>
    reg:hasUnconstrained <http://rdaregistry.info/Elements/u/P60725> ;
    reg:lexicalAlias <http://rdaregistry.info/Elements/e/videoMusicExpression.en> ;
    reg:name "videoMusicExpression"@en ;
    reg:status <http://metadataregistry.org/uri/RegStatus/1001> ;
    rdakit:toolkitDefinition "An expression of a musical work that is used in a video."@en ;
    rdakit:toolkitLabel "video music (expression)"@en ;
    a rdf:Property ;
    rdfs:domain <http://rdaregistry.info/Elements/c/C10006> ;
    rdfs:isDefinedBy <http://rdaregistry.info/Elements/e/> ;
    rdfs:label "is video music (expression)"@en ;
    rdfs:range <http://rdaregistry.info/Elements/c/C10006> ;
    rdfs:subPropertyOf <http://rdaregistry.info/Elements/e/P20243> ;
    owl:inverseOf <http://rdaregistry.info/Elements/e/P20246> ;
    skos:definition "Relates an expression to an expression of a musical work that is used in a video."@en .

<http://rdaregistry.info/Elements/e/P20246>
    reg:hasUnconstrained <http://rdaregistry.info/Elements/u/P60726> ;
    reg:lexicalAlias <http://rdaregistry.info/Elements/e/musicForVideoExpression.en> ;
    reg:name "musicForVideoExpression"@en ;
    reg:status <http://metadataregistry.org/uri/RegStatus/1001> ;
    rdakit:toolkitDefinition "An expression of a work that uses the musical work in a video."@en ;
    rdakit:toolkitLabel "music for video (expression)"@en ;
    a rdf:Property ;
    rdfs:domain <http://rdaregistry.info/Elements/c/C10006> ;
    rdfs:isDefinedBy <http://rdaregistry.info/Elements/e/> ;
    rdfs:label "is music for video (expression)"@en ;
    rdfs:range <http://rdaregistry.info/Elements/c/C10006> ;
    rdfs:subPropertyOf <http://rdaregistry.info/Elements/e/P20244> ;
    owl:inverseOf <http://rdaregistry.info/Elements/e/P20245> ;
    skos:definition "Relates an expression to an expression of a work that uses the musical work in a video."@en .

<http://rdaregistry.info/Elements/e/P20247>
    reg:hasUnconstrained <http://rdaregistry.info/Elements/u/P60727> ;
    reg:lexicalAlias <http://rdaregistry.info/Elements/e/televisionProgramMusicExpression.en> ;
    reg:name "televisionProgramMusicExpression"@en ;
    reg:status <http://metadataregistry.org/uri/RegStatus/1001> ;
    rdakit:toolkitDefinition "An expression of a musical work that is used in a television program."@en ;
    rdakit:toolkitLabel "television program music (expression)"@en ;
    a rdf:Property ;
    rdfs:domain <http://rdaregistry.info/Elements/c/C10006> ;
    rdfs:isDefinedBy <http://rdaregistry.info/Elements/e/> ;
    rdfs:label "is television program music (expression)"@en ;
    rdfs:range <http://rdaregistry.info/Elements/c/C10006> ;
    rdfs:subPropertyOf <http://rdaregistry.info/Elements/e/P20243> ;
    owl:inverseOf <http://rdaregistry.info/Elements/e/P20248> ;
    skos:definition "Relates an expression to an expression of a musical work that is used in a television program."@en .

<http://rdaregistry.info/Elements/e/P20248>
    reg:hasUnconstrained <http://rdaregistry.info/Elements/u/P60728> ;
    reg:lexicalAlias <http://rdaregistry.info/Elements/e/musicForTelevisionProgramExpression.en> ;
    reg:name "musicForTelevisionProgramExpression"@en ;
    reg:status <http://metadataregistry.org/uri/RegStatus/1001> ;
    rdakit:toolkitDefinition "An expression of a work that uses the musical work in a television program."@en ;
    rdakit:toolkitLabel "music for television program (expression)"@en ;
    a rdf:Property ;
    rdfs:domain <http://rdaregistry.info/Elements/c/C10006> ;
    rdfs:isDefinedBy <http://rdaregistry.info/Elements/e/> ;
    rdfs:label "is music for television program (expression)"@en ;
    rdfs:range <http://rdaregistry.info/Elements/c/C10006> ;
    rdfs:subPropertyOf <http://rdaregistry.info/Elements/e/P20244> ;
    owl:inverseOf <http://rdaregistry.info/Elements/e/P20247> ;
    skos:definition "Relates an expression to an expression of a work that uses the musical work in a television program."@en .

<http://rdaregistry.info/Elements/e/P20249>
    reg:hasUnconstrained <http://rdaregistry.info/Elements/u/P60729> ;
    reg:lexicalAlias <http://rdaregistry.info/Elements/e/radioProgramMusicExpression.en> ;
    reg:name "radioProgramMusicExpression"@en ;
    reg:status <http://metadataregistry.org/uri/RegStatus/1001> ;
    rdakit:toolkitDefinition "An expression of a musical work that is used in a radio program."@en ;
    rdakit:toolkitLabel "radio program music (expression)"@en ;
    a rdf:Property ;
    rdfs:domain <http://rdaregistry.info/Elements/c/C10006> ;
    rdfs:isDefinedBy <http://rdaregistry.info/Elements/e/> ;
    rdfs:label "is radio program music (expression)"@en ;
    rdfs:range <http://rdaregistry.info/Elements/c/C10006> ;
    rdfs:subPropertyOf <http://rdaregistry.info/Elements/e/P20243> ;
    owl:inverseOf <http://rdaregistry.info/Elements/e/P20250> ;
    skos:definition "Relates an expression to an expression of a musical work that is used in a radio program."@en .

<http://rdaregistry.info/Elements/e/P20250>
    reg:hasUnconstrained <http://rdaregistry.info/Elements/u/P60730> ;
    reg:lexicalAlias <http://rdaregistry.info/Elements/e/musicForRadioProgramExpression.en> ;
    reg:name "musicForRadioProgramExpression"@en ;
    reg:status <http://metadataregistry.org/uri/RegStatus/1001> ;
    rdakit:toolkitDefinition "An expression of a work that uses the musical work in a radio program."@en ;
    rdakit:toolkitLabel "music for radio program (expression)"@en ;
    a rdf:Property ;
    rdfs:domain <http://rdaregistry.info/Elements/c/C10006> ;
    rdfs:isDefinedBy <http://rdaregistry.info/Elements/e/> ;
    rdfs:label "is music for radio program (expression)"@en ;
    rdfs:range <http://rdaregistry.info/Elements/c/C10006> ;
    rdfs:subPropertyOf <http://rdaregistry.info/Elements/e/P20244> ;
    owl:inverseOf <http://rdaregistry.info/Elements/e/P20249> ;
    skos:definition "Relates an expression to an expression of a work that uses the musical work in a radio program."@en .

<http://rdaregistry.info/Elements/e/P20251>
    reg:hasUnconstrained <http://rdaregistry.info/Elements/u/P60731> ;
    reg:lexicalAlias <http://rdaregistry.info/Elements/e/motionPictureMusicExpression.en> ;
    reg:name "motionPictureMusicExpression"@en ;
    reg:status <http://metadataregistry.org/uri/RegStatus/1001> ;
    rdakit:toolkitDefinition "An expression of a musical work that is used in a motion picture."@en ;
    rdakit:toolkitLabel "motion picture music (expression)"@en ;
    a rdf:Property ;
    rdfs:domain <http://rdaregistry.info/Elements/c/C10006> ;
    rdfs:isDefinedBy <http://rdaregistry.info/Elements/e/> ;
    rdfs:label "is motion picture music (expression)"@en ;
    rdfs:range <http://rdaregistry.info/Elements/c/C10006> ;
    rdfs:subPropertyOf <http://rdaregistry.info/Elements/e/P20243> ;
    owl:inverseOf <http://rdaregistry.info/Elements/e/P20252> ;
    skos:definition "Relates an expression to an expression of a musical work that is used in a motion picture."@en .

<http://rdaregistry.info/Elements/e/P20252>
    reg:hasUnconstrained <http://rdaregistry.info/Elements/u/P60732> ;
    reg:lexicalAlias <http://rdaregistry.info/Elements/e/musicForMotionPictureExpression.en> ;
    reg:name "musicForMotionPictureExpression"@en ;
    reg:status <http://metadataregistry.org/uri/RegStatus/1001> ;
    rdakit:toolkitDefinition "An expression of a work that uses the musical work in a motion picture."@en ;
    rdakit:toolkitLabel "music for motion picture (expression)"@en ;
    a rdf:Property ;
    rdfs:domain <http://rdaregistry.info/Elements/c/C10006> ;
    rdfs:isDefinedBy <http://rdaregistry.info/Elements/e/> ;
    rdfs:label "is music for motion picture (expression)"@en ;
    rdfs:range <http://rdaregistry.info/Elements/c/C10006> ;
    rdfs:subPropertyOf <http://rdaregistry.info/Elements/e/P20244> ;
    owl:inverseOf <http://rdaregistry.info/Elements/e/P20251> ;
    skos:definition "Relates an expression to an expression of a work that uses the musical work in a motion picture."@en .

<http://rdaregistry.info/Elements/e/P20253>
    reg:hasUnconstrained <http://rdaregistry.info/Elements/u/P60740> ;
    reg:lexicalAlias <http://rdaregistry.info/Elements/e/choreographyExpression.en> ;
    reg:name "choreographyExpression"@en ;
    reg:status <http://metadataregistry.org/uri/RegStatus/1001> ;
    rdakit:toolkitDefinition "An expression of a work that provides the choreography for use in the related expression."@en ;
    rdakit:toolkitLabel "choreography (expression)"@en ;
    a rdf:Property ;
    rdfs:domain <http://rdaregistry.info/Elements/c/C10006> ;
    rdfs:isDefinedBy <http://rdaregistry.info/Elements/e/> ;
    rdfs:label "is choreography (expression)"@en ;
    rdfs:range <http://rdaregistry.info/Elements/c/C10006> ;
    rdfs:subPropertyOf <http://rdaregistry.info/Elements/e/P20100> ;
    owl:inverseOf <http://rdaregistry.info/Elements/e/P20254> ;
    skos:definition "Relates an expression to an expression of a work that provides the choreography for use in the related expression."@en .

<http://rdaregistry.info/Elements/e/P20254>
    reg:hasUnconstrained <http://rdaregistry.info/Elements/u/P60741> ;
    reg:lexicalAlias <http://rdaregistry.info/Elements/e/choreographyForExpression.en> ;
    reg:name "choreographyForExpression"@en ;
    reg:status <http://metadataregistry.org/uri/RegStatus/1001> ;
    rdakit:toolkitDefinition "An expression of a work that uses the choreography of the related expression."@en ;
    rdakit:toolkitLabel "choreography for (expression)"@en ;
    a rdf:Property ;
    rdfs:domain <http://rdaregistry.info/Elements/c/C10006> ;
    rdfs:isDefinedBy <http://rdaregistry.info/Elements/e/> ;
    rdfs:label "is choreography for (expression)"@en ;
    rdfs:range <http://rdaregistry.info/Elements/c/C10006> ;
    rdfs:subPropertyOf <http://rdaregistry.info/Elements/e/P20100> ;
    owl:inverseOf <http://rdaregistry.info/Elements/e/P20253> ;
    skos:definition "Relates an expression to an expression of a work that uses the choreography of the related expression."@en .

<http://rdaregistry.info/Elements/e/P20255>
    reg:hasUnconstrained <http://rdaregistry.info/Elements/u/P60742> ;
    reg:lexicalAlias <http://rdaregistry.info/Elements/e/adaptedAsGraphicNovelExpression.en> ;
    reg:name "adaptedAsGraphicNovelExpression"@en ;
    reg:status <http://metadataregistry.org/uri/RegStatus/1001> ;
    rdakit:toolkitDefinition "A graphic novel based on the source expression."@en ;
    rdakit:toolkitLabel "adapted as graphic novel (expression)"@en ;
    a rdf:Property ;
    rdfs:domain <http://rdaregistry.info/Elements/c/C10006> ;
    rdfs:isDefinedBy <http://rdaregistry.info/Elements/e/> ;
    rdfs:label "is adapted as graphic novel (expression)"@en ;
    rdfs:range <http://rdaregistry.info/Elements/c/C10006> ;
    rdfs:subPropertyOf <http://rdaregistry.info/Elements/e/P20153> ;
    owl:inverseOf <http://rdaregistry.info/Elements/e/P20256> ;
    skos:definition "Relates an expression to a graphic novel based on the source expression."@en .

<http://rdaregistry.info/Elements/e/P20256>
    reg:hasUnconstrained <http://rdaregistry.info/Elements/u/P60743> ;
    reg:lexicalAlias <http://rdaregistry.info/Elements/e/graphicNovelizationOfExpression.en> ;
    reg:name "graphicNovelizationOfExpression"@en ;
    reg:status <http://metadataregistry.org/uri/RegStatus/1001> ;
    rdakit:toolkitDefinition "An expression of a work that has been adapated as a graphic novel."@en ;
    rdakit:toolkitLabel "graphic novelization of (expression)"@en ;
    a rdf:Property ;
    rdfs:domain <http://rdaregistry.info/Elements/c/C10006> ;
    rdfs:isDefinedBy <http://rdaregistry.info/Elements/e/> ;
    rdfs:label "is graphic novelization of (expression)"@en ;
    rdfs:range <http://rdaregistry.info/Elements/c/C10006> ;
    rdfs:subPropertyOf <http://rdaregistry.info/Elements/e/P20152> ;
    owl:inverseOf <http://rdaregistry.info/Elements/e/P20255> ;
    skos:definition "Relates an expression to an expression of a work that has been adapated as a graphic novel."@en .

<http://rdaregistry.info/Elements/e/P20257>
    reg:hasUnconstrained <http://rdaregistry.info/Elements/u/P60748> ;
    reg:lexicalAlias <http://rdaregistry.info/Elements/e/visualEffectsProvider.en> ;
    reg:name "visualEffectsProvider"@en ;
    reg:status <http://metadataregistry.org/uri/RegStatus/1001> ;
    rdakit:toolkitDefinition "A person, family, or corporate body contributing to an expression of a moving image work by designing and creating post-production visual effects."@en ;
    rdakit:toolkitLabel "visual effects provider"@en ;
    a rdf:Property ;
    rdfs:domain <http://rdaregistry.info/Elements/c/C10006> ;
    rdfs:isDefinedBy <http://rdaregistry.info/Elements/e/> ;
    rdfs:label "has visual effects provider"@en ;
    rdfs:range <http://rdaregistry.info/Elements/c/C10002> ;
    rdfs:subPropertyOf <http://rdaregistry.info/Elements/e/P20053> ;
    owl:inverseOf <http://rdaregistry.info/Elements/a/P50243> ;
    skos:definition "Relates an expression to a person, family, or corporate body contributing to an expression of a moving image work by designing and creating post-production visual effects."@en .

<http://rdaregistry.info/Elements/e/P20258>
    reg:hasUnconstrained <http://rdaregistry.info/Elements/u/P60749> ;
    reg:lexicalAlias <http://rdaregistry.info/Elements/e/specialEffectsProvider.en> ;
    reg:name "specialEffectsProvider"@en ;
    reg:status <http://metadataregistry.org/uri/RegStatus/1001> ;
    rdakit:toolkitDefinition "A person, family, or corporate body contributing to an expression of a moving image or audio work by designing and creating on-set special effects (on-set mechanical effects and in-camera optical effects)."@en ;
    rdakit:toolkitLabel "special effects provider"@en ;
    a rdf:Property ;
    rdfs:domain <http://rdaregistry.info/Elements/c/C10006> ;
    rdfs:isDefinedBy <http://rdaregistry.info/Elements/e/> ;
    rdfs:label "has special effects provider"@en ;
    rdfs:range <http://rdaregistry.info/Elements/c/C10002> ;
    rdfs:subPropertyOf <http://rdaregistry.info/Elements/e/P20053> ;
    owl:inverseOf <http://rdaregistry.info/Elements/a/P50244> ;
    skos:definition "Relates an expression to a person, family, or corporate body contributing to an expression of a moving image or audio work by designing and creating on-set special effects (on-set mechanical effects and in-camera optical effects)."@en .

<http://rdaregistry.info/Elements/e/P20259>
    reg:hasUnconstrained <http://rdaregistry.info/Elements/u/P60750> ;
    reg:lexicalAlias <http://rdaregistry.info/Elements/e/letterer.en> ;
    reg:name "letterer"@en ;
    reg:status <http://metadataregistry.org/uri/RegStatus/1001> ;
    rdakit:toolkitDefinition "An illustrator contributing to an expression of a comic book, graphic novel, etc., by drawing the text and graphic sound effects."@en ;
    rdakit:toolkitLabel "letterer"@en ;
    a rdf:Property ;
    rdfs:domain <http://rdaregistry.info/Elements/c/C10006> ;
    rdfs:isDefinedBy <http://rdaregistry.info/Elements/e/> ;
    rdfs:label "has letterer"@en ;
    rdfs:range <http://rdaregistry.info/Elements/c/C10002> ;
    rdfs:subPropertyOf <http://rdaregistry.info/Elements/e/P20051> ;
    owl:inverseOf <http://rdaregistry.info/Elements/a/P50245> ;
    skos:definition "Relates an expression to an illustrator contributing to an expression of a comic book, graphic novel, etc., by drawing the text and graphic sound effects."@en .

<http://rdaregistry.info/Elements/e/P20260>
    reg:hasUnconstrained <http://rdaregistry.info/Elements/u/P60760> ;
    reg:lexicalAlias <http://rdaregistry.info/Elements/e/detailsOfAspectRatio.en> ;
    reg:name "detailsOfAspectRatio"@en ;
    reg:status <http://metadataregistry.org/uri/RegStatus/1001> ;
    rdakit:instructionNumber "7.19.1.4" ;
    rdakit:toolkitDefinition "Details of the ratio of the width to the height of a moving image."@en ;
    rdakit:toolkitLabel "details of aspect ratio"@en ;
    a rdf:Property ;
    rdfs:domain <http://rdaregistry.info/Elements/c/C10006> ;
    rdfs:isDefinedBy <http://rdaregistry.info/Elements/e/> ;
    rdfs:label "has details of aspect ratio"@en ;
    skos:definition "Relates an expression to details of the ratio of the width to the height of a moving image."@en .

<http://rdaregistry.info/Elements/e/P20261>
    reg:hasUnconstrained <http://rdaregistry.info/Elements/u/P60761> ;
    reg:lexicalAlias <http://rdaregistry.info/Elements/e/detailsOfColourContent.en> ;
    reg:name "detailsOfColourContent"@en ;
    reg:status <http://metadataregistry.org/uri/RegStatus/1001> ;
    rdakit:instructionNumber "7.17.1.4" ;
    rdakit:toolkitDefinition "Details of the presence of colour, tone, etc., in the content of a resource, and the specific colours, tones, etc., (including black and white) present."@en ;
    rdakit:toolkitLabel "details of colour content"@en ;
    a rdf:Property ;
    rdfs:domain <http://rdaregistry.info/Elements/c/C10006> ;
    rdfs:isDefinedBy <http://rdaregistry.info/Elements/e/> ;
    rdfs:label "has details of colour content"@en ;
    skos:altLabel "has details of color content"@en ;
    skos:definition "Relates an expression to details of the presence of colour, tone, etc., in the content of a resource, and the specific colours, tones, etc., (including black and white) present."@en .

<http://rdaregistry.info/Elements/e/P20262>
    reg:hasUnconstrained <http://rdaregistry.info/Elements/u/P60762> ;
    reg:lexicalAlias <http://rdaregistry.info/Elements/e/detailsOfFormOfMusicalNotation.en> ;
    reg:name "detailsOfFormOfMusicalNotation"@en ;
    reg:status <http://metadataregistry.org/uri/RegStatus/1001> ;
    rdakit:instructionNumber "7.13.3.4" ;
    rdakit:toolkitDefinition "Details of the set of characters and/or symbols used to express the musical content of a resource."@en ;
    rdakit:toolkitLabel "details of form of musical notation"@en ;
    a rdf:Property ;
    rdfs:domain <http://rdaregistry.info/Elements/c/C10006> ;
    rdfs:isDefinedBy <http://rdaregistry.info/Elements/e/> ;
    rdfs:label "has details of form of musical notation"@en ;
    skos:definition "Relates an expression to details of the set of characters and/or symbols used to express the musical content of a resource."@en .

<http://rdaregistry.info/Elements/e/P20263>
    reg:hasUnconstrained <http://rdaregistry.info/Elements/u/P60763> ;
    reg:lexicalAlias <http://rdaregistry.info/Elements/e/detailsOfFormOfNotatedMovement.en> ;
    reg:name "detailsOfFormOfNotatedMovement"@en ;
    reg:status <http://metadataregistry.org/uri/RegStatus/1001> ;
    rdakit:instructionNumber "7.13.5.4" ;
    rdakit:toolkitDefinition "Details of the set of characters and/or symbols used to express the movement content of a resource."@en ;
    rdakit:toolkitLabel "details of form of notated movement"@en ;
    a rdf:Property ;
    rdfs:domain <http://rdaregistry.info/Elements/c/C10006> ;
    rdfs:isDefinedBy <http://rdaregistry.info/Elements/e/> ;
    rdfs:label "has details of form of notated movement"@en ;
    skos:definition "Relates an expression to details of the set of characters and/or symbols used to express the movement content of a resource."@en .

<http://rdaregistry.info/Elements/e/P20264>
    reg:hasUnconstrained <http://rdaregistry.info/Elements/u/P60764> ;
    reg:lexicalAlias <http://rdaregistry.info/Elements/e/detailsOfFormatOfNotatedMusic.en> ;
    reg:name "detailsOfFormatOfNotatedMusic"@en ;
    reg:status <http://metadataregistry.org/uri/RegStatus/1001> ;
    rdakit:instructionNumber "7.20.1.4" ;
    rdakit:toolkitDefinition "Details of the musical or physical layout of the content of a resource that is presented in the form of musical notation."@en ;
    rdakit:toolkitLabel "details of format of notated music"@en ;
    a rdf:Property ;
    rdfs:domain <http://rdaregistry.info/Elements/c/C10006> ;
    rdfs:isDefinedBy <http://rdaregistry.info/Elements/e/> ;
    rdfs:label "has details of format of notated music"@en ;
    skos:definition "Relates an expression to details of the musical or physical layout of the content of a resource that is presented in the form of musical notation."@en .

<http://rdaregistry.info/Elements/e/P20265>
    reg:hasUnconstrained <http://rdaregistry.info/Elements/u/P60765> ;
    reg:lexicalAlias <http://rdaregistry.info/Elements/e/detailsOfFormOfTactileNotation.en> ;
    reg:name "detailsOfFormOfTactileNotation"@en ;
    reg:status <http://metadataregistry.org/uri/RegStatus/1001> ;
    rdakit:instructionNumber "7.13.4.4" ;
    rdakit:toolkitDefinition "Details of the set of characters and/or symbols used to express the content of a resource in a form that can be perceived through touch."@en ;
    rdakit:toolkitLabel "details of form of tactile notation"@en ;
    a rdf:Property ;
    rdfs:domain <http://rdaregistry.info/Elements/c/C10006> ;
    rdfs:isDefinedBy <http://rdaregistry.info/Elements/e/> ;
    rdfs:label "has details of form of tactile notation"@en ;
    skos:definition "Relates an expression to details of the set of characters and/or symbols used to express the content of a resource in a form that can be perceived through touch."@en .

<http://rdaregistry.info/Elements/e/P20266>
    reg:hasUnconstrained <http://rdaregistry.info/Elements/u/P60766> ;
    reg:lexicalAlias <http://rdaregistry.info/Elements/e/detailsOfScript.en> ;
    reg:name "detailsOfScript"@en ;
    reg:status <http://metadataregistry.org/uri/RegStatus/1001> ;
    rdakit:instructionNumber "7.13.2.4" ;
    rdakit:toolkitDefinition "Details of the set of characters and/or symbols used to express the written language content of a resource."@en ;
    rdakit:toolkitLabel "details of script"@en ;
    a rdf:Property ;
    rdfs:domain <http://rdaregistry.info/Elements/c/C10006> ;
    rdfs:isDefinedBy <http://rdaregistry.info/Elements/e/> ;
    rdfs:label "has details of script"@en ;
    skos:definition "Relates an expression to details of the set of characters and/or symbols used to express the written language content of a resource."@en .

<http://rdaregistry.info/Elements/e/P20267>
    reg:hasUnconstrained <http://rdaregistry.info/Elements/u/P60804> ;
    reg:lexicalAlias <http://rdaregistry.info/Elements/e/detailsOfIllustrativeContent.en> ;
    reg:name "detailsOfIllustrativeContent"@en ;
    reg:status <http://metadataregistry.org/uri/RegStatus/1001> ;
    rdakit:instructionNumber "7.15.1.4" ;
    rdakit:toolkitDefinition "Details of content intended to illustrate the primary content of a resource."@en ;
    rdakit:toolkitLabel "details of illustrative content"@en ;
    a rdf:Property ;
    rdfs:domain <http://rdaregistry.info/Elements/c/C10006> ;
    rdfs:isDefinedBy <http://rdaregistry.info/Elements/e/> ;
    rdfs:label "has details of illustrative content"@en ;
    skos:definition "Relates an expression to details of content intended to illustrate the primary content of a resource."@en .

<http://rdaregistry.info/Elements/e/P20268>
    reg:hasSubproperty <http://rdaregistry.info/Elements/e/P20269> ;
    reg:hasUnconstrained <http://rdaregistry.info/Elements/u/P60806> ;
    reg:lexicalAlias <http://rdaregistry.info/Elements/e/subjectOfExpression.en> ;
    reg:name "subjectOfExpression"@en ;
    reg:status <http://metadataregistry.org/uri/RegStatus/1001> ;
    rdakit:toolkitDefinition "A work that is about the expression."@en ;
    rdakit:toolkitLabel "subject of (expression)"@en ;
    a rdf:Property ;
    rdfs:domain <http://rdaregistry.info/Elements/c/C10006> ;
    rdfs:isDefinedBy <http://rdaregistry.info/Elements/e/> ;
    rdfs:label "is subject of (expression)"@en ;
    rdfs:range <http://rdaregistry.info/Elements/c/C10001> ;
    rdfs:subPropertyOf <http://rdaregistry.info/Elements/w/P10283> ;
    owl:inverseOf <http://rdaregistry.info/Elements/w/P10258> ;
    skos:definition "Relates an expression to a work that is about the expression."@en .

<http://rdaregistry.info/Elements/e/P20269>
    reg:hasSubproperty <http://rdaregistry.info/Elements/e/P20270>, <http://rdaregistry.info/Elements/e/P20271>, <http://rdaregistry.info/Elements/e/P20272>, <http://rdaregistry.info/Elements/e/P20273>, <http://rdaregistry.info/Elements/e/P20274> ;
    reg:hasUnconstrained <http://rdaregistry.info/Elements/u/P60215> ;
    reg:lexicalAlias <http://rdaregistry.info/Elements/e/describedInExpression.en> ;
    reg:name "describedInExpression"@en ;
    reg:status <http://metadataregistry.org/uri/RegStatus/1001> ;
    rdakit:toolkitDefinition "A work that describes a described expression."@en ;
    rdakit:toolkitLabel "described in (expression)"@en ;
    a rdf:Property ;
    rdfs:domain <http://rdaregistry.info/Elements/c/C10006> ;
    rdfs:isDefinedBy <http://rdaregistry.info/Elements/e/> ;
    rdfs:label "is described in (expression)"@en ;
    rdfs:range <http://rdaregistry.info/Elements/c/C10001> ;
    rdfs:subPropertyOf <http://rdaregistry.info/Elements/e/P20268> ;
    owl:inverseOf <http://rdaregistry.info/Elements/w/P10277> ;
    skos:definition "Relates an expression to a work that describes a described expression."@en .

<http://rdaregistry.info/Elements/e/P20270>
    reg:hasUnconstrained <http://rdaregistry.info/Elements/u/P60219> ;
    reg:lexicalAlias <http://rdaregistry.info/Elements/e/analysedInExpression.en> ;
    reg:name "analysedInExpression"@en ;
    reg:status <http://metadataregistry.org/uri/RegStatus/1001> ;
    rdakit:toolkitDefinition "A work that examines the source expression to identify its components and their relations."@en ;
    rdakit:toolkitLabel "analysed in (expression)"@en ;
    a rdf:Property ;
    rdfs:domain <http://rdaregistry.info/Elements/c/C10006> ;
    rdfs:isDefinedBy <http://rdaregistry.info/Elements/e/> ;
    rdfs:label "is analysed in (expression)"@en ;
    rdfs:range <http://rdaregistry.info/Elements/c/C10001> ;
    rdfs:subPropertyOf <http://rdaregistry.info/Elements/e/P20269> ;
    owl:inverseOf <http://rdaregistry.info/Elements/w/P10278> ;
    skos:definition "Relates a expression to a work that examines the source expression to identify its components and their relations."@en .

<http://rdaregistry.info/Elements/e/P20271>
    reg:hasUnconstrained <http://rdaregistry.info/Elements/u/P60213> ;
    reg:lexicalAlias <http://rdaregistry.info/Elements/e/commentaryInExpression.en> ;
    reg:name "commentaryInExpression"@en ;
    reg:status <http://metadataregistry.org/uri/RegStatus/1001> ;
    rdakit:toolkitDefinition "A work that contains a set of explanatory or critical notes on the described expression."@en ;
    rdakit:toolkitLabel "commentary in (expression)"@en ;
    a rdf:Property ;
    rdfs:domain <http://rdaregistry.info/Elements/c/C10006> ;
    rdfs:isDefinedBy <http://rdaregistry.info/Elements/e/> ;
    rdfs:label "is commentary in (expression)"@en ;
    rdfs:range <http://rdaregistry.info/Elements/c/C10001> ;
    rdfs:subPropertyOf <http://rdaregistry.info/Elements/e/P20269> ;
    owl:inverseOf <http://rdaregistry.info/Elements/w/P10282> ;
    skos:definition "Relates a expression to a work that contains a set of explanatory or critical notes on the described expression."@en .

<http://rdaregistry.info/Elements/e/P20272>
    reg:hasUnconstrained <http://rdaregistry.info/Elements/u/P60212> ;
    reg:lexicalAlias <http://rdaregistry.info/Elements/e/critiquedInExpression.en> ;
    reg:name "critiquedInExpression"@en ;
    reg:status <http://metadataregistry.org/uri/RegStatus/1001> ;
    rdakit:toolkitDefinition "A work that contains a critical evaluation of the described expression."@en ;
    rdakit:toolkitLabel "critiqued in (expression)"@en ;
    a rdf:Property ;
    rdfs:domain <http://rdaregistry.info/Elements/c/C10006> ;
    rdfs:isDefinedBy <http://rdaregistry.info/Elements/e/> ;
    rdfs:label "is critiqued in (expression)"@en ;
    rdfs:range <http://rdaregistry.info/Elements/c/C10001> ;
    rdfs:subPropertyOf <http://rdaregistry.info/Elements/e/P20269> ;
    owl:inverseOf <http://rdaregistry.info/Elements/w/P10281> ;
    skos:definition "Relates a expression to a work that contains a critical evaluation of the described expression."@en .

<http://rdaregistry.info/Elements/e/P20273>
    reg:hasUnconstrained <http://rdaregistry.info/Elements/u/P60218> ;
    reg:lexicalAlias <http://rdaregistry.info/Elements/e/evaluatedInExpression.en> ;
    reg:name "evaluatedInExpression"@en ;
    reg:status <http://metadataregistry.org/uri/RegStatus/1001> ;
    rdakit:toolkitDefinition "A work that examines or judges the described expression."@en ;
    rdakit:toolkitLabel "evaluated in (expression)"@en ;
    a rdf:Property ;
    rdfs:domain <http://rdaregistry.info/Elements/c/C10006> ;
    rdfs:isDefinedBy <http://rdaregistry.info/Elements/e/> ;
    rdfs:label "is evaluated in (expression)"@en ;
    rdfs:range <http://rdaregistry.info/Elements/c/C10001> ;
    rdfs:subPropertyOf <http://rdaregistry.info/Elements/e/P20269> ;
    owl:inverseOf <http://rdaregistry.info/Elements/w/P10279> ;
    skos:definition "Relates a expression to a work that examines or judges the described expression."@en .

<http://rdaregistry.info/Elements/e/P20274>
    reg:hasUnconstrained <http://rdaregistry.info/Elements/u/P60211> ;
    reg:lexicalAlias <http://rdaregistry.info/Elements/e/reviewedInExpression.en> ;
    reg:name "reviewedInExpression"@en ;
    reg:status <http://metadataregistry.org/uri/RegStatus/1001> ;
    rdakit:toolkitDefinition "A work that contains a brief evaluation of the described expression."@en ;
    rdakit:toolkitLabel "reviewed in (expression)"@en ;
    a rdf:Property ;
    rdfs:domain <http://rdaregistry.info/Elements/c/C10006> ;
    rdfs:isDefinedBy <http://rdaregistry.info/Elements/e/> ;
    rdfs:label "is reviewed in (expression)"@en ;
    rdfs:range <http://rdaregistry.info/Elements/c/C10001> ;
    rdfs:subPropertyOf <http://rdaregistry.info/Elements/e/P20269> ;
    owl:inverseOf <http://rdaregistry.info/Elements/w/P10280> ;
    skos:definition "Relates a expression to a work that contains a brief evaluation of the described expression."@en .

<http://rdaregistry.info/Elements/e/P20275>
    reg:hasUnconstrained <http://rdaregistry.info/Elements/u/P60809> ;
    reg:lexicalAlias <http://rdaregistry.info/Elements/e/writerOfForeword.en> ;
    reg:name "writerOfForeword"@en ;
    reg:status <http://metadataregistry.org/uri/RegStatus/1001> ;
    rdakit:toolkitDefinition "A person, family, or corporate body contributing to an expression of a work by providing a foreword to the original work."@en ;
    rdakit:toolkitLabel "writer of foreword"@en ;
    a rdf:Property ;
    rdfs:domain <http://rdaregistry.info/Elements/c/C10006> ;
    rdfs:isDefinedBy <http://rdaregistry.info/Elements/e/> ;
    rdfs:label "has writer of foreword"@en ;
    rdfs:range <http://rdaregistry.info/Elements/c/C10002> ;
    rdfs:subPropertyOf <http://rdaregistry.info/Elements/e/P20046> ;
    owl:inverseOf <http://rdaregistry.info/Elements/a/P50254> ;
    skos:definition "Relates an expression to a person, family, or corporate body contributing to an expression of a work by providing a foreword to the original work."@en .

<http://rdaregistry.info/Elements/e/P20276>
    reg:hasUnconstrained <http://rdaregistry.info/Elements/u/P60811> ;
    reg:lexicalAlias <http://rdaregistry.info/Elements/e/soundDesigner.en> ;
    reg:name "soundDesigner"@en ;
    reg:status <http://metadataregistry.org/uri/RegStatus/1001> ;
    rdakit:toolkitDefinition "A person, family, or corporate body contributing to an expression of a work by designing and creating audio/sound components."@en ;
    rdakit:toolkitLabel "sound designer"@en ;
    a rdf:Property ;
    rdfs:domain <http://rdaregistry.info/Elements/c/C10006> ;
    rdfs:isDefinedBy <http://rdaregistry.info/Elements/e/> ;
    rdfs:label "has sound designer"@en ;
    rdfs:range <http://rdaregistry.info/Elements/c/C10002> ;
    rdfs:subPropertyOf <http://rdaregistry.info/Elements/e/P20053> ;
    owl:inverseOf <http://rdaregistry.info/Elements/a/P50255> ;
    skos:definition "Relates an expression to a person, family, or corporate body contributing to an expression of a work by designing and creating audio/sound components."@en .

<http://rdaregistry.info/Elements/e/P20277>
    reg:hasUnconstrained <http://rdaregistry.info/Elements/u/P60813> ;
    reg:lexicalAlias <http://rdaregistry.info/Elements/e/lightingDesigner.en> ;
    reg:name "lightingDesigner"@en ;
    reg:status <http://metadataregistry.org/uri/RegStatus/1001> ;
    rdakit:toolkitDefinition "A person, family, or corporate body contributing to an expression of a work by designing and creating lighting components."@en ;
    rdakit:toolkitLabel "lighting designer"@en ;
    a rdf:Property ;
    rdfs:domain <http://rdaregistry.info/Elements/c/C10006> ;
    rdfs:isDefinedBy <http://rdaregistry.info/Elements/e/> ;
    rdfs:label "has lighting designer"@en ;
    rdfs:range <http://rdaregistry.info/Elements/c/C10002> ;
    rdfs:subPropertyOf <http://rdaregistry.info/Elements/e/P20053> ;
    owl:inverseOf <http://rdaregistry.info/Elements/a/P50256> ;
    skos:definition "Relates an expression to a person, family, or corporate body contributing to an expression of a work by designing and creating lighting components."@en .

<http://rdaregistry.info/Elements/e/P20278>
    reg:hasUnconstrained <http://rdaregistry.info/Elements/u/P60823> ;
    reg:lexicalAlias <http://rdaregistry.info/Elements/e/detailsOfDuration.en> ;
    reg:name "detailsOfDuration"@en ;
    reg:status <http://metadataregistry.org/uri/RegStatus/1001> ;
    rdakit:instructionNumber "7.22.1.5" ;
    rdakit:toolkitDefinition "The playing time, running time, performance time, etc., of the content of a resource."@en ;
    rdakit:toolkitLabel "details of duration"@en ;
    a rdf:Property ;
    rdfs:domain <http://rdaregistry.info/Elements/c/C10006> ;
    rdfs:isDefinedBy <http://rdaregistry.info/Elements/e/> ;
    rdfs:label "has details of duration"@en ;
    skos:definition "Relates an expression to details of the playing time, running time, performance time, etc., of the content of a resource."@en .

<http://rdaregistry.info/Elements/e/P20279>
    reg:hasUnconstrained <http://rdaregistry.info/Elements/u/P60824> ;
    reg:lexicalAlias <http://rdaregistry.info/Elements/e/onScreenParticipant.en> ;
    reg:name "onScreenParticipant"@en ;
    reg:status <http://metadataregistry.org/uri/RegStatus/1001> ;
    rdakit:toolkitDefinition "A person, family, or corporate body contributing to an expression of a nonfiction moving image work by taking an active role as a participant."@en ;
    rdakit:toolkitLabel "on-screen participant"@en ;
    a rdf:Property ;
    rdfs:domain <http://rdaregistry.info/Elements/c/C10006> ;
    rdfs:isDefinedBy <http://rdaregistry.info/Elements/e/> ;
    rdfs:label "has on-screen participant"@en ;
    rdfs:range <http://rdaregistry.info/Elements/c/C10002> ;
    rdfs:subPropertyOf <http://rdaregistry.info/Elements/e/P20053> ;
    owl:inverseOf <http://rdaregistry.info/Elements/a/P50261> ;
    skos:definition "Relates an expression to a person, family. or corporate body contributing to an expression of a nonfiction moving image work by taking an active role as a participant."@en .

<http://rdaregistry.info/Elements/e/P20280>
    reg:hasUnconstrained <http://rdaregistry.info/Elements/u/P60828> ;
    reg:lexicalAlias <http://rdaregistry.info/Elements/e/softwareDeveloper.en> ;
    reg:name "softwareDeveloper"@en ;
    reg:status <http://metadataregistry.org/uri/RegStatus/1001> ;
    rdakit:toolkitDefinition "A person, family, or corporate body contributing to an expression of a work by researching, designing, implementing, or testing the software."@en ;
    rdakit:toolkitLabel "software developer"@en ;
    a rdf:Property ;
    rdfs:domain <http://rdaregistry.info/Elements/c/C10006> ;
    rdfs:isDefinedBy <http://rdaregistry.info/Elements/e/> ;
    rdfs:label "has software developer"@en ;
    rdfs:range <http://rdaregistry.info/Elements/c/C10002> ;
    rdfs:subPropertyOf <http://rdaregistry.info/Elements/e/P20053> ;
    owl:inverseOf <http://rdaregistry.info/Elements/a/P50263> ;
    skos:definition "Relates an expression to a person, family, or corporate body contributing to an expression of a work by researching, designing, implementing, or testing the software."@en .

<http://rdaregistry.info/Elements/e/P20281>
    reg:hasUnconstrained <http://rdaregistry.info/Elements/u/P60830> ;
    reg:lexicalAlias <http://rdaregistry.info/Elements/e/oratorioAdaptationOfExpression.en> ;
    reg:name "oratorioAdaptationOfExpression"@en ;
    reg:status <http://metadataregistry.org/uri/RegStatus/1001> ;
    rdakit:toolkitDefinition "An expression of a work that has been adapted as an oratorio."@en ;
    rdakit:toolkitLabel "oratorio adaptaion of (expression)"@en ;
    a rdf:Property ;
    rdfs:domain <http://rdaregistry.info/Elements/c/C10006> ;
    rdfs:isDefinedBy <http://rdaregistry.info/Elements/e/> ;
    rdfs:label "is oratorio adaptation of (expression)"@en ;
    rdfs:range <http://rdaregistry.info/Elements/c/C10006> ;
    rdfs:subPropertyOf <http://rdaregistry.info/Elements/e/P20152> ;
    owl:inverseOf <http://rdaregistry.info/Elements/e/P20282> ;
    skos:definition "Relates an expression to an expression of a work that has been adapted as an oratorio."@en .

<http://rdaregistry.info/Elements/e/P20282>
    reg:hasUnconstrained <http://rdaregistry.info/Elements/u/P60831> ;
    reg:lexicalAlias <http://rdaregistry.info/Elements/e/adaptedAsOratorioExpression.en> ;
    reg:name "adaptedAsOratorioExpression"@en ;
    reg:status <http://metadataregistry.org/uri/RegStatus/1001> ;
    rdakit:toolkitDefinition "An expression of an oratorio based on the source expression."@en ;
    rdakit:toolkitLabel "adapted as oratorio (expression)"@en ;
    a rdf:Property ;
    rdfs:domain <http://rdaregistry.info/Elements/c/C10006> ;
    rdfs:isDefinedBy <http://rdaregistry.info/Elements/e/> ;
    rdfs:label "is adapted as oratorio (expression)"@en ;
    rdfs:range <http://rdaregistry.info/Elements/c/C10006> ;
    rdfs:subPropertyOf <http://rdaregistry.info/Elements/e/P20153> ;
    owl:inverseOf <http://rdaregistry.info/Elements/e/P20281> ;
    skos:definition "Relates an expression to an expression of an oratorio based on the source expression."@en .

<http://rdaregistry.info/Elements/e/P20283>
    reg:hasUnconstrained <http://rdaregistry.info/Elements/u/P60838> ;
    reg:lexicalAlias <http://rdaregistry.info/Elements/e/colourist.en> ;
    reg:name "colourist"@en ;
    reg:status <http://metadataregistry.org/uri/RegStatus/1001> ;
    rdakit:toolkitDefinition "A person, family, or corporate body contributing to an expression of a work by applying colour to drawings, prints, photographs, maps, moving images, etc."@en ;
    rdakit:toolkitLabel "colourist"@en ;
    a rdf:Property ;
    rdfs:domain <http://rdaregistry.info/Elements/c/C10006> ;
    rdfs:isDefinedBy <http://rdaregistry.info/Elements/e/> ;
    rdfs:label "has colourist"@en ;
    rdfs:range <http://rdaregistry.info/Elements/c/C10002> ;
    rdfs:subPropertyOf <http://rdaregistry.info/Elements/e/P20053> ;
    owl:inverseOf <http://rdaregistry.info/Elements/a/P50266> ;
    skos:definition "Relates an expression to a person, family, or corporate body contributing to an expression of a work by applying colour to drawings, prints, photographs, maps, moving images, etc."@en .

<http://rdaregistry.info/Elements/e/P20284>
    reg:hasUnconstrained <http://rdaregistry.info/Elements/u/P60840> ;
    reg:lexicalAlias <http://rdaregistry.info/Elements/e/makeUpArtist.en> ;
    reg:name "makeUpArtist"@en ;
    reg:status <http://metadataregistry.org/uri/RegStatus/1001> ;
    rdakit:toolkitDefinition "A person, family, or corporate body contributing to an expression of a work by applying make-up and prosthetics for a moving image production or for a musical or dramatic presentation or entertainment."@en ;
    rdakit:toolkitLabel "make-up artist"@en ;
    a rdf:Property ;
    rdfs:domain <http://rdaregistry.info/Elements/c/C10006> ;
    rdfs:isDefinedBy <http://rdaregistry.info/Elements/e/> ;
    rdfs:label "has make-up artist"@en ;
    rdfs:range <http://rdaregistry.info/Elements/c/C10002> ;
    rdfs:subPropertyOf <http://rdaregistry.info/Elements/e/P20053> ;
    owl:inverseOf <http://rdaregistry.info/Elements/a/P50267> ;
    skos:definition "Relates an expression to a person, family, or corporate body contributing to an expression of a work by applying make-up and prosthetics for a moving image production or for a musical or dramatic presentation or entertainment."@en .

<http://rdaregistry.info/Elements/e/P20285>
    reg:hasUnconstrained <http://rdaregistry.info/Elements/u/P60842> ;
    reg:lexicalAlias <http://rdaregistry.info/Elements/e/choralConductor.en> ;
    reg:name "choralConductor"@en ;
    reg:status <http://metadataregistry.org/uri/RegStatus/1001> ;
    rdakit:toolkitDefinition "A conductor contributing to an expression of a musical work by leading a choral performing group in a musical or dramatic presentation, etc."@en ;
    rdakit:toolkitLabel "choral conductor"@en ;
    a rdf:Property ;
    rdfs:domain <http://rdaregistry.info/Elements/c/C10006> ;
    rdfs:isDefinedBy <http://rdaregistry.info/Elements/e/> ;
    rdfs:label "has choral conductor"@en ;
    rdfs:range <http://rdaregistry.info/Elements/c/C10002> ;
    rdfs:subPropertyOf <http://rdaregistry.info/Elements/e/P20011> ;
    owl:inverseOf <http://rdaregistry.info/Elements/a/P50268> ;
    skos:definition "Relates an expression to a conductor contributing to an expression of a musical work by leading a choral performing group in a musical or dramatic presentation, etc."@en .

<http://rdaregistry.info/Elements/e/P20286>
    reg:hasUnconstrained <http://rdaregistry.info/Elements/u/P60844> ;
    reg:lexicalAlias <http://rdaregistry.info/Elements/e/instrumentalConductor.en> ;
    reg:name "instrumentalConductor"@en ;
    reg:status <http://metadataregistry.org/uri/RegStatus/1001> ;
    rdakit:toolkitDefinition "A conductor contributing to an expression of a musical work by leading an instrumental performing group in a musical or dramatic presentation, etc."@en ;
    rdakit:toolkitLabel "instrumental conductor"@en ;
    a rdf:Property ;
    rdfs:domain <http://rdaregistry.info/Elements/c/C10006> ;
    rdfs:isDefinedBy <http://rdaregistry.info/Elements/e/> ;
    rdfs:label "has instrumental conductor"@en ;
    rdfs:range <http://rdaregistry.info/Elements/c/C10002> ;
    rdfs:subPropertyOf <http://rdaregistry.info/Elements/e/P20011> ;
    owl:inverseOf <http://rdaregistry.info/Elements/a/P50269> ;
    skos:definition "Relates an expression to a conductor contributing to an expression of a musical work by leading an instrumental performing group in a musical or dramatic presentation, etc."@en .

