@prefix rdf: <http://www.w3.org/1999/02/22-rdf-syntax-ns#> .
@prefix rdfs: <http://www.w3.org/2000/01/rdf-schema#> .
@prefix skos: <http://www.w3.org/2004/02/skos/core#> .
@prefix dc: <http://purl.org/dc/elements/1.1/> .
@prefix dct: <http://purl.org/dc/terms/> .
@prefix owl: <http://www.w3.org/2002/07/owl#> .
@prefix foaf: <http://xmlns.com/foaf/0.1/> .
@prefix reg: <http://metadataregistry.org/uri/profile/RegAp/> .
@prefix status: <http://metadataregistry.org/uri/RegStatus/> .

<http://metadataregistry.org/uri/RegStatus/1001>
    a skos:Concept ;
    skos:prefLabel "Published"@en .

<http://metadataregistry.org/uri/RegStatus/1008>
    a skos:Concept ;
    skos:prefLabel "Deprecated"@en .

<http://rdaregistry.info/Elements/i/>
    dc:title "RDA Item properties"@en ;
    skos:note "Properties derived from RDA elements and relationship designators with the domain of RDA Item."@en .

<http://rdaregistry.info/Elements/i/P40001>
    reg:hasUnconstrained <http://rdaregistry.info/Elements/u/P60052> ;
    reg:lexicalAlias "http://rdaregistry.info/Elements/i/identifierForTheItem"@en ;
    reg:name "identifierForTheItem"@en ;
    reg:status <http://metadataregistry.org/uri/RegStatus/1001> ;
    a rdf:Property ;
    rdfs:domain <http://rdaregistry.info/Elements/c/C10003> ;
    rdfs:isDefinedBy <http://rdaregistry.info/Elements/i/> ;
    rdfs:label "has identifier for the item"@en ;
    skos:definition "Relates an item to a character string associated with an item that serves to differentiate that item from other items."@en .

<http://rdaregistry.info/Elements/i/P40002>
    reg:status <http://metadataregistry.org/uri/RegStatus/1008> ;
    rdfs:isDefinedBy <http://rdaregistry.info/Elements/i/> .

<http://rdaregistry.info/Elements/i/P40003>
    reg:hasUnconstrained <http://rdaregistry.info/Elements/u/P60056> ;
    reg:lexicalAlias "http://rdaregistry.info/Elements/i/noteOnItemSpecificCarrierCharacteristic"@en ;
    reg:name "noteOnItemSpecificCarrierCharacteristic"@en ;
    reg:status <http://metadataregistry.org/uri/RegStatus/1001> ;
    a rdf:Property ;
    rdfs:domain <http://rdaregistry.info/Elements/c/C10003> ;
    rdfs:isDefinedBy <http://rdaregistry.info/Elements/i/> ;
    rdfs:label "has note on item-specific carrier characteristic"@en ;
    skos:definition "Relates an item to a note providing additional information about carrier characteristics that are specific to the item being described and are assumed not to apply to other items exemplifying the same manifestation."@en .

<http://rdaregistry.info/Elements/i/P40004>
    reg:hasUnconstrained <http://rdaregistry.info/Elements/u/P60066> ;
    reg:lexicalAlias "http://rdaregistry.info/Elements/i/collector"@en ;
    reg:name "collector"@en ;
    reg:status <http://metadataregistry.org/uri/RegStatus/1001> ;
    a rdf:Property ;
    rdfs:domain <http://rdaregistry.info/Elements/c/C10003> ;
    rdfs:isDefinedBy <http://rdaregistry.info/Elements/i/> ;
    rdfs:label "has collector"@en ;
    rdfs:range <http://rdaregistry.info/Elements/c/C10002> ;
    rdfs:subPropertyOf <http://rdaregistry.info/Elements/i/P40017>, <http://rdaregistry.info/Elements/u/P60066> ;
    owl:inverseOf <http://rdaregistry.info/Elements/a/P50045> ;
    skos:definition "Relates an item to a curator who brings together items from various sources that are then arranged, described, and cataloged as a collection."@en .

<http://rdaregistry.info/Elements/i/P40005>
    reg:hasUnconstrained <http://rdaregistry.info/Elements/u/P60067> ;
    reg:lexicalAlias "http://rdaregistry.info/Elements/i/collectionRegistrar"@en ;
    reg:name "collectionRegistrar"@en ;
    reg:status <http://metadataregistry.org/uri/RegStatus/1001> ;
    a rdf:Property ;
    rdfs:domain <http://rdaregistry.info/Elements/c/C10003> ;
    rdfs:isDefinedBy <http://rdaregistry.info/Elements/i/> ;
    rdfs:label "has collection registrar "@en ;
    rdfs:range <http://rdaregistry.info/Elements/c/C10002> ;
    rdfs:subPropertyOf <http://rdaregistry.info/Elements/i/P40017>, <http://rdaregistry.info/Elements/u/P60067> ;
    owl:inverseOf <http://rdaregistry.info/Elements/a/P50046> ;
    skos:definition "Relates an item to a curator who lists or inventories the items in an aggregate work such as a collection of items or works."@en .

<http://rdaregistry.info/Elements/i/P40006>
    reg:hasUnconstrained <http://rdaregistry.info/Elements/u/P60068> ;
    reg:lexicalAlias "http://rdaregistry.info/Elements/i/depositor"@en ;
    reg:name "depositor"@en ;
    reg:status <http://metadataregistry.org/uri/RegStatus/1001> ;
    a rdf:Property ;
    rdfs:domain <http://rdaregistry.info/Elements/c/C10003> ;
    rdfs:isDefinedBy <http://rdaregistry.info/Elements/i/> ;
    rdfs:label "has depositor"@en ;
    rdfs:range <http://rdaregistry.info/Elements/c/C10002> ;
    rdfs:subPropertyOf <http://rdaregistry.info/Elements/i/P40018>, <http://rdaregistry.info/Elements/u/P60068> ;
    owl:inverseOf <http://rdaregistry.info/Elements/a/P50047> ;
    skos:definition "Relates an item to a current owner of an item who deposited the item into the custody of another person, family, or corporate body, while still retaining ownership."@en .

<http://rdaregistry.info/Elements/i/P40007>
    reg:hasUnconstrained <http://rdaregistry.info/Elements/u/P60091> ;
    reg:lexicalAlias "http://rdaregistry.info/Elements/i/donor"@en ;
    reg:name "donor"@en ;
    reg:status <http://metadataregistry.org/uri/RegStatus/1001> ;
    a rdf:Property ;
    rdfs:domain <http://rdaregistry.info/Elements/c/C10003> ;
    rdfs:isDefinedBy <http://rdaregistry.info/Elements/i/> ;
    rdfs:label "has donor"@en ;
    rdfs:range <http://rdaregistry.info/Elements/c/C10002> ;
    rdfs:subPropertyOf <http://rdaregistry.info/Elements/i/P40019>, <http://rdaregistry.info/Elements/u/P60091> ;
    owl:inverseOf <http://rdaregistry.info/Elements/a/P50066> ;
    skos:definition "Relates an item to a former owner of an item who donated that item to another owner."@en .

<http://rdaregistry.info/Elements/i/P40008>
    reg:hasUnconstrained <http://rdaregistry.info/Elements/u/P60092> ;
    reg:lexicalAlias "http://rdaregistry.info/Elements/i/seller"@en ;
    reg:name "seller"@en ;
    reg:status <http://metadataregistry.org/uri/RegStatus/1001> ;
    a rdf:Property ;
    rdfs:domain <http://rdaregistry.info/Elements/c/C10003> ;
    rdfs:isDefinedBy <http://rdaregistry.info/Elements/i/> ;
    rdfs:label "has seller"@en ;
    rdfs:range <http://rdaregistry.info/Elements/c/C10002> ;
    rdfs:subPropertyOf <http://rdaregistry.info/Elements/i/P40019>, <http://rdaregistry.info/Elements/u/P60092> ;
    owl:inverseOf <http://rdaregistry.info/Elements/a/P50067> ;
    skos:definition "Relates an item to a former owner of an item who sold that item to another owner."@en .

<http://rdaregistry.info/Elements/i/P40009>
    reg:hasUnconstrained <http://rdaregistry.info/Elements/u/P60101> ;
    reg:lexicalAlias "http://rdaregistry.info/Elements/i/containedInItem"@en ;
    reg:name "containedInItem"@en ;
    reg:status <http://metadataregistry.org/uri/RegStatus/1001> ;
    a rdf:Property ;
    rdfs:domain <http://rdaregistry.info/Elements/c/C10003> ;
    rdfs:isDefinedBy <http://rdaregistry.info/Elements/i/> ;
    rdfs:label "is contained in (item)"@en ;
    rdfs:range <http://rdaregistry.info/Elements/c/C10003> ;
    rdfs:subPropertyOf <http://rdaregistry.info/Elements/i/P40054>, <http://rdaregistry.info/Elements/u/P60101> ;
    owl:inverseOf <http://rdaregistry.info/Elements/i/P40034> ;
    skos:definition "Relates an item to a larger item of which the item is a discrete component."@en .

<http://rdaregistry.info/Elements/i/P40010>
    reg:hasUnconstrained <http://rdaregistry.info/Elements/u/P60133> ;
    reg:lexicalAlias "http://rdaregistry.info/Elements/i/noteOnDimensionsOfItem"@en ;
    reg:name "noteOnDimensionsOfItem"@en ;
    reg:status <http://metadataregistry.org/uri/RegStatus/1001> ;
    a rdf:Property ;
    rdfs:domain <http://rdaregistry.info/Elements/c/C10003> ;
    rdfs:isDefinedBy <http://rdaregistry.info/Elements/i/> ;
    rdfs:label "has note on dimensions of item"@en ;
    rdfs:subPropertyOf <http://rdaregistry.info/Elements/i/P40003> ;
    skos:definition "Relates an item to a note providing information on the dimensions of the specific item being described that is not recorded as part of the dimensions element."@en .

<http://rdaregistry.info/Elements/i/P40011>
    reg:hasUnconstrained <http://rdaregistry.info/Elements/u/P60134> ;
    reg:lexicalAlias "http://rdaregistry.info/Elements/i/noteOnExtentOfItem"@en ;
    reg:name "noteOnExtentOfItem"@en ;
    reg:status <http://metadataregistry.org/uri/RegStatus/1001> ;
    a rdf:Property ;
    rdfs:domain <http://rdaregistry.info/Elements/c/C10003> ;
    rdfs:isDefinedBy <http://rdaregistry.info/Elements/i/> ;
    rdfs:label "has note on extent of item"@en ;
    rdfs:subPropertyOf <http://rdaregistry.info/Elements/i/P40003> ;
    skos:definition "Relates an item to a note providing information on the extent of the specific item being described that is not recorded as part of the extent element."@en .

<http://rdaregistry.info/Elements/i/P40012>
    reg:hasUnconstrained <http://rdaregistry.info/Elements/u/P60421> ;
    reg:lexicalAlias "http://rdaregistry.info/Elements/i/illuminator"@en ;
    reg:name "illuminator"@en ;
    reg:status <http://metadataregistry.org/uri/RegStatus/1001> ;
    a rdf:Property ;
    rdfs:domain <http://rdaregistry.info/Elements/c/C10003> ;
    rdfs:isDefinedBy <http://rdaregistry.info/Elements/i/> ;
    rdfs:label "has illuminator"@en ;
    rdfs:range <http://rdaregistry.info/Elements/c/C10004> ;
    rdfs:subPropertyOf <http://rdaregistry.info/Elements/i/P40023>, <http://rdaregistry.info/Elements/u/P60421> ;
    owl:inverseOf <http://rdaregistry.info/Elements/a/P50092> ;
    skos:definition "Relates an item to a person providing decoration to a specific item using precious metals or color, often with elaborate designs and motifs."@en .

<http://rdaregistry.info/Elements/i/P40013>
    reg:hasUnconstrained <http://rdaregistry.info/Elements/u/P60458> ;
    reg:lexicalAlias "http://rdaregistry.info/Elements/i/binder"@en ;
    reg:name "binder"@en ;
    reg:status <http://metadataregistry.org/uri/RegStatus/1001> ;
    a rdf:Property ;
    rdfs:domain <http://rdaregistry.info/Elements/c/C10003> ;
    rdfs:isDefinedBy <http://rdaregistry.info/Elements/i/> ;
    rdfs:label "has binder"@en ;
    rdfs:range <http://rdaregistry.info/Elements/c/C10004> ;
    rdfs:subPropertyOf <http://rdaregistry.info/Elements/i/P40023>, <http://rdaregistry.info/Elements/u/P60458> ;
    owl:inverseOf <http://rdaregistry.info/Elements/a/P50123> ;
    skos:definition "Relates an item to a person who binds an item."@en .

<http://rdaregistry.info/Elements/i/P40014>
    reg:hasUnconstrained <http://rdaregistry.info/Elements/u/P60460> ;
    reg:lexicalAlias "http://rdaregistry.info/Elements/i/inscriber"@en ;
    reg:name "inscriber"@en ;
    reg:status <http://metadataregistry.org/uri/RegStatus/1001> ;
    a rdf:Property ;
    rdfs:domain <http://rdaregistry.info/Elements/c/C10003> ;
    rdfs:isDefinedBy <http://rdaregistry.info/Elements/i/> ;
    rdfs:label "has inscriber"@en ;
    rdfs:range <http://rdaregistry.info/Elements/c/C10004> ;
    rdfs:subPropertyOf <http://rdaregistry.info/Elements/i/P40023>, <http://rdaregistry.info/Elements/u/P60460> ;
    owl:inverseOf <http://rdaregistry.info/Elements/a/P50125> ;
    skos:definition "Relates an item to a person who has written a statement of dedication or gift on an item."@en .

<http://rdaregistry.info/Elements/i/P40015>
    reg:hasUnconstrained <http://rdaregistry.info/Elements/u/P60464> ;
    reg:lexicalAlias "http://rdaregistry.info/Elements/i/annotator"@en ;
    reg:name "annotator"@en ;
    reg:status <http://metadataregistry.org/uri/RegStatus/1001> ;
    a rdf:Property ;
    rdfs:domain <http://rdaregistry.info/Elements/c/C10003> ;
    rdfs:isDefinedBy <http://rdaregistry.info/Elements/i/> ;
    rdfs:label "has annotator"@en ;
    rdfs:range <http://rdaregistry.info/Elements/c/C10004> ;
    rdfs:subPropertyOf <http://rdaregistry.info/Elements/i/P40023>, <http://rdaregistry.info/Elements/u/P60464> ;
    owl:inverseOf <http://rdaregistry.info/Elements/a/P50128> ;
    skos:definition "Relates an item to a person who makes manuscript annotations on an item."@en .

<http://rdaregistry.info/Elements/i/P40016>
    reg:hasUnconstrained <http://rdaregistry.info/Elements/u/P60466> ;
    reg:lexicalAlias "http://rdaregistry.info/Elements/i/autographer"@en ;
    reg:name "autographer"@en ;
    reg:status <http://metadataregistry.org/uri/RegStatus/1001> ;
    a rdf:Property ;
    rdfs:domain <http://rdaregistry.info/Elements/c/C10003> ;
    rdfs:isDefinedBy <http://rdaregistry.info/Elements/i/> ;
    rdfs:label "has autographer "@en ;
    rdfs:range <http://rdaregistry.info/Elements/c/C10004> ;
    rdfs:subPropertyOf <http://rdaregistry.info/Elements/i/P40023>, <http://rdaregistry.info/Elements/u/P60466> ;
    owl:inverseOf <http://rdaregistry.info/Elements/a/P50129> ;
    skos:definition "Relates an item to a person whose manuscript signature appears on an item."@en .

<http://rdaregistry.info/Elements/i/P40017>
    reg:hasSubproperty <http://rdaregistry.info/Elements/i/P40004>, <http://rdaregistry.info/Elements/i/P40005> ;
    reg:hasUnconstrained <http://rdaregistry.info/Elements/u/P60376> ;
    reg:lexicalAlias "http://rdaregistry.info/Elements/i/curator"@en ;
    reg:name "curator"@en ;
    reg:status <http://metadataregistry.org/uri/RegStatus/1001> ;
    a rdf:Property ;
    rdfs:domain <http://rdaregistry.info/Elements/c/C10003> ;
    rdfs:isDefinedBy <http://rdaregistry.info/Elements/i/> ;
    rdfs:label "has curator"@en ;
    rdfs:range <http://rdaregistry.info/Elements/c/C10002> ;
    rdfs:subPropertyOf <http://rdaregistry.info/Elements/i/P40023>, <http://rdaregistry.info/Elements/u/P60376> ;
    owl:inverseOf <http://rdaregistry.info/Elements/a/P50133> ;
    skos:definition "Relates an item to a person, family, or corporate body conceiving, aggregating, and/or organizing an exhibition, collection, or other item."@en .

<http://rdaregistry.info/Elements/i/P40018>
    reg:hasSubproperty <http://rdaregistry.info/Elements/i/P40006> ;
    reg:hasUnconstrained <http://rdaregistry.info/Elements/u/P60400> ;
    reg:lexicalAlias "http://rdaregistry.info/Elements/i/currentOwner"@en ;
    reg:name "currentOwner"@en ;
    reg:status <http://metadataregistry.org/uri/RegStatus/1001> ;
    a rdf:Property ;
    rdfs:domain <http://rdaregistry.info/Elements/c/C10003> ;
    rdfs:isDefinedBy <http://rdaregistry.info/Elements/i/> ;
    rdfs:label "has current owner"@en ;
    rdfs:range <http://rdaregistry.info/Elements/c/C10002> ;
    rdfs:subPropertyOf <http://rdaregistry.info/Elements/i/P40021>, <http://rdaregistry.info/Elements/u/P60400> ;
    owl:inverseOf <http://rdaregistry.info/Elements/a/P50162> ;
    skos:definition "Relates an item to a person, family, or corporate body currently having legal possession of an item."@en .

<http://rdaregistry.info/Elements/i/P40019>
    reg:hasSubproperty <http://rdaregistry.info/Elements/i/P40007>, <http://rdaregistry.info/Elements/i/P40008> ;
    reg:hasUnconstrained <http://rdaregistry.info/Elements/u/P60401> ;
    reg:lexicalAlias "http://rdaregistry.info/Elements/i/formerOwner"@en ;
    reg:name "formerOwner"@en ;
    reg:status <http://metadataregistry.org/uri/RegStatus/1001> ;
    a rdf:Property ;
    rdfs:domain <http://rdaregistry.info/Elements/c/C10003> ;
    rdfs:isDefinedBy <http://rdaregistry.info/Elements/i/> ;
    rdfs:label "has former owner"@en ;
    rdfs:range <http://rdaregistry.info/Elements/c/C10002> ;
    rdfs:subPropertyOf <http://rdaregistry.info/Elements/i/P40021>, <http://rdaregistry.info/Elements/u/P60401> ;
    owl:inverseOf <http://rdaregistry.info/Elements/a/P50163> ;
    skos:definition "Relates an item to a person, family, or corporate body formerly having legal possession of an item."@en .

<http://rdaregistry.info/Elements/i/P40020>
    reg:hasUnconstrained <http://rdaregistry.info/Elements/u/P60402> ;
    reg:lexicalAlias "http://rdaregistry.info/Elements/i/custodian"@en ;
    reg:name "custodian"@en ;
    reg:status <http://metadataregistry.org/uri/RegStatus/1001> ;
    a rdf:Property ;
    rdfs:domain <http://rdaregistry.info/Elements/c/C10003> ;
    rdfs:isDefinedBy <http://rdaregistry.info/Elements/i/> ;
    rdfs:label "has custodian"@en ;
    rdfs:range <http://rdaregistry.info/Elements/c/C10002> ;
    owl:inverseOf <http://rdaregistry.info/Elements/a/P50164> ;
    skos:definition "Relates an item to a person, family, or corporate body having legal custody of an item."@en .

<http://rdaregistry.info/Elements/i/P40021>
    reg:hasSubproperty <http://rdaregistry.info/Elements/i/P40018>, <http://rdaregistry.info/Elements/i/P40019> ;
    reg:hasUnconstrained <http://rdaregistry.info/Elements/u/P60404> ;
    reg:lexicalAlias "http://rdaregistry.info/Elements/i/owner"@en ;
    reg:name "owner"@en ;
    reg:status <http://metadataregistry.org/uri/RegStatus/1001> ;
    a rdf:Property ;
    rdfs:domain <http://rdaregistry.info/Elements/c/C10003> ;
    rdfs:isDefinedBy <http://rdaregistry.info/Elements/i/> ;
    rdfs:label "has owner"@en ;
    rdfs:range <http://rdaregistry.info/Elements/c/C10002> ;
    owl:inverseOf <http://rdaregistry.info/Elements/a/P50165> ;
    skos:definition "Relates an item to a person, family, or corporate body having legal possession of an item."@en .

<http://rdaregistry.info/Elements/i/P40022>
    reg:hasUnconstrained <http://rdaregistry.info/Elements/u/P60406> ;
    reg:lexicalAlias "http://rdaregistry.info/Elements/i/honoureeOfItem"@en ;
    reg:name "honoureeOfItem"@en ;
    reg:status <http://metadataregistry.org/uri/RegStatus/1001> ;
    a rdf:Property ;
    rdfs:domain <http://rdaregistry.info/Elements/c/C10003> ;
    rdfs:isDefinedBy <http://rdaregistry.info/Elements/i/> ;
    rdfs:label "has honouree (item) "@en ;
    rdfs:range <http://rdaregistry.info/Elements/c/C10002> ;
    rdfs:subPropertyOf <http://rdaregistry.info/Elements/i/P40023>, <http://rdaregistry.info/Elements/u/P60406> ;
    owl:inverseOf <http://rdaregistry.info/Elements/a/P50167> ;
    skos:definition "Relates an item to a person, family, or corporate body honoured by an item, e.g., a person to whom a copy is presented."@en .

<http://rdaregistry.info/Elements/i/P40023>
    reg:hasSubproperty <http://rdaregistry.info/Elements/i/P40012>, <http://rdaregistry.info/Elements/i/P40013>, <http://rdaregistry.info/Elements/i/P40014>, <http://rdaregistry.info/Elements/i/P40015>, <http://rdaregistry.info/Elements/i/P40016>, <http://rdaregistry.info/Elements/i/P40017>, <http://rdaregistry.info/Elements/i/P40022>, <http://rdaregistry.info/Elements/i/P40024>, <http://rdaregistry.info/Elements/i/P40025> ;
    reg:hasUnconstrained <http://rdaregistry.info/Elements/u/P60374> ;
    reg:lexicalAlias "http://rdaregistry.info/Elements/i/otherPFCItem"@en ;
    reg:name "otherPFCItem"@en ;
    reg:status <http://metadataregistry.org/uri/RegStatus/1001> ;
    a rdf:Property ;
    rdfs:domain <http://rdaregistry.info/Elements/c/C10003> ;
    rdfs:isDefinedBy <http://rdaregistry.info/Elements/i/> ;
    rdfs:label "has other person, family, or corporate body associated with an item"@en ;
    rdfs:range <http://rdaregistry.info/Elements/c/C10002> ;
    owl:inverseOf <http://rdaregistry.info/Elements/a/P50182> ;
    skos:definition "Relates an item to a person, family, or corporate body other than an owner or custodian associated with an item."@en ;
    skos:scopeNote "Includes curators, binders, restorationists, etc."@en .

<http://rdaregistry.info/Elements/i/P40024>
    reg:hasUnconstrained <http://rdaregistry.info/Elements/u/P60450> ;
    reg:lexicalAlias "http://rdaregistry.info/Elements/i/restorationist"@en ;
    reg:name "restorationist"@en ;
    reg:status <http://metadataregistry.org/uri/RegStatus/1001> ;
    a rdf:Property ;
    rdfs:domain <http://rdaregistry.info/Elements/c/C10003> ;
    rdfs:isDefinedBy <http://rdaregistry.info/Elements/i/> ;
    rdfs:label "has restorationist"@en ;
    rdfs:range <http://rdaregistry.info/Elements/c/C10002> ;
    rdfs:subPropertyOf <http://rdaregistry.info/Elements/i/P40023>, <http://rdaregistry.info/Elements/u/P60450> ;
    owl:inverseOf <http://rdaregistry.info/Elements/a/P50206> ;
    skos:definition "Relates an item to a person, family, or corporate body responsible for the set of technical, editorial, and intellectual procedures aimed at compensating for the degradation of an item by bringing it back to a state as close as possible to its original condition."@en .

<http://rdaregistry.info/Elements/i/P40025>
    reg:hasUnconstrained <http://rdaregistry.info/Elements/u/P60455> ;
    reg:lexicalAlias "http://rdaregistry.info/Elements/i/dedicateeOfItem"@en ;
    reg:name "dedicateeOfItem"@en ;
    reg:status <http://metadataregistry.org/uri/RegStatus/1001> ;
    a rdf:Property ;
    rdfs:domain <http://rdaregistry.info/Elements/c/C10003> ;
    rdfs:isDefinedBy <http://rdaregistry.info/Elements/i/> ;
    rdfs:label "has dedicatee (item) "@en ;
    rdfs:range <http://rdaregistry.info/Elements/c/C10002> ;
    rdfs:subPropertyOf <http://rdaregistry.info/Elements/i/P40023>, <http://rdaregistry.info/Elements/u/P60455> ;
    owl:inverseOf <http://rdaregistry.info/Elements/a/P50210> ;
    skos:definition "Relates an item to a person, family, or corporate body to whom an item is dedicated."@en .

<http://rdaregistry.info/Elements/i/P40026>
    reg:hasUnconstrained <http://rdaregistry.info/Elements/u/P60176> ;
    reg:lexicalAlias "http://rdaregistry.info/Elements/i/custodialHistoryOfItem"@en ;
    reg:name "custodialHistoryOfItem"@en ;
    reg:status <http://metadataregistry.org/uri/RegStatus/1001> ;
    a rdf:Property ;
    rdfs:domain <http://rdaregistry.info/Elements/c/C10003> ;
    rdfs:isDefinedBy <http://rdaregistry.info/Elements/i/> ;
    rdfs:label "has custodial history of item"@en ;
    skos:definition "Relates an item to a record of previous ownership or custodianship of an item."@en .

<http://rdaregistry.info/Elements/i/P40027>
    reg:hasUnconstrained <http://rdaregistry.info/Elements/u/P60469> ;
    reg:lexicalAlias "http://rdaregistry.info/Elements/i/electronicReproductionOfItem"@en ;
    reg:name "electronicReproductionOfItem"@en ;
    reg:status <http://metadataregistry.org/uri/RegStatus/1001> ;
    a rdf:Property ;
    rdfs:domain <http://rdaregistry.info/Elements/c/C10003> ;
    rdfs:isDefinedBy <http://rdaregistry.info/Elements/i/> ;
    rdfs:label "is electronic reproduction of (item)"@en ;
    rdfs:range <http://rdaregistry.info/Elements/c/C10003> ;
    rdfs:subPropertyOf <http://rdaregistry.info/Elements/i/P40042>, <http://rdaregistry.info/Elements/u/P60469> ;
    owl:inverseOf <http://rdaregistry.info/Elements/i/P40057> ;
    skos:definition "Relates an item to an item in an analog format that is transferred to a digital format."@en .

<http://rdaregistry.info/Elements/i/P40028>
    reg:hasUnconstrained <http://rdaregistry.info/Elements/u/P60470> ;
    reg:lexicalAlias "http://rdaregistry.info/Elements/i/noteOnItem"@en ;
    reg:name "noteOnItem"@en ;
    reg:status <http://metadataregistry.org/uri/RegStatus/1001> ;
    a rdf:Property ;
    rdfs:domain <http://rdaregistry.info/Elements/c/C10003> ;
    rdfs:isDefinedBy <http://rdaregistry.info/Elements/i/> ;
    rdfs:label "has note on item"@en ;
    skos:definition "Relates an item to a note providing information on attributes of the item."@en .

<http://rdaregistry.info/Elements/i/P40029>
    reg:hasSubproperty <http://rdaregistry.info/Elements/i/P40032>, <http://rdaregistry.info/Elements/i/P40035>, <http://rdaregistry.info/Elements/i/P40036> ;
    reg:hasUnconstrained <http://rdaregistry.info/Elements/u/P60196> ;
    reg:lexicalAlias "http://rdaregistry.info/Elements/i/accompaniedByItem"@en ;
    reg:name "accompaniedByItem"@en ;
    reg:status <http://metadataregistry.org/uri/RegStatus/1001> ;
    a rdf:Property ;
    rdfs:domain <http://rdaregistry.info/Elements/c/C10003> ;
    rdfs:isDefinedBy <http://rdaregistry.info/Elements/i/> ;
    rdfs:label "is accompanied by (item)"@en ;
    rdfs:range <http://rdaregistry.info/Elements/c/C10003> ;
    rdfs:subPropertyOf <http://rdaregistry.info/Elements/i/P40051>, <http://rdaregistry.info/Elements/u/P60196> ;
    owl:inverseOf <http://rdaregistry.info/Elements/i/P40029> ;
    skos:definition "Relates an item to an item brought together with another item after being issued."@en .

<http://rdaregistry.info/Elements/i/P40030>
    reg:hasSubproperty <http://rdaregistry.info/Elements/i/P40033>, <http://rdaregistry.info/Elements/i/P40037>, <http://rdaregistry.info/Elements/i/P40040>, <http://rdaregistry.info/Elements/i/P40041>, <http://rdaregistry.info/Elements/i/P40043> ;
    reg:name "descriptionOfItem"@en ;
    reg:status <http://metadataregistry.org/uri/RegStatus/1008> ;
    a rdf:Property ;
    rdfs:domain <http://rdaregistry.info/Elements/c/C10003> ;
    rdfs:isDefinedBy <http://rdaregistry.info/Elements/i/> ;
    rdfs:label "is description of (item)"@en ;
    rdfs:range <http://rdaregistry.info/Elements/c/C10003> ;
    rdfs:subPropertyOf <http://rdaregistry.info/Elements/i/P40052>, <http://rdaregistry.info/Elements/u/P60190> ;
    owl:sameAs <http://rdaregistry.info/Elements/i/descriptionOfItem> ;
    skos:definition "Relates an item to an item described by a describing work."@en .

<http://rdaregistry.info/Elements/i/P40031>
    reg:hasSubproperty <http://rdaregistry.info/Elements/i/P40042>, <http://rdaregistry.info/Elements/i/P40055> ;
    reg:hasUnconstrained <http://rdaregistry.info/Elements/u/P60191> ;
    reg:lexicalAlias "http://rdaregistry.info/Elements/i/equivalentItem"@en ;
    reg:name "equivalentItem"@en ;
    reg:status <http://metadataregistry.org/uri/RegStatus/1001> ;
    a rdf:Property ;
    rdfs:domain <http://rdaregistry.info/Elements/c/C10003> ;
    rdfs:isDefinedBy <http://rdaregistry.info/Elements/i/> ;
    rdfs:label "is equivalent (item)"@en ;
    rdfs:range <http://rdaregistry.info/Elements/c/C10003> ;
    rdfs:subPropertyOf <http://rdaregistry.info/Elements/i/P40053>, <http://rdaregistry.info/Elements/u/P60191> ;
    owl:inverseOf <http://rdaregistry.info/Elements/i/P40031> ;
    skos:definition "Relates an item to an item that exemplifies a manifestation that embodies the same expression of a work."@en .

<http://rdaregistry.info/Elements/i/P40032>
    reg:hasUnconstrained <http://rdaregistry.info/Elements/u/P60237> ;
    reg:lexicalAlias "http://rdaregistry.info/Elements/i/boundWith"@en ;
    reg:name "boundWith"@en ;
    reg:status <http://metadataregistry.org/uri/RegStatus/1001> ;
    a rdf:Property ;
    rdfs:domain <http://rdaregistry.info/Elements/c/C10003> ;
    rdfs:isDefinedBy <http://rdaregistry.info/Elements/i/> ;
    rdfs:label "is bound with"@en ;
    rdfs:range <http://rdaregistry.info/Elements/c/C10003> ;
    rdfs:subPropertyOf <http://rdaregistry.info/Elements/i/P40029>, <http://rdaregistry.info/Elements/u/P60237> ;
    owl:inverseOf <http://rdaregistry.info/Elements/i/P40032> ;
    skos:definition "Relates an item to an item that has been bound within the same binding as the item being described."@en .

<http://rdaregistry.info/Elements/i/P40033>
    reg:name "analysisOfItem"@en ;
    reg:status <http://metadataregistry.org/uri/RegStatus/1008> ;
    a rdf:Property ;
    rdfs:domain <http://rdaregistry.info/Elements/c/C10003> ;
    rdfs:isDefinedBy <http://rdaregistry.info/Elements/i/> ;
    rdfs:label "is analysis of (item)"@en ;
    rdfs:range <http://rdaregistry.info/Elements/c/C10003> ;
    rdfs:subPropertyOf <http://rdaregistry.info/Elements/i/P40030>, <http://rdaregistry.info/Elements/u/P60239> ;
    owl:sameAs <http://rdaregistry.info/Elements/i/analysisOfItem> ;
    skos:definition "Relates an item to an item that has been examined to identify its components and their relations."@en .

<http://rdaregistry.info/Elements/i/P40034>
    reg:hasUnconstrained <http://rdaregistry.info/Elements/u/P60249> ;
    reg:lexicalAlias "http://rdaregistry.info/Elements/i/containerOfItem"@en ;
    reg:name "containerOfItem"@en ;
    reg:status <http://metadataregistry.org/uri/RegStatus/1001> ;
    a rdf:Property ;
    rdfs:domain <http://rdaregistry.info/Elements/c/C10003> ;
    rdfs:isDefinedBy <http://rdaregistry.info/Elements/i/> ;
    rdfs:label "is container of (item)"@en ;
    rdfs:range <http://rdaregistry.info/Elements/c/C10003> ;
    rdfs:subPropertyOf <http://rdaregistry.info/Elements/i/P40054>, <http://rdaregistry.info/Elements/u/P60249> ;
    owl:inverseOf <http://rdaregistry.info/Elements/i/P40009> ;
    skos:definition "Relates an item to an item that is a discrete component of a larger item."@en .

<http://rdaregistry.info/Elements/i/P40035>
    reg:hasUnconstrained <http://rdaregistry.info/Elements/u/P60257> ;
    reg:lexicalAlias "http://rdaregistry.info/Elements/i/onDiscWithItem"@en ;
    reg:name "onDiscWithItem"@en ;
    reg:status <http://metadataregistry.org/uri/RegStatus/1001> ;
    a rdf:Property ;
    rdfs:domain <http://rdaregistry.info/Elements/c/C10003> ;
    rdfs:isDefinedBy <http://rdaregistry.info/Elements/i/> ;
    rdfs:label "is on disc with (item)"@en ;
    rdfs:range <http://rdaregistry.info/Elements/c/C10003> ;
    rdfs:subPropertyOf <http://rdaregistry.info/Elements/i/P40029>, <http://rdaregistry.info/Elements/u/P60257> ;
    owl:inverseOf <http://rdaregistry.info/Elements/i/P40035> ;
    skos:definition "Relates an item to an item that is contained on the same disc with the item being described."@en .

<http://rdaregistry.info/Elements/i/P40036>
    reg:hasUnconstrained <http://rdaregistry.info/Elements/u/P60258> ;
    reg:lexicalAlias "http://rdaregistry.info/Elements/i/filmedWithItem"@en ;
    reg:name "filmedWithItem"@en ;
    reg:status <http://metadataregistry.org/uri/RegStatus/1001> ;
    a rdf:Property ;
    rdfs:domain <http://rdaregistry.info/Elements/c/C10003> ;
    rdfs:isDefinedBy <http://rdaregistry.info/Elements/i/> ;
    rdfs:label "is filmed with (item)"@en ;
    rdfs:range <http://rdaregistry.info/Elements/c/C10003> ;
    rdfs:subPropertyOf <http://rdaregistry.info/Elements/i/P40029>, <http://rdaregistry.info/Elements/u/P60258> ;
    owl:inverseOf <http://rdaregistry.info/Elements/i/P40036> ;
    skos:definition "Relates an item to an item that is contained on the same microform with the item being described."@en .

<http://rdaregistry.info/Elements/i/P40037>
    reg:name "evaluationOfItem"@en ;
    reg:status <http://metadataregistry.org/uri/RegStatus/1008> ;
    a rdf:Property ;
    rdfs:domain <http://rdaregistry.info/Elements/c/C10003> ;
    rdfs:isDefinedBy <http://rdaregistry.info/Elements/i/> ;
    rdfs:label "is evaluation of (item)"@en ;
    rdfs:range <http://rdaregistry.info/Elements/c/C10003> ;
    rdfs:subPropertyOf <http://rdaregistry.info/Elements/i/P40030>, <http://rdaregistry.info/Elements/u/P60255> ;
    owl:sameAs <http://rdaregistry.info/Elements/i/evaluationOfItem> ;
    skos:definition "Relates an item to an item that is examined or judged."@en .

<http://rdaregistry.info/Elements/i/P40038>
    reg:hasUnconstrained <http://rdaregistry.info/Elements/u/P60168> ;
    reg:lexicalAlias "http://rdaregistry.info/Elements/i/reprintOfItem"@en ;
    reg:name "reprintOfItem"@en ;
    reg:status <http://metadataregistry.org/uri/RegStatus/1001> ;
    a rdf:Property ;
    rdfs:domain <http://rdaregistry.info/Elements/c/C10003> ;
    rdfs:isDefinedBy <http://rdaregistry.info/Elements/i/> ;
    rdfs:label "is reprint of (item)"@en ;
    rdfs:range <http://rdaregistry.info/Elements/c/C10003> ;
    rdfs:subPropertyOf <http://rdaregistry.info/Elements/i/P40042>, <http://rdaregistry.info/Elements/u/P60168> ;
    owl:inverseOf <http://rdaregistry.info/Elements/i/P40060> ;
    skos:definition "Relates an item to an item that exemplifies a printed manifestation that is used as the basis for a reissue of a manifestation."@en .

<http://rdaregistry.info/Elements/i/P40039>
    reg:hasUnconstrained <http://rdaregistry.info/Elements/u/P60287> ;
    reg:lexicalAlias "http://rdaregistry.info/Elements/i/digitalTransferOfItem"@en ;
    reg:name "digitalTransferOfItem"@en ;
    reg:status <http://metadataregistry.org/uri/RegStatus/1001> ;
    a rdf:Property ;
    rdfs:domain <http://rdaregistry.info/Elements/c/C10003> ;
    rdfs:isDefinedBy <http://rdaregistry.info/Elements/i/> ;
    rdfs:label "is digital transfer of (item)"@en ;
    rdfs:range <http://rdaregistry.info/Elements/c/C10003> ;
    rdfs:subPropertyOf <http://rdaregistry.info/Elements/i/P40042>, <http://rdaregistry.info/Elements/u/P60287> ;
    owl:inverseOf <http://rdaregistry.info/Elements/i/P40056> ;
    skos:definition "Relates an item to an item in a digital format that is transferred to another digital format. "@en .

<http://rdaregistry.info/Elements/i/P40040>
    reg:name "reviewOfItem"@en ;
    reg:status <http://metadataregistry.org/uri/RegStatus/1008> ;
    a rdf:Property ;
    rdfs:domain <http://rdaregistry.info/Elements/c/C10003> ;
    rdfs:isDefinedBy <http://rdaregistry.info/Elements/i/> ;
    rdfs:label "is review of (item)"@en ;
    rdfs:range <http://rdaregistry.info/Elements/c/C10003> ;
    rdfs:subPropertyOf <http://rdaregistry.info/Elements/i/P40030>, <http://rdaregistry.info/Elements/u/P60288> ;
    owl:sameAs <http://rdaregistry.info/Elements/i/reviewOfItem> ;
    skos:definition "Relates an item to an item used as the basis for a brief evaluation."@en .

<http://rdaregistry.info/Elements/i/P40041>
    reg:name "critiqueOfItem"@en ;
    reg:status <http://metadataregistry.org/uri/RegStatus/1008> ;
    a rdf:Property ;
    rdfs:domain <http://rdaregistry.info/Elements/c/C10003> ;
    rdfs:isDefinedBy <http://rdaregistry.info/Elements/i/> ;
    rdfs:label "is critique of (item)"@en ;
    rdfs:range <http://rdaregistry.info/Elements/c/C10003> ;
    rdfs:subPropertyOf <http://rdaregistry.info/Elements/i/P40030>, <http://rdaregistry.info/Elements/u/P60292> ;
    owl:sameAs <http://rdaregistry.info/Elements/i/critiqueOfItem> ;
    skos:definition "Relates an item to an item used as the basis for a critical evaluation."@en .

<http://rdaregistry.info/Elements/i/P40042>
    reg:hasSubproperty <http://rdaregistry.info/Elements/i/P40027>, <http://rdaregistry.info/Elements/i/P40038>, <http://rdaregistry.info/Elements/i/P40039>, <http://rdaregistry.info/Elements/i/P40045> ;
    reg:hasUnconstrained <http://rdaregistry.info/Elements/u/P60297> ;
    reg:lexicalAlias "http://rdaregistry.info/Elements/i/reproductionOfItem"@en ;
    reg:name "reproductionOfItem"@en ;
    reg:status <http://metadataregistry.org/uri/RegStatus/1001> ;
    a rdf:Property ;
    rdfs:domain <http://rdaregistry.info/Elements/c/C10003> ;
    rdfs:isDefinedBy <http://rdaregistry.info/Elements/i/> ;
    rdfs:label "is reproduction of (item)"@en ;
    rdfs:range <http://rdaregistry.info/Elements/c/C10003> ;
    rdfs:subPropertyOf <http://rdaregistry.info/Elements/i/P40031>, <http://rdaregistry.info/Elements/u/P60297> ;
    owl:inverseOf <http://rdaregistry.info/Elements/i/P40055> ;
    skos:definition "Relates an item to an item that is used as the basis for a reproduction."@en .

<http://rdaregistry.info/Elements/i/P40043>
    reg:name "commentaryOnItem"@en ;
    reg:status <http://metadataregistry.org/uri/RegStatus/1008> ;
    a rdf:Property ;
    rdfs:domain <http://rdaregistry.info/Elements/c/C10003> ;
    rdfs:isDefinedBy <http://rdaregistry.info/Elements/i/> ;
    rdfs:label "is commentary on (item)"@en ;
    rdfs:range <http://rdaregistry.info/Elements/c/C10003> ;
    rdfs:subPropertyOf <http://rdaregistry.info/Elements/i/P40030>, <http://rdaregistry.info/Elements/u/P60298> ;
    owl:sameAs <http://rdaregistry.info/Elements/i/commentaryOnItem> ;
    skos:definition "Relates an item to an item used as the basis for a set of explanatory or critical notes."@en .

<http://rdaregistry.info/Elements/i/P40044>
    reg:hasUnconstrained <http://rdaregistry.info/Elements/u/P60299> ;
    reg:lexicalAlias "http://rdaregistry.info/Elements/i/preservationFacsimileOfItem"@en ;
    reg:name "preservationFacsimileOfItem"@en ;
    reg:status <http://metadataregistry.org/uri/RegStatus/1001> ;
    a rdf:Property ;
    rdfs:domain <http://rdaregistry.info/Elements/c/C10003> ;
    rdfs:isDefinedBy <http://rdaregistry.info/Elements/i/> ;
    rdfs:label "is preservation facsimile of (item)"@en ;
    rdfs:range <http://rdaregistry.info/Elements/c/C10003> ;
    rdfs:subPropertyOf <http://rdaregistry.info/Elements/i/P40045>, <http://rdaregistry.info/Elements/u/P60299> ;
    owl:inverseOf <http://rdaregistry.info/Elements/i/P40059> ;
    skos:definition "Relates an item to an item that is used as the basis for an exact reproduction on preservation-quality media, such as acid-free permanent or archival paper."@en .

<http://rdaregistry.info/Elements/i/P40045>
    reg:hasSubproperty <http://rdaregistry.info/Elements/i/P40044> ;
    reg:hasUnconstrained <http://rdaregistry.info/Elements/u/P60301> ;
    reg:lexicalAlias "http://rdaregistry.info/Elements/i/facsimileOfItem"@en ;
    reg:name "facsimileOfItem"@en ;
    reg:status <http://metadataregistry.org/uri/RegStatus/1001> ;
    a rdf:Property ;
    rdfs:domain <http://rdaregistry.info/Elements/c/C10003> ;
    rdfs:isDefinedBy <http://rdaregistry.info/Elements/i/> ;
    rdfs:label "is facsimile of (item)"@en ;
    rdfs:range <http://rdaregistry.info/Elements/c/C10003> ;
    rdfs:subPropertyOf <http://rdaregistry.info/Elements/i/P40042>, <http://rdaregistry.info/Elements/u/P60301> ;
    owl:inverseOf <http://rdaregistry.info/Elements/i/P40058> ;
    skos:definition "Relates an item to an item that is used as the basis for an exact reproduction."@en .

<http://rdaregistry.info/Elements/i/P40046>
    reg:hasSubproperty <http://rdaregistry.info/Elements/i/P40052>, <http://rdaregistry.info/Elements/i/P40053>, <http://rdaregistry.info/Elements/i/P40054> ;
    reg:lexicalAlias "http://rdaregistry.info/Elements/i/relatedItemOfItem"@en ;
    reg:name "relatedItemOfItem"@en ;
    reg:status <http://metadataregistry.org/uri/RegStatus/1001> ;
    a rdf:Property ;
    rdfs:domain <http://rdaregistry.info/Elements/c/C10003> ;
    rdfs:isDefinedBy <http://rdaregistry.info/Elements/i/> ;
    rdfs:label "has related item of item"@en ;
    rdfs:range <http://rdaregistry.info/Elements/c/C10003> ;
    owl:inverseOf <http://rdaregistry.info/Elements/i/P40046> ;
    skos:definition "Relates an item to an item, represented by an identifier or a description, that is related to the item being described (e.g., an item used as the basis for a microform reproduction)."@en .

<http://rdaregistry.info/Elements/i/P40047>
    reg:hasUnconstrained <http://rdaregistry.info/Elements/u/P60496> ;
    reg:lexicalAlias "http://rdaregistry.info/Elements/i/restrictionsOnAccessToItem"@en ;
    reg:name "restrictionsOnAccessToItem"@en ;
    reg:status <http://metadataregistry.org/uri/RegStatus/1001> ;
    a rdf:Property ;
    rdfs:domain <http://rdaregistry.info/Elements/c/C10003> ;
    rdfs:isDefinedBy <http://rdaregistry.info/Elements/i/> ;
    rdfs:label "has restrictions on access to item"@en ;
    skos:definition "Relates an item to limitations placed on access to an item."@en .

<http://rdaregistry.info/Elements/i/P40048>
    reg:hasUnconstrained <http://rdaregistry.info/Elements/u/P60497> ;
    reg:lexicalAlias "http://rdaregistry.info/Elements/i/restrictionsOnUseOfItem"@en ;
    reg:name "restrictionsOnUseOfItem"@en ;
    reg:status <http://metadataregistry.org/uri/RegStatus/1001> ;
    a rdf:Property ;
    rdfs:domain <http://rdaregistry.info/Elements/c/C10003> ;
    rdfs:isDefinedBy <http://rdaregistry.info/Elements/i/> ;
    rdfs:label "has restrictions on use of item"@en ;
    skos:definition "Relates an item to limitations placed on uses such as reproduction, publication, exhibition, etc."@en .

<http://rdaregistry.info/Elements/i/P40049>
    reg:lexicalAlias "http://rdaregistry.info/Elements/i/manifestationExemplified"@en ;
    reg:name "manifestationExemplified"@en ;
    reg:status <http://metadataregistry.org/uri/RegStatus/1001> ;
    a rdf:Property ;
    rdfs:domain <http://rdaregistry.info/Elements/c/C10003> ;
    rdfs:isDefinedBy <http://rdaregistry.info/Elements/i/> ;
    rdfs:label "has manifestation exemplified"@en ;
    rdfs:range <http://rdaregistry.info/Elements/c/C10007> ;
    owl:inverseOf <http://rdaregistry.info/Elements/m/P30103> ;
    skos:definition "Relates an item to the manifestation exemplified by an item."@en .

<http://rdaregistry.info/Elements/i/P40050>
    reg:hasUnconstrained <http://rdaregistry.info/Elements/u/P60583> ;
    reg:lexicalAlias "http://rdaregistry.info/Elements/i/immediateSourceOfAcquisitionOfItem"@en ;
    reg:name "immediateSourceOfAcquisitionOfItem"@en ;
    reg:status <http://metadataregistry.org/uri/RegStatus/1001> ;
    a rdf:Property ;
    rdfs:domain <http://rdaregistry.info/Elements/c/C10003> ;
    rdfs:isDefinedBy <http://rdaregistry.info/Elements/i/> ;
    rdfs:label "has immediate source of acquisition of item"@en ;
    skos:definition "Relates an item to the source from which the agency directly acquired an item and the circumstances under which it was received."@en .

<http://rdaregistry.info/Elements/i/P40051>
    reg:hasSubproperty <http://rdaregistry.info/Elements/i/P40029> ;
    reg:hasUnconstrained <http://rdaregistry.info/Elements/u/P60709> ;
    reg:lexicalAlias "http://rdaregistry.info/Elements/i/accompanyingItemRelationship"@en ;
    reg:name "accompanyingItemRelationship"@en ;
    reg:status <http://metadataregistry.org/uri/RegStatus/1001> ;
    a rdf:Property ;
    rdfs:domain <http://rdaregistry.info/Elements/c/C10003> ;
    rdfs:isDefinedBy <http://rdaregistry.info/Elements/i/> ;
    rdfs:label "has accompanying item relationship with"@en ;
    rdfs:range <http://rdaregistry.info/Elements/c/C10003> ;
    rdfs:subPropertyOf <http://rdaregistry.info/Elements/i/P40046> ;
    owl:inverseOf <http://rdaregistry.info/Elements/i/P40051> ;
    skos:definition "Relates an item to an item that accompanies or is accompanied by the item."@en .

<http://rdaregistry.info/Elements/i/P40052>
    reg:hasSubproperty <http://rdaregistry.info/Elements/i/P40030> ;
    reg:name "descriptiveItemRelationship"@en ;
    reg:status <http://metadataregistry.org/uri/RegStatus/1008> ;
    a rdf:Property ;
    rdfs:domain <http://rdaregistry.info/Elements/c/C10003> ;
    rdfs:isDefinedBy <http://rdaregistry.info/Elements/i/> ;
    rdfs:label "has descriptive item relationship with"@en ;
    rdfs:range <http://rdaregistry.info/Elements/c/C10003> ;
    rdfs:subPropertyOf <http://rdaregistry.info/Elements/i/P40046>, <http://rdaregistry.info/Elements/u/P60711> ;
    owl:sameAs <http://rdaregistry.info/Elements/i/descriptiveItemRelationship> ;
    skos:definition "Relates an item to a work that is a description of the item."@en .

<http://rdaregistry.info/Elements/i/P40053>
    reg:hasSubproperty <http://rdaregistry.info/Elements/i/P40031> ;
    reg:hasUnconstrained <http://rdaregistry.info/Elements/u/P60712> ;
    reg:lexicalAlias "http://rdaregistry.info/Elements/i/equivalentItemRelationship"@en ;
    reg:name "equivalentItemRelationship"@en ;
    reg:status <http://metadataregistry.org/uri/RegStatus/1001> ;
    a rdf:Property ;
    rdfs:domain <http://rdaregistry.info/Elements/c/C10003> ;
    rdfs:isDefinedBy <http://rdaregistry.info/Elements/i/> ;
    rdfs:label "has equivalent item relationship with"@en ;
    rdfs:range <http://rdaregistry.info/Elements/c/C10003> ;
    rdfs:subPropertyOf <http://rdaregistry.info/Elements/i/P40046>, <http://rdaregistry.info/Elements/u/P60712> ;
    owl:inverseOf <http://rdaregistry.info/Elements/i/P40053> ;
    skos:definition "Relates an item to an item that is equivalent to the item."@en .

<http://rdaregistry.info/Elements/i/P40054>
    reg:hasSubproperty <http://rdaregistry.info/Elements/i/P40009>, <http://rdaregistry.info/Elements/i/P40034> ;
    reg:hasUnconstrained <http://rdaregistry.info/Elements/u/P60714> ;
    reg:lexicalAlias "http://rdaregistry.info/Elements/i/wholePartItemRelationship"@en ;
    reg:name "wholePartItemRelationship"@en ;
    reg:status <http://metadataregistry.org/uri/RegStatus/1001> ;
    a rdf:Property ;
    rdfs:domain <http://rdaregistry.info/Elements/c/C10003> ;
    rdfs:isDefinedBy <http://rdaregistry.info/Elements/i/> ;
    rdfs:label "has whole-part item relationship with"@en ;
    rdfs:range <http://rdaregistry.info/Elements/c/C10003> ;
    rdfs:subPropertyOf <http://rdaregistry.info/Elements/i/P40046>, <http://rdaregistry.info/Elements/u/P60714> ;
    skos:definition "Relates an item to an item that is contained in or contains the item."@en .

<http://rdaregistry.info/Elements/i/P40055>
    reg:hasSubproperty <http://rdaregistry.info/Elements/i/P40056>, <http://rdaregistry.info/Elements/i/P40057>, <http://rdaregistry.info/Elements/i/P40058>, <http://rdaregistry.info/Elements/i/P40060> ;
    reg:hasUnconstrained <http://rdaregistry.info/Elements/u/P60272> ;
    reg:lexicalAlias "http://rdaregistry.info/Elements/i/reproducedAsItem"@en ;
    reg:name "reproducedAsItem"@en ;
    reg:status <http://metadataregistry.org/uri/RegStatus/1001> ;
    a rdf:Property ;
    rdfs:domain <http://rdaregistry.info/Elements/c/C10003> ;
    rdfs:isDefinedBy <http://rdaregistry.info/Elements/i/> ;
    rdfs:label "is reproduced as (item)"@en ;
    rdfs:range <http://rdaregistry.info/Elements/c/C10003> ;
    rdfs:subPropertyOf <http://rdaregistry.info/Elements/i/P40031> ;
    owl:inverseOf <http://rdaregistry.info/Elements/i/P40042> ;
    skos:definition "Relates an item to an item that reproduces another item."@en .

<http://rdaregistry.info/Elements/i/P40056>
    reg:hasUnconstrained <http://rdaregistry.info/Elements/u/P60200> ;
    reg:lexicalAlias "http://rdaregistry.info/Elements/i/digitalTransferItem"@en ;
    reg:name "digitalTransferItem"@en ;
    reg:status <http://metadataregistry.org/uri/RegStatus/1001> ;
    a rdf:Property ;
    rdfs:domain <http://rdaregistry.info/Elements/c/C10003> ;
    rdfs:isDefinedBy <http://rdaregistry.info/Elements/i/> ;
    rdfs:label "is digital transfer (item)"@en ;
    rdfs:range <http://rdaregistry.info/Elements/c/C10003> ;
    rdfs:subPropertyOf <http://rdaregistry.info/Elements/i/P40055> ;
    owl:inverseOf <http://rdaregistry.info/Elements/i/P40039> ;
    skos:definition "Relates an item to an item in a digital format that results from the transfer of an item in another digital format."@en .

<http://rdaregistry.info/Elements/i/P40057>
    reg:hasUnconstrained <http://rdaregistry.info/Elements/u/P60083> ;
    reg:lexicalAlias "http://rdaregistry.info/Elements/i/electronicReproductionItem"@en ;
    reg:name "electronicReproductionItem"@en ;
    reg:status <http://metadataregistry.org/uri/RegStatus/1001> ;
    a rdf:Property ;
    rdfs:domain <http://rdaregistry.info/Elements/c/C10003> ;
    rdfs:isDefinedBy <http://rdaregistry.info/Elements/i/> ;
    rdfs:label "is electronic reproduction (item)"@en ;
    rdfs:range <http://rdaregistry.info/Elements/c/C10003> ;
    rdfs:subPropertyOf <http://rdaregistry.info/Elements/i/P40055> ;
    owl:inverseOf <http://rdaregistry.info/Elements/i/P40027> ;
    skos:definition "Relates an item to an item in a digital format that is the result of the transfer of an item in analog format."@en .

<http://rdaregistry.info/Elements/i/P40058>
    reg:hasSubproperty <http://rdaregistry.info/Elements/i/P40059> ;
    reg:hasUnconstrained <http://rdaregistry.info/Elements/u/P60217> ;
    reg:lexicalAlias "http://rdaregistry.info/Elements/i/facsimileItem"@en ;
    reg:name "facsimileItem"@en ;
    reg:status <http://metadataregistry.org/uri/RegStatus/1001> ;
    a rdf:Property ;
    rdfs:domain <http://rdaregistry.info/Elements/c/C10003> ;
    rdfs:isDefinedBy <http://rdaregistry.info/Elements/i/> ;
    rdfs:label "is facsimile (item)"@en ;
    rdfs:range <http://rdaregistry.info/Elements/c/C10003> ;
    rdfs:subPropertyOf <http://rdaregistry.info/Elements/i/P40055> ;
    owl:inverseOf <http://rdaregistry.info/Elements/i/P40045> ;
    skos:definition "Relates an item to an item that exactly reproduces an item."@en .

<http://rdaregistry.info/Elements/i/P40059>
    reg:hasUnconstrained <http://rdaregistry.info/Elements/u/P60179> ;
    reg:lexicalAlias "http://rdaregistry.info/Elements/i/preservationFacsimileItem"@en ;
    reg:name "preservationFacsimileItem"@en ;
    reg:status <http://metadataregistry.org/uri/RegStatus/1001> ;
    a rdf:Property ;
    rdfs:domain <http://rdaregistry.info/Elements/c/C10003> ;
    rdfs:isDefinedBy <http://rdaregistry.info/Elements/i/> ;
    rdfs:label "is preservation facsimile (item)"@en ;
    rdfs:range <http://rdaregistry.info/Elements/c/C10003> ;
    rdfs:subPropertyOf <http://rdaregistry.info/Elements/i/P40058> ;
    owl:inverseOf <http://rdaregistry.info/Elements/i/P40044> ;
    skos:definition "Relates an item to an item that consists of an exact reproduction on preservation-quality media, such as acid-free permanent or archival paper."@en .

<http://rdaregistry.info/Elements/i/P40060>
    reg:hasUnconstrained <http://rdaregistry.info/Elements/u/P60271> ;
    reg:lexicalAlias "http://rdaregistry.info/Elements/i/reprintedAsItem"@en ;
    reg:name "reprintedAsItem"@en ;
    reg:status <http://metadataregistry.org/uri/RegStatus/1001> ;
    a rdf:Property ;
    rdfs:domain <http://rdaregistry.info/Elements/c/C10003> ;
    rdfs:isDefinedBy <http://rdaregistry.info/Elements/i/> ;
    rdfs:label "is reprinted as (item)"@en ;
    rdfs:range <http://rdaregistry.info/Elements/c/C10003> ;
    rdfs:subPropertyOf <http://rdaregistry.info/Elements/i/P40055> ;
    owl:inverseOf <http://rdaregistry.info/Elements/i/P40038> ;
    skos:definition "Relates an item to an item that is a reissue of an item that exemplifies another printed manifestation."@en .

<http://rdaregistry.info/Elements/i/P40061>
    reg:hasSubproperty <http://rdaregistry.info/Elements/i/P40062> ;
    reg:hasUnconstrained <http://rdaregistry.info/Elements/u/P60806> ;
    reg:lexicalAlias "http://rdaregistry.info/Elements/i/subjectOfItem"@en ;
    reg:name "subjectOfItem"@en ;
    reg:status <http://metadataregistry.org/uri/RegStatus/1001> ;
    a rdf:Property ;
    rdfs:domain <http://rdaregistry.info/Elements/c/C10003> ;
    rdfs:isDefinedBy <http://rdaregistry.info/Elements/i/> ;
    rdfs:label "is subject of (item)"@en ;
    rdfs:range <http://rdaregistry.info/Elements/c/C10001> ;
    rdfs:subPropertyOf <http://rdaregistry.info/Elements/w/P10283> ;
    owl:inverseOf <http://rdaregistry.info/Elements/w/P10260> ;
    skos:definition "Relates an item to a work that is about the item."@en .

<http://rdaregistry.info/Elements/i/P40062>
    reg:hasSubproperty <http://rdaregistry.info/Elements/i/P40063>, <http://rdaregistry.info/Elements/i/P40064>, <http://rdaregistry.info/Elements/i/P40065>, <http://rdaregistry.info/Elements/i/P40066>, <http://rdaregistry.info/Elements/i/P40067> ;
    reg:hasUnconstrained <http://rdaregistry.info/Elements/u/P60215> ;
    reg:lexicalAlias "http://rdaregistry.info/Elements/i/describedInItem"@en ;
    reg:name "describedInItem"@en ;
    reg:status <http://metadataregistry.org/uri/RegStatus/1001> ;
    a rdf:Property ;
    rdfs:domain <http://rdaregistry.info/Elements/c/C10003> ;
    rdfs:isDefinedBy <http://rdaregistry.info/Elements/i/> ;
    rdfs:label "is described in (item)"@en ;
    rdfs:range <http://rdaregistry.info/Elements/c/C10001> ;
    rdfs:subPropertyOf <http://rdaregistry.info/Elements/i/P40061> ;
    owl:inverseOf <http://rdaregistry.info/Elements/w/P10265> ;
    skos:definition "Relates an item to a work that describes a described item."@en .

<http://rdaregistry.info/Elements/i/P40063>
    reg:hasUnconstrained <http://rdaregistry.info/Elements/u/P60219> ;
    reg:lexicalAlias "http://rdaregistry.info/Elements/i/analysedInItem"@en ;
    reg:name "analysedInItem"@en ;
    reg:status <http://metadataregistry.org/uri/RegStatus/1001> ;
    a rdf:Property ;
    rdfs:domain <http://rdaregistry.info/Elements/c/C10003> ;
    rdfs:isDefinedBy <http://rdaregistry.info/Elements/i/> ;
    rdfs:label "is analysed in (item)"@en ;
    rdfs:range <http://rdaregistry.info/Elements/c/C10001> ;
    rdfs:subPropertyOf <http://rdaregistry.info/Elements/i/P40062> ;
    owl:inverseOf <http://rdaregistry.info/Elements/w/P10266> ;
    skos:definition "Relates an item to a work that examines the source item to identify its components and their relations. "@en .

<http://rdaregistry.info/Elements/i/P40064>
    reg:hasUnconstrained <http://rdaregistry.info/Elements/u/P60213> ;
    reg:lexicalAlias "http://rdaregistry.info/Elements/i/commentaryInItem"@en ;
    reg:name "commentaryInItem"@en ;
    reg:status <http://metadataregistry.org/uri/RegStatus/1001> ;
    a rdf:Property ;
    rdfs:domain <http://rdaregistry.info/Elements/c/C10003> ;
    rdfs:isDefinedBy <http://rdaregistry.info/Elements/i/> ;
    rdfs:label "is commentary in (item) "@en ;
    rdfs:range <http://rdaregistry.info/Elements/c/C10001> ;
    rdfs:subPropertyOf <http://rdaregistry.info/Elements/i/P40062> ;
    owl:inverseOf <http://rdaregistry.info/Elements/w/P10270> ;
    skos:definition "Relates an item to a work that contains a set of explanatory or critical notes on the described item."@en .

<http://rdaregistry.info/Elements/i/P40065>
    reg:hasUnconstrained <http://rdaregistry.info/Elements/u/P60212> ;
    reg:lexicalAlias "http://rdaregistry.info/Elements/i/critiquedInItem"@en ;
    reg:name "critiquedInItem"@en ;
    reg:status <http://metadataregistry.org/uri/RegStatus/1001> ;
    a rdf:Property ;
    rdfs:domain <http://rdaregistry.info/Elements/c/C10003> ;
    rdfs:isDefinedBy <http://rdaregistry.info/Elements/i/> ;
    rdfs:label "is critiqued in (item)"@en ;
    rdfs:range <http://rdaregistry.info/Elements/c/C10001> ;
    rdfs:subPropertyOf <http://rdaregistry.info/Elements/i/P40062> ;
    owl:inverseOf <http://rdaregistry.info/Elements/w/P10269> ;
    skos:definition "Relates an item to a work that contains a critical evaluation of the described item."@en .

<http://rdaregistry.info/Elements/i/P40066>
    reg:hasUnconstrained <http://rdaregistry.info/Elements/u/P60218> ;
    reg:lexicalAlias "http://rdaregistry.info/Elements/i/evaluatedInItem"@en ;
    reg:name "evaluatedInItem"@en ;
    reg:status <http://metadataregistry.org/uri/RegStatus/1001> ;
    a rdf:Property ;
    rdfs:domain <http://rdaregistry.info/Elements/c/C10003> ;
    rdfs:isDefinedBy <http://rdaregistry.info/Elements/i/> ;
    rdfs:label "is evaluated in (item)"@en ;
    rdfs:range <http://rdaregistry.info/Elements/c/C10001> ;
    rdfs:subPropertyOf <http://rdaregistry.info/Elements/i/P40062> ;
    owl:inverseOf <http://rdaregistry.info/Elements/w/P10267> ;
    skos:definition "Relates an item to a work that examines or judges the described item. "@en .

<http://rdaregistry.info/Elements/i/P40067>
    reg:hasUnconstrained <http://rdaregistry.info/Elements/u/P60211> ;
    reg:lexicalAlias "http://rdaregistry.info/Elements/i/reviewedInItem"@en ;
    reg:name "reviewedInItem"@en ;
    reg:status <http://metadataregistry.org/uri/RegStatus/1001> ;
    a rdf:Property ;
    rdfs:domain <http://rdaregistry.info/Elements/c/C10003> ;
    rdfs:isDefinedBy <http://rdaregistry.info/Elements/i/> ;
    rdfs:label "is reviewed in (item)"@en ;
    rdfs:range <http://rdaregistry.info/Elements/c/C10001> ;
    rdfs:subPropertyOf <http://rdaregistry.info/Elements/i/P40062> ;
    owl:inverseOf <http://rdaregistry.info/Elements/w/P10268> ;
    skos:definition "Relates an item to a work that contains a brief evaluation of the described item."@en .

