@prefix dc: <http://purl.org/dc/elements/1.1/> .
@prefix foaf: <http://xmlns.com/foaf/0.1/> .
@prefix rdakit: <http://metadataregistry.org/uri/profile/rdakit/> .
@prefix rdf: <http://www.w3.org/1999/02/22-rdf-syntax-ns#> .
@prefix rdfs: <http://www.w3.org/2000/01/rdf-schema#> .
@prefix reg: <http://metadataregistry.org/uri/profile/regap/> .
@prefix skos: <http://www.w3.org/2004/02/skos/core#> .
@prefix xml: <http://www.w3.org/XML/1998/namespace> .
@prefix xsd: <http://www.w3.org/2001/XMLSchema#> .

<http://rdaregistry.info/Elements/a/P50001> a rdf:Property ;
    rdfs:label "is respondent of"@en,
        "est le répondant de"@fr ;
    rdakit:instructionNumber "18.5" ;
    rdakit:toolkitDefinition "A thesis provided by the praeses in an academic disputation that is defended or opposed by a candidate for a degree."@en,
        "Candidat à un diplôme universitaire qui défend ou réfute la thèse proposée par le praeses lors d’une soutenance de thèse."@fr ;
    rdakit:toolkitLabel "respondent of"@en,
        "répondant de"@fr ;
    reg:hasSubproperty <http://rdaregistry.info/Elements/a/datatype/P50001>,
        <http://rdaregistry.info/Elements/a/object/P50001> ;
    reg:hasUnconstrained <http://rdaregistry.info/Elements/u/P60001> ;
    reg:lexicalAlias <http://rdaregistry.info/Elements/a/respondentOf.en> ;
    reg:name "respondentOf"@en ;
    reg:status <http://metadataregistry.org/uri/RegStatus/1001> ;
    rdfs:domain <http://rdaregistry.info/Elements/c/C10004> ;
    rdfs:isDefinedBy <http://rdaregistry.info/Elements/a/> ;
    rdfs:subPropertyOf <http://rdaregistry.info/Elements/a/P50204> ;
    skos:definition "Relates a candidate for a degree who defends or opposes a thesis provided by the praeses in an academic disputation to a work."@en,
        "Met un candidat à un diplôme universitaire qui défend ou réfute la thèse proposée par le praeses lors d’une soutenance de thèse en relation avec l’œuvre."@fr .

<http://rdaregistry.info/Elements/a/P50002> a rdf:Property ;
    rdfs:label "is appellee corporate body of"@en,
        "est la collectivité intimée de"@fr ;
    rdakit:instructionNumber "18.5" ;
    rdakit:toolkitDefinition "A legal work of a higher court recording a decision of a lower court that appeals against a corporate body."@en,
        "Collectivité contre laquelle un appel a été formé."@fr ;
    rdakit:toolkitLabel "appellee corporate body of"@en,
        "collectivité intimée de"@fr ;
    reg:hasSubproperty <http://rdaregistry.info/Elements/a/datatype/P50002>,
        <http://rdaregistry.info/Elements/a/object/P50002> ;
    reg:hasUnconstrained <http://rdaregistry.info/Elements/u/P60601> ;
    reg:lexicalAlias <http://rdaregistry.info/Elements/a/appelleeCorporateBodyOf.en> ;
    reg:name "appelleeCorporateBodyOf"@en ;
    reg:status <http://metadataregistry.org/uri/RegStatus/1001> ;
    rdfs:domain <http://rdaregistry.info/Elements/c/C10005> ;
    rdfs:isDefinedBy <http://rdaregistry.info/Elements/a/> ;
    rdfs:subPropertyOf <http://rdaregistry.info/Elements/a/P50087> ;
    skos:definition "Relates a corporate body against whom an appeal is taken on a decision of a lower court recorded in a legal work of a higher court to a work."@en,
        "Met une collectivité contre laquelle un appel a été formé en relation avec l’œuvre."@fr .

<http://rdaregistry.info/Elements/a/P50003> a rdf:Property ;
    rdfs:label "is degree granting institution of"@en,
        "est l’institution conférant des diplômes universitaires de"@fr ;
    rdakit:instructionNumber "18.5" ;
    rdakit:toolkitDefinition "An academic degree that is granted to a corporate body."@en,
        "Collectivité conférant un diplôme universitaire."@fr ;
    rdakit:toolkitLabel "degree granting institution of"@en,
        "institution conférant des diplômes universitaires de"@fr ;
    reg:hasSubproperty <http://rdaregistry.info/Elements/a/datatype/P50003>,
        <http://rdaregistry.info/Elements/a/object/P50003> ;
    reg:hasUnconstrained <http://rdaregistry.info/Elements/u/P60002> ;
    reg:lexicalAlias <http://rdaregistry.info/Elements/a/degreeGrantingInstitutionOf.en> ;
    reg:name "degreeGrantingInstitutionOf"@en ;
    reg:status <http://metadataregistry.org/uri/RegStatus/1001> ;
    rdfs:domain <http://rdaregistry.info/Elements/c/C10005> ;
    rdfs:isDefinedBy <http://rdaregistry.info/Elements/a/> ;
    rdfs:subPropertyOf <http://rdaregistry.info/Elements/a/P50131> ;
    skos:definition "Relates a corporate body granting an academic degree to a work."@en,
        "Met une collectivité conférant un diplôme universitaire en relation avec l’œuvre."@fr .

<http://rdaregistry.info/Elements/a/P50004> a rdf:Property ;
    rdfs:label "is host institution of"@en,
        "est l’institution hôte de"@fr ;
    rdakit:instructionNumber "18.5" ;
    rdakit:toolkitDefinition "An event, exhibit, conference, etc., which gave rise to a work that is hosted by a corporate body having little or no responsibility for the content of the work."@en,
        "Collectivité accueillant l’événement, l’exposition, le congrès, etc."@fr ;
    rdakit:toolkitLabel "host institution of"@en,
        "institution hôte de"@fr ;
    reg:hasSubproperty <http://rdaregistry.info/Elements/a/datatype/P50004>,
        <http://rdaregistry.info/Elements/a/object/P50004> ;
    reg:hasUnconstrained <http://rdaregistry.info/Elements/u/P60003> ;
    reg:lexicalAlias <http://rdaregistry.info/Elements/a/hostInstitutionOf.en> ;
    reg:name "hostInstitutionOf"@en ;
    reg:status <http://metadataregistry.org/uri/RegStatus/1001> ;
    rdfs:domain <http://rdaregistry.info/Elements/c/C10005> ;
    rdfs:isDefinedBy <http://rdaregistry.info/Elements/a/> ;
    rdfs:subPropertyOf <http://rdaregistry.info/Elements/a/P50131> ;
    skos:definition "Relates a corporate body hosting an event, exhibit, conference, etc., which gave rise to a work to a work."@en,
        "Met une collectivité accueillant l’événement, l’exposition, le congrès, etc. en relation avec l’œuvre."@fr .

<http://rdaregistry.info/Elements/a/P50005> a rdf:Property ;
    rdfs:label "is production company of"@en,
        "est la société de production de"@fr ;
    rdakit:instructionNumber "18.5" ;
    rdakit:toolkitDefinition "A work that includes the financial, technical, and organizational management of a production for stage, screen, sound recording, television, webcast, etc."@en,
        "Collectivité responsable de la gestion financière, technique et organisationnelle de la production d’un spectacle, d’un film, d’un enregistrement audio, d’une émission de télévision, d’une webémission, etc."@fr ;
    rdakit:toolkitLabel "production company of"@en,
        "société de production de"@fr ;
    reg:hasSubproperty <http://rdaregistry.info/Elements/a/datatype/P50005>,
        <http://rdaregistry.info/Elements/a/object/P50005> ;
    reg:hasUnconstrained <http://rdaregistry.info/Elements/u/P60004> ;
    reg:lexicalAlias <http://rdaregistry.info/Elements/a/productionCompanyOf.en> ;
    reg:name "productionCompanyOf"@en ;
    reg:status <http://metadataregistry.org/uri/RegStatus/1001> ;
    rdfs:domain <http://rdaregistry.info/Elements/c/C10005> ;
    rdfs:isDefinedBy <http://rdaregistry.info/Elements/a/> ;
    rdfs:subPropertyOf <http://rdaregistry.info/Elements/a/P50131> ;
    skos:definition "Relates a corporate body that is responsible for financial, technical, and organizational management of a production for stage, screen, sound recording, television, webcast, etc to a work."@en,
        "Met une collectivité responsable de la gestion financière, technique et organisationnelle de la production d’un spectacle, d’un film, d’un enregistrement audio, d’une émission de télévision, d’une webémission, etc. en relation avec l’œuvre."@fr .

<http://rdaregistry.info/Elements/a/P50006> a rdf:Property ;
    rdfs:label "has identifier for corporate body"@en,
        "a pour identifiant de la collectivité"@fr,
        "har identifikator för institutionen"@sv ;
    rdakit:instructionNumber "11.12" ;
    rdakit:toolkitDefinition "A character string uniquely associated with a corporate body, or with a surrogate such as an authority record for a corporate body."@en,
        "Una cadena de caracteres singularmente asociada con una entidad corporativa, o con un substituto de una entidad corporativa (p.ej., un registro de autoridad)."@es,
        "Chaîne de caractères associée de manière unique à une collectivité ou à un substitut d’une collectivité (par exemple, une notice d’autorité)."@fr ;
    rdakit:toolkitLabel "identifier for corporate body"@en,
        "identificador de la entidad corporativa"@es,
        "identifiant de la collectivité"@fr,
        "identifikator för institutionen"@sv ;
    reg:hasSubproperty <http://rdaregistry.info/Elements/a/datatype/P50006> ;
    reg:hasUnconstrained <http://rdaregistry.info/Elements/u/P60053> ;
    reg:lexicalAlias <http://rdaregistry.info/Elements/a/identifierForCorporateBody.en> ;
    reg:name "identifierForCorporateBody"@en ;
    reg:status <http://metadataregistry.org/uri/RegStatus/1001> ;
    rdfs:domain <http://rdaregistry.info/Elements/c/C10005> ;
    rdfs:isDefinedBy <http://rdaregistry.info/Elements/a/> ;
    skos:definition "Relates a corporate body to a character string uniquely associated with a corporate body, or with a surrogate such as an authority record for a corporate body."@en,
        "Met une collectivité en relation avec une chaîne de caractères associée de manière unique à une collectivité ou à un substitut d’une collectivité (par exemple, une notice d’autorité)."@fr ;
    skos:scopeNote "The identifier serves to differentiate a corporate body from other corporate bodies."@en,
        "L’identifiant sert à distinguer cette collectivité d’autres collectivités."@fr .

<http://rdaregistry.info/Elements/a/P50007> a rdf:Property ;
    rdfs:label "has founding corporate body"@en,
        "a pour collectivité fondatrice"@fr ;
    rdakit:instructionNumber "29.5" ;
    rdakit:toolkitDefinition "A corporate body that founded another corporate body."@en,
        "Una entidad corporativa que fundó a otra entidad corporativa."@es,
        "Collectivité qui a fondé l’autre collectivité."@fr ;
    rdakit:toolkitLabel "founding corporate body"@en,
        "entidad corporativa fundadora"@es,
        "collectivité fondatrice"@fr ;
    reg:hasSubproperty <http://rdaregistry.info/Elements/a/datatype/P50007>,
        <http://rdaregistry.info/Elements/a/object/P50007> ;
    reg:hasUnconstrained <http://rdaregistry.info/Elements/u/P60694> ;
    reg:lexicalAlias <http://rdaregistry.info/Elements/a/foundingCorporateBody.en> ;
    reg:name "foundingCorporateBody"@en ;
    reg:status <http://metadataregistry.org/uri/RegStatus/1001> ;
    rdfs:domain <http://rdaregistry.info/Elements/c/C10005> ;
    rdfs:isDefinedBy <http://rdaregistry.info/Elements/a/> ;
    skos:definition "Relates a corporate body to a corporate body that founded another corporate body."@en,
        "Met une collectivité en relation avec une collectivité qui a fondé l’autre collectivité."@fr .

<http://rdaregistry.info/Elements/a/P50008> a rdf:Property ;
    rdfs:label "has hierarchical superior"@en,
        "a pour supérieur hiérarchique"@fr ;
    rdakit:instructionNumber "29.5" ;
    rdakit:toolkitDefinition "A corporate body that is hierarchically superior to another corporate body."@en,
        "Una entidad corporativa que es jerárquicamente superior a otra entidad corporativa."@es,
        "Collectivité qui est hiérarchiquement supérieure à l’autre collectivité."@fr ;
    rdakit:toolkitLabel "hierarchical superior"@en,
        "superior jerárquica"@es,
        "supérieur hiérarchique"@fr ;
    reg:hasSubproperty <http://rdaregistry.info/Elements/a/datatype/P50008>,
        <http://rdaregistry.info/Elements/a/object/P50008> ;
    reg:hasUnconstrained <http://rdaregistry.info/Elements/u/P60680> ;
    reg:lexicalAlias <http://rdaregistry.info/Elements/a/hierarchicalSuperior.en> ;
    reg:name "hierarchicalSuperior"@en ;
    reg:status <http://metadataregistry.org/uri/RegStatus/1001> ;
    rdfs:domain <http://rdaregistry.info/Elements/c/C10005> ;
    rdfs:isDefinedBy <http://rdaregistry.info/Elements/a/> ;
    skos:definition "Relates a corporate body to a corporate body that is hierarchically superior to another corporate body."@en,
        "Met une collectivité en relation avec une collectivité qui est hiérarchiquement supérieure à l’autre collectivité."@fr .

<http://rdaregistry.info/Elements/a/P50009> a rdf:Property ;
    rdfs:label "has sponsored corporate body of corporate body"@en,
        "a pour collectivité commanditée"@fr ;
    rdakit:instructionNumber "29.5" ;
    rdakit:toolkitDefinition "A corporate body that is sponsored by another corporate body."@en,
        "Una entidad corporativa que es patrocinada por otra entidad corporativa."@es,
        "Collectivité commanditée par l’autre collectivité."@fr ;
    rdakit:toolkitLabel "sponsored corporate body of corporate body"@en,
        "entidad corporativa patrocinada"@es,
        "collectivité commanditée"@fr ;
    reg:hasSubproperty <http://rdaregistry.info/Elements/a/datatype/P50009>,
        <http://rdaregistry.info/Elements/a/object/P50009> ;
    reg:hasUnconstrained <http://rdaregistry.info/Elements/u/P60688> ;
    reg:lexicalAlias <http://rdaregistry.info/Elements/a/sponsoredCorporateBodyOfCorporateBody.en> ;
    reg:name "sponsoredCorporateBodyOfCorporateBody"@en ;
    reg:status <http://metadataregistry.org/uri/RegStatus/1001> ;
    rdfs:domain <http://rdaregistry.info/Elements/c/C10005> ;
    rdfs:isDefinedBy <http://rdaregistry.info/Elements/a/> ;
    skos:definition "Relates a corporate body to a corporate body that is sponsored by another corporate body."@en,
        "Met une collectivité en relation avec une collectivité commanditée par l’autre collectivité."@fr .

<http://rdaregistry.info/Elements/a/P50010> a rdf:Property ;
    rdfs:label "has hierarchical subordinate"@en,
        "a pour subordonné hiérarchique"@fr ;
    rdakit:instructionNumber "29.5" ;
    rdakit:toolkitDefinition "A corporate body that is subordinate to another corporate body."@en,
        "Una entidad corporativa que es subordinada a otra entidad corporativa."@es,
        "Collectivité qui est subordonnée à l’autre collectivité."@fr ;
    rdakit:toolkitLabel "hierarchical subordinate"@en,
        "subordinada jerárquica"@es,
        "subordonné hiérarchique"@fr ;
    reg:hasSubproperty <http://rdaregistry.info/Elements/a/datatype/P50010>,
        <http://rdaregistry.info/Elements/a/object/P50010> ;
    reg:hasUnconstrained <http://rdaregistry.info/Elements/u/P60681> ;
    reg:lexicalAlias <http://rdaregistry.info/Elements/a/hierarchicalSubordinate.en> ;
    reg:name "hierarchicalSubordinate"@en ;
    reg:status <http://metadataregistry.org/uri/RegStatus/1001> ;
    rdfs:domain <http://rdaregistry.info/Elements/c/C10005> ;
    rdfs:isDefinedBy <http://rdaregistry.info/Elements/a/> ;
    skos:definition "Relates a corporate body to a corporate body that is subordinate to another corporate body."@en,
        "Met une collectivité en relation avec une collectivité qui est subordonnée à l’autre collectivité."@fr .

<http://rdaregistry.info/Elements/a/P50011> a rdf:Property ;
    rdfs:label "has mergee"@en,
        "a pour collectivité fusionnée"@fr ;
    rdakit:instructionNumber "29.5" ;
    rdakit:toolkitDefinition "A corporate body that merged with another corporate body to form a third."@en,
        "Una entidad corporativa que se fusionó con otra entidad corporativa para formar una tercera."@es,
        "Collectivité qui a fusionné avec l’autre collectivité pour en former une troisième."@fr ;
    rdakit:toolkitLabel "mergee"@en,
        "fusionada con"@es,
        "collectivité fusionnée"@fr ;
    reg:hasSubproperty <http://rdaregistry.info/Elements/a/datatype/P50011>,
        <http://rdaregistry.info/Elements/a/object/P50011> ;
    reg:hasUnconstrained <http://rdaregistry.info/Elements/u/P60682> ;
    reg:lexicalAlias <http://rdaregistry.info/Elements/a/mergee.en> ;
    reg:name "mergee"@en ;
    reg:status <http://metadataregistry.org/uri/RegStatus/1001> ;
    rdfs:domain <http://rdaregistry.info/Elements/c/C10005> ;
    rdfs:isDefinedBy <http://rdaregistry.info/Elements/a/> ;
    skos:definition "Relates a corporate body to a corporate body that merged with another corporate body to form a third."@en,
        "Met une collectivité en relation avec une collectivité qui a fusionné avec l’autre collectivité pour en former une troisième."@fr .

<http://rdaregistry.info/Elements/a/P50012> a rdf:Property ;
    rdfs:label "has predecessor"@en,
        "a pour prédécesseur"@fr ;
    rdakit:instructionNumber "29.5" ;
    rdakit:toolkitDefinition "A corporate body that precedes another corporate body."@en,
        "Una entidad corporativa que precede a otra entidad corporativa"@es,
        "Collectivité qui précède l’autre collectivité."@fr ;
    rdakit:toolkitLabel "predecessor"@en,
        "predecesora"@es,
        "prédécesseur"@fr ;
    reg:hasSubproperty <http://rdaregistry.info/Elements/a/datatype/P50012>,
        <http://rdaregistry.info/Elements/a/object/P50012> ;
    reg:hasUnconstrained <http://rdaregistry.info/Elements/u/P60683> ;
    reg:lexicalAlias <http://rdaregistry.info/Elements/a/predecessor.en> ;
    reg:name "predecessor"@en ;
    reg:status <http://metadataregistry.org/uri/RegStatus/1001> ;
    rdfs:domain <http://rdaregistry.info/Elements/c/C10005> ;
    rdfs:isDefinedBy <http://rdaregistry.info/Elements/a/> ;
    skos:definition "Relates a corporate body to a corporate body that precedes another corporate body."@en,
        "Met une collectivité en relation avec une collectivité qui précède l’autre collectivité."@fr .

<http://rdaregistry.info/Elements/a/P50013> a rdf:Property ;
    rdfs:label "has product of merger"@en,
        "a pour résultat de fusion"@fr ;
    rdakit:instructionNumber "29.5" ;
    rdakit:toolkitDefinition "A corporate body that resulted from a merger of two or more other corporate bodies."@en,
        "Una entidad corporativa que resulta de la fusión de dos o más entidades corporativas."@es,
        "Collectivité résultant d’une fusion entre deux ou plusieurs autres collectivités."@fr ;
    rdakit:toolkitLabel "product of merger"@en,
        "producto de fusión de"@es,
        "résultat de fusion"@fr ;
    reg:hasSubproperty <http://rdaregistry.info/Elements/a/datatype/P50013>,
        <http://rdaregistry.info/Elements/a/object/P50013> ;
    reg:hasUnconstrained <http://rdaregistry.info/Elements/u/P60684> ;
    reg:lexicalAlias <http://rdaregistry.info/Elements/a/productOfAMerger.en> ;
    reg:name "productOfAMerger"@en ;
    reg:status <http://metadataregistry.org/uri/RegStatus/1001> ;
    rdfs:domain <http://rdaregistry.info/Elements/c/C10005> ;
    rdfs:isDefinedBy <http://rdaregistry.info/Elements/a/> ;
    skos:definition "Relates a corporate body to a corporate body that resulted from a merger of two or more other corporate bodies."@en,
        "Met une collectivité en relation avec une collectivité résultant d’une fusion entre deux ou plusieurs autres collectivités."@fr .

<http://rdaregistry.info/Elements/a/P50014> a rdf:Property ;
    rdfs:label "has product of split"@en,
        "a pour résultat de scission"@fr ;
    rdakit:instructionNumber "29.5" ;
    rdakit:toolkitDefinition "A corporate body that resulted from a split or division of another corporate body."@en,
        "Una entidad corporativa que resulta de la escisión o división de otra entidad corporativa."@es,
        "Collectivité résultant d’une scission ou division de l’autre collectivité."@fr ;
    rdakit:toolkitLabel "product of split"@en,
        "producto de escisión de"@es,
        "résultat de scission"@fr ;
    reg:hasSubproperty <http://rdaregistry.info/Elements/a/datatype/P50014>,
        <http://rdaregistry.info/Elements/a/object/P50014> ;
    reg:hasUnconstrained <http://rdaregistry.info/Elements/u/P60685> ;
    reg:lexicalAlias <http://rdaregistry.info/Elements/a/productOfASplit.en> ;
    reg:name "productOfASplit"@en ;
    reg:status <http://metadataregistry.org/uri/RegStatus/1001> ;
    rdfs:domain <http://rdaregistry.info/Elements/c/C10005> ;
    rdfs:isDefinedBy <http://rdaregistry.info/Elements/a/> ;
    skos:definition "Relates a corporate body to a corporate body that resulted from a split or division of another corporate body."@en,
        "Met une collectivité en relation avec une collectivité résultant d’une scission ou division de l’autre collectivité."@fr .

<http://rdaregistry.info/Elements/a/P50015> a rdf:Property ;
    rdfs:label "has sponsoring corporate body"@en,
        "a pour collectivité commanditaire"@fr ;
    rdakit:instructionNumber "29.5" ;
    rdakit:toolkitDefinition "A corporate body that sponsors another corporate body."@en,
        "Una entidad corporativa que patrocina a otra entidad corporativa."@es,
        "Collectivité qui commandite l’autre collectivité."@fr ;
    rdakit:toolkitLabel "sponsoring corporate body"@en,
        "entidad corporativa patrocinadora"@es,
        "collectivité commanditaire"@fr ;
    reg:hasSubproperty <http://rdaregistry.info/Elements/a/datatype/P50015>,
        <http://rdaregistry.info/Elements/a/object/P50015> ;
    reg:hasUnconstrained <http://rdaregistry.info/Elements/u/P60676> ;
    reg:lexicalAlias <http://rdaregistry.info/Elements/a/sponsoringCorporateBody.en> ;
    reg:name "sponsoringCorporateBody"@en ;
    reg:status <http://metadataregistry.org/uri/RegStatus/1001> ;
    rdfs:domain <http://rdaregistry.info/Elements/c/C10005> ;
    rdfs:isDefinedBy <http://rdaregistry.info/Elements/a/> ;
    skos:definition "Relates a corporate body to a corporate body that sponsors another corporate body."@en,
        "Met une collectivité en relation avec une collectivité qui commandite l’autre collectivité."@fr .

<http://rdaregistry.info/Elements/a/P50016> a rdf:Property ;
    rdfs:label "has successor"@en,
        "a pour successeur"@fr ;
    rdakit:instructionNumber "29.5" ;
    rdakit:toolkitDefinition "A corporate body that succeeds or follows another corporate body."@en,
        "Una entidad corporativa que sucede o continúa a otra entidad corporativa."@es,
        "Collectivité qui succède ou fait suite à l’autre collectivité."@fr ;
    rdakit:toolkitLabel "successor"@en,
        "sucesora"@es,
        "successeur"@fr ;
    reg:hasSubproperty <http://rdaregistry.info/Elements/a/datatype/P50016>,
        <http://rdaregistry.info/Elements/a/object/P50016> ;
    reg:hasUnconstrained <http://rdaregistry.info/Elements/u/P60686> ;
    reg:lexicalAlias <http://rdaregistry.info/Elements/a/successor.en> ;
    reg:name "successor"@en ;
    reg:status <http://metadataregistry.org/uri/RegStatus/1001> ;
    rdfs:domain <http://rdaregistry.info/Elements/c/C10005> ;
    rdfs:isDefinedBy <http://rdaregistry.info/Elements/a/> ;
    skos:definition "Relates a corporate body to a corporate body that succeeds or follows another corporate body."@en,
        "Met une collectivité en relation avec une collectivité qui succède ou fait suite à l’autre collectivité."@fr .

<http://rdaregistry.info/Elements/a/P50017> a rdf:Property ;
    rdfs:label "has founded corporate body of corporate body"@en,
        "a pour collectivité fondée de la collectivité"@fr ;
    rdakit:instructionNumber "29.5" ;
    rdakit:toolkitDefinition "A corporate body that another corporate body founded."@en,
        "Una entidad corporativa fundada por la otra entidad corporativa."@es,
        "Collectivité que l’autre collectivité a fondée."@fr ;
    rdakit:toolkitLabel "founded corporate body of corporate body"@en,
        "entidad corporativa fundada"@es,
        "collectivité fondée de la collectivité"@fr ;
    reg:hasSubproperty <http://rdaregistry.info/Elements/a/datatype/P50017>,
        <http://rdaregistry.info/Elements/a/object/P50017> ;
    reg:hasUnconstrained <http://rdaregistry.info/Elements/u/P60687> ;
    reg:lexicalAlias <http://rdaregistry.info/Elements/a/foundedCorporateBodyOfCorporateBody.en> ;
    reg:name "foundedCorporateBodyOfCorporateBody"@en ;
    reg:status <http://metadataregistry.org/uri/RegStatus/1001> ;
    rdfs:domain <http://rdaregistry.info/Elements/c/C10005> ;
    rdfs:isDefinedBy <http://rdaregistry.info/Elements/a/> ;
    skos:definition "Relates a corporate body to a corporate body that another corporate body founded."@en,
        "Met une collectivité en relation avec une collectivité que l’autre collectivité a fondée."@fr .

<http://rdaregistry.info/Elements/a/P50018> a rdf:Property ;
    reg:status <http://metadataregistry.org/uri/RegStatus/1008> ;
    rdfs:isDefinedBy <http://rdaregistry.info/Elements/a/> .

<http://rdaregistry.info/Elements/a/P50019> a rdf:Property ;
    rdfs:label "has number of conference, etc."@en,
        "a pour numéro d’ordre d’un congrès, etc."@fr,
        "har ordningsnummer för konferens etc."@sv ;
    rdakit:instructionNumber "11.6" ;
    rdakit:toolkitDefinition "A designation of the sequencing of a conference, etc., within a series of conferences, etc."@en,
        "Una designación de la secuencia de una conferencia, etc., dentro de una serie de conferencias, etc."@es,
        "Indication d’ordre séquentiel d’un congrès, etc. à l’intérieur d’une série de congrès, etc."@fr ;
    rdakit:toolkitLabel "number of conference, etc."@en,
        "número de una conferencia, etc."@es,
        "numéro d’ordre d’un congrès, etc."@fr,
        "ordningsnummer för konferens etc."@sv ;
    reg:hasSubproperty <http://rdaregistry.info/Elements/a/datatype/P50019> ;
    reg:hasUnconstrained <http://rdaregistry.info/Elements/u/P60079> ;
    reg:lexicalAlias <http://rdaregistry.info/Elements/a/numberOfConferenceEtc.en> ;
    reg:name "numberOfConferenceEtc"@en ;
    reg:status <http://metadataregistry.org/uri/RegStatus/1001> ;
    rdfs:domain <http://rdaregistry.info/Elements/c/C10005> ;
    rdfs:isDefinedBy <http://rdaregistry.info/Elements/a/> ;
    skos:definition "Relates a corporate body to a designation of the sequencing of a conference, etc., within a series of conferences, etc."@en,
        "Met une collectivité en relation avec une indication d’ordre séquentiel d’un congrès, etc. à l’intérieur d’une série de congrès, etc."@fr .

<http://rdaregistry.info/Elements/a/P50020> a rdf:Property ;
    rdfs:label "has founding family"@en,
        "a pour famille fondatrice"@fr ;
    rdakit:instructionNumber "29.5" ;
    rdakit:toolkitDefinition "A family that founded a corporate body."@en,
        "Una familia que fundó la entidad corporativa."@es,
        "Famille qui a fondé la collectivité."@fr ;
    rdakit:toolkitLabel "founding family"@en,
        "familia fundadora"@es,
        "famille fondatrice"@fr ;
    reg:hasSubproperty <http://rdaregistry.info/Elements/a/datatype/P50020>,
        <http://rdaregistry.info/Elements/a/object/P50020> ;
    reg:hasUnconstrained <http://rdaregistry.info/Elements/u/P60694> ;
    reg:lexicalAlias <http://rdaregistry.info/Elements/a/foundingFamily.en> ;
    reg:name "foundingFamily"@en ;
    reg:status <http://metadataregistry.org/uri/RegStatus/1001> ;
    rdfs:domain <http://rdaregistry.info/Elements/c/C10005> ;
    rdfs:isDefinedBy <http://rdaregistry.info/Elements/a/> ;
    skos:definition "Relates a corporate body to a family that founded a corporate body."@en,
        "Met une collectivité en relation avec une famille qui a fondé la collectivité."@fr .

<http://rdaregistry.info/Elements/a/P50021> a rdf:Property ;
    rdfs:label "has sponsoring family"@en,
        "a pour famille commanditaire"@fr ;
    rdakit:instructionNumber "29.5" ;
    rdakit:toolkitDefinition "A family that sponsors a corporate body."@en,
        "Una familia que patrocina la entidad corporativa."@es,
        "Famille qui commandite la collectivité."@fr ;
    rdakit:toolkitLabel "sponsoring family"@en,
        "familia patrocinadora"@es,
        "famille commanditaire"@fr ;
    reg:hasSubproperty <http://rdaregistry.info/Elements/a/datatype/P50021>,
        <http://rdaregistry.info/Elements/a/object/P50021> ;
    reg:hasUnconstrained <http://rdaregistry.info/Elements/u/P60676> ;
    reg:lexicalAlias <http://rdaregistry.info/Elements/a/sponsoringFamily.en> ;
    reg:name "sponsoringFamily"@en ;
    reg:status <http://metadataregistry.org/uri/RegStatus/1001> ;
    rdfs:domain <http://rdaregistry.info/Elements/c/C10005> ;
    rdfs:isDefinedBy <http://rdaregistry.info/Elements/a/> ;
    skos:definition "Relates a corporate body to a family that sponsors a corporate body."@en,
        "Met une collectivité en relation avec une famille qui commandite la collectivité."@fr .

<http://rdaregistry.info/Elements/a/P50022> a rdf:Property ;
    rdfs:label "has field of activity of corporate body"@en,
        "a pour domaine d’activité de la collectivité"@fr ;
    rdakit:instructionNumber "11.1" ;
    rdakit:toolkitDefinition "A field of business in which a corporate body is engaged or an area of competence, responsibility, jurisdiction, etc. of a corporate body."@en,
        "Un campo de negocios al que la entidad corporativa está dedicada y/o su área de competencia, responsabilidad, jurisdicción, etc."@es,
        "Champ d’activité dans lequel s’investit la collectivité, sa zone de compétence, de responsabilité, de juridiction, etc."@fr ;
    rdakit:toolkitLabel "field of activity of corporate body"@en,
        "campo de actividad de la entidad corporativa"@es,
        "domaine d’activité de la collectivité"@fr ;
    reg:hasSubproperty <http://rdaregistry.info/Elements/a/datatype/P50022> ;
    reg:hasUnconstrained <http://rdaregistry.info/Elements/u/P60089> ;
    reg:lexicalAlias <http://rdaregistry.info/Elements/a/fieldOfActivityOfCorporateBody.en> ;
    reg:name "fieldOfActivityOfCorporateBody"@en ;
    reg:status <http://metadataregistry.org/uri/RegStatus/1001> ;
    rdfs:domain <http://rdaregistry.info/Elements/c/C10005> ;
    rdfs:isDefinedBy <http://rdaregistry.info/Elements/a/> ;
    skos:definition "Relates a corporate body to a field of business in which a corporate body is engaged or an area of competence, responsibility, jurisdiction, etc. of a corporate body."@en,
        "Met une collectivité en relation avec un champ d’activité dans lequel s’investit la collectivité, sa zone de compétence, de responsabilité, de juridiction, etc."@fr .

<http://rdaregistry.info/Elements/a/P50023> a rdf:Property ;
    rdfs:label "has language of corporate body"@en,
        "a pour langue de la collectivité"@fr ;
    rdakit:instructionNumber "11.8" ;
    rdakit:toolkitDefinition "A language a corporate body uses in its communications."@en,
        "Lengua o lenguas que usa la entidad corporativa en sus comunicaciones"@es,
        "Langue que la collectivité utilise pour sa communication."@fr ;
    rdakit:toolkitLabel "language of corporate body"@en,
        "lengua de la entidad corporativa"@es,
        "langue de la collectivité"@fr ;
    reg:hasSubproperty <http://rdaregistry.info/Elements/a/datatype/P50023> ;
    reg:hasUnconstrained <http://rdaregistry.info/Elements/u/P60098> ;
    reg:lexicalAlias <http://rdaregistry.info/Elements/a/languageOfCorporateBody.en> ;
    reg:name "languageOfCorporateBody"@en ;
    reg:status <http://metadataregistry.org/uri/RegStatus/1001> ;
    rdfs:domain <http://rdaregistry.info/Elements/c/C10005> ;
    rdfs:isDefinedBy <http://rdaregistry.info/Elements/a/> ;
    skos:definition "Relates a corporate body to a language a corporate body uses in its communications."@en,
        "Met une collectivité en relation avec une langue que la collectivité utilise pour sa communication."@fr .

<http://rdaregistry.info/Elements/a/P50024> a rdf:Property ;
    rdfs:label "has location of conference, etc."@en,
        "a pour lieu du congrès, etc."@fr,
        "har konferensort"@sv ;
    rdakit:instructionNumber "11.3.2" ;
    rdakit:toolkitDefinition "A place or places in which a conference, congress, meeting, exhibition, fair, festival, etc., was held."@en,
        "Una localidad en la que se se realizó una conferencia, congreso, reunión, exposición, feria, festival, etc."@es,
        "Localité où un congrès, une conférence, une réunion, une exposition, une foire, un festival, etc. s’est tenu."@fr ;
    rdakit:toolkitLabel "location of conference, etc."@en,
        "lugar de la conferencia, etc."@es,
        "lieu du congrès, etc."@fr,
        "konferensort"@sv ;
    reg:hasSubproperty <http://rdaregistry.info/Elements/a/datatype/P50024> ;
    reg:hasUnconstrained <http://rdaregistry.info/Elements/u/P60107> ;
    reg:lexicalAlias <http://rdaregistry.info/Elements/a/locationOfConferenceEtc.en> ;
    reg:name "locationOfConferenceEtc"@en ;
    reg:status <http://metadataregistry.org/uri/RegStatus/1001> ;
    rdfs:domain <http://rdaregistry.info/Elements/c/C10005> ;
    rdfs:isDefinedBy <http://rdaregistry.info/Elements/a/> ;
    rdfs:subPropertyOf <http://rdaregistry.info/Elements/a/P50031> ;
    skos:definition "Relates a corporate body to a place or places in which a conference, congress, meeting, exhibition, fair, festival, etc., was held."@en,
        "Met une collectivité en relation avec une localité où un congrès, une conférence, une réunion, une exposition, une foire, un festival, etc. s’est tenu."@fr .

<http://rdaregistry.info/Elements/a/P50025> a rdf:Property ;
    rdfs:label "has variant name for corporate body"@en,
        "a pour variante de nom de la collectivité"@fr,
        "har variantnamn för institutionen"@sv ;
    rdakit:instructionNumber "11.2.3" ;
    rdakit:toolkitDefinition "A name or form of name by which a corporate body is known that differs from a name or form of name chosen as a preferred name."@en,
        "Un nombre o una forma de un nombre mediante el cual se conoce a una entidad corporativa que difiere del nombre o la forma del nombre escogido como el nombre preferido."@es,
        "Nom ou forme de nom sous laquelle une collectivité est connue et qui diffère du nom ou de la forme de nom choisie comme nom privilégié."@fr ;
    rdakit:toolkitLabel "variant name for corporate body"@en,
        "variante del nombre de la entidad corporativa"@es,
        "variante de nom de la collectivité"@fr,
        "variantnamn för institutionen"@sv ;
    reg:hasSubproperty <http://rdaregistry.info/Elements/a/datatype/P50025> ;
    reg:hasUnconstrained <http://rdaregistry.info/Elements/u/P60119> ;
    reg:lexicalAlias <http://rdaregistry.info/Elements/a/variantNameForCorporateBody.en> ;
    reg:name "variantNameForCorporateBody"@en ;
    reg:status <http://metadataregistry.org/uri/RegStatus/1001> ;
    rdfs:domain <http://rdaregistry.info/Elements/c/C10005> ;
    rdfs:isDefinedBy <http://rdaregistry.info/Elements/a/> ;
    rdfs:subPropertyOf <http://rdaregistry.info/Elements/a/P50032> ;
    skos:definition "Relates a corporate body to a name or form of name by which a corporate body is known that differs from a name or form of name chosen as a preferred name."@en,
        "Met une collectivité en relation avec un nom ou forme de nom sous laquelle une collectivité est connue et qui diffère du nom ou de la forme de nom choisie comme nom privilégié."@fr ;
    skos:scopeNote "Variant name for corporate body includes a name or form of name used by a corporate body or found in reference sources, a name resulting from a different transliteration of a name, etc."@en .

<http://rdaregistry.info/Elements/a/P50026> a rdf:Property ;
    rdfs:label "has employee"@en,
        "a pour employé"@fr ;
    rdakit:instructionNumber "29.5" ;
    rdakit:toolkitDefinition "A person employed by a corporate body."@en,
        "Una persona empleada por la entidad corporativa."@es,
        "Personne employée par la collectivité."@fr ;
    rdakit:toolkitLabel "employee"@en,
        "empleado"@es,
        "employé"@fr ;
    reg:hasSubproperty <http://rdaregistry.info/Elements/a/datatype/P50026>,
        <http://rdaregistry.info/Elements/a/object/P50026> ;
    reg:hasUnconstrained <http://rdaregistry.info/Elements/u/P60629> ;
    reg:lexicalAlias <http://rdaregistry.info/Elements/a/employee.en> ;
    reg:name "employee"@en ;
    reg:status <http://metadataregistry.org/uri/RegStatus/1001> ;
    rdfs:domain <http://rdaregistry.info/Elements/c/C10005> ;
    rdfs:isDefinedBy <http://rdaregistry.info/Elements/a/> ;
    skos:definition "Relates a corporate body to a person employed by a corporate body."@en,
        "Met une collectivité en relation avec une personne employée par la collectivité."@fr .

<http://rdaregistry.info/Elements/a/P50028> a rdf:Property ;
    rdfs:label "has sponsor"@en,
        "a pour personne commanditaire"@fr ;
    rdakit:instructionNumber "29.5" ;
    rdakit:toolkitDefinition "A person sponsoring a corporate body."@en,
        "Una persona que patrocina la entidad corporativa"@es,
        "Personne qui commandite la collectivité."@fr ;
    rdakit:toolkitLabel "sponsor"@en,
        "patrocinador"@es,
        "personne commanditaire"@fr ;
    reg:hasSubproperty <http://rdaregistry.info/Elements/a/datatype/P50028>,
        <http://rdaregistry.info/Elements/a/object/P50028> ;
    reg:hasUnconstrained <http://rdaregistry.info/Elements/u/P60676> ;
    reg:lexicalAlias <http://rdaregistry.info/Elements/a/sponsor.en> ;
    reg:name "sponsor"@en ;
    reg:status <http://metadataregistry.org/uri/RegStatus/1001> ;
    rdfs:domain <http://rdaregistry.info/Elements/c/C10005> ;
    rdfs:isDefinedBy <http://rdaregistry.info/Elements/a/> ;
    skos:definition "Relates a corporate body to a person sponsoring a corporate body."@en,
        "Met une collectivité en relation avec une personne qui commandite la collectivité."@fr .

<http://rdaregistry.info/Elements/a/P50029> a rdf:Property ;
    rdfs:label "has founder"@en,
        "a pour fondateur"@fr ;
    rdakit:instructionNumber "29.5" ;
    rdakit:toolkitDefinition "A person who founded a corporate body."@en,
        "Una persona que fundó la entidad corporativa."@es,
        "Personne qui a fondé la collectivité."@fr ;
    rdakit:toolkitLabel "founder"@en,
        "fundador"@es,
        "fondateur"@fr ;
    reg:hasSubproperty <http://rdaregistry.info/Elements/a/datatype/P50029>,
        <http://rdaregistry.info/Elements/a/object/P50029> ;
    reg:hasUnconstrained <http://rdaregistry.info/Elements/u/P60694> ;
    reg:lexicalAlias <http://rdaregistry.info/Elements/a/founder.en> ;
    reg:name "founder"@en ;
    reg:status <http://metadataregistry.org/uri/RegStatus/1001> ;
    rdfs:domain <http://rdaregistry.info/Elements/c/C10005> ;
    rdfs:isDefinedBy <http://rdaregistry.info/Elements/a/> ;
    skos:definition "Relates a corporate body to a person who founded a corporate body."@en,
        "Met une collectivité en relation avec une personne qui a fondé la collectivité."@fr .

<http://rdaregistry.info/Elements/a/P50030> a rdf:Property ;
    rdfs:label "has member"@en,
        "a pour membre"@fr ;
    rdakit:instructionNumber "29.5" ;
    rdakit:toolkitDefinition "A person who is a member of a corporate body."@en,
        "Una persona que es miembro de una entidad corporativa."@es,
        "Personne qui est membre du groupe d’interprètes, de l’expédition, etc."@fr ;
    rdakit:toolkitLabel "member"@en,
        "miembro"@es,
        "membre"@fr ;
    reg:hasSubproperty <http://rdaregistry.info/Elements/a/datatype/P50030>,
        <http://rdaregistry.info/Elements/a/object/P50030> ;
    reg:hasUnconstrained <http://rdaregistry.info/Elements/u/P60697> ;
    reg:lexicalAlias <http://rdaregistry.info/Elements/a/member.en> ;
    reg:name "member"@en ;
    reg:status <http://metadataregistry.org/uri/RegStatus/1001> ;
    rdfs:domain <http://rdaregistry.info/Elements/c/C10005> ;
    rdfs:isDefinedBy <http://rdaregistry.info/Elements/a/> ;
    skos:definition "Relates a corporate body to a person who is a member of a corporate body."@en,
        "Met une collectivité en relation avec une personne qui est membre du groupe d’interprètes, de l’expédition, etc."@fr .

<http://rdaregistry.info/Elements/a/P50034> a rdf:Property ;
    rdfs:label "has associated institution"@en,
        "a pour institution associée"@fr,
        "har samhörande institution"@sv ;
    rdakit:instructionNumber "11.5" ;
    rdakit:toolkitDefinition "An institution commonly associated with a corporate body."@en,
        "Una institución comúnmente asociada con una entidad corporativa."@es,
        "Institution communément associée à une collectivité."@fr ;
    rdakit:toolkitLabel "associated institution"@en,
        "institución asociada"@es,
        "institution associée"@fr,
        "samhörande institution"@sv ;
    reg:hasSubproperty <http://rdaregistry.info/Elements/a/datatype/P50034> ;
    reg:hasUnconstrained <http://rdaregistry.info/Elements/u/P60482> ;
    reg:lexicalAlias <http://rdaregistry.info/Elements/a/associatedInstitution.en> ;
    reg:name "associatedInstitution"@en ;
    reg:status <http://metadataregistry.org/uri/RegStatus/1001> ;
    rdfs:domain <http://rdaregistry.info/Elements/c/C10005> ;
    rdfs:isDefinedBy <http://rdaregistry.info/Elements/a/> ;
    skos:definition "Relates a corporate body to an institution commonly associated with a corporate body."@en,
        "Met une collectivité en relation avec une institution communément associée à une collectivité."@fr .

<http://rdaregistry.info/Elements/a/P50035> a rdf:Property ;
    rdfs:label "has corporate history"@en,
        "a pour historique de la collectivité"@fr,
        "har institutionshistoria"@sv ;
    rdakit:instructionNumber "11.11" ;
    rdakit:toolkitDefinition "A summary of historical information about a corporate body."@en,
        "Información histórica de una entidad corporativa"@es,
        "Information historique sur la collectivité."@fr ;
    rdakit:toolkitLabel "corporate history"@en,
        "historia corporativa"@es,
        "historique de la collectivité"@fr,
        "institutionshistoria"@sv ;
    reg:hasSubproperty <http://rdaregistry.info/Elements/a/datatype/P50035> ;
    reg:hasUnconstrained <http://rdaregistry.info/Elements/u/P60484> ;
    reg:lexicalAlias <http://rdaregistry.info/Elements/a/corporateHistory.en> ;
    reg:name "corporateHistory"@en ;
    reg:status <http://metadataregistry.org/uri/RegStatus/1001> ;
    rdfs:domain <http://rdaregistry.info/Elements/c/C10005> ;
    rdfs:isDefinedBy <http://rdaregistry.info/Elements/a/> ;
    skos:definition "Relates a corporate body to a summary of historical information about a corporate body."@en,
        "Met une collectivité en relation avec une information historique sur la collectivité."@fr .

<http://rdaregistry.info/Elements/a/P50036> a rdf:Property ;
    rdfs:label "has address of corporate body"@en,
        "a pour adresse de la collectivité"@fr ;
    rdakit:instructionNumber "11.9" ;
    rdakit:toolkitDefinition "An address of a corporate body."@en,
        "La dirección de una entidad corporativa."@es,
        "L’adresse du siège social ou des bureaux, l’adresse électronique ou l’adresse du site Web de la collectivité."@fr ;
    rdakit:toolkitLabel "address of corporate body"@en,
        "dirección de la entidad corporativa"@es,
        "adresse de la collectivité"@fr ;
    reg:hasSubproperty <http://rdaregistry.info/Elements/a/datatype/P50036> ;
    reg:hasUnconstrained <http://rdaregistry.info/Elements/u/P60512> ;
    reg:lexicalAlias <http://rdaregistry.info/Elements/a/addressOfCorporateBody.en> ;
    reg:name "addressOfCorporateBody"@en ;
    reg:status <http://metadataregistry.org/uri/RegStatus/1001> ;
    rdfs:domain <http://rdaregistry.info/Elements/c/C10005> ;
    rdfs:isDefinedBy <http://rdaregistry.info/Elements/a/> ;
    skos:definition "Relates a corporate body to an address of a corporate body."@en,
        "Met une collectivité en relation avec l’adresse du siège social ou des bureaux, l’adresse électronique ou l’adresse du site Web de la collectivité."@fr .

<http://rdaregistry.info/Elements/a/P50051> a rdf:Property ;
    rdfs:label "has type of family"@en,
        "a pour type de famille"@fr,
        "har typ av familj/släkt"@sv ;
    rdakit:instructionNumber "10.3" ;
    rdakit:toolkitDefinition "A categorization or generic descriptor for a type of family."@en,
        "Una categorización o descriptor genérico del tipo de familia."@es,
        "Catégorie ou descripteur générique pour le type de famille."@fr ;
    rdakit:toolkitLabel "type of family"@en,
        "tipo de familia"@es,
        "type de famille"@fr,
        "typ av familj/släkt"@sv ;
    reg:hasSubproperty <http://rdaregistry.info/Elements/a/datatype/P50051> ;
    reg:hasUnconstrained <http://rdaregistry.info/Elements/u/P60047> ;
    reg:lexicalAlias <http://rdaregistry.info/Elements/a/typeOfFamily.en> ;
    reg:name "typeOfFamily"@en ;
    reg:status <http://metadataregistry.org/uri/RegStatus/1001> ;
    rdfs:domain <http://rdaregistry.info/Elements/c/C10008> ;
    rdfs:isDefinedBy <http://rdaregistry.info/Elements/a/> ;
    skos:definition "Relates a family to a categorization or generic descriptor for a type of family."@en,
        "Met une famille en relation avec une catégorie ou descripteur générique pour le type de famille."@fr .

<http://rdaregistry.info/Elements/a/P50052> a rdf:Property ;
    rdfs:label "has identifier for family"@en,
        "a pour identifiant de la famille"@fr,
        "har identifikator för familjen/släkten"@sv ;
    rdakit:instructionNumber "10.1" ;
    rdakit:toolkitDefinition "A character string uniquely associated with a family, or with a surrogate such as an authority record for a family."@en,
        "Una cadena de caracteres solamente asociada con una familia, o con un sustituto de una familia (por ej., un registro de autoridad)."@es,
        "Chaîne de caractères associée de manière unique à une famille ou à un substitut d’une famille (par exemple, une notice d’autorité)."@fr ;
    rdakit:toolkitLabel "identifier for family"@en,
        "identificador de la familia"@es,
        "identifiant de la famille"@fr,
        "identifikator för familjen/släkten"@sv ;
    reg:hasSubproperty <http://rdaregistry.info/Elements/a/datatype/P50052> ;
    reg:hasUnconstrained <http://rdaregistry.info/Elements/u/P60053> ;
    reg:lexicalAlias <http://rdaregistry.info/Elements/a/identifierForFamily.en> ;
    reg:name "identifierForFamily"@en ;
    reg:status <http://metadataregistry.org/uri/RegStatus/1001> ;
    rdfs:domain <http://rdaregistry.info/Elements/c/C10008> ;
    rdfs:isDefinedBy <http://rdaregistry.info/Elements/a/> ;
    skos:definition "Relates a family to a character string uniquely associated with a family, or with a surrogate such as an authority record for a family."@en,
        "Met une famille en relation avec une chaîne de caractères associée de manière unique à une famille ou à un substitut d’une famille (par exemple, une notice d’autorité)."@fr ;
    skos:scopeNote "The identifier serves to differentiate a family from other families."@en,
        "L’identifiant sert à distinguer cette famille d’autres familles."@fr .

<http://rdaregistry.info/Elements/a/P50053> a rdf:Property ;
    rdfs:label "has descendant family"@en,
        "a pour famille descendante"@fr ;
    rdakit:instructionNumber "29.5" ;
    rdakit:toolkitDefinition "A family descended from another family."@en,
        "Una familia que desciende de otra familia."@es,
        "Famille descendant de l’autre famille."@fr ;
    rdakit:toolkitLabel "descendant family"@en,
        "familia descendiente"@es,
        "famille descendante"@fr ;
    reg:hasSubproperty <http://rdaregistry.info/Elements/a/datatype/P50053>,
        <http://rdaregistry.info/Elements/a/object/P50053> ;
    reg:hasUnconstrained <http://rdaregistry.info/Elements/u/P60686> ;
    reg:lexicalAlias <http://rdaregistry.info/Elements/a/descendantFamily.en> ;
    reg:name "descendantFamily"@en ;
    reg:status <http://metadataregistry.org/uri/RegStatus/1001> ;
    rdfs:domain <http://rdaregistry.info/Elements/c/C10008> ;
    rdfs:isDefinedBy <http://rdaregistry.info/Elements/a/> ;
    skos:definition "Relates a family to a family descended from another family."@en,
        "Met une famille en relation avec une famille descendant de l’autre famille."@fr .

<http://rdaregistry.info/Elements/a/P50057> a rdf:Property ;
    rdfs:label "has place associated with family"@en,
        "a pour lieu associé à la famille"@fr,
        "har ort förknippad med familjen/släkten"@sv ;
    rdakit:instructionNumber "10.5" ;
    rdakit:toolkitDefinition "A place where a family resides or has resided or has some connection."@en,
        "Un lugar donde reside la familia, o donde ha residido o que tiene alguna conexión."@es,
        "Lieu où une famille réside ou a résidé ou avec lequel elle a une relation quelconque."@fr ;
    rdakit:toolkitLabel "place associated with family"@en,
        "lugar asociado con la familia"@es,
        "lieu associé à la famille"@fr,
        "ort förknippad med familjen/släkten"@sv ;
    reg:hasSubproperty <http://rdaregistry.info/Elements/a/datatype/P50057> ;
    reg:hasUnconstrained <http://rdaregistry.info/Elements/u/P60325> ;
    reg:lexicalAlias <http://rdaregistry.info/Elements/a/placeAssociatedWithFamily.en> ;
    reg:name "placeAssociatedWithFamily"@en ;
    reg:status <http://metadataregistry.org/uri/RegStatus/1001> ;
    rdfs:domain <http://rdaregistry.info/Elements/c/C10008> ;
    rdfs:isDefinedBy <http://rdaregistry.info/Elements/a/> ;
    skos:definition "Relates a family to a place where a family resides or has resided or has some connection."@en,
        "Met une famille en relation avec un lieu où une famille réside ou a résidé ou avec lequel elle a une relation quelconque."@fr .

<http://rdaregistry.info/Elements/a/P50058> a rdf:Property ;
    rdfs:label "has date associated with family"@en,
        "a pour date associée à la famille"@fr,
        "har tid förknippad med famliljen/släkten"@sv ;
    rdakit:instructionNumber "10.4" ;
    rdakit:toolkitDefinition "A significant date associated with a family."@en,
        "Una fecha significativa asociada con la familia."@es,
        "Date importante associée à une famille."@fr ;
    rdakit:toolkitLabel "date associated with family"@en,
        "fecha asociada con la familia"@es,
        "date associée à la famille"@fr,
        "tid förknippad med famliljen/släkten"@sv ;
    reg:hasSubproperty <http://rdaregistry.info/Elements/a/datatype/P50058> ;
    reg:hasUnconstrained <http://rdaregistry.info/Elements/u/P60324> ;
    reg:lexicalAlias <http://rdaregistry.info/Elements/a/dateAssociatedWithFamily.en> ;
    reg:name "dateAssociatedWithFamily"@en ;
    reg:status <http://metadataregistry.org/uri/RegStatus/1001> ;
    rdfs:domain <http://rdaregistry.info/Elements/c/C10008> ;
    rdfs:isDefinedBy <http://rdaregistry.info/Elements/a/> ;
    skos:definition "Relates a family to a significant date associated with a family."@en,
        "Met une famille en relation avec une date importante associée à une famille."@fr .

<http://rdaregistry.info/Elements/a/P50059> a rdf:Property ;
    rdfs:label "has hereditary title"@en,
        "a pour titre héréditaire"@fr,
        "har ärvd titel"@sv ;
    rdakit:instructionNumber "10.7" ;
    rdakit:toolkitDefinition "A title of nobility, etc., associated with a family."@en,
        "Un título de nobleza, etc., asociado con una familia."@es,
        "Titre de noblesse, etc. associé à une famille."@fr ;
    rdakit:toolkitLabel "hereditary title"@en,
        "título hereditario"@es,
        "titre héréditaire"@fr,
        "ärvd titel"@sv ;
    reg:hasSubproperty <http://rdaregistry.info/Elements/a/datatype/P50059> ;
    reg:hasUnconstrained <http://rdaregistry.info/Elements/u/P60356> ;
    reg:lexicalAlias <http://rdaregistry.info/Elements/a/hereditaryTitle.en> ;
    reg:name "hereditaryTitle"@en ;
    reg:status <http://metadataregistry.org/uri/RegStatus/1001> ;
    rdfs:domain <http://rdaregistry.info/Elements/c/C10008> ;
    rdfs:isDefinedBy <http://rdaregistry.info/Elements/a/> ;
    skos:definition "Relates a family to a title of nobility, etc., associated with a family."@en,
        "Met une famille en relation avec un titre de noblesse, etc. associé à une famille."@fr .

<http://rdaregistry.info/Elements/a/P50060> a rdf:Property ;
    rdfs:label "has prominent member of family"@en,
        "a pour membre illustre de la famille"@fr,
        "har välkänd medlem av familjen/släkten"@sv ;
    rdakit:instructionNumber "10.6" ;
    rdakit:toolkitDefinition "A well-known individual who is a member of a family."@en,
        "Un individuo ampliamente conocido, que es miembro de una familia."@es,
        "Individu jouissant d’une certaine notoriété et qui est membre d’une famille."@fr ;
    rdakit:toolkitLabel "prominent member of family"@en,
        "miembro prominente de la familia"@es,
        "membre illustre de la famille"@fr,
        "välkänd medlem av familjen/släkten"@sv ;
    reg:hasSubproperty <http://rdaregistry.info/Elements/a/datatype/P50060> ;
    reg:hasUnconstrained <http://rdaregistry.info/Elements/u/P60362> ;
    reg:lexicalAlias <http://rdaregistry.info/Elements/a/prominentMemberOfFamily.en> ;
    reg:name "prominentMemberOfFamily"@en ;
    reg:status <http://metadataregistry.org/uri/RegStatus/1001> ;
    rdfs:domain <http://rdaregistry.info/Elements/c/C10008> ;
    rdfs:isDefinedBy <http://rdaregistry.info/Elements/a/> ;
    skos:definition "Relates a family to a well-known individual who is a member of a family."@en,
        "Met une famille en relation avec un individu jouissant d’une certaine notoriété et qui est membre d’une famille."@fr .

<http://rdaregistry.info/Elements/a/P50062> a rdf:Property ;
    rdfs:label "has founded corporate body of family"@en,
        "a pour collectivité fondée de la famille"@fr ;
    rdakit:instructionNumber "29.5" ;
    rdakit:toolkitDefinition "An organization that a family founded."@en,
        "Una entidad corporativa que la familia fundó."@es,
        "Organisation que la famille a fondée."@fr ;
    rdakit:toolkitLabel "founded corporate body of family"@en,
        "entidad corporativa fundada"@es,
        "collectivité fondée de la famille"@fr ;
    reg:hasSubproperty <http://rdaregistry.info/Elements/a/datatype/P50062>,
        <http://rdaregistry.info/Elements/a/object/P50062> ;
    reg:hasUnconstrained <http://rdaregistry.info/Elements/u/P60687> ;
    reg:lexicalAlias <http://rdaregistry.info/Elements/a/foundedCorporateBodyOfFamily.en> ;
    reg:name "foundedCorporateBodyOfFamily"@en ;
    reg:status <http://metadataregistry.org/uri/RegStatus/1001> ;
    rdfs:domain <http://rdaregistry.info/Elements/c/C10008> ;
    rdfs:isDefinedBy <http://rdaregistry.info/Elements/a/> ;
    skos:definition "Relates a family to an organization that a family founded."@en,
        "Met une famille en relation avec une organisation que la famille a fondée."@fr .

<http://rdaregistry.info/Elements/a/P50063> a rdf:Property ;
    rdfs:label "has sponsored corporate body of family"@en,
        "a pour collectivité commanditée"@fr ;
    rdakit:instructionNumber "29.5" ;
    rdakit:toolkitDefinition "An organization that a family sponsors."@en,
        "Una entidad corporativa que la familia patrocina."@es,
        "Organisation que la famille commandite."@fr ;
    rdakit:toolkitLabel "sponsored corporate body of family"@en,
        "entidad corporativa patrocinada"@es,
        "collectivité commanditée"@fr ;
    reg:hasSubproperty <http://rdaregistry.info/Elements/a/datatype/P50063>,
        <http://rdaregistry.info/Elements/a/object/P50063> ;
    reg:hasUnconstrained <http://rdaregistry.info/Elements/u/P60688> ;
    reg:lexicalAlias <http://rdaregistry.info/Elements/a/sponsoredCorporateBodyOfFamily.en> ;
    reg:name "sponsoredCorporateBodyOfFamily"@en ;
    reg:status <http://metadataregistry.org/uri/RegStatus/1001> ;
    rdfs:domain <http://rdaregistry.info/Elements/c/C10008> ;
    rdfs:isDefinedBy <http://rdaregistry.info/Elements/a/> ;
    skos:definition "Relates a family to an organization that a family sponsors."@en,
        "Met une famille en relation avec une organisation que la famille commandite."@fr .

<http://rdaregistry.info/Elements/a/P50064> a rdf:Property ;
    rdfs:label "has family history"@en,
        "a pour historique de la famille"@fr ;
    rdakit:instructionNumber "10.9" ;
    rdakit:toolkitDefinition "A summary of information about the history of a family and/or its members."@en,
        "Información biográfica sobre la familia y sus miembros"@es,
        "Information biographique sur la famille et ses membres."@fr ;
    rdakit:toolkitLabel "family history"@en,
        "historia de la familia"@es,
        "historique de la famille"@fr ;
    reg:hasSubproperty <http://rdaregistry.info/Elements/a/datatype/P50064> ;
    reg:hasUnconstrained <http://rdaregistry.info/Elements/u/P60484> ;
    reg:lexicalAlias <http://rdaregistry.info/Elements/a/familyHistory.en> ;
    reg:name "familyHistory"@en ;
    reg:status <http://metadataregistry.org/uri/RegStatus/1001> ;
    rdfs:domain <http://rdaregistry.info/Elements/c/C10008> ;
    rdfs:isDefinedBy <http://rdaregistry.info/Elements/a/> ;
    skos:definition "Relates a family to a summary of information about the history of a family and/or its members."@en,
        "Met une famille en relation avec une information biographique sur la famille et ses membres."@fr .

<http://rdaregistry.info/Elements/a/P50093> a rdf:Property ;
    rdfs:label "has undifferentiated name indicator"@en,
        "a pour indicateur de nom indifférencié"@fr,
        "har indikator för odifferentierat namn"@sv ;
    rdakit:instructionNumber "8.11" ;
    rdakit:toolkitDefinition "A categorization indicating that the core elements recorded are insufficient to differentiate between two or more persons with the same name."@en,
        "Una categorización que indica que los elementos núcleo registrados son insuficientes para diferenciar dos o más personas con el mismo nombre."@es,
        "Catégorisation indiquant que les éléments fondamentaux enregistrés sont insuffisants pour distinguer deux ou plusieurs personnes portant le même nom."@fr ;
    rdakit:toolkitLabel "undifferentiated name indicator"@en,
        "indicador de nombre no diferenciado"@es,
        "indicateur de nom indifférencié"@fr,
        "indikator för odifferentierat namn"@sv ;
    reg:hasSubproperty <http://rdaregistry.info/Elements/a/datatype/P50093> ;
    reg:hasUnconstrained <http://rdaregistry.info/Elements/u/P60046> ;
    reg:lexicalAlias <http://rdaregistry.info/Elements/a/undifferentiatedNameIndicator.en> ;
    reg:name "undifferentiatedNameIndicator"@en ;
    reg:status <http://metadataregistry.org/uri/RegStatus/1001> ;
    rdfs:domain <http://rdaregistry.info/Elements/c/C10004> ;
    rdfs:isDefinedBy <http://rdaregistry.info/Elements/a/> ;
    skos:definition "Relates a person to a categorization indicating that the core elements recorded are insufficient to differentiate between two or more persons with the same name."@en,
        "Met une personne en relation avec une catégorisation indiquant que les éléments fondamentaux enregistrés sont insuffisants pour distinguer deux ou plusieurs personnes portant le même nom."@fr .

<http://rdaregistry.info/Elements/a/P50094> a rdf:Property ;
    rdfs:label "has identifier for person"@en,
        "a pour identifiant de la personne"@fr,
        "har identifikator för personen"@sv ;
    rdakit:instructionNumber "9.18" ;
    rdakit:toolkitDefinition "A character string uniquely associated with a person, or with a surrogate such as an authority record for a person."@en,
        "Una cadena de caracteres asociados de manera unívoca con una persona, o un sustituto de la persona (p.ej., un registro de autoridad)."@es,
        "Chaîne de caractères associée de manière unique à une personne ou à un substitut d’une personne (par exemple, une notice d’autorité)."@fr ;
    rdakit:toolkitLabel "identifier for person"@en,
        "identificador de la persona"@es,
        "identifiant de la personne"@fr,
        "identifikator för personen"@sv ;
    reg:hasSubproperty <http://rdaregistry.info/Elements/a/datatype/P50094> ;
    reg:hasUnconstrained <http://rdaregistry.info/Elements/u/P60053> ;
    reg:lexicalAlias <http://rdaregistry.info/Elements/a/identifierForPerson.en> ;
    reg:name "identifierForPerson"@en ;
    reg:status <http://metadataregistry.org/uri/RegStatus/1001> ;
    rdfs:domain <http://rdaregistry.info/Elements/c/C10004> ;
    rdfs:isDefinedBy <http://rdaregistry.info/Elements/a/> ;
    skos:definition "Relates a person to a character string uniquely associated with a person, or with a surrogate such as an authority record for a person."@en,
        "Met une personne en relation avec une chaîne de caractères associée de manière unique à une personne ou à un substitut d’une personne (par exemple, une notice d’autorité)."@fr ;
    skos:scopeNote "The identifier serves to differentiate that person from other persons."@en,
        "L’identifiant sert à distinguer cette personne d’autres personnes."@fr .

<http://rdaregistry.info/Elements/a/P50095> a rdf:Property ;
    rdfs:label "has corporate body"@en,
        "a pour collectivité"@fr ;
    rdakit:instructionNumber "29.5" ;
    rdakit:toolkitDefinition "A corporate body of which a person is a member."@en,
        "Una entidad corporativa de la cual es miembro una persona."@es,
        "Collectivité (groupe d’interprètes, expédition, etc) dont la personne est membre."@fr ;
    rdakit:toolkitLabel "corporate body"@en,
        "entidad corporativa"@es,
        "collectivité"@fr ;
    reg:hasSubproperty <http://rdaregistry.info/Elements/a/datatype/P50095>,
        <http://rdaregistry.info/Elements/a/object/P50095> ;
    reg:hasUnconstrained <http://rdaregistry.info/Elements/u/P60648> ;
    reg:lexicalAlias <http://rdaregistry.info/Elements/a/corporateBody.en> ;
    reg:name "corporateBody"@en ;
    reg:status <http://metadataregistry.org/uri/RegStatus/1001> ;
    rdfs:domain <http://rdaregistry.info/Elements/c/C10004> ;
    rdfs:isDefinedBy <http://rdaregistry.info/Elements/a/> ;
    skos:definition "Relates a person to a corporate body of which a person is a member."@en,
        "Met une personne en relation avec une collectivité (groupe d’interprètes, expédition, etc) dont la personne est membre."@fr .

<http://rdaregistry.info/Elements/a/P50096> a rdf:Property ;
    rdfs:label "has employer"@en,
        "a pour employeur"@fr ;
    rdakit:instructionNumber "29.5" ;
    rdakit:toolkitDefinition "A corporate body that employs a person."@en,
        "Una entidad corporativa que emplea a la persona."@es,
        "Collectivité qui emploie la personne."@fr ;
    rdakit:toolkitLabel "employer"@en,
        "empleador"@es,
        "employeur"@fr ;
    reg:hasSubproperty <http://rdaregistry.info/Elements/a/datatype/P50096>,
        <http://rdaregistry.info/Elements/a/object/P50096> ;
    reg:hasUnconstrained <http://rdaregistry.info/Elements/u/P60679> ;
    reg:lexicalAlias <http://rdaregistry.info/Elements/a/employer.en> ;
    reg:name "employer"@en ;
    reg:status <http://metadataregistry.org/uri/RegStatus/1001> ;
    rdfs:domain <http://rdaregistry.info/Elements/c/C10004> ;
    rdfs:isDefinedBy <http://rdaregistry.info/Elements/a/> ;
    skos:definition "Relates a person to a corporate body that employs a person."@en,
        "Met une personne en relation avec une collectivité qui emploie la personne."@fr .

<http://rdaregistry.info/Elements/a/P50097> a rdf:Property ;
    rdfs:label "has country associated with person"@en,
        "a pour pays associé à la personne"@fr,
        "har land förknippat med personen"@sv ;
    rdakit:instructionNumber "9.1" ;
    rdakit:toolkitDefinition "A country with which a person is identified."@en,
        "Un país con el que se identifica la persona"@es,
        "Pays auquel une personne est identifiée."@fr ;
    rdakit:toolkitLabel "country associated with person"@en,
        "país asociado con la persona"@es,
        "pays associé à la personne"@fr,
        "land förknippat med personen"@sv ;
    reg:hasSubproperty <http://rdaregistry.info/Elements/a/datatype/P50097> ;
    reg:hasUnconstrained <http://rdaregistry.info/Elements/u/P60063> ;
    reg:lexicalAlias <http://rdaregistry.info/Elements/a/countryAssociatedWithPerson.en> ;
    reg:name "countryAssociatedWithPerson"@en ;
    reg:status <http://metadataregistry.org/uri/RegStatus/1001> ;
    rdfs:domain <http://rdaregistry.info/Elements/c/C10004> ;
    rdfs:isDefinedBy <http://rdaregistry.info/Elements/a/> ;
    skos:definition "Relates a person to a country with which a person is identified."@en,
        "Met une personne en relation avec un pays auquel une personne est identifiée."@fr .

<http://rdaregistry.info/Elements/a/P50099> a rdf:Property ;
    rdfs:label "has descendants"@en,
        "a pour descendants"@fr ;
    rdakit:instructionNumber "29.5" ;
    rdakit:toolkitDefinition "A family descended from a particular person."@en,
        "Una familia que desciende de una persona determinada."@es,
        "Famille descendant de la personne particulière."@fr ;
    rdakit:toolkitLabel "descendants"@en,
        "descendientes"@es,
        "descendants"@fr ;
    reg:hasSubproperty <http://rdaregistry.info/Elements/a/datatype/P50099>,
        <http://rdaregistry.info/Elements/a/object/P50099> ;
    reg:hasUnconstrained <http://rdaregistry.info/Elements/u/P60686> ;
    reg:lexicalAlias <http://rdaregistry.info/Elements/a/descendants.en> ;
    reg:name "descendants"@en ;
    reg:status <http://metadataregistry.org/uri/RegStatus/1001> ;
    rdfs:domain <http://rdaregistry.info/Elements/c/C10004> ;
    rdfs:isDefinedBy <http://rdaregistry.info/Elements/a/> ;
    skos:definition "Relates a person to a family descended from a particular person."@en,
        "Met une personne en relation avec une famille descendant de la personne particulière."@fr .

<http://rdaregistry.info/Elements/a/P50100> a rdf:Property ;
    rdfs:label "has field of activity of person"@en,
        "a pour domaine d’activité de la personne"@fr ;
    rdakit:instructionNumber "9.15" ;
    rdakit:toolkitDefinition "A field of endeavour, area of expertise, etc., in which a person is engaged or was engaged."@en,
        "Un área de trabajo, área de pericia, etc., en el que la persona está o estuvo involucrada."@es,
        "Champ d’action, domaine du savoir, etc. dans lequel s’investit ou s’est investie la personne."@fr ;
    rdakit:toolkitLabel "field of activity of person"@en,
        "campo de actividad de la persona"@es,
        "domaine d’activité de la personne"@fr ;
    reg:hasSubproperty <http://rdaregistry.info/Elements/a/datatype/P50100> ;
    reg:hasUnconstrained <http://rdaregistry.info/Elements/u/P60089> ;
    reg:lexicalAlias <http://rdaregistry.info/Elements/a/fieldOfActivityOfPerson.en> ;
    reg:name "fieldOfActivityOfPerson"@en ;
    reg:status <http://metadataregistry.org/uri/RegStatus/1001> ;
    rdfs:domain <http://rdaregistry.info/Elements/c/C10004> ;
    rdfs:isDefinedBy <http://rdaregistry.info/Elements/a/> ;
    skos:definition "Relates a person to a field of endeavour, area of expertise, etc., in which a person is engaged or was engaged."@en,
        "Met une personne en relation avec un champ d’action, un domaine du savoir, etc. dans lequel s’investit ou s’est investie la personne."@fr .

<http://rdaregistry.info/Elements/a/P50101> a rdf:Property ;
    rdfs:label "has affiliation"@en,
        "a pour affiliation"@fr,
        "har organisatorisk tillhörighet"@sv ;
    rdakit:instructionNumber "9.13" ;
    rdakit:toolkitDefinition "A group with which a person is affiliated or has been affiliated through employment, membership, cultural identity, etc."@en,
        "Un grupo con el que la persona está afiliada, o ha estado afiliada, mediante empleo, membresía, identidad cultural, etc."@es,
        "Groupe auquel une personne est ou a été affiliée par recrutement, acquisition de la qualité de membre, identité culturelle, etc."@fr ;
    rdakit:toolkitLabel "affiliation"@en,
        "afiliación"@es,
        "affiliation"@fr,
        "organisatorisk tillhörighet"@sv ;
    reg:hasSubproperty <http://rdaregistry.info/Elements/a/datatype/P50101> ;
    reg:hasUnconstrained <http://rdaregistry.info/Elements/u/P60095> ;
    reg:lexicalAlias <http://rdaregistry.info/Elements/a/affiliation.en> ;
    reg:name "affiliation"@en ;
    reg:status <http://metadataregistry.org/uri/RegStatus/1001> ;
    rdfs:domain <http://rdaregistry.info/Elements/c/C10004> ;
    rdfs:isDefinedBy <http://rdaregistry.info/Elements/a/> ;
    skos:definition "Relates a person to a group with which a person is affiliated or has been affiliated through employment, membership, cultural identity, etc."@en,
        "Met une personne en relation avec un groupe auquel une personne est ou a été affiliée par recrutement, acquisition de la qualité de membre, identité culturelle, etc."@fr .

<http://rdaregistry.info/Elements/a/P50102> a rdf:Property ;
    rdfs:label "has language of person"@en,
        "a pour langue de la personne"@fr ;
    rdakit:instructionNumber "9.14" ;
    rdakit:toolkitDefinition "A language a person uses when writing for publication, broadcasting, etc."@en,
        "Una lengua que una persona utiliza cuando escribe para publicaciones, transmisiones, etc."@es,
        "Langue utilisée par la personne quand elle écrit en vue d’une publication, d’une radiodiffusion, etc."@fr ;
    rdakit:toolkitLabel "language of person"@en,
        "lengua de la persona"@es,
        "langue de la personne"@fr ;
    reg:hasSubproperty <http://rdaregistry.info/Elements/a/datatype/P50102> ;
    reg:hasUnconstrained <http://rdaregistry.info/Elements/u/P60098> ;
    reg:lexicalAlias <http://rdaregistry.info/Elements/a/languageOfPerson.en> ;
    reg:name "languageOfPerson"@en ;
    reg:status <http://metadataregistry.org/uri/RegStatus/1001> ;
    rdfs:domain <http://rdaregistry.info/Elements/c/C10004> ;
    rdfs:isDefinedBy <http://rdaregistry.info/Elements/a/> ;
    skos:definition "Relates a person to a language a person uses when writing for publication, broadcasting, etc."@en,
        "Met une personne en relation avec une langue utilisée par la personne quand elle écrit en vue d’une publication, d’une radiodiffusion, etc."@fr .

<http://rdaregistry.info/Elements/a/P50104> a rdf:Property ;
    rdfs:label "has profession or occupation"@en,
        "a pour profession ou occupation"@fr,
        "har yrke eller sysselsättning"@sv ;
    rdakit:instructionNumber "9.16" ;
    rdakit:toolkitDefinition "A person's vocation or avocation."@en,
        "Vocación o pasatiempo de una persona."@es,
        "La profession ou le passe-temps d’une personne."@fr ;
    rdakit:toolkitLabel "profession or occupation"@en,
        "profesión u ocupación"@es,
        "profession ou occupation"@fr,
        "yrke eller sysselsättning"@sv ;
    reg:hasSubproperty <http://rdaregistry.info/Elements/a/datatype/P50104> ;
    reg:hasUnconstrained <http://rdaregistry.info/Elements/u/P60468> ;
    reg:lexicalAlias <http://rdaregistry.info/Elements/a/professionOrOccupation.en> ;
    reg:name "professionOrOccupation"@en ;
    reg:status <http://metadataregistry.org/uri/RegStatus/1001> ;
    rdfs:domain <http://rdaregistry.info/Elements/c/C10004> ;
    rdfs:isDefinedBy <http://rdaregistry.info/Elements/a/> ;
    skos:definition "Relates a person to a person's vocation or avocation."@en,
        "Met une personne en relation avec la profession ou le passe-temps d’une personne."@fr .

<http://rdaregistry.info/Elements/a/P50105> a rdf:Property ;
    rdfs:label "has alternate identity"@en,
        "a pour identité alternative"@fr ;
    rdakit:instructionNumber "29.5" ;
    rdakit:toolkitDefinition "A pseudonymous or other identity assumed by a person."@en,
        "Un seudónimo u otra identidad asumida por la persona."@es,
        "Pseudonyme ou autre identité adoptée par la personne."@fr ;
    rdakit:toolkitLabel "alternate identity"@en,
        "identidad alternativa"@es,
        "identité alternative"@fr ;
    reg:hasSubproperty <http://rdaregistry.info/Elements/a/datatype/P50105>,
        <http://rdaregistry.info/Elements/a/object/P50105> ;
    reg:hasUnconstrained <http://rdaregistry.info/Elements/u/P60036> ;
    reg:lexicalAlias <http://rdaregistry.info/Elements/a/alternateIdentity.en> ;
    reg:name "alternateIdentity"@en ;
    reg:status <http://metadataregistry.org/uri/RegStatus/1001> ;
    rdfs:domain <http://rdaregistry.info/Elements/c/C10004> ;
    rdfs:isDefinedBy <http://rdaregistry.info/Elements/a/> ;
    skos:definition "Relates a person to a pseudonymous or other identity assumed by a person."@en,
        "Met une personne en relation avec un pseudonyme ou une autre identité adoptée par la personne."@fr .

<http://rdaregistry.info/Elements/a/P50106> a rdf:Property ;
    rdfs:label "has real identity"@en,
        "a pour identité réelle"@fr ;
    rdakit:instructionNumber "29.5" ;
    rdakit:toolkitDefinition "A real person who assumes an alternate identity."@en,
        "Una persona real que asume la identidad alternativa."@es,
        "Personne réelle qui adopte l’identité alternative."@fr ;
    rdakit:toolkitLabel "real identity"@en,
        "identidad real"@es,
        "identité réelle"@fr ;
    reg:hasSubproperty <http://rdaregistry.info/Elements/a/datatype/P50106>,
        <http://rdaregistry.info/Elements/a/object/P50106> ;
    reg:hasUnconstrained <http://rdaregistry.info/Elements/u/P60037> ;
    reg:lexicalAlias <http://rdaregistry.info/Elements/a/realIdentity.en> ;
    reg:name "realIdentity"@en ;
    reg:status <http://metadataregistry.org/uri/RegStatus/1001> ;
    rdfs:domain <http://rdaregistry.info/Elements/c/C10004> ;
    rdfs:isDefinedBy <http://rdaregistry.info/Elements/a/> ;
    skos:definition "Relates a person to a real person who assumes an alternate identity."@en,
        "Met une personne en relation avec une personne réelle qui adopte l’identité alternative."@fr .

<http://rdaregistry.info/Elements/a/P50108> a rdf:Property ;
    rdfs:label "has other designation associated with person"@en,
        "a pour autre information associée à la personne"@fr,
        "har övrig beteckning förknippad med personen"@sv ;
    rdakit:instructionNumber "9.6" ;
    rdakit:toolkitDefinition "A term other than a title that is associated with a person."@en,
        "Un término diferente de un título que está asociado con el nombre de la persona."@es,
        "Terme, autre qu’un titre, associé à un nom de personne."@fr ;
    rdakit:toolkitLabel "other designation associated with person"@en,
        "otra designación asociada con la persona"@es,
        "autre information associée à la personne"@fr,
        "övrig beteckning förknippad med personen"@sv ;
    reg:hasSubproperty <http://rdaregistry.info/Elements/a/datatype/P50108> ;
    reg:hasUnconstrained <http://rdaregistry.info/Elements/u/P60370> ;
    reg:lexicalAlias <http://rdaregistry.info/Elements/a/otherDesignationAssociatedWithPerson.en> ;
    reg:name "otherDesignationAssociatedWithPerson"@en ;
    reg:status <http://metadataregistry.org/uri/RegStatus/1001> ;
    rdfs:domain <http://rdaregistry.info/Elements/c/C10004> ;
    rdfs:isDefinedBy <http://rdaregistry.info/Elements/a/> ;
    skos:definition "Relates a person to a term other than a title that is associated with a person's name."@en,
        "Met une personne en relation avec un terme, autre qu’un titre, associé à un nom de personne."@fr .

<http://rdaregistry.info/Elements/a/P50109> a rdf:Property ;
    rdfs:label "has place of residence, etc."@en,
        "a pour lieu de résidence"@fr,
        "har bostadsort"@sv ;
    rdakit:instructionNumber "9.11" ;
    rdakit:toolkitDefinition "A town, city, province, state, and/or country in which a person resides or has resided, or another significant place associated with a person other than place of birth, place of death, or residence."@en,
        "Un poblado, ciudad, provincia, estado y/o país en el que residió o ha residido una persona, u otro lugar significativo asociado con la persona diferente del lugar de nacimiento, fallecimiento o residencia (por ej., un lugar donde la persona ha trabajado o estudiado)."@es,
        "Municipalité, ville, province, État et/ou pays où une personne réside ou a résidé, ou autre lieu important associé à la personne et autre qu’un lieu de naissance, de décès ou de résidence (par exemple, un lieu où la personne a travaillé ou étudié)."@fr ;
    rdakit:toolkitLabel "place of residence, etc."@en,
        "lugar de residencia"@es,
        "lieu de résidence"@fr,
        "bostadsort"@sv ;
    reg:hasSubproperty <http://rdaregistry.info/Elements/a/datatype/P50109> ;
    reg:hasUnconstrained <http://rdaregistry.info/Elements/u/P60360> ;
    reg:lexicalAlias <http://rdaregistry.info/Elements/a/placeOfResidenceEtc.en> ;
    reg:name "placeOfResidenceEtc"@en ;
    reg:status <http://metadataregistry.org/uri/RegStatus/1001> ;
    rdfs:domain <http://rdaregistry.info/Elements/c/C10004> ;
    rdfs:isDefinedBy <http://rdaregistry.info/Elements/a/> ;
    skos:definition "Relates a person to a town, city, province, state, and/or country in which a person resides or has resided, or another significant place associated with the person other than place of birth, place of death, or residence."@en,
        "Met une personne en relation avec une municipalité, une ville, une province, un État et/ou un pays où une personne réside ou a résidé, ou un autre lieu important associé à la personne et autre qu’un lieu de naissance, de décès ou de résidence (par exemple, un lieu où la personne a travaillé ou étudié)."@fr ;
    skos:scopeNote "A place where a person has worked or studied is included."@en .

<http://rdaregistry.info/Elements/a/P50110> a rdf:Property ;
    rdfs:label "has title of person"@en,
        "a pour titre de la personne"@fr ;
    rdakit:instructionNumber "9.4" ;
    rdakit:toolkitDefinition "A word or phrase indicative of royalty, nobility, ecclesiastical rank or office, or a term of address for a person of religious vocation."@en,
        "Una palabra o frase que indica realeza, nobleza o rango o cargo eclesiástico o un término de tratamiento de una persona de vocación religiosa."@es,
        "Mot ou expression indiquant la royauté, la noblesse ou un rang ou une fonction ecclésiastiques, un terme de politesse pour une personne à vocation religieuse ou un autre terme indiquant un rang, un honneur ou une fonction."@fr ;
    rdakit:toolkitLabel "title of person"@en,
        "título de la persona"@es,
        "titre de la personne"@fr ;
    reg:hasSubproperty <http://rdaregistry.info/Elements/a/datatype/P50110> ;
    reg:hasUnconstrained <http://rdaregistry.info/Elements/u/P60363> ;
    reg:lexicalAlias <http://rdaregistry.info/Elements/a/titleOfPerson.en> ;
    reg:name "titleOfPerson"@en ;
    reg:status <http://metadataregistry.org/uri/RegStatus/1001> ;
    rdfs:domain <http://rdaregistry.info/Elements/c/C10004> ;
    rdfs:isDefinedBy <http://rdaregistry.info/Elements/a/> ;
    skos:definition "Relates a person to a word or phrase indicative of royalty, nobility, ecclesiastical rank or office, or a term of address for a person of religious vocation."@en,
        "Met une personne en relation avec un mot ou une expression indiquant la royauté, la noblesse ou un rang ou une fonction ecclésiastiques, un terme de politesse pour une personne à vocation religieuse ou un autre terme indiquant un rang, un honneur ou une fonction."@fr ;
    skos:scopeNote "A title of the person includes other terms indicative of rank, honour, or office, including initials or abbreviations representing an academic degree, or membership in an organization, and excludes terms of address that simply indicate gender or marital status such as Mr. or Mrs."@en,
        "Le titre de la personne exclut les termes de politesse qui indiquent simplement le sexe ou le statut marital (par exemple, M., Mme)."@fr .

<http://rdaregistry.info/Elements/a/P50112> a rdf:Property ;
    rdfs:label "has founded corporate body of person"@en,
        "a pour collectivité fondée de la personne"@fr ;
    rdakit:instructionNumber "29.5" ;
    rdakit:toolkitDefinition "An organization that a person founded."@en,
        "Una organización que la persona fundó."@es,
        "Organisation que la personne a fondée."@fr ;
    rdakit:toolkitLabel "founded corporate body of person"@en,
        "entidad corporativa fundada"@es,
        "collectivité fondée de la personne"@fr ;
    reg:hasSubproperty <http://rdaregistry.info/Elements/a/datatype/P50112>,
        <http://rdaregistry.info/Elements/a/object/P50112> ;
    reg:hasUnconstrained <http://rdaregistry.info/Elements/u/P60687> ;
    reg:lexicalAlias <http://rdaregistry.info/Elements/a/foundedCorporateBodyOfPerson.en> ;
    reg:name "foundedCorporateBodyOfPerson"@en ;
    reg:status <http://metadataregistry.org/uri/RegStatus/1001> ;
    rdfs:domain <http://rdaregistry.info/Elements/c/C10004> ;
    rdfs:isDefinedBy <http://rdaregistry.info/Elements/a/> ;
    skos:definition "Relates a person to an organization that a person founded."@en,
        "Met une personne en relation avec une organisation que la personne a fondée."@fr .

<http://rdaregistry.info/Elements/a/P50113> a rdf:Property ;
    rdfs:label "has biographical information"@en,
        "a pour information biographique"@fr,
        "har biografisk information"@sv ;
    rdakit:instructionNumber "9.17" ;
    rdakit:toolkitDefinition "A summary of information about the life or history of a person."@en,
        "Información perteneciente a la vida o historia de una persona."@es,
        "Information relative à la vie ou à l’histoire d’une personne."@fr ;
    rdakit:toolkitLabel "biographical information"@en,
        "información biográfica"@es,
        "information biographique"@fr,
        "biografisk information"@sv ;
    reg:hasSubproperty <http://rdaregistry.info/Elements/a/datatype/P50113> ;
    reg:hasUnconstrained <http://rdaregistry.info/Elements/u/P60492> ;
    reg:lexicalAlias <http://rdaregistry.info/Elements/a/biographicalInformation.en> ;
    reg:name "biographicalInformation"@en ;
    reg:status <http://metadataregistry.org/uri/RegStatus/1001> ;
    rdfs:domain <http://rdaregistry.info/Elements/c/C10004> ;
    rdfs:isDefinedBy <http://rdaregistry.info/Elements/a/> ;
    skos:definition "Relates a person to a summary of information about the life or history of a person."@en,
        "Met une personne en relation avec une information relative à la vie ou à l’histoire d’une personne."@fr .

<http://rdaregistry.info/Elements/a/P50114> a rdf:Property ;
    rdfs:label "has address of person"@en,
        "a pour adresse de la personne"@fr ;
    rdakit:instructionNumber "9.12" ;
    rdakit:toolkitDefinition "An address of a person."@en,
        "La dirección de una persona."@es,
        "L’adresse du lieu de résidence, de travail, l’adresse de l’employeur d’une personne et/ou son adresse électronique ou son adresse de site Web."@fr ;
    rdakit:toolkitLabel "address of person"@en,
        "dirección de la persona"@es,
        "adresse de la personne"@fr ;
    reg:hasSubproperty <http://rdaregistry.info/Elements/a/datatype/P50114> ;
    reg:hasUnconstrained <http://rdaregistry.info/Elements/u/P60512> ;
    reg:lexicalAlias <http://rdaregistry.info/Elements/a/addressOfPerson.en> ;
    reg:name "addressOfPerson"@en ;
    reg:status <http://metadataregistry.org/uri/RegStatus/1001> ;
    rdfs:domain <http://rdaregistry.info/Elements/c/C10004> ;
    rdfs:isDefinedBy <http://rdaregistry.info/Elements/a/> ;
    skos:definition "Relates a person to an address of a person's place of residence, business, or employer, and/or an e-mail or internet address."@en,
        "Met une personne en relation avec l’adresse du lieu de résidence, de travail, l’adresse de l’employeur d’une personne et/ou son adresse électronique ou son adresse de site Web."@fr .

<http://rdaregistry.info/Elements/a/P50115> a rdf:Property ;
    rdfs:label "has fuller form of name"@en,
        "a pour forme développée du nom"@fr,
        "har fullständig namnform"@sv ;
    rdakit:instructionNumber "9.5" ;
    rdakit:toolkitDefinition "A name or names associated with a person that includes the fuller form of a part of any name represented only by an initial, abbreviation, or shortened or otherwise modified variant in the form chosen as the preferred name and/or a part of the name not included in the form chosen as the preferred name."@en,
        "La forma completa de una parte de un nombre representado solo por una inicial o abreviatura en la forma escogida como el nombre preferido, o una parte del nombre no incluida en la forma elegida como el nombre preferido."@es,
        "La forme développée d’une partie d’un nom représentée seulement par une initiale ou une abréviation dans la forme choisie comme nom privilégié, ou une partie du nom non incluse dans la forme choisie comme nom privilégié."@fr ;
    rdakit:toolkitLabel "fuller form of name"@en,
        "forma más completa del nombre"@es,
        "forme développée du nom"@fr,
        "fullständig namnform"@sv ;
    reg:hasSubproperty <http://rdaregistry.info/Elements/a/datatype/P50115> ;
    reg:hasUnconstrained <http://rdaregistry.info/Elements/u/P60530> ;
    reg:lexicalAlias <http://rdaregistry.info/Elements/a/fullerFormOfName.en> ;
    reg:name "fullerFormOfName"@en ;
    reg:status <http://metadataregistry.org/uri/RegStatus/1001> ;
    rdfs:domain <http://rdaregistry.info/Elements/c/C10004> ;
    rdfs:isDefinedBy <http://rdaregistry.info/Elements/a/> ;
    skos:definition "Relates a person to a name or names associated with a person that includes the fuller form of a part of any name represented only by an initial, abbreviation, or shortened or otherwise modified variant in the form chosen as the preferred name and/or a part of the name not included in the form chosen as the preferred name."@en,
        "Met une personne en relation avec la forme développée d’une partie d’un nom représentée seulement par une initiale ou une abréviation dans la forme choisie comme nom privilégié, ou une partie du nom non incluse dans la forme choisie comme nom privilégié."@fr .

<http://rdaregistry.info/Elements/a/P50116> a rdf:Property ;
    rdfs:label "has gender"@en,
        "a pour sexe"@fr,
        "har kön"@sv ;
    rdakit:instructionNumber "9.7" ;
    rdakit:toolkitDefinition "A gender with which a person identifies."@en,
        "El género con el que se identifica la persona."@es,
        "Le sexe auquel une personne s’identifie."@fr ;
    rdakit:toolkitLabel "gender"@en,
        "género"@es,
        "sexe"@fr,
        "kön"@sv ;
    reg:hasSubproperty <http://rdaregistry.info/Elements/a/datatype/P50116> ;
    reg:hasUnconstrained <http://rdaregistry.info/Elements/u/P60531> ;
    reg:lexicalAlias <http://rdaregistry.info/Elements/a/gender.en> ;
    reg:name "gender"@en ;
    reg:status <http://metadataregistry.org/uri/RegStatus/1001> ;
    rdfs:domain <http://rdaregistry.info/Elements/c/C10004> ;
    rdfs:isDefinedBy <http://rdaregistry.info/Elements/a/> ;
    skos:definition "Relates a person to a gender with which a person identifies."@en,
        "Met une personne en relation avec le sexe auquel une personne s’identifie."@fr .

<http://rdaregistry.info/Elements/a/P50118> a rdf:Property ;
    rdfs:label "has place of death"@en,
        "a pour lieu de décès"@fr,
        "har dödsort"@sv ;
    rdakit:instructionNumber "9.9" ;
    rdakit:toolkitDefinition "A town, city, province, state, and/or country in which a person died."@en,
        "El poblado, ciudad, provincia, estado y/o país en el que murió la persona."@es,
        "La municipalité, la ville, la province, l’État et/ou le pays où une personne est morte."@fr ;
    rdakit:toolkitLabel "place of death"@en,
        "lugar de fallecimiento"@es,
        "lieu de décès"@fr,
        "dödsort"@sv ;
    reg:hasSubproperty <http://rdaregistry.info/Elements/a/datatype/P50118> ;
    reg:hasUnconstrained <http://rdaregistry.info/Elements/u/P60592> ;
    reg:lexicalAlias <http://rdaregistry.info/Elements/a/placeOfDeath.en> ;
    reg:name "placeOfDeath"@en ;
    reg:status <http://metadataregistry.org/uri/RegStatus/1001> ;
    rdfs:domain <http://rdaregistry.info/Elements/c/C10004> ;
    rdfs:isDefinedBy <http://rdaregistry.info/Elements/a/> ;
    skos:definition "Relates a person to a town, city, province, state, and/or country in which a person died."@en,
        "Met une personne en relation avec la municipalité, la ville, la province, l’État et/ou le pays où une personne est morte."@fr .

<http://rdaregistry.info/Elements/a/P50119> a rdf:Property ;
    rdfs:label "has place of birth"@en,
        "a pour lieu de naissance"@fr,
        "har födelseort"@sv ;
    rdakit:instructionNumber "9.8" ;
    rdakit:toolkitDefinition "A town, city, province, state, and/or country in which a person was born."@en,
        "El poblado, ciudad, provincia, estado y/o país en el que nació la persona."@es,
        "La municipalité, la ville, la province, l’État et/ou le pays où une personne est née."@fr ;
    rdakit:toolkitLabel "place of birth"@en,
        "lugar de nacimiento"@es,
        "lieu de naissance"@fr,
        "födelseort"@sv ;
    reg:hasSubproperty <http://rdaregistry.info/Elements/a/datatype/P50119> ;
    reg:hasUnconstrained <http://rdaregistry.info/Elements/u/P60593> ;
    reg:lexicalAlias <http://rdaregistry.info/Elements/a/placeOfBirth.en> ;
    reg:name "placeOfBirth"@en ;
    reg:status <http://metadataregistry.org/uri/RegStatus/1001> ;
    rdfs:domain <http://rdaregistry.info/Elements/c/C10004> ;
    rdfs:isDefinedBy <http://rdaregistry.info/Elements/a/> ;
    skos:definition "Relates a person to a town, city, province, state, and/or country in which a person was born."@en,
        "Met une personne en relation avec la municipalité, la ville, la province, l’État et/ou le pays où une personne est née."@fr .

<http://rdaregistry.info/Elements/a/P50122> a rdf:Property ;
    rdfs:label "is appellant person of"@en,
        "est la personne appelante de"@fr ;
    rdakit:instructionNumber "18.5" ;
    rdakit:toolkitDefinition "A legal work of a higher court recording a decision of a lower court that is appealed by a person."@en,
        "Personne qui en appelle de la décision d’un tribunal inférieur."@fr ;
    rdakit:toolkitLabel "appellant person of"@en,
        "personne appelante de"@fr ;
    reg:hasSubproperty <http://rdaregistry.info/Elements/a/datatype/P50122>,
        <http://rdaregistry.info/Elements/a/object/P50122> ;
    reg:hasUnconstrained <http://rdaregistry.info/Elements/u/P60691> ;
    reg:lexicalAlias <http://rdaregistry.info/Elements/a/appellantPersonOf.en> ;
    reg:name "appellantPersonOf"@en ;
    reg:status <http://metadataregistry.org/uri/RegStatus/1001> ;
    rdfs:domain <http://rdaregistry.info/Elements/c/C10004> ;
    rdfs:isDefinedBy <http://rdaregistry.info/Elements/a/> ;
    rdfs:subPropertyOf <http://rdaregistry.info/Elements/a/P50088> ;
    skos:definition "Relates a person who appeals a decision of a lower court recorded in a legal work of a higher court to a work."@en,
        "Met une personne qui en appelle de la décision d’un tribunal inférieur en relation avec l’œuvre."@fr .

<http://rdaregistry.info/Elements/a/P50148> a rdf:Property ;
    rdfs:label "is court reporter of"@en,
        "est le rapporteur judiciaire de"@fr ;
    rdakit:instructionNumber "18.5" ;
    rdakit:toolkitDefinition "An expression of a work that incorporates a contribution of preparing a court's opinions for publication."@en,
        "Personne, famille ou collectivité contribuant à une expression d’une œuvre en préparant les opinions d’un tribunal aux fins de publication."@fr ;
    rdakit:toolkitLabel "court reporter of"@en,
        "rapporteur judiciaire de"@fr ;
    reg:hasSubproperty <http://rdaregistry.info/Elements/a/datatype/P50148>,
        <http://rdaregistry.info/Elements/a/object/P50148> ;
    reg:hasUnconstrained <http://rdaregistry.info/Elements/u/P60616> ;
    reg:lexicalAlias <http://rdaregistry.info/Elements/a/courtReporterOf.en> ;
    reg:name "courtReporterOf"@en ;
    reg:status <http://metadataregistry.org/uri/RegStatus/1001> ;
    rdfs:domain <http://rdaregistry.info/Elements/c/C10002> ;
    rdfs:isDefinedBy <http://rdaregistry.info/Elements/a/> ;
    rdfs:subPropertyOf <http://rdaregistry.info/Elements/a/P50161> ;
    skos:definition "Relates an agent contributing to an expression of a work by preparing a court's opinions for publication to an expression."@en,
        "Met une personne, famille ou collectivité contribuant à une expression d’une œuvre en préparant les opinions d’un tribunal aux fins de publication en relation avec l’expression."@fr .

<http://rdaregistry.info/Elements/a/P50164> a rdf:Property ;
    rdfs:label "is custodian of"@en,
        "est le dépositaire de"@fr ;
    rdakit:instructionNumber "18.5" ;
    rdakit:toolkitDefinition "An item in the legal custody of an agent."@en,
        "Personne, famille ou collectivité à qui est confiée la garde légale d’un item."@fr ;
    rdakit:toolkitLabel "custodian of"@en,
        "dépositaire de"@fr ;
    reg:hasSubproperty <http://rdaregistry.info/Elements/a/datatype/P50164>,
        <http://rdaregistry.info/Elements/a/object/P50164> ;
    reg:hasUnconstrained <http://rdaregistry.info/Elements/u/P60631> ;
    reg:lexicalAlias <http://rdaregistry.info/Elements/a/custodianOf.en> ;
    reg:name "custodianOf"@en ;
    reg:status <http://metadataregistry.org/uri/RegStatus/1001> ;
    rdfs:domain <http://rdaregistry.info/Elements/c/C10002> ;
    rdfs:isDefinedBy <http://rdaregistry.info/Elements/a/> ;
    rdfs:subPropertyOf <http://rdaregistry.info/Elements/a/P50308> ;
    skos:definition "Relates an agent having legal custody of an item to an item."@en,
        "Met une personne, famille ou collectivité à qui est confiée la garde légale d’un item en relation avec l’item."@fr .

<http://rdaregistry.info/Elements/a/P50180> a rdf:Property ;
    rdfs:label "is presenter of"@en,
        "est le présentateur de"@fr ;
    rdakit:instructionNumber "18.5" ;
    rdakit:toolkitDefinition "A manifestation for moving image materials with an \"X presents:\" credit for an agent who is probably associated with production, finance, or distribution in some way."@en,
        "Personne, famille ou collectivité mentionnée dans un générique d’images animées sous la forme « X présente » et qui est probablement associée d’une façon quelconque à la production, au financement ou à la distribution."@fr ;
    rdakit:toolkitLabel "presenter of"@en,
        "présentateur de"@fr ;
    reg:hasSubproperty <http://rdaregistry.info/Elements/a/datatype/P50180>,
        <http://rdaregistry.info/Elements/a/object/P50180> ;
    reg:hasUnconstrained <http://rdaregistry.info/Elements/u/P60647> ;
    reg:lexicalAlias <http://rdaregistry.info/Elements/a/presenterOf.en> ;
    reg:name "presenterOf"@en ;
    reg:status <http://metadataregistry.org/uri/RegStatus/1001> ;
    rdfs:domain <http://rdaregistry.info/Elements/c/C10002> ;
    rdfs:isDefinedBy <http://rdaregistry.info/Elements/a/> ;
    rdfs:subPropertyOf <http://rdaregistry.info/Elements/a/P50161> ;
    skos:definition "Relates an agent mentioned in an \"X presents:\" credit for moving image materials and who is probably associated with production, finance, or distribution in some way to an expression."@en,
        "Met une personne, famille ou collectivité mentionnée dans un générique d’images animées sous la forme « X présente » et qui est probablement associée d’une façon quelconque à la production, au financement ou à la distribution en relation avec l’expression."@fr .

<http://rdaregistry.info/Elements/a/P50181> a rdf:Property ;
    rdfs:label "is other agent associated with manifestation of"@en,
        "est l’autre personne, famille ou collectivité associée à une manifestation de"@fr ;
    rdakit:toolkitDefinition "A manifestation associated with an agent other than a producer, publisher, distributor, or manufacturer."@en,
        "Personne, famille ou collectivité, autre qu’un producteur, un éditeur, un diffuseur ou distributeur ou bien un fabricant, associée à une manifestation."@fr ;
    rdakit:toolkitLabel "other agent associated with manifestation of"@en,
        "autre personne, famille ou collectivité associée à une manifestation de"@fr ;
    reg:hasSubproperty <http://rdaregistry.info/Elements/a/datatype/P50181>,
        <http://rdaregistry.info/Elements/a/object/P50181> ;
    reg:hasUnconstrained <http://rdaregistry.info/Elements/u/P60602> ;
    reg:lexicalAlias <http://rdaregistry.info/Elements/a/otherAgentManifestationOf.en> ;
    reg:name "otherAgentManifestationOf"@en ;
    reg:status <http://metadataregistry.org/uri/RegStatus/1001> ;
    rdfs:domain <http://rdaregistry.info/Elements/c/C10002> ;
    rdfs:isDefinedBy <http://rdaregistry.info/Elements/a/> ;
    rdfs:subPropertyOf <http://rdaregistry.info/Elements/a/P50307> ;
    skos:definition "Relates an agent other than a producer, publisher, distributor, or manufacturer associated with a manifestation to a manifestation."@en,
        "Met une personne, famille ou collectivité, autre qu’un producteur, un éditeur, un diffuseur ou distributeur ou bien un fabricant, associée à une manifestation en relation avec la manifestation."@fr ;
    skos:scopeNote "Book designers, platemakers, etc., are included."@en,
        "Comprend les graphistes, les graveurs de planches, etc."@fr .

<http://rdaregistry.info/Elements/a/P50200> a rdf:Property ;
    rdfs:label "is producer of unpublished manifestation of"@en,
        "est le producteur d’une ressource non publiée de"@fr ;
    rdakit:toolkitDefinition "A manifestation that is inscribed, fabricated, constructed, etc."@en,
        "Personne, famille ou collectivité responsable de la scription, de la fabrication, de la construction, etc. d’une ressource sous une forme non publiée."@fr ;
    rdakit:toolkitLabel "producer of unpublished manifestation of"@en,
        "producteur d’une ressource non publiée de"@fr ;
    reg:hasSubproperty <http://rdaregistry.info/Elements/a/datatype/P50200>,
        <http://rdaregistry.info/Elements/a/object/P50200> ;
    reg:hasUnconstrained <http://rdaregistry.info/Elements/u/P60817> ;
    reg:lexicalAlias <http://rdaregistry.info/Elements/a/producerOfUnpublishedManifestationOf.en> ;
    reg:name "producerOfUnpublishedManifestationOf"@en ;
    reg:status <http://metadataregistry.org/uri/RegStatus/1001> ;
    rdfs:domain <http://rdaregistry.info/Elements/c/C10002> ;
    rdfs:isDefinedBy <http://rdaregistry.info/Elements/a/> ;
    rdfs:subPropertyOf <http://rdaregistry.info/Elements/a/P50307> ;
    skos:definition "Relates an agent to a manifestation that is inscribed, fabricated, constructed, etc."@en,
        "Met une personne, famille ou collectivité responsable de la scription, de la fabrication, de la construction, etc. d’une ressource sous une forme non publiée en relation avec la manifestation."@fr .

<http://rdaregistry.info/Elements/a/P50227> a rdf:Property ;
    rdfs:label "is writer of afterword of"@en,
        "est l’auteur d’après-propos de"@fr ;
    rdakit:instructionNumber "18.5" ;
    rdakit:toolkitDefinition "An expression that incorporates a contribution of providing an afterword to an original work."@en,
        "Personne, famille ou collectivité contribuant à une expression d’une œuvre en fournissant un après-propos à l’œuvre originale."@fr ;
    rdakit:toolkitLabel "writer of afterword of"@en,
        "auteur d’après-propos de"@fr ;
    reg:hasSubproperty <http://rdaregistry.info/Elements/a/datatype/P50227>,
        <http://rdaregistry.info/Elements/a/object/P50227> ;
    reg:hasUnconstrained <http://rdaregistry.info/Elements/u/P60717> ;
    reg:lexicalAlias <http://rdaregistry.info/Elements/a/writerOfAfterwordOf.en> ;
    reg:name "writerOfAfterwordOf"@en ;
    reg:status <http://metadataregistry.org/uri/RegStatus/1001> ;
    rdfs:domain <http://rdaregistry.info/Elements/c/C10002> ;
    rdfs:isDefinedBy <http://rdaregistry.info/Elements/a/> ;
    rdfs:subPropertyOf <http://rdaregistry.info/Elements/a/P50154> ;
    skos:definition "Relates an agent contributing to an expression of a work by providing an afterword to an original work to an expression."@en,
        "Met une personne, famille ou collectivité contribuant à une expression d’une œuvre en fournissant un après-propos à l’œuvre originale en relation avec l’expression."@fr .

<http://rdaregistry.info/Elements/a/P50228> a rdf:Property ;
    rdfs:label "is writer of postface of"@en,
        "est le postfacier de"@fr ;
    rdakit:instructionNumber "18.5" ;
    rdakit:toolkitDefinition "An expression that incorporates a contribution of providing a postface to an original work."@en,
        "Personne, famille ou collectivité contribuant à une expression d’une œuvre en fournissant une postface à l’œuvre originale."@fr ;
    rdakit:toolkitLabel "writer of postface of"@en,
        "postfacier de"@fr ;
    reg:hasSubproperty <http://rdaregistry.info/Elements/a/datatype/P50228>,
        <http://rdaregistry.info/Elements/a/object/P50228> ;
    reg:hasUnconstrained <http://rdaregistry.info/Elements/u/P60718> ;
    reg:lexicalAlias <http://rdaregistry.info/Elements/a/writerOfPostfaceOf.en> ;
    reg:name "writerOfPostfaceOf"@en ;
    reg:status <http://metadataregistry.org/uri/RegStatus/1001> ;
    rdfs:domain <http://rdaregistry.info/Elements/c/C10002> ;
    rdfs:isDefinedBy <http://rdaregistry.info/Elements/a/> ;
    rdfs:subPropertyOf <http://rdaregistry.info/Elements/a/P50154> ;
    skos:definition "Relates an agent contributing to an expression of a work by providing a postface to an original work to an expression."@en,
        "Met une personne, famille ou collectivité contribuant à une expression d’une œuvre en fournissant une postface à l’œuvre originale en relation avec l’expression."@fr .

<http://rdaregistry.info/Elements/a/P50229> a rdf:Property ;
    rdfs:label "has predecessor of split"@en,
        "a pour prédécesseur avant scission"@fr ;
    rdakit:instructionNumber "29.5" ;
    rdakit:toolkitDefinition "A corporate body that split or divided into another corporate body."@en,
        "Una entidad corporativa que se separa o divide en otra entidad corporativa."@es,
        "Collectivité qui s’est scindée ou s’est divisée pour former l’autre collectivité."@fr ;
    rdakit:toolkitLabel "predecessor of split"@en,
        "predecesora de la división"@es,
        "prédécesseur avant scission"@fr ;
    reg:hasSubproperty <http://rdaregistry.info/Elements/a/datatype/P50229>,
        <http://rdaregistry.info/Elements/a/object/P50229> ;
    reg:hasUnconstrained <http://rdaregistry.info/Elements/u/P60733> ;
    reg:lexicalAlias <http://rdaregistry.info/Elements/a/predecessorOfSplit.en> ;
    reg:name "predecessorOfSplit"@en ;
    reg:status <http://metadataregistry.org/uri/RegStatus/1001> ;
    rdfs:domain <http://rdaregistry.info/Elements/c/C10005> ;
    rdfs:isDefinedBy <http://rdaregistry.info/Elements/a/> ;
    skos:definition "Relates a corporate body to a corporate body that split or divided into another corporate body."@en,
        "Met une collectivité en relation avec une collectivité qui s’est scindée ou s’est divisée pour former l’autre collectivité."@fr .

<http://rdaregistry.info/Elements/a/P50230> a rdf:Property ;
    rdfs:label "has membership corporate body"@en,
        "a pour collectivité d’affiliation"@fr ;
    rdakit:instructionNumber "29.5" ;
    rdakit:toolkitDefinition "A corporate body formed from the membership of other corporate bodies."@en,
        "Una entidad corporativa formada de la membresía de otras entidades corporativas."@es,
        "Collectivité formée par le regroupement de collectivités membres."@fr ;
    rdakit:toolkitLabel "membership corporate body"@en,
        "entidad corporativa por membresía"@es,
        "collectivité d’affiliation"@fr ;
    reg:hasSubproperty <http://rdaregistry.info/Elements/a/datatype/P50230>,
        <http://rdaregistry.info/Elements/a/object/P50230> ;
    reg:hasUnconstrained <http://rdaregistry.info/Elements/u/P60648> ;
    reg:lexicalAlias <http://rdaregistry.info/Elements/a/membershipCorporateBody.en> ;
    reg:name "membershipCorporateBody"@en ;
    reg:status <http://metadataregistry.org/uri/RegStatus/1001> ;
    rdfs:domain <http://rdaregistry.info/Elements/c/C10005> ;
    rdfs:isDefinedBy <http://rdaregistry.info/Elements/a/> ;
    skos:definition "Relates a corporate body to a corporate body formed from the membership of other corporate bodies."@en,
        "Met une collectivité en relation avec une collectivité formée par le regroupement de collectivités membres."@fr .

<http://rdaregistry.info/Elements/a/P50231> a rdf:Property ;
    rdfs:label "has corporate member"@en,
        "a pour collectivité membre"@fr ;
    rdakit:instructionNumber "29.5" ;
    rdakit:toolkitDefinition "A corporate body that is a member of another corporate body."@en,
        "Una entidad corporativa que es miembro de otra entidad corporativa."@es,
        "Collectivité qui est membre de l’autre collectivité."@fr ;
    rdakit:toolkitLabel "corporate member"@en,
        "miembro corporativo"@es,
        "collectivité membre"@fr ;
    reg:hasSubproperty <http://rdaregistry.info/Elements/a/datatype/P50231>,
        <http://rdaregistry.info/Elements/a/object/P50231> ;
    reg:hasUnconstrained <http://rdaregistry.info/Elements/u/P60697> ;
    reg:lexicalAlias <http://rdaregistry.info/Elements/a/corporateMember.en> ;
    reg:name "corporateMember"@en ;
    reg:status <http://metadataregistry.org/uri/RegStatus/1001> ;
    rdfs:domain <http://rdaregistry.info/Elements/c/C10005> ;
    rdfs:isDefinedBy <http://rdaregistry.info/Elements/a/> ;
    skos:definition "Relates a corporate body to a corporate body that is a member of another corporate body."@en,
        "Met une collectivité en relation avec une collectivité qui est membre de l’autre collectivité."@fr .

<http://rdaregistry.info/Elements/a/P50232> a rdf:Property ;
    rdfs:label "has component of merger"@en,
        "a pour composante d’une fusion"@fr ;
    rdakit:instructionNumber "29.5" ;
    rdakit:toolkitDefinition "A corporate body that formed another corporate body by merging with one or more other corporate bodies."@en,
        "Una entidad corporativa que forma otra entidad corporativa mediante la fusión con otra u otras entidades corporativas."@es,
        "Collectivité qui a formé l’autre collectivité en fusionnant avec une ou plusieurs autres collectivités."@fr ;
    rdakit:toolkitLabel "component of merger"@en,
        "componente de una fusión"@es,
        "composante d’une fusion"@fr ;
    reg:hasSubproperty <http://rdaregistry.info/Elements/a/datatype/P50232>,
        <http://rdaregistry.info/Elements/a/object/P50232> ;
    reg:hasUnconstrained <http://rdaregistry.info/Elements/u/P60736> ;
    reg:lexicalAlias <http://rdaregistry.info/Elements/a/componentOfMerger.en> ;
    reg:name "componentOfAMerger"@en ;
    reg:status <http://metadataregistry.org/uri/RegStatus/1001> ;
    rdfs:domain <http://rdaregistry.info/Elements/c/C10005> ;
    rdfs:isDefinedBy <http://rdaregistry.info/Elements/a/> ;
    skos:definition "Relates a corporate body to a corporate body that formed another corporate body by merging with one or more other corporate bodies."@en,
        "Met une collectivité en relation avec une collectivité qui a formé l’autre collectivité en fusionnant avec une ou plusieurs autres collectivités."@fr .

<http://rdaregistry.info/Elements/a/P50233> a rdf:Property ;
    rdfs:label "has family"@en,
        "a pour famille"@fr ;
    rdakit:instructionNumber "29.5" ;
    rdakit:toolkitDefinition "A family to which a person belongs."@en,
        "Una familia a la cual la persona pertenece."@es,
        "Famille à laquelle la personne appartient."@fr ;
    rdakit:toolkitLabel "family"@en,
        "familia"@es,
        "famille"@fr ;
    reg:hasSubproperty <http://rdaregistry.info/Elements/a/datatype/P50233>,
        <http://rdaregistry.info/Elements/a/object/P50233> ;
    reg:hasUnconstrained <http://rdaregistry.info/Elements/u/P60697> ;
    reg:lexicalAlias <http://rdaregistry.info/Elements/a/family.en> ;
    reg:name "family"@en ;
    reg:status <http://metadataregistry.org/uri/RegStatus/1001> ;
    rdfs:domain <http://rdaregistry.info/Elements/c/C10004> ;
    rdfs:isDefinedBy <http://rdaregistry.info/Elements/a/> ;
    skos:definition "Relates a person to a family to which a person belongs."@en,
        "Met une personne en relation avec une famille à laquelle la personne appartient."@fr .

<http://rdaregistry.info/Elements/a/P50235> a rdf:Property ;
    rdfs:label "has language of family"@en,
        "a pour langue de la famille"@fr ;
    rdakit:instructionNumber "10.8" ;
    rdakit:toolkitDefinition "A language a family uses in its communications."@en,
        "Una lengua que una familia usa para sus comunicaciones."@es,
        "Langue que la famille utilise pour sa communication."@fr ;
    rdakit:toolkitLabel "language of family"@en,
        "lengua de la familia"@es,
        "langue de la famille"@fr ;
    reg:hasSubproperty <http://rdaregistry.info/Elements/a/datatype/P50235> ;
    reg:hasUnconstrained <http://rdaregistry.info/Elements/u/P60098> ;
    reg:lexicalAlias <http://rdaregistry.info/Elements/a/languageOfFamily.en> ;
    reg:name "languageOfFamily"@en ;
    reg:status <http://metadataregistry.org/uri/RegStatus/1001> ;
    rdfs:domain <http://rdaregistry.info/Elements/c/C10008> ;
    rdfs:isDefinedBy <http://rdaregistry.info/Elements/a/> ;
    skos:definition "Relates a family to a language a family uses in its communications."@en,
        "Met une famille en relation avec une langue que la famille utilise pour sa communication."@fr .

<http://rdaregistry.info/Elements/a/P50236> a rdf:Property ;
    rdfs:label "has period of activity of corporate body"@en,
        "har verksamhetstid för institutionen"@sv ;
    rdakit:instructionNumber "11.4.5" ;
    rdakit:toolkitDefinition "A date or range of dates indicative of the period in which a corporate body was active."@en,
        "Una fecha o rango de fechas que indican el período en el que la entidad corporativa estaba activa."@es ;
    rdakit:toolkitLabel "period of activity of corporate body"@en,
        "período de actividad de la entidad corporativa"@es,
        "verksamhetstid för institutionen"@sv ;
    reg:hasSubproperty <http://rdaregistry.info/Elements/a/datatype/P50236> ;
    reg:hasUnconstrained <http://rdaregistry.info/Elements/u/P60076> ;
    reg:lexicalAlias <http://rdaregistry.info/Elements/a/periodOfActivityOfCorporateBody.en> ;
    reg:name "periodOfActivityOfCorporateBody"@en ;
    reg:status <http://metadataregistry.org/uri/RegStatus/1001> ;
    rdfs:domain <http://rdaregistry.info/Elements/c/C10005> ;
    rdfs:isDefinedBy <http://rdaregistry.info/Elements/a/> ;
    rdfs:subPropertyOf <http://rdaregistry.info/Elements/a/P50040> ;
    skos:definition "Relates a corporate body to a date or range of dates indicative of the period in which a corporate body was active."@en .

<http://rdaregistry.info/Elements/a/P50237> a rdf:Property ;
    rdfs:label "has type of corporate body"@en,
        "a pour type de collectivité"@fr ;
    rdakit:instructionNumber "11.7.1.4" ;
    rdakit:toolkitDefinition "A categorization for a type of corporate body."@en,
        "Type de collectivité."@fr ;
    rdakit:toolkitLabel "type of corporate body"@en,
        "tipo de entidad corporativa"@es,
        "type de collectivité"@fr ;
    reg:hasSubproperty <http://rdaregistry.info/Elements/a/datatype/P50237> ;
    reg:hasUnconstrained <http://rdaregistry.info/Elements/u/P60047> ;
    reg:lexicalAlias <http://rdaregistry.info/Elements/a/typeOfCorporateBody.en> ;
    reg:name "typeOfCorporateBody"@en ;
    reg:status <http://metadataregistry.org/uri/RegStatus/1001> ;
    rdfs:domain <http://rdaregistry.info/Elements/c/C10005> ;
    rdfs:isDefinedBy <http://rdaregistry.info/Elements/a/> ;
    rdfs:subPropertyOf <http://rdaregistry.info/Elements/a/P50033> ;
    skos:definition "Relates a corporate body to a type of corporate body."@en,
        "Met une collectivité en relation avec le type de collectivité."@fr .

<http://rdaregistry.info/Elements/a/P50238> a rdf:Property ;
    rdfs:label "has type of jurisdiction"@en,
        "a pour type de juridiction"@fr ;
    rdakit:instructionNumber "11.7.1.5" ;
    rdakit:toolkitDefinition "A categorization for a type of corporate body."@en,
        "Type de juridiction."@fr ;
    rdakit:toolkitLabel "type of jurisdiction"@en,
        "tipo de jurisdicción"@es,
        "type de juridiction"@fr ;
    reg:hasSubproperty <http://rdaregistry.info/Elements/a/datatype/P50238> ;
    reg:hasUnconstrained <http://rdaregistry.info/Elements/u/P60047> ;
    reg:lexicalAlias <http://rdaregistry.info/Elements/a/typeOfJurisdiction.en> ;
    reg:name "typeOfJurisdiction"@en ;
    reg:status <http://metadataregistry.org/uri/RegStatus/1001> ;
    rdfs:domain <http://rdaregistry.info/Elements/c/C10005> ;
    rdfs:isDefinedBy <http://rdaregistry.info/Elements/a/> ;
    rdfs:subPropertyOf <http://rdaregistry.info/Elements/a/P50033> ;
    skos:definition "Relates a corporate body to a type of jurisdiction."@en,
        "Met une collectivité en relation avec le type de juridiction."@fr .

<http://rdaregistry.info/Elements/a/P50239> a rdf:Property ;
    rdfs:label "has other designation"@en,
        "a pour autre information"@fr ;
    rdakit:instructionNumber "11.7.1.6" ;
    rdakit:toolkitDefinition "A characteristic other than place associated with corporate body, date associated with corporate body, associated institution, type of corporate body, or type of jurisdiction."@en,
        "Autre information."@fr ;
    rdakit:toolkitLabel "other designation"@en,
        "otra designación"@es,
        "autre information"@fr ;
    reg:hasSubproperty <http://rdaregistry.info/Elements/a/datatype/P50239> ;
    reg:hasUnconstrained <http://rdaregistry.info/Elements/u/P60370> ;
    reg:lexicalAlias <http://rdaregistry.info/Elements/a/otherDesignation.en> ;
    reg:name "otherDesignation"@en ;
    reg:status <http://metadataregistry.org/uri/RegStatus/1001> ;
    rdfs:domain <http://rdaregistry.info/Elements/c/C10005> ;
    rdfs:isDefinedBy <http://rdaregistry.info/Elements/a/> ;
    rdfs:subPropertyOf <http://rdaregistry.info/Elements/a/P50033> ;
    skos:definition "Relates a corporate body to another designation."@en,
        "Met une collectivité en relation avec l’autre information."@fr .

<http://rdaregistry.info/Elements/a/P50240> a rdf:Property ;
    rdfs:label "has broader affiliated body"@en,
        "a pour collectivité affiliée plus vaste"@fr ;
    rdakit:instructionNumber "29.5" ;
    rdakit:toolkitDefinition "A corporate body that acts for a local affiliated body and others at a broader organizational level."@en,
        "Una entidad corporativa que actúa para la entidad afiliada local y otras en un nivel organizacional más amplio."@es,
        "Collectivité qui agit pour la collectivité affiliée locale et pour d’autres à un niveau organisationnel plus vaste."@fr ;
    rdakit:toolkitLabel "broader affiliated body"@en,
        "entidad afiliada amplia"@es,
        "collectivité affiliée plus vaste"@fr ;
    reg:hasSubproperty <http://rdaregistry.info/Elements/a/datatype/P50240>,
        <http://rdaregistry.info/Elements/a/object/P50240> ;
    reg:hasUnconstrained <http://rdaregistry.info/Elements/u/P60738> ;
    reg:lexicalAlias <http://rdaregistry.info/Elements/a/broaderAffiliatedBody.en> ;
    reg:name "broaderAffiliatedBody"@en ;
    reg:status <http://metadataregistry.org/uri/RegStatus/1001> ;
    rdfs:domain <http://rdaregistry.info/Elements/c/C10005> ;
    rdfs:isDefinedBy <http://rdaregistry.info/Elements/a/> ;
    skos:definition "Relates a corporate body to a corporate body that acts for a local affiliated body and others at a broader organizational level."@en,
        "Met une collectivité en relation avec une collectivité qui agit pour la collectivité affiliée locale et pour d’autres à un niveau organisationnel plus vaste."@fr .

<http://rdaregistry.info/Elements/a/P50241> a rdf:Property ;
    rdfs:label "has local affiliate"@en,
        "a pour collectivité affiliée locale"@fr ;
    rdakit:instructionNumber "29.5" ;
    rdakit:toolkitDefinition "A local corporate body affiliated with a broader body which acts for it and others at a broader organizational level."@en,
        "Una entidad corporativa afiliada a otra más amplia que actúa para ella y para otras en un nivel organizacional más amplio."@es,
        "Collectivité locale affiliée avec la collectivité plus vaste qui agit pour elle et pour d’autres à un niveau organisationnel plus vaste."@fr ;
    rdakit:toolkitLabel "local affiliate"@en,
        "afiliado local"@es,
        "collectivité affiliée locale"@fr ;
    reg:hasSubproperty <http://rdaregistry.info/Elements/a/datatype/P50241>,
        <http://rdaregistry.info/Elements/a/object/P50241> ;
    reg:hasUnconstrained <http://rdaregistry.info/Elements/u/P60739> ;
    reg:lexicalAlias <http://rdaregistry.info/Elements/a/localAffiliate.en> ;
    reg:name "localAffiliate"@en ;
    reg:status <http://metadataregistry.org/uri/RegStatus/1001> ;
    rdfs:domain <http://rdaregistry.info/Elements/c/C10005> ;
    rdfs:isDefinedBy <http://rdaregistry.info/Elements/a/> ;
    skos:definition "Relates a corporate body to a local corporate body affiliated with a broader body which acts for it and others at a broader organizational level."@en,
        "Met une collectivité en relation avec une collectivité locale affiliée avec la collectivité plus vaste qui agit pour elle et pour d’autres à un niveau organisationnel plus vaste."@fr .

<http://rdaregistry.info/Elements/a/P50242> a rdf:Property ;
    rdfs:label "is papermaker of"@en,
        "est le papetier de"@fr ;
    rdakit:instructionNumber "18.5" ;
    rdakit:toolkitDefinition "A manifestation using paper produced to manufacture a manifestation."@en,
        "Personne, famille ou collectivité responsable de la production du papier utilisé pour fabriquer une manifestation."@fr ;
    rdakit:toolkitLabel "papermaker of"@en,
        "papetier de"@fr ;
    reg:hasSubproperty <http://rdaregistry.info/Elements/a/datatype/P50242>,
        <http://rdaregistry.info/Elements/a/object/P50242> ;
    reg:hasUnconstrained <http://rdaregistry.info/Elements/u/P60747> ;
    reg:lexicalAlias <http://rdaregistry.info/Elements/a/papermakerOf.en> ;
    reg:name "papermakerOf"@en ;
    reg:status <http://metadataregistry.org/uri/RegStatus/1001> ;
    rdfs:domain <http://rdaregistry.info/Elements/c/C10002> ;
    rdfs:isDefinedBy <http://rdaregistry.info/Elements/a/> ;
    rdfs:subPropertyOf <http://rdaregistry.info/Elements/a/P50202> ;
    skos:definition "Relates an agent responsible for the production of paper used to manufacture a manifestation to a manifestation."@en,
        "Met une personne, famille ou collectivité responsable de la production du papier utilisé pour fabriquer une manifestation en relation avec la manifestation."@fr .

<http://rdaregistry.info/Elements/a/P50243> a rdf:Property ;
    rdfs:label "is visual effects provider of"@en,
        "est le fournisseur d’effets visuels de"@fr ;
    rdakit:instructionNumber "18.5" ;
    rdakit:toolkitDefinition "An expression of a moving image work that involves a responsibility for designing and creating post-production visual effects."@en,
        "Personne, famille ou collectivité contribuant à une expression d’une œuvre d’images animées en concevant et en créant des effets visuels en postproduction."@fr ;
    rdakit:toolkitLabel "visual effects provider of"@en,
        "fournisseur d’effets visuels de"@fr ;
    reg:hasSubproperty <http://rdaregistry.info/Elements/a/datatype/P50243>,
        <http://rdaregistry.info/Elements/a/object/P50243> ;
    reg:hasUnconstrained <http://rdaregistry.info/Elements/u/P60754> ;
    reg:lexicalAlias <http://rdaregistry.info/Elements/a/visualEffectsProviderOf.en> ;
    reg:name "visualEffectsProviderOf"@en ;
    reg:status <http://metadataregistry.org/uri/RegStatus/1001> ;
    rdfs:domain <http://rdaregistry.info/Elements/c/C10002> ;
    rdfs:isDefinedBy <http://rdaregistry.info/Elements/a/> ;
    rdfs:subPropertyOf <http://rdaregistry.info/Elements/a/P50161> ;
    skos:definition "Relates an agent contributing to an expression of a moving image work by designing and creating post-production visual effects to an expression."@en,
        "Met une personne, famille ou collectivité contribuant à une expression d’une œuvre d’images animées en concevant et en créant des effets visuels en postproduction en relation avec l’expression."@fr .

<http://rdaregistry.info/Elements/a/P50244> a rdf:Property ;
    rdfs:label "is special effects provider of"@en,
        "est le fournisseur d’effets spéciaux de"@fr ;
    rdakit:instructionNumber "18.5" ;
    rdakit:toolkitDefinition "An expression of a moving image or audio work that involves a responsibility for designing and creating on-set special effects, such as on-set mechanical effects and in-camera optical effects."@en,
        "Personne, famille ou collectivité contribuant à une expression d’une œuvre d’images animées ou d’une œuvre audio en concevant et en créant des effets spéciaux de plateau (effets mécaniques de plateau et effets d’optique dans la caméra)."@fr ;
    rdakit:toolkitLabel "special effects provider of"@en,
        "fournisseur d’effets spéciaux de"@fr ;
    reg:hasSubproperty <http://rdaregistry.info/Elements/a/datatype/P50244>,
        <http://rdaregistry.info/Elements/a/object/P50244> ;
    reg:hasUnconstrained <http://rdaregistry.info/Elements/u/P60755> ;
    reg:lexicalAlias <http://rdaregistry.info/Elements/a/specialEffectsProviderOf.en> ;
    reg:name "specialEffectsProviderOf"@en ;
    reg:status <http://metadataregistry.org/uri/RegStatus/1001> ;
    rdfs:domain <http://rdaregistry.info/Elements/c/C10002> ;
    rdfs:isDefinedBy <http://rdaregistry.info/Elements/a/> ;
    rdfs:subPropertyOf <http://rdaregistry.info/Elements/a/P50161> ;
    skos:definition "Relates an agent contributing to an expression of a moving image or audio work by designing and creating on-set special effects, such as on-set mechanical effects and in-camera optical effects, to an expression."@en,
        "Met une personne, famille ou collectivité contribuant à une expression d’une œuvre d’images animées ou d’une œuvre audio en concevant et en créant des effets spéciaux de plateau (effets mécaniques de plateau et effets d’optique dans la caméra) en relation avec l’expression."@fr .

<http://rdaregistry.info/Elements/a/P50245> a rdf:Property ;
    rdfs:label "is letterer of"@en,
        "est le lettreur de"@fr ;
    rdakit:instructionNumber "18.5" ;
    rdakit:toolkitDefinition "An expression of a comic book, graphic novel, etc. that incorporates an illustrating contribution."@en,
        "Illustrateur contribuant à une expression d’une bande dessinée, d’un roman graphique, etc. en dessinant le texte et les effets sonores graphiques."@fr ;
    rdakit:toolkitLabel "letterer of"@en,
        "lettreur de"@fr ;
    reg:hasSubproperty <http://rdaregistry.info/Elements/a/datatype/P50245>,
        <http://rdaregistry.info/Elements/a/object/P50245> ;
    reg:hasUnconstrained <http://rdaregistry.info/Elements/u/P60756> ;
    reg:lexicalAlias <http://rdaregistry.info/Elements/a/lettererOf.en> ;
    reg:name "lettererOf"@en ;
    reg:status <http://metadataregistry.org/uri/RegStatus/1001> ;
    rdfs:domain <http://rdaregistry.info/Elements/c/C10002> ;
    rdfs:isDefinedBy <http://rdaregistry.info/Elements/a/> ;
    rdfs:subPropertyOf <http://rdaregistry.info/Elements/a/P50159> ;
    skos:definition "Relates an illustrator contributing to an expression of a comic book, graphic novel, etc. to an expression."@en,
        "Met un illustrateur contribuant à une expression d’une bande dessinée, d’un roman graphique, etc. en dessinant le texte et les effets sonores graphiques en relation avec l’expression."@fr .

<http://rdaregistry.info/Elements/a/P50246> a rdf:Property ;
    rdfs:label "is calligrapher of"@en,
        "est le calligraphe de"@fr ;
    rdakit:instructionNumber "18.5" ;
    rdakit:toolkitDefinition "A work of calligraphy that involves an artistic responsibility for the focus of interest in the aesthetic value of its penmanship or graphic artistry, regardless of whether the same person, etc. also authored the inscribed text."@en,
        "Artiste responsable de la création d’une œuvre de calligraphie où l’accent est mis sur la valeur esthétique de la calligraphie ou du graphisme, peu importe que la même personne, etc. soit aussi l’auteur du texte calligraphié."@fr ;
    rdakit:toolkitLabel "calligrapher of"@en,
        "calligraphe de"@fr ;
    reg:hasSubproperty <http://rdaregistry.info/Elements/a/datatype/P50246>,
        <http://rdaregistry.info/Elements/a/object/P50246> ;
    reg:hasUnconstrained <http://rdaregistry.info/Elements/u/P60758> ;
    reg:lexicalAlias <http://rdaregistry.info/Elements/a/calligrapherOf.en> ;
    reg:name "calligrapherOf"@en ;
    reg:status <http://metadataregistry.org/uri/RegStatus/1001> ;
    rdfs:domain <http://rdaregistry.info/Elements/c/C10002> ;
    rdfs:isDefinedBy <http://rdaregistry.info/Elements/a/> ;
    rdfs:subPropertyOf <http://rdaregistry.info/Elements/a/P50192> ;
    skos:definition "Relates an artist responsible for creating a work of calligraphy where the focus of interest lies in the aesthetic value of its penmanship or graphic artistry, regardless of whether the same person, etc to a work."@en,
        "Met un artiste responsable de la création d’une œuvre de calligraphie où l’accent est mis sur la valeur esthétique de la calligraphie ou du graphisme, peu importe que la même personne, etc. soit aussi l’auteur du texte calligraphié, en relation avec l’œuvre."@fr .

<http://rdaregistry.info/Elements/a/P50247> a rdf:Property ;
    rdfs:label "is book artist of"@en,
        "est l’artiste du livre de"@fr ;
    rdakit:instructionNumber "18.5" ;
    rdakit:toolkitDefinition "A work that involves an artistic responsibility for creating art works that exploit the book form or alter its physical structure as part of the content."@en,
        "Artiste responsable de la création d’œuvres d’art qui exploitent la forme livre ou qui modifient sa structure physique comme partie du contenu de l’œuvre."@fr ;
    rdakit:toolkitLabel "book artist of"@en,
        "artiste du livre de"@fr ;
    reg:hasSubproperty <http://rdaregistry.info/Elements/a/datatype/P50247>,
        <http://rdaregistry.info/Elements/a/object/P50247> ;
    reg:hasUnconstrained <http://rdaregistry.info/Elements/u/P60759> ;
    reg:lexicalAlias <http://rdaregistry.info/Elements/a/bookArtistOf.en> ;
    reg:name "bookArtistOf"@en ;
    reg:status <http://metadataregistry.org/uri/RegStatus/1001> ;
    rdfs:domain <http://rdaregistry.info/Elements/c/C10002> ;
    rdfs:isDefinedBy <http://rdaregistry.info/Elements/a/> ;
    rdfs:subPropertyOf <http://rdaregistry.info/Elements/a/P50192> ;
    skos:definition "Relates an artist resonsible for creating art works that exploit the book form or alter its physical structure as part of the content to a work."@en,
        "Met un artiste responsable de la création d’œuvres d’art qui exploitent la forme livre ou qui modifient sa structure physique comme partie du contenu de l’œuvre en relation avec l’œuvre."@fr .

<http://rdaregistry.info/Elements/a/P50248> a rdf:Property ;
    rdfs:label "is rapporteur of"@en,
        "est le rapporteur de"@fr ;
    rdakit:instructionNumber "18.5" ;
    rdakit:seeAlso <http://rdaregistry.info/Elements/a/P50212> ;
    rdakit:toolkitDefinition "A work that involves a responsibility for reporting on the proceedings of the meetings of an organization."@en,
        "Auteur nommé par une organisation pour rédiger les comptes rendus de ses réunions."@fr ;
    rdakit:toolkitLabel "rapporteur of"@en,
        "rapporteur de"@fr ;
    reg:hasSubproperty <http://rdaregistry.info/Elements/a/datatype/P50248>,
        <http://rdaregistry.info/Elements/a/object/P50248> ;
    reg:hasUnconstrained <http://rdaregistry.info/Elements/u/P60757> ;
    reg:lexicalAlias <http://rdaregistry.info/Elements/a/rapporteurOf.en> ;
    reg:name "rapporteurOf"@en ;
    reg:status <http://metadataregistry.org/uri/RegStatus/1001> ;
    rdfs:domain <http://rdaregistry.info/Elements/c/C10002> ;
    rdfs:isDefinedBy <http://rdaregistry.info/Elements/a/> ;
    rdfs:subPropertyOf <http://rdaregistry.info/Elements/a/P50195> ;
    skos:definition "Relates an author who is appointed by an organization to report on the proceedings of its meetings to a work."@en,
        "Met un auteur nommé par une organisation pour rédiger les comptes rendus de ses réunions en relation avec l’œuvre."@fr .

<http://rdaregistry.info/Elements/a/P50249> a rdf:Property ;
    rdfs:label "is subject of (person)"@en ;
    rdakit:toolkitDefinition "A work that is about a person."@en ;
    rdakit:toolkitLabel "subject of (person)"@en ;
    reg:hasSubproperty <http://rdaregistry.info/Elements/a/datatype/P50249>,
        <http://rdaregistry.info/Elements/a/object/P50249> ;
    reg:hasUnconstrained <http://rdaregistry.info/Elements/u/P60806> ;
    reg:lexicalAlias <http://rdaregistry.info/Elements/a/subjectOfPerson.en> ;
    reg:name "subjectOfPerson"@en ;
    reg:status <http://metadataregistry.org/uri/RegStatus/1001> ;
    rdfs:domain <http://rdaregistry.info/Elements/c/C10004> ;
    rdfs:isDefinedBy <http://rdaregistry.info/Elements/a/> ;
    rdfs:subPropertyOf <http://rdaregistry.info/Elements/a/P50366> ;
    skos:definition "Relates a person to a work that is about a person."@en .

<http://rdaregistry.info/Elements/a/P50250> a rdf:Property ;
    rdfs:label "is subject of (family)"@en ;
    rdakit:toolkitDefinition "A work that is about a family."@en ;
    rdakit:toolkitLabel "subject of (family)"@en ;
    reg:hasSubproperty <http://rdaregistry.info/Elements/a/datatype/P50250>,
        <http://rdaregistry.info/Elements/a/object/P50250> ;
    reg:hasUnconstrained <http://rdaregistry.info/Elements/u/P60806> ;
    reg:lexicalAlias <http://rdaregistry.info/Elements/a/subjectOfFamily.en> ;
    reg:name "subjectOfFamily"@en ;
    reg:status <http://metadataregistry.org/uri/RegStatus/1001> ;
    rdfs:domain <http://rdaregistry.info/Elements/c/C10008> ;
    rdfs:isDefinedBy <http://rdaregistry.info/Elements/a/> ;
    rdfs:subPropertyOf <http://rdaregistry.info/Elements/a/P50367> ;
    skos:definition "Relates a family to a work that is about a family."@en .

<http://rdaregistry.info/Elements/a/P50251> a rdf:Property ;
    rdfs:label "is subject of (corporate body)"@en ;
    rdakit:toolkitDefinition "A work that is about a corporate body."@en ;
    rdakit:toolkitLabel "subject of (corporate body)"@en ;
    reg:hasSubproperty <http://rdaregistry.info/Elements/a/datatype/P50251>,
        <http://rdaregistry.info/Elements/a/object/P50251> ;
    reg:hasUnconstrained <http://rdaregistry.info/Elements/u/P60806> ;
    reg:lexicalAlias <http://rdaregistry.info/Elements/a/subjectOfCorporateBody.en> ;
    reg:name "subjectOfCorporateBody"@en ;
    reg:status <http://metadataregistry.org/uri/RegStatus/1001> ;
    rdfs:domain <http://rdaregistry.info/Elements/c/C10005> ;
    rdfs:isDefinedBy <http://rdaregistry.info/Elements/a/> ;
    rdfs:subPropertyOf <http://rdaregistry.info/Elements/a/P50367> ;
    skos:definition "Relates a corporate body to a work that is about a corporate body."@en .

<http://rdaregistry.info/Elements/a/P50252> a rdf:Property ;
    rdfs:label "has graduate"@en ;
    rdakit:instructionNumber "29.5" ;
    rdakit:toolkitDefinition "A person who receives an academic degree from a granting institution or faculty."@en,
        "Una persona que recibe un grado académico de una institución o facultad otorgante."@es ;
    rdakit:toolkitLabel "graduate"@en,
        "graduado"@es ;
    reg:hasSubproperty <http://rdaregistry.info/Elements/a/datatype/P50252>,
        <http://rdaregistry.info/Elements/a/object/P50252> ;
    reg:hasUnconstrained <http://rdaregistry.info/Elements/u/P60807> ;
    reg:lexicalAlias <http://rdaregistry.info/Elements/a/graduate.en> ;
    reg:name "graduate"@en ;
    reg:status <http://metadataregistry.org/uri/RegStatus/1001> ;
    rdfs:domain <http://rdaregistry.info/Elements/c/C10005> ;
    rdfs:isDefinedBy <http://rdaregistry.info/Elements/a/> ;
    skos:definition "Relates a corporate body to a person who receives an academic degree from a granting institution or faculty."@en .

<http://rdaregistry.info/Elements/a/P50253> a rdf:Property ;
    rdfs:label "is graduate of"@en ;
    rdakit:instructionNumber "29.5" ;
    rdakit:toolkitDefinition "An institution or faculty that granted an academic degree to a person."@en,
        "Una institución o facultad que otorgó un grado académico a la persona."@es ;
    rdakit:toolkitLabel "graduate of"@en,
        "graduado de"@es ;
    reg:hasSubproperty <http://rdaregistry.info/Elements/a/datatype/P50253>,
        <http://rdaregistry.info/Elements/a/object/P50253> ;
    reg:hasUnconstrained <http://rdaregistry.info/Elements/u/P60808> ;
    reg:lexicalAlias <http://rdaregistry.info/Elements/a/graduateOf.en> ;
    reg:name "graduateOf"@en ;
    reg:status <http://metadataregistry.org/uri/RegStatus/1001> ;
    rdfs:domain <http://rdaregistry.info/Elements/c/C10004> ;
    rdfs:isDefinedBy <http://rdaregistry.info/Elements/a/> ;
    skos:definition "Relates a person to an institution or faculty that granted an academic degree to a person."@en .

<http://rdaregistry.info/Elements/a/P50254> a rdf:Property ;
    rdfs:label "is writer of foreword of"@en ;
    rdakit:instructionNumber "18.5" ;
    rdakit:toolkitDefinition "An expression of a work that incorporates a contribution of providing a foreword to an original work."@en ;
    rdakit:toolkitLabel "writer of foreword of"@en ;
    reg:hasSubproperty <http://rdaregistry.info/Elements/a/datatype/P50254>,
        <http://rdaregistry.info/Elements/a/object/P50254> ;
    reg:hasUnconstrained <http://rdaregistry.info/Elements/u/P60810> ;
    reg:lexicalAlias <http://rdaregistry.info/Elements/a/writerOfForewordOf.en> ;
    reg:name "writerOfForewordOf"@en ;
    reg:status <http://metadataregistry.org/uri/RegStatus/1001> ;
    rdfs:domain <http://rdaregistry.info/Elements/c/C10002> ;
    rdfs:isDefinedBy <http://rdaregistry.info/Elements/a/> ;
    rdfs:subPropertyOf <http://rdaregistry.info/Elements/a/P50154> ;
    skos:definition "Relates an agent contributing to an expression of a work by providing a foreword to an original work to an expression."@en .

<http://rdaregistry.info/Elements/a/P50255> a rdf:Property ;
    rdfs:label "is sound designer of"@en ;
    rdakit:instructionNumber "18.5" ;
    rdakit:toolkitDefinition "An expression of a work that incorporates a contribution of designing and creating audio or sound components."@en ;
    rdakit:toolkitLabel "sound designer of"@en ;
    reg:hasSubproperty <http://rdaregistry.info/Elements/a/datatype/P50255>,
        <http://rdaregistry.info/Elements/a/object/P50255> ;
    reg:hasUnconstrained <http://rdaregistry.info/Elements/u/P60812> ;
    reg:lexicalAlias <http://rdaregistry.info/Elements/a/soundDesignerOf.en> ;
    reg:name "soundDesignerOf"@en ;
    reg:status <http://metadataregistry.org/uri/RegStatus/1001> ;
    rdfs:domain <http://rdaregistry.info/Elements/c/C10002> ;
    rdfs:isDefinedBy <http://rdaregistry.info/Elements/a/> ;
    rdfs:subPropertyOf <http://rdaregistry.info/Elements/a/P50161> ;
    skos:definition "Relates an agent contributing to an expression of a work by designing and creating audio or sound components to an expression."@en .

<http://rdaregistry.info/Elements/a/P50256> a rdf:Property ;
    rdfs:label "is lighting designer of"@en ;
    rdakit:instructionNumber "18.5" ;
    rdakit:toolkitDefinition "An expression of a work that incorporates a contribution of designing and creating lighting components."@en ;
    rdakit:toolkitLabel "lighting designer of"@en ;
    reg:hasSubproperty <http://rdaregistry.info/Elements/a/datatype/P50256>,
        <http://rdaregistry.info/Elements/a/object/P50256> ;
    reg:hasUnconstrained <http://rdaregistry.info/Elements/u/P60814> ;
    reg:lexicalAlias <http://rdaregistry.info/Elements/a/lightingDesignerOf.en> ;
    reg:name "lightingDesignerOf"@en ;
    reg:status <http://metadataregistry.org/uri/RegStatus/1001> ;
    rdfs:domain <http://rdaregistry.info/Elements/c/C10002> ;
    rdfs:isDefinedBy <http://rdaregistry.info/Elements/a/> ;
    rdfs:subPropertyOf <http://rdaregistry.info/Elements/a/P50161> ;
    skos:definition "Relates an agent contributing to an expression of a work by designing and creating lighting components to an expression."@en .

<http://rdaregistry.info/Elements/a/P50257> a rdf:Property ;
    rdfs:label "is degree committee member of"@en ;
    rdakit:instructionNumber "18.5" ;
    rdakit:toolkitDefinition "A work that involves a responsibility for serving on a committee that supervises a student's thesis or dissertation."@en ;
    rdakit:toolkitLabel "degree committee member of"@en ;
    reg:hasSubproperty <http://rdaregistry.info/Elements/a/datatype/P50257>,
        <http://rdaregistry.info/Elements/a/object/P50257> ;
    reg:hasUnconstrained <http://rdaregistry.info/Elements/u/P60816> ;
    reg:lexicalAlias <http://rdaregistry.info/Elements/a/degreeCommitteeMemberOf.en> ;
    reg:name "degreeCommitteeMemberOf"@en ;
    reg:status <http://metadataregistry.org/uri/RegStatus/1001> ;
    rdfs:domain <http://rdaregistry.info/Elements/c/C10004> ;
    rdfs:isDefinedBy <http://rdaregistry.info/Elements/a/> ;
    rdfs:subPropertyOf <http://rdaregistry.info/Elements/a/P50131> ;
    skos:definition "Relates a person serving on a committee that supervises a student's thesis or dissertation to a work."@en .

<http://rdaregistry.info/Elements/a/P50258> a rdf:Property ;
    rdfs:label "is defendant corporate body of"@en,
        "est la collectivité défenderesse de"@fr ;
    rdakit:instructionNumber "18.5" ;
    rdakit:toolkitDefinition "A work that involves a responsibility for being a corporate body accused in a criminal proceeding or sued in a civil proceeding."@en,
        "Collectivité qui est accusée dans une poursuite criminelle ou contre laquelle une poursuite civile est intentée."@fr ;
    rdakit:toolkitLabel "defendant corporate body of"@en,
        "collectivité défenderesse de"@fr ;
    reg:hasSubproperty <http://rdaregistry.info/Elements/a/datatype/P50258>,
        <http://rdaregistry.info/Elements/a/object/P50258> ;
    reg:hasUnconstrained <http://rdaregistry.info/Elements/u/P60698> ;
    reg:lexicalAlias <http://rdaregistry.info/Elements/a/defendantCorporateBodyOf.en> ;
    reg:name "defendantCorporateBodyOf"@en ;
    reg:status <http://metadataregistry.org/uri/RegStatus/1001> ;
    rdfs:domain <http://rdaregistry.info/Elements/c/C10005> ;
    rdfs:isDefinedBy <http://rdaregistry.info/Elements/a/> ;
    rdfs:subPropertyOf <http://rdaregistry.info/Elements/a/P50090> ;
    skos:definition "Relates a corporate body who is accused in a criminal proceeding or sued in a civil proceeding to a work."@en,
        "Met une collectivité qui est accusée dans une poursuite criminelle ou contre laquelle une poursuite civile est intentée en relation avec l’œuvre."@fr .

<http://rdaregistry.info/Elements/a/P50259> a rdf:Property ;
    rdfs:label "is defendant person of"@en,
        "est la personne défenderesse de"@fr ;
    rdakit:instructionNumber "18.5" ;
    rdakit:toolkitDefinition "A work that involves a responsibility for being a person accused in a criminal proceeding or sued in a civil proceeding."@en,
        "Personne qui est accusée dans une poursuite criminelle ou contre laquelle une poursuite civile est intentée."@fr ;
    rdakit:toolkitLabel "defendant person of"@en,
        "personne défenderesse de"@fr ;
    reg:hasSubproperty <http://rdaregistry.info/Elements/a/datatype/P50259>,
        <http://rdaregistry.info/Elements/a/object/P50259> ;
    reg:hasUnconstrained <http://rdaregistry.info/Elements/u/P60698> ;
    reg:lexicalAlias <http://rdaregistry.info/Elements/a/defendantPersonOf.en> ;
    reg:name "defendantPersonOf"@en ;
    reg:status <http://metadataregistry.org/uri/RegStatus/1001> ;
    rdfs:domain <http://rdaregistry.info/Elements/c/C10004> ;
    rdfs:isDefinedBy <http://rdaregistry.info/Elements/a/> ;
    rdfs:subPropertyOf <http://rdaregistry.info/Elements/a/P50090> ;
    skos:definition "Relates a person who is accused in a criminal proceeding or sued in a civil proceeding to a work."@en,
        "Met une personne qui est accusée dans une poursuite criminelle ou contre laquelle une poursuite civile est intentée en relation avec l’œuvre."@fr .

<http://rdaregistry.info/Elements/a/P50260> a rdf:Property ;
    rdfs:label "has other place associated with corporate body"@en,
        "har övrig ort förknippad med institutionen"@sv ;
    rdakit:instructionNumber "11.3.3" ;
    rdakit:toolkitDefinition "A place associated with a corporate body other than location of a conference, etc."@en,
        "Un lugar asociado con una entidad corporativa diferente al lugar de una conferencia, etc."@es ;
    rdakit:toolkitLabel "other place associated with corporate body"@en,
        "otro lugar asociado con la entidad corporativa"@es,
        "övrig ort förknippad med institutionen"@sv ;
    reg:hasSubproperty <http://rdaregistry.info/Elements/a/datatype/P50260> ;
    reg:hasUnconstrained <http://rdaregistry.info/Elements/u/P60325> ;
    reg:lexicalAlias <http://rdaregistry.info/Elements/a/otherPlaceAssociatedWithCorporateBody.en> ;
    reg:name "otherPlaceAssociatedWithCorporateBody"@en ;
    reg:status <http://metadataregistry.org/uri/RegStatus/1001> ;
    rdfs:domain <http://rdaregistry.info/Elements/c/C10005> ;
    rdfs:isDefinedBy <http://rdaregistry.info/Elements/a/> ;
    rdfs:subPropertyOf <http://rdaregistry.info/Elements/a/P50031> ;
    skos:definition "Relates a corporate body to a place associated with a corporate body other than location of a conference, etc."@en ;
    skos:scopeNote "Other place associated with a corporate body includes a country, state, province, local place, etc., associated with a corporate body and the location of headquarters of a corporate body."@en .

<http://rdaregistry.info/Elements/a/P50262> a rdf:Property ;
    rdfs:label "is commissioning body of"@en ;
    rdakit:instructionNumber "18.5" ;
    rdakit:toolkitDefinition "A work that involves a responsibility for commissioning a work."@en ;
    rdakit:toolkitLabel "commissioning body of"@en ;
    reg:hasSubproperty <http://rdaregistry.info/Elements/a/datatype/P50262>,
        <http://rdaregistry.info/Elements/a/object/P50262> ;
    reg:hasUnconstrained <http://rdaregistry.info/Elements/u/P60827> ;
    reg:lexicalAlias <http://rdaregistry.info/Elements/a/commissioningBodyOf.en> ;
    reg:name "commissioningBodyOf"@en ;
    reg:status <http://metadataregistry.org/uri/RegStatus/1001> ;
    rdfs:domain <http://rdaregistry.info/Elements/c/C10002> ;
    rdfs:isDefinedBy <http://rdaregistry.info/Elements/a/> ;
    rdfs:subPropertyOf <http://rdaregistry.info/Elements/a/P50131> ;
    skos:definition "Relates an agent responsible for commissioning a work to a work."@en .

<http://rdaregistry.info/Elements/a/P50263> a rdf:Property ;
    rdfs:label "is software developer of"@en ;
    rdakit:instructionNumber "18.5" ;
    rdakit:toolkitDefinition "An expression of a work that incorporates a contribution of researching, designing, implementing, or testing software."@en ;
    rdakit:toolkitLabel "software developer of"@en ;
    reg:hasSubproperty <http://rdaregistry.info/Elements/a/datatype/P50263>,
        <http://rdaregistry.info/Elements/a/object/P50263> ;
    reg:hasUnconstrained <http://rdaregistry.info/Elements/u/P60829> ;
    reg:lexicalAlias <http://rdaregistry.info/Elements/a/softwareDeveloperOf.en> ;
    reg:name "softwareDeveloperOf"@en ;
    reg:status <http://metadataregistry.org/uri/RegStatus/1001> ;
    rdfs:domain <http://rdaregistry.info/Elements/c/C10002> ;
    rdfs:isDefinedBy <http://rdaregistry.info/Elements/a/> ;
    rdfs:subPropertyOf <http://rdaregistry.info/Elements/a/P50161> ;
    skos:definition "Relates an agent contributing to an expression of a work by researching, designing, implementing, or testing software to an expression."@en .

<http://rdaregistry.info/Elements/a/P50264> a rdf:Property ;
    rdfs:label "is participant in treaty of"@en,
        "est le participant à un traité de"@fr ;
    rdakit:instructionNumber "18.5" ;
    rdakit:toolkitDefinition "A work that is signed, ratified, or acceded to a treaty."@en,
        "Gouvernement, organisation internationale intergouvernementale ou autre collectivité qui a signé ou ratifié un traité ou y a adhéré."@fr ;
    rdakit:toolkitLabel "participant in treaty of"@en,
        "participant à un traité de"@fr ;
    reg:hasSubproperty <http://rdaregistry.info/Elements/a/datatype/P50264>,
        <http://rdaregistry.info/Elements/a/object/P50264> ;
    reg:hasUnconstrained <http://rdaregistry.info/Elements/u/P60835> ;
    reg:lexicalAlias <http://rdaregistry.info/Elements/a/participantInTreatyOf.en> ;
    reg:name "participantInTreatyOf"@en ;
    reg:status <http://metadataregistry.org/uri/RegStatus/1001> ;
    rdfs:domain <http://rdaregistry.info/Elements/c/C10005> ;
    rdfs:isDefinedBy <http://rdaregistry.info/Elements/a/> ;
    rdfs:subPropertyOf <http://rdaregistry.info/Elements/a/P50131> ;
    skos:definition "Relates a government, international intergovernmental body, or other corporate body that has signed, ratified, or acceded to a treaty to a work."@en,
        "Met un gouvernement, une organisation internationale intergouvernementale ou une autre collectivité qui a signé ou ratifié un traité ou y a adhéré en relation avec l’œuvre."@fr .

<http://rdaregistry.info/Elements/a/P50265> a rdf:Property ;
    rdfs:label "is researcher of"@en ;
    rdakit:instructionNumber "18.5" ;
    rdakit:toolkitDefinition "A work that involves a responsibility for research in support of the creation of a work."@en ;
    rdakit:toolkitLabel "researcher of"@en ;
    reg:hasSubproperty <http://rdaregistry.info/Elements/a/datatype/P50265>,
        <http://rdaregistry.info/Elements/a/object/P50265> ;
    reg:hasUnconstrained <http://rdaregistry.info/Elements/u/P60837> ;
    reg:lexicalAlias <http://rdaregistry.info/Elements/a/researcherOf.en> ;
    reg:name "researcherOf"@en ;
    reg:status <http://metadataregistry.org/uri/RegStatus/1001> ;
    rdfs:domain <http://rdaregistry.info/Elements/c/C10002> ;
    rdfs:isDefinedBy <http://rdaregistry.info/Elements/a/> ;
    rdfs:subPropertyOf <http://rdaregistry.info/Elements/a/P50131> ;
    skos:definition "Relates an agent who does research in support of the creation of a work to a work."@en .

<http://rdaregistry.info/Elements/a/P50266> a rdf:Property ;
    rdfs:label "is colourist of"@en ;
    rdakit:instructionNumber "18.5" ;
    rdakit:toolkitDefinition "An expression of a work that incorporates a contribution of applying colour to drawings, prints, photographs, maps, moving images, etc."@en ;
    rdakit:toolkitLabel "colourist of"@en ;
    reg:hasSubproperty <http://rdaregistry.info/Elements/a/datatype/P50266>,
        <http://rdaregistry.info/Elements/a/object/P50266> ;
    reg:hasUnconstrained <http://rdaregistry.info/Elements/u/P60839> ;
    reg:lexicalAlias <http://rdaregistry.info/Elements/a/colouristOf.en> ;
    reg:name "colouristOf"@en ;
    reg:status <http://metadataregistry.org/uri/RegStatus/1001> ;
    rdfs:domain <http://rdaregistry.info/Elements/c/C10002> ;
    rdfs:isDefinedBy <http://rdaregistry.info/Elements/a/> ;
    rdfs:subPropertyOf <http://rdaregistry.info/Elements/a/P50161> ;
    skos:definition "Relates an agent contributing to an expression of a work by applying colour to drawings, prints, photographs, maps, moving images, etc. to an expression."@en .

<http://rdaregistry.info/Elements/a/P50267> a rdf:Property ;
    rdfs:label "is make-up artist of"@en ;
    rdakit:instructionNumber "18.5" ;
    rdakit:toolkitDefinition "An expression of a work that incorporates a contribution of applying make-up and prosthetics for a moving image production or for a musical or dramatic presentation or entertainment."@en ;
    rdakit:toolkitLabel "make-up artist of"@en ;
    reg:hasSubproperty <http://rdaregistry.info/Elements/a/datatype/P50267>,
        <http://rdaregistry.info/Elements/a/object/P50267> ;
    reg:hasUnconstrained <http://rdaregistry.info/Elements/u/P60841> ;
    reg:lexicalAlias <http://rdaregistry.info/Elements/a/makeUpArtistOf.en> ;
    reg:name "makeUpArtistOf"@en ;
    reg:status <http://metadataregistry.org/uri/RegStatus/1001> ;
    rdfs:domain <http://rdaregistry.info/Elements/c/C10002> ;
    rdfs:isDefinedBy <http://rdaregistry.info/Elements/a/> ;
    rdfs:subPropertyOf <http://rdaregistry.info/Elements/a/P50161> ;
    skos:definition "Relates an agent contributing to an expression of a work by applying make-up and prosthetics for a moving image production or for a musical or dramatic presentation or entertainment to an expression."@en .

<http://rdaregistry.info/Elements/a/P50268> a rdf:Property ;
    rdfs:label "is choral conductor of"@en ;
    rdakit:instructionNumber "18.5" ;
    rdakit:toolkitDefinition "An expression of a musical work that incorporates a contribution of leading a choral performing group in a musical or dramatic presentation, etc."@en ;
    rdakit:toolkitLabel "choral conductor of"@en ;
    reg:hasSubproperty <http://rdaregistry.info/Elements/a/datatype/P50268>,
        <http://rdaregistry.info/Elements/a/object/P50268> ;
    reg:hasUnconstrained <http://rdaregistry.info/Elements/u/P60843> ;
    reg:lexicalAlias <http://rdaregistry.info/Elements/a/choralConductorOf.en> ;
    reg:name "choralConductorOf"@en ;
    reg:status <http://metadataregistry.org/uri/RegStatus/1001> ;
    rdfs:domain <http://rdaregistry.info/Elements/c/C10002> ;
    rdfs:isDefinedBy <http://rdaregistry.info/Elements/a/> ;
    rdfs:subPropertyOf <http://rdaregistry.info/Elements/a/P50070> ;
    skos:definition "Relates a conductor contributing to an expression of a musical work by leading a choral performing group in a musical or dramatic presentation, etc. to an expression."@en .

<http://rdaregistry.info/Elements/a/P50269> a rdf:Property ;
    rdfs:label "is instrumental conductor of"@en ;
    rdakit:instructionNumber "18.5" ;
    rdakit:toolkitDefinition "An expression of a musical work that incorporates a conducting contribution by leading an instrumental performing group in a musical or dramatic presentation, etc."@en ;
    rdakit:toolkitLabel "instrumental conductor of"@en ;
    reg:hasSubproperty <http://rdaregistry.info/Elements/a/datatype/P50269>,
        <http://rdaregistry.info/Elements/a/object/P50269> ;
    reg:hasUnconstrained <http://rdaregistry.info/Elements/u/P60845> ;
    reg:lexicalAlias <http://rdaregistry.info/Elements/a/instrumentalConductorOf.en> ;
    reg:name "instrumentalConductorOf"@en ;
    reg:status <http://metadataregistry.org/uri/RegStatus/1001> ;
    rdfs:domain <http://rdaregistry.info/Elements/c/C10002> ;
    rdfs:isDefinedBy <http://rdaregistry.info/Elements/a/> ;
    rdfs:subPropertyOf <http://rdaregistry.info/Elements/a/P50070> ;
    skos:definition "Relates a conductor contributing to an expression of a musical work by leading an instrumental performing group in a musical or dramatic presentation, etc. to an expression."@en .

<http://rdaregistry.info/Elements/a/P50270> a rdf:Property ;
    rdfs:label "is organizer of"@en,
        "est l’organisateur de"@fr ;
    rdakit:instructionNumber "18.5" ;
    rdakit:toolkitDefinition "A work that involves a responsibility for organizing an exhibit, event, conference, etc., which gave rise to a work."@en,
        "Personne, famille ou collectivité organisant l’exposition, l’événement, le congrès, etc. qui a donné lieu à la création d’une œuvre."@fr ;
    rdakit:toolkitLabel "organizer of"@en,
        "organisateur de"@fr ;
    reg:hasSubproperty <http://rdaregistry.info/Elements/a/datatype/P50270>,
        <http://rdaregistry.info/Elements/a/object/P50270> ;
    reg:hasUnconstrained <http://rdaregistry.info/Elements/u/P60850> ;
    reg:lexicalAlias <http://rdaregistry.info/Elements/a/organizerOf.en> ;
    reg:name "organizerOf"@en ;
    reg:status <http://metadataregistry.org/uri/RegStatus/1001> ;
    rdfs:domain <http://rdaregistry.info/Elements/c/C10002> ;
    rdfs:isDefinedBy <http://rdaregistry.info/Elements/a/> ;
    rdfs:subPropertyOf <http://rdaregistry.info/Elements/a/P50131> ;
    skos:definition "Relates an agent organizing an exhibit, event, conference, etc., which gave rise to a work to a work."@en,
        "Met une personne, famille ou collectivité organisant l’exposition, l’événement, le congrès, etc. qui a donné lieu à la création d’une œuvre en relation avec l’œuvre."@fr .

<http://rdaregistry.info/Elements/a/P50271> a rdf:Property ;
    rdfs:label "is censor of"@en ;
    rdakit:instructionNumber "18.5" ;
    rdakit:seeAlso <http://rdaregistry.info/Elements/a/P50195> ;
    rdakit:toolkitDefinition "An expression of a work that involves a responsibility for revising the content for the purpose of suppressing parts deemed objectionable on moral, political, military, or other grounds, but leaving the nature and content substantially unchanged."@en ;
    rdakit:toolkitLabel "censor of"@en ;
    reg:hasSubproperty <http://rdaregistry.info/Elements/a/datatype/P50271>,
        <http://rdaregistry.info/Elements/a/object/P50271> ;
    reg:hasUnconstrained <http://rdaregistry.info/Elements/u/P60852> ;
    reg:lexicalAlias <http://rdaregistry.info/Elements/a/censorOf.en> ;
    reg:name "censorOf"@en ;
    reg:status <http://metadataregistry.org/uri/RegStatus/1001> ;
    rdfs:domain <http://rdaregistry.info/Elements/c/C10002> ;
    rdfs:isDefinedBy <http://rdaregistry.info/Elements/a/> ;
    rdfs:subPropertyOf <http://rdaregistry.info/Elements/a/P50161> ;
    skos:definition "Relates an agent contributing to an expression of a work by revising the content for the purpose of suppressing parts deemed objectionable on moral, political, military, or other grounds, but leaving the nature and content substantially unchanged to an expression."@en .

<http://rdaregistry.info/Elements/a/P50272> a rdf:Property ;
    rdfs:label "is photographer (expression) of"@en ;
    rdakit:instructionNumber "18.5" ;
    rdakit:seeAlso <http://rdaregistry.info/Elements/a/P50190> ;
    rdakit:toolkitDefinition "An expression of a work that incorporates an illustrating contribution of providing supplementary photographic content to an original work."@en ;
    rdakit:toolkitLabel "photographer (expression) of"@en ;
    reg:hasSubproperty <http://rdaregistry.info/Elements/a/datatype/P50272>,
        <http://rdaregistry.info/Elements/a/object/P50272> ;
    reg:hasUnconstrained <http://rdaregistry.info/Elements/u/P60658> ;
    reg:lexicalAlias <http://rdaregistry.info/Elements/a/photographerExpressionOf.en> ;
    reg:name "photographerExpressionOf"@en ;
    reg:status <http://metadataregistry.org/uri/RegStatus/1001> ;
    rdfs:domain <http://rdaregistry.info/Elements/c/C10002> ;
    rdfs:isDefinedBy <http://rdaregistry.info/Elements/a/> ;
    rdfs:subPropertyOf <http://rdaregistry.info/Elements/a/P50161> ;
    skos:definition "Relates an illustrator contributing to an expression of a work by providing supplementary photographic content to an original work to an expression."@en .

<http://rdaregistry.info/Elements/a/P50273> a rdf:Property ;
    rdfs:label "is restorationist (expression) of"@en ;
    rdakit:instructionNumber "18.5" ;
    rdakit:toolkitDefinition "An expression of a work that incorporates a contribution of restoring and/or combining earlier expressions, which may be damaged or fragmentary, to create a new expression."@en ;
    rdakit:toolkitLabel "restorationist (expression) of"@en ;
    reg:hasSubproperty <http://rdaregistry.info/Elements/a/datatype/P50273>,
        <http://rdaregistry.info/Elements/a/object/P50273> ;
    reg:hasUnconstrained <http://rdaregistry.info/Elements/u/P60674> ;
    reg:lexicalAlias <http://rdaregistry.info/Elements/a/restorationistExpressionOf.en> ;
    reg:name "restorationistExpressionOf"@en ;
    reg:status <http://metadataregistry.org/uri/RegStatus/1001> ;
    rdfs:domain <http://rdaregistry.info/Elements/c/C10002> ;
    rdfs:isDefinedBy <http://rdaregistry.info/Elements/a/> ;
    rdfs:subPropertyOf <http://rdaregistry.info/Elements/a/P50161> ;
    skos:definition "Relates an agent who contributes to an expression of a work by restoring and/or combining earlier expressions, which may be damaged or fragmentary, to create a new expression to an expression."@en .

<http://rdaregistry.info/Elements/a/P50275> a rdf:Property ;
    rdfs:label "has assistant"@en ;
    rdakit:instructionNumber "29.5" ;
    rdakit:toolkitDefinition "A colleague who helps another person."@en ;
    rdakit:toolkitLabel "assistant"@en ;
    reg:hasSubproperty <http://rdaregistry.info/Elements/a/datatype/P50275>,
        <http://rdaregistry.info/Elements/a/object/P50275> ;
    reg:hasUnconstrained <http://rdaregistry.info/Elements/u/P60857> ;
    reg:lexicalAlias <http://rdaregistry.info/Elements/a/assistant.en> ;
    reg:name "assistant"@en ;
    reg:status <http://metadataregistry.org/uri/RegStatus/1001> ;
    rdfs:domain <http://rdaregistry.info/Elements/c/C10004> ;
    rdfs:isDefinedBy <http://rdaregistry.info/Elements/a/> ;
    rdfs:subPropertyOf <http://rdaregistry.info/Elements/a/P50274> ;
    skos:definition "Relates a person to a colleague who helps another person."@en .

<http://rdaregistry.info/Elements/a/P50276> a rdf:Property ;
    rdfs:label "is assistant to"@en ;
    rdakit:instructionNumber "29.5" ;
    rdakit:toolkitDefinition "A colleague who is helped by another person."@en ;
    rdakit:toolkitLabel "assistant to"@en ;
    reg:hasSubproperty <http://rdaregistry.info/Elements/a/datatype/P50276>,
        <http://rdaregistry.info/Elements/a/object/P50276> ;
    reg:hasUnconstrained <http://rdaregistry.info/Elements/u/P60858> ;
    reg:lexicalAlias <http://rdaregistry.info/Elements/a/assistantTo.en> ;
    reg:name "assistantTo"@en ;
    reg:status <http://metadataregistry.org/uri/RegStatus/1001> ;
    rdfs:domain <http://rdaregistry.info/Elements/c/C10004> ;
    rdfs:isDefinedBy <http://rdaregistry.info/Elements/a/> ;
    rdfs:subPropertyOf <http://rdaregistry.info/Elements/a/P50274> ;
    skos:definition "Relates a person to a colleague who is helped by another person."@en .

<http://rdaregistry.info/Elements/a/P50277> a rdf:Property ;
    rdfs:label "has co-worker"@en ;
    rdakit:instructionNumber "29.5" ;
    rdakit:toolkitDefinition "A colleague who works with or shares a task with another person."@en ;
    rdakit:toolkitLabel "co-worker"@en ;
    reg:hasSubproperty <http://rdaregistry.info/Elements/a/datatype/P50277>,
        <http://rdaregistry.info/Elements/a/object/P50277> ;
    reg:hasUnconstrained <http://rdaregistry.info/Elements/u/P60859> ;
    reg:lexicalAlias <http://rdaregistry.info/Elements/a/coworker.en> ;
    reg:name "coworker"@en ;
    reg:status <http://metadataregistry.org/uri/RegStatus/1001> ;
    rdfs:domain <http://rdaregistry.info/Elements/c/C10004> ;
    rdfs:isDefinedBy <http://rdaregistry.info/Elements/a/> ;
    rdfs:subPropertyOf <http://rdaregistry.info/Elements/a/P50274> ;
    skos:definition "Relates a person to a colleague who works with or shares a task with another person."@en .

<http://rdaregistry.info/Elements/a/P50278> a rdf:Property ;
    rdfs:label "has partner"@en ;
    rdakit:instructionNumber "29.5" ;
    rdakit:toolkitDefinition "A colleague working with another person in an activity of common interest, most often, a business partnership."@en ;
    rdakit:toolkitLabel "partner"@en ;
    reg:hasSubproperty <http://rdaregistry.info/Elements/a/datatype/P50278>,
        <http://rdaregistry.info/Elements/a/object/P50278> ;
    reg:hasUnconstrained <http://rdaregistry.info/Elements/u/P60860> ;
    reg:lexicalAlias <http://rdaregistry.info/Elements/a/partner.en> ;
    reg:name "partner"@en ;
    reg:status <http://metadataregistry.org/uri/RegStatus/1001> ;
    rdfs:domain <http://rdaregistry.info/Elements/c/C10004> ;
    rdfs:isDefinedBy <http://rdaregistry.info/Elements/a/> ;
    rdfs:subPropertyOf <http://rdaregistry.info/Elements/a/P50274> ;
    skos:definition "Relates a person to a colleague working with another person in an activity of common interest, most often, a business partnership."@en .

<http://rdaregistry.info/Elements/a/P50279> a rdf:Property ;
    rdfs:label "has fellow student"@en ;
    rdakit:instructionNumber "29.5" ;
    rdakit:toolkitDefinition "An associate of another student who is also formally engaged in learning."@en ;
    rdakit:toolkitLabel "fellow student"@en ;
    reg:hasSubproperty <http://rdaregistry.info/Elements/a/datatype/P50279>,
        <http://rdaregistry.info/Elements/a/object/P50279> ;
    reg:hasUnconstrained <http://rdaregistry.info/Elements/u/P60861> ;
    reg:lexicalAlias <http://rdaregistry.info/Elements/a/fellowStudent.en> ;
    reg:name "fellowStudent"@en ;
    reg:status <http://metadataregistry.org/uri/RegStatus/1001> ;
    rdfs:domain <http://rdaregistry.info/Elements/c/C10004> ;
    rdfs:isDefinedBy <http://rdaregistry.info/Elements/a/> ;
    rdfs:subPropertyOf <http://rdaregistry.info/Elements/a/P50220> ;
    skos:definition "Relates a person to an associate of another student who is also formally engaged in learning."@en .

<http://rdaregistry.info/Elements/a/P50280> a rdf:Property ;
    rdfs:label "has friend"@en ;
    rdakit:instructionNumber "29.5" ;
    rdakit:toolkitDefinition "A person who shares a bond of mutual affection or regard with another person."@en ;
    rdakit:toolkitLabel "friend"@en ;
    reg:hasSubproperty <http://rdaregistry.info/Elements/a/datatype/P50280>,
        <http://rdaregistry.info/Elements/a/object/P50280> ;
    reg:hasUnconstrained <http://rdaregistry.info/Elements/u/P60854> ;
    reg:lexicalAlias <http://rdaregistry.info/Elements/a/friend.en> ;
    reg:name "friend"@en ;
    reg:status <http://metadataregistry.org/uri/RegStatus/1001> ;
    rdfs:domain <http://rdaregistry.info/Elements/c/C10004> ;
    rdfs:isDefinedBy <http://rdaregistry.info/Elements/a/> ;
    rdfs:subPropertyOf <http://rdaregistry.info/Elements/a/P50220> ;
    skos:definition "Relates a person to a person who shares a bond of mutual affection or regard with another person."@en .

<http://rdaregistry.info/Elements/a/P50281> a rdf:Property ;
    rdfs:label "has student"@en ;
    rdakit:instructionNumber "29.5" ;
    rdakit:toolkitDefinition "A person who receives instruction from another person."@en ;
    rdakit:toolkitLabel "student"@en ;
    reg:hasSubproperty <http://rdaregistry.info/Elements/a/datatype/P50281>,
        <http://rdaregistry.info/Elements/a/object/P50281> ;
    reg:hasUnconstrained <http://rdaregistry.info/Elements/u/P60862> ;
    reg:lexicalAlias <http://rdaregistry.info/Elements/a/student.en> ;
    reg:name "student"@en ;
    reg:status <http://metadataregistry.org/uri/RegStatus/1001> ;
    rdfs:domain <http://rdaregistry.info/Elements/c/C10004> ;
    rdfs:isDefinedBy <http://rdaregistry.info/Elements/a/> ;
    rdfs:subPropertyOf <http://rdaregistry.info/Elements/a/P50220> ;
    skos:definition "Relates a person to a person who receives instruction from another person."@en .

<http://rdaregistry.info/Elements/a/P50282> a rdf:Property ;
    rdfs:label "has teacher"@en ;
    rdakit:instructionNumber "29.5" ;
    rdakit:toolkitDefinition "A person who instructs another person."@en ;
    rdakit:toolkitLabel "teacher"@en ;
    reg:hasSubproperty <http://rdaregistry.info/Elements/a/datatype/P50282>,
        <http://rdaregistry.info/Elements/a/object/P50282> ;
    reg:hasUnconstrained <http://rdaregistry.info/Elements/u/P60863> ;
    reg:lexicalAlias <http://rdaregistry.info/Elements/a/teacher.en> ;
    reg:name "teacher"@en ;
    reg:status <http://metadataregistry.org/uri/RegStatus/1001> ;
    rdfs:domain <http://rdaregistry.info/Elements/c/C10004> ;
    rdfs:isDefinedBy <http://rdaregistry.info/Elements/a/> ;
    rdfs:subPropertyOf <http://rdaregistry.info/Elements/a/P50220> ;
    skos:definition "Relates a person to a person who instructs another person."@en .

<http://rdaregistry.info/Elements/a/P50283> a rdf:Property ;
    rdfs:label "has enrolled student"@en ;
    rdakit:instructionNumber "29.5" ;
    rdakit:toolkitDefinition "A person who receives instruction at an educational institution."@en ;
    rdakit:toolkitLabel "enrolled student"@en ;
    reg:hasSubproperty <http://rdaregistry.info/Elements/a/datatype/P50283>,
        <http://rdaregistry.info/Elements/a/object/P50283> ;
    reg:hasUnconstrained <http://rdaregistry.info/Elements/u/P60855> ;
    reg:lexicalAlias <http://rdaregistry.info/Elements/a/enrolledStudent.en> ;
    reg:name "enrolledStudent"@en ;
    reg:status <http://metadataregistry.org/uri/RegStatus/1001> ;
    rdfs:domain <http://rdaregistry.info/Elements/c/C10005> ;
    rdfs:isDefinedBy <http://rdaregistry.info/Elements/a/> ;
    rdfs:subPropertyOf <http://rdaregistry.info/Elements/a/P50220> ;
    skos:definition "Relates a corporate body to a person who receives instruction at an educational institution."@en .

<http://rdaregistry.info/Elements/a/P50284> a rdf:Property ;
    rdfs:label "has chief executive"@en ;
    rdakit:instructionNumber "29.5" ;
    rdakit:toolkitDefinition "An officer who is the top ranking official of a corporate body."@en ;
    rdakit:toolkitLabel "chief executive"@en ;
    reg:hasSubproperty <http://rdaregistry.info/Elements/a/datatype/P50284>,
        <http://rdaregistry.info/Elements/a/object/P50284> ;
    reg:hasUnconstrained <http://rdaregistry.info/Elements/u/P60864> ;
    reg:lexicalAlias <http://rdaregistry.info/Elements/a/chiefExecutive.en> ;
    reg:name "chiefExecutive"@en ;
    reg:status <http://metadataregistry.org/uri/RegStatus/1001> ;
    rdfs:domain <http://rdaregistry.info/Elements/c/C10005> ;
    rdfs:isDefinedBy <http://rdaregistry.info/Elements/a/> ;
    rdfs:subPropertyOf <http://rdaregistry.info/Elements/a/P50027> ;
    skos:definition "Relates a corporate body to an officer who is the top ranking official of a corporate body."@en .

<http://rdaregistry.info/Elements/a/P50285> a rdf:Property ;
    rdfs:label "has trustee"@en ;
    rdakit:instructionNumber "29.5" ;
    rdakit:toolkitDefinition "An officer granted the powers of administration in a corporate body in order to act for its benefit."@en ;
    rdakit:toolkitLabel "trustee"@en ;
    reg:hasSubproperty <http://rdaregistry.info/Elements/a/datatype/P50285>,
        <http://rdaregistry.info/Elements/a/object/P50285> ;
    reg:hasUnconstrained <http://rdaregistry.info/Elements/u/P60866> ;
    reg:lexicalAlias <http://rdaregistry.info/Elements/a/trustee.en> ;
    reg:name "trustee"@en ;
    reg:status <http://metadataregistry.org/uri/RegStatus/1001> ;
    rdfs:domain <http://rdaregistry.info/Elements/c/C10005> ;
    rdfs:isDefinedBy <http://rdaregistry.info/Elements/a/> ;
    rdfs:subPropertyOf <http://rdaregistry.info/Elements/a/P50027> ;
    skos:definition "Relates a corporate body to an officer granted the powers of administration in a corporate body in order to act for its benefit."@en .

<http://rdaregistry.info/Elements/a/P50286> a rdf:Property ;
    rdfs:label "is chief executive of"@en ;
    rdakit:instructionNumber "29.5" ;
    rdakit:toolkitDefinition "A corporate body in which an officer is the top ranking official."@en ;
    rdakit:toolkitLabel "chief executive of"@en ;
    reg:hasSubproperty <http://rdaregistry.info/Elements/a/datatype/P50286>,
        <http://rdaregistry.info/Elements/a/object/P50286> ;
    reg:hasUnconstrained <http://rdaregistry.info/Elements/u/P60865> ;
    reg:lexicalAlias <http://rdaregistry.info/Elements/a/chiefExecutiveOf.en> ;
    reg:name "chiefExecutiveOf"@en ;
    reg:status <http://metadataregistry.org/uri/RegStatus/1001> ;
    rdfs:domain <http://rdaregistry.info/Elements/c/C10004> ;
    rdfs:isDefinedBy <http://rdaregistry.info/Elements/a/> ;
    rdfs:subPropertyOf <http://rdaregistry.info/Elements/a/P50234> ;
    skos:definition "Relates a person to a corporate body in which an officer is the top ranking official."@en .

<http://rdaregistry.info/Elements/a/P50287> a rdf:Property ;
    rdfs:label "is trustee of"@en ;
    rdakit:instructionNumber "29.5" ;
    rdakit:toolkitDefinition "A corporate body that grants the powers of administration to an officer in order to act for its benefit."@en ;
    rdakit:toolkitLabel "trustee of"@en ;
    reg:hasSubproperty <http://rdaregistry.info/Elements/a/datatype/P50287>,
        <http://rdaregistry.info/Elements/a/object/P50287> ;
    reg:hasUnconstrained <http://rdaregistry.info/Elements/u/P60867> ;
    reg:lexicalAlias <http://rdaregistry.info/Elements/a/trusteeOf.en> ;
    reg:name "trusteeOf"@en ;
    reg:status <http://metadataregistry.org/uri/RegStatus/1001> ;
    rdfs:domain <http://rdaregistry.info/Elements/c/C10004> ;
    rdfs:isDefinedBy <http://rdaregistry.info/Elements/a/> ;
    rdfs:subPropertyOf <http://rdaregistry.info/Elements/a/P50234> ;
    skos:definition "Relates a person to a corporate body that grants the powers of administration to an officer in order to act for its benefit."@en .

<http://rdaregistry.info/Elements/a/P50288> a rdf:Property ;
    rdfs:label "is student at"@en ;
    rdakit:instructionNumber "29.5" ;
    rdakit:toolkitDefinition "An educational institution that provides instruction to a person."@en ;
    rdakit:toolkitLabel "student at"@en ;
    reg:hasSubproperty <http://rdaregistry.info/Elements/a/datatype/P50288>,
        <http://rdaregistry.info/Elements/a/object/P50288> ;
    reg:hasUnconstrained <http://rdaregistry.info/Elements/u/P60856> ;
    reg:lexicalAlias <http://rdaregistry.info/Elements/a/studentAt.en> ;
    reg:name "studentAt"@en ;
    reg:status <http://metadataregistry.org/uri/RegStatus/1001> ;
    rdfs:domain <http://rdaregistry.info/Elements/c/C10004> ;
    rdfs:isDefinedBy <http://rdaregistry.info/Elements/a/> ;
    rdfs:subPropertyOf <http://rdaregistry.info/Elements/a/P50218> ;
    skos:definition "Relates a person to an educational institution that provides instruction to a person."@en .

<http://rdaregistry.info/Elements/a/P50289> a rdf:Property ;
    rdfs:label "is editorial director of"@en ;
    rdakit:instructionNumber "18.5" ;
    rdakit:seeAlso <http://rdaregistry.info/Elements/a/P50156> ;
    rdakit:toolkitDefinition "A work that includes a legal and/or intellectual responsibility other than creation for the content of a serial, integrating resource, or multipart monographic work."@en ;
    rdakit:toolkitLabel "editorial director of"@en ;
    reg:hasSubproperty <http://rdaregistry.info/Elements/a/datatype/P50289>,
        <http://rdaregistry.info/Elements/a/object/P50289> ;
    reg:hasUnconstrained <http://rdaregistry.info/Elements/u/P60870> ;
    reg:lexicalAlias <http://rdaregistry.info/Elements/a/editorialDirectorOf.en> ;
    reg:name "editorialDirectorOf"@en ;
    reg:status <http://metadataregistry.org/uri/RegStatus/1001> ;
    rdfs:domain <http://rdaregistry.info/Elements/c/C10002> ;
    rdfs:isDefinedBy <http://rdaregistry.info/Elements/a/> ;
    rdfs:subPropertyOf <http://rdaregistry.info/Elements/a/P50131> ;
    skos:definition "Relates an agent responsible for the legal and/or intellectual responsibility other than creation for the content of a serial, integrating resource, or multipart monographic work to a work."@en,
        "Relates an agent responsible for the legal or intellectual responsibility other than creation for the content of a serial, integrating resource, or multipart monographic work to a work."@en .

<http://rdaregistry.info/Elements/a/P50290> a rdf:Property ;
    rdfs:label "is founder of work of"@en ;
    rdakit:instructionNumber "18.5" ;
    rdakit:toolkitDefinition "A work that involves a responsibility for establishing a serial, integrating resource, or multipart monograph."@en ;
    rdakit:toolkitLabel "founder of work of"@en ;
    reg:hasSubproperty <http://rdaregistry.info/Elements/a/datatype/P50290>,
        <http://rdaregistry.info/Elements/a/object/P50290> ;
    reg:hasUnconstrained <http://rdaregistry.info/Elements/u/P60872> ;
    reg:lexicalAlias <http://rdaregistry.info/Elements/a/founderOfWorkOf.en> ;
    reg:name "founderOfWorkOf"@en ;
    reg:status <http://metadataregistry.org/uri/RegStatus/1001> ;
    rdfs:domain <http://rdaregistry.info/Elements/c/C10002> ;
    rdfs:isDefinedBy <http://rdaregistry.info/Elements/a/> ;
    rdfs:subPropertyOf <http://rdaregistry.info/Elements/a/P50131> ;
    skos:definition "Relates an agent responsible for establishing a serial, integrating resource, or multipart monograph to a work."@en .

<http://rdaregistry.info/Elements/a/P50291> a rdf:Property ;
    rdfs:label "has surname"@en ;
    rdakit:instructionNumber "18.5" ;
    rdakit:toolkitDefinition "A name used as a family name."@en ;
    rdakit:toolkitLabel "surname"@en ;
    reg:hasSubproperty <http://rdaregistry.info/Elements/a/datatype/P50291> ;
    reg:hasUnconstrained <http://rdaregistry.info/Elements/u/P60878> ;
    reg:lexicalAlias <http://rdaregistry.info/Elements/a/surname.en> ;
    reg:name "surname"@en ;
    reg:status <http://metadataregistry.org/uri/RegStatus/1001> ;
    rdfs:domain <http://rdaregistry.info/Elements/c/C10004> ;
    rdfs:isDefinedBy <http://rdaregistry.info/Elements/a/> ;
    skos:definition "Relates a person to a name used as a family name."@en ;
    skos:scopeNote "Names used as family names by Romans of classical times are excluded."@en .

<http://rdaregistry.info/Elements/a/P50292> a rdf:Property ;
    rdfs:label "has given name"@en ;
    rdakit:instructionNumber "18.5" ;
    rdakit:toolkitDefinition "A name given to a person at birth or at some later point in addition to, or instead of, a surname."@en ;
    rdakit:toolkitLabel "given name"@en ;
    reg:hasSubproperty <http://rdaregistry.info/Elements/a/datatype/P50292> ;
    reg:hasUnconstrained <http://rdaregistry.info/Elements/u/P60879> ;
    reg:lexicalAlias <http://rdaregistry.info/Elements/a/givenName.en> ;
    reg:name "givenName"@en ;
    reg:status <http://metadataregistry.org/uri/RegStatus/1001> ;
    rdfs:domain <http://rdaregistry.info/Elements/c/C10004> ;
    rdfs:isDefinedBy <http://rdaregistry.info/Elements/a/> ;
    skos:definition "Relates a person to a name given to a person at birth or at some later point in addition to, or instead of, a surname."@en .

<http://rdaregistry.info/Elements/a/P50294> a rdf:Property ;
    rdfs:label "is casting director of"@en ;
    rdakit:instructionNumber "18.5" ;
    rdakit:toolkitDefinition "A work that incorporates a contribution of responsibility for most aspects of assigning parts and duties to performers."@en ;
    rdakit:toolkitLabel "casting director of"@en ;
    reg:hasSubproperty <http://rdaregistry.info/Elements/a/datatype/P50294>,
        <http://rdaregistry.info/Elements/a/object/P50294> ;
    reg:hasUnconstrained <http://rdaregistry.info/Elements/u/P60882> ;
    reg:lexicalAlias <http://rdaregistry.info/Elements/a/castingDirectorOf.en> ;
    reg:name "castingDirectorOf"@en ;
    reg:status <http://metadataregistry.org/uri/RegStatus/1001> ;
    rdfs:domain <http://rdaregistry.info/Elements/c/C10002> ;
    rdfs:isDefinedBy <http://rdaregistry.info/Elements/a/> ;
    rdfs:subPropertyOf <http://rdaregistry.info/Elements/a/P50204> ;
    skos:definition "Relates an agent to a work that incorporates a contribution of responsibility for most aspects of assigning parts and duties to performers."@en .

<http://rdaregistry.info/Elements/a/P50295> a rdf:Property ;
    rdfs:label "is audio producer of"@en ;
    rdakit:instructionNumber "18.5" ;
    rdakit:toolkitDefinition "A work that involves a responsibility for most of the business aspects of an audio recording."@en ;
    rdakit:toolkitLabel "audio producer of"@en ;
    reg:hasSubproperty <http://rdaregistry.info/Elements/a/datatype/P50295>,
        <http://rdaregistry.info/Elements/a/object/P50295> ;
    reg:hasUnconstrained <http://rdaregistry.info/Elements/u/P60883> ;
    reg:lexicalAlias <http://rdaregistry.info/Elements/a/audioProducerOf.en> ;
    reg:name "audioProducerOf"@en ;
    reg:status <http://metadataregistry.org/uri/RegStatus/1001> ;
    rdfs:domain <http://rdaregistry.info/Elements/c/C10002> ;
    rdfs:isDefinedBy <http://rdaregistry.info/Elements/a/> ;
    rdfs:subPropertyOf <http://rdaregistry.info/Elements/a/P50201> ;
    skos:definition "Relates an agent to a work that involves a responsibility for most of the business aspects of an audio recording."@en .

<http://rdaregistry.info/Elements/a/P50299> a rdf:Property ;
    rdfs:label "is dubbing director of"@en ;
    rdakit:instructionNumber "18.5" ;
    rdakit:toolkitDefinition "An expression of a work that incorporates a contribution of responsibility for the general management and supervision of the process of adding new dialogue or other sounds to complete a sound track."@en ;
    rdakit:toolkitLabel "dubbing director of"@en ;
    reg:hasSubproperty <http://rdaregistry.info/Elements/a/datatype/P50299>,
        <http://rdaregistry.info/Elements/a/object/P50299> ;
    reg:hasUnconstrained <http://rdaregistry.info/Elements/u/P60887> ;
    reg:lexicalAlias <http://rdaregistry.info/Elements/a/dubbingDirectorOf.en> ;
    reg:name "dubbingDirectorOf"@en ;
    reg:status <http://metadataregistry.org/uri/RegStatus/1001> ;
    rdfs:domain <http://rdaregistry.info/Elements/c/C10002> ;
    rdfs:isDefinedBy <http://rdaregistry.info/Elements/a/> ;
    rdfs:subPropertyOf <http://rdaregistry.info/Elements/a/P50161> ;
    skos:definition "Relates an agent to an expression of a work that incorporates a contribution of responsibility for the general management and supervision of the process of adding new dialogue or other sounds to complete a sound track."@en .

<http://rdaregistry.info/Elements/a/P50300> a rdf:Property ;
    rdfs:label "is music programmer of"@en ;
    rdakit:instructionNumber "18.5" ;
    rdakit:seeAlso <http://rdaregistry.info/Elements/a/P50187> ;
    rdakit:toolkitDefinition "An expression of a musical work that incorporates a contribution of using electronic audio devices and/or computer software to generate sounds."@en ;
    rdakit:toolkitLabel "music programmer of"@en ;
    reg:hasSubproperty <http://rdaregistry.info/Elements/a/datatype/P50300>,
        <http://rdaregistry.info/Elements/a/object/P50300> ;
    reg:hasUnconstrained <http://rdaregistry.info/Elements/u/P60888> ;
    reg:lexicalAlias <http://rdaregistry.info/Elements/a/musicProgrammerOf.en> ;
    reg:name "musicProgrammerOf"@en ;
    reg:status <http://metadataregistry.org/uri/RegStatus/1001> ;
    rdfs:domain <http://rdaregistry.info/Elements/c/C10002> ;
    rdfs:isDefinedBy <http://rdaregistry.info/Elements/a/> ;
    rdfs:subPropertyOf <http://rdaregistry.info/Elements/a/P50161> ;
    skos:definition "Relates an agent to an expression of a musical work that incorporates a contribution of using electronic audio devices and/or computer software to generate sounds."@en,
        "Relates an agent to an expression of a musical work that incorporates a contribution of using electronic audio devices or computer software to generate sounds."@en ;
    skos:scopeNote "The creation of a new musical work is excluded"@en .

<http://rdaregistry.info/Elements/a/P50301> a rdf:Property ;
    rdfs:label "has absorbed corporate body"@en ;
    rdakit:instructionNumber "29.5" ;
    rdakit:toolkitDefinition "A corporate body that was absorbed by another corporate body."@en ;
    rdakit:toolkitLabel "absorbed corporate body"@en ;
    reg:hasSubproperty <http://rdaregistry.info/Elements/a/datatype/P50301>,
        <http://rdaregistry.info/Elements/a/object/P50301> ;
    reg:hasUnconstrained <http://rdaregistry.info/Elements/u/P60901> ;
    reg:lexicalAlias <http://rdaregistry.info/Elements/a/absorbedCorporateBody.en> ;
    reg:name "absorbedCorporateBody"@en ;
    reg:status <http://metadataregistry.org/uri/RegStatus/1001> ;
    rdfs:domain <http://rdaregistry.info/Elements/c/C10005> ;
    rdfs:isDefinedBy <http://rdaregistry.info/Elements/a/> ;
    skos:definition "Relates a corporate body to a corporate body that was absorbed by another corporate body."@en .

<http://rdaregistry.info/Elements/a/P50302> a rdf:Property ;
    rdfs:label "has absorbing corporate body"@en ;
    rdakit:instructionNumber "29.5" ;
    rdakit:toolkitDefinition "A corporate body that absorbed another corporate body."@en ;
    rdakit:toolkitLabel "absorbing corporate body"@en ;
    reg:hasSubproperty <http://rdaregistry.info/Elements/a/datatype/P50302>,
        <http://rdaregistry.info/Elements/a/object/P50302> ;
    reg:hasUnconstrained <http://rdaregistry.info/Elements/u/P60902> ;
    reg:lexicalAlias <http://rdaregistry.info/Elements/a/absorbingCorporateBody.en> ;
    reg:name "absorbingCorporateBody"@en ;
    reg:status <http://metadataregistry.org/uri/RegStatus/1001> ;
    rdfs:domain <http://rdaregistry.info/Elements/c/C10005> ;
    rdfs:isDefinedBy <http://rdaregistry.info/Elements/a/> ;
    skos:definition "Relates a corporate body to a corporate body that absorbed another corporate body."@en .

<http://rdaregistry.info/Elements/a/P50303> a rdf:Property ;
    rdfs:label "has jointly held conference"@en ;
    rdakit:instructionNumber "29.5" ;
    rdakit:toolkitDefinition "A conference that is jointly held with another conference."@en ;
    rdakit:toolkitLabel "jointly held conference"@en ;
    reg:hasSubproperty <http://rdaregistry.info/Elements/a/datatype/P50303>,
        <http://rdaregistry.info/Elements/a/object/P50303> ;
    reg:hasUnconstrained <http://rdaregistry.info/Elements/u/P60903> ;
    reg:lexicalAlias <http://rdaregistry.info/Elements/a/jointlyHeldConference.en> ;
    reg:name "jointlyHeldConference"@en ;
    reg:status <http://metadataregistry.org/uri/RegStatus/1001> ;
    rdfs:domain <http://rdaregistry.info/Elements/c/C10005> ;
    rdfs:isDefinedBy <http://rdaregistry.info/Elements/a/> ;
    skos:definition "Relates a conference to a conference that is jointly held with another conference."@en .

<http://metadataregistry.org/uri/RegStatus/1008> a skos:Concept ;
    skos:prefLabel "Deprecated"@en .

<http://rdaregistry.info/Elements/a/P50037> a rdf:Property ;
    rdfs:label "has date of establishment"@en,
        "a pour date de fondation"@fr,
        "har tid för institutionens grundande"@sv ;
    rdakit:instructionNumber "11.4.3" ;
    rdakit:toolkitDefinition "A date on which a corporate body was established or founded."@en,
        "La fecha en que se estableció o fundó una entidad corporativa."@es,
        "La date à laquelle une collectivité a été établie ou fondée."@fr ;
    rdakit:toolkitLabel "date of establishment"@en,
        "fecha de establecimiento"@es,
        "date de fondation"@fr,
        "tid för institutionens grundande"@sv ;
    reg:hasSubproperty <http://rdaregistry.info/Elements/a/datatype/P50037> ;
    reg:hasUnconstrained <http://rdaregistry.info/Elements/u/P60524> ;
    reg:lexicalAlias <http://rdaregistry.info/Elements/a/dateOfEstablishment.en> ;
    reg:name "dateOfEstablishment"@en ;
    reg:status <http://metadataregistry.org/uri/RegStatus/1001> ;
    rdfs:domain <http://rdaregistry.info/Elements/c/C10005> ;
    rdfs:isDefinedBy <http://rdaregistry.info/Elements/a/> ;
    rdfs:subPropertyOf <http://rdaregistry.info/Elements/a/P50040> ;
    skos:definition "Relates a corporate body to a date on which a corporate body was established or founded."@en,
        "Met une collectivité en relation avec la date à laquelle une collectivité a été établie ou fondée."@fr .

<http://rdaregistry.info/Elements/a/P50038> a rdf:Property ;
    rdfs:label "has date of termination"@en,
        "a pour date de cessation"@fr,
        "har tid för institutionens upphörande"@sv ;
    rdakit:instructionNumber "11.4.4" ;
    rdakit:toolkitDefinition "A date on which a corporate body was terminated or dissolved."@en,
        "La fecha en la que una entidad corporativa fue concluida o disuelta."@es,
        "La date à laquelle une collectivité a cessé son activité ou a été dissoute."@fr ;
    rdakit:toolkitLabel "date of termination"@en,
        "fecha de terminación"@es,
        "date de cessation"@fr,
        "tid för institutionens upphörande"@sv ;
    reg:hasSubproperty <http://rdaregistry.info/Elements/a/datatype/P50038> ;
    reg:hasUnconstrained <http://rdaregistry.info/Elements/u/P60525> ;
    reg:lexicalAlias <http://rdaregistry.info/Elements/a/dateOfTermination.en> ;
    reg:name "dateOfTermination"@en ;
    reg:status <http://metadataregistry.org/uri/RegStatus/1001> ;
    rdfs:domain <http://rdaregistry.info/Elements/c/C10005> ;
    rdfs:isDefinedBy <http://rdaregistry.info/Elements/a/> ;
    rdfs:subPropertyOf <http://rdaregistry.info/Elements/a/P50040> ;
    skos:definition "Relates a corporate body to a date on which a corporate body was terminated or dissolved."@en,
        "Met une collectivité en relation avec la date à laquelle une collectivité a cessé son activité ou a été dissoute."@fr .

<http://rdaregistry.info/Elements/a/P50039> a rdf:Property ;
    rdfs:label "has date of conference, etc."@en,
        "a pour date du congrès, etc."@fr,
        "har tid för konferens"@sv ;
    rdakit:instructionNumber "11.4.2" ;
    rdakit:toolkitDefinition "A date or range of dates on which a conference, congress, meeting, exhibition, fair, festival, etc., was held."@en,
        "La fecha o rango de fechas en las que se realizó una conferencia, congreso, reunión, exposición, feria, festival, etc."@es,
        "La date ou la fourchette de dates à laquelle un congrès, une conférence, une réunion, une exposition, une foire, un festival, etc. s’est tenu."@fr ;
    rdakit:toolkitLabel "date of conference, etc."@en,
        "fecha de la conferencia, etc."@es,
        "date du congrès, etc."@fr,
        "tid för konferens"@sv ;
    reg:hasSubproperty <http://rdaregistry.info/Elements/a/datatype/P50039> ;
    reg:hasUnconstrained <http://rdaregistry.info/Elements/u/P60526> ;
    reg:lexicalAlias <http://rdaregistry.info/Elements/a/dateOfConferenceEtc.en> ;
    reg:name "dateOfConferenceEtc"@en ;
    reg:status <http://metadataregistry.org/uri/RegStatus/1001> ;
    rdfs:domain <http://rdaregistry.info/Elements/c/C10005> ;
    rdfs:isDefinedBy <http://rdaregistry.info/Elements/a/> ;
    rdfs:subPropertyOf <http://rdaregistry.info/Elements/a/P50040> ;
    skos:definition "Relates a corporate body to a date or range of dates on which a conference, congress, meeting, exhibition, fair, festival, etc., was held."@en,
        "Met une collectivité en relation avec la date ou la fourchette de dates à laquelle un congrès, une conférence, une réunion, une exposition, une foire, un festival, etc. s’est tenu."@fr .

<http://rdaregistry.info/Elements/a/P50041> a rdf:Property ;
    rdfs:label "has preferred name for corporate body"@en,
        "a pour nom privilégié de la collectivité"@fr,
        "har föredraget namn för institutionen"@sv ;
    rdakit:instructionNumber "11.2.2" ;
    rdakit:toolkitDefinition "A name or form of name chosen to identify a corporate body."@en,
        "El nombre o la forma del nombre elegida para identificar la entidad corporativa."@es,
        "Le nom ou la forme de nom choisie pour identifier la collectivité."@fr ;
    rdakit:toolkitLabel "preferred name for corporate body"@en,
        "nombre preferido de la entidad corporativa"@es,
        "nom privilégié de la collectivité"@fr,
        "föredraget namn för institutionen"@sv ;
    reg:hasSubproperty <http://rdaregistry.info/Elements/a/datatype/P50041> ;
    reg:hasUnconstrained <http://rdaregistry.info/Elements/u/P60549> ;
    reg:lexicalAlias <http://rdaregistry.info/Elements/a/preferredNameForCorporateBody.en> ;
    reg:name "preferredNameForCorporateBody"@en ;
    reg:status <http://metadataregistry.org/uri/RegStatus/1001> ;
    rdfs:domain <http://rdaregistry.info/Elements/c/C10005> ;
    rdfs:isDefinedBy <http://rdaregistry.info/Elements/a/> ;
    rdfs:subPropertyOf <http://rdaregistry.info/Elements/a/P50032> ;
    skos:definition "Relates a corporate body to a name or form of name chosen to identify a corporate body."@en,
        "Met une collectivité en relation avec le nom ou la forme de nom choisie pour identifier la collectivité."@fr .

<http://rdaregistry.info/Elements/a/P50042> a rdf:Property ;
    rdfs:label "is appellant corporate body of"@en,
        "est la collectivité appelante de"@fr ;
    rdakit:instructionNumber "18.5" ;
    rdakit:toolkitDefinition "A legal work of a higher court recording a decision of a lower court that is appealed by a corporate body."@en,
        "Collectivité qui en appelle de la décision d’un tribunal inférieur."@fr ;
    rdakit:toolkitLabel "appellant corporate body of"@en,
        "collectivité appelante de"@fr ;
    reg:hasSubproperty <http://rdaregistry.info/Elements/a/datatype/P50042>,
        <http://rdaregistry.info/Elements/a/object/P50042> ;
    reg:hasUnconstrained <http://rdaregistry.info/Elements/u/P60691> ;
    reg:lexicalAlias <http://rdaregistry.info/Elements/a/appellantCorporateBodyOf.en> ;
    reg:name "appellantCorporateBodyOf"@en ;
    reg:status <http://metadataregistry.org/uri/RegStatus/1001> ;
    rdfs:domain <http://rdaregistry.info/Elements/c/C10005> ;
    rdfs:isDefinedBy <http://rdaregistry.info/Elements/a/> ;
    rdfs:subPropertyOf <http://rdaregistry.info/Elements/a/P50088> ;
    skos:definition "Relates a corporate body who appeals a decision of a lower court recorded in a legal work of a higher court to a work."@en,
        "Met une collectivité qui en appelle de la décision d’un tribunal inférieur en relation avec l’œuvre."@fr .

<http://rdaregistry.info/Elements/a/P50043> a rdf:Property ;
    rdfs:label "is plaintiff corporate body of"@en,
        "est la collectivité demanderesse de"@fr ;
    rdakit:instructionNumber "18.5" ;
    rdakit:toolkitDefinition "A work that involves a responsibility for bringing a suit in a civil proceeding by a corporate body."@en,
        "Collectivité qui intente une poursuite civile."@fr ;
    rdakit:toolkitLabel "plaintiff corporate body of"@en,
        "collectivité demanderesse de"@fr ;
    reg:hasSubproperty <http://rdaregistry.info/Elements/a/datatype/P50043>,
        <http://rdaregistry.info/Elements/a/object/P50043> ;
    reg:hasUnconstrained <http://rdaregistry.info/Elements/u/P60693> ;
    reg:lexicalAlias <http://rdaregistry.info/Elements/a/plaintiffCorporateBodyOf.en> ;
    reg:name "plaintiffCorporateBodyOf"@en ;
    reg:status <http://metadataregistry.org/uri/RegStatus/1001> ;
    rdfs:domain <http://rdaregistry.info/Elements/c/C10005> ;
    rdfs:isDefinedBy <http://rdaregistry.info/Elements/a/> ;
    rdfs:subPropertyOf <http://rdaregistry.info/Elements/a/P50089> ;
    skos:definition "Relates a corporate body who brings a suit in a civil proceeding to a work."@en,
        "Met une collectivité qui intente une poursuite civile en relation avec l’œuvre."@fr .

<http://rdaregistry.info/Elements/a/P50044> a rdf:Property ;
    rdfs:label "is court governed of"@en,
        "est le tribunal régi de"@fr ;
    rdakit:instructionNumber "18.5" ;
    rdakit:toolkitDefinition "A work of a court governed by court rules, regardless of their official nature."@en,
        "Tribunal régi par des règles de pratique, sans égard à leur nature officielle (par exemple, lois, règlements)."@fr ;
    rdakit:toolkitLabel "court governed of"@en,
        "tribunal régi de"@fr ;
    reg:hasSubproperty <http://rdaregistry.info/Elements/a/datatype/P50044>,
        <http://rdaregistry.info/Elements/a/object/P50044> ;
    reg:hasUnconstrained <http://rdaregistry.info/Elements/u/P60005> ;
    reg:lexicalAlias <http://rdaregistry.info/Elements/a/courtGovernedOf.en> ;
    reg:name "courtGovernedOf"@en ;
    reg:status <http://metadataregistry.org/uri/RegStatus/1001> ;
    rdfs:domain <http://rdaregistry.info/Elements/c/C10005> ;
    rdfs:isDefinedBy <http://rdaregistry.info/Elements/a/> ;
    rdfs:subPropertyOf <http://rdaregistry.info/Elements/a/P50131> ;
    skos:definition "Relates a court governed by court rules, regardless of their official nature to a work."@en,
        "Met un tribunal régi par des règles de pratique, sans égard à leur nature officielle (par exemple, lois, règlements) en relation avec l’œuvre."@fr .

<http://rdaregistry.info/Elements/a/P50045> a rdf:Property ;
    rdfs:label "is collector of"@en,
        "est le collectionneur de"@fr ;
    rdakit:instructionNumber "18.5" ;
    rdakit:toolkitDefinition "An item brought together with items from various sources that are then arranged, described, and cataloged as a collection."@en,
        "Conservateur qui rassemble des items de diverses sources qui sont subséquemment arrangés, décrits et catalogués comme une collection."@fr ;
    rdakit:toolkitLabel "collector of"@en,
        "collectionneur de"@fr ;
    reg:hasSubproperty <http://rdaregistry.info/Elements/a/datatype/P50045>,
        <http://rdaregistry.info/Elements/a/object/P50045> ;
    reg:hasUnconstrained <http://rdaregistry.info/Elements/u/P60006> ;
    reg:lexicalAlias <http://rdaregistry.info/Elements/a/collectorOf.en> ;
    reg:name "collectorOf"@en ;
    reg:status <http://metadataregistry.org/uri/RegStatus/1001> ;
    rdfs:domain <http://rdaregistry.info/Elements/c/C10002> ;
    rdfs:isDefinedBy <http://rdaregistry.info/Elements/a/> ;
    rdfs:subPropertyOf <http://rdaregistry.info/Elements/a/P50133> ;
    skos:definition "Relates a curator who brings together items from various sources that are then arranged, described, and cataloged as a collection to an item."@en,
        "Met un conservateur qui rassemble des items de diverses sources qui sont subséquemment arrangés, décrits et catalogués comme une collection en relation avec l’item."@fr .

<http://rdaregistry.info/Elements/a/P50046> a rdf:Property ;
    rdfs:label "is collection registrar of"@en,
        "est le conservateur de collections de"@fr ;
    rdakit:instructionNumber "18.5" ;
    rdakit:toolkitDefinition "An item that is listed or inventoried in an aggregate work such as a collection of items or works."@en,
        "Conservateur qui dresse une liste et un inventaire des items faisant partie d’une œuvre agrégative telle qu’une collection d’items ou d’œuvres."@fr ;
    rdakit:toolkitLabel "collection registrar of"@en,
        "conservateur de collections de"@fr ;
    reg:hasSubproperty <http://rdaregistry.info/Elements/a/datatype/P50046>,
        <http://rdaregistry.info/Elements/a/object/P50046> ;
    reg:hasUnconstrained <http://rdaregistry.info/Elements/u/P60007> ;
    reg:lexicalAlias <http://rdaregistry.info/Elements/a/collectionRegistrarOf.en> ;
    reg:name "collectionRegistrarOf"@en ;
    reg:status <http://metadataregistry.org/uri/RegStatus/1001> ;
    rdfs:domain <http://rdaregistry.info/Elements/c/C10002> ;
    rdfs:isDefinedBy <http://rdaregistry.info/Elements/a/> ;
    rdfs:subPropertyOf <http://rdaregistry.info/Elements/a/P50133> ;
    skos:definition "Relates a curator who lists or inventories the items in an aggregate work such as a collection of items or works to an item."@en,
        "Met un conservateur qui dresse une liste et un inventaire des items faisant partie d’une œuvre agrégative telle qu’une collection d’items ou d’œuvres en relation avec l’item."@fr .

<http://rdaregistry.info/Elements/a/P50047> a rdf:Property ;
    rdfs:label "is depositor of"@en,
        "est le déposant de"@fr ;
    rdakit:instructionNumber "18.5" ;
    rdakit:toolkitDefinition "An item deposited into the custody of another agent, while still retaining ownership."@en,
        "Propriétaire actuel d’un item qui a déposé l’item sous la garde d’une autre personne, famille ou collectivité tout en en conservant la propriété."@fr ;
    rdakit:toolkitLabel "depositor of"@en,
        "déposant de"@fr ;
    reg:hasSubproperty <http://rdaregistry.info/Elements/a/datatype/P50047>,
        <http://rdaregistry.info/Elements/a/object/P50047> ;
    reg:hasUnconstrained <http://rdaregistry.info/Elements/u/P60008> ;
    reg:lexicalAlias <http://rdaregistry.info/Elements/a/depositorOf.en> ;
    reg:name "depositorOf"@en ;
    reg:status <http://metadataregistry.org/uri/RegStatus/1001> ;
    rdfs:domain <http://rdaregistry.info/Elements/c/C10002> ;
    rdfs:isDefinedBy <http://rdaregistry.info/Elements/a/> ;
    rdfs:subPropertyOf <http://rdaregistry.info/Elements/a/P50162> ;
    skos:definition "Relates a current owner of an item who deposited the item into the custody of another agent, while still retaining ownership to an item."@en,
        "Met un propriétaire actuel d’un item qui a déposé l’item sous la garde d’une autre personne, famille ou collectivité tout en en conservant la propriété en relation avec l’item."@fr .

<http://rdaregistry.info/Elements/a/P50048> a rdf:Property ;
    rdfs:label "is film director of"@en,
        "est le réalisateur de films de"@fr ;
    rdakit:instructionNumber "18.5" ;
    rdakit:toolkitDefinition "A work that involves a responsibility for the general management and supervision of a filmed performance."@en,
        "Réalisateur responsable de la gestion et de la supervision générales d’une prestation filmée."@fr ;
    rdakit:toolkitLabel "film director of"@en,
        "réalisateur de films de"@fr ;
    reg:hasSubproperty <http://rdaregistry.info/Elements/a/datatype/P50048>,
        <http://rdaregistry.info/Elements/a/object/P50048> ;
    reg:hasUnconstrained <http://rdaregistry.info/Elements/u/P60009> ;
    reg:lexicalAlias <http://rdaregistry.info/Elements/a/filmDirectorOf.en> ;
    reg:name "filmDirectorOf"@en ;
    reg:status <http://metadataregistry.org/uri/RegStatus/1001> ;
    rdfs:domain <http://rdaregistry.info/Elements/c/C10002> ;
    rdfs:isDefinedBy <http://rdaregistry.info/Elements/a/> ;
    rdfs:subPropertyOf <http://rdaregistry.info/Elements/a/P50205> ;
    skos:definition "Relates a director responsible for the general management and supervision of a filmed performance to a work."@en,
        "Met un réalisateur responsable de la gestion et de la supervision générales d’une prestation filmée en relation avec l’œuvre."@fr .

<http://rdaregistry.info/Elements/a/P50049> a rdf:Property ;
    rdfs:label "is radio director of"@en,
        "est le réalisateur d’émissions de radio de"@fr ;
    rdakit:instructionNumber "18.5" ;
    rdakit:toolkitDefinition "A work that involves a responsibility for the general management and supervision of a radio program."@en,
        "Réalisateur responsable de la gestion et de la supervision générales d’une émission de radio."@fr ;
    rdakit:toolkitLabel "radio director of"@en,
        "réalisateur d’émissions de radio de"@fr ;
    reg:hasSubproperty <http://rdaregistry.info/Elements/a/datatype/P50049>,
        <http://rdaregistry.info/Elements/a/object/P50049> ;
    reg:hasUnconstrained <http://rdaregistry.info/Elements/u/P60010> ;
    reg:lexicalAlias <http://rdaregistry.info/Elements/a/radioDirectorOf.en> ;
    reg:name "radioDirectorOf"@en ;
    reg:status <http://metadataregistry.org/uri/RegStatus/1001> ;
    rdfs:domain <http://rdaregistry.info/Elements/c/C10002> ;
    rdfs:isDefinedBy <http://rdaregistry.info/Elements/a/> ;
    rdfs:subPropertyOf <http://rdaregistry.info/Elements/a/P50205> ;
    skos:definition "Relates a director responsible for the general management and supervision of a radio program to a work."@en,
        "Met un réalisateur responsable de la gestion et de la supervision générales d’une émission de radio en relation avec l’œuvre."@fr .

<http://rdaregistry.info/Elements/a/P50050> a rdf:Property ;
    rdfs:label "is television director of"@en,
        "est le réalisateur d’émissions de télévision de"@fr ;
    rdakit:instructionNumber "18.5" ;
    rdakit:toolkitDefinition "A work that involves a responsibility for the general management and supervision of a television program."@en,
        "Réalisateur responsable de la gestion et de la supervision générales d’une émission de télévision."@fr ;
    rdakit:toolkitLabel "television director of"@en,
        "réalisateur d’émissions de télévision de"@fr ;
    reg:hasSubproperty <http://rdaregistry.info/Elements/a/datatype/P50050>,
        <http://rdaregistry.info/Elements/a/object/P50050> ;
    reg:hasUnconstrained <http://rdaregistry.info/Elements/u/P60011> ;
    reg:lexicalAlias <http://rdaregistry.info/Elements/a/televisionDirectorOf.en> ;
    reg:name "televisionDirectorOf"@en ;
    reg:status <http://metadataregistry.org/uri/RegStatus/1001> ;
    rdfs:domain <http://rdaregistry.info/Elements/c/C10002> ;
    rdfs:isDefinedBy <http://rdaregistry.info/Elements/a/> ;
    rdfs:subPropertyOf <http://rdaregistry.info/Elements/a/P50205> ;
    skos:definition "Relates a director responsible for the general management and supervision of a television program to a work."@en,
        "Met un réalisateur responsable de la gestion et de la supervision générales d’une émission de télévision en relation avec l’œuvre."@fr .

<http://rdaregistry.info/Elements/a/P50054> a rdf:Property ;
    rdfs:label "has variant name for family"@en,
        "a pour variante de nom de la famille"@fr,
        "har variantnamn för familjen/släkten"@sv ;
    rdakit:instructionNumber "10.2.3" ;
    rdakit:toolkitDefinition "A name or form of name by which a family is known that differs from a name or form of name chosen as a preferred name."@en,
        "Un nombre o una forma del nombre mediante el cual se conoce una familia, que difiere del nombre o la forma del nombre elegida como el nombre preferido."@es,
        "Nom ou forme de nom sous laquelle une famille est connue et qui diffère du nom ou de la forme de nom choisie comme nom privilégié."@fr ;
    rdakit:toolkitLabel "variant name for family"@en,
        "variante del nombre de la familia"@es,
        "variante de nom de la famille"@fr,
        "variantnamn för familjen/släkten"@sv ;
    reg:hasSubproperty <http://rdaregistry.info/Elements/a/datatype/P50054> ;
    reg:hasUnconstrained <http://rdaregistry.info/Elements/u/P60119> ;
    reg:lexicalAlias <http://rdaregistry.info/Elements/a/variantNameForFamily.en> ;
    reg:name "variantNameForFamily"@en ;
    reg:status <http://metadataregistry.org/uri/RegStatus/1001> ;
    rdfs:domain <http://rdaregistry.info/Elements/c/C10008> ;
    rdfs:isDefinedBy <http://rdaregistry.info/Elements/a/> ;
    rdfs:subPropertyOf <http://rdaregistry.info/Elements/a/P50061> ;
    skos:definition "Relates a family to a name or form of name by which a family is known that differs from a name or form of name chosen as a preferred name."@en,
        "Met une famille en relation avec un nom ou une forme de nom sous laquelle une famille est connue et qui diffère du nom ou de la forme de nom choisie comme nom privilégié."@fr ;
    skos:scopeNote "Variant name for family includes a name or form of name used by a family or found in reference sources, a name resulting from a different transliteration of a name, etc."@en .

<http://rdaregistry.info/Elements/a/P50055> a rdf:Property ;
    rdfs:label "has progenitor"@en,
        "a pour ancêtre"@fr ;
    rdakit:instructionNumber "29.5" ;
    rdakit:toolkitDefinition "A person from whom a family is descended."@en,
        "Una persona de la cual desciende la familia."@es,
        "Personne de qui la famille descend."@fr ;
    rdakit:toolkitLabel "progenitor"@en,
        "progenitor"@es,
        "ancêtre"@fr ;
    reg:hasSubproperty <http://rdaregistry.info/Elements/a/datatype/P50055>,
        <http://rdaregistry.info/Elements/a/object/P50055> ;
    reg:hasUnconstrained <http://rdaregistry.info/Elements/u/P60683> ;
    reg:lexicalAlias <http://rdaregistry.info/Elements/a/progenitor.en> ;
    reg:name "progenitor"@en ;
    reg:status <http://metadataregistry.org/uri/RegStatus/1001> ;
    rdfs:domain <http://rdaregistry.info/Elements/c/C10008> ;
    rdfs:isDefinedBy <http://rdaregistry.info/Elements/a/> ;
    rdfs:subPropertyOf <http://rdaregistry.info/Elements/a/P50056> ;
    skos:definition "Relates a family to a person from whom a family is descended."@en,
        "Met une famille en relation avec une personne de qui la famille descend."@fr .

<http://rdaregistry.info/Elements/a/P50056> a rdf:Property ;
    rdfs:label "has family member"@en,
        "a pour membre de la famille"@fr ;
    rdakit:instructionNumber "29.5" ;
    rdakit:toolkitDefinition "A person who is a member of a family."@en,
        "Una persona que es un miembro de la familia."@es,
        "Personne qui est membre de la famille."@fr ;
    rdakit:toolkitLabel "family member"@en,
        "miembro de la familia"@es,
        "membre de la famille"@fr ;
    reg:hasSubproperty <http://rdaregistry.info/Elements/a/P50055>,
        <http://rdaregistry.info/Elements/a/datatype/P50056>,
        <http://rdaregistry.info/Elements/a/object/P50056> ;
    reg:hasUnconstrained <http://rdaregistry.info/Elements/u/P60648> ;
    reg:lexicalAlias <http://rdaregistry.info/Elements/a/familyMember.en> ;
    reg:name "familyMember"@en ;
    reg:status <http://metadataregistry.org/uri/RegStatus/1001> ;
    rdfs:domain <http://rdaregistry.info/Elements/c/C10008> ;
    rdfs:isDefinedBy <http://rdaregistry.info/Elements/a/> ;
    skos:definition "Relates a family to a person who is a member of a family."@en,
        "Met une famille en relation avec une personne qui est membre de la famille."@fr .

<http://rdaregistry.info/Elements/a/P50065> a rdf:Property ;
    rdfs:label "has preferred name for family"@en,
        "a pour nom privilégié de la famille"@fr,
        "har föredraget namn för familjen/släkten"@sv ;
    rdakit:instructionNumber "10.2.2" ;
    rdakit:toolkitDefinition "A name or form of name chosen to identify a family."@en,
        "El nombre o la forma del nombre elegida para identificar la familia."@es,
        "Le nom ou la forme de nom choisie pour identifier la famille."@fr ;
    rdakit:toolkitLabel "preferred name for family"@en,
        "nombre preferido de la familia"@es,
        "nom privilégié de la famille"@fr,
        "föredraget namn för familjen/släkten"@sv ;
    reg:hasSubproperty <http://rdaregistry.info/Elements/a/datatype/P50065> ;
    reg:hasUnconstrained <http://rdaregistry.info/Elements/u/P60549> ;
    reg:lexicalAlias <http://rdaregistry.info/Elements/a/preferredNameForFamily.en> ;
    reg:name "preferredNameForFamily"@en ;
    reg:status <http://metadataregistry.org/uri/RegStatus/1001> ;
    rdfs:domain <http://rdaregistry.info/Elements/c/C10008> ;
    rdfs:isDefinedBy <http://rdaregistry.info/Elements/a/> ;
    rdfs:subPropertyOf <http://rdaregistry.info/Elements/a/P50061> ;
    skos:definition "Relates a family to a name or form of name chosen to identify a family."@en,
        "Met une famille en relation avec le nom ou la forme de nom choisie pour identifier la famille."@fr .

<http://rdaregistry.info/Elements/a/P50066> a rdf:Property ;
    rdfs:label "is donor of"@en,
        "est le donateur de"@fr ;
    rdakit:instructionNumber "18.5" ;
    rdakit:toolkitDefinition "An item donated to another owner."@en,
        "Ancien propriétaire d’un item qui a fait don de cet item à un autre propriétaire."@fr ;
    rdakit:toolkitLabel "donor of"@en,
        "donateur de"@fr ;
    reg:hasSubproperty <http://rdaregistry.info/Elements/a/datatype/P50066>,
        <http://rdaregistry.info/Elements/a/object/P50066> ;
    reg:hasUnconstrained <http://rdaregistry.info/Elements/u/P60012> ;
    reg:lexicalAlias <http://rdaregistry.info/Elements/a/donorOf.en> ;
    reg:name "donorOf"@en ;
    reg:status <http://metadataregistry.org/uri/RegStatus/1001> ;
    rdfs:domain <http://rdaregistry.info/Elements/c/C10002> ;
    rdfs:isDefinedBy <http://rdaregistry.info/Elements/a/> ;
    rdfs:subPropertyOf <http://rdaregistry.info/Elements/a/P50163> ;
    skos:definition "Relates a former owner of an item who donated that item to another owner to an item."@en,
        "Met un ancien propriétaire d’un item qui a fait don de cet item à un autre propriétaire en relation avec l’item."@fr .

<http://rdaregistry.info/Elements/a/P50067> a rdf:Property ;
    rdfs:label "is seller of"@en,
        "est le vendeur de"@fr ;
    rdakit:instructionNumber "18.5" ;
    rdakit:toolkitDefinition "An item sold to another owner."@en,
        "Ancien propriétaire d’un item qui a vendu cet item à un autre propriétaire."@fr ;
    rdakit:toolkitLabel "seller of"@en,
        "vendeur de"@fr ;
    reg:hasSubproperty <http://rdaregistry.info/Elements/a/datatype/P50067>,
        <http://rdaregistry.info/Elements/a/object/P50067> ;
    reg:hasUnconstrained <http://rdaregistry.info/Elements/u/P60013> ;
    reg:lexicalAlias <http://rdaregistry.info/Elements/a/sellerOf.en> ;
    reg:name "sellerOf"@en ;
    reg:status <http://metadataregistry.org/uri/RegStatus/1001> ;
    rdfs:domain <http://rdaregistry.info/Elements/c/C10002> ;
    rdfs:isDefinedBy <http://rdaregistry.info/Elements/a/> ;
    rdfs:subPropertyOf <http://rdaregistry.info/Elements/a/P50163> ;
    skos:definition "Relates a former owner of an item who sold that item to another owner to an item."@en,
        "Met un ancien propriétaire d’un item qui a vendu cet item à un autre propriétaire en relation avec l’item."@fr .

<http://rdaregistry.info/Elements/a/P50068> a rdf:Property ;
    rdfs:label "is enacting jurisdiction of"@en,
        "est la juridiction promulgatrice de"@fr ;
    rdakit:instructionNumber "18.5" ;
    rdakit:toolkitDefinition "A work enacting a law, regulation, constitution, court rule, etc."@en,
        "Juridiction promulguant une loi, un règlement, une constitution, une règle de pratique de tribunal, etc."@fr ;
    rdakit:toolkitLabel "enacting jurisdiction of"@en,
        "juridiction promulgatrice de"@fr ;
    reg:hasSubproperty <http://rdaregistry.info/Elements/a/datatype/P50068>,
        <http://rdaregistry.info/Elements/a/object/P50068> ;
    reg:hasUnconstrained <http://rdaregistry.info/Elements/u/P60014> ;
    reg:lexicalAlias <http://rdaregistry.info/Elements/a/enactingJurisdictionOf.en> ;
    reg:name "enactingJurisdictionOf"@en ;
    reg:status <http://metadataregistry.org/uri/RegStatus/1001> ;
    rdfs:domain <http://rdaregistry.info/Elements/c/C10005> ;
    rdfs:isDefinedBy <http://rdaregistry.info/Elements/a/> ;
    rdfs:subPropertyOf <http://rdaregistry.info/Elements/a/P50204> ;
    skos:definition "Relates a jurisdiction enacting a law, regulation, constitution, court rule, etc. to a work."@en,
        "Met une juridiction promulguant une loi, un règlement, une constitution, une règle de pratique de tribunal, etc. en relation avec l’œuvre."@fr .

<http://rdaregistry.info/Elements/a/P50069> a rdf:Property ;
    rdfs:label "is jurisdiction governed of"@en,
        "est la juridiction régie de"@fr ;
    rdakit:instructionNumber "18.5" ;
    rdakit:toolkitDefinition "A law, regulation, etc., that was enacted by another jurisdiction."@en,
        "Juridiction régie par une loi, un règlement, etc. qui a été promulgué par une autre juridiction."@fr ;
    rdakit:toolkitLabel "jurisdiction governed of"@en,
        "juridiction régie de"@fr ;
    reg:hasSubproperty <http://rdaregistry.info/Elements/a/datatype/P50069>,
        <http://rdaregistry.info/Elements/a/object/P50069> ;
    reg:hasUnconstrained <http://rdaregistry.info/Elements/u/P60015> ;
    reg:lexicalAlias <http://rdaregistry.info/Elements/a/jurisdictionGovernedOf.en> ;
    reg:name "jurisdictionGovernedOf"@en ;
    reg:status <http://metadataregistry.org/uri/RegStatus/1001> ;
    rdfs:domain <http://rdaregistry.info/Elements/c/C10005> ;
    rdfs:isDefinedBy <http://rdaregistry.info/Elements/a/> ;
    rdfs:subPropertyOf <http://rdaregistry.info/Elements/a/P50131> ;
    skos:definition "Relates a jurisdiction governed by a law, regulation, etc., that was enacted by another jurisdiction to a work."@en,
        "Met une juridiction régie par une loi, un règlement, etc. qui a été promulgué par une autre juridiction en relation avec l’œuvre."@fr .

<http://rdaregistry.info/Elements/a/P50073> a rdf:Property ;
    rdfs:label "is dancer of"@en,
        "est le danseur de"@fr ;
    rdakit:instructionNumber "18.5" ;
    rdakit:toolkitDefinition "An expression of a work that incorporates a performance of dancing in a musical, dramatic, etc., presentation."@en,
        "Interprète contribuant à une expression d’une œuvre en dansant dans une représentation musicale ou dramatique, etc."@fr ;
    rdakit:toolkitLabel "dancer of"@en,
        "danseur de"@fr ;
    reg:hasSubproperty <http://rdaregistry.info/Elements/a/datatype/P50073>,
        <http://rdaregistry.info/Elements/a/object/P50073> ;
    reg:hasUnconstrained <http://rdaregistry.info/Elements/u/P60019> ;
    reg:lexicalAlias <http://rdaregistry.info/Elements/a/dancerOf.en> ;
    reg:name "dancerOf"@en ;
    reg:status <http://metadataregistry.org/uri/RegStatus/1001> ;
    rdfs:domain <http://rdaregistry.info/Elements/c/C10002> ;
    rdfs:isDefinedBy <http://rdaregistry.info/Elements/a/> ;
    rdfs:subPropertyOf <http://rdaregistry.info/Elements/a/P50147> ;
    skos:definition "Relates a performer contributing to an expression of a work by dancing in a musical, dramatic, etc., presentation to an expression."@en,
        "Met un interprète contribuant à une expression d’une œuvre en dansant dans une représentation musicale ou dramatique, etc. en relation avec l’expression."@fr .

<http://rdaregistry.info/Elements/a/P50074> a rdf:Property ;
    rdfs:label "is instructor of"@en,
        "est l’enseignant de"@fr ;
    rdakit:instructionNumber "18.5" ;
    rdakit:toolkitDefinition "An expression of a work that incorporates a performance of teaching or providing a demonstration."@en,
        "Interprète contribuant à une expression d’une œuvre en transmettant des connaissances par la théorie ou la pratique."@fr ;
    rdakit:toolkitLabel "instructor of"@en,
        "enseignant de"@fr ;
    reg:hasSubproperty <http://rdaregistry.info/Elements/a/datatype/P50074>,
        <http://rdaregistry.info/Elements/a/object/P50074> ;
    reg:hasUnconstrained <http://rdaregistry.info/Elements/u/P60020> ;
    reg:lexicalAlias <http://rdaregistry.info/Elements/a/instructorOf.en> ;
    reg:name "instructorOf"@en ;
    reg:status <http://metadataregistry.org/uri/RegStatus/1001> ;
    rdfs:domain <http://rdaregistry.info/Elements/c/C10002> ;
    rdfs:isDefinedBy <http://rdaregistry.info/Elements/a/> ;
    rdfs:subPropertyOf <http://rdaregistry.info/Elements/a/P50147> ;
    skos:definition "Relates a performer contributing to an expression of a work by teaching or providing a demonstration to an expression."@en,
        "Met un interprète contribuant à une expression d’une œuvre en transmettant des connaissances par la théorie ou la pratique en relation avec l’expression."@fr .

<http://rdaregistry.info/Elements/a/P50075> a rdf:Property ;
    rdfs:label "is host of"@en,
        "est l’hôte de"@fr ;
    rdakit:instructionNumber "18.5" ;
    rdakit:toolkitDefinition "An expression of a work that incorporates a performance of leading a program, often broadcast, that includes other guests, performers, etc."@en,
        "Interprète contribuant à une expression d’une œuvre en dirigeant une émission (souvent diffusée) qui comprend d’autres invités, interprètes, etc. (par exemple, un animateur d’émission-débat)."@fr ;
    rdakit:toolkitLabel "host of"@en,
        "hôte de"@fr ;
    reg:hasSubproperty <http://rdaregistry.info/Elements/a/datatype/P50075>,
        <http://rdaregistry.info/Elements/a/object/P50075> ;
    reg:hasUnconstrained <http://rdaregistry.info/Elements/u/P60021> ;
    reg:lexicalAlias <http://rdaregistry.info/Elements/a/hostOf.en> ;
    reg:name "hostOf"@en ;
    reg:status <http://metadataregistry.org/uri/RegStatus/1001> ;
    rdfs:domain <http://rdaregistry.info/Elements/c/C10002> ;
    rdfs:isDefinedBy <http://rdaregistry.info/Elements/a/> ;
    rdfs:subPropertyOf <http://rdaregistry.info/Elements/a/P50147> ;
    skos:definition "Relates a performer contributing to an expression of a work by leading a program, often broadcast, that includes other guests, performers, etc., to an expression."@en,
        "Met un interprète contribuant à une expression d’une œuvre en dirigeant une émission (souvent diffusée) qui comprend d’autres invités, interprètes, etc. (par exemple, un animateur d’émission-débat) en relation avec l’expression."@fr .

<http://rdaregistry.info/Elements/a/P50076> a rdf:Property ;
    rdfs:label "is moderator of"@en,
        "est le modérateur de"@fr ;
    rdakit:instructionNumber "18.5" ;
    rdakit:toolkitDefinition "An expression of a work that incorporates a performance of leading a program, often broadcast, where topics are discussed, usually with participation of experts in fields related to the discussion."@en,
        "Interprète contribuant à une expression d’une œuvre en dirigeant une émission (souvent diffusée) où des sujets sont discutés, habituellement avec la participation d’experts dans les domaines reliés à la discussion."@fr ;
    rdakit:toolkitLabel "moderator of"@en,
        "modérateur de"@fr ;
    reg:hasSubproperty <http://rdaregistry.info/Elements/a/datatype/P50076>,
        <http://rdaregistry.info/Elements/a/object/P50076> ;
    reg:hasUnconstrained <http://rdaregistry.info/Elements/u/P60022> ;
    reg:lexicalAlias <http://rdaregistry.info/Elements/a/moderatorOf.en> ;
    reg:name "moderatorOf"@en ;
    reg:status <http://metadataregistry.org/uri/RegStatus/1001> ;
    rdfs:domain <http://rdaregistry.info/Elements/c/C10002> ;
    rdfs:isDefinedBy <http://rdaregistry.info/Elements/a/> ;
    rdfs:subPropertyOf <http://rdaregistry.info/Elements/a/P50147> ;
    skos:definition "Relates a performer contributing to an expression of a work by leading a program, often broadcast, where topics are discussed, usually with participation of experts in fields related to the discussion to an expression."@en,
        "Met un interprète contribuant à une expression d’une œuvre en dirigeant une émission (souvent diffusée) où des sujets sont discutés, habituellement avec la participation d’experts dans les domaines reliés à la discussion en relation avec l’expression."@fr .

<http://rdaregistry.info/Elements/a/P50077> a rdf:Property ;
    rdfs:label "is puppeteer of"@en,
        "est le marionnettiste de"@fr ;
    rdakit:instructionNumber "18.5" ;
    rdakit:toolkitDefinition "An expression of a work that incorporates a performance of manipulating, controlling, or directing puppets or marionettes in a moving image production or a musical or dramatic presentation or entertainment."@en,
        "Interprète contribuant à une expression d’une œuvre en manipulant, en contrôlant ou en dirigeant des marionnettes dans une production d’images animées ou bien dans une représentation ou un spectacle musical ou dramatique."@fr ;
    rdakit:toolkitLabel "puppeteer of"@en,
        "marionnettiste de"@fr ;
    reg:hasSubproperty <http://rdaregistry.info/Elements/a/datatype/P50077>,
        <http://rdaregistry.info/Elements/a/object/P50077> ;
    reg:hasUnconstrained <http://rdaregistry.info/Elements/u/P60023> ;
    reg:lexicalAlias <http://rdaregistry.info/Elements/a/puppeteerOf.en> ;
    reg:name "puppeteerOf"@en ;
    reg:status <http://metadataregistry.org/uri/RegStatus/1001> ;
    rdfs:domain <http://rdaregistry.info/Elements/c/C10002> ;
    rdfs:isDefinedBy <http://rdaregistry.info/Elements/a/> ;
    rdfs:subPropertyOf <http://rdaregistry.info/Elements/a/P50147> ;
    skos:definition "Relates a performer contributing to an expression of a work by manipulating, controlling, or directing puppets or marionettes in a moving image production or a musical or dramatic presentation or entertainment to an expression."@en,
        "Met un interprète contribuant à une expression d’une œuvre en manipulant, en contrôlant ou en dirigeant des marionnettes dans une production d’images animées ou bien dans une représentation ou un spectacle musical ou dramatique en relation avec l’expression."@fr .

<http://rdaregistry.info/Elements/a/P50078> a rdf:Property ;
    rdfs:label "is panelist of"@en,
        "est le panéliste de"@fr ;
    rdakit:instructionNumber "18.5" ;
    rdakit:toolkitDefinition "An expression of a work that incorporates a performance of participating in a program, often broadcast, where topics are discussed, usually with participation of experts in fields related to the discussion."@en,
        "Interprète contribuant à une expression d’une œuvre en participant à une émission (souvent diffusée) où des sujets sont discutés, habituellement avec la participation d’experts dans les domaines reliés à la discussion."@fr ;
    rdakit:toolkitLabel "panelist of"@en,
        "panéliste de"@fr ;
    reg:hasSubproperty <http://rdaregistry.info/Elements/a/datatype/P50078>,
        <http://rdaregistry.info/Elements/a/object/P50078> ;
    reg:hasUnconstrained <http://rdaregistry.info/Elements/u/P60024> ;
    reg:lexicalAlias <http://rdaregistry.info/Elements/a/panelistOf.en> ;
    reg:name "panelistOf"@en ;
    reg:status <http://metadataregistry.org/uri/RegStatus/1001> ;
    rdfs:domain <http://rdaregistry.info/Elements/c/C10002> ;
    rdfs:isDefinedBy <http://rdaregistry.info/Elements/a/> ;
    rdfs:subPropertyOf <http://rdaregistry.info/Elements/a/P50147> ;
    skos:definition "Relates a performer contributing to an expression of a work by participating in a program, often broadcast, where topics are discussed, usually with participation of experts in fields related to the discussion to an expression."@en,
        "Met un interprète contribuant à une expression d’une œuvre en participant à une émission (souvent diffusée) où des sujets sont discutés, habituellement avec la participation d’experts dans les domaines reliés à la discussion en relation avec l’expression."@fr .

<http://rdaregistry.info/Elements/a/P50079> a rdf:Property ;
    rdfs:label "is instrumentalist of"@en,
        "est l’instrumentiste de"@fr ;
    rdakit:instructionNumber "18.5" ;
    rdakit:toolkitDefinition "An expression of a work that incorporates a performance of playing a musical instrument."@en,
        "Interprète contribuant à une expression d’une œuvre en jouant d’un instrument de musique."@fr ;
    rdakit:toolkitLabel "instrumentalist of"@en,
        "instrumentiste de"@fr ;
    reg:hasSubproperty <http://rdaregistry.info/Elements/a/datatype/P50079>,
        <http://rdaregistry.info/Elements/a/object/P50079> ;
    reg:hasUnconstrained <http://rdaregistry.info/Elements/u/P60025> ;
    reg:lexicalAlias <http://rdaregistry.info/Elements/a/instrumentalistOf.en> ;
    reg:name "instrumentalistOf"@en ;
    reg:status <http://metadataregistry.org/uri/RegStatus/1001> ;
    rdfs:domain <http://rdaregistry.info/Elements/c/C10002> ;
    rdfs:isDefinedBy <http://rdaregistry.info/Elements/a/> ;
    rdfs:subPropertyOf <http://rdaregistry.info/Elements/a/P50147> ;
    skos:definition "Relates a performer contributing to an expression of a work by playing a musical instrument to an expression."@en,
        "Met un interprète contribuant à une expression d’une œuvre en jouant d’un instrument de musique en relation avec l’expression."@fr .

<http://rdaregistry.info/Elements/a/P50080> a rdf:Property ;
    rdfs:label "is commentator of"@en,
        "est le commentateur de"@fr ;
    rdakit:instructionNumber "18.5" ;
    rdakit:toolkitDefinition "An expression of a work that incorporates a performance of providing interpretation, analysis, or a discussion of the subject matter on a recording, film, or other audiovisual medium."@en,
        "Interprète contribuant à une expression d’une œuvre en fournissant une interprétation, une analyse ou une explication du sujet sur un enregistrement, un film ou un autre support audiovisuel."@fr ;
    rdakit:toolkitLabel "commentator of"@en,
        "commentateur de"@fr ;
    reg:hasSubproperty <http://rdaregistry.info/Elements/a/datatype/P50080>,
        <http://rdaregistry.info/Elements/a/object/P50080> ;
    reg:hasUnconstrained <http://rdaregistry.info/Elements/u/P60026> ;
    reg:lexicalAlias <http://rdaregistry.info/Elements/a/commentatorOf.en> ;
    reg:name "commentatorOf"@en ;
    reg:status <http://metadataregistry.org/uri/RegStatus/1001> ;
    rdfs:domain <http://rdaregistry.info/Elements/c/C10002> ;
    rdfs:isDefinedBy <http://rdaregistry.info/Elements/a/> ;
    rdfs:subPropertyOf <http://rdaregistry.info/Elements/a/P50147> ;
    skos:definition "Relates a performer contributing to an expression of a work by providing interpretation, analysis, or a discussion of the subject matter on a recording, film, or other audiovisual medium to an expression."@en,
        "Met un interprète contribuant à une expression d’une œuvre en fournissant une interprétation, une analyse ou une explication du sujet sur un enregistrement, un film ou un autre support audiovisuel en relation avec l’expression."@fr .

<http://rdaregistry.info/Elements/a/P50081> a rdf:Property ;
    rdfs:label "is narrator of"@en,
        "est le narrateur de"@fr ;
    rdakit:instructionNumber "18.5" ;
    rdakit:toolkitDefinition "An expression of a work that incorporates a performance of reading aloud or giving an account of an act, occurrence, course of events, etc."@en,
        "Interprète contribuant à une expression d’une œuvre en lisant à voix haute ou en rendant compte d’une action, d’une situation, du déroulement des événements, etc."@fr ;
    rdakit:toolkitLabel "narrator of"@en,
        "narrateur de"@fr ;
    reg:hasSubproperty <http://rdaregistry.info/Elements/a/datatype/P50081>,
        <http://rdaregistry.info/Elements/a/object/P50081> ;
    reg:hasUnconstrained <http://rdaregistry.info/Elements/u/P60028> ;
    reg:lexicalAlias <http://rdaregistry.info/Elements/a/narratorOf.en> ;
    reg:name "narratorOf"@en ;
    reg:status <http://metadataregistry.org/uri/RegStatus/1001> ;
    rdfs:domain <http://rdaregistry.info/Elements/c/C10002> ;
    rdfs:isDefinedBy <http://rdaregistry.info/Elements/a/> ;
    rdfs:subPropertyOf <http://rdaregistry.info/Elements/a/P50147> ;
    skos:definition "Relates a performer contributing to an expression of a work by reading aloud or giving an account of an act, occurrence, course of events, etc. to an expression."@en,
        "Met un interprète contribuant à une expression d’une œuvre en lisant à voix haute ou en rendant compte d’une action, d’une situation, du déroulement des événements, etc. en relation avec l’expression."@fr .

<http://rdaregistry.info/Elements/a/P50082> a rdf:Property ;
    rdfs:label "is storyteller of"@en,
        "est le conteur de"@fr ;
    rdakit:instructionNumber "18.5" ;
    rdakit:toolkitDefinition "An expression of a work that incorporates a performance of relaying a creator's original story with dramatic or theatrical interpretation."@en,
        "Interprète contribuant à une expression d’une œuvre en racontant l’histoire originale d’un créateur dans une interprétation dramatique ou théâtrale."@fr ;
    rdakit:toolkitLabel "storyteller of"@en,
        "conteur de"@fr ;
    reg:hasSubproperty <http://rdaregistry.info/Elements/a/datatype/P50082>,
        <http://rdaregistry.info/Elements/a/object/P50082> ;
    reg:hasUnconstrained <http://rdaregistry.info/Elements/u/P60029> ;
    reg:lexicalAlias <http://rdaregistry.info/Elements/a/storytellerOf.en> ;
    reg:name "storytellerOf"@en ;
    reg:status <http://metadataregistry.org/uri/RegStatus/1001> ;
    rdfs:domain <http://rdaregistry.info/Elements/c/C10002> ;
    rdfs:isDefinedBy <http://rdaregistry.info/Elements/a/> ;
    rdfs:subPropertyOf <http://rdaregistry.info/Elements/a/P50147> ;
    skos:definition "Relates a performer contributing to an expression of a work by relaying a creator's original story with dramatic or theatrical interpretation to an expression."@en,
        "Met un interprète contribuant à une expression d’une œuvre en racontant l’histoire originale d’un créateur dans une interprétation dramatique ou théâtrale en relation avec l’expression."@fr .

<http://rdaregistry.info/Elements/a/P50083> a rdf:Property ;
    rdfs:label "is speaker of"@en,
        "est l’orateur de"@fr ;
    rdakit:instructionNumber "18.5" ;
    rdakit:toolkitDefinition "An expression of a work that incorporates a performance of speaking words, such as a lecture, speech, etc."@en,
        "Interprète contribuant à une expression d’une œuvre en énonçant des paroles, telles qu’un exposé, un discours, etc."@fr ;
    rdakit:toolkitLabel "speaker of"@en,
        "orateur de"@fr ;
    reg:hasSubproperty <http://rdaregistry.info/Elements/a/datatype/P50083>,
        <http://rdaregistry.info/Elements/a/object/P50083> ;
    reg:hasUnconstrained <http://rdaregistry.info/Elements/u/P60030> ;
    reg:lexicalAlias <http://rdaregistry.info/Elements/a/speakerOf.en> ;
    reg:name "speakerOf"@en ;
    reg:status <http://metadataregistry.org/uri/RegStatus/1001> ;
    rdfs:domain <http://rdaregistry.info/Elements/c/C10002> ;
    rdfs:isDefinedBy <http://rdaregistry.info/Elements/a/> ;
    rdfs:subPropertyOf <http://rdaregistry.info/Elements/a/P50147> ;
    skos:definition "Relates a performer contributing to an expression of a work by speaking words, such as a lecture, speech, etc. to an expression."@en,
        "Met un interprète contribuant à une expression d’une œuvre en énonçant des paroles, telles qu’un exposé, un discours, etc., en relation avec l’expression."@fr .

<http://rdaregistry.info/Elements/a/P50084> a rdf:Property ;
    rdfs:label "is singer of"@en,
        "est le chanteur de"@fr ;
    rdakit:instructionNumber "18.5" ;
    rdakit:toolkitDefinition "An expression of a work that incorporates a performance of using his/her/their voice, with or without instrumental accompaniment, to produce music."@en,
        "Interprète contribuant à une expression d’une œuvre en utilisant sa voix, avec ou sans accompagnement instrumental, pour produire de la musique."@fr ;
    rdakit:toolkitLabel "singer of"@en,
        "chanteur de"@fr ;
    reg:hasSubproperty <http://rdaregistry.info/Elements/a/datatype/P50084>,
        <http://rdaregistry.info/Elements/a/object/P50084> ;
    reg:hasUnconstrained <http://rdaregistry.info/Elements/u/P60031> ;
    reg:lexicalAlias <http://rdaregistry.info/Elements/a/singerOf.en> ;
    reg:name "singerOf"@en ;
    reg:status <http://metadataregistry.org/uri/RegStatus/1001> ;
    rdfs:domain <http://rdaregistry.info/Elements/c/C10002> ;
    rdfs:isDefinedBy <http://rdaregistry.info/Elements/a/> ;
    rdfs:subPropertyOf <http://rdaregistry.info/Elements/a/P50147> ;
    skos:definition "Relates a performer contributing to an expression of a work by using his/her/their voice, with or without instrumental accompaniment, to produce music to an expression."@en,
        "Met un interprète contribuant à une expression d’une œuvre en utilisant sa voix, avec ou sans accompagnement instrumental, pour produire de la musique en relation avec l’expression."@fr ;
    skos:scopeNote "A singer's performance may or may not include actual words."@en,
        "La prestation d’un chanteur peut inclure ou non des paroles."@fr .

<http://rdaregistry.info/Elements/a/P50085> a rdf:Property ;
    rdfs:label "is appellee person of"@en,
        "est la personne intimée de"@fr ;
    rdakit:instructionNumber "18.5" ;
    rdakit:toolkitDefinition "A legal work of a higher court recording a decision of a lower court that appeals against a person."@en,
        "Personne contre laquelle un appel a été formé."@fr ;
    rdakit:toolkitLabel "appellee person of"@en,
        "personne intimée de"@fr ;
    reg:hasSubproperty <http://rdaregistry.info/Elements/a/datatype/P50085>,
        <http://rdaregistry.info/Elements/a/object/P50085> ;
    reg:hasUnconstrained <http://rdaregistry.info/Elements/u/P60601> ;
    reg:lexicalAlias <http://rdaregistry.info/Elements/a/appelleePersonOf.en> ;
    reg:name "appelleePersonOf"@en ;
    reg:status <http://metadataregistry.org/uri/RegStatus/1001> ;
    rdfs:domain <http://rdaregistry.info/Elements/c/C10004> ;
    rdfs:isDefinedBy <http://rdaregistry.info/Elements/a/> ;
    rdfs:subPropertyOf <http://rdaregistry.info/Elements/a/P50087> ;
    skos:definition "Relates a person against whom an appeal is taken on a decision of a lower court recorded in a legal work of a higher court to a work."@en,
        "Met une personne contre laquelle un appel a été formé en relation avec l’œuvre."@fr .

<http://rdaregistry.info/Elements/a/P50086> a rdf:Property ;
    rdfs:label "is medium of"@en,
        "est le médium de"@fr ;
    rdakit:instructionNumber "18.5" ;
    rdakit:toolkitDefinition "A work that involves a responsibility for a communication between the earthly world and a world of spirits."@en,
        "Personne tenue pour être un canal de communication entre le monde terrestre et le monde des esprits."@fr ;
    rdakit:toolkitLabel "medium of"@en,
        "médium de"@fr ;
    reg:hasSubproperty <http://rdaregistry.info/Elements/a/datatype/P50086>,
        <http://rdaregistry.info/Elements/a/object/P50086> ;
    reg:hasUnconstrained <http://rdaregistry.info/Elements/u/P60032> ;
    reg:lexicalAlias <http://rdaregistry.info/Elements/a/mediumOf.en> ;
    reg:name "mediumOf"@en ;
    reg:status <http://metadataregistry.org/uri/RegStatus/1001> ;
    rdfs:domain <http://rdaregistry.info/Elements/c/C10004> ;
    rdfs:isDefinedBy <http://rdaregistry.info/Elements/a/> ;
    rdfs:subPropertyOf <http://rdaregistry.info/Elements/a/P50131> ;
    skos:definition "Relates a person held to be a channel of communication between the earthly world and a world of spirits to a work."@en,
        "Met une personne tenue pour être un canal de communication entre le monde terrestre et le monde des esprits en relation avec l’œuvre."@fr .

<http://rdaregistry.info/Elements/a/P50091> a rdf:Property ;
    rdfs:label "is degree supervisor of"@en,
        "est le superviseur académique de"@fr ;
    rdakit:instructionNumber "18.5" ;
    rdakit:toolkitDefinition "A work that involves a responsibility as an advisor or supervisor of thesis or dissertation research, overseeing either an academic degree or thesis."@en,
        "Personne supervisant un diplôme universitaire de niveau supérieur."@fr ;
    rdakit:toolkitLabel "degree supervisor of"@en,
        "superviseur académique de"@fr ;
    reg:hasSubproperty <http://rdaregistry.info/Elements/a/datatype/P50091>,
        <http://rdaregistry.info/Elements/a/object/P50091> ;
    reg:hasUnconstrained <http://rdaregistry.info/Elements/u/P60649> ;
    reg:lexicalAlias <http://rdaregistry.info/Elements/a/degreeSupervisorOf.en> ;
    reg:name "degreeSupervisorOf"@en ;
    reg:status <http://metadataregistry.org/uri/RegStatus/1001> ;
    rdfs:domain <http://rdaregistry.info/Elements/c/C10004> ;
    rdfs:isDefinedBy <http://rdaregistry.info/Elements/a/> ;
    rdfs:subPropertyOf <http://rdaregistry.info/Elements/a/P50131> ;
    skos:definition "Relates a person, such as an advisor or supervisor of thesis or dissertation research, overseeing either an academic degree or thesis to a work."@en,
        "Met une personne supervisant un diplôme universitaire de niveau supérieur en relation avec l’œuvre."@fr .

<http://rdaregistry.info/Elements/a/P50092> a rdf:Property ;
    rdfs:label "is illuminator of"@en,
        "est l’enlumineur de"@fr ;
    rdakit:instructionNumber "18.5" ;
    rdakit:toolkitDefinition "An item decorated using precious metals or color, often with elaborate designs and motifs."@en,
        "Personne ornant un item spécifique en utilisant des métaux précieux ou de la couleur, souvent avec des dessins et des motifs élaborés."@fr ;
    rdakit:toolkitLabel "illuminator of"@en,
        "enlumineur de"@fr ;
    reg:hasSubproperty <http://rdaregistry.info/Elements/a/datatype/P50092>,
        <http://rdaregistry.info/Elements/a/object/P50092> ;
    reg:hasUnconstrained <http://rdaregistry.info/Elements/u/P60650> ;
    reg:lexicalAlias <http://rdaregistry.info/Elements/a/illuminatorOf.en> ;
    reg:name "illuminatorOf"@en ;
    reg:status <http://metadataregistry.org/uri/RegStatus/1001> ;
    rdfs:domain <http://rdaregistry.info/Elements/c/C10004> ;
    rdfs:isDefinedBy <http://rdaregistry.info/Elements/a/> ;
    rdfs:subPropertyOf <http://rdaregistry.info/Elements/a/P50182> ;
    skos:definition "Relates a person providing decoration to a specific item using precious metals or color, often with elaborate designs and motifs to an item."@en,
        "Met une personne ornant un item spécifique en utilisant des métaux précieux ou de la couleur, souvent avec des dessins et des motifs élaborés, en relation avec l’item."@fr .

<http://rdaregistry.info/Elements/a/P50098> a rdf:Property ;
    rdfs:label "has period of activity of person"@en,
        "a pour période d’activité de la personne"@fr,
        "har verksamhetstid för personen"@sv ;
    rdakit:instructionNumber "9.3.4" ;
    rdakit:toolkitDefinition "A date or range of dates indicative of the period in which a person was active in his or her primary field of endeavour."@en,
        "La fecha o rango de fechas que indica el período en el que una persona fue activa en su campo primario de desempeño."@es,
        "La date ou la fourchette de dates indicative de la période pendant laquelle une personne a été active dans son principal domaine d’activité."@fr ;
    rdakit:toolkitLabel "period of activity of person"@en,
        "período de actividad de la persona"@es,
        "période d’activité de la personne"@fr,
        "verksamhetstid för personen"@sv ;
    reg:hasSubproperty <http://rdaregistry.info/Elements/a/datatype/P50098> ;
    reg:hasUnconstrained <http://rdaregistry.info/Elements/u/P60076> ;
    reg:lexicalAlias <http://rdaregistry.info/Elements/a/periodOfActivityOfPerson.en> ;
    reg:name "periodOfActivityOfPerson"@en ;
    reg:status <http://metadataregistry.org/uri/RegStatus/1001> ;
    rdfs:domain <http://rdaregistry.info/Elements/c/C10004> ;
    rdfs:isDefinedBy <http://rdaregistry.info/Elements/a/> ;
    rdfs:subPropertyOf <http://rdaregistry.info/Elements/a/P50107> ;
    skos:definition "Relates a person to a date or range of dates indicative of the period in which a person was active in his or her primary field of endeavour."@en,
        "Met une personne en relation avec la date ou la fourchette de dates indicative de la période pendant laquelle une personne a été active dans son principal domaine d’activité."@fr .

<http://rdaregistry.info/Elements/a/P50103> a rdf:Property ;
    rdfs:label "has variant name for person"@en,
        "a pour variante de nom de la personne"@fr,
        "har variantnamn för personen"@sv ;
    rdakit:instructionNumber "9.2.3" ;
    rdakit:toolkitDefinition "A name or form of name by which a person is known that differs from a name or form of name chosen as a preferred name."@en,
        "Un nombre o forma del nombre mediante el cual se conoce una persona que difiere del nombre o forma del nombre elegido como el nombre preferido."@es,
        "Nom ou forme de nom sous laquelle une personne est connue et qui diffère du nom ou de la forme de nom choisie comme nom privilégié."@fr ;
    rdakit:toolkitLabel "variant name for person"@en,
        "variante del nombre de la persona"@es,
        "variante de nom de la personne"@fr,
        "variantnamn för personen"@sv ;
    reg:hasSubproperty <http://rdaregistry.info/Elements/a/datatype/P50103> ;
    reg:hasUnconstrained <http://rdaregistry.info/Elements/u/P60119> ;
    reg:lexicalAlias <http://rdaregistry.info/Elements/a/variantNameForPerson.en> ;
    reg:name "variantNameForPerson"@en ;
    reg:status <http://metadataregistry.org/uri/RegStatus/1001> ;
    rdfs:domain <http://rdaregistry.info/Elements/c/C10004> ;
    rdfs:isDefinedBy <http://rdaregistry.info/Elements/a/> ;
    rdfs:subPropertyOf <http://rdaregistry.info/Elements/a/P50111> ;
    skos:definition "Relates a person to a name or form of name by which a person is known that differs from a name or form of name chosen as a preferred name."@en,
        "Met une personne en relation avec un nom ou une forme de nom sous laquelle une personne est connue et qui diffère du nom ou de la forme de nom choisie comme nom privilégié."@fr ;
    skos:scopeNote "Variant name for person includes a name or form of name used by a person or found in reference sources, a name resulting from a different transliteration of a name, etc."@en .

<http://rdaregistry.info/Elements/a/P50117> a rdf:Property ;
    rdfs:label "has preferred name for person"@en,
        "a pour nom privilégié de la personne"@fr ;
    rdakit:instructionNumber "9.2.2" ;
    rdakit:toolkitDefinition "A name or form of name chosen to identify a person."@en,
        "El nombre o forma del nombre elegido para identificar la persona."@es,
        "Le nom ou la forme de nom choisie pour identifier la personne."@fr ;
    rdakit:toolkitLabel "preferred name for person"@en,
        "nombre preferido de la persona"@es,
        "nom privilégié de la personne"@fr ;
    reg:hasSubproperty <http://rdaregistry.info/Elements/a/datatype/P50117> ;
    reg:hasUnconstrained <http://rdaregistry.info/Elements/u/P60549> ;
    reg:lexicalAlias <http://rdaregistry.info/Elements/a/preferredNameForPerson.en> ;
    reg:name "preferredNameForPerson"@en ;
    reg:status <http://metadataregistry.org/uri/RegStatus/1001> ;
    rdfs:domain <http://rdaregistry.info/Elements/c/C10004> ;
    rdfs:isDefinedBy <http://rdaregistry.info/Elements/a/> ;
    rdfs:subPropertyOf <http://rdaregistry.info/Elements/a/P50111> ;
    skos:definition "Relates a person to a name or form of name chosen to identify a person."@en,
        "Met une personne en relation avec le nom ou la forme de nom choisie pour identifier la personne."@fr .

<http://rdaregistry.info/Elements/a/P50120> a rdf:Property ;
    rdfs:label "has date of death"@en,
        "a pour date de décès"@fr,
        "har dödstid"@sv ;
    rdakit:instructionNumber "9.3.3" ;
    rdakit:toolkitDefinition "A year a person died."@en,
        "El año en que murió la persona."@es,
        "L’année de mort d’une personne."@fr ;
    rdakit:toolkitLabel "date of death"@en,
        "fecha de fallecimiento"@es,
        "date de décès"@fr,
        "dödstid"@sv ;
    reg:hasSubproperty <http://rdaregistry.info/Elements/a/datatype/P50120> ;
    reg:hasUnconstrained <http://rdaregistry.info/Elements/u/P60598> ;
    reg:lexicalAlias <http://rdaregistry.info/Elements/a/dateOfDeath.en> ;
    reg:name "dateOfDeath"@en ;
    reg:status <http://metadataregistry.org/uri/RegStatus/1001> ;
    rdfs:domain <http://rdaregistry.info/Elements/c/C10004> ;
    rdfs:isDefinedBy <http://rdaregistry.info/Elements/a/> ;
    rdfs:subPropertyOf <http://rdaregistry.info/Elements/a/P50107> ;
    skos:definition "Relates a person to a year a person died."@en,
        "Met une personne en relation avec l’année de mort d’une personne."@fr ;
    skos:scopeNote "Date of death may also include the month or month and day of the person's death."@en,
        "La date de décès peut aussi inclure le mois et le jour de la mort de la personne."@fr .

<http://rdaregistry.info/Elements/a/P50121> a rdf:Property ;
    rdfs:label "has date of birth"@en,
        "a pour date de naissance"@fr,
        "has date of birth"@sv ;
    rdakit:instructionNumber "9.3.2" ;
    rdakit:toolkitDefinition "A year a person was born."@en,
        "El año en que nació la persona."@es,
        "L’année de naissance d’une personne."@fr ;
    rdakit:toolkitLabel "date of birth"@en,
        "fecha de nacimiento"@es,
        "date de naissance"@fr,
        "födelsetid"@sv ;
    reg:hasSubproperty <http://rdaregistry.info/Elements/a/datatype/P50121> ;
    reg:hasUnconstrained <http://rdaregistry.info/Elements/u/P60599> ;
    reg:lexicalAlias <http://rdaregistry.info/Elements/a/dateOfBirth.en> ;
    reg:name "dateOfBirth"@en ;
    reg:status <http://metadataregistry.org/uri/RegStatus/1001> ;
    rdfs:domain <http://rdaregistry.info/Elements/c/C10004> ;
    rdfs:isDefinedBy <http://rdaregistry.info/Elements/a/> ;
    rdfs:subPropertyOf <http://rdaregistry.info/Elements/a/P50107> ;
    skos:definition "Relates a person to a year a person was born."@en,
        "Met une personne en relation avec l’année de naissance d’une personne."@fr ;
    skos:scopeNote "Date of birth may also include the month or month and day of the person's birth."@en,
        "La date de naissance peut aussi inclure le mois et le jour de naissance de la personne."@fr .

<http://rdaregistry.info/Elements/a/P50123> a rdf:Property ;
    rdfs:label "is binder of"@en,
        "est le relieur de"@fr ;
    rdakit:instructionNumber "18.5" ;
    rdakit:toolkitDefinition "An item that is bound."@en,
        "Personne qui relie un item."@fr ;
    rdakit:toolkitLabel "binder of"@en,
        "relieur de"@fr ;
    reg:hasSubproperty <http://rdaregistry.info/Elements/a/datatype/P50123>,
        <http://rdaregistry.info/Elements/a/object/P50123> ;
    reg:hasUnconstrained <http://rdaregistry.info/Elements/u/P60692> ;
    reg:lexicalAlias <http://rdaregistry.info/Elements/a/binderOf.en> ;
    reg:name "binderOf"@en ;
    reg:status <http://metadataregistry.org/uri/RegStatus/1001> ;
    rdfs:domain <http://rdaregistry.info/Elements/c/C10004> ;
    rdfs:isDefinedBy <http://rdaregistry.info/Elements/a/> ;
    rdfs:subPropertyOf <http://rdaregistry.info/Elements/a/P50182> ;
    skos:definition "Relates a person who binds an item to an item."@en,
        "Met une personne qui relie un item en relation avec l’item."@fr .

<http://rdaregistry.info/Elements/a/P50124> a rdf:Property ;
    rdfs:label "is plaintiff person of"@en,
        "est la personne demanderesse de"@fr ;
    rdakit:instructionNumber "18.5" ;
    rdakit:toolkitDefinition "A work that involves a responsibility for bringing a suit in a civil proceeding by a person."@en,
        "Personne qui intente une poursuite civile."@fr ;
    rdakit:toolkitLabel "plaintiff person of"@en,
        "personne demanderesse de"@fr ;
    reg:hasSubproperty <http://rdaregistry.info/Elements/a/datatype/P50124>,
        <http://rdaregistry.info/Elements/a/object/P50124> ;
    reg:hasUnconstrained <http://rdaregistry.info/Elements/u/P60693> ;
    reg:lexicalAlias <http://rdaregistry.info/Elements/a/plaintiffPersonOf.en> ;
    reg:name "plaintiffPersonOf"@en ;
    reg:status <http://metadataregistry.org/uri/RegStatus/1001> ;
    rdfs:domain <http://rdaregistry.info/Elements/c/C10004> ;
    rdfs:isDefinedBy <http://rdaregistry.info/Elements/a/> ;
    rdfs:subPropertyOf <http://rdaregistry.info/Elements/a/P50089> ;
    skos:definition "Relates a person who brings a suit in a civil proceeding to a work."@en,
        "Met une personne qui intente une poursuite civile en relation avec l’œuvre."@fr .

<http://rdaregistry.info/Elements/a/P50125> a rdf:Property ;
    rdfs:label "is inscriber of"@en,
        "est le dédicateur (item) de"@fr ;
    rdakit:instructionNumber "18.5" ;
    rdakit:toolkitDefinition "An item with a statement of dedication or gift written on it."@en,
        "Personne qui a écrit une dédicace ou une mention de don sur un item."@fr ;
    rdakit:toolkitLabel "inscriber of"@en,
        "dédicateur (item) de"@fr ;
    reg:hasSubproperty <http://rdaregistry.info/Elements/a/datatype/P50125>,
        <http://rdaregistry.info/Elements/a/object/P50125> ;
    reg:hasUnconstrained <http://rdaregistry.info/Elements/u/P60695> ;
    reg:lexicalAlias <http://rdaregistry.info/Elements/a/inscriberOf.en> ;
    reg:name "inscriberOf"@en ;
    reg:status <http://metadataregistry.org/uri/RegStatus/1001> ;
    rdfs:domain <http://rdaregistry.info/Elements/c/C10004> ;
    rdfs:isDefinedBy <http://rdaregistry.info/Elements/a/> ;
    rdfs:subPropertyOf <http://rdaregistry.info/Elements/a/P50182> ;
    skos:definition "Relates a person who has written a statement of dedication or gift on an item to an item."@en,
        "Met une personne qui a écrit une dédicace ou une mention de don sur un item en relation avec l’item."@fr .

<http://rdaregistry.info/Elements/a/P50126> a rdf:Property ;
    rdfs:label "is judge of"@en,
        "est le juge de"@fr ;
    rdakit:instructionNumber "18.5" ;
    rdakit:toolkitDefinition "A work that involves a responsibility for hearing and decision on legal matters in court."@en,
        "Personne qui entend des causes juridiques et rend jugement dans un tribunal."@fr ;
    rdakit:toolkitLabel "judge of"@en,
        "juge de"@fr ;
    reg:hasSubproperty <http://rdaregistry.info/Elements/a/datatype/P50126>,
        <http://rdaregistry.info/Elements/a/object/P50126> ;
    reg:hasUnconstrained <http://rdaregistry.info/Elements/u/P60696> ;
    reg:lexicalAlias <http://rdaregistry.info/Elements/a/judgeOf.en> ;
    reg:name "judgeOf"@en ;
    reg:status <http://metadataregistry.org/uri/RegStatus/1001> ;
    rdfs:domain <http://rdaregistry.info/Elements/c/C10004> ;
    rdfs:isDefinedBy <http://rdaregistry.info/Elements/a/> ;
    rdfs:subPropertyOf <http://rdaregistry.info/Elements/a/P50131> ;
    skos:definition "Relates a person who hears and decides on legal matters in court to a work."@en,
        "Met une personne qui entend des causes juridiques et rend jugement dans un tribunal en relation avec l’œuvre."@fr .

<http://rdaregistry.info/Elements/a/P50127> a rdf:Property ;
    rdfs:label "is praeses of"@en,
        "est le praeses de"@fr ;
    rdakit:instructionNumber "18.5" ;
    rdakit:toolkitDefinition "A work that involves a responsibility as a faculty moderator of an academic disputation, normally proposing a thesis and participating in the ensuing disputation."@en,
        "Personne qui est le président d’une soutenance de thèse, proposant normalement la thèse et participant au débat qui s’ensuit."@fr ;
    rdakit:toolkitLabel "praeses of"@en,
        "praeses de"@fr ;
    reg:hasSubproperty <http://rdaregistry.info/Elements/a/datatype/P50127>,
        <http://rdaregistry.info/Elements/a/object/P50127> ;
    reg:hasUnconstrained <http://rdaregistry.info/Elements/u/P60699> ;
    reg:lexicalAlias <http://rdaregistry.info/Elements/a/praesesOf.en> ;
    reg:name "praesesOf"@en ;
    reg:status <http://metadataregistry.org/uri/RegStatus/1001> ;
    rdfs:domain <http://rdaregistry.info/Elements/c/C10004> ;
    rdfs:isDefinedBy <http://rdaregistry.info/Elements/a/> ;
    rdfs:subPropertyOf <http://rdaregistry.info/Elements/a/P50204> ;
    skos:definition "Relates a person who is a faculty moderator of an academic disputation, normally proposing a thesis and participating in the ensuing disputation to a work."@en,
        "Met une personne qui est le président d’une soutenance de thèse, proposant normalement la thèse et participant au débat qui s’ensuit en relation avec l’œuvre."@fr .

<http://rdaregistry.info/Elements/a/P50128> a rdf:Property ;
    rdfs:label "is annotator of"@en,
        "est l’annotateur de"@fr ;
    rdakit:instructionNumber "18.5" ;
    rdakit:toolkitDefinition "An item with manuscript annotations."@en,
        "Personne qui rédige des annotations manuscrites sur un item."@fr ;
    rdakit:toolkitLabel "annotator of"@en,
        "annotateur de"@fr ;
    reg:hasSubproperty <http://rdaregistry.info/Elements/a/datatype/P50128>,
        <http://rdaregistry.info/Elements/a/object/P50128> ;
    reg:hasUnconstrained <http://rdaregistry.info/Elements/u/P60700> ;
    reg:lexicalAlias <http://rdaregistry.info/Elements/a/annotatorOf.en> ;
    reg:name "annotatorOf"@en ;
    reg:status <http://metadataregistry.org/uri/RegStatus/1001> ;
    rdfs:domain <http://rdaregistry.info/Elements/c/C10004> ;
    rdfs:isDefinedBy <http://rdaregistry.info/Elements/a/> ;
    rdfs:subPropertyOf <http://rdaregistry.info/Elements/a/P50182> ;
    skos:definition "Relates a person who makes manuscript annotations on an item to an item."@en,
        "Met une personne qui rédige des annotations manuscrites sur un item en relation avec l’item."@fr .

<http://rdaregistry.info/Elements/a/P50129> a rdf:Property ;
    rdfs:label "is autographer of"@en,
        "est le signataire autographe de"@fr ;
    rdakit:instructionNumber "18.5" ;
    rdakit:toolkitDefinition "An item with a manuscript signature appearing on it."@en,
        "Personne dont la signature manuscrite figure sur un item."@fr ;
    rdakit:toolkitLabel "autographer of"@en,
        "signataire autographe de"@fr ;
    reg:hasSubproperty <http://rdaregistry.info/Elements/a/datatype/P50129>,
        <http://rdaregistry.info/Elements/a/object/P50129> ;
    reg:hasUnconstrained <http://rdaregistry.info/Elements/u/P60702> ;
    reg:lexicalAlias <http://rdaregistry.info/Elements/a/autographerOf.en> ;
    reg:name "autographerOf"@en ;
    reg:status <http://metadataregistry.org/uri/RegStatus/1001> ;
    rdfs:domain <http://rdaregistry.info/Elements/c/C10004> ;
    rdfs:isDefinedBy <http://rdaregistry.info/Elements/a/> ;
    rdfs:subPropertyOf <http://rdaregistry.info/Elements/a/P50182> ;
    skos:definition "Relates a person whose manuscript signature appears on an item to an item."@en,
        "Met une personne dont la signature manuscrite figure sur un item en relation avec l’item."@fr .

<http://rdaregistry.info/Elements/a/P50130> a rdf:Property ;
    rdfs:label "is issuing body of"@en,
        "est l’organisme de publication de"@fr ;
    rdakit:instructionNumber "18.5" ;
    rdakit:toolkitDefinition "A work that involves a responsibility for issuing a work, such as an official organ of the body."@en,
        "Personne, famille ou collectivité publiant une œuvre, tel un organe officiel de l’organisme."@fr ;
    rdakit:toolkitLabel "issuing body of"@en,
        "organisme de publication de"@fr ;
    reg:hasSubproperty <http://rdaregistry.info/Elements/a/datatype/P50130>,
        <http://rdaregistry.info/Elements/a/object/P50130> ;
    reg:hasUnconstrained <http://rdaregistry.info/Elements/u/P60703> ;
    reg:lexicalAlias <http://rdaregistry.info/Elements/a/issuingBodyOf.en> ;
    reg:name "issuingBodyOf"@en ;
    reg:status <http://metadataregistry.org/uri/RegStatus/1001> ;
    rdfs:domain <http://rdaregistry.info/Elements/c/C10002> ;
    rdfs:isDefinedBy <http://rdaregistry.info/Elements/a/> ;
    rdfs:subPropertyOf <http://rdaregistry.info/Elements/a/P50131> ;
    skos:definition "Relates an agent issuing a work, such as an official organ of the body to a work."@en,
        "Met une personne, famille ou collectivité publiant une œuvre, tel un organe officiel de l’organisme, en relation avec l’œuvre."@fr .

<http://rdaregistry.info/Elements/a/P50132> a rdf:Property ;
    rdfs:label "is dedicator of"@en,
        "est le dédicateur de"@fr ;
    rdakit:instructionNumber "18.5" ;
    rdakit:toolkitDefinition "A work that is dedicated to an agent."@en,
        "Personne, famille ou collectivité par qui une œuvre est dédiée."@fr ;
    rdakit:toolkitLabel "dedicator of"@en,
        "dédicateur de"@fr ;
    reg:hasSubproperty <http://rdaregistry.info/Elements/a/datatype/P50132>,
        <http://rdaregistry.info/Elements/a/object/P50132> ;
    reg:hasUnconstrained <http://rdaregistry.info/Elements/u/P60603> ;
    reg:lexicalAlias <http://rdaregistry.info/Elements/a/dedicatorOf.en> ;
    reg:name "dedicatorOf"@en ;
    reg:status <http://metadataregistry.org/uri/RegStatus/1001> ;
    rdfs:domain <http://rdaregistry.info/Elements/c/C10002> ;
    rdfs:isDefinedBy <http://rdaregistry.info/Elements/a/> ;
    rdfs:subPropertyOf <http://rdaregistry.info/Elements/a/P50131> ;
    skos:definition "Relates an agent by whom a work is dedicated to a work."@en,
        "Met une personne, famille ou collectivité par qui une œuvre est dédiée en relation avec l’œuvre."@fr .

<http://rdaregistry.info/Elements/a/P50134> a rdf:Property ;
    rdfs:label "is composer (expression) of"@en,
        "est le compositeur (expression) de"@fr ;
    rdakit:instructionNumber "18.5" ;
    rdakit:toolkitDefinition "An expression that incorporates a contribution of adding music to a work that originally lacked it, by composing new music to substitute for original music, or by composing new music to supplement existing music."@en,
        "Personne, famille ou collectivité contribuant à une expression en ajoutant de la musique à une œuvre qui n’en avait pas à l’origine, en composant une nouvelle musique pour remplacer la musique originale ou en composant une nouvelle musique pour compléter la musique existante."@fr ;
    rdakit:toolkitLabel "composer (expression) of"@en,
        "compositeur (expression) de"@fr ;
    reg:hasSubproperty <http://rdaregistry.info/Elements/a/datatype/P50134>,
        <http://rdaregistry.info/Elements/a/object/P50134> ;
    reg:hasUnconstrained <http://rdaregistry.info/Elements/u/P60655> ;
    reg:lexicalAlias <http://rdaregistry.info/Elements/a/composerExpressionOf.en> ;
    reg:name "composerExpressionOf"@en ;
    reg:status <http://metadataregistry.org/uri/RegStatus/1001> ;
    rdfs:domain <http://rdaregistry.info/Elements/c/C10002> ;
    rdfs:isDefinedBy <http://rdaregistry.info/Elements/a/> ;
    rdfs:subPropertyOf <http://rdaregistry.info/Elements/a/P50161> ;
    skos:definition "Relates an agent contributing to an expression by adding music to a work that originally lacked it, by composing new music to substitute for the original music, or by composing new music to supplement the existing music, to an expression."@en,
        "Met une personne, famille ou collectivité contribuant à une expression en ajoutant de la musique à une œuvre qui n’en avait pas à l’origine, en composant une nouvelle musique pour remplacer la musique originale ou en composant une nouvelle musique pour compléter la musique existante en relation avec l’expression."@fr .

<http://rdaregistry.info/Elements/a/P50135> a rdf:Property ;
    rdfs:label "is surveyor of"@en,
        "est l’arpenteur de"@fr ;
    rdakit:instructionNumber "18.5" ;
    rdakit:toolkitDefinition "An expression of a cartographic work that incorporates a contribution of providing measurements or dimensional relationships for a geographic area represented."@en,
        "Personne, famille ou collectivité contribuant à une expression d’une œuvre cartographique en fournissant les mesures ou les relations dimensionnelles pour l’aire géographique représentée."@fr ;
    rdakit:toolkitLabel "surveyor of"@en,
        "arpenteur de"@fr ;
    reg:hasSubproperty <http://rdaregistry.info/Elements/a/datatype/P50135>,
        <http://rdaregistry.info/Elements/a/object/P50135> ;
    reg:hasUnconstrained <http://rdaregistry.info/Elements/u/P60605> ;
    reg:lexicalAlias <http://rdaregistry.info/Elements/a/surveyorOf.en> ;
    reg:name "surveyorOf"@en ;
    reg:status <http://metadataregistry.org/uri/RegStatus/1001> ;
    rdfs:domain <http://rdaregistry.info/Elements/c/C10002> ;
    rdfs:isDefinedBy <http://rdaregistry.info/Elements/a/> ;
    rdfs:subPropertyOf <http://rdaregistry.info/Elements/a/P50161> ;
    skos:definition "Relates an agent contributing to an expression of a cartographic work by providing measurements or dimensional relationships for a geographic area represented to an expression."@en,
        "Met une personne, famille ou collectivité contribuant à une expression d’une œuvre cartographique en fournissant les mesures ou les relations dimensionnelles pour l’aire géographique représentée en relation avec l’expression."@fr .

<http://rdaregistry.info/Elements/a/P50136> a rdf:Property ;
    rdfs:label "is animator of"@en,
        "est l’animateur de"@fr ;
    rdakit:instructionNumber "18.5" ;
    rdakit:seeAlso <http://rdaregistry.info/Elements/a/P50192> ;
    rdakit:toolkitDefinition "An expression of a moving image work or computer program that incorporates a contribution of giving apparent movement to inanimate objects or drawings."@en,
        "Personne, famille ou collectivité contribuant à une expression d’une œuvre d’images animées ou d’un programme informatique en donnant l’illusion du mouvement à des objets inanimés ou à des dessins."@fr ;
    rdakit:toolkitLabel "animator of"@en,
        "animateur de"@fr ;
    reg:hasSubproperty <http://rdaregistry.info/Elements/a/datatype/P50136>,
        <http://rdaregistry.info/Elements/a/object/P50136> ;
    reg:hasUnconstrained <http://rdaregistry.info/Elements/u/P60606> ;
    reg:lexicalAlias <http://rdaregistry.info/Elements/a/animatorOf.en> ;
    reg:name "animatorOf"@en ;
    reg:status <http://metadataregistry.org/uri/RegStatus/1001> ;
    rdfs:domain <http://rdaregistry.info/Elements/c/C10002> ;
    rdfs:isDefinedBy <http://rdaregistry.info/Elements/a/> ;
    rdfs:subPropertyOf <http://rdaregistry.info/Elements/a/P50161> ;
    skos:definition "Relates an agent contributing to an expression of a moving image work or computer program by giving apparent movement to inanimate objects or drawings to an expression."@en,
        "Met une personne, famille ou collectivité contribuant à une expression d’une œuvre d’images animées ou d’un programme informatique en donnant l’illusion du mouvement à des objets inanimés ou à des dessins en relation avec l’expression."@fr .

<http://rdaregistry.info/Elements/a/P50139> a rdf:Property ;
    rdfs:label "is stage director of"@en,
        "est le metteur en scène de"@fr ;
    rdakit:instructionNumber "18.5" ;
    rdakit:toolkitDefinition "An expression of a stage work that incorporates a contribution of the general management and supervision of a performance."@en,
        "Personne, famille ou collectivité contribuant à une expression d’une œuvre scénique par la gestion et la supervision générales d’une prestation."@fr ;
    rdakit:toolkitLabel "stage director of"@en,
        "metteur en scène de"@fr ;
    reg:hasSubproperty <http://rdaregistry.info/Elements/a/datatype/P50139>,
        <http://rdaregistry.info/Elements/a/object/P50139> ;
    reg:hasUnconstrained <http://rdaregistry.info/Elements/u/P60627> ;
    reg:lexicalAlias <http://rdaregistry.info/Elements/a/stageDirectorOf.en> ;
    reg:name "stageDirectorOf"@en ;
    reg:status <http://metadataregistry.org/uri/RegStatus/1001> ;
    rdfs:domain <http://rdaregistry.info/Elements/c/C10002> ;
    rdfs:isDefinedBy <http://rdaregistry.info/Elements/a/> ;
    rdfs:subPropertyOf <http://rdaregistry.info/Elements/a/P50161> ;
    skos:definition "Relates an agent contributing to an expression of a stage work through the general management and supervision of a performance to an expression."@en,
        "Met une personne, famille ou collectivité contribuant à une expression d’une œuvre scénique par la gestion et la supervision générales d’une prestation en relation avec l’expression."@fr .

<http://rdaregistry.info/Elements/a/P50140> a rdf:Property ;
    rdfs:label "is interviewer (expression) of"@en,
        "est l’intervieweur (expression) de"@fr ;
    rdakit:instructionNumber "18.5" ;
    rdakit:toolkitDefinition "An expression of a work that incorporates a contribution of acting as an interviewer, reporter, pollster, or some other information gathering agent."@en,
        "Personne, famille ou collectivité contribuant à une expression d’une œuvre en agissant à titre d’intervieweur, de journaliste, de sondeur ou d’autre agent recueillant de l’information."@fr ;
    rdakit:toolkitLabel "interviewer (expression) of"@en,
        "intervieweur (expression) de"@fr ;
    reg:hasSubproperty <http://rdaregistry.info/Elements/a/datatype/P50140>,
        <http://rdaregistry.info/Elements/a/object/P50140> ;
    reg:hasUnconstrained <http://rdaregistry.info/Elements/u/P60659> ;
    reg:lexicalAlias <http://rdaregistry.info/Elements/a/interviewerExpressionOf.en> ;
    reg:name "interviewerExpressionOf"@en ;
    reg:status <http://metadataregistry.org/uri/RegStatus/1001> ;
    rdfs:domain <http://rdaregistry.info/Elements/c/C10002> ;
    rdfs:isDefinedBy <http://rdaregistry.info/Elements/a/> ;
    rdfs:subPropertyOf <http://rdaregistry.info/Elements/a/P50161> ;
    skos:definition "Relates an agent contributing to an expression of a work by acting as an interviewer, reporter, pollster, or some other information gathering agent to an expression."@en,
        "Met une personne, famille ou collectivité contribuant à une expression d’une œuvre en agissant à titre d’intervieweur, de journaliste, de sondeur ou d’autre agent recueillant de l’information en relation avec l’expression."@fr .

<http://rdaregistry.info/Elements/a/P50141> a rdf:Property ;
    rdfs:label "is draftsman of"@en,
        "est le dessinateur industriel de"@fr ;
    rdakit:instructionNumber "18.5" ;
    rdakit:toolkitDefinition "An expression of a work by an architect, inventor, etc., that incorporates a contribution of making detailed plans or drawings for buildings, ships, aircraft, machines, objects, etc."@en,
        "Personne, famille ou collectivité contribuant à une expression d’une œuvre par un architecte, un inventeur, etc. en effectuant des plans ou des dessins détaillés pour des bâtiments, des navires, des avions, des machines, des objets, etc."@fr ;
    rdakit:toolkitLabel "draftsman of"@en,
        "dessinateur industriel de"@fr ;
    reg:hasSubproperty <http://rdaregistry.info/Elements/a/datatype/P50141>,
        <http://rdaregistry.info/Elements/a/object/P50141> ;
    reg:hasUnconstrained <http://rdaregistry.info/Elements/u/P60609> ;
    reg:lexicalAlias <http://rdaregistry.info/Elements/a/draftsmanOf.en> ;
    reg:name "draftsmanOf"@en ;
    reg:status <http://metadataregistry.org/uri/RegStatus/1001> ;
    rdfs:domain <http://rdaregistry.info/Elements/c/C10002> ;
    rdfs:isDefinedBy <http://rdaregistry.info/Elements/a/> ;
    rdfs:subPropertyOf <http://rdaregistry.info/Elements/a/P50161> ;
    skos:definition "Relates an agent contributing to an expression of a work by an architect, inventor, etc., by making detailed plans or drawings for buildings, ships, aircraft, machines, objects, etc. to an expression."@en,
        "Met une personne, famille ou collectivité contribuant à une expression d’une œuvre par un architecte, un inventeur, etc. en effectuant des plans ou des dessins détaillés pour des bâtiments, des navires, des avions, des machines, des objets, etc. en relation avec l’expression."@fr .

<http://rdaregistry.info/Elements/a/P50142> a rdf:Property ;
    rdfs:label "is transcriber of"@en,
        "est le transcripteur de"@fr ;
    rdakit:instructionNumber "18.5" ;
    rdakit:seeAlso <http://rdaregistry.info/Elements/a/P50137> ;
    rdakit:toolkitDefinition "An expression of a work that incorporates a contribution of writing down or notating previously unwritten or unnotated content, or by changing it from one system of notation to another."@en,
        "Personne, famille ou collectivité contribuant à une expression d’une œuvre en écrivant ou en notant un contenu auparavant non écrit ou non noté, ou bien en le transposant d’un système de notation à un autre."@fr ;
    rdakit:toolkitLabel "transcriber of"@en,
        "transcripteur de"@fr ;
    reg:hasSubproperty <http://rdaregistry.info/Elements/a/datatype/P50142>,
        <http://rdaregistry.info/Elements/a/object/P50142> ;
    reg:hasUnconstrained <http://rdaregistry.info/Elements/u/P60610> ;
    reg:lexicalAlias <http://rdaregistry.info/Elements/a/transcriberOf.en> ;
    reg:name "transcriberOf"@en ;
    reg:status <http://metadataregistry.org/uri/RegStatus/1001> ;
    rdfs:domain <http://rdaregistry.info/Elements/c/C10002> ;
    rdfs:isDefinedBy <http://rdaregistry.info/Elements/a/> ;
    rdfs:subPropertyOf <http://rdaregistry.info/Elements/a/P50161> ;
    skos:definition "Relates an agent contributing to an expression of a work by writing down or notating previously unwritten or unnotated content, or by changing it from one system of notation to another to an expression."@en,
        "Met une personne, famille ou collectivité contribuant à une expression d’une œuvre en écrivant ou en notant un contenu auparavant non écrit ou non noté, ou bien en le transposant d’un système de notation à un autre en relation avec l’expression."@fr .

<http://rdaregistry.info/Elements/a/P50143> a rdf:Property ;
    rdfs:label "is musical director of"@en,
        "est le directeur musical de"@fr ;
    rdakit:instructionNumber "18.5" ;
    rdakit:toolkitDefinition "An expression of a work that incorporates a contribution of coordinating the activities of composers, sound editors, and sound mixers for a moving image production or for a musical or dramatic presentation or entertainment."@en,
        "Personne, famille ou collectivité contribuant à une expression d’une œuvre en coordonnant les activités du compositeur, du monteur son et des mixeurs de son pour une production d’images animées ou bien pour une représentation ou un spectacle dramatique ou musical."@fr ;
    rdakit:toolkitLabel "musical director of"@en,
        "directeur musical de"@fr ;
    reg:hasSubproperty <http://rdaregistry.info/Elements/a/datatype/P50143>,
        <http://rdaregistry.info/Elements/a/object/P50143> ;
    reg:hasUnconstrained <http://rdaregistry.info/Elements/u/P60611> ;
    reg:lexicalAlias <http://rdaregistry.info/Elements/a/musicalDirectorOf.en> ;
    reg:name "musicalDirectorOf"@en ;
    reg:status <http://metadataregistry.org/uri/RegStatus/1001> ;
    rdfs:domain <http://rdaregistry.info/Elements/c/C10002> ;
    rdfs:isDefinedBy <http://rdaregistry.info/Elements/a/> ;
    rdfs:subPropertyOf <http://rdaregistry.info/Elements/a/P50161> ;
    skos:definition "Relates an agent contributing to an expression of a work by coordinating the activities of composers, sound editors, and sound mixers for a moving image production or for a musical or dramatic presentation or entertainment to an expression."@en,
        "Met une personne, famille ou collectivité contribuant à une expression d’une œuvre en coordonnant les activités du compositeur, du monteur son et des mixeurs de son pour une production d’images animées ou bien pour une représentation ou un spectacle dramatique ou musical en relation avec l’expression."@fr .

<http://rdaregistry.info/Elements/a/P50144> a rdf:Property ;
    rdfs:label "is costume designer of"@en,
        "est le créateur de costumes de"@fr ;
    rdakit:instructionNumber "18.5" ;
    rdakit:toolkitDefinition "An expression of a work that incorporates a contribution of designing costumes for a moving image production or for a musical or dramatic presentation or entertainment."@en,
        "Personne, famille ou collectivité contribuant à une expression d’une œuvre en créant les costumes pour une production d’images animées ou bien pour une représentation ou un spectacle musical ou dramatique."@fr ;
    rdakit:toolkitLabel "costume designer of"@en,
        "créateur de costumes de"@fr ;
    reg:hasSubproperty <http://rdaregistry.info/Elements/a/datatype/P50144>,
        <http://rdaregistry.info/Elements/a/object/P50144> ;
    reg:hasUnconstrained <http://rdaregistry.info/Elements/u/P60612> ;
    reg:lexicalAlias <http://rdaregistry.info/Elements/a/costumeDesignerOf.en> ;
    reg:name "costumeDesignerOf"@en ;
    reg:status <http://metadataregistry.org/uri/RegStatus/1001> ;
    rdfs:domain <http://rdaregistry.info/Elements/c/C10002> ;
    rdfs:isDefinedBy <http://rdaregistry.info/Elements/a/> ;
    rdfs:subPropertyOf <http://rdaregistry.info/Elements/a/P50161> ;
    skos:definition "Relates an agent contributing to an expression of a work by designing costumes for a moving image production or for a musical or dramatic presentation or entertainment to an expression."@en,
        "Met une personne, famille ou collectivité contribuant à une expression d’une œuvre en créant les costumes pour une production d’images animées ou bien pour une représentation ou un spectacle musical ou dramatique en relation avec l’expression."@fr .

<http://rdaregistry.info/Elements/a/P50145> a rdf:Property ;
    rdfs:label "is translator of"@en,
        "est le traducteur de"@fr ;
    rdakit:instructionNumber "18.5" ;
    rdakit:toolkitDefinition "An expression of a work that incorporates a contribution of expressing the linguistic content of the work in a language different from that of previous expressions of an original work."@en,
        "Personne, famille ou collectivité contribuant à une expression d’une œuvre en exprimant le texte original de l’œuvre dans une langue différente de celle de l’œuvre originale."@fr ;
    rdakit:toolkitLabel "translator of"@en,
        "traducteur de"@fr ;
    reg:hasSubproperty <http://rdaregistry.info/Elements/a/datatype/P50145>,
        <http://rdaregistry.info/Elements/a/object/P50145> ;
    reg:hasUnconstrained <http://rdaregistry.info/Elements/u/P60613> ;
    reg:lexicalAlias <http://rdaregistry.info/Elements/a/translatorOf.en> ;
    reg:name "translatorOf"@en ;
    reg:status <http://metadataregistry.org/uri/RegStatus/1001> ;
    rdfs:domain <http://rdaregistry.info/Elements/c/C10002> ;
    rdfs:isDefinedBy <http://rdaregistry.info/Elements/a/> ;
    rdfs:subPropertyOf <http://rdaregistry.info/Elements/a/P50161> ;
    skos:definition "Relates an agent contributing to an expression of a work by expressing the linguistic content of the work in a language different from that of previous expressions of an original work to an expression."@en,
        "Met une personne, famille ou collectivité contribuant à une expression d’une œuvre en exprimant le texte original de l’œuvre dans une langue différente de celle de l’œuvre originale en relation avec l’expression."@fr ;
    skos:scopeNote "A translator may also translate linguistic content between forms of the same language from different time periods."@en,
        "Un traducteur peut aussi traduire un texte depuis une forme ancienne d’une langue vers la forme moderne."@fr .

<http://rdaregistry.info/Elements/a/P50146> a rdf:Property ;
    rdfs:label "is art director of"@en,
        "est le directeur artistique de"@fr ;
    rdakit:instructionNumber "18.5" ;
    rdakit:toolkitDefinition "An expression of a work that incorporates a contribution of overseeing artists and craftspeople who build sets for moving image productions."@en,
        "Personne, famille ou collectivité contribuant à une expression d’une œuvre en supervisant les artistes et les artisans qui construisent les décors pour des productions d’images animées."@fr ;
    rdakit:toolkitLabel "art director of"@en,
        "directeur artistique de"@fr ;
    reg:hasSubproperty <http://rdaregistry.info/Elements/a/datatype/P50146>,
        <http://rdaregistry.info/Elements/a/object/P50146> ;
    reg:hasUnconstrained <http://rdaregistry.info/Elements/u/P60614> ;
    reg:lexicalAlias <http://rdaregistry.info/Elements/a/artDirectorOf.en> ;
    reg:name "artDirectorOf"@en ;
    reg:status <http://metadataregistry.org/uri/RegStatus/1001> ;
    rdfs:domain <http://rdaregistry.info/Elements/c/C10002> ;
    rdfs:isDefinedBy <http://rdaregistry.info/Elements/a/> ;
    rdfs:subPropertyOf <http://rdaregistry.info/Elements/a/P50161> ;
    skos:definition "Relates an agent contributing to an expression of a work by overseeing artists and craftspeople who build sets for moving image productions to an expression."@en,
        "Met une personne, famille ou collectivité contribuant à une expression d’une œuvre en supervisant les artistes et les artisans qui construisent les décors pour des productions d’images animées en relation avec l’expression."@fr .

<http://rdaregistry.info/Elements/a/P50149> a rdf:Property ;
    rdfs:label "is writer of preface of"@en,
        "est le préfacier de"@fr ;
    rdakit:instructionNumber "18.5" ;
    rdakit:toolkitDefinition "An expression of a work that incorporates a contribution of providing a preface to an original work."@en,
        "Personne, famille ou collectivité contribuant à une expression d’une œuvre en fournissant une préface à l’œuvre originale."@fr ;
    rdakit:toolkitLabel "writer of preface of"@en,
        "préfacier de"@fr ;
    reg:hasSubproperty <http://rdaregistry.info/Elements/a/datatype/P50149>,
        <http://rdaregistry.info/Elements/a/object/P50149> ;
    reg:hasUnconstrained <http://rdaregistry.info/Elements/u/P60617> ;
    reg:lexicalAlias <http://rdaregistry.info/Elements/a/writerOfPrefaceOf.en> ;
    reg:name "writerOfPrefaceOf"@en ;
    reg:status <http://metadataregistry.org/uri/RegStatus/1001> ;
    rdfs:domain <http://rdaregistry.info/Elements/c/C10002> ;
    rdfs:isDefinedBy <http://rdaregistry.info/Elements/a/> ;
    rdfs:subPropertyOf <http://rdaregistry.info/Elements/a/P50154> ;
    skos:definition "Relates an agent contributing to an expression of a work by providing a preface to an original work to an expression."@en,
        "Met une personne, famille ou collectivité contribuant à une expression d’une œuvre en fournissant une préface à l’œuvre originale en relation avec l’expression."@fr .

<http://rdaregistry.info/Elements/a/P50150> a rdf:Property ;
    rdfs:label "is cartographer (expression) of"@en,
        "est le cartographe (expression) de"@fr ;
    rdakit:instructionNumber "18.5" ;
    rdakit:toolkitDefinition "An expression of a work that incorporates a contribution of providing additional cartography, or by modifying previous cartography."@en,
        "Personne, famille ou collectivité contribuant à une expression d’une œuvre en fournissant une cartographie additionnelle ou en modifiant la cartographie antérieure."@fr ;
    rdakit:toolkitLabel "cartographer (expression) of"@en,
        "cartographe (expression) de"@fr ;
    reg:hasSubproperty <http://rdaregistry.info/Elements/a/datatype/P50150>,
        <http://rdaregistry.info/Elements/a/object/P50150> ;
    reg:hasUnconstrained <http://rdaregistry.info/Elements/u/P60654> ;
    reg:lexicalAlias <http://rdaregistry.info/Elements/a/cartographerExpressionOf.en> ;
    reg:name "cartographerExpressionOf"@en ;
    reg:status <http://metadataregistry.org/uri/RegStatus/1001> ;
    rdfs:domain <http://rdaregistry.info/Elements/c/C10002> ;
    rdfs:isDefinedBy <http://rdaregistry.info/Elements/a/> ;
    rdfs:subPropertyOf <http://rdaregistry.info/Elements/a/P50161> ;
    skos:definition "Relates an agent contributing to an expression of a work by providing additional cartography, or by modifying previous cartography to an expression."@en,
        "Met une personne, famille ou collectivité contribuant à une expression d’une œuvre en fournissant une cartographie additionnelle ou en modifiant la cartographie antérieure en relation avec l’expression."@fr .

<http://rdaregistry.info/Elements/a/P50151> a rdf:Property ;
    rdfs:label "is choreographer (expression) of"@en,
        "est le chorégraphe (expression) de"@fr ;
    rdakit:instructionNumber "18.5" ;
    rdakit:toolkitDefinition "An expression of a work that incorporates a contribution of providing additional choreography, or by modifying previous choreography."@en,
        "Personne, famille ou collectivité contribuant à une expression d’une œuvre en fournissant une chorégraphie additionnelle ou en modifiant la chorégraphie antérieure."@fr ;
    rdakit:toolkitLabel "choreographer (expression) of"@en,
        "chorégraphe (expression) de"@fr ;
    reg:hasSubproperty <http://rdaregistry.info/Elements/a/datatype/P50151>,
        <http://rdaregistry.info/Elements/a/object/P50151> ;
    reg:hasUnconstrained <http://rdaregistry.info/Elements/u/P60662> ;
    reg:lexicalAlias <http://rdaregistry.info/Elements/a/choreographerExpressionOf.en> ;
    reg:name "choreographerExpressionOf"@en ;
    reg:status <http://metadataregistry.org/uri/RegStatus/1001> ;
    rdfs:domain <http://rdaregistry.info/Elements/c/C10002> ;
    rdfs:isDefinedBy <http://rdaregistry.info/Elements/a/> ;
    rdfs:subPropertyOf <http://rdaregistry.info/Elements/a/P50161> ;
    skos:definition "Relates an agent contributing to an expression of a work by providing additional choreography, or by modifying previous choreography to an expression."@en,
        "Met une personne, famille ou collectivité contribuant à une expression d’une œuvre en fournissant une chorégraphie additionnelle ou en modifiant la chorégraphie antérieure en relation avec l’expression."@fr .

<http://rdaregistry.info/Elements/a/P50152> a rdf:Property ;
    rdfs:label "is writer of added commentary of"@en,
        "est l’auteur de commentaire ajouté de"@fr ;
    rdakit:instructionNumber "18.5" ;
    rdakit:toolkitDefinition "An expression of a work that incorporates a contribution of providing an interpretation or critical explanation to an original work."@en,
        "Personne, famille ou collectivité contribuant à une expression d’une œuvre en fournissant une interprétation ou une critique de l’œuvre originale."@fr ;
    rdakit:toolkitLabel "writer of added commentary of"@en,
        "auteur de commentaire ajouté de"@fr ;
    reg:hasSubproperty <http://rdaregistry.info/Elements/a/datatype/P50152>,
        <http://rdaregistry.info/Elements/a/object/P50152> ;
    reg:hasUnconstrained <http://rdaregistry.info/Elements/u/P60618> ;
    reg:lexicalAlias <http://rdaregistry.info/Elements/a/writerOfAddedCommentaryOf.en> ;
    reg:name "writerOfAddedCommentaryOf"@en ;
    reg:status <http://metadataregistry.org/uri/RegStatus/1001> ;
    rdfs:domain <http://rdaregistry.info/Elements/c/C10002> ;
    rdfs:isDefinedBy <http://rdaregistry.info/Elements/a/> ;
    rdfs:subPropertyOf <http://rdaregistry.info/Elements/a/P50154> ;
    skos:definition "Relates an agent contributing to an expression of a work by providing an interpretation or critical explanation of an original work to an expression."@en,
        "Met une personne, famille ou collectivité contribuant à une expression d’une œuvre en fournissant une interprétation ou une critique de l’œuvre originale en relation avec l’expression."@fr .

<http://rdaregistry.info/Elements/a/P50153> a rdf:Property ;
    rdfs:label "is writer of introduction of"@en,
        "est l’auteur d’introduction de"@fr ;
    rdakit:instructionNumber "18.5" ;
    rdakit:toolkitDefinition "An expression of a work that incorporates a contribution of providing an introduction to an original work."@en,
        "Personne, famille ou collectivité contribuant à une expression d’une œuvre en fournissant une introduction à l’œuvre originale."@fr ;
    rdakit:toolkitLabel "writer of introduction of"@en,
        "auteur d’introduction de"@fr ;
    reg:hasSubproperty <http://rdaregistry.info/Elements/a/datatype/P50153>,
        <http://rdaregistry.info/Elements/a/object/P50153> ;
    reg:hasUnconstrained <http://rdaregistry.info/Elements/u/P60619> ;
    reg:lexicalAlias <http://rdaregistry.info/Elements/a/writerOfIntroductionOf.en> ;
    reg:name "writerOfIntroductionOf"@en ;
    reg:status <http://metadataregistry.org/uri/RegStatus/1001> ;
    rdfs:domain <http://rdaregistry.info/Elements/c/C10002> ;
    rdfs:isDefinedBy <http://rdaregistry.info/Elements/a/> ;
    rdfs:subPropertyOf <http://rdaregistry.info/Elements/a/P50154> ;
    skos:definition "Relates an agent contributing to an expression of a work by providing an introduction to an original work to an expression."@en,
        "Met une personne, famille ou collectivité contribuant à une expression d’une œuvre en fournissant une introduction à l’œuvre originale en relation avec l’expression."@fr .

<http://rdaregistry.info/Elements/a/P50155> a rdf:Property ;
    rdfs:label "is interviewee (expression) of"@en,
        "est l’interviewé (expression) de"@fr ;
    rdakit:instructionNumber "18.5" ;
    rdakit:toolkitDefinition "An expression of a work that incorporates a contribution of responding to an interviewer, usually a reporter, pollster, or some other information gathering agent."@en,
        "Personne, famille ou collectivité contribuant à une expression d’une œuvre en répondant à un intervieweur, habituellement un journaliste, un sondeur ou un autre agent recueillant de l’information."@fr ;
    rdakit:toolkitLabel "interviewee (expression) of"@en,
        "interviewé (expression) de"@fr ;
    reg:hasSubproperty <http://rdaregistry.info/Elements/a/datatype/P50155>,
        <http://rdaregistry.info/Elements/a/object/P50155> ;
    reg:hasUnconstrained <http://rdaregistry.info/Elements/u/P60661> ;
    reg:lexicalAlias <http://rdaregistry.info/Elements/a/intervieweeExpressionOf.en> ;
    reg:name "intervieweeExpressionOf"@en ;
    reg:status <http://metadataregistry.org/uri/RegStatus/1001> ;
    rdfs:domain <http://rdaregistry.info/Elements/c/C10002> ;
    rdfs:isDefinedBy <http://rdaregistry.info/Elements/a/> ;
    rdfs:subPropertyOf <http://rdaregistry.info/Elements/a/P50161> ;
    skos:definition "Relates an agent contributing to an expression of a work by responding to an interviewer, usually a reporter, pollster, or some other information gathering agent to an expression."@en,
        "Met une personne, famille ou collectivité contribuant à une expression d’une œuvre en répondant à un intervieweur, habituellement un journaliste, un sondeur ou un autre agent recueillant de l’information en relation avec l’expression."@fr .

<http://rdaregistry.info/Elements/a/P50157> a rdf:Property ;
    rdfs:label "is abridger of"@en,
        "est l’abréviateur de"@fr ;
    rdakit:instructionNumber "18.5" ;
    rdakit:seeAlso <http://rdaregistry.info/Elements/a/P50195> ;
    rdakit:toolkitDefinition "An expression of a work that incorporates a contribution of shortening or condensing the original work but leaving the nature and content substantially unchanged."@en,
        "Personne, famille ou collectivité contribuant à une expression d’une œuvre en abrégeant ou en condensant l’œuvre originale tout en conservant la nature et le contenu de l’œuvre originale sensiblement inchangés."@fr ;
    rdakit:toolkitLabel "abridger of"@en,
        "abréviateur de"@fr ;
    reg:hasSubproperty <http://rdaregistry.info/Elements/a/datatype/P50157>,
        <http://rdaregistry.info/Elements/a/object/P50157> ;
    reg:hasUnconstrained <http://rdaregistry.info/Elements/u/P60622> ;
    reg:lexicalAlias <http://rdaregistry.info/Elements/a/abridgerOf.en> ;
    reg:name "abridgerOf"@en ;
    reg:status <http://metadataregistry.org/uri/RegStatus/1001> ;
    rdfs:domain <http://rdaregistry.info/Elements/c/C10002> ;
    rdfs:isDefinedBy <http://rdaregistry.info/Elements/a/> ;
    rdfs:subPropertyOf <http://rdaregistry.info/Elements/a/P50161> ;
    skos:definition "Relates an agent contributing to an expression of a work by shortening or condensing the original work but leaving the nature and content substantially unchanged to an expression."@en,
        "Met une personne, famille ou collectivité contribuant à une expression d’une œuvre en abrégeant ou en condensant l’œuvre originale tout en conservant la nature et le contenu de l’œuvre originale sensiblement inchangés en relation avec l’expression."@fr .

<http://rdaregistry.info/Elements/a/P50158> a rdf:Property ;
    rdfs:label "is recording engineer of"@en,
        "est l’ingénieur du son de"@fr ;
    rdakit:instructionNumber "18.5" ;
    rdakit:toolkitDefinition "An expression of a work that incorporates a contribution to the audio content of supervising the technical aspects of a recording session."@en,
        "Personne, famille ou collectivité contribuant à une expression d’une œuvre en supervisant les aspects techniques d’une séance d’enregistrement sonore ou vidéo."@fr ;
    rdakit:toolkitLabel "recording engineer of"@en,
        "ingénieur du son de"@fr ;
    reg:hasSubproperty <http://rdaregistry.info/Elements/a/datatype/P50158>,
        <http://rdaregistry.info/Elements/a/object/P50158> ;
    reg:hasUnconstrained <http://rdaregistry.info/Elements/u/P60623> ;
    reg:lexicalAlias <http://rdaregistry.info/Elements/a/recordingEngineerOf.en> ;
    reg:name "recordingEngineerOf"@en ;
    reg:status <http://metadataregistry.org/uri/RegStatus/1001> ;
    rdfs:domain <http://rdaregistry.info/Elements/c/C10002> ;
    rdfs:isDefinedBy <http://rdaregistry.info/Elements/a/> ;
    rdfs:subPropertyOf <http://rdaregistry.info/Elements/a/P50296> ;
    skos:definition "Relates an audio engineer contributing to the audio content of an expression by supervising the technical aspects of a recording session to an expression."@en,
        "Met une personne, famille ou collectivité contribuant à une expression d’une œuvre en supervisant les aspects techniques d’une séance d’enregistrement sonore ou vidéo en relation avec l’expression."@fr .

<http://rdaregistry.info/Elements/a/P50160> a rdf:Property ;
    rdfs:label "is recordist of"@en,
        "est l’opérateur d’enregistrement de"@fr ;
    rdakit:instructionNumber "18.5" ;
    rdakit:toolkitDefinition "An expression of a work that incorporates a contribution of using a recording device to capture sound and/or video during a recording session, including field recordings of natural sounds, folkloric events, music, etc."@en,
        "Personne, famille ou collectivité contribuant à une expression d’une œuvre en utilisant un appareil d’enregistrement pour capter le son et/ou la vidéo durant une séance d’enregistrement, y compris les enregistrements de terrain de sons naturels, de prestations folkloriques, de musique, etc."@fr ;
    rdakit:toolkitLabel "recordist of"@en,
        "opérateur d’enregistrement de"@fr ;
    reg:hasSubproperty <http://rdaregistry.info/Elements/a/datatype/P50160>,
        <http://rdaregistry.info/Elements/a/object/P50160> ;
    reg:hasUnconstrained <http://rdaregistry.info/Elements/u/P60625> ;
    reg:lexicalAlias <http://rdaregistry.info/Elements/a/recordistOf.en> ;
    reg:name "recordistOf"@en ;
    reg:status <http://metadataregistry.org/uri/RegStatus/1001> ;
    rdfs:domain <http://rdaregistry.info/Elements/c/C10002> ;
    rdfs:isDefinedBy <http://rdaregistry.info/Elements/a/> ;
    rdfs:subPropertyOf <http://rdaregistry.info/Elements/a/P50161> ;
    skos:definition "Relates an agent contributing to an expression of a work by using a recording device to capture sound and/or video during a recording session, including field recordings of natural sounds, folkloric events, music, etc. to an expression."@en,
        "Met une personne, famille ou collectivité contribuant à une expression d’une œuvre en utilisant un appareil d’enregistrement pour capter le son et/ou la vidéo durant une séance d’enregistrement, y compris les enregistrements de terrain de sons naturels, de prestations folkloriques, de musique, etc., en relation avec l’expression."@fr .

<http://rdaregistry.info/Elements/a/P50166> a rdf:Property ;
    rdfs:label "is honouree of"@en,
        "est l’entité honorée de"@fr ;
    rdakit:instructionNumber "18.5" ;
    rdakit:toolkitDefinition "A work honouring an agent."@en,
        "Personne, famille ou collectivité honorée par une œuvre (par exemple, une personne à qui sont offerts des mélanges)."@fr ;
    rdakit:toolkitLabel "honouree of"@en,
        "entité honorée de"@fr ;
    reg:hasSubproperty <http://rdaregistry.info/Elements/a/datatype/P50166>,
        <http://rdaregistry.info/Elements/a/object/P50166> ;
    reg:hasUnconstrained <http://rdaregistry.info/Elements/u/P60634> ;
    reg:lexicalAlias <http://rdaregistry.info/Elements/a/honoureeOf.en> ;
    reg:name "honoureeOf"@en ;
    reg:status <http://metadataregistry.org/uri/RegStatus/1001> ;
    rdfs:domain <http://rdaregistry.info/Elements/c/C10002> ;
    rdfs:isDefinedBy <http://rdaregistry.info/Elements/a/> ;
    rdfs:subPropertyOf <http://rdaregistry.info/Elements/a/P50131> ;
    skos:altLabel "honoree of"@en ;
    skos:definition "Relates an agent honoured by a work to a work."@en,
        "Met une personne, famille ou collectivité honorée par une œuvre (par exemple, une personne à qui sont offerts des mélanges) en relation avec l’œuvre."@fr .

<http://rdaregistry.info/Elements/a/P50167> a rdf:Property ;
    rdfs:label "is honouree (item) of"@en,
        "est l’entité honorée (item) de"@fr ;
    rdakit:instructionNumber "18.5" ;
    rdakit:toolkitDefinition "An item honouring an agent."@en,
        "Personne, famille ou collectivité honorée par un item, par exemple, une personne à qui un exemplaire est offert."@fr ;
    rdakit:toolkitLabel "honouree (item) of"@en,
        "entité honorée (item) de"@fr ;
    reg:hasSubproperty <http://rdaregistry.info/Elements/a/datatype/P50167>,
        <http://rdaregistry.info/Elements/a/object/P50167> ;
    reg:hasUnconstrained <http://rdaregistry.info/Elements/u/P60634> ;
    reg:lexicalAlias <http://rdaregistry.info/Elements/a/honoureeOfItemOf.en> ;
    reg:name "honoureeOfItemOf"@en ;
    reg:status <http://metadataregistry.org/uri/RegStatus/1001> ;
    rdfs:domain <http://rdaregistry.info/Elements/c/C10002> ;
    rdfs:isDefinedBy <http://rdaregistry.info/Elements/a/> ;
    rdfs:subPropertyOf <http://rdaregistry.info/Elements/a/P50182> ;
    skos:altLabel "honoree (item) of"@en ;
    skos:definition "Relates an agent honoured by an item to an item."@en,
        "Met une personne, famille ou collectivité honorée par un item, par exemple, une personne à qui un exemplaire est offert, en relation avec l’item."@fr .

<http://rdaregistry.info/Elements/a/P50168> a rdf:Property ;
    rdfs:label "is broadcaster of"@en,
        "est le diffuseur de"@fr ;
    rdakit:instructionNumber "18.5" ;
    rdakit:toolkitDefinition "A manifestation that is broadcast to an audience via radio, television, webcast, etc."@en,
        "Personne, famille ou collectivité prenant part à la diffusion d’une manifestation à un public par la radio, la télévision, la webdiffusion, etc."@fr ;
    rdakit:toolkitLabel "broadcaster of"@en,
        "diffuseur de"@fr ;
    reg:hasSubproperty <http://rdaregistry.info/Elements/a/datatype/P50168>,
        <http://rdaregistry.info/Elements/a/object/P50168> ;
    reg:hasUnconstrained <http://rdaregistry.info/Elements/u/P60635> ;
    reg:lexicalAlias <http://rdaregistry.info/Elements/a/broadcasterOf.en> ;
    reg:name "broadcasterOf"@en ;
    reg:status <http://metadataregistry.org/uri/RegStatus/1001> ;
    rdfs:domain <http://rdaregistry.info/Elements/c/C10002> ;
    rdfs:isDefinedBy <http://rdaregistry.info/Elements/a/> ;
    rdfs:subPropertyOf <http://rdaregistry.info/Elements/a/P50203> ;
    skos:definition "Relates an agent involved in broadcasting a manifestation to an audience via radio, television, webcast, etc. to a manifestation."@en,
        "Met une personne, famille ou collectivité prenant part à la diffusion d’une manifestation à un public par la radio, la télévision, la webdiffusion, etc. en relation avec la manifestation."@fr .

<http://rdaregistry.info/Elements/a/P50169> a rdf:Property ;
    rdfs:label "is film distributor of"@en,
        "est le distributeur de films de"@fr ;
    rdakit:instructionNumber "18.5" ;
    rdakit:toolkitDefinition "A moving image manifestation distributed to theatres or other distribution channels."@en,
        "Personne, famille ou collectivité prenant part à la distribution d’une manifestation d’images animées aux salles de cinéma ou aux autres réseaux de distribution."@fr ;
    rdakit:toolkitLabel "film distributor of"@en,
        "distributeur de films de"@fr ;
    reg:hasSubproperty <http://rdaregistry.info/Elements/a/datatype/P50169>,
        <http://rdaregistry.info/Elements/a/object/P50169> ;
    reg:hasUnconstrained <http://rdaregistry.info/Elements/u/P60636> ;
    reg:lexicalAlias <http://rdaregistry.info/Elements/a/filmDistributorOf.en> ;
    reg:name "filmDistributorOf"@en ;
    reg:status <http://metadataregistry.org/uri/RegStatus/1001> ;
    rdfs:domain <http://rdaregistry.info/Elements/c/C10002> ;
    rdfs:isDefinedBy <http://rdaregistry.info/Elements/a/> ;
    rdfs:subPropertyOf <http://rdaregistry.info/Elements/a/P50199> ;
    skos:definition "Relates an agent involved in distributing a moving image manifestation to theatres or other distribution channels to a manifestation."@en,
        "Met une personne, famille ou collectivité prenant part à la distribution d’une manifestation d’images animées aux salles de cinéma ou aux autres réseaux de distribution en relation avec la manifestation."@fr .

<http://rdaregistry.info/Elements/a/P50170> a rdf:Property ;
    rdfs:label "is book designer of"@en,
        "est le graphiste de"@fr ;
    rdakit:instructionNumber "18.5" ;
    rdakit:toolkitDefinition "A manifestation manufactured by an agent responsible for the entire graphic design of a book, including arrangement of type and illustration, choice of materials, and process used."@en,
        "Personne, famille ou collectivité prenant part à la fabrication d’une manifestation en étant responsable de toute la conception graphique d’un livre, y compris la composition typographique, l’arrangement des illustrations, le choix des matériaux et le processus utilisé."@fr ;
    rdakit:toolkitLabel "book designer of"@en,
        "graphiste de"@fr ;
    reg:hasSubproperty <http://rdaregistry.info/Elements/a/datatype/P50170>,
        <http://rdaregistry.info/Elements/a/object/P50170> ;
    reg:hasUnconstrained <http://rdaregistry.info/Elements/u/P60637> ;
    reg:lexicalAlias <http://rdaregistry.info/Elements/a/bookDesignerOf.en> ;
    reg:name "bookDesignerOf"@en ;
    reg:status <http://metadataregistry.org/uri/RegStatus/1001> ;
    rdfs:domain <http://rdaregistry.info/Elements/c/C10002> ;
    rdfs:isDefinedBy <http://rdaregistry.info/Elements/a/> ;
    rdfs:subPropertyOf <http://rdaregistry.info/Elements/a/P50202> ;
    skos:definition "Relates an agent involved in manufacturing a manifestation by being responsible for the entire graphic design of a book, including arrangement of type and illustration, choice of materials, and process used to a manifestation."@en,
        "Met une personne, famille ou collectivité prenant part à la fabrication d’une manifestation en étant responsable de toute la conception graphique d’un livre, y compris la composition typographique, l’arrangement des illustrations, le choix des matériaux et le processus utilisé, en relation avec la manifestation."@fr .

<http://rdaregistry.info/Elements/a/P50171> a rdf:Property ;
    rdfs:label "is engraver of"@en,
        "est le graveur de"@fr ;
    rdakit:instructionNumber "18.5" ;
    rdakit:toolkitDefinition "A manifestation manufactured by an agent responsible for cutting letters, figures, etc., on a surface such as a wooden or metal plate used for printing."@en,
        "Personne, famille ou collectivité prenant part à la fabrication d’une manifestation en gravant des lettres, des figures, etc. sur une surface telle qu’une plaque de bois ou de métal utilisée pour l’impression."@fr ;
    rdakit:toolkitLabel "engraver of"@en,
        "graveur de"@fr ;
    reg:hasSubproperty <http://rdaregistry.info/Elements/a/datatype/P50171>,
        <http://rdaregistry.info/Elements/a/object/P50171> ;
    reg:hasUnconstrained <http://rdaregistry.info/Elements/u/P60638> ;
    reg:lexicalAlias <http://rdaregistry.info/Elements/a/engraverOf.en> ;
    reg:name "engraverOf"@en ;
    reg:status <http://metadataregistry.org/uri/RegStatus/1001> ;
    rdfs:domain <http://rdaregistry.info/Elements/c/C10002> ;
    rdfs:isDefinedBy <http://rdaregistry.info/Elements/a/> ;
    rdfs:subPropertyOf <http://rdaregistry.info/Elements/a/P50202> ;
    skos:definition "Relates an agent involved in manufacturing a manifestation by cutting letters, figures, etc., on a surface such as a wooden or metal plate used for printing to a manifestation."@en,
        "Met une personne, famille ou collectivité prenant part à la fabrication d’une manifestation en gravant des lettres, des figures, etc. sur une surface telle qu’une plaque de bois ou de métal utilisée pour l’impression en relation avec la manifestation."@fr .

<http://rdaregistry.info/Elements/a/P50172> a rdf:Property ;
    rdfs:label "is braille embosser of"@en,
        "est le producteur braille de"@fr ;
    rdakit:instructionNumber "18.5" ;
    rdakit:toolkitDefinition "A manifestation manufactured by an agent responsible for embossing braille cells using a stylus, special embossing printer, or other device."@en,
        "Personne, famille ou collectivité prenant part à la fabrication d’une manifestation par l’embossage de cellules braille au moyen d’un poinçon, d’une imprimante spéciale ou d’un autre appareil."@fr ;
    rdakit:toolkitLabel "braille embosser of"@en,
        "producteur braille de"@fr ;
    reg:hasSubproperty <http://rdaregistry.info/Elements/a/datatype/P50172>,
        <http://rdaregistry.info/Elements/a/object/P50172> ;
    reg:hasUnconstrained <http://rdaregistry.info/Elements/u/P60639> ;
    reg:lexicalAlias <http://rdaregistry.info/Elements/a/brailleEmbosserOf.en> ;
    reg:name "brailleEmbosserOf"@en ;
    reg:status <http://metadataregistry.org/uri/RegStatus/1001> ;
    rdfs:domain <http://rdaregistry.info/Elements/c/C10002> ;
    rdfs:isDefinedBy <http://rdaregistry.info/Elements/a/> ;
    rdfs:subPropertyOf <http://rdaregistry.info/Elements/a/P50202> ;
    skos:definition "Relates an agent involved in manufacturing a manifestation by embossing braille cells using a stylus, special embossing printer, or other device to a manifestation."@en,
        "Met une personne, famille ou collectivité prenant part à la fabrication d’une manifestation par l’embossage de cellules braille au moyen d’un poinçon, d’une imprimante spéciale ou d’un autre appareil en relation avec la manifestation."@fr .

<http://rdaregistry.info/Elements/a/P50173> a rdf:Property ;
    rdfs:label "is printmaker of"@en,
        "est le graveur d’estampes de"@fr ;
    rdakit:instructionNumber "18.5" ;
    rdakit:toolkitDefinition "A manifestation manufactured by an agent responsible for making a relief, intaglio, or planographic printing surface."@en,
        "Personne, famille ou collectivité prenant part à la fabrication d’une manifestation en préparant un élément d’impression en relief, en creux ou planographique."@fr ;
    rdakit:toolkitLabel "printmaker of"@en,
        "graveur d’estampes de"@fr ;
    reg:hasSubproperty <http://rdaregistry.info/Elements/a/datatype/P50173>,
        <http://rdaregistry.info/Elements/a/object/P50173> ;
    reg:hasUnconstrained <http://rdaregistry.info/Elements/u/P60640> ;
    reg:lexicalAlias <http://rdaregistry.info/Elements/a/printmakerOf.en> ;
    reg:name "printmakerOf"@en ;
    reg:status <http://metadataregistry.org/uri/RegStatus/1001> ;
    rdfs:domain <http://rdaregistry.info/Elements/c/C10002> ;
    rdfs:isDefinedBy <http://rdaregistry.info/Elements/a/> ;
    rdfs:subPropertyOf <http://rdaregistry.info/Elements/a/P50202> ;
    skos:definition "Relates an agent involved in manufacturing a manifestation by making a relief, intaglio, or planographic printing surface to a manifestation."@en,
        "Met une personne, famille ou collectivité prenant part à la fabrication d’une manifestation en préparant un élément d’impression en relief, en creux ou planographique en relation avec la manifestation."@fr .

<http://rdaregistry.info/Elements/a/P50174> a rdf:Property ;
    rdfs:label "is caster of"@en,
        "est le fondeur de"@fr ;
    rdakit:instructionNumber "18.5" ;
    rdakit:toolkitDefinition "A manifestation manufactured by an agent responsible for pouring a liquid or molten substance into a mold and leaving it to solidify to take the shape of the mold."@en,
        "Personne, famille ou collectivité prenant part à la fabrication d’une manifestation en versant un liquide ou une substance fondue dans un moule et en laissant ce liquide ou cette substance se solidifier pour prendre la forme du moule."@fr ;
    rdakit:toolkitLabel "caster of"@en,
        "fondeur de"@fr ;
    reg:hasSubproperty <http://rdaregistry.info/Elements/a/datatype/P50174>,
        <http://rdaregistry.info/Elements/a/object/P50174> ;
    reg:hasUnconstrained <http://rdaregistry.info/Elements/u/P60641> ;
    reg:lexicalAlias <http://rdaregistry.info/Elements/a/casterOf.en> ;
    reg:name "casterOf"@en ;
    reg:status <http://metadataregistry.org/uri/RegStatus/1001> ;
    rdfs:domain <http://rdaregistry.info/Elements/c/C10002> ;
    rdfs:isDefinedBy <http://rdaregistry.info/Elements/a/> ;
    rdfs:subPropertyOf <http://rdaregistry.info/Elements/a/P50202> ;
    skos:definition "Relates an agent involved in manufacturing a manifestation by pouring a liquid or molten substance into a mold and leaving it to solidify to take the shape of the mold to a manifestation."@en,
        "Met une personne, famille ou collectivité prenant part à la fabrication d’une manifestation en versant un liquide ou une substance fondue dans un moule et en laissant ce liquide ou cette substance se solidifier pour prendre la forme du moule en relation avec la manifestation."@fr .

<http://rdaregistry.info/Elements/a/P50175> a rdf:Property ;
    rdfs:label "is lithographer of"@en,
        "est le lithographe de"@fr ;
    rdakit:instructionNumber "18.5" ;
    rdakit:toolkitDefinition "A manifestation manufactured by an agent responsible for preparing a stone or plate for lithographic printing."@en,
        "Personne, famille ou collectivité prenant part à la fabrication d’une manifestation en préparant une pierre ou une plaque pour l’impression lithographique, y compris un artiste graphique créant un dessin directement sur la surface à partir de laquelle l’impression sera effectuée."@fr ;
    rdakit:toolkitLabel "lithographer of"@en,
        "lithographe de"@fr ;
    reg:hasSubproperty <http://rdaregistry.info/Elements/a/datatype/P50175>,
        <http://rdaregistry.info/Elements/a/object/P50175> ;
    reg:hasUnconstrained <http://rdaregistry.info/Elements/u/P60642> ;
    reg:lexicalAlias <http://rdaregistry.info/Elements/a/lithographerOf.en> ;
    reg:name "lithographerOf"@en ;
    reg:status <http://metadataregistry.org/uri/RegStatus/1001> ;
    rdfs:domain <http://rdaregistry.info/Elements/c/C10002> ;
    rdfs:isDefinedBy <http://rdaregistry.info/Elements/a/> ;
    rdfs:subPropertyOf <http://rdaregistry.info/Elements/a/P50202> ;
    skos:definition "Relates an agent involved in manufacturing a manifestation by preparing a stone or plate for lithographic printing."@en,
        "Met une personne, famille ou collectivité prenant part à la fabrication d’une manifestation en préparant une pierre ou une plaque pour l’impression lithographique, y compris un artiste graphique créant un dessin directement sur la surface à partir de laquelle l’impression sera effectuée, en relation avec la manifestation."@fr ;
    skos:scopeNote "A lithographer includes a graphic artist creating a design directly on the surface from which printing will be done."@en .

<http://rdaregistry.info/Elements/a/P50176> a rdf:Property ;
    rdfs:label "is platemaker of"@en,
        "est le graveur de planches de"@fr ;
    rdakit:instructionNumber "18.5" ;
    rdakit:toolkitDefinition "A manifestation manufactured by an agent responsible for preparing plates used in the production of printed images or text."@en,
        "Personne, famille ou collectivité prenant part à la fabrication d’une manifestation en préparant les planches utilisées dans la production d’images et/ou de textes imprimés."@fr ;
    rdakit:toolkitLabel "platemaker of"@en,
        "graveur de planches de"@fr ;
    reg:hasSubproperty <http://rdaregistry.info/Elements/a/datatype/P50176>,
        <http://rdaregistry.info/Elements/a/object/P50176> ;
    reg:hasUnconstrained <http://rdaregistry.info/Elements/u/P60643> ;
    reg:lexicalAlias <http://rdaregistry.info/Elements/a/platemakerOf.en> ;
    reg:name "platemakerOf"@en ;
    reg:status <http://metadataregistry.org/uri/RegStatus/1001> ;
    rdfs:domain <http://rdaregistry.info/Elements/c/C10002> ;
    rdfs:isDefinedBy <http://rdaregistry.info/Elements/a/> ;
    rdfs:subPropertyOf <http://rdaregistry.info/Elements/a/P50202> ;
    skos:definition "Relates an agent involved in manufacturing a manifestation by preparing plates used in the production of printed images or text to a manifestation."@en,
        "Met une personne, famille ou collectivité prenant part à la fabrication d’une manifestation en préparant les planches utilisées dans la production d’images et/ou de textes imprimés en relation avec la manifestation."@fr .

<http://rdaregistry.info/Elements/a/P50177> a rdf:Property ;
    rdfs:label "is etcher of"@en,
        "est l’aquafortiste de"@fr ;
    rdakit:instructionNumber "18.5" ;
    rdakit:toolkitDefinition "A manifestation manufactured by an agent responsible for subjecting metal, glass, or some other surface used for printing, to acid or another corrosive substance."@en,
        "Personne, famille ou collectivité prenant part à la fabrication d’une manifestation en soumettant à l’acide ou à une autre substance corrosive du métal, du verre ou une autre surface utilisée pour l’impression."@fr ;
    rdakit:toolkitLabel "etcher of"@en,
        "aquafortiste de"@fr ;
    reg:hasSubproperty <http://rdaregistry.info/Elements/a/datatype/P50177>,
        <http://rdaregistry.info/Elements/a/object/P50177> ;
    reg:hasUnconstrained <http://rdaregistry.info/Elements/u/P60644> ;
    reg:lexicalAlias <http://rdaregistry.info/Elements/a/etcherOf.en> ;
    reg:name "etcherOf"@en ;
    reg:status <http://metadataregistry.org/uri/RegStatus/1001> ;
    rdfs:domain <http://rdaregistry.info/Elements/c/C10002> ;
    rdfs:isDefinedBy <http://rdaregistry.info/Elements/a/> ;
    rdfs:subPropertyOf <http://rdaregistry.info/Elements/a/P50202> ;
    skos:definition "Relates an agent involved in manufacturing a manifestation by subjecting metal, glass, or some other surface used for printing, to acid or another corrosive substance to a manifestation."@en,
        "Met une personne, famille ou collectivité prenant part à la fabrication d’une manifestation en soumettant à l’acide ou à une autre substance corrosive du métal, du verre ou une autre surface utilisée pour l’impression en relation avec la manifestation."@fr .

<http://rdaregistry.info/Elements/a/P50178> a rdf:Property ;
    rdfs:label "is collotyper of"@en,
        "est le phototypeur de"@fr ;
    rdakit:instructionNumber "18.5" ;
    rdakit:toolkitDefinition "A manifestation manufactured by an agent responsible for using a photomechanical process for making prints directly from a hardened film of gelatin or other colloid that has ink-receptive and ink-repellent surfaces."@en,
        "Personne, famille ou collectivité prenant part à la fabrication d’une manifestation d’épreuves photographiques faites à partir d’un film de gélatine ou d’un autre colloïde ayant des surfaces acceptant ou repoussant l’encre."@fr ;
    rdakit:toolkitLabel "collotyper of"@en,
        "phototypeur de"@fr ;
    reg:hasSubproperty <http://rdaregistry.info/Elements/a/datatype/P50178>,
        <http://rdaregistry.info/Elements/a/object/P50178> ;
    reg:hasUnconstrained <http://rdaregistry.info/Elements/u/P60645> ;
    reg:lexicalAlias <http://rdaregistry.info/Elements/a/collotyperOf.en> ;
    reg:name "collotyperOf"@en ;
    reg:status <http://metadataregistry.org/uri/RegStatus/1001> ;
    rdfs:domain <http://rdaregistry.info/Elements/c/C10002> ;
    rdfs:isDefinedBy <http://rdaregistry.info/Elements/a/> ;
    rdfs:subPropertyOf <http://rdaregistry.info/Elements/a/P50202> ;
    skos:definition "Relates an agent involved in manufacturing a manifestation using a photomechanical process for making prints directly from a hardened film of gelatin or other colloid that has ink-receptive and ink-repellent surfaces to a manifestation."@en,
        "Met une personne, famille ou collectivité prenant part à la fabrication d’une manifestation d’épreuves photographiques faites à partir d’un film de gélatine ou d’un autre colloïde ayant des surfaces acceptant ou repoussant l’encre en relation avec la manifestation."@fr .

<http://rdaregistry.info/Elements/a/P50179> a rdf:Property ;
    rdfs:label "is printer of"@en,
        "est l’imprimeur de"@fr ;
    rdakit:instructionNumber "18.5" ;
    rdakit:toolkitDefinition "A manifestation of printed text, notated music, etc., manufactured by an agent from type or plates, such as a book, newspaper, magazine, broadside, score, etc."@en,
        "Personne, famille ou collectivité prenant part à la fabrication d’une manifestation de texte imprimé, de musique notée, etc. à partir de caractères ou de planches, telle qu’un livre, un journal, une revue, un placard, une partition, etc."@fr ;
    rdakit:toolkitLabel "printer of"@en,
        "imprimeur de"@fr ;
    reg:hasSubproperty <http://rdaregistry.info/Elements/a/datatype/P50179>,
        <http://rdaregistry.info/Elements/a/object/P50179> ;
    reg:hasUnconstrained <http://rdaregistry.info/Elements/u/P60646> ;
    reg:lexicalAlias <http://rdaregistry.info/Elements/a/printerOf.en> ;
    reg:name "printerOf"@en ;
    reg:status <http://metadataregistry.org/uri/RegStatus/1001> ;
    rdfs:domain <http://rdaregistry.info/Elements/c/C10002> ;
    rdfs:isDefinedBy <http://rdaregistry.info/Elements/a/> ;
    rdfs:subPropertyOf <http://rdaregistry.info/Elements/a/P50202> ;
    skos:definition "Relates an agent involved in manufacturing a manifestation of printed text, notated music, etc., from type or plates, such as a book, newspaper, magazine, broadside, score, etc. to a manifestation."@en,
        "Met une personne, famille ou collectivité prenant part à la fabrication d’une manifestation de texte imprimé, de musique notée, etc. à partir de caractères ou de planches, telle qu’un livre, un journal, une revue, un placard, une partition, etc., en relation avec la manifestation."@fr .

<http://rdaregistry.info/Elements/a/P50183> a rdf:Property ;
    rdfs:label "is editor of moving image work of"@en,
        "est le monteur d’œuvre d’images animées de"@fr ;
    rdakit:instructionNumber "18.5" ;
    rdakit:toolkitDefinition "An expression that incorporates a contribution of assembling, arranging, and trimming film, video, or other moving image formats, including both visual and audio aspects."@en,
        "Personne, famille ou collectivité responsable de l’assemblage, de l’arrangement et du découpage de film, de vidéo ou d’autres formats d’images animées, y compris les aspects visuels et sonores."@fr ;
    rdakit:toolkitLabel "editor of moving image work of"@en,
        "monteur d’œuvre d’images animées de"@fr ;
    reg:hasSubproperty <http://rdaregistry.info/Elements/a/datatype/P50183>,
        <http://rdaregistry.info/Elements/a/object/P50183> ;
    reg:hasUnconstrained <http://rdaregistry.info/Elements/u/P60651> ;
    reg:lexicalAlias <http://rdaregistry.info/Elements/a/editorOfMovingImageWorkOf.en> ;
    reg:name "editorOfMovingImageWorkOf"@en ;
    reg:status <http://metadataregistry.org/uri/RegStatus/1001> ;
    rdfs:domain <http://rdaregistry.info/Elements/c/C10002> ;
    rdfs:isDefinedBy <http://rdaregistry.info/Elements/a/> ;
    rdfs:subPropertyOf <http://rdaregistry.info/Elements/a/P50161> ;
    skos:definition "Relates an agent responsible for assembling, arranging, and trimming film, video, or other moving image formats, including both visual and audio aspects to an expression."@en,
        "Met une personne, famille ou collectivité responsable de l’assemblage, de l’arrangement et du découpage de film, de vidéo ou d’autres formats d’images animées, y compris les aspects visuels et sonores, en relation avec l’expression."@fr .

<http://rdaregistry.info/Elements/a/P50184> a rdf:Property ;
    rdfs:label "is programmer of"@en,
        "est le programmeur de"@fr ;
    rdakit:instructionNumber "18.5" ;
    rdakit:toolkitDefinition "A work that involves a creation responsibility for a computer program."@en,
        "Personne, famille ou collectivité responsable de la création d’un programme informatique."@fr ;
    rdakit:toolkitLabel "programmer of"@en,
        "programmeur de"@fr ;
    reg:hasSubproperty <http://rdaregistry.info/Elements/a/datatype/P50184>,
        <http://rdaregistry.info/Elements/a/object/P50184> ;
    reg:hasUnconstrained <http://rdaregistry.info/Elements/u/P60652> ;
    reg:lexicalAlias <http://rdaregistry.info/Elements/a/programmerOf.en> ;
    reg:name "programmerOf"@en ;
    reg:status <http://metadataregistry.org/uri/RegStatus/1001> ;
    rdfs:domain <http://rdaregistry.info/Elements/c/C10002> ;
    rdfs:isDefinedBy <http://rdaregistry.info/Elements/a/> ;
    rdfs:subPropertyOf <http://rdaregistry.info/Elements/a/P50204> ;
    skos:definition "Relates an agent responsible for creating a computer program to a work."@en,
        "Met une personne, famille ou collectivité responsable de la création d’un programme informatique en relation avec l’œuvre."@fr .

<http://rdaregistry.info/Elements/a/P50185> a rdf:Property ;
    rdfs:label "is designer of"@en,
        "est le designer de"@fr ;
    rdakit:instructionNumber "18.5" ;
    rdakit:toolkitDefinition "A work that involves a creation responsibility for a design for an object."@en,
        "Personne, famille ou collectivité responsable de la conception d’un objet."@fr ;
    rdakit:toolkitLabel "designer of"@en,
        "designer de"@fr ;
    reg:hasSubproperty <http://rdaregistry.info/Elements/a/datatype/P50185>,
        <http://rdaregistry.info/Elements/a/object/P50185> ;
    reg:hasUnconstrained <http://rdaregistry.info/Elements/u/P60653> ;
    reg:lexicalAlias <http://rdaregistry.info/Elements/a/designerOf.en> ;
    reg:name "designerOf"@en ;
    reg:status <http://metadataregistry.org/uri/RegStatus/1001> ;
    rdfs:domain <http://rdaregistry.info/Elements/c/C10002> ;
    rdfs:isDefinedBy <http://rdaregistry.info/Elements/a/> ;
    rdfs:subPropertyOf <http://rdaregistry.info/Elements/a/P50204> ;
    skos:definition "Relates an agent responsible for creating a design for an object to a work."@en,
        "Met une personne, famille ou collectivité responsable de la conception d’un objet en relation avec l’œuvre."@fr .

<http://rdaregistry.info/Elements/a/P50186> a rdf:Property ;
    rdfs:label "is cartographer of"@en,
        "est le cartographe de"@fr ;
    rdakit:instructionNumber "18.5" ;
    rdakit:toolkitDefinition "A cartographic work that involves a creation responsibility for a map, atlas, globe, etc."@en,
        "Personne, famille ou collectivité responsable de la création d’une carte, d’un atlas, d’un globe ou d’une autre œuvre cartographique."@fr ;
    rdakit:toolkitLabel "cartographer of"@en,
        "cartographe de"@fr ;
    reg:hasSubproperty <http://rdaregistry.info/Elements/a/datatype/P50186>,
        <http://rdaregistry.info/Elements/a/object/P50186> ;
    reg:hasUnconstrained <http://rdaregistry.info/Elements/u/P60654> ;
    reg:lexicalAlias <http://rdaregistry.info/Elements/a/cartographerOf.en> ;
    reg:name "cartographerOf"@en ;
    reg:status <http://metadataregistry.org/uri/RegStatus/1001> ;
    rdfs:domain <http://rdaregistry.info/Elements/c/C10002> ;
    rdfs:isDefinedBy <http://rdaregistry.info/Elements/a/> ;
    rdfs:subPropertyOf <http://rdaregistry.info/Elements/a/P50204> ;
    skos:definition "Relates an agent responsible for creating a map, atlas, globe, or other cartographic work to a work."@en,
        "Met une personne, famille ou collectivité responsable de la création d’une carte, d’un atlas, d’un globe ou d’une autre œuvre cartographique en relation avec l’œuvre."@fr .

<http://rdaregistry.info/Elements/a/P50188> a rdf:Property ;
    rdfs:label "is inventor of"@en,
        "est l’inventeur de"@fr ;
    rdakit:instructionNumber "18.5" ;
    rdakit:toolkitDefinition "A work that involves a creation responsibility for a new device or process."@en,
        "Personne, famille ou collectivité responsable de la création d’un nouveau dispositif ou procédé."@fr ;
    rdakit:toolkitLabel "inventor of"@en,
        "inventeur de"@fr ;
    reg:hasSubproperty <http://rdaregistry.info/Elements/a/datatype/P50188>,
        <http://rdaregistry.info/Elements/a/object/P50188> ;
    reg:hasUnconstrained <http://rdaregistry.info/Elements/u/P60656> ;
    reg:lexicalAlias <http://rdaregistry.info/Elements/a/inventorOf.en> ;
    reg:name "inventorOf"@en ;
    reg:status <http://metadataregistry.org/uri/RegStatus/1001> ;
    rdfs:domain <http://rdaregistry.info/Elements/c/C10002> ;
    rdfs:isDefinedBy <http://rdaregistry.info/Elements/a/> ;
    rdfs:subPropertyOf <http://rdaregistry.info/Elements/a/P50204> ;
    skos:definition "Relates an agent responsible for creating a new device or process to a work."@en,
        "Met une personne, famille ou collectivité responsable de la création d’un nouveau dispositif ou procédé en relation avec l’œuvre."@fr .

<http://rdaregistry.info/Elements/a/P50189> a rdf:Property ;
    rdfs:label "is compiler of"@en,
        "est le compilateur de"@fr ;
    rdakit:instructionNumber "18.5" ;
    rdakit:seeAlso <http://rdaregistry.info/Elements/a/P50156> ;
    rdakit:toolkitDefinition "A work that involves a creation responsibility for a new work such as a bibliography or a directory by selecting, arranging, aggregating, and editing data, information, etc."@en,
        "Personne, famille ou collectivité responsable de la création d’une nouvelle œuvre (par exemple, une bibliographie, un répertoire) en sélectionnant, en organisant, en regroupant et en éditant des données, de l’information, etc."@fr ;
    rdakit:toolkitLabel "compiler of"@en,
        "compilateur de"@fr ;
    reg:hasSubproperty <http://rdaregistry.info/Elements/a/datatype/P50189>,
        <http://rdaregistry.info/Elements/a/object/P50189> ;
    reg:hasUnconstrained <http://rdaregistry.info/Elements/u/P60657> ;
    reg:lexicalAlias <http://rdaregistry.info/Elements/a/compilerOf.en> ;
    reg:name "compilerOf"@en ;
    reg:status <http://metadataregistry.org/uri/RegStatus/1001> ;
    rdfs:domain <http://rdaregistry.info/Elements/c/C10002> ;
    rdfs:isDefinedBy <http://rdaregistry.info/Elements/a/> ;
    rdfs:subPropertyOf <http://rdaregistry.info/Elements/a/P50204> ;
    skos:definition "Relates an agent responsible for creating a new work such as a bibliography or a directory by selecting, arranging, aggregating, and editing data, information, etc., to a work."@en,
        "Met une personne, famille ou collectivité responsable de la création d’une nouvelle œuvre (par exemple, une bibliographie, un répertoire) en sélectionnant, en organisant, en regroupant et en éditant des données, de l’information, etc. en relation avec l’œuvre."@fr .

<http://rdaregistry.info/Elements/a/P50191> a rdf:Property ;
    rdfs:label "is interviewer of"@en,
        "est l’intervieweur de"@fr ;
    rdakit:instructionNumber "18.5" ;
    rdakit:toolkitDefinition "A work that involves a creation responsibility for acting as an interviewer, reporter, pollster, or some other information gathering agent."@en,
        "Personne, famille ou collectivité responsable de la création d’une œuvre en agissant à titre d’intervieweur, de journaliste, de sondeur ou d’autre agent recueillant de l’information."@fr ;
    rdakit:toolkitLabel "interviewer of"@en,
        "intervieweur de"@fr ;
    reg:hasSubproperty <http://rdaregistry.info/Elements/a/datatype/P50191>,
        <http://rdaregistry.info/Elements/a/object/P50191> ;
    reg:hasUnconstrained <http://rdaregistry.info/Elements/u/P60659> ;
    reg:lexicalAlias <http://rdaregistry.info/Elements/a/interviewerOf.en> ;
    reg:name "interviewerOf"@en ;
    reg:status <http://metadataregistry.org/uri/RegStatus/1001> ;
    rdfs:domain <http://rdaregistry.info/Elements/c/C10002> ;
    rdfs:isDefinedBy <http://rdaregistry.info/Elements/a/> ;
    rdfs:subPropertyOf <http://rdaregistry.info/Elements/a/P50204> ;
    skos:definition "Relates an agent responsible for creating a work by acting as an interviewer, reporter, pollster, or some other information gathering agent to a work."@en,
        "Met une personne, famille ou collectivité responsable de la création d’une œuvre en agissant à titre d’intervieweur, de journaliste, de sondeur ou d’autre agent recueillant de l’information en relation avec l’œuvre."@fr .

<http://rdaregistry.info/Elements/a/P50193> a rdf:Property ;
    rdfs:label "is interviewee of"@en,
        "est l’interviewé de"@fr ;
    rdakit:instructionNumber "18.5" ;
    rdakit:toolkitDefinition "A work that involves a creation responsibility for responding to an interviewer, usually a reporter, pollster, or some other information gathering agent."@en,
        "Personne, famille ou collectivité responsable de la création d’une œuvre en répondant à un intervieweur, habituellement un journaliste, un sondeur ou un autre agent recueillant de l’information."@fr ;
    rdakit:toolkitLabel "interviewee of"@en,
        "interviewé de"@fr ;
    reg:hasSubproperty <http://rdaregistry.info/Elements/a/datatype/P50193>,
        <http://rdaregistry.info/Elements/a/object/P50193> ;
    reg:hasUnconstrained <http://rdaregistry.info/Elements/u/P60661> ;
    reg:lexicalAlias <http://rdaregistry.info/Elements/a/intervieweeOf.en> ;
    reg:name "intervieweeOf"@en ;
    reg:status <http://metadataregistry.org/uri/RegStatus/1001> ;
    rdfs:domain <http://rdaregistry.info/Elements/c/C10002> ;
    rdfs:isDefinedBy <http://rdaregistry.info/Elements/a/> ;
    rdfs:subPropertyOf <http://rdaregistry.info/Elements/a/P50204> ;
    skos:definition "Relates an agent responsible for creating a work by responding to an interviewer, usually a reporter, pollster, or some other information gathering agent to a work."@en,
        "Met une personne, famille ou collectivité responsable de la création d’une œuvre en répondant à un intervieweur, habituellement un journaliste, un sondeur ou un autre agent recueillant de l’information en relation avec l’œuvre."@fr .

<http://rdaregistry.info/Elements/a/P50194> a rdf:Property ;
    rdfs:label "is choreographer of"@en,
        "est le chorégraphe de"@fr ;
    rdakit:instructionNumber "18.5" ;
    rdakit:toolkitDefinition "A work of movement that involves a creation responsibility."@en,
        "Personne, famille ou collectivité responsable de la création d’une œuvre de mouvement."@fr ;
    rdakit:toolkitLabel "choreographer of"@en,
        "chorégraphe de"@fr ;
    reg:hasSubproperty <http://rdaregistry.info/Elements/a/datatype/P50194>,
        <http://rdaregistry.info/Elements/a/object/P50194> ;
    reg:hasUnconstrained <http://rdaregistry.info/Elements/u/P60662> ;
    reg:lexicalAlias <http://rdaregistry.info/Elements/a/choreographerOf.en> ;
    reg:name "choreographerOf"@en ;
    reg:status <http://metadataregistry.org/uri/RegStatus/1001> ;
    rdfs:domain <http://rdaregistry.info/Elements/c/C10002> ;
    rdfs:isDefinedBy <http://rdaregistry.info/Elements/a/> ;
    rdfs:subPropertyOf <http://rdaregistry.info/Elements/a/P50204> ;
    skos:definition "Relates an agent responsible for creating a work of movement to a work."@en,
        "Met une personne, famille ou collectivité responsable de la création d’une œuvre de mouvement en relation avec l’œuvre."@fr .

<http://rdaregistry.info/Elements/a/P50197> a rdf:Property ;
    rdfs:label "is filmmaker of"@en,
        "est le cinéaste de"@fr ;
    rdakit:instructionNumber "18.5" ;
    rdakit:toolkitDefinition "A work that involves a creation responsibility for an independent or personal film."@en,
        "Personne, famille ou collectivité responsable de la création d’un film indépendant ou personnel."@fr ;
    rdakit:toolkitLabel "filmmaker of"@en,
        "cinéaste de"@fr ;
    reg:hasSubproperty <http://rdaregistry.info/Elements/a/datatype/P50197>,
        <http://rdaregistry.info/Elements/a/object/P50197> ;
    reg:hasUnconstrained <http://rdaregistry.info/Elements/u/P60665> ;
    reg:lexicalAlias <http://rdaregistry.info/Elements/a/filmmakerOf.en> ;
    reg:name "filmmakerOf"@en ;
    reg:status <http://metadataregistry.org/uri/RegStatus/1001> ;
    rdfs:domain <http://rdaregistry.info/Elements/c/C10002> ;
    rdfs:isDefinedBy <http://rdaregistry.info/Elements/a/> ;
    rdfs:subPropertyOf <http://rdaregistry.info/Elements/a/P50204> ;
    skos:definition "Relates an agent responsible for creating an independent or personal film to a work."@en,
        "Met une personne, famille ou collectivité responsable de la création d’un film indépendant ou personnel en relation avec l’œuvre."@fr ;
    skos:scopeNote "A filmmaker is individually responsible for the conception and execution of all aspects of the film."@en,
        "Un cinéaste est responsable à titre individuel de la conception et de l’exécution de tous les aspects du film."@fr .

<http://rdaregistry.info/Elements/a/P50198> a rdf:Property ;
    rdfs:label "is production designer of"@en,
        "est le chef décorateur de"@fr ;
    rdakit:instructionNumber "18.5" ;
    rdakit:toolkitDefinition "An expression that incorporates a contribution of designing the overall visual appearance of a moving image production."@en,
        "Personne, famille ou collectivité responsable de concevoir l’aspect visuel global d’une production d’images animées."@fr ;
    rdakit:toolkitLabel "production designer of"@en,
        "chef décorateur de"@fr ;
    reg:hasSubproperty <http://rdaregistry.info/Elements/a/datatype/P50198>,
        <http://rdaregistry.info/Elements/a/object/P50198> ;
    reg:hasUnconstrained <http://rdaregistry.info/Elements/u/P60666> ;
    reg:lexicalAlias <http://rdaregistry.info/Elements/a/productionDesignerOf.en> ;
    reg:name "productionDesignerOf"@en ;
    reg:status <http://metadataregistry.org/uri/RegStatus/1001> ;
    rdfs:domain <http://rdaregistry.info/Elements/c/C10002> ;
    rdfs:isDefinedBy <http://rdaregistry.info/Elements/a/> ;
    rdfs:subPropertyOf <http://rdaregistry.info/Elements/a/P50161> ;
    skos:definition "Relates an agent responsible for designing the overall visual appearance of a moving image production to an expression."@en,
        "Met une personne, famille ou collectivité responsable de concevoir l’aspect visuel global d’une production d’images animées en relation avec l’expression."@fr .

<http://rdaregistry.info/Elements/a/P50199> a rdf:Property ;
    rdfs:label "is distributor of"@en,
        "est le diffuseur ou distributeur de"@fr ;
    rdakit:toolkitDefinition "A manifestation that is distributed."@en,
        "Personne, famille ou collectivité responsable de la diffusion ou de la distribution d’une ressource."@fr ;
    rdakit:toolkitLabel "distributor of"@en,
        "diffuseur ou distributeur de"@fr ;
    reg:hasSubproperty <http://rdaregistry.info/Elements/a/P50169>,
        <http://rdaregistry.info/Elements/a/datatype/P50199>,
        <http://rdaregistry.info/Elements/a/object/P50199> ;
    reg:hasUnconstrained <http://rdaregistry.info/Elements/u/P60667> ;
    reg:lexicalAlias <http://rdaregistry.info/Elements/a/distributorOf.en> ;
    reg:name "distributorOf"@en ;
    reg:status <http://metadataregistry.org/uri/RegStatus/1001> ;
    rdfs:domain <http://rdaregistry.info/Elements/c/C10002> ;
    rdfs:isDefinedBy <http://rdaregistry.info/Elements/a/> ;
    rdfs:subPropertyOf <http://rdaregistry.info/Elements/a/P50307> ;
    skos:definition "Relates an agent responsible for distributing a manifestation to a manifestation."@en,
        "Met une personne, famille ou collectivité responsable de la diffusion ou de la distribution d’une ressource en relation avec la manifestation."@fr .

<http://rdaregistry.info/Elements/a/P50203> a rdf:Property ;
    rdfs:label "is publisher of"@en,
        "est l’éditeur de"@fr ;
    rdakit:toolkitDefinition "A manifestation that is published, released, or issued."@en,
        "Personne, famille ou collectivité responsable de la publication, de la mise à disposition ou de l’édition d’une ressource."@fr ;
    rdakit:toolkitLabel "publisher of"@en,
        "éditeur de"@fr ;
    reg:hasSubproperty <http://rdaregistry.info/Elements/a/P50168>,
        <http://rdaregistry.info/Elements/a/datatype/P50203>,
        <http://rdaregistry.info/Elements/a/object/P50203> ;
    reg:hasUnconstrained <http://rdaregistry.info/Elements/u/P60670> ;
    reg:lexicalAlias <http://rdaregistry.info/Elements/a/publisherOf.en> ;
    reg:name "publisherOf"@en ;
    reg:status <http://metadataregistry.org/uri/RegStatus/1001> ;
    rdfs:domain <http://rdaregistry.info/Elements/c/C10002> ;
    rdfs:isDefinedBy <http://rdaregistry.info/Elements/a/> ;
    rdfs:subPropertyOf <http://rdaregistry.info/Elements/a/P50307> ;
    skos:definition "Relates an agent responsible for publishing, releasing, or issuing a manifestation to a manifestation."@en,
        "Met une personne, famille ou collectivité responsable de la publication, de la mise à disposition ou de l’édition d’une ressource en relation avec la manifestation."@fr .

<http://rdaregistry.info/Elements/a/P50206> a rdf:Property ;
    rdfs:label "is restorationist of"@en,
        "est le restaurateur de"@fr ;
    rdakit:instructionNumber "18.5" ;
    rdakit:toolkitDefinition "An item compensated for degradation by bringing it back to a state as close as possible to its original condition using a set of technical, editorial, and intellectual procedures."@en,
        "Personne, famille ou collectivité responsable de l’ensemble des procédures techniques, éditoriales et intellectuelles destinées à compenser la dégradation d’un item en le ramenant à un état aussi près que possible de sa condition originelle."@fr ;
    rdakit:toolkitLabel "restorationist of"@en,
        "restaurateur de"@fr ;
    reg:hasSubproperty <http://rdaregistry.info/Elements/a/datatype/P50206>,
        <http://rdaregistry.info/Elements/a/object/P50206> ;
    reg:hasUnconstrained <http://rdaregistry.info/Elements/u/P60674> ;
    reg:lexicalAlias <http://rdaregistry.info/Elements/a/restorationistOf.en> ;
    reg:name "restorationistOf"@en ;
    reg:status <http://metadataregistry.org/uri/RegStatus/1001> ;
    rdfs:domain <http://rdaregistry.info/Elements/c/C10002> ;
    rdfs:isDefinedBy <http://rdaregistry.info/Elements/a/> ;
    rdfs:subPropertyOf <http://rdaregistry.info/Elements/a/P50182> ;
    skos:definition "Relates an agent responsible for the set of technical, editorial, and intellectual procedures aimed at compensating for the degradation of an item by bringing it back to a state as close as possible to its original condition to an item."@en,
        "Met une personne, famille ou collectivité responsable de l’ensemble des procédures techniques, éditoriales et intellectuelles destinées à compenser la dégradation d’un item en le ramenant à un état aussi près que possible de sa condition originelle en relation avec l’item."@fr .

<http://rdaregistry.info/Elements/a/P50207> a rdf:Property ;
    rdfs:label "is director of photography of"@en,
        "est le directeur de la photographie de"@fr ;
    rdakit:instructionNumber "18.5" ;
    rdakit:toolkitDefinition "A work that involves a responsibility for capturing images, either electronically or on film or video stock, and often selecting and arranging the lighting."@en,
        "Personne, famille ou collectivité qui capte des images, de manière électronique ou bien sur film ou vidéo, et qui, souvent, choisit et dispose l’éclairage."@fr ;
    rdakit:toolkitLabel "director of photography of"@en,
        "directeur de la photographie de"@fr ;
    reg:hasSubproperty <http://rdaregistry.info/Elements/a/datatype/P50207>,
        <http://rdaregistry.info/Elements/a/object/P50207> ;
    reg:hasUnconstrained <http://rdaregistry.info/Elements/u/P60678> ;
    reg:lexicalAlias <http://rdaregistry.info/Elements/a/directorOfPhotographyOf.en> ;
    reg:name "directorOfPhotographyOf"@en ;
    reg:status <http://metadataregistry.org/uri/RegStatus/1001> ;
    rdfs:domain <http://rdaregistry.info/Elements/c/C10002> ;
    rdfs:isDefinedBy <http://rdaregistry.info/Elements/a/> ;
    rdfs:subPropertyOf <http://rdaregistry.info/Elements/a/P50131> ;
    skos:definition "Relates an agent that captures images, either electronically or on film or video stock, and often selects and arranges the lighting to a work."@en,
        "Met une personne, famille ou collectivité qui capte des images, de manière électronique ou bien sur film ou vidéo, et qui, souvent, choisit et dispose l’éclairage en relation avec l’œuvre."@fr ;
    skos:scopeNote "A director of photography for a movie is also called a chief cinematographer."@en,
        "Le directeur de la photographie pour un film est également appelé le chef opérateur de prise de vues."@fr .

<http://rdaregistry.info/Elements/a/P50208> a rdf:Property ;
    rdfs:label "is dedicatee of"@en,
        "est le dédicataire de"@fr ;
    rdakit:instructionNumber "18.5" ;
    rdakit:toolkitDefinition "A work that is dedicated to an agent."@en,
        "Personne, famille ou collectivité à qui une œuvre est dédiée."@fr ;
    rdakit:toolkitLabel "dedicatee of"@en,
        "dédicataire de"@fr ;
    reg:hasSubproperty <http://rdaregistry.info/Elements/a/datatype/P50208>,
        <http://rdaregistry.info/Elements/a/object/P50208> ;
    reg:hasUnconstrained <http://rdaregistry.info/Elements/u/P60689> ;
    reg:lexicalAlias <http://rdaregistry.info/Elements/a/dedicateeOf.en> ;
    reg:name "dedicateeOf"@en ;
    reg:status <http://metadataregistry.org/uri/RegStatus/1001> ;
    rdfs:domain <http://rdaregistry.info/Elements/c/C10002> ;
    rdfs:isDefinedBy <http://rdaregistry.info/Elements/a/> ;
    rdfs:subPropertyOf <http://rdaregistry.info/Elements/a/P50131> ;
    skos:definition "Relates an agent to whom a work is dedicated to a work."@en,
        "Met une personne, famille ou collectivité à qui une œuvre est dédiée en relation avec l’œuvre."@fr .

<http://rdaregistry.info/Elements/a/P50209> a rdf:Property ;
    rdfs:label "is addressee of"@en,
        "est le destinataire de"@fr ;
    rdakit:instructionNumber "18.5" ;
    rdakit:toolkitDefinition "A work or part of a work that is addressed to an agent."@en,
        "Personne, famille ou collectivité à qui une œuvre ou une partie d’œuvre est adressée."@fr ;
    rdakit:toolkitLabel "addressee of"@en,
        "destinataire de"@fr ;
    reg:hasSubproperty <http://rdaregistry.info/Elements/a/datatype/P50209>,
        <http://rdaregistry.info/Elements/a/object/P50209> ;
    reg:hasUnconstrained <http://rdaregistry.info/Elements/u/P60690> ;
    reg:lexicalAlias <http://rdaregistry.info/Elements/a/addresseeOf.en> ;
    reg:name "addresseeOf"@en ;
    reg:status <http://metadataregistry.org/uri/RegStatus/1001> ;
    rdfs:domain <http://rdaregistry.info/Elements/c/C10002> ;
    rdfs:isDefinedBy <http://rdaregistry.info/Elements/a/> ;
    rdfs:subPropertyOf <http://rdaregistry.info/Elements/a/P50131> ;
    skos:definition "Relates an agent to whom a work or part of a work is addressed to a work."@en,
        "Met une personne, famille ou collectivité à qui une œuvre ou une partie d’œuvre est adressée en relation avec l’œuvre."@fr .

<http://rdaregistry.info/Elements/a/P50210> a rdf:Property ;
    rdfs:label "is dedicatee (item) of"@en,
        "est le dédicataire (item) de"@fr ;
    rdakit:instructionNumber "18.5" ;
    rdakit:toolkitDefinition "An item that is dedicated to an agent."@en,
        "Personne, famille ou collectivité à qui un item est dédié."@fr ;
    rdakit:toolkitLabel "dedicatee (item) of"@en,
        "dédicataire (item) de"@fr ;
    reg:hasSubproperty <http://rdaregistry.info/Elements/a/datatype/P50210>,
        <http://rdaregistry.info/Elements/a/object/P50210> ;
    reg:hasUnconstrained <http://rdaregistry.info/Elements/u/P60689> ;
    reg:lexicalAlias <http://rdaregistry.info/Elements/a/dedicateeOfItemOf.en> ;
    reg:name "dedicateeOfItemOf"@en ;
    reg:status <http://metadataregistry.org/uri/RegStatus/1001> ;
    rdfs:domain <http://rdaregistry.info/Elements/c/C10002> ;
    rdfs:isDefinedBy <http://rdaregistry.info/Elements/a/> ;
    rdfs:subPropertyOf <http://rdaregistry.info/Elements/a/P50182> ;
    skos:definition "Relates an agent to whom an item is dedicated to an item."@en,
        "Met une personne, famille ou collectivité à qui un item est dédié en relation avec l’item."@fr .

<http://rdaregistry.info/Elements/a/P50211> a rdf:Property ;
    rdfs:label "is consultant of"@en,
        "est le consultant de"@fr ;
    rdakit:instructionNumber "18.5" ;
    rdakit:toolkitDefinition "A work that involves a responsibility for providing consultation services, and often making recommendations, for another agent that is represented as the creator of a work."@en,
        "Personne, famille ou collectivité qui fournit des services de consultation et fait souvent des recommandations à une autre personne, famille ou collectivité représentée comme créatrice de l’œuvre."@fr ;
    rdakit:toolkitLabel "consultant of"@en,
        "consultant de"@fr ;
    reg:hasSubproperty <http://rdaregistry.info/Elements/a/datatype/P50211>,
        <http://rdaregistry.info/Elements/a/object/P50211> ;
    reg:hasUnconstrained <http://rdaregistry.info/Elements/u/P60701> ;
    reg:lexicalAlias <http://rdaregistry.info/Elements/a/consultantOf.en> ;
    reg:name "consultantOf"@en ;
    reg:status <http://metadataregistry.org/uri/RegStatus/1001> ;
    rdfs:domain <http://rdaregistry.info/Elements/c/C10002> ;
    rdfs:isDefinedBy <http://rdaregistry.info/Elements/a/> ;
    rdfs:subPropertyOf <http://rdaregistry.info/Elements/a/P50131> ;
    skos:definition "Relates an agent who provides consultation services, and often makes recommendations, for another agent that is represented as the creator of a work to a work."@en,
        "Met une personne, famille ou collectivité qui fournit des services de consultation et fait souvent des recommandations à une autre personne, famille ou collectivité représentée comme créatrice de l’œuvre en relation avec l’œuvre."@fr .

<http://rdaregistry.info/Elements/a/P50213> a rdf:Property ;
    rdfs:label "is film producer of"@en,
        "est le producteur de films de"@fr ;
    rdakit:instructionNumber "18.5" ;
    rdakit:toolkitDefinition "A work that involves a production responsibility for most of the business aspects of a film."@en,
        "Producteur responsable de la majeure partie des aspects financiers, techniques et artistiques d’un film."@fr ;
    rdakit:toolkitLabel "film producer of"@en,
        "producteur de films de"@fr ;
    reg:hasSubproperty <http://rdaregistry.info/Elements/a/datatype/P50213>,
        <http://rdaregistry.info/Elements/a/object/P50213> ;
    reg:hasUnconstrained <http://rdaregistry.info/Elements/u/P60033> ;
    reg:lexicalAlias <http://rdaregistry.info/Elements/a/filmProducerOf.en> ;
    reg:name "filmProducerOf"@en ;
    reg:status <http://metadataregistry.org/uri/RegStatus/1001> ;
    rdfs:domain <http://rdaregistry.info/Elements/c/C10002> ;
    rdfs:isDefinedBy <http://rdaregistry.info/Elements/a/> ;
    rdfs:subPropertyOf <http://rdaregistry.info/Elements/a/P50201> ;
    skos:definition "Relates a producer responsible for most of the business aspects of a film to a work."@en,
        "Met un producteur responsable de la majeure partie des aspects financiers, techniques et artistiques d’un film en relation avec l’œuvre."@fr .

<http://rdaregistry.info/Elements/a/P50214> a rdf:Property ;
    rdfs:label "is radio producer of"@en,
        "est le producteur d’émissions de radio de"@fr ;
    rdakit:instructionNumber "18.5" ;
    rdakit:toolkitDefinition "A work that involves a production responsibility for most of the business aspects of a radio program."@en,
        "Producteur responsable de la majeure partie des aspects financiers, techniques et artistiques d’une émission de radio."@fr ;
    rdakit:toolkitLabel "radio producer of"@en,
        "producteur d’émissions de radio de"@fr ;
    reg:hasSubproperty <http://rdaregistry.info/Elements/a/datatype/P50214>,
        <http://rdaregistry.info/Elements/a/object/P50214> ;
    reg:hasUnconstrained <http://rdaregistry.info/Elements/u/P60034> ;
    reg:lexicalAlias <http://rdaregistry.info/Elements/a/radioProducerOf.en> ;
    reg:name "radioProducerOf"@en ;
    reg:status <http://metadataregistry.org/uri/RegStatus/1001> ;
    rdfs:domain <http://rdaregistry.info/Elements/c/C10002> ;
    rdfs:isDefinedBy <http://rdaregistry.info/Elements/a/> ;
    rdfs:subPropertyOf <http://rdaregistry.info/Elements/a/P50201> ;
    skos:definition "Relates a producer responsible for most of the business aspects of a radio program to a work."@en,
        "Met un producteur responsable de la majeure partie des aspects financiers, techniques et artistiques d’une émission de radio en relation avec l’œuvre."@fr .

<http://rdaregistry.info/Elements/a/P50215> a rdf:Property ;
    rdfs:label "is television producer of"@en,
        "est le producteur d’émissions de télévision de"@fr ;
    rdakit:instructionNumber "18.5" ;
    rdakit:toolkitDefinition "A work that involves a production responsibility for most of the business aspects of a television program."@en,
        "Producteur responsable de la majeure partie des aspects financiers, techniques et artistiques d’une émission de télévision."@fr ;
    rdakit:toolkitLabel "television producer of"@en,
        "producteur d’émissions de télévision de"@fr ;
    reg:hasSubproperty <http://rdaregistry.info/Elements/a/datatype/P50215>,
        <http://rdaregistry.info/Elements/a/object/P50215> ;
    reg:hasUnconstrained <http://rdaregistry.info/Elements/u/P60035> ;
    reg:lexicalAlias <http://rdaregistry.info/Elements/a/televisionProducerOf.en> ;
    reg:name "televisionProducerOf"@en ;
    reg:status <http://metadataregistry.org/uri/RegStatus/1001> ;
    rdfs:domain <http://rdaregistry.info/Elements/c/C10002> ;
    rdfs:isDefinedBy <http://rdaregistry.info/Elements/a/> ;
    rdfs:subPropertyOf <http://rdaregistry.info/Elements/a/P50201> ;
    skos:definition "Relates a producer responsible for most of the business aspects of a television program to a work."@en,
        "Met un producteur responsable de la majeure partie des aspects financiers, techniques et artistiques d’une émission de télévision en relation avec l’œuvre."@fr .

<http://rdaregistry.info/Elements/a/P50216> a rdf:Property ;
    rdfs:label "is writer of added lyrics of"@en,
        "est l’auteur de paroles ajoutées de"@fr ;
    rdakit:instructionNumber "18.5" ;
    rdakit:seeAlso <http://rdaregistry.info/Elements/a/P50224> ;
    rdakit:toolkitDefinition "An expression of a musical work that incorporates a contribution of writing words added to an expression."@en,
        "Auteur de paroles ajoutées à une expression d’une œuvre musicale."@fr ;
    rdakit:toolkitLabel "writer of added lyrics of"@en,
        "auteur de paroles ajoutées de"@fr ;
    reg:hasSubproperty <http://rdaregistry.info/Elements/a/datatype/P50216>,
        <http://rdaregistry.info/Elements/a/object/P50216> ;
    reg:hasUnconstrained <http://rdaregistry.info/Elements/u/P60600> ;
    reg:lexicalAlias <http://rdaregistry.info/Elements/a/writerOfAddedLyricsOf.en> ;
    reg:name "writerOfAddedLyricsOf"@en ;
    reg:status <http://metadataregistry.org/uri/RegStatus/1001> ;
    rdfs:domain <http://rdaregistry.info/Elements/c/C10002> ;
    rdfs:isDefinedBy <http://rdaregistry.info/Elements/a/> ;
    rdfs:subPropertyOf <http://rdaregistry.info/Elements/a/P50138> ;
    skos:definition "Relates a writer of words added to an expression of a musical work to an expression."@en,
        "Met un auteur de paroles ajoutées à une expression d’une œuvre musicale en relation avec l’expression."@fr .

<http://rdaregistry.info/Elements/a/P50217> a rdf:Property ;
    rdfs:label "is voice actor of"@en,
        "est la voix de"@fr ;
    rdakit:instructionNumber "18.5" ;
    rdakit:toolkitDefinition "An expression that incorporates an acting contribution of providing the voice for characters in radio and audio productions and for animated characters in moving image works, as well as by providing voice-overs in radio and television commercials, dubbed expressions, etc."@en,
        "Acteur contribuant à une expression d’une œuvre en prêtant sa voix à des personnages dans des productions radiophoniques et audio et à des personnages animés dans des œuvres d’images animées, de même qu’en prêtant sa voix hors champ dans des messages publicitaires à la radio et à la télévision, du doublage, etc."@fr ;
    rdakit:toolkitLabel "voice actor of"@en,
        "voix de"@fr ;
    reg:hasSubproperty <http://rdaregistry.info/Elements/a/datatype/P50217>,
        <http://rdaregistry.info/Elements/a/object/P50217> ;
    reg:hasUnconstrained <http://rdaregistry.info/Elements/u/P60027> ;
    reg:lexicalAlias <http://rdaregistry.info/Elements/a/voiceActorOf.en> ;
    reg:name "voiceActorOf"@en ;
    reg:status <http://metadataregistry.org/uri/RegStatus/1001> ;
    rdfs:domain <http://rdaregistry.info/Elements/c/C10002> ;
    rdfs:isDefinedBy <http://rdaregistry.info/Elements/a/> ;
    rdfs:subPropertyOf <http://rdaregistry.info/Elements/a/P50071> ;
    skos:definition "Relates an actor contributing to an expression of a work by providing the voice for characters in radio and audio productions and for animated characters in moving image works, as well as by providing voice-overs in radio and television commercials, dubbed expressions, etc., to an expression."@en,
        "Met un acteur contribuant à une expression d’une œuvre en prêtant sa voix à des personnages dans des productions radiophoniques et audio et à des personnages animés dans des œuvres d’images animées, de même qu’en prêtant sa voix hors champ dans des messages publicitaires à la radio et à la télévision, du doublage, etc. en relation avec l’expression."@fr .

<http://rdaregistry.info/Elements/a/P50221> a rdf:Property ;
    rdfs:label "is landscape architect of"@en,
        "est l’architecte paysagiste de"@fr ;
    rdakit:instructionNumber "18.5" ;
    rdakit:toolkitDefinition "A landscape work that involves an architectural responsibility."@en,
        "Architecte responsable de la création d’œuvres paysagères."@fr ;
    rdakit:toolkitLabel "landscape architect of"@en,
        "architecte paysagiste de"@fr ;
    reg:hasSubproperty <http://rdaregistry.info/Elements/a/datatype/P50221>,
        <http://rdaregistry.info/Elements/a/object/P50221> ;
    reg:hasUnconstrained <http://rdaregistry.info/Elements/u/P60704> ;
    reg:lexicalAlias <http://rdaregistry.info/Elements/a/landscapeArchitectOf.en> ;
    reg:name "landscapeArchitectOf"@en ;
    reg:status <http://metadataregistry.org/uri/RegStatus/1001> ;
    rdfs:domain <http://rdaregistry.info/Elements/c/C10002> ;
    rdfs:isDefinedBy <http://rdaregistry.info/Elements/a/> ;
    rdfs:subPropertyOf <http://rdaregistry.info/Elements/a/P50196> ;
    skos:definition "Relates an architect responsible for creating landscape works to a work."@en,
        "Met un architecte responsable de la création d’œuvres paysagères en relation avec l’œuvre."@fr .

<http://rdaregistry.info/Elements/a/P50222> a rdf:Property ;
    rdfs:label "is sculptor of"@en,
        "est le sculpteur de"@fr ;
    rdakit:instructionNumber "18.5" ;
    rdakit:toolkitDefinition "A three-dimensional work that involves an artistic responsibility for modeling, carving, or similar technique."@en,
        "Artiste responsable de la création d’une œuvre tridimensionnelle par le modelage, la taille ou une technique similaire."@fr ;
    rdakit:toolkitLabel "sculptor of"@en,
        "sculpteur de"@fr ;
    reg:hasSubproperty <http://rdaregistry.info/Elements/a/datatype/P50222>,
        <http://rdaregistry.info/Elements/a/object/P50222> ;
    reg:hasUnconstrained <http://rdaregistry.info/Elements/u/P60705> ;
    reg:lexicalAlias <http://rdaregistry.info/Elements/a/sculptorOf.en> ;
    reg:name "sculptorOf"@en ;
    reg:status <http://metadataregistry.org/uri/RegStatus/1001> ;
    rdfs:domain <http://rdaregistry.info/Elements/c/C10002> ;
    rdfs:isDefinedBy <http://rdaregistry.info/Elements/a/> ;
    rdfs:subPropertyOf <http://rdaregistry.info/Elements/a/P50192> ;
    skos:definition "Relates an artist responsible for creating a three-dimensional work by modeling, carving, or similar technique to a work."@en,
        "Met un artiste responsable de la création d’une œuvre tridimensionnelle par le modelage, la taille ou une technique similaire en relation avec l’œuvre."@fr .

<http://rdaregistry.info/Elements/a/P50223> a rdf:Property ;
    rdfs:label "is screenwriter of"@en,
        "est le scénariste de"@fr ;
    rdakit:instructionNumber "18.5" ;
    rdakit:toolkitDefinition "A work that involves an authoring responsibility for a screenplay, script, or scene."@en,
        "Auteur d’un scénario, d’un script ou d’une scène."@fr ;
    rdakit:toolkitLabel "screenwriter of"@en,
        "scénariste de"@fr ;
    reg:hasSubproperty <http://rdaregistry.info/Elements/a/datatype/P50223>,
        <http://rdaregistry.info/Elements/a/object/P50223> ;
    reg:hasUnconstrained <http://rdaregistry.info/Elements/u/P60706> ;
    reg:lexicalAlias <http://rdaregistry.info/Elements/a/screenwriterOf.en> ;
    reg:name "screenwriterOf"@en ;
    reg:status <http://metadataregistry.org/uri/RegStatus/1001> ;
    rdfs:domain <http://rdaregistry.info/Elements/c/C10002> ;
    rdfs:isDefinedBy <http://rdaregistry.info/Elements/a/> ;
    rdfs:subPropertyOf <http://rdaregistry.info/Elements/a/P50195> ;
    skos:definition "Relates an author of a screenplay, script, or scene to a work."@en,
        "Met un auteur d’un scénario, d’un script ou d’une scène en relation avec l’œuvre."@fr .

<http://rdaregistry.info/Elements/a/P50226> a rdf:Property ;
    rdfs:label "is sponsoring body of"@en,
        "est le commanditaire de"@fr ;
    rdakit:instructionNumber "18.5" ;
    rdakit:toolkitDefinition "A work that involves a responsibility for sponsoring some aspect of a work, e.g., funding research, sponsoring an event."@en,
        "Personne, famille ou collectivité commanditant certains aspects d’une œuvre, par exemple, le financement de la recherche, le parrainage d’un événement."@fr ;
    rdakit:toolkitLabel "sponsoring body of"@en,
        "commanditaire de"@fr ;
    reg:hasSubproperty <http://rdaregistry.info/Elements/a/datatype/P50226>,
        <http://rdaregistry.info/Elements/a/object/P50226> ;
    reg:hasUnconstrained <http://rdaregistry.info/Elements/u/P60675> ;
    reg:lexicalAlias <http://rdaregistry.info/Elements/a/sponsoringBodyOf.en> ;
    reg:name "sponsoringBodyOf"@en ;
    reg:status <http://metadataregistry.org/uri/RegStatus/1001> ;
    rdfs:domain <http://rdaregistry.info/Elements/c/C10002> ;
    rdfs:isDefinedBy <http://rdaregistry.info/Elements/a/> ;
    rdfs:subPropertyOf <http://rdaregistry.info/Elements/a/P50131> ;
    skos:definition "Relates an agent sponsoring some aspect of a work, e.g., funding research, sponsoring an event, to a work."@en,
        "Met une personne, famille ou collectivité commanditant certains aspects d’une œuvre, par exemple, le financement de la recherche, le parrainage d’un événement, en relation avec l’œuvre."@fr .

<http://rdaregistry.info/Elements/a/P50261> a rdf:Property ;
    rdfs:label "is on-screen participant of"@en ;
    rdakit:instructionNumber "18.5" ;
    rdakit:seeAlso <http://rdaregistry.info/Elements/a/P50072> ;
    rdakit:toolkitDefinition "An expression of a nonfiction moving image work that incorporates a contribution of taking an active role as a participant."@en ;
    rdakit:toolkitLabel "on-screen participant of"@en ;
    reg:hasSubproperty <http://rdaregistry.info/Elements/a/datatype/P50261>,
        <http://rdaregistry.info/Elements/a/object/P50261> ;
    reg:hasUnconstrained <http://rdaregistry.info/Elements/u/P60825> ;
    reg:lexicalAlias <http://rdaregistry.info/Elements/a/onScreenParticipantOf.en> ;
    reg:name "onscreenParticipantOf"@en ;
    reg:status <http://metadataregistry.org/uri/RegStatus/1001> ;
    rdfs:domain <http://rdaregistry.info/Elements/c/C10002> ;
    rdfs:isDefinedBy <http://rdaregistry.info/Elements/a/> ;
    rdfs:subPropertyOf <http://rdaregistry.info/Elements/a/P50161> ;
    skos:definition "Relates an agent contributing to an expression of a nonfiction moving image work by taking an active role as a participant to an expression."@en .

<http://rdaregistry.info/Elements/a/P50293> a rdf:Property ;
    rdfs:label "is remix artist of"@en ;
    rdakit:instructionNumber "18.5" ;
    rdakit:seeAlso <http://rdaregistry.info/Elements/a/P50298> ;
    rdakit:toolkitDefinition "An audio work created by manipulating, recombining, mixing, and reproducing previously recorded sounds."@en ;
    rdakit:toolkitLabel "remix artist of"@en ;
    reg:hasSubproperty <http://rdaregistry.info/Elements/a/datatype/P50293>,
        <http://rdaregistry.info/Elements/a/object/P50293> ;
    reg:hasUnconstrained <http://rdaregistry.info/Elements/u/P60881> ;
    reg:lexicalAlias <http://rdaregistry.info/Elements/a/remixArtistOf.en> ;
    reg:name "remixArtistOf"@en ;
    reg:status <http://metadataregistry.org/uri/RegStatus/1001> ;
    rdfs:domain <http://rdaregistry.info/Elements/c/C10002> ;
    rdfs:isDefinedBy <http://rdaregistry.info/Elements/a/> ;
    rdfs:subPropertyOf <http://rdaregistry.info/Elements/a/P50204> ;
    skos:definition "Relates an agent to an audio work created by manipulating, recombining, mixing, and reproducing previously recorded sounds."@en ;
    skos:scopeNote "Remixing activities that do not substantially change the nature and content of the original work, and mixing recorded tracks together to appear as one continuous track are excluded."@en .

<http://rdaregistry.info/Elements/a/P50297> a rdf:Property ;
    rdfs:label "is mixing engineer of"@en ;
    rdakit:instructionNumber "18.5" ;
    rdakit:seeAlso <http://rdaregistry.info/Elements/a/P50293> ;
    rdakit:toolkitDefinition "An expression of a work that incorporates a contribution to the audio content of manipulating, mixing and assembling the multiple tracks of a recording."@en ;
    rdakit:toolkitLabel "mixing engineer of"@en ;
    reg:hasSubproperty <http://rdaregistry.info/Elements/a/datatype/P50297>,
        <http://rdaregistry.info/Elements/a/object/P50297> ;
    reg:hasUnconstrained <http://rdaregistry.info/Elements/u/P60885> ;
    reg:lexicalAlias <http://rdaregistry.info/Elements/a/mixingEngineerOf.en> ;
    reg:name "mixingEngineerOf"@en ;
    reg:status <http://metadataregistry.org/uri/RegStatus/1001> ;
    rdfs:domain <http://rdaregistry.info/Elements/c/C10002> ;
    rdfs:isDefinedBy <http://rdaregistry.info/Elements/a/> ;
    rdfs:subPropertyOf <http://rdaregistry.info/Elements/a/P50296> ;
    skos:definition "Relates an agent to an expression of a work that incorporates a contribution to the audio content of manipulating, mixing and assembling the multiple tracks of a recording."@en ;
    skos:scopeNote "Remixing activities that substantially change the nature and content of the original work, resulting in a new work, are excluded."@en .

<http://rdaregistry.info/Elements/a/P50298> a rdf:Property ;
    rdfs:label "is DJ of"@en ;
    rdakit:instructionNumber "18.5" ;
    rdakit:seeAlso <http://rdaregistry.info/Elements/a/P50297> ;
    rdakit:toolkitDefinition "An expression of a work that incorporates a contribution of mixing recorded tracks together during a live performance or in a recording studio to appear as one continuous track."@en ;
    rdakit:toolkitLabel "DJ of"@en ;
    reg:hasSubproperty <http://rdaregistry.info/Elements/a/datatype/P50298>,
        <http://rdaregistry.info/Elements/a/object/P50298> ;
    reg:hasUnconstrained <http://rdaregistry.info/Elements/u/P60886> ;
    reg:lexicalAlias <http://rdaregistry.info/Elements/a/DJOf.en> ;
    reg:name "DJOf"@en ;
    reg:status <http://metadataregistry.org/uri/RegStatus/1001> ;
    rdfs:domain <http://rdaregistry.info/Elements/c/C10002> ;
    rdfs:isDefinedBy <http://rdaregistry.info/Elements/a/> ;
    rdfs:subPropertyOf <http://rdaregistry.info/Elements/a/P50161> ;
    skos:definition "Relates an agent to an expression of a work that incorporates a contribution of mixing recorded tracks together during a live performance or in a recording studio to appear as one continuous track."@en ;
    skos:scopeNote "An expression of a work that incorporates a contribution of mixing recorded tracks together during a live performance or in a recording studio to appear as one continuous track."@en .

<http://rdaregistry.info/Elements/a/P50311> a rdf:Property ;
    rdfs:label "has related work (person)"@en ;
    reg:hasSubproperty <http://rdaregistry.info/Elements/a/datatype/P50311>,
        <http://rdaregistry.info/Elements/a/object/P50311> ;
    reg:lexicalAlias <http://rdaregistry.info/Elements/a/relatedWorkPerson.en> ;
    reg:name "relatedWorkPerson"@en ;
    reg:status <http://metadataregistry.org/uri/RegStatus/1001> ;
    rdfs:domain <http://rdaregistry.info/Elements/c/C10004> ;
    rdfs:isDefinedBy <http://rdaregistry.info/Elements/a/> ;
    rdfs:subPropertyOf <http://rdaregistry.info/Elements/a/P50305>,
        <http://rdaregistry.info/Elements/a/P50310> ;
    skos:definition "Relates a person to a work associated with a person being described."@en .

<http://rdaregistry.info/Elements/a/P50312> a rdf:Property ;
    rdfs:label "has related expression (person)"@en ;
    reg:hasSubproperty <http://rdaregistry.info/Elements/a/datatype/P50312>,
        <http://rdaregistry.info/Elements/a/object/P50312> ;
    reg:lexicalAlias <http://rdaregistry.info/Elements/a/relatedExpressionPerson.en> ;
    reg:name "relatedExpressionPerson"@en ;
    reg:status <http://metadataregistry.org/uri/RegStatus/1001> ;
    rdfs:domain <http://rdaregistry.info/Elements/c/C10004> ;
    rdfs:isDefinedBy <http://rdaregistry.info/Elements/a/> ;
    rdfs:subPropertyOf <http://rdaregistry.info/Elements/a/P50306>,
        <http://rdaregistry.info/Elements/a/P50310> ;
    skos:definition "Relates a person to an expression associated with a person being described."@en .

<http://rdaregistry.info/Elements/a/P50313> a rdf:Property ;
    rdfs:label "has related manifestation (person)"@en ;
    reg:hasSubproperty <http://rdaregistry.info/Elements/a/datatype/P50313>,
        <http://rdaregistry.info/Elements/a/object/P50313> ;
    reg:lexicalAlias <http://rdaregistry.info/Elements/a/relatedManifestationPerson.en> ;
    reg:name "relatedManifestationPerson"@en ;
    reg:status <http://metadataregistry.org/uri/RegStatus/1001> ;
    rdfs:domain <http://rdaregistry.info/Elements/c/C10004> ;
    rdfs:isDefinedBy <http://rdaregistry.info/Elements/a/> ;
    rdfs:subPropertyOf <http://rdaregistry.info/Elements/a/P50307>,
        <http://rdaregistry.info/Elements/a/P50310> ;
    skos:definition "Relates a person to a manifestation associated with a person being described."@en .

<http://rdaregistry.info/Elements/a/P50314> a rdf:Property ;
    rdfs:label "has related item (person)"@en ;
    reg:hasSubproperty <http://rdaregistry.info/Elements/a/datatype/P50314>,
        <http://rdaregistry.info/Elements/a/object/P50314> ;
    reg:lexicalAlias <http://rdaregistry.info/Elements/a/relatedItemPerson.en> ;
    reg:name "relatedItemPerson"@en ;
    reg:status <http://metadataregistry.org/uri/RegStatus/1001> ;
    rdfs:domain <http://rdaregistry.info/Elements/c/C10004> ;
    rdfs:isDefinedBy <http://rdaregistry.info/Elements/a/> ;
    rdfs:subPropertyOf <http://rdaregistry.info/Elements/a/P50308>,
        <http://rdaregistry.info/Elements/a/P50310> ;
    skos:definition "Relates a person to an item associated with a person being described."@en .

<http://rdaregistry.info/Elements/a/P50316> a rdf:Property ;
    rdfs:label "has related person (person)"@en ;
    reg:hasSubproperty <http://rdaregistry.info/Elements/a/datatype/P50316>,
        <http://rdaregistry.info/Elements/a/object/P50316> ;
    reg:lexicalAlias <http://rdaregistry.info/Elements/a/relatedPersonPerson.en> ;
    reg:name "relatedPersonPerson"@en ;
    reg:status <http://metadataregistry.org/uri/RegStatus/1001> ;
    rdfs:domain <http://rdaregistry.info/Elements/c/C10004> ;
    rdfs:isDefinedBy <http://rdaregistry.info/Elements/a/> ;
    rdfs:subPropertyOf <http://rdaregistry.info/Elements/a/P50220>,
        <http://rdaregistry.info/Elements/a/P50315> ;
    skos:definition "Relates a person to a person who is associated with a person being described."@en .

<http://rdaregistry.info/Elements/a/P50317> a rdf:Property ;
    rdfs:label "has related family (person)"@en ;
    reg:hasSubproperty <http://rdaregistry.info/Elements/a/datatype/P50317>,
        <http://rdaregistry.info/Elements/a/object/P50317> ;
    reg:lexicalAlias <http://rdaregistry.info/Elements/a/relatedFamilyPerson.en> ;
    reg:name "relatedFamilyPerson"@en ;
    reg:status <http://metadataregistry.org/uri/RegStatus/1001> ;
    rdfs:domain <http://rdaregistry.info/Elements/c/C10004> ;
    rdfs:isDefinedBy <http://rdaregistry.info/Elements/a/> ;
    rdfs:subPropertyOf <http://rdaregistry.info/Elements/a/P50219>,
        <http://rdaregistry.info/Elements/a/P50345> ;
    skos:definition "Relates a person to a family associated with a person being described."@en .

<http://rdaregistry.info/Elements/a/P50318> a rdf:Property ;
    rdfs:label "has related corporate body (person)"@en ;
    reg:hasSubproperty <http://rdaregistry.info/Elements/a/datatype/P50318>,
        <http://rdaregistry.info/Elements/a/object/P50318> ;
    reg:lexicalAlias <http://rdaregistry.info/Elements/a/relatedCorporateBodyPerson.en> ;
    reg:name "relatedCorporateBodyPerson"@en ;
    reg:status <http://metadataregistry.org/uri/RegStatus/1001> ;
    rdfs:domain <http://rdaregistry.info/Elements/c/C10004> ;
    rdfs:isDefinedBy <http://rdaregistry.info/Elements/a/> ;
    rdfs:subPropertyOf <http://rdaregistry.info/Elements/a/P50218>,
        <http://rdaregistry.info/Elements/a/P50345> ;
    skos:definition "Relates a person to a corporate body associated with a person being described."@en .

<http://rdaregistry.info/Elements/a/P50320> a rdf:Property ;
    rdfs:label "has related work (family)"@en ;
    reg:hasSubproperty <http://rdaregistry.info/Elements/a/datatype/P50320>,
        <http://rdaregistry.info/Elements/a/object/P50320> ;
    reg:lexicalAlias <http://rdaregistry.info/Elements/a/relatedWorkFamily.en> ;
    reg:name "relatedWorkFamily"@en ;
    reg:status <http://metadataregistry.org/uri/RegStatus/1001> ;
    rdfs:domain <http://rdaregistry.info/Elements/c/C10008> ;
    rdfs:isDefinedBy <http://rdaregistry.info/Elements/a/> ;
    rdfs:subPropertyOf <http://rdaregistry.info/Elements/a/P50319>,
        <http://rdaregistry.info/Elements/a/P50357> ;
    skos:definition "Relates a family to a work associated with a family being described."@en .

<http://rdaregistry.info/Elements/a/P50321> a rdf:Property ;
    rdfs:label "has related expression (family)"@en ;
    reg:hasSubproperty <http://rdaregistry.info/Elements/a/datatype/P50321>,
        <http://rdaregistry.info/Elements/a/object/P50321> ;
    reg:lexicalAlias <http://rdaregistry.info/Elements/a/relatedExpressionFamily.en> ;
    reg:name "relatedExpressionFamily"@en ;
    reg:status <http://metadataregistry.org/uri/RegStatus/1001> ;
    rdfs:domain <http://rdaregistry.info/Elements/c/C10008> ;
    rdfs:isDefinedBy <http://rdaregistry.info/Elements/a/> ;
    rdfs:subPropertyOf <http://rdaregistry.info/Elements/a/P50319>,
        <http://rdaregistry.info/Elements/a/P50361> ;
    skos:definition "Relates a family to an expression associated with a family being described."@en .

<http://rdaregistry.info/Elements/a/P50322> a rdf:Property ;
    rdfs:label "has related manifestation (family)"@en ;
    reg:hasSubproperty <http://rdaregistry.info/Elements/a/datatype/P50322>,
        <http://rdaregistry.info/Elements/a/object/P50322> ;
    reg:lexicalAlias <http://rdaregistry.info/Elements/a/relatedManifestationFamily.en> ;
    reg:name "relatedManifestationFamily"@en ;
    reg:status <http://metadataregistry.org/uri/RegStatus/1001> ;
    rdfs:domain <http://rdaregistry.info/Elements/c/C10008> ;
    rdfs:isDefinedBy <http://rdaregistry.info/Elements/a/> ;
    rdfs:subPropertyOf <http://rdaregistry.info/Elements/a/P50319>,
        <http://rdaregistry.info/Elements/a/P50364> ;
    skos:definition "Relates a family to a manifestation associated with a family being described."@en .

<http://rdaregistry.info/Elements/a/P50323> a rdf:Property ;
    rdfs:label "has related item (family)"@en ;
    reg:hasSubproperty <http://rdaregistry.info/Elements/a/datatype/P50323>,
        <http://rdaregistry.info/Elements/a/object/P50323> ;
    reg:lexicalAlias <http://rdaregistry.info/Elements/a/relatedItemFamily.en> ;
    reg:name "relatedItemFamily"@en ;
    reg:status <http://metadataregistry.org/uri/RegStatus/1001> ;
    rdfs:domain <http://rdaregistry.info/Elements/c/C10008> ;
    rdfs:isDefinedBy <http://rdaregistry.info/Elements/a/> ;
    rdfs:subPropertyOf <http://rdaregistry.info/Elements/a/P50319>,
        <http://rdaregistry.info/Elements/a/P50363> ;
    skos:definition "Relates a family to an item associated with a family being described."@en .

<http://rdaregistry.info/Elements/a/P50325> a rdf:Property ;
    rdfs:label "has related person (family)"@en ;
    reg:hasSubproperty <http://rdaregistry.info/Elements/a/datatype/P50325>,
        <http://rdaregistry.info/Elements/a/object/P50325> ;
    reg:lexicalAlias <http://rdaregistry.info/Elements/a/relatedPersonFamily.en> ;
    reg:name "relatedPersonFamily"@en ;
    reg:status <http://metadataregistry.org/uri/RegStatus/1001> ;
    rdfs:domain <http://rdaregistry.info/Elements/c/C10008> ;
    rdfs:isDefinedBy <http://rdaregistry.info/Elements/a/> ;
    rdfs:subPropertyOf <http://rdaregistry.info/Elements/a/P50324>,
        <http://rdaregistry.info/Elements/a/P50365> ;
    skos:definition "Relates a family to a person who is associated with a family being described."@en .

<http://rdaregistry.info/Elements/a/P50326> a rdf:Property ;
    rdfs:label "has related family (family)"@en ;
    reg:hasSubproperty <http://rdaregistry.info/Elements/a/datatype/P50326>,
        <http://rdaregistry.info/Elements/a/object/P50326> ;
    reg:lexicalAlias <http://rdaregistry.info/Elements/a/relatedFamilyFamily.en> ;
    reg:name "relatedFamilyFamily"@en ;
    reg:status <http://metadataregistry.org/uri/RegStatus/1001> ;
    rdfs:domain <http://rdaregistry.info/Elements/c/C10008> ;
    rdfs:isDefinedBy <http://rdaregistry.info/Elements/a/> ;
    rdfs:subPropertyOf <http://rdaregistry.info/Elements/a/P50353>,
        <http://rdaregistry.info/Elements/a/P50362> ;
    skos:definition "Relates a family to a family associated with a family being described."@en .

<http://rdaregistry.info/Elements/a/P50327> a rdf:Property ;
    rdfs:label "has related corporate body (family)"@en ;
    reg:hasSubproperty <http://rdaregistry.info/Elements/a/datatype/P50327>,
        <http://rdaregistry.info/Elements/a/object/P50327> ;
    reg:lexicalAlias <http://rdaregistry.info/Elements/a/relatedCorporateBodyFamily.en> ;
    reg:name "relatedCorporateBodyFamily"@en ;
    reg:status <http://metadataregistry.org/uri/RegStatus/1001> ;
    rdfs:domain <http://rdaregistry.info/Elements/c/C10008> ;
    rdfs:isDefinedBy <http://rdaregistry.info/Elements/a/> ;
    rdfs:subPropertyOf <http://rdaregistry.info/Elements/a/P50353>,
        <http://rdaregistry.info/Elements/a/P50359> ;
    skos:definition "Relates a family to a corporate body associated with a family being described."@en .

<http://rdaregistry.info/Elements/a/P50329> a rdf:Property ;
    rdfs:label "has related work (corporate body)"@en ;
    reg:hasSubproperty <http://rdaregistry.info/Elements/a/datatype/P50329>,
        <http://rdaregistry.info/Elements/a/object/P50329> ;
    reg:lexicalAlias <http://rdaregistry.info/Elements/a/relatedWorkCorporateBody.en> ;
    reg:name "relatedWorkCorporateBody"@en ;
    reg:status <http://metadataregistry.org/uri/RegStatus/1001> ;
    rdfs:domain <http://rdaregistry.info/Elements/c/C10005> ;
    rdfs:isDefinedBy <http://rdaregistry.info/Elements/a/> ;
    rdfs:subPropertyOf <http://rdaregistry.info/Elements/a/P50305>,
        <http://rdaregistry.info/Elements/a/P50357> ;
    skos:definition "Relates a corporate body to a work associated with a corporate body being described."@en .

<http://rdaregistry.info/Elements/a/P50330> a rdf:Property ;
    rdfs:label "has related expression (corporate body)"@en ;
    reg:hasSubproperty <http://rdaregistry.info/Elements/a/datatype/P50330>,
        <http://rdaregistry.info/Elements/a/object/P50330> ;
    reg:lexicalAlias <http://rdaregistry.info/Elements/a/relatedExpressionCorporateBody.en> ;
    reg:name "relatedExpressionCorporateBody"@en ;
    reg:status <http://metadataregistry.org/uri/RegStatus/1001> ;
    rdfs:domain <http://rdaregistry.info/Elements/c/C10005> ;
    rdfs:isDefinedBy <http://rdaregistry.info/Elements/a/> ;
    rdfs:subPropertyOf <http://rdaregistry.info/Elements/a/P50306>,
        <http://rdaregistry.info/Elements/a/P50361> ;
    skos:definition "Relates a corporate body to an expression associated with a corporate body being described."@en .

<http://rdaregistry.info/Elements/a/P50331> a rdf:Property ;
    rdfs:label "has related manifestation (corporate body)"@en ;
    reg:hasSubproperty <http://rdaregistry.info/Elements/a/datatype/P50331>,
        <http://rdaregistry.info/Elements/a/object/P50331> ;
    reg:lexicalAlias <http://rdaregistry.info/Elements/a/relatedManifestationCorporateBody.en> ;
    reg:name "relatedManifestationCorporateBody"@en ;
    reg:status <http://metadataregistry.org/uri/RegStatus/1001> ;
    rdfs:domain <http://rdaregistry.info/Elements/c/C10005> ;
    rdfs:isDefinedBy <http://rdaregistry.info/Elements/a/> ;
    rdfs:subPropertyOf <http://rdaregistry.info/Elements/a/P50307>,
        <http://rdaregistry.info/Elements/a/P50364> ;
    skos:definition "Relates a corporate body to a manifestation associated with a corporate body being described."@en .

<http://rdaregistry.info/Elements/a/P50332> a rdf:Property ;
    rdfs:label "has related item (corporate body)"@en ;
    reg:hasSubproperty <http://rdaregistry.info/Elements/a/datatype/P50332>,
        <http://rdaregistry.info/Elements/a/object/P50332> ;
    reg:lexicalAlias <http://rdaregistry.info/Elements/a/relatedItemCorporateBody.en> ;
    reg:name "relatedItemCorporateBody"@en ;
    reg:status <http://metadataregistry.org/uri/RegStatus/1001> ;
    rdfs:domain <http://rdaregistry.info/Elements/c/C10005> ;
    rdfs:isDefinedBy <http://rdaregistry.info/Elements/a/> ;
    rdfs:subPropertyOf <http://rdaregistry.info/Elements/a/P50308>,
        <http://rdaregistry.info/Elements/a/P50363> ;
    skos:definition "Relates a corporate body to an item associated with a corporate body described."@en .

<http://rdaregistry.info/Elements/a/P50334> a rdf:Property ;
    rdfs:label "has related person (corporate body)"@en ;
    reg:hasSubproperty <http://rdaregistry.info/Elements/a/datatype/P50334>,
        <http://rdaregistry.info/Elements/a/object/P50334> ;
    reg:lexicalAlias <http://rdaregistry.info/Elements/a/relatedPersonCorporateBody.en> ;
    reg:name "relatedPersonCorporateBody"@en ;
    reg:status <http://metadataregistry.org/uri/RegStatus/1001> ;
    rdfs:domain <http://rdaregistry.info/Elements/c/C10005> ;
    rdfs:isDefinedBy <http://rdaregistry.info/Elements/a/> ;
    rdfs:subPropertyOf <http://rdaregistry.info/Elements/a/P50333>,
        <http://rdaregistry.info/Elements/a/P50365> ;
    skos:definition "Relates a corporate body to a person who is associated with a corporate body being described."@en .

<http://rdaregistry.info/Elements/a/P50335> a rdf:Property ;
    rdfs:label "has related family (corporate body)"@en ;
    reg:hasSubproperty <http://rdaregistry.info/Elements/a/datatype/P50335>,
        <http://rdaregistry.info/Elements/a/object/P50335> ;
    reg:lexicalAlias <http://rdaregistry.info/Elements/a/relatedFamilyCorporateBody.en> ;
    reg:name "relatedFamilyCorporateBody"@en ;
    reg:status <http://metadataregistry.org/uri/RegStatus/1001> ;
    rdfs:domain <http://rdaregistry.info/Elements/c/C10005> ;
    rdfs:isDefinedBy <http://rdaregistry.info/Elements/a/> ;
    rdfs:subPropertyOf <http://rdaregistry.info/Elements/a/P50333>,
        <http://rdaregistry.info/Elements/a/P50362> ;
    skos:definition "Relates a corporate body to a family associated with a corporate body being described."@en .

<http://rdaregistry.info/Elements/a/P50336> a rdf:Property ;
    rdfs:label "has related corporate body (corporate body)"@en ;
    reg:hasSubproperty <http://rdaregistry.info/Elements/a/datatype/P50336>,
        <http://rdaregistry.info/Elements/a/object/P50336> ;
    reg:lexicalAlias <http://rdaregistry.info/Elements/a/relatedCorporateBodyCorporateBody.en> ;
    reg:name "relatedCorporateBodyCorporateBody"@en ;
    reg:status <http://metadataregistry.org/uri/RegStatus/1001> ;
    rdfs:domain <http://rdaregistry.info/Elements/c/C10005> ;
    rdfs:isDefinedBy <http://rdaregistry.info/Elements/a/> ;
    rdfs:subPropertyOf <http://rdaregistry.info/Elements/a/P50333>,
        <http://rdaregistry.info/Elements/a/P50359> ;
    skos:definition "Relates a corporate body to a corporate body associated with a corporate body being described."@en .

<http://rdaregistry.info/Elements/a/P50346> a rdf:Property ;
    rdfs:label "has related place (person)"@en ;
    reg:hasSubproperty <http://rdaregistry.info/Elements/a/datatype/P50346>,
        <http://rdaregistry.info/Elements/a/object/P50346> ;
    reg:lexicalAlias <http://rdaregistry.info/Elements/a/relatedPlacePerson.en> ;
    reg:name "relatedPlacePerson"@en ;
    reg:status <http://metadataregistry.org/uri/RegStatus/1001> ;
    rdfs:domain <http://rdaregistry.info/Elements/c/C10004> ;
    rdfs:isDefinedBy <http://rdaregistry.info/Elements/a/> ;
    rdfs:subPropertyOf <http://rdaregistry.info/Elements/a/P50310>,
        <http://rdaregistry.info/Elements/a/P50338> ;
    skos:definition "Relates a person to a place associated with a person."@en .

<http://rdaregistry.info/Elements/a/P50347> a rdf:Property ;
    rdfs:label "has related time-span (person)"@en ;
    reg:hasSubproperty <http://rdaregistry.info/Elements/a/datatype/P50347>,
        <http://rdaregistry.info/Elements/a/object/P50347> ;
    reg:lexicalAlias <http://rdaregistry.info/Elements/a/relatedTimespanPerson.en> ;
    reg:name "relatedTimespanPerson"@en ;
    reg:status <http://metadataregistry.org/uri/RegStatus/1001> ;
    rdfs:domain <http://rdaregistry.info/Elements/c/C10004> ;
    rdfs:isDefinedBy <http://rdaregistry.info/Elements/a/> ;
    rdfs:subPropertyOf <http://rdaregistry.info/Elements/a/P50310>,
        <http://rdaregistry.info/Elements/a/P50339> ;
    skos:definition "Relates a person to a time-span associated with a person."@en .

<http://rdaregistry.info/Elements/a/P50348> a rdf:Property ;
    rdfs:label "has related nomen (person)"@en ;
    reg:hasSubproperty <http://rdaregistry.info/Elements/a/datatype/P50348>,
        <http://rdaregistry.info/Elements/a/object/P50348> ;
    reg:lexicalAlias <http://rdaregistry.info/Elements/a/relatedNomenPerson.en> ;
    reg:name "relatedNomenPerson"@en ;
    reg:status <http://metadataregistry.org/uri/RegStatus/1001> ;
    rdfs:domain <http://rdaregistry.info/Elements/c/C10004> ;
    rdfs:isDefinedBy <http://rdaregistry.info/Elements/a/> ;
    rdfs:subPropertyOf <http://rdaregistry.info/Elements/a/P50310>,
        <http://rdaregistry.info/Elements/a/P50340> ;
    skos:definition "Relates a person to a nomen associated with a person."@en .

<http://rdaregistry.info/Elements/a/P50349> a rdf:Property ;
    rdfs:label "has related collective agent (corporate body)"@en ;
    reg:hasSubproperty <http://rdaregistry.info/Elements/a/datatype/P50349>,
        <http://rdaregistry.info/Elements/a/object/P50349> ;
    reg:lexicalAlias <http://rdaregistry.info/Elements/a/relatedCollectiveAgentCorporateBody.en> ;
    reg:name "relatedCollectiveAgentCorporateBody"@en ;
    reg:status <http://metadataregistry.org/uri/RegStatus/1001> ;
    rdfs:domain <http://rdaregistry.info/Elements/c/C10005> ;
    rdfs:isDefinedBy <http://rdaregistry.info/Elements/a/> ;
    rdfs:subPropertyOf <http://rdaregistry.info/Elements/a/P50328>,
        <http://rdaregistry.info/Elements/a/P50341> ;
    skos:definition "Relates a corporate body to a collective agent associated with a corporate body."@en .

<http://rdaregistry.info/Elements/a/P50350> a rdf:Property ;
    rdfs:label "has related place (corporate body)"@en ;
    reg:hasSubproperty <http://rdaregistry.info/Elements/a/datatype/P50350>,
        <http://rdaregistry.info/Elements/a/object/P50350> ;
    reg:lexicalAlias <http://rdaregistry.info/Elements/a/relatedPlaceCorporateBody.en> ;
    reg:name "relatedPlaceCorporateBody"@en ;
    reg:status <http://metadataregistry.org/uri/RegStatus/1001> ;
    rdfs:domain <http://rdaregistry.info/Elements/c/C10005> ;
    rdfs:isDefinedBy <http://rdaregistry.info/Elements/a/> ;
    rdfs:subPropertyOf <http://rdaregistry.info/Elements/a/P50328>,
        <http://rdaregistry.info/Elements/a/P50342> ;
    skos:definition "Relates a corporate body to a place associated with a corporate body."@en .

<http://rdaregistry.info/Elements/a/P50351> a rdf:Property ;
    rdfs:label "has related time-span (corporate body)"@en ;
    reg:hasSubproperty <http://rdaregistry.info/Elements/a/datatype/P50351>,
        <http://rdaregistry.info/Elements/a/object/P50351> ;
    reg:lexicalAlias <http://rdaregistry.info/Elements/a/relatedTimespanCorporateBody.en> ;
    reg:name "relatedTimespanCorporateBody"@en ;
    reg:status <http://metadataregistry.org/uri/RegStatus/1001> ;
    rdfs:domain <http://rdaregistry.info/Elements/c/C10005> ;
    rdfs:isDefinedBy <http://rdaregistry.info/Elements/a/> ;
    rdfs:subPropertyOf <http://rdaregistry.info/Elements/a/P50328>,
        <http://rdaregistry.info/Elements/a/P50343> ;
    skos:definition "Relates a corporate body to a time-span associated with a corporate body."@en .

<http://rdaregistry.info/Elements/a/P50352> a rdf:Property ;
    rdfs:label "has related nomen (corporate body)"@en ;
    reg:hasSubproperty <http://rdaregistry.info/Elements/a/datatype/P50352>,
        <http://rdaregistry.info/Elements/a/object/P50352> ;
    reg:lexicalAlias <http://rdaregistry.info/Elements/a/relatedNomenCorporateBody.en> ;
    reg:name "relatedNomenCorporateBody"@en ;
    reg:status <http://metadataregistry.org/uri/RegStatus/1001> ;
    rdfs:domain <http://rdaregistry.info/Elements/c/C10005> ;
    rdfs:isDefinedBy <http://rdaregistry.info/Elements/a/> ;
    rdfs:subPropertyOf <http://rdaregistry.info/Elements/a/P50328>,
        <http://rdaregistry.info/Elements/a/P50344> ;
    skos:definition "Relates a corporate body to a nomen associated with a corporate body."@en .

<http://rdaregistry.info/Elements/a/P50354> a rdf:Property ;
    rdfs:label "has related place (family)"@en ;
    reg:hasSubproperty <http://rdaregistry.info/Elements/a/datatype/P50354>,
        <http://rdaregistry.info/Elements/a/object/P50354> ;
    reg:lexicalAlias <http://rdaregistry.info/Elements/a/relatedPlaceFamily.en> ;
    reg:name "relatedPlaceFamily"@en ;
    reg:status <http://metadataregistry.org/uri/RegStatus/1001> ;
    rdfs:domain <http://rdaregistry.info/Elements/c/C10008> ;
    rdfs:isDefinedBy <http://rdaregistry.info/Elements/a/> ;
    rdfs:subPropertyOf <http://rdaregistry.info/Elements/a/P50319>,
        <http://rdaregistry.info/Elements/a/P50342> ;
    skos:definition "Relates a family to a place associated with a family."@en .

<http://rdaregistry.info/Elements/a/P50355> a rdf:Property ;
    rdfs:label "has related time-span (family)"@en ;
    reg:hasSubproperty <http://rdaregistry.info/Elements/a/datatype/P50355>,
        <http://rdaregistry.info/Elements/a/object/P50355> ;
    reg:lexicalAlias <http://rdaregistry.info/Elements/a/relatedTimespanFamily.en> ;
    reg:name "relatedTimespanFamily"@en ;
    reg:status <http://metadataregistry.org/uri/RegStatus/1001> ;
    rdfs:domain <http://rdaregistry.info/Elements/c/C10008> ;
    rdfs:isDefinedBy <http://rdaregistry.info/Elements/a/> ;
    rdfs:subPropertyOf <http://rdaregistry.info/Elements/a/P50319>,
        <http://rdaregistry.info/Elements/a/P50343> ;
    skos:definition "Relates a family to a time-span associated with a family."@en .

<http://rdaregistry.info/Elements/a/P50356> a rdf:Property ;
    rdfs:label "has related nomen (family)"@en ;
    reg:hasSubproperty <http://rdaregistry.info/Elements/a/datatype/P50356>,
        <http://rdaregistry.info/Elements/a/object/P50356> ;
    reg:lexicalAlias <http://rdaregistry.info/Elements/a/relatedNomenFamily.en> ;
    reg:name "relatedNomenFamily"@en ;
    reg:status <http://metadataregistry.org/uri/RegStatus/1001> ;
    rdfs:domain <http://rdaregistry.info/Elements/c/C10008> ;
    rdfs:isDefinedBy <http://rdaregistry.info/Elements/a/> ;
    rdfs:subPropertyOf <http://rdaregistry.info/Elements/a/P50319>,
        <http://rdaregistry.info/Elements/a/P50344> ;
    skos:definition "Relates a family to a nomen associated with a family."@en .

<http://rdaregistry.info/Elements/a/P50027> a rdf:Property ;
    rdfs:label "has officer"@en,
        "a pour titulaire"@fr ;
    rdakit:instructionNumber "29.5" ;
    rdakit:toolkitDefinition "A person holding an office in or commanding a corporate body."@en,
        "Una persona que tiene un cargo en la entidad corporativa."@es,
        "Personne qui exerce une fonction administrative ou officielle dans la collectivité."@fr ;
    rdakit:toolkitLabel "officer"@en,
        "funcionario"@es,
        "titulaire"@fr ;
    reg:hasSubproperty <http://rdaregistry.info/Elements/a/datatype/P50027>,
        <http://rdaregistry.info/Elements/a/object/P50027>,
        <http://rdaregistry.info/Elements/a/object/P50284>,
        <http://rdaregistry.info/Elements/a/object/P50285> ;
    reg:hasUnconstrained <http://rdaregistry.info/Elements/u/P60633> ;
    reg:lexicalAlias <http://rdaregistry.info/Elements/a/officer.en> ;
    reg:name "officer"@en ;
    reg:status <http://metadataregistry.org/uri/RegStatus/1001> ;
    rdfs:domain <http://rdaregistry.info/Elements/c/C10005> ;
    rdfs:isDefinedBy <http://rdaregistry.info/Elements/a/> ;
    skos:definition "Relates a corporate body to a person holding an office in or commanding a corporate body."@en,
        "Met une collectivité en relation avec une personne qui exerce une fonction administrative ou officielle dans la collectivité."@fr .

<http://rdaregistry.info/Elements/a/P50031> a rdf:Property ;
    rdfs:label "has place associated with corporate body"@en,
        "a pour lieu associé à la collectivité"@fr,
        "har ort förknippad med institutionen"@sv ;
    rdakit:instructionNumber "11.3" ;
    rdakit:toolkitDefinition "A significant location associated with a corporate body."@en,
        "Un lugar significativo asociado con una entidad corporativa."@es,
        "Localisation significative associée à une collectivité."@fr ;
    rdakit:toolkitLabel "place associated with corporate body"@en,
        "lugar asociado con la entidad corporativa"@es,
        "lieu associé à la collectivité"@fr,
        "ort förknippad med institutionen"@sv ;
    reg:hasSubproperty <http://rdaregistry.info/Elements/a/datatype/P50031> ;
    reg:hasUnconstrained <http://rdaregistry.info/Elements/u/P60325> ;
    reg:lexicalAlias <http://rdaregistry.info/Elements/a/placeAssociatedWithCorporateBody.en> ;
    reg:name "placeAssociatedWithCorporateBody"@en ;
    reg:status <http://metadataregistry.org/uri/RegStatus/1001> ;
    rdfs:domain <http://rdaregistry.info/Elements/c/C10005> ;
    rdfs:isDefinedBy <http://rdaregistry.info/Elements/a/> ;
    skos:definition "Relates a corporate body to a significant location associated with a corporate body."@en,
        "Met une collectivité en relation avec une localisation significative associée à une collectivité."@fr .

<http://rdaregistry.info/Elements/a/P50032> a rdf:Property ;
    rdfs:label "has name of corporate body"@en,
        "a pour nom de collectivité"@fr,
        "har institutionsnamn"@sv ;
    rdakit:instructionNumber "11.2" ;
    rdakit:toolkitDefinition "A word, character, or group of words and/or characters by which a corporate body is known."@en,
        "Una palabra, carácter o grupo de palabras y/o caracteres mediante los cuales se conoce una entidad corporativa."@es,
        "Mot, caractère ou groupe de mots et/ou de caractères sous lequel une collectivité est connue."@fr ;
    rdakit:toolkitLabel "name of corporate body"@en,
        "nombre de la entidad corporativa"@es,
        "nom de collectivité"@fr,
        "institutionsnamn"@sv ;
    reg:hasSubproperty <http://rdaregistry.info/Elements/a/P50041>,
        <http://rdaregistry.info/Elements/a/datatype/P50032> ;
    reg:hasUnconstrained <http://rdaregistry.info/Elements/u/P60368> ;
    reg:lexicalAlias <http://rdaregistry.info/Elements/a/nameOfCorporateBody.en> ;
    reg:name "nameOfCorporateBody"@en ;
    reg:status <http://metadataregistry.org/uri/RegStatus/1001> ;
    rdfs:domain <http://rdaregistry.info/Elements/c/C10005> ;
    rdfs:isDefinedBy <http://rdaregistry.info/Elements/a/> ;
    skos:definition "Relates a corporate body to a word, character, or group of words and/or characters by which a corporate body is known."@en,
        "Met une collectivité en relation avec un mot, un caractère ou un groupe de mots et/ou de caractères sous lequel une collectivité est connue."@fr .

<http://rdaregistry.info/Elements/a/P50061> a rdf:Property ;
    rdfs:label "has name of family"@en,
        "a pour nom de famille"@fr ;
    rdakit:instructionNumber "10.2" ;
    rdakit:toolkitDefinition "A word, character, or group of words and/or characters by which a family is known."@en,
        "Una palabra, un carácter o grupo de palabras y/o caracteres mediante los cuales se conoce una familia."@es,
        "Mot, caractère ou groupe de mots et/ou de caractères sous lequel une famille est connue."@fr ;
    rdakit:toolkitLabel "name of family"@en,
        "nombre de la familia"@es,
        "nom de famille"@fr ;
    reg:hasSubproperty <http://rdaregistry.info/Elements/a/P50054>,
        <http://rdaregistry.info/Elements/a/P50065>,
        <http://rdaregistry.info/Elements/a/datatype/P50061> ;
    reg:hasUnconstrained <http://rdaregistry.info/Elements/u/P60368> ;
    reg:lexicalAlias <http://rdaregistry.info/Elements/a/nameOfFamily.en> ;
    reg:name "nameOfFamily"@en ;
    reg:status <http://metadataregistry.org/uri/RegStatus/1001> ;
    rdfs:domain <http://rdaregistry.info/Elements/c/C10008> ;
    rdfs:isDefinedBy <http://rdaregistry.info/Elements/a/> ;
    skos:definition "Relates a family to a word, character, or group of words and/or characters by which a family is known."@en,
        "Met une famille en relation avec un mot, un caractère ou un groupe de mots et/ou de caractères sous lequel une famille est connue."@fr .

<http://rdaregistry.info/Elements/a/P50071> a rdf:Property ;
    rdfs:label "is actor of"@en,
        "est l’acteur de"@fr ;
    rdakit:instructionNumber "18.5" ;
    rdakit:toolkitDefinition "An expression of a work that incorporates a performance of acting as a cast member or player in a musical or dramatic presentation, etc."@en,
        "Interprète contribuant à une expression d’une œuvre en agissant à titre de membre d’une distribution artistique ou de comédien dans une représentation musicale ou dramatique, etc."@fr ;
    rdakit:toolkitLabel "actor of"@en,
        "acteur de"@fr ;
    reg:hasSubproperty <http://rdaregistry.info/Elements/a/P50217>,
        <http://rdaregistry.info/Elements/a/datatype/P50071>,
        <http://rdaregistry.info/Elements/a/object/P50071> ;
    reg:hasUnconstrained <http://rdaregistry.info/Elements/u/P60017> ;
    reg:lexicalAlias <http://rdaregistry.info/Elements/a/actorOf.en> ;
    reg:name "actorOf"@en ;
    reg:status <http://metadataregistry.org/uri/RegStatus/1001> ;
    rdfs:domain <http://rdaregistry.info/Elements/c/C10002> ;
    rdfs:isDefinedBy <http://rdaregistry.info/Elements/a/> ;
    rdfs:subPropertyOf <http://rdaregistry.info/Elements/a/P50147> ;
    skos:definition "Relates a performer contributing to an expression of a work by acting as a cast member or player in a musical or dramatic presentation, etc. to an expression."@en,
        "Met un interprète contribuant à une expression d’une œuvre en agissant à titre de membre d’une distribution artistique ou de comédien dans une représentation musicale ou dramatique, etc. en relation avec l’expression."@fr .

<http://rdaregistry.info/Elements/a/P50072> a rdf:Property ;
    rdfs:label "is on-screen presenter of"@en,
        "est le présentateur à l’écran de"@fr ;
    rdakit:instructionNumber "18.5" ;
    rdakit:seeAlso <http://rdaregistry.info/Elements/a/P50261> ;
    rdakit:toolkitDefinition "An expression of a work that incorporates a performance of appearing on screen to provide contextual or background information."@en,
        "Interprète contribuant à une expression d’une œuvre en apparaissant à l’écran pour fournir de l’information contextuelle ou complémentaire."@fr ;
    rdakit:toolkitLabel "on-screen presenter of"@en,
        "présentateur à l’écran de"@fr ;
    reg:hasSubproperty <http://rdaregistry.info/Elements/a/datatype/P50072>,
        <http://rdaregistry.info/Elements/a/object/P50072> ;
    reg:hasUnconstrained <http://rdaregistry.info/Elements/u/P60018> ;
    reg:lexicalAlias <http://rdaregistry.info/Elements/a/onScreenPresenterOf.en> ;
    reg:name "onScreenPresenterOf"@en ;
    reg:status <http://metadataregistry.org/uri/RegStatus/1001> ;
    rdfs:domain <http://rdaregistry.info/Elements/c/C10002> ;
    rdfs:isDefinedBy <http://rdaregistry.info/Elements/a/> ;
    rdfs:subPropertyOf <http://rdaregistry.info/Elements/a/P50147> ;
    skos:definition "Relates a performer contributing to an expression of a work by appearing on screen to provide contextual or background information to an expression."@en,
        "Met un interprète contribuant à une expression d’une œuvre en apparaissant à l’écran pour fournir de l’information contextuelle ou complémentaire en relation avec l’expression."@fr ;
    skos:scopeNote "An on-screen presenter may appear in nonfiction moving image materials or in introductions to fiction moving image materials."@en,
        "Un présentateur à l’écran peut apparaître dans des images animées de non fiction ou dans des introductions à des images animées de fiction."@fr .

<http://rdaregistry.info/Elements/a/P50111> a rdf:Property ;
    rdfs:label "has name of person"@en,
        "a pour nom de personne"@fr,
        "har personnamn"@sv ;
    rdakit:instructionNumber "9.2" ;
    rdakit:toolkitDefinition "A word, character, or group of words and/or characters by which a person is known."@en,
        "Una palabra, carácter o grupo de palabras y/o caracteres mediante el cual se conoce una persona."@es,
        "Mot, caractère ou groupe de mots et/ou de caractères sous lequel une personne est connue."@fr ;
    rdakit:toolkitLabel "name of person"@en,
        "nombre de la persona"@es,
        "nom de personne"@fr,
        "personnamn"@sv ;
    reg:hasSubproperty <http://rdaregistry.info/Elements/a/P50103>,
        <http://rdaregistry.info/Elements/a/P50117>,
        <http://rdaregistry.info/Elements/a/datatype/P50111> ;
    reg:hasUnconstrained <http://rdaregistry.info/Elements/u/P60368> ;
    reg:lexicalAlias <http://rdaregistry.info/Elements/a/nameOfPerson.en> ;
    reg:name "nameOfPerson"@en ;
    reg:status <http://metadataregistry.org/uri/RegStatus/1001> ;
    rdfs:domain <http://rdaregistry.info/Elements/c/C10004> ;
    rdfs:isDefinedBy <http://rdaregistry.info/Elements/a/> ;
    skos:definition "Relates a person to a word, character, or group of words and/or characters by which a person is known."@en,
        "Met une personne en relation avec un mot, un caractère ou un groupe de mots et/ou de caractères sous lequel une personne est connue."@fr .

<http://rdaregistry.info/Elements/a/P50137> a rdf:Property ;
    rdfs:label "is arranger of music of"@en,
        "est l’arrangeur de musique de"@fr ;
    rdakit:instructionNumber "18.5" ;
    rdakit:seeAlso <http://rdaregistry.info/Elements/a/P50187> ;
    rdakit:toolkitDefinition "An expression of a musical work that incorporates a contribution of rewriting a composition for a medium of performance different from that for which the work was originally intended."@en,
        "Personne, famille ou collectivité contribuant à une expression d’une œuvre musicale en réécrivant la composition pour une distribution d’exécution différente de celle à laquelle l’œuvre est originellement destinée."@fr ;
    rdakit:toolkitLabel "arranger of music of"@en,
        "arrangeur de musique de"@fr ;
    reg:hasSubproperty <http://rdaregistry.info/Elements/a/datatype/P50137>,
        <http://rdaregistry.info/Elements/a/object/P50137> ;
    reg:hasUnconstrained <http://rdaregistry.info/Elements/u/P60607> ;
    reg:lexicalAlias <http://rdaregistry.info/Elements/a/arrangerOfMusicOf.en> ;
    reg:name "arrangerOfMusicOf"@en ;
    reg:status <http://metadataregistry.org/uri/RegStatus/1001> ;
    rdfs:domain <http://rdaregistry.info/Elements/c/C10002> ;
    rdfs:isDefinedBy <http://rdaregistry.info/Elements/a/> ;
    rdfs:subPropertyOf <http://rdaregistry.info/Elements/a/P50161> ;
    skos:definition "Relates an agent contributing to an expression of a musical work by rewriting a composition for a medium of performance different from that for which the work was originally intended to an expression."@en,
        "Met une personne, famille ou collectivité contribuant à une expression d’une œuvre musicale en réécrivant la composition pour une distribution d’exécution différente de celle à laquelle l’œuvre est originellement destinée en relation avec l’expression."@fr ;
    skos:scopeNote "An arranger of music may also modify the work for the same medium of performance, etc., keeping the musical substance of the original composition essentially unchanged."@en,
        "Un arrangeur de musique peut aussi modifier l’œuvre pour la même distribution d’exécution, etc. tout en gardant la substance musicale de la composition originale essentiellement inchangée."@fr .

<http://rdaregistry.info/Elements/a/P50138> a rdf:Property ;
    rdfs:label "is writer of added text of"@en,
        "est l’auteur de texte ajouté de"@fr ;
    rdakit:instructionNumber "18.5" ;
    rdakit:toolkitDefinition "An expression of a primarily non-textual work that incorporates a contribution of providing text, such as captions for photographs or descriptions of maps."@en,
        "Personne, famille ou collectivité contribuant à une expression d’une œuvre essentiellement non textuelle en fournissant un texte pour l’œuvre non textuelle (par exemple, en écrivant des légendes pour des photographies, des descriptions de cartes géographiques)."@fr ;
    rdakit:toolkitLabel "writer of added text of"@en,
        "auteur de texte ajouté de"@fr ;
    reg:hasSubproperty <http://rdaregistry.info/Elements/a/P50216>,
        <http://rdaregistry.info/Elements/a/datatype/P50138>,
        <http://rdaregistry.info/Elements/a/object/P50138> ;
    reg:hasUnconstrained <http://rdaregistry.info/Elements/u/P60608> ;
    reg:lexicalAlias <http://rdaregistry.info/Elements/a/writerOfAddedTextOf.en> ;
    reg:name "writerOfAddedTextOf"@en ;
    reg:status <http://metadataregistry.org/uri/RegStatus/1001> ;
    rdfs:domain <http://rdaregistry.info/Elements/c/C10002> ;
    rdfs:isDefinedBy <http://rdaregistry.info/Elements/a/> ;
    rdfs:subPropertyOf <http://rdaregistry.info/Elements/a/P50154> ;
    skos:definition "Relates an agent contributing to an expression of a primarily non-textual work by providing text, such as captions for photographs or descriptions of maps, to an expression."@en,
        "Met une personne, famille ou collectivité contribuant à une expression d’une œuvre essentiellement non textuelle en fournissant un texte pour l’œuvre non textuelle (par exemple, en écrivant des légendes pour des photographies, des descriptions de cartes géographiques) en relation avec l’expression."@fr .

<http://rdaregistry.info/Elements/a/P50159> a rdf:Property ;
    rdfs:label "is illustrator of"@en,
        "est l’illustrateur de"@fr ;
    rdakit:instructionNumber "18.5" ;
    rdakit:toolkitDefinition "An expression of a work that incorporates a contribution of supplementing the primary content with drawings, diagrams, photographs, etc."@en,
        "Personne, famille ou collectivité contribuant à une expression d’une œuvre en complétant le contenu principal avec des dessins, des diagrammes, des photographies, etc."@fr ;
    rdakit:toolkitLabel "illustrator of"@en,
        "illustrateur de"@fr ;
    reg:hasSubproperty <http://rdaregistry.info/Elements/a/datatype/P50159>,
        <http://rdaregistry.info/Elements/a/object/P50159>,
        <http://rdaregistry.info/Elements/a/object/P50245> ;
    reg:hasUnconstrained <http://rdaregistry.info/Elements/u/P60624> ;
    reg:lexicalAlias <http://rdaregistry.info/Elements/a/illustratorOf.en> ;
    reg:name "illustratorOf"@en ;
    reg:status <http://metadataregistry.org/uri/RegStatus/1001> ;
    rdfs:domain <http://rdaregistry.info/Elements/c/C10002> ;
    rdfs:isDefinedBy <http://rdaregistry.info/Elements/a/> ;
    rdfs:subPropertyOf <http://rdaregistry.info/Elements/a/P50161> ;
    skos:definition "Relates an agent contributing to an expression of a work by supplementing the primary content with drawings, diagrams, photographs, etc. to an expression."@en,
        "Met une personne, famille ou collectivité contribuant à une expression d’une œuvre en complétant le contenu principal avec des dessins, des diagrammes, des photographies, etc. en relation avec l’expression."@fr .

<http://rdaregistry.info/Elements/a/P50162> a rdf:Property ;
    rdfs:label "is current owner of"@en,
        "est le propriétaire actuel de"@fr ;
    rdakit:instructionNumber "18.5" ;
    rdakit:toolkitDefinition "An item currently in the legal possession of an agent."@en,
        "Personne, famille ou collectivité possédant légalement un item."@fr ;
    rdakit:toolkitLabel "current owner of"@en,
        "propriétaire actuel de"@fr ;
    reg:hasSubproperty <http://rdaregistry.info/Elements/a/P50047>,
        <http://rdaregistry.info/Elements/a/datatype/P50162>,
        <http://rdaregistry.info/Elements/a/object/P50162> ;
    reg:hasUnconstrained <http://rdaregistry.info/Elements/u/P60628> ;
    reg:lexicalAlias <http://rdaregistry.info/Elements/a/currentOwnerOf.en> ;
    reg:name "currentOwnerOf"@en ;
    reg:status <http://metadataregistry.org/uri/RegStatus/1001> ;
    rdfs:domain <http://rdaregistry.info/Elements/c/C10002> ;
    rdfs:isDefinedBy <http://rdaregistry.info/Elements/a/> ;
    rdfs:subPropertyOf <http://rdaregistry.info/Elements/a/P50165> ;
    skos:definition "Relates an agent currently having legal possession of an item to an item."@en,
        "Met une personne, famille ou collectivité possédant légalement un item en relation avec l’item."@fr .

<http://rdaregistry.info/Elements/a/P50165> a rdf:Property ;
    rdfs:label "is owner of"@en,
        "est le propriétaire de"@fr ;
    rdakit:toolkitDefinition "An item in the legal possession of an agent."@en,
        "Personne, famille ou collectivité possédant légalement un item."@fr ;
    rdakit:toolkitLabel "owner of"@en,
        "propriétaire de"@fr ;
    reg:hasSubproperty <http://rdaregistry.info/Elements/a/P50162>,
        <http://rdaregistry.info/Elements/a/P50163>,
        <http://rdaregistry.info/Elements/a/datatype/P50165>,
        <http://rdaregistry.info/Elements/a/object/P50165> ;
    reg:hasUnconstrained <http://rdaregistry.info/Elements/u/P60632> ;
    reg:lexicalAlias <http://rdaregistry.info/Elements/a/ownerOf.en> ;
    reg:name "ownerOf"@en ;
    reg:status <http://metadataregistry.org/uri/RegStatus/1001> ;
    rdfs:domain <http://rdaregistry.info/Elements/c/C10002> ;
    rdfs:isDefinedBy <http://rdaregistry.info/Elements/a/> ;
    rdfs:subPropertyOf <http://rdaregistry.info/Elements/a/P50308> ;
    skos:definition "Relates an agent having legal possession of an item to an item."@en,
        "Met une personne, famille ou collectivité possédant légalement un item en relation avec l’item."@fr .

<http://rdaregistry.info/Elements/a/P50190> a rdf:Property ;
    rdfs:label "is photographer of"@en,
        "est le photographe de"@fr ;
    rdakit:instructionNumber "18.5" ;
    rdakit:toolkitDefinition "A photographic work that involves a creation responsibility."@en,
        "Personne, famille ou collectivité responsable de la création d’une œuvre photographique."@fr ;
    rdakit:toolkitLabel "photographer of"@en,
        "photographe de"@fr ;
    reg:hasSubproperty <http://rdaregistry.info/Elements/a/datatype/P50190>,
        <http://rdaregistry.info/Elements/a/object/P50190> ;
    reg:hasUnconstrained <http://rdaregistry.info/Elements/u/P60658> ;
    reg:lexicalAlias <http://rdaregistry.info/Elements/a/photographerOf.en> ;
    reg:name "photographerOf"@en ;
    reg:status <http://metadataregistry.org/uri/RegStatus/1001> ;
    rdfs:domain <http://rdaregistry.info/Elements/c/C10002> ;
    rdfs:isDefinedBy <http://rdaregistry.info/Elements/a/> ;
    rdfs:subPropertyOf <http://rdaregistry.info/Elements/a/P50204> ;
    skos:definition "Relates an agent responsible for creating a photographic work to a work."@en,
        "Met une personne, famille ou collectivité responsable de la création d’une œuvre photographique en relation avec l’œuvre."@fr .

<http://rdaregistry.info/Elements/a/P50196> a rdf:Property ;
    rdfs:label "is architect of"@en,
        "est l’architecte de"@fr ;
    rdakit:instructionNumber "18.5" ;
    rdakit:toolkitDefinition "A work that involves a responsibility for creating an architectural design, including a pictorial representation intended to show how a building, etc., will look when completed."@en,
        "Personne, famille ou collectivité responsable d’une création architecturale, y compris une représentation illustrée conçue pour montrer de quoi aura l’air un bâtiment, etc. une fois terminé."@fr ;
    rdakit:toolkitLabel "architect of"@en,
        "architecte de"@fr ;
    reg:hasSubproperty <http://rdaregistry.info/Elements/a/P50221>,
        <http://rdaregistry.info/Elements/a/datatype/P50196>,
        <http://rdaregistry.info/Elements/a/object/P50196> ;
    reg:hasUnconstrained <http://rdaregistry.info/Elements/u/P60664> ;
    reg:lexicalAlias <http://rdaregistry.info/Elements/a/architectOf.en> ;
    reg:name "architectOf"@en ;
    reg:status <http://metadataregistry.org/uri/RegStatus/1001> ;
    rdfs:domain <http://rdaregistry.info/Elements/c/C10002> ;
    rdfs:isDefinedBy <http://rdaregistry.info/Elements/a/> ;
    rdfs:subPropertyOf <http://rdaregistry.info/Elements/a/P50204> ;
    skos:definition "Relates an agent responsible for creating an architectural design, including a pictorial representation intended to show how a building, etc., will look when completed to a work."@en,
        "Met une personne, famille ou collectivité responsable d’une création architecturale, y compris une représentation illustrée conçue pour montrer de quoi aura l’air un bâtiment, etc. une fois terminé, en relation avec l’œuvre."@fr .

<http://rdaregistry.info/Elements/a/P50212> a rdf:Property ;
    rdfs:label "is minute taker of"@en,
        "est le procès-verbaliste de"@fr ;
    rdakit:instructionNumber "18.5" ;
    rdakit:toolkitDefinition "An expression that incorporates a contribution of recording the minutes of a meeting."@en,
        "Personne, famille ou collectivité responsable de rédiger le procès-verbal d’une réunion."@fr ;
    rdakit:toolkitLabel "minute taker of"@en,
        "procès-verbaliste de"@fr ;
    reg:hasSubproperty <http://rdaregistry.info/Elements/a/datatype/P50212>,
        <http://rdaregistry.info/Elements/a/object/P50212> ;
    reg:hasUnconstrained <http://rdaregistry.info/Elements/u/P60671> ;
    reg:lexicalAlias <http://rdaregistry.info/Elements/a/minuteTakerOf.en> ;
    reg:name "minuteTakerOf"@en ;
    reg:status <http://metadataregistry.org/uri/RegStatus/1001> ;
    rdfs:domain <http://rdaregistry.info/Elements/c/C10002> ;
    rdfs:isDefinedBy <http://rdaregistry.info/Elements/a/> ;
    rdfs:subPropertyOf <http://rdaregistry.info/Elements/a/P50161> ;
    skos:definition "Relates an agent responsible for recording the minutes of a meeting to an expression."@en,
        "Met une personne, famille ou collectivité responsable de rédiger le procès-verbal d’une réunion en relation avec l’expression."@fr .

<http://rdaregistry.info/Elements/a/P50225> a rdf:Property ;
    rdfs:label "is librettist of"@en,
        "est le librettiste de"@fr ;
    rdakit:instructionNumber "18.5" ;
    rdakit:seeAlso <http://rdaregistry.info/Elements/a/P50224> ;
    rdakit:toolkitDefinition "A work that involves an authoring responsibility for the words of an opera or other musical stage work, or an oratorio."@en,
        "Auteur des paroles d’un opéra ou d’une autre œuvre scénique ou d’un oratorio."@fr ;
    rdakit:toolkitLabel "librettist of"@en,
        "librettiste de"@fr ;
    reg:hasSubproperty <http://rdaregistry.info/Elements/a/datatype/P50225>,
        <http://rdaregistry.info/Elements/a/object/P50225> ;
    reg:hasUnconstrained <http://rdaregistry.info/Elements/u/P60708> ;
    reg:lexicalAlias <http://rdaregistry.info/Elements/a/librettistOf.en> ;
    reg:name "librettistOf"@en ;
    reg:status <http://metadataregistry.org/uri/RegStatus/1001> ;
    rdfs:domain <http://rdaregistry.info/Elements/c/C10002> ;
    rdfs:isDefinedBy <http://rdaregistry.info/Elements/a/> ;
    rdfs:subPropertyOf <http://rdaregistry.info/Elements/a/P50195> ;
    skos:definition "Relates an author of the words of an opera or other musical stage work, or an oratorio to a work."@en,
        "Met un auteur des paroles d’un opéra ou d’une autre œuvre scénique ou d’un oratorio en relation avec l’œuvre."@fr .

<http://rdaregistry.info/Elements/a/P50234> a rdf:Property ;
    rdfs:label "is officer of"@en,
        "a pour collectivité administrée"@fr ;
    rdakit:instructionNumber "29.5" ;
    rdakit:toolkitDefinition "A corporate body that a person commands or in which a person holds an office."@en,
        "Una entidad corporativa en la cual una persona tiene un cargo."@es,
        "Collectivité dans laquelle la personne exerce une fonction administrative ou officielle."@fr ;
    rdakit:toolkitLabel "officer of"@en,
        "entidad corporativa sede"@es,
        "collectivité administrée"@fr ;
    reg:hasSubproperty <http://rdaregistry.info/Elements/a/datatype/P50234>,
        <http://rdaregistry.info/Elements/a/object/P50234>,
        <http://rdaregistry.info/Elements/a/object/P50286>,
        <http://rdaregistry.info/Elements/a/object/P50287> ;
    reg:hasUnconstrained <http://rdaregistry.info/Elements/u/P60737> ;
    reg:lexicalAlias <http://rdaregistry.info/Elements/a/officerOf.en> ;
    reg:name "officerOf"@en ;
    reg:status <http://metadataregistry.org/uri/RegStatus/1001> ;
    rdfs:domain <http://rdaregistry.info/Elements/c/C10004> ;
    rdfs:isDefinedBy <http://rdaregistry.info/Elements/a/> ;
    skos:definition "Relates a person to a corporate body that a person commands or in which a person holds an office."@en,
        "Met une personne en relation avec une collectivité dans laquelle la personne exerce une fonction administrative ou officielle."@fr .

<http://rdaregistry.info/Elements/a/P50296> a rdf:Property ;
    rdfs:label "is audio engineer of"@en ;
    rdakit:instructionNumber "18.5" ;
    rdakit:toolkitDefinition "An expression of a work that incorporates a contribution to the audio content of managing the technical aspects of sound during the processes of recording, mixing, and reproduction."@en ;
    rdakit:toolkitLabel "audio engineer of"@en ;
    reg:hasSubproperty <http://rdaregistry.info/Elements/a/datatype/P50296>,
        <http://rdaregistry.info/Elements/a/object/P50296>,
        <http://rdaregistry.info/Elements/a/object/P50297> ;
    reg:hasUnconstrained <http://rdaregistry.info/Elements/u/P60884> ;
    reg:lexicalAlias <http://rdaregistry.info/Elements/a/audioEngineerOf.en> ;
    reg:name "audioEngineerOf"@en ;
    reg:status <http://metadataregistry.org/uri/RegStatus/1001> ;
    rdfs:domain <http://rdaregistry.info/Elements/c/C10002> ;
    rdfs:isDefinedBy <http://rdaregistry.info/Elements/a/> ;
    rdfs:subPropertyOf <http://rdaregistry.info/Elements/a/P50161> ;
    skos:definition "Relates an agent to an expression of a work that incorporates a contribution to the audio content of managing the technical aspects of sound during the processes of recording, mixing, and reproduction."@en .

<http://rdaregistry.info/Elements/a/P50366> a rdf:Property ;
    rdfs:label "is subject of (agent)"@en ;
    reg:lexicalAlias <http://rdaregistry.info/Elements/a/subjectOfAgent.en> ;
    reg:name "subjectOfAgent"@en ;
    reg:status <http://metadataregistry.org/uri/RegStatus/1001> ;
    rdfs:domain <http://rdaregistry.info/Elements/c/C10011> ;
    rdfs:isDefinedBy <http://rdaregistry.info/Elements/a/> ;
    rdfs:subPropertyOf <http://rdaregistry.info/Elements/w/P10283> ;
    skos:definition "Relates an agent to a work that is about an agent."@en .

<http://rdaregistry.info/Elements/a/P50367> a rdf:Property ;
    rdfs:label "is subject of (collective agent)"@en ;
    reg:lexicalAlias <http://rdaregistry.info/Elements/a/subjectOfCollectiveAgent.en> ;
    reg:name "subjectOfCollectiveAgent"@en ;
    reg:status <http://metadataregistry.org/uri/RegStatus/1001> ;
    rdfs:domain <http://rdaregistry.info/Elements/c/C10011> ;
    rdfs:isDefinedBy <http://rdaregistry.info/Elements/a/> ;
    rdfs:subPropertyOf <http://rdaregistry.info/Elements/a/P50366> ;
    skos:definition "Relates a collective agent to a work that is about a collective agent."@en .

<http://rdaregistry.info/Elements/a/P50033> a rdf:Property ;
    rdfs:label "has other designation associated with corporate body"@en,
        "a pour autre information associée à la collectivité"@fr,
        "har övrig beteckning förknippad med institutionen"@sv ;
    rdakit:instructionNumber "11.7" ;
    rdakit:toolkitDefinition "A word, phrase, or abbreviation indicating incorporation or legal status of a corporate body, or any term serving to differentiate a corporate body from other corporate bodies, persons, etc."@en,
        "Una palabra, frase o abreviatura que indica la incorporación o la condición legal de una entidad corporativa, o cualquier término que diferencia la entidad de otras entidades corporativas, personas, etc."@es,
        "Mot, locution ou abréviation indiquant le statut commercial ou juridique d’une collectivité ou tout terme permettant de différencier la collectivité d’autres collectivités, personnes, etc."@fr ;
    rdakit:toolkitLabel "other designation associated with corporate body"@en,
        "otra designación asociada con la entidad corporativa"@es,
        "autre information associée à la collectivité"@fr,
        "övrig beteckning förknippad med institutionen"@sv ;
    reg:hasSubproperty <http://rdaregistry.info/Elements/a/datatype/P50033> ;
    reg:hasUnconstrained <http://rdaregistry.info/Elements/u/P60370> ;
    reg:lexicalAlias <http://rdaregistry.info/Elements/a/otherDesignationAssociatedWithCorporateBody.en> ;
    reg:name "otherDesignationAssociatedWithCorporateBody"@en ;
    reg:status <http://metadataregistry.org/uri/RegStatus/1001> ;
    rdfs:domain <http://rdaregistry.info/Elements/c/C10005> ;
    rdfs:isDefinedBy <http://rdaregistry.info/Elements/a/> ;
    skos:definition "Relates a corporate body to a word, phrase, or abbreviation indicating incorporation or legal status of a corporate body, or any term serving to differentiate a corporate body from other corporate bodies, persons, etc."@en,
        "Met une collectivité en relation avec un mot, une locution ou une abréviation indiquant le statut commercial ou juridique d’une collectivité ou tout terme permettant de différencier la collectivité d’autres collectivités, personnes, etc."@fr .

<http://rdaregistry.info/Elements/a/P50070> a rdf:Property ;
    rdfs:label "is conductor of"@en,
        "est le chef d’orchestre de"@fr ;
    rdakit:instructionNumber "18.5" ;
    rdakit:toolkitDefinition "An expression of a musical work that incorporates a performance of leading of a performing group in a musical or dramatic presentation, etc."@en,
        "Interprète contribuant à une expression d’une œuvre musicale en dirigeant un groupe d’interprètes (orchestre, chorale, opéra, etc.) dans une représentation musicale ou dramatique, etc."@fr ;
    rdakit:toolkitLabel "conductor of"@en,
        "chef d’orchestre de"@fr ;
    reg:hasSubproperty <http://rdaregistry.info/Elements/a/datatype/P50070>,
        <http://rdaregistry.info/Elements/a/object/P50070>,
        <http://rdaregistry.info/Elements/a/object/P50268>,
        <http://rdaregistry.info/Elements/a/object/P50269> ;
    reg:hasUnconstrained <http://rdaregistry.info/Elements/u/P60016> ;
    reg:lexicalAlias <http://rdaregistry.info/Elements/a/conductorOf.en> ;
    reg:name "conductorOf"@en ;
    reg:status <http://metadataregistry.org/uri/RegStatus/1001> ;
    rdfs:domain <http://rdaregistry.info/Elements/c/C10002> ;
    rdfs:isDefinedBy <http://rdaregistry.info/Elements/a/> ;
    rdfs:subPropertyOf <http://rdaregistry.info/Elements/a/P50147> ;
    skos:definition "Relates a performer contributing to an expression of a musical work by leading a performing group in a musical or dramatic presentation, etc. to an expression."@en,
        "Met un interprète contribuant à une expression d’une œuvre musicale en dirigeant un groupe d’interprètes (orchestre, chorale, opéra, etc.) dans une représentation musicale ou dramatique, etc. en relation avec l’expression."@fr .

<http://rdaregistry.info/Elements/a/P50087> a rdf:Property ;
    rdfs:label "is appellee of"@en,
        "est l’intimé de"@fr ;
    rdakit:instructionNumber "18.5" ;
    rdakit:toolkitDefinition "A legal work of a higher court recording a decision of a lower court that appeals against a person or corporate body."@en,
        "Personne ou collectivité contre laquelle un appel a été formé."@fr ;
    rdakit:toolkitLabel "appellee of"@en,
        "intimé de"@fr ;
    reg:hasSubproperty <http://rdaregistry.info/Elements/a/P50085>,
        <http://rdaregistry.info/Elements/a/datatype/P50087>,
        <http://rdaregistry.info/Elements/a/object/P50087> ;
    reg:hasUnconstrained <http://rdaregistry.info/Elements/u/P60601> ;
    reg:lexicalAlias <http://rdaregistry.info/Elements/a/appelleeOf.en> ;
    reg:name "appelleeOf"@en ;
    reg:status <http://metadataregistry.org/uri/RegStatus/1001> ;
    rdfs:isDefinedBy <http://rdaregistry.info/Elements/a/> ;
    rdfs:subPropertyOf <http://rdaregistry.info/Elements/a/P50131> ;
    skos:definition "Relates a person or corporate body against whom an appeal is taken on a decision of a lower court recorded in a legal work of a higher court to a work."@en,
        "Met une personne ou collectivité contre laquelle un appel a été formé en relation avec l’œuvre."@fr .

<http://rdaregistry.info/Elements/a/P50088> a rdf:Property ;
    rdfs:label "is appellant of"@en,
        "est l’appelant de"@fr ;
    rdakit:instructionNumber "18.5" ;
    rdakit:toolkitDefinition "A legal work of a higher court recording a decision of a lower court that is appealed by a person or corporate body."@en,
        "Personne ou collectivité qui en appelle de la décision d’un tribunal inférieur."@fr ;
    rdakit:toolkitLabel "appellant of"@en,
        "appelant de"@fr ;
    reg:hasSubproperty <http://rdaregistry.info/Elements/a/P50042>,
        <http://rdaregistry.info/Elements/a/datatype/P50088>,
        <http://rdaregistry.info/Elements/a/object/P50088>,
        <http://rdaregistry.info/Elements/a/object/P50122> ;
    reg:hasUnconstrained <http://rdaregistry.info/Elements/u/P60691> ;
    reg:lexicalAlias <http://rdaregistry.info/Elements/a/appellantOf.en> ;
    reg:name "appellantOf"@en ;
    reg:status <http://metadataregistry.org/uri/RegStatus/1001> ;
    rdfs:isDefinedBy <http://rdaregistry.info/Elements/a/> ;
    rdfs:subPropertyOf <http://rdaregistry.info/Elements/a/P50131> ;
    skos:definition "Relates a person or corporate body who appeals the decision of a lower court recorded in a legal work of a higher court to a work."@en,
        "Met une personne ou collectivité qui en appelle de la décision d’un tribunal inférieur en relation avec l’œuvre."@fr .

<http://rdaregistry.info/Elements/a/P50089> a rdf:Property ;
    rdfs:label "is plaintiff of"@en,
        "est le demandeur de"@fr ;
    rdakit:instructionNumber "18.5" ;
    rdakit:toolkitDefinition "A work that involves a responsibility for bringing a suit in a civil proceeding by a person or corporate body."@en,
        "Personne ou collectivité qui intente une poursuite civile."@fr ;
    rdakit:toolkitLabel "plaintiff of"@en,
        "demandeur de"@fr ;
    reg:hasSubproperty <http://rdaregistry.info/Elements/a/P50043>,
        <http://rdaregistry.info/Elements/a/P50124>,
        <http://rdaregistry.info/Elements/a/datatype/P50089>,
        <http://rdaregistry.info/Elements/a/object/P50089> ;
    reg:hasUnconstrained <http://rdaregistry.info/Elements/u/P60693> ;
    reg:lexicalAlias <http://rdaregistry.info/Elements/a/plaintiffOf.en> ;
    reg:name "plaintiffOf"@en ;
    reg:status <http://metadataregistry.org/uri/RegStatus/1001> ;
    rdfs:isDefinedBy <http://rdaregistry.info/Elements/a/> ;
    rdfs:subPropertyOf <http://rdaregistry.info/Elements/a/P50131> ;
    skos:definition "Relates a person or corporate body who brings a suit in a civil proceeding to a work."@en,
        "Met une personne ou collectivité qui intente une poursuite civile en relation avec l’œuvre."@fr .

<http://rdaregistry.info/Elements/a/P50090> a rdf:Property ;
    rdfs:label "is defendant of"@en,
        "est le défendeur de"@fr ;
    rdakit:instructionNumber "18.5" ;
    rdakit:toolkitDefinition "A work that involves a responsibility for being a person or corporate body accused in a criminal proceeding or sued in a civil proceeding."@en,
        "Personne ou collectivité qui est accusée dans une poursuite criminelle ou contre laquelle une poursuite civile est intentée."@fr ;
    rdakit:toolkitLabel "defendant of"@en,
        "défendeur de"@fr ;
    reg:hasSubproperty <http://rdaregistry.info/Elements/a/datatype/P50090>,
        <http://rdaregistry.info/Elements/a/object/P50090>,
        <http://rdaregistry.info/Elements/a/object/P50258>,
        <http://rdaregistry.info/Elements/a/object/P50259> ;
    reg:hasUnconstrained <http://rdaregistry.info/Elements/u/P60698> ;
    reg:lexicalAlias <http://rdaregistry.info/Elements/a/defendantOf.en> ;
    reg:name "defendantOf"@en ;
    reg:status <http://metadataregistry.org/uri/RegStatus/1001> ;
    rdfs:isDefinedBy <http://rdaregistry.info/Elements/a/> ;
    rdfs:subPropertyOf <http://rdaregistry.info/Elements/a/P50131> ;
    skos:definition "Relates a person or corporate body who is accused in a criminal proceeding or sued in a civil proceeding to a work."@en,
        "Met une personne ou collectivité qui est accusée dans une poursuite criminelle ou contre laquelle une poursuite civile est intentée en relation avec l’œuvre."@fr .

<http://rdaregistry.info/Elements/a/P50107> a rdf:Property ;
    rdfs:label "has date associated with person"@en,
        "a pour date associée à la personne"@fr,
        "har tid förknippad med personen"@sv ;
    rdakit:instructionNumber "9.3" ;
    rdakit:toolkitDefinition "A significant date associated with a person."@en,
        "Una fecha significativa asociada con la persona (p.ej., fecha de nacimiento, fecha de fallecimiento)."@es,
        "Date importante associée à une personne (par exemple, date de naissance, date de décès)."@fr ;
    rdakit:toolkitLabel "date associated with person"@en,
        "fecha asociada con la persona"@es,
        "date associée à la personne"@fr,
        "tid förknippad med personen"@sv ;
    reg:hasSubproperty <http://rdaregistry.info/Elements/a/P50098>,
        <http://rdaregistry.info/Elements/a/P50120>,
        <http://rdaregistry.info/Elements/a/P50121>,
        <http://rdaregistry.info/Elements/a/datatype/P50107> ;
    reg:hasUnconstrained <http://rdaregistry.info/Elements/u/P60324> ;
    reg:lexicalAlias <http://rdaregistry.info/Elements/a/dateAssociatedWithPerson.en> ;
    reg:name "dateAssociatedWithPerson"@en ;
    reg:status <http://metadataregistry.org/uri/RegStatus/1001> ;
    rdfs:domain <http://rdaregistry.info/Elements/c/C10004> ;
    rdfs:isDefinedBy <http://rdaregistry.info/Elements/a/> ;
    skos:definition "Relates a person to a significant date associated with a person."@en,
        "Met une personne en relation avec une date importante associée à une personne (par exemple, date de naissance, date de décès)."@fr .

<http://rdaregistry.info/Elements/a/P50133> a rdf:Property ;
    rdfs:label "is curator of"@en,
        "est le conservateur de"@fr ;
    rdakit:instructionNumber "18.5" ;
    rdakit:toolkitDefinition "An item that is conceived, aggregated, and/or organized in an exhibition, collection, or other item."@en,
        "Personne, famille ou collectivité concevant, regroupant et/ou organisant une exposition, une collection ou un autre item."@fr ;
    rdakit:toolkitLabel "curator of"@en,
        "conservateur de"@fr ;
    reg:hasSubproperty <http://rdaregistry.info/Elements/a/P50045>,
        <http://rdaregistry.info/Elements/a/P50046>,
        <http://rdaregistry.info/Elements/a/datatype/P50133>,
        <http://rdaregistry.info/Elements/a/object/P50133> ;
    reg:hasUnconstrained <http://rdaregistry.info/Elements/u/P60604> ;
    reg:lexicalAlias <http://rdaregistry.info/Elements/a/curatorOf.en> ;
    reg:name "curatorOf"@en ;
    reg:status <http://metadataregistry.org/uri/RegStatus/1001> ;
    rdfs:domain <http://rdaregistry.info/Elements/c/C10002> ;
    rdfs:isDefinedBy <http://rdaregistry.info/Elements/a/> ;
    rdfs:subPropertyOf <http://rdaregistry.info/Elements/a/P50182> ;
    skos:definition "Relates an agent conceiving, aggregating, or organizing an exhibition, collection, or other item to an item."@en,
        "Met une personne, famille ou collectivité concevant, regroupant et/ou organisant une exposition, une collection ou un autre item en relation avec l’item."@fr .

<http://rdaregistry.info/Elements/a/P50156> a rdf:Property ;
    rdfs:label "is editor of"@en,
        "est l’éditeur intellectuel de"@fr ;
    rdakit:instructionNumber "18.5" ;
    rdakit:seeAlso <http://rdaregistry.info/Elements/a/P50195> ;
    rdakit:toolkitDefinition "An expression of a work that incorporates a contribution of revising or clarifying the content, or by selecting and putting together works, or parts of works, by one or more creators."@en,
        "Personne, famille ou collectivité contribuant à une expression d’une œuvre en révisant ou en clarifiant le contenu, ou bien en choisissant et en rassemblant des œuvres, ou des parties d’œuvres, d’un ou de plusieurs créateurs."@fr ;
    rdakit:toolkitLabel "editor of"@en,
        "éditeur intellectuel de"@fr ;
    reg:hasSubproperty <http://rdaregistry.info/Elements/a/datatype/P50156>,
        <http://rdaregistry.info/Elements/a/object/P50156> ;
    reg:hasUnconstrained <http://rdaregistry.info/Elements/u/P60621> ;
    reg:lexicalAlias <http://rdaregistry.info/Elements/a/editorOf.en> ;
    reg:name "editorOf"@en ;
    reg:status <http://metadataregistry.org/uri/RegStatus/1001> ;
    rdfs:domain <http://rdaregistry.info/Elements/c/C10002> ;
    rdfs:isDefinedBy <http://rdaregistry.info/Elements/a/> ;
    rdfs:subPropertyOf <http://rdaregistry.info/Elements/a/P50161> ;
    skos:definition "Relates an agent contributing to an expression of a work by revising or clarifying the content, or by selecting and putting together works, or parts of works, by one or more creators to an expression."@en,
        "Met une personne, famille ou collectivité contribuant à une expression d’une œuvre en révisant ou en clarifiant le contenu, ou bien en choisissant et en rassemblant des œuvres, ou des parties d’œuvres, d’un ou de plusieurs créateurs en relation avec l’expression."@fr ;
    skos:scopeNote "Contributions may include adding an introduction, notes, or other critical matter, or preparing the expression of a work for production, publication, or distribution."@en,
        "Les contributions peuvent inclure l’ajout d’une introduction, de notes ou d’autres textes critiques, ou bien la préparation de l’expression d’une œuvre aux fins de production, de publication ou de diffusion/distribution."@fr .

<http://rdaregistry.info/Elements/a/P50163> a rdf:Property ;
    rdfs:label "is former owner of"@en,
        "est l’ancien propriétaire de"@fr ;
    rdakit:instructionNumber "18.5" ;
    rdakit:toolkitDefinition "An item formerly in the legal possession of an agent."@en,
        "Personne, famille ou collectivité ayant auparavant possédé légalement un item."@fr ;
    rdakit:toolkitLabel "former owner of"@en,
        "ancien propriétaire de"@fr ;
    reg:hasSubproperty <http://rdaregistry.info/Elements/a/P50066>,
        <http://rdaregistry.info/Elements/a/P50067>,
        <http://rdaregistry.info/Elements/a/datatype/P50163>,
        <http://rdaregistry.info/Elements/a/object/P50163> ;
    reg:hasUnconstrained <http://rdaregistry.info/Elements/u/P60630> ;
    reg:lexicalAlias <http://rdaregistry.info/Elements/a/formerOwnerOf.en> ;
    reg:name "formerOwnerOf"@en ;
    reg:status <http://metadataregistry.org/uri/RegStatus/1001> ;
    rdfs:domain <http://rdaregistry.info/Elements/c/C10002> ;
    rdfs:isDefinedBy <http://rdaregistry.info/Elements/a/> ;
    rdfs:subPropertyOf <http://rdaregistry.info/Elements/a/P50165> ;
    skos:definition "Relates an agent formerly having legal possession of an item to an item."@en,
        "Met une personne, famille ou collectivité ayant auparavant possédé légalement un item en relation avec l’item."@fr .

<http://rdaregistry.info/Elements/a/P50187> a rdf:Property ;
    rdfs:label "is composer of"@en,
        "est le compositeur de"@fr ;
    rdakit:instructionNumber "18.5" ;
    rdakit:toolkitDefinition "A musical work that involves a creation responsibility."@en,
        "Personne, famille ou collectivité responsable de la création d’une œuvre musicale."@fr ;
    rdakit:toolkitLabel "composer of"@en,
        "compositeur de"@fr ;
    reg:hasSubproperty <http://rdaregistry.info/Elements/a/datatype/P50187>,
        <http://rdaregistry.info/Elements/a/object/P50187> ;
    reg:hasUnconstrained <http://rdaregistry.info/Elements/u/P60655> ;
    reg:lexicalAlias <http://rdaregistry.info/Elements/a/composerOf.en> ;
    reg:name "composerOf"@en ;
    reg:status <http://metadataregistry.org/uri/RegStatus/1001> ;
    rdfs:domain <http://rdaregistry.info/Elements/c/C10002> ;
    rdfs:isDefinedBy <http://rdaregistry.info/Elements/a/> ;
    rdfs:subPropertyOf <http://rdaregistry.info/Elements/a/P50204> ;
    skos:definition "Relates an agent responsible for creating a musical work to a work."@en,
        "Met une personne, famille ou collectivité responsable de la création d’une œuvre musicale en relation avec l’œuvre."@fr .

<http://rdaregistry.info/Elements/a/P50224> a rdf:Property ;
    rdfs:label "is lyricist of"@en,
        "est le parolier de"@fr ;
    rdakit:instructionNumber "18.5" ;
    rdakit:seeAlso <http://rdaregistry.info/Elements/a/P50225> ;
    rdakit:toolkitDefinition "A work that involves an authoring responsibility for the words of a popular song, including a song or songs from a musical."@en,
        "Auteur des paroles d’une chanson populaire, y compris une ou plusieurs chansons d’une comédie musicale."@fr ;
    rdakit:toolkitLabel "lyricist of"@en,
        "parolier de"@fr ;
    reg:hasSubproperty <http://rdaregistry.info/Elements/a/datatype/P50224>,
        <http://rdaregistry.info/Elements/a/object/P50224> ;
    reg:hasUnconstrained <http://rdaregistry.info/Elements/u/P60707> ;
    reg:lexicalAlias <http://rdaregistry.info/Elements/a/lyricistOf.en> ;
    reg:name "lyricistOf"@en ;
    reg:status <http://metadataregistry.org/uri/RegStatus/1001> ;
    rdfs:domain <http://rdaregistry.info/Elements/c/C10002> ;
    rdfs:isDefinedBy <http://rdaregistry.info/Elements/a/> ;
    rdfs:subPropertyOf <http://rdaregistry.info/Elements/a/P50195> ;
    skos:definition "Relates an author of the words of a popular song, including a song or songs from a musical to a work."@en,
        "Met un auteur des paroles d’une chanson populaire, y compris une ou plusieurs chansons d’une comédie musicale, en relation avec l’œuvre."@fr .

<http://rdaregistry.info/Elements/a/P50315> a rdf:Property ;
    rdfs:label "has related agent (person)"@en ;
    reg:hasSubproperty <http://rdaregistry.info/Elements/a/P50316>,
        <http://rdaregistry.info/Elements/a/P50345>,
        <http://rdaregistry.info/Elements/a/datatype/P50315>,
        <http://rdaregistry.info/Elements/a/object/P50315> ;
    reg:lexicalAlias <http://rdaregistry.info/Elements/a/relatedAgentPerson.en> ;
    reg:name "relatedAgentPerson"@en ;
    reg:status <http://metadataregistry.org/uri/RegStatus/1001> ;
    rdfs:domain <http://rdaregistry.info/Elements/c/C10004> ;
    rdfs:isDefinedBy <http://rdaregistry.info/Elements/a/> ;
    rdfs:subPropertyOf <http://rdaregistry.info/Elements/a/P50309>,
        <http://rdaregistry.info/Elements/a/P50310> ;
    skos:definition "Relates a person to an agent associated with a person being described."@en .

<http://rdaregistry.info/Elements/a/P50324> a rdf:Property ;
    rdfs:label "has related agent (family)"@en ;
    reg:hasSubproperty <http://rdaregistry.info/Elements/a/P50325>,
        <http://rdaregistry.info/Elements/a/P50353>,
        <http://rdaregistry.info/Elements/a/datatype/P50324>,
        <http://rdaregistry.info/Elements/a/object/P50324> ;
    reg:lexicalAlias <http://rdaregistry.info/Elements/a/relatedAgentFamily.en> ;
    reg:name "relatedAgentFamily"@en ;
    reg:status <http://metadataregistry.org/uri/RegStatus/1001> ;
    rdfs:domain <http://rdaregistry.info/Elements/c/C10008> ;
    rdfs:isDefinedBy <http://rdaregistry.info/Elements/a/> ;
    rdfs:subPropertyOf <http://rdaregistry.info/Elements/a/P50319>,
        <http://rdaregistry.info/Elements/a/P50358> ;
    skos:definition "Relates a family to an agent associated with a family being described."@en .

<http://rdaregistry.info/Elements/a/P50338> a rdf:Property ;
    rdfs:label "has related place (agent)"@en ;
    reg:hasSubproperty <http://rdaregistry.info/Elements/a/datatype/P50338>,
        <http://rdaregistry.info/Elements/a/object/P50338> ;
    reg:lexicalAlias <http://rdaregistry.info/Elements/a/relatedPlaceAgent.en> ;
    reg:name "relatedPlaceAgent"@en ;
    reg:status <http://metadataregistry.org/uri/RegStatus/1001> ;
    rdfs:domain <http://rdaregistry.info/Elements/c/C10002> ;
    rdfs:isDefinedBy <http://rdaregistry.info/Elements/a/> ;
    rdfs:subPropertyOf <http://rdaregistry.info/Elements/a/P50304>,
        <http://rdaregistry.info/Elements/x/P00006> ;
    skos:definition "Relates an agent to a place associated with an agent."@en .

<http://rdaregistry.info/Elements/a/P50339> a rdf:Property ;
    rdfs:label "has related time-span (agent)"@en ;
    reg:hasSubproperty <http://rdaregistry.info/Elements/a/datatype/P50339>,
        <http://rdaregistry.info/Elements/a/object/P50339> ;
    reg:lexicalAlias <http://rdaregistry.info/Elements/a/relatedTimespanAgent.en> ;
    reg:name "relatedTimespanAgent"@en ;
    reg:status <http://metadataregistry.org/uri/RegStatus/1001> ;
    rdfs:domain <http://rdaregistry.info/Elements/c/C10002> ;
    rdfs:isDefinedBy <http://rdaregistry.info/Elements/a/> ;
    rdfs:subPropertyOf <http://rdaregistry.info/Elements/a/P50304>,
        <http://rdaregistry.info/Elements/x/P00006> ;
    skos:definition "Relates an agent to a time-span associated with an agent."@en .

<http://rdaregistry.info/Elements/a/P50340> a rdf:Property ;
    rdfs:label "has related nomen (agent)"@en ;
    reg:hasSubproperty <http://rdaregistry.info/Elements/a/datatype/P50340>,
        <http://rdaregistry.info/Elements/a/object/P50340> ;
    reg:lexicalAlias <http://rdaregistry.info/Elements/a/relatedNomenAgent.en> ;
    reg:name "relatedNomenAgent"@en ;
    reg:status <http://metadataregistry.org/uri/RegStatus/1001> ;
    rdfs:domain <http://rdaregistry.info/Elements/c/C10002> ;
    rdfs:isDefinedBy <http://rdaregistry.info/Elements/a/> ;
    rdfs:subPropertyOf <http://rdaregistry.info/Elements/a/P50304>,
        <http://rdaregistry.info/Elements/x/P00006> ;
    skos:definition "Relates an agent to a nomen associated with an agent."@en .

<http://rdaregistry.info/Elements/a/P50342> a rdf:Property ;
    rdfs:label "has related place (collective agent)"@en ;
    reg:hasSubproperty <http://rdaregistry.info/Elements/a/datatype/P50342>,
        <http://rdaregistry.info/Elements/a/object/P50342> ;
    reg:lexicalAlias <http://rdaregistry.info/Elements/a/relatedPlaceCollectiveAgent.en> ;
    reg:name "relatedPlaceCollectiveAgent"@en ;
    reg:status <http://metadataregistry.org/uri/RegStatus/1001> ;
    rdfs:domain <http://rdaregistry.info/Elements/c/C10011> ;
    rdfs:isDefinedBy <http://rdaregistry.info/Elements/a/> ;
    rdfs:subPropertyOf <http://rdaregistry.info/Elements/a/P50338>,
        <http://rdaregistry.info/Elements/a/P50360> ;
    skos:definition "Relates a collective agent to a place associated with a collective agent."@en .

<http://rdaregistry.info/Elements/a/P50343> a rdf:Property ;
    rdfs:label "has related time-span (collective agent)"@en ;
    reg:hasSubproperty <http://rdaregistry.info/Elements/a/datatype/P50343>,
        <http://rdaregistry.info/Elements/a/object/P50343> ;
    reg:lexicalAlias <http://rdaregistry.info/Elements/a/relatedTimespanCollectiveAgent.en> ;
    reg:name "relatedTimespanCollectiveAgent"@en ;
    reg:status <http://metadataregistry.org/uri/RegStatus/1001> ;
    rdfs:domain <http://rdaregistry.info/Elements/c/C10011> ;
    rdfs:isDefinedBy <http://rdaregistry.info/Elements/a/> ;
    rdfs:subPropertyOf <http://rdaregistry.info/Elements/a/P50339>,
        <http://rdaregistry.info/Elements/a/P50360> ;
    skos:definition "Relates a collective agent to a time-span associated with a collective agent."@en .

<http://rdaregistry.info/Elements/a/P50344> a rdf:Property ;
    rdfs:label "has related nomen (collective agent)"@en ;
    reg:hasSubproperty <http://rdaregistry.info/Elements/a/datatype/P50344>,
        <http://rdaregistry.info/Elements/a/object/P50344> ;
    reg:lexicalAlias <http://rdaregistry.info/Elements/a/relatedNomenCollectiveAgent.en> ;
    reg:name "relatedNomenCollectiveAgent"@en ;
    reg:status <http://metadataregistry.org/uri/RegStatus/1001> ;
    rdfs:domain <http://rdaregistry.info/Elements/c/C10011> ;
    rdfs:isDefinedBy <http://rdaregistry.info/Elements/a/> ;
    rdfs:subPropertyOf <http://rdaregistry.info/Elements/a/P50340>,
        <http://rdaregistry.info/Elements/a/P50360> ;
    skos:definition "Relates a collective agent to a nomen associated with a collective agent."@en .

<http://rdaregistry.info/Elements/a/P50345> a rdf:Property ;
    rdfs:label "has related collective agent (person)"@en ;
    reg:hasSubproperty <http://rdaregistry.info/Elements/a/P50317>,
        <http://rdaregistry.info/Elements/a/P50318>,
        <http://rdaregistry.info/Elements/a/datatype/P50345>,
        <http://rdaregistry.info/Elements/a/object/P50345> ;
    reg:lexicalAlias <http://rdaregistry.info/Elements/a/relatedCollectiveAgentPerson.en> ;
    reg:name "relatedCollectiveAgentPerson"@en ;
    reg:status <http://metadataregistry.org/uri/RegStatus/1001> ;
    rdfs:domain <http://rdaregistry.info/Elements/c/C10004> ;
    rdfs:isDefinedBy <http://rdaregistry.info/Elements/a/> ;
    rdfs:subPropertyOf <http://rdaregistry.info/Elements/a/P50315>,
        <http://rdaregistry.info/Elements/a/P50337> ;
    skos:definition "Relates a person to a collective agent associated with a person."@en .

<http://rdaregistry.info/Elements/a/P50353> a rdf:Property ;
    rdfs:label "has related collective agent (family)"@en ;
    reg:hasSubproperty <http://rdaregistry.info/Elements/a/P50326>,
        <http://rdaregistry.info/Elements/a/P50327>,
        <http://rdaregistry.info/Elements/a/datatype/P50353>,
        <http://rdaregistry.info/Elements/a/object/P50353> ;
    reg:lexicalAlias <http://rdaregistry.info/Elements/a/relatedCollectiveAgentFamily.en> ;
    reg:name "relatedCollectiveAgentFamily"@en ;
    reg:status <http://metadataregistry.org/uri/RegStatus/1001> ;
    rdfs:domain <http://rdaregistry.info/Elements/c/C10008> ;
    rdfs:isDefinedBy <http://rdaregistry.info/Elements/a/> ;
    rdfs:subPropertyOf <http://rdaregistry.info/Elements/a/P50324>,
        <http://rdaregistry.info/Elements/a/P50341> ;
    skos:definition "Relates a family to a collective agent associated with a family."@en .

<http://rdaregistry.info/Elements/a/P50357> a rdf:Property ;
    rdfs:label "has related work (collective agent)"@en ;
    reg:hasSubproperty <http://rdaregistry.info/Elements/a/datatype/P50357>,
        <http://rdaregistry.info/Elements/a/object/P50357> ;
    reg:lexicalAlias <http://rdaregistry.info/Elements/a/relatedWorkCollectiveAgent.en> ;
    reg:name "relatedWorkCollectiveAgent"@en ;
    reg:status <http://metadataregistry.org/uri/RegStatus/1001> ;
    rdfs:domain <http://rdaregistry.info/Elements/c/C10011> ;
    rdfs:isDefinedBy <http://rdaregistry.info/Elements/a/> ;
    rdfs:subPropertyOf <http://rdaregistry.info/Elements/a/P50305>,
        <http://rdaregistry.info/Elements/a/P50360> ;
    skos:definition "Relates a collective agent to a work associated with a collective agent being described."@en .

<http://rdaregistry.info/Elements/a/P50359> a rdf:Property ;
    rdfs:label "has related corporate body (collective agent)"@en ;
    reg:hasSubproperty <http://rdaregistry.info/Elements/a/datatype/P50359>,
        <http://rdaregistry.info/Elements/a/object/P50359> ;
    reg:lexicalAlias <http://rdaregistry.info/Elements/a/relatedCorporateBodyCollectiveAgent.en> ;
    reg:name "relatedCorporateBodyCollectiveAgent"@en ;
    reg:status <http://metadataregistry.org/uri/RegStatus/1001> ;
    rdfs:domain <http://rdaregistry.info/Elements/c/C10011> ;
    rdfs:isDefinedBy <http://rdaregistry.info/Elements/a/> ;
    rdfs:subPropertyOf <http://rdaregistry.info/Elements/a/P50218>,
        <http://rdaregistry.info/Elements/a/P50341> ;
    skos:definition "Relates a collective agent to a corporate body associated with a collective agent."@en .

<http://rdaregistry.info/Elements/a/P50361> a rdf:Property ;
    rdfs:label "has related expression (collective agent)"@en ;
    reg:hasSubproperty <http://rdaregistry.info/Elements/a/datatype/P50361>,
        <http://rdaregistry.info/Elements/a/object/P50361> ;
    reg:lexicalAlias <http://rdaregistry.info/Elements/a/relatedExpressionCollectiveAgent.en> ;
    reg:name "relatedExpressionCollectiveAgent"@en ;
    reg:status <http://metadataregistry.org/uri/RegStatus/1001> ;
    rdfs:domain <http://rdaregistry.info/Elements/c/C10011> ;
    rdfs:isDefinedBy <http://rdaregistry.info/Elements/a/> ;
    rdfs:subPropertyOf <http://rdaregistry.info/Elements/a/P50306>,
        <http://rdaregistry.info/Elements/a/P50360> ;
    skos:definition "Relates a collective agent to an expression associated with a collective agent."@en .

<http://rdaregistry.info/Elements/a/P50362> a rdf:Property ;
    rdfs:label "has related family (collective agent)"@en ;
    reg:hasSubproperty <http://rdaregistry.info/Elements/a/datatype/P50362>,
        <http://rdaregistry.info/Elements/a/object/P50362> ;
    reg:lexicalAlias <http://rdaregistry.info/Elements/a/relatedFamilyCollectiveAgent.en> ;
    reg:name "relatedFamilyCollectiveAgent"@en ;
    reg:status <http://metadataregistry.org/uri/RegStatus/1001> ;
    rdfs:domain <http://rdaregistry.info/Elements/c/C10011> ;
    rdfs:isDefinedBy <http://rdaregistry.info/Elements/a/> ;
    rdfs:subPropertyOf <http://rdaregistry.info/Elements/a/P50219>,
        <http://rdaregistry.info/Elements/a/P50341> ;
    skos:definition "Relates a collective agent to a family associated with a collective agent."@en .

<http://rdaregistry.info/Elements/a/P50363> a rdf:Property ;
    rdfs:label "has related item (collective agent)"@en ;
    reg:hasSubproperty <http://rdaregistry.info/Elements/a/datatype/P50363>,
        <http://rdaregistry.info/Elements/a/object/P50363> ;
    reg:lexicalAlias <http://rdaregistry.info/Elements/a/relatedItemCollectiveAgent.en> ;
    reg:name "relatedItemCollectiveAgent"@en ;
    reg:status <http://metadataregistry.org/uri/RegStatus/1001> ;
    rdfs:domain <http://rdaregistry.info/Elements/c/C10011> ;
    rdfs:isDefinedBy <http://rdaregistry.info/Elements/a/> ;
    rdfs:subPropertyOf <http://rdaregistry.info/Elements/a/P50308>,
        <http://rdaregistry.info/Elements/a/P50360> ;
    skos:definition "Relates a collective agent to an item associated with a collective agent."@en .

<http://rdaregistry.info/Elements/a/P50364> a rdf:Property ;
    rdfs:label "has related manifestation (collective agent)"@en ;
    reg:hasSubproperty <http://rdaregistry.info/Elements/a/datatype/P50364>,
        <http://rdaregistry.info/Elements/a/object/P50364> ;
    reg:lexicalAlias <http://rdaregistry.info/Elements/a/relatedManifestationCollectiveAgent.en> ;
    reg:name "relatedManifestationCollectiveAgent"@en ;
    reg:status <http://metadataregistry.org/uri/RegStatus/1001> ;
    rdfs:domain <http://rdaregistry.info/Elements/c/C10011> ;
    rdfs:isDefinedBy <http://rdaregistry.info/Elements/a/> ;
    rdfs:subPropertyOf <http://rdaregistry.info/Elements/a/P50307>,
        <http://rdaregistry.info/Elements/a/P50360> ;
    skos:definition "Relates a collective agent to a manifestation associated with a collective agent."@en .

<http://rdaregistry.info/Elements/a/P50365> a rdf:Property ;
    rdfs:label "has related person (collective agent)"@en ;
    reg:hasSubproperty <http://rdaregistry.info/Elements/a/datatype/P50365>,
        <http://rdaregistry.info/Elements/a/object/P50365> ;
    reg:lexicalAlias <http://rdaregistry.info/Elements/a/relatedPersonCollectiveAgent.en> ;
    reg:name "relatedPersonCollectiveAgent"@en ;
    reg:status <http://metadataregistry.org/uri/RegStatus/1001> ;
    rdfs:domain <http://rdaregistry.info/Elements/c/C10011> ;
    rdfs:isDefinedBy <http://rdaregistry.info/Elements/a/> ;
    rdfs:subPropertyOf <http://rdaregistry.info/Elements/a/P50220>,
        <http://rdaregistry.info/Elements/a/P50358> ;
    skos:definition "Relates a collective agent to a person associated with a collective agent."@en .

<http://rdaregistry.info/Elements/a/P50040> a rdf:Property ;
    rdfs:label "has date associated with corporate body"@en,
        "a pour date associée à la collectivité"@fr,
        "har tid förknippad med institutionen"@sv ;
    rdakit:instructionNumber "11.4" ;
    rdakit:toolkitDefinition "A significant date associated with the history of a corporate body."@en,
        "Una fecha significativa asociada con la historia de una entidad corporativa, incluyendo fechas de conferencia, fechas de terminación, y período de actividad."@es,
        "Date importante associée à l’histoire d’une collectivité, telle que la date de fondation ou la date de cessation."@fr ;
    rdakit:toolkitLabel "date associated with corporate body"@en,
        "fecha asociada con la entidad corporativa"@es,
        "date associée à la collectivité"@fr,
        "tid förknippad med institutionen"@sv ;
    reg:hasSubproperty <http://rdaregistry.info/Elements/a/P50037>,
        <http://rdaregistry.info/Elements/a/P50038>,
        <http://rdaregistry.info/Elements/a/P50039>,
        <http://rdaregistry.info/Elements/a/datatype/P50040> ;
    reg:hasUnconstrained <http://rdaregistry.info/Elements/u/P60324> ;
    reg:lexicalAlias <http://rdaregistry.info/Elements/a/dateAssociatedWithCorporateBody.en> ;
    reg:name "dateAssociatedWithCorporateBody"@en ;
    reg:status <http://metadataregistry.org/uri/RegStatus/1001> ;
    rdfs:domain <http://rdaregistry.info/Elements/c/C10005> ;
    rdfs:isDefinedBy <http://rdaregistry.info/Elements/a/> ;
    skos:definition "Relates a corporate body to a significant date associated with the history of a corporate body."@en,
        "Met une collectivité en relation avec une date importante associée à l’histoire d’une collectivité, telle que la date de fondation ou la date de cessation."@fr .

<http://rdaregistry.info/Elements/a/P50205> a rdf:Property ;
    rdfs:label "is director of"@en,
        "est le réalisateur de"@fr ;
    rdakit:instructionNumber "18.5" ;
    rdakit:toolkitDefinition "A work that involves a responsibility for the general management and supervision of a filmed performance, a radio or television program, etc."@en,
        "Personne, famille ou collectivité responsable de la gestion et de la supervision générales d’une prestation filmée, d’une émission de radio ou de télévision, etc."@fr ;
    rdakit:toolkitLabel "director of"@en,
        "réalisateur de"@fr ;
    reg:hasSubproperty <http://rdaregistry.info/Elements/a/P50048>,
        <http://rdaregistry.info/Elements/a/P50049>,
        <http://rdaregistry.info/Elements/a/P50050>,
        <http://rdaregistry.info/Elements/a/datatype/P50205>,
        <http://rdaregistry.info/Elements/a/object/P50205> ;
    reg:hasUnconstrained <http://rdaregistry.info/Elements/u/P60673> ;
    reg:lexicalAlias <http://rdaregistry.info/Elements/a/directorOf.en> ;
    reg:name "directorOf"@en ;
    reg:status <http://metadataregistry.org/uri/RegStatus/1001> ;
    rdfs:domain <http://rdaregistry.info/Elements/c/C10002> ;
    rdfs:isDefinedBy <http://rdaregistry.info/Elements/a/> ;
    rdfs:subPropertyOf <http://rdaregistry.info/Elements/a/P50131> ;
    skos:definition "Relates an agent responsible for the general management and supervision of a filmed performance, a radio or television program, etc. to a work."@en,
        "Met une personne, famille ou collectivité responsable de la gestion et de la supervision générales d’une prestation filmée, d’une émission de radio ou de télévision, etc. en relation avec l’œuvre."@fr .

<http://rdaregistry.info/Elements/a/P50219> a rdf:Property ;
    rdfs:label "has related family (agent)"@en ;
    reg:hasSubproperty <http://rdaregistry.info/Elements/a/datatype/P50219>,
        <http://rdaregistry.info/Elements/a/object/P50219> ;
    reg:lexicalAlias <http://rdaregistry.info/Elements/a/relatedFamilyAgent.en> ;
    reg:name "relatedFamilyAgent"@en ;
    reg:status <http://metadataregistry.org/uri/RegStatus/1001> ;
    rdfs:domain <http://rdaregistry.info/Elements/c/C10002> ;
    rdfs:isDefinedBy <http://rdaregistry.info/Elements/a/> ;
    rdfs:subPropertyOf <http://rdaregistry.info/Elements/a/P50337>,
        <http://rdaregistry.info/Elements/x/P00006> ;
    skos:definition "Relates an agent to a family associated with an agent being identified."@en .

<http://rdaregistry.info/Elements/a/P50274> a rdf:Property ;
    rdfs:label "has colleague"@en ;
    rdakit:instructionNumber "29.5" ;
    rdakit:toolkitDefinition "A fellow member of a profession, staff, or academic faculty."@en ;
    rdakit:toolkitLabel "colleague"@en ;
    reg:hasSubproperty <http://rdaregistry.info/Elements/a/datatype/P50274>,
        <http://rdaregistry.info/Elements/a/object/P50274>,
        <http://rdaregistry.info/Elements/a/object/P50275>,
        <http://rdaregistry.info/Elements/a/object/P50276>,
        <http://rdaregistry.info/Elements/a/object/P50277>,
        <http://rdaregistry.info/Elements/a/object/P50278> ;
    reg:hasUnconstrained <http://rdaregistry.info/Elements/u/P60853> ;
    reg:lexicalAlias <http://rdaregistry.info/Elements/a/colleague.en> ;
    reg:name "colleague"@en ;
    reg:status <http://metadataregistry.org/uri/RegStatus/1001> ;
    rdfs:domain <http://rdaregistry.info/Elements/c/C10004> ;
    rdfs:isDefinedBy <http://rdaregistry.info/Elements/a/> ;
    rdfs:subPropertyOf <http://rdaregistry.info/Elements/a/P50220> ;
    skos:definition "Relates a person to a fellow member of a profession, staff, or academic faculty."@en .

<http://rdaregistry.info/Elements/a/P50333> a rdf:Property ;
    rdfs:label "has related agent (corporate body)"@en ;
    reg:hasSubproperty <http://rdaregistry.info/Elements/a/P50334>,
        <http://rdaregistry.info/Elements/a/P50335>,
        <http://rdaregistry.info/Elements/a/P50336>,
        <http://rdaregistry.info/Elements/a/datatype/P50333>,
        <http://rdaregistry.info/Elements/a/object/P50333> ;
    reg:lexicalAlias <http://rdaregistry.info/Elements/a/relatedAgentCorporateBody.en> ;
    reg:name "relatedAgentCorporateBody"@en ;
    reg:status <http://metadataregistry.org/uri/RegStatus/1001> ;
    rdfs:domain <http://rdaregistry.info/Elements/c/C10005> ;
    rdfs:isDefinedBy <http://rdaregistry.info/Elements/a/> ;
    rdfs:subPropertyOf <http://rdaregistry.info/Elements/a/P50309>,
        <http://rdaregistry.info/Elements/a/P50358> ;
    skos:definition "Relates a corporate body to an agent associated with a corporate body being described."@en .

<http://rdaregistry.info/Elements/a/P50192> a rdf:Property ;
    rdfs:label "is artist of"@en,
        "est l’artiste de"@fr ;
    rdakit:instructionNumber "18.5" ;
    rdakit:toolkitDefinition "A work that involves a creation responsibility for conceiving, and often implementing, an original graphic design, drawing, painting, etc."@en,
        "Personne, famille ou collectivité responsable de la création d’une œuvre par la conception et souvent par la réalisation d’un graphisme, d’une peinture, d’un dessin, etc. original."@fr ;
    rdakit:toolkitLabel "artist of"@en,
        "artiste de"@fr ;
    reg:hasSubproperty <http://rdaregistry.info/Elements/a/P50222>,
        <http://rdaregistry.info/Elements/a/datatype/P50192>,
        <http://rdaregistry.info/Elements/a/object/P50192>,
        <http://rdaregistry.info/Elements/a/object/P50246>,
        <http://rdaregistry.info/Elements/a/object/P50247> ;
    reg:hasUnconstrained <http://rdaregistry.info/Elements/u/P60660> ;
    reg:lexicalAlias <http://rdaregistry.info/Elements/a/artistOf.en> ;
    reg:name "artistOf"@en ;
    reg:status <http://metadataregistry.org/uri/RegStatus/1001> ;
    rdfs:domain <http://rdaregistry.info/Elements/c/C10002> ;
    rdfs:isDefinedBy <http://rdaregistry.info/Elements/a/> ;
    rdfs:subPropertyOf <http://rdaregistry.info/Elements/a/P50204> ;
    skos:definition "Relates an agent responsible for creating a work by conceiving, and often implementing, an original graphic design, drawing, painting, etc. to a work."@en,
        "Met une personne, famille ou collectivité responsable de la création d’une œuvre par la conception et souvent par la réalisation d’un graphisme, d’une peinture, d’un dessin, etc. original en relation avec l’œuvre."@fr .

<http://rdaregistry.info/Elements/a/P50201> a rdf:Property ;
    rdfs:label "is producer of"@en,
        "est le producteur de"@fr ;
    rdakit:toolkitDefinition "A work that involves a responsibility for most of the business aspects of a production for screen, sound recording, television, webcast, etc."@en,
        "Personne, famille ou collectivité responsable de la majeure partie des aspects financiers, techniques et artistiques de la production d’un film, d’un enregistrement audio, d’une émission de télévision, d’une webémission, etc."@fr ;
    rdakit:toolkitLabel "producer of"@en,
        "producteur de"@fr ;
    reg:hasSubproperty <http://rdaregistry.info/Elements/a/P50213>,
        <http://rdaregistry.info/Elements/a/P50214>,
        <http://rdaregistry.info/Elements/a/P50215>,
        <http://rdaregistry.info/Elements/a/datatype/P50201>,
        <http://rdaregistry.info/Elements/a/object/P50201>,
        <http://rdaregistry.info/Elements/a/object/P50295> ;
    reg:hasUnconstrained <http://rdaregistry.info/Elements/u/P60668> ;
    reg:lexicalAlias <http://rdaregistry.info/Elements/a/producerOf.en> ;
    reg:name "producerOf"@en ;
    reg:status <http://metadataregistry.org/uri/RegStatus/1001> ;
    rdfs:domain <http://rdaregistry.info/Elements/c/C10002> ;
    rdfs:isDefinedBy <http://rdaregistry.info/Elements/a/> ;
    rdfs:subPropertyOf <http://rdaregistry.info/Elements/a/P50131> ;
    skos:definition "Relates an agent responsible for most of the business aspects of a production for screen, sound recording, television, webcast, etc. to a work."@en,
        "Met une personne, famille ou collectivité responsable de la majeure partie des aspects financiers, techniques et artistiques de la production d’un film, d’un enregistrement audio, d’une émission de télévision, d’une webémission, etc. en relation avec l’œuvre."@fr ;
    skos:scopeNote "A producer is generally responsible for fund raising, managing the production, hiring key personnel, arranging for distributors, etc."@en,
        "Le producteur est généralement responsable d’assurer le financement, de gérer la production, de recruter le personnel clé, d’organiser la distribution, etc."@fr .

<http://rdaregistry.info/Elements/a/P50218> a rdf:Property ;
    rdfs:label "has related corporate body (agent)"@en ;
    reg:hasSubproperty <http://rdaregistry.info/Elements/a/datatype/P50218>,
        <http://rdaregistry.info/Elements/a/object/P50218>,
        <http://rdaregistry.info/Elements/a/object/P50288> ;
    reg:lexicalAlias <http://rdaregistry.info/Elements/a/relatedCorporateBodyAgent.en> ;
    reg:name "relatedCorporateBodyAgent"@en ;
    reg:status <http://metadataregistry.org/uri/RegStatus/1001> ;
    rdfs:domain <http://rdaregistry.info/Elements/c/C10002> ;
    rdfs:isDefinedBy <http://rdaregistry.info/Elements/a/> ;
    rdfs:subPropertyOf <http://rdaregistry.info/Elements/a/P50337>,
        <http://rdaregistry.info/Elements/x/P00006> ;
    skos:definition "Relates an agent to a corporate body associated with an agent being identified."@en .

<http://rdaregistry.info/Elements/a/P50306> a rdf:Property ;
    rdfs:label "has related expression (agent)"@en ;
    reg:hasSubproperty <http://rdaregistry.info/Elements/a/P50330>,
        <http://rdaregistry.info/Elements/a/datatype/P50306>,
        <http://rdaregistry.info/Elements/a/object/P50306> ;
    reg:lexicalAlias <http://rdaregistry.info/Elements/a/relatedExpressionAgent.en> ;
    reg:name "relatedExpressionAgent"@en ;
    reg:status <http://metadataregistry.org/uri/RegStatus/1001> ;
    rdfs:domain <http://rdaregistry.info/Elements/c/C10002> ;
    rdfs:isDefinedBy <http://rdaregistry.info/Elements/a/> ;
    rdfs:subPropertyOf <http://rdaregistry.info/Elements/a/P50304>,
        <http://rdaregistry.info/Elements/x/P00006> ;
    skos:definition "Relates an agent to an expression associated with an agent being described."@en .

<http://rdaregistry.info/Elements/a/P50328> a rdf:Property ;
    rdfs:label "has related entity (corporate body)"@en ;
    reg:hasSubproperty <http://rdaregistry.info/Elements/a/P50349>,
        <http://rdaregistry.info/Elements/a/P50350>,
        <http://rdaregistry.info/Elements/a/P50351>,
        <http://rdaregistry.info/Elements/a/P50352>,
        <http://rdaregistry.info/Elements/a/datatype/P50328>,
        <http://rdaregistry.info/Elements/a/object/P50328> ;
    reg:lexicalAlias <http://rdaregistry.info/Elements/a/relatedEntityCorporateBody.en> ;
    reg:name "relatedEntityCorporateBody"@en ;
    reg:status <http://metadataregistry.org/uri/RegStatus/1001> ;
    rdfs:domain <http://rdaregistry.info/Elements/c/C10005> ;
    rdfs:isDefinedBy <http://rdaregistry.info/Elements/a/> ;
    rdfs:subPropertyOf <http://rdaregistry.info/Elements/a/P50360> ;
    skos:definition "Relates a corporate body to an entity associated with a corporate body being described."@en .

<http://rdaregistry.info/Elements/a/P50337> a rdf:Property ;
    rdfs:label "has related collective agent (agent)"@en ;
    reg:hasSubproperty <http://rdaregistry.info/Elements/a/P50218>,
        <http://rdaregistry.info/Elements/a/P50219>,
        <http://rdaregistry.info/Elements/a/datatype/P50337>,
        <http://rdaregistry.info/Elements/a/object/P50337> ;
    reg:lexicalAlias <http://rdaregistry.info/Elements/a/relatedCollectiveAgentAgent.en> ;
    reg:name "relatedCollectiveAgentAgent"@en ;
    reg:status <http://metadataregistry.org/uri/RegStatus/1001> ;
    rdfs:domain <http://rdaregistry.info/Elements/c/C10002> ;
    rdfs:isDefinedBy <http://rdaregistry.info/Elements/a/> ;
    rdfs:subPropertyOf <http://rdaregistry.info/Elements/a/P50309>,
        <http://rdaregistry.info/Elements/x/P00006> ;
    skos:definition "Relates an agent to a collective agent associated with an agent."@en .

<http://rdaregistry.info/Elements/a/P50341> a rdf:Property ;
    rdfs:label "has related collective agent (collective agent)"@en ;
    reg:hasSubproperty <http://rdaregistry.info/Elements/a/P50359>,
        <http://rdaregistry.info/Elements/a/P50362>,
        <http://rdaregistry.info/Elements/a/datatype/P50341>,
        <http://rdaregistry.info/Elements/a/object/P50341> ;
    reg:lexicalAlias <http://rdaregistry.info/Elements/a/relatedCollectiveAgentCollectiveAgent.en> ;
    reg:name "relatedCollectiveAgentCollectiveAgent"@en ;
    reg:status <http://metadataregistry.org/uri/RegStatus/1001> ;
    rdfs:domain <http://rdaregistry.info/Elements/c/C10011> ;
    rdfs:isDefinedBy <http://rdaregistry.info/Elements/a/> ;
    rdfs:subPropertyOf <http://rdaregistry.info/Elements/a/P50337>,
        <http://rdaregistry.info/Elements/a/P50358> ;
    skos:definition "Relates a collective agent to a collective agent associated with a collective agent."@en .

<http://rdaregistry.info/Elements/a/P50358> a rdf:Property ;
    rdfs:label "has related agent (collective agent)"@en ;
    reg:hasSubproperty <http://rdaregistry.info/Elements/a/P50218>,
        <http://rdaregistry.info/Elements/a/P50219>,
        <http://rdaregistry.info/Elements/a/P50341>,
        <http://rdaregistry.info/Elements/a/P50365>,
        <http://rdaregistry.info/Elements/a/datatype/P50358>,
        <http://rdaregistry.info/Elements/a/object/P50358> ;
    reg:lexicalAlias <http://rdaregistry.info/Elements/a/relatedAgentCollectiveAgent.en> ;
    reg:name "relatedAgentCollectiveAgent"@en ;
    reg:status <http://metadataregistry.org/uri/RegStatus/1001> ;
    rdfs:domain <http://rdaregistry.info/Elements/c/C10011> ;
    rdfs:isDefinedBy <http://rdaregistry.info/Elements/a/> ;
    rdfs:subPropertyOf <http://rdaregistry.info/Elements/a/P50309>,
        <http://rdaregistry.info/Elements/a/P50360> ;
    skos:definition "Relates a collective agent to an agent associated with a collective agent,"@en .

<http://rdaregistry.info/Elements/a/P50305> a rdf:Property ;
    rdfs:label "has related work (agent)"@en ;
    reg:hasSubproperty <http://rdaregistry.info/Elements/a/P50329>,
        <http://rdaregistry.info/Elements/a/datatype/P50305>,
        <http://rdaregistry.info/Elements/a/object/P50305> ;
    reg:lexicalAlias <http://rdaregistry.info/Elements/a/relatedWorkAgent.en> ;
    reg:name "relatedWorkAgent"@en ;
    reg:status <http://metadataregistry.org/uri/RegStatus/1001> ;
    rdfs:domain <http://rdaregistry.info/Elements/c/C10002> ;
    rdfs:isDefinedBy <http://rdaregistry.info/Elements/a/> ;
    rdfs:subPropertyOf <http://rdaregistry.info/Elements/a/P50304>,
        <http://rdaregistry.info/Elements/x/P00006> ;
    skos:definition "Relates an agent to a work associated with an agent being described."@en .

<http://rdaregistry.info/Elements/a/P50309> a rdf:Property ;
    rdfs:label "has related agent (agent)"@en ;
    reg:hasSubproperty <http://rdaregistry.info/Elements/a/P50220>,
        <http://rdaregistry.info/Elements/a/P50333>,
        <http://rdaregistry.info/Elements/a/P50337>,
        <http://rdaregistry.info/Elements/a/datatype/P50309>,
        <http://rdaregistry.info/Elements/a/object/P50309> ;
    reg:lexicalAlias <http://rdaregistry.info/Elements/a/relatedAgentAgent.en> ;
    reg:name "relatedAgentAgent"@en ;
    reg:status <http://metadataregistry.org/uri/RegStatus/1001> ;
    rdfs:domain <http://rdaregistry.info/Elements/c/C10002> ;
    rdfs:isDefinedBy <http://rdaregistry.info/Elements/a/> ;
    rdfs:subPropertyOf <http://rdaregistry.info/Elements/a/P50304>,
        <http://rdaregistry.info/Elements/x/P00006> ;
    skos:definition "Relates an agent to an agent associated with an agent being described."@en .

<http://rdaregistry.info/Elements/a/P50308> a rdf:Property ;
    rdfs:label "has related item (agent)"@en ;
    reg:hasSubproperty <http://rdaregistry.info/Elements/a/P50332>,
        <http://rdaregistry.info/Elements/a/datatype/P50308>,
        <http://rdaregistry.info/Elements/a/object/P50308> ;
    reg:lexicalAlias <http://rdaregistry.info/Elements/a/relatedItemAgent.en> ;
    reg:name "relatedItemAgent"@en ;
    reg:status <http://metadataregistry.org/uri/RegStatus/1001> ;
    rdfs:domain <http://rdaregistry.info/Elements/c/C10002> ;
    rdfs:isDefinedBy <http://rdaregistry.info/Elements/a/> ;
    rdfs:subPropertyOf <http://rdaregistry.info/Elements/a/P50304>,
        <http://rdaregistry.info/Elements/x/P00006> ;
    skos:definition "Relates an agent to an item associated with an agent being described."@en .

<http://rdaregistry.info/Elements/a/P50154> a rdf:Property ;
    rdfs:label "is writer of supplementary textual content of"@en,
        "est l’auteur de contenu textuel supplémentaire de"@fr ;
    rdakit:instructionNumber "18.5" ;
    rdakit:toolkitDefinition "An expression of a work that incorporates a contribution of providing supplementary textual content, such as an introduction or a preface, to an original work."@en,
        "Personne, famille ou collectivité contribuant à une expression d’une œuvre en fournissant du contenu textuel supplémentaire (par exemple, une introduction, une préface) à l’œuvre originale."@fr ;
    rdakit:toolkitLabel "writer of supplementary textual content of"@en,
        "auteur de contenu textuel supplémentaire de"@fr ;
    reg:hasSubproperty <http://rdaregistry.info/Elements/a/P50138>,
        <http://rdaregistry.info/Elements/a/P50149>,
        <http://rdaregistry.info/Elements/a/P50152>,
        <http://rdaregistry.info/Elements/a/P50153>,
        <http://rdaregistry.info/Elements/a/datatype/P50154>,
        <http://rdaregistry.info/Elements/a/object/P50154>,
        <http://rdaregistry.info/Elements/a/object/P50254> ;
    reg:hasUnconstrained <http://rdaregistry.info/Elements/u/P60620> ;
    reg:lexicalAlias <http://rdaregistry.info/Elements/a/writerOfSupplementaryTextualContentOf.en> ;
    reg:name "writerOfSupplementaryTextualContentOf"@en ;
    reg:status <http://metadataregistry.org/uri/RegStatus/1001> ;
    rdfs:domain <http://rdaregistry.info/Elements/c/C10002> ;
    rdfs:isDefinedBy <http://rdaregistry.info/Elements/a/> ;
    rdfs:subPropertyOf <http://rdaregistry.info/Elements/a/P50161> ;
    skos:definition "Relates an agent contributing to an expression of a work by providing supplementary textual content, such as an introduction or a preface, to an original work to an expression."@en,
        "Met une personne, famille ou collectivité contribuant à une expression d’une œuvre en fournissant du contenu textuel supplémentaire (par exemple, une introduction, une préface) à l’œuvre originale en relation avec l’expression."@fr .

<http://rdaregistry.info/Elements/a/P50195> a rdf:Property ;
    rdfs:label "is author of"@en,
        "est l’auteur de"@fr ;
    rdakit:instructionNumber "18.5" ;
    rdakit:toolkitDefinition "A work that is primarily textual in content, regardless of media  type or genre, that involves a creation responsibility."@en,
        "Personne, famille ou collectivité responsable de la création d’une œuvre dont le contenu est principalement textuel quel que soit le type de média (par exemple, texte imprimé, parole énoncée, texte électronique, texte tactile) ou le genre (par exemple, poèmes, romans, scénarios, blogues)."@fr ;
    rdakit:toolkitLabel "author of"@en,
        "auteur de"@fr ;
    reg:hasSubproperty <http://rdaregistry.info/Elements/a/P50223>,
        <http://rdaregistry.info/Elements/a/P50224>,
        <http://rdaregistry.info/Elements/a/P50225>,
        <http://rdaregistry.info/Elements/a/datatype/P50195>,
        <http://rdaregistry.info/Elements/a/object/P50195>,
        <http://rdaregistry.info/Elements/a/object/P50248> ;
    reg:hasUnconstrained <http://rdaregistry.info/Elements/u/P60663> ;
    reg:lexicalAlias <http://rdaregistry.info/Elements/a/authorOf.en> ;
    reg:name "authorOf"@en ;
    reg:status <http://metadataregistry.org/uri/RegStatus/1001> ;
    rdfs:domain <http://rdaregistry.info/Elements/c/C10002> ;
    rdfs:isDefinedBy <http://rdaregistry.info/Elements/a/> ;
    rdfs:subPropertyOf <http://rdaregistry.info/Elements/a/P50204> ;
    skos:definition "Relates an agent responsible for creating a work that is primarily textual in content, regardless of media  type or genre to a work."@en,
        "Met une personne, famille ou collectivité responsable de la création d’une œuvre dont le contenu est principalement textuel quel que soit le type de média (par exemple, texte imprimé, parole énoncée, texte électronique, texte tactile) ou le genre (par exemple, poèmes, romans, scénarios, blogues) en relation avec l’œuvre."@fr .

<http://rdaregistry.info/Elements/a/P50182> a rdf:Property ;
    rdfs:label "is other agent associated with item of"@en,
        "est l’autre personne, famille ou collectivité associée à un item de"@fr ;
    rdakit:toolkitDefinition "An item associated with an agent other than an owner or custodian."@en,
        "Personne, famille ou collectivité, autre qu’un propriétaire ou un dépositaire, associée à un item."@fr ;
    rdakit:toolkitLabel "other agent associated with item of"@en,
        "autre personne, famille ou collectivité associée à un item de"@fr ;
    reg:hasSubproperty <http://rdaregistry.info/Elements/a/P50092>,
        <http://rdaregistry.info/Elements/a/P50123>,
        <http://rdaregistry.info/Elements/a/P50125>,
        <http://rdaregistry.info/Elements/a/P50128>,
        <http://rdaregistry.info/Elements/a/P50129>,
        <http://rdaregistry.info/Elements/a/P50133>,
        <http://rdaregistry.info/Elements/a/P50167>,
        <http://rdaregistry.info/Elements/a/P50206>,
        <http://rdaregistry.info/Elements/a/P50210>,
        <http://rdaregistry.info/Elements/a/datatype/P50182>,
        <http://rdaregistry.info/Elements/a/object/P50182> ;
    reg:hasUnconstrained <http://rdaregistry.info/Elements/u/P60602> ;
    reg:lexicalAlias <http://rdaregistry.info/Elements/a/otherAgentItemOf.en> ;
    reg:name "otherAgentItemOf"@en ;
    reg:status <http://metadataregistry.org/uri/RegStatus/1001> ;
    rdfs:domain <http://rdaregistry.info/Elements/c/C10002> ;
    rdfs:isDefinedBy <http://rdaregistry.info/Elements/a/> ;
    rdfs:subPropertyOf <http://rdaregistry.info/Elements/a/P50308> ;
    skos:definition "Relates an agent other than an owner or custodian associated with an item to an item."@en,
        "Met une personne, famille ou collectivité, autre qu’un propriétaire ou un dépositaire, associée à un item en relation avec l’item."@fr ;
    skos:scopeNote "Curators, binders, restorationists, etc., are included."@en,
        "Comprend les conservateurs, les relieurs, les restaurateurs, etc."@fr .

<http://rdaregistry.info/Elements/a/P50220> a rdf:Property ;
    rdfs:label "has related person (agent)"@en ;
    reg:hasSubproperty <http://rdaregistry.info/Elements/a/datatype/P50220>,
        <http://rdaregistry.info/Elements/a/object/P50220>,
        <http://rdaregistry.info/Elements/a/object/P50274>,
        <http://rdaregistry.info/Elements/a/object/P50279>,
        <http://rdaregistry.info/Elements/a/object/P50280>,
        <http://rdaregistry.info/Elements/a/object/P50281>,
        <http://rdaregistry.info/Elements/a/object/P50282>,
        <http://rdaregistry.info/Elements/a/object/P50283> ;
    reg:lexicalAlias <http://rdaregistry.info/Elements/a/relatedPersonAgent.en> ;
    reg:name "relatedPersonAgent"@en ;
    reg:status <http://metadataregistry.org/uri/RegStatus/1001> ;
    rdfs:domain <http://rdaregistry.info/Elements/c/C10002> ;
    rdfs:isDefinedBy <http://rdaregistry.info/Elements/a/> ;
    rdfs:subPropertyOf <http://rdaregistry.info/Elements/a/P50309>,
        <http://rdaregistry.info/Elements/x/P00006> ;
    skos:definition "Relates an agent to a person who is associated with an agent being identified."@en .

<http://rdaregistry.info/Elements/a/P50307> a rdf:Property ;
    rdfs:label "has related manifestation (agent)"@en ;
    reg:hasSubproperty <http://rdaregistry.info/Elements/a/P50331>,
        <http://rdaregistry.info/Elements/a/datatype/P50307>,
        <http://rdaregistry.info/Elements/a/object/P50307> ;
    reg:lexicalAlias <http://rdaregistry.info/Elements/a/relatedManifestationAgent.en> ;
    reg:name "relatedManifestationAgent"@en ;
    reg:status <http://metadataregistry.org/uri/RegStatus/1001> ;
    rdfs:domain <http://rdaregistry.info/Elements/c/C10002> ;
    rdfs:isDefinedBy <http://rdaregistry.info/Elements/a/> ;
    rdfs:subPropertyOf <http://rdaregistry.info/Elements/a/P50304>,
        <http://rdaregistry.info/Elements/x/P00006> ;
    skos:definition "Relates an agent to a manifestation associated with an agent being described."@en .

<http://rdaregistry.info/Elements/a/P50310> a rdf:Property ;
    rdfs:label "has related entity (person)"@en ;
    reg:hasSubproperty <http://rdaregistry.info/Elements/a/P50311>,
        <http://rdaregistry.info/Elements/a/P50312>,
        <http://rdaregistry.info/Elements/a/P50313>,
        <http://rdaregistry.info/Elements/a/P50314>,
        <http://rdaregistry.info/Elements/a/P50315>,
        <http://rdaregistry.info/Elements/a/P50346>,
        <http://rdaregistry.info/Elements/a/P50347>,
        <http://rdaregistry.info/Elements/a/P50348>,
        <http://rdaregistry.info/Elements/a/datatype/P50310>,
        <http://rdaregistry.info/Elements/a/object/P50310> ;
    reg:lexicalAlias <http://rdaregistry.info/Elements/a/relatedEntityPerson.en> ;
    reg:name "relatedEntityPerson"@en ;
    reg:status <http://metadataregistry.org/uri/RegStatus/1001> ;
    rdfs:domain <http://rdaregistry.info/Elements/c/C10004> ;
    rdfs:isDefinedBy <http://rdaregistry.info/Elements/a/> ;
    rdfs:subPropertyOf <http://rdaregistry.info/Elements/a/P50304> ;
    skos:definition "Relates a person to an entity associated with a person being described."@en .

<http://rdaregistry.info/Elements/a/P50319> a rdf:Property ;
    rdfs:label "has related entity (family)"@en ;
    reg:hasSubproperty <http://rdaregistry.info/Elements/a/P50320>,
        <http://rdaregistry.info/Elements/a/P50321>,
        <http://rdaregistry.info/Elements/a/P50322>,
        <http://rdaregistry.info/Elements/a/P50323>,
        <http://rdaregistry.info/Elements/a/P50324>,
        <http://rdaregistry.info/Elements/a/P50354>,
        <http://rdaregistry.info/Elements/a/P50355>,
        <http://rdaregistry.info/Elements/a/P50356>,
        <http://rdaregistry.info/Elements/a/datatype/P50319>,
        <http://rdaregistry.info/Elements/a/object/P50319> ;
    reg:lexicalAlias <http://rdaregistry.info/Elements/a/relatedEntityFamily.en> ;
    reg:name "relatedEntityFamily"@en ;
    reg:status <http://metadataregistry.org/uri/RegStatus/1001> ;
    rdfs:domain <http://rdaregistry.info/Elements/c/C10008> ;
    rdfs:isDefinedBy <http://rdaregistry.info/Elements/a/> ;
    rdfs:subPropertyOf <http://rdaregistry.info/Elements/a/P50360> ;
    skos:definition "Relates a family to an entity associated with a family being described."@en .

<http://rdaregistry.info/Elements/a/P50304> a rdf:Property ;
    rdfs:label "has related entity (agent)"@en ;
    reg:hasSubproperty <http://rdaregistry.info/Elements/a/P50305>,
        <http://rdaregistry.info/Elements/a/P50306>,
        <http://rdaregistry.info/Elements/a/P50307>,
        <http://rdaregistry.info/Elements/a/P50308>,
        <http://rdaregistry.info/Elements/a/P50309>,
        <http://rdaregistry.info/Elements/a/P50310>,
        <http://rdaregistry.info/Elements/a/P50319>,
        <http://rdaregistry.info/Elements/a/P50328>,
        <http://rdaregistry.info/Elements/a/P50338>,
        <http://rdaregistry.info/Elements/a/P50339>,
        <http://rdaregistry.info/Elements/a/P50340>,
        <http://rdaregistry.info/Elements/a/P50360>,
        <http://rdaregistry.info/Elements/a/datatype/P50304>,
        <http://rdaregistry.info/Elements/a/object/P50304> ;
    reg:lexicalAlias <http://rdaregistry.info/Elements/a/relatedEntityAgent.en> ;
    reg:name "relatedEntityAgent"@en ;
    reg:status <http://metadataregistry.org/uri/RegStatus/1001> ;
    rdfs:domain <http://rdaregistry.info/Elements/c/C10002> ;
    rdfs:isDefinedBy <http://rdaregistry.info/Elements/a/> ;
    rdfs:subPropertyOf <http://rdaregistry.info/Elements/x/P00001> ;
    skos:definition "Relates an agent to an entity associated with an agent being described."@en .

<http://rdaregistry.info/Elements/a/P50202> a rdf:Property ;
    rdfs:label "is manufacturer of"@en,
        "est le fabricant de"@fr ;
    rdakit:toolkitDefinition "A manifestation that is printed, duplicated, cast, etc."@en,
        "Personne, famille ou collectivité responsable de l’impression, de la reproduction, du moulage, etc. d’une ressource sous une forme publiée."@fr ;
    rdakit:toolkitLabel "manufacturer of"@en,
        "fabricant de"@fr ;
    reg:hasSubproperty <http://rdaregistry.info/Elements/a/P50170>,
        <http://rdaregistry.info/Elements/a/P50171>,
        <http://rdaregistry.info/Elements/a/P50172>,
        <http://rdaregistry.info/Elements/a/P50173>,
        <http://rdaregistry.info/Elements/a/P50174>,
        <http://rdaregistry.info/Elements/a/P50175>,
        <http://rdaregistry.info/Elements/a/P50176>,
        <http://rdaregistry.info/Elements/a/P50177>,
        <http://rdaregistry.info/Elements/a/P50178>,
        <http://rdaregistry.info/Elements/a/P50179>,
        <http://rdaregistry.info/Elements/a/datatype/P50202>,
        <http://rdaregistry.info/Elements/a/object/P50202>,
        <http://rdaregistry.info/Elements/a/object/P50242> ;
    reg:hasUnconstrained <http://rdaregistry.info/Elements/u/P60669> ;
    reg:lexicalAlias <http://rdaregistry.info/Elements/a/manufacturerOf.en> ;
    reg:name "manufacturerOf"@en ;
    reg:status <http://metadataregistry.org/uri/RegStatus/1001> ;
    rdfs:domain <http://rdaregistry.info/Elements/c/C10002> ;
    rdfs:isDefinedBy <http://rdaregistry.info/Elements/a/> ;
    rdfs:subPropertyOf <http://rdaregistry.info/Elements/a/P50307> ;
    skos:definition "Relates an agent responsible for printing, duplicating, casting, etc. to a manifestation."@en,
        "Met une personne, famille ou collectivité responsable de l’impression, de la reproduction, du moulage, etc. d’une ressource sous une forme publiée en relation avec la manifestation."@fr .

<http://rdaregistry.info/Elements/a/P50360> a rdf:Property ;
    rdfs:label "has related entity (collective agent)"@en ;
    reg:hasSubproperty <http://rdaregistry.info/Elements/a/P50342>,
        <http://rdaregistry.info/Elements/a/P50343>,
        <http://rdaregistry.info/Elements/a/P50344>,
        <http://rdaregistry.info/Elements/a/P50357>,
        <http://rdaregistry.info/Elements/a/P50358>,
        <http://rdaregistry.info/Elements/a/P50361>,
        <http://rdaregistry.info/Elements/a/P50363>,
        <http://rdaregistry.info/Elements/a/P50364>,
        <http://rdaregistry.info/Elements/a/datatype/P50360>,
        <http://rdaregistry.info/Elements/a/object/P50360> ;
    reg:lexicalAlias <http://rdaregistry.info/Elements/a/relatedEntityCollectiveAgent.en> ;
    reg:name "relatedEntityCollectiveAgent"@en ;
    reg:status <http://metadataregistry.org/uri/RegStatus/1001> ;
    rdfs:domain <http://rdaregistry.info/Elements/c/C10011> ;
    rdfs:isDefinedBy <http://rdaregistry.info/Elements/a/> ;
    rdfs:subPropertyOf <http://rdaregistry.info/Elements/a/P50304> ;
    skos:definition "Relates a collective agent to an entity associated with a collective agent."@en .

<http://rdaregistry.info/Elements/a/P50147> a rdf:Property ;
    rdfs:label "is performer of"@en,
        "est l’interprète de"@fr ;
    rdakit:instructionNumber "18.5" ;
    rdakit:toolkitDefinition "An expression of a work that incorporates a contribution of performing music, acting, dancing, speaking, etc."@en,
        "Personne, famille ou collectivité contribuant à une expression d’une œuvre en exécutant de la musique, en jouant, en dansant, en parlant, etc. souvent dans une représentation musicale ou dramatique, etc."@fr ;
    rdakit:toolkitLabel "performer of"@en,
        "interprète de"@fr ;
    reg:hasSubproperty <http://rdaregistry.info/Elements/a/P50070>,
        <http://rdaregistry.info/Elements/a/P50071>,
        <http://rdaregistry.info/Elements/a/P50072>,
        <http://rdaregistry.info/Elements/a/P50073>,
        <http://rdaregistry.info/Elements/a/P50074>,
        <http://rdaregistry.info/Elements/a/P50075>,
        <http://rdaregistry.info/Elements/a/P50076>,
        <http://rdaregistry.info/Elements/a/P50077>,
        <http://rdaregistry.info/Elements/a/P50078>,
        <http://rdaregistry.info/Elements/a/P50079>,
        <http://rdaregistry.info/Elements/a/P50080>,
        <http://rdaregistry.info/Elements/a/P50081>,
        <http://rdaregistry.info/Elements/a/P50082>,
        <http://rdaregistry.info/Elements/a/P50083>,
        <http://rdaregistry.info/Elements/a/P50084>,
        <http://rdaregistry.info/Elements/a/datatype/P50147>,
        <http://rdaregistry.info/Elements/a/object/P50147> ;
    reg:hasUnconstrained <http://rdaregistry.info/Elements/u/P60615> ;
    reg:lexicalAlias <http://rdaregistry.info/Elements/a/performerOf.en> ;
    reg:name "performerOf"@en ;
    reg:status <http://metadataregistry.org/uri/RegStatus/1001> ;
    rdfs:domain <http://rdaregistry.info/Elements/c/C10002> ;
    rdfs:isDefinedBy <http://rdaregistry.info/Elements/a/> ;
    rdfs:subPropertyOf <http://rdaregistry.info/Elements/a/P50161> ;
    skos:definition "Relates an agent contributing to an expression of a work by performing music, acting, dancing, speaking, etc. to an expression."@en,
        "Met une personne, famille ou collectivité contribuant à une expression d’une œuvre en exécutant de la musique, en jouant, en dansant, en parlant, etc. souvent dans une représentation musicale ou dramatique, etc. en relation avec l’expression."@fr .

<http://rdaregistry.info/Elements/a/P50204> a rdf:Property ;
    rdfs:label "is creator of"@en,
        "est le créateur de"@fr ;
    rdakit:toolkitDefinition "A work that involves a creation responsibility."@en,
        "Personne, famille ou collectivité responsable de la création d’une œuvre."@fr ;
    rdakit:toolkitLabel "creator of"@en,
        "créateur de"@fr ;
    reg:hasSubproperty <http://rdaregistry.info/Elements/a/P50068>,
        <http://rdaregistry.info/Elements/a/P50127>,
        <http://rdaregistry.info/Elements/a/P50184>,
        <http://rdaregistry.info/Elements/a/P50185>,
        <http://rdaregistry.info/Elements/a/P50186>,
        <http://rdaregistry.info/Elements/a/P50187>,
        <http://rdaregistry.info/Elements/a/P50188>,
        <http://rdaregistry.info/Elements/a/P50189>,
        <http://rdaregistry.info/Elements/a/P50190>,
        <http://rdaregistry.info/Elements/a/P50191>,
        <http://rdaregistry.info/Elements/a/P50192>,
        <http://rdaregistry.info/Elements/a/P50193>,
        <http://rdaregistry.info/Elements/a/P50194>,
        <http://rdaregistry.info/Elements/a/P50195>,
        <http://rdaregistry.info/Elements/a/P50196>,
        <http://rdaregistry.info/Elements/a/P50197>,
        <http://rdaregistry.info/Elements/a/datatype/P50204>,
        <http://rdaregistry.info/Elements/a/object/P50204>,
        <http://rdaregistry.info/Elements/a/object/P50293>,
        <http://rdaregistry.info/Elements/a/object/P50294> ;
    reg:hasUnconstrained <http://rdaregistry.info/Elements/u/P60672> ;
    reg:lexicalAlias <http://rdaregistry.info/Elements/a/creatorOf.en> ;
    reg:name "creatorOf"@en ;
    reg:status <http://metadataregistry.org/uri/RegStatus/1001> ;
    rdfs:domain <http://rdaregistry.info/Elements/c/C10002> ;
    rdfs:isDefinedBy <http://rdaregistry.info/Elements/a/> ;
    rdfs:subPropertyOf <http://rdaregistry.info/Elements/a/P50305> ;
    skos:definition "Relates an agent responsible for the creation of a work to a work."@en,
        "Met une personne, famille ou collectivité responsable de la création d’une œuvre en relation avec l’œuvre."@fr .

<http://rdaregistry.info/Elements/a/P50131> a rdf:Property ;
    rdfs:label "is other agent associated with work of"@en,
        "est l’autre personne, famille ou collectivité associée à une œuvre de"@fr ;
    rdakit:toolkitDefinition "A work associated with an agent other than a creator."@en,
        "Personne, famille ou collectivité associée à une œuvre autrement que comme créateur."@fr ;
    rdakit:toolkitLabel "other agent associated with work of"@en,
        "autre personne, famille ou collectivité associée à une œuvre de"@fr ;
    reg:hasSubproperty <http://rdaregistry.info/Elements/a/P50044>,
        <http://rdaregistry.info/Elements/a/P50069>,
        <http://rdaregistry.info/Elements/a/P50086>,
        <http://rdaregistry.info/Elements/a/P50087>,
        <http://rdaregistry.info/Elements/a/P50088>,
        <http://rdaregistry.info/Elements/a/P50089>,
        <http://rdaregistry.info/Elements/a/P50090>,
        <http://rdaregistry.info/Elements/a/P50091>,
        <http://rdaregistry.info/Elements/a/P50126>,
        <http://rdaregistry.info/Elements/a/P50130>,
        <http://rdaregistry.info/Elements/a/P50132>,
        <http://rdaregistry.info/Elements/a/P50166>,
        <http://rdaregistry.info/Elements/a/P50201>,
        <http://rdaregistry.info/Elements/a/P50205>,
        <http://rdaregistry.info/Elements/a/P50207>,
        <http://rdaregistry.info/Elements/a/P50208>,
        <http://rdaregistry.info/Elements/a/P50209>,
        <http://rdaregistry.info/Elements/a/P50211>,
        <http://rdaregistry.info/Elements/a/P50226>,
        <http://rdaregistry.info/Elements/a/datatype/P50131>,
        <http://rdaregistry.info/Elements/a/object/P50131>,
        <http://rdaregistry.info/Elements/a/object/P50257>,
        <http://rdaregistry.info/Elements/a/object/P50262>,
        <http://rdaregistry.info/Elements/a/object/P50264>,
        <http://rdaregistry.info/Elements/a/object/P50265>,
        <http://rdaregistry.info/Elements/a/object/P50270>,
        <http://rdaregistry.info/Elements/a/object/P50289>,
        <http://rdaregistry.info/Elements/a/object/P50290> ;
    reg:hasUnconstrained <http://rdaregistry.info/Elements/u/P60602> ;
    reg:lexicalAlias <http://rdaregistry.info/Elements/a/otherAgentWorkOf.en> ;
    reg:name "otherAgentWorkOf"@en ;
    reg:status <http://metadataregistry.org/uri/RegStatus/1001> ;
    rdfs:domain <http://rdaregistry.info/Elements/c/C10002> ;
    rdfs:isDefinedBy <http://rdaregistry.info/Elements/a/> ;
    rdfs:subPropertyOf <http://rdaregistry.info/Elements/a/P50305> ;
    skos:definition "Relates an agent associated with a work other than as a creator to a work."@en,
        "Met une personne, famille ou collectivité associée à une œuvre autrement que comme créateur en relation avec l’œuvre."@fr ;
    skos:scopeNote "Agents to whom correspondence is addressed, agents honoured by a festschrift, directors, cinematographers, sponsoring bodies, production companies, institutions, etc., hosting an exhibition or event, etc., are included."@en,
        "Comprend les personnes, etc. à qui une correspondance est adressée, les personnes, etc. à qui sont offerts des mélanges, les réalisateurs, les directeurs de la photographie, les commanditaires, les sociétés de production, les institutions, etc. accueillant une exposition ou un évènement, etc."@fr .

<http://rdaregistry.info/Elements/a/P50161> a rdf:Property ;
    rdfs:label "is contributor of"@en,
        "est le contributeur de"@fr ;
    rdakit:toolkitDefinition "An expression that incorporates a contribution."@en,
        "Personne, famille ou collectivité contribuant à une expression."@fr ;
    rdakit:toolkitLabel "contributor of"@en,
        "contributeur de"@fr ;
    reg:hasSubproperty <http://rdaregistry.info/Elements/a/P50134>,
        <http://rdaregistry.info/Elements/a/P50135>,
        <http://rdaregistry.info/Elements/a/P50136>,
        <http://rdaregistry.info/Elements/a/P50137>,
        <http://rdaregistry.info/Elements/a/P50139>,
        <http://rdaregistry.info/Elements/a/P50140>,
        <http://rdaregistry.info/Elements/a/P50141>,
        <http://rdaregistry.info/Elements/a/P50142>,
        <http://rdaregistry.info/Elements/a/P50143>,
        <http://rdaregistry.info/Elements/a/P50144>,
        <http://rdaregistry.info/Elements/a/P50145>,
        <http://rdaregistry.info/Elements/a/P50146>,
        <http://rdaregistry.info/Elements/a/P50147>,
        <http://rdaregistry.info/Elements/a/P50150>,
        <http://rdaregistry.info/Elements/a/P50151>,
        <http://rdaregistry.info/Elements/a/P50154>,
        <http://rdaregistry.info/Elements/a/P50155>,
        <http://rdaregistry.info/Elements/a/P50156>,
        <http://rdaregistry.info/Elements/a/P50157>,
        <http://rdaregistry.info/Elements/a/P50158>,
        <http://rdaregistry.info/Elements/a/P50159>,
        <http://rdaregistry.info/Elements/a/P50160>,
        <http://rdaregistry.info/Elements/a/P50183>,
        <http://rdaregistry.info/Elements/a/P50198>,
        <http://rdaregistry.info/Elements/a/P50212>,
        <http://rdaregistry.info/Elements/a/datatype/P50161>,
        <http://rdaregistry.info/Elements/a/object/P50161>,
        <http://rdaregistry.info/Elements/a/object/P50180>,
        <http://rdaregistry.info/Elements/a/object/P50243>,
        <http://rdaregistry.info/Elements/a/object/P50244>,
        <http://rdaregistry.info/Elements/a/object/P50255>,
        <http://rdaregistry.info/Elements/a/object/P50256>,
        <http://rdaregistry.info/Elements/a/object/P50261>,
        <http://rdaregistry.info/Elements/a/object/P50263>,
        <http://rdaregistry.info/Elements/a/object/P50266>,
        <http://rdaregistry.info/Elements/a/object/P50267>,
        <http://rdaregistry.info/Elements/a/object/P50271>,
        <http://rdaregistry.info/Elements/a/object/P50272>,
        <http://rdaregistry.info/Elements/a/object/P50273>,
        <http://rdaregistry.info/Elements/a/object/P50296>,
        <http://rdaregistry.info/Elements/a/object/P50298>,
        <http://rdaregistry.info/Elements/a/object/P50299>,
        <http://rdaregistry.info/Elements/a/object/P50300> ;
    reg:hasUnconstrained <http://rdaregistry.info/Elements/u/P60626> ;
    reg:lexicalAlias <http://rdaregistry.info/Elements/a/contributorOf.en> ;
    reg:name "contributorOf"@en ;
    reg:status <http://metadataregistry.org/uri/RegStatus/1001> ;
    rdfs:domain <http://rdaregistry.info/Elements/c/C10002> ;
    rdfs:isDefinedBy <http://rdaregistry.info/Elements/a/> ;
    rdfs:subPropertyOf <http://rdaregistry.info/Elements/a/P50306> ;
    skos:definition "Relates an agent contributing to an expression to an expression."@en,
        "Met une personne, famille ou collectivité contribuant à une expression en relation avec l’expression."@fr ;
    skos:scopeNote "Editors, translators, arrangers of music, performers, etc., are included."@en,
        "Les contributeurs incluent les éditeurs intellectuels, les traducteurs, les arrangeurs de musique, les interprètes, etc."@fr .

<http://metadataregistry.org/uri/RegStatus/1001> a skos:Concept ;
    skos:prefLabel "Published"@en .

<http://rdaregistry.info/Elements/a/> dc:title "RDA Agent properties"@en ;
    skos:note "Properties derived from RDA elements and relationship designators with the domain of RDA Agent and its sub-classes Person, Family, and Corporate Body."@en ;
    foaf:homepage <http://www.rdaregistry.info/Elements/a/> .

