@prefix dc: <http://purl.org/dc/elements/1.1/> .
@prefix foaf: <http://xmlns.com/foaf/0.1/> .
@prefix rdakit: <http://metadataregistry.org/uri/profile/rdakit/> .
@prefix rdf: <http://www.w3.org/1999/02/22-rdf-syntax-ns#> .
@prefix rdfs: <http://www.w3.org/2000/01/rdf-schema#> .
@prefix reg: <http://metadataregistry.org/uri/profile/regap/> .
@prefix skos: <http://www.w3.org/2004/02/skos/core#> .
@prefix xml: <http://www.w3.org/XML/1998/namespace> .
@prefix xsd: <http://www.w3.org/2001/XMLSchema#> .

<http://rdaregistry.info/Elements/n/P80065> a rdf:Property ;
    rdfs:label "has intended audience of nomen"@en ;
    rdakit:hasElementType "5" ;
    rdakit:toolkitDefinition "A class of users for which a nomen is intended."@en ;
    rdakit:toolkitLabel "intended audience of nomen"@en ;
    reg:hasSubproperty <http://rdaregistry.info/Elements/n/datatype/P80065> ;
    reg:lexicalAlias <http://rdaregistry.info/Elements/n/intendedAudienceOfNomen.en> ;
    reg:name "intendedAudienceOfNomen"@en ;
    reg:status <http://metadataregistry.org/uri/RegStatus/1001> ;
    rdfs:domain <http://rdaregistry.info/Elements/c/C10012> ;
    rdfs:isDefinedBy <http://rdaregistry.info/Elements/n/> ;
    skos:definition "Relates a nomen to a class of users for which a nomen is intended."@en .

<http://rdaregistry.info/Elements/n/P80066> a rdf:Property ;
    rdfs:label "has language of nomen"@en ;
    rdakit:hasElementType "5" ;
    rdakit:toolkitDefinition "A language of an appellation."@en ;
    rdakit:toolkitLabel "language of nomen"@en ;
    reg:hasSubproperty <http://rdaregistry.info/Elements/n/datatype/P80066> ;
    reg:lexicalAlias <http://rdaregistry.info/Elements/n/languageOfNomen.en> ;
    reg:name "languageOfNomen"@en ;
    reg:status <http://metadataregistry.org/uri/RegStatus/1001> ;
    rdfs:domain <http://rdaregistry.info/Elements/c/C10012> ;
    rdfs:isDefinedBy <http://rdaregistry.info/Elements/n/> ;
    skos:definition "Relates a nomen to a language of an appellation."@en .

<http://rdaregistry.info/Elements/n/P80067> a rdf:Property ;
    rdfs:label "has context of use"@en ;
    rdakit:hasElementType "6" ;
    rdakit:toolkitDefinition "The circumstances or situation in which an appellation of an RDA entity is used."@en ;
    rdakit:toolkitLabel "context of use"@en ;
    reg:hasSubproperty <http://rdaregistry.info/Elements/n/datatype/P80067> ;
    reg:hasUnconstrained <http://rdaregistry.info/Elements/u/P61119> ;
    reg:lexicalAlias <http://rdaregistry.info/Elements/n/contextOfUse.en> ;
    reg:name "contextOfUse"@en ;
    reg:status <http://metadataregistry.org/uri/RegStatus/1001> ;
    rdfs:domain <http://rdaregistry.info/Elements/c/C10012> ;
    rdfs:isDefinedBy <http://rdaregistry.info/Elements/n/> ;
    skos:altLabel "scope of usage"@en ;
    skos:definition "Relates a nomen to the circumstances or situation in which an appellation of an RDA entity is used."@en .

<http://rdaregistry.info/Elements/n/P80068> a rdf:Property ;
    rdfs:label "has nomen string"@en ;
    rdakit:hasElementType "6" ;
    rdakit:toolkitDefinition "The combination of signs that forms an appellation associated with an entity."@en ;
    rdakit:toolkitLabel "nomen string"@en ;
    reg:hasSubproperty <http://rdaregistry.info/Elements/n/datatype/P80068> ;
    reg:hasUnconstrained <http://rdaregistry.info/Elements/u/P60913> ;
    reg:lexicalAlias <http://rdaregistry.info/Elements/n/nomenString.en> ;
    reg:name "nomenString"@en ;
    reg:status <http://metadataregistry.org/uri/RegStatus/1001> ;
    rdfs:domain <http://rdaregistry.info/Elements/c/C10012> ;
    rdfs:isDefinedBy <http://rdaregistry.info/Elements/n/> ;
    skos:definition "Relates a nomen to the combination of signs that forms an appellation associated with an entity."@en ;
    skos:scopeNote "The string can be expressed as a notation in any form, such as a combination of signs within a writing system, chemical structure symbols, mathematical notation, or by any other kind of sign, such as sounds, etc."@en .

<http://rdaregistry.info/Elements/n/P80069> a rdf:Property ;
    rdfs:label "has scheme of nomen"@en ;
    rdakit:hasElementType "5" ;
    rdakit:toolkitDefinition "A scheme in which an appellation is established."@en ;
    rdakit:toolkitLabel "scheme of nomen"@en ;
    reg:hasSubproperty <http://rdaregistry.info/Elements/n/datatype/P80069> ;
    reg:hasUnconstrained <http://rdaregistry.info/Elements/u/P61156> ;
    reg:lexicalAlias <http://rdaregistry.info/Elements/n/schemeOfNomen.en> ;
    reg:name "schemeOfNomen"@en ;
    reg:status <http://metadataregistry.org/uri/RegStatus/1001> ;
    rdfs:domain <http://rdaregistry.info/Elements/c/C10012> ;
    rdfs:isDefinedBy <http://rdaregistry.info/Elements/n/> ;
    skos:definition "Relates a nomen to a scheme in which an appellation is established."@en ;
    skos:scopeNote "The scheme can be a value or vocabulary encoding scheme or a syntax encoding scheme."@en .

<http://rdaregistry.info/Elements/n/P80070> a rdf:Property ;
    rdfs:label "has script of nomen"@en ;
    rdakit:hasElementType "5" ;
    rdakit:toolkitDefinition "A set of characters or symbols with which an appellation is formed."@en ;
    rdakit:toolkitLabel "script of nomen"@en ;
    reg:hasSubproperty <http://rdaregistry.info/Elements/n/datatype/P80070> ;
    reg:hasUnconstrained <http://rdaregistry.info/Elements/u/P61157> ;
    reg:lexicalAlias <http://rdaregistry.info/Elements/n/scriptOfNomen.en> ;
    reg:name "scriptOfNomen"@en ;
    reg:status <http://metadataregistry.org/uri/RegStatus/1001> ;
    rdfs:domain <http://rdaregistry.info/Elements/c/C10012> ;
    rdfs:isDefinedBy <http://rdaregistry.info/Elements/n/> ;
    skos:definition "Relates a nomen to a set of characters or symbols with which an appellation is formed."@en .

<http://rdaregistry.info/Elements/n/P80071> a rdf:Property ;
    rdfs:label "has note on nomen"@en ;
    rdakit:hasElementType "6" ;
    rdakit:toolkitDefinition "A broad unstructured description of one or more attributes of a nomen."@en ;
    rdakit:toolkitLabel "note on nomen"@en ;
    reg:hasSubproperty <http://rdaregistry.info/Elements/n/datatype/P80071>,
        <http://rdaregistry.info/Elements/n/object/P80071> ;
    reg:hasUnconstrained <http://rdaregistry.info/Elements/u/P60936> ;
    reg:lexicalAlias <http://rdaregistry.info/Elements/n/noteOnNomen.en> ;
    reg:name "noteOnNomen"@en ;
    reg:status <http://metadataregistry.org/uri/RegStatus/1001> ;
    rdfs:domain <http://rdaregistry.info/Elements/c/C10012> ;
    rdfs:isDefinedBy <http://rdaregistry.info/Elements/n/> ;
    rdfs:subPropertyOf <http://rdaregistry.info/Elements/x/P00015> ;
    skos:definition "Relates a nomen to a broad unstructured description of one or more attributes of a nomen."@en .

<http://rdaregistry.info/Elements/n/P80078> a rdf:Property ;
    rdfs:label "has category of nomen"@en ;
    rdakit:hasElementType "5" ;
    rdakit:toolkitDefinition "A type to which a nomen belongs."@en ;
    rdakit:toolkitLabel "category of nomen"@en ;
    reg:hasSubproperty <http://rdaregistry.info/Elements/n/datatype/P80078> ;
    reg:hasUnconstrained <http://rdaregistry.info/Elements/u/P60944> ;
    reg:lexicalAlias <http://rdaregistry.info/Elements/n/categoryOfNomen.en> ;
    reg:name "categoryOfNomen"@en ;
    reg:status <http://metadataregistry.org/uri/RegStatus/1001> ;
    rdfs:domain <http://rdaregistry.info/Elements/c/C10012> ;
    rdfs:isDefinedBy <http://rdaregistry.info/Elements/n/> ;
    rdfs:subPropertyOf <http://rdaregistry.info/Elements/x/P00029> ;
    skos:altLabel "type of nomen"@en ;
    skos:definition "Relates a nomen to a type to which a nomen belongs."@en .

<http://rdaregistry.info/Elements/n/P80139> a rdf:Property ;
    rdfs:label "has reference source"@en ;
    rdakit:hasElementType "3" ;
    rdakit:toolkitDefinition "A source in which there is evidence for the use of a nomen."@en ;
    rdakit:toolkitLabel "reference source"@en ;
    reg:hasSubproperty <http://rdaregistry.info/Elements/n/datatype/P80139> ;
    reg:hasUnconstrained <http://rdaregistry.info/Elements/u/P61159> ;
    reg:lexicalAlias <http://rdaregistry.info/Elements/n/referenceSource.en> ;
    reg:name "referenceSource"@en ;
    reg:status <http://metadataregistry.org/uri/RegStatus/1001> ;
    rdfs:domain <http://rdaregistry.info/Elements/c/C10012> ;
    rdfs:isDefinedBy <http://rdaregistry.info/Elements/n/> ;
    skos:altLabel "source consulted"@en ;
    skos:definition "Relates a nomen to a source in which there is evidence for the use of a nomen."@en .

<http://rdaregistry.info/Elements/n/P80167> a rdf:Property ;
    rdfs:label "has scope of usage (Deprecated)"@en ;
    rdakit:hasElementType "3" ;
    rdakit:toolkitDefinition "A type or form of work associated with the usage of a name of agent."@en ;
    rdakit:toolkitLabel "scope of usage"@en ;
    reg:hasSubproperty <http://rdaregistry.info/Elements/n/datatype/P80167> ;
    reg:hasUnconstrained <http://rdaregistry.info/Elements/u/P60822> ;
    reg:lexicalAlias <http://rdaregistry.info/Elements/n/scopeOfUsage.en> ;
    reg:name "scopeOfUsage"@en ;
    reg:status <http://metadataregistry.org/uri/RegStatus/1008> ;
    rdfs:domain <http://rdaregistry.info/Elements/c/C10012> ;
    rdfs:isDefinedBy <http://rdaregistry.info/Elements/n/> ;
    skos:definition "Relates a nomen to a type or form of work associated with the usage of a name of agent."@en .

<http://rdaregistry.info/Elements/n/P80168> a rdf:Property ;
    rdfs:label "has status of identification"@en ;
    rdakit:hasElementType "3" ;
    rdakit:toolkitDefinition "An indication of a level of authentication of the nomen of an entity."@en ;
    rdakit:toolkitLabel "status of identification"@en ;
    reg:hasSubproperty <http://rdaregistry.info/Elements/n/datatype/P80168> ;
    reg:hasUnconstrained <http://rdaregistry.info/Elements/u/P61160> ;
    reg:lexicalAlias <http://rdaregistry.info/Elements/n/statusOfIdentification.en> ;
    reg:name "statusOfIdentification"@en ;
    reg:status <http://metadataregistry.org/uri/RegStatus/1001> ;
    rdfs:domain <http://rdaregistry.info/Elements/c/C10012> ;
    rdfs:isDefinedBy <http://rdaregistry.info/Elements/n/> ;
    skos:definition "Relates a nomen to an indication of a level of authentication of the nomen of an entity."@en .

<http://rdaregistry.info/Elements/n/P80169> a rdf:Property ;
    rdfs:label "has undifferentiated name indicator"@en ;
    rdakit:hasElementType "3" ;
    rdakit:toolkitDefinition "A categorization indicating that a nomen is insufficient to differentiate between two or more entities."@en ;
    rdakit:toolkitLabel "undifferentiated name indicator"@en ;
    reg:hasSubproperty <http://rdaregistry.info/Elements/n/datatype/P80169> ;
    reg:hasUnconstrained <http://rdaregistry.info/Elements/u/P60046> ;
    reg:lexicalAlias <http://rdaregistry.info/Elements/n/undifferentiatedNameIndicator.en> ;
    reg:name "undifferentiatedNameIndicator"@en ;
    reg:status <http://metadataregistry.org/uri/RegStatus/1001> ;
    rdfs:domain <http://rdaregistry.info/Elements/c/C10012> ;
    rdfs:isDefinedBy <http://rdaregistry.info/Elements/n/> ;
    skos:definition "Relates a nomen to a categorization indicating that a nomen is insufficient to differentiate between two or more entities."@en .

<http://rdaregistry.info/Elements/n/P80014> a rdf:Property ;
    rdfs:label "is subject nomen of"@en ;
    rdakit:hasElementType "2" ;
    rdakit:toolkitDefinition "A work that is about a nomen."@en ;
    rdakit:toolkitLabel "subject nomen of"@en ;
    reg:hasSubproperty <http://rdaregistry.info/Elements/n/P80178>,
        <http://rdaregistry.info/Elements/n/datatype/P80014>,
        <http://rdaregistry.info/Elements/n/object/P80014> ;
    reg:hasUnconstrained <http://rdaregistry.info/Elements/u/P60806> ;
    reg:lexicalAlias <http://rdaregistry.info/Elements/n/subjectNomenOf.en> ;
    reg:name "subjectNomenOf"@en ;
    reg:status <http://metadataregistry.org/uri/RegStatus/1001> ;
    rdfs:domain <http://rdaregistry.info/Elements/c/C10012> ;
    rdfs:isDefinedBy <http://rdaregistry.info/Elements/n/> ;
    rdfs:subPropertyOf <http://rdaregistry.info/Elements/n/P80001>,
        <http://rdaregistry.info/Elements/x/P00014> ;
    skos:altLabel "subject of (nomen)"@en ;
    skos:definition "Relates a nomen to a work that is about a nomen."@en .

<http://rdaregistry.info/Elements/n/P80042> a rdf:Property ;
    rdfs:label "is identifier for place of"@en ;
    rdakit:hasElementType "2" ;
    rdakit:toolkitDefinition "A place that has an appellation of place that is a reference code taken from a vocabulary encoding scheme."@en ;
    rdakit:toolkitLabel "identifier for place of"@en ;
    reg:hasSubproperty <http://rdaregistry.info/Elements/n/datatype/P80042>,
        <http://rdaregistry.info/Elements/n/object/P80042> ;
    reg:hasUnconstrained <http://rdaregistry.info/Elements/u/P60928> ;
    reg:lexicalAlias <http://rdaregistry.info/Elements/n/identifierForPlaceOf.en> ;
    reg:name "identifierForPlaceOf"@en ;
    reg:status <http://metadataregistry.org/uri/RegStatus/1001> ;
    rdfs:domain <http://rdaregistry.info/Elements/c/C10012> ;
    rdfs:isDefinedBy <http://rdaregistry.info/Elements/n/> ;
    rdfs:subPropertyOf <http://rdaregistry.info/Elements/n/P80041>,
        <http://rdaregistry.info/Elements/n/P80160> ;
    skos:definition "Relates a nomen to a place that has an appellation of place that is a reference code taken from a vocabulary encoding scheme."@en .

<http://rdaregistry.info/Elements/n/P80046> a rdf:Property ;
    rdfs:label "is identifier for expression of"@en ;
    rdakit:hasElementType "2" ;
    rdakit:toolkitDefinition "An expression that has an appellation of expression that is a reference code taken from a vocabulary encoding scheme."@en ;
    rdakit:toolkitLabel "identifier for expression of"@en ;
    reg:hasSubproperty <http://rdaregistry.info/Elements/n/datatype/P80046>,
        <http://rdaregistry.info/Elements/n/object/P80046> ;
    reg:hasUnconstrained <http://rdaregistry.info/Elements/u/P60938> ;
    reg:lexicalAlias <http://rdaregistry.info/Elements/n/identifierForExpressionOf.en> ;
    reg:name "identifierForExpressionOf"@en ;
    reg:status <http://metadataregistry.org/uri/RegStatus/1001> ;
    rdfs:domain <http://rdaregistry.info/Elements/c/C10012> ;
    rdfs:isDefinedBy <http://rdaregistry.info/Elements/n/> ;
    rdfs:subPropertyOf <http://rdaregistry.info/Elements/n/P80038>,
        <http://rdaregistry.info/Elements/n/P80160> ;
    skos:definition "Relates a nomen to an expression that has an appellation of expression that is a reference code taken from a vocabulary encoding scheme."@en .

<http://rdaregistry.info/Elements/n/P80047> a rdf:Property ;
    rdfs:label "is identifier for item of"@en ;
    rdakit:hasElementType "2" ;
    rdakit:toolkitDefinition "An item that has an appellation of item that is a reference code taken from a vocabulary encoding scheme."@en ;
    rdakit:toolkitLabel "identifier for item of"@en ;
    reg:hasSubproperty <http://rdaregistry.info/Elements/n/datatype/P80047>,
        <http://rdaregistry.info/Elements/n/object/P80047> ;
    reg:hasUnconstrained <http://rdaregistry.info/Elements/u/P60938> ;
    reg:lexicalAlias <http://rdaregistry.info/Elements/n/identifierForItemOf.en> ;
    reg:name "identifierForItemOf"@en ;
    reg:status <http://metadataregistry.org/uri/RegStatus/1001> ;
    rdfs:domain <http://rdaregistry.info/Elements/c/C10012> ;
    rdfs:isDefinedBy <http://rdaregistry.info/Elements/n/> ;
    rdfs:subPropertyOf <http://rdaregistry.info/Elements/n/P80016>,
        <http://rdaregistry.info/Elements/n/P80160> ;
    skos:definition "Relates a nomen to an item that has an appellation of item that is a reference code taken from a vocabulary encoding scheme."@en .

<http://rdaregistry.info/Elements/n/P80050> a rdf:Property ;
    rdfs:label "is identifier for timespan of"@en ;
    rdakit:hasElementType "2" ;
    rdakit:toolkitDefinition "A timespan that has an appellation of timespan that is a reference code taken from a vocabulary encoding scheme."@en ;
    rdakit:toolkitLabel "identifier for timespan of"@en ;
    reg:hasSubproperty <http://rdaregistry.info/Elements/n/datatype/P80050>,
        <http://rdaregistry.info/Elements/n/object/P80050> ;
    reg:hasUnconstrained <http://rdaregistry.info/Elements/u/P60928> ;
    reg:lexicalAlias <http://rdaregistry.info/Elements/n/identifierForTimespanOf.en> ;
    reg:name "identifierForTimespanOf"@en ;
    reg:status <http://metadataregistry.org/uri/RegStatus/1001> ;
    rdfs:domain <http://rdaregistry.info/Elements/c/C10012> ;
    rdfs:isDefinedBy <http://rdaregistry.info/Elements/n/> ;
    rdfs:subPropertyOf <http://rdaregistry.info/Elements/n/P80043>,
        <http://rdaregistry.info/Elements/n/P80160> ;
    skos:definition "Relates a nomen to a timespan that has an appellation of timespan that is a reference code taken from a vocabulary encoding scheme."@en .

<http://rdaregistry.info/Elements/n/P80057> a rdf:Property ;
    rdfs:label "is abbreviated title of"@en ;
    rdakit:hasElementType "2" ;
    rdakit:toolkitDefinition "A manifestation that has a title of manifestation that has been abbreviated for purposes of indexing or identification."@en ;
    rdakit:toolkitLabel "abbreviated title of"@en ;
    reg:hasSubproperty <http://rdaregistry.info/Elements/n/datatype/P80057>,
        <http://rdaregistry.info/Elements/n/object/P80057> ;
    reg:hasUnconstrained <http://rdaregistry.info/Elements/u/P61111> ;
    reg:lexicalAlias <http://rdaregistry.info/Elements/n/abbreviatedTitleOf.en> ;
    reg:name "abbreviatedTitleOf"@en ;
    reg:status <http://metadataregistry.org/uri/RegStatus/1001> ;
    rdfs:domain <http://rdaregistry.info/Elements/c/C10012> ;
    rdfs:isDefinedBy <http://rdaregistry.info/Elements/n/> ;
    rdfs:subPropertyOf <http://rdaregistry.info/Elements/n/P80111> ;
    skos:definition "Relates a nomen to a manifestation that has a title of manifestation that has been abbreviated for purposes of indexing or identification."@en .

<http://rdaregistry.info/Elements/n/P80058> a rdf:Property ;
    rdfs:label "has part nomen"@en ;
    rdakit:hasElementType "2" ;
    rdakit:toolkitDefinition "A nomen that is a discrete component of another nomen."@en ;
    rdakit:toolkitLabel "part nomen"@en ;
    reg:hasSubproperty <http://rdaregistry.info/Elements/n/datatype/P80058>,
        <http://rdaregistry.info/Elements/n/object/P80058> ;
    reg:hasUnconstrained <http://rdaregistry.info/Elements/u/P61114> ;
    reg:lexicalAlias <http://rdaregistry.info/Elements/n/partNomen.en> ;
    reg:name "partNomen"@en ;
    reg:status <http://metadataregistry.org/uri/RegStatus/1001> ;
    rdfs:domain <http://rdaregistry.info/Elements/c/C10012> ;
    rdfs:isDefinedBy <http://rdaregistry.info/Elements/n/> ;
    rdfs:subPropertyOf <http://rdaregistry.info/Elements/n/P80009> ;
    skos:definition "Relates a nomen to a nomen that is a discrete component of another nomen."@en .

<http://rdaregistry.info/Elements/n/P80059> a rdf:Property ;
    rdfs:label "is part of nomen"@en ;
    rdakit:hasElementType "2" ;
    rdakit:toolkitDefinition "A nomen that has another nomen as a discrete component."@en ;
    rdakit:toolkitLabel "part of nomen"@en ;
    reg:hasSubproperty <http://rdaregistry.info/Elements/n/datatype/P80059>,
        <http://rdaregistry.info/Elements/n/object/P80059> ;
    reg:hasUnconstrained <http://rdaregistry.info/Elements/u/P61115> ;
    reg:lexicalAlias <http://rdaregistry.info/Elements/n/partOfNomen.en> ;
    reg:name "partOfNomen"@en ;
    reg:status <http://metadataregistry.org/uri/RegStatus/1001> ;
    rdfs:domain <http://rdaregistry.info/Elements/c/C10012> ;
    rdfs:isDefinedBy <http://rdaregistry.info/Elements/n/> ;
    rdfs:subPropertyOf <http://rdaregistry.info/Elements/n/P80009> ;
    skos:definition "Relates a nomen to a nomen that has another nomen as a discrete component."@en .

<http://rdaregistry.info/Elements/n/P80060> a rdf:Property ;
    rdfs:label "has derivation"@en ;
    rdakit:hasElementType "2" ;
    rdakit:toolkitDefinition "A nomen that is based on another nomen."@en ;
    rdakit:toolkitLabel "derivation"@en ;
    reg:hasSubproperty <http://rdaregistry.info/Elements/n/datatype/P80060>,
        <http://rdaregistry.info/Elements/n/object/P80060> ;
    reg:hasUnconstrained <http://rdaregistry.info/Elements/u/P61121> ;
    reg:lexicalAlias <http://rdaregistry.info/Elements/n/derivation.en> ;
    reg:name "derivation"@en ;
    reg:status <http://metadataregistry.org/uri/RegStatus/1001> ;
    rdfs:domain <http://rdaregistry.info/Elements/c/C10012> ;
    rdfs:isDefinedBy <http://rdaregistry.info/Elements/n/> ;
    rdfs:subPropertyOf <http://rdaregistry.info/Elements/n/P80009> ;
    skos:definition "Relates a nomen to a nomen that is based on another nomen."@en .

<http://rdaregistry.info/Elements/n/P80061> a rdf:Property ;
    rdfs:label "is derivation of"@en ;
    rdakit:hasElementType "2" ;
    rdakit:toolkitDefinition "A nomen that is used as the basis of another nomen."@en ;
    rdakit:toolkitLabel "derivation of"@en ;
    reg:hasSubproperty <http://rdaregistry.info/Elements/n/datatype/P80061>,
        <http://rdaregistry.info/Elements/n/object/P80061> ;
    reg:hasUnconstrained <http://rdaregistry.info/Elements/u/P61122> ;
    reg:lexicalAlias <http://rdaregistry.info/Elements/n/derivationOf.en> ;
    reg:name "derivationOf"@en ;
    reg:status <http://metadataregistry.org/uri/RegStatus/1001> ;
    rdfs:domain <http://rdaregistry.info/Elements/c/C10012> ;
    rdfs:isDefinedBy <http://rdaregistry.info/Elements/n/> ;
    rdfs:subPropertyOf <http://rdaregistry.info/Elements/n/P80009> ;
    skos:definition "Relates a nomen to a nomen that is used as the basis of another nomen."@en .

<http://rdaregistry.info/Elements/n/P80072> a rdf:Property ;
    rdfs:label "is key title of"@en ;
    rdakit:hasElementType "2" ;
    rdakit:toolkitDefinition "A work that has a title of work that is assigned by an ISSN registration agency."@en ;
    rdakit:toolkitLabel "key title of"@en ;
    reg:hasSubproperty <http://rdaregistry.info/Elements/n/datatype/P80072> ;
    reg:hasUnconstrained <http://rdaregistry.info/Elements/u/P61118> ;
    reg:lexicalAlias <http://rdaregistry.info/Elements/n/keyTitleOf.en> ;
    reg:name "keyTitleOf"@en ;
    reg:status <http://metadataregistry.org/uri/RegStatus/1001> ;
    rdfs:domain <http://rdaregistry.info/Elements/c/C10012> ;
    rdfs:isDefinedBy <http://rdaregistry.info/Elements/n/> ;
    rdfs:subPropertyOf <http://rdaregistry.info/Elements/n/P80064> ;
    skos:definition "Relates a nomen to a work that has a title of work that is assigned by an ISSN registration agency."@en .

<http://rdaregistry.info/Elements/n/P80081> a rdf:Property ;
    rdfs:label "is authorized access point for timespan of"@en ;
    rdakit:hasElementType "2" ;
    rdakit:toolkitDefinition "A timespan that has an access point for timespan that is selected for preference in a specific vocabulary encoding scheme."@en ;
    rdakit:toolkitLabel "authorized access point for timespan of"@en ;
    reg:hasSubproperty <http://rdaregistry.info/Elements/n/datatype/P80081>,
        <http://rdaregistry.info/Elements/n/object/P80081> ;
    reg:hasUnconstrained <http://rdaregistry.info/Elements/u/P60918> ;
    reg:lexicalAlias <http://rdaregistry.info/Elements/n/authorizedAccessPointForTimespanOf.en> ;
    reg:name "authorizedAccessPointForTimespanOf"@en ;
    reg:status <http://metadataregistry.org/uri/RegStatus/1001> ;
    rdfs:domain <http://rdaregistry.info/Elements/c/C10012> ;
    rdfs:isDefinedBy <http://rdaregistry.info/Elements/n/> ;
    rdfs:subPropertyOf <http://rdaregistry.info/Elements/n/P80026>,
        <http://rdaregistry.info/Elements/n/P80162> ;
    skos:definition "Relates a nomen to a timespan that has an access point for timespan that is selected for preference in a specific vocabulary encoding scheme."@en .

<http://rdaregistry.info/Elements/n/P80084> a rdf:Property ;
    rdfs:label "is variant name of timespan of"@en ;
    rdakit:hasElementType "2" ;
    rdakit:toolkitDefinition "A timespan that has a name of timespan that is not selected for preference in a specific application or context."@en ;
    rdakit:toolkitLabel "variant name of timespan of"@en ;
    reg:hasSubproperty <http://rdaregistry.info/Elements/n/datatype/P80084>,
        <http://rdaregistry.info/Elements/n/object/P80084> ;
    reg:hasUnconstrained <http://rdaregistry.info/Elements/u/P60932> ;
    reg:lexicalAlias <http://rdaregistry.info/Elements/n/variantNameOfTimespanOf.en> ;
    reg:name "variantNameOfTimespanOf"@en ;
    reg:status <http://metadataregistry.org/uri/RegStatus/1001> ;
    rdfs:domain <http://rdaregistry.info/Elements/c/C10012> ;
    rdfs:isDefinedBy <http://rdaregistry.info/Elements/n/> ;
    rdfs:subPropertyOf <http://rdaregistry.info/Elements/n/P80044>,
        <http://rdaregistry.info/Elements/n/P80164> ;
    skos:definition "Relates a nomen to a timespan that has a name of timespan that is not selected for preference in a specific application or context."@en .

<http://rdaregistry.info/Elements/n/P80085> a rdf:Property ;
    rdfs:label "is authorized access point for place of"@en ;
    rdakit:hasElementType "2" ;
    rdakit:toolkitDefinition "A place that has an access point for place that is selected for preference in a specific vocabulary encoding scheme."@en ;
    rdakit:toolkitLabel "authorized access point for place of"@en ;
    reg:hasSubproperty <http://rdaregistry.info/Elements/n/datatype/P80085>,
        <http://rdaregistry.info/Elements/n/object/P80085> ;
    reg:hasUnconstrained <http://rdaregistry.info/Elements/u/P60918> ;
    reg:lexicalAlias <http://rdaregistry.info/Elements/n/authorizedAccessPointForPlaceOf.en> ;
    reg:name "authorizedAccessPointForPlaceOf"@en ;
    reg:status <http://metadataregistry.org/uri/RegStatus/1001> ;
    rdfs:domain <http://rdaregistry.info/Elements/c/C10012> ;
    rdfs:isDefinedBy <http://rdaregistry.info/Elements/n/> ;
    rdfs:subPropertyOf <http://rdaregistry.info/Elements/n/P80025>,
        <http://rdaregistry.info/Elements/n/P80162> ;
    skos:definition "Relates a nomen to a place that has an access point for place that is selected for preference in a specific vocabulary encoding scheme."@en .

<http://rdaregistry.info/Elements/n/P80088> a rdf:Property ;
    rdfs:label "is variant name of place of"@en ;
    rdakit:hasElementType "2" ;
    rdakit:toolkitDefinition "A place that has a name of place that is not selected for preference in a specific application or context."@en ;
    rdakit:toolkitLabel "variant name of place of"@en ;
    reg:hasSubproperty <http://rdaregistry.info/Elements/n/datatype/P80088>,
        <http://rdaregistry.info/Elements/n/object/P80088> ;
    reg:hasUnconstrained <http://rdaregistry.info/Elements/u/P60922> ;
    reg:lexicalAlias <http://rdaregistry.info/Elements/n/variantNameOfPlaceOf.en> ;
    reg:name "variantNameOfPlaceOf"@en ;
    reg:status <http://metadataregistry.org/uri/RegStatus/1001> ;
    rdfs:domain <http://rdaregistry.info/Elements/c/C10012> ;
    rdfs:isDefinedBy <http://rdaregistry.info/Elements/n/> ;
    rdfs:subPropertyOf <http://rdaregistry.info/Elements/n/P80051>,
        <http://rdaregistry.info/Elements/n/P80164> ;
    skos:definition "Relates a nomen to a place that has a name of place that is not selected for preference in a specific application or context."@en .

<http://rdaregistry.info/Elements/n/P80089> a rdf:Property ;
    rdfs:label "is authorized access point for manifestation of"@en ;
    rdakit:hasElementType "2" ;
    rdakit:toolkitDefinition "A manifestation that has an access point for manifestation that is selected for preference in a specific vocabulary encoding scheme."@en ;
    rdakit:toolkitLabel "authorized access point for manifestation of"@en ;
    reg:hasSubproperty <http://rdaregistry.info/Elements/n/datatype/P80089>,
        <http://rdaregistry.info/Elements/n/object/P80089> ;
    reg:hasUnconstrained <http://rdaregistry.info/Elements/u/P60918> ;
    reg:lexicalAlias <http://rdaregistry.info/Elements/n/authorizedAccessPointForManifestationOf.en> ;
    reg:name "authorizedAccessPointForManifestationOf"@en ;
    reg:status <http://metadataregistry.org/uri/RegStatus/1001> ;
    rdfs:domain <http://rdaregistry.info/Elements/c/C10012> ;
    rdfs:isDefinedBy <http://rdaregistry.info/Elements/n/> ;
    rdfs:subPropertyOf <http://rdaregistry.info/Elements/n/P80024>,
        <http://rdaregistry.info/Elements/n/P80162> ;
    skos:definition "Relates a nomen to a manifestation that has an access point for manifestation that is selected for preference in a specific vocabulary encoding scheme."@en .

<http://rdaregistry.info/Elements/n/P80091> a rdf:Property ;
    rdfs:label "is authorized access point for item of"@en ;
    rdakit:hasElementType "2" ;
    rdakit:toolkitDefinition "An item that has an access point for item that is selected for preference in a specific vocabulary encoding scheme."@en ;
    rdakit:toolkitLabel "authorized access point for item of"@en ;
    reg:hasSubproperty <http://rdaregistry.info/Elements/n/datatype/P80091>,
        <http://rdaregistry.info/Elements/n/object/P80091> ;
    reg:hasUnconstrained <http://rdaregistry.info/Elements/u/P60918> ;
    reg:lexicalAlias <http://rdaregistry.info/Elements/n/authorizedAccessPointForItemOf.en> ;
    reg:name "authorizedAccessPointForItemOf"@en ;
    reg:status <http://metadataregistry.org/uri/RegStatus/1001> ;
    rdfs:domain <http://rdaregistry.info/Elements/c/C10012> ;
    rdfs:isDefinedBy <http://rdaregistry.info/Elements/n/> ;
    rdfs:subPropertyOf <http://rdaregistry.info/Elements/n/P80015>,
        <http://rdaregistry.info/Elements/n/P80162> ;
    skos:definition "Relates a nomen to an item that has an access point for item that is selected for preference in a specific vocabulary encoding scheme."@en .

<http://rdaregistry.info/Elements/n/P80094> a rdf:Property ;
    rdfs:label "is variant title of item of"@en ;
    rdakit:hasElementType "2" ;
    rdakit:toolkitDefinition "An item that has a title of item that is not selected for preference in a specific application or context."@en ;
    rdakit:toolkitLabel "variant title of item of"@en ;
    reg:hasSubproperty <http://rdaregistry.info/Elements/n/datatype/P80094>,
        <http://rdaregistry.info/Elements/n/object/P80094> ;
    reg:hasUnconstrained <http://rdaregistry.info/Elements/u/P60925> ;
    reg:lexicalAlias <http://rdaregistry.info/Elements/n/variantTitleOfItemOf.en> ;
    reg:name "variantTitleOfItemOf"@en ;
    reg:status <http://metadataregistry.org/uri/RegStatus/1001> ;
    rdfs:domain <http://rdaregistry.info/Elements/c/C10012> ;
    rdfs:isDefinedBy <http://rdaregistry.info/Elements/n/> ;
    rdfs:subPropertyOf <http://rdaregistry.info/Elements/n/P80017>,
        <http://rdaregistry.info/Elements/n/P80164> ;
    skos:definition "Relates a nomen to an item that has a title of item that is not selected for preference in a specific application or context."@en .

<http://rdaregistry.info/Elements/n/P80095> a rdf:Property ;
    rdfs:label "is authorized access point for expression of"@en ;
    rdakit:hasElementType "2" ;
    rdakit:toolkitDefinition "An expression that has an access point for expression that is selected for preference in a specific vocabulary encoding scheme."@en ;
    rdakit:toolkitLabel "authorized access point for expression of"@en ;
    reg:hasSubproperty <http://rdaregistry.info/Elements/n/datatype/P80095>,
        <http://rdaregistry.info/Elements/n/object/P80095> ;
    reg:hasUnconstrained <http://rdaregistry.info/Elements/u/P60918> ;
    reg:lexicalAlias <http://rdaregistry.info/Elements/n/authorizedAccessPointForExpressionOf.en> ;
    reg:name "authorizedAccessPointForExpressionOf"@en ;
    reg:status <http://metadataregistry.org/uri/RegStatus/1001> ;
    rdfs:domain <http://rdaregistry.info/Elements/c/C10012> ;
    rdfs:isDefinedBy <http://rdaregistry.info/Elements/n/> ;
    rdfs:subPropertyOf <http://rdaregistry.info/Elements/n/P80023>,
        <http://rdaregistry.info/Elements/n/P80162> ;
    skos:definition "Relates a nomen to an expression that has an access point for expression that is selected for preference in a specific vocabulary encoding scheme."@en .

<http://rdaregistry.info/Elements/n/P80098> a rdf:Property ;
    rdfs:label "is variant title of expression of"@en ;
    rdakit:hasElementType "2" ;
    rdakit:toolkitDefinition "An expression that has a title of expression that is not selected for preference in a specific application or context."@en ;
    rdakit:toolkitLabel "variant title of expression of"@en ;
    reg:hasSubproperty <http://rdaregistry.info/Elements/n/datatype/P80098>,
        <http://rdaregistry.info/Elements/n/object/P80098> ;
    reg:hasUnconstrained <http://rdaregistry.info/Elements/u/P60925> ;
    reg:lexicalAlias <http://rdaregistry.info/Elements/n/variantTitleOfExpressionOf.en> ;
    reg:name "variantTitleOfExpressionOf"@en ;
    reg:status <http://metadataregistry.org/uri/RegStatus/1001> ;
    rdfs:domain <http://rdaregistry.info/Elements/c/C10012> ;
    rdfs:isDefinedBy <http://rdaregistry.info/Elements/n/> ;
    rdfs:subPropertyOf <http://rdaregistry.info/Elements/n/P80039>,
        <http://rdaregistry.info/Elements/n/P80164> ;
    skos:definition "Relates a nomen to an expression that has a title of expression that is not selected for preference in a specific application or context."@en .

<http://rdaregistry.info/Elements/n/P80110> a rdf:Property ;
    rdfs:label "is variant title of work of"@en ;
    rdakit:hasElementType "2" ;
    rdakit:toolkitDefinition "A work that has a title of work that is not selected for preference in a specific application or context."@en ;
    rdakit:toolkitLabel "variant title of work of"@en ;
    reg:hasSubproperty <http://rdaregistry.info/Elements/n/datatype/P80110>,
        <http://rdaregistry.info/Elements/n/object/P80110> ;
    reg:hasUnconstrained <http://rdaregistry.info/Elements/u/P60925> ;
    reg:lexicalAlias <http://rdaregistry.info/Elements/n/variantTitleOfWorkOf.en> ;
    reg:name "variantTitleOfWorkOf"@en ;
    reg:status <http://metadataregistry.org/uri/RegStatus/1001> ;
    rdfs:domain <http://rdaregistry.info/Elements/c/C10012> ;
    rdfs:isDefinedBy <http://rdaregistry.info/Elements/n/> ;
    rdfs:subPropertyOf <http://rdaregistry.info/Elements/n/P80064>,
        <http://rdaregistry.info/Elements/n/P80164> ;
    skos:definition "Relates a nomen to a work that has a title of work that is not selected for preference in a specific application or context."@en ;
    skos:scopeNote "A variant title of work includes a title or form of title appearing on a manifestation of the work or found in reference sources, a title resulting from a different transliteration of a title, etc."@en .

<http://rdaregistry.info/Elements/n/P80113> a rdf:Property ;
    rdfs:label "is equivalent to"@en ;
    rdakit:hasElementType "2" ;
    rdakit:toolkitDefinition "A nomen that is an appellation of the same entity as another nomen."@en ;
    rdakit:toolkitLabel "equivalent to"@en ;
    reg:hasSubproperty <http://rdaregistry.info/Elements/n/datatype/P80113>,
        <http://rdaregistry.info/Elements/n/object/P80113> ;
    reg:hasUnconstrained <http://rdaregistry.info/Elements/u/P61123> ;
    reg:lexicalAlias <http://rdaregistry.info/Elements/n/equivalentTo.en> ;
    reg:name "equivalentTo"@en ;
    reg:status <http://metadataregistry.org/uri/RegStatus/1001> ;
    rdfs:domain <http://rdaregistry.info/Elements/c/C10012> ;
    rdfs:isDefinedBy <http://rdaregistry.info/Elements/n/> ;
    rdfs:subPropertyOf <http://rdaregistry.info/Elements/n/P80009> ;
    skos:definition "Relates a nomen to a nomen that is an appellation of the same entity as another nomen."@en .

<http://rdaregistry.info/Elements/n/P80120> a rdf:Property ;
    rdfs:label "is opus number of"@en ;
    rdakit:hasElementType "2" ;
    rdakit:toolkitDefinition "A musical work that has an identifier for work that is a numeric designation assigned from a list of works of a composer indicating chronological order of composition."@en ;
    rdakit:toolkitLabel "opus number of"@en ;
    reg:hasSubproperty <http://rdaregistry.info/Elements/n/datatype/P80120> ;
    reg:hasUnconstrained <http://rdaregistry.info/Elements/u/P60962> ;
    reg:lexicalAlias <http://rdaregistry.info/Elements/n/opusNumberOf.en> ;
    reg:name "opusNumberOf"@en ;
    reg:status <http://metadataregistry.org/uri/RegStatus/1001> ;
    rdfs:domain <http://rdaregistry.info/Elements/c/C10012> ;
    rdfs:isDefinedBy <http://rdaregistry.info/Elements/n/> ;
    rdfs:subPropertyOf <http://rdaregistry.info/Elements/n/P80119> ;
    skos:definition "Relates a nomen to a musical work that has an identifier for work that is a numeric designation assigned from a list of works of a composer indicating chronological order of composition."@en .

<http://rdaregistry.info/Elements/n/P80121> a rdf:Property ;
    rdfs:label "is serial number of musical work of"@en ;
    rdakit:hasElementType "2" ;
    rdakit:toolkitDefinition "A musical work that has a numeric designation of musical work assigned by a composer or a reference source that indicates a sequence of musical works that share the same title or that share the same title and the same representative medium of performance."@en ;
    rdakit:toolkitLabel "serial number of musical work of"@en ;
    reg:hasSubproperty <http://rdaregistry.info/Elements/n/datatype/P80121> ;
    reg:hasUnconstrained <http://rdaregistry.info/Elements/u/P60961> ;
    reg:lexicalAlias <http://rdaregistry.info/Elements/n/serialNumberOfMusicalWorkOf.en> ;
    reg:name "serialNumberOfMusicalWorkOf"@en ;
    reg:status <http://metadataregistry.org/uri/RegStatus/1001> ;
    rdfs:domain <http://rdaregistry.info/Elements/c/C10012> ;
    rdfs:isDefinedBy <http://rdaregistry.info/Elements/n/> ;
    rdfs:subPropertyOf <http://rdaregistry.info/Elements/n/P80119> ;
    skos:definition "Relates a nomen to a musical work that has a numeric designation of musical work assigned by a composer or a reference source that indicates a sequence of musical works that share the same title or that share the same title and the same representative medium of performance."@en .

<http://rdaregistry.info/Elements/n/P80122> a rdf:Property ;
    rdfs:label "is thematic index number of"@en ;
    rdakit:hasElementType "2" ;
    rdakit:toolkitDefinition "A musical work that has an identifier for work that is a numeric designation assigned from a list of works of a composer, usually arranged in chronological order or by categories, with the theme given for each composition or for each section of large compositions."@en ;
    rdakit:toolkitLabel "thematic index number of"@en ;
    reg:hasSubproperty <http://rdaregistry.info/Elements/n/datatype/P80122>,
        <http://rdaregistry.info/Elements/n/object/P80113>,
        <http://rdaregistry.info/Elements/n/object/P80122> ;
    reg:hasUnconstrained <http://rdaregistry.info/Elements/u/P60960> ;
    reg:lexicalAlias <http://rdaregistry.info/Elements/n/thematicIndexNumberOf.en> ;
    reg:name "thematicIndexNumberOf"@en ;
    reg:status <http://metadataregistry.org/uri/RegStatus/1001> ;
    rdfs:domain <http://rdaregistry.info/Elements/c/C10012> ;
    rdfs:isDefinedBy <http://rdaregistry.info/Elements/n/> ;
    rdfs:subPropertyOf <http://rdaregistry.info/Elements/n/P80119> ;
    skos:definition "Relates a nomen to a musical work that has an identifier for work that is a numeric designation assigned from a list of works of a composer, usually arranged in chronological order or by categories, with the theme given for each composition or for each section of large compositions."@en .

<http://rdaregistry.info/Elements/n/P80123> a rdf:Property ;
    rdfs:label "is earlier title proper of"@en ;
    rdakit:hasElementType "2" ;
    reg:hasSubproperty <http://rdaregistry.info/Elements/n/object/P80123> ;
    reg:name "earlierTitleProperOf"@en ;
    reg:status <http://metadataregistry.org/uri/RegStatus/1008> ;
    rdfs:isDefinedBy <http://rdaregistry.info/Elements/n/> .

<http://rdaregistry.info/Elements/n/P80124> a rdf:Property ;
    rdfs:label "is later title proper of (Deprecated)"@en ;
    rdakit:hasElementType "2" ;
    reg:hasSubproperty <http://rdaregistry.info/Elements/n/object/P80124> ;
    reg:lexicalAlias <http://rdaregistry.info/Elements/n/laterTitleProperOf.en> ;
    reg:name "laterTitleProperOf"@en ;
    reg:status <http://metadataregistry.org/uri/RegStatus/1008> ;
    rdfs:isDefinedBy <http://rdaregistry.info/Elements/n/> .

<http://rdaregistry.info/Elements/n/P80127> a rdf:Property ;
    rdfs:label "is parallel name of distributor of"@en ;
    rdakit:hasElementType "2" ;
    rdakit:toolkitDefinition "A manifestation that has a name of distributor in another language or script."@en ;
    rdakit:toolkitLabel "parallel name of distributor of"@en ;
    reg:hasSubproperty <http://rdaregistry.info/Elements/n/datatype/P80127> ;
    reg:hasUnconstrained <http://rdaregistry.info/Elements/u/P60946> ;
    reg:lexicalAlias <http://rdaregistry.info/Elements/n/parallelNameOfDistributorOf.en> ;
    reg:name "parallelNameOfDistributorOf"@en ;
    reg:status <http://metadataregistry.org/uri/RegStatus/1001> ;
    rdfs:domain <http://rdaregistry.info/Elements/c/C10012> ;
    rdfs:isDefinedBy <http://rdaregistry.info/Elements/n/> ;
    rdfs:subPropertyOf <http://rdaregistry.info/Elements/n/P80115> ;
    skos:definition "Relates a nomen to a manifestation that has a name of distributor in another language or script."@en .

<http://rdaregistry.info/Elements/n/P80128> a rdf:Property ;
    rdfs:label "is parallel name of manufacturer of"@en ;
    rdakit:hasElementType "2" ;
    rdakit:toolkitDefinition "A manifestation that has a name of manufacturer in another language or script."@en ;
    rdakit:toolkitLabel "parallel name of manufacturer of"@en ;
    reg:hasSubproperty <http://rdaregistry.info/Elements/n/datatype/P80128> ;
    reg:hasUnconstrained <http://rdaregistry.info/Elements/u/P60948> ;
    reg:lexicalAlias <http://rdaregistry.info/Elements/n/parallelNameOfManufacturerOf.en> ;
    reg:name "parallelNameOfManufacturerOf"@en ;
    reg:status <http://metadataregistry.org/uri/RegStatus/1001> ;
    rdfs:domain <http://rdaregistry.info/Elements/c/C10012> ;
    rdfs:isDefinedBy <http://rdaregistry.info/Elements/n/> ;
    rdfs:subPropertyOf <http://rdaregistry.info/Elements/n/P80116> ;
    skos:definition "Relates a nomen to a manifestation that has a name of manufacturer in another language or script."@en .

<http://rdaregistry.info/Elements/n/P80129> a rdf:Property ;
    rdfs:label "is parallel name of producer of"@en ;
    rdakit:hasElementType "2" ;
    rdakit:toolkitDefinition "A manifestation that has a name of producer in another language or script."@en ;
    rdakit:toolkitLabel "parallel name of producer of"@en ;
    reg:hasSubproperty <http://rdaregistry.info/Elements/n/datatype/P80129> ;
    reg:hasUnconstrained <http://rdaregistry.info/Elements/u/P60949> ;
    reg:lexicalAlias <http://rdaregistry.info/Elements/n/parallelNameOfProducerOf.en> ;
    reg:name "parallelNameOfProducerOf"@en ;
    reg:status <http://metadataregistry.org/uri/RegStatus/1001> ;
    rdfs:domain <http://rdaregistry.info/Elements/c/C10012> ;
    rdfs:isDefinedBy <http://rdaregistry.info/Elements/n/> ;
    rdfs:subPropertyOf <http://rdaregistry.info/Elements/n/P80117> ;
    skos:definition "Relates a nomen to a manifestation that has a name of producer in another language or script."@en .

<http://rdaregistry.info/Elements/n/P80130> a rdf:Property ;
    rdfs:label "is parallel name of publisher of"@en ;
    rdakit:hasElementType "2" ;
    rdakit:toolkitDefinition "A manifestation that has a name of publisher in another language or script."@en ;
    rdakit:toolkitLabel "parallel name of publisher of"@en ;
    reg:hasSubproperty <http://rdaregistry.info/Elements/n/datatype/P80130> ;
    reg:hasUnconstrained <http://rdaregistry.info/Elements/u/P60950> ;
    reg:lexicalAlias <http://rdaregistry.info/Elements/n/parallelNameOfPublisherOf.en> ;
    reg:name "parallelNameOfPublisherOf"@en ;
    reg:status <http://metadataregistry.org/uri/RegStatus/1001> ;
    rdfs:domain <http://rdaregistry.info/Elements/c/C10012> ;
    rdfs:isDefinedBy <http://rdaregistry.info/Elements/n/> ;
    rdfs:subPropertyOf <http://rdaregistry.info/Elements/n/P80118> ;
    skos:definition "Relates a nomen to a manifestation that has a name of publisher in another language or script."@en .

<http://rdaregistry.info/Elements/n/P80137> a rdf:Property ;
    rdfs:label "is parallel title proper of subseries of (Deprecated)"@en ;
    rdakit:hasElementType "2" ;
    rdakit:toolkitDefinition "A manifestation that has a title proper of subseries in another language or script. (Deprecated)"@en ;
    rdakit:toolkitLabel "parallel title proper of subseries of (Deprecated)"@en ;
    reg:hasSubproperty <http://rdaregistry.info/Elements/n/datatype/P80137> ;
    reg:lexicalAlias <http://rdaregistry.info/Elements/n/parallelTitleProperOfSubseriesOf.en> ;
    reg:name "parallelTitleProperOfSubseriesOf"@en ;
    reg:status <http://metadataregistry.org/uri/RegStatus/1008> ;
    rdfs:domain <http://rdaregistry.info/Elements/c/C10012> ;
    rdfs:isDefinedBy <http://rdaregistry.info/Elements/n/> ;
    rdfs:subPropertyOf <http://rdaregistry.info/Elements/n/P80126>,
        <http://rdaregistry.info/Elements/n/P80136> ;
    skos:definition "Relates a nomen to a manifestation that has a title proper of subseries in another language or script. (Deprecated)"@en .

<http://rdaregistry.info/Elements/n/P80138> a rdf:Property ;
    rdfs:label "is fingerprint of"@en ;
    rdakit:hasElementType "2" ;
    rdakit:toolkitDefinition "A manifestation that has an identifier for manifestation that consists of a group of characters from specified locations in a manifestation combined with a date of publication or other element."@en ;
    rdakit:toolkitLabel "fingerprint of"@en ;
    reg:hasSubproperty <http://rdaregistry.info/Elements/n/datatype/P80138>,
        <http://rdaregistry.info/Elements/n/object/P80138> ;
    reg:hasUnconstrained <http://rdaregistry.info/Elements/u/P61158> ;
    reg:lexicalAlias <http://rdaregistry.info/Elements/n/fingerprintOf.en> ;
    reg:name "fingerprintOf"@en ;
    reg:status <http://metadataregistry.org/uri/RegStatus/1001> ;
    rdfs:domain <http://rdaregistry.info/Elements/c/C10012> ;
    rdfs:isDefinedBy <http://rdaregistry.info/Elements/n/> ;
    rdfs:subPropertyOf <http://rdaregistry.info/Elements/n/P80048> ;
    skos:definition "Relates a nomen to a manifestation that has an identifier for manifestation that consists of a group of characters from specified locations in a manifestation combined with a date of publication or other element."@en .

<http://rdaregistry.info/Elements/n/P80150> a rdf:Property ;
    rdfs:label "is address of corporate body of"@en ;
    rdakit:hasElementType "2" ;
    reg:name "addressOfCorporateBodyOf"@en ;
    reg:status <http://metadataregistry.org/uri/RegStatus/1008> ;
    rdfs:isDefinedBy <http://rdaregistry.info/Elements/n/> .

<http://rdaregistry.info/Elements/n/P80151> a rdf:Property ;
    rdfs:label "is address of person of"@en ;
    rdakit:hasElementType "2" ;
    reg:name "addressOfPersonOf"@en ;
    reg:status <http://metadataregistry.org/uri/RegStatus/1008> ;
    rdfs:isDefinedBy <http://rdaregistry.info/Elements/n/> .

<http://rdaregistry.info/Elements/n/P80152> a rdf:Property ;
    rdfs:label "is address of family of"@en ;
    rdakit:hasElementType "2" ;
    reg:name "addressOfFamilyOf"@en ;
    reg:status <http://metadataregistry.org/uri/RegStatus/1008> ;
    rdfs:isDefinedBy <http://rdaregistry.info/Elements/n/> .

<http://rdaregistry.info/Elements/n/P80153> a rdf:Property ;
    rdfs:label "is address of agent of"@en ;
    rdakit:hasElementType "2" ;
    reg:name "addressOfAgentOf"@en ;
    reg:status <http://metadataregistry.org/uri/RegStatus/1008> ;
    rdfs:isDefinedBy <http://rdaregistry.info/Elements/n/> .

<http://rdaregistry.info/Elements/n/P80154> a rdf:Property ;
    rdfs:label "is address of collective agent of"@en ;
    rdakit:hasElementType "2" ;
    reg:name "addressOfCollectiveAgentOf"@en ;
    reg:status <http://metadataregistry.org/uri/RegStatus/1008> ;
    rdfs:isDefinedBy <http://rdaregistry.info/Elements/n/> .

<http://rdaregistry.info/Elements/n/P80155> a rdf:Property ;
    rdfs:label "is plate number for notated music of"@en ;
    rdakit:hasElementType "2" ;
    rdakit:toolkitDefinition "A manifestation of a notated music expression that has an identifier for manifestation other than a publisher number for notated music, assigned by a publisher to indicate the printing plate used in the printing process."@en ;
    rdakit:toolkitLabel "plate number for notated music of"@en ;
    reg:hasSubproperty <http://rdaregistry.info/Elements/n/datatype/P80155> ;
    reg:hasUnconstrained <http://rdaregistry.info/Elements/u/P60988> ;
    reg:lexicalAlias <http://rdaregistry.info/Elements/n/plateNumberForNotatedMusicOf.en> ;
    reg:name "plateNumberForNotatedMusicOf"@en ;
    reg:status <http://metadataregistry.org/uri/RegStatus/1001> ;
    rdfs:domain <http://rdaregistry.info/Elements/c/C10012> ;
    rdfs:isDefinedBy <http://rdaregistry.info/Elements/n/> ;
    rdfs:subPropertyOf <http://rdaregistry.info/Elements/n/P80048> ;
    skos:definition "Relates a nomen to a manifestation of a notated music expression that has an identifier for manifestation other than a publisher number for notated music, assigned by a publisher to indicate the printing plate used in the printing process."@en ;
    skos:scopeNote "The number normally appears at the bottom of each page, and sometimes on the title page. The number may include initials, abbreviations, or words identifying the publisher, or followed by a number corresponding to the number of pages or plates or a number corresponding to an individual page or plate."@en .

<http://rdaregistry.info/Elements/n/P80156> a rdf:Property ;
    rdfs:label "is publisher number for notated music of"@en ;
    rdakit:hasElementType "2" ;
    rdakit:toolkitDefinition "A manifestation of a notated music expression that has an identifier for manifestation other than a plate number for notated music, assigned by a publisher."@en ;
    rdakit:toolkitLabel "publisher number for notated music of"@en ;
    reg:hasSubproperty <http://rdaregistry.info/Elements/n/datatype/P80156> ;
    reg:hasUnconstrained <http://rdaregistry.info/Elements/u/P60989> ;
    reg:lexicalAlias <http://rdaregistry.info/Elements/n/publisherNumberForNotatedMusicOf.en> ;
    reg:name "publisherNumberForNotatedMusicOf"@en ;
    reg:status <http://metadataregistry.org/uri/RegStatus/1001> ;
    rdfs:domain <http://rdaregistry.info/Elements/c/C10012> ;
    rdfs:isDefinedBy <http://rdaregistry.info/Elements/n/> ;
    rdfs:subPropertyOf <http://rdaregistry.info/Elements/n/P80048> ;
    skos:definition "Relates a nomen to a manifestation of a notated music expression that has an identifier for manifestation other than a plate number for notated music, assigned by a publisher."@en .

<http://rdaregistry.info/Elements/n/P80157> a rdf:Property ;
    rdfs:label "is alternate identity of person of"@en ;
    rdakit:hasElementType "2" ;
    rdakit:toolkitDefinition "A person that has an appellation of person that is a pseudonym or other assumed identity."@en ;
    rdakit:toolkitLabel "alternate identity of person of"@en ;
    reg:hasSubproperty <http://rdaregistry.info/Elements/n/datatype/P80157> ;
    reg:hasUnconstrained <http://rdaregistry.info/Elements/u/P61112> ;
    reg:lexicalAlias <http://rdaregistry.info/Elements/n/alternateIdentityOfPersonOf.en> ;
    reg:name "alternateIdentityOfPersonOf"@en ;
    reg:status <http://metadataregistry.org/uri/RegStatus/1001> ;
    rdfs:domain <http://rdaregistry.info/Elements/c/C10012> ;
    rdfs:isDefinedBy <http://rdaregistry.info/Elements/n/> ;
    rdfs:subPropertyOf <http://rdaregistry.info/Elements/n/P80032> ;
    skos:definition "Relates a nomen to a person that has an appellation of person that is a pseudonym or other assumed identity."@en .

<http://rdaregistry.info/Elements/n/P80158> a rdf:Property ;
    rdfs:label "is real identity of person of"@en ;
    rdakit:hasElementType "2" ;
    rdakit:toolkitDefinition "A person that has an appellation of person that is a real identity."@en ;
    rdakit:toolkitLabel "real identity of person of"@en ;
    reg:hasSubproperty <http://rdaregistry.info/Elements/n/datatype/P80158> ;
    reg:hasUnconstrained <http://rdaregistry.info/Elements/u/P61113> ;
    reg:lexicalAlias <http://rdaregistry.info/Elements/n/realIdentityOfPersonOf.en> ;
    reg:name "realIdentityOfPersonOf"@en ;
    reg:status <http://metadataregistry.org/uri/RegStatus/1001> ;
    rdfs:domain <http://rdaregistry.info/Elements/c/C10012> ;
    rdfs:isDefinedBy <http://rdaregistry.info/Elements/n/> ;
    rdfs:subPropertyOf <http://rdaregistry.info/Elements/n/P80032> ;
    skos:definition "Relates a nomen to a person that has an appellation of person that is a real identity."@en .

<http://rdaregistry.info/Elements/n/P80166> a rdf:Property ;
    rdfs:label "has date of usage"@en ;
    rdakit:hasElementType "3" ;
    rdakit:toolkitDefinition "A date or range of dates that is associated with the use of an appellation of an RDA entity."@en ;
    rdakit:toolkitLabel "date of usage"@en ;
    reg:hasSubproperty <http://rdaregistry.info/Elements/n/datatype/P80166>,
        <http://rdaregistry.info/Elements/n/object/P80166> ;
    reg:hasUnconstrained <http://rdaregistry.info/Elements/u/P61120> ;
    reg:lexicalAlias <http://rdaregistry.info/Elements/n/dateOfUsage.en> ;
    reg:name "dateOfUsage"@en ;
    reg:status <http://metadataregistry.org/uri/RegStatus/1001> ;
    rdfs:domain <http://rdaregistry.info/Elements/c/C10012> ;
    rdfs:isDefinedBy <http://rdaregistry.info/Elements/n/> ;
    rdfs:subPropertyOf <http://rdaregistry.info/Elements/n/P80008> ;
    skos:definition "Relates a nomen to a date or range of dates that is associated with the use of an appellation of an RDA entity."@en .

<http://rdaregistry.info/Elements/n/P80170> a rdf:Property ;
    rdfs:label "is ISSN of"@en ;
    rdakit:hasElementType "2" ;
    rdakit:toolkitDefinition "A work that has an identifier assigned by an ISSN registration agency."@en ;
    rdakit:toolkitLabel "ISSN of"@en ;
    reg:hasSubproperty <http://rdaregistry.info/Elements/n/datatype/P80170>,
        <http://rdaregistry.info/Elements/n/object/P80170> ;
    reg:hasUnconstrained <http://rdaregistry.info/Elements/u/P61117> ;
    reg:lexicalAlias <http://rdaregistry.info/Elements/n/issnOf.en> ;
    reg:name "issnOf" ;
    reg:status <http://metadataregistry.org/uri/RegStatus/1001> ;
    rdfs:domain <http://rdaregistry.info/Elements/c/C10012> ;
    rdfs:isDefinedBy <http://rdaregistry.info/Elements/n/> ;
    rdfs:subPropertyOf <http://rdaregistry.info/Elements/n/P80049> ;
    skos:altLabel "International Standard Serial Number of"@en ;
    skos:definition "Relates a nomen to a work that has an identifier assigned by an ISSN registration agency."@en .

<http://rdaregistry.info/Elements/n/P80174> a rdf:Property ;
    rdfs:label "has related entity of nomen"@en ;
    rdakit:hasElementType "1" ;
    rdakit:toolkitDefinition "An entity that is associated with a nomen."@en ;
    rdakit:toolkitLabel "related entity of nomen"@en ;
    reg:hasUnconstrained <http://rdaregistry.info/Elements/u/P61037> ;
    reg:lexicalAlias <http://rdaregistry.info/Elements/n/relatedEntityOfNomen.en> ;
    reg:name "relatedEntityOfNomen" ;
    reg:status <http://metadataregistry.org/uri/RegStatus/1001> ;
    rdfs:domain <http://rdaregistry.info/Elements/c/C10012> ;
    rdfs:isDefinedBy <http://rdaregistry.info/Elements/n/> ;
    rdfs:subPropertyOf <http://rdaregistry.info/Elements/x/P00028> ;
    skos:definition "Relates a nomen to an entity that is associated with a nomen."@en .

<http://rdaregistry.info/Elements/n/P80175> a rdf:Property ;
    rdfs:label "is given name of"@en ;
    rdakit:hasElementType "2" ;
    rdakit:toolkitDefinition "A person who uses a name given at birth or at some later point in addition to, or instead of, a surname."@en ;
    rdakit:toolkitLabel "given name of"@en ;
    reg:hasSubproperty <http://rdaregistry.info/Elements/n/object/P80175> ;
    reg:lexicalAlias <http://rdaregistry.info/Elements/n/giveNameOf.en> ;
    reg:name "givenNameOf" ;
    reg:status <http://metadataregistry.org/uri/RegStatus/1001> ;
    rdfs:domain <http://rdaregistry.info/Elements/c/C10012> ;
    rdfs:isDefinedBy <http://rdaregistry.info/Elements/n/> ;
    rdfs:subPropertyOf <http://rdaregistry.info/Elements/n/P80056> ;
    skos:definition "Relates a nomen to a person who uses a name given at birth or at some later point in addition to, or instead of, a surname."@en .

<http://rdaregistry.info/Elements/n/P80176> a rdf:Property ;
    rdfs:label "is surname of"@en ;
    rdakit:hasElementType "2" ;
    rdakit:toolkitDefinition "A person who uses a family name."@en ;
    rdakit:toolkitLabel "surname of"@en ;
    reg:hasSubproperty <http://rdaregistry.info/Elements/n/object/P80176> ;
    reg:lexicalAlias <http://rdaregistry.info/Elements/n/surnameOf.en> ;
    reg:name "surnameOf" ;
    reg:status <http://metadataregistry.org/uri/RegStatus/1001> ;
    rdfs:domain <http://rdaregistry.info/Elements/c/C10012> ;
    rdfs:isDefinedBy <http://rdaregistry.info/Elements/n/> ;
    rdfs:subPropertyOf <http://rdaregistry.info/Elements/n/P80056> ;
    skos:definition "Relates a nomen to a person who uses a family name."@en .

<http://rdaregistry.info/Elements/n/P80177> a rdf:Property ;
    rdfs:label "is fuller form of name of"@en ;
    rdakit:hasElementType "2" ;
    rdakit:toolkitDefinition "A person who has a fuller form of a name or part of a name represented by an initial, abbreviation, or shortened or otherwise modified form."@en ;
    rdakit:toolkitLabel "fuller form of name of"@en ;
    reg:hasSubproperty <http://rdaregistry.info/Elements/n/object/P80177> ;
    reg:lexicalAlias <http://rdaregistry.info/Elements/n/fullerFormOfNameOf.en> ;
    reg:name "fullerFormOfNameOf" ;
    reg:status <http://metadataregistry.org/uri/RegStatus/1001> ;
    rdfs:domain <http://rdaregistry.info/Elements/c/C10012> ;
    rdfs:isDefinedBy <http://rdaregistry.info/Elements/n/> ;
    rdfs:subPropertyOf <http://rdaregistry.info/Elements/n/P80056> ;
    skos:definition "Relates a nomen to a person who has a fuller form of a name or part of a name represented by an initial, abbreviation, or shortened or otherwise modified form."@en .

<http://rdaregistry.info/Elements/n/P80178> a rdf:Property ;
    rdfs:label "is nomen described in"@en ;
    rdakit:hasElementType "2" ;
    rdakit:toolkitDefinition "A work that describes a nomen."@en ;
    rdakit:toolkitLabel "nomen described in"@en ;
    reg:hasSubproperty <http://rdaregistry.info/Elements/n/datatype/P80178>,
        <http://rdaregistry.info/Elements/n/object/P80178> ;
    reg:hasUnconstrained <http://rdaregistry.info/Elements/u/P60215> ;
    reg:lexicalAlias <http://rdaregistry.info/Elements/n/nomenDescribedIn.en> ;
    reg:name "nomenDescribedIn" ;
    reg:status <http://metadataregistry.org/uri/RegStatus/1001> ;
    rdfs:domain <http://rdaregistry.info/Elements/c/C10012> ;
    rdfs:isDefinedBy <http://rdaregistry.info/Elements/n/> ;
    rdfs:subPropertyOf <http://rdaregistry.info/Elements/n/P80014> ;
    skos:definition "Relates a nomen to a work that describes a nomen."@en .

<http://rdaregistry.info/Elements/n/P80002> a rdf:Property ;
    rdfs:label "has related expression of nomen"@en ;
    rdakit:hasElementType "1" ;
    rdakit:toolkitDefinition "An expression that is associated with a nomen."@en ;
    rdakit:toolkitLabel "related expression of nomen"@en ;
    reg:hasSubproperty <http://rdaregistry.info/Elements/n/P80038>,
        <http://rdaregistry.info/Elements/n/datatype/P80002>,
        <http://rdaregistry.info/Elements/n/object/P80002> ;
    reg:hasUnconstrained <http://rdaregistry.info/Elements/u/P61030> ;
    reg:lexicalAlias <http://rdaregistry.info/Elements/n/relatedExpressionOfNomen.en> ;
    reg:name "relatedExpressionOfNomen"@en ;
    reg:status <http://metadataregistry.org/uri/RegStatus/1001> ;
    rdfs:domain <http://rdaregistry.info/Elements/c/C10012> ;
    rdfs:isDefinedBy <http://rdaregistry.info/Elements/n/> ;
    rdfs:subPropertyOf <http://rdaregistry.info/Elements/n/P80010>,
        <http://rdaregistry.info/Elements/x/P00003> ;
    skos:definition "Relates a nomen to an expression that is associated with a nomen."@en .

<http://rdaregistry.info/Elements/n/P80004> a rdf:Property ;
    rdfs:label "has related item of nomen"@en ;
    rdakit:hasElementType "1" ;
    rdakit:toolkitDefinition "An item that is associated with a nomen."@en ;
    rdakit:toolkitLabel "related item of nomen"@en ;
    reg:hasSubproperty <http://rdaregistry.info/Elements/n/P80016>,
        <http://rdaregistry.info/Elements/n/datatype/P80004>,
        <http://rdaregistry.info/Elements/n/object/P80004> ;
    reg:hasUnconstrained <http://rdaregistry.info/Elements/u/P61030> ;
    reg:lexicalAlias <http://rdaregistry.info/Elements/n/relatedItemOfNomen.en> ;
    reg:name "relatedItemOfNomen"@en ;
    reg:status <http://metadataregistry.org/uri/RegStatus/1001> ;
    rdfs:domain <http://rdaregistry.info/Elements/c/C10012> ;
    rdfs:isDefinedBy <http://rdaregistry.info/Elements/n/> ;
    rdfs:subPropertyOf <http://rdaregistry.info/Elements/n/P80010>,
        <http://rdaregistry.info/Elements/x/P00005> ;
    skos:definition "Relates a nomen to an item that is associated with a nomen."@en .

<http://rdaregistry.info/Elements/n/P80007> a rdf:Property ;
    rdfs:label "has related place of nomen"@en ;
    rdakit:hasElementType "1" ;
    rdakit:toolkitDefinition "A place that is associated with a nomen."@en ;
    rdakit:toolkitLabel "related place of nomen"@en ;
    reg:hasSubproperty <http://rdaregistry.info/Elements/n/P80041>,
        <http://rdaregistry.info/Elements/n/datatype/P80007>,
        <http://rdaregistry.info/Elements/n/object/P80007> ;
    reg:hasUnconstrained <http://rdaregistry.info/Elements/u/P61028> ;
    reg:lexicalAlias <http://rdaregistry.info/Elements/n/relatedPlaceOfNomen.en> ;
    reg:name "relatedPlaceOfNomen"@en ;
    reg:status <http://metadataregistry.org/uri/RegStatus/1001> ;
    rdfs:domain <http://rdaregistry.info/Elements/c/C10012> ;
    rdfs:isDefinedBy <http://rdaregistry.info/Elements/n/> ;
    rdfs:subPropertyOf <http://rdaregistry.info/Elements/n/P80010>,
        <http://rdaregistry.info/Elements/x/P00010> ;
    skos:definition "Relates a nomen to a place associated with a nomen."@en .

<http://rdaregistry.info/Elements/n/P80035> a rdf:Property ;
    rdfs:label "is identifier for corporate body of"@en ;
    rdakit:hasElementType "2" ;
    rdakit:toolkitDefinition "A corporate body who has an appellation of corporate body that is a reference code taken from a vocabulary encoding scheme."@en ;
    rdakit:toolkitLabel "identifier for corporate body of"@en ;
    reg:hasSubproperty <http://rdaregistry.info/Elements/n/datatype/P80035>,
        <http://rdaregistry.info/Elements/n/object/P80035> ;
    reg:hasUnconstrained <http://rdaregistry.info/Elements/u/P60937> ;
    reg:lexicalAlias <http://rdaregistry.info/Elements/n/identifierForCorporateBodyOf.en> ;
    reg:name "identifierForCorporateBodyOf"@en ;
    reg:status <http://metadataregistry.org/uri/RegStatus/1001> ;
    rdfs:domain <http://rdaregistry.info/Elements/c/C10012> ;
    rdfs:isDefinedBy <http://rdaregistry.info/Elements/n/> ;
    rdfs:subPropertyOf <http://rdaregistry.info/Elements/n/P80030>,
        <http://rdaregistry.info/Elements/n/P80034> ;
    skos:definition "Relates a nomen to a corporate body who has an appellation of corporate body that is a reference code taken from a vocabulary encoding scheme."@en .

<http://rdaregistry.info/Elements/n/P80036> a rdf:Property ;
    rdfs:label "is identifier for family of"@en ;
    rdakit:hasElementType "2" ;
    rdakit:toolkitDefinition "A family who has an appellation of family that is a reference code taken from a vocabulary encoding scheme."@en ;
    rdakit:toolkitLabel "identifier for family of"@en ;
    reg:hasSubproperty <http://rdaregistry.info/Elements/n/datatype/P80036>,
        <http://rdaregistry.info/Elements/n/object/P80036> ;
    reg:hasUnconstrained <http://rdaregistry.info/Elements/u/P60937> ;
    reg:lexicalAlias <http://rdaregistry.info/Elements/n/identifierForFamilyOf.en> ;
    reg:name "identifierForFamilyOf"@en ;
    reg:status <http://metadataregistry.org/uri/RegStatus/1001> ;
    rdfs:domain <http://rdaregistry.info/Elements/c/C10012> ;
    rdfs:isDefinedBy <http://rdaregistry.info/Elements/n/> ;
    rdfs:subPropertyOf <http://rdaregistry.info/Elements/n/P80031>,
        <http://rdaregistry.info/Elements/n/P80034> ;
    skos:definition "Relates a nomen to a family who has an appellation of family that is a reference code taken from a vocabulary encoding scheme."@en .

<http://rdaregistry.info/Elements/n/P80037> a rdf:Property ;
    rdfs:label "is identifier for person of"@en ;
    rdakit:hasElementType "2" ;
    rdakit:toolkitDefinition "A person who has an appellation of person that is a reference code taken from a vocabulary encoding scheme."@en ;
    rdakit:toolkitLabel "identifier for person of"@en ;
    reg:hasSubproperty <http://rdaregistry.info/Elements/n/datatype/P80037>,
        <http://rdaregistry.info/Elements/n/object/P80037> ;
    reg:hasUnconstrained <http://rdaregistry.info/Elements/u/P60937> ;
    reg:lexicalAlias <http://rdaregistry.info/Elements/n/identifierForPersonOf.en> ;
    reg:name "identifierForPersonOf"@en ;
    reg:status <http://metadataregistry.org/uri/RegStatus/1001> ;
    rdfs:domain <http://rdaregistry.info/Elements/c/C10012> ;
    rdfs:isDefinedBy <http://rdaregistry.info/Elements/n/> ;
    rdfs:subPropertyOf <http://rdaregistry.info/Elements/n/P80032>,
        <http://rdaregistry.info/Elements/n/P80033> ;
    skos:definition "Relates a nomen to a person who has an appellation of person that is a reference code taken from a vocabulary encoding scheme."@en .

<http://rdaregistry.info/Elements/n/P80063> a rdf:Property ;
    rdfs:label "is title proper of"@en ;
    rdakit:hasElementType "2" ;
    rdakit:toolkitDefinition "A manifestation that has a title of manifestation that is selected for preference in a specific application or context."@en ;
    rdakit:toolkitLabel "title proper of"@en ;
    reg:hasSubproperty <http://rdaregistry.info/Elements/n/P80123>,
        <http://rdaregistry.info/Elements/n/P80124>,
        <http://rdaregistry.info/Elements/n/P80125>,
        <http://rdaregistry.info/Elements/n/P80135>,
        <http://rdaregistry.info/Elements/n/datatype/P80063>,
        <http://rdaregistry.info/Elements/n/object/P80063> ;
    reg:hasUnconstrained <http://rdaregistry.info/Elements/u/P60957> ;
    reg:lexicalAlias <http://rdaregistry.info/Elements/n/titleProperOf.en> ;
    reg:name "titleProperOf"@en ;
    reg:status <http://metadataregistry.org/uri/RegStatus/1001> ;
    rdfs:domain <http://rdaregistry.info/Elements/c/C10012> ;
    rdfs:isDefinedBy <http://rdaregistry.info/Elements/n/> ;
    rdfs:subPropertyOf <http://rdaregistry.info/Elements/n/P80062> ;
    skos:definition "Relates a nomen to a manifestation that has a title of manifestation that is selected for preference in a specific application or context."@en .

<http://rdaregistry.info/Elements/n/P80075> a rdf:Property ;
    rdfs:label "is assigned by corporate body"@en ;
    rdakit:hasElementType "2" ;
    rdakit:toolkitDefinition "A corporate body who assigns a nomen to an entity."@en ;
    rdakit:toolkitLabel "assigned by corporate body"@en ;
    reg:hasSubproperty <http://rdaregistry.info/Elements/n/datatype/P80075>,
        <http://rdaregistry.info/Elements/n/object/P80075> ;
    reg:hasUnconstrained <http://rdaregistry.info/Elements/u/P60943> ;
    reg:lexicalAlias <http://rdaregistry.info/Elements/n/assignedByCorporateBody.en> ;
    reg:name "assignedByCorporateBody"@en ;
    reg:status <http://metadataregistry.org/uri/RegStatus/1001> ;
    rdfs:domain <http://rdaregistry.info/Elements/c/C10012> ;
    rdfs:isDefinedBy <http://rdaregistry.info/Elements/n/> ;
    rdfs:subPropertyOf <http://rdaregistry.info/Elements/n/P80013>,
        <http://rdaregistry.info/Elements/n/P80074> ;
    skos:definition "Relates a nomen to a corporate body who assigns a nomen to an entity."@en .

<http://rdaregistry.info/Elements/n/P80076> a rdf:Property ;
    rdfs:label "is assigned by family"@en ;
    rdakit:hasElementType "2" ;
    rdakit:toolkitDefinition "A family who assigns a nomen to an entity."@en ;
    rdakit:toolkitLabel "assigned by family"@en ;
    reg:hasSubproperty <http://rdaregistry.info/Elements/n/datatype/P80076>,
        <http://rdaregistry.info/Elements/n/object/P80076> ;
    reg:hasUnconstrained <http://rdaregistry.info/Elements/u/P60943> ;
    reg:lexicalAlias <http://rdaregistry.info/Elements/n/assignedByFamily.en> ;
    reg:name "assignedByFamily"@en ;
    reg:status <http://metadataregistry.org/uri/RegStatus/1001> ;
    rdfs:domain <http://rdaregistry.info/Elements/c/C10012> ;
    rdfs:isDefinedBy <http://rdaregistry.info/Elements/n/> ;
    rdfs:subPropertyOf <http://rdaregistry.info/Elements/n/P80012>,
        <http://rdaregistry.info/Elements/n/P80074> ;
    skos:definition "Relates a nomen to a family who assigns a nomen to an entity."@en .

<http://rdaregistry.info/Elements/n/P80077> a rdf:Property ;
    rdfs:label "is assigned by person"@en ;
    rdakit:hasElementType "2" ;
    rdakit:toolkitDefinition "A person who assigns a nomen to an entity."@en ;
    rdakit:toolkitLabel "assigned by person"@en ;
    reg:hasSubproperty <http://rdaregistry.info/Elements/n/datatype/P80077>,
        <http://rdaregistry.info/Elements/n/object/P80077> ;
    reg:hasUnconstrained <http://rdaregistry.info/Elements/u/P60943> ;
    reg:lexicalAlias <http://rdaregistry.info/Elements/n/assignedByPerson.en> ;
    reg:name "assignedByPerson"@en ;
    reg:status <http://metadataregistry.org/uri/RegStatus/1001> ;
    rdfs:domain <http://rdaregistry.info/Elements/c/C10012> ;
    rdfs:isDefinedBy <http://rdaregistry.info/Elements/n/> ;
    rdfs:subPropertyOf <http://rdaregistry.info/Elements/n/P80011>,
        <http://rdaregistry.info/Elements/n/P80073> ;
    skos:definition "Relates a nomen to a person who assigns a nomen to an entity."@en .

<http://rdaregistry.info/Elements/n/P80079> a rdf:Property ;
    rdfs:label "is authorized access point for work of"@en ;
    rdakit:hasElementType "2" ;
    rdakit:toolkitDefinition "A work that has an access point for work that is selected for preference in a specific vocabulary encoding scheme."@en ;
    rdakit:toolkitLabel "authorized access point for work of"@en ;
    reg:hasSubproperty <http://rdaregistry.info/Elements/n/P80173>,
        <http://rdaregistry.info/Elements/n/datatype/P80079>,
        <http://rdaregistry.info/Elements/n/object/P80079> ;
    reg:hasUnconstrained <http://rdaregistry.info/Elements/u/P60918> ;
    reg:lexicalAlias <http://rdaregistry.info/Elements/n/authorizedAccessPointForWorkOf.en> ;
    reg:name "authorizedAccessPointForWorkOf"@en ;
    reg:status <http://metadataregistry.org/uri/RegStatus/1001> ;
    rdfs:domain <http://rdaregistry.info/Elements/c/C10012> ;
    rdfs:isDefinedBy <http://rdaregistry.info/Elements/n/> ;
    rdfs:subPropertyOf <http://rdaregistry.info/Elements/n/P80027>,
        <http://rdaregistry.info/Elements/n/P80162> ;
    skos:definition "Relates a nomen to a work that has an access point for work that is selected for preference in a specific vocabulary encoding scheme."@en .

<http://rdaregistry.info/Elements/n/P80080> a rdf:Property ;
    rdfs:label "is variant access point for work of"@en ;
    rdakit:hasElementType "2" ;
    rdakit:toolkitDefinition "A work that has an access point for work that is not selected for preference in a specific vocabulary encoding scheme."@en ;
    rdakit:toolkitLabel "variant access point for work of"@en ;
    reg:hasSubproperty <http://rdaregistry.info/Elements/n/datatype/P80080>,
        <http://rdaregistry.info/Elements/n/object/P80080> ;
    reg:hasUnconstrained <http://rdaregistry.info/Elements/u/P60934> ;
    reg:lexicalAlias <http://rdaregistry.info/Elements/n/variantAccessPointForWorkOf.en> ;
    reg:name "variantAccessPointForWorkOf"@en ;
    reg:status <http://metadataregistry.org/uri/RegStatus/1001> ;
    rdfs:domain <http://rdaregistry.info/Elements/c/C10012> ;
    rdfs:isDefinedBy <http://rdaregistry.info/Elements/n/> ;
    rdfs:subPropertyOf <http://rdaregistry.info/Elements/n/P80027>,
        <http://rdaregistry.info/Elements/n/P80165> ;
    skos:definition "Relates a nomen to a work that has an access point for work that is not selected for preference in a specific vocabulary encoding scheme."@en .

<http://rdaregistry.info/Elements/n/P80082> a rdf:Property ;
    rdfs:label "is variant access point for timespan of"@en ;
    rdakit:hasElementType "2" ;
    rdakit:toolkitDefinition "A timespan that has an access point for timespan that is not selected for preference in a specific vocabulary encoding scheme."@en ;
    rdakit:toolkitLabel "variant access point for timespan of"@en ;
    reg:hasSubproperty <http://rdaregistry.info/Elements/n/datatype/P80082>,
        <http://rdaregistry.info/Elements/n/object/P80082> ;
    reg:hasUnconstrained <http://rdaregistry.info/Elements/u/P60934> ;
    reg:lexicalAlias <http://rdaregistry.info/Elements/n/variantAccessPointForTimespanOf.en> ;
    reg:name "variantAccessPointForTimespanOf"@en ;
    reg:status <http://metadataregistry.org/uri/RegStatus/1001> ;
    rdfs:domain <http://rdaregistry.info/Elements/c/C10012> ;
    rdfs:isDefinedBy <http://rdaregistry.info/Elements/n/> ;
    rdfs:subPropertyOf <http://rdaregistry.info/Elements/n/P80026>,
        <http://rdaregistry.info/Elements/n/P80165> ;
    skos:definition "Relates a nomen to a timespan that has an access point for timespan that is not selected for preference in a specific vocabulary encoding scheme."@en .

<http://rdaregistry.info/Elements/n/P80083> a rdf:Property ;
    rdfs:label "is preferred name of timespan of"@en ;
    rdakit:hasElementType "2" ;
    rdakit:toolkitDefinition "A timespan that has a name of timespan that is selected for preference in a specific application or context."@en ;
    rdakit:toolkitLabel "preferred name of timespan of"@en ;
    reg:hasSubproperty <http://rdaregistry.info/Elements/n/datatype/P80083>,
        <http://rdaregistry.info/Elements/n/object/P80083> ;
    reg:hasUnconstrained <http://rdaregistry.info/Elements/u/P60924> ;
    reg:lexicalAlias <http://rdaregistry.info/Elements/n/preferredNameOfTimespanOf.en> ;
    reg:name "preferredNameOfTimespanOf"@en ;
    reg:status <http://metadataregistry.org/uri/RegStatus/1001> ;
    rdfs:domain <http://rdaregistry.info/Elements/c/C10012> ;
    rdfs:isDefinedBy <http://rdaregistry.info/Elements/n/> ;
    rdfs:subPropertyOf <http://rdaregistry.info/Elements/n/P80044>,
        <http://rdaregistry.info/Elements/n/P80163> ;
    skos:definition "Relates a nomen to a timespan that has a name of timespan that is selected for preference in a specific application or context."@en .

<http://rdaregistry.info/Elements/n/P80086> a rdf:Property ;
    rdfs:label "is variant access point for place of"@en ;
    rdakit:hasElementType "2" ;
    rdakit:toolkitDefinition "A place that has an access point for place that is not selected for preference in a specific vocabulary encoding scheme."@en ;
    rdakit:toolkitLabel "variant access point for place of"@en ;
    reg:hasSubproperty <http://rdaregistry.info/Elements/n/datatype/P80086>,
        <http://rdaregistry.info/Elements/n/object/P80086> ;
    reg:hasUnconstrained <http://rdaregistry.info/Elements/u/P60934> ;
    reg:lexicalAlias <http://rdaregistry.info/Elements/n/variantAccessPointForPlaceOf.en> ;
    reg:name "variantAccessPointForPlaceOf"@en ;
    reg:status <http://metadataregistry.org/uri/RegStatus/1001> ;
    rdfs:domain <http://rdaregistry.info/Elements/c/C10012> ;
    rdfs:isDefinedBy <http://rdaregistry.info/Elements/n/> ;
    rdfs:subPropertyOf <http://rdaregistry.info/Elements/n/P80025>,
        <http://rdaregistry.info/Elements/n/P80165> ;
    skos:definition "Relates a nomen to a place that has an access point for place that is not selected for preference in a specific vocabulary encoding scheme."@en .

<http://rdaregistry.info/Elements/n/P80087> a rdf:Property ;
    rdfs:label "is preferred name of place of"@en ;
    rdakit:hasElementType "2" ;
    rdakit:toolkitDefinition "A place that has a name of place that is selected for preference in a specific application or context."@en ;
    rdakit:toolkitLabel "preferred name of place of"@en ;
    reg:hasSubproperty <http://rdaregistry.info/Elements/n/datatype/P80087>,
        <http://rdaregistry.info/Elements/n/object/P80087> ;
    reg:hasUnconstrained <http://rdaregistry.info/Elements/u/P60923> ;
    reg:lexicalAlias <http://rdaregistry.info/Elements/n/preferredNameOfPlaceOf.en> ;
    reg:name "preferredNameOfPlaceOf"@en ;
    reg:status <http://metadataregistry.org/uri/RegStatus/1001> ;
    rdfs:domain <http://rdaregistry.info/Elements/c/C10012> ;
    rdfs:isDefinedBy <http://rdaregistry.info/Elements/n/> ;
    rdfs:subPropertyOf <http://rdaregistry.info/Elements/n/P80051>,
        <http://rdaregistry.info/Elements/n/P80163> ;
    skos:definition "Relates a nomen to a place that has a name of place that is selected for preference in a specific application or context."@en .

<http://rdaregistry.info/Elements/n/P80090> a rdf:Property ;
    rdfs:label "is variant access point for manifestation of"@en ;
    rdakit:hasElementType "2" ;
    rdakit:toolkitDefinition "A manifestation that has an access point for manifestation that is not selected for preference in a specific vocabulary encoding scheme."@en ;
    rdakit:toolkitLabel "variant access point for manifestation of"@en ;
    reg:hasSubproperty <http://rdaregistry.info/Elements/n/datatype/P80090>,
        <http://rdaregistry.info/Elements/n/object/P80090> ;
    reg:hasUnconstrained <http://rdaregistry.info/Elements/u/P60934> ;
    reg:lexicalAlias <http://rdaregistry.info/Elements/n/variantAccessPointForManifestationOf.en> ;
    reg:name "variantAccessPointForManifestationOf"@en ;
    reg:status <http://metadataregistry.org/uri/RegStatus/1001> ;
    rdfs:domain <http://rdaregistry.info/Elements/c/C10012> ;
    rdfs:isDefinedBy <http://rdaregistry.info/Elements/n/> ;
    rdfs:subPropertyOf <http://rdaregistry.info/Elements/n/P80024>,
        <http://rdaregistry.info/Elements/n/P80165> ;
    skos:definition "Relates a nomen to a manifestation that has an access point for manifestation that is not selected for preference in a specific vocabulary encoding scheme."@en .

<http://rdaregistry.info/Elements/n/P80092> a rdf:Property ;
    rdfs:label "is variant access point for item of"@en ;
    rdakit:hasElementType "2" ;
    rdakit:toolkitDefinition "An item that has an access point for item that is not selected for preference in a specific vocabulary encoding scheme."@en ;
    rdakit:toolkitLabel "variant access point for item of"@en ;
    reg:hasSubproperty <http://rdaregistry.info/Elements/n/datatype/P80092>,
        <http://rdaregistry.info/Elements/n/object/P80092> ;
    reg:hasUnconstrained <http://rdaregistry.info/Elements/u/P60934> ;
    reg:lexicalAlias <http://rdaregistry.info/Elements/n/variantAccessPointForItemOf.en> ;
    reg:name "variantAccessPointForItemOf"@en ;
    reg:status <http://metadataregistry.org/uri/RegStatus/1001> ;
    rdfs:domain <http://rdaregistry.info/Elements/c/C10012> ;
    rdfs:isDefinedBy <http://rdaregistry.info/Elements/n/> ;
    rdfs:subPropertyOf <http://rdaregistry.info/Elements/n/P80015>,
        <http://rdaregistry.info/Elements/n/P80165> ;
    skos:definition "Relates a nomen to an item that has an access point for item that is not selected for preference in a specific vocabulary encoding scheme."@en .

<http://rdaregistry.info/Elements/n/P80093> a rdf:Property ;
    rdfs:label "is preferred title of item of"@en ;
    rdakit:hasElementType "2" ;
    rdakit:toolkitDefinition "An item that has a title of item that is selected for preference in a specific application or context."@en ;
    rdakit:toolkitLabel "preferred title of item of"@en ;
    reg:hasSubproperty <http://rdaregistry.info/Elements/n/datatype/P80093>,
        <http://rdaregistry.info/Elements/n/object/P80093> ;
    reg:hasUnconstrained <http://rdaregistry.info/Elements/u/P60933> ;
    reg:lexicalAlias <http://rdaregistry.info/Elements/n/preferredTitleOfItemOf.en> ;
    reg:name "preferredTitleOfItemOf"@en ;
    reg:status <http://metadataregistry.org/uri/RegStatus/1001> ;
    rdfs:domain <http://rdaregistry.info/Elements/c/C10012> ;
    rdfs:isDefinedBy <http://rdaregistry.info/Elements/n/> ;
    rdfs:subPropertyOf <http://rdaregistry.info/Elements/n/P80017>,
        <http://rdaregistry.info/Elements/n/P80163> ;
    skos:definition "Relates a nomen to an item that has a title of item that is selected for preference in a specific application or context."@en .

<http://rdaregistry.info/Elements/n/P80096> a rdf:Property ;
    rdfs:label "is variant access point for expression of"@en ;
    rdakit:hasElementType "2" ;
    rdakit:toolkitDefinition "An expression that has an access point for expression that is not selected for preference in a specific vocabulary encoding scheme."@en ;
    rdakit:toolkitLabel "variant access point for expression of"@en ;
    reg:hasSubproperty <http://rdaregistry.info/Elements/n/datatype/P80096>,
        <http://rdaregistry.info/Elements/n/object/P80096> ;
    reg:hasUnconstrained <http://rdaregistry.info/Elements/u/P60934> ;
    reg:lexicalAlias <http://rdaregistry.info/Elements/n/variantAccessPointForExpressionOf.en> ;
    reg:name "variantAccessPointForExpressionOf"@en ;
    reg:status <http://metadataregistry.org/uri/RegStatus/1001> ;
    rdfs:domain <http://rdaregistry.info/Elements/c/C10012> ;
    rdfs:isDefinedBy <http://rdaregistry.info/Elements/n/> ;
    rdfs:subPropertyOf <http://rdaregistry.info/Elements/n/P80023>,
        <http://rdaregistry.info/Elements/n/P80165> ;
    skos:definition "Relates a nomen to an expression that has an access point for expression that is not selected for preference in a specific vocabulary encoding scheme."@en .

<http://rdaregistry.info/Elements/n/P80097> a rdf:Property ;
    rdfs:label "is preferred title of expression of"@en ;
    rdakit:hasElementType "2" ;
    rdakit:toolkitDefinition "An expression that has a title of expression that is selected for preference in a specific application or context."@en ;
    rdakit:toolkitLabel "preferred title of expression of"@en ;
    reg:hasSubproperty <http://rdaregistry.info/Elements/n/datatype/P80097>,
        <http://rdaregistry.info/Elements/n/object/P80097> ;
    reg:hasUnconstrained <http://rdaregistry.info/Elements/u/P60933> ;
    reg:lexicalAlias <http://rdaregistry.info/Elements/n/preferredTitleOfExpressionOf.en> ;
    reg:name "preferredTitleOfExpressionOf"@en ;
    reg:status <http://metadataregistry.org/uri/RegStatus/1001> ;
    rdfs:domain <http://rdaregistry.info/Elements/c/C10012> ;
    rdfs:isDefinedBy <http://rdaregistry.info/Elements/n/> ;
    rdfs:subPropertyOf <http://rdaregistry.info/Elements/n/P80039>,
        <http://rdaregistry.info/Elements/n/P80163> ;
    skos:definition "Relates a nomen to an expression that has a title of expression that is selected for preference in a specific application or context."@en .

<http://rdaregistry.info/Elements/n/P80103> a rdf:Property ;
    rdfs:label "is authorized access point for corporate body of"@en ;
    rdakit:hasElementType "2" ;
    rdakit:toolkitDefinition "A corporate body who has an access point for corporate body that is selected for preference in a specific vocabulary encoding scheme."@en ;
    rdakit:toolkitLabel "authorized access point for corporate body of"@en ;
    reg:hasSubproperty <http://rdaregistry.info/Elements/n/datatype/P80103>,
        <http://rdaregistry.info/Elements/n/object/P80103> ;
    reg:hasUnconstrained <http://rdaregistry.info/Elements/u/P60918> ;
    reg:lexicalAlias <http://rdaregistry.info/Elements/n/authorizedAccessPointForCorporateBodyOf.en> ;
    reg:name "authorizedAccessPointForCorporateBodyOf"@en ;
    reg:status <http://metadataregistry.org/uri/RegStatus/1001> ;
    rdfs:domain <http://rdaregistry.info/Elements/c/C10012> ;
    rdfs:isDefinedBy <http://rdaregistry.info/Elements/n/> ;
    rdfs:subPropertyOf <http://rdaregistry.info/Elements/n/P80020>,
        <http://rdaregistry.info/Elements/n/P80101> ;
    skos:definition "Relates a nomen to a corporate body who has an access point for corporate body that is selected for preference in a specific vocabulary encoding scheme."@en .

<http://rdaregistry.info/Elements/n/P80104> a rdf:Property ;
    rdfs:label "is variant access point for corporate body of"@en ;
    rdakit:hasElementType "2" ;
    rdakit:toolkitDefinition "A corporate body who has an access point for corporate body that is not selected for preference in a specific vocabulary encoding scheme."@en ;
    rdakit:toolkitLabel "variant access point for corporate body of"@en ;
    reg:hasSubproperty <http://rdaregistry.info/Elements/n/datatype/P80104>,
        <http://rdaregistry.info/Elements/n/object/P80104> ;
    reg:hasUnconstrained <http://rdaregistry.info/Elements/u/P60934> ;
    reg:lexicalAlias <http://rdaregistry.info/Elements/n/variantAccessPointForCorporateBodyOf.en> ;
    reg:name "variantAccessPointForCorporateBodyOf"@en ;
    reg:status <http://metadataregistry.org/uri/RegStatus/1001> ;
    rdfs:domain <http://rdaregistry.info/Elements/c/C10012> ;
    rdfs:isDefinedBy <http://rdaregistry.info/Elements/n/> ;
    rdfs:subPropertyOf <http://rdaregistry.info/Elements/n/P80020>,
        <http://rdaregistry.info/Elements/n/P80102> ;
    skos:definition "Relates a nomen to a corporate body who has an access point for corporate body that is not selected for preference in a specific vocabulary encoding scheme."@en .

<http://rdaregistry.info/Elements/n/P80105> a rdf:Property ;
    rdfs:label "is authorized access point for family of"@en ;
    rdakit:hasElementType "2" ;
    rdakit:toolkitDefinition "A family who has an access point for family that is selected for preference in a specific vocabulary encoding scheme."@en ;
    rdakit:toolkitLabel "authorized access point for family of"@en ;
    reg:hasSubproperty <http://rdaregistry.info/Elements/n/datatype/P80105>,
        <http://rdaregistry.info/Elements/n/object/P80105> ;
    reg:hasUnconstrained <http://rdaregistry.info/Elements/u/P60918> ;
    reg:lexicalAlias <http://rdaregistry.info/Elements/n/authorizedAccessPointForFamilyOf.en> ;
    reg:name "authorizedAccessPointForFamilyOf"@en ;
    reg:status <http://metadataregistry.org/uri/RegStatus/1001> ;
    rdfs:domain <http://rdaregistry.info/Elements/c/C10012> ;
    rdfs:isDefinedBy <http://rdaregistry.info/Elements/n/> ;
    rdfs:subPropertyOf <http://rdaregistry.info/Elements/n/P80021>,
        <http://rdaregistry.info/Elements/n/P80101> ;
    skos:definition "Relates a nomen to a family who has an access point for family that is selected for preference in a specific vocabulary encoding scheme."@en .

<http://rdaregistry.info/Elements/n/P80106> a rdf:Property ;
    rdfs:label "is variant access point for family of"@en ;
    rdakit:hasElementType "2" ;
    rdakit:toolkitDefinition "A family who has an access point for family that is not selected for preference in a specific vocabulary encoding scheme."@en ;
    rdakit:toolkitLabel "variant access point for family of"@en ;
    reg:hasSubproperty <http://rdaregistry.info/Elements/n/datatype/P80106>,
        <http://rdaregistry.info/Elements/n/object/P80106> ;
    reg:hasUnconstrained <http://rdaregistry.info/Elements/u/P60934> ;
    reg:lexicalAlias <http://rdaregistry.info/Elements/n/variantAccessPointForFamilyOf.en> ;
    reg:name "variantAccessPointForFamilyOf"@en ;
    reg:status <http://metadataregistry.org/uri/RegStatus/1001> ;
    rdfs:domain <http://rdaregistry.info/Elements/c/C10012> ;
    rdfs:isDefinedBy <http://rdaregistry.info/Elements/n/> ;
    rdfs:subPropertyOf <http://rdaregistry.info/Elements/n/P80021>,
        <http://rdaregistry.info/Elements/n/P80102> ;
    skos:definition "Relates a nomen to a family who has an access point for family that is not selected for preference in a specific vocabulary encoding scheme."@en .

<http://rdaregistry.info/Elements/n/P80107> a rdf:Property ;
    rdfs:label "is authorized access point for person of"@en ;
    rdakit:hasElementType "2" ;
    rdakit:toolkitDefinition "A person who has an access point for person that is selected for preference in a specific vocabulary encoding scheme."@en ;
    rdakit:toolkitLabel "authorized access point for person of"@en ;
    reg:hasSubproperty <http://rdaregistry.info/Elements/n/datatype/P80107>,
        <http://rdaregistry.info/Elements/n/object/P80107> ;
    reg:hasUnconstrained <http://rdaregistry.info/Elements/u/P60918> ;
    reg:lexicalAlias <http://rdaregistry.info/Elements/n/authorizedAccessPointForPersonOf.en> ;
    reg:name "authorizedAccessPointForPersonOf"@en ;
    reg:status <http://metadataregistry.org/uri/RegStatus/1001> ;
    rdfs:domain <http://rdaregistry.info/Elements/c/C10012> ;
    rdfs:isDefinedBy <http://rdaregistry.info/Elements/n/> ;
    rdfs:subPropertyOf <http://rdaregistry.info/Elements/n/P80022>,
        <http://rdaregistry.info/Elements/n/P80099> ;
    skos:definition "Relates a nomen to a person who has an access point for person that is selected for preference in a specific vocabulary encoding scheme."@en .

<http://rdaregistry.info/Elements/n/P80108> a rdf:Property ;
    rdfs:label "is variant access point for person of"@en ;
    rdakit:hasElementType "2" ;
    rdakit:toolkitDefinition "A person who has an access point for person that is not selected for preference in a specific vocabulary encoding scheme."@en ;
    rdakit:toolkitLabel "variant access point for person of"@en ;
    reg:hasSubproperty <http://rdaregistry.info/Elements/n/datatype/P80108>,
        <http://rdaregistry.info/Elements/n/object/P80108> ;
    reg:hasUnconstrained <http://rdaregistry.info/Elements/u/P60934> ;
    reg:lexicalAlias <http://rdaregistry.info/Elements/n/variantAccessPointForPersonOf.en> ;
    reg:name "variantAccessPointForPersonOf"@en ;
    reg:status <http://metadataregistry.org/uri/RegStatus/1001> ;
    rdfs:domain <http://rdaregistry.info/Elements/c/C10012> ;
    rdfs:isDefinedBy <http://rdaregistry.info/Elements/n/> ;
    rdfs:subPropertyOf <http://rdaregistry.info/Elements/n/P80022>,
        <http://rdaregistry.info/Elements/n/P80100> ;
    skos:definition "Relates a nomen to a person who has an access point for person that is not selected for preference in a specific vocabulary encoding scheme."@en .

<http://rdaregistry.info/Elements/n/P80109> a rdf:Property ;
    rdfs:label "is preferred title of work of"@en ;
    rdakit:hasElementType "2" ;
    rdakit:toolkitDefinition "A work that has a title of work that is selected for preference in a specific application or context."@en ;
    rdakit:toolkitLabel "preferred title of work of"@en ;
    reg:hasSubproperty <http://rdaregistry.info/Elements/n/datatype/P80109>,
        <http://rdaregistry.info/Elements/n/object/P80109> ;
    reg:hasUnconstrained <http://rdaregistry.info/Elements/u/P60933> ;
    reg:lexicalAlias <http://rdaregistry.info/Elements/n/preferredTitleOfWorkOf.en> ;
    reg:name "preferredTitleOfWorkOf"@en ;
    reg:status <http://metadataregistry.org/uri/RegStatus/1001> ;
    rdfs:domain <http://rdaregistry.info/Elements/c/C10012> ;
    rdfs:isDefinedBy <http://rdaregistry.info/Elements/n/> ;
    rdfs:subPropertyOf <http://rdaregistry.info/Elements/n/P80064>,
        <http://rdaregistry.info/Elements/n/P80163> ;
    skos:definition "Relates a nomen to a work that has a title of work that is selected for preference in a specific application or context."@en .

<http://rdaregistry.info/Elements/n/P80111> a rdf:Property ;
    rdfs:label "is variant title of manifestation of"@en ;
    rdakit:hasElementType "2" ;
    rdakit:toolkitDefinition "A manifestation that has a title of manifestation that is not selected for preference in a specific application or context."@en ;
    rdakit:toolkitLabel "variant title of manifestation of"@en ;
    reg:hasSubproperty <http://rdaregistry.info/Elements/n/P80057>,
        <http://rdaregistry.info/Elements/n/datatype/P80111>,
        <http://rdaregistry.info/Elements/n/object/P80111> ;
    reg:hasUnconstrained <http://rdaregistry.info/Elements/u/P60925> ;
    reg:lexicalAlias <http://rdaregistry.info/Elements/n/variantTitleOfManifestationOf.en> ;
    reg:name "variantTitleOfManifestationOf"@en ;
    reg:status <http://metadataregistry.org/uri/RegStatus/1001> ;
    rdfs:domain <http://rdaregistry.info/Elements/c/C10012> ;
    rdfs:isDefinedBy <http://rdaregistry.info/Elements/n/> ;
    rdfs:subPropertyOf <http://rdaregistry.info/Elements/n/P80062>,
        <http://rdaregistry.info/Elements/n/P80164> ;
    skos:definition "Relates a nomen to a manifestation that has a title of manifestation that is not selected for preference in a specific application or context."@en .

<http://rdaregistry.info/Elements/n/P80115> a rdf:Property ;
    rdfs:label "is name of distributor of"@en ;
    rdakit:hasElementType "2" ;
    rdakit:toolkitDefinition "A manifestation that is published that has a name of agent who is responsible for distribution."@en ;
    rdakit:toolkitLabel "name of distributor of"@en ;
    reg:hasSubproperty <http://rdaregistry.info/Elements/n/P80127>,
        <http://rdaregistry.info/Elements/n/datatype/P80115> ;
    reg:hasUnconstrained <http://rdaregistry.info/Elements/u/P60946> ;
    reg:lexicalAlias <http://rdaregistry.info/Elements/n/nameOfDistributorOf.en> ;
    reg:name "nameOfDistributorOf"@en ;
    reg:status <http://metadataregistry.org/uri/RegStatus/1001> ;
    rdfs:domain <http://rdaregistry.info/Elements/c/C10012> ;
    rdfs:isDefinedBy <http://rdaregistry.info/Elements/n/> ;
    rdfs:subPropertyOf <http://rdaregistry.info/Elements/n/P80114> ;
    skos:definition "Relates a nomen to a manifestation that is published that has a name of agent who is responsible for distribution."@en .

<http://rdaregistry.info/Elements/n/P80116> a rdf:Property ;
    rdfs:label "is name of manufacturer of"@en ;
    rdakit:hasElementType "2" ;
    rdakit:toolkitDefinition "A manifestation that is published that has a name of agent who is responsible for printing, duplication, casting, etc."@en ;
    rdakit:toolkitLabel "name of manufacturer of"@en ;
    reg:hasSubproperty <http://rdaregistry.info/Elements/n/P80128>,
        <http://rdaregistry.info/Elements/n/datatype/P80116> ;
    reg:hasUnconstrained <http://rdaregistry.info/Elements/u/P60948> ;
    reg:lexicalAlias <http://rdaregistry.info/Elements/n/nameOfManufacturerOf.en> ;
    reg:name "nameOfManufacturerOf"@en ;
    reg:status <http://metadataregistry.org/uri/RegStatus/1001> ;
    rdfs:domain <http://rdaregistry.info/Elements/c/C10012> ;
    rdfs:isDefinedBy <http://rdaregistry.info/Elements/n/> ;
    rdfs:subPropertyOf <http://rdaregistry.info/Elements/n/P80114> ;
    skos:definition "Relates a nomen to a manifestation that is published that has a name of agent who is responsible for printing, duplication, casting, etc."@en .

<http://rdaregistry.info/Elements/n/P80117> a rdf:Property ;
    rdfs:label "is name of producer of"@en ;
    rdakit:hasElementType "2" ;
    rdakit:toolkitDefinition "A manifestation that is unpublished that has a name of agent who is responsible for inscription, fabrication, construction, etc."@en ;
    rdakit:toolkitLabel "name of producer of"@en ;
    reg:hasSubproperty <http://rdaregistry.info/Elements/n/P80129>,
        <http://rdaregistry.info/Elements/n/datatype/P80117> ;
    reg:hasUnconstrained <http://rdaregistry.info/Elements/u/P60949> ;
    reg:lexicalAlias <http://rdaregistry.info/Elements/n/nameOfProducerOf.en> ;
    reg:name "nameOfProducerOf"@en ;
    reg:status <http://metadataregistry.org/uri/RegStatus/1001> ;
    rdfs:domain <http://rdaregistry.info/Elements/c/C10012> ;
    rdfs:isDefinedBy <http://rdaregistry.info/Elements/n/> ;
    rdfs:subPropertyOf <http://rdaregistry.info/Elements/n/P80114> ;
    skos:definition "Relates a nomen to a manifestation that is unpublished that has a name of agent who is responsible for inscription, fabrication, construction, etc."@en .

<http://rdaregistry.info/Elements/n/P80118> a rdf:Property ;
    rdfs:label "is name of publisher of"@en ;
    rdakit:hasElementType "2" ;
    rdakit:toolkitDefinition "A manifestation that is published that has a name of agent who is responsible for its publication."@en ;
    rdakit:toolkitLabel "name of publisher of"@en ;
    reg:hasSubproperty <http://rdaregistry.info/Elements/n/P80130>,
        <http://rdaregistry.info/Elements/n/datatype/P80118> ;
    reg:hasUnconstrained <http://rdaregistry.info/Elements/u/P60950> ;
    reg:lexicalAlias <http://rdaregistry.info/Elements/n/nameOfPublisherOf.en> ;
    reg:name "nameOfPublisherOf"@en ;
    reg:status <http://metadataregistry.org/uri/RegStatus/1001> ;
    rdfs:domain <http://rdaregistry.info/Elements/c/C10012> ;
    rdfs:isDefinedBy <http://rdaregistry.info/Elements/n/> ;
    rdfs:subPropertyOf <http://rdaregistry.info/Elements/n/P80114> ;
    skos:definition "Relates a nomen to a manifestation that is published that has a name of agent who is responsible for its publication."@en ;
    skos:scopeNote "Publication includes release and issuance."@en .

<http://rdaregistry.info/Elements/n/P80126> a rdf:Property ;
    rdfs:label "is title proper of subseries of (Deprecated)"@en ;
    rdakit:hasElementType "2" ;
    rdakit:toolkitDefinition "A manifestation of an issue of a subseries that has a name of series appearing on it. (Deprecated)"@en ;
    rdakit:toolkitLabel "title proper of subseries of (Deprecated)"@en ;
    reg:hasSubproperty <http://rdaregistry.info/Elements/n/datatype/P80126> ;
    reg:hasUnconstrained <http://rdaregistry.info/Elements/u/P60959> ;
    reg:lexicalAlias <http://rdaregistry.info/Elements/n/titleProperOfSubseriesOf.en> ;
    reg:name "titleProperOfSubseriesOf"@en ;
    reg:status <http://metadataregistry.org/uri/RegStatus/1008> ;
    rdfs:domain <http://rdaregistry.info/Elements/c/C10012> ;
    rdfs:isDefinedBy <http://rdaregistry.info/Elements/n/> ;
    rdfs:subPropertyOf <http://rdaregistry.info/Elements/n/P80125> ;
    skos:definition "Relates a nomen to a manifestation of an issue of a subseries that has a name of series appearing on it. (Deprecated)"@en .

<http://rdaregistry.info/Elements/n/P80135> a rdf:Property ;
    rdfs:label "is parallel title proper of"@en ;
    rdakit:hasElementType "2" ;
    rdakit:toolkitDefinition "A manifestation that has a title proper in another language or script."@en ;
    rdakit:toolkitLabel "parallel title proper of"@en ;
    reg:hasSubproperty <http://rdaregistry.info/Elements/n/P80136>,
        <http://rdaregistry.info/Elements/n/datatype/P80135> ;
    reg:hasUnconstrained <http://rdaregistry.info/Elements/u/P61116> ;
    reg:lexicalAlias <http://rdaregistry.info/Elements/n/parallelTitleProperOf.en> ;
    reg:name "parallelTitleProperOf"@en ;
    reg:status <http://metadataregistry.org/uri/RegStatus/1001> ;
    rdfs:domain <http://rdaregistry.info/Elements/c/C10012> ;
    rdfs:isDefinedBy <http://rdaregistry.info/Elements/n/> ;
    rdfs:subPropertyOf <http://rdaregistry.info/Elements/n/P80063> ;
    skos:definition "Relates a nomen to a manifestation that has a title proper in another language or script."@en .

<http://rdaregistry.info/Elements/n/P80136> a rdf:Property ;
    rdfs:label "is parallel title of series of"@en ;
    rdakit:hasElementType "2" ;
    rdakit:toolkitDefinition "A manifestation that has a title of series in another language or script."@en ;
    rdakit:toolkitLabel "parallel title of series of"@en ;
    reg:hasSubproperty <http://rdaregistry.info/Elements/n/P80137>,
        <http://rdaregistry.info/Elements/n/datatype/P80136> ;
    reg:lexicalAlias <http://rdaregistry.info/Elements/n/parallelTitleOfSeriesOf.en> ;
    reg:name "parallelTitleOfSeriesOf"@en ;
    reg:status <http://metadataregistry.org/uri/RegStatus/1001> ;
    rdfs:domain <http://rdaregistry.info/Elements/c/C10012> ;
    rdfs:isDefinedBy <http://rdaregistry.info/Elements/n/> ;
    rdfs:subPropertyOf <http://rdaregistry.info/Elements/n/P80125>,
        <http://rdaregistry.info/Elements/n/P80135> ;
    skos:definition "Relates a nomen to a manifestation that has a title of series in another language or script."@en .

<http://rdaregistry.info/Elements/n/P80144> a rdf:Property ;
    rdfs:label "is preferred name of corporate body of"@en ;
    rdakit:hasElementType "2" ;
    rdakit:toolkitDefinition "A corporate body who has a name of corporate body that is selected for preference in a specific application or context."@en ;
    rdakit:toolkitLabel "preferred name of corporate body of"@en ;
    reg:hasSubproperty <http://rdaregistry.info/Elements/n/datatype/P80144> ;
    reg:hasUnconstrained <http://rdaregistry.info/Elements/u/P60927> ;
    reg:lexicalAlias <http://rdaregistry.info/Elements/n/preferredNameOfCorporateBodyOf.en> ;
    reg:name "preferredNameOfCorporateBodyOf"@en ;
    reg:status <http://metadataregistry.org/uri/RegStatus/1001> ;
    rdfs:domain <http://rdaregistry.info/Elements/c/C10012> ;
    rdfs:isDefinedBy <http://rdaregistry.info/Elements/n/> ;
    rdfs:subPropertyOf <http://rdaregistry.info/Elements/n/P80054>,
        <http://rdaregistry.info/Elements/n/P80141> ;
    skos:definition "Relates a nomen to a corporate body who has a name of corporate body that is selected for preference in a specific application or context."@en .

<http://rdaregistry.info/Elements/n/P80145> a rdf:Property ;
    rdfs:label "is preferred name of family of"@en ;
    rdakit:hasElementType "2" ;
    rdakit:toolkitDefinition "A family who has a name of family that is selected for preference in a specific application or context."@en ;
    rdakit:toolkitLabel "preferred name of family of"@en ;
    reg:hasSubproperty <http://rdaregistry.info/Elements/n/datatype/P80145> ;
    reg:hasUnconstrained <http://rdaregistry.info/Elements/u/P60927> ;
    reg:lexicalAlias <http://rdaregistry.info/Elements/n/preferredNameOfFamilyOf.en> ;
    reg:name "preferredNameOfFamilyOf"@en ;
    reg:status <http://metadataregistry.org/uri/RegStatus/1001> ;
    rdfs:domain <http://rdaregistry.info/Elements/c/C10012> ;
    rdfs:isDefinedBy <http://rdaregistry.info/Elements/n/> ;
    rdfs:subPropertyOf <http://rdaregistry.info/Elements/n/P80055>,
        <http://rdaregistry.info/Elements/n/P80141> ;
    skos:definition "Relates a nomen to a family who has a name of family that is selected for preference in a specific application or context."@en .

<http://rdaregistry.info/Elements/n/P80146> a rdf:Property ;
    rdfs:label "is preferred name of person of"@en ;
    rdakit:hasElementType "2" ;
    rdakit:toolkitDefinition "A person who has a name of person that is selected for preference in a specific application or context."@en ;
    rdakit:toolkitLabel "preferred name of person of"@en ;
    reg:hasSubproperty <http://rdaregistry.info/Elements/n/datatype/P80146> ;
    reg:hasUnconstrained <http://rdaregistry.info/Elements/u/P60927> ;
    reg:lexicalAlias <http://rdaregistry.info/Elements/n/preferredNameOfPersonOf.en> ;
    reg:name "preferredNameOfPersonOf"@en ;
    reg:status <http://metadataregistry.org/uri/RegStatus/1001> ;
    rdfs:domain <http://rdaregistry.info/Elements/c/C10012> ;
    rdfs:isDefinedBy <http://rdaregistry.info/Elements/n/> ;
    rdfs:subPropertyOf <http://rdaregistry.info/Elements/n/P80056>,
        <http://rdaregistry.info/Elements/n/P80140> ;
    skos:definition "Relates a nomen to a person who has a name of person that is selected for preference in a specific application or context."@en .

<http://rdaregistry.info/Elements/n/P80147> a rdf:Property ;
    rdfs:label "is variant name of corporate body of"@en ;
    rdakit:hasElementType "2" ;
    rdakit:toolkitDefinition "A corporate body who has a name of corporate body that is not selected for preference in a specific application or context."@en ;
    rdakit:toolkitLabel "variant name of corporate body of"@en ;
    reg:hasSubproperty <http://rdaregistry.info/Elements/n/datatype/P80147> ;
    reg:hasUnconstrained <http://rdaregistry.info/Elements/u/P60921> ;
    reg:lexicalAlias <http://rdaregistry.info/Elements/n/variantNameOfCorporateBodyOf.en> ;
    reg:name "variantNameOfCorporateBodyOf"@en ;
    reg:status <http://metadataregistry.org/uri/RegStatus/1001> ;
    rdfs:domain <http://rdaregistry.info/Elements/c/C10012> ;
    rdfs:isDefinedBy <http://rdaregistry.info/Elements/n/> ;
    rdfs:subPropertyOf <http://rdaregistry.info/Elements/n/P80054>,
        <http://rdaregistry.info/Elements/n/P80143> ;
    skos:definition "Relates a nomen to a corporate body who has a name of corporate body that is not selected for preference in a specific application or context."@en .

<http://rdaregistry.info/Elements/n/P80148> a rdf:Property ;
    rdfs:label "is variant name of family of"@en ;
    rdakit:hasElementType "2" ;
    rdakit:toolkitDefinition "A family who has a name of family that is not selected for preference in a specific application or context."@en ;
    rdakit:toolkitLabel "variant name of family of"@en ;
    reg:hasSubproperty <http://rdaregistry.info/Elements/n/datatype/P80148> ;
    reg:hasUnconstrained <http://rdaregistry.info/Elements/u/P60921> ;
    reg:lexicalAlias <http://rdaregistry.info/Elements/n/variantNameOfFamilyOf.en> ;
    reg:name "variantNameOfFamilyOf"@en ;
    reg:status <http://metadataregistry.org/uri/RegStatus/1001> ;
    rdfs:domain <http://rdaregistry.info/Elements/c/C10012> ;
    rdfs:isDefinedBy <http://rdaregistry.info/Elements/n/> ;
    rdfs:subPropertyOf <http://rdaregistry.info/Elements/n/P80055>,
        <http://rdaregistry.info/Elements/n/P80143> ;
    skos:definition "Relates a nomen to a family who has a name of family that is not selected for preference in a specific application or context."@en .

<http://rdaregistry.info/Elements/n/P80149> a rdf:Property ;
    rdfs:label "is variant name of person of"@en ;
    rdakit:hasElementType "2" ;
    rdakit:toolkitDefinition "A person who has a name of person that is not selected for preference in a specific application or context."@en ;
    rdakit:toolkitLabel "variant name of person of"@en ;
    reg:hasSubproperty <http://rdaregistry.info/Elements/n/datatype/P80149> ;
    reg:hasUnconstrained <http://rdaregistry.info/Elements/u/P60921> ;
    reg:lexicalAlias <http://rdaregistry.info/Elements/n/variantNameOfPersonOf.en> ;
    reg:name "variantNameOfPersonOf"@en ;
    reg:status <http://metadataregistry.org/uri/RegStatus/1001> ;
    rdfs:domain <http://rdaregistry.info/Elements/c/C10012> ;
    rdfs:isDefinedBy <http://rdaregistry.info/Elements/n/> ;
    rdfs:subPropertyOf <http://rdaregistry.info/Elements/n/P80056>,
        <http://rdaregistry.info/Elements/n/P80142> ;
    skos:definition "Relates a nomen to a person who has a name of person that is not selected for preference in a specific application or context."@en .

<http://rdaregistry.info/Elements/n/P80172> a rdf:Property ;
    rdfs:label "is identifier for work group of"@en ;
    rdakit:hasElementType "2" ;
    rdakit:toolkitDefinition "A work that has an appellation of work that is a reference code taken from a vocabulary encoding scheme used to identify a work group."@en ;
    rdakit:toolkitLabel "identifier for work group of"@en ;
    reg:hasSubproperty <http://rdaregistry.info/Elements/n/datatype/P80172>,
        <http://rdaregistry.info/Elements/n/object/P80172> ;
    reg:hasUnconstrained <http://rdaregistry.info/Elements/u/P60938> ;
    reg:lexicalAlias <http://rdaregistry.info/Elements/n/identifierForWorkGroupOf.en> ;
    reg:name "identifierForWorkGroupOf" ;
    reg:status <http://metadataregistry.org/uri/RegStatus/1001> ;
    rdfs:domain <http://rdaregistry.info/Elements/c/C10012> ;
    rdfs:isDefinedBy <http://rdaregistry.info/Elements/n/> ;
    rdfs:subPropertyOf <http://rdaregistry.info/Elements/n/P80049>,
        <http://rdaregistry.info/Elements/n/P80171> ;
    skos:definition "Relates a nomen to a work that has an appellation of work that is a reference code taken from a vocabulary encoding scheme used to identify a work group."@en .

<http://rdaregistry.info/Elements/n/P80173> a rdf:Property ;
    rdfs:label "is authorized access point for work group of"@en ;
    rdakit:hasElementType "2" ;
    rdakit:toolkitDefinition "A work that has an access point for work that is selected for preference in a specific vocabulary encoding scheme used to identify a work group."@en ;
    rdakit:toolkitLabel "authorized access point for work group of"@en ;
    reg:hasSubproperty <http://rdaregistry.info/Elements/n/datatype/P80173>,
        <http://rdaregistry.info/Elements/n/object/P80173> ;
    reg:hasUnconstrained <http://rdaregistry.info/Elements/u/P60918> ;
    reg:lexicalAlias <http://rdaregistry.info/Elements/n/authorizedAccessPointForWorkGroupOf.en> ;
    reg:name "authorizedAccessPointForWorkGroupOf" ;
    reg:status <http://metadataregistry.org/uri/RegStatus/1001> ;
    rdfs:domain <http://rdaregistry.info/Elements/c/C10012> ;
    rdfs:isDefinedBy <http://rdaregistry.info/Elements/n/> ;
    rdfs:subPropertyOf <http://rdaregistry.info/Elements/n/P80079>,
        <http://rdaregistry.info/Elements/n/P80171> ;
    skos:definition "Relates a nomen to a work that has an access point for work that is selected for preference in a specific vocabulary encoding scheme used to identify a work group."@en .

<http://rdaregistry.info/Elements/n/P80001> a rdf:Property ;
    rdfs:label "has related work of nomen"@en ;
    rdakit:hasElementType "1" ;
    rdakit:toolkitDefinition "A work that is associated with a nomen."@en ;
    rdakit:toolkitLabel "related work of nomen"@en ;
    reg:hasSubproperty <http://rdaregistry.info/Elements/n/P80045>,
        <http://rdaregistry.info/Elements/n/datatype/P80001>,
        <http://rdaregistry.info/Elements/n/object/P80001> ;
    reg:hasUnconstrained <http://rdaregistry.info/Elements/u/P61030> ;
    reg:lexicalAlias <http://rdaregistry.info/Elements/n/relatedWorkOfNomen.en> ;
    reg:name "relatedWorkOfNomen"@en ;
    reg:status <http://metadataregistry.org/uri/RegStatus/1001> ;
    rdfs:domain <http://rdaregistry.info/Elements/c/C10012> ;
    rdfs:isDefinedBy <http://rdaregistry.info/Elements/n/> ;
    rdfs:subPropertyOf <http://rdaregistry.info/Elements/n/P80010>,
        <http://rdaregistry.info/Elements/x/P00002> ;
    skos:definition "Relates a nomen to a work that is associated with a nomen."@en .

<http://rdaregistry.info/Elements/n/P80003> a rdf:Property ;
    rdfs:label "has related manifestation of nomen"@en ;
    rdakit:hasElementType "1" ;
    rdakit:toolkitDefinition "A manifestation that is associated with a nomen."@en ;
    rdakit:toolkitLabel "related manifestation of nomen"@en ;
    reg:hasSubproperty <http://rdaregistry.info/Elements/n/P80040>,
        <http://rdaregistry.info/Elements/n/P80114>,
        <http://rdaregistry.info/Elements/n/datatype/P80003>,
        <http://rdaregistry.info/Elements/n/object/P80003> ;
    reg:hasUnconstrained <http://rdaregistry.info/Elements/u/P61030> ;
    reg:lexicalAlias <http://rdaregistry.info/Elements/n/relatedManifestationOfNomen.en> ;
    reg:name "relatedManifestationOfNomen"@en ;
    reg:status <http://metadataregistry.org/uri/RegStatus/1001> ;
    rdfs:domain <http://rdaregistry.info/Elements/c/C10012> ;
    rdfs:isDefinedBy <http://rdaregistry.info/Elements/n/> ;
    rdfs:subPropertyOf <http://rdaregistry.info/Elements/n/P80010>,
        <http://rdaregistry.info/Elements/x/P00004> ;
    skos:definition "Relates a nomen to a manifestation that is associated with a nomen."@en .

<http://rdaregistry.info/Elements/n/P80008> a rdf:Property ;
    rdfs:label "has related timespan of nomen"@en ;
    rdakit:hasElementType "1" ;
    rdakit:toolkitDefinition "A timespan that is associated with a nomen."@en ;
    rdakit:toolkitLabel "related timespan of nomen"@en ;
    reg:hasSubproperty <http://rdaregistry.info/Elements/n/P80043>,
        <http://rdaregistry.info/Elements/n/P80166>,
        <http://rdaregistry.info/Elements/n/datatype/P80008>,
        <http://rdaregistry.info/Elements/n/object/P80008> ;
    reg:hasUnconstrained <http://rdaregistry.info/Elements/u/P61029> ;
    reg:lexicalAlias <http://rdaregistry.info/Elements/n/relatedTimespanOfNomen.en> ;
    reg:name "relatedTimespanOfNomen"@en ;
    reg:status <http://metadataregistry.org/uri/RegStatus/1001> ;
    rdfs:domain <http://rdaregistry.info/Elements/c/C10012> ;
    rdfs:isDefinedBy <http://rdaregistry.info/Elements/n/> ;
    rdfs:subPropertyOf <http://rdaregistry.info/Elements/n/P80010>,
        <http://rdaregistry.info/Elements/x/P00011> ;
    skos:definition "Relates a nomen to a timespan that is associated with a nomen."@en .

<http://rdaregistry.info/Elements/n/P80011> a rdf:Property ;
    rdfs:label "has related person of nomen"@en ;
    rdakit:hasElementType "1" ;
    rdakit:toolkitDefinition "A person who is associated with a nomen."@en ;
    rdakit:toolkitLabel "related person of nomen"@en ;
    reg:hasSubproperty <http://rdaregistry.info/Elements/n/P80032>,
        <http://rdaregistry.info/Elements/n/P80077>,
        <http://rdaregistry.info/Elements/n/P80151>,
        <http://rdaregistry.info/Elements/n/datatype/P80011>,
        <http://rdaregistry.info/Elements/n/object/P80011> ;
    reg:hasUnconstrained <http://rdaregistry.info/Elements/u/P61027> ;
    reg:lexicalAlias <http://rdaregistry.info/Elements/n/relatedPersonOfNomen.en> ;
    reg:name "relatedPersonOfNomen"@en ;
    reg:status <http://metadataregistry.org/uri/RegStatus/1001> ;
    rdfs:domain <http://rdaregistry.info/Elements/c/C10012> ;
    rdfs:isDefinedBy <http://rdaregistry.info/Elements/n/> ;
    rdfs:subPropertyOf <http://rdaregistry.info/Elements/n/P80005>,
        <http://rdaregistry.info/Elements/x/P00007> ;
    skos:definition "Relates a nomen to a person who is associated with a nomen."@en .

<http://rdaregistry.info/Elements/n/P80012> a rdf:Property ;
    rdfs:label "has related family of nomen"@en ;
    rdakit:hasElementType "1" ;
    rdakit:toolkitDefinition "A family who is associated with a nomen."@en ;
    rdakit:toolkitLabel "related family of nomen"@en ;
    reg:hasSubproperty <http://rdaregistry.info/Elements/n/P80031>,
        <http://rdaregistry.info/Elements/n/P80076>,
        <http://rdaregistry.info/Elements/n/P80152>,
        <http://rdaregistry.info/Elements/n/datatype/P80012>,
        <http://rdaregistry.info/Elements/n/object/P80012> ;
    reg:hasUnconstrained <http://rdaregistry.info/Elements/u/P61027> ;
    reg:lexicalAlias <http://rdaregistry.info/Elements/n/relatedFamilyOfNomen.en> ;
    reg:name "relatedFamilyOfNomen"@en ;
    reg:status <http://metadataregistry.org/uri/RegStatus/1001> ;
    rdfs:domain <http://rdaregistry.info/Elements/c/C10012> ;
    rdfs:isDefinedBy <http://rdaregistry.info/Elements/n/> ;
    rdfs:subPropertyOf <http://rdaregistry.info/Elements/n/P80006>,
        <http://rdaregistry.info/Elements/x/P00008> ;
    skos:definition "Relates a nomen to a family who is associated with a nomen."@en .

<http://rdaregistry.info/Elements/n/P80013> a rdf:Property ;
    rdfs:label "has related corporate body of nomen"@en ;
    rdakit:hasElementType "1" ;
    rdakit:toolkitDefinition "A corporate body who is associated with a nomen."@en ;
    rdakit:toolkitLabel "related corporate body of nomen"@en ;
    reg:hasSubproperty <http://rdaregistry.info/Elements/n/P80030>,
        <http://rdaregistry.info/Elements/n/P80075>,
        <http://rdaregistry.info/Elements/n/P80150>,
        <http://rdaregistry.info/Elements/n/datatype/P80013>,
        <http://rdaregistry.info/Elements/n/object/P80013> ;
    reg:hasUnconstrained <http://rdaregistry.info/Elements/u/P61027> ;
    reg:lexicalAlias <http://rdaregistry.info/Elements/n/relatedCorporateBodyOfNomen.en> ;
    reg:name "relatedCorporateBodyOfNomen"@en ;
    reg:status <http://metadataregistry.org/uri/RegStatus/1001> ;
    rdfs:domain <http://rdaregistry.info/Elements/c/C10012> ;
    rdfs:isDefinedBy <http://rdaregistry.info/Elements/n/> ;
    rdfs:subPropertyOf <http://rdaregistry.info/Elements/n/P80006>,
        <http://rdaregistry.info/Elements/x/P00009> ;
    skos:definition "Relates a nomen to a corporate body who is associated with a nomen."@en .

<http://rdaregistry.info/Elements/n/P80015> a rdf:Property ;
    rdfs:label "is access point for item of"@en ;
    rdakit:hasElementType "2" ;
    rdakit:toolkitDefinition "An item that has an appellation in natural language that is taken from a vocabulary encoding scheme or is constructed using a string encoding scheme."@en ;
    rdakit:toolkitLabel "access point for item of"@en ;
    reg:hasSubproperty <http://rdaregistry.info/Elements/n/P80092>,
        <http://rdaregistry.info/Elements/n/datatype/P80015>,
        <http://rdaregistry.info/Elements/n/object/P80015> ;
    reg:hasUnconstrained <http://rdaregistry.info/Elements/u/P60910> ;
    reg:lexicalAlias <http://rdaregistry.info/Elements/n/accessPointForItemOf.en> ;
    reg:name "accessPointForItemOf"@en ;
    reg:status <http://metadataregistry.org/uri/RegStatus/1001> ;
    rdfs:domain <http://rdaregistry.info/Elements/c/C10012> ;
    rdfs:isDefinedBy <http://rdaregistry.info/Elements/n/> ;
    rdfs:subPropertyOf <http://rdaregistry.info/Elements/n/P80016>,
        <http://rdaregistry.info/Elements/n/P80159> ;
    skos:definition "Relates a nomen to an item that has an appellation in natural language that is taken from a vocabulary encoding scheme or is constructed using a string encoding scheme."@en .

<http://rdaregistry.info/Elements/n/P80017> a rdf:Property ;
    rdfs:label "is title of item of"@en ;
    rdakit:hasElementType "2" ;
    rdakit:toolkitDefinition "An item that has an appellation of item in natural language and phrasing used in common discourse."@en ;
    rdakit:toolkitLabel "title of item of"@en ;
    reg:hasSubproperty <http://rdaregistry.info/Elements/n/P80093>,
        <http://rdaregistry.info/Elements/n/datatype/P80017>,
        <http://rdaregistry.info/Elements/n/object/P80017> ;
    reg:hasUnconstrained <http://rdaregistry.info/Elements/u/P60912> ;
    reg:lexicalAlias <http://rdaregistry.info/Elements/n/titleOfItemOf.en> ;
    reg:name "titleOfItemOf"@en ;
    reg:status <http://metadataregistry.org/uri/RegStatus/1001> ;
    rdfs:domain <http://rdaregistry.info/Elements/c/C10012> ;
    rdfs:isDefinedBy <http://rdaregistry.info/Elements/n/> ;
    rdfs:subPropertyOf <http://rdaregistry.info/Elements/n/P80016>,
        <http://rdaregistry.info/Elements/n/P80161> ;
    skos:definition "Relates a nomen to an item that has an appellation of item in natural language and phrasing used in common discourse."@en .

<http://rdaregistry.info/Elements/n/P80023> a rdf:Property ;
    rdfs:label "is access point for expression of"@en ;
    rdakit:hasElementType "2" ;
    rdakit:toolkitDefinition "An expression that has an appellation in natural language that is taken from a vocabulary encoding scheme or is constructed using a string encoding scheme."@en ;
    rdakit:toolkitLabel "access point for expression of"@en ;
    reg:hasSubproperty <http://rdaregistry.info/Elements/n/P80096>,
        <http://rdaregistry.info/Elements/n/datatype/P80023>,
        <http://rdaregistry.info/Elements/n/object/P80023> ;
    reg:hasUnconstrained <http://rdaregistry.info/Elements/u/P60910> ;
    reg:lexicalAlias <http://rdaregistry.info/Elements/n/accessPointForExpressionOf.en> ;
    reg:name "accessPointForExpressionOf"@en ;
    reg:status <http://metadataregistry.org/uri/RegStatus/1001> ;
    rdfs:domain <http://rdaregistry.info/Elements/c/C10012> ;
    rdfs:isDefinedBy <http://rdaregistry.info/Elements/n/> ;
    rdfs:subPropertyOf <http://rdaregistry.info/Elements/n/P80038>,
        <http://rdaregistry.info/Elements/n/P80159> ;
    skos:definition "Relates a nomen to an expression that has an appellation in natural language that is taken from a vocabulary encoding scheme or is constructed using a string encoding scheme."@en .

<http://rdaregistry.info/Elements/n/P80024> a rdf:Property ;
    rdfs:label "is access point for manifestation of"@en ;
    rdakit:hasElementType "2" ;
    rdakit:toolkitDefinition "A manifestation that has an appellation in natural language that is taken from a vocabulary encoding scheme or is constructed using a string encoding scheme."@en ;
    rdakit:toolkitLabel "access point for manifestation of"@en ;
    reg:hasSubproperty <http://rdaregistry.info/Elements/n/P80090>,
        <http://rdaregistry.info/Elements/n/datatype/P80024>,
        <http://rdaregistry.info/Elements/n/object/P80024> ;
    reg:hasUnconstrained <http://rdaregistry.info/Elements/u/P60910> ;
    reg:lexicalAlias <http://rdaregistry.info/Elements/n/accessPointForManifestationOf.en> ;
    reg:name "accessPointForManifestationOf"@en ;
    reg:status <http://metadataregistry.org/uri/RegStatus/1001> ;
    rdfs:domain <http://rdaregistry.info/Elements/c/C10012> ;
    rdfs:isDefinedBy <http://rdaregistry.info/Elements/n/> ;
    rdfs:subPropertyOf <http://rdaregistry.info/Elements/n/P80040>,
        <http://rdaregistry.info/Elements/n/P80159> ;
    skos:definition "Relates a nomen to a manifestation that has an appellation in natural language that is taken from a vocabulary encoding scheme or is constructed using a string encoding scheme."@en .

<http://rdaregistry.info/Elements/n/P80025> a rdf:Property ;
    rdfs:label "is access point for place of"@en ;
    rdakit:hasElementType "2" ;
    rdakit:toolkitDefinition "A place that has an appellation in natural language that is taken from a vocabulary encoding scheme or is constructed using a string encoding scheme."@en ;
    rdakit:toolkitLabel "access point for place of"@en ;
    reg:hasSubproperty <http://rdaregistry.info/Elements/n/P80086>,
        <http://rdaregistry.info/Elements/n/P80107>,
        <http://rdaregistry.info/Elements/n/P80108>,
        <http://rdaregistry.info/Elements/n/datatype/P80025>,
        <http://rdaregistry.info/Elements/n/object/P80025> ;
    reg:hasUnconstrained <http://rdaregistry.info/Elements/u/P60910> ;
    reg:lexicalAlias <http://rdaregistry.info/Elements/n/accessPointForPlaceOf.en> ;
    reg:name "accessPointForPlaceOf"@en ;
    reg:status <http://metadataregistry.org/uri/RegStatus/1001> ;
    rdfs:domain <http://rdaregistry.info/Elements/c/C10012> ;
    rdfs:isDefinedBy <http://rdaregistry.info/Elements/n/> ;
    rdfs:subPropertyOf <http://rdaregistry.info/Elements/n/P80041>,
        <http://rdaregistry.info/Elements/n/P80159> ;
    skos:definition "Relates a nomen to a place that has an appellation in natural language that is taken from a vocabulary encoding scheme or is constructed using a string encoding scheme."@en .

<http://rdaregistry.info/Elements/n/P80026> a rdf:Property ;
    rdfs:label "is access point for timespan of"@en ;
    rdakit:hasElementType "2" ;
    rdakit:toolkitDefinition "A timespan that has an appellation in natural language that is taken from a vocabulary encoding scheme or is constructed using a string encoding scheme."@en ;
    rdakit:toolkitLabel "access point for timespan of"@en ;
    reg:hasSubproperty <http://rdaregistry.info/Elements/n/P80082>,
        <http://rdaregistry.info/Elements/n/datatype/P80026>,
        <http://rdaregistry.info/Elements/n/object/P80026> ;
    reg:hasUnconstrained <http://rdaregistry.info/Elements/u/P60910> ;
    reg:lexicalAlias <http://rdaregistry.info/Elements/n/accessPointForTimespanOf.en> ;
    reg:name "accessPointForTimespanOf"@en ;
    reg:status <http://metadataregistry.org/uri/RegStatus/1001> ;
    rdfs:domain <http://rdaregistry.info/Elements/c/C10012> ;
    rdfs:isDefinedBy <http://rdaregistry.info/Elements/n/> ;
    rdfs:subPropertyOf <http://rdaregistry.info/Elements/n/P80043>,
        <http://rdaregistry.info/Elements/n/P80159> ;
    skos:definition "Relates a nomen to a timespan that has an appellation in natural language that is taken from a vocabulary encoding scheme or is constructed using a string encoding scheme."@en .

<http://rdaregistry.info/Elements/n/P80027> a rdf:Property ;
    rdfs:label "is access point for work of"@en ;
    rdakit:hasElementType "2" ;
    rdakit:toolkitDefinition "A work that has an appellation in natural language that is taken from a vocabulary encoding scheme or is constructed using a string encoding scheme."@en ;
    rdakit:toolkitLabel "access point for work of"@en ;
    reg:hasSubproperty <http://rdaregistry.info/Elements/n/P80080>,
        <http://rdaregistry.info/Elements/n/datatype/P80027>,
        <http://rdaregistry.info/Elements/n/object/P80027> ;
    reg:hasUnconstrained <http://rdaregistry.info/Elements/u/P60910> ;
    reg:lexicalAlias <http://rdaregistry.info/Elements/n/accessPointForWorkOf.en> ;
    reg:name "accessPointForWorkOf"@en ;
    reg:status <http://metadataregistry.org/uri/RegStatus/1001> ;
    rdfs:domain <http://rdaregistry.info/Elements/c/C10012> ;
    rdfs:isDefinedBy <http://rdaregistry.info/Elements/n/> ;
    rdfs:subPropertyOf <http://rdaregistry.info/Elements/n/P80045>,
        <http://rdaregistry.info/Elements/n/P80159> ;
    skos:definition "Relates a nomen to a work that has an appellation in natural language that is taken from a vocabulary encoding scheme or is constructed using a string encoding scheme."@en .

<http://rdaregistry.info/Elements/n/P80033> a rdf:Property ;
    rdfs:label "is identifier for agent of"@en ;
    rdakit:hasElementType "2" ;
    rdakit:toolkitDefinition "An agent who has an appellation of agent that is a reference code taken from a vocabulary encoding scheme."@en ;
    rdakit:toolkitLabel "identifier for agent of"@en ;
    reg:hasSubproperty <http://rdaregistry.info/Elements/n/P80034>,
        <http://rdaregistry.info/Elements/n/P80037>,
        <http://rdaregistry.info/Elements/n/datatype/P80033>,
        <http://rdaregistry.info/Elements/n/object/P80033> ;
    reg:hasUnconstrained <http://rdaregistry.info/Elements/u/P60937> ;
    reg:lexicalAlias <http://rdaregistry.info/Elements/n/identifierForAgentOf.en> ;
    reg:name "identifierForAgentOf"@en ;
    reg:status <http://metadataregistry.org/uri/RegStatus/1001> ;
    rdfs:domain <http://rdaregistry.info/Elements/c/C10012> ;
    rdfs:isDefinedBy <http://rdaregistry.info/Elements/n/> ;
    rdfs:subPropertyOf <http://rdaregistry.info/Elements/n/P80028>,
        <http://rdaregistry.info/Elements/n/P80160> ;
    skos:definition "Relates a nomen to an agent who has an appellation of agent that is a reference code taken from a vocabulary encoding scheme."@en .

<http://rdaregistry.info/Elements/n/P80039> a rdf:Property ;
    rdfs:label "is title of expression of"@en ;
    rdakit:hasElementType "2" ;
    rdakit:toolkitDefinition "An expression that has an appellation of expression in natural language and phrasing used in common discourse."@en ;
    rdakit:toolkitLabel "title of expression of"@en ;
    reg:hasSubproperty <http://rdaregistry.info/Elements/n/P80097>,
        <http://rdaregistry.info/Elements/n/datatype/P80039>,
        <http://rdaregistry.info/Elements/n/object/P80039> ;
    reg:hasUnconstrained <http://rdaregistry.info/Elements/u/P60912> ;
    reg:lexicalAlias <http://rdaregistry.info/Elements/n/titleOfExpressionOf.en> ;
    reg:name "titleOfExpressionOf"@en ;
    reg:status <http://metadataregistry.org/uri/RegStatus/1001> ;
    rdfs:domain <http://rdaregistry.info/Elements/c/C10012> ;
    rdfs:isDefinedBy <http://rdaregistry.info/Elements/n/> ;
    rdfs:subPropertyOf <http://rdaregistry.info/Elements/n/P80038>,
        <http://rdaregistry.info/Elements/n/P80161> ;
    skos:definition "Relates a nomen to an expression that has an appellation of expression in natural language and phrasing used in common discourse."@en .

<http://rdaregistry.info/Elements/n/P80044> a rdf:Property ;
    rdfs:label "is name of timespan of"@en ;
    rdakit:hasElementType "2" ;
    rdakit:toolkitDefinition "A timespan that has an appellation of timespan in natural language and phrasing used in common discourse."@en ;
    rdakit:toolkitLabel "name of timespan of"@en ;
    reg:hasSubproperty <http://rdaregistry.info/Elements/n/P80083>,
        <http://rdaregistry.info/Elements/n/datatype/P80044>,
        <http://rdaregistry.info/Elements/n/object/P80044> ;
    reg:hasUnconstrained <http://rdaregistry.info/Elements/u/P60920> ;
    reg:lexicalAlias <http://rdaregistry.info/Elements/n/nameOfTimespanOf.en> ;
    reg:name "nameOfTimespanOf"@en ;
    reg:status <http://metadataregistry.org/uri/RegStatus/1001> ;
    rdfs:domain <http://rdaregistry.info/Elements/c/C10012> ;
    rdfs:isDefinedBy <http://rdaregistry.info/Elements/n/> ;
    rdfs:subPropertyOf <http://rdaregistry.info/Elements/n/P80043>,
        <http://rdaregistry.info/Elements/n/P80161> ;
    skos:definition "Relates a nomen to a timespan that has an appellation of timespan in natural language and phrasing used in common discourse."@en .

<http://rdaregistry.info/Elements/n/P80051> a rdf:Property ;
    rdfs:label "is name of place of"@en ;
    rdakit:hasElementType "2" ;
    rdakit:toolkitDefinition "A place that has an appellation of place in natural language and phrasing used in common discourse."@en ;
    rdakit:toolkitLabel "name of place of"@en ;
    reg:hasSubproperty <http://rdaregistry.info/Elements/n/P80087>,
        <http://rdaregistry.info/Elements/n/datatype/P80051>,
        <http://rdaregistry.info/Elements/n/object/P80051> ;
    reg:hasUnconstrained <http://rdaregistry.info/Elements/u/P60920> ;
    reg:lexicalAlias <http://rdaregistry.info/Elements/n/nameOfPlaceOf.en> ;
    reg:name "nameOfPlaceOf"@en ;
    reg:status <http://metadataregistry.org/uri/RegStatus/1001> ;
    rdfs:domain <http://rdaregistry.info/Elements/c/C10012> ;
    rdfs:isDefinedBy <http://rdaregistry.info/Elements/n/> ;
    rdfs:subPropertyOf <http://rdaregistry.info/Elements/n/P80041>,
        <http://rdaregistry.info/Elements/n/P80161> ;
    skos:definition "Relates a nomen to a place that has an appellation of place in natural language and phrasing used in common discourse."@en .

<http://rdaregistry.info/Elements/n/P80073> a rdf:Property ;
    rdfs:label "is assigned by agent"@en ;
    rdakit:hasElementType "2" ;
    rdakit:toolkitDefinition "An agent who assigns a nomen to an entity."@en ;
    rdakit:toolkitLabel "assigned by agent"@en ;
    reg:hasSubproperty <http://rdaregistry.info/Elements/n/P80074>,
        <http://rdaregistry.info/Elements/n/P80077>,
        <http://rdaregistry.info/Elements/n/datatype/P80073>,
        <http://rdaregistry.info/Elements/n/object/P80073> ;
    reg:hasUnconstrained <http://rdaregistry.info/Elements/u/P60943> ;
    reg:lexicalAlias <http://rdaregistry.info/Elements/n/assignedByAgent.en> ;
    reg:name "assignedByAgent"@en ;
    reg:status <http://metadataregistry.org/uri/RegStatus/1001> ;
    rdfs:domain <http://rdaregistry.info/Elements/c/C10012> ;
    rdfs:isDefinedBy <http://rdaregistry.info/Elements/n/> ;
    rdfs:subPropertyOf <http://rdaregistry.info/Elements/n/P80005> ;
    skos:definition "Relates a nomen to an agent who assigns a nomen to an entity."@en .

<http://rdaregistry.info/Elements/n/P80099> a rdf:Property ;
    rdfs:label "is authorized access point for agent of"@en ;
    rdakit:hasElementType "2" ;
    rdakit:toolkitDefinition "An agent who has an access point for agent that is selected for preference in a specific vocabulary encoding scheme."@en ;
    rdakit:toolkitLabel "authorized access point for agent of"@en ;
    reg:hasSubproperty <http://rdaregistry.info/Elements/n/P80101>,
        <http://rdaregistry.info/Elements/n/P80107>,
        <http://rdaregistry.info/Elements/n/datatype/P80099>,
        <http://rdaregistry.info/Elements/n/object/P80099> ;
    reg:hasUnconstrained <http://rdaregistry.info/Elements/u/P60918> ;
    reg:lexicalAlias <http://rdaregistry.info/Elements/n/authorizedAccessPointForAgentOf.en> ;
    reg:name "authorizedAccessPointForAgentOf"@en ;
    reg:status <http://metadataregistry.org/uri/RegStatus/1001> ;
    rdfs:domain <http://rdaregistry.info/Elements/c/C10012> ;
    rdfs:isDefinedBy <http://rdaregistry.info/Elements/n/> ;
    rdfs:subPropertyOf <http://rdaregistry.info/Elements/n/P80018>,
        <http://rdaregistry.info/Elements/n/P80162> ;
    skos:definition "Relates a nomen to an agent who has an access point for agent that is selected for preference in a specific vocabulary encoding scheme."@en .

<http://rdaregistry.info/Elements/n/P80125> a rdf:Property ;
    rdfs:label "is title of series of"@en ;
    rdakit:hasElementType "2" ;
    rdakit:toolkitDefinition "A manifestation that has a title that identifies a series to which a manifestation belongs."@en ;
    rdakit:toolkitLabel "title of series of"@en ;
    reg:hasSubproperty <http://rdaregistry.info/Elements/n/P80126>,
        <http://rdaregistry.info/Elements/n/datatype/P80125> ;
    reg:hasUnconstrained <http://rdaregistry.info/Elements/u/P60958> ;
    reg:lexicalAlias <http://rdaregistry.info/Elements/n/titleOfSeriesOf.en> ;
    reg:name "titleOfSeriesOf"@en ;
    reg:status <http://metadataregistry.org/uri/RegStatus/1001> ;
    rdfs:domain <http://rdaregistry.info/Elements/c/C10012> ;
    rdfs:isDefinedBy <http://rdaregistry.info/Elements/n/> ;
    rdfs:subPropertyOf <http://rdaregistry.info/Elements/n/P80062> ;
    skos:definition "Relates a nomen to a manifestation that has a title that identifies a series to which a manifestation belongs."@en .

<http://rdaregistry.info/Elements/n/P80142> a rdf:Property ;
    rdfs:label "is variant name of agent of"@en ;
    rdakit:hasElementType "2" ;
    rdakit:toolkitDefinition "An agent who has a name of agent that is not selected for preference in a specific application or context."@en ;
    rdakit:toolkitLabel "variant name of agent of"@en ;
    reg:hasSubproperty <http://rdaregistry.info/Elements/n/P80143>,
        <http://rdaregistry.info/Elements/n/P80149>,
        <http://rdaregistry.info/Elements/n/datatype/P80142> ;
    reg:hasUnconstrained <http://rdaregistry.info/Elements/u/P60921> ;
    reg:lexicalAlias <http://rdaregistry.info/Elements/n/variantNameOfAgentOf.en> ;
    reg:name "variantNameOfAgentOf"@en ;
    reg:status <http://metadataregistry.org/uri/RegStatus/1001> ;
    rdfs:domain <http://rdaregistry.info/Elements/c/C10012> ;
    rdfs:isDefinedBy <http://rdaregistry.info/Elements/n/> ;
    rdfs:subPropertyOf <http://rdaregistry.info/Elements/n/P80052>,
        <http://rdaregistry.info/Elements/n/P80164> ;
    skos:definition "Relates a nomen to an agent who has a name of agent that is not selected for preference in a specific application or context."@en .

<http://rdaregistry.info/Elements/n/P80171> a rdf:Property ;
    rdfs:label "is appellation of work group of"@en ;
    rdakit:hasElementType "2" ;
    rdakit:toolkitDefinition "A work that is referred to by a nomen used within a given scheme or context to refer to a work as a member of a work group."@en ;
    rdakit:toolkitLabel "appellation of work group of"@en ;
    reg:hasSubproperty <http://rdaregistry.info/Elements/n/P80172>,
        <http://rdaregistry.info/Elements/n/P80173>,
        <http://rdaregistry.info/Elements/n/datatype/P80171>,
        <http://rdaregistry.info/Elements/n/object/P80171> ;
    reg:hasUnconstrained <http://rdaregistry.info/Elements/u/P60911> ;
    reg:lexicalAlias <http://rdaregistry.info/Elements/n/appellationOfWorkGroupOf.en> ;
    reg:name "appellationOfWorkGroupOf" ;
    reg:status <http://metadataregistry.org/uri/RegStatus/1001> ;
    rdfs:domain <http://rdaregistry.info/Elements/c/C10012> ;
    rdfs:isDefinedBy <http://rdaregistry.info/Elements/n/> ;
    rdfs:subPropertyOf <http://rdaregistry.info/Elements/n/P80045> ;
    skos:definition "Relates a nomen to work that is referred to by a nomen used within a given scheme or context to refer to a work as a member of a work group."@en .

<http://rdaregistry.info/Elements/n/P80020> a rdf:Property ;
    rdfs:label "is access point for corporate body of"@en ;
    rdakit:hasElementType "2" ;
    rdakit:toolkitDefinition "A corporate body who has an appellation in natural language that is taken from a vocabulary encoding scheme or is constructed using a string encoding scheme."@en ;
    rdakit:toolkitLabel "access point for corporate body of"@en ;
    reg:hasSubproperty <http://rdaregistry.info/Elements/n/P80103>,
        <http://rdaregistry.info/Elements/n/P80104>,
        <http://rdaregistry.info/Elements/n/datatype/P80020>,
        <http://rdaregistry.info/Elements/n/object/P80020> ;
    reg:hasUnconstrained <http://rdaregistry.info/Elements/u/P60910> ;
    reg:lexicalAlias <http://rdaregistry.info/Elements/n/accessPointForCorporateBodyOf.en> ;
    reg:name "accessPointForCorporateBodyOf"@en ;
    reg:status <http://metadataregistry.org/uri/RegStatus/1001> ;
    rdfs:domain <http://rdaregistry.info/Elements/c/C10012> ;
    rdfs:isDefinedBy <http://rdaregistry.info/Elements/n/> ;
    rdfs:subPropertyOf <http://rdaregistry.info/Elements/n/P80019>,
        <http://rdaregistry.info/Elements/n/P80030> ;
    skos:definition "Relates a nomen to a corporate body who has an appellation in natural language that is taken from a vocabulary encoding scheme or is constructed using a string encoding scheme."@en .

<http://rdaregistry.info/Elements/n/P80021> a rdf:Property ;
    rdfs:label "is access point for family of"@en ;
    rdakit:hasElementType "2" ;
    rdakit:toolkitDefinition "A family who has an appellation in natural language that is taken from a vocabulary encoding scheme or is constructed using a string encoding scheme."@en ;
    rdakit:toolkitLabel "access point for family of"@en ;
    reg:hasSubproperty <http://rdaregistry.info/Elements/n/P80105>,
        <http://rdaregistry.info/Elements/n/P80106>,
        <http://rdaregistry.info/Elements/n/datatype/P80021>,
        <http://rdaregistry.info/Elements/n/object/P80021> ;
    reg:hasUnconstrained <http://rdaregistry.info/Elements/u/P60910> ;
    reg:lexicalAlias <http://rdaregistry.info/Elements/n/accessPointForFamilyOf.en> ;
    reg:name "accessPointForFamilyOf"@en ;
    reg:status <http://metadataregistry.org/uri/RegStatus/1001> ;
    rdfs:domain <http://rdaregistry.info/Elements/c/C10012> ;
    rdfs:isDefinedBy <http://rdaregistry.info/Elements/n/> ;
    rdfs:subPropertyOf <http://rdaregistry.info/Elements/n/P80019>,
        <http://rdaregistry.info/Elements/n/P80031> ;
    skos:definition "Relates a nomen to a family who has an appellation in natural language that is taken from a vocabulary encoding scheme or is constructed using a string encoding scheme."@en .

<http://rdaregistry.info/Elements/n/P80022> a rdf:Property ;
    rdfs:label "is access point for person of"@en ;
    rdakit:hasElementType "2" ;
    rdakit:toolkitDefinition "A person who has an appellation in natural language that is taken from a vocabulary encoding scheme or is constructed using a string encoding scheme."@en ;
    rdakit:toolkitLabel "access point for person of"@en ;
    reg:hasSubproperty <http://rdaregistry.info/Elements/n/datatype/P80022>,
        <http://rdaregistry.info/Elements/n/object/P80022> ;
    reg:hasUnconstrained <http://rdaregistry.info/Elements/u/P60910> ;
    reg:lexicalAlias <http://rdaregistry.info/Elements/n/accessPointForPersonOf.en> ;
    reg:name "accessPointForPersonOf"@en ;
    reg:status <http://metadataregistry.org/uri/RegStatus/1001> ;
    rdfs:domain <http://rdaregistry.info/Elements/c/C10012> ;
    rdfs:isDefinedBy <http://rdaregistry.info/Elements/n/> ;
    rdfs:subPropertyOf <http://rdaregistry.info/Elements/n/P80018>,
        <http://rdaregistry.info/Elements/n/P80032> ;
    skos:definition "Relates a nomen to a person who has an appellation in natural language that is taken from a vocabulary encoding scheme or is constructed using a string encoding scheme."@en .

<http://rdaregistry.info/Elements/n/P80034> a rdf:Property ;
    rdfs:label "is identifier for collective agent of"@en ;
    rdakit:hasElementType "2" ;
    rdakit:toolkitDefinition "A collective agent who has an appellation of collective agent that is a reference code taken from a vocabulary encoding scheme."@en ;
    rdakit:toolkitLabel "identifier for collective agent of"@en ;
    reg:hasSubproperty <http://rdaregistry.info/Elements/n/P80035>,
        <http://rdaregistry.info/Elements/n/P80036>,
        <http://rdaregistry.info/Elements/n/datatype/P80034>,
        <http://rdaregistry.info/Elements/n/object/P80034> ;
    reg:hasUnconstrained <http://rdaregistry.info/Elements/u/P60937> ;
    reg:lexicalAlias <http://rdaregistry.info/Elements/n/identifierForCollectiveAgentOf.en> ;
    reg:name "identifierForCollectiveAgentOf"@en ;
    reg:status <http://metadataregistry.org/uri/RegStatus/1001> ;
    rdfs:domain <http://rdaregistry.info/Elements/c/C10012> ;
    rdfs:isDefinedBy <http://rdaregistry.info/Elements/n/> ;
    rdfs:subPropertyOf <http://rdaregistry.info/Elements/n/P80029>,
        <http://rdaregistry.info/Elements/n/P80033> ;
    skos:definition "Relates a nomen to a collective agent who has an appellation of collective agent that is a reference code taken from a vocabulary encoding scheme."@en .

<http://rdaregistry.info/Elements/n/P80048> a rdf:Property ;
    rdfs:label "is identifier for manifestation of"@en ;
    rdakit:hasElementType "2" ;
    rdakit:toolkitDefinition "A manifestation that has an appellation of manifestation that is a reference code taken from a vocabulary encoding scheme."@en ;
    rdakit:toolkitLabel "identifier for manifestation of"@en ;
    reg:hasSubproperty <http://rdaregistry.info/Elements/n/P80138>,
        <http://rdaregistry.info/Elements/n/P80155>,
        <http://rdaregistry.info/Elements/n/P80156>,
        <http://rdaregistry.info/Elements/n/datatype/P80048>,
        <http://rdaregistry.info/Elements/n/object/P80048> ;
    reg:hasUnconstrained <http://rdaregistry.info/Elements/u/P60938> ;
    reg:lexicalAlias <http://rdaregistry.info/Elements/n/identifierForManifestationOf.en> ;
    reg:name "identifierForManifestationOf"@en ;
    reg:status <http://metadataregistry.org/uri/RegStatus/1001> ;
    rdfs:domain <http://rdaregistry.info/Elements/c/C10012> ;
    rdfs:isDefinedBy <http://rdaregistry.info/Elements/n/> ;
    rdfs:subPropertyOf <http://rdaregistry.info/Elements/n/P80040>,
        <http://rdaregistry.info/Elements/n/P80160> ;
    skos:definition "Relates a nomen to a manifestation that has an appellation of manifestation that is a reference code taken from a vocabulary encoding scheme."@en .

<http://rdaregistry.info/Elements/n/P80049> a rdf:Property ;
    rdfs:label "is identifier for work of"@en ;
    rdakit:hasElementType "2" ;
    rdakit:toolkitDefinition "A work that has an appellation of work that is a reference code taken from a vocabulary encoding scheme."@en ;
    rdakit:toolkitLabel "identifier for work of"@en ;
    reg:hasSubproperty <http://rdaregistry.info/Elements/n/P80119>,
        <http://rdaregistry.info/Elements/n/P80170>,
        <http://rdaregistry.info/Elements/n/P80172>,
        <http://rdaregistry.info/Elements/n/datatype/P80049>,
        <http://rdaregistry.info/Elements/n/object/P80049> ;
    reg:hasUnconstrained <http://rdaregistry.info/Elements/u/P60938> ;
    reg:lexicalAlias <http://rdaregistry.info/Elements/n/identifierForWorkOf.en> ;
    reg:name "identifierForWorkOf"@en ;
    reg:status <http://metadataregistry.org/uri/RegStatus/1001> ;
    rdfs:domain <http://rdaregistry.info/Elements/c/C10012> ;
    rdfs:isDefinedBy <http://rdaregistry.info/Elements/n/> ;
    rdfs:subPropertyOf <http://rdaregistry.info/Elements/n/P80045>,
        <http://rdaregistry.info/Elements/n/P80160> ;
    skos:definition "Relates a nomen to a work that has an appellation of work that is a reference code taken from a vocabulary encoding scheme."@en .

<http://rdaregistry.info/Elements/n/P80054> a rdf:Property ;
    rdfs:label "is name of corporate body of"@en ;
    rdakit:hasElementType "2" ;
    rdakit:toolkitDefinition "A corporate body who has an appellation of corporate body in natural language and phrasing used in common discourse."@en ;
    rdakit:toolkitLabel "name of corporate body of"@en ;
    reg:hasSubproperty <http://rdaregistry.info/Elements/n/P80144>,
        <http://rdaregistry.info/Elements/n/P80147>,
        <http://rdaregistry.info/Elements/n/datatype/P80054>,
        <http://rdaregistry.info/Elements/n/object/P80054> ;
    reg:hasUnconstrained <http://rdaregistry.info/Elements/u/P60920> ;
    reg:lexicalAlias <http://rdaregistry.info/Elements/n/nameOfCorporateBodyOf.en> ;
    reg:name "nameOfCorporateBodyOf"@en ;
    reg:status <http://metadataregistry.org/uri/RegStatus/1001> ;
    rdfs:domain <http://rdaregistry.info/Elements/c/C10012> ;
    rdfs:isDefinedBy <http://rdaregistry.info/Elements/n/> ;
    rdfs:subPropertyOf <http://rdaregistry.info/Elements/n/P80030>,
        <http://rdaregistry.info/Elements/n/P80053> ;
    skos:definition "Relates a nomen to a corporate body who has an appellation of corporate body in natural language and phrasing used in common discourse."@en .

<http://rdaregistry.info/Elements/n/P80055> a rdf:Property ;
    rdfs:label "is name of family of"@en ;
    rdakit:hasElementType "2" ;
    rdakit:toolkitDefinition "A family who has an appellation of family in natural language and phrasing used in common discourse."@en ;
    rdakit:toolkitLabel "name of family of"@en ;
    reg:hasSubproperty <http://rdaregistry.info/Elements/n/P80145>,
        <http://rdaregistry.info/Elements/n/P80148>,
        <http://rdaregistry.info/Elements/n/datatype/P80055>,
        <http://rdaregistry.info/Elements/n/object/P80055> ;
    reg:hasUnconstrained <http://rdaregistry.info/Elements/u/P60920> ;
    reg:lexicalAlias <http://rdaregistry.info/Elements/n/nameOfFamilyOf.en> ;
    reg:name "nameOfFamilyOf"@en ;
    reg:status <http://metadataregistry.org/uri/RegStatus/1001> ;
    rdfs:domain <http://rdaregistry.info/Elements/c/C10012> ;
    rdfs:isDefinedBy <http://rdaregistry.info/Elements/n/> ;
    rdfs:subPropertyOf <http://rdaregistry.info/Elements/n/P80031>,
        <http://rdaregistry.info/Elements/n/P80053> ;
    skos:definition "Relates a nomen to a family who has an appellation of family in natural language and phrasing used in common discourse."@en .

<http://rdaregistry.info/Elements/n/P80062> a rdf:Property ;
    rdfs:label "is title of manifestation of"@en ;
    rdakit:hasElementType "2" ;
    rdakit:toolkitDefinition "A manifestation that has an appellation of manifestation in natural language and phrasing used in common discourse."@en ;
    rdakit:toolkitLabel "title of manifestation of"@en ;
    reg:hasSubproperty <http://rdaregistry.info/Elements/n/P80063>,
        <http://rdaregistry.info/Elements/n/datatype/P80062>,
        <http://rdaregistry.info/Elements/n/object/P80062> ;
    reg:hasUnconstrained <http://rdaregistry.info/Elements/u/P60912> ;
    reg:lexicalAlias <http://rdaregistry.info/Elements/n/titleOfManifestationOf.en> ;
    reg:name "titleOfManifestationOf"@en ;
    reg:status <http://metadataregistry.org/uri/RegStatus/1001> ;
    rdfs:domain <http://rdaregistry.info/Elements/c/C10012> ;
    rdfs:isDefinedBy <http://rdaregistry.info/Elements/n/> ;
    rdfs:subPropertyOf <http://rdaregistry.info/Elements/n/P80040>,
        <http://rdaregistry.info/Elements/n/P80161> ;
    skos:definition "Relates a nomen to a manifestation that has an appellation of manifestation in natural language and phrasing used in common discourse."@en .

<http://rdaregistry.info/Elements/n/P80064> a rdf:Property ;
    rdfs:label "is title of work of"@en ;
    rdakit:hasElementType "2" ;
    rdakit:toolkitDefinition "A work that has an appellation of work in natural language and phrasing used in common discourse."@en ;
    rdakit:toolkitLabel "title of work of"@en ;
    reg:hasSubproperty <http://rdaregistry.info/Elements/n/P80072>,
        <http://rdaregistry.info/Elements/n/P80109>,
        <http://rdaregistry.info/Elements/n/datatype/P80064>,
        <http://rdaregistry.info/Elements/n/object/P80064> ;
    reg:hasUnconstrained <http://rdaregistry.info/Elements/u/P60912> ;
    reg:lexicalAlias <http://rdaregistry.info/Elements/n/titleOfWorkOf.en> ;
    reg:name "titleOfWorkOf"@en ;
    reg:status <http://metadataregistry.org/uri/RegStatus/1001> ;
    rdfs:domain <http://rdaregistry.info/Elements/c/C10012> ;
    rdfs:isDefinedBy <http://rdaregistry.info/Elements/n/> ;
    rdfs:subPropertyOf <http://rdaregistry.info/Elements/n/P80045>,
        <http://rdaregistry.info/Elements/n/P80161> ;
    skos:definition "Relates a nomen to a work that has an appellation of work in natural language and phrasing used in common discourse."@en .

<http://rdaregistry.info/Elements/n/P80074> a rdf:Property ;
    rdfs:label "is assigned by collective agent"@en ;
    rdakit:hasElementType "2" ;
    rdakit:toolkitDefinition "A collective agent who assigns a nomen to an entity."@en ;
    rdakit:toolkitLabel "assigned by collective agent"@en ;
    reg:hasSubproperty <http://rdaregistry.info/Elements/n/P80075>,
        <http://rdaregistry.info/Elements/n/P80076>,
        <http://rdaregistry.info/Elements/n/datatype/P80074>,
        <http://rdaregistry.info/Elements/n/object/P80074> ;
    reg:hasUnconstrained <http://rdaregistry.info/Elements/u/P60943> ;
    reg:lexicalAlias <http://rdaregistry.info/Elements/n/assignedByCollectiveAgent.en> ;
    reg:name "assignedByCollectiveAgent"@en ;
    reg:status <http://metadataregistry.org/uri/RegStatus/1001> ;
    rdfs:domain <http://rdaregistry.info/Elements/c/C10012> ;
    rdfs:isDefinedBy <http://rdaregistry.info/Elements/n/> ;
    rdfs:subPropertyOf <http://rdaregistry.info/Elements/n/P80006>,
        <http://rdaregistry.info/Elements/n/P80073> ;
    skos:definition "Relates a nomen to a collective agent who assigns a nomen to an entity."@en .

<http://rdaregistry.info/Elements/n/P80100> a rdf:Property ;
    rdfs:label "is variant access point for agent of"@en ;
    rdakit:hasElementType "2" ;
    rdakit:toolkitDefinition "An agent who has an access point for agent that is not selected for preference in a specific vocabulary encoding scheme."@en ;
    rdakit:toolkitLabel "variant access point for agent of"@en ;
    reg:hasSubproperty <http://rdaregistry.info/Elements/n/P80102>,
        <http://rdaregistry.info/Elements/n/P80108>,
        <http://rdaregistry.info/Elements/n/datatype/P80100>,
        <http://rdaregistry.info/Elements/n/object/P80100> ;
    reg:hasUnconstrained <http://rdaregistry.info/Elements/u/P60934> ;
    reg:lexicalAlias <http://rdaregistry.info/Elements/n/variantAccessPointForAgentOf.en> ;
    reg:name "variantAccessPointForAgentOf"@en ;
    reg:status <http://metadataregistry.org/uri/RegStatus/1001> ;
    rdfs:domain <http://rdaregistry.info/Elements/c/C10012> ;
    rdfs:isDefinedBy <http://rdaregistry.info/Elements/n/> ;
    rdfs:subPropertyOf <http://rdaregistry.info/Elements/n/P80018>,
        <http://rdaregistry.info/Elements/n/P80165> ;
    skos:definition "Relates a nomen to an agent who has an access point for agent that is not selected for preference in a specific vocabulary encoding scheme."@en .

<http://rdaregistry.info/Elements/n/P80101> a rdf:Property ;
    rdfs:label "is authorized access point for collective agent of"@en ;
    rdakit:hasElementType "2" ;
    rdakit:toolkitDefinition "A collective agent who has an access point for collective agent that is selected for preference in a specific vocabulary encoding scheme."@en ;
    rdakit:toolkitLabel "authorized access point for collective agent of"@en ;
    reg:hasSubproperty <http://rdaregistry.info/Elements/n/P80103>,
        <http://rdaregistry.info/Elements/n/P80105>,
        <http://rdaregistry.info/Elements/n/datatype/P80101>,
        <http://rdaregistry.info/Elements/n/object/P80101> ;
    reg:hasUnconstrained <http://rdaregistry.info/Elements/u/P60918> ;
    reg:lexicalAlias <http://rdaregistry.info/Elements/n/authorizedAccessPointForCollectiveAgentOf.en> ;
    reg:name "authorizedAccessPointForCollectiveAgentOf"@en ;
    reg:status <http://metadataregistry.org/uri/RegStatus/1001> ;
    rdfs:domain <http://rdaregistry.info/Elements/c/C10012> ;
    rdfs:isDefinedBy <http://rdaregistry.info/Elements/n/> ;
    rdfs:subPropertyOf <http://rdaregistry.info/Elements/n/P80019>,
        <http://rdaregistry.info/Elements/n/P80099> ;
    skos:definition "Relates a nomen to a collective agent who has an access point for collective agent that is selected for preference in a specific vocabulary encoding scheme."@en .

<http://rdaregistry.info/Elements/n/P80102> a rdf:Property ;
    rdfs:label "is variant access point for collective agent of"@en ;
    rdakit:hasElementType "2" ;
    rdakit:toolkitDefinition "A collective agent who has an access point for collective agent that is not selected for preference in a specific vocabulary encoding scheme."@en ;
    rdakit:toolkitLabel "variant access point for collective agent of"@en ;
    reg:hasSubproperty <http://rdaregistry.info/Elements/n/P80104>,
        <http://rdaregistry.info/Elements/n/P80106>,
        <http://rdaregistry.info/Elements/n/datatype/P80102>,
        <http://rdaregistry.info/Elements/n/object/P80102> ;
    reg:hasUnconstrained <http://rdaregistry.info/Elements/u/P60934> ;
    reg:lexicalAlias <http://rdaregistry.info/Elements/n/variantAccessPointForCollectiveAgentOf.en> ;
    reg:name "variantAccessPointForCollectiveAgentOf"@en ;
    reg:status <http://metadataregistry.org/uri/RegStatus/1001> ;
    rdfs:domain <http://rdaregistry.info/Elements/c/C10012> ;
    rdfs:isDefinedBy <http://rdaregistry.info/Elements/n/> ;
    rdfs:subPropertyOf <http://rdaregistry.info/Elements/n/P80019>,
        <http://rdaregistry.info/Elements/n/P80100> ;
    skos:definition "Relates a nomen to a collective agent who has an access point for collective agent that is not selected for preference in a specific vocabulary encoding scheme."@en .

<http://rdaregistry.info/Elements/n/P80119> a rdf:Property ;
    rdfs:label "is numeric designation of musical work of"@en ;
    rdakit:hasElementType "2" ;
    rdakit:toolkitDefinition "A musical work that has an identifier for work that is a serial number, opus number, or thematic index number assigned to a musical work by a composer, publisher, or a musicologist. "@en ;
    rdakit:toolkitLabel "numeric designation of musical work of"@en ;
    reg:hasSubproperty <http://rdaregistry.info/Elements/n/P80120>,
        <http://rdaregistry.info/Elements/n/P80121>,
        <http://rdaregistry.info/Elements/n/P80122>,
        <http://rdaregistry.info/Elements/n/datatype/P80119> ;
    reg:hasUnconstrained <http://rdaregistry.info/Elements/u/P60963> ;
    reg:lexicalAlias <http://rdaregistry.info/Elements/n/numericDesignationOfMusicalWorkOf.en> ;
    reg:name "numericDesignationOfMusicalWorkOf"@en ;
    reg:status <http://metadataregistry.org/uri/RegStatus/1001> ;
    rdfs:domain <http://rdaregistry.info/Elements/c/C10012> ;
    rdfs:isDefinedBy <http://rdaregistry.info/Elements/n/> ;
    rdfs:subPropertyOf <http://rdaregistry.info/Elements/n/P80049> ;
    skos:definition "Relates a nomen to a musical work that has an identifier for work that is a serial number, opus number, or thematic index number assigned to a musical work by a composer, publisher, or a musicologist. "@en .

<http://rdaregistry.info/Elements/n/P80140> a rdf:Property ;
    rdfs:label "is preferred name of agent of"@en ;
    rdakit:hasElementType "2" ;
    rdakit:toolkitDefinition "An agent who has a name of agent that is selected for preference in a specific application or context."@en ;
    rdakit:toolkitLabel "preferred name of agent of"@en ;
    reg:hasSubproperty <http://rdaregistry.info/Elements/n/P80141>,
        <http://rdaregistry.info/Elements/n/P80146>,
        <http://rdaregistry.info/Elements/n/datatype/P80140> ;
    reg:hasUnconstrained <http://rdaregistry.info/Elements/u/P60927> ;
    reg:lexicalAlias <http://rdaregistry.info/Elements/n/preferredNameOfAgentOf.en> ;
    reg:name "preferredNameOfAgentOf"@en ;
    reg:status <http://metadataregistry.org/uri/RegStatus/1001> ;
    rdfs:domain <http://rdaregistry.info/Elements/c/C10012> ;
    rdfs:isDefinedBy <http://rdaregistry.info/Elements/n/> ;
    rdfs:subPropertyOf <http://rdaregistry.info/Elements/n/P80052>,
        <http://rdaregistry.info/Elements/n/P80163> ;
    skos:definition "Relates a nomen to an agent who has a name of agent that is selected for preference in a specific application or context."@en .

<http://rdaregistry.info/Elements/n/P80141> a rdf:Property ;
    rdfs:label "is preferred name of collective agent of"@en ;
    rdakit:hasElementType "2" ;
    rdakit:toolkitDefinition "A collective agent who has a name of collective agent that is selected for preference in a specific application or context."@en ;
    rdakit:toolkitLabel "preferred name of collective agent of"@en ;
    reg:hasSubproperty <http://rdaregistry.info/Elements/n/P80144>,
        <http://rdaregistry.info/Elements/n/P80145>,
        <http://rdaregistry.info/Elements/n/datatype/P80141> ;
    reg:hasUnconstrained <http://rdaregistry.info/Elements/u/P60927> ;
    reg:lexicalAlias <http://rdaregistry.info/Elements/n/preferredNameOfCollectiveAgentOf.en> ;
    reg:name "preferredNameOfCollectiveAgentOf"@en ;
    reg:status <http://metadataregistry.org/uri/RegStatus/1001> ;
    rdfs:domain <http://rdaregistry.info/Elements/c/C10012> ;
    rdfs:isDefinedBy <http://rdaregistry.info/Elements/n/> ;
    rdfs:subPropertyOf <http://rdaregistry.info/Elements/n/P80053>,
        <http://rdaregistry.info/Elements/n/P80140> ;
    skos:definition "Relates a nomen to a collective agent who has a name of collective agent that is selected for preference in a specific application or context."@en .

<http://rdaregistry.info/Elements/n/P80143> a rdf:Property ;
    rdfs:label "is variant name of collective agent of"@en ;
    rdakit:hasElementType "2" ;
    rdakit:toolkitDefinition "A collective agent who has a name of collective agent that is not selected for preference in a specific application or context."@en ;
    rdakit:toolkitLabel "variant name of collective agent of"@en ;
    reg:hasSubproperty <http://rdaregistry.info/Elements/n/P80147>,
        <http://rdaregistry.info/Elements/n/P80148>,
        <http://rdaregistry.info/Elements/n/datatype/P80143> ;
    reg:hasUnconstrained <http://rdaregistry.info/Elements/u/P60921> ;
    reg:lexicalAlias <http://rdaregistry.info/Elements/n/variantNameOfCollectiveAgentOf.en> ;
    reg:name "variantNameOfCollectiveAgentOf"@en ;
    reg:status <http://metadataregistry.org/uri/RegStatus/1001> ;
    rdfs:domain <http://rdaregistry.info/Elements/c/C10012> ;
    rdfs:isDefinedBy <http://rdaregistry.info/Elements/n/> ;
    rdfs:subPropertyOf <http://rdaregistry.info/Elements/n/P80053>,
        <http://rdaregistry.info/Elements/n/P80142> ;
    skos:definition "Relates a nomen to a collective agent who has a name of collective agent that is not selected for preference in a specific application or context."@en .

<http://rdaregistry.info/Elements/n/P80005> a rdf:Property ;
    rdfs:label "has related agent of nomen"@en ;
    rdakit:hasElementType "1" ;
    rdakit:toolkitDefinition "An agent who is associated with a nomen."@en ;
    rdakit:toolkitLabel "related agent of nomen"@en ;
    reg:hasSubproperty <http://rdaregistry.info/Elements/n/P80006>,
        <http://rdaregistry.info/Elements/n/P80011>,
        <http://rdaregistry.info/Elements/n/P80028>,
        <http://rdaregistry.info/Elements/n/P80073>,
        <http://rdaregistry.info/Elements/n/P80153>,
        <http://rdaregistry.info/Elements/n/datatype/P80005>,
        <http://rdaregistry.info/Elements/n/object/P80005> ;
    reg:hasUnconstrained <http://rdaregistry.info/Elements/u/P61027> ;
    reg:lexicalAlias <http://rdaregistry.info/Elements/n/relatedAgentOfNomen.en> ;
    reg:name "relatedAgentOfNomen"@en ;
    reg:status <http://metadataregistry.org/uri/RegStatus/1001> ;
    rdfs:domain <http://rdaregistry.info/Elements/c/C10012> ;
    rdfs:isDefinedBy <http://rdaregistry.info/Elements/n/> ;
    rdfs:subPropertyOf <http://rdaregistry.info/Elements/n/P80010>,
        <http://rdaregistry.info/Elements/x/P00006> ;
    skos:definition "Relates a nomen to an agent who is associated with a nomen."@en .

<http://rdaregistry.info/Elements/n/P80006> a rdf:Property ;
    rdfs:label "has related collective agent of nomen"@en ;
    rdakit:hasElementType "1" ;
    rdakit:toolkitDefinition "A collective agent who is associated with a nomen."@en ;
    rdakit:toolkitLabel "related collective agent of nomen"@en ;
    reg:hasSubproperty <http://rdaregistry.info/Elements/n/P80012>,
        <http://rdaregistry.info/Elements/n/P80013>,
        <http://rdaregistry.info/Elements/n/P80029>,
        <http://rdaregistry.info/Elements/n/P80074>,
        <http://rdaregistry.info/Elements/n/P80154>,
        <http://rdaregistry.info/Elements/n/datatype/P80006>,
        <http://rdaregistry.info/Elements/n/object/P80006> ;
    reg:hasUnconstrained <http://rdaregistry.info/Elements/u/P61027> ;
    reg:lexicalAlias <http://rdaregistry.info/Elements/n/relatedCollectiveAgentOfNomen.en> ;
    reg:name "relatedCollectiveAgentOfNomen"@en ;
    reg:status <http://metadataregistry.org/uri/RegStatus/1001> ;
    rdfs:domain <http://rdaregistry.info/Elements/c/C10012> ;
    rdfs:isDefinedBy <http://rdaregistry.info/Elements/n/> ;
    rdfs:subPropertyOf <http://rdaregistry.info/Elements/n/P80005>,
        <http://rdaregistry.info/Elements/x/P00012> ;
    skos:definition "Relates a nomen to a collective agent who is associated with a nomen."@en .

<http://rdaregistry.info/Elements/n/P80016> a rdf:Property ;
    rdfs:label "is appellation of item of"@en ;
    rdakit:hasElementType "2" ;
    rdakit:toolkitDefinition "An item that is referred to by a nomen used within a given scheme or context."@en ;
    rdakit:toolkitLabel "appellation of item of"@en ;
    reg:hasSubproperty <http://rdaregistry.info/Elements/n/datatype/P80016>,
        <http://rdaregistry.info/Elements/n/object/P80016> ;
    reg:hasUnconstrained <http://rdaregistry.info/Elements/u/P60911> ;
    reg:lexicalAlias <http://rdaregistry.info/Elements/n/appellationOfItemOf.en> ;
    reg:name "appellationOfItemOf"@en ;
    reg:status <http://metadataregistry.org/uri/RegStatus/1001> ;
    rdfs:domain <http://rdaregistry.info/Elements/c/C10012> ;
    rdfs:isDefinedBy <http://rdaregistry.info/Elements/n/> ;
    rdfs:subPropertyOf <http://rdaregistry.info/Elements/n/P80004>,
        <http://rdaregistry.info/Elements/n/P80112> ;
    skos:definition "Relates a nomen to an item that is referred to by a nomen used within a given scheme or context."@en .

<http://rdaregistry.info/Elements/n/P80018> a rdf:Property ;
    rdfs:label "is access point for agent of"@en ;
    rdakit:hasElementType "2" ;
    rdakit:toolkitDefinition "An agent who has an appellation in natural language that is taken from a vocabulary encoding scheme or is constructed using a string encoding scheme."@en ;
    rdakit:toolkitLabel "access point for agent of"@en ;
    reg:hasSubproperty <http://rdaregistry.info/Elements/n/P80019>,
        <http://rdaregistry.info/Elements/n/P80022>,
        <http://rdaregistry.info/Elements/n/P80100>,
        <http://rdaregistry.info/Elements/n/datatype/P80018>,
        <http://rdaregistry.info/Elements/n/object/P80018> ;
    reg:hasUnconstrained <http://rdaregistry.info/Elements/u/P60910> ;
    reg:lexicalAlias <http://rdaregistry.info/Elements/n/accessPointForAgentOf.en> ;
    reg:name "accessPointForAgentOf"@en ;
    reg:status <http://metadataregistry.org/uri/RegStatus/1001> ;
    rdfs:domain <http://rdaregistry.info/Elements/c/C10012> ;
    rdfs:isDefinedBy <http://rdaregistry.info/Elements/n/> ;
    rdfs:subPropertyOf <http://rdaregistry.info/Elements/n/P80028>,
        <http://rdaregistry.info/Elements/n/P80159> ;
    skos:definition "Relates a nomen to an agent who has an appellation in natural language that is taken from a vocabulary encoding scheme or is constructed using a string encoding scheme."@en .

<http://rdaregistry.info/Elements/n/P80030> a rdf:Property ;
    rdfs:label "is appellation of corporate body of"@en ;
    rdakit:hasElementType "2" ;
    rdakit:toolkitDefinition "A corporate body who is referred to by a nomen used within a given scheme or context."@en ;
    rdakit:toolkitLabel "appellation of corporate body of"@en ;
    reg:hasSubproperty <http://rdaregistry.info/Elements/n/P80020>,
        <http://rdaregistry.info/Elements/n/P80035>,
        <http://rdaregistry.info/Elements/n/P80054>,
        <http://rdaregistry.info/Elements/n/datatype/P80030>,
        <http://rdaregistry.info/Elements/n/object/P80030> ;
    reg:hasUnconstrained <http://rdaregistry.info/Elements/u/P60911> ;
    reg:lexicalAlias <http://rdaregistry.info/Elements/n/appellationOfCorporateBodyOf.en> ;
    reg:name "appellationOfCorporateBodyOf"@en ;
    reg:status <http://metadataregistry.org/uri/RegStatus/1001> ;
    rdfs:domain <http://rdaregistry.info/Elements/c/C10012> ;
    rdfs:isDefinedBy <http://rdaregistry.info/Elements/n/> ;
    rdfs:subPropertyOf <http://rdaregistry.info/Elements/n/P80013>,
        <http://rdaregistry.info/Elements/n/P80029> ;
    skos:definition "Relates a nomen to a corporate body who is referred to by a nomen used within a given scheme or context."@en .

<http://rdaregistry.info/Elements/n/P80031> a rdf:Property ;
    rdfs:label "is appellation of family of"@en ;
    rdakit:hasElementType "2" ;
    rdakit:toolkitDefinition "A family who is referred to by a nomen used within a given scheme or context."@en ;
    rdakit:toolkitLabel "appellation of family of"@en ;
    reg:hasSubproperty <http://rdaregistry.info/Elements/n/P80021>,
        <http://rdaregistry.info/Elements/n/P80036>,
        <http://rdaregistry.info/Elements/n/P80055>,
        <http://rdaregistry.info/Elements/n/datatype/P80031>,
        <http://rdaregistry.info/Elements/n/object/P80031> ;
    reg:hasUnconstrained <http://rdaregistry.info/Elements/u/P60911> ;
    reg:lexicalAlias <http://rdaregistry.info/Elements/n/appellationOfFamilyOf.en> ;
    reg:name "appellationOfFamilyOf"@en ;
    reg:status <http://metadataregistry.org/uri/RegStatus/1001> ;
    rdfs:domain <http://rdaregistry.info/Elements/c/C10012> ;
    rdfs:isDefinedBy <http://rdaregistry.info/Elements/n/> ;
    rdfs:subPropertyOf <http://rdaregistry.info/Elements/n/P80012>,
        <http://rdaregistry.info/Elements/n/P80029> ;
    skos:definition "Relates a nomen to a family who is referred to by a nomen used within a given scheme or context."@en .

<http://rdaregistry.info/Elements/n/P80038> a rdf:Property ;
    rdfs:label "is appellation of expression of"@en ;
    rdakit:hasElementType "2" ;
    rdakit:toolkitDefinition "An expression that is referred to by a nomen used within a given scheme or context."@en ;
    rdakit:toolkitLabel "appellation of expression of"@en ;
    reg:hasSubproperty <http://rdaregistry.info/Elements/n/datatype/P80038>,
        <http://rdaregistry.info/Elements/n/object/P80038> ;
    reg:hasUnconstrained <http://rdaregistry.info/Elements/u/P60911> ;
    reg:lexicalAlias <http://rdaregistry.info/Elements/n/appellationOfExpressionOf.en> ;
    reg:name "appellationOfExpressionOf"@en ;
    reg:status <http://metadataregistry.org/uri/RegStatus/1001> ;
    rdfs:domain <http://rdaregistry.info/Elements/c/C10012> ;
    rdfs:isDefinedBy <http://rdaregistry.info/Elements/n/> ;
    rdfs:subPropertyOf <http://rdaregistry.info/Elements/n/P80002>,
        <http://rdaregistry.info/Elements/n/P80112> ;
    skos:definition "Relates a nomen to an expression that is referred to by a nomen used within a given scheme or context."@en .

<http://rdaregistry.info/Elements/n/P80040> a rdf:Property ;
    rdfs:label "is appellation of manifestation of"@en ;
    rdakit:hasElementType "2" ;
    rdakit:toolkitDefinition "A manifestation that is referred to by a nomen used within a given scheme or context."@en ;
    rdakit:toolkitLabel "appellation of manifestation of"@en ;
    reg:hasSubproperty <http://rdaregistry.info/Elements/n/datatype/P80040>,
        <http://rdaregistry.info/Elements/n/object/P80040> ;
    reg:hasUnconstrained <http://rdaregistry.info/Elements/u/P60911> ;
    reg:lexicalAlias <http://rdaregistry.info/Elements/n/appellationOfManifestationOf.en> ;
    reg:name "appellationOfManifestationOf"@en ;
    reg:status <http://metadataregistry.org/uri/RegStatus/1001> ;
    rdfs:domain <http://rdaregistry.info/Elements/c/C10012> ;
    rdfs:isDefinedBy <http://rdaregistry.info/Elements/n/> ;
    rdfs:subPropertyOf <http://rdaregistry.info/Elements/n/P80003>,
        <http://rdaregistry.info/Elements/n/P80112> ;
    skos:definition "Relates a nomen to a manifestation that is referred to by a nomen used within a given scheme or context."@en .

<http://rdaregistry.info/Elements/n/P80041> a rdf:Property ;
    rdfs:label "is appellation of place of"@en ;
    rdakit:hasElementType "2" ;
    rdakit:toolkitDefinition "A place that is referred to by a nomen used within a given scheme or context."@en ;
    rdakit:toolkitLabel "appellation of place of"@en ;
    reg:hasSubproperty <http://rdaregistry.info/Elements/n/datatype/P80041>,
        <http://rdaregistry.info/Elements/n/object/P80041> ;
    reg:hasUnconstrained <http://rdaregistry.info/Elements/u/P60911> ;
    reg:lexicalAlias <http://rdaregistry.info/Elements/n/appellationOfPlaceOf.en> ;
    reg:name "appellationOfPlaceOf"@en ;
    reg:status <http://metadataregistry.org/uri/RegStatus/1001> ;
    rdfs:domain <http://rdaregistry.info/Elements/c/C10012> ;
    rdfs:isDefinedBy <http://rdaregistry.info/Elements/n/> ;
    rdfs:subPropertyOf <http://rdaregistry.info/Elements/n/P80007>,
        <http://rdaregistry.info/Elements/n/P80112> ;
    skos:definition "Relates a nomen to a place that is referred to by a nomen used within a given scheme or context."@en .

<http://rdaregistry.info/Elements/n/P80043> a rdf:Property ;
    rdfs:label "is appellation of timespan of"@en ;
    rdakit:hasElementType "2" ;
    rdakit:toolkitDefinition "A timespan that is referred to by a nomen used within a given scheme or context."@en ;
    rdakit:toolkitLabel "appellation of timespan of"@en ;
    reg:hasSubproperty <http://rdaregistry.info/Elements/n/datatype/P80043>,
        <http://rdaregistry.info/Elements/n/object/P80043> ;
    reg:hasUnconstrained <http://rdaregistry.info/Elements/u/P60911> ;
    reg:lexicalAlias <http://rdaregistry.info/Elements/n/appellationOfTimespanOf.en> ;
    reg:name "appellationOfTimespanOf"@en ;
    reg:status <http://metadataregistry.org/uri/RegStatus/1001> ;
    rdfs:domain <http://rdaregistry.info/Elements/c/C10012> ;
    rdfs:isDefinedBy <http://rdaregistry.info/Elements/n/> ;
    rdfs:subPropertyOf <http://rdaregistry.info/Elements/n/P80008>,
        <http://rdaregistry.info/Elements/n/P80112> ;
    skos:definition "Relates a nomen to a timespan that is referred to by a nomen used within a given scheme or context."@en .

<http://rdaregistry.info/Elements/n/P80009> a rdf:Property ;
    rdfs:label "has related nomen of nomen"@en ;
    rdakit:hasElementType "1" ;
    rdakit:toolkitDefinition "A nomen that is associated with a nomen."@en ;
    rdakit:toolkitLabel "related nomen of nomen"@en ;
    reg:hasSubproperty <http://rdaregistry.info/Elements/n/P80058>,
        <http://rdaregistry.info/Elements/n/P80059>,
        <http://rdaregistry.info/Elements/n/P80060>,
        <http://rdaregistry.info/Elements/n/P80061>,
        <http://rdaregistry.info/Elements/n/P80113>,
        <http://rdaregistry.info/Elements/n/datatype/P80009>,
        <http://rdaregistry.info/Elements/n/object/P80009> ;
    reg:hasUnconstrained <http://rdaregistry.info/Elements/u/P61026> ;
    reg:lexicalAlias <http://rdaregistry.info/Elements/n/relatedNomenOfNomen.en> ;
    reg:name "relatedNomenOfNomen"@en ;
    reg:status <http://metadataregistry.org/uri/RegStatus/1001> ;
    rdfs:domain <http://rdaregistry.info/Elements/c/C10012> ;
    rdfs:isDefinedBy <http://rdaregistry.info/Elements/n/> ;
    rdfs:subPropertyOf <http://rdaregistry.info/Elements/n/P80010>,
        <http://rdaregistry.info/Elements/x/P00013> ;
    skos:definition "Relates a nomen to a nomen that is associated with a nomen."@en .

<http://rdaregistry.info/Elements/n/P80019> a rdf:Property ;
    rdfs:label "is access point for collective agent of"@en ;
    rdakit:hasElementType "2" ;
    rdakit:toolkitDefinition "A collective agent who has an appellation in natural language that is taken from a vocabulary encoding scheme or is constructed using a string encoding scheme."@en ;
    rdakit:toolkitLabel "access point for collective agent of"@en ;
    reg:hasSubproperty <http://rdaregistry.info/Elements/n/P80020>,
        <http://rdaregistry.info/Elements/n/P80021>,
        <http://rdaregistry.info/Elements/n/P80101>,
        <http://rdaregistry.info/Elements/n/P80102>,
        <http://rdaregistry.info/Elements/n/datatype/P80019>,
        <http://rdaregistry.info/Elements/n/object/P80019> ;
    reg:hasUnconstrained <http://rdaregistry.info/Elements/u/P60910> ;
    reg:lexicalAlias <http://rdaregistry.info/Elements/n/accessPointForCollectiveAgentOf.en> ;
    reg:name "accessPointForCollectiveAgentOf"@en ;
    reg:status <http://metadataregistry.org/uri/RegStatus/1001> ;
    rdfs:domain <http://rdaregistry.info/Elements/c/C10012> ;
    rdfs:isDefinedBy <http://rdaregistry.info/Elements/n/> ;
    rdfs:subPropertyOf <http://rdaregistry.info/Elements/n/P80018>,
        <http://rdaregistry.info/Elements/n/P80029> ;
    skos:definition "Relates a nomen to a collective agent who has an appellation in natural language that is taken from a vocabulary encoding scheme or is constructed using a string encoding scheme."@en .

<http://rdaregistry.info/Elements/n/P80045> a rdf:Property ;
    rdfs:label "is appellation of work of"@en ;
    rdakit:hasElementType "2" ;
    rdakit:toolkitDefinition "A work that is referred to by a nomen used within a given scheme or context."@en ;
    rdakit:toolkitLabel "appellation of work of"@en ;
    reg:hasSubproperty <http://rdaregistry.info/Elements/n/P80171>,
        <http://rdaregistry.info/Elements/n/datatype/P80045>,
        <http://rdaregistry.info/Elements/n/object/P80045> ;
    reg:hasUnconstrained <http://rdaregistry.info/Elements/u/P60911> ;
    reg:lexicalAlias <http://rdaregistry.info/Elements/n/appellationOfWorkOf.en> ;
    reg:name "appellationOfWorkOf"@en ;
    reg:status <http://metadataregistry.org/uri/RegStatus/1001> ;
    rdfs:domain <http://rdaregistry.info/Elements/c/C10012> ;
    rdfs:isDefinedBy <http://rdaregistry.info/Elements/n/> ;
    rdfs:subPropertyOf <http://rdaregistry.info/Elements/n/P80001>,
        <http://rdaregistry.info/Elements/n/P80112> ;
    skos:definition "Relates a nomen to a work that is referred to by a nomen used within a given scheme or context."@en .

<http://rdaregistry.info/Elements/n/P80052> a rdf:Property ;
    rdfs:label "is name of agent of"@en ;
    rdakit:hasElementType "2" ;
    rdakit:toolkitDefinition "An agent who has an appellation of agent in natural language and phrasing used in common discourse."@en ;
    rdakit:toolkitLabel "name of agent of"@en ;
    reg:hasSubproperty <http://rdaregistry.info/Elements/n/P80053>,
        <http://rdaregistry.info/Elements/n/P80056>,
        <http://rdaregistry.info/Elements/n/P80114>,
        <http://rdaregistry.info/Elements/n/P80140>,
        <http://rdaregistry.info/Elements/n/datatype/P80052>,
        <http://rdaregistry.info/Elements/n/object/P80052> ;
    reg:hasUnconstrained <http://rdaregistry.info/Elements/u/P60920> ;
    reg:lexicalAlias <http://rdaregistry.info/Elements/n/nameOfAgentOf.en> ;
    reg:name "nameOfAgentOf"@en ;
    reg:status <http://metadataregistry.org/uri/RegStatus/1001> ;
    rdfs:domain <http://rdaregistry.info/Elements/c/C10012> ;
    rdfs:isDefinedBy <http://rdaregistry.info/Elements/n/> ;
    rdfs:subPropertyOf <http://rdaregistry.info/Elements/n/P80028>,
        <http://rdaregistry.info/Elements/n/P80161> ;
    skos:definition "Relates a nomen to an agent who has an appellation of agent in natural language and phrasing used in common discourse."@en .

<http://rdaregistry.info/Elements/n/P80053> a rdf:Property ;
    rdfs:label "is name of collective agent of"@en ;
    rdakit:hasElementType "2" ;
    rdakit:toolkitDefinition "A collective agent who has an appellation of collective agent in natural language and phrasing used in common discourse."@en ;
    rdakit:toolkitLabel "name of collective agent of"@en ;
    reg:hasSubproperty <http://rdaregistry.info/Elements/n/P80054>,
        <http://rdaregistry.info/Elements/n/P80055>,
        <http://rdaregistry.info/Elements/n/P80141>,
        <http://rdaregistry.info/Elements/n/P80143>,
        <http://rdaregistry.info/Elements/n/datatype/P80053>,
        <http://rdaregistry.info/Elements/n/object/P80053> ;
    reg:hasUnconstrained <http://rdaregistry.info/Elements/u/P60920> ;
    reg:lexicalAlias <http://rdaregistry.info/Elements/n/nameOfCollectiveAgentOf.en> ;
    reg:name "nameOfCollectiveAgentOf"@en ;
    reg:status <http://metadataregistry.org/uri/RegStatus/1001> ;
    rdfs:domain <http://rdaregistry.info/Elements/c/C10012> ;
    rdfs:isDefinedBy <http://rdaregistry.info/Elements/n/> ;
    rdfs:subPropertyOf <http://rdaregistry.info/Elements/n/P80029>,
        <http://rdaregistry.info/Elements/n/P80052> ;
    skos:definition "Relates a nomen to a collective agent who has an appellation of collective agent in natural language and phrasing used in common discourse."@en .

<http://rdaregistry.info/Elements/n/P80114> a rdf:Property ;
    rdfs:label "is name of agent of manifestation of"@en ;
    rdakit:hasElementType "2" ;
    rdakit:toolkitDefinition "A manifestation that has a name of agent who is responsible for distribution, printing, duplication, casting, publication, release, issue, etc., or inscription, fabrication, construction, etc."@en ;
    rdakit:toolkitLabel "name of agent of manifestation of"@en ;
    reg:hasSubproperty <http://rdaregistry.info/Elements/n/P80115>,
        <http://rdaregistry.info/Elements/n/P80116>,
        <http://rdaregistry.info/Elements/n/P80117>,
        <http://rdaregistry.info/Elements/n/P80118>,
        <http://rdaregistry.info/Elements/n/datatype/P80114>,
        <http://rdaregistry.info/Elements/n/object/P80114> ;
    reg:lexicalAlias <http://rdaregistry.info/Elements/n/nameOfAgentOfManifestationOf.en> ;
    reg:name "nameOfAgentOfManifestationOf"@en ;
    reg:status <http://metadataregistry.org/uri/RegStatus/1001> ;
    rdfs:domain <http://rdaregistry.info/Elements/c/C10012> ;
    rdfs:isDefinedBy <http://rdaregistry.info/Elements/n/> ;
    rdfs:subPropertyOf <http://rdaregistry.info/Elements/n/P80003>,
        <http://rdaregistry.info/Elements/n/P80052> ;
    skos:definition "Relates a nomen to a manifestation that has a name of agent who is responsible for distribution, printing, duplication, casting, publication, release, issue, etc., or inscription, fabrication, construction, etc."@en .

<http://rdaregistry.info/Elements/n/P80028> a rdf:Property ;
    rdfs:label "is appellation of agent of"@en ;
    rdakit:hasElementType "2" ;
    rdakit:toolkitDefinition "An agent who is referred to by a nomen used within a given scheme or context."@en ;
    rdakit:toolkitLabel "appellation of agent of"@en ;
    reg:hasSubproperty <http://rdaregistry.info/Elements/n/P80029>,
        <http://rdaregistry.info/Elements/n/P80032>,
        <http://rdaregistry.info/Elements/n/datatype/P80028>,
        <http://rdaregistry.info/Elements/n/object/P80028> ;
    reg:hasUnconstrained <http://rdaregistry.info/Elements/u/P60911> ;
    reg:lexicalAlias <http://rdaregistry.info/Elements/n/appellationOfAgentOf.en> ;
    reg:name "appellationOfAgentOf"@en ;
    reg:status <http://metadataregistry.org/uri/RegStatus/1001> ;
    rdfs:domain <http://rdaregistry.info/Elements/c/C10012> ;
    rdfs:isDefinedBy <http://rdaregistry.info/Elements/n/> ;
    rdfs:subPropertyOf <http://rdaregistry.info/Elements/n/P80005>,
        <http://rdaregistry.info/Elements/n/P80112> ;
    skos:definition "Relates a nomen to an agent who is referred to by a nomen used within a given scheme or context."@en .

<http://rdaregistry.info/Elements/n/P80029> a rdf:Property ;
    rdfs:label "is appellation of collective agent of"@en ;
    rdakit:hasElementType "2" ;
    rdakit:toolkitDefinition "A collective agent who is referred to by a nomen used within a given scheme or context."@en ;
    rdakit:toolkitLabel "appellation of collective agent of"@en ;
    reg:hasSubproperty <http://rdaregistry.info/Elements/n/P80019>,
        <http://rdaregistry.info/Elements/n/P80030>,
        <http://rdaregistry.info/Elements/n/P80031>,
        <http://rdaregistry.info/Elements/n/P80034>,
        <http://rdaregistry.info/Elements/n/P80053>,
        <http://rdaregistry.info/Elements/n/datatype/P80029>,
        <http://rdaregistry.info/Elements/n/object/P80029> ;
    reg:hasUnconstrained <http://rdaregistry.info/Elements/u/P60911> ;
    reg:lexicalAlias <http://rdaregistry.info/Elements/n/appellationOfCollectiveAgentOf.en> ;
    reg:name "appellationOfCollectiveAgentOf"@en ;
    reg:status <http://metadataregistry.org/uri/RegStatus/1001> ;
    rdfs:domain <http://rdaregistry.info/Elements/c/C10012> ;
    rdfs:isDefinedBy <http://rdaregistry.info/Elements/n/> ;
    rdfs:subPropertyOf <http://rdaregistry.info/Elements/n/P80006>,
        <http://rdaregistry.info/Elements/n/P80028> ;
    skos:definition "Relates a nomen to a collective agent who is referred to by a nomen used within a given scheme or context."@en .

<http://rdaregistry.info/Elements/n/P80032> a rdf:Property ;
    rdfs:label "is appellation of person of"@en ;
    rdakit:hasElementType "2" ;
    rdakit:toolkitDefinition "A person who is referred to by a nomen used within a given scheme or context."@en ;
    rdakit:toolkitLabel "appellation of person of"@en ;
    reg:hasSubproperty <http://rdaregistry.info/Elements/n/P80022>,
        <http://rdaregistry.info/Elements/n/P80037>,
        <http://rdaregistry.info/Elements/n/P80056>,
        <http://rdaregistry.info/Elements/n/P80157>,
        <http://rdaregistry.info/Elements/n/P80158>,
        <http://rdaregistry.info/Elements/n/datatype/P80032>,
        <http://rdaregistry.info/Elements/n/object/P80032> ;
    reg:hasUnconstrained <http://rdaregistry.info/Elements/u/P60911> ;
    reg:lexicalAlias <http://rdaregistry.info/Elements/n/appellationOfPersonOf.en> ;
    reg:name "appellationOfPersonOf"@en ;
    reg:status <http://metadataregistry.org/uri/RegStatus/1001> ;
    rdfs:domain <http://rdaregistry.info/Elements/c/C10012> ;
    rdfs:isDefinedBy <http://rdaregistry.info/Elements/n/> ;
    rdfs:subPropertyOf <http://rdaregistry.info/Elements/n/P80011>,
        <http://rdaregistry.info/Elements/n/P80028> ;
    skos:definition "Relates a nomen to a person who is referred to by a nomen used within a given scheme or context."@en .

<http://rdaregistry.info/Elements/n/P80056> a rdf:Property ;
    rdfs:label "is name of person of"@en ;
    rdakit:hasElementType "2" ;
    rdakit:toolkitDefinition "A person who has an appellation of person in natural language and phrasing used in common discourse."@en ;
    rdakit:toolkitLabel "name of person of"@en ;
    reg:hasSubproperty <http://rdaregistry.info/Elements/n/P80146>,
        <http://rdaregistry.info/Elements/n/P80149>,
        <http://rdaregistry.info/Elements/n/P80175>,
        <http://rdaregistry.info/Elements/n/P80176>,
        <http://rdaregistry.info/Elements/n/P80177>,
        <http://rdaregistry.info/Elements/n/datatype/P80056>,
        <http://rdaregistry.info/Elements/n/object/P80056> ;
    reg:hasUnconstrained <http://rdaregistry.info/Elements/u/P60920> ;
    reg:lexicalAlias <http://rdaregistry.info/Elements/n/nameOfPersonOf.en> ;
    reg:name "nameOfPersonOf"@en ;
    reg:status <http://metadataregistry.org/uri/RegStatus/1001> ;
    rdfs:domain <http://rdaregistry.info/Elements/c/C10012> ;
    rdfs:isDefinedBy <http://rdaregistry.info/Elements/n/> ;
    rdfs:subPropertyOf <http://rdaregistry.info/Elements/n/P80032>,
        <http://rdaregistry.info/Elements/n/P80052> ;
    skos:definition "Relates a nomen to a person who has an appellation of person in natural language and phrasing used in common discourse."@en .

<http://rdaregistry.info/Elements/n/P80163> a rdf:Property ;
    rdfs:label "is preferred name of RDA entity of"@en ;
    rdakit:hasElementType "2" ;
    rdakit:toolkitDefinition "An RDA entity that has a name of RDA entity that is selected for preference in a specific application or context."@en ;
    rdakit:toolkitLabel "preferred name of RDA entity of"@en ;
    reg:hasSubproperty <http://rdaregistry.info/Elements/n/P80083>,
        <http://rdaregistry.info/Elements/n/P80087>,
        <http://rdaregistry.info/Elements/n/P80093>,
        <http://rdaregistry.info/Elements/n/P80097>,
        <http://rdaregistry.info/Elements/n/P80109>,
        <http://rdaregistry.info/Elements/n/P80140>,
        <http://rdaregistry.info/Elements/n/datatype/P80163> ;
    reg:hasUnconstrained <http://rdaregistry.info/Elements/u/P60951> ;
    reg:lexicalAlias <http://rdaregistry.info/Elements/n/preferredNameOfRDAEntityOf.en> ;
    reg:name "preferredNameOfRDAEntityOf"@en ;
    reg:status <http://metadataregistry.org/uri/RegStatus/1001> ;
    rdfs:domain <http://rdaregistry.info/Elements/c/C10012> ;
    rdfs:isDefinedBy <http://rdaregistry.info/Elements/n/> ;
    rdfs:subPropertyOf <http://rdaregistry.info/Elements/n/P80161> ;
    skos:definition "Relates a nomen to an RDA entity that has a name of RDA entity that is selected for preference in a specific application or context."@en .

<http://rdaregistry.info/Elements/n/P80160> a rdf:Property ;
    rdfs:label "is identifier for RDA entity of"@en ;
    rdakit:hasElementType "2" ;
    rdakit:toolkitDefinition "An RDA entity that has an appellation of work that is a reference code taken from a vocabulary encoding scheme."@en ;
    rdakit:toolkitLabel "identifier for RDA entity of"@en ;
    reg:hasSubproperty <http://rdaregistry.info/Elements/n/P80033>,
        <http://rdaregistry.info/Elements/n/P80042>,
        <http://rdaregistry.info/Elements/n/P80046>,
        <http://rdaregistry.info/Elements/n/P80047>,
        <http://rdaregistry.info/Elements/n/P80048>,
        <http://rdaregistry.info/Elements/n/P80049>,
        <http://rdaregistry.info/Elements/n/P80050>,
        <http://rdaregistry.info/Elements/n/datatype/P80160> ;
    reg:hasUnconstrained <http://rdaregistry.info/Elements/u/P60928> ;
    reg:lexicalAlias <http://rdaregistry.info/Elements/n/identifierForRDAEntityOf.en> ;
    reg:name "identifierForRDAEntityOf"@en ;
    reg:status <http://metadataregistry.org/uri/RegStatus/1001> ;
    rdfs:domain <http://rdaregistry.info/Elements/c/C10012> ;
    rdfs:isDefinedBy <http://rdaregistry.info/Elements/n/> ;
    rdfs:subPropertyOf <http://rdaregistry.info/Elements/n/P80112> ;
    skos:definition "Relates a nomen to an RDA entity that has an appellation of RDA Entity that is a reference code taken from a vocabulary encoding scheme."@en .

<http://rdaregistry.info/Elements/n/P80162> a rdf:Property ;
    rdfs:label "is authorized access point for RDA entity of"@en ;
    rdakit:hasElementType "2" ;
    rdakit:toolkitDefinition "An RDA entity that has an access point for RDA entity that is selected for preference in a specific vocabulary encoding scheme."@en ;
    rdakit:toolkitLabel "authorized access point for RDA entity of"@en ;
    reg:hasSubproperty <http://rdaregistry.info/Elements/n/P80079>,
        <http://rdaregistry.info/Elements/n/P80081>,
        <http://rdaregistry.info/Elements/n/P80085>,
        <http://rdaregistry.info/Elements/n/P80089>,
        <http://rdaregistry.info/Elements/n/P80091>,
        <http://rdaregistry.info/Elements/n/P80095>,
        <http://rdaregistry.info/Elements/n/P80099>,
        <http://rdaregistry.info/Elements/n/datatype/P80162> ;
    reg:hasUnconstrained <http://rdaregistry.info/Elements/u/P60918> ;
    reg:lexicalAlias <http://rdaregistry.info/Elements/n/authorizedAccessPointForRDAEntityOf.en> ;
    reg:name "authorizedAccessPointForRDAEntityOf"@en ;
    reg:status <http://metadataregistry.org/uri/RegStatus/1001> ;
    rdfs:domain <http://rdaregistry.info/Elements/c/C10012> ;
    rdfs:isDefinedBy <http://rdaregistry.info/Elements/n/> ;
    rdfs:subPropertyOf <http://rdaregistry.info/Elements/n/P80159> ;
    skos:definition "Relates a nomen to an RDA entity that has an access point for RDA entity that is selected for preference in a specific vocabulary encoding scheme."@en .

<http://rdaregistry.info/Elements/n/P80164> a rdf:Property ;
    rdfs:label "is variant name of RDA entity of"@en ;
    rdakit:hasElementType "2" ;
    rdakit:toolkitDefinition "An RDA entity that has a name of RDA entity that is not selected for preference in a specific application or context."@en ;
    rdakit:toolkitLabel "variant name of RDA entity of"@en ;
    reg:hasSubproperty <http://rdaregistry.info/Elements/n/P80084>,
        <http://rdaregistry.info/Elements/n/P80088>,
        <http://rdaregistry.info/Elements/n/P80094>,
        <http://rdaregistry.info/Elements/n/P80098>,
        <http://rdaregistry.info/Elements/n/P80110>,
        <http://rdaregistry.info/Elements/n/P80111>,
        <http://rdaregistry.info/Elements/n/P80142>,
        <http://rdaregistry.info/Elements/n/datatype/P80164> ;
    reg:hasUnconstrained <http://rdaregistry.info/Elements/u/P60952> ;
    reg:lexicalAlias <http://rdaregistry.info/Elements/n/variantNameOfRDAEntityOf.en> ;
    reg:name "variantNameOfRDAEntityOf"@en ;
    reg:status <http://metadataregistry.org/uri/RegStatus/1001> ;
    rdfs:domain <http://rdaregistry.info/Elements/c/C10012> ;
    rdfs:isDefinedBy <http://rdaregistry.info/Elements/n/> ;
    rdfs:subPropertyOf <http://rdaregistry.info/Elements/n/P80161> ;
    skos:definition "Relates a nomen to an RDA entity that has a name of RDA entity that is not selected for preference in a specific application or context."@en .

<http://rdaregistry.info/Elements/n/P80165> a rdf:Property ;
    rdfs:label "is variant access point for RDA entity of"@en ;
    rdakit:hasElementType "2" ;
    rdakit:toolkitDefinition "An RDA entity that has an access point for RDA entity that is not selected for preference in a specific vocabulary encoding scheme."@en ;
    rdakit:toolkitLabel "variant access point for RDA entity of"@en ;
    reg:hasSubproperty <http://rdaregistry.info/Elements/n/P80080>,
        <http://rdaregistry.info/Elements/n/P80082>,
        <http://rdaregistry.info/Elements/n/P80086>,
        <http://rdaregistry.info/Elements/n/P80090>,
        <http://rdaregistry.info/Elements/n/P80092>,
        <http://rdaregistry.info/Elements/n/P80096>,
        <http://rdaregistry.info/Elements/n/P80100>,
        <http://rdaregistry.info/Elements/n/datatype/P80165> ;
    reg:hasUnconstrained <http://rdaregistry.info/Elements/u/P60952> ;
    reg:lexicalAlias <http://rdaregistry.info/Elements/n/variantAccessPointForRDAEntityOf.en> ;
    reg:name "variantAccessPointForRDAEntityOf"@en ;
    reg:status <http://metadataregistry.org/uri/RegStatus/1001> ;
    rdfs:domain <http://rdaregistry.info/Elements/c/C10012> ;
    rdfs:isDefinedBy <http://rdaregistry.info/Elements/n/> ;
    rdfs:subPropertyOf <http://rdaregistry.info/Elements/n/P80159> ;
    skos:definition "Relates a nomen to an RDA entity that has an access point for entity that is not selected for preference in a specific vocabulary encoding scheme."@en .

<http://rdaregistry.info/Elements/n/P80010> a rdf:Property ;
    rdfs:label "has related RDA entity of nomen"@en ;
    rdakit:hasElementType "1" ;
    rdakit:toolkitDefinition "An RDA entity that is associated with a nomen."@en ;
    rdakit:toolkitLabel "related RDA entity of nomen"@en ;
    reg:hasSubproperty <http://rdaregistry.info/Elements/n/P80001>,
        <http://rdaregistry.info/Elements/n/P80002>,
        <http://rdaregistry.info/Elements/n/P80003>,
        <http://rdaregistry.info/Elements/n/P80004>,
        <http://rdaregistry.info/Elements/n/P80005>,
        <http://rdaregistry.info/Elements/n/P80007>,
        <http://rdaregistry.info/Elements/n/P80008>,
        <http://rdaregistry.info/Elements/n/P80009>,
        <http://rdaregistry.info/Elements/n/P80112>,
        <http://rdaregistry.info/Elements/n/datatype/P80010>,
        <http://rdaregistry.info/Elements/n/object/P80010> ;
    reg:hasUnconstrained <http://rdaregistry.info/Elements/u/P61037> ;
    reg:lexicalAlias <http://rdaregistry.info/Elements/n/relatedRDAEntityOfNomen.en> ;
    reg:name "relatedRDAEntityOfNomen"@en ;
    reg:status <http://metadataregistry.org/uri/RegStatus/1001> ;
    rdfs:domain <http://rdaregistry.info/Elements/c/C10012> ;
    rdfs:isDefinedBy <http://rdaregistry.info/Elements/n/> ;
    rdfs:subPropertyOf <http://rdaregistry.info/Elements/n/P80174>,
        <http://rdaregistry.info/Elements/x/P00001> ;
    skos:definition "Relates a nomen to an RDA entity that is associated with a nomen."@en .

<http://metadataregistry.org/uri/RegStatus/1008> a skos:Concept ;
    skos:prefLabel "Deprecated"@en .

<http://rdaregistry.info/Elements/n/P80159> a rdf:Property ;
    rdfs:label "is access point for RDA entity of"@en ;
    rdakit:hasElementType "2" ;
    rdakit:toolkitDefinition "An RDA entity that has an appellation in natural language that is taken from a vocabulary encoding scheme or is constructed using a string encoding scheme."@en ;
    rdakit:toolkitLabel "access point for RDA entity of"@en ;
    reg:hasSubproperty <http://rdaregistry.info/Elements/n/P80015>,
        <http://rdaregistry.info/Elements/n/P80018>,
        <http://rdaregistry.info/Elements/n/P80023>,
        <http://rdaregistry.info/Elements/n/P80024>,
        <http://rdaregistry.info/Elements/n/P80025>,
        <http://rdaregistry.info/Elements/n/P80026>,
        <http://rdaregistry.info/Elements/n/P80027>,
        <http://rdaregistry.info/Elements/n/P80162>,
        <http://rdaregistry.info/Elements/n/P80165>,
        <http://rdaregistry.info/Elements/n/datatype/P80159> ;
    reg:hasUnconstrained <http://rdaregistry.info/Elements/u/P60910> ;
    reg:lexicalAlias <http://rdaregistry.info/Elements/n/accessPointForRDAEntityOf.en> ;
    reg:name "accessPointForRDAEntityOf"@en ;
    reg:status <http://metadataregistry.org/uri/RegStatus/1001> ;
    rdfs:domain <http://rdaregistry.info/Elements/c/C10012> ;
    rdfs:isDefinedBy <http://rdaregistry.info/Elements/n/> ;
    rdfs:subPropertyOf <http://rdaregistry.info/Elements/n/P80112> ;
    skos:definition "Relates a nomen to an RDA entity that has an appellation in natural language that is taken from a vocabulary encoding scheme or is constructed using a string encoding scheme."@en .

<http://rdaregistry.info/Elements/n/P80161> a rdf:Property ;
    rdfs:label "is name of RDA entity of"@en ;
    rdakit:hasElementType "2" ;
    rdakit:toolkitDefinition "An RDA entity that has an appellation of RDA entity in natural language and phrasing used in common discourse."@en ;
    rdakit:toolkitLabel "name of RDA entity of"@en ;
    reg:hasSubproperty <http://rdaregistry.info/Elements/n/P80017>,
        <http://rdaregistry.info/Elements/n/P80039>,
        <http://rdaregistry.info/Elements/n/P80044>,
        <http://rdaregistry.info/Elements/n/P80051>,
        <http://rdaregistry.info/Elements/n/P80052>,
        <http://rdaregistry.info/Elements/n/P80062>,
        <http://rdaregistry.info/Elements/n/P80064>,
        <http://rdaregistry.info/Elements/n/P80163>,
        <http://rdaregistry.info/Elements/n/P80164>,
        <http://rdaregistry.info/Elements/n/datatype/P80161> ;
    reg:hasUnconstrained <http://rdaregistry.info/Elements/u/P60947> ;
    reg:lexicalAlias <http://rdaregistry.info/Elements/n/nameOfRDAEntityOf.en> ;
    reg:name "nameOfRDAEntityOf"@en ;
    reg:status <http://metadataregistry.org/uri/RegStatus/1001> ;
    rdfs:domain <http://rdaregistry.info/Elements/c/C10012> ;
    rdfs:isDefinedBy <http://rdaregistry.info/Elements/n/> ;
    rdfs:subPropertyOf <http://rdaregistry.info/Elements/n/P80112> ;
    skos:definition "Relates a nomen to an RDA entity that has an appellation of RDA entity in natural language and phrasing used in common discourse."@en .

<http://rdaregistry.info/Elements/n/P80112> a rdf:Property ;
    rdfs:label "is appellation of RDA entity of"@en ;
    rdakit:hasElementType "2" ;
    rdakit:toolkitDefinition "An RDA entity that is referred to by a nomen used within a given scheme or context."@en ;
    rdakit:toolkitLabel "appellation of RDA entity of"@en ;
    reg:hasSubproperty <http://rdaregistry.info/Elements/n/P80016>,
        <http://rdaregistry.info/Elements/n/P80028>,
        <http://rdaregistry.info/Elements/n/P80038>,
        <http://rdaregistry.info/Elements/n/P80040>,
        <http://rdaregistry.info/Elements/n/P80041>,
        <http://rdaregistry.info/Elements/n/P80043>,
        <http://rdaregistry.info/Elements/n/P80045>,
        <http://rdaregistry.info/Elements/n/P80112>,
        <http://rdaregistry.info/Elements/n/P80159>,
        <http://rdaregistry.info/Elements/n/P80160>,
        <http://rdaregistry.info/Elements/n/P80161>,
        <http://rdaregistry.info/Elements/n/datatype/P80112> ;
    reg:hasUnconstrained <http://rdaregistry.info/Elements/u/P60911> ;
    reg:lexicalAlias <http://rdaregistry.info/Elements/n/appellationOfRDAEntityOf.en> ;
    reg:name "appellationOfRDAEntityOf"@en ;
    reg:status <http://metadataregistry.org/uri/RegStatus/1001> ;
    rdfs:domain <http://rdaregistry.info/Elements/c/C10012> ;
    rdfs:isDefinedBy <http://rdaregistry.info/Elements/n/> ;
    rdfs:subPropertyOf <http://rdaregistry.info/Elements/n/P80010>,
        <http://rdaregistry.info/Elements/n/P80112> ;
    skos:definition "Relates a nomen to an RDA entity that is referred to by a nomen used within a given scheme or context."@en .

<http://metadataregistry.org/uri/RegStatus/1001> a skos:Concept ;
    skos:prefLabel "Published"@en .

<http://rdaregistry.info/Elements/n/> dc:title "RDA Nomen properties"@en ;
    skos:note "Properties derived from RDA elements with the domain of RDA Nomen."@en .

