@prefix dc: <http://purl.org/dc/elements/1.1/> .
@prefix foaf: <http://xmlns.com/foaf/0.1/> .
@prefix rdakit: <http://metadataregistry.org/uri/profile/rdakit/> .
@prefix rdf: <http://www.w3.org/1999/02/22-rdf-syntax-ns#> .
@prefix rdfs: <http://www.w3.org/2000/01/rdf-schema#> .
@prefix reg: <http://metadataregistry.org/uri/profile/regap/> .
@prefix skos: <http://www.w3.org/2004/02/skos/core#> .
@prefix xml: <http://www.w3.org/XML/1998/namespace> .
@prefix xsd: <http://www.w3.org/2001/XMLSchema#> .

<http://rdaregistry.info/Elements/t/P70014> a rdf:Property ;
    rdfs:label "is subject timespan of"@en ;
    rdakit:hasElementType "2" ;
    rdakit:toolkitDefinition "A work that is about a timespan."@en ;
    rdakit:toolkitLabel "subject timespan of"@en ;
    reg:hasSubproperty <http://rdaregistry.info/Elements/t/datatype/P70014>,
        <http://rdaregistry.info/Elements/t/object/P70014> ;
    reg:lexicalAlias <http://rdaregistry.info/Elements/t/subjectTimespanOf.en> ;
    reg:name "subjectTimespanOf"@en ;
    reg:status <http://metadataregistry.org/uri/RegStatus/1001> ;
    rdfs:domain <http://rdaregistry.info/Elements/c/C10010> ;
    rdfs:isDefinedBy <http://rdaregistry.info/Elements/t/> ;
    rdfs:subPropertyOf <http://rdaregistry.info/Elements/w/P10283> ;
    skos:definition "Relates a timespan to a work that is about a timespan."@en .

<http://rdaregistry.info/Elements/t/P70039> a rdf:Property ;
    rdfs:label "has beginning"@en ;
    rdakit:hasElementType "3" ;
    rdakit:toolkitDefinition "The time at which a timespan starts."@en ;
    rdakit:toolkitLabel "beginning"@en ;
    reg:hasSubproperty <http://rdaregistry.info/Elements/t/datatype/P70039> ;
    reg:hasUnconstrained <http://rdaregistry.info/Elements/u/P60998> ;
    reg:lexicalAlias <http://rdaregistry.info/Elements/t/beginning,en.en> ;
    reg:name "beginning"@en ;
    reg:status <http://metadataregistry.org/uri/RegStatus/1001> ;
    rdfs:domain <http://rdaregistry.info/Elements/c/C10010> ;
    rdfs:isDefinedBy <http://rdaregistry.info/Elements/t/> ;
    skos:definition "Relates a timespan to the time at which the timespan starts."@en .

<http://rdaregistry.info/Elements/t/P70040> a rdf:Property ;
    rdfs:label "has ending"@en ;
    rdakit:hasElementType "3" ;
    rdakit:toolkitDefinition "The time at which a timespan ends."@en ;
    rdakit:toolkitLabel "ending"@en ;
    reg:hasSubproperty <http://rdaregistry.info/Elements/t/datatype/P70040> ;
    reg:hasUnconstrained <http://rdaregistry.info/Elements/u/P61000> ;
    reg:lexicalAlias <http://rdaregistry.info/Elements/t/ending.en> ;
    reg:name "ending"@en ;
    reg:status <http://metadataregistry.org/uri/RegStatus/1001> ;
    rdfs:domain <http://rdaregistry.info/Elements/c/C10010> ;
    rdfs:isDefinedBy <http://rdaregistry.info/Elements/t/> ;
    skos:definition "Relates a timespan to the time at which the timespan ends."@en ;
    skos:scopeNote "A time may be represented at different levels of granularity by a calendrical timespan."@en .

<http://rdaregistry.info/Elements/t/P70045> a rdf:Property ;
    rdfs:label "has note on timespan"@en ;
    rdakit:hasElementType "6" ;
    rdakit:toolkitDefinition "A broad unstructured description of one or more attributes of a timespan."@en ;
    rdakit:toolkitLabel "note on timespan"@en ;
    reg:hasSubproperty <http://rdaregistry.info/Elements/t/datatype/P70045> ;
    reg:hasUnconstrained <http://rdaregistry.info/Elements/u/P60936> ;
    reg:lexicalAlias <http://rdaregistry.info/Elements/t/noteOnTimespan.en> ;
    reg:name "noteOnTimespan"@en ;
    reg:status <http://metadataregistry.org/uri/RegStatus/1001> ;
    rdfs:domain <http://rdaregistry.info/Elements/c/C10010> ;
    rdfs:isDefinedBy <http://rdaregistry.info/Elements/t/> ;
    skos:definition "Relates a timespan to a broad unstructured description of one or more attributes of a timespan."@en .

<http://rdaregistry.info/Elements/t/P70004> a rdf:Property ;
    rdfs:label "has related item of timespan"@en ;
    rdakit:hasElementType "1" ;
    rdakit:toolkitDefinition "An item that is associated with a timespan."@en ;
    rdakit:toolkitLabel "related item of timespan"@en ;
    reg:hasSubproperty <http://rdaregistry.info/Elements/t/datatype/P70004>,
        <http://rdaregistry.info/Elements/t/object/P70004> ;
    reg:hasUnconstrained <http://rdaregistry.info/Elements/u/P61012> ;
    reg:lexicalAlias <http://rdaregistry.info/Elements/t/relatedItemOfTimespan.en> ;
    reg:name "relatedItemOfTimespan"@en ;
    reg:status <http://metadataregistry.org/uri/RegStatus/1001> ;
    rdfs:domain <http://rdaregistry.info/Elements/c/C10010> ;
    rdfs:isDefinedBy <http://rdaregistry.info/Elements/t/> ;
    rdfs:subPropertyOf <http://rdaregistry.info/Elements/t/P70010> ;
    skos:definition "Relates a timespan to an item that is associated with a timespan."@en .

<http://rdaregistry.info/Elements/t/P70007> a rdf:Property ;
    rdfs:label "has related place of timespan"@en ;
    rdakit:hasElementType "1" ;
    rdakit:toolkitDefinition "A place that is associated with a timespan."@en ;
    rdakit:toolkitLabel "related place of timespan"@en ;
    reg:hasSubproperty <http://rdaregistry.info/Elements/t/datatype/P70007>,
        <http://rdaregistry.info/Elements/t/object/P70007> ;
    reg:hasUnconstrained <http://rdaregistry.info/Elements/u/P61015> ;
    reg:lexicalAlias <http://rdaregistry.info/Elements/t/relatedPlaceOfTimespan.en> ;
    reg:name "relatedPlaceOfTimespan"@en ;
    reg:status <http://metadataregistry.org/uri/RegStatus/1001> ;
    rdfs:domain <http://rdaregistry.info/Elements/c/C10010> ;
    rdfs:isDefinedBy <http://rdaregistry.info/Elements/t/> ;
    rdfs:subPropertyOf <http://rdaregistry.info/Elements/t/P70010> ;
    skos:definition "Relates a timespan to a place that is associated with a timespan."@en .

<http://rdaregistry.info/Elements/t/P70018> a rdf:Property ;
    rdfs:label "has identifier for timespan"@en ;
    rdakit:hasElementType "3" ;
    rdakit:toolkitDefinition "An appellation of timepsan that consists of a code, number, or other string, usually independent of natural language and social naming conventions, used to identify a timespan."@en ;
    rdakit:toolkitLabel "identifier for timespan"@en ;
    reg:hasSubproperty <http://rdaregistry.info/Elements/t/datatype/P70018>,
        <http://rdaregistry.info/Elements/t/object/P70018> ;
    reg:hasUnconstrained <http://rdaregistry.info/Elements/u/P60919> ;
    reg:lexicalAlias <http://rdaregistry.info/Elements/t/identifierForTimespan.en> ;
    reg:name "identifierForTimespan"@en ;
    reg:status <http://metadataregistry.org/uri/RegStatus/1001> ;
    rdfs:domain <http://rdaregistry.info/Elements/c/C10010> ;
    rdfs:isDefinedBy <http://rdaregistry.info/Elements/t/> ;
    rdfs:subPropertyOf <http://rdaregistry.info/Elements/t/P70016> ;
    skos:definition "Relates a timespan to an appellation of timepsan that consists of a code, number, or other string, usually independent of natural language and social naming conventions, used to identify a timespan."@en .

<http://rdaregistry.info/Elements/t/P70019> a rdf:Property ;
    rdfs:label "is copyright date of"@en ;
    rdakit:hasElementType "2" ;
    rdakit:toolkitDefinition "A manifestation that is associated with a claim of protection under copyright or a similar regime during a timespan."@en ;
    rdakit:toolkitLabel "copyright date of"@en ;
    reg:hasSubproperty <http://rdaregistry.info/Elements/t/datatype/P70019>,
        <http://rdaregistry.info/Elements/t/object/P70019> ;
    reg:lexicalAlias <http://rdaregistry.info/Elements/t/copyrightDateOf.en> ;
    reg:name "copyrightDateOf"@en ;
    reg:status <http://metadataregistry.org/uri/RegStatus/1001> ;
    rdfs:domain <http://rdaregistry.info/Elements/c/C10010> ;
    rdfs:isDefinedBy <http://rdaregistry.info/Elements/t/> ;
    rdfs:subPropertyOf <http://rdaregistry.info/Elements/t/P70020> ;
    skos:definition "Relates a timespan to a manifestation that is associated with a claim of protection under copyright or a similar regime during a timespan."@en .

<http://rdaregistry.info/Elements/t/P70021> a rdf:Property ;
    rdfs:label "is epoch of"@en ;
    rdakit:hasElementType "2" ;
    rdakit:toolkitDefinition "A work that refers to measurements of position for a body or orientation for an orbit."@en ;
    rdakit:toolkitLabel "epoch of"@en ;
    reg:hasSubproperty <http://rdaregistry.info/Elements/t/datatype/P70021>,
        <http://rdaregistry.info/Elements/t/object/P70021> ;
    reg:hasUnconstrained <http://rdaregistry.info/Elements/u/P60991> ;
    reg:lexicalAlias <http://rdaregistry.info/Elements/t/epochOf.en> ;
    reg:name "epochOf"@en ;
    reg:status <http://metadataregistry.org/uri/RegStatus/1001> ;
    rdfs:domain <http://rdaregistry.info/Elements/c/C10010> ;
    rdfs:isDefinedBy <http://rdaregistry.info/Elements/t/> ;
    rdfs:subPropertyOf <http://rdaregistry.info/Elements/t/P70001> ;
    skos:definition "Relates a timespan to a work that refers to measurements of position for a body or orientation for an orbit."@en .

<http://rdaregistry.info/Elements/t/P70023> a rdf:Property ;
    rdfs:label "is date of capture of"@en ;
    rdakit:hasElementType "2" ;
    rdakit:toolkitDefinition "An expression that is recorded, filmed, etc., during a timespan."@en ;
    rdakit:toolkitLabel "date of capture of"@en ;
    reg:hasSubproperty <http://rdaregistry.info/Elements/t/datatype/P70023>,
        <http://rdaregistry.info/Elements/t/object/P70023> ;
    reg:hasUnconstrained <http://rdaregistry.info/Elements/u/P60976> ;
    reg:lexicalAlias <http://rdaregistry.info/Elements/t/dateOfCaptureOf.en> ;
    reg:name "dateOfCaptureOf"@en ;
    reg:status <http://metadataregistry.org/uri/RegStatus/1001> ;
    rdfs:domain <http://rdaregistry.info/Elements/c/C10010> ;
    rdfs:isDefinedBy <http://rdaregistry.info/Elements/t/> ;
    rdfs:subPropertyOf <http://rdaregistry.info/Elements/t/P70024> ;
    skos:definition "Relates a timespan to an expression that is recorded, filmed, etc., during a timespan."@en .

<http://rdaregistry.info/Elements/t/P70025> a rdf:Property ;
    rdfs:label "is date of distribution of"@en ;
    rdakit:hasElementType "2" ;
    rdakit:toolkitDefinition "A manifestation that is a published manifestation that is distributed during a timespan."@en ;
    rdakit:toolkitLabel "date of distribution of"@en ;
    reg:hasSubproperty <http://rdaregistry.info/Elements/t/datatype/P70025>,
        <http://rdaregistry.info/Elements/t/object/P70025> ;
    reg:hasUnconstrained <http://rdaregistry.info/Elements/u/P60979> ;
    reg:lexicalAlias <http://rdaregistry.info/Elements/t/dateOfDistributionOf.en> ;
    reg:name "dateOfDistributionOf"@en ;
    reg:status <http://metadataregistry.org/uri/RegStatus/1001> ;
    rdfs:domain <http://rdaregistry.info/Elements/c/C10010> ;
    rdfs:isDefinedBy <http://rdaregistry.info/Elements/t/> ;
    rdfs:subPropertyOf <http://rdaregistry.info/Elements/t/P70020> ;
    skos:definition "Relates a timespan to a manifestation that is a published manifestation that is distributed during a timespan."@en .

<http://rdaregistry.info/Elements/t/P70026> a rdf:Property ;
    rdfs:label "is date of manufacture of"@en ;
    rdakit:hasElementType "2" ;
    rdakit:toolkitDefinition "A manifestation that is a published manifesation that is printed, duplicated, cast, etc., during a timespan."@en ;
    rdakit:toolkitLabel "date of manufacture of"@en ;
    reg:hasSubproperty <http://rdaregistry.info/Elements/t/datatype/P70026>,
        <http://rdaregistry.info/Elements/t/object/P70026> ;
    reg:hasUnconstrained <http://rdaregistry.info/Elements/u/P60981> ;
    reg:lexicalAlias <http://rdaregistry.info/Elements/t/dateOfManufactureOf.en> ;
    reg:name "dateOfManufactureOf"@en ;
    reg:status <http://metadataregistry.org/uri/RegStatus/1001> ;
    rdfs:domain <http://rdaregistry.info/Elements/c/C10010> ;
    rdfs:isDefinedBy <http://rdaregistry.info/Elements/t/> ;
    rdfs:subPropertyOf <http://rdaregistry.info/Elements/t/P70020> ;
    skos:definition "Relates a timespan to a manifestation that is a published manifesation that is printed, duplicated, cast, etc., during a timespan."@en .

<http://rdaregistry.info/Elements/t/P70027> a rdf:Property ;
    rdfs:label "is date of production of"@en ;
    rdakit:hasElementType "2" ;
    rdakit:toolkitDefinition "A manifestation that is an unpublished manifestation that is inscribed, fabricated, constructed, etc., during a timespan."@en ;
    rdakit:toolkitLabel "date of production of"@en ;
    reg:hasSubproperty <http://rdaregistry.info/Elements/t/datatype/P70027>,
        <http://rdaregistry.info/Elements/t/object/P70027> ;
    reg:hasUnconstrained <http://rdaregistry.info/Elements/u/P60982> ;
    reg:lexicalAlias <http://rdaregistry.info/Elements/t/dateOfProductionOf.en> ;
    reg:name "dateOfProductionOf"@en ;
    reg:status <http://metadataregistry.org/uri/RegStatus/1001> ;
    rdfs:domain <http://rdaregistry.info/Elements/c/C10010> ;
    rdfs:isDefinedBy <http://rdaregistry.info/Elements/t/> ;
    rdfs:subPropertyOf <http://rdaregistry.info/Elements/t/P70020> ;
    skos:definition "Relates a timespan to a manifestation that is an unpublished manifestation that is inscribed, fabricated, constructed, etc., during a timespan."@en .

<http://rdaregistry.info/Elements/t/P70028> a rdf:Property ;
    rdfs:label "is date of publication of"@en ;
    rdakit:hasElementType "2" ;
    rdakit:toolkitDefinition "A manifestation that is published, released, or issued in a published form during a timespan."@en ;
    rdakit:toolkitLabel "date of publication of"@en ;
    reg:hasSubproperty <http://rdaregistry.info/Elements/t/datatype/P70028>,
        <http://rdaregistry.info/Elements/t/object/P70028> ;
    reg:hasUnconstrained <http://rdaregistry.info/Elements/u/P60983> ;
    reg:lexicalAlias <http://rdaregistry.info/Elements/t/dateOfPublicationOf.en> ;
    reg:name "dateOfPublicationOf"@en ;
    reg:status <http://metadataregistry.org/uri/RegStatus/1001> ;
    rdfs:domain <http://rdaregistry.info/Elements/c/C10010> ;
    rdfs:isDefinedBy <http://rdaregistry.info/Elements/t/> ;
    rdfs:subPropertyOf <http://rdaregistry.info/Elements/t/P70020> ;
    skos:definition "Relates a timespan to a manifestation that is published, released, or issued in a published form during a timespan."@en .

<http://rdaregistry.info/Elements/t/P70029> a rdf:Property ;
    rdfs:label "is date of birth of"@en ;
    rdakit:hasElementType "2" ;
    rdakit:toolkitDefinition "A person who was born during a timespan."@en ;
    rdakit:toolkitLabel "date of birth of"@en ;
    reg:hasSubproperty <http://rdaregistry.info/Elements/t/datatype/P70029>,
        <http://rdaregistry.info/Elements/t/object/P70029> ;
    reg:hasUnconstrained <http://rdaregistry.info/Elements/u/P60975> ;
    reg:lexicalAlias <http://rdaregistry.info/Elements/t/dateOfBirthOf.en> ;
    reg:name "dateOfBirthOf"@en ;
    reg:status <http://metadataregistry.org/uri/RegStatus/1001> ;
    rdfs:domain <http://rdaregistry.info/Elements/c/C10010> ;
    rdfs:isDefinedBy <http://rdaregistry.info/Elements/t/> ;
    rdfs:subPropertyOf <http://rdaregistry.info/Elements/t/P70038> ;
    skos:definition "Relates a timespan to a person who was born during a timespan."@en .

<http://rdaregistry.info/Elements/t/P70030> a rdf:Property ;
    rdfs:label "is date of death of"@en ;
    rdakit:hasElementType "2" ;
    rdakit:toolkitDefinition "A person who died during a timespan."@en ;
    rdakit:toolkitLabel "date of death of"@en ;
    reg:hasSubproperty <http://rdaregistry.info/Elements/t/datatype/P70030>,
        <http://rdaregistry.info/Elements/t/object/P70030> ;
    reg:hasUnconstrained <http://rdaregistry.info/Elements/u/P60978> ;
    reg:lexicalAlias <http://rdaregistry.info/Elements/t/dateOfDeathOf.en> ;
    reg:name "dateOfDeathOf"@en ;
    reg:status <http://metadataregistry.org/uri/RegStatus/1001> ;
    rdfs:domain <http://rdaregistry.info/Elements/c/C10010> ;
    rdfs:isDefinedBy <http://rdaregistry.info/Elements/t/> ;
    rdfs:subPropertyOf <http://rdaregistry.info/Elements/t/P70038> ;
    skos:definition "Relates a timespan to a person who died during a timespan."@en .

<http://rdaregistry.info/Elements/t/P70031> a rdf:Property ;
    rdfs:label "is date of conference, etc. of"@en ;
    rdakit:hasElementType "2" ;
    rdakit:toolkitDefinition "A conference, exhibition, or other event that gives rise to a work that is held during a timespan."@en ;
    rdakit:toolkitLabel "date of conference, etc. of"@en ;
    reg:hasSubproperty <http://rdaregistry.info/Elements/t/datatype/P70031>,
        <http://rdaregistry.info/Elements/t/object/P70031> ;
    reg:hasUnconstrained <http://rdaregistry.info/Elements/u/P60977> ;
    reg:lexicalAlias <http://rdaregistry.info/Elements/t/dateOfConferenceEtcOf.en> ;
    reg:name "dateOfConferenceEtcOf"@en ;
    reg:status <http://metadataregistry.org/uri/RegStatus/1001> ;
    rdfs:domain <http://rdaregistry.info/Elements/c/C10010> ;
    rdfs:isDefinedBy <http://rdaregistry.info/Elements/t/> ;
    rdfs:subPropertyOf <http://rdaregistry.info/Elements/t/P70036> ;
    skos:definition "Relates a timespan to a conference, exhibition, or other event that gives rise to a work that is held during a timespan."@en .

<http://rdaregistry.info/Elements/t/P70032> a rdf:Property ;
    rdfs:label "is date of establishment of"@en ;
    rdakit:hasElementType "2" ;
    rdakit:toolkitDefinition "A corporate body who is established or founded during a timespan."@en ;
    rdakit:toolkitLabel "date of establishment of"@en ;
    reg:hasSubproperty <http://rdaregistry.info/Elements/t/datatype/P70032>,
        <http://rdaregistry.info/Elements/t/object/P70032> ;
    reg:hasUnconstrained <http://rdaregistry.info/Elements/u/P60980> ;
    reg:lexicalAlias <http://rdaregistry.info/Elements/t/dateOfEstablishmentOf.en> ;
    reg:name "dateOfEstablishmentOf"@en ;
    reg:status <http://metadataregistry.org/uri/RegStatus/1001> ;
    rdfs:domain <http://rdaregistry.info/Elements/c/C10010> ;
    rdfs:isDefinedBy <http://rdaregistry.info/Elements/t/> ;
    rdfs:subPropertyOf <http://rdaregistry.info/Elements/t/P70036> ;
    skos:definition "Relates a timespan to a corporate body who is established or founded during a timespan."@en .

<http://rdaregistry.info/Elements/t/P70033> a rdf:Property ;
    rdfs:label "is date of termination of"@en ;
    rdakit:hasElementType "2" ;
    rdakit:toolkitDefinition "A corporate body who is terminated or dissolved during a timespan."@en ;
    rdakit:toolkitLabel "date of termination of"@en ;
    reg:hasSubproperty <http://rdaregistry.info/Elements/t/datatype/P70033>,
        <http://rdaregistry.info/Elements/t/object/P70033> ;
    reg:hasUnconstrained <http://rdaregistry.info/Elements/u/P60985> ;
    reg:lexicalAlias <http://rdaregistry.info/Elements/t/dateOfTerminationOf.en> ;
    reg:name "dateOfTerminationOf"@en ;
    reg:status <http://metadataregistry.org/uri/RegStatus/1001> ;
    rdfs:domain <http://rdaregistry.info/Elements/c/C10010> ;
    rdfs:isDefinedBy <http://rdaregistry.info/Elements/t/> ;
    rdfs:subPropertyOf <http://rdaregistry.info/Elements/t/P70036> ;
    skos:definition "Relates a timespan to a corporate body who is terminated or dissolved during a timespan."@en .

<http://rdaregistry.info/Elements/t/P70034> a rdf:Property ;
    rdfs:label "is part of timespan"@en ;
    rdakit:hasElementType "2" ;
    rdakit:toolkitDefinition "A timespan that is a component of another timespan."@en ;
    rdakit:toolkitLabel "part of timespan"@en ;
    reg:hasSubproperty <http://rdaregistry.info/Elements/t/datatype/P70034>,
        <http://rdaregistry.info/Elements/t/object/P70034> ;
    reg:hasUnconstrained <http://rdaregistry.info/Elements/u/P61002> ;
    reg:lexicalAlias <http://rdaregistry.info/Elements/t/partOfTimespan.en> ;
    reg:name "partOfTimespan"@en ;
    reg:status <http://metadataregistry.org/uri/RegStatus/1001> ;
    rdfs:domain <http://rdaregistry.info/Elements/c/C10010> ;
    rdfs:isDefinedBy <http://rdaregistry.info/Elements/t/> ;
    rdfs:subPropertyOf <http://rdaregistry.info/Elements/t/P70008> ;
    skos:definition "Relates a timespan to a timespan that is a component of another timespan."@en .

<http://rdaregistry.info/Elements/t/P70035> a rdf:Property ;
    rdfs:label "has part timespan"@en ;
    rdakit:hasElementType "2" ;
    rdakit:toolkitDefinition "A timespan that has another timespan as a component."@en ;
    rdakit:toolkitLabel "part timespan"@en ;
    reg:hasSubproperty <http://rdaregistry.info/Elements/t/datatype/P70035>,
        <http://rdaregistry.info/Elements/t/object/P70035> ;
    reg:hasUnconstrained <http://rdaregistry.info/Elements/u/P61004> ;
    reg:lexicalAlias <http://rdaregistry.info/Elements/t/partTimespan.en> ;
    reg:name "partTimespan"@en ;
    reg:status <http://metadataregistry.org/uri/RegStatus/1001> ;
    rdfs:domain <http://rdaregistry.info/Elements/c/C10010> ;
    rdfs:isDefinedBy <http://rdaregistry.info/Elements/t/> ;
    rdfs:subPropertyOf <http://rdaregistry.info/Elements/t/P70008> ;
    skos:definition "Relates a timespan to a timespan that has another timespan as a component."@en .

<http://rdaregistry.info/Elements/t/P70041> a rdf:Property ;
    rdfs:label "is duration of"@en ;
    rdakit:hasElementType "3" ;
    rdakit:toolkitDefinition "An expression that has an extent of expression that is a playing time, performance time, running time, or other timespan."@en ;
    rdakit:toolkitLabel "duration of"@en ;
    reg:hasSubproperty <http://rdaregistry.info/Elements/t/datatype/P70041>,
        <http://rdaregistry.info/Elements/t/object/P70041> ;
    reg:lexicalAlias <http://rdaregistry.info/Elements/t/durationOf.en> ;
    reg:name "durationOf"@en ;
    reg:status <http://metadataregistry.org/uri/RegStatus/1001> ;
    rdfs:domain <http://rdaregistry.info/Elements/c/C10010> ;
    rdfs:isDefinedBy <http://rdaregistry.info/Elements/t/> ;
    rdfs:subPropertyOf <http://rdaregistry.info/Elements/t/P70002> ;
    skos:definition "Relates a timespan to an expression that has an extent of expression that is a playing time, performance time, running time, or other timespan."@en .

<http://rdaregistry.info/Elements/t/P70042> a rdf:Property ;
    rdfs:label "is equinox of"@en ;
    rdakit:hasElementType "2" ;
    rdakit:toolkitDefinition "A work that uses a point of intersection of the ecliptic and the celestial equator, occupied by the sun when its declination is 0°."@en ;
    rdakit:toolkitLabel "equinox of"@en ;
    reg:hasSubproperty <http://rdaregistry.info/Elements/t/datatype/P70042>,
        <http://rdaregistry.info/Elements/t/object/P70042> ;
    reg:hasUnconstrained <http://rdaregistry.info/Elements/u/P60992> ;
    reg:lexicalAlias <http://rdaregistry.info/Elements/t/equinoxOf.en> ;
    reg:name "equinoxOf"@en ;
    reg:status <http://metadataregistry.org/uri/RegStatus/1001> ;
    rdfs:domain <http://rdaregistry.info/Elements/c/C10010> ;
    rdfs:isDefinedBy <http://rdaregistry.info/Elements/t/> ;
    rdfs:subPropertyOf <http://rdaregistry.info/Elements/t/P70001> ;
    skos:definition "Relates a timespan to a work that uses a point of intersection of the ecliptic and the celestial equator, occupied by the sun when its declination is 0°."@en .

<http://rdaregistry.info/Elements/t/P70046> a rdf:Property ;
    rdfs:label "is year degree granted of"@en ;
    rdakit:hasElementType "2" ;
    rdakit:toolkitDefinition "A work that is an academic degree conferred by a granting institution or faculty during a timespan."@en ;
    rdakit:toolkitLabel "year degree granted of"@en ;
    reg:hasSubproperty <http://rdaregistry.info/Elements/t/datatype/P70046>,
        <http://rdaregistry.info/Elements/t/object/P70046> ;
    reg:lexicalAlias <http://rdaregistry.info/Elements/t/yearDegreeGrantedOf.en> ;
    reg:name "yearDegreeGrantedOf"@en ;
    reg:status <http://metadataregistry.org/uri/RegStatus/1001> ;
    rdfs:domain <http://rdaregistry.info/Elements/c/C10010> ;
    rdfs:isDefinedBy <http://rdaregistry.info/Elements/t/> ;
    rdfs:subPropertyOf <http://rdaregistry.info/Elements/t/P70022> ;
    skos:definition "Relates a timespan to a work that is an academic degree conferred by a granting institution or faculty during a timespan."@en .

<http://rdaregistry.info/Elements/t/P70047> a rdf:Property ;
    rdfs:label "has authorized access point for timespan"@en ;
    rdakit:hasElementType "3" ;
    rdakit:toolkitDefinition "An access point for timespan that is selected for preference in a specific vocabulary encoding scheme."@en ;
    rdakit:toolkitLabel "authorized access point for timespan"@en ;
    reg:hasSubproperty <http://rdaregistry.info/Elements/t/datatype/P70047>,
        <http://rdaregistry.info/Elements/t/object/P70047> ;
    reg:hasUnconstrained <http://rdaregistry.info/Elements/u/P60916> ;
    reg:lexicalAlias <http://rdaregistry.info/Elements/t/authorizedAccessPointForTimespan.en> ;
    reg:name "authorizedAccessPointForTimespan"@en ;
    reg:status <http://metadataregistry.org/uri/RegStatus/1001> ;
    rdfs:domain <http://rdaregistry.info/Elements/c/C10010> ;
    rdfs:isDefinedBy <http://rdaregistry.info/Elements/t/> ;
    rdfs:subPropertyOf <http://rdaregistry.info/Elements/t/P70015> ;
    skos:definition "Relates a timespan to an access point for timespan that is selected for preference in a specific vocabulary encoding scheme."@en .

<http://rdaregistry.info/Elements/t/P70048> a rdf:Property ;
    rdfs:label "has variant access point for timespan"@en ;
    rdakit:hasElementType "3" ;
    rdakit:toolkitDefinition "An access point for timespan that is not selected for preference in a specific vocabulary encoding scheme."@en ;
    rdakit:toolkitLabel "variant access point for timespan"@en ;
    reg:hasSubproperty <http://rdaregistry.info/Elements/t/datatype/P70048>,
        <http://rdaregistry.info/Elements/t/object/P70048> ;
    reg:hasUnconstrained <http://rdaregistry.info/Elements/u/P60917> ;
    reg:lexicalAlias <http://rdaregistry.info/Elements/t/variantAccessPointForTimespan.en> ;
    reg:name "variantAccessPointForTimespan"@en ;
    reg:status <http://metadataregistry.org/uri/RegStatus/1001> ;
    rdfs:domain <http://rdaregistry.info/Elements/c/C10010> ;
    rdfs:isDefinedBy <http://rdaregistry.info/Elements/t/> ;
    rdfs:subPropertyOf <http://rdaregistry.info/Elements/t/P70015> ;
    skos:definition "Relates a timespan to an access point for timespan that is not selected for preference in a specific vocabulary encoding scheme."@en .

<http://rdaregistry.info/Elements/t/P70049> a rdf:Property ;
    rdfs:label "has preferred name of timespan"@en ;
    rdakit:hasElementType "3" ;
    rdakit:toolkitDefinition "A name of timespan that is selected for preference in a specific application or context."@en ;
    rdakit:toolkitLabel "preferred name of timespan"@en ;
    reg:hasSubproperty <http://rdaregistry.info/Elements/t/datatype/P70049>,
        <http://rdaregistry.info/Elements/t/object/P70049> ;
    reg:hasUnconstrained <http://rdaregistry.info/Elements/u/P60930> ;
    reg:lexicalAlias <http://rdaregistry.info/Elements/t/preferredNameOfTimespan.en> ;
    reg:name "preferredNameOfTimespan"@en ;
    reg:status <http://metadataregistry.org/uri/RegStatus/1001> ;
    rdfs:domain <http://rdaregistry.info/Elements/c/C10010> ;
    rdfs:isDefinedBy <http://rdaregistry.info/Elements/t/> ;
    rdfs:subPropertyOf <http://rdaregistry.info/Elements/t/P70017> ;
    skos:definition "Relates a timespan to a name of timespan that is selected for preference in a specific application or context."@en .

<http://rdaregistry.info/Elements/t/P70050> a rdf:Property ;
    rdfs:label "has variant name of timespan"@en ;
    rdakit:hasElementType "3" ;
    rdakit:toolkitDefinition "A name of timespan that is not selected for preference in a specific application or context."@en ;
    rdakit:toolkitLabel "variant name of timespan"@en ;
    reg:hasSubproperty <http://rdaregistry.info/Elements/t/datatype/P70050>,
        <http://rdaregistry.info/Elements/t/object/P70050> ;
    reg:hasUnconstrained <http://rdaregistry.info/Elements/u/P60926> ;
    reg:lexicalAlias <http://rdaregistry.info/Elements/t/variantNameOfTimespan.en> ;
    reg:name "variantNameOfTimespan"@en ;
    reg:status <http://metadataregistry.org/uri/RegStatus/1001> ;
    rdfs:domain <http://rdaregistry.info/Elements/c/C10010> ;
    rdfs:isDefinedBy <http://rdaregistry.info/Elements/t/> ;
    rdfs:subPropertyOf <http://rdaregistry.info/Elements/t/P70017> ;
    skos:definition "Relates a timespan to a name of timespan that is not selected for preference in a specific application or context."@en .

<http://rdaregistry.info/Elements/t/P70054> a rdf:Property ;
    rdfs:label "is date of capture of representative expression of"@en ;
    rdakit:hasElementType "2" ;
    rdakit:toolkitDefinition "A work associated with a representative expression that is recorded, filmed, etc., during a timespan."@en ;
    rdakit:toolkitLabel "date of capture of representative expression of"@en ;
    reg:hasSubproperty <http://rdaregistry.info/Elements/t/datatype/P70054> ;
    reg:hasUnconstrained <http://rdaregistry.info/Elements/u/P60976> ;
    reg:lexicalAlias <http://rdaregistry.info/Elements/t/dateOfCaptureOfRepresentativeExpressionOf.en> ;
    reg:name "dateOfCaptureOfRepresentativeExpressionOf"@en ;
    reg:status <http://metadataregistry.org/uri/RegStatus/1001> ;
    rdfs:domain <http://rdaregistry.info/Elements/c/C10010> ;
    rdfs:isDefinedBy <http://rdaregistry.info/Elements/t/> ;
    rdfs:subPropertyOf <http://rdaregistry.info/Elements/t/P70001> ;
    skos:definition "Relates a timespan to a work associated with a representative expression that is recorded, filmed, etc., during a timespan."@en .

<http://rdaregistry.info/Elements/t/P70055> a rdf:Property ;
    rdfs:label "is duration of representative expression of"@en ;
    rdakit:hasElementType "2" ;
    rdakit:toolkitDefinition "A work that has an extent of expression of a representative expression that is a playing time, performance time, running time, or other timespan."@en ;
    rdakit:toolkitLabel "duration of representative expression of"@en ;
    reg:hasSubproperty <http://rdaregistry.info/Elements/t/datatype/P70055> ;
    reg:lexicalAlias <http://rdaregistry.info/Elements/t/durationOfRepresentativeExpressionOf.en> ;
    reg:name "durationOfRepresentativeExpressionOf"@en ;
    reg:status <http://metadataregistry.org/uri/RegStatus/1001> ;
    rdfs:domain <http://rdaregistry.info/Elements/c/C10010> ;
    rdfs:isDefinedBy <http://rdaregistry.info/Elements/t/> ;
    rdfs:subPropertyOf <http://rdaregistry.info/Elements/t/P70001> ;
    skos:definition "Relates a timespan to a work that has an extent of expression of a representative expression that is a playing time, performance time, running time, or other timespan."@en .

<http://rdaregistry.info/Elements/t/P70056> a rdf:Property ;
    rdfs:label "is date of usage of"@en ;
    rdakit:hasElementType "3" ;
    rdakit:toolkitDefinition "An appellation of an RDA entity used during a timespan."@en ;
    rdakit:toolkitLabel "date of usage of"@en ;
    reg:hasSubproperty <http://rdaregistry.info/Elements/t/datatype/P70056>,
        <http://rdaregistry.info/Elements/t/object/P70056> ;
    reg:hasUnconstrained <http://rdaregistry.info/Elements/u/P60986> ;
    reg:lexicalAlias <http://rdaregistry.info/Elements/t/dateOfUsageOf.en> ;
    reg:name "dateOfUsageOf"@en ;
    reg:status <http://metadataregistry.org/uri/RegStatus/1001> ;
    rdfs:domain <http://rdaregistry.info/Elements/c/C10010> ;
    rdfs:isDefinedBy <http://rdaregistry.info/Elements/t/> ;
    rdfs:subPropertyOf <http://rdaregistry.info/Elements/t/P70009> ;
    skos:definition "Relates a timespan to an appellation of an RDA entity used during a timespan."@en .

<http://rdaregistry.info/Elements/t/P70057> a rdf:Property ;
    rdfs:label "is date of representative expression of"@en ;
    rdakit:hasElementType "2" ;
    rdakit:toolkitDefinition "A work that is associated with an earlist timespan of a representative expression."@en ;
    rdakit:toolkitLabel "date of representative expression of"@en ;
    reg:hasSubproperty <http://rdaregistry.info/Elements/t/datatype/P70057>,
        <http://rdaregistry.info/Elements/t/object/P70057> ;
    reg:hasUnconstrained <http://rdaregistry.info/Elements/u/P60984> ;
    reg:lexicalAlias <http://rdaregistry.info/Elements/t/dateOfRepresentativeExpressionOf.en> ;
    reg:name "dateOfRepresentativeExpressionOf" ;
    reg:status <http://metadataregistry.org/uri/RegStatus/1001> ;
    rdfs:domain <http://rdaregistry.info/Elements/c/C10010> ;
    rdfs:isDefinedBy <http://rdaregistry.info/Elements/t/> ;
    rdfs:subPropertyOf <http://rdaregistry.info/Elements/t/P70001> ;
    skos:definition "Relates a timespan to a work that is associated with an earliest timespan of a representative expression."@en .

<http://rdaregistry.info/Elements/t/P70003> a rdf:Property ;
    rdfs:label "has related manifestation of timespan"@en ;
    rdakit:hasElementType "1" ;
    rdakit:toolkitDefinition "A manifestation that is associated with a timespan."@en ;
    rdakit:toolkitLabel "related manifestation of timespan"@en ;
    reg:hasSubproperty <http://rdaregistry.info/Elements/t/P70020>,
        <http://rdaregistry.info/Elements/t/datatype/P70003>,
        <http://rdaregistry.info/Elements/t/object/P70003> ;
    reg:hasUnconstrained <http://rdaregistry.info/Elements/u/P61012> ;
    reg:lexicalAlias <http://rdaregistry.info/Elements/t/relatedManifestationOfTimespan.en> ;
    reg:name "relatedManifestationOfTimespan"@en ;
    reg:status <http://metadataregistry.org/uri/RegStatus/1001> ;
    rdfs:domain <http://rdaregistry.info/Elements/c/C10010> ;
    rdfs:isDefinedBy <http://rdaregistry.info/Elements/t/> ;
    rdfs:subPropertyOf <http://rdaregistry.info/Elements/t/P70010> ;
    skos:definition "Relates a timespan to a manifestation that is associated with a timespan."@en .

<http://rdaregistry.info/Elements/t/P70011> a rdf:Property ;
    rdfs:label "has related person of timespan"@en ;
    rdakit:hasElementType "1" ;
    rdakit:toolkitDefinition "A person who is associated with a timespan."@en ;
    rdakit:toolkitLabel "related person of timespan"@en ;
    reg:hasSubproperty <http://rdaregistry.info/Elements/t/P70038>,
        <http://rdaregistry.info/Elements/t/datatype/P70011>,
        <http://rdaregistry.info/Elements/t/object/P70011> ;
    reg:hasUnconstrained <http://rdaregistry.info/Elements/u/P61010> ;
    reg:lexicalAlias <http://rdaregistry.info/Elements/t/relatedPersonOfTimespan.en> ;
    reg:name "relatedPersonOfTimespan"@en ;
    reg:status <http://metadataregistry.org/uri/RegStatus/1001> ;
    rdfs:domain <http://rdaregistry.info/Elements/c/C10010> ;
    rdfs:isDefinedBy <http://rdaregistry.info/Elements/t/> ;
    rdfs:subPropertyOf <http://rdaregistry.info/Elements/t/P70005> ;
    skos:definition "Relates a timespan to a person who is associated with a timespan."@en .

<http://rdaregistry.info/Elements/t/P70012> a rdf:Property ;
    rdfs:label "has related family of timespan"@en ;
    rdakit:hasElementType "1" ;
    rdakit:toolkitDefinition "A family who is associated with a timespan."@en ;
    rdakit:toolkitLabel "related family of timespan"@en ;
    reg:hasSubproperty <http://rdaregistry.info/Elements/t/P70037>,
        <http://rdaregistry.info/Elements/t/datatype/P70012>,
        <http://rdaregistry.info/Elements/t/object/P70012> ;
    reg:hasUnconstrained <http://rdaregistry.info/Elements/u/P61010> ;
    reg:lexicalAlias <http://rdaregistry.info/Elements/t/relatedFamilyOfTimespan.en> ;
    reg:name "relatedFamilyOfTimespan"@en ;
    reg:status <http://metadataregistry.org/uri/RegStatus/1001> ;
    rdfs:domain <http://rdaregistry.info/Elements/c/C10010> ;
    rdfs:isDefinedBy <http://rdaregistry.info/Elements/t/> ;
    rdfs:subPropertyOf <http://rdaregistry.info/Elements/t/P70006> ;
    skos:definition "Relates a timespan to a family who is associated with a timespan."@en .

<http://rdaregistry.info/Elements/t/P70013> a rdf:Property ;
    rdfs:label "has related corporate body of timespan"@en ;
    rdakit:hasElementType "1" ;
    rdakit:toolkitDefinition "A corporate body who is associated with a timespan."@en ;
    rdakit:toolkitLabel "related corporate body of timespan"@en ;
    reg:hasSubproperty <http://rdaregistry.info/Elements/t/P70036>,
        <http://rdaregistry.info/Elements/t/datatype/P70013>,
        <http://rdaregistry.info/Elements/t/object/P70013> ;
    reg:hasUnconstrained <http://rdaregistry.info/Elements/u/P61010> ;
    reg:lexicalAlias <http://rdaregistry.info/Elements/t/relatedCorporateBodyOfTimespan.en> ;
    reg:name "relatedCorporateBodyOfTimespan"@en ;
    reg:status <http://metadataregistry.org/uri/RegStatus/1001> ;
    rdfs:domain <http://rdaregistry.info/Elements/c/C10010> ;
    rdfs:isDefinedBy <http://rdaregistry.info/Elements/t/> ;
    rdfs:subPropertyOf <http://rdaregistry.info/Elements/t/P70006> ;
    skos:definition "Relates a timespan to a corporate body who is associated with a timespan."@en .

<http://rdaregistry.info/Elements/t/P70022> a rdf:Property ;
    rdfs:label "is date of work of"@en ;
    rdakit:hasElementType "2" ;
    rdakit:toolkitDefinition "A work that is associated with an earliest timespan of a work."@en ;
    rdakit:toolkitLabel "date of work of"@en ;
    reg:hasSubproperty <http://rdaregistry.info/Elements/t/P70046>,
        <http://rdaregistry.info/Elements/t/datatype/P70022>,
        <http://rdaregistry.info/Elements/t/object/P70022> ;
    reg:hasUnconstrained <http://rdaregistry.info/Elements/u/P60984> ;
    reg:lexicalAlias <http://rdaregistry.info/Elements/t/dateOfWorkOf.en> ;
    reg:name "dateOfWorkOf"@en ;
    reg:status <http://metadataregistry.org/uri/RegStatus/1001> ;
    rdfs:domain <http://rdaregistry.info/Elements/c/C10010> ;
    rdfs:isDefinedBy <http://rdaregistry.info/Elements/t/> ;
    rdfs:subPropertyOf <http://rdaregistry.info/Elements/t/P70001> ;
    skos:definition "Relates a timespan to a work that is associated with an earliest timespan of a work."@en .

<http://rdaregistry.info/Elements/t/P70024> a rdf:Property ;
    rdfs:label "is date of expression of"@en ;
    rdakit:hasElementType "2" ;
    rdakit:toolkitDefinition "An expression that is associated with an earliest timespan."@en ;
    rdakit:toolkitLabel "date of expression of"@en ;
    reg:hasSubproperty <http://rdaregistry.info/Elements/t/P70023>,
        <http://rdaregistry.info/Elements/t/datatype/P70024>,
        <http://rdaregistry.info/Elements/t/object/P70024> ;
    reg:hasUnconstrained <http://rdaregistry.info/Elements/u/P60984> ;
    reg:lexicalAlias <http://rdaregistry.info/Elements/t/dateOfExpressionOf.en> ;
    reg:name "dateOfExpressionOf"@en ;
    reg:status <http://metadataregistry.org/uri/RegStatus/1001> ;
    rdfs:domain <http://rdaregistry.info/Elements/c/C10010> ;
    rdfs:isDefinedBy <http://rdaregistry.info/Elements/t/> ;
    rdfs:subPropertyOf <http://rdaregistry.info/Elements/t/P70002> ;
    skos:definition "Relates a timespan to an expression that is associated with an earliest timespan."@en .

<http://rdaregistry.info/Elements/t/P70037> a rdf:Property ;
    rdfs:label "is date associated with family of"@en ;
    rdakit:hasElementType "2" ;
    rdakit:toolkitDefinition "A family who has a significant association with a timespan."@en ;
    rdakit:toolkitLabel "date associated with family of"@en ;
    reg:hasSubproperty <http://rdaregistry.info/Elements/t/P70053>,
        <http://rdaregistry.info/Elements/t/datatype/P70037>,
        <http://rdaregistry.info/Elements/t/object/P70037> ;
    reg:hasUnconstrained <http://rdaregistry.info/Elements/u/P60974> ;
    reg:lexicalAlias <http://rdaregistry.info/Elements/t/dateAssociatedWithFamilyOf.en> ;
    reg:name "dateAssociatedWithFamilyOf"@en ;
    reg:status <http://metadataregistry.org/uri/RegStatus/1001> ;
    rdfs:domain <http://rdaregistry.info/Elements/c/C10010> ;
    rdfs:isDefinedBy <http://rdaregistry.info/Elements/t/> ;
    rdfs:subPropertyOf <http://rdaregistry.info/Elements/t/P70012> ;
    skos:definition "Relates a timespan to a family who has a significant association with a timespan."@en .

<http://rdaregistry.info/Elements/t/P70043> a rdf:Property ;
    rdfs:label "is period of activity of corporate body of"@en ;
    rdakit:hasElementType "2" ;
    rdakit:toolkitDefinition "A corporate body who is active in its primary field of endeavour during a timespan."@en ;
    rdakit:toolkitLabel "period of activity of corporate body of"@en ;
    reg:hasSubproperty <http://rdaregistry.info/Elements/t/datatype/P70043>,
        <http://rdaregistry.info/Elements/t/object/P70043> ;
    reg:hasUnconstrained <http://rdaregistry.info/Elements/u/P60990> ;
    reg:lexicalAlias <http://rdaregistry.info/Elements/t/periodOfActivityOfCorporateBodyOf.en> ;
    reg:name "periodOfActivityOfCorporateBodyOf"@en ;
    reg:status <http://metadataregistry.org/uri/RegStatus/1001> ;
    rdfs:domain <http://rdaregistry.info/Elements/c/C10010> ;
    rdfs:isDefinedBy <http://rdaregistry.info/Elements/t/> ;
    rdfs:subPropertyOf <http://rdaregistry.info/Elements/t/P70036>,
        <http://rdaregistry.info/Elements/t/P70052> ;
    skos:definition "Relates a timespan to a corporate body who is active in its primary field of endeavour during a timespan."@en .

<http://rdaregistry.info/Elements/t/P70044> a rdf:Property ;
    rdfs:label "is period of activity of person of"@en ;
    rdakit:hasElementType "2" ;
    rdakit:toolkitDefinition "A person who is active in their primary field of endeavour during a timespan."@en ;
    rdakit:toolkitLabel "period of activity of person of"@en ;
    reg:hasSubproperty <http://rdaregistry.info/Elements/t/datatype/P70044>,
        <http://rdaregistry.info/Elements/t/object/P70044> ;
    reg:hasUnconstrained <http://rdaregistry.info/Elements/u/P60990> ;
    reg:lexicalAlias <http://rdaregistry.info/Elements/t/periodOfActivityOfPersonOf.en> ;
    reg:name "periodOfActivityOfPersonOf"@en ;
    reg:status <http://metadataregistry.org/uri/RegStatus/1001> ;
    rdfs:domain <http://rdaregistry.info/Elements/c/C10010> ;
    rdfs:isDefinedBy <http://rdaregistry.info/Elements/t/> ;
    rdfs:subPropertyOf <http://rdaregistry.info/Elements/t/P70038>,
        <http://rdaregistry.info/Elements/t/P70051> ;
    skos:definition "Relates a timespan to a person who is active in their primary field of endeavour during a timespan."@en .

<http://rdaregistry.info/Elements/t/P70053> a rdf:Property ;
    rdfs:label "is period of activity of family of"@en ;
    rdakit:hasElementType "2" ;
    rdakit:toolkitDefinition "A family who is active in its primary field of endeavour during a timespan."@en ;
    rdakit:toolkitLabel "period of activity of family of"@en ;
    reg:hasSubproperty <http://rdaregistry.info/Elements/t/datatype/P70053> ;
    reg:hasUnconstrained <http://rdaregistry.info/Elements/u/P60990> ;
    reg:lexicalAlias <http://rdaregistry.info/Elements/t/periodOfActivityOfFamilyOf.en> ;
    reg:name "periodOfActivityOfFamilyOf"@en ;
    reg:status <http://metadataregistry.org/uri/RegStatus/1001> ;
    rdfs:domain <http://rdaregistry.info/Elements/c/C10010> ;
    rdfs:isDefinedBy <http://rdaregistry.info/Elements/t/> ;
    rdfs:subPropertyOf <http://rdaregistry.info/Elements/t/P70037>,
        <http://rdaregistry.info/Elements/t/P70052> ;
    skos:definition "Relates a timespan to a family who is active in its primary field of endeavour during a timespan."@en .

<http://rdaregistry.info/Elements/t/P70002> a rdf:Property ;
    rdfs:label "has related expression of timespan"@en ;
    rdakit:hasElementType "1" ;
    rdakit:toolkitDefinition "An expression that is associated with a timespan."@en ;
    rdakit:toolkitLabel "related expression of timespan"@en ;
    reg:hasSubproperty <http://rdaregistry.info/Elements/t/P70024>,
        <http://rdaregistry.info/Elements/t/P70041>,
        <http://rdaregistry.info/Elements/t/datatype/P70002>,
        <http://rdaregistry.info/Elements/t/object/P70002> ;
    reg:hasUnconstrained <http://rdaregistry.info/Elements/u/P61012> ;
    reg:lexicalAlias <http://rdaregistry.info/Elements/t/relatedExpressionOfTimespan.en> ;
    reg:name "relatedExpressionOfTimespan"@en ;
    reg:status <http://metadataregistry.org/uri/RegStatus/1001> ;
    rdfs:domain <http://rdaregistry.info/Elements/c/C10010> ;
    rdfs:isDefinedBy <http://rdaregistry.info/Elements/t/> ;
    rdfs:subPropertyOf <http://rdaregistry.info/Elements/t/P70010> ;
    skos:definition "Relates a timespan to an expression that is associated with a timespan."@en .

<http://rdaregistry.info/Elements/t/P70008> a rdf:Property ;
    rdfs:label "has related timespan of timespan"@en ;
    rdakit:hasElementType "1" ;
    rdakit:toolkitDefinition "A timespan that is associated with a timespan."@en ;
    rdakit:toolkitLabel "related timespan of timespan"@en ;
    reg:hasSubproperty <http://rdaregistry.info/Elements/t/P70034>,
        <http://rdaregistry.info/Elements/t/P70035>,
        <http://rdaregistry.info/Elements/t/datatype/P70008>,
        <http://rdaregistry.info/Elements/t/object/P70008> ;
    reg:hasUnconstrained <http://rdaregistry.info/Elements/u/P61017> ;
    reg:lexicalAlias <http://rdaregistry.info/Elements/t/relatedTimespanOfTimespan.en> ;
    reg:name "relatedTimespanOfTimespan"@en ;
    reg:status <http://metadataregistry.org/uri/RegStatus/1001> ;
    rdfs:domain <http://rdaregistry.info/Elements/c/C10010> ;
    rdfs:isDefinedBy <http://rdaregistry.info/Elements/t/> ;
    rdfs:subPropertyOf <http://rdaregistry.info/Elements/t/P70010> ;
    skos:definition "Relates a timespan to a timespan that is associated with a timespan."@en .

<http://rdaregistry.info/Elements/t/P70009> a rdf:Property ;
    rdfs:label "has related nomen of timespan"@en ;
    rdakit:hasElementType "1" ;
    rdakit:toolkitDefinition "A nomen that is associated with a timespan."@en ;
    rdakit:toolkitLabel "related nomen of timespan"@en ;
    reg:hasSubproperty <http://rdaregistry.info/Elements/t/P70016>,
        <http://rdaregistry.info/Elements/t/P70056>,
        <http://rdaregistry.info/Elements/t/datatype/P70009>,
        <http://rdaregistry.info/Elements/t/object/P70009> ;
    reg:hasUnconstrained <http://rdaregistry.info/Elements/u/P61024> ;
    reg:lexicalAlias <http://rdaregistry.info/Elements/t/relatedNomenOfTimespan.en> ;
    reg:name "relatedNomenOfTimespan"@en ;
    reg:status <http://metadataregistry.org/uri/RegStatus/1001> ;
    rdfs:domain <http://rdaregistry.info/Elements/c/C10010> ;
    rdfs:isDefinedBy <http://rdaregistry.info/Elements/t/> ;
    rdfs:subPropertyOf <http://rdaregistry.info/Elements/t/P70010> ;
    skos:definition "Relates a timespan to a nomen that is associated with a timespan."@en .

<http://rdaregistry.info/Elements/t/P70015> a rdf:Property ;
    rdfs:label "has access point for timespan"@en ;
    rdakit:hasElementType "3" ;
    rdakit:toolkitDefinition "An appellation of timespan in natural language that is taken from a vocabulary encoding scheme or is constructed using a string encoding scheme."@en ;
    rdakit:toolkitLabel "access point for timespan"@en ;
    reg:hasSubproperty <http://rdaregistry.info/Elements/t/P70047>,
        <http://rdaregistry.info/Elements/t/P70048>,
        <http://rdaregistry.info/Elements/t/datatype/P70015>,
        <http://rdaregistry.info/Elements/t/object/P70015> ;
    reg:hasUnconstrained <http://rdaregistry.info/Elements/u/P60906> ;
    reg:lexicalAlias <http://rdaregistry.info/Elements/t/accessPointForTimespan.en> ;
    reg:name "accessPointForTimespan"@en ;
    reg:status <http://metadataregistry.org/uri/RegStatus/1001> ;
    rdfs:domain <http://rdaregistry.info/Elements/c/C10010> ;
    rdfs:isDefinedBy <http://rdaregistry.info/Elements/t/> ;
    rdfs:subPropertyOf <http://rdaregistry.info/Elements/t/P70016> ;
    skos:definition "Relates a timespan to an appellation of timespan in natural language that is taken from a vocabulary encoding scheme or is constructed using a string encoding scheme."@en .

<http://rdaregistry.info/Elements/t/P70017> a rdf:Property ;
    rdfs:label "has name of timespan"@en ;
    rdakit:hasElementType "3" ;
    rdakit:toolkitDefinition "An appellation of timespan in natural language and phrasing used in common discourse."@en ;
    rdakit:toolkitLabel "name of timespan"@en ;
    reg:hasSubproperty <http://rdaregistry.info/Elements/t/P70049>,
        <http://rdaregistry.info/Elements/t/P70050>,
        <http://rdaregistry.info/Elements/t/datatype/P70017>,
        <http://rdaregistry.info/Elements/t/object/P70017> ;
    reg:hasUnconstrained <http://rdaregistry.info/Elements/u/P60935> ;
    reg:lexicalAlias <http://rdaregistry.info/Elements/t/nameOfTimespan.en> ;
    reg:name "nameOfTimespan"@en ;
    reg:status <http://metadataregistry.org/uri/RegStatus/1001> ;
    rdfs:domain <http://rdaregistry.info/Elements/c/C10010> ;
    rdfs:isDefinedBy <http://rdaregistry.info/Elements/t/> ;
    rdfs:subPropertyOf <http://rdaregistry.info/Elements/t/P70016> ;
    skos:definition "Relates a timespan to an appellation of timespan in natural language and phrasing used in common discourse."@en .

<http://rdaregistry.info/Elements/t/P70051> a rdf:Property ;
    rdfs:label "is period of activity of agent of"@en ;
    rdakit:hasElementType "2" ;
    rdakit:toolkitDefinition "An agent who is active in its primary field of endeavour during a timespan."@en ;
    rdakit:toolkitLabel "period of activity of agent of"@en ;
    reg:hasSubproperty <http://rdaregistry.info/Elements/t/P70044>,
        <http://rdaregistry.info/Elements/t/datatype/P70051> ;
    reg:hasUnconstrained <http://rdaregistry.info/Elements/u/P60990> ;
    reg:lexicalAlias <http://rdaregistry.info/Elements/t/periodOfActivityOfAgentOf.en> ;
    reg:name "periodOfActivityOfAgentOf"@en ;
    reg:status <http://metadataregistry.org/uri/RegStatus/1001> ;
    rdfs:domain <http://rdaregistry.info/Elements/c/C10010> ;
    rdfs:isDefinedBy <http://rdaregistry.info/Elements/t/> ;
    rdfs:subPropertyOf <http://rdaregistry.info/Elements/t/P70005> ;
    skos:definition "Relates a timespan to an agent who is active in its primary field of endeavour during a timespan."@en .

<http://rdaregistry.info/Elements/t/P70052> a rdf:Property ;
    rdfs:label "is period of activity of collective agent of"@en ;
    rdakit:hasElementType "2" ;
    rdakit:toolkitDefinition "A collective agent who is active in its primary field of endeavour during a timespan."@en ;
    rdakit:toolkitLabel "period of activity of collective agent of"@en ;
    reg:hasSubproperty <http://rdaregistry.info/Elements/t/P70043>,
        <http://rdaregistry.info/Elements/t/P70053>,
        <http://rdaregistry.info/Elements/t/datatype/P70052> ;
    reg:hasUnconstrained <http://rdaregistry.info/Elements/u/P60990> ;
    reg:lexicalAlias <http://rdaregistry.info/Elements/t/periodOfActivityOfCollectiveAgentOf.en> ;
    reg:name "periodOfActivityOfCollectiveAgentOf"@en ;
    reg:status <http://metadataregistry.org/uri/RegStatus/1001> ;
    rdfs:domain <http://rdaregistry.info/Elements/c/C10010> ;
    rdfs:isDefinedBy <http://rdaregistry.info/Elements/t/> ;
    rdfs:subPropertyOf <http://rdaregistry.info/Elements/t/P70006>,
        <http://rdaregistry.info/Elements/t/P70051> ;
    skos:definition "Relates a timespan to a collective agent who is active in its primary field of endeavour during a timespan."@en .

<http://rdaregistry.info/Elements/t/P70005> a rdf:Property ;
    rdfs:label "has related agent of timespan"@en ;
    rdakit:hasElementType "1" ;
    rdakit:toolkitDefinition "An agent who is associated with a timespan."@en ;
    rdakit:toolkitLabel "related agent of timespan"@en ;
    reg:hasSubproperty <http://rdaregistry.info/Elements/t/P70006>,
        <http://rdaregistry.info/Elements/t/P70011>,
        <http://rdaregistry.info/Elements/t/P70051>,
        <http://rdaregistry.info/Elements/t/datatype/P70005>,
        <http://rdaregistry.info/Elements/t/object/P70005> ;
    reg:hasUnconstrained <http://rdaregistry.info/Elements/u/P61010> ;
    reg:lexicalAlias <http://rdaregistry.info/Elements/t/relatedAgentOfTimespan.en> ;
    reg:name "relatedAgentOfTimespan"@en ;
    reg:status <http://metadataregistry.org/uri/RegStatus/1001> ;
    rdfs:domain <http://rdaregistry.info/Elements/c/C10010> ;
    rdfs:isDefinedBy <http://rdaregistry.info/Elements/t/> ;
    rdfs:subPropertyOf <http://rdaregistry.info/Elements/t/P70010> ;
    skos:definition "Relates a timespan to an agent who is associated with a timespan."@en .

<http://rdaregistry.info/Elements/t/P70006> a rdf:Property ;
    rdfs:label "has related collective agent of timespan"@en ;
    rdakit:hasElementType "1" ;
    rdakit:toolkitDefinition "A collective agent who is associated with a timespan."@en ;
    rdakit:toolkitLabel "related collective agent of timespan"@en ;
    reg:hasSubproperty <http://rdaregistry.info/Elements/t/P70012>,
        <http://rdaregistry.info/Elements/t/P70013>,
        <http://rdaregistry.info/Elements/t/P70052>,
        <http://rdaregistry.info/Elements/t/datatype/P70006>,
        <http://rdaregistry.info/Elements/t/object/P70006> ;
    reg:hasUnconstrained <http://rdaregistry.info/Elements/u/P61010> ;
    reg:lexicalAlias <http://rdaregistry.info/Elements/t/relatedCollectiveAgentOfTimespan.en> ;
    reg:name "relatedCollectiveAgentOfTimespan"@en ;
    reg:status <http://metadataregistry.org/uri/RegStatus/1001> ;
    rdfs:domain <http://rdaregistry.info/Elements/c/C10010> ;
    rdfs:isDefinedBy <http://rdaregistry.info/Elements/t/> ;
    rdfs:subPropertyOf <http://rdaregistry.info/Elements/t/P70005> ;
    skos:definition "Relates a timespan to a collective agent who is associated with a timespan."@en .

<http://rdaregistry.info/Elements/t/P70016> a rdf:Property ;
    rdfs:label "has appellation of timespan"@en ;
    rdakit:hasElementType "3" ;
    rdakit:toolkitDefinition "A nomen used within a given scheme or context to refer to a timespan."@en ;
    rdakit:toolkitLabel "appellation of timespan"@en ;
    reg:hasSubproperty <http://rdaregistry.info/Elements/t/P70015>,
        <http://rdaregistry.info/Elements/t/P70017>,
        <http://rdaregistry.info/Elements/t/P70018>,
        <http://rdaregistry.info/Elements/t/datatype/P70016>,
        <http://rdaregistry.info/Elements/t/object/P70016> ;
    reg:hasUnconstrained <http://rdaregistry.info/Elements/u/P60909> ;
    reg:lexicalAlias <http://rdaregistry.info/Elements/t/appellationOfTimespan.en> ;
    reg:name "appellationOfTimespan"@en ;
    reg:status <http://metadataregistry.org/uri/RegStatus/1001> ;
    rdfs:domain <http://rdaregistry.info/Elements/c/C10010> ;
    rdfs:isDefinedBy <http://rdaregistry.info/Elements/t/> ;
    rdfs:subPropertyOf <http://rdaregistry.info/Elements/t/P70009> ;
    skos:definition "Relates a timespan to a nomen used within a given scheme or context to refer to a timespan."@en .

<http://rdaregistry.info/Elements/t/P70038> a rdf:Property ;
    rdfs:label "is date associated with person of"@en ;
    rdakit:hasElementType "2" ;
    rdakit:toolkitDefinition "A person who has a significant association with a timespan."@en ;
    rdakit:toolkitLabel "date associated with person of"@en ;
    reg:hasSubproperty <http://rdaregistry.info/Elements/t/P70029>,
        <http://rdaregistry.info/Elements/t/P70030>,
        <http://rdaregistry.info/Elements/t/P70044>,
        <http://rdaregistry.info/Elements/t/datatype/P70038>,
        <http://rdaregistry.info/Elements/t/object/P70038> ;
    reg:hasUnconstrained <http://rdaregistry.info/Elements/u/P60974> ;
    reg:lexicalAlias <http://rdaregistry.info/Elements/t/dateAssociatedWithPersonOf.en> ;
    reg:name "dateAssociatedWithPersonOf"@en ;
    reg:status <http://metadataregistry.org/uri/RegStatus/1001> ;
    rdfs:domain <http://rdaregistry.info/Elements/c/C10010> ;
    rdfs:isDefinedBy <http://rdaregistry.info/Elements/t/> ;
    rdfs:subPropertyOf <http://rdaregistry.info/Elements/t/P70011> ;
    skos:definition "Relates a timespan to a person who has a significant association with a timespan."@en .

<http://rdaregistry.info/Elements/t/P70036> a rdf:Property ;
    rdfs:label "is date associated with corporate body of"@en ;
    rdakit:hasElementType "2" ;
    rdakit:toolkitDefinition "A corporate body who has a significant association with a timespan."@en ;
    rdakit:toolkitLabel "date associated with corporate body of"@en ;
    reg:hasSubproperty <http://rdaregistry.info/Elements/t/P70031>,
        <http://rdaregistry.info/Elements/t/P70032>,
        <http://rdaregistry.info/Elements/t/P70033>,
        <http://rdaregistry.info/Elements/t/P70043>,
        <http://rdaregistry.info/Elements/t/datatype/P70036>,
        <http://rdaregistry.info/Elements/t/object/P70036> ;
    reg:hasUnconstrained <http://rdaregistry.info/Elements/u/P60974> ;
    reg:lexicalAlias <http://rdaregistry.info/Elements/t/dateAssociatedWithCorporateBodyOf.en> ;
    reg:name "dateAssociatedWithCorporateBodyOf"@en ;
    reg:status <http://metadataregistry.org/uri/RegStatus/1001> ;
    rdfs:domain <http://rdaregistry.info/Elements/c/C10010> ;
    rdfs:isDefinedBy <http://rdaregistry.info/Elements/t/> ;
    rdfs:subPropertyOf <http://rdaregistry.info/Elements/t/P70013> ;
    skos:definition "Relates a timespan to a corporate body who has a significant association with a timespan."@en .

<http://rdaregistry.info/Elements/t/P70020> a rdf:Property ;
    rdfs:label "is date of manifestation of"@en ;
    rdakit:hasElementType "2" ;
    rdakit:toolkitDefinition "A manifestation that is a published manifestation that is published, released, issued, printed, duplicated, cast, distributed, etc., or an unpublished manifestation that is inscribed, fabricated, constructed, etc., during a timespan."@en ;
    rdakit:toolkitLabel "date of manifestation of"@en ;
    reg:hasSubproperty <http://rdaregistry.info/Elements/t/P70019>,
        <http://rdaregistry.info/Elements/t/P70025>,
        <http://rdaregistry.info/Elements/t/P70026>,
        <http://rdaregistry.info/Elements/t/P70027>,
        <http://rdaregistry.info/Elements/t/P70028>,
        <http://rdaregistry.info/Elements/t/datatype/P70020>,
        <http://rdaregistry.info/Elements/t/object/P70020> ;
    reg:hasUnconstrained <http://rdaregistry.info/Elements/u/P60984> ;
    reg:lexicalAlias <http://rdaregistry.info/Elements/t/dateOfManifestationOf.en> ;
    reg:name "dateOfManifestationOf"@en ;
    reg:status <http://metadataregistry.org/uri/RegStatus/1001> ;
    rdfs:domain <http://rdaregistry.info/Elements/c/C10010> ;
    rdfs:isDefinedBy <http://rdaregistry.info/Elements/t/> ;
    rdfs:subPropertyOf <http://rdaregistry.info/Elements/t/P70003> ;
    skos:definition "Relates a timespan to a manifestation that is published, released, issued, printed, duplicated, cast, distributed, etc., in a published form or is inscribed, fabricated, constructed, etc., in a unpublished form during a timespan."@en .

<http://rdaregistry.info/Elements/t/P70001> a rdf:Property ;
    rdfs:label "has related work of timespan"@en ;
    rdakit:hasElementType "1" ;
    rdakit:toolkitDefinition "A work that is associated with a timespan."@en ;
    rdakit:toolkitLabel "related work of timespan"@en ;
    reg:hasSubproperty <http://rdaregistry.info/Elements/t/P70021>,
        <http://rdaregistry.info/Elements/t/P70022>,
        <http://rdaregistry.info/Elements/t/P70042>,
        <http://rdaregistry.info/Elements/t/P70054>,
        <http://rdaregistry.info/Elements/t/P70055>,
        <http://rdaregistry.info/Elements/t/P70057>,
        <http://rdaregistry.info/Elements/t/datatype/P70001>,
        <http://rdaregistry.info/Elements/t/object/P70001> ;
    reg:hasUnconstrained <http://rdaregistry.info/Elements/u/P61012> ;
    reg:lexicalAlias <http://rdaregistry.info/Elements/t/relatedWorkOfTimespan.en> ;
    reg:name "relatedWorkOfTimespan"@en ;
    reg:status <http://metadataregistry.org/uri/RegStatus/1001> ;
    rdfs:domain <http://rdaregistry.info/Elements/c/C10010> ;
    rdfs:isDefinedBy <http://rdaregistry.info/Elements/t/> ;
    rdfs:subPropertyOf <http://rdaregistry.info/Elements/t/P70010> ;
    skos:definition "Relates a timespan to a work that is associated with a timespan."@en .

<http://rdaregistry.info/Elements/t/P70010> a rdf:Property ;
    rdfs:label "has related RDA entity of timespan"@en ;
    rdakit:hasElementType "1" ;
    rdakit:toolkitDefinition "An RDA entity that is associated with a timespan."@en ;
    rdakit:toolkitLabel "related RDA entity of timespan"@en ;
    reg:hasSubproperty <http://rdaregistry.info/Elements/t/P70001>,
        <http://rdaregistry.info/Elements/t/P70002>,
        <http://rdaregistry.info/Elements/t/P70003>,
        <http://rdaregistry.info/Elements/t/P70004>,
        <http://rdaregistry.info/Elements/t/P70005>,
        <http://rdaregistry.info/Elements/t/P70007>,
        <http://rdaregistry.info/Elements/t/P70008>,
        <http://rdaregistry.info/Elements/t/P70009>,
        <http://rdaregistry.info/Elements/t/datatype/P70010>,
        <http://rdaregistry.info/Elements/t/object/P70010> ;
    reg:hasUnconstrained <http://rdaregistry.info/Elements/u/P61035> ;
    reg:lexicalAlias <http://rdaregistry.info/Elements/t/relatedRDAEntityOfTimespan.en> ;
    reg:name "relatedRDAEntityOfTimespan"@en ;
    reg:status <http://metadataregistry.org/uri/RegStatus/1001> ;
    rdfs:domain <http://rdaregistry.info/Elements/c/C10010> ;
    rdfs:isDefinedBy <http://rdaregistry.info/Elements/t/> ;
    skos:definition "Relates a timespan to an RDA entity that is associated with a timespan."@en .

<http://metadataregistry.org/uri/RegStatus/1001> a skos:Concept ;
    skos:prefLabel "Published"@en .

<http://rdaregistry.info/Elements/t/> dc:title "RDA Timespan properties"@en ;
    skos:note "Properties derived from RDA elements and relationship designators with the domain of RDA Timespan. Warning! This element set is under development as part of the RDA Toolkit Restructure and Redesign Project. The last stable version can be found in release v2.7.3 of RDA Vocabularies in the RDA Registry."@en .

